<?xml version="1.0" encoding = "UTF-8"?>
<rdf:RDF
    xmlns:dc="http://purl.org/dc/elements/1.1/"
    xmlns:rdakit="http://metadataregistry.org/uri/profile/rdakit/"
    xmlns:rdf="http://www.w3.org/1999/02/22-rdf-syntax-ns#"
    xmlns:reg="http://metadataregistry.org/uri/profile/regap/"
    xmlns:owl="http://www.w3.org/2002/07/owl#"
    xmlns:skos="http://www.w3.org/2004/02/skos/core#">

<owl:Ontology rdf:about="http://rdaregistry.info/termList/AspectRatio" />
<!-- Scheme: RDA Aspect Ratio Designation -->
    <skos:ConceptScheme rdf:about="http://rdaregistry.info/termList/AspectRatio">
        <dc:title>RDA Aspect Ratio Designation</dc:title>
    </skos:ConceptScheme>

<!-- Concept: full screen  -->
    <skos:Concept rdf:about="http://rdaregistry.info/termList/AspectRatio/1001" xml:lang="en">
      <skos:inScheme rdf:resource="http://rdaregistry.info/termList/AspectRatio"/>
      <reg:status rdf:resource="http://metadataregistry.org/uri/RegStatus/1001"/>
      <reg:identifier rdf:resource="http://metadataregistry.org/concepts/727"/>
      <skos:prefLabel xml:lang="en">full screen</skos:prefLabel>
      <skos:definition xml:lang="en">An aspect ratio designation for a moving image resource of less than 1.5:1.</skos:definition>
      <skos:prefLabel xml:lang="de">Vollbild</skos:prefLabel>
      <skos:prefLabel xml:lang="fr">plein écran</skos:prefLabel>
      <skos:definition xml:lang="de">Ein Bildformat einer Bewegtbildressource von weniger als 1,5:1.</skos:definition>
      <skos:definition xml:lang="fr">Désignation de format d’image pour une ressource d’images animées dont le format d’image est inférieur à 1,5:1.</skos:definition>
      <skos:prefLabel xml:lang="es">pantalla completa</skos:prefLabel>
      <skos:definition xml:lang="es">Proporción dimensional de un recurso de imagen en movimiento menor que 1.5:1.</skos:definition>
      <rdakit:toolkitLabel xml:lang="en">full screen</rdakit:toolkitLabel>
      <rdakit:toolkitLabel xml:lang="fr">plein écran</rdakit:toolkitLabel>
      <rdakit:toolkitDefinition xml:lang="en">An aspect ratio designation for a moving image resource of less than 1.5:1.</rdakit:toolkitDefinition>
      <rdakit:toolkitDefinition xml:lang="fr">Désignation de format d’image pour une ressource d’images animées dont le format d’image est inférieur à 1,5:1.</rdakit:toolkitDefinition>
      <rdakit:toolkitLabel xml:lang="de">Vollbild</rdakit:toolkitLabel>
      <rdakit:toolkitDefinition xml:lang="de">Ein Bildformat einer Bewegtbildressource von weniger als 1,5:1.</rdakit:toolkitDefinition>
      <rdakit:toolkitLabel xml:lang="es">pantalla completa</rdakit:toolkitLabel>
      <rdakit:toolkitDefinition xml:lang="es">Proporción dimensional de un recurso de imagen en movimiento menor que 1.5:1.</rdakit:toolkitDefinition>
      <skos:prefLabel xml:lang="zh">全屏</skos:prefLabel>
      <rdakit:toolkitLabel xml:lang="zh">全屏</rdakit:toolkitLabel>
      <skos:definition xml:lang="zh">动态图像资源的宽高比小于1.5：1。</skos:definition>
      <rdakit:toolkitDefinition xml:lang="zh">动态图像资源的宽高比小于1.5：1。</rdakit:toolkitDefinition>
      <skos:altLabel xml:lang="en">full-screen</skos:altLabel>
      <skos:prefLabel xml:lang="nl">full screen</skos:prefLabel>
      <rdakit:toolkitLabel xml:lang="nl">full screen</rdakit:toolkitLabel>
      <skos:definition xml:lang="nl">Aspectratio voor een resource met bewegend beeld minder dan 1.5:1</skos:definition>
      <rdakit:toolkitDefinition xml:lang="nl">Aspectratio voor een resource met bewegend beeld minder dan 1.5:1</rdakit:toolkitDefinition>
      <skos:prefLabel xml:lang="it">a tutto schermo</skos:prefLabel>
      <rdakit:toolkitLabel xml:lang="it">a tutto schermo</rdakit:toolkitLabel>
      <skos:prefLabel xml:lang="fi">full screen</skos:prefLabel>
      <rdakit:toolkitLabel xml:lang="fi">full screen</rdakit:toolkitLabel>
      <skos:prefLabel xml:lang="sv">normalbild</skos:prefLabel>
      <rdakit:toolkitLabel xml:lang="sv">normalbild</rdakit:toolkitLabel>
      <skos:prefLabel xml:lang="vi">toàn màn hình</skos:prefLabel>
      <skos:altLabel xml:lang="vi">toàn-màn-hình</skos:altLabel>
      <rdakit:toolkitLabel xml:lang="vi">toàn màn hình</rdakit:toolkitLabel>
      <skos:definition xml:lang="vi">Định danh tỷ lệ bề ngoài cho tài nguyên hình ảnh động nhỏ hơn 1,5:1.</skos:definition>
      <rdakit:toolkitDefinition xml:lang="vi">Định danh tỷ lệ về ngoài cho tài nguyên hình ảnh động nhỏ hơn 1,5:1.</rdakit:toolkitDefinition>
      <skos:prefLabel xml:lang="ca">pantalla completa</skos:prefLabel>
      <rdakit:toolkitLabel xml:lang="ca">pantalla completa</rdakit:toolkitLabel>
      <skos:definition xml:lang="ca">Relació d’aspecte d’un recurs d’imatge en moviment de menys d’1,5:1.</skos:definition>
      <rdakit:toolkitDefinition xml:lang="ca">Relació d’aspecte d’un recurs d’imatge en moviment de menys d’1,5:1.</rdakit:toolkitDefinition>
      <skos:prefLabel xml:lang="no">fullskjerm</skos:prefLabel>
      <rdakit:toolkitLabel xml:lang="no">fullskjerm</rdakit:toolkitLabel>
      <skos:definition xml:lang="no">En betegnelse for bildesideforhold på under 1,5:1 for en levende bilde-ressurs.</skos:definition>
      <rdakit:toolkitDefinition xml:lang="no">En betegnelse for bildesideforhold på under 1,5:1 for en levende bilde-ressurs.</rdakit:toolkitDefinition>
      <skos:prefLabel xml:lang="da">fuldskærm</skos:prefLabel>
      <rdakit:toolkitLabel xml:lang="da">fuldskærm</rdakit:toolkitLabel>
      <skos:definition xml:lang="da">Billedformat for en levende billedressource på mindre end 1,5:1.</skos:definition>
      <rdakit:toolkitDefinition xml:lang="da">Billedformat for en levende billedressource på mindre end 1,5:1.</rdakit:toolkitDefinition>
      <skos:definition xml:lang="fi">Liikkuvan kuvan kuvasuhde, joka on pienempi kuin 1.5:1.</skos:definition>
      <rdakit:toolkitDefinition xml:lang="fi">Liikkuvan kuvan kuvasuhde, joka on pienempi kuin 1.5:1.</rdakit:toolkitDefinition>
    </skos:Concept>
<!-- Concept: mixed aspect ratio  -->
    <skos:Concept rdf:about="http://rdaregistry.info/termList/AspectRatio/1003" xml:lang="en">
      <skos:inScheme rdf:resource="http://rdaregistry.info/termList/AspectRatio"/>
      <reg:status rdf:resource="http://metadataregistry.org/uri/RegStatus/1001"/>
      <reg:identifier rdf:resource="http://metadataregistry.org/concepts/729"/>
      <skos:prefLabel xml:lang="en">mixed aspect ratio</skos:prefLabel>
      <skos:definition xml:lang="en">An aspect ratio designation for a moving image resource that includes multiple aspect ratios within the same resource.</skos:definition>
      <skos:prefLabel xml:lang="de">gemischt</skos:prefLabel>
      <skos:prefLabel xml:lang="fr">mixte</skos:prefLabel>
      <skos:definition xml:lang="de">Ein Bildformat einer Bewegtbildressource, die mehrere Bildformate innerhalb derselben Ressource enthält.</skos:definition>
      <skos:definition xml:lang="fr">Désignation de format d’image pour une ressource d’images animées comprenant divers formats d’image à l’intérieur de la même ressource.</skos:definition>
      <skos:prefLabel xml:lang="es">mixta</skos:prefLabel>
      <rdakit:toolkitLabel xml:lang="en">mixed aspect ratio</rdakit:toolkitLabel>
      <rdakit:toolkitLabel xml:lang="fr">mixte</rdakit:toolkitLabel>
      <rdakit:toolkitDefinition xml:lang="en">An aspect ratio designation for a moving image resource that includes multiple aspect ratios within the same resource.</rdakit:toolkitDefinition>
      <rdakit:toolkitDefinition xml:lang="fr">Désignation de format d’image pour une ressource d’images animées comprenant divers formats d’image à l’intérieur de la même ressource.</rdakit:toolkitDefinition>
      <rdakit:toolkitLabel xml:lang="de">gemischt</rdakit:toolkitLabel>
      <rdakit:toolkitDefinition xml:lang="de">Ein Bildformat einer Bewegtbildressource, die mehrere Bildformate innerhalb derselben Ressource enthält.</rdakit:toolkitDefinition>
      <rdakit:toolkitLabel xml:lang="es">mixta</rdakit:toolkitLabel>
      <skos:prefLabel xml:lang="zh">混合</skos:prefLabel>
      <rdakit:toolkitLabel xml:lang="zh">混合</rdakit:toolkitLabel>
      <skos:definition xml:lang="zh">在同一资源中动态图像资源包括多种宽高比。</skos:definition>
      <rdakit:toolkitDefinition xml:lang="zh">在同一资源中动态图像资源包括多种宽高比。</rdakit:toolkitDefinition>
      <skos:definition xml:lang="es">Proporción dimensional de un recurso que incluye múltiples proporciones dimensionales dentro del mismo recurso.</skos:definition>
      <rdakit:toolkitDefinition xml:lang="es">Proporción dimensional de un recurso que incluye múltiples proporciones dimensionales dentro del mismo recurso.</rdakit:toolkitDefinition>
      <skos:prefLabel xml:lang="nl">gemengd</skos:prefLabel>
      <rdakit:toolkitLabel xml:lang="nl">gemengd</rdakit:toolkitLabel>
      <skos:definition xml:lang="nl">Aspectratio voor een resource met bewegend beeld dat meerdere aspectratio's bevat binnen dezelfde resource</skos:definition>
      <rdakit:toolkitDefinition xml:lang="nl">Aspectratio voor een resource met bewegend beeld dat meerdere aspectratio's bevat binnen dezelfde resource</rdakit:toolkitDefinition>
      <skos:prefLabel xml:lang="it">misto</skos:prefLabel>
      <rdakit:toolkitLabel xml:lang="it">misto</rdakit:toolkitLabel>
      <skos:prefLabel xml:lang="fi">yhdistelmä (kuvasuhde)</skos:prefLabel>
      <rdakit:toolkitLabel xml:lang="fi">yhdistelmä (kuvasuhde)</rdakit:toolkitLabel>
      <skos:prefLabel xml:lang="sv">blandade bildförhållanden</skos:prefLabel>
      <rdakit:toolkitLabel xml:lang="sv">blandade bildförhållanden</rdakit:toolkitLabel>
      <skos:prefLabel xml:lang="vi">tỷ lệ bề ngoài hỗn hợp</skos:prefLabel>
      <rdakit:toolkitLabel xml:lang="vi">tỷ lệ bề ngoài hỗn hợp</rdakit:toolkitLabel>
      <skos:definition xml:lang="vi">Định danh tỷ lệ bề ngoài cho tài nguyên hình ảnh động bao gồm nhiều tỷ lệ bề ngoài bên trong cùng tài nguyên.</skos:definition>
      <rdakit:toolkitDefinition xml:lang="vi">Định danh tỷ lệ về ngoài cho tài nguyên hình ảnh động bao gồm các tỷ lệ bề ngoài khác nhau bên trong cùng tài nguyên.</rdakit:toolkitDefinition>
      <skos:prefLabel xml:lang="ca">relació d’aspecte mixta</skos:prefLabel>
      <rdakit:toolkitLabel xml:lang="ca">relació d’aspecte mixta</rdakit:toolkitLabel>
      <skos:definition xml:lang="ca">Relació d’aspecte d’un recurs d’imatges en moviment que inclou diverses relacions d’aspecte dins del mateix recurs.</skos:definition>
      <rdakit:toolkitDefinition xml:lang="ca">Relació d’aspecte d’un recurs d’imatges en moviment que inclou diverses relacions d’aspecte dins del mateix recurs.</rdakit:toolkitDefinition>
      <skos:prefLabel xml:lang="no">blandet bildesideforhold</skos:prefLabel>
      <rdakit:toolkitLabel xml:lang="no">blandet bildesideforhold</rdakit:toolkitLabel>
      <skos:definition xml:lang="no">En betegnelse for bildesideforhold for en levende bilde-ressurs som har flere ulike bildesideforhold innenfor samme ressurs.</skos:definition>
      <rdakit:toolkitDefinition xml:lang="no">En betegnelse for bildesideforhold for en levende bilde-ressurs som har flere ulike bildesideforhold innenfor samme ressurs.</rdakit:toolkitDefinition>
      <skos:prefLabel xml:lang="da">blandet billedformat</skos:prefLabel>
      <rdakit:toolkitLabel xml:lang="da">blandet billedformat</rdakit:toolkitLabel>
      <skos:definition xml:lang="da">Billedformat for en levende billedressource, der omfatter flere billedformater inden for samme ressource</skos:definition>
      <rdakit:toolkitDefinition xml:lang="da">Billedformat for en levende billedressource, der omfatter flere billedformater inden for samme ressource</rdakit:toolkitDefinition>
      <skos:definition xml:lang="fi">Kuvasuhde liikkuvaa kuvaa sisältävälle aineistolle, joka käsittää useita eri kuvasuhteita.</skos:definition>
      <rdakit:toolkitDefinition xml:lang="fi">Kuvasuhde liikkuvaa kuvaa sisältävälle aineistolle, joka käsittää useita eri kuvasuhteita.</rdakit:toolkitDefinition>
    </skos:Concept>
<!-- Concept: wide screen  -->
    <skos:Concept rdf:about="http://rdaregistry.info/termList/AspectRatio/1002" xml:lang="en">
      <skos:inScheme rdf:resource="http://rdaregistry.info/termList/AspectRatio"/>
      <reg:status rdf:resource="http://metadataregistry.org/uri/RegStatus/1001"/>
      <reg:identifier rdf:resource="http://metadataregistry.org/concepts/728"/>
      <skos:prefLabel xml:lang="en">wide screen</skos:prefLabel>
      <skos:definition xml:lang="en">An aspect ratio designation for a moving image resource of 1.5:1 or greater.</skos:definition>
      <skos:prefLabel xml:lang="de">Breitbild</skos:prefLabel>
      <skos:prefLabel xml:lang="fr">écran large</skos:prefLabel>
      <skos:definition xml:lang="de">Ein Bildformat einer Bewegtbildressource von 1,5:1 oder höher.</skos:definition>
      <skos:prefLabel xml:lang="es">pantalla ancha</skos:prefLabel>
      <skos:definition xml:lang="fr">Désignation de format d’image d’une ressource d’images animées dont le format d’image est égal ou supérieur à 1,5:1.</skos:definition>
      <rdakit:toolkitLabel xml:lang="en">wide screen</rdakit:toolkitLabel>
      <rdakit:toolkitLabel xml:lang="fr">écran large</rdakit:toolkitLabel>
      <rdakit:toolkitDefinition xml:lang="en">An aspect ratio designation for a moving image resource of 1.5:1 or greater.</rdakit:toolkitDefinition>
      <rdakit:toolkitDefinition xml:lang="fr">Désignation de format d’image d’une ressource d’images animées dont le format d’image est égal ou supérieur à 1,5:1.</rdakit:toolkitDefinition>
      <rdakit:toolkitLabel xml:lang="de">Breitbild</rdakit:toolkitLabel>
      <rdakit:toolkitDefinition xml:lang="de">Ein Bildformat einer Bewegtbildressource von 1,5:1 oder höher.</rdakit:toolkitDefinition>
      <rdakit:toolkitLabel xml:lang="es">pantalla ancha</rdakit:toolkitLabel>
      <skos:prefLabel xml:lang="zh">宽屏</skos:prefLabel>
      <rdakit:toolkitLabel xml:lang="zh">宽屏</rdakit:toolkitLabel>
      <skos:definition xml:lang="zh">动态图像的宽高比为1.5:1或更大。</skos:definition>
      <rdakit:toolkitDefinition xml:lang="zh">动态图像的宽高比为1.5:1或更大。</rdakit:toolkitDefinition>
      <skos:altLabel xml:lang="en">wide-screen</skos:altLabel>
      <skos:definition xml:lang="es">Proporción dimensional de un recurso de imagen en movimiento de 1.5:1 o mayor.</skos:definition>
      <rdakit:toolkitDefinition xml:lang="es">Proporción dimensional de un recurso de imagen en movimiento de 1.5:1 o mayor.</rdakit:toolkitDefinition>
      <skos:prefLabel xml:lang="nl">widescreen</skos:prefLabel>
      <rdakit:toolkitLabel xml:lang="nl">widescreen</rdakit:toolkitLabel>
      <skos:definition xml:lang="nl">Aspectratio voor een resource met bewegend beeld van 1.5:1 of meer</skos:definition>
      <rdakit:toolkitDefinition xml:lang="nl">Aspectratio voor een resource met bewegend beeld van 1.5:1 of meer</rdakit:toolkitDefinition>
      <skos:prefLabel xml:lang="it">a schermo panoramico</skos:prefLabel>
      <rdakit:toolkitLabel xml:lang="it">a schermo panoramico</rdakit:toolkitLabel>
      <skos:prefLabel xml:lang="fi">wide screen</skos:prefLabel>
      <rdakit:toolkitLabel xml:lang="fi">wide screen</rdakit:toolkitLabel>
      <skos:prefLabel xml:lang="sv">bredbild</skos:prefLabel>
      <rdakit:toolkitLabel xml:lang="sv">bredbild</rdakit:toolkitLabel>
      <skos:prefLabel xml:lang="vi">màn hình rộng</skos:prefLabel>
      <skos:altLabel xml:lang="vi">màn-hình-rộng</skos:altLabel>
      <rdakit:toolkitLabel xml:lang="vi">màn hình rộng</rdakit:toolkitLabel>
      <skos:definition xml:lang="vi">Định danh tỷ lệ bề ngoài cho tài nguyên hình ảnh động bằng 1,5:1 hoặc lớn hơn.</skos:definition>
      <rdakit:toolkitDefinition xml:lang="vi">Định danh tỷ lệ về ngoài cho tài nguyên hình ảnh động là 1,5:1 hoặc lớn hơn.</rdakit:toolkitDefinition>
      <skos:prefLabel xml:lang="ca">pantalla panoràmica</skos:prefLabel>
      <rdakit:toolkitLabel xml:lang="ca">pantalla panoràmica</rdakit:toolkitLabel>
      <skos:definition xml:lang="ca">Relació d’aspecte d’un recurs d’imatges en moviment igual o superior 1,5:1.</skos:definition>
      <rdakit:toolkitDefinition xml:lang="ca">Relació d’aspecte d’un recurs d’imatges en moviment igual o superior 1,5:1.</rdakit:toolkitDefinition>
      <skos:prefLabel xml:lang="no">widescreen</skos:prefLabel>
      <rdakit:toolkitLabel xml:lang="no">widescreen</rdakit:toolkitLabel>
      <skos:definition xml:lang="no">En betegnelse for bildesideforhold på 1,5:1 eller mer for en levende bilde-ressurs.</skos:definition>
      <rdakit:toolkitDefinition xml:lang="no">En betegnelse for bildesideforhold på 1,5:1 eller mer for en levende bilde-ressurs.</rdakit:toolkitDefinition>
      <skos:prefLabel xml:lang="da">wide screen</skos:prefLabel>
      <rdakit:toolkitLabel xml:lang="da">wide screen</rdakit:toolkitLabel>
      <skos:definition xml:lang="da">Billedformat for en levende billedressource på 1,5:1 eller større.</skos:definition>
      <rdakit:toolkitDefinition xml:lang="da">Billedformat for en levende billedressource på 1,5:1 eller større.</rdakit:toolkitDefinition>
      <skos:definition xml:lang="fi">Liikkuvan kuvan kuvasuhde, joka on 1.5:1 tai suurempi.</skos:definition>
      <rdakit:toolkitDefinition xml:lang="fi">Liikkuvan kuvan kuvasuhde, joka on 1.5:1 tai suurempi.</rdakit:toolkitDefinition>
    </skos:Concept>

<!-- Status properties used in this document  -->
    <skos:Concept rdf:about="http://metadataregistry.org/uri/RegStatus/1001">
        <skos:prefLabel xml:lang="en">Published</skos:prefLabel>
    </skos:Concept>

</rdf:RDF>
