<?xml version="1.0" encoding = "UTF-8"?>
<rdf:RDF
    xmlns:dc="http://purl.org/dc/elements/1.1/"
    xmlns:rdakit="http://metadataregistry.org/uri/profile/rdakit/"
    xmlns:rdf="http://www.w3.org/1999/02/22-rdf-syntax-ns#"
    xmlns:reg="http://metadataregistry.org/uri/profile/regap/"
    xmlns:owl="http://www.w3.org/2002/07/owl#"
    xmlns:skos="http://www.w3.org/2004/02/skos/core#">

<owl:Ontology rdf:about="http://rdaregistry.info/termList/bookFormat" />
<!-- Scheme: RDA Bibliographic Format -->
    <skos:ConceptScheme rdf:about="http://rdaregistry.info/termList/bookFormat">
        <dc:title>RDA Bibliographic Format</dc:title>
    </skos:ConceptScheme>

<!-- Concept: 128mo  -->
    <skos:Concept rdf:about="http://rdaregistry.info/termList/bookFormat/1014" xml:lang="en">
      <skos:inScheme rdf:resource="http://rdaregistry.info/termList/bookFormat"/>
      <reg:status rdf:resource="http://metadataregistry.org/uri/RegStatus/1001"/>
      <reg:identifier rdf:resource="http://metadataregistry.org/concepts/9509"/>
      <skos:prefLabel xml:lang="en">128mo</skos:prefLabel>
      <skos:altLabel xml:lang="en">one hundred twenty-eightmo</skos:altLabel>
      <rdakit:toolkitLabel xml:lang="en">128mo</rdakit:toolkitLabel>
      <skos:definition xml:lang="en">A bibliographic format consisting of one or more leaves that are 1/128 of the whole sheet.</skos:definition>
      <rdakit:toolkitDefinition xml:lang="en">A bibliographic format consisting of one or more leaves that are 1/128 of the whole sheet.</rdakit:toolkitDefinition>
      <skos:prefLabel xml:lang="ca">128º</skos:prefLabel>
      <skos:altLabel xml:lang="ca">cent vint-i-vuitau</skos:altLabel>
      <rdakit:toolkitLabel xml:lang="ca">128º</rdakit:toolkitLabel>
      <skos:definition xml:lang="ca">Format bibliogràfic que consisteix en un o més fulls que són 1/128 del full sencer.</skos:definition>
      <rdakit:toolkitDefinition xml:lang="ca">Format bibliogràfic que consisteix en un o més fulls que són 1/128 del full sencer.</rdakit:toolkitDefinition>
      <skos:prefLabel xml:lang="vi">128mo</skos:prefLabel>
      <skos:altLabel xml:lang="vi">khổ một trăm hai tám</skos:altLabel>
      <rdakit:toolkitLabel xml:lang="vi">128mo</rdakit:toolkitLabel>
      <skos:definition xml:lang="vi">Định dạng thư mục có chứa một hoặc nhiều hơn tờ in bằng 1/128 của toàn bộ tờ.</skos:definition>
      <rdakit:toolkitDefinition xml:lang="vi">Định dạng thư mục có chứa một hoặc nhiều hơn tờ in bằng 1/128 của toàn bộ tờ.</rdakit:toolkitDefinition>
      <skos:prefLabel xml:lang="de">128°</skos:prefLabel>
      <skos:altLabel xml:lang="de">Centesimovigesimo octavo</skos:altLabel>
      <rdakit:toolkitLabel xml:lang="de">128°</rdakit:toolkitLabel>
      <skos:definition xml:lang="de">Ein Buchformat, das aus einem oder mehreren Blättern besteht, das/die 1/128 des ganzen Bogens ist/sind.</skos:definition>
      <rdakit:toolkitDefinition xml:lang="de">Ein Buchformat, das aus einem oder mehreren Blättern besteht, das/die 1/128 des ganzen Bogens ist/sind.</rdakit:toolkitDefinition>
      <skos:prefLabel xml:lang="da">128o</skos:prefLabel>
      <rdakit:toolkitLabel xml:lang="da">128o</rdakit:toolkitLabel>
      <skos:definition xml:lang="da">Bibliografisk format, der består af et eller flere blade, der er 1/128 af et helt ark.</skos:definition>
      <rdakit:toolkitDefinition xml:lang="da">Bibliografisk format, der består af et eller flere blade, der er 1/128 af et helt ark.</rdakit:toolkitDefinition>
      <skos:prefLabel xml:lang="fi">128:o</skos:prefLabel>
      <rdakit:toolkitLabel xml:lang="fi">128:o</rdakit:toolkitLabel>
      <skos:definition xml:lang="fi">Kirjan formaatti muodostuu yhdestä tai useammasta lehdestä, jotka ovat kooltaan 1/128 painoarkista.</skos:definition>
      <rdakit:toolkitDefinition xml:lang="fi">Kirjan formaatti muodostuu yhdestä tai useammasta lehdestä, jotka ovat kooltaan 1/128 painoarkista.</rdakit:toolkitDefinition>
      <skos:prefLabel xml:lang="fr">128º</skos:prefLabel>
      <skos:altLabel xml:lang="fr">in-cent-vingt-huit</skos:altLabel>
      <rdakit:toolkitLabel xml:lang="fr">128º</rdakit:toolkitLabel>
      <skos:definition xml:lang="fr">Format bibliographique qui consiste en un ou plusieurs feuillets formant chacun 1/128 de la feuille complète.</skos:definition>
      <rdakit:toolkitDefinition xml:lang="fr">Format bibliographique qui consiste en un ou plusieurs feuillets formant chacun 1/128 de la feuille complète.</rdakit:toolkitDefinition>
      <skos:definition xml:lang="no">Et bokformat som består av ett eller flere blad som er 1/128 av et ark.</skos:definition>
      <rdakit:toolkitDefinition xml:lang="no">Et bokformat som består av ett eller flere blad som er 1/128 av et ark.</rdakit:toolkitDefinition>
    </skos:Concept>
<!-- Concept: 12mo  -->
    <skos:Concept rdf:about="http://rdaregistry.info/termList/bookFormat/1004" xml:lang="en">
      <skos:inScheme rdf:resource="http://rdaregistry.info/termList/bookFormat"/>
      <reg:status rdf:resource="http://metadataregistry.org/uri/RegStatus/1001"/>
      <reg:identifier rdf:resource="http://metadataregistry.org/concepts/853"/>
      <skos:prefLabel xml:lang="en">12mo</skos:prefLabel>
      <skos:definition xml:lang="en">A bibliographic format consisting of one or more leaves that are 1/12 of the whole sheet.</skos:definition>
      <skos:altLabel xml:lang="en">duodecimo</skos:altLabel>
      <skos:altLabel xml:lang="en">twelvemo</skos:altLabel>
      <skos:definition xml:lang="fr">Format bibliographique qui consiste en un ou plusieurs feuillets formant chacun 1/12 de la feuille complète.</skos:definition>
      <skos:altLabel xml:lang="fr">in-douze</skos:altLabel>
      <skos:prefLabel xml:lang="fr">12º</skos:prefLabel>
      <skos:definition xml:lang="de">Ein Buchformat, das aus einem oder mehreren Blättern besteht, das/die 1/12 des ganzen Bogens ist/sind.</skos:definition>
      <skos:altLabel xml:lang="de">Duodecimo</skos:altLabel>
      <skos:prefLabel xml:lang="de">12°</skos:prefLabel>
      <skos:altLabel xml:lang="es">doceavo</skos:altLabel>
      <skos:prefLabel xml:lang="es">12vo</skos:prefLabel>
      <skos:definition xml:lang="es">Un formato de libro que consiste en una o más hojas que son 1/12 del folio completo.</skos:definition>
      <rdakit:toolkitLabel xml:lang="en">12mo</rdakit:toolkitLabel>
      <rdakit:toolkitLabel xml:lang="fr">12º</rdakit:toolkitLabel>
      <rdakit:toolkitDefinition xml:lang="en">A bibliographic format consisting of one or more leaves that are 1/12 of the whole sheet.</rdakit:toolkitDefinition>
      <rdakit:toolkitDefinition xml:lang="fr">Format bibliographique qui consiste en un ou plusieurs feuillets formant chacun 1/12 de la feuille complète.</rdakit:toolkitDefinition>
      <rdakit:toolkitLabel xml:lang="de">12°</rdakit:toolkitLabel>
      <rdakit:toolkitDefinition xml:lang="de">Ein Buchformat, das aus einem oder mehreren Blättern besteht, das/die 1/12 des ganzen Bogens ist/sind.</rdakit:toolkitDefinition>
      <rdakit:toolkitLabel xml:lang="es">12vo</rdakit:toolkitLabel>
      <rdakit:toolkitDefinition xml:lang="es">Un formato de libro que consiste en una o más hojas que son 1/12 del folio completo.</rdakit:toolkitDefinition>
      <skos:prefLabel xml:lang="zh">12开</skos:prefLabel>
      <skos:altLabel xml:lang="zh">十二开</skos:altLabel>
      <rdakit:toolkitLabel xml:lang="zh">12开</rdakit:toolkitLabel>
      <skos:definition xml:lang="zh">图书的一种开本，由一叶或多叶全张纸的1/12组成。</skos:definition>
      <rdakit:toolkitDefinition xml:lang="zh">图书的一种开本，由一叶或多叶全张纸的1/12组成。</rdakit:toolkitDefinition>
      <skos:prefLabel xml:lang="nl">12mo</skos:prefLabel>
      <rdakit:toolkitLabel xml:lang="nl">12mo</rdakit:toolkitLabel>
      <skos:definition xml:lang="nl">Een boekformaat dat bestaat uit één of meer bladen die 1/12 van een heel vel zijn.</skos:definition>
      <rdakit:toolkitDefinition xml:lang="nl">Een boekformaat dat bestaat uit één of meer bladen die 1/12 van een heel vel zijn.</rdakit:toolkitDefinition>
      <skos:prefLabel xml:lang="it">in 12mo</skos:prefLabel>
      <rdakit:toolkitLabel xml:lang="it">in 12mo</rdakit:toolkitLabel>
      <skos:prefLabel xml:lang="fi">12:o</skos:prefLabel>
      <rdakit:toolkitLabel xml:lang="fi">12:o</rdakit:toolkitLabel>
      <skos:prefLabel xml:lang="ca">12º</skos:prefLabel>
      <skos:altLabel xml:lang="ca">dotzau</skos:altLabel>
      <rdakit:toolkitLabel xml:lang="ca">12º</rdakit:toolkitLabel>
      <skos:definition xml:lang="ca">Format bibliogràfic que consisteix en un o més fulls que són 1/12 del full sencer.</skos:definition>
      <rdakit:toolkitDefinition xml:lang="ca">Format bibliogràfic que consisteix en un o més fulls que són 1/12 del full sencer.</rdakit:toolkitDefinition>
      <skos:prefLabel xml:lang="vi">12mo</skos:prefLabel>
      <skos:altLabel xml:lang="vi">khổ nười hai</skos:altLabel>
      <rdakit:toolkitLabel xml:lang="vi">12mo</rdakit:toolkitLabel>
      <skos:definition xml:lang="vi">Định dạng thư mục có chứa một hoặc nhiều hơn tờ in bằng 1/12 của toàn bộ tờ.</skos:definition>
      <rdakit:toolkitDefinition xml:lang="vi">Định dạng thư mục có chứa một hoặc nhiều hơn tờ in bằng 1/12 của toàn bộ tờ.</rdakit:toolkitDefinition>
      <skos:altLabel xml:lang="de">Duodez</skos:altLabel>
      <skos:prefLabel xml:lang="da">12o</skos:prefLabel>
      <skos:altLabel xml:lang="da">duodesformat</skos:altLabel>
      <rdakit:toolkitLabel xml:lang="da">12o</rdakit:toolkitLabel>
      <skos:definition xml:lang="da">Bibliografisk format, der består af et eller flere blade, der er 1/12 af et helt ark.</skos:definition>
      <rdakit:toolkitDefinition xml:lang="da">Bibliografisk format, der består af et eller flere blade, der er 1/12 af et helt ark.</rdakit:toolkitDefinition>
      <skos:definition xml:lang="fi">Kirjan formaatti muodostuu yhdestä tai useammasta lehdestä, jotka ovat kooltaan 1/12 painoarkista.</skos:definition>
      <rdakit:toolkitDefinition xml:lang="fi">Kirjan formaatti muodostuu yhdestä tai useammasta lehdestä, jotka ovat kooltaan 1/12 painoarkista.</rdakit:toolkitDefinition>
      <skos:prefLabel xml:lang="no">duodesformat</skos:prefLabel>
      <rdakit:toolkitLabel xml:lang="no">duodesformat</rdakit:toolkitLabel>
      <skos:definition xml:lang="no">Et bokformat som består av ett eller flere blad som er 1/12 av et ark.</skos:definition>
      <rdakit:toolkitDefinition xml:lang="no">Et bokformat som består av ett eller flere blad som er 1/12 av et ark.</rdakit:toolkitDefinition>
    </skos:Concept>
<!-- Concept: 16mo  -->
    <skos:Concept rdf:about="http://rdaregistry.info/termList/bookFormat/1005" xml:lang="en">
      <skos:inScheme rdf:resource="http://rdaregistry.info/termList/bookFormat"/>
      <reg:status rdf:resource="http://metadataregistry.org/uri/RegStatus/1001"/>
      <reg:identifier rdf:resource="http://metadataregistry.org/concepts/854"/>
      <skos:prefLabel xml:lang="en">16mo</skos:prefLabel>
      <skos:definition xml:lang="en">A bibliographic format consisting of one or more leaves that are 1/16 of the whole sheet.</skos:definition>
      <skos:altLabel xml:lang="en">decimo-sexto</skos:altLabel>
      <skos:altLabel xml:lang="en">sexto-decimo</skos:altLabel>
      <skos:altLabel xml:lang="en">sixteenmo</skos:altLabel>
      <skos:definition xml:lang="fr">Format bibliographique qui consiste en un ou plusieurs feuillets formant chacun 1/16 de la feuille complète.</skos:definition>
      <skos:prefLabel xml:lang="fr">16º</skos:prefLabel>
      <skos:altLabel xml:lang="fr">in-seize</skos:altLabel>
      <skos:definition xml:lang="de">Ein Buchformat, das aus einem oder mehreren Blättern besteht, das/die 1/16 des ganzen Bogens ist/sind.</skos:definition>
      <skos:altLabel xml:lang="de">Sedecimo</skos:altLabel>
      <skos:prefLabel xml:lang="de">16°</skos:prefLabel>
      <skos:altLabel xml:lang="es">dieciseisavo</skos:altLabel>
      <skos:prefLabel xml:lang="es">16vo</skos:prefLabel>
      <skos:definition xml:lang="es">Un formato de libro que consiste en una o más hojas que son 1/16 del folio completo.</skos:definition>
      <rdakit:toolkitLabel xml:lang="en">16mo</rdakit:toolkitLabel>
      <rdakit:toolkitLabel xml:lang="fr">16º</rdakit:toolkitLabel>
      <rdakit:toolkitDefinition xml:lang="en">A bibliographic format consisting of one or more leaves that are 1/16 of the whole sheet.</rdakit:toolkitDefinition>
      <rdakit:toolkitDefinition xml:lang="fr">Format bibliographique qui consiste en un ou plusieurs feuillets formant chacun 1/16 de la feuille complète.</rdakit:toolkitDefinition>
      <rdakit:toolkitLabel xml:lang="de">16°</rdakit:toolkitLabel>
      <rdakit:toolkitDefinition xml:lang="de">Ein Buchformat, das aus einem oder mehreren Blättern besteht, das/die 1/16 des ganzen Bogens ist/sind.</rdakit:toolkitDefinition>
      <rdakit:toolkitLabel xml:lang="es">16vo</rdakit:toolkitLabel>
      <rdakit:toolkitDefinition xml:lang="es">Un formato de libro que consiste en una o más hojas que son 1/16 del folio completo.</rdakit:toolkitDefinition>
      <skos:prefLabel xml:lang="zh">16开</skos:prefLabel>
      <skos:altLabel xml:lang="zh">十六开</skos:altLabel>
      <rdakit:toolkitLabel xml:lang="zh">16开</rdakit:toolkitLabel>
      <skos:definition xml:lang="zh">图书的一种开本，由一叶或多叶全张纸的1/16组成。</skos:definition>
      <rdakit:toolkitDefinition xml:lang="zh">图书的一种开本，由一叶或多叶全张纸的1/16组成。</rdakit:toolkitDefinition>
      <skos:prefLabel xml:lang="nl">16mo</skos:prefLabel>
      <rdakit:toolkitLabel xml:lang="nl">16mo</rdakit:toolkitLabel>
      <skos:definition xml:lang="nl">Een boekformaat dat bestaat uit één of meer bladen die 1/16 van een heel vel zijn.</skos:definition>
      <rdakit:toolkitDefinition xml:lang="nl">Een boekformaat dat bestaat uit één of meer bladen die 1/16 van een heel vel zijn.</rdakit:toolkitDefinition>
      <skos:prefLabel xml:lang="it">in 16mo</skos:prefLabel>
      <rdakit:toolkitLabel xml:lang="it">in 16mo</rdakit:toolkitLabel>
      <skos:prefLabel xml:lang="fi">16:o</skos:prefLabel>
      <rdakit:toolkitLabel xml:lang="fi">16:o</rdakit:toolkitLabel>
      <skos:prefLabel xml:lang="ca">16º</skos:prefLabel>
      <skos:altLabel xml:lang="ca">setzau</skos:altLabel>
      <rdakit:toolkitLabel xml:lang="ca">16º</rdakit:toolkitLabel>
      <skos:definition xml:lang="ca">Format bibliogràfic que consisteix en un o més fulls que són 1/16 del full sencer.</skos:definition>
      <rdakit:toolkitDefinition xml:lang="ca">Format bibliogràfic que consisteix en un o més fulls que són 1/16 del full sencer.</rdakit:toolkitDefinition>
      <skos:prefLabel xml:lang="vi">16mo</skos:prefLabel>
      <skos:altLabel xml:lang="vi">khổ mười tám</skos:altLabel>
      <rdakit:toolkitLabel xml:lang="vi">16mo</rdakit:toolkitLabel>
      <skos:definition xml:lang="vi">Định dạng thư mục có chứa một hoặc nhiều hơn tờ in bằng 1/16 của toàn bộ tờ.</skos:definition>
      <rdakit:toolkitDefinition xml:lang="vi">Định dạng thư mục có chứa một hoặc nhiều hơn tờ in bằng 1/16 của toàn bộ tờ.</rdakit:toolkitDefinition>
      <skos:altLabel xml:lang="de">Sedez</skos:altLabel>
      <skos:altLabel xml:lang="de">Sextodecimo</skos:altLabel>
      <skos:altLabel xml:lang="de">Decimo sexto</skos:altLabel>
      <skos:prefLabel xml:lang="da">16o</skos:prefLabel>
      <rdakit:toolkitLabel xml:lang="da">16o</rdakit:toolkitLabel>
      <skos:definition xml:lang="da">Bibliografisk format, der består af et eller flere blade, der er 1/16 af et helt ark.</skos:definition>
      <rdakit:toolkitDefinition xml:lang="da">Bibliografisk format, der består af et eller flere blade, der er 1/16 af et helt ark.</rdakit:toolkitDefinition>
      <skos:definition xml:lang="fi">Kirjan formaatti muodostuu yhdestä tai useammasta lehdestä, jotka ovat kooltaan 1/16 painoarkista.</skos:definition>
      <rdakit:toolkitDefinition xml:lang="fi">Kirjan formaatti muodostuu yhdestä tai useammasta lehdestä, jotka ovat kooltaan 1/16 painoarkista.</rdakit:toolkitDefinition>
      <skos:prefLabel xml:lang="no">sedesformat</skos:prefLabel>
      <rdakit:toolkitLabel xml:lang="no">sedesformat</rdakit:toolkitLabel>
      <skos:definition xml:lang="no">Et bokformat som består av ett eller flere blad som er 1/16 av et ark.</skos:definition>
      <rdakit:toolkitDefinition xml:lang="no">Et bokformat som består av ett eller flere blad som er 1/16 av et ark.</rdakit:toolkitDefinition>
    </skos:Concept>
<!-- Concept: 18mo  -->
    <skos:Concept rdf:about="http://rdaregistry.info/termList/bookFormat/1010" xml:lang="en">
      <skos:inScheme rdf:resource="http://rdaregistry.info/termList/bookFormat"/>
      <reg:status rdf:resource="http://metadataregistry.org/uri/RegStatus/1001"/>
      <reg:identifier rdf:resource="http://metadataregistry.org/concepts/9505"/>
      <skos:prefLabel xml:lang="en">18mo</skos:prefLabel>
      <skos:altLabel xml:lang="en">eighteenmo</skos:altLabel>
      <rdakit:toolkitLabel xml:lang="en">18mo</rdakit:toolkitLabel>
      <skos:definition xml:lang="en">A bibliographic format consisting of one or more leaves that are 1/18 of the whole sheet.</skos:definition>
      <rdakit:toolkitDefinition xml:lang="en">A bibliographic format consisting of one or more leaves that are 1/18 of the whole sheet.</rdakit:toolkitDefinition>
      <skos:altLabel xml:lang="en">octodecimo</skos:altLabel>
      <skos:prefLabel xml:lang="ca">18º</skos:prefLabel>
      <skos:altLabel xml:lang="ca">divuitau</skos:altLabel>
      <rdakit:toolkitLabel xml:lang="ca">18º</rdakit:toolkitLabel>
      <skos:definition xml:lang="ca">Format bibliogràfic que consisteix en un o més fulls que són 1/18 del full sencer.</skos:definition>
      <rdakit:toolkitDefinition xml:lang="ca">Format bibliogràfic que consisteix en un o més fulls que són 1/18 del full sencer.</rdakit:toolkitDefinition>
      <skos:prefLabel xml:lang="vi">18mo</skos:prefLabel>
      <skos:altLabel xml:lang="vi">khổ mười tám</skos:altLabel>
      <rdakit:toolkitLabel xml:lang="vi">18mo</rdakit:toolkitLabel>
      <skos:definition xml:lang="vi">Định dạng thư mục có chứa một hoặc nhiều hơn tờ in bằng 1/18 của toàn bộ tờ.</skos:definition>
      <rdakit:toolkitDefinition xml:lang="vi">Định dạng thư mục có chứa một hoặc nhiều hơn tờ in bằng 1/18 của toàn bộ tờ.</rdakit:toolkitDefinition>
      <skos:prefLabel xml:lang="de">18°</skos:prefLabel>
      <skos:altLabel xml:lang="de">Decimo octavo</skos:altLabel>
      <rdakit:toolkitLabel xml:lang="de">18°</rdakit:toolkitLabel>
      <skos:definition xml:lang="de">Ein Buchformat, das aus einem oder mehreren Blättern besteht, das/die 1/18 des ganzen Bogens ist/sind.</skos:definition>
      <rdakit:toolkitDefinition xml:lang="de">Ein Buchformat, das aus einem oder mehreren Blättern besteht, das/die 1/18 des ganzen Bogens ist/sind.</rdakit:toolkitDefinition>
      <skos:altLabel xml:lang="de">Oktodez</skos:altLabel>
      <skos:altLabel xml:lang="de">Octodecimo</skos:altLabel>
      <skos:prefLabel xml:lang="da">18o</skos:prefLabel>
      <rdakit:toolkitLabel xml:lang="da">18o</rdakit:toolkitLabel>
      <skos:definition xml:lang="da">Bibliografisk format, der består af et eller flere blade, der er 1/18 af et helt ark.</skos:definition>
      <rdakit:toolkitDefinition xml:lang="da">Bibliografisk format, der består af et eller flere blade, der er 1/18 af et helt ark.</rdakit:toolkitDefinition>
      <skos:prefLabel xml:lang="fi">18:o</skos:prefLabel>
      <rdakit:toolkitLabel xml:lang="fi">18:o</rdakit:toolkitLabel>
      <skos:definition xml:lang="fi">Kirjan formaatti muodostuu yhdestä tai useammasta lehdestä, jotka ovat kooltaan 1/18 painoarkista.</skos:definition>
      <rdakit:toolkitDefinition xml:lang="fi">Kirjan formaatti muodostuu yhdestä tai useammasta lehdestä, jotka ovat kooltaan 1/18 painoarkista.</rdakit:toolkitDefinition>
      <skos:prefLabel xml:lang="fr">18º</skos:prefLabel>
      <skos:altLabel xml:lang="fr">in-dix-huit</skos:altLabel>
      <rdakit:toolkitLabel xml:lang="fr">18º</rdakit:toolkitLabel>
      <skos:definition xml:lang="fr">Format bibliographique qui consiste en un ou plusieurs feuillets formant chacun 1/18 de la feuille complète.</skos:definition>
      <rdakit:toolkitDefinition xml:lang="fr">Format bibliographique qui consiste en un ou plusieurs feuillets formant chacun 1/18 de la feuille complète.</rdakit:toolkitDefinition>
      <skos:definition xml:lang="no">Et bokformat som består av ett eller flere blad som er 1/18 av et ark.</skos:definition>
      <rdakit:toolkitDefinition xml:lang="no">Et bokformat som består av ett eller flere blad som er 1/18 av et ark.</rdakit:toolkitDefinition>
    </skos:Concept>
<!-- Concept: 24mo  -->
    <skos:Concept rdf:about="http://rdaregistry.info/termList/bookFormat/1006" xml:lang="en">
      <skos:inScheme rdf:resource="http://rdaregistry.info/termList/bookFormat"/>
      <reg:status rdf:resource="http://metadataregistry.org/uri/RegStatus/1001"/>
      <reg:identifier rdf:resource="http://metadataregistry.org/concepts/855"/>
      <skos:prefLabel xml:lang="en">24mo</skos:prefLabel>
      <skos:definition xml:lang="en">A bibliographic format consisting of one or more leaves that are 1/24 of the whole sheet.</skos:definition>
      <skos:altLabel xml:lang="en">vigesimo-quarto</skos:altLabel>
      <skos:altLabel xml:lang="en">twenty-fourmo</skos:altLabel>
      <skos:definition xml:lang="fr">Format bibliographique qui consiste en un ou plusieurs feuillets formant chacun 1/24 de la feuille complète.</skos:definition>
      <skos:altLabel xml:lang="fr">in-vingt-quatre</skos:altLabel>
      <skos:prefLabel xml:lang="fr">24º</skos:prefLabel>
      <skos:definition xml:lang="de">Ein Buchformat, das aus einem oder mehreren Blättern besteht, das/die 1/24 des ganzen Bogens ist/sind.</skos:definition>
      <skos:altLabel xml:lang="de">Vigesimo quarto</skos:altLabel>
      <skos:prefLabel xml:lang="de">24°</skos:prefLabel>
      <skos:altLabel xml:lang="en">vicesimo-­quarto</skos:altLabel>
      <skos:prefLabel xml:lang="es">24vo</skos:prefLabel>
      <skos:altLabel xml:lang="es">veinticuatroavo</skos:altLabel>
      <skos:definition xml:lang="es">Un formato de libro que consiste en una o más hojas que son 1/24 del folio completo.</skos:definition>
      <rdakit:toolkitLabel xml:lang="en">24mo</rdakit:toolkitLabel>
      <rdakit:toolkitLabel xml:lang="fr">24º</rdakit:toolkitLabel>
      <rdakit:toolkitDefinition xml:lang="en">A bibliographic format consisting of one or more leaves that are 1/24 of the whole sheet.</rdakit:toolkitDefinition>
      <rdakit:toolkitDefinition xml:lang="fr">Format bibliographique qui consiste en un ou plusieurs feuillets formant chacun 1/24 de la feuille complète.</rdakit:toolkitDefinition>
      <rdakit:toolkitLabel xml:lang="de">24°</rdakit:toolkitLabel>
      <rdakit:toolkitDefinition xml:lang="de">Ein Buchformat, das aus einem oder mehreren Blättern besteht, das/die 1/24 des ganzen Bogens ist/sind.</rdakit:toolkitDefinition>
      <rdakit:toolkitLabel xml:lang="es">24vo</rdakit:toolkitLabel>
      <rdakit:toolkitDefinition xml:lang="es">Un formato de libro que consiste en una o más hojas que son 1/24 del folio completo.</rdakit:toolkitDefinition>
      <skos:prefLabel xml:lang="zh">24开</skos:prefLabel>
      <skos:altLabel xml:lang="zh">二十四开</skos:altLabel>
      <rdakit:toolkitLabel xml:lang="zh">24开</rdakit:toolkitLabel>
      <skos:definition xml:lang="zh">图书的一种开本，由一叶或多叶全张纸的1/24组成。</skos:definition>
      <rdakit:toolkitDefinition xml:lang="zh">图书的一种开本，由一叶或多叶全张纸的1/24组成。</rdakit:toolkitDefinition>
      <skos:prefLabel xml:lang="nl">24mo</skos:prefLabel>
      <rdakit:toolkitLabel xml:lang="nl">24mo</rdakit:toolkitLabel>
      <skos:definition xml:lang="nl">Een boekformaat dat bestaat uit één of meer bladen die 1/24 van een heel vel zijn.</skos:definition>
      <rdakit:toolkitDefinition xml:lang="nl">Een boekformaat dat bestaat uit één of meer bladen die 1/24 van een heel vel zijn.</rdakit:toolkitDefinition>
      <skos:prefLabel xml:lang="it">in 24mo</skos:prefLabel>
      <rdakit:toolkitLabel xml:lang="it">in 24mo</rdakit:toolkitLabel>
      <skos:prefLabel xml:lang="fi">24:o</skos:prefLabel>
      <rdakit:toolkitLabel xml:lang="fi">24:o</rdakit:toolkitLabel>
      <skos:prefLabel xml:lang="ca">24º</skos:prefLabel>
      <skos:altLabel xml:lang="ca">vint-i-quatrau</skos:altLabel>
      <rdakit:toolkitLabel xml:lang="ca">24º</rdakit:toolkitLabel>
      <skos:definition xml:lang="ca">Format bibliogràfic que consisteix en un o més fulls que són 1/24 del full sencer.</skos:definition>
      <rdakit:toolkitDefinition xml:lang="ca">Format bibliogràfic que consisteix en un o més fulls que són 1/24 del full sencer.</rdakit:toolkitDefinition>
      <skos:prefLabel xml:lang="vi">24mo</skos:prefLabel>
      <skos:altLabel xml:lang="vi">khổ hai tư</skos:altLabel>
      <rdakit:toolkitLabel xml:lang="vi">24mo</rdakit:toolkitLabel>
      <skos:definition xml:lang="vi">Định dạng thư mục có chứa một hoặc nhiều hơn tờ in bằng 1/24 của toàn bộ tờ.</skos:definition>
      <rdakit:toolkitDefinition xml:lang="vi">Định dạng thư mục có chứa một hoặc nhiều hơn tờ in bằng 1/24 của toàn bộ tờ.</rdakit:toolkitDefinition>
      <skos:altLabel xml:lang="de">Vicesimo quarto</skos:altLabel>
      <skos:prefLabel xml:lang="da">24o</skos:prefLabel>
      <rdakit:toolkitLabel xml:lang="da">24o</rdakit:toolkitLabel>
      <skos:definition xml:lang="da">Bibliografisk format, der består af et eller flere blade, der er 1/24 af et helt ark.</skos:definition>
      <rdakit:toolkitDefinition xml:lang="da">Bibliografisk format, der består af et eller flere blade, der er 1/24 af et helt ark.</rdakit:toolkitDefinition>
      <skos:definition xml:lang="fi">Kirjan formaatti muodostuu yhdestä tai useammasta lehdestä, jotka ovat kooltaan 1/24 painoarkista.</skos:definition>
      <rdakit:toolkitDefinition xml:lang="fi">Kirjan formaatti muodostuu yhdestä tai useammasta lehdestä, jotka ovat kooltaan 1/24 painoarkista.</rdakit:toolkitDefinition>
      <skos:definition xml:lang="no">Et bokformat som består av ett eller flere blad som er 1/24 av et ark.</skos:definition>
      <rdakit:toolkitDefinition xml:lang="no">Et bokformat som består av ett eller flere blad som er 1/24 av et ark.</rdakit:toolkitDefinition>
    </skos:Concept>
<!-- Concept: 32mo  -->
    <skos:Concept rdf:about="http://rdaregistry.info/termList/bookFormat/1007" xml:lang="en">
      <skos:inScheme rdf:resource="http://rdaregistry.info/termList/bookFormat"/>
      <reg:status rdf:resource="http://metadataregistry.org/uri/RegStatus/1001"/>
      <reg:identifier rdf:resource="http://metadataregistry.org/concepts/856"/>
      <skos:prefLabel xml:lang="en">32mo</skos:prefLabel>
      <skos:definition xml:lang="en">A bibliographic format consisting of one or more leaves that are 1/32 of the whole sheet.</skos:definition>
      <skos:altLabel xml:lang="en">trigesimo-secundo</skos:altLabel>
      <skos:altLabel xml:lang="en">thirty-twomo</skos:altLabel>
      <skos:definition xml:lang="fr">Format bibliographique qui consiste en un ou plusieurs feuillets formant chacun 1/32 de la feuille complète.</skos:definition>
      <skos:altLabel xml:lang="fr">in-trente-deux</skos:altLabel>
      <skos:prefLabel xml:lang="fr">32º</skos:prefLabel>
      <skos:definition xml:lang="de">Ein Buchformat, das aus einem oder mehreren Blättern besteht, das/die 1/32 des ganzen Bogens ist/sind.</skos:definition>
      <skos:altLabel xml:lang="de">Trigesimo secundo</skos:altLabel>
      <skos:prefLabel xml:lang="de">32°</skos:prefLabel>
      <skos:altLabel xml:lang="en">tricesimo‐secundo</skos:altLabel>
      <skos:prefLabel xml:lang="es">32vo</skos:prefLabel>
      <skos:altLabel xml:lang="es">treintaidosavo</skos:altLabel>
      <skos:definition xml:lang="es">Un formato de libro que consiste en una o más hojas que son 1/32 del folio completo.</skos:definition>
      <rdakit:toolkitLabel xml:lang="en">32mo</rdakit:toolkitLabel>
      <rdakit:toolkitLabel xml:lang="fr">32º</rdakit:toolkitLabel>
      <rdakit:toolkitDefinition xml:lang="en">A bibliographic format consisting of one or more leaves that are 1/32 of the whole sheet.</rdakit:toolkitDefinition>
      <rdakit:toolkitDefinition xml:lang="fr">Format bibliographique qui consiste en un ou plusieurs feuillets formant chacun 1/32 de la feuille complète.</rdakit:toolkitDefinition>
      <rdakit:toolkitLabel xml:lang="de">32°</rdakit:toolkitLabel>
      <rdakit:toolkitDefinition xml:lang="de">Ein Buchformat, das aus einem oder mehreren Blättern besteht, das/die 1/32 des ganzen Bogens ist/sind.</rdakit:toolkitDefinition>
      <rdakit:toolkitLabel xml:lang="es">32vo</rdakit:toolkitLabel>
      <rdakit:toolkitDefinition xml:lang="es">Un formato de libro que consiste en una o más hojas que son 1/32 del folio completo.</rdakit:toolkitDefinition>
      <skos:prefLabel xml:lang="zh">32开</skos:prefLabel>
      <skos:altLabel xml:lang="zh">三十二开</skos:altLabel>
      <rdakit:toolkitLabel xml:lang="zh">32开</rdakit:toolkitLabel>
      <skos:definition xml:lang="zh">图书的一种开本，由一叶或多叶全张纸的1/32组成。</skos:definition>
      <rdakit:toolkitDefinition xml:lang="zh">图书的一种开本，由一叶或多叶全张纸的1/32组成。</rdakit:toolkitDefinition>
      <skos:prefLabel xml:lang="nl">32mo</skos:prefLabel>
      <rdakit:toolkitLabel xml:lang="nl">32mo</rdakit:toolkitLabel>
      <skos:definition xml:lang="nl">Een boekformaat dat bestaat uit één of meer bladen die 1/32 van een heel vel zijn.</skos:definition>
      <rdakit:toolkitDefinition xml:lang="nl">Een boekformaat dat bestaat uit één of meer bladen die 1/32 van een heel vel zijn.</rdakit:toolkitDefinition>
      <skos:prefLabel xml:lang="it">in 32mo</skos:prefLabel>
      <rdakit:toolkitLabel xml:lang="it">in 32mo</rdakit:toolkitLabel>
      <skos:prefLabel xml:lang="fi">32:o</skos:prefLabel>
      <rdakit:toolkitLabel xml:lang="fi">32:o</rdakit:toolkitLabel>
      <skos:prefLabel xml:lang="ca">32º</skos:prefLabel>
      <skos:altLabel xml:lang="ca">trenta-dosau</skos:altLabel>
      <rdakit:toolkitLabel xml:lang="ca">32º</rdakit:toolkitLabel>
      <skos:definition xml:lang="ca">Format bibliogràfic que consisteix en un o més fulls que són 1/32 del full sencer.</skos:definition>
      <rdakit:toolkitDefinition xml:lang="ca">Format bibliogràfic que consisteix en un o més fulls que són 1/32 del full sencer.</rdakit:toolkitDefinition>
      <skos:prefLabel xml:lang="vi">32mo</skos:prefLabel>
      <skos:altLabel xml:lang="vi">khổ ba hai</skos:altLabel>
      <rdakit:toolkitLabel xml:lang="vi">32mo</rdakit:toolkitLabel>
      <skos:definition xml:lang="vi">Định dạng thư mục có chứa một hoặc nhiều hơn tờ in bằng 1/32 của toàn bộ tờ.</skos:definition>
      <rdakit:toolkitDefinition xml:lang="vi">Định dạng thư mục có chứa một hoặc nhiều hơn tờ in bằng 1/32 của toàn bộ tờ.</rdakit:toolkitDefinition>
      <skos:altLabel xml:lang="de">Tricesimo secundo</skos:altLabel>
      <skos:altLabel xml:lang="de">Tregesimo secundo</skos:altLabel>
      <skos:prefLabel xml:lang="da">32o</skos:prefLabel>
      <rdakit:toolkitLabel xml:lang="da">32o</rdakit:toolkitLabel>
      <skos:definition xml:lang="da">Bibliografisk format, der består af et eller flere blade, der er 1/32 af et helt ark.</skos:definition>
      <rdakit:toolkitDefinition xml:lang="da">Bibliografisk format, der består af et eller flere blade, der er 1/32 af et helt ark.</rdakit:toolkitDefinition>
      <skos:definition xml:lang="fi">Kirjan formaatti muodostuu yhdestä tai useammasta lehdestä, jotka ovat kooltaan 1/32 painoarkista.</skos:definition>
      <rdakit:toolkitDefinition xml:lang="fi">Kirjan formaatti muodostuu yhdestä tai useammasta lehdestä, jotka ovat kooltaan 1/32 painoarkista.</rdakit:toolkitDefinition>
      <skos:definition xml:lang="no">Et bokformat som består av ett eller flere blad som er 1/32 av et ark.</skos:definition>
      <rdakit:toolkitDefinition xml:lang="no">Et bokformat som består av ett eller flere blad som er 1/32 av et ark.</rdakit:toolkitDefinition>
    </skos:Concept>
<!-- Concept: 36mo  -->
    <skos:Concept rdf:about="http://rdaregistry.info/termList/bookFormat/1011" xml:lang="en">
      <skos:inScheme rdf:resource="http://rdaregistry.info/termList/bookFormat"/>
      <reg:status rdf:resource="http://metadataregistry.org/uri/RegStatus/1001"/>
      <reg:identifier rdf:resource="http://metadataregistry.org/concepts/9506"/>
      <skos:prefLabel xml:lang="en">36mo</skos:prefLabel>
      <skos:altLabel xml:lang="en">thirty-sixmo</skos:altLabel>
      <rdakit:toolkitLabel xml:lang="en">36mo</rdakit:toolkitLabel>
      <skos:definition xml:lang="en">A bibliographic format consisting of one or more leaves that are 1/36 of the whole sheet.</skos:definition>
      <rdakit:toolkitDefinition xml:lang="en">A bibliographic format consisting of one or more leaves that are 1/36 of the whole sheet.</rdakit:toolkitDefinition>
      <skos:prefLabel xml:lang="ca">36º</skos:prefLabel>
      <skos:altLabel xml:lang="ca">trenta-sisau</skos:altLabel>
      <rdakit:toolkitLabel xml:lang="ca">36º</rdakit:toolkitLabel>
      <skos:definition xml:lang="ca">Format bibliogràfic que consisteix en un o més fulls que són 1/36 del full sencer.</skos:definition>
      <rdakit:toolkitDefinition xml:lang="ca">Format bibliogràfic que consisteix en un o més fulls que són 1/36 del full sencer.</rdakit:toolkitDefinition>
      <skos:prefLabel xml:lang="vi">36mo</skos:prefLabel>
      <skos:altLabel xml:lang="vi">khổ ba sáu</skos:altLabel>
      <rdakit:toolkitLabel xml:lang="vi">36mo</rdakit:toolkitLabel>
      <skos:definition xml:lang="vi">Định dạng thư mục có chứa một hoặc nhiều hơn tờ in bằng 1/36 của toàn bộ tờ.</skos:definition>
      <rdakit:toolkitDefinition xml:lang="vi">Định dạng thư mục có chứa một hoặc nhiều hơn tờ in bằng 1/36 của toàn bộ tờ.</rdakit:toolkitDefinition>
      <skos:prefLabel xml:lang="de">36°</skos:prefLabel>
      <skos:altLabel xml:lang="de">Trigesimo sexto</skos:altLabel>
      <rdakit:toolkitLabel xml:lang="de">36°</rdakit:toolkitLabel>
      <skos:definition xml:lang="de">Ein Buchformat, das aus einem oder mehreren Blättern besteht, das/die 1/36 des ganzen Bogens ist/sind.</skos:definition>
      <rdakit:toolkitDefinition xml:lang="de">Ein Buchformat, das aus einem oder mehreren Blättern besteht, das/die 1/36 des ganzen Bogens ist/sind.</rdakit:toolkitDefinition>
      <skos:prefLabel xml:lang="da">36o</skos:prefLabel>
      <rdakit:toolkitLabel xml:lang="da">36o</rdakit:toolkitLabel>
      <skos:definition xml:lang="da">Bibliografisk format, der består af et eller flere blade, der er 1/36 af et helt ark.</skos:definition>
      <rdakit:toolkitDefinition xml:lang="da">Bibliografisk format, der består af et eller flere blade, der er 1/36 af et helt ark.</rdakit:toolkitDefinition>
      <skos:prefLabel xml:lang="fi">36:o</skos:prefLabel>
      <rdakit:toolkitLabel xml:lang="fi">36:o</rdakit:toolkitLabel>
      <skos:definition xml:lang="fi">Kirjan formaatti muodostuu yhdestä tai useammasta lehdestä, jotka ovat kooltaan 1/36 painoarkista.</skos:definition>
      <rdakit:toolkitDefinition xml:lang="fi">Kirjan formaatti muodostuu yhdestä tai useammasta lehdestä, jotka ovat kooltaan 1/36 painoarkista.</rdakit:toolkitDefinition>
      <skos:prefLabel xml:lang="fr">36º</skos:prefLabel>
      <skos:altLabel xml:lang="fr">in-trente-six</skos:altLabel>
      <rdakit:toolkitLabel xml:lang="fr">36º</rdakit:toolkitLabel>
      <skos:definition xml:lang="fr">Format bibliographique qui consiste en un ou plusieurs feuillets formant chacun 1/36 de la feuille complète.</skos:definition>
      <rdakit:toolkitDefinition xml:lang="fr">Format bibliographique qui consiste en un ou plusieurs feuillets formant chacun 1/36 de la feuille complète.</rdakit:toolkitDefinition>
      <skos:definition xml:lang="no">Et bokformat som består av ett eller flere blad som er 1/36 av et ark.</skos:definition>
      <rdakit:toolkitDefinition xml:lang="no">Et bokformat som består av ett eller flere blad som er 1/36 av et ark.</rdakit:toolkitDefinition>
    </skos:Concept>
<!-- Concept: 48mo  -->
    <skos:Concept rdf:about="http://rdaregistry.info/termList/bookFormat/1008" xml:lang="en">
      <skos:inScheme rdf:resource="http://rdaregistry.info/termList/bookFormat"/>
      <reg:status rdf:resource="http://metadataregistry.org/uri/RegStatus/1001"/>
      <reg:identifier rdf:resource="http://metadataregistry.org/concepts/857"/>
      <skos:prefLabel xml:lang="en">48mo</skos:prefLabel>
      <skos:definition xml:lang="en">A bibliographic format consisting of one or more leaves that are 1/48 of the whole sheet.</skos:definition>
      <skos:altLabel xml:lang="en">forty-eightmo</skos:altLabel>
      <skos:definition xml:lang="fr">Format bibliographique qui consiste en un ou plusieurs feuillets formant chacun 1/48 de la feuille complète.</skos:definition>
      <skos:altLabel xml:lang="fr">in-quarante-huit</skos:altLabel>
      <skos:prefLabel xml:lang="fr">48º</skos:prefLabel>
      <skos:definition xml:lang="de">Ein Buchformat, das aus einem oder mehreren Blättern besteht, das/die 1/48 des ganzen Bogens ist/sind.</skos:definition>
      <skos:altLabel xml:lang="de">Quadragesimo octavo</skos:altLabel>
      <skos:prefLabel xml:lang="de">48°</skos:prefLabel>
      <skos:prefLabel xml:lang="es">48vo</skos:prefLabel>
      <skos:altLabel xml:lang="es">cuarentiochoavo</skos:altLabel>
      <skos:definition xml:lang="es">Un formato de libro que consiste en una o más hojas que son 1/48 del folio completo.</skos:definition>
      <rdakit:toolkitLabel xml:lang="en">48mo</rdakit:toolkitLabel>
      <rdakit:toolkitLabel xml:lang="fr">48º</rdakit:toolkitLabel>
      <rdakit:toolkitDefinition xml:lang="en">A bibliographic format consisting of one or more leaves that are 1/48 of the whole sheet.</rdakit:toolkitDefinition>
      <rdakit:toolkitDefinition xml:lang="fr">Format bibliographique qui consiste en un ou plusieurs feuillets formant chacun 1/48 de la feuille complète.</rdakit:toolkitDefinition>
      <rdakit:toolkitLabel xml:lang="de">48°</rdakit:toolkitLabel>
      <rdakit:toolkitDefinition xml:lang="de">Ein Buchformat, das aus einem oder mehreren Blättern besteht, das/die 1/48 des ganzen Bogens ist/sind.</rdakit:toolkitDefinition>
      <rdakit:toolkitLabel xml:lang="es">48vo</rdakit:toolkitLabel>
      <rdakit:toolkitDefinition xml:lang="es">Un formato de libro que consiste en una o más hojas que son 1/48 del folio completo.</rdakit:toolkitDefinition>
      <skos:prefLabel xml:lang="zh">48开</skos:prefLabel>
      <skos:altLabel xml:lang="zh">四十八开</skos:altLabel>
      <rdakit:toolkitLabel xml:lang="zh">48开</rdakit:toolkitLabel>
      <skos:definition xml:lang="zh">图书的一种开本，由一叶或多叶全张纸的1/48组成。</skos:definition>
      <rdakit:toolkitDefinition xml:lang="zh">图书的一种开本，由一叶或多叶全张纸的1/48组成。</rdakit:toolkitDefinition>
      <skos:prefLabel xml:lang="nl">48mo</skos:prefLabel>
      <rdakit:toolkitLabel xml:lang="nl">48mo</rdakit:toolkitLabel>
      <skos:definition xml:lang="nl">Een boekformaat dat bestaat uit één of meer bladen die 1/48 van een heel vel zijn.</skos:definition>
      <rdakit:toolkitDefinition xml:lang="nl">Een boekformaat dat bestaat uit één of meer bladen die 1/48 van een heel vel zijn.</rdakit:toolkitDefinition>
      <skos:prefLabel xml:lang="it">in 48mo</skos:prefLabel>
      <rdakit:toolkitLabel xml:lang="it">in 48mo</rdakit:toolkitLabel>
      <skos:prefLabel xml:lang="fi">48:o</skos:prefLabel>
      <rdakit:toolkitLabel xml:lang="fi">48:o</rdakit:toolkitLabel>
      <skos:prefLabel xml:lang="ca">48º</skos:prefLabel>
      <skos:altLabel xml:lang="ca">quaranta-vuitau</skos:altLabel>
      <rdakit:toolkitLabel xml:lang="ca">48º</rdakit:toolkitLabel>
      <skos:definition xml:lang="ca">Format bibliogràfic que consisteix en un o més fulls que són 1/48 del full sencer.</skos:definition>
      <rdakit:toolkitDefinition xml:lang="ca">Format bibliogràfic que consisteix en un o més fulls que són 1/48 del full sencer.</rdakit:toolkitDefinition>
      <skos:prefLabel xml:lang="vi">48mo</skos:prefLabel>
      <skos:altLabel xml:lang="vi">khổ bốn tám</skos:altLabel>
      <rdakit:toolkitLabel xml:lang="vi">48mo</rdakit:toolkitLabel>
      <skos:definition xml:lang="vi">Định dạng thư mục có chứa một hoặc nhiều hơn tờ in bằng 1/48 của toàn bộ tờ.</skos:definition>
      <rdakit:toolkitDefinition xml:lang="vi">Định dạng thư mục có chứa một hoặc nhiều hơn tờ in bằng 1/48 của toàn bộ tờ.</rdakit:toolkitDefinition>
      <skos:prefLabel xml:lang="da">48o</skos:prefLabel>
      <rdakit:toolkitLabel xml:lang="da">48o</rdakit:toolkitLabel>
      <skos:definition xml:lang="da">Bibliografisk format, der består af et eller flere blade, der er 1/48 af et helt ark.</skos:definition>
      <rdakit:toolkitDefinition xml:lang="da">Bibliografisk format, der består af et eller flere blade, der er 1/48 af et helt ark.</rdakit:toolkitDefinition>
      <skos:definition xml:lang="fi">Kirjan formaatti muodostuu yhdestä tai useammasta lehdestä, jotka ovat kooltaan 1/48 painoarkista.</skos:definition>
      <rdakit:toolkitDefinition xml:lang="fi">Kirjan formaatti muodostuu yhdestä tai useammasta lehdestä, jotka ovat kooltaan 1/48 painoarkista.</rdakit:toolkitDefinition>
      <skos:definition xml:lang="no">Et bokformat som består av ett eller flere blad som er 1/48 av et ark.</skos:definition>
      <rdakit:toolkitDefinition xml:lang="no">Et bokformat som består av ett eller flere blad som er 1/48 av et ark.</rdakit:toolkitDefinition>
    </skos:Concept>
<!-- Concept: 4to  -->
    <skos:Concept rdf:about="http://rdaregistry.info/termList/bookFormat/1002" xml:lang="en">
      <skos:inScheme rdf:resource="http://rdaregistry.info/termList/bookFormat"/>
      <reg:status rdf:resource="http://metadataregistry.org/uri/RegStatus/1001"/>
      <reg:identifier rdf:resource="http://metadataregistry.org/concepts/851"/>
      <skos:prefLabel xml:lang="en">4to</skos:prefLabel>
      <skos:definition xml:lang="en">A bibliographic format consisting of one or more leaves that are 1/4 of the whole sheet.</skos:definition>
      <skos:altLabel xml:lang="en">quarto</skos:altLabel>
      <skos:definition xml:lang="fr">Format bibliographique qui consiste en un ou plusieurs feuillets formant chacun 1/4 de la feuille complète.</skos:definition>
      <skos:altLabel xml:lang="fr">in-quarto</skos:altLabel>
      <skos:prefLabel xml:lang="fr">4º</skos:prefLabel>
      <skos:definition xml:lang="de">Ein Buchformat, das aus einem oder mehreren Blättern besteht, das/die 1/4 des ganzen Bogens ist/sind.</skos:definition>
      <skos:altLabel xml:lang="de">Quart</skos:altLabel>
      <skos:prefLabel xml:lang="de">4°</skos:prefLabel>
      <skos:prefLabel xml:lang="es">4to</skos:prefLabel>
      <skos:altLabel xml:lang="es">cuarto</skos:altLabel>
      <skos:definition xml:lang="es">Un formato de libro que consiste en una o más hojas que son 1/4 del folio completo.</skos:definition>
      <rdakit:toolkitLabel xml:lang="en">4to</rdakit:toolkitLabel>
      <rdakit:toolkitLabel xml:lang="fr">4º</rdakit:toolkitLabel>
      <rdakit:toolkitDefinition xml:lang="en">A bibliographic format consisting of one or more leaves that are 1/4 of the whole sheet.</rdakit:toolkitDefinition>
      <rdakit:toolkitDefinition xml:lang="fr">Format bibliographique qui consiste en un ou plusieurs feuillets formant chacun 1/4 de la feuille complète.</rdakit:toolkitDefinition>
      <rdakit:toolkitLabel xml:lang="de">4°</rdakit:toolkitLabel>
      <rdakit:toolkitDefinition xml:lang="de">Ein Buchformat, das aus einem oder mehreren Blättern besteht, das/die 1/4 des ganzen Bogens ist/sind.</rdakit:toolkitDefinition>
      <rdakit:toolkitLabel xml:lang="es">4to</rdakit:toolkitLabel>
      <rdakit:toolkitDefinition xml:lang="es">Un formato de libro que consiste en una o más hojas que son 1/4 del folio completo.</rdakit:toolkitDefinition>
      <skos:prefLabel xml:lang="zh">4开</skos:prefLabel>
      <skos:altLabel xml:lang="zh">四开</skos:altLabel>
      <rdakit:toolkitLabel xml:lang="zh">4开</rdakit:toolkitLabel>
      <skos:definition xml:lang="zh">图书的一种开本，由一叶或多叶全张纸的1/4组成。</skos:definition>
      <rdakit:toolkitDefinition xml:lang="zh">图书的一种开本，由一叶或多叶全张纸的1/4组成。</rdakit:toolkitDefinition>
      <skos:prefLabel xml:lang="nl">4to</skos:prefLabel>
      <rdakit:toolkitLabel xml:lang="nl">4to</rdakit:toolkitLabel>
      <skos:definition xml:lang="nl">Een boekformaat dat bestaat uit één of meer bladen die 1/4 van een heel vel zijn.</skos:definition>
      <rdakit:toolkitDefinition xml:lang="nl">Een boekformaat dat bestaat uit één of meer bladen die 1/4 van een heel vel zijn.</rdakit:toolkitDefinition>
      <skos:prefLabel xml:lang="it">in 4to</skos:prefLabel>
      <rdakit:toolkitLabel xml:lang="it">in 4to</rdakit:toolkitLabel>
      <skos:prefLabel xml:lang="fi">4:o</skos:prefLabel>
      <rdakit:toolkitLabel xml:lang="fi">4:o</rdakit:toolkitLabel>
      <skos:prefLabel xml:lang="ca">4º</skos:prefLabel>
      <skos:altLabel xml:lang="ca">quart</skos:altLabel>
      <rdakit:toolkitLabel xml:lang="ca">4º</rdakit:toolkitLabel>
      <skos:definition xml:lang="ca">Format bibliogràfic que consisteix en un o més fulls que són 1/4 del full sencer.</skos:definition>
      <rdakit:toolkitDefinition xml:lang="ca">Format bibliogràfic que consisteix en un o més fulls que són 1/4 del full sencer.</rdakit:toolkitDefinition>
      <skos:prefLabel xml:lang="vi">4to</skos:prefLabel>
      <skos:altLabel xml:lang="vi">khổ bốn</skos:altLabel>
      <rdakit:toolkitLabel xml:lang="vi">4to</rdakit:toolkitLabel>
      <skos:definition xml:lang="vi">Định dạng thư mục có chứa một hoặc nhiều hơn tờ in bằng 1/4 của toàn bộ tờ.</skos:definition>
      <rdakit:toolkitDefinition xml:lang="vi">Định dạng thư mục có chứa một hoặc nhiều hơn tờ in bằng 1/4 của toàn bộ tờ.</rdakit:toolkitDefinition>
      <skos:prefLabel xml:lang="da">4o</skos:prefLabel>
      <skos:altLabel xml:lang="da">kvartformat</skos:altLabel>
      <rdakit:toolkitLabel xml:lang="da">4o</rdakit:toolkitLabel>
      <skos:definition xml:lang="da">Bibliografisk format, der består af et eller flere blade, der er 1/4 af et helt ark.</skos:definition>
      <rdakit:toolkitDefinition xml:lang="da">Bibliografisk format, der består af et eller flere blade, der er 1/4 af et helt ark.</rdakit:toolkitDefinition>
      <skos:definition xml:lang="fi">Kirjan formaatti muodostuu yhdestä tai useammasta lehdestä, jotka ovat kooltaan 1/4 painoarkista.</skos:definition>
      <rdakit:toolkitDefinition xml:lang="fi">Kirjan formaatti muodostuu yhdestä tai useammasta lehdestä, jotka ovat kooltaan 1/4 painoarkista.</rdakit:toolkitDefinition>
      <skos:prefLabel xml:lang="no">kvartformat</skos:prefLabel>
      <rdakit:toolkitLabel xml:lang="no">kvartformat</rdakit:toolkitLabel>
      <skos:definition xml:lang="no">Et bokformat som består av ett eller flere blad som er 1/4 av et ark.</skos:definition>
      <rdakit:toolkitDefinition xml:lang="no">Et bokformat som består av ett eller flere blad som er 1/4 av et ark.</rdakit:toolkitDefinition>
    </skos:Concept>
<!-- Concept: 64mo  -->
    <skos:Concept rdf:about="http://rdaregistry.info/termList/bookFormat/1009" xml:lang="en">
      <skos:inScheme rdf:resource="http://rdaregistry.info/termList/bookFormat"/>
      <reg:status rdf:resource="http://metadataregistry.org/uri/RegStatus/1001"/>
      <reg:identifier rdf:resource="http://metadataregistry.org/concepts/858"/>
      <skos:prefLabel xml:lang="en">64mo</skos:prefLabel>
      <skos:definition xml:lang="en">A bibliographic format consisting of one or more leaves that are 1/64 of the whole sheet.</skos:definition>
      <skos:altLabel xml:lang="en">sixty-fourmo</skos:altLabel>
      <skos:prefLabel xml:lang="fr">64º</skos:prefLabel>
      <skos:definition xml:lang="fr">Format bibliographique qui consiste en un ou plusieurs feuillets formant chacun 1/64 de la feuille complète.</skos:definition>
      <skos:altLabel xml:lang="fr">in-soixante-quatre</skos:altLabel>
      <skos:definition xml:lang="de">Ein Buchformat, das aus einem oder mehreren Blättern besteht, das/die 1/64 des ganzen Bogens ist/sind.</skos:definition>
      <skos:altLabel xml:lang="de">Sexagesimo quarto</skos:altLabel>
      <skos:prefLabel xml:lang="de">64°</skos:prefLabel>
      <skos:prefLabel xml:lang="es">64vo</skos:prefLabel>
      <skos:altLabel xml:lang="es">sesentaicuatroavo</skos:altLabel>
      <skos:definition xml:lang="es">Un formato de libro que consiste en una o más hojas que son 1/64 del folio completo.</skos:definition>
      <rdakit:toolkitLabel xml:lang="en">64mo</rdakit:toolkitLabel>
      <rdakit:toolkitLabel xml:lang="fr">64º</rdakit:toolkitLabel>
      <rdakit:toolkitDefinition xml:lang="en">A bibliographic format consisting of one or more leaves that are 1/64 of the whole sheet.</rdakit:toolkitDefinition>
      <rdakit:toolkitDefinition xml:lang="fr">Format bibliographique qui consiste en un ou plusieurs feuillets formant chacun 1/64 de la feuille complète.</rdakit:toolkitDefinition>
      <rdakit:toolkitLabel xml:lang="de">64°</rdakit:toolkitLabel>
      <rdakit:toolkitDefinition xml:lang="de">Ein Buchformat, das aus einem oder mehreren Blättern besteht, das/die 1/64 des ganzen Bogens ist/sind.</rdakit:toolkitDefinition>
      <rdakit:toolkitLabel xml:lang="es">64vo</rdakit:toolkitLabel>
      <rdakit:toolkitDefinition xml:lang="es">Un formato de libro que consiste en una o más hojas que son 1/64 del folio completo.</rdakit:toolkitDefinition>
      <skos:prefLabel xml:lang="zh">64开</skos:prefLabel>
      <skos:altLabel xml:lang="zh">六十四开</skos:altLabel>
      <rdakit:toolkitLabel xml:lang="zh">64开</rdakit:toolkitLabel>
      <skos:definition xml:lang="zh">图书的一种开本，由一叶或多叶全张纸的1/64组成。</skos:definition>
      <rdakit:toolkitDefinition xml:lang="zh">图书的一种开本，由一叶或多叶全张纸的1/64组成。</rdakit:toolkitDefinition>
      <skos:prefLabel xml:lang="nl">64mo</skos:prefLabel>
      <rdakit:toolkitLabel xml:lang="nl">64mo</rdakit:toolkitLabel>
      <skos:definition xml:lang="nl">Een boekformaat dat bestaat uit één of meer bladen die 1/64 van een heel vel zijn.</skos:definition>
      <rdakit:toolkitDefinition xml:lang="nl">Een boekformaat dat bestaat uit één of meer bladen die 1/64 van een heel vel zijn.</rdakit:toolkitDefinition>
      <skos:prefLabel xml:lang="it">in 64mo</skos:prefLabel>
      <rdakit:toolkitLabel xml:lang="it">in 64mo</rdakit:toolkitLabel>
      <skos:prefLabel xml:lang="fi">64:o</skos:prefLabel>
      <rdakit:toolkitLabel xml:lang="fi">64:o</rdakit:toolkitLabel>
      <skos:prefLabel xml:lang="ca">64º</skos:prefLabel>
      <skos:altLabel xml:lang="ca">seixanta-quatrau</skos:altLabel>
      <rdakit:toolkitLabel xml:lang="ca">64º</rdakit:toolkitLabel>
      <skos:definition xml:lang="ca">Format bibliogràfic que consisteix en un o més fulls que són 1/64 del full sencer.</skos:definition>
      <rdakit:toolkitDefinition xml:lang="ca">Format bibliogràfic que consisteix en un o més fulls que són 1/64 del full sencer.</rdakit:toolkitDefinition>
      <skos:prefLabel xml:lang="vi">64mo</skos:prefLabel>
      <skos:altLabel xml:lang="vi">khổ sái tư</skos:altLabel>
      <rdakit:toolkitLabel xml:lang="vi">64mo</rdakit:toolkitLabel>
      <skos:definition xml:lang="vi">Định dạng thư mục có chứa một hoặc nhiều hơn tờ in bằng 1/64 của toàn bộ tờ.</skos:definition>
      <rdakit:toolkitDefinition xml:lang="vi">Định dạng thư mục có chứa một hoặc nhiều hơn tờ in bằng 1/64 của toàn bộ tờ.</rdakit:toolkitDefinition>
      <skos:prefLabel xml:lang="da">64o</skos:prefLabel>
      <rdakit:toolkitLabel xml:lang="da">64o</rdakit:toolkitLabel>
      <skos:definition xml:lang="da">Bibliografisk format, der består af et eller flere blade, der er 1/64 af et helt ark.</skos:definition>
      <rdakit:toolkitDefinition xml:lang="da">Bibliografisk format, der består af et eller flere blade, der er 1/64 af et helt ark.</rdakit:toolkitDefinition>
      <skos:definition xml:lang="fi">Kirjan formaatti muodostuu yhdestä tai useammasta lehdestä, jotka ovat kooltaan 1/64 painoarkista.</skos:definition>
      <rdakit:toolkitDefinition xml:lang="fi">Kirjan formaatti muodostuu yhdestä tai useammasta lehdestä, jotka ovat kooltaan 1/64 painoarkista.</rdakit:toolkitDefinition>
      <skos:definition xml:lang="no">Et bokformat som består av ett eller flere blad som er 1/64 av et ark.</skos:definition>
      <rdakit:toolkitDefinition xml:lang="no">Et bokformat som består av ett eller flere blad som er 1/64 av et ark.</rdakit:toolkitDefinition>
    </skos:Concept>
<!-- Concept: 72mo  -->
    <skos:Concept rdf:about="http://rdaregistry.info/termList/bookFormat/1012" xml:lang="en">
      <skos:inScheme rdf:resource="http://rdaregistry.info/termList/bookFormat"/>
      <reg:status rdf:resource="http://metadataregistry.org/uri/RegStatus/1001"/>
      <reg:identifier rdf:resource="http://metadataregistry.org/concepts/9507"/>
      <skos:prefLabel xml:lang="en">72mo</skos:prefLabel>
      <skos:altLabel xml:lang="en">seventy-twomo</skos:altLabel>
      <rdakit:toolkitLabel xml:lang="en">72mo</rdakit:toolkitLabel>
      <skos:definition xml:lang="en">A bibliographic format consisting of one or more leaves that are 1/72 of the whole sheet.</skos:definition>
      <rdakit:toolkitDefinition xml:lang="en">A bibliographic format consisting of one or more leaves that are 1/72 of the whole sheet.</rdakit:toolkitDefinition>
      <skos:prefLabel xml:lang="ca">72º</skos:prefLabel>
      <skos:altLabel xml:lang="ca">setanta-dosau</skos:altLabel>
      <rdakit:toolkitLabel xml:lang="ca">72º</rdakit:toolkitLabel>
      <skos:definition xml:lang="ca">Format bibliogràfic que consisteix en un o més fulls que són 1/72 del full sencer.</skos:definition>
      <rdakit:toolkitDefinition xml:lang="ca">Format bibliogràfic que consisteix en un o més fulls que són 1/72 del full sencer.</rdakit:toolkitDefinition>
      <skos:prefLabel xml:lang="vi">72mo</skos:prefLabel>
      <skos:altLabel xml:lang="vi">khổ bảy hai</skos:altLabel>
      <rdakit:toolkitLabel xml:lang="vi">72mo</rdakit:toolkitLabel>
      <skos:definition xml:lang="vi">Định dạng thư mục có chứa một hoặc nhiều hơn tờ in bằng 1/72 của toàn bộ tờ.</skos:definition>
      <rdakit:toolkitDefinition xml:lang="vi">Định dạng thư mục có chứa một hoặc nhiều hơn tờ in bằng 1/72 của toàn bộ tờ.</rdakit:toolkitDefinition>
      <skos:prefLabel xml:lang="de">72°</skos:prefLabel>
      <skos:altLabel xml:lang="de">Septuagesimo secundo</skos:altLabel>
      <rdakit:toolkitLabel xml:lang="de">72°</rdakit:toolkitLabel>
      <skos:definition xml:lang="de">Ein Buchformat, das aus einem oder mehreren Blättern besteht, das/die 1/72 des ganzen Bogens ist/sind.</skos:definition>
      <rdakit:toolkitDefinition xml:lang="de">Ein Buchformat, das aus einem oder mehreren Blättern besteht, das/die 1/72 des ganzen Bogens ist/sind.</rdakit:toolkitDefinition>
      <skos:prefLabel xml:lang="da">72o</skos:prefLabel>
      <rdakit:toolkitLabel xml:lang="da">72o</rdakit:toolkitLabel>
      <skos:definition xml:lang="da">Bibliografisk format, der består af et eller flere blade, der er 1/72 af et helt ark.</skos:definition>
      <rdakit:toolkitDefinition xml:lang="da">Bibliografisk format, der består af et eller flere blade, der er 1/72 af et helt ark.</rdakit:toolkitDefinition>
      <skos:prefLabel xml:lang="fi">72:o</skos:prefLabel>
      <rdakit:toolkitLabel xml:lang="fi">72:o</rdakit:toolkitLabel>
      <skos:definition xml:lang="fi">Kirjan formaatti muodostuu yhdestä tai useammasta lehdestä, jotka ovat kooltaan 1/72 painoarkista.</skos:definition>
      <rdakit:toolkitDefinition xml:lang="fi">Kirjan formaatti muodostuu yhdestä tai useammasta lehdestä, jotka ovat kooltaan 1/72 painoarkista.</rdakit:toolkitDefinition>
      <skos:prefLabel xml:lang="fr">72º</skos:prefLabel>
      <skos:altLabel xml:lang="fr">in-soixante-douze</skos:altLabel>
      <rdakit:toolkitLabel xml:lang="fr">72º</rdakit:toolkitLabel>
      <skos:definition xml:lang="fr">Format bibliographique qui consiste en un ou plusieurs feuillets formant chacun 1/72 de la feuille complète.</skos:definition>
      <rdakit:toolkitDefinition xml:lang="fr">Format bibliographique qui consiste en un ou plusieurs feuillets formant chacun 1/72 de la feuille complète.</rdakit:toolkitDefinition>
      <skos:definition xml:lang="no">Et bokformat som består av ett eller flere blad som er 1/72 av et ark.</skos:definition>
      <rdakit:toolkitDefinition xml:lang="no">Et bokformat som består av ett eller flere blad som er 1/72 av et ark.</rdakit:toolkitDefinition>
    </skos:Concept>
<!-- Concept: 8vo  -->
    <skos:Concept rdf:about="http://rdaregistry.info/termList/bookFormat/1003" xml:lang="en">
      <skos:inScheme rdf:resource="http://rdaregistry.info/termList/bookFormat"/>
      <reg:status rdf:resource="http://metadataregistry.org/uri/RegStatus/1001"/>
      <reg:identifier rdf:resource="http://metadataregistry.org/concepts/852"/>
      <skos:prefLabel xml:lang="en">8vo</skos:prefLabel>
      <skos:definition xml:lang="en">A bibliographic format consisting of one or more leaves that are 1/8 of the whole sheet.</skos:definition>
      <skos:altLabel xml:lang="en">octavo</skos:altLabel>
      <skos:definition xml:lang="fr">Format bibliographique qui consiste en un ou plusieurs feuillets formant chacun 1/8 de la feuille complète.</skos:definition>
      <skos:altLabel xml:lang="fr">in-octavo</skos:altLabel>
      <skos:prefLabel xml:lang="fr">8º</skos:prefLabel>
      <skos:definition xml:lang="de">Ein Buchformat, das aus einem oder mehreren Blättern besteht, das/die 1/8 des ganzen Bogens ist/sind.</skos:definition>
      <skos:altLabel xml:lang="de">Octavo</skos:altLabel>
      <skos:prefLabel xml:lang="de">8°</skos:prefLabel>
      <skos:prefLabel xml:lang="es">8vo</skos:prefLabel>
      <skos:altLabel xml:lang="es">octavo</skos:altLabel>
      <skos:definition xml:lang="es">Un formato de libro que consiste en una o más hojas que son 1/8 del folio completo.</skos:definition>
      <rdakit:toolkitLabel xml:lang="en">8vo</rdakit:toolkitLabel>
      <rdakit:toolkitLabel xml:lang="fr">8º</rdakit:toolkitLabel>
      <rdakit:toolkitDefinition xml:lang="en">A bibliographic format consisting of one or more leaves that are 1/8 of the whole sheet.</rdakit:toolkitDefinition>
      <rdakit:toolkitDefinition xml:lang="fr">Format bibliographique qui consiste en un ou plusieurs feuillets formant chacun 1/8 de la feuille complète.</rdakit:toolkitDefinition>
      <rdakit:toolkitLabel xml:lang="de">8°</rdakit:toolkitLabel>
      <rdakit:toolkitDefinition xml:lang="de">Ein Buchformat, das aus einem oder mehreren Blättern besteht, das/die 1/8 des ganzen Bogens ist/sind.</rdakit:toolkitDefinition>
      <rdakit:toolkitLabel xml:lang="es">8vo</rdakit:toolkitLabel>
      <rdakit:toolkitDefinition xml:lang="es">Un formato de libro que consiste en una o más hojas que son 1/8 del folio completo.</rdakit:toolkitDefinition>
      <skos:prefLabel xml:lang="zh">8开</skos:prefLabel>
      <skos:altLabel xml:lang="zh">八开</skos:altLabel>
      <rdakit:toolkitLabel xml:lang="zh">8开</rdakit:toolkitLabel>
      <skos:definition xml:lang="zh">图书的一种开本，由一叶或多叶全张纸的1/8组成。</skos:definition>
      <rdakit:toolkitDefinition xml:lang="zh">图书的一种开本，由一叶或多叶全张纸的1/8组成。</rdakit:toolkitDefinition>
      <skos:prefLabel xml:lang="nl">8vo</skos:prefLabel>
      <rdakit:toolkitLabel xml:lang="nl">8vo</rdakit:toolkitLabel>
      <skos:definition xml:lang="nl">Een boekformaat dat bestaat uit één of meer bladen die 1/8 van een heel vel zijn.</skos:definition>
      <rdakit:toolkitDefinition xml:lang="nl">Een boekformaat dat bestaat uit één of meer bladen die 1/8 van een heel vel zijn.</rdakit:toolkitDefinition>
      <skos:prefLabel xml:lang="it">in 8vo</skos:prefLabel>
      <rdakit:toolkitLabel xml:lang="it">in 8vo</rdakit:toolkitLabel>
      <skos:prefLabel xml:lang="fi">8:o</skos:prefLabel>
      <rdakit:toolkitLabel xml:lang="fi">8:o</rdakit:toolkitLabel>
      <skos:prefLabel xml:lang="ca">8º</skos:prefLabel>
      <skos:altLabel xml:lang="ca">octau</skos:altLabel>
      <rdakit:toolkitLabel xml:lang="ca">8º</rdakit:toolkitLabel>
      <skos:definition xml:lang="ca">Format bibliogràfic que consisteix en un o més fulls que són 1/8 del full sencer.</skos:definition>
      <rdakit:toolkitDefinition xml:lang="ca">Format bibliogràfic que consisteix en un o més fulls que són 1/8 del full sencer.</rdakit:toolkitDefinition>
      <skos:prefLabel xml:lang="vi">8vo</skos:prefLabel>
      <skos:altLabel xml:lang="vi">khổ tám</skos:altLabel>
      <rdakit:toolkitLabel xml:lang="vi">8vo</rdakit:toolkitLabel>
      <skos:definition xml:lang="vi">Định dạng thư mục có chứa một hoặc nhiều hơn tờ in bằng 1/8 của toàn bộ tờ.</skos:definition>
      <rdakit:toolkitDefinition xml:lang="vi">Định dạng thư mục có chứa một hoặc nhiều hơn tờ in bằng 1/8 của toàn bộ tờ.</rdakit:toolkitDefinition>
      <skos:altLabel xml:lang="de">Oktav</skos:altLabel>
      <skos:prefLabel xml:lang="da">8o</skos:prefLabel>
      <skos:altLabel xml:lang="da">oktavformat</skos:altLabel>
      <rdakit:toolkitLabel xml:lang="da">8o</rdakit:toolkitLabel>
      <skos:definition xml:lang="da">Bibliografisk format, der består af et eller flere blade, der er 1/8 af et helt ark.</skos:definition>
      <rdakit:toolkitDefinition xml:lang="da">Bibliografisk format, der består af et eller flere blade, der er 1/8 af et helt ark.</rdakit:toolkitDefinition>
      <skos:definition xml:lang="fi">Kirjan formaatti muodostuu yhdestä tai useammasta lehdestä, jotka ovat kooltaan 1/8 painoarkista.</skos:definition>
      <rdakit:toolkitDefinition xml:lang="fi">Kirjan formaatti muodostuu yhdestä tai useammasta lehdestä, jotka ovat kooltaan 1/8 painoarkista.</rdakit:toolkitDefinition>
      <skos:prefLabel xml:lang="no">oktavformat</skos:prefLabel>
      <rdakit:toolkitLabel xml:lang="no">oktavformat</rdakit:toolkitLabel>
      <skos:definition xml:lang="no">Et bokformat som består av ett eller flere blad som er 1/8 av et ark.</skos:definition>
      <rdakit:toolkitDefinition xml:lang="no">Et bokformat som består av ett eller flere blad som er 1/8 av et ark.</rdakit:toolkitDefinition>
    </skos:Concept>
<!-- Concept: 96mo  -->
    <skos:Concept rdf:about="http://rdaregistry.info/termList/bookFormat/1013" xml:lang="en">
      <skos:inScheme rdf:resource="http://rdaregistry.info/termList/bookFormat"/>
      <reg:status rdf:resource="http://metadataregistry.org/uri/RegStatus/1001"/>
      <reg:identifier rdf:resource="http://metadataregistry.org/concepts/9508"/>
      <skos:prefLabel xml:lang="en">96mo</skos:prefLabel>
      <skos:altLabel xml:lang="en">ninety-sixmo</skos:altLabel>
      <rdakit:toolkitLabel xml:lang="en">96mo</rdakit:toolkitLabel>
      <skos:definition xml:lang="en">A bibliographic format consisting of one or more leaves that are 1/96 of the whole sheet.</skos:definition>
      <rdakit:toolkitDefinition xml:lang="en">A bibliographic format consisting of one or more leaves that are 1/96 of the whole sheet.</rdakit:toolkitDefinition>
      <skos:prefLabel xml:lang="ca">96º</skos:prefLabel>
      <skos:altLabel xml:lang="ca">noranta-sisau</skos:altLabel>
      <rdakit:toolkitLabel xml:lang="ca">96º</rdakit:toolkitLabel>
      <skos:definition xml:lang="ca">Format bibliogràfic que consisteix en un o més fulls que són 1/96 del full sencer.</skos:definition>
      <rdakit:toolkitDefinition xml:lang="ca">Format bibliogràfic que consisteix en un o més fulls que són 1/96 del full sencer.</rdakit:toolkitDefinition>
      <skos:prefLabel xml:lang="vi">96mo</skos:prefLabel>
      <skos:altLabel xml:lang="vi">khổ chín sáu</skos:altLabel>
      <rdakit:toolkitLabel xml:lang="vi">96mo</rdakit:toolkitLabel>
      <skos:definition xml:lang="vi">Định dạng thư mục có chứa một hoặc nhiều hơn tờ in bằng 1/96 của toàn bộ tờ.</skos:definition>
      <rdakit:toolkitDefinition xml:lang="vi">Định dạng thư mục có chứa một hoặc nhiều hơn tờ in bằng 1/96 của toàn bộ tờ.</rdakit:toolkitDefinition>
      <skos:prefLabel xml:lang="de">96°</skos:prefLabel>
      <skos:altLabel xml:lang="de">Nonagesimo sexto</skos:altLabel>
      <rdakit:toolkitLabel xml:lang="de">96°</rdakit:toolkitLabel>
      <skos:definition xml:lang="de">Ein Buchformat, das aus einem oder mehreren Blättern besteht, das/die 1/96 des ganzen Bogens ist/sind.</skos:definition>
      <rdakit:toolkitDefinition xml:lang="de">Ein Buchformat, das aus einem oder mehreren Blättern besteht, das/die 1/96 des ganzen Bogens ist/sind.</rdakit:toolkitDefinition>
      <skos:prefLabel xml:lang="da">96o</skos:prefLabel>
      <rdakit:toolkitLabel xml:lang="da">96o</rdakit:toolkitLabel>
      <skos:definition xml:lang="da">Bibliografisk format, der består af et eller flere blade, der er 1/96 af et helt ark.</skos:definition>
      <rdakit:toolkitDefinition xml:lang="da">Bibliografisk format, der består af et eller flere blade, der er 1/96 af et helt ark.</rdakit:toolkitDefinition>
      <skos:prefLabel xml:lang="fi">96:o</skos:prefLabel>
      <rdakit:toolkitLabel xml:lang="fi">96:o</rdakit:toolkitLabel>
      <skos:definition xml:lang="fi">Kirjan formaatti muodostuu yhdestä tai useammasta lehdestä, jotka ovat kooltaan 1/96 painoarkista.</skos:definition>
      <rdakit:toolkitDefinition xml:lang="fi">Kirjan formaatti muodostuu yhdestä tai useammasta lehdestä, jotka ovat kooltaan 1/96 painoarkista.</rdakit:toolkitDefinition>
      <skos:prefLabel xml:lang="fr">96º</skos:prefLabel>
      <skos:altLabel xml:lang="fr">in-quatre-vingt-seize</skos:altLabel>
      <rdakit:toolkitLabel xml:lang="fr">96º</rdakit:toolkitLabel>
      <skos:definition xml:lang="fr">Format bibliographique qui consiste en un ou plusieurs feuillets formant chacun 1/96 de la feuille complète.</skos:definition>
      <rdakit:toolkitDefinition xml:lang="fr">Format bibliographique qui consiste en un ou plusieurs feuillets formant chacun 1/96 de la feuille complète.</rdakit:toolkitDefinition>
      <skos:definition xml:lang="no">Et bokformat som består av ett eller flere blad som er 1/96 av et ark.</skos:definition>
      <rdakit:toolkitDefinition xml:lang="no">Et bokformat som består av ett eller flere blad som er 1/96 av et ark.</rdakit:toolkitDefinition>
    </skos:Concept>
<!-- Concept: folio  -->
    <skos:Concept rdf:about="http://rdaregistry.info/termList/bookFormat/1001" xml:lang="en">
      <skos:inScheme rdf:resource="http://rdaregistry.info/termList/bookFormat"/>
      <reg:status rdf:resource="http://metadataregistry.org/uri/RegStatus/1001"/>
      <reg:identifier rdf:resource="http://metadataregistry.org/concepts/850"/>
      <skos:prefLabel xml:lang="en">folio</skos:prefLabel>
      <skos:definition xml:lang="en">A bibliographic format consisting of one or more leaves that are 1/2 of the whole sheet.</skos:definition>
      <skos:definition xml:lang="de">Ein Buchformat, das aus einem oder mehreren Blättern besteht, das/die 1/2 des ganzen Bogens ist/sind.</skos:definition>
      <skos:definition xml:lang="fr">Format bibliographique qui consiste en un ou plusieurs feuillets formant chacun 1/2 de la feuille complète.</skos:definition>
      <skos:altLabel xml:lang="fr">in-folio</skos:altLabel>
      <skos:prefLabel xml:lang="fr">2º</skos:prefLabel>
      <skos:prefLabel xml:lang="es">folio</skos:prefLabel>
      <skos:prefLabel xml:lang="de">2°</skos:prefLabel>
      <skos:altLabel xml:lang="en">2o</skos:altLabel>
      <rdakit:toolkitLabel xml:lang="en">folio</rdakit:toolkitLabel>
      <rdakit:toolkitLabel xml:lang="fr">2º</rdakit:toolkitLabel>
      <rdakit:toolkitDefinition xml:lang="en">A bibliographic format consisting of one or more leaves that are 1/2 of the whole sheet.</rdakit:toolkitDefinition>
      <rdakit:toolkitDefinition xml:lang="fr">Format bibliographique qui consiste en un ou plusieurs feuillets formant chacun 1/2 de la feuille complète.</rdakit:toolkitDefinition>
      <rdakit:toolkitLabel xml:lang="de">2°</rdakit:toolkitLabel>
      <rdakit:toolkitDefinition xml:lang="de">Ein Buchformat, das aus einem oder mehreren Blättern besteht, das/die 1/2 des ganzen Bogens ist/sind.</rdakit:toolkitDefinition>
      <rdakit:toolkitLabel xml:lang="es">folio</rdakit:toolkitLabel>
      <skos:prefLabel xml:lang="zh">对开</skos:prefLabel>
      <skos:altLabel xml:lang="zh">对开</skos:altLabel>
      <rdakit:toolkitLabel xml:lang="zh">对开</rdakit:toolkitLabel>
      <skos:definition xml:lang="zh">图书的一种开本，由一叶或多叶全张纸的1/2组成。</skos:definition>
      <rdakit:toolkitDefinition xml:lang="zh">图书的一种开本，由一叶或多叶全张纸的1/2组成。</rdakit:toolkitDefinition>
      <skos:definition xml:lang="es">Un formato de libro que consiste en una o más hojas que son 1/2 del folio completo.</skos:definition>
      <rdakit:toolkitDefinition xml:lang="es">Un formato de libro que consiste en una o más hojas que son 1/2 del folio completo.</rdakit:toolkitDefinition>
      <skos:prefLabel xml:lang="nl">folio</skos:prefLabel>
      <rdakit:toolkitLabel xml:lang="nl">folio</rdakit:toolkitLabel>
      <skos:definition xml:lang="nl">Een boekformaat dat bestaat uit één of meer bladen die 1/2 van een heel vel zijn.</skos:definition>
      <rdakit:toolkitDefinition xml:lang="nl">Een boekformaat dat bestaat uit één of meer bladen die 1/2 van een heel vel zijn.</rdakit:toolkitDefinition>
      <skos:prefLabel xml:lang="it">in folio</skos:prefLabel>
      <rdakit:toolkitLabel xml:lang="it">in folio</rdakit:toolkitLabel>
      <skos:prefLabel xml:lang="fi">2:o</skos:prefLabel>
      <rdakit:toolkitLabel xml:lang="fi">2:o</rdakit:toolkitLabel>
      <skos:prefLabel xml:lang="ca">2º</skos:prefLabel>
      <skos:altLabel xml:lang="ca">folio</skos:altLabel>
      <rdakit:toolkitLabel xml:lang="ca">2º</rdakit:toolkitLabel>
      <skos:definition xml:lang="ca">Format bibliogràfic que consisteix en un o més fulls que són la meitat del full sencer.</skos:definition>
      <rdakit:toolkitDefinition xml:lang="ca">Format bibliogràfic que consisteix en un o més fulls que són la meitat del full sencer.</rdakit:toolkitDefinition>
      <skos:prefLabel xml:lang="vi">folio</skos:prefLabel>
      <skos:altLabel xml:lang="vi">khổ hai</skos:altLabel>
      <rdakit:toolkitLabel xml:lang="vi">folio</rdakit:toolkitLabel>
      <skos:definition xml:lang="vi">Định dạng thư mục có chứa một hoặc nhiều hơn tờ in bằng 1/2 của toàn bộ tờ.</skos:definition>
      <rdakit:toolkitDefinition xml:lang="vi">Định dạng thư mục có chứa một hoặc nhiều hơn tờ in bằng 1/2 của toàn bộ tờ.</rdakit:toolkitDefinition>
      <skos:altLabel xml:lang="de">Folio</skos:altLabel>
      <skos:prefLabel xml:lang="da">folio</skos:prefLabel>
      <skos:altLabel xml:lang="da">2o</skos:altLabel>
      <rdakit:toolkitLabel xml:lang="da">folio</rdakit:toolkitLabel>
      <skos:definition xml:lang="da">Bibliografisk format, der består af et eller flere blade, der er halvdelen af et helt ark.</skos:definition>
      <rdakit:toolkitDefinition xml:lang="da">Bibliografisk format, der består af et eller flere blade, der er halvdelen af et helt ark.</rdakit:toolkitDefinition>
      <skos:definition xml:lang="fi">Kirjan formaatti muodostuu yhdestä tai useammasta lehdestä, jotka ovat kooltaan 1/2 painoarkista</skos:definition>
      <rdakit:toolkitDefinition xml:lang="fi">Kirjan formaatti muodostuu yhdestä tai useammasta lehdestä, jotka ovat kooltaan 1/2 painoarkista</rdakit:toolkitDefinition>
      <skos:prefLabel xml:lang="no">folio</skos:prefLabel>
      <rdakit:toolkitLabel xml:lang="no">folio</rdakit:toolkitLabel>
      <skos:definition xml:lang="no">Et bokformat som består av ett eller flere blad som er 1/2 av et ark.</skos:definition>
      <rdakit:toolkitDefinition xml:lang="no">Et bokformat som består av ett eller flere blad som er 1/2 av et ark.</rdakit:toolkitDefinition>
    </skos:Concept>
<!-- Concept: full-sheet  -->
    <skos:Concept rdf:about="http://rdaregistry.info/termList/bookFormat/1015" xml:lang="en">
      <skos:inScheme rdf:resource="http://rdaregistry.info/termList/bookFormat"/>
      <reg:status rdf:resource="http://metadataregistry.org/uri/RegStatus/1001"/>
      <reg:identifier rdf:resource="http://metadataregistry.org/concepts/9510"/>
      <skos:prefLabel xml:lang="en">full-sheet</skos:prefLabel>
      <rdakit:toolkitLabel xml:lang="en">full-sheet</rdakit:toolkitLabel>
      <skos:definition xml:lang="en">A bibliographic format consisting of one or more sheets that have not been cut or folded.</skos:definition>
      <rdakit:toolkitDefinition xml:lang="en">A bibliographic format consisting of one or more sheets that have not been cut or folded.</rdakit:toolkitDefinition>
      <skos:altLabel xml:lang="en">full sheet</skos:altLabel>
      <skos:prefLabel xml:lang="ca">full complet</skos:prefLabel>
      <rdakit:toolkitLabel xml:lang="ca">full complet</rdakit:toolkitLabel>
      <skos:definition xml:lang="ca">Format bibliogràfic que consisteix en un o més fulls que no han estat tallats o plegats.</skos:definition>
      <rdakit:toolkitDefinition xml:lang="ca">Format bibliogràfic que consisteix en un o més fulls que no han estat tallats o plegats.</rdakit:toolkitDefinition>
      <skos:prefLabel xml:lang="vi">toàn tờ</skos:prefLabel>
      <skos:altLabel xml:lang="vi">toàn-tờ</skos:altLabel>
      <rdakit:toolkitLabel xml:lang="vi">toàn tờ</rdakit:toolkitLabel>
      <skos:definition xml:lang="vi">Định dạng thư mục có chứa một hoặc nhiều hơn tờ không bị cắt hoặc gấp.</skos:definition>
      <rdakit:toolkitDefinition xml:lang="vi">Định dạng thư mục có chứa một hoặc nhiều hơn tờ không bị cắt hoặc gấp.</rdakit:toolkitDefinition>
      <skos:prefLabel xml:lang="de">Ungefalzter Bogen</skos:prefLabel>
      <skos:altLabel xml:lang="de">Doppelfolio</skos:altLabel>
      <rdakit:toolkitLabel xml:lang="de">Ungefalzter Bogen</rdakit:toolkitLabel>
      <skos:definition xml:lang="de">Ein Buchformat, das aus einem oder mehreren Blättern besteht, die weder geschnitten noch gefaltet sind.</skos:definition>
      <rdakit:toolkitDefinition xml:lang="de">Ein Buchformat, das aus einem oder mehreren Blättern besteht, die weder geschnitten noch gefaltet sind.</rdakit:toolkitDefinition>
      <skos:altLabel xml:lang="de">Atlasformat</skos:altLabel>
      <skos:prefLabel xml:lang="da">helt ark</skos:prefLabel>
      <rdakit:toolkitLabel xml:lang="da">helt ark</rdakit:toolkitLabel>
      <skos:definition xml:lang="da">Bibliografisk format, der består af et eller flere ark, der ikke er blevet skåret eller foldet.</skos:definition>
      <rdakit:toolkitDefinition xml:lang="da">Bibliografisk format, der består af et eller flere ark, der ikke er blevet skåret eller foldet.</rdakit:toolkitDefinition>
      <skos:prefLabel xml:lang="fi">kokoarkki</skos:prefLabel>
      <rdakit:toolkitLabel xml:lang="fi">kokoarkki</rdakit:toolkitLabel>
      <skos:definition xml:lang="fi">Kirjan formaatti muodostuu yhdestä tai useammasta lehdestä, joita ei ole leikattu tai taitettu.</skos:definition>
      <rdakit:toolkitDefinition xml:lang="fi">Kirjan formaatti muodostuu yhdestä tai useammasta lehdestä, joita ei ole leikattu tai taitettu.</rdakit:toolkitDefinition>
      <skos:prefLabel xml:lang="fr">in-plano</skos:prefLabel>
      <rdakit:toolkitLabel xml:lang="fr">in-plano</rdakit:toolkitLabel>
      <skos:definition xml:lang="fr">Format bibliographique qui consiste en une ou plusieurs feuilles n’ayant été ni coupées ni pliées.</skos:definition>
      <rdakit:toolkitDefinition xml:lang="fr">Format bibliographique qui consiste en une ou plusieurs feuilles n’ayant été ni coupées ni pliées.</rdakit:toolkitDefinition>
      <skos:prefLabel xml:lang="no">planoark</skos:prefLabel>
      <rdakit:toolkitLabel xml:lang="no">planoark</rdakit:toolkitLabel>
      <skos:definition xml:lang="no">Et bokformat som består av ett eller flere ark som verken er brettet eller beskåret.</skos:definition>
      <rdakit:toolkitDefinition xml:lang="no">Et bokformat som består av ett eller flere ark som verken er brettet eller beskåret.</rdakit:toolkitDefinition>
    </skos:Concept>

<!-- Status properties used in this document  -->
    <skos:Concept rdf:about="http://metadataregistry.org/uri/RegStatus/1001">
        <skos:prefLabel xml:lang="en">Published</skos:prefLabel>
    </skos:Concept>

</rdf:RDF>
