<?xml version="1.0" encoding = "UTF-8"?>
<rdf:RDF
    xmlns:dc="http://purl.org/dc/elements/1.1/"
    xmlns:rdakit="http://metadataregistry.org/uri/profile/rdakit/"
    xmlns:rdf="http://www.w3.org/1999/02/22-rdf-syntax-ns#"
    xmlns:reg="http://metadataregistry.org/uri/profile/regap/"
    xmlns:owl="http://www.w3.org/2002/07/owl#"
    xmlns:skos="http://www.w3.org/2004/02/skos/core#">

<owl:Ontology rdf:about="http://rdaregistry.info/termList/configPlayback" />
<!-- Scheme: RDA Configuration of Playback Channels -->
    <skos:ConceptScheme rdf:about="http://rdaregistry.info/termList/configPlayback">
        <dc:title>RDA Configuration of Playback Channels</dc:title>
    </skos:ConceptScheme>

<!-- Concept: mono  -->
    <skos:Concept rdf:about="http://rdaregistry.info/termList/configPlayback/1001" xml:lang="en">
      <skos:inScheme rdf:resource="http://rdaregistry.info/termList/configPlayback"/>
      <reg:status rdf:resource="http://metadataregistry.org/uri/RegStatus/1001"/>
      <reg:identifier rdf:resource="http://metadataregistry.org/concepts/874"/>
      <skos:prefLabel xml:lang="en">mono</skos:prefLabel>
      <rdakit:toolkitLabel xml:lang="en">mono</rdakit:toolkitLabel>
      <skos:definition xml:lang="en">A configuration of playback channels consisting of a single channel for monophonic sound.</skos:definition>
      <rdakit:toolkitDefinition xml:lang="en">A configuration of playback channels consisting of a single channel for monophonic sound.</rdakit:toolkitDefinition>
      <skos:prefLabel xml:lang="it">mono</skos:prefLabel>
      <rdakit:toolkitLabel xml:lang="it">mono</rdakit:toolkitLabel>
      <skos:prefLabel xml:lang="de">Mono</skos:prefLabel>
      <rdakit:toolkitLabel xml:lang="de">Mono</rdakit:toolkitLabel>
      <skos:prefLabel xml:lang="fr">mono</skos:prefLabel>
      <rdakit:toolkitLabel xml:lang="fr">mono</rdakit:toolkitLabel>
      <skos:prefLabel xml:lang="es">mono</skos:prefLabel>
      <rdakit:toolkitLabel xml:lang="es">mono</rdakit:toolkitLabel>
      <skos:prefLabel xml:lang="fi">mono</skos:prefLabel>
      <rdakit:toolkitLabel xml:lang="fi">mono</rdakit:toolkitLabel>
      <skos:prefLabel xml:lang="vi">đơn</skos:prefLabel>
      <rdakit:toolkitLabel xml:lang="vi">đơn</rdakit:toolkitLabel>
      <skos:definition xml:lang="vi">Cấu hình kênh phát lại gồm có một kênh đơn lẻ cho âm thanh đơn sắc.</skos:definition>
      <rdakit:toolkitDefinition xml:lang="vi">Cấu hình kênh phát lại gồm có một kênh đơn lẻ cho âm thanh đơn sắc.</rdakit:toolkitDefinition>
      <skos:definition xml:lang="de">Eine Konfiguration der Wiedergabekanäle, die aus einem Kanal für eine monophone Aufnahme besteht.</skos:definition>
      <rdakit:toolkitDefinition xml:lang="de">Eine Konfiguration der Wiedergabekanäle, die aus einem Kanal für eine monophone Aufnahme besteht.</rdakit:toolkitDefinition>
      <skos:prefLabel xml:lang="da">mono</skos:prefLabel>
      <rdakit:toolkitLabel xml:lang="da">mono</rdakit:toolkitLabel>
      <skos:definition xml:lang="da">Konfiguration af afspilningskanaler, der består af en enkel kanal for monografisk lyd.</skos:definition>
      <rdakit:toolkitDefinition xml:lang="da">Konfiguration af afspilningskanaler, der består af en enkel kanal for monografisk lyd.</rdakit:toolkitDefinition>
      <skos:prefLabel xml:lang="ca">mono</skos:prefLabel>
      <rdakit:toolkitLabel xml:lang="ca">mono</rdakit:toolkitLabel>
      <skos:definition xml:lang="fi">Yhdestä kanavasta koostuva monofonisen äänen äänikanava.</skos:definition>
      <rdakit:toolkitDefinition xml:lang="fi">Yhdestä kanavasta koostuva monofonisen äänen äänikanava.</rdakit:toolkitDefinition>
      <skos:definition xml:lang="fr">Configuration des canaux de reproduction qui consiste en un seul canal pour le son monophonique.</skos:definition>
      <rdakit:toolkitDefinition xml:lang="fr">Configuration des canaux de reproduction qui consiste en un seul canal pour le son monophonique.</rdakit:toolkitDefinition>
      <skos:prefLabel xml:lang="no">mono</skos:prefLabel>
      <rdakit:toolkitLabel xml:lang="no">mono</rdakit:toolkitLabel>
      <skos:definition xml:lang="no">En konfigurasjon av kanaler for avspilling som består av én enkelt kanal for monofonisk lyd.</skos:definition>
      <rdakit:toolkitDefinition xml:lang="no">En konfigurasjon av kanaler for avspilling som består av én enkelt kanal for monofonisk lyd.</rdakit:toolkitDefinition>
    </skos:Concept>
<!-- Concept: quadraphonic  -->
    <skos:Concept rdf:about="http://rdaregistry.info/termList/configPlayback/1003" xml:lang="en">
      <skos:inScheme rdf:resource="http://rdaregistry.info/termList/configPlayback"/>
      <reg:status rdf:resource="http://metadataregistry.org/uri/RegStatus/1001"/>
      <reg:identifier rdf:resource="http://metadataregistry.org/concepts/876"/>
      <skos:prefLabel xml:lang="en">quadraphonic</skos:prefLabel>
      <rdakit:toolkitLabel xml:lang="en">quadraphonic</rdakit:toolkitLabel>
      <skos:definition xml:lang="en">A configuration of playback channels consisting of four channels for quadraphonic sound.</skos:definition>
      <rdakit:toolkitDefinition xml:lang="en">A configuration of playback channels consisting of four channels for quadraphonic sound.</rdakit:toolkitDefinition>
      <skos:prefLabel xml:lang="it">quadrifonico</skos:prefLabel>
      <rdakit:toolkitLabel xml:lang="it">quadrifonico</rdakit:toolkitLabel>
      <skos:prefLabel xml:lang="de">Quadro</skos:prefLabel>
      <rdakit:toolkitLabel xml:lang="de">Quadro</rdakit:toolkitLabel>
      <skos:prefLabel xml:lang="fr">quadriphonique</skos:prefLabel>
      <rdakit:toolkitLabel xml:lang="fr">quadriphonique</rdakit:toolkitLabel>
      <skos:prefLabel xml:lang="es">cuadrafónico</skos:prefLabel>
      <rdakit:toolkitLabel xml:lang="es">cuadrafónico</rdakit:toolkitLabel>
      <skos:prefLabel xml:lang="fi">kvadrofoninen</skos:prefLabel>
      <rdakit:toolkitLabel xml:lang="fi">kvadrofoninen</rdakit:toolkitLabel>
      <skos:prefLabel xml:lang="vi">bốn kênh</skos:prefLabel>
      <rdakit:toolkitLabel xml:lang="vi">bốn kênh</rdakit:toolkitLabel>
      <skos:definition xml:lang="vi">Cấu hình kênh phát lại gồm có bốn kênh cho âm thanh bậc bốn.</skos:definition>
      <rdakit:toolkitDefinition xml:lang="vi">Cấu hình kênh phát lại gồm có bốn kênh cho âm thanh bậc bốn.</rdakit:toolkitDefinition>
      <skos:definition xml:lang="de">Eine Konfiguration der Wiedergabekanäle, die aus vier Kanälen für eine quadrophonische Aufnahme besteht.</skos:definition>
      <rdakit:toolkitDefinition xml:lang="de">Eine Konfiguration der Wiedergabekanäle, die aus vier Kanälen für eine quadrophonische Aufnahme besteht.</rdakit:toolkitDefinition>
      <skos:prefLabel xml:lang="da">kvadrofonisk</skos:prefLabel>
      <rdakit:toolkitLabel xml:lang="da">kvadrofonisk</rdakit:toolkitLabel>
      <skos:definition xml:lang="da">Konfiguration af afspilningskanaler, der består af fire kanaler for kvadrofonisk lyd.</skos:definition>
      <rdakit:toolkitDefinition xml:lang="da">Konfiguration af afspilningskanaler, der består af fire kanaler for kvadrofonisk lyd.</rdakit:toolkitDefinition>
      <skos:prefLabel xml:lang="ca">quadrifònic</skos:prefLabel>
      <rdakit:toolkitLabel xml:lang="ca">quadrifònic</rdakit:toolkitLabel>
      <skos:definition xml:lang="fi">Neljästä kanavasta koostuva kvadrofonisen äänen äänikanava.</skos:definition>
      <rdakit:toolkitDefinition xml:lang="fi">Neljästä kanavasta koostuva kvadrofonisen äänen äänikanava.</rdakit:toolkitDefinition>
      <skos:definition xml:lang="fr">Configuration des canaux de reproduction qui consiste en quatre canaux pour le son quadriphonique.</skos:definition>
      <rdakit:toolkitDefinition xml:lang="fr">Configuration des canaux de reproduction qui consiste en quatre canaux pour le son quadriphonique.</rdakit:toolkitDefinition>
      <skos:prefLabel xml:lang="no">kvadrofonisk</skos:prefLabel>
      <rdakit:toolkitLabel xml:lang="no">kvadrofonisk</rdakit:toolkitLabel>
      <skos:definition xml:lang="no">En konfigurasjon av kanaler for avspilling som består av fire kanaler for kvadrofonisk lyd.</skos:definition>
      <rdakit:toolkitDefinition xml:lang="no">En konfigurasjon av kanaler for avspilling som består av fire kanaler for kvadrofonisk lyd.</rdakit:toolkitDefinition>
    </skos:Concept>
<!-- Concept: stereo  -->
    <skos:Concept rdf:about="http://rdaregistry.info/termList/configPlayback/1002" xml:lang="en">
      <skos:inScheme rdf:resource="http://rdaregistry.info/termList/configPlayback"/>
      <reg:status rdf:resource="http://metadataregistry.org/uri/RegStatus/1001"/>
      <reg:identifier rdf:resource="http://metadataregistry.org/concepts/875"/>
      <skos:prefLabel xml:lang="en">stereo</skos:prefLabel>
      <rdakit:toolkitLabel xml:lang="en">stereo</rdakit:toolkitLabel>
      <skos:definition xml:lang="en">A configuration of playback channels consisting of two channels for stereophonic sound.</skos:definition>
      <rdakit:toolkitDefinition xml:lang="en">A configuration of playback channels consisting of two channels for stereophonic sound.</rdakit:toolkitDefinition>
      <skos:prefLabel xml:lang="it">stereo</skos:prefLabel>
      <rdakit:toolkitLabel xml:lang="it">stereo</rdakit:toolkitLabel>
      <skos:prefLabel xml:lang="de">Stereo</skos:prefLabel>
      <rdakit:toolkitLabel xml:lang="de">Stereo</rdakit:toolkitLabel>
      <skos:prefLabel xml:lang="fr">stéréo</skos:prefLabel>
      <rdakit:toolkitLabel xml:lang="fr">stéréo</rdakit:toolkitLabel>
      <skos:prefLabel xml:lang="es">estéreo</skos:prefLabel>
      <rdakit:toolkitLabel xml:lang="es">estéreo</rdakit:toolkitLabel>
      <skos:prefLabel xml:lang="fi">stereo</skos:prefLabel>
      <rdakit:toolkitLabel xml:lang="fi">stereo</rdakit:toolkitLabel>
      <skos:prefLabel xml:lang="vi">nổi</skos:prefLabel>
      <rdakit:toolkitLabel xml:lang="vi">nổi</rdakit:toolkitLabel>
      <skos:definition xml:lang="vi">Cấu hình kênh phát lại gồm có hai kênh cho âm thanh nổi.</skos:definition>
      <rdakit:toolkitDefinition xml:lang="vi">Cấu hình kênh phát lại gồm có hai kênh cho âm thanh nổi.</rdakit:toolkitDefinition>
      <skos:definition xml:lang="de">Eine Konfiguration der Wiedergabekanäle, die aus zwei Kanälen für eine stereophone Aufnahme besteht.</skos:definition>
      <rdakit:toolkitDefinition xml:lang="de">Eine Konfiguration der Wiedergabekanäle, die aus zwei Kanälen für eine stereophone Aufnahme besteht.</rdakit:toolkitDefinition>
      <skos:prefLabel xml:lang="da">stereo</skos:prefLabel>
      <rdakit:toolkitLabel xml:lang="da">stereo</rdakit:toolkitLabel>
      <skos:definition xml:lang="da">Konfiguration af afspilningskanaler, der består af to kanaler for stereofonisk lyd.</skos:definition>
      <rdakit:toolkitDefinition xml:lang="da">Konfiguration af afspilningskanaler, der består af to kanaler for stereofonisk lyd.</rdakit:toolkitDefinition>
      <skos:prefLabel xml:lang="ca">estèreo</skos:prefLabel>
      <rdakit:toolkitLabel xml:lang="ca">estèreo</rdakit:toolkitLabel>
      <skos:definition xml:lang="fi">Kahdesta kanavasta koostuva stereofonisen äänen äänikanava.</skos:definition>
      <rdakit:toolkitDefinition xml:lang="fi">Kahdesta kanavasta koostuva stereofonisen äänen äänikanava.</rdakit:toolkitDefinition>
      <skos:definition xml:lang="fr">Configuration des canaux de reproduction qui consiste en deux canaux pour le son stéréophonique.</skos:definition>
      <rdakit:toolkitDefinition xml:lang="fr">Configuration des canaux de reproduction qui consiste en deux canaux pour le son stéréophonique.</rdakit:toolkitDefinition>
      <skos:prefLabel xml:lang="no">stereo</skos:prefLabel>
      <rdakit:toolkitLabel xml:lang="no">stereo</rdakit:toolkitLabel>
      <skos:definition xml:lang="no">En konfigurasjon av kanaler for avspilling som består av to kanaler for stereofonisk lyd.</skos:definition>
      <rdakit:toolkitDefinition xml:lang="no">En konfigurasjon av kanaler for avspilling som består av to kanaler for stereofonisk lyd.</rdakit:toolkitDefinition>
    </skos:Concept>
<!-- Concept: surround  -->
    <skos:Concept rdf:about="http://rdaregistry.info/termList/configPlayback/1004" xml:lang="en">
      <skos:inScheme rdf:resource="http://rdaregistry.info/termList/configPlayback"/>
      <reg:status rdf:resource="http://metadataregistry.org/uri/RegStatus/1001"/>
      <reg:identifier rdf:resource="http://metadataregistry.org/concepts/877"/>
      <skos:prefLabel xml:lang="en">surround</skos:prefLabel>
      <rdakit:toolkitLabel xml:lang="en">surround</rdakit:toolkitLabel>
      <skos:definition xml:lang="en">A configuration of playback channels consisting of more than four channels for surround sound.</skos:definition>
      <rdakit:toolkitDefinition xml:lang="en">A configuration of playback channels consisting of more than four channels for surround sound.</rdakit:toolkitDefinition>
      <skos:prefLabel xml:lang="it">surround</skos:prefLabel>
      <rdakit:toolkitLabel xml:lang="it">surround</rdakit:toolkitLabel>
      <skos:prefLabel xml:lang="de">Surround</skos:prefLabel>
      <rdakit:toolkitLabel xml:lang="de">Surround</rdakit:toolkitLabel>
      <skos:prefLabel xml:lang="fr">ambiophonique</skos:prefLabel>
      <rdakit:toolkitLabel xml:lang="fr">ambiophonique</rdakit:toolkitLabel>
      <skos:prefLabel xml:lang="es">sonido global</skos:prefLabel>
      <rdakit:toolkitLabel xml:lang="es">sonido global</rdakit:toolkitLabel>
      <skos:prefLabel xml:lang="fi">surround</skos:prefLabel>
      <rdakit:toolkitLabel xml:lang="fi">surround</rdakit:toolkitLabel>
      <skos:prefLabel xml:lang="vi">lan toả</skos:prefLabel>
      <rdakit:toolkitLabel xml:lang="vi">lan toả</rdakit:toolkitLabel>
      <skos:definition xml:lang="vi">Cấu hình kênh phát lại gồm có nhiều hơn bốn kênh cho âm thanh lan toả.</skos:definition>
      <rdakit:toolkitDefinition xml:lang="vi">Cấu hình kênh phát lại gồm có nhiều hơn bốn kênh cho âm thanh lan toả.</rdakit:toolkitDefinition>
      <skos:definition xml:lang="de">Eine Konfiguration der Wiedergabekanäle, die aus mehr als vier Kanälen für eine Surround-Aufnahme besteht.</skos:definition>
      <rdakit:toolkitDefinition xml:lang="de">Eine Konfiguration der Wiedergabekanäle, die aus mehr als vier Kanälen für eine Surround-Aufnahme besteht.</rdakit:toolkitDefinition>
      <skos:prefLabel xml:lang="da">surround</skos:prefLabel>
      <rdakit:toolkitLabel xml:lang="da">surround</rdakit:toolkitLabel>
      <skos:definition xml:lang="da">Konfiguration af afspilningskanaler, der består af flere end fire kanaler for surroundsound.</skos:definition>
      <rdakit:toolkitDefinition xml:lang="da">Konfiguration af afspilningskanaler, der består af flere end fire kanaler for surroundsound.</rdakit:toolkitDefinition>
      <skos:prefLabel xml:lang="ca">so envoltant</skos:prefLabel>
      <rdakit:toolkitLabel xml:lang="ca">so envoltant</rdakit:toolkitLabel>
      <skos:definition xml:lang="fi">Useammasta kuin neljästä kanavasta koostuva surround-äänen äänikanava.</skos:definition>
      <rdakit:toolkitDefinition xml:lang="fi">Useammasta kuin neljästä kanavasta koostuva surround-äänen äänikanava.</rdakit:toolkitDefinition>
      <skos:definition xml:lang="fr">Configuration des canaux de reproduction qui consiste en plus de quatre canaux pour le son ambiophonique.</skos:definition>
      <rdakit:toolkitDefinition xml:lang="fr">Configuration des canaux de reproduction qui consiste en plus de quatre canaux pour le son ambiophonique.</rdakit:toolkitDefinition>
      <skos:prefLabel xml:lang="no">surround</skos:prefLabel>
      <rdakit:toolkitLabel xml:lang="no">surround</rdakit:toolkitLabel>
      <skos:definition xml:lang="no">En konfigurasjon av kanaler for avspilling som består av mer enn fire kanaler for surroundlyd.</skos:definition>
      <rdakit:toolkitDefinition xml:lang="no">En konfigurasjon av kanaler for avspilling som består av mer enn fire kanaler for surroundlyd.</rdakit:toolkitDefinition>
    </skos:Concept>

<!-- Status properties used in this document  -->
    <skos:Concept rdf:about="http://metadataregistry.org/uri/RegStatus/1001">
        <skos:prefLabel xml:lang="en">Published</skos:prefLabel>
    </skos:Concept>

</rdf:RDF>
