<?xml version="1.0" encoding = "UTF-8"?>
<rdf:RDF
    xmlns:dc="http://purl.org/dc/elements/1.1/"
    xmlns:rdakit="http://metadataregistry.org/uri/profile/rdakit/"
    xmlns:rdf="http://www.w3.org/1999/02/22-rdf-syntax-ns#"
    xmlns:reg="http://metadataregistry.org/uri/profile/regap/"
    xmlns:owl="http://www.w3.org/2002/07/owl#"
    xmlns:skos="http://www.w3.org/2004/02/skos/core#">

<owl:Ontology rdf:about="http://rdaregistry.info/termList/frequency" />
<!-- Scheme: RDA Frequency -->
    <skos:ConceptScheme rdf:about="http://rdaregistry.info/termList/frequency">
        <dc:title>RDA Frequency</dc:title>
    </skos:ConceptScheme>

<!-- Concept: annual  -->
    <skos:Concept rdf:about="http://rdaregistry.info/termList/frequency/1013" xml:lang="en">
      <skos:inScheme rdf:resource="http://rdaregistry.info/termList/frequency"/>
      <reg:status rdf:resource="http://metadataregistry.org/uri/RegStatus/1001"/>
      <reg:identifier rdf:resource="http://metadataregistry.org/concepts/757"/>
      <skos:prefLabel xml:lang="en">annual</skos:prefLabel>
      <skos:definition xml:lang="en">A frequency for a manifestation issued or updated once every year.</skos:definition>
      <skos:prefLabel xml:lang="de">jährlich</skos:prefLabel>
      <skos:prefLabel xml:lang="fr">annuel</skos:prefLabel>
      <skos:definition xml:lang="de">Eine Erscheinungsfrequenz für eine Manifestation, die einmal pro Jahr erscheint oder aktualisiert wird.</skos:definition>
      <skos:definition xml:lang="fr">Périodicité d’une manifestation publiée ou mise à jour une fois par année.</skos:definition>
      <skos:prefLabel xml:lang="es">anual</skos:prefLabel>
      <skos:definition xml:lang="es">Frecuencia de un recurso publicado o actualizado una vez cada año.</skos:definition>
      <rdakit:toolkitLabel xml:lang="en">annual</rdakit:toolkitLabel>
      <rdakit:toolkitLabel xml:lang="fr">annuel</rdakit:toolkitLabel>
      <rdakit:toolkitDefinition xml:lang="en">A frequency for a manifestation issued or updated once every year.</rdakit:toolkitDefinition>
      <rdakit:toolkitDefinition xml:lang="fr">Périodicité d’une manifestation publiée ou mise à jour une fois par année.</rdakit:toolkitDefinition>
      <rdakit:toolkitLabel xml:lang="es">anual</rdakit:toolkitLabel>
      <rdakit:toolkitDefinition xml:lang="es">Frecuencia de un recurso publicado o actualizado una vez cada año.</rdakit:toolkitDefinition>
      <skos:prefLabel xml:lang="zh">每年</skos:prefLabel>
      <rdakit:toolkitLabel xml:lang="zh">每年</rdakit:toolkitLabel>
      <skos:definition xml:lang="zh">资源的发行或更新频率为每年一次。</skos:definition>
      <rdakit:toolkitDefinition xml:lang="zh">资源的发行或更新频率为每年一次。</rdakit:toolkitDefinition>
      <skos:prefLabel xml:lang="nl">jaarlijks</skos:prefLabel>
      <rdakit:toolkitLabel xml:lang="nl">jaarlijks</rdakit:toolkitLabel>
      <skos:definition xml:lang="nl">Frequentie voor een resource die eens per jaar uitgegeven of bijgewerkt wordt.</skos:definition>
      <rdakit:toolkitDefinition xml:lang="nl">Frequentie voor een resource die eens per jaar uitgegeven of bijgewerkt wordt.</rdakit:toolkitDefinition>
      <rdakit:toolkitLabel xml:lang="de">jährlich</rdakit:toolkitLabel>
      <rdakit:toolkitDefinition xml:lang="de">Eine Erscheinungsfrequenz für eine Manifestation, die einmal pro Jahr erscheint oder aktualisiert wird.</rdakit:toolkitDefinition>
      <skos:prefLabel xml:lang="it">annuale</skos:prefLabel>
      <rdakit:toolkitLabel xml:lang="it">annuale</rdakit:toolkitLabel>
      <skos:prefLabel xml:lang="fi">vuosittain</skos:prefLabel>
      <rdakit:toolkitLabel xml:lang="fi">vuosittain</rdakit:toolkitLabel>
      <skos:prefLabel xml:lang="ar">سنوي</skos:prefLabel>
      <skos:prefLabel xml:lang="da">årlig</skos:prefLabel>
      <rdakit:toolkitLabel xml:lang="da">årlig</rdakit:toolkitLabel>
      <skos:definition xml:lang="da">Frekvens for en ressource, der udgives eller opdateres en gang om året.</skos:definition>
      <rdakit:toolkitDefinition xml:lang="da">Frekvens for en ressource, der udgives eller opdateres en gang om året.</rdakit:toolkitDefinition>
      <skos:prefLabel xml:lang="ca">anual</skos:prefLabel>
      <rdakit:toolkitLabel xml:lang="ca">anual</rdakit:toolkitLabel>
      <skos:definition xml:lang="ca">Periodicitat d’una manifestació que es publica o s’actualitza una vegada cada any.</skos:definition>
      <rdakit:toolkitDefinition xml:lang="ca">Periodicitat d’una manifestació que es publica o s’actualitza una vegada cada any.</rdakit:toolkitDefinition>
      <skos:prefLabel xml:lang="vi">hàng năm</skos:prefLabel>
      <rdakit:toolkitLabel xml:lang="vi">hàng năm</rdakit:toolkitLabel>
      <skos:definition xml:lang="vi">Tần số của biểu thị được công bố hoặc cập nhật một lần mỗi năm.</skos:definition>
      <rdakit:toolkitDefinition xml:lang="vi">Tần số của biểu thị được công bố hoặc cập nhật một lần mỗi năm.</rdakit:toolkitDefinition>
      <skos:definition xml:lang="fi">Ilmestymis- tai päivittymistiheys aineistolle, joka ilmestyy tai päivittyy kerran vuodessa.</skos:definition>
      <rdakit:toolkitDefinition xml:lang="fi">Ilmestymis- tai päivittymistiheys aineistolle, joka ilmestyy tai päivittyy kerran vuodessa.</rdakit:toolkitDefinition>
      <skos:prefLabel xml:lang="no">årlig</skos:prefLabel>
      <rdakit:toolkitLabel xml:lang="no">årlig</rdakit:toolkitLabel>
      <skos:definition xml:lang="no">En frekvens for en manifestasjon som blir utgitt eller oppdatert en gang hvert år.</skos:definition>
      <rdakit:toolkitDefinition xml:lang="no">En frekvens for en manifestasjon som blir utgitt eller oppdatert en gang hvert år.</rdakit:toolkitDefinition>
    </skos:Concept>
<!-- Concept: biennial  -->
    <skos:Concept rdf:about="http://rdaregistry.info/termList/frequency/1014" xml:lang="en">
      <skos:inScheme rdf:resource="http://rdaregistry.info/termList/frequency"/>
      <reg:status rdf:resource="http://metadataregistry.org/uri/RegStatus/1001"/>
      <reg:identifier rdf:resource="http://metadataregistry.org/concepts/758"/>
      <skos:prefLabel xml:lang="en">biennial</skos:prefLabel>
      <skos:definition xml:lang="en">A frequency for a manifestation issued or updated once every two years.</skos:definition>
      <skos:prefLabel xml:lang="de">alle zwei Jahre</skos:prefLabel>
      <skos:prefLabel xml:lang="fr">biennal</skos:prefLabel>
      <skos:definition xml:lang="de">Eine Erscheinungsfrequenz für eine Manifestation, die alle zwei Jahre erscheint oder aktualisiert wird.</skos:definition>
      <skos:definition xml:lang="fr">Périodicité d’une manifestation publiée ou mise à jour tous les deux ans.</skos:definition>
      <skos:definition xml:lang="es">Frecuencia de un recurso publicado o actualizado una vez cada dos años.</skos:definition>
      <skos:prefLabel xml:lang="es">bienal</skos:prefLabel>
      <rdakit:toolkitLabel xml:lang="en">biennial</rdakit:toolkitLabel>
      <rdakit:toolkitLabel xml:lang="fr">biennal</rdakit:toolkitLabel>
      <rdakit:toolkitDefinition xml:lang="en">A frequency for a manifestation issued or updated once every two years.</rdakit:toolkitDefinition>
      <rdakit:toolkitDefinition xml:lang="fr">Périodicité d’une manifestation publiée ou mise à jour tous les deux ans.</rdakit:toolkitDefinition>
      <rdakit:toolkitLabel xml:lang="es">bienal</rdakit:toolkitLabel>
      <rdakit:toolkitDefinition xml:lang="es">Frecuencia de un recurso publicado o actualizado una vez cada dos años.</rdakit:toolkitDefinition>
      <skos:prefLabel xml:lang="zh">双年</skos:prefLabel>
      <rdakit:toolkitLabel xml:lang="zh">双年</rdakit:toolkitLabel>
      <skos:definition xml:lang="zh">资源的发行或更新频率为每两年一次。</skos:definition>
      <rdakit:toolkitDefinition xml:lang="zh">资源的发行或更新频率为每两年一次。</rdakit:toolkitDefinition>
      <skos:prefLabel xml:lang="nl">eens per twee jaar</skos:prefLabel>
      <rdakit:toolkitLabel xml:lang="nl">eens per twee jaar</rdakit:toolkitLabel>
      <skos:definition xml:lang="nl">Frequentie voor een resource die eens in de twee jaar uitgegeven of bijgewerkt wordt.</skos:definition>
      <rdakit:toolkitDefinition xml:lang="nl">Frequentie voor een resource die eens in de twee jaar uitgegeven of bijgewerkt wordt.</rdakit:toolkitDefinition>
      <rdakit:toolkitLabel xml:lang="de">alle zwei Jahre</rdakit:toolkitLabel>
      <rdakit:toolkitDefinition xml:lang="de">Eine Erscheinungsfrequenz für eine Manifestation, die alle zwei Jahre erscheint oder aktualisiert wird.</rdakit:toolkitDefinition>
      <skos:prefLabel xml:lang="it">biennale</skos:prefLabel>
      <rdakit:toolkitLabel xml:lang="it">biennale</rdakit:toolkitLabel>
      <skos:prefLabel xml:lang="fi">kerran kahdessa vuodessa</skos:prefLabel>
      <rdakit:toolkitLabel xml:lang="fi">kerran kahdessa vuodessa</rdakit:toolkitLabel>
      <skos:prefLabel xml:lang="ar">مرة كل سنتين</skos:prefLabel>
      <skos:prefLabel xml:lang="sv">vartannat år</skos:prefLabel>
      <rdakit:toolkitLabel xml:lang="sv">vartannat år</rdakit:toolkitLabel>
      <skos:prefLabel xml:lang="da">hvert 2. år</skos:prefLabel>
      <rdakit:toolkitLabel xml:lang="da">hvert 2. år</rdakit:toolkitLabel>
      <skos:definition xml:lang="da">Frekvens for en ressource, der udgives eller opdateres hvert andet år.</skos:definition>
      <rdakit:toolkitDefinition xml:lang="da">Frekvens for en ressource, der udgives eller opdateres hvert andet år.</rdakit:toolkitDefinition>
      <skos:prefLabel xml:lang="ca">biennal</skos:prefLabel>
      <rdakit:toolkitLabel xml:lang="ca">biennal</rdakit:toolkitLabel>
      <skos:definition xml:lang="ca">Periodicitat d’una manifestació que es publica o s’actualitza cada dos anys.</skos:definition>
      <rdakit:toolkitDefinition xml:lang="ca">Periodicitat d’una manifestació que es publica o s’actualitza cada dos anys.</rdakit:toolkitDefinition>
      <skos:prefLabel xml:lang="vi">hàng hai năm</skos:prefLabel>
      <rdakit:toolkitLabel xml:lang="vi">hàng hai năm</rdakit:toolkitLabel>
      <skos:definition xml:lang="vi">Tần số của biểu thị được công bố hoặc cập nhật hai năm một lần.</skos:definition>
      <rdakit:toolkitDefinition xml:lang="vi">Tần số của biểu thị được công bố hoặc cập nhật hai năm một lần.</rdakit:toolkitDefinition>
      <skos:definition xml:lang="fi">Ilmestymis- tai päivittymistiheys aineistolle, joka ilmestyy tai päivittyy kerran kahdessa vuodessa.</skos:definition>
      <rdakit:toolkitDefinition xml:lang="fi">Ilmestymis- tai päivittymistiheys aineistolle, joka ilmestyy tai päivittyy kerran kahdessa vuodessa.</rdakit:toolkitDefinition>
      <skos:prefLabel xml:lang="no">hvert annet år</skos:prefLabel>
      <rdakit:toolkitLabel xml:lang="no">hvert annet år</rdakit:toolkitLabel>
      <skos:definition xml:lang="no">En frekvens for en manifestasjon som blir utgitt eller oppdatert en gang hvert annet år.</skos:definition>
      <rdakit:toolkitDefinition xml:lang="no">En frekvens for en manifestasjon som blir utgitt eller oppdatert en gang hvert annet år.</rdakit:toolkitDefinition>
    </skos:Concept>
<!-- Concept: bimonthly  -->
    <skos:Concept rdf:about="http://rdaregistry.info/termList/frequency/1007" xml:lang="en">
      <skos:inScheme rdf:resource="http://rdaregistry.info/termList/frequency"/>
      <reg:status rdf:resource="http://metadataregistry.org/uri/RegStatus/1001"/>
      <reg:identifier rdf:resource="http://metadataregistry.org/concepts/751"/>
      <skos:prefLabel xml:lang="en">bimonthly</skos:prefLabel>
      <skos:definition xml:lang="en">A frequency for a manifestation issued or updated once every two months.</skos:definition>
      <skos:prefLabel xml:lang="de">alle zwei Monate</skos:prefLabel>
      <skos:prefLabel xml:lang="fr">bimestriel</skos:prefLabel>
      <skos:definition xml:lang="de">Eine Erscheinungsfrequenz für eine Manifestation, die alle zwei Monate erscheint oder aktualisiert wird.</skos:definition>
      <skos:definition xml:lang="fr">Périodicité d’une manifestation publiée ou mise à jour tous les deux mois.</skos:definition>
      <skos:prefLabel xml:lang="es">bimestral</skos:prefLabel>
      <skos:definition xml:lang="es">Frecuencia de un recurso publicado o actualizado una vez cada dos meses.</skos:definition>
      <rdakit:toolkitLabel xml:lang="en">bimonthly</rdakit:toolkitLabel>
      <rdakit:toolkitLabel xml:lang="fr">bimestriel</rdakit:toolkitLabel>
      <rdakit:toolkitDefinition xml:lang="en">A frequency for a manifestation issued or updated once every two months.</rdakit:toolkitDefinition>
      <rdakit:toolkitDefinition xml:lang="fr">Périodicité d’une manifestation publiée ou mise à jour tous les deux mois.</rdakit:toolkitDefinition>
      <rdakit:toolkitLabel xml:lang="es">bimestral</rdakit:toolkitLabel>
      <rdakit:toolkitDefinition xml:lang="es">Frecuencia de un recurso publicado o actualizado una vez cada dos meses.</rdakit:toolkitDefinition>
      <skos:prefLabel xml:lang="zh">双月</skos:prefLabel>
      <rdakit:toolkitLabel xml:lang="zh">双月</rdakit:toolkitLabel>
      <skos:definition xml:lang="zh">资源的发行或更新频率为每两月一次。</skos:definition>
      <rdakit:toolkitDefinition xml:lang="zh">资源的发行或更新频率为每两月一次。</rdakit:toolkitDefinition>
      <skos:prefLabel xml:lang="nl">eens per twee maanden</skos:prefLabel>
      <rdakit:toolkitLabel xml:lang="nl">eens per twee maanden</rdakit:toolkitLabel>
      <skos:definition xml:lang="nl">Frequentie voor een resource die eens in de twee maanden uitgegeven of bijgewerkt wordt.</skos:definition>
      <rdakit:toolkitDefinition xml:lang="nl">Frequentie voor een resource die eens in de twee maanden uitgegeven of bijgewerkt wordt.</rdakit:toolkitDefinition>
      <rdakit:toolkitLabel xml:lang="de">alle zwei Monate</rdakit:toolkitLabel>
      <rdakit:toolkitDefinition xml:lang="de">Eine Erscheinungsfrequenz für eine Manifestation, die alle zwei Monate erscheint oder aktualisiert wird.</rdakit:toolkitDefinition>
      <skos:prefLabel xml:lang="it">bimensile</skos:prefLabel>
      <rdakit:toolkitLabel xml:lang="it">bimensile</rdakit:toolkitLabel>
      <skos:prefLabel xml:lang="fi">kerran kahdessa kuukaudessa</skos:prefLabel>
      <rdakit:toolkitLabel xml:lang="fi">kerran kahdessa kuukaudessa</rdakit:toolkitLabel>
      <skos:prefLabel xml:lang="ar">كل شهرين</skos:prefLabel>
      <skos:prefLabel xml:lang="sv">varannan månad</skos:prefLabel>
      <rdakit:toolkitLabel xml:lang="sv">varannan månad</rdakit:toolkitLabel>
      <skos:prefLabel xml:lang="da">hver 2. måned</skos:prefLabel>
      <rdakit:toolkitLabel xml:lang="da">hver 2. måned</rdakit:toolkitLabel>
      <skos:definition xml:lang="da">Frekvens for en ressource, der udgives eller opdateres hver anden måned.</skos:definition>
      <rdakit:toolkitDefinition xml:lang="da">Frekvens for en ressource, der udgives eller opdateres hver anden måned.</rdakit:toolkitDefinition>
      <skos:prefLabel xml:lang="ca">bimestral</skos:prefLabel>
      <rdakit:toolkitLabel xml:lang="ca">bimestral</rdakit:toolkitLabel>
      <skos:definition xml:lang="ca">Periodicitat d’una manifestació que es publica o s’actualitza cada dos mesos.</skos:definition>
      <rdakit:toolkitDefinition xml:lang="ca">Periodicitat d’una manifestació que es publica o s’actualitza cada dos mesos.</rdakit:toolkitDefinition>
      <skos:prefLabel xml:lang="vi">hàng hai tháng</skos:prefLabel>
      <rdakit:toolkitLabel xml:lang="vi">hàng hai tháng</rdakit:toolkitLabel>
      <skos:definition xml:lang="vi">Tần số của biểu thị được công bố hoặc cập nhật hai tháng một lần.</skos:definition>
      <rdakit:toolkitDefinition xml:lang="vi">Tần số của biểu thị được công bố hoặc cập nhật hai tháng một lần.</rdakit:toolkitDefinition>
      <skos:definition xml:lang="fi">Ilmestymis- tai päivittymistiheys aineistolle, joka ilmestyy tai päivittyy kerran kahdessa kuukaudessa.</skos:definition>
      <rdakit:toolkitDefinition xml:lang="fi">Ilmestymis- tai päivittymistiheys aineistolle, joka ilmestyy tai päivittyy kerran kahdessa kuukaudessa.</rdakit:toolkitDefinition>
      <skos:prefLabel xml:lang="no">hver annen måned</skos:prefLabel>
      <rdakit:toolkitLabel xml:lang="no">hver annen måned</rdakit:toolkitLabel>
      <skos:definition xml:lang="no">En frekvens for en manifestasjon som blir utgitt eller oppdatert en gang hver annen måned.</skos:definition>
      <rdakit:toolkitDefinition xml:lang="no">En frekvens for en manifestasjon som blir utgitt eller oppdatert en gang hver annen måned.</rdakit:toolkitDefinition>
    </skos:Concept>
<!-- Concept: biweekly  -->
    <skos:Concept rdf:about="http://rdaregistry.info/termList/frequency/1003" xml:lang="en">
      <skos:inScheme rdf:resource="http://rdaregistry.info/termList/frequency"/>
      <reg:status rdf:resource="http://metadataregistry.org/uri/RegStatus/1001"/>
      <reg:identifier rdf:resource="http://metadataregistry.org/concepts/747"/>
      <skos:prefLabel xml:lang="en">biweekly</skos:prefLabel>
      <skos:definition xml:lang="en">A frequency for a manifestation issued or updated once every two weeks.</skos:definition>
      <skos:altLabel xml:lang="en">fortnightly</skos:altLabel>
      <skos:prefLabel xml:lang="de">alle zwei Wochen</skos:prefLabel>
      <skos:prefLabel xml:lang="fr">toutes les deux semaines</skos:prefLabel>
      <skos:definition xml:lang="de">Eine Erscheinungsfrequenz für eine Manifestation, die einmal alle zwei Wochen erscheint oder aktualisiert wird.</skos:definition>
      <skos:altLabel xml:lang="de">vierzehntäglich</skos:altLabel>
      <skos:definition xml:lang="fr">Périodicité d’une manifestation publiée ou mise à jour toutes les deux semaines.</skos:definition>
      <skos:altLabel xml:lang="fr">tous les quinze jours</skos:altLabel>
      <skos:prefLabel xml:lang="es">bisemanal</skos:prefLabel>
      <rdakit:toolkitLabel xml:lang="en">biweekly</rdakit:toolkitLabel>
      <rdakit:toolkitLabel xml:lang="fr">toutes les deux semaines</rdakit:toolkitLabel>
      <rdakit:toolkitDefinition xml:lang="en">A frequency for a manifestation issued or updated once every two weeks.</rdakit:toolkitDefinition>
      <rdakit:toolkitDefinition xml:lang="fr">Périodicité d’une manifestation publiée ou mise à jour toutes les deux semaines.</rdakit:toolkitDefinition>
      <rdakit:toolkitLabel xml:lang="es">bisemanal</rdakit:toolkitLabel>
      <skos:prefLabel xml:lang="zh">双周</skos:prefLabel>
      <skos:altLabel xml:lang="zh">隔周发行</skos:altLabel>
      <rdakit:toolkitLabel xml:lang="zh">双周</rdakit:toolkitLabel>
      <skos:definition xml:lang="zh">资源的发行或更新频率为每两周一次。</skos:definition>
      <rdakit:toolkitDefinition xml:lang="zh">资源的发行或更新频率为每两周一次。</rdakit:toolkitDefinition>
      <skos:scopeNote xml:lang="zh">用于：隔周发行</skos:scopeNote>
      <skos:altLabel xml:lang="es">quincenal</skos:altLabel>
      <skos:definition xml:lang="es">Frecuencia de un recurso publicado o actualizado una vez cada dos semanas.</skos:definition>
      <rdakit:toolkitDefinition xml:lang="es">Frecuencia de un recurso publicado o actualizado una vez cada dos semanas.</rdakit:toolkitDefinition>
      <skos:prefLabel xml:lang="nl">eens per twee weken</skos:prefLabel>
      <rdakit:toolkitLabel xml:lang="nl">eens per twee weken</rdakit:toolkitLabel>
      <skos:definition xml:lang="nl">Frequentie voor een resource die eens per twee weken uitgegeven of bijgewerkt wordt.</skos:definition>
      <rdakit:toolkitDefinition xml:lang="nl">Frequentie voor een resource die eens per twee weken uitgegeven of bijgewerkt wordt.</rdakit:toolkitDefinition>
      <rdakit:toolkitLabel xml:lang="de">alle zwei Wochen</rdakit:toolkitLabel>
      <rdakit:toolkitDefinition xml:lang="de">Eine Erscheinungsfrequenz für eine Manifestation, die einmal alle zwei Wochen erscheint oder aktualisiert wird.</rdakit:toolkitDefinition>
      <skos:prefLabel xml:lang="it">ogni due settimane</skos:prefLabel>
      <rdakit:toolkitLabel xml:lang="it">ogni due settimane</rdakit:toolkitLabel>
      <skos:prefLabel xml:lang="fi">kerran kahdessa viikossa</skos:prefLabel>
      <rdakit:toolkitLabel xml:lang="fi">kerran kahdessa viikossa</rdakit:toolkitLabel>
      <skos:prefLabel xml:lang="ar">كل أسبوعين</skos:prefLabel>
      <skos:prefLabel xml:lang="sv">varannan vecka</skos:prefLabel>
      <rdakit:toolkitLabel xml:lang="sv">varannan vecka</rdakit:toolkitLabel>
      <skos:prefLabel xml:lang="da">hver 2. uge</skos:prefLabel>
      <rdakit:toolkitLabel xml:lang="da">hver 2. uge</rdakit:toolkitLabel>
      <skos:definition xml:lang="da">Frekvens for en ressource, der udgives eller opdateres hver anden uge.</skos:definition>
      <rdakit:toolkitDefinition xml:lang="da">Frekvens for en ressource, der udgives eller opdateres hver anden uge.</rdakit:toolkitDefinition>
      <skos:prefLabel xml:lang="ca">quinzenal</skos:prefLabel>
      <rdakit:toolkitLabel xml:lang="ca">quinzenal</rdakit:toolkitLabel>
      <skos:definition xml:lang="ca">Periodicitat d’una manifestació que es publica o s’actualitza cada dues setmanes.</skos:definition>
      <rdakit:toolkitDefinition xml:lang="ca">Periodicitat d’una manifestació que es publica o s’actualitza cada dues setmanes.</rdakit:toolkitDefinition>
      <skos:prefLabel xml:lang="vi">hàng hai tuần</skos:prefLabel>
      <skos:altLabel xml:lang="vi">hai tuần một lần</skos:altLabel>
      <rdakit:toolkitLabel xml:lang="vi">hàng hai tuần</rdakit:toolkitLabel>
      <skos:definition xml:lang="vi">Tần số cho mộtbiểu thị được công bốhoặc cập nhậthai tuần một lần.</skos:definition>
      <rdakit:toolkitDefinition xml:lang="vi">Tần số cho mộtbiểu thị được công bốhoặc cập nhậthai tuần một lần.</rdakit:toolkitDefinition>
      <skos:definition xml:lang="fi">Ilmestymis- tai päivittymistiheys aineistolle, joka ilmestyy tai päivittyy kerran kahdessa viikossa.</skos:definition>
      <rdakit:toolkitDefinition xml:lang="fi">Ilmestymis- tai päivittymistiheys aineistolle, joka ilmestyy tai päivittyy kerran kahdessa viikossa.</rdakit:toolkitDefinition>
      <skos:prefLabel xml:lang="no">hver annen uke</skos:prefLabel>
      <skos:altLabel xml:lang="no">hver 14. dag</skos:altLabel>
      <rdakit:toolkitLabel xml:lang="no">hver annen uke</rdakit:toolkitLabel>
      <skos:definition xml:lang="no">En frekvens for en manifestasjon som blir utgitt eller oppdatert en gang hver annen uke.</skos:definition>
      <rdakit:toolkitDefinition xml:lang="no">En frekvens for en manifestasjon som blir utgitt eller oppdatert en gang hver annen uke.</rdakit:toolkitDefinition>
    </skos:Concept>
<!-- Concept: daily  -->
    <skos:Concept rdf:about="http://rdaregistry.info/termList/frequency/1001" xml:lang="en">
      <skos:inScheme rdf:resource="http://rdaregistry.info/termList/frequency"/>
      <reg:status rdf:resource="http://metadataregistry.org/uri/RegStatus/1001"/>
      <reg:identifier rdf:resource="http://metadataregistry.org/concepts/745"/>
      <skos:prefLabel xml:lang="en">daily</skos:prefLabel>
      <skos:definition xml:lang="en">A frequency for a manifestation issued or updated once every day, usually exclusive of nonworking days.</skos:definition>
      <skos:prefLabel xml:lang="de">täglich</skos:prefLabel>
      <skos:prefLabel xml:lang="fr">quotidien</skos:prefLabel>
      <skos:definition xml:lang="de">Eine Erscheinungsfrequenz für eine Manifestation, die jeden Tag erscheint oder aktualisiert wird, normalerweise nicht an Tagen, die keine Arbeitstage sind.</skos:definition>
      <skos:definition xml:lang="fr">Périodicité d’une manifestation publiée ou mise à jour une fois par jour, habituellement à l’exclusion des jours non ouvrables.</skos:definition>
      <skos:prefLabel xml:lang="es">diario</skos:prefLabel>
      <skos:definition xml:lang="es">Frecuencia de un recurso publicado o actualizado una vez cada día, generalmente exclusivo de días no laborables.</skos:definition>
      <rdakit:toolkitLabel xml:lang="en">daily</rdakit:toolkitLabel>
      <rdakit:toolkitLabel xml:lang="fr">quotidien</rdakit:toolkitLabel>
      <rdakit:toolkitDefinition xml:lang="en">A frequency for a manifestation issued or updated once every day, usually exclusive of nonworking days.</rdakit:toolkitDefinition>
      <rdakit:toolkitDefinition xml:lang="fr">Périodicité d’une manifestation publiée ou mise à jour une fois par jour, habituellement à l’exclusion des jours non ouvrables.</rdakit:toolkitDefinition>
      <rdakit:toolkitLabel xml:lang="es">diario</rdakit:toolkitLabel>
      <rdakit:toolkitDefinition xml:lang="es">Frecuencia de un recurso publicado o actualizado una vez cada día, generalmente exclusivo de días no laborables.</rdakit:toolkitDefinition>
      <skos:prefLabel xml:lang="zh">每日</skos:prefLabel>
      <rdakit:toolkitLabel xml:lang="zh">每日</rdakit:toolkitLabel>
      <skos:definition xml:lang="zh">资源的发行或更新频率为每天一次，通常不包括非工作日。</skos:definition>
      <rdakit:toolkitDefinition xml:lang="zh">资源的发行或更新频率为每天一次，通常不包括非工作日。</rdakit:toolkitDefinition>
      <skos:prefLabel xml:lang="nl">dagelijks</skos:prefLabel>
      <rdakit:toolkitLabel xml:lang="nl">dagelijks</rdakit:toolkitLabel>
      <skos:definition xml:lang="nl">Frequentie voor een resource die elke dag uitgegeven of bijgewerkt wordt, meestal uitgezonderd dagen waarop niet gewerkt wordt.</skos:definition>
      <rdakit:toolkitDefinition xml:lang="nl">Frequentie voor een resource die elke dag uitgegeven of bijgewerkt wordt, meestal uitgezonderd dagen waarop niet gewerkt wordt.</rdakit:toolkitDefinition>
      <rdakit:toolkitLabel xml:lang="de">täglich</rdakit:toolkitLabel>
      <rdakit:toolkitDefinition xml:lang="de">Eine Erscheinungsfrequenz für eine Manifestation, die jeden Tag erscheint oder aktualisiert wird, normalerweise nicht an Tagen, die keine Arbeitstage sind.</rdakit:toolkitDefinition>
      <skos:prefLabel xml:lang="it">quotidiano</skos:prefLabel>
      <rdakit:toolkitLabel xml:lang="it">quotidiano</rdakit:toolkitLabel>
      <skos:prefLabel xml:lang="fi">päivittäin</skos:prefLabel>
      <rdakit:toolkitLabel xml:lang="fi">päivittäin</rdakit:toolkitLabel>
      <skos:prefLabel xml:lang="ar">يوميا</skos:prefLabel>
      <skos:prefLabel xml:lang="sv">daglig</skos:prefLabel>
      <rdakit:toolkitLabel xml:lang="sv">daglig</rdakit:toolkitLabel>
      <skos:prefLabel xml:lang="da">daglig</skos:prefLabel>
      <rdakit:toolkitLabel xml:lang="da">daglig</rdakit:toolkitLabel>
      <skos:definition xml:lang="da">Frekvens for en manifestation, der udgives eller opdateres hver dag, normalt med undtagelse af søn- og helligdage</skos:definition>
      <rdakit:toolkitDefinition xml:lang="da">Frekvens for en manifestation, der udgives eller opdateres hver dag, normalt med undtagelse af søn- og helligdage</rdakit:toolkitDefinition>
      <skos:prefLabel xml:lang="ca">diari</skos:prefLabel>
      <rdakit:toolkitLabel xml:lang="ca">diari</rdakit:toolkitLabel>
      <skos:definition xml:lang="ca">Periodicitat d’una manifestació que es publica o s’actualitza una vegada cada dia, normalment exclosos els dies no laborables.</skos:definition>
      <rdakit:toolkitDefinition xml:lang="ca">Periodicitat d’una manifestació que es publica o s’actualitza una vegada cada dia, normalment exclosos els dies no laborables.</rdakit:toolkitDefinition>
      <skos:prefLabel xml:lang="vi">hàng ngày</skos:prefLabel>
      <rdakit:toolkitLabel xml:lang="vi">hàng ngày</rdakit:toolkitLabel>
      <skos:definition xml:lang="vi">Tần số của biểu thị được công bố hoặc cập nhật mỗi ngày, thường không bao gồm không làm việc.</skos:definition>
      <rdakit:toolkitDefinition xml:lang="vi">Tần số của biểu thị được công bố hoặc cập nhật mỗi ngày, thường không bao gồm không làm việc.</rdakit:toolkitDefinition>
      <skos:altLabel xml:lang="fi">joka päivä</skos:altLabel>
      <skos:definition xml:lang="fi">Ilmestymis- tai päivittymistiheys aineistolle, joka ilmestyy tai päivittyy kerran päivässä, yleensä arkipäivisin.</skos:definition>
      <rdakit:toolkitDefinition xml:lang="fi">Ilmestymis- tai päivittymistiheys aineistolle, joka ilmestyy tai päivittyy kerran päivässä, yleensä arkipäivisin.</rdakit:toolkitDefinition>
      <skos:prefLabel xml:lang="no">daglig</skos:prefLabel>
      <rdakit:toolkitLabel xml:lang="no">daglig</rdakit:toolkitLabel>
      <skos:definition xml:lang="no">Frekvens for en manifestasjon som blir utgitt eller oppdatert hver dag, vanligvis bare på arbeidsdager.</skos:definition>
      <rdakit:toolkitDefinition xml:lang="no">Frekvens for en manifestasjon som blir utgitt eller oppdatert hver dag, vanligvis bare på arbeidsdager.</rdakit:toolkitDefinition>
    </skos:Concept>
<!-- Concept: irregular  -->
    <skos:Concept rdf:about="http://rdaregistry.info/termList/frequency/1016" xml:lang="en">
      <skos:inScheme rdf:resource="http://rdaregistry.info/termList/frequency"/>
      <reg:status rdf:resource="http://metadataregistry.org/uri/RegStatus/1001"/>
      <reg:identifier rdf:resource="http://metadataregistry.org/concepts/760"/>
      <skos:prefLabel xml:lang="en">irregular</skos:prefLabel>
      <skos:definition xml:lang="en">A frequency for a manifestation issued with no consistent interval between issues.</skos:definition>
      <skos:prefLabel xml:lang="de">unregelmäßig</skos:prefLabel>
      <skos:prefLabel xml:lang="fr">irrégulier</skos:prefLabel>
      <skos:definition xml:lang="de">Eine Erscheinungsfrequenz für eine Manifestation, die ohne einheitliches Intervall zwischen den Ausgaben erscheint oder aktualisiert wird.</skos:definition>
      <skos:definition xml:lang="fr">Périodicité d’une manifestation publiée à intervalles irréguliers.</skos:definition>
      <skos:definition xml:lang="es">Frecuencia de un recurso publicado sin intervalos consistentes entre entregas.</skos:definition>
      <skos:prefLabel xml:lang="es">irregular</skos:prefLabel>
      <rdakit:toolkitLabel xml:lang="en">irregular</rdakit:toolkitLabel>
      <rdakit:toolkitLabel xml:lang="fr">irrégulier</rdakit:toolkitLabel>
      <rdakit:toolkitDefinition xml:lang="en">A frequency for a manifestation issued with no consistent interval between issues.</rdakit:toolkitDefinition>
      <rdakit:toolkitDefinition xml:lang="fr">Périodicité d’une manifestation publiée à intervalles irréguliers.</rdakit:toolkitDefinition>
      <rdakit:toolkitLabel xml:lang="es">irregular</rdakit:toolkitLabel>
      <rdakit:toolkitDefinition xml:lang="es">Frecuencia de un recurso publicado sin intervalos consistentes entre entregas.</rdakit:toolkitDefinition>
      <skos:prefLabel xml:lang="zh">不定期</skos:prefLabel>
      <rdakit:toolkitLabel xml:lang="zh">不定期</rdakit:toolkitLabel>
      <skos:definition xml:lang="zh">资源发行的频率不规律。</skos:definition>
      <rdakit:toolkitDefinition xml:lang="zh">资源发行的频率不规律。</rdakit:toolkitDefinition>
      <skos:prefLabel xml:lang="nl">onregelmatig</skos:prefLabel>
      <rdakit:toolkitLabel xml:lang="nl">onregelmatig</rdakit:toolkitLabel>
      <skos:definition xml:lang="nl">Frequentie voor een resource uitgegeven zonder vast interval tussen de nummers.</skos:definition>
      <rdakit:toolkitDefinition xml:lang="nl">Frequentie voor een resource uitgegeven zonder vast interval tussen de nummers.</rdakit:toolkitDefinition>
      <rdakit:toolkitLabel xml:lang="de">unregelmäßig</rdakit:toolkitLabel>
      <rdakit:toolkitDefinition xml:lang="de">Eine Erscheinungsfrequenz für eine Manifestation, die ohne einheitliches Intervall zwischen den Ausgaben erscheint oder aktualisiert wird.</rdakit:toolkitDefinition>
      <skos:prefLabel xml:lang="it">irregolare</skos:prefLabel>
      <rdakit:toolkitLabel xml:lang="it">irregolare</rdakit:toolkitLabel>
      <skos:prefLabel xml:lang="fi">epäsäännöllinen</skos:prefLabel>
      <rdakit:toolkitLabel xml:lang="fi">epäsäännöllinen</rdakit:toolkitLabel>
      <skos:prefLabel xml:lang="ar">غير منتظم</skos:prefLabel>
      <skos:prefLabel xml:lang="sv">oregelbunden</skos:prefLabel>
      <rdakit:toolkitLabel xml:lang="sv">oregelbunden</rdakit:toolkitLabel>
      <skos:prefLabel xml:lang="da">uregelmæssig</skos:prefLabel>
      <rdakit:toolkitLabel xml:lang="da">uregelmæssig</rdakit:toolkitLabel>
      <skos:definition xml:lang="da">Frekvens for en ressource, der udgives uden konsekvent interval mellem numre.</skos:definition>
      <rdakit:toolkitDefinition xml:lang="da">Frekvens for en ressource, der udgives uden konsekvent interval mellem numre.</rdakit:toolkitDefinition>
      <skos:prefLabel xml:lang="ca">irregular</skos:prefLabel>
      <rdakit:toolkitLabel xml:lang="ca">irregular</rdakit:toolkitLabel>
      <skos:definition xml:lang="ca">Periodicitat d’una manifestació que es publica a intervals entre números que no són constants.</skos:definition>
      <rdakit:toolkitDefinition xml:lang="ca">Periodicitat d’una manifestació que es publica a intervals entre números que no són constants.</rdakit:toolkitDefinition>
      <skos:prefLabel xml:lang="vi">bất thường</skos:prefLabel>
      <rdakit:toolkitLabel xml:lang="vi">bất thường</rdakit:toolkitLabel>
      <skos:definition xml:lang="vi">Tần số của biểu thị được công bố không có khoảng thời gian cố định giữa các số.</skos:definition>
      <rdakit:toolkitDefinition xml:lang="vi">Tần số của biểu thị được công bố không có khoảng thời gian cố định giữa các số.</rdakit:toolkitDefinition>
      <skos:definition xml:lang="fi">Ilmestymis- tai päivittymistiheys aineistolle, joka ilmestyy tai päivittyy epäsäännöllisesti.</skos:definition>
      <rdakit:toolkitDefinition xml:lang="fi">Ilmestymis- tai päivittymistiheys aineistolle, joka ilmestyy tai päivittyy epäsäännöllisesti.</rdakit:toolkitDefinition>
      <skos:prefLabel xml:lang="no">uregelmessig</skos:prefLabel>
      <rdakit:toolkitLabel xml:lang="no">uregelmessig</rdakit:toolkitLabel>
      <skos:definition xml:lang="no">En frekvens for en manifestasjon utgitt uten faste intervaller mellom heftene.</skos:definition>
      <rdakit:toolkitDefinition xml:lang="no">En frekvens for en manifestasjon utgitt uten faste intervaller mellom heftene.</rdakit:toolkitDefinition>
    </skos:Concept>
<!-- Concept: monthly  -->
    <skos:Concept rdf:about="http://rdaregistry.info/termList/frequency/1008" xml:lang="en">
      <skos:inScheme rdf:resource="http://rdaregistry.info/termList/frequency"/>
      <reg:status rdf:resource="http://metadataregistry.org/uri/RegStatus/1001"/>
      <reg:identifier rdf:resource="http://metadataregistry.org/concepts/752"/>
      <skos:prefLabel xml:lang="en">monthly</skos:prefLabel>
      <skos:definition xml:lang="en">A frequency for a manifestation issued or updated once every month.</skos:definition>
      <skos:prefLabel xml:lang="de">monatlich</skos:prefLabel>
      <skos:prefLabel xml:lang="fr">mensuel</skos:prefLabel>
      <skos:definition xml:lang="de">Eine Erscheinungsfrequenz für eine Manifestation, die einmal pro Monat erscheint oder aktualisiert wird.</skos:definition>
      <skos:definition xml:lang="fr">Périodicité d’une manifestation publiée ou mise à jour une fois par mois.</skos:definition>
      <skos:prefLabel xml:lang="es">mensual</skos:prefLabel>
      <skos:definition xml:lang="es">Frecuencia de un recurso publicado o actualizado una vez al mes.</skos:definition>
      <rdakit:toolkitLabel xml:lang="en">monthly</rdakit:toolkitLabel>
      <rdakit:toolkitLabel xml:lang="fr">mensuel</rdakit:toolkitLabel>
      <rdakit:toolkitDefinition xml:lang="en">A frequency for a manifestation issued or updated once every month.</rdakit:toolkitDefinition>
      <rdakit:toolkitDefinition xml:lang="fr">Périodicité d’une manifestation publiée ou mise à jour une fois par mois.</rdakit:toolkitDefinition>
      <rdakit:toolkitLabel xml:lang="es">mensual</rdakit:toolkitLabel>
      <rdakit:toolkitDefinition xml:lang="es">Frecuencia de un recurso publicado o actualizado una vez al mes.</rdakit:toolkitDefinition>
      <skos:prefLabel xml:lang="zh">每月</skos:prefLabel>
      <rdakit:toolkitLabel xml:lang="zh">每月</rdakit:toolkitLabel>
      <skos:definition xml:lang="zh">资源的发行或更新频率为每月一次。</skos:definition>
      <rdakit:toolkitDefinition xml:lang="zh">资源的发行或更新频率为每月一次。</rdakit:toolkitDefinition>
      <skos:prefLabel xml:lang="nl">maandelijks</skos:prefLabel>
      <rdakit:toolkitLabel xml:lang="nl">maandelijks</rdakit:toolkitLabel>
      <skos:definition xml:lang="nl">Frequentie voor een resource die eens per maand uitgegeven of bijgewerkt wordt.</skos:definition>
      <rdakit:toolkitDefinition xml:lang="nl">Frequentie voor een resource die eens per maand uitgegeven of bijgewerkt wordt.</rdakit:toolkitDefinition>
      <rdakit:toolkitLabel xml:lang="de">monatlich</rdakit:toolkitLabel>
      <rdakit:toolkitDefinition xml:lang="de">Eine Erscheinungsfrequenz für eine Manifestation, die einmal pro Monat erscheint oder aktualisiert wird.</rdakit:toolkitDefinition>
      <skos:prefLabel xml:lang="it">mensile</skos:prefLabel>
      <rdakit:toolkitLabel xml:lang="it">mensile</rdakit:toolkitLabel>
      <skos:prefLabel xml:lang="fi">kuukausittain</skos:prefLabel>
      <rdakit:toolkitLabel xml:lang="fi">kuukausittain</rdakit:toolkitLabel>
      <skos:prefLabel xml:lang="ar">شهري</skos:prefLabel>
      <skos:prefLabel xml:lang="sv">1 nr/månad</skos:prefLabel>
      <rdakit:toolkitLabel xml:lang="sv">1 nr/månad</rdakit:toolkitLabel>
      <skos:prefLabel xml:lang="da">månedlig</skos:prefLabel>
      <rdakit:toolkitLabel xml:lang="da">månedlig</rdakit:toolkitLabel>
      <skos:definition xml:lang="da">Frekvens for en ressource, der udgives eller opdateres hver måned.</skos:definition>
      <rdakit:toolkitDefinition xml:lang="da">Frekvens for en ressource, der udgives eller opdateres hver måned.</rdakit:toolkitDefinition>
      <skos:prefLabel xml:lang="ca">mensual</skos:prefLabel>
      <rdakit:toolkitLabel xml:lang="ca">mensual</rdakit:toolkitLabel>
      <skos:definition xml:lang="ca">Periodicitat d’una manifestació que es publica o s’actualitza una vegada cada mes.</skos:definition>
      <rdakit:toolkitDefinition xml:lang="ca">Periodicitat d’una manifestació que es publica o s’actualitza una vegada cada mes.</rdakit:toolkitDefinition>
      <skos:prefLabel xml:lang="vi">hàng tháng</skos:prefLabel>
      <rdakit:toolkitLabel xml:lang="vi">hàng tháng</rdakit:toolkitLabel>
      <skos:definition xml:lang="vi">Tần số cho mộtbiểu thị được công bốhoặc cập nhậtmộtlần mỗitháng.</skos:definition>
      <rdakit:toolkitDefinition xml:lang="vi">Tần số cho mộtbiểu thị được công bốhoặc cập nhậtmộtlần mỗitháng.</rdakit:toolkitDefinition>
      <skos:altLabel xml:lang="fi">joka kuukausi</skos:altLabel>
      <skos:definition xml:lang="fi">Ilmestymis- tai päivittymistiheys aineistolle, joka ilmestyy tai päivittyy kerran kuukaudessa.</skos:definition>
      <rdakit:toolkitDefinition xml:lang="fi">Ilmestymis- tai päivittymistiheys aineistolle, joka ilmestyy tai päivittyy kerran kuukaudessa.</rdakit:toolkitDefinition>
      <skos:prefLabel xml:lang="no">månedlig</skos:prefLabel>
      <rdakit:toolkitLabel xml:lang="no">månedlig</rdakit:toolkitLabel>
      <skos:definition xml:lang="no">En frekvens for en manifestasjon som blir utgitt eller oppdatert en gang hver måned.</skos:definition>
      <rdakit:toolkitDefinition xml:lang="no">En frekvens for en manifestasjon som blir utgitt eller oppdatert en gang hver måned.</rdakit:toolkitDefinition>
    </skos:Concept>
<!-- Concept: quarterly  -->
    <skos:Concept rdf:about="http://rdaregistry.info/termList/frequency/1010" xml:lang="en">
      <skos:inScheme rdf:resource="http://rdaregistry.info/termList/frequency"/>
      <reg:status rdf:resource="http://metadataregistry.org/uri/RegStatus/1001"/>
      <reg:identifier rdf:resource="http://metadataregistry.org/concepts/754"/>
      <skos:prefLabel xml:lang="en">quarterly</skos:prefLabel>
      <skos:definition xml:lang="en">A frequency for a manifestation issued or updated once every three months.</skos:definition>
      <skos:prefLabel xml:lang="de">vierteljährlich</skos:prefLabel>
      <skos:prefLabel xml:lang="fr">trimestriel</skos:prefLabel>
      <skos:definition xml:lang="de">Eine Erscheinungsfrequenz für eine Manifestation, die einmal alle drei Monate erscheint oder aktualisiert wird.</skos:definition>
      <skos:definition xml:lang="fr">Périodicité d’une manifestation publiée ou mise à jour tous les trois mois.</skos:definition>
      <skos:definition xml:lang="es">Frecuencia de un recurso publicado o actualizado una vez cada tres meses.</skos:definition>
      <skos:prefLabel xml:lang="es">trimestral</skos:prefLabel>
      <rdakit:toolkitLabel xml:lang="en">quarterly</rdakit:toolkitLabel>
      <rdakit:toolkitLabel xml:lang="fr">trimestriel</rdakit:toolkitLabel>
      <rdakit:toolkitDefinition xml:lang="en">A frequency for a manifestation issued or updated once every three months.</rdakit:toolkitDefinition>
      <rdakit:toolkitDefinition xml:lang="fr">Périodicité d’une manifestation publiée ou mise à jour tous les trois mois.</rdakit:toolkitDefinition>
      <rdakit:toolkitLabel xml:lang="es">trimestral</rdakit:toolkitLabel>
      <rdakit:toolkitDefinition xml:lang="es">Frecuencia de un recurso publicado o actualizado una vez cada tres meses.</rdakit:toolkitDefinition>
      <skos:prefLabel xml:lang="zh">每季度</skos:prefLabel>
      <rdakit:toolkitLabel xml:lang="zh">每季度</rdakit:toolkitLabel>
      <skos:definition xml:lang="zh">资源发行或更新的频率为每三个月一次。</skos:definition>
      <rdakit:toolkitDefinition xml:lang="zh">资源发行或更新的频率为每三个月一次。</rdakit:toolkitDefinition>
      <skos:prefLabel xml:lang="nl">eens per kwartaal</skos:prefLabel>
      <rdakit:toolkitLabel xml:lang="nl">eens per kwartaal</rdakit:toolkitLabel>
      <skos:definition xml:lang="nl">Frequentie voor een resource die eens per drie maanden uitgegeven of bijgewerkt wordt.</skos:definition>
      <rdakit:toolkitDefinition xml:lang="nl">Frequentie voor een resource die eens per drie maanden uitgegeven of bijgewerkt wordt.</rdakit:toolkitDefinition>
      <rdakit:toolkitLabel xml:lang="de">vierteljährlich</rdakit:toolkitLabel>
      <rdakit:toolkitDefinition xml:lang="de">Eine Erscheinungsfrequenz für eine Manifestation, die einmal alle drei Monate erscheint oder aktualisiert wird.</rdakit:toolkitDefinition>
      <skos:prefLabel xml:lang="it">trimestrale</skos:prefLabel>
      <rdakit:toolkitLabel xml:lang="it">trimestrale</rdakit:toolkitLabel>
      <skos:prefLabel xml:lang="fi">neljä kertaa vuodessa</skos:prefLabel>
      <rdakit:toolkitLabel xml:lang="fi">neljä kertaa vuodessa</rdakit:toolkitLabel>
      <skos:prefLabel xml:lang="ar">فصلي</skos:prefLabel>
      <skos:prefLabel xml:lang="sv">1 nr/kvartal</skos:prefLabel>
      <rdakit:toolkitLabel xml:lang="sv">1 nr/kvartal</rdakit:toolkitLabel>
      <skos:prefLabel xml:lang="da">kvartalsvis</skos:prefLabel>
      <rdakit:toolkitLabel xml:lang="da">kvartalsvis</rdakit:toolkitLabel>
      <skos:definition xml:lang="da">Frekvens for en ressource, der udgives eller opdateres kvartalsvis.</skos:definition>
      <rdakit:toolkitDefinition xml:lang="da">Frekvens for en ressource, der udgives eller opdateres kvartalsvis.</rdakit:toolkitDefinition>
      <skos:prefLabel xml:lang="ca">trimestral</skos:prefLabel>
      <rdakit:toolkitLabel xml:lang="ca">trimestral</rdakit:toolkitLabel>
      <skos:definition xml:lang="ca">Periodicitat d’una manifestació que es publica o s’actualitza una vegada cada tres mesos.</skos:definition>
      <rdakit:toolkitDefinition xml:lang="ca">Periodicitat d’una manifestació que es publica o s’actualitza una vegada cada tres mesos.</rdakit:toolkitDefinition>
      <skos:prefLabel xml:lang="vi">hàng quý</skos:prefLabel>
      <rdakit:toolkitLabel xml:lang="vi">hàng quý</rdakit:toolkitLabel>
      <skos:definition xml:lang="vi">Tần số của một biểu thị được công bố hoặc cập nhật một lần mỗi ba tháng.</skos:definition>
      <rdakit:toolkitDefinition xml:lang="vi">Tần số của một biểu thị được công bố hoặc cập nhật một lần mỗi ba tháng.</rdakit:toolkitDefinition>
      <skos:definition xml:lang="fi">Ilmestymis- tai päivittymistiheys aineistolle, joka ilmestyy tai päivittyy neljä kertaa vuodessa.</skos:definition>
      <rdakit:toolkitDefinition xml:lang="fi">Ilmestymis- tai päivittymistiheys aineistolle, joka ilmestyy tai päivittyy neljä kertaa vuodessa.</rdakit:toolkitDefinition>
      <skos:prefLabel xml:lang="no">kvartalsvis</skos:prefLabel>
      <rdakit:toolkitLabel xml:lang="no">kvartalsvis</rdakit:toolkitLabel>
      <skos:definition xml:lang="no">En frekvens for en manifestasjon som blir utgitt eller oppdatert en gang hver tredje måned.</skos:definition>
      <rdakit:toolkitDefinition xml:lang="no">En frekvens for en manifestasjon som blir utgitt eller oppdatert en gang hver tredje måned.</rdakit:toolkitDefinition>
    </skos:Concept>
<!-- Concept: semiannual  -->
    <skos:Concept rdf:about="http://rdaregistry.info/termList/frequency/1012" xml:lang="en">
      <skos:inScheme rdf:resource="http://rdaregistry.info/termList/frequency"/>
      <reg:status rdf:resource="http://metadataregistry.org/uri/RegStatus/1001"/>
      <reg:identifier rdf:resource="http://metadataregistry.org/concepts/756"/>
      <skos:prefLabel xml:lang="en">semiannual</skos:prefLabel>
      <skos:definition xml:lang="en">A frequency for a manifestation issued or updated twice every year.</skos:definition>
      <skos:prefLabel xml:lang="de">halbjährlich</skos:prefLabel>
      <skos:prefLabel xml:lang="fr">semestriel</skos:prefLabel>
      <skos:definition xml:lang="de">Eine Erscheinungsfrequenz für eine Manifestation, die zweimal pro Jahr erscheint oder aktualisiert wird.</skos:definition>
      <skos:definition xml:lang="fr">Périodicité d’une manifestation publiée ou mise à jour deux fois par année.</skos:definition>
      <skos:prefLabel xml:lang="es">semestral</skos:prefLabel>
      <rdakit:toolkitLabel xml:lang="en">semiannual</rdakit:toolkitLabel>
      <rdakit:toolkitLabel xml:lang="fr">semestriel</rdakit:toolkitLabel>
      <rdakit:toolkitDefinition xml:lang="en">A frequency for a manifestation issued or updated twice every year.</rdakit:toolkitDefinition>
      <rdakit:toolkitDefinition xml:lang="fr">Périodicité d’une manifestation publiée ou mise à jour deux fois par année.</rdakit:toolkitDefinition>
      <rdakit:toolkitLabel xml:lang="es">semestral</rdakit:toolkitLabel>
      <skos:prefLabel xml:lang="zh">每半年</skos:prefLabel>
      <rdakit:toolkitLabel xml:lang="zh">每半年</rdakit:toolkitLabel>
      <skos:definition xml:lang="zh">资源发行或更新的频率为每年两次。</skos:definition>
      <rdakit:toolkitDefinition xml:lang="zh">资源发行或更新的频率为每年两次。</rdakit:toolkitDefinition>
      <skos:definition xml:lang="es">Frecuencia de un recurso publicado o actualizado dos veces al año.</skos:definition>
      <rdakit:toolkitDefinition xml:lang="es">Frecuencia de un recurso publicado o actualizado dos veces al año.</rdakit:toolkitDefinition>
      <skos:prefLabel xml:lang="nl">twee keer per jaar</skos:prefLabel>
      <rdakit:toolkitLabel xml:lang="nl">twee keer per jaar</rdakit:toolkitLabel>
      <skos:definition xml:lang="nl">Frequentie voor een resource die twee keer per jaar uitgegeven of bijgewerkt wordt.</skos:definition>
      <rdakit:toolkitDefinition xml:lang="nl">Frequentie voor een resource die twee keer per jaar uitgegeven of bijgewerkt wordt.</rdakit:toolkitDefinition>
      <rdakit:toolkitLabel xml:lang="de">halbjährlich</rdakit:toolkitLabel>
      <rdakit:toolkitDefinition xml:lang="de">Eine Erscheinungsfrequenz für eine Manifestation, die zweimal pro Jahr erscheint oder aktualisiert wird.</rdakit:toolkitDefinition>
      <skos:prefLabel xml:lang="it">semestrale</skos:prefLabel>
      <rdakit:toolkitLabel xml:lang="it">semestrale</rdakit:toolkitLabel>
      <skos:prefLabel xml:lang="fi">kaksi kertaa vuodessa</skos:prefLabel>
      <rdakit:toolkitLabel xml:lang="fi">kaksi kertaa vuodessa</rdakit:toolkitLabel>
      <skos:prefLabel xml:lang="ar">نصف سنوي</skos:prefLabel>
      <skos:prefLabel xml:lang="sv">2 nr/år</skos:prefLabel>
      <rdakit:toolkitLabel xml:lang="sv">2 nr/år</rdakit:toolkitLabel>
      <skos:prefLabel xml:lang="da">2 gange om året</skos:prefLabel>
      <rdakit:toolkitLabel xml:lang="da">2 gange om året</rdakit:toolkitLabel>
      <skos:definition xml:lang="da">Frekvens for en ressource, der udgives eller opdateres halvårligt.</skos:definition>
      <rdakit:toolkitDefinition xml:lang="da">Frekvens for en ressource, der udgives eller opdateres halvårligt.</rdakit:toolkitDefinition>
      <skos:prefLabel xml:lang="ca">semestral</skos:prefLabel>
      <rdakit:toolkitLabel xml:lang="ca">semestral</rdakit:toolkitLabel>
      <skos:definition xml:lang="ca">Periodicitat d’una manifestació que es publica o s’actualitza dues vegades cada any.</skos:definition>
      <rdakit:toolkitDefinition xml:lang="ca">Periodicitat d’una manifestació que es publica o s’actualitza dues vegades cada any.</rdakit:toolkitDefinition>
      <skos:prefLabel xml:lang="vi">hàng nửa năm</skos:prefLabel>
      <rdakit:toolkitLabel xml:lang="vi">hàng nửa năm</rdakit:toolkitLabel>
      <skos:definition xml:lang="vi">Tần số cho mộtbiểu thị được công bốhoặc cập nhật hai lần mỗi năm.</skos:definition>
      <rdakit:toolkitDefinition xml:lang="vi">Tần số cho mộtbiểu thị được công bốhoặc cập nhật hai lần mỗi năm.</rdakit:toolkitDefinition>
      <skos:definition xml:lang="fi">Ilmestymis- tai päivittymistiheys aineistolle, joka ilmestyy tai päivittyy kaksi kertaa vuodessa.</skos:definition>
      <rdakit:toolkitDefinition xml:lang="fi">Ilmestymis- tai päivittymistiheys aineistolle, joka ilmestyy tai päivittyy kaksi kertaa vuodessa.</rdakit:toolkitDefinition>
      <skos:prefLabel xml:lang="no">halvårlig</skos:prefLabel>
      <rdakit:toolkitLabel xml:lang="no">halvårlig</rdakit:toolkitLabel>
      <skos:definition xml:lang="no">En frekvens for en manifestasjon som blir utgitt eller oppdatert to ganger hvert år.</skos:definition>
      <rdakit:toolkitDefinition xml:lang="no">En frekvens for en manifestasjon som blir utgitt eller oppdatert to ganger hvert år.</rdakit:toolkitDefinition>
    </skos:Concept>
<!-- Concept: semimonthly  -->
    <skos:Concept rdf:about="http://rdaregistry.info/termList/frequency/1009" xml:lang="en">
      <skos:inScheme rdf:resource="http://rdaregistry.info/termList/frequency"/>
      <reg:status rdf:resource="http://metadataregistry.org/uri/RegStatus/1001"/>
      <reg:identifier rdf:resource="http://metadataregistry.org/concepts/753"/>
      <skos:prefLabel xml:lang="en">semimonthly</skos:prefLabel>
      <skos:definition xml:lang="en">A frequency for a manifestation issued or updated twice every month.</skos:definition>
      <skos:prefLabel xml:lang="de">zweimal pro Monat</skos:prefLabel>
      <skos:prefLabel xml:lang="fr">bimensuel</skos:prefLabel>
      <skos:definition xml:lang="de">Eine Erscheinungsfrequenz für eine Manifestation, die zweimal pro Monat erscheint oder aktualisiert wird.</skos:definition>
      <skos:definition xml:lang="fr">Périodicité d’une manifestation publiée ou mise à jour deux fois par mois.</skos:definition>
      <skos:prefLabel xml:lang="es">bimensual</skos:prefLabel>
      <skos:definition xml:lang="es">Frecuencia de un recurso publicado o actualizado dos veces en el mes.</skos:definition>
      <rdakit:toolkitLabel xml:lang="en">semimonthly</rdakit:toolkitLabel>
      <rdakit:toolkitLabel xml:lang="fr">bimensuel</rdakit:toolkitLabel>
      <rdakit:toolkitDefinition xml:lang="en">A frequency for a manifestation issued or updated twice every month.</rdakit:toolkitDefinition>
      <rdakit:toolkitDefinition xml:lang="fr">Périodicité d’une manifestation publiée ou mise à jour deux fois par mois.</rdakit:toolkitDefinition>
      <rdakit:toolkitLabel xml:lang="es">bimensual</rdakit:toolkitLabel>
      <rdakit:toolkitDefinition xml:lang="es">Frecuencia de un recurso publicado o actualizado dos veces en el mes.</rdakit:toolkitDefinition>
      <skos:prefLabel xml:lang="zh">每半月</skos:prefLabel>
      <rdakit:toolkitLabel xml:lang="zh">每半月</rdakit:toolkitLabel>
      <skos:definition xml:lang="zh">资源发行或更新的频率为每月两次。</skos:definition>
      <rdakit:toolkitDefinition xml:lang="zh">资源发行或更新的频率为每月两次。</rdakit:toolkitDefinition>
      <skos:prefLabel xml:lang="nl">twee keer per maand</skos:prefLabel>
      <rdakit:toolkitLabel xml:lang="nl">twee keer per maand</rdakit:toolkitLabel>
      <skos:definition xml:lang="nl">Frequentie voor een resource die twee keer per maand uitgegeven of bijgewerkt wordt.</skos:definition>
      <rdakit:toolkitDefinition xml:lang="nl">Frequentie voor een resource die twee keer per maand uitgegeven of bijgewerkt wordt.</rdakit:toolkitDefinition>
      <rdakit:toolkitLabel xml:lang="de">zweimal pro Monat</rdakit:toolkitLabel>
      <rdakit:toolkitDefinition xml:lang="de">Eine Erscheinungsfrequenz für eine Manifestation, die zweimal pro Monat erscheint oder aktualisiert wird.</rdakit:toolkitDefinition>
      <skos:prefLabel xml:lang="it">due volte al mese</skos:prefLabel>
      <rdakit:toolkitLabel xml:lang="it">due volte al mese</rdakit:toolkitLabel>
      <skos:prefLabel xml:lang="fi">kaksi kertaa kuukaudessa</skos:prefLabel>
      <rdakit:toolkitLabel xml:lang="fi">kaksi kertaa kuukaudessa</rdakit:toolkitLabel>
      <skos:prefLabel xml:lang="ar">نصف شهري</skos:prefLabel>
      <skos:prefLabel xml:lang="sv">2 nr/månad</skos:prefLabel>
      <rdakit:toolkitLabel xml:lang="sv">2 nr/månad</rdakit:toolkitLabel>
      <skos:prefLabel xml:lang="da">2 gange om måneden</skos:prefLabel>
      <rdakit:toolkitLabel xml:lang="da">2 gange om måneden</rdakit:toolkitLabel>
      <skos:definition xml:lang="da">Frekvens for en ressource, der udgives eller opdateres to gange om måneden.</skos:definition>
      <rdakit:toolkitDefinition xml:lang="da">Frekvens for en ressource, der udgives eller opdateres to gange om måneden.</rdakit:toolkitDefinition>
      <skos:prefLabel xml:lang="ca">bimensual</skos:prefLabel>
      <rdakit:toolkitLabel xml:lang="ca">bimensual</rdakit:toolkitLabel>
      <skos:definition xml:lang="ca">Periodicitat d’una manifestació que es publica o s’actualitza dues vegades cada mes.</skos:definition>
      <rdakit:toolkitDefinition xml:lang="ca">Periodicitat d’una manifestació que es publica o s’actualitza dues vegades cada mes.</rdakit:toolkitDefinition>
      <skos:prefLabel xml:lang="vi">hàng nửa tháng</skos:prefLabel>
      <rdakit:toolkitLabel xml:lang="vi">hàng nửa tháng</rdakit:toolkitLabel>
      <skos:definition xml:lang="vi">Tần số cho mộtbiểu thị được công bốhoặc cập nhậthailần mỗitháng.</skos:definition>
      <rdakit:toolkitDefinition xml:lang="vi">Tần số cho mộtbiểu thị được công bốhoặc cập nhậthailần mỗitháng.</rdakit:toolkitDefinition>
      <skos:definition xml:lang="fi">Ilmestymis- tai päivittymistiheys aineistolle, joka ilmestyy tai päivittyy kaksi kertaa kuukaudessa.</skos:definition>
      <rdakit:toolkitDefinition xml:lang="fi">Ilmestymis- tai päivittymistiheys aineistolle, joka ilmestyy tai päivittyy kaksi kertaa kuukaudessa.</rdakit:toolkitDefinition>
      <skos:prefLabel xml:lang="no">to ganger i måneden</skos:prefLabel>
      <rdakit:toolkitLabel xml:lang="no">to ganger i måneden</rdakit:toolkitLabel>
      <skos:definition xml:lang="no">En frekvens for en manifestasjon som blir utgitt eller oppdatert to ganger hver måned.</skos:definition>
      <rdakit:toolkitDefinition xml:lang="no">En frekvens for en manifestasjon som blir utgitt eller oppdatert to ganger hver måned.</rdakit:toolkitDefinition>
    </skos:Concept>
<!-- Concept: semiweekly  -->
    <skos:Concept rdf:about="http://rdaregistry.info/termList/frequency/1005" xml:lang="en">
      <skos:inScheme rdf:resource="http://rdaregistry.info/termList/frequency"/>
      <reg:status rdf:resource="http://metadataregistry.org/uri/RegStatus/1001"/>
      <reg:identifier rdf:resource="http://metadataregistry.org/concepts/749"/>
      <skos:prefLabel xml:lang="en">semiweekly</skos:prefLabel>
      <skos:definition xml:lang="en">A frequency for a manifestation issued or updated twice every week.</skos:definition>
      <skos:prefLabel xml:lang="de">zweimal pro Woche</skos:prefLabel>
      <skos:prefLabel xml:lang="fr">bihebdomadaire</skos:prefLabel>
      <skos:definition xml:lang="de">Eine Erscheinungsfrequenz für eine Manifestation, die zweimal pro Woche erscheint oder aktualisiert wird.</skos:definition>
      <skos:definition xml:lang="fr">Périodicité d’une manifestation publiée ou mise à jour deux fois par semaine.</skos:definition>
      <rdakit:toolkitLabel xml:lang="en">semiweekly</rdakit:toolkitLabel>
      <rdakit:toolkitLabel xml:lang="fr">bihebdomadaire</rdakit:toolkitLabel>
      <rdakit:toolkitDefinition xml:lang="en">A frequency for a manifestation issued or updated twice every week.</rdakit:toolkitDefinition>
      <rdakit:toolkitDefinition xml:lang="fr">Périodicité d’une manifestation publiée ou mise à jour deux fois par semaine.</rdakit:toolkitDefinition>
      <skos:prefLabel xml:lang="zh">每半周</skos:prefLabel>
      <rdakit:toolkitLabel xml:lang="zh">每半周</rdakit:toolkitLabel>
      <skos:definition xml:lang="zh">资源的发行或更新频率为每周两次。</skos:definition>
      <rdakit:toolkitDefinition xml:lang="zh">资源的发行或更新频率为每周两次。</rdakit:toolkitDefinition>
      <skos:prefLabel xml:lang="es">semisemanal</skos:prefLabel>
      <rdakit:toolkitLabel xml:lang="es">semisemanal</rdakit:toolkitLabel>
      <skos:definition xml:lang="es">Frecuencia de un recurso publicado o actualizado dos veces en la semana.</skos:definition>
      <rdakit:toolkitDefinition xml:lang="es">Frecuencia de un recurso publicado o actualizado dos veces en la semana.</rdakit:toolkitDefinition>
      <skos:prefLabel xml:lang="nl">twee keer per week</skos:prefLabel>
      <rdakit:toolkitLabel xml:lang="nl">twee keer per week</rdakit:toolkitLabel>
      <skos:definition xml:lang="nl">Frequentie voor een resource die twee keer per week uitgegeven of bijgewerkt wordt.</skos:definition>
      <rdakit:toolkitDefinition xml:lang="nl">Frequentie voor een resource die twee keer per week uitgegeven of bijgewerkt wordt.</rdakit:toolkitDefinition>
      <rdakit:toolkitLabel xml:lang="de">zweimal pro Woche</rdakit:toolkitLabel>
      <rdakit:toolkitDefinition xml:lang="de">Eine Erscheinungsfrequenz für eine Manifestation, die zweimal pro Woche erscheint oder aktualisiert wird.</rdakit:toolkitDefinition>
      <skos:prefLabel xml:lang="it">bisettimanale</skos:prefLabel>
      <rdakit:toolkitLabel xml:lang="it">bisettimanale</rdakit:toolkitLabel>
      <skos:prefLabel xml:lang="fi">kaksi kertaa viikossa</skos:prefLabel>
      <rdakit:toolkitLabel xml:lang="fi">kaksi kertaa viikossa</rdakit:toolkitLabel>
      <skos:prefLabel xml:lang="ar">نصف اسبوعي</skos:prefLabel>
      <skos:prefLabel xml:lang="sv">2 nr/vecka</skos:prefLabel>
      <rdakit:toolkitLabel xml:lang="sv">2 nr/vecka</rdakit:toolkitLabel>
      <skos:prefLabel xml:lang="da">2 gange om ugen</skos:prefLabel>
      <rdakit:toolkitLabel xml:lang="da">2 gange om ugen</rdakit:toolkitLabel>
      <skos:definition xml:lang="da">Frekvens for en ressource, der udgives eller opdateres to gange om ugen.</skos:definition>
      <rdakit:toolkitDefinition xml:lang="da">Frekvens for en ressource, der udgives eller opdateres to gange om ugen.</rdakit:toolkitDefinition>
      <skos:prefLabel xml:lang="ca">bisetmanal</skos:prefLabel>
      <rdakit:toolkitLabel xml:lang="ca">bisetmanal</rdakit:toolkitLabel>
      <skos:definition xml:lang="ca">Periodicitat d’una manifestació que es publica o s’actualitza dues vegades cada setmana.</skos:definition>
      <rdakit:toolkitDefinition xml:lang="ca">Periodicitat d’una manifestació que es publica o s’actualitza dues vegades cada setmana.</rdakit:toolkitDefinition>
      <skos:prefLabel xml:lang="vi">hàng nửa tuần</skos:prefLabel>
      <rdakit:toolkitLabel xml:lang="vi">hàng nửa tuần</rdakit:toolkitLabel>
      <skos:definition xml:lang="vi">Tần số cho mộtbiểu thị được công bốhoặc cập nhậthailần mỗituần.</skos:definition>
      <rdakit:toolkitDefinition xml:lang="vi">Tần số cho mộtbiểu thị được công bốhoặc cập nhậthailần mỗituần.</rdakit:toolkitDefinition>
      <skos:definition xml:lang="fi">Ilmestymis- tai päivittymistiheys aineistolle, joka ilmestyy tai päivittyy kaksi kertaa viikossa.</skos:definition>
      <rdakit:toolkitDefinition xml:lang="fi">Ilmestymis- tai päivittymistiheys aineistolle, joka ilmestyy tai päivittyy kaksi kertaa viikossa.</rdakit:toolkitDefinition>
      <skos:prefLabel xml:lang="no">to ganger i uken</skos:prefLabel>
      <rdakit:toolkitLabel xml:lang="no">to ganger i uken</rdakit:toolkitLabel>
      <skos:definition xml:lang="no">En frekvens for en manifestasjon som blir utgitt eller oppdatert to ganger hver uke.</skos:definition>
      <rdakit:toolkitDefinition xml:lang="no">En frekvens for en manifestasjon som blir utgitt eller oppdatert to ganger hver uke.</rdakit:toolkitDefinition>
    </skos:Concept>
<!-- Concept: three times a month  -->
    <skos:Concept rdf:about="http://rdaregistry.info/termList/frequency/1006" xml:lang="en">
      <skos:inScheme rdf:resource="http://rdaregistry.info/termList/frequency"/>
      <reg:status rdf:resource="http://metadataregistry.org/uri/RegStatus/1001"/>
      <reg:identifier rdf:resource="http://metadataregistry.org/concepts/750"/>
      <skos:prefLabel xml:lang="en">three times a month</skos:prefLabel>
      <skos:definition xml:lang="en">A frequency for a manifestation issued or updated three times every month.</skos:definition>
      <skos:prefLabel xml:lang="de">dreimal pro Monat</skos:prefLabel>
      <skos:prefLabel xml:lang="fr">trois fois par mois</skos:prefLabel>
      <skos:definition xml:lang="de">Eine Erscheinungsfrequenz für eine Manifestation, die dreimal pro Monat erscheint oder aktualisiert wird.</skos:definition>
      <skos:definition xml:lang="fr">Périodicité d’une manifestation publiée ou mise à jour trois fois par mois.</skos:definition>
      <skos:prefLabel xml:lang="es">tres veces en un mes</skos:prefLabel>
      <skos:definition xml:lang="es">Frecuencia de un recurso publicado o actualizado tres veces al mes.</skos:definition>
      <rdakit:toolkitLabel xml:lang="en">three times a month</rdakit:toolkitLabel>
      <rdakit:toolkitLabel xml:lang="fr">trois fois par mois</rdakit:toolkitLabel>
      <rdakit:toolkitDefinition xml:lang="en">A frequency for a manifestation issued or updated three times every month.</rdakit:toolkitDefinition>
      <rdakit:toolkitDefinition xml:lang="fr">Périodicité d’une manifestation publiée ou mise à jour trois fois par mois.</rdakit:toolkitDefinition>
      <rdakit:toolkitLabel xml:lang="es">tres veces en un mes</rdakit:toolkitLabel>
      <rdakit:toolkitDefinition xml:lang="es">Frecuencia de un recurso publicado o actualizado tres veces al mes.</rdakit:toolkitDefinition>
      <skos:prefLabel xml:lang="zh">每月三次</skos:prefLabel>
      <rdakit:toolkitLabel xml:lang="zh">每月三次</rdakit:toolkitLabel>
      <skos:definition xml:lang="zh">资源发行或更新的频率为每月三次。</skos:definition>
      <rdakit:toolkitDefinition xml:lang="zh">资源发行或更新的频率为每月三次。</rdakit:toolkitDefinition>
      <skos:prefLabel xml:lang="nl">drie keer per maand</skos:prefLabel>
      <rdakit:toolkitLabel xml:lang="nl">drie keer per maand</rdakit:toolkitLabel>
      <skos:definition xml:lang="nl">Frequentie voor een resource die drie keer per maand uitgegeven of bijgewerkt wordt.</skos:definition>
      <rdakit:toolkitDefinition xml:lang="nl">Frequentie voor een resource die drie keer per maand uitgegeven of bijgewerkt wordt.</rdakit:toolkitDefinition>
      <rdakit:toolkitLabel xml:lang="de">dreimal pro Monat</rdakit:toolkitLabel>
      <rdakit:toolkitDefinition xml:lang="de">Eine Erscheinungsfrequenz für eine Manifestation, die dreimal pro Monat erscheint oder aktualisiert wird.</rdakit:toolkitDefinition>
      <skos:prefLabel xml:lang="it">tre volte al mese</skos:prefLabel>
      <rdakit:toolkitLabel xml:lang="it">tre volte al mese</rdakit:toolkitLabel>
      <skos:prefLabel xml:lang="fi">kolme kertaa kuukaudessa</skos:prefLabel>
      <rdakit:toolkitLabel xml:lang="fi">kolme kertaa kuukaudessa</rdakit:toolkitLabel>
      <skos:prefLabel xml:lang="ar">ثلاث مرات  في الشهر</skos:prefLabel>
      <skos:prefLabel xml:lang="sv">3 nr/månad</skos:prefLabel>
      <rdakit:toolkitLabel xml:lang="sv">3 nr/månad</rdakit:toolkitLabel>
      <skos:prefLabel xml:lang="da">3 gange om ugen</skos:prefLabel>
      <rdakit:toolkitLabel xml:lang="da">3 gange om ugen</rdakit:toolkitLabel>
      <skos:definition xml:lang="da">Frekvens for en ressource, der udgives eller opdateres tre gange om måneden.</skos:definition>
      <rdakit:toolkitDefinition xml:lang="da">Frekvens for en ressource, der udgives eller opdateres tre gange om måneden.</rdakit:toolkitDefinition>
      <skos:prefLabel xml:lang="ca">tres vegades al mes</skos:prefLabel>
      <rdakit:toolkitLabel xml:lang="ca">tres vegades al mes</rdakit:toolkitLabel>
      <skos:definition xml:lang="ca">Periodicitat d’una manifestació que es publica o s’actualitza tres vegades cada mes.</skos:definition>
      <rdakit:toolkitDefinition xml:lang="ca">Periodicitat d’una manifestació que es publica o s’actualitza tres vegades cada mes.</rdakit:toolkitDefinition>
      <skos:prefLabel xml:lang="vi">ba lần một tháng</skos:prefLabel>
      <rdakit:toolkitLabel xml:lang="vi">ba lần một tháng</rdakit:toolkitLabel>
      <skos:definition xml:lang="vi">Tần số cho mộtbiểu thị được công bốhoặc cập nhật ba lần mỗi tháng.</skos:definition>
      <rdakit:toolkitDefinition xml:lang="vi">Tần số cho mộtbiểu thị được công bốhoặc cập nhật ba lần mỗi tháng.</rdakit:toolkitDefinition>
      <skos:definition xml:lang="fi">Ilmestymis- tai päivittymistiheys aineistolle, joka ilmestyy tai päivittyy kolme kertaa kuussa.</skos:definition>
      <rdakit:toolkitDefinition xml:lang="fi">Ilmestymis- tai päivittymistiheys aineistolle, joka ilmestyy tai päivittyy kolme kertaa kuussa.</rdakit:toolkitDefinition>
      <skos:prefLabel xml:lang="no">tre ganger i måneden</skos:prefLabel>
      <rdakit:toolkitLabel xml:lang="no">tre ganger i måneden</rdakit:toolkitLabel>
      <skos:definition xml:lang="no">En frekvens for en manifestasjon som blir utgitt eller oppdatert tre ganger hver måned.</skos:definition>
      <rdakit:toolkitDefinition xml:lang="no">En frekvens for en manifestasjon som blir utgitt eller oppdatert tre ganger hver måned.</rdakit:toolkitDefinition>
    </skos:Concept>
<!-- Concept: three times a week  -->
    <skos:Concept rdf:about="http://rdaregistry.info/termList/frequency/1002" xml:lang="en">
      <skos:inScheme rdf:resource="http://rdaregistry.info/termList/frequency"/>
      <reg:status rdf:resource="http://metadataregistry.org/uri/RegStatus/1001"/>
      <reg:identifier rdf:resource="http://metadataregistry.org/concepts/746"/>
      <skos:prefLabel xml:lang="en">three times a week</skos:prefLabel>
      <skos:definition xml:lang="en">A frequency for a manifestation issued or updated three times every week.</skos:definition>
      <skos:prefLabel xml:lang="de">dreimal pro Woche</skos:prefLabel>
      <skos:prefLabel xml:lang="fr">trois fois par semaine</skos:prefLabel>
      <skos:definition xml:lang="de">Eine Erscheinungsfrequenz für eine Manifestation, die dreimal pro Woche erscheint oder aktualisiert wird.</skos:definition>
      <skos:definition xml:lang="fr">Périodicité d’une manifestation publiée ou mise à jour trois fois par semaine.</skos:definition>
      <skos:prefLabel xml:lang="es">tres veces por semana</skos:prefLabel>
      <skos:definition xml:lang="es">Frecuencia de un recurso publicado o actualizado tres veces por semana.</skos:definition>
      <rdakit:toolkitLabel xml:lang="en">three times a week</rdakit:toolkitLabel>
      <rdakit:toolkitLabel xml:lang="fr">trois fois par semaine</rdakit:toolkitLabel>
      <rdakit:toolkitDefinition xml:lang="en">A frequency for a manifestation issued or updated three times every week.</rdakit:toolkitDefinition>
      <rdakit:toolkitDefinition xml:lang="fr">Périodicité d’une manifestation publiée ou mise à jour trois fois par semaine.</rdakit:toolkitDefinition>
      <rdakit:toolkitLabel xml:lang="es">tres veces por semana</rdakit:toolkitLabel>
      <rdakit:toolkitDefinition xml:lang="es">Frecuencia de un recurso publicado o actualizado tres veces por semana.</rdakit:toolkitDefinition>
      <skos:prefLabel xml:lang="zh">每周三次</skos:prefLabel>
      <rdakit:toolkitLabel xml:lang="zh">每周三次</rdakit:toolkitLabel>
      <skos:definition xml:lang="zh">资源发行或更新的频率为每周三次。</skos:definition>
      <rdakit:toolkitDefinition xml:lang="zh">资源发行或更新的频率为每周三次。</rdakit:toolkitDefinition>
      <skos:prefLabel xml:lang="nl">drie keer per week</skos:prefLabel>
      <rdakit:toolkitLabel xml:lang="nl">drie keer per week</rdakit:toolkitLabel>
      <skos:definition xml:lang="nl">Frequentie voor een resource die drie keer per week uitgegeven of bijgewerkt wordt.</skos:definition>
      <rdakit:toolkitDefinition xml:lang="nl">Frequentie voor een resource die drie keer per week uitgegeven of bijgewerkt wordt.</rdakit:toolkitDefinition>
      <rdakit:toolkitLabel xml:lang="de">dreimal pro Woche</rdakit:toolkitLabel>
      <rdakit:toolkitDefinition xml:lang="de">Eine Erscheinungsfrequenz für eine Manifestation, die dreimal pro Woche erscheint oder aktualisiert wird.</rdakit:toolkitDefinition>
      <skos:prefLabel xml:lang="it">tre volte alla settimana</skos:prefLabel>
      <rdakit:toolkitLabel xml:lang="it">tre volte alla settimana</rdakit:toolkitLabel>
      <skos:prefLabel xml:lang="fi">kolme kertaa viikossa</skos:prefLabel>
      <rdakit:toolkitLabel xml:lang="fi">kolme kertaa viikossa</rdakit:toolkitLabel>
      <skos:prefLabel xml:lang="ar">ثلاث مرات في الاسبوع</skos:prefLabel>
      <skos:prefLabel xml:lang="sv">3 nr/vecka</skos:prefLabel>
      <rdakit:toolkitLabel xml:lang="sv">3 nr/vecka</rdakit:toolkitLabel>
      <skos:prefLabel xml:lang="da">3 gange om ugen</skos:prefLabel>
      <rdakit:toolkitLabel xml:lang="da">3 gange om ugen</rdakit:toolkitLabel>
      <skos:definition xml:lang="da">Frekvens for en ressource, der udgives eller opdateres tre gange om ugen.</skos:definition>
      <rdakit:toolkitDefinition xml:lang="da">Frekvens for en ressource, der udgives eller opdateres tre gange om ugen.</rdakit:toolkitDefinition>
      <skos:prefLabel xml:lang="ca">tres vegades a la setmana</skos:prefLabel>
      <rdakit:toolkitLabel xml:lang="ca">tres vegades a la setmana</rdakit:toolkitLabel>
      <skos:definition xml:lang="ca">Periodicitat d’una manifestació que es publica o s’actualitza tres vegades cada setmana.</skos:definition>
      <rdakit:toolkitDefinition xml:lang="ca">Periodicitat d’una manifestació que es publica o s’actualitza tres vegades cada setmana.</rdakit:toolkitDefinition>
      <skos:prefLabel xml:lang="vi">ba lần một tuần</skos:prefLabel>
      <rdakit:toolkitLabel xml:lang="vi">ba lần một tuần</rdakit:toolkitLabel>
      <skos:definition xml:lang="vi">Tần số cho mộtbiểu thị được công bốhoặc cập nhật ba lần mỗituần.</skos:definition>
      <rdakit:toolkitDefinition xml:lang="vi">Tần số cho mộtbiểu thị được công bốhoặc cập nhật ba lần mỗituần.</rdakit:toolkitDefinition>
      <skos:definition xml:lang="fi">Ilmestymis- tai päivittymistiheys aineistolle, joka ilmestyy tai päivittyy kolme kertaa viikossa.</skos:definition>
      <rdakit:toolkitDefinition xml:lang="fi">Ilmestymis- tai päivittymistiheys aineistolle, joka ilmestyy tai päivittyy kolme kertaa viikossa.</rdakit:toolkitDefinition>
      <skos:prefLabel xml:lang="no">tre ganger i uken</skos:prefLabel>
      <rdakit:toolkitLabel xml:lang="no">tre ganger i uken</rdakit:toolkitLabel>
      <skos:definition xml:lang="no">En frekvens for en manifestasjon som blir utgitt eller oppdatert tre ganger hver uke.</skos:definition>
      <rdakit:toolkitDefinition xml:lang="no">En frekvens for en manifestasjon som blir utgitt eller oppdatert tre ganger hver uke.</rdakit:toolkitDefinition>
    </skos:Concept>
<!-- Concept: three times a year  -->
    <skos:Concept rdf:about="http://rdaregistry.info/termList/frequency/1011" xml:lang="en">
      <skos:inScheme rdf:resource="http://rdaregistry.info/termList/frequency"/>
      <reg:status rdf:resource="http://metadataregistry.org/uri/RegStatus/1001"/>
      <reg:identifier rdf:resource="http://metadataregistry.org/concepts/755"/>
      <skos:prefLabel xml:lang="en">three times a year</skos:prefLabel>
      <skos:definition xml:lang="en">A frequency for a manifestation issued or updated three times every year.</skos:definition>
      <skos:prefLabel xml:lang="de">dreimal pro Jahr</skos:prefLabel>
      <skos:prefLabel xml:lang="fr">trois fois par an</skos:prefLabel>
      <skos:definition xml:lang="de">Eine Erscheinungsfrequenz für eine Manifestation, die dreimal pro Jahr erscheint oder aktualisiert wird.</skos:definition>
      <skos:definition xml:lang="fr">Périodicité d’une manifestation publiée ou mise à jour trois fois par année.</skos:definition>
      <skos:definition xml:lang="es">Frecuencia de un recurso publicado o actualizado tres veces al año.</skos:definition>
      <skos:prefLabel xml:lang="es">tres veces al año</skos:prefLabel>
      <rdakit:toolkitLabel xml:lang="en">three times a year</rdakit:toolkitLabel>
      <rdakit:toolkitLabel xml:lang="fr">trois fois par an</rdakit:toolkitLabel>
      <rdakit:toolkitDefinition xml:lang="en">A frequency for a manifestation issued or updated three times every year.</rdakit:toolkitDefinition>
      <rdakit:toolkitDefinition xml:lang="fr">Périodicité d’une manifestation publiée ou mise à jour trois fois par année.</rdakit:toolkitDefinition>
      <rdakit:toolkitLabel xml:lang="es">tres veces al año</rdakit:toolkitLabel>
      <rdakit:toolkitDefinition xml:lang="es">Frecuencia de un recurso publicado o actualizado tres veces al año.</rdakit:toolkitDefinition>
      <skos:prefLabel xml:lang="zh">每年三次</skos:prefLabel>
      <rdakit:toolkitLabel xml:lang="zh">每年三次</rdakit:toolkitLabel>
      <skos:definition xml:lang="zh">资源发行或更新的频率为每年三次。</skos:definition>
      <rdakit:toolkitDefinition xml:lang="zh">资源发行或更新的频率为每年三次。</rdakit:toolkitDefinition>
      <skos:prefLabel xml:lang="nl">drie keer per jaar</skos:prefLabel>
      <rdakit:toolkitLabel xml:lang="nl">drie keer per jaar</rdakit:toolkitLabel>
      <skos:definition xml:lang="nl">Frequentie voor een resource die drie keer per jaar uitgegeven of bijgewerkt wordt.</skos:definition>
      <rdakit:toolkitDefinition xml:lang="nl">Frequentie voor een resource die drie keer per jaar uitgegeven of bijgewerkt wordt.</rdakit:toolkitDefinition>
      <rdakit:toolkitLabel xml:lang="de">dreimal pro Jahr</rdakit:toolkitLabel>
      <rdakit:toolkitDefinition xml:lang="de">Eine Erscheinungsfrequenz für eine Manifestation, die dreimal pro Jahr erscheint oder aktualisiert wird.</rdakit:toolkitDefinition>
      <skos:prefLabel xml:lang="it">tre volte all'anno</skos:prefLabel>
      <rdakit:toolkitLabel xml:lang="it">tre volte all'anno</rdakit:toolkitLabel>
      <skos:prefLabel xml:lang="fi">kolme kertaa vuodessa</skos:prefLabel>
      <rdakit:toolkitLabel xml:lang="fi">kolme kertaa vuodessa</rdakit:toolkitLabel>
      <skos:prefLabel xml:lang="ar">ثلاث مرات في السنة</skos:prefLabel>
      <skos:prefLabel xml:lang="sv">3 nr/år</skos:prefLabel>
      <rdakit:toolkitLabel xml:lang="sv">3 nr/år</rdakit:toolkitLabel>
      <skos:prefLabel xml:lang="da">3 gange om året</skos:prefLabel>
      <rdakit:toolkitLabel xml:lang="da">3 gange om året</rdakit:toolkitLabel>
      <skos:definition xml:lang="da">Frekvens for en ressource, der udgives eller opdateres tre gange om året.</skos:definition>
      <rdakit:toolkitDefinition xml:lang="da">Frekvens for en ressource, der udgives eller opdateres tre gange om året.</rdakit:toolkitDefinition>
      <skos:prefLabel xml:lang="ca">tres vegades a l’any</skos:prefLabel>
      <rdakit:toolkitLabel xml:lang="ca">tres vegades a l’any</rdakit:toolkitLabel>
      <skos:definition xml:lang="ca">Periodicitat d’una manifestació que es publica o s’actualitza tres vegades cada any.</skos:definition>
      <rdakit:toolkitDefinition xml:lang="ca">Periodicitat d’una manifestació que es publica o s’actualitza tres vegades cada any.</rdakit:toolkitDefinition>
      <skos:prefLabel xml:lang="vi">ba lần một năm</skos:prefLabel>
      <rdakit:toolkitLabel xml:lang="vi">ba lần một năm</rdakit:toolkitLabel>
      <skos:definition xml:lang="vi">Tần số cho mộtbiểu thị được công bốhoặc cập nhật ba lần mỗinăm.</skos:definition>
      <rdakit:toolkitDefinition xml:lang="vi">Tần số cho mộtbiểu thị được công bốhoặc cập nhật ba lần mỗinăm.</rdakit:toolkitDefinition>
      <skos:definition xml:lang="fi">Ilmestymis- tai päivittymistiheys aineistolle, joka ilmestyy tai päivittyy kolme kertaa vuodessa.</skos:definition>
      <rdakit:toolkitDefinition xml:lang="fi">Ilmestymis- tai päivittymistiheys aineistolle, joka ilmestyy tai päivittyy kolme kertaa vuodessa.</rdakit:toolkitDefinition>
      <skos:prefLabel xml:lang="no">tre ganger i året</skos:prefLabel>
      <rdakit:toolkitLabel xml:lang="no">tre ganger i året</rdakit:toolkitLabel>
      <skos:definition xml:lang="no">En frekvens for en manifestasjon som blir utgitt eller oppdatert tre ganger hvert år.</skos:definition>
      <rdakit:toolkitDefinition xml:lang="no">En frekvens for en manifestasjon som blir utgitt eller oppdatert tre ganger hvert år.</rdakit:toolkitDefinition>
    </skos:Concept>
<!-- Concept: triennial  -->
    <skos:Concept rdf:about="http://rdaregistry.info/termList/frequency/1015" xml:lang="en">
      <skos:inScheme rdf:resource="http://rdaregistry.info/termList/frequency"/>
      <reg:status rdf:resource="http://metadataregistry.org/uri/RegStatus/1001"/>
      <reg:identifier rdf:resource="http://metadataregistry.org/concepts/759"/>
      <skos:prefLabel xml:lang="en">triennial</skos:prefLabel>
      <skos:definition xml:lang="en">A frequency for a manifestation issued or updated once every three years.</skos:definition>
      <skos:prefLabel xml:lang="de">alle drei Jahre</skos:prefLabel>
      <skos:prefLabel xml:lang="fr">triennal</skos:prefLabel>
      <skos:definition xml:lang="de">Eine Erscheinungsfrequenz für eine Manifestation, die einmal alle drei Jahre erscheint oder aktualisiert wird.</skos:definition>
      <skos:definition xml:lang="fr">Périodicité d’une manifestation publiée ou mise à jour tous les trois ans.</skos:definition>
      <skos:definition xml:lang="es">Frecuencia de un recurso publicado o actualizado una vez cada tres años.</skos:definition>
      <skos:prefLabel xml:lang="es">trienal</skos:prefLabel>
      <rdakit:toolkitLabel xml:lang="en">triennial</rdakit:toolkitLabel>
      <rdakit:toolkitLabel xml:lang="fr">triennal</rdakit:toolkitLabel>
      <rdakit:toolkitDefinition xml:lang="en">A frequency for a manifestation issued or updated once every three years.</rdakit:toolkitDefinition>
      <rdakit:toolkitDefinition xml:lang="fr">Périodicité d’une manifestation publiée ou mise à jour tous les trois ans.</rdakit:toolkitDefinition>
      <rdakit:toolkitLabel xml:lang="es">trienal</rdakit:toolkitLabel>
      <rdakit:toolkitDefinition xml:lang="es">Frecuencia de un recurso publicado o actualizado una vez cada tres años.</rdakit:toolkitDefinition>
      <skos:prefLabel xml:lang="zh">每三年</skos:prefLabel>
      <rdakit:toolkitLabel xml:lang="zh">每三年</rdakit:toolkitLabel>
      <skos:definition xml:lang="zh">资源发行或更新的频率为每三年一次。</skos:definition>
      <rdakit:toolkitDefinition xml:lang="zh">资源发行或更新的频率为每三年一次。</rdakit:toolkitDefinition>
      <skos:prefLabel xml:lang="nl">eens per drie jaar</skos:prefLabel>
      <rdakit:toolkitLabel xml:lang="nl">eens per drie jaar</rdakit:toolkitLabel>
      <skos:definition xml:lang="nl">Frequentie voor een resource die eens in de drie jaar uitgegeven of bijgewerkt wordt.</skos:definition>
      <rdakit:toolkitDefinition xml:lang="nl">Frequentie voor een resource die eens in de drie jaar uitgegeven of bijgewerkt wordt.</rdakit:toolkitDefinition>
      <rdakit:toolkitLabel xml:lang="de">alle drei Jahre</rdakit:toolkitLabel>
      <rdakit:toolkitDefinition xml:lang="de">Eine Erscheinungsfrequenz für eine Manifestation, die einmal alle drei Jahre erscheint oder aktualisiert wird.</rdakit:toolkitDefinition>
      <skos:prefLabel xml:lang="it">triennale</skos:prefLabel>
      <rdakit:toolkitLabel xml:lang="it">triennale</rdakit:toolkitLabel>
      <skos:prefLabel xml:lang="fi">kerran kolmessa vuodessa</skos:prefLabel>
      <rdakit:toolkitLabel xml:lang="fi">kerran kolmessa vuodessa</rdakit:toolkitLabel>
      <skos:prefLabel xml:lang="ar">مرة كل ثلاث سنوات</skos:prefLabel>
      <skos:prefLabel xml:lang="sv">var tredje år</skos:prefLabel>
      <rdakit:toolkitLabel xml:lang="sv">var tredje år</rdakit:toolkitLabel>
      <skos:prefLabel xml:lang="da">hvert 3. år</skos:prefLabel>
      <rdakit:toolkitLabel xml:lang="da">hvert 3. år</rdakit:toolkitLabel>
      <skos:definition xml:lang="da">Frekvens for en ressource, der udgives eller opdateres hvert tredje år.</skos:definition>
      <rdakit:toolkitDefinition xml:lang="da">Frekvens for en ressource, der udgives eller opdateres hvert tredje år.</rdakit:toolkitDefinition>
      <skos:prefLabel xml:lang="ca">triennal</skos:prefLabel>
      <rdakit:toolkitLabel xml:lang="ca">triennal</rdakit:toolkitLabel>
      <skos:definition xml:lang="ca">Periodicitat d’una manifestació que es publica o s’actualitza una vegada cada tres anys.</skos:definition>
      <rdakit:toolkitDefinition xml:lang="ca">Periodicitat d’una manifestació que es publica o s’actualitza una vegada cada tres anys.</rdakit:toolkitDefinition>
      <skos:prefLabel xml:lang="vi">hàng ba năm</skos:prefLabel>
      <rdakit:toolkitLabel xml:lang="vi">hàng ba năm</rdakit:toolkitLabel>
      <skos:definition xml:lang="vi">Tần số của biểu thị được công bố hoặc cập nhật ba năm một lần.</skos:definition>
      <rdakit:toolkitDefinition xml:lang="vi">Tần số của biểu thị được công bố hoặc cập nhật ba năm một lần.</rdakit:toolkitDefinition>
      <skos:definition xml:lang="fi">Ilmestymis- tai päivittymistiheys aineistolle, joka ilmestyy tai päivittyy kerran kolmessa vuodessa.</skos:definition>
      <rdakit:toolkitDefinition xml:lang="fi">Ilmestymis- tai päivittymistiheys aineistolle, joka ilmestyy tai päivittyy kerran kolmessa vuodessa.</rdakit:toolkitDefinition>
      <skos:prefLabel xml:lang="no">hvert tredje år</skos:prefLabel>
      <rdakit:toolkitLabel xml:lang="no">hvert tredje år</rdakit:toolkitLabel>
      <skos:definition xml:lang="no">En frekvens for en manifestasjon som blir utgitt eller oppdatert en gang hvert tredje år.</skos:definition>
      <rdakit:toolkitDefinition xml:lang="no">En frekvens for en manifestasjon som blir utgitt eller oppdatert en gang hvert tredje år.</rdakit:toolkitDefinition>
    </skos:Concept>
<!-- Concept: weekly  -->
    <skos:Concept rdf:about="http://rdaregistry.info/termList/frequency/1004" xml:lang="en">
      <skos:inScheme rdf:resource="http://rdaregistry.info/termList/frequency"/>
      <reg:status rdf:resource="http://metadataregistry.org/uri/RegStatus/1001"/>
      <reg:identifier rdf:resource="http://metadataregistry.org/concepts/748"/>
      <skos:prefLabel xml:lang="en">weekly</skos:prefLabel>
      <skos:definition xml:lang="en">A frequency for a manifestation issued or updated once every week.</skos:definition>
      <skos:prefLabel xml:lang="de">wöchentlich</skos:prefLabel>
      <skos:prefLabel xml:lang="fr">hebdomadaire</skos:prefLabel>
      <skos:definition xml:lang="de">Eine Erscheinungsfrequenz für eine Manifestation, die einmal pro Woche erscheint oder aktualisiert wird.</skos:definition>
      <skos:definition xml:lang="fr">Périodicité d’une manifestation publiée ou mise à jour une fois par semaine.</skos:definition>
      <skos:prefLabel xml:lang="es">semanal</skos:prefLabel>
      <rdakit:toolkitLabel xml:lang="en">weekly</rdakit:toolkitLabel>
      <rdakit:toolkitLabel xml:lang="fr">hebdomadaire</rdakit:toolkitLabel>
      <rdakit:toolkitDefinition xml:lang="en">A frequency for a manifestation issued or updated once every week.</rdakit:toolkitDefinition>
      <rdakit:toolkitDefinition xml:lang="fr">Périodicité d’une manifestation publiée ou mise à jour une fois par semaine.</rdakit:toolkitDefinition>
      <rdakit:toolkitLabel xml:lang="es">semanal</rdakit:toolkitLabel>
      <skos:prefLabel xml:lang="zh">每周</skos:prefLabel>
      <rdakit:toolkitLabel xml:lang="zh">每周</rdakit:toolkitLabel>
      <skos:definition xml:lang="zh">资源的发行或更新频率为每周一次。</skos:definition>
      <rdakit:toolkitDefinition xml:lang="zh">资源的发行或更新频率为每周一次。</rdakit:toolkitDefinition>
      <skos:definition xml:lang="es">Frecuencia de un recurso publicado o actualizado una vez por semana.</skos:definition>
      <rdakit:toolkitDefinition xml:lang="es">Frecuencia de un recurso publicado o actualizado una vez por semana.</rdakit:toolkitDefinition>
      <skos:prefLabel xml:lang="nl">wekelijks</skos:prefLabel>
      <rdakit:toolkitLabel xml:lang="nl">wekelijks</rdakit:toolkitLabel>
      <skos:definition xml:lang="nl">Frequentie voor een resource die eens per week uitgegeven of bijgewerkt wordt.</skos:definition>
      <rdakit:toolkitDefinition xml:lang="nl">Frequentie voor een resource die eens per week uitgegeven of bijgewerkt wordt.</rdakit:toolkitDefinition>
      <rdakit:toolkitLabel xml:lang="de">wöchentlich</rdakit:toolkitLabel>
      <rdakit:toolkitDefinition xml:lang="de">Eine Erscheinungsfrequenz für eine Manifestation, die einmal pro Woche erscheint oder aktualisiert wird.</rdakit:toolkitDefinition>
      <skos:prefLabel xml:lang="it">settimanale</skos:prefLabel>
      <rdakit:toolkitLabel xml:lang="it">settimanale</rdakit:toolkitLabel>
      <skos:prefLabel xml:lang="fi">viikoittain</skos:prefLabel>
      <rdakit:toolkitLabel xml:lang="fi">viikoittain</rdakit:toolkitLabel>
      <skos:prefLabel xml:lang="ar">اسبوعي</skos:prefLabel>
      <skos:prefLabel xml:lang="sv">1 nr/vecka</skos:prefLabel>
      <rdakit:toolkitLabel xml:lang="sv">1 nr/vecka</rdakit:toolkitLabel>
      <skos:prefLabel xml:lang="da">ugentlig</skos:prefLabel>
      <rdakit:toolkitLabel xml:lang="da">ugentlig</rdakit:toolkitLabel>
      <skos:definition xml:lang="da">Frekvens for en ressource, der udgives eller opdateres hver uge.</skos:definition>
      <rdakit:toolkitDefinition xml:lang="da">Frekvens for en ressource, der udgives eller opdateres hver uge.</rdakit:toolkitDefinition>
      <skos:prefLabel xml:lang="ca">setmanal</skos:prefLabel>
      <rdakit:toolkitLabel xml:lang="ca">setmanal</rdakit:toolkitLabel>
      <skos:definition xml:lang="ca">Periodicitat d’una manifestació que es publica o s’actualitza una vegada cada setmana.</skos:definition>
      <rdakit:toolkitDefinition xml:lang="ca">Periodicitat d’una manifestació que es publica o s’actualitza una vegada cada setmana.</rdakit:toolkitDefinition>
      <skos:prefLabel xml:lang="vi">hàng tuần</skos:prefLabel>
      <rdakit:toolkitLabel xml:lang="vi">hàng tuần</rdakit:toolkitLabel>
      <skos:definition xml:lang="vi">Tần số cho mộtbiểu thị được công bốhoặc cập nhậtmộtlần mỗituần.</skos:definition>
      <rdakit:toolkitDefinition xml:lang="vi">Tần số cho mộtbiểu thị được công bốhoặc cập nhậtmộtlần mỗituần.</rdakit:toolkitDefinition>
      <skos:definition xml:lang="fi">Ilmestymis- tai päivittymistiheys aineistolle, joka ilmestyy tai päivittyy kerran viikossa.</skos:definition>
      <rdakit:toolkitDefinition xml:lang="fi">Ilmestymis- tai päivittymistiheys aineistolle, joka ilmestyy tai päivittyy kerran viikossa.</rdakit:toolkitDefinition>
      <skos:prefLabel xml:lang="no">ukentlig</skos:prefLabel>
      <rdakit:toolkitLabel xml:lang="no">ukentlig</rdakit:toolkitLabel>
      <skos:definition xml:lang="no">En frekvens for en manifestasjon som blir utgitt eller oppdatert en gang hver uke.</skos:definition>
      <rdakit:toolkitDefinition xml:lang="no">En frekvens for en manifestasjon som blir utgitt eller oppdatert en gang hver uke.</rdakit:toolkitDefinition>
    </skos:Concept>

<!-- Status properties used in this document  -->
    <skos:Concept rdf:about="http://metadataregistry.org/uri/RegStatus/1001">
        <skos:prefLabel xml:lang="en">Published</skos:prefLabel>
    </skos:Concept>

</rdf:RDF>
