<?xml version="1.0" encoding = "UTF-8"?>
<rdf:RDF
    xmlns:dc="http://purl.org/dc/elements/1.1/"
    xmlns:rdakit="http://metadataregistry.org/uri/profile/rdakit/"
    xmlns:rdf="http://www.w3.org/1999/02/22-rdf-syntax-ns#"
    xmlns:reg="http://metadataregistry.org/uri/profile/regap/"
    xmlns:owl="http://www.w3.org/2002/07/owl#"
    xmlns:skos="http://www.w3.org/2004/02/skos/core#">

<owl:Ontology rdf:about="http://rdaregistry.info/termList/layout" />
<!-- Scheme: RDA Layout -->
    <skos:ConceptScheme rdf:about="http://rdaregistry.info/termList/layout">
        <dc:title>RDA Layout</dc:title>
    </skos:ConceptScheme>

<!-- Concept: back to back  -->
    <skos:Concept rdf:about="http://rdaregistry.info/termList/layout/1003" xml:lang="en">
      <skos:inScheme rdf:resource="http://rdaregistry.info/termList/layout"/>
      <reg:status rdf:resource="http://metadataregistry.org/uri/RegStatus/1001"/>
      <reg:identifier rdf:resource="http://metadataregistry.org/concepts/8436"/>
      <skos:prefLabel xml:lang="en">back to back</skos:prefLabel>
      <rdakit:toolkitLabel xml:lang="en">back to back</rdakit:toolkitLabel>
      <skos:definition xml:lang="en">A layout in which the same image is represented in more than one language on each side of a sheet.</skos:definition>
      <rdakit:toolkitDefinition xml:lang="en">A layout in which the same image is represented in more than one language on each side of a sheet.</rdakit:toolkitDefinition>
      <skos:scopeNote xml:lang="en">This term applies to cartographic images.</skos:scopeNote>
      <skos:prefLabel xml:lang="it">back-to-back</skos:prefLabel>
      <rdakit:toolkitLabel xml:lang="it">back-to-back</rdakit:toolkitLabel>
      <skos:prefLabel xml:lang="de">back to back</skos:prefLabel>
      <rdakit:toolkitLabel xml:lang="de">back to back</rdakit:toolkitLabel>
      <skos:definition xml:lang="de">Ein Layout, in dem das gleiche Bild in mehr als einer Sprache auf jeder Seite eines Blattes dargestellt wird.</skos:definition>
      <rdakit:toolkitDefinition xml:lang="de">Ein Layout, in dem das gleiche Bild in mehr als einer Sprache auf jeder Seite eines Blattes dargestellt wird.</rdakit:toolkitDefinition>
      <skos:scopeNote xml:lang="de">Dieser Terminus trifft auf kartografische Bilder zu.</skos:scopeNote>
      <skos:prefLabel xml:lang="fi">kääntöpuolilla</skos:prefLabel>
      <rdakit:toolkitLabel xml:lang="fi">kääntöpuolilla</rdakit:toolkitLabel>
      <skos:definition xml:lang="fi">Layout, jossa sama kuva esitetään useammalla kuin yhdellä kielellä arkin molemmin puolin.</skos:definition>
      <rdakit:toolkitDefinition xml:lang="fi">Layout, jossa sama kuva esitetään useammalla kuin yhdellä kielellä arkin molemmin puolin.</rdakit:toolkitDefinition>
      <skos:scopeNote xml:lang="fi">Termi koskee kartografisia kuvia.</skos:scopeNote>
      <skos:prefLabel xml:lang="vi">giáp lưng</skos:prefLabel>
      <rdakit:toolkitLabel xml:lang="vi">giáp lưng</rdakit:toolkitLabel>
      <skos:definition xml:lang="vi">Sắp đặt trong đó cùng một hình ảnh được trình bày theo hai hoặc nhiều hơn ngôn ngữ trên mỗi mặt của tờ.</skos:definition>
      <rdakit:toolkitDefinition xml:lang="vi">Sắp đặt trong đó cùng một hình ảnh được trình bày theo hai hoặc nhiều hơn ngôn ngữ trên mỗi mặt của tờ.</rdakit:toolkitDefinition>
      <skos:scopeNote xml:lang="vi">Thuật ngữ này áp dụng cho hình ảnh bản đồ.</skos:scopeNote>
      <skos:prefLabel xml:lang="da">back to back</skos:prefLabel>
      <rdakit:toolkitLabel xml:lang="da">back to back</rdakit:toolkitLabel>
      <skos:definition xml:lang="da">Layout hvor det samme billede er repræsenteret ved mere end ét sprog på hver side af et ark.</skos:definition>
      <rdakit:toolkitDefinition xml:lang="da">Layout hvor det samme billede er repræsenteret ved mere end ét sprog på hver side af et ark.</rdakit:toolkitDefinition>
      <skos:scopeNote xml:lang="da">Denne term anvendes til kartografiske billeder.</skos:scopeNote>
      <skos:prefLabel xml:lang="fr">dos à dos</skos:prefLabel>
      <rdakit:toolkitLabel xml:lang="fr">dos à dos</rdakit:toolkitLabel>
      <skos:definition xml:lang="fr">Disposition dans laquelle la même image est présentée dans plus d’une langue sur chaque côté d’une feuille.</skos:definition>
      <rdakit:toolkitDefinition xml:lang="fr">Disposition dans laquelle la même image est présentée dans plus d’une langue sur chaque côté d’une feuille.</rdakit:toolkitDefinition>
      <skos:scopeNote xml:lang="fr">Ce terme s’applique aux images cartographiques.</skos:scopeNote>
      <skos:prefLabel xml:lang="no">back to back</skos:prefLabel>
      <rdakit:toolkitLabel xml:lang="no">back to back</rdakit:toolkitLabel>
      <skos:definition xml:lang="no">Et oppsett der det samme bildet er gjengitt på mer enn ett språk på hver side av et ark.</skos:definition>
      <rdakit:toolkitDefinition xml:lang="no">Et oppsett der det samme bildet er gjengitt på mer enn ett språk på hver side av et ark.</rdakit:toolkitDefinition>
      <skos:scopeNote xml:lang="no">Dette begrepet gjelder kartografiske bilder.</skos:scopeNote>
    </skos:Concept>
<!-- Concept: bar by bar  -->
    <skos:Concept rdf:about="http://rdaregistry.info/termList/layout/1004" xml:lang="en">
      <skos:inScheme rdf:resource="http://rdaregistry.info/termList/layout"/>
      <reg:status rdf:resource="http://metadataregistry.org/uri/RegStatus/1001"/>
      <reg:identifier rdf:resource="http://metadataregistry.org/concepts/8437"/>
      <skos:prefLabel xml:lang="en">bar by bar</skos:prefLabel>
      <rdakit:toolkitLabel xml:lang="en">bar by bar</rdakit:toolkitLabel>
      <skos:definition xml:lang="en">A layout consisting of music displayed in indented paragraphs with all of the parts for each measure written consecutively.</skos:definition>
      <rdakit:toolkitDefinition xml:lang="en">A layout consisting of music displayed in indented paragraphs with all of the parts for each measure written consecutively.</rdakit:toolkitDefinition>
      <skos:scopeNote xml:lang="en">This term applies to tactile music resources.</skos:scopeNote>
      <skos:prefLabel xml:lang="it">battuta per battuta</skos:prefLabel>
      <rdakit:toolkitLabel xml:lang="it">battuta per battuta</rdakit:toolkitLabel>
      <skos:prefLabel xml:lang="de">Takt für Takt</skos:prefLabel>
      <rdakit:toolkitLabel xml:lang="de">Takt für Takt</rdakit:toolkitLabel>
      <skos:definition xml:lang="de">Ein Layout, bei dem Noten in eingerückten Absätzen dargestellt werden, wobei alle Stimmen für jeden Takt nacheinander folgend geschrieben sind.</skos:definition>
      <rdakit:toolkitDefinition xml:lang="de">Ein Layout, bei dem Noten in eingerückten Absätzen dargestellt werden, wobei alle Stimmen für jeden Takt nacheinander folgend geschrieben sind.</rdakit:toolkitDefinition>
      <skos:scopeNote xml:lang="de">Dieser Terminus trifft auf taktile Musikressourcen zu.</skos:scopeNote>
      <skos:prefLabel xml:lang="fi">tahdit peräkkäin</skos:prefLabel>
      <rdakit:toolkitLabel xml:lang="fi">tahdit peräkkäin</rdakit:toolkitLabel>
      <skos:definition xml:lang="fi">Layout, joka koostuu sisennetyissä kappaleissa esitetystä nuottikirjoituksesta, ja jossa jokaisen tahdin stemmat on merkitty peräkkäin.</skos:definition>
      <rdakit:toolkitDefinition xml:lang="fi">Layout, joka koostuu sisennetyissä kappaleissa esitetystä nuottikirjoituksesta, ja jossa jokaisen tahdin stemmat on merkitty peräkkäin.</rdakit:toolkitDefinition>
      <skos:scopeNote xml:lang="fi">Termi koskee taktiileja musiikkiaineistoja.</skos:scopeNote>
      <skos:prefLabel xml:lang="vi">gạch nhịp sau gạch nhịp</skos:prefLabel>
      <rdakit:toolkitLabel xml:lang="vi">gạch nhịp sau gạch nhịp</rdakit:toolkitLabel>
      <skos:definition xml:lang="vi">Sắp đặt bao gồm có âm nhạc được hiện trong các đoạn dự kiến với tất cả các phần cho mỗi nhịp được viết liên tiếp.</skos:definition>
      <rdakit:toolkitDefinition xml:lang="vi">Sắp đặt bao gồm có âm nhạc được hiện trong các đoạn dự kiến với tất cả các phần cho mỗi nhịp được viết liên tiếp.</rdakit:toolkitDefinition>
      <skos:scopeNote xml:lang="vi">Thuật ngữ này áp dụng cho tài nguyên âm nhạc xúc giác.</skos:scopeNote>
      <skos:prefLabel xml:lang="da">takt for takt</skos:prefLabel>
      <rdakit:toolkitLabel xml:lang="da">takt for takt</rdakit:toolkitLabel>
      <skos:definition xml:lang="da">Layout bestående af musik vist i indrykkede afsnit med alle stemmerne for hver takt skrevet efter hinanden.</skos:definition>
      <rdakit:toolkitDefinition xml:lang="da">Layout bestående af musik vist i indrykkede afsnit med alle stemmerne for hver takt skrevet efter hinanden.</rdakit:toolkitDefinition>
      <skos:scopeNote xml:lang="da">Denne term anvendes til taktile musik-ressourcer.</skos:scopeNote>
      <skos:prefLabel xml:lang="fr">mesure par mesure</skos:prefLabel>
      <rdakit:toolkitLabel xml:lang="fr">mesure par mesure</rdakit:toolkitLabel>
      <skos:definition xml:lang="fr">Disposition qui consiste en musique présentée sous forme de paragraphes en retrait dans lesquels toutes les parties figurant dans une même mesure sont écrites l’une à la suite de l’autre.</skos:definition>
      <rdakit:toolkitDefinition xml:lang="fr">Disposition qui consiste en musique présentée sous forme de paragraphes en retrait dans lesquels toutes les parties figurant dans une même mesure sont écrites l’une à la suite de l’autre.</rdakit:toolkitDefinition>
      <skos:scopeNote xml:lang="fr">Ce terme s’applique aux ressources de musique tactile.</skos:scopeNote>
      <skos:prefLabel xml:lang="no">bar by bar</skos:prefLabel>
      <rdakit:toolkitLabel xml:lang="no">bar by bar</rdakit:toolkitLabel>
      <skos:definition xml:lang="no">Et oppsett som består av noter vist i avsnitt med innrykk der alle stemmene for hver takt er skrevet fortløpende.</skos:definition>
      <rdakit:toolkitDefinition xml:lang="no">Et oppsett som består av noter vist i avsnitt med innrykk der alle stemmene for hver takt er skrevet fortløpende.</rdakit:toolkitDefinition>
      <skos:scopeNote xml:lang="no">Dette begrepet gjelder taktile musikkressurser.</skos:scopeNote>
    </skos:Concept>
<!-- Concept: bar over bar  -->
    <skos:Concept rdf:about="http://rdaregistry.info/termList/layout/1005" xml:lang="en">
      <skos:inScheme rdf:resource="http://rdaregistry.info/termList/layout"/>
      <reg:status rdf:resource="http://metadataregistry.org/uri/RegStatus/1001"/>
      <reg:identifier rdf:resource="http://metadataregistry.org/concepts/8438"/>
      <skos:prefLabel xml:lang="en">bar over bar</skos:prefLabel>
      <rdakit:toolkitLabel xml:lang="en">bar over bar</rdakit:toolkitLabel>
      <skos:definition xml:lang="en">A layout consisting of measures displayed in units called parallels and that the beginning of each part’s measure is vertically aligned with the beginning of the same measure for the other part or parts.</skos:definition>
      <rdakit:toolkitDefinition xml:lang="en">A layout consisting of measures displayed in units called parallels and that the beginning of each part’s measure is vertically aligned with the beginning of the same measure for the other part or parts.</rdakit:toolkitDefinition>
      <skos:scopeNote xml:lang="en">This term applies to tactile music resources.</skos:scopeNote>
      <skos:prefLabel xml:lang="it">battuta sopra battuta</skos:prefLabel>
      <rdakit:toolkitLabel xml:lang="it">battuta sopra battuta</rdakit:toolkitLabel>
      <skos:prefLabel xml:lang="de">Takt über Takt</skos:prefLabel>
      <rdakit:toolkitLabel xml:lang="de">Takt über Takt</rdakit:toolkitLabel>
      <skos:definition xml:lang="de">Ein Layout, bei dem Noten in Einheiten, sogenannten Parallelen, dargestellt werden, wobei der Beginn eines Takts bei jeder Stimme senkrecht über dem gleichen Takt für jede andere Stimme steht.</skos:definition>
      <rdakit:toolkitDefinition xml:lang="de">Ein Layout, bei dem Noten in Einheiten, sogenannten Parallelen, dargestellt werden, wobei der Beginn eines Takts bei jeder Stimme senkrecht über dem gleichen Takt für jede andere Stimme steht.</rdakit:toolkitDefinition>
      <skos:scopeNote xml:lang="de">Dieser Terminus trifft auf taktile Musikressourcen zu.</skos:scopeNote>
      <skos:prefLabel xml:lang="fi">tahdit allekkain</skos:prefLabel>
      <rdakit:toolkitLabel xml:lang="fi">tahdit allekkain</rdakit:toolkitLabel>
      <skos:definition xml:lang="fi">Layout, joka koostuu rinnakkaisissa yksiköissä esitetyistä tahdeista siten, että kunkin stemman tahdin alku on pystysuuntaisesti tasattu toisen stemman tai stemmojen saman tahdin alun kanssa.</skos:definition>
      <rdakit:toolkitDefinition xml:lang="fi">Layout, joka koostuu rinnakkaisissa yksiköissä esitetyistä tahdeista siten, että kunkin stemman tahdin alku on pystysuuntaisesti tasattu toisen stemman tai stemmojen saman tahdin alun kanssa.</rdakit:toolkitDefinition>
      <skos:scopeNote xml:lang="fi">Termi koskee taktiileja musiikkiaineistoja.</skos:scopeNote>
      <skos:prefLabel xml:lang="vi">gạch nhịp trên gạch nhịp</skos:prefLabel>
      <rdakit:toolkitLabel xml:lang="vi">gạch nhịp trên gạch nhịp</rdakit:toolkitLabel>
      <skos:definition xml:lang="vi">Sắp đặt gồm có các nhịp được hiện thành các đơn vị gọi là tương đương bắt đầu mỗi nhịp được sắp hàng dọc với bắt đầu bằng cùng nhịp cho mỗi phần hoặc các phần.</skos:definition>
      <rdakit:toolkitDefinition xml:lang="vi">Sắp đặt gồm có các nhịp được hiện thành các đơn vị gọi là tương đương bắt đầu mỗi nhịp được sắp hàng dọc với bắt đầu bằng cùng nhịp cho mỗi phần hoặc các phần.</rdakit:toolkitDefinition>
      <skos:scopeNote xml:lang="vi">Thuật ngữ này áp dụng cho tài nguyên âm nhạc xúc giác.</skos:scopeNote>
      <skos:prefLabel xml:lang="da">takt over takt</skos:prefLabel>
      <rdakit:toolkitLabel xml:lang="da">takt over takt</rdakit:toolkitLabel>
      <skos:definition xml:lang="da">Layout bestående af musik vist i enheder kaldet paralleller og hvor starten af hver stemmes takt er på linje med starten af den samme takt for den anden stemme eller stemmer.</skos:definition>
      <rdakit:toolkitDefinition xml:lang="da">Layout bestående af musik vist i enheder kaldet paralleller og hvor starten af hver stemmes takt er på linje med starten af den samme takt for den anden stemme eller stemmer.</rdakit:toolkitDefinition>
      <skos:scopeNote xml:lang="da">Denne term anvendes til taktile musik-ressourcer.</skos:scopeNote>
      <skos:prefLabel xml:lang="fr">mesure sur mesure</skos:prefLabel>
      <rdakit:toolkitLabel xml:lang="fr">mesure sur mesure</rdakit:toolkitLabel>
      <skos:definition xml:lang="fr">Disposition qui consiste en mesures présentées sous forme d’unités appelées parallèles dans lesquelles le début de chaque mesure dans une partie donnée est aligné verticalement avec le début de la même mesure dans la ou les autres parties.</skos:definition>
      <rdakit:toolkitDefinition xml:lang="fr">Disposition qui consiste en mesures présentées sous forme d’unités appelées parallèles dans lesquelles le début de chaque mesure dans une partie donnée est aligné verticalement avec le début de la même mesure dans la ou les autres parties.</rdakit:toolkitDefinition>
      <skos:scopeNote xml:lang="fr">Ce terme s’applique aux ressources de musique tactile.</skos:scopeNote>
      <skos:prefLabel xml:lang="no">bar over bar</skos:prefLabel>
      <rdakit:toolkitLabel xml:lang="no">bar over bar</rdakit:toolkitLabel>
      <skos:definition xml:lang="no">Et oppsett som består av takter som vises i parallelle enheter der begynnelsen takten for hver stemme er på loddrett linje med begynnelsen av samme takten for alle de andre stemmene.</skos:definition>
      <rdakit:toolkitDefinition xml:lang="no">Et oppsett som består av takter som vises i parallelle enheter der begynnelsen takten for hver stemme er på loddrett linje med begynnelsen av samme takten for alle de andre stemmene.</rdakit:toolkitDefinition>
      <skos:scopeNote xml:lang="no">Dette begrepet gjelder taktile musikkressurser.</skos:scopeNote>
    </skos:Concept>
<!-- Concept: both sides  -->
    <skos:Concept rdf:about="http://rdaregistry.info/termList/layout/1006" xml:lang="en">
      <skos:inScheme rdf:resource="http://rdaregistry.info/termList/layout"/>
      <reg:status rdf:resource="http://metadataregistry.org/uri/RegStatus/1001"/>
      <reg:identifier rdf:resource="http://metadataregistry.org/concepts/8439"/>
      <skos:prefLabel xml:lang="en">both sides</skos:prefLabel>
      <rdakit:toolkitLabel xml:lang="en">both sides</rdakit:toolkitLabel>
      <skos:definition xml:lang="en">A layout that is continued at the same scale on both sides of a sheet or sheets.</skos:definition>
      <rdakit:toolkitDefinition xml:lang="en">A layout that is continued at the same scale on both sides of a sheet or sheets.</rdakit:toolkitDefinition>
      <skos:scopeNote xml:lang="en">This term applies to cartographic images.</skos:scopeNote>
      <skos:prefLabel xml:lang="it">entrambi i lati</skos:prefLabel>
      <rdakit:toolkitLabel xml:lang="it">entrambi i lati</rdakit:toolkitLabel>
      <skos:prefLabel xml:lang="de">beidseitig</skos:prefLabel>
      <rdakit:toolkitLabel xml:lang="de">beidseitig</rdakit:toolkitLabel>
      <skos:definition xml:lang="de">Ein Layout, das im selben Maßstab auf beiden Seiten eines Blattes fortgesetzt wird.</skos:definition>
      <rdakit:toolkitDefinition xml:lang="de">Ein Layout, das im selben Maßstab auf beiden Seiten eines Blattes fortgesetzt wird.</rdakit:toolkitDefinition>
      <skos:scopeNote xml:lang="de">Dieser Terminus trifft auf kartografische Bilder zu.</skos:scopeNote>
      <skos:prefLabel xml:lang="fi">molemmilla puolilla</skos:prefLabel>
      <rdakit:toolkitLabel xml:lang="fi">molemmilla puolilla</rdakit:toolkitLabel>
      <skos:definition xml:lang="fi">Layout, joka jatkuu samassa mittakaavassa arkin tai arkkien molemmilla puolilla.</skos:definition>
      <rdakit:toolkitDefinition xml:lang="fi">Layout, joka jatkuu samassa mittakaavassa arkin tai arkkien molemmilla puolilla.</rdakit:toolkitDefinition>
      <skos:scopeNote xml:lang="fi">Termi koskee kartografisia kuvia.</skos:scopeNote>
      <skos:prefLabel xml:lang="vi">cả hai mặt</skos:prefLabel>
      <rdakit:toolkitLabel xml:lang="vi">cả hai mặt</rdakit:toolkitLabel>
      <skos:definition xml:lang="vi">Sắp đặt được tiếp tục theo cùng tỷ lệ trên cả hai mặt của tờ hoặc các tờ.</skos:definition>
      <rdakit:toolkitDefinition xml:lang="vi">Sắp đặt được tiếp tục theo cùng tỷ lệ trên cả hai mặt của tờ hoặc các tờ.</rdakit:toolkitDefinition>
      <skos:scopeNote xml:lang="vi">Thuật ngữ này áp dụng cho hình ảnh bản đồ.</skos:scopeNote>
      <skos:prefLabel xml:lang="da">begge sider</skos:prefLabel>
      <rdakit:toolkitLabel xml:lang="da">begge sider</rdakit:toolkitLabel>
      <skos:definition xml:lang="da">Layout der er fortsat i samme målestoksforhold på begge sider af et eller flere ark.</skos:definition>
      <rdakit:toolkitDefinition xml:lang="da">Layout der er fortsat i samme målestoksforhold på begge sider af et eller flere ark.</rdakit:toolkitDefinition>
      <skos:scopeNote xml:lang="da">Denne term anvendes til kartografiske billeder.</skos:scopeNote>
      <skos:prefLabel xml:lang="fr">recto verso</skos:prefLabel>
      <rdakit:toolkitLabel xml:lang="fr">recto verso</rdakit:toolkitLabel>
      <skos:definition xml:lang="fr">Disposition qui se poursuit à la même échelle sur les deux côtés d’une ou plusieurs feuilles.</skos:definition>
      <rdakit:toolkitDefinition xml:lang="fr">Disposition qui se poursuit à la même échelle sur les deux côtés d’une ou plusieurs feuilles.</rdakit:toolkitDefinition>
      <skos:scopeNote xml:lang="fr">Ce terme s’applique aux images cartographiques.</skos:scopeNote>
      <skos:prefLabel xml:lang="no">begge sider</skos:prefLabel>
      <rdakit:toolkitLabel xml:lang="no">begge sider</rdakit:toolkitLabel>
      <skos:definition xml:lang="no">Et oppsett som fortsetter i samme målestokk på gegge sider av ett eller flere ark.</skos:definition>
      <rdakit:toolkitDefinition xml:lang="no">Et oppsett som fortsetter i samme målestokk på gegge sider av ett eller flere ark.</rdakit:toolkitDefinition>
      <skos:scopeNote xml:lang="no">Dette begrepet gjelder kartografiske bilder.</skos:scopeNote>
    </skos:Concept>
<!-- Concept: double line spacing  -->
    <skos:Concept rdf:about="http://rdaregistry.info/termList/layout/1017" xml:lang="en">
      <skos:inScheme rdf:resource="http://rdaregistry.info/termList/layout"/>
      <reg:status rdf:resource="http://metadataregistry.org/uri/RegStatus/1001"/>
      <reg:identifier rdf:resource="http://metadataregistry.org/concepts/8450"/>
      <skos:prefLabel xml:lang="en">double line spacing</skos:prefLabel>
      <rdakit:toolkitLabel xml:lang="en">double line spacing</rdakit:toolkitLabel>
      <skos:definition xml:lang="en">A layout containing a full blank line between lines of text.</skos:definition>
      <rdakit:toolkitDefinition xml:lang="en">A layout containing a full blank line between lines of text.</rdakit:toolkitDefinition>
      <skos:scopeNote xml:lang="en">This term applies to tactile text.</skos:scopeNote>
      <skos:prefLabel xml:lang="it">interlinea doppia</skos:prefLabel>
      <rdakit:toolkitLabel xml:lang="it">interlinea doppia</rdakit:toolkitLabel>
      <skos:prefLabel xml:lang="de">doppelter Zeilenabstand</skos:prefLabel>
      <rdakit:toolkitLabel xml:lang="de">doppelter Zeilenabstand</rdakit:toolkitLabel>
      <skos:definition xml:lang="de">Ein Layout, das eine ganze Leerzeile zwischen den Zeilen eines Textes enthält.</skos:definition>
      <rdakit:toolkitDefinition xml:lang="de">Ein Layout, das eine ganze Leerzeile zwischen den Zeilen eines Textes enthält.</rdakit:toolkitDefinition>
      <skos:scopeNote xml:lang="de">Dieser Terminus trifft auf taktilen Text zu.</skos:scopeNote>
      <skos:prefLabel xml:lang="fi">harvennettu riviväli</skos:prefLabel>
      <rdakit:toolkitLabel xml:lang="fi">harvennettu riviväli</rdakit:toolkitLabel>
      <skos:definition xml:lang="fi">Layout, jossa tekstirivien välillä on tyhjä rivi.</skos:definition>
      <rdakit:toolkitDefinition xml:lang="fi">Layout, jossa tekstirivien välillä on tyhjä rivi.</rdakit:toolkitDefinition>
      <skos:scopeNote xml:lang="fi">Termi koskee taktiilia tekstiä.</skos:scopeNote>
      <skos:prefLabel xml:lang="vi">cách dòng đúp</skos:prefLabel>
      <rdakit:toolkitLabel xml:lang="vi">cách dòng đúp</rdakit:toolkitLabel>
      <skos:definition xml:lang="vi">Sắp đặt có chứa một dòng trống hoàn toàn giữa các dòng văn bản.</skos:definition>
      <rdakit:toolkitDefinition xml:lang="vi">Sắp đặt có chứa một dòng trống hoàn toàn giữa các dòng văn bản.</rdakit:toolkitDefinition>
      <skos:scopeNote xml:lang="vi">Thuật ngữ này áp dụng cho văn bản xúc giác.</skos:scopeNote>
      <skos:prefLabel xml:lang="da">dobbelt linjeafstand</skos:prefLabel>
      <rdakit:toolkitLabel xml:lang="da">dobbelt linjeafstand</rdakit:toolkitLabel>
      <skos:definition xml:lang="da">Layout indeholdende en hel blank linje mellem linjer med tekst.</skos:definition>
      <rdakit:toolkitDefinition xml:lang="da">Layout indeholdende en hel blank linje mellem linjer med tekst.</rdakit:toolkitDefinition>
      <skos:scopeNote xml:lang="da">Denne term anvendes til taktil tekst.</skos:scopeNote>
      <skos:prefLabel xml:lang="fr">double interligne</skos:prefLabel>
      <rdakit:toolkitLabel xml:lang="fr">double interligne</rdakit:toolkitLabel>
      <skos:definition xml:lang="fr">Disposition comprenant une ligne vide complète entre les lignes de texte.</skos:definition>
      <rdakit:toolkitDefinition xml:lang="fr">Disposition comprenant une ligne vide complète entre les lignes de texte.</rdakit:toolkitDefinition>
      <skos:scopeNote xml:lang="fr">Ce terme s’applique au texte tactile.</skos:scopeNote>
      <skos:prefLabel xml:lang="no">dobbel linjeavstand</skos:prefLabel>
      <rdakit:toolkitLabel xml:lang="no">dobbel linjeavstand</rdakit:toolkitLabel>
      <skos:definition xml:lang="no">Et oppsett med en hel tom linje mellom hver tekstlinje.</skos:definition>
      <rdakit:toolkitDefinition xml:lang="no">Et oppsett med en hel tom linje mellom hver tekstlinje.</rdakit:toolkitDefinition>
      <skos:scopeNote xml:lang="no">Dette begrepet gjelder taktil tekst.</skos:scopeNote>
    </skos:Concept>
<!-- Concept: double sided  -->
    <skos:Concept rdf:about="http://rdaregistry.info/termList/layout/1001" xml:lang="en">
      <skos:inScheme rdf:resource="http://rdaregistry.info/termList/layout"/>
      <reg:status rdf:resource="http://metadataregistry.org/uri/RegStatus/1001"/>
      <reg:identifier rdf:resource="http://metadataregistry.org/concepts/836"/>
      <skos:prefLabel xml:lang="en">double sided</skos:prefLabel>
      <rdakit:toolkitLabel xml:lang="en">double sided</rdakit:toolkitLabel>
      <skos:definition xml:lang="en">A layout that uses both sides of a sheet.</skos:definition>
      <rdakit:toolkitDefinition xml:lang="en">A layout that uses both sides of a sheet.</rdakit:toolkitDefinition>
      <skos:scopeNote xml:lang="en">This term applies to sheets and tactile text.</skos:scopeNote>
      <skos:prefLabel xml:lang="it">fronte retro</skos:prefLabel>
      <rdakit:toolkitLabel xml:lang="it">fronte retro</rdakit:toolkitLabel>
      <skos:prefLabel xml:lang="de">doppelseitig</skos:prefLabel>
      <rdakit:toolkitLabel xml:lang="de">doppelseitig</rdakit:toolkitLabel>
      <skos:definition xml:lang="de">Ein Layout, das beide Seiten eines Blatts verwendet.</skos:definition>
      <rdakit:toolkitDefinition xml:lang="de">Ein Layout, das beide Seiten eines Blatts verwendet.</rdakit:toolkitDefinition>
      <skos:scopeNote xml:lang="de">Dieser Terminus trifft auf Blätter und taktilen Text zu.</skos:scopeNote>
      <skos:prefLabel xml:lang="fi">kaksipuolinen</skos:prefLabel>
      <rdakit:toolkitLabel xml:lang="fi">kaksipuolinen</rdakit:toolkitLabel>
      <skos:definition xml:lang="fi">Layout molemmin puolin arkkia.</skos:definition>
      <rdakit:toolkitDefinition xml:lang="fi">Layout molemmin puolin arkkia.</rdakit:toolkitDefinition>
      <skos:scopeNote xml:lang="fi">Termi koskee arkkeja sekä taktiilia tekstiä.</skos:scopeNote>
      <skos:prefLabel xml:lang="vi">hai mặt</skos:prefLabel>
      <rdakit:toolkitLabel xml:lang="vi">hai mặt</rdakit:toolkitLabel>
      <skos:definition xml:lang="vi">Sắp đặt sử dụng cả hai mặt của tờ.</skos:definition>
      <rdakit:toolkitDefinition xml:lang="vi">Sắp đặt sử dụng cả hai mặt của tờ.</rdakit:toolkitDefinition>
      <skos:scopeNote xml:lang="vi">Thuật ngữ này áp dụng cho tờ và văn bản xúc giác.</skos:scopeNote>
      <skos:prefLabel xml:lang="da">dobbeltsidet</skos:prefLabel>
      <rdakit:toolkitLabel xml:lang="da">dobbeltsidet</rdakit:toolkitLabel>
      <skos:definition xml:lang="da">Layout der anvender begge sider af et ark.</skos:definition>
      <rdakit:toolkitDefinition xml:lang="da">Layout der anvender begge sider af et ark.</rdakit:toolkitDefinition>
      <skos:scopeNote xml:lang="da">Denne term anvendes til ark og taktil tekst.</skos:scopeNote>
      <skos:prefLabel xml:lang="fr">double face</skos:prefLabel>
      <rdakit:toolkitLabel xml:lang="fr">double face</rdakit:toolkitLabel>
      <skos:definition xml:lang="fr">Disposition qui utilise les deux côtés d’une feuille.</skos:definition>
      <rdakit:toolkitDefinition xml:lang="fr">Disposition qui utilise les deux côtés d’une feuille.</rdakit:toolkitDefinition>
      <skos:scopeNote xml:lang="fr">Ce terme s’applique aux feuilles et au texte tactile.</skos:scopeNote>
      <skos:prefLabel xml:lang="no">tosidig</skos:prefLabel>
      <rdakit:toolkitLabel xml:lang="no">tosidig</rdakit:toolkitLabel>
      <skos:definition xml:lang="no">Et oppsett som bruker begge sider av et ark.</skos:definition>
      <rdakit:toolkitDefinition xml:lang="no">Et oppsett som bruker begge sider av et ark.</rdakit:toolkitDefinition>
      <skos:scopeNote xml:lang="no">Dette begrepet gjelder ark og taktil tekst.</skos:scopeNote>
    </skos:Concept>
<!-- Concept: line by line  -->
    <skos:Concept rdf:about="http://rdaregistry.info/termList/layout/1007" xml:lang="en">
      <skos:inScheme rdf:resource="http://rdaregistry.info/termList/layout"/>
      <reg:status rdf:resource="http://metadataregistry.org/uri/RegStatus/1001"/>
      <reg:identifier rdf:resource="http://metadataregistry.org/concepts/8440"/>
      <skos:prefLabel xml:lang="en">line by line</skos:prefLabel>
      <rdakit:toolkitLabel xml:lang="en">line by line</rdakit:toolkitLabel>
      <skos:definition xml:lang="en">A layout consisting of lines of text that alternate with lines of music for the preceding text.</skos:definition>
      <rdakit:toolkitDefinition xml:lang="en">A layout consisting of lines of text that alternate with lines of music for the preceding text.</rdakit:toolkitDefinition>
      <skos:scopeNote xml:lang="en">This term applies to tactile music resources.</skos:scopeNote>
      <skos:prefLabel xml:lang="it">linea per linea</skos:prefLabel>
      <rdakit:toolkitLabel xml:lang="it">linea per linea</rdakit:toolkitLabel>
      <skos:prefLabel xml:lang="de">Linie für Linie</skos:prefLabel>
      <rdakit:toolkitLabel xml:lang="de">Linie für Linie</rdakit:toolkitLabel>
      <skos:definition xml:lang="de">Ein Layout, bei dem sich Textzeilen mit Notenzeilen, die zum vorhergehenden Text gehören, abwechseln.</skos:definition>
      <rdakit:toolkitDefinition xml:lang="de">Ein Layout, bei dem sich Textzeilen mit Notenzeilen, die zum vorhergehenden Text gehören, abwechseln.</rdakit:toolkitDefinition>
      <skos:scopeNote xml:lang="de">Dieser Terminus trifft auf taktile Musikressourcen zu.</skos:scopeNote>
      <skos:prefLabel xml:lang="fi">säkeet peräkkäin</skos:prefLabel>
      <rdakit:toolkitLabel xml:lang="fi">säkeet peräkkäin</rdakit:toolkitLabel>
      <skos:definition xml:lang="fi">Layout, joka koostuu tekstisäkeistä, jotka vuorottelevat edeltävään tekstiin liittyvien nuottisäkeiden kanssa.</skos:definition>
      <rdakit:toolkitDefinition xml:lang="fi">Layout, joka koostuu tekstisäkeistä, jotka vuorottelevat edeltävään tekstiin liittyvien nuottisäkeiden kanssa.</rdakit:toolkitDefinition>
      <skos:scopeNote xml:lang="fi">Termi koskee taktiileja musiikkiaineistoja.</skos:scopeNote>
      <skos:prefLabel xml:lang="vi">dòng sau dòng</skos:prefLabel>
      <rdakit:toolkitLabel xml:lang="vi">dòng sau dòng</rdakit:toolkitLabel>
      <skos:definition xml:lang="vi">Sắp đặt gồm có các dòng của văn bản xen kẽ với các dòng âm nhạc đối với văn bản có trước.</skos:definition>
      <rdakit:toolkitDefinition xml:lang="vi">Sắp đặt gồm có các dòng của văn bản xen kẽ với các dòng âm nhạc đối với văn bản có trước.</rdakit:toolkitDefinition>
      <skos:scopeNote xml:lang="vi">Thuật ngữ này áp dụng cho tài nguyên âm nhạc xúc giác.</skos:scopeNote>
      <skos:prefLabel xml:lang="da">linje for linje</skos:prefLabel>
      <rdakit:toolkitLabel xml:lang="da">linje for linje</rdakit:toolkitLabel>
      <skos:definition xml:lang="da">Layout bestående skiftevis af linjer med tekst og linjer med musik til den foregående tekst.</skos:definition>
      <rdakit:toolkitDefinition xml:lang="da">Layout bestående skiftevis af linjer med tekst og linjer med musik til den foregående tekst.</rdakit:toolkitDefinition>
      <skos:scopeNote xml:lang="da">Denne term anvendes til taktile musik-ressourcer.</skos:scopeNote>
      <skos:prefLabel xml:lang="fr">ligne par ligne</skos:prefLabel>
      <rdakit:toolkitLabel xml:lang="fr">ligne par ligne</rdakit:toolkitLabel>
      <skos:definition xml:lang="fr">Disposition qui consiste en lignes de texte qui alternent avec des lignes de musique correspondant au texte qui précède.</skos:definition>
      <rdakit:toolkitDefinition xml:lang="fr">Disposition qui consiste en lignes de texte qui alternent avec des lignes de musique correspondant au texte qui précède.</rdakit:toolkitDefinition>
      <skos:scopeNote xml:lang="fr">Ce terme s’applique aux ressources de musique tactile.</skos:scopeNote>
      <skos:prefLabel xml:lang="no">line by line</skos:prefLabel>
      <rdakit:toolkitLabel xml:lang="no">line by line</rdakit:toolkitLabel>
      <skos:definition xml:lang="no">Et oppsett som består av vekselvis linjer med tekst og linjer med musikk til teksten på linjen over.</skos:definition>
      <rdakit:toolkitDefinition xml:lang="no">Et oppsett som består av vekselvis linjer med tekst og linjer med musikk til teksten på linjen over.</rdakit:toolkitDefinition>
      <skos:scopeNote xml:lang="no">Dette begrepet gjelder taktile musikkressurser.</skos:scopeNote>
    </skos:Concept>
<!-- Concept: line over line  -->
    <skos:Concept rdf:about="http://rdaregistry.info/termList/layout/1008" xml:lang="en">
      <skos:inScheme rdf:resource="http://rdaregistry.info/termList/layout"/>
      <reg:status rdf:resource="http://metadataregistry.org/uri/RegStatus/1001"/>
      <reg:identifier rdf:resource="http://metadataregistry.org/concepts/8441"/>
      <skos:prefLabel xml:lang="en">line over line</skos:prefLabel>
      <rdakit:toolkitLabel xml:lang="en">line over line</rdakit:toolkitLabel>
      <skos:definition xml:lang="en">A layout consisting of measures displayed in parallels, but the measures are not necessarily aligned.</skos:definition>
      <rdakit:toolkitDefinition xml:lang="en">A layout consisting of measures displayed in parallels, but the measures are not necessarily aligned.</rdakit:toolkitDefinition>
      <skos:scopeNote xml:lang="en">This term applies to tactile music resources.</skos:scopeNote>
      <skos:prefLabel xml:lang="it">linea sopra linea</skos:prefLabel>
      <rdakit:toolkitLabel xml:lang="it">linea sopra linea</rdakit:toolkitLabel>
      <skos:prefLabel xml:lang="de">Linie über Linie</skos:prefLabel>
      <rdakit:toolkitLabel xml:lang="de">Linie über Linie</rdakit:toolkitLabel>
      <skos:definition xml:lang="de">Ein Layout, bei dem Takte in parallelen Linien dargestellt werden, wobei die Takte aber nicht zwingend bündig ausgerichtet sind.</skos:definition>
      <rdakit:toolkitDefinition xml:lang="de">Ein Layout, bei dem Takte in parallelen Linien dargestellt werden, wobei die Takte aber nicht zwingend bündig ausgerichtet sind.</rdakit:toolkitDefinition>
      <skos:scopeNote xml:lang="de">Dieser Terminus trifft auf taktile Musikressourcen zu.</skos:scopeNote>
      <skos:prefLabel xml:lang="fi">säkeet allekkain</skos:prefLabel>
      <rdakit:toolkitLabel xml:lang="fi">säkeet allekkain</rdakit:toolkitLabel>
      <skos:definition xml:lang="fi">Layout, joka koostuu rinnakkaisina esitetyistä tahdeista, mutta tahteja ei ole välttämättä tasattu.</skos:definition>
      <rdakit:toolkitDefinition xml:lang="fi">Layout, joka koostuu rinnakkaisina esitetyistä tahdeista, mutta tahteja ei ole välttämättä tasattu.</rdakit:toolkitDefinition>
      <skos:scopeNote xml:lang="fi">Termi koskee taktiileja musiikkiaineistoja.</skos:scopeNote>
      <skos:prefLabel xml:lang="vi">dòng trên dòng</skos:prefLabel>
      <rdakit:toolkitLabel xml:lang="vi">dòng trên dòng</rdakit:toolkitLabel>
      <skos:definition xml:lang="vi">Sắp đặt gồm có các nhịp được hiện song song, nhưng các nhịp đó không cần thẳng hàng.</skos:definition>
      <rdakit:toolkitDefinition xml:lang="vi">Sắp đặt gồm có các nhịp được hiện song song, nhưng các nhịp đó không cần thẳng hàng.</rdakit:toolkitDefinition>
      <skos:scopeNote xml:lang="vi">Thuật ngữ này áp dụng cho tài nguyên âm nhạc xúc giác.</skos:scopeNote>
      <skos:prefLabel xml:lang="da">linje over linje</skos:prefLabel>
      <rdakit:toolkitLabel xml:lang="da">linje over linje</rdakit:toolkitLabel>
      <skos:definition xml:lang="da">Layout bestående af takter vist som paralleller, men hvor takterne ikke nødvendigvis er på linje med hinanden.</skos:definition>
      <rdakit:toolkitDefinition xml:lang="da">Layout bestående af takter vist som paralleller, men hvor takterne ikke nødvendigvis er på linje med hinanden.</rdakit:toolkitDefinition>
      <skos:scopeNote xml:lang="da">Denne term anvendes til taktile musik-ressourcer.</skos:scopeNote>
      <skos:prefLabel xml:lang="fr">ligne sur ligne</skos:prefLabel>
      <rdakit:toolkitLabel xml:lang="fr">ligne sur ligne</rdakit:toolkitLabel>
      <skos:definition xml:lang="fr">Disposition qui consiste en mesures présentées sous forme de parallèles, mais dans lesquels les mesures ne sont pas nécessairement alignées les unes avec les autres.</skos:definition>
      <rdakit:toolkitDefinition xml:lang="fr">Disposition qui consiste en mesures présentées sous forme de parallèles, mais dans lesquels les mesures ne sont pas nécessairement alignées les unes avec les autres.</rdakit:toolkitDefinition>
      <skos:scopeNote xml:lang="fr">Ce terme s’applique aux ressources de musique tactile.</skos:scopeNote>
      <skos:prefLabel xml:lang="no">line over line</skos:prefLabel>
      <rdakit:toolkitLabel xml:lang="no">line over line</rdakit:toolkitLabel>
      <skos:definition xml:lang="no">Et oppsett som består av takter som vises parallelt, men taktene er ikke nødvendigvis på linje.</skos:definition>
      <rdakit:toolkitDefinition xml:lang="no">Et oppsett som består av takter som vises parallelt, men taktene er ikke nødvendigvis på linje.</rdakit:toolkitDefinition>
      <skos:scopeNote xml:lang="no">Dette begrepet gjelder taktile musikkressurser.</skos:scopeNote>
    </skos:Concept>
<!-- Concept: melody chord system  -->
    <skos:Concept rdf:about="http://rdaregistry.info/termList/layout/1009" xml:lang="en">
      <skos:inScheme rdf:resource="http://rdaregistry.info/termList/layout"/>
      <reg:status rdf:resource="http://metadataregistry.org/uri/RegStatus/1001"/>
      <reg:identifier rdf:resource="http://metadataregistry.org/concepts/8442"/>
      <skos:prefLabel xml:lang="en">melody chord system</skos:prefLabel>
      <rdakit:toolkitLabel xml:lang="en">melody chord system</rdakit:toolkitLabel>
      <skos:definition xml:lang="en">A layout consisting of chord symbols and melody presented in paragraphs with music braille used for the chord symbols.</skos:definition>
      <rdakit:toolkitDefinition xml:lang="en">A layout consisting of chord symbols and melody presented in paragraphs with music braille used for the chord symbols.</rdakit:toolkitDefinition>
      <skos:scopeNote xml:lang="en">This term applies to tactile music resources.</skos:scopeNote>
      <skos:prefLabel xml:lang="it">sistema di melodia accordale</skos:prefLabel>
      <rdakit:toolkitLabel xml:lang="it">sistema di melodia accordale</rdakit:toolkitLabel>
      <skos:prefLabel xml:lang="de">Melodie-Akkordsystem</skos:prefLabel>
      <rdakit:toolkitLabel xml:lang="de">Melodie-Akkordsystem</rdakit:toolkitLabel>
      <skos:definition xml:lang="de">Ein Layout bei dem Akkordsymbole und Tonfolgen in Absätzen dargestellt werden, wobei Braille-Notenschrift für die Akkordsymbole verwendet wird.</skos:definition>
      <rdakit:toolkitDefinition xml:lang="de">Ein Layout bei dem Akkordsymbole und Tonfolgen in Absätzen dargestellt werden, wobei Braille-Notenschrift für die Akkordsymbole verwendet wird.</rdakit:toolkitDefinition>
      <skos:scopeNote xml:lang="de">Dieser Terminus trifft auf taktile Musikressourcen zu.</skos:scopeNote>
      <skos:prefLabel xml:lang="fi">melody chord system</skos:prefLabel>
      <rdakit:toolkitLabel xml:lang="fi">melody chord system</rdakit:toolkitLabel>
      <skos:definition xml:lang="fi">Layout, joka koostuu sointumerkeistä ja melodiasta kappaleisiin jaettuina, ja jossa sointumerkit on merkitty pistekirjoituksella.</skos:definition>
      <rdakit:toolkitDefinition xml:lang="fi">Layout, joka koostuu sointumerkeistä ja melodiasta kappaleisiin jaettuina, ja jossa sointumerkit on merkitty pistekirjoituksella.</rdakit:toolkitDefinition>
      <skos:scopeNote xml:lang="fi">Termi koskee taktiileja musiikkiaineistoja.</skos:scopeNote>
      <skos:prefLabel xml:lang="vi">hệ thống hợp âm giai điệu</skos:prefLabel>
      <rdakit:toolkitLabel xml:lang="vi">hệ thống hợp âm giai điệu</rdakit:toolkitLabel>
      <skos:definition xml:lang="vi">Sắp đặt gồm có ký hiệu hơp âm và giai điệu được trình bày trong các đoạn với mã braille âm nhạc được dùng cho ký hiệu hợp âm.</skos:definition>
      <rdakit:toolkitDefinition xml:lang="vi">Sắp đặt gồm có ký hiệu hơp âm và giai điệu được trình bày trong các đoạn với mã braille âm nhạc được dùng cho ký hiệu hợp âm.</rdakit:toolkitDefinition>
      <skos:scopeNote xml:lang="vi">Thuật ngữ này áp dụng cho tài nguyên âm nhạc xúc giác.</skos:scopeNote>
      <skos:prefLabel xml:lang="da">melodi-akkordsystem</skos:prefLabel>
      <rdakit:toolkitLabel xml:lang="da">melodi-akkordsystem</rdakit:toolkitLabel>
      <skos:definition xml:lang="da">Layout bestående af becifring og melodi præsenteret i afsnit med musik-braille anvendt for becifring.</skos:definition>
      <rdakit:toolkitDefinition xml:lang="da">Layout bestående af becifring og melodi præsenteret i afsnit med musik-braille anvendt for becifring.</rdakit:toolkitDefinition>
      <skos:scopeNote xml:lang="da">Denne term anvendes til taktile musik-ressourcer.</skos:scopeNote>
      <skos:prefLabel xml:lang="fr">système mélodie/accords</skos:prefLabel>
      <rdakit:toolkitLabel xml:lang="fr">système mélodie/accords</rdakit:toolkitLabel>
      <skos:definition xml:lang="fr">Disposition qui consiste en accords chiffrés et en une mélodie présentés sous forme de paragraphes, les accords chiffrés étant représentés à l’aide du braille musical.</skos:definition>
      <rdakit:toolkitDefinition xml:lang="fr">Disposition qui consiste en accords chiffrés et en une mélodie présentés sous forme de paragraphes, les accords chiffrés étant représentés à l’aide du braille musical.</rdakit:toolkitDefinition>
      <skos:scopeNote xml:lang="fr">Ce terme s’applique aux ressources de musique tactile.</skos:scopeNote>
      <skos:prefLabel xml:lang="no">melodiakkordsystem</skos:prefLabel>
      <rdakit:toolkitLabel xml:lang="no">melodiakkordsystem</rdakit:toolkitLabel>
      <skos:definition xml:lang="no">Et oppsett som består av akkordsymboler og melodi vist i avsnitt, der musikalsk punktskrift brukes for akkordsymbolene.</skos:definition>
      <rdakit:toolkitDefinition xml:lang="no">Et oppsett som består av akkordsymboler og melodi vist i avsnitt, der musikalsk punktskrift brukes for akkordsymbolene.</rdakit:toolkitDefinition>
      <skos:scopeNote xml:lang="no">Dette begrepet gjelder taktile musikkressurser.</skos:scopeNote>
    </skos:Concept>
<!-- Concept: open score  -->
    <skos:Concept rdf:about="http://rdaregistry.info/termList/layout/1010" xml:lang="en">
      <skos:inScheme rdf:resource="http://rdaregistry.info/termList/layout"/>
      <reg:status rdf:resource="http://metadataregistry.org/uri/RegStatus/1001"/>
      <reg:identifier rdf:resource="http://metadataregistry.org/concepts/8443"/>
      <skos:prefLabel xml:lang="en">open score</skos:prefLabel>
      <rdakit:toolkitLabel xml:lang="en">open score</rdakit:toolkitLabel>
      <skos:definition xml:lang="en">A layout consisting of music presented in parallels.</skos:definition>
      <rdakit:toolkitDefinition xml:lang="en">A layout consisting of music presented in parallels.</rdakit:toolkitDefinition>
      <skos:scopeNote xml:lang="en">Open score is similar to bar over bar, but used for ensemble scores. This term applies to tactile music resources.</skos:scopeNote>
      <skos:prefLabel xml:lang="it">partitura a parti late</skos:prefLabel>
      <rdakit:toolkitLabel xml:lang="it">partitura a parti late</rdakit:toolkitLabel>
      <skos:prefLabel xml:lang="de">open score</skos:prefLabel>
      <rdakit:toolkitLabel xml:lang="de">open score</rdakit:toolkitLabel>
      <skos:definition xml:lang="de">Ein Layout, bei dem Noten in parallelen Linien dargestellt werden.</skos:definition>
      <rdakit:toolkitDefinition xml:lang="de">Ein Layout, bei dem Noten in parallelen Linien dargestellt werden.</rdakit:toolkitDefinition>
      <skos:scopeNote xml:lang="de">Open score ist dem Layout &quot;Takt über Takt&quot; ähnlich, wird aber für Ensemble-Partituren verwendet. Dieser Terminus trifft auf taktile Musikressourcen zu.</skos:scopeNote>
      <skos:prefLabel xml:lang="fi">avoin partituuri</skos:prefLabel>
      <rdakit:toolkitLabel xml:lang="fi">avoin partituuri</rdakit:toolkitLabel>
      <skos:definition xml:lang="fi">Layout, joka koostuu rinnakkain esitetystä nuottikirjoituksesta.</skos:definition>
      <rdakit:toolkitDefinition xml:lang="fi">Layout, joka koostuu rinnakkain esitetystä nuottikirjoituksesta.</rdakit:toolkitDefinition>
      <skos:scopeNote xml:lang="fi">Open score muistuttaa tahdit allekkain -layoutia, mutta sitä käytetään yhtyenuoteissa. Tämä termi koskee taktiileja musiikkiaineistoja.</skos:scopeNote>
      <skos:prefLabel xml:lang="vi">bảng tổng phổ mở</skos:prefLabel>
      <rdakit:toolkitLabel xml:lang="vi">bảng tổng phổ mở</rdakit:toolkitLabel>
      <skos:definition xml:lang="vi">Sắp đặt gồm có âm nhạc được trình bày trong các đường song song.</skos:definition>
      <rdakit:toolkitDefinition xml:lang="vi">Sắp đặt gồm có âm nhạc được trình bày trong các đường song song.</rdakit:toolkitDefinition>
      <skos:scopeNote xml:lang="vi">Bảng tổng phổ mở tương tự như gạch nhịp sau gạch nhịp nhưng được dùng cho bảng tổng phổ đồng diễn. Thuật ngữ này áp dụng cho tài nguyên âm nhạc xúc giác.</skos:scopeNote>
      <skos:prefLabel xml:lang="da">partitur</skos:prefLabel>
      <rdakit:toolkitLabel xml:lang="da">partitur</rdakit:toolkitLabel>
      <skos:definition xml:lang="da">Layout bestående af musik præsenteret i paralleller.</skos:definition>
      <rdakit:toolkitDefinition xml:lang="da">Layout bestående af musik præsenteret i paralleller.</rdakit:toolkitDefinition>
      <skos:scopeNote xml:lang="da">Partitur er det samme som takt over takt men bruges for ensemble-partiturer. Denne term anvendes til taktile musik-ressourcer.</skos:scopeNote>
      <skos:prefLabel xml:lang="fr">partition ouverte</skos:prefLabel>
      <rdakit:toolkitLabel xml:lang="fr">partition ouverte</rdakit:toolkitLabel>
      <skos:definition xml:lang="fr">Disposition qui consiste en musique présentée sous forme de parallèles.</skos:definition>
      <rdakit:toolkitDefinition xml:lang="fr">Disposition qui consiste en musique présentée sous forme de parallèles.</rdakit:toolkitDefinition>
      <skos:scopeNote xml:lang="fr">La disposition en partition ouverte est semblable à la disposition mesure sur mesure, mais est utilisée pour les partitions de musique d’ensemble. Ce terme s’applique aux ressources de musique tactile.</skos:scopeNote>
      <skos:prefLabel xml:lang="no">open score</skos:prefLabel>
      <rdakit:toolkitLabel xml:lang="no">open score</rdakit:toolkitLabel>
      <skos:definition xml:lang="no">Et oppsett som består av musikk som vises parallellt.</skos:definition>
      <rdakit:toolkitDefinition xml:lang="no">Et oppsett som består av musikk som vises parallellt.</rdakit:toolkitDefinition>
      <skos:scopeNote xml:lang="no">Open score ligner bar over bar, men brukes for ensembler. Dette begrepet gjelder taktile musikkressurser.</skos:scopeNote>
    </skos:Concept>
<!-- Concept: outline  -->
    <skos:Concept rdf:about="http://rdaregistry.info/termList/layout/1011" xml:lang="en">
      <skos:inScheme rdf:resource="http://rdaregistry.info/termList/layout"/>
      <reg:status rdf:resource="http://metadataregistry.org/uri/RegStatus/1001"/>
      <reg:identifier rdf:resource="http://metadataregistry.org/concepts/8444"/>
      <skos:prefLabel xml:lang="en">outline</skos:prefLabel>
      <rdakit:toolkitLabel xml:lang="en">outline</rdakit:toolkitLabel>
      <skos:definition xml:lang="en">A layout consisting of music in the outline format.</skos:definition>
      <rdakit:toolkitDefinition xml:lang="en">A layout consisting of music in the outline format.</rdakit:toolkitDefinition>
      <skos:scopeNote xml:lang="en">This term applies to tactile music resources.</skos:scopeNote>
      <skos:prefLabel xml:lang="it">outline</skos:prefLabel>
      <rdakit:toolkitLabel xml:lang="it">outline</rdakit:toolkitLabel>
      <skos:prefLabel xml:lang="de">outline</skos:prefLabel>
      <rdakit:toolkitLabel xml:lang="de">outline</rdakit:toolkitLabel>
      <skos:definition xml:lang="de">Ein Layout, bei dem Noten im Outline Format dargestellt werden.</skos:definition>
      <rdakit:toolkitDefinition xml:lang="de">Ein Layout, bei dem Noten im Outline Format dargestellt werden.</rdakit:toolkitDefinition>
      <skos:scopeNote xml:lang="de">Dieser Terminus trifft auf taktile Musikressourcen zu.</skos:scopeNote>
      <skos:prefLabel xml:lang="fi">outline</skos:prefLabel>
      <rdakit:toolkitLabel xml:lang="fi">outline</rdakit:toolkitLabel>
      <skos:definition xml:lang="fi">Layout, joka koostuu outline-muotoisesta nuottikirjoituksesta.</skos:definition>
      <rdakit:toolkitDefinition xml:lang="fi">Layout, joka koostuu outline-muotoisesta nuottikirjoituksesta.</rdakit:toolkitDefinition>
      <skos:scopeNote xml:lang="fi">Termi koskee taktiileja musiikkiaineistoja.</skos:scopeNote>
      <skos:prefLabel xml:lang="vi">phác thảo</skos:prefLabel>
      <rdakit:toolkitLabel xml:lang="vi">phác thảo</rdakit:toolkitLabel>
      <skos:definition xml:lang="vi">Sắp đặt gồm có âm nhạc trong định dạng phác thảo</skos:definition>
      <rdakit:toolkitDefinition xml:lang="vi">Sắp đặt gồm có âm nhạc trong định dạng phác thảo</rdakit:toolkitDefinition>
      <skos:scopeNote xml:lang="vi">Thuật ngữ này áp dụng cho tài nguyên âm nhạc xúc giác.</skos:scopeNote>
      <skos:prefLabel xml:lang="da">outline</skos:prefLabel>
      <rdakit:toolkitLabel xml:lang="da">outline</rdakit:toolkitLabel>
      <skos:definition xml:lang="da">Layout bestående af musik i outline-format.</skos:definition>
      <rdakit:toolkitDefinition xml:lang="da">Layout bestående af musik i outline-format.</rdakit:toolkitDefinition>
      <skos:scopeNote xml:lang="da">Denne term anvendes til taktile musik-ressourcer.</skos:scopeNote>
      <skos:prefLabel xml:lang="fr">notation simplifiée</skos:prefLabel>
      <rdakit:toolkitLabel xml:lang="fr">notation simplifiée</rdakit:toolkitLabel>
      <skos:definition xml:lang="fr">Disposition qui consiste en musique présentée sous forme de notation simplifiée.</skos:definition>
      <rdakit:toolkitDefinition xml:lang="fr">Disposition qui consiste en musique présentée sous forme de notation simplifiée.</rdakit:toolkitDefinition>
      <skos:scopeNote xml:lang="fr">Ce terme s’applique aux ressources de musique tactile.</skos:scopeNote>
      <skos:prefLabel xml:lang="no">skisse</skos:prefLabel>
      <rdakit:toolkitLabel xml:lang="no">skisse</rdakit:toolkitLabel>
      <skos:definition xml:lang="no">Et oppsett som består av musikk i skisseformat.</skos:definition>
      <rdakit:toolkitDefinition xml:lang="no">Et oppsett som består av musikk i skisseformat.</rdakit:toolkitDefinition>
      <skos:scopeNote xml:lang="no">Dette begrepet gjelder taktile musikkressurser.</skos:scopeNote>
    </skos:Concept>
<!-- Concept: paragraph  -->
    <skos:Concept rdf:about="http://rdaregistry.info/termList/layout/1012" xml:lang="en">
      <skos:inScheme rdf:resource="http://rdaregistry.info/termList/layout"/>
      <reg:status rdf:resource="http://metadataregistry.org/uri/RegStatus/1001"/>
      <reg:identifier rdf:resource="http://metadataregistry.org/concepts/8445"/>
      <skos:prefLabel xml:lang="en">paragraph</skos:prefLabel>
      <rdakit:toolkitLabel xml:lang="en">paragraph</rdakit:toolkitLabel>
      <skos:definition xml:lang="en">A layout in braille consisting of music displayed in paragraphs with one part per paragraph.</skos:definition>
      <rdakit:toolkitDefinition xml:lang="en">A layout in braille consisting of music displayed in paragraphs with one part per paragraph.</rdakit:toolkitDefinition>
      <skos:scopeNote xml:lang="en">This term applies to tactile music resources.</skos:scopeNote>
      <skos:prefLabel xml:lang="it">paragrafo</skos:prefLabel>
      <rdakit:toolkitLabel xml:lang="it">paragrafo</rdakit:toolkitLabel>
      <skos:prefLabel xml:lang="de">paragraph</skos:prefLabel>
      <rdakit:toolkitLabel xml:lang="de">paragraph</rdakit:toolkitLabel>
      <skos:definition xml:lang="de">Ein Layout in Braille, bei dem Noten in Absätzen dargestellt werden, wobei es pro Stimme einen Absatz gibt.</skos:definition>
      <rdakit:toolkitDefinition xml:lang="de">Ein Layout in Braille, bei dem Noten in Absätzen dargestellt werden, wobei es pro Stimme einen Absatz gibt.</rdakit:toolkitDefinition>
      <skos:scopeNote xml:lang="de">Dieser Terminus trifft auf taktile Musikressourcen zu.</skos:scopeNote>
      <skos:prefLabel xml:lang="fi">paragrafi</skos:prefLabel>
      <rdakit:toolkitLabel xml:lang="fi">paragrafi</rdakit:toolkitLabel>
      <skos:definition xml:lang="fi">Pistekirjoituslayout, joka koostuu kappaleittain esitetystä nuottikirjoituksesta, yksi stemma kappaletta kohden.</skos:definition>
      <rdakit:toolkitDefinition xml:lang="fi">Pistekirjoituslayout, joka koostuu kappaleittain esitetystä nuottikirjoituksesta, yksi stemma kappaletta kohden.</rdakit:toolkitDefinition>
      <skos:scopeNote xml:lang="fi">Termi koskee taktiileja musiikkiaineistoja.</skos:scopeNote>
      <skos:prefLabel xml:lang="vi">đoạn</skos:prefLabel>
      <rdakit:toolkitLabel xml:lang="vi">đoạn</rdakit:toolkitLabel>
      <skos:definition xml:lang="vi">Sắp đặt theo mã braille gồm có âm nhạc hiện theo đoạn với một phần trong một đoạn.</skos:definition>
      <rdakit:toolkitDefinition xml:lang="vi">Sắp đặt theo mã braille gồm có âm nhạc hiện theo đoạn với một phần trong một đoạn.</rdakit:toolkitDefinition>
      <skos:scopeNote xml:lang="vi">Thuật ngữ này áp dụng cho tài nguyên âm nhạc xúc giác.</skos:scopeNote>
      <skos:prefLabel xml:lang="da">afsnit</skos:prefLabel>
      <rdakit:toolkitLabel xml:lang="da">afsnit</rdakit:toolkitLabel>
      <skos:definition xml:lang="da">Layout i braille bestående af musik vist i afsnit med en stemme per afsnit.</skos:definition>
      <rdakit:toolkitDefinition xml:lang="da">Layout i braille bestående af musik vist i afsnit med en stemme per afsnit.</rdakit:toolkitDefinition>
      <skos:scopeNote xml:lang="da">Denne term anvendes til taktile musik-ressourcer.</skos:scopeNote>
      <skos:prefLabel xml:lang="fr">paragraphe</skos:prefLabel>
      <rdakit:toolkitLabel xml:lang="fr">paragraphe</rdakit:toolkitLabel>
      <skos:definition xml:lang="fr">Disposition en braille qui consiste en musique présentée sous forme de paragraphes contenant chacun une partie.</skos:definition>
      <rdakit:toolkitDefinition xml:lang="fr">Disposition en braille qui consiste en musique présentée sous forme de paragraphes contenant chacun une partie.</rdakit:toolkitDefinition>
      <skos:scopeNote xml:lang="fr">Ce terme s’applique aux ressources de musique tactile.</skos:scopeNote>
      <skos:prefLabel xml:lang="no">avsnitt</skos:prefLabel>
      <rdakit:toolkitLabel xml:lang="no">avsnitt</rdakit:toolkitLabel>
      <skos:definition xml:lang="no">Et oppsett i punktskrift der musikk vises i avsnitt med ett instrument per avsnitt.</skos:definition>
      <rdakit:toolkitDefinition xml:lang="no">Et oppsett i punktskrift der musikk vises i avsnitt med ett instrument per avsnitt.</rdakit:toolkitDefinition>
      <skos:scopeNote xml:lang="no">Dette begrepet gjelder taktile musikkressurser.</skos:scopeNote>
    </skos:Concept>
<!-- Concept: section by section  -->
    <skos:Concept rdf:about="http://rdaregistry.info/termList/layout/1013" xml:lang="en">
      <skos:inScheme rdf:resource="http://rdaregistry.info/termList/layout"/>
      <reg:status rdf:resource="http://metadataregistry.org/uri/RegStatus/1001"/>
      <reg:identifier rdf:resource="http://metadataregistry.org/concepts/8446"/>
      <skos:prefLabel xml:lang="en">section by section</skos:prefLabel>
      <rdakit:toolkitLabel xml:lang="en">section by section</rdakit:toolkitLabel>
      <skos:definition xml:lang="en">A layout consisting of hand or part signs that are prominent in the left margin.</skos:definition>
      <rdakit:toolkitDefinition xml:lang="en">A layout consisting of hand or part signs that are prominent in the left margin.</rdakit:toolkitDefinition>
      <skos:scopeNote xml:lang="en">This term applies to tactile music resources.</skos:scopeNote>
      <skos:prefLabel xml:lang="it">sezione per sezione</skos:prefLabel>
      <rdakit:toolkitLabel xml:lang="it">sezione per sezione</rdakit:toolkitLabel>
      <skos:prefLabel xml:lang="de">section by section</skos:prefLabel>
      <rdakit:toolkitLabel xml:lang="de">section by section</rdakit:toolkitLabel>
      <skos:definition xml:lang="de">Ein Layout, das aus Hand- oder Stimmenzeichen besteht, die am linken Rand zu sehen sind.</skos:definition>
      <rdakit:toolkitDefinition xml:lang="de">Ein Layout, das aus Hand- oder Stimmenzeichen besteht, die am linken Rand zu sehen sind.</rdakit:toolkitDefinition>
      <skos:scopeNote xml:lang="de">Dieser Terminus trifft auf taktile Musikressourcen zu.</skos:scopeNote>
      <skos:prefLabel xml:lang="fi">osat peräkkäin</skos:prefLabel>
      <rdakit:toolkitLabel xml:lang="fi">osat peräkkäin</rdakit:toolkitLabel>
      <skos:definition xml:lang="fi">Layout, joka koostuu käsi- tai stemmamerkeistä, jotka on ryhmitelty vasemmassa marginaalissa.</skos:definition>
      <rdakit:toolkitDefinition xml:lang="fi">Layout, joka koostuu käsi- tai stemmamerkeistä, jotka on ryhmitelty vasemmassa marginaalissa.</rdakit:toolkitDefinition>
      <skos:scopeNote xml:lang="fi">Termi koskee taktiileja musiikkiaineistoja.</skos:scopeNote>
      <skos:prefLabel xml:lang="vi">mục sau mục</skos:prefLabel>
      <rdakit:toolkitLabel xml:lang="vi">mục sau mục</rdakit:toolkitLabel>
      <skos:definition xml:lang="vi">Sặp đặt gồm có ký hiệu tay hoặc phần nổi bật trên lề trái.</skos:definition>
      <rdakit:toolkitDefinition xml:lang="vi">Sặp đặt gồm có ký hiệu tay hoặc phần nổi bật trên lề trái.</rdakit:toolkitDefinition>
      <skos:scopeNote xml:lang="vi">Thuật ngữ này áp dụng cho tài nguyên âm nhạc xúc giác.</skos:scopeNote>
      <skos:prefLabel xml:lang="da">sektion for sektion</skos:prefLabel>
      <rdakit:toolkitLabel xml:lang="da">sektion for sektion</rdakit:toolkitLabel>
      <skos:definition xml:lang="da">Layout bestående af tegn for hånd eller stemme fremhævet i den venstre margen.</skos:definition>
      <rdakit:toolkitDefinition xml:lang="da">Layout bestående af tegn for hånd eller stemme fremhævet i den venstre margen.</rdakit:toolkitDefinition>
      <skos:scopeNote xml:lang="da">Denne term anvendes til taktile musik-ressourcer.</skos:scopeNote>
      <skos:prefLabel xml:lang="fr">section par section</skos:prefLabel>
      <rdakit:toolkitLabel xml:lang="fr">section par section</rdakit:toolkitLabel>
      <skos:definition xml:lang="fr">Disposition qui consiste en signes pour les mains ou les parties figurant clairement dans la marge de gauche.</skos:definition>
      <rdakit:toolkitDefinition xml:lang="fr">Disposition qui consiste en signes pour les mains ou les parties figurant clairement dans la marge de gauche.</rdakit:toolkitDefinition>
      <skos:scopeNote xml:lang="fr">Ce terme s’applique aux ressources de musique tactile.</skos:scopeNote>
      <skos:prefLabel xml:lang="no">section by section</skos:prefLabel>
      <rdakit:toolkitLabel xml:lang="no">section by section</rdakit:toolkitLabel>
      <skos:definition xml:lang="no">Et oppsett som består av tegn for hånd eller stemme som vises tydelig i venstre marg.</skos:definition>
      <rdakit:toolkitDefinition xml:lang="no">Et oppsett som består av tegn for hånd eller stemme som vises tydelig i venstre marg.</rdakit:toolkitDefinition>
      <skos:scopeNote xml:lang="no">Dette begrepet gjelder taktile musikkressurser.</skos:scopeNote>
    </skos:Concept>
<!-- Concept: short form scoring  -->
    <skos:Concept rdf:about="http://rdaregistry.info/termList/layout/1014" xml:lang="en">
      <skos:inScheme rdf:resource="http://rdaregistry.info/termList/layout"/>
      <reg:status rdf:resource="http://metadataregistry.org/uri/RegStatus/1001"/>
      <reg:identifier rdf:resource="http://metadataregistry.org/concepts/8447"/>
      <skos:prefLabel xml:lang="en">short form scoring</skos:prefLabel>
      <rdakit:toolkitLabel xml:lang="en">short form scoring</rdakit:toolkitLabel>
      <skos:definition xml:lang="en">A layout consisting of words, chord symbols, and melody presented in parallels with literary braille used for the chord symbols.</skos:definition>
      <rdakit:toolkitDefinition xml:lang="en">A layout consisting of words, chord symbols, and melody presented in parallels with literary braille used for the chord symbols.</rdakit:toolkitDefinition>
      <skos:scopeNote xml:lang="en">Short form scoring is used chiefly for popular and folk music. This term applies to tactile music resources.</skos:scopeNote>
      <skos:prefLabel xml:lang="it">partitura a parti strette</skos:prefLabel>
      <rdakit:toolkitLabel xml:lang="it">partitura a parti strette</rdakit:toolkitLabel>
      <skos:prefLabel xml:lang="de">short form scoring</skos:prefLabel>
      <rdakit:toolkitLabel xml:lang="de">short form scoring</rdakit:toolkitLabel>
      <skos:definition xml:lang="de">Ein Layout, bei dem Text, Akkordsymbole und Tonfolgen in parallelen Linien dargestellt werden. Für die Akkordsymbole werden Braille-Buchstaben verwendet.</skos:definition>
      <rdakit:toolkitDefinition xml:lang="de">Ein Layout, bei dem Text, Akkordsymbole und Tonfolgen in parallelen Linien dargestellt werden. Für die Akkordsymbole werden Braille-Buchstaben verwendet.</rdakit:toolkitDefinition>
      <skos:scopeNote xml:lang="de">Kurzform-Partituren werden hauptsächlich im Bereich der Volks- und Populärmusik verwendet. Der Terminus trifft auf taktile Musikressourcen zu.</skos:scopeNote>
      <skos:prefLabel xml:lang="fi">short form scoring</skos:prefLabel>
      <rdakit:toolkitLabel xml:lang="fi">short form scoring</rdakit:toolkitLabel>
      <skos:definition xml:lang="fi">Layout, joka koostuu rinnakkain esitetyistä sanoista, sointumerkeistä ja melodiasta, ja jossa sointumerkeille on käytetty kirjallista pistekirjoitusta.</skos:definition>
      <rdakit:toolkitDefinition xml:lang="fi">Layout, joka koostuu rinnakkain esitetyistä sanoista, sointumerkeistä ja melodiasta, ja jossa sointumerkeille on käytetty kirjallista pistekirjoitusta.</rdakit:toolkitDefinition>
      <skos:scopeNote xml:lang="fi">Short form scoringia käytetään pääasiassa populaari- ja kansanmusiikissa. Termi koskee taktiileja musiikkiaineistoja.</skos:scopeNote>
      <skos:prefLabel xml:lang="vi">tổng phổ hình thái ngắn</skos:prefLabel>
      <rdakit:toolkitLabel xml:lang="vi">tổng phổ hình thái ngắn</rdakit:toolkitLabel>
      <skos:definition xml:lang="vi">Sắp đặt gồm có từ, ký hiệu hợp âm, và giai điệu được trình bày trong các đường song song với mã braille văn học được dùng cho ký hiệu hợp âm.</skos:definition>
      <rdakit:toolkitDefinition xml:lang="vi">Sắp đặt gồm có từ, ký hiệu hợp âm, và giai điệu được trình bày trong các đường song song với mã braille văn học được dùng cho ký hiệu hợp âm.</rdakit:toolkitDefinition>
      <skos:scopeNote xml:lang="vi">Tổng phổ hình thái ngắn được dùng chủ yếu cho âm nhạc đại chúng và dân gian. Thuật ngữ này áp dụng cho tài nguyên âm nhạc xúc giác.</skos:scopeNote>
      <skos:prefLabel xml:lang="da">short form scoring</skos:prefLabel>
      <rdakit:toolkitLabel xml:lang="da">short form scoring</rdakit:toolkitLabel>
      <skos:definition xml:lang="da">Layout bestående af ord, becifring og melodi præsenteret i paralleller med braille-tekst anvendt for becifring.</skos:definition>
      <rdakit:toolkitDefinition xml:lang="da">Layout bestående af ord, becifring og melodi præsenteret i paralleller med braille-tekst anvendt for becifring.</rdakit:toolkitDefinition>
      <skos:scopeNote xml:lang="da">Short form scoring er anvendt primært for populær- og folkemusik. Denne term anvendes til taktile musik-ressourcer.</skos:scopeNote>
      <skos:prefLabel xml:lang="fr">notation abrégée</skos:prefLabel>
      <rdakit:toolkitLabel xml:lang="fr">notation abrégée</rdakit:toolkitLabel>
      <skos:definition xml:lang="fr">Disposition qui consiste en paroles, en accords chiffrés et en une mélodie présentés en parallèles, les accords chiffrés étant représentés à l’aide du braille littéraire.</skos:definition>
      <rdakit:toolkitDefinition xml:lang="fr">Disposition qui consiste en paroles, en accords chiffrés et en une mélodie présentés en parallèles, les accords chiffrés étant représentés à l’aide du braille littéraire.</rdakit:toolkitDefinition>
      <skos:scopeNote xml:lang="fr">La disposition en notation abrégée est utilisée principalement pour la musique populaire et folklorique. Ce terme s’applique aux ressources de musique tactile.</skos:scopeNote>
      <skos:prefLabel xml:lang="no">short form scoring</skos:prefLabel>
      <rdakit:toolkitLabel xml:lang="no">short form scoring</rdakit:toolkitLabel>
      <skos:definition xml:lang="no">Et oppsett som består av ord, akkordsymboler og melodi vist parallellt, der punktskrift brukes for akkordsymbolene.</skos:definition>
      <rdakit:toolkitDefinition xml:lang="no">Et oppsett som består av ord, akkordsymboler og melodi vist parallellt, der punktskrift brukes for akkordsymbolene.</rdakit:toolkitDefinition>
      <skos:scopeNote xml:lang="no">Short form scoring brukes hovedsakelig for populær- og folkemusikk. Dette begrepet gjelder taktile musikkressurser.</skos:scopeNote>
    </skos:Concept>
<!-- Concept: single line  -->
    <skos:Concept rdf:about="http://rdaregistry.info/termList/layout/1015" xml:lang="en">
      <skos:inScheme rdf:resource="http://rdaregistry.info/termList/layout"/>
      <reg:status rdf:resource="http://metadataregistry.org/uri/RegStatus/1001"/>
      <reg:identifier rdf:resource="http://metadataregistry.org/concepts/8448"/>
      <skos:prefLabel xml:lang="en">single line</skos:prefLabel>
      <rdakit:toolkitLabel xml:lang="en">single line</rdakit:toolkitLabel>
      <skos:definition xml:lang="en">A layout consisting of music for single instrumental parts or solos presented in segments of two to five lines, the initial line displaying a measure number or rehearsal designation.</skos:definition>
      <rdakit:toolkitDefinition xml:lang="en">A layout consisting of music for single instrumental parts or solos presented in segments of two to five lines, the initial line displaying a measure number or rehearsal designation.</rdakit:toolkitDefinition>
      <skos:scopeNote xml:lang="en">This term applies to tactile music resources.</skos:scopeNote>
      <skos:prefLabel xml:lang="it">linea singola</skos:prefLabel>
      <rdakit:toolkitLabel xml:lang="it">linea singola</rdakit:toolkitLabel>
      <skos:prefLabel xml:lang="de">single line</skos:prefLabel>
      <rdakit:toolkitLabel xml:lang="de">single line</rdakit:toolkitLabel>
      <skos:definition xml:lang="de">Ein Layout, bei dem Noten für Einzelinstrumentalstimmen oder Solos in Segmenten von zwei bis fünf Linien dargestellt sind, wobei die erste Linie eine Taktzahl oder eine Probeanweisung enthält.</skos:definition>
      <rdakit:toolkitDefinition xml:lang="de">Ein Layout, bei dem Noten für Einzelinstrumentalstimmen oder Solos in Segmenten von zwei bis fünf Linien dargestellt sind, wobei die erste Linie eine Taktzahl oder eine Probeanweisung enthält.</rdakit:toolkitDefinition>
      <skos:scopeNote xml:lang="de">Dieser Terminus trifft auf taktile Musikressourcen zu.</skos:scopeNote>
      <skos:prefLabel xml:lang="fi">yksirivinen</skos:prefLabel>
      <rdakit:toolkitLabel xml:lang="fi">yksirivinen</rdakit:toolkitLabel>
      <skos:definition xml:lang="fi">Layout, joka koostuu nuottikirjoituksesta yksittäisille soitinstemmoille tai -sooloille, jotka on esitetty kahden–viiden rivin lohkoissa, joissa ensimmäinen rivi osoittaa tahti- tai harjoitusnumeron.</skos:definition>
      <rdakit:toolkitDefinition xml:lang="fi">Layout, joka koostuu nuottikirjoituksesta yksittäisille soitinstemmoille tai -sooloille, jotka on esitetty kahden–viiden rivin lohkoissa, joissa ensimmäinen rivi osoittaa tahti- tai harjoitusnumeron.</rdakit:toolkitDefinition>
      <skos:scopeNote xml:lang="fi">Termi koskee taktiileja musiikkiaineistoja.</skos:scopeNote>
      <skos:prefLabel xml:lang="vi">dòng đơn</skos:prefLabel>
      <rdakit:toolkitLabel xml:lang="vi">dòng đơn</rdakit:toolkitLabel>
      <skos:definition xml:lang="vi">Sắp đặt gồm có âm nhạc cho các phần nhạc khí đơn hoặc độc tấu trình bày trên các đoạn từ hai tới năm dòng, dòng đầu hiện chỉ số nhịp điệu hoặc định danh diễn tập.</skos:definition>
      <rdakit:toolkitDefinition xml:lang="vi">Sắp đặt gồm có âm nhạc cho các phần nhạc khí đơn hoặc độc tấu trình bày trên các đoạn từ hai tới năm dòng, dòng đầu hiện chỉ số nhịp điệu hoặc định danh diễn tập.</rdakit:toolkitDefinition>
      <skos:scopeNote xml:lang="vi">Thuật ngữ này áp dụng cho tài nguyên âm nhạc xúc giác.</skos:scopeNote>
      <skos:prefLabel xml:lang="da">enkel linje</skos:prefLabel>
      <rdakit:toolkitLabel xml:lang="da">enkel linje</rdakit:toolkitLabel>
      <skos:definition xml:lang="da">Layout bestående af musik for enkelte instrumentstemmer eller soloer præsenteret i segmenter af to til fem linjer, hvor den første linje viser et taktnummer eller et prøveciffer.</skos:definition>
      <rdakit:toolkitDefinition xml:lang="da">Layout bestående af musik for enkelte instrumentstemmer eller soloer præsenteret i segmenter af to til fem linjer, hvor den første linje viser et taktnummer eller et prøveciffer.</rdakit:toolkitDefinition>
      <skos:scopeNote xml:lang="da">Denne term anvendes til taktile musik-ressourcer.</skos:scopeNote>
      <skos:prefLabel xml:lang="fr">ligne individuelle</skos:prefLabel>
      <rdakit:toolkitLabel xml:lang="fr">ligne individuelle</rdakit:toolkitLabel>
      <skos:definition xml:lang="fr">Disposition qui consiste en musique pour parties instrumentales ou solos individuels présentée en segments de deux à cinq lignes, la première présentant un numéro de mesure ou un repère de répétition.</skos:definition>
      <rdakit:toolkitDefinition xml:lang="fr">Disposition qui consiste en musique pour parties instrumentales ou solos individuels présentée en segments de deux à cinq lignes, la première présentant un numéro de mesure ou un repère de répétition.</rdakit:toolkitDefinition>
      <skos:scopeNote xml:lang="fr">Ce terme s’applique aux ressources de musique tactile.</skos:scopeNote>
      <skos:prefLabel xml:lang="no">enkeltlinje</skos:prefLabel>
      <rdakit:toolkitLabel xml:lang="no">enkeltlinje</rdakit:toolkitLabel>
      <skos:definition xml:lang="no">Ett oppsett som består av musikk for de enkelte instrumentalstemmene eller soloutøverne vist i segmenter med to til fem linjer der den første linjen viser et taktnummer eller en betegnelse for øvelse.</skos:definition>
      <rdakit:toolkitDefinition xml:lang="no">Ett oppsett som består av musikk for de enkelte instrumentalstemmene eller soloutøverne vist i segmenter med to til fem linjer der den første linjen viser et taktnummer eller en betegnelse for øvelse.</rdakit:toolkitDefinition>
      <skos:scopeNote xml:lang="no">Dette begrepet gjelder taktile musikkressurser.</skos:scopeNote>
    </skos:Concept>
<!-- Concept: single sided  -->
    <skos:Concept rdf:about="http://rdaregistry.info/termList/layout/1002" xml:lang="en">
      <skos:inScheme rdf:resource="http://rdaregistry.info/termList/layout"/>
      <reg:status rdf:resource="http://metadataregistry.org/uri/RegStatus/1001"/>
      <reg:identifier rdf:resource="http://metadataregistry.org/concepts/837"/>
      <skos:prefLabel xml:lang="en">single sided</skos:prefLabel>
      <rdakit:toolkitLabel xml:lang="en">single sided</rdakit:toolkitLabel>
      <skos:definition xml:lang="en">A layout that uses only one side of a sheet.</skos:definition>
      <rdakit:toolkitDefinition xml:lang="en">A layout that uses only one side of a sheet.</rdakit:toolkitDefinition>
      <skos:scopeNote xml:lang="en">This term applies to sheets and tactile text.</skos:scopeNote>
      <skos:prefLabel xml:lang="it">facciata singola</skos:prefLabel>
      <rdakit:toolkitLabel xml:lang="it">facciata singola</rdakit:toolkitLabel>
      <skos:prefLabel xml:lang="de">einseitig</skos:prefLabel>
      <rdakit:toolkitLabel xml:lang="de">einseitig</rdakit:toolkitLabel>
      <skos:definition xml:lang="de">Ein Layout, das ausschließlich eine Seite eines Blatts verwendet.</skos:definition>
      <rdakit:toolkitDefinition xml:lang="de">Ein Layout, das ausschließlich eine Seite eines Blatts verwendet.</rdakit:toolkitDefinition>
      <skos:scopeNote xml:lang="de">Dieser Terminus trifft auf Blätter und taktilen Text zu.</skos:scopeNote>
      <skos:prefLabel xml:lang="fi">yksipuolinen</skos:prefLabel>
      <rdakit:toolkitLabel xml:lang="fi">yksipuolinen</rdakit:toolkitLabel>
      <skos:definition xml:lang="fi">Layout vain arkin toisella puolella.</skos:definition>
      <rdakit:toolkitDefinition xml:lang="fi">Layout vain arkin toisella puolella.</rdakit:toolkitDefinition>
      <skos:scopeNote xml:lang="fi">Termi koskee arkkeja sekä taktiilia tekstiä.</skos:scopeNote>
      <skos:prefLabel xml:lang="vi">một mặt</skos:prefLabel>
      <rdakit:toolkitLabel xml:lang="vi">một mặt</rdakit:toolkitLabel>
      <skos:definition xml:lang="vi">Sắp đặt sử dụng chỉ một mặt của tờ.</skos:definition>
      <rdakit:toolkitDefinition xml:lang="vi">Sắp đặt sử dụng chỉ một mặt của tờ.</rdakit:toolkitDefinition>
      <skos:scopeNote xml:lang="vi">Thuật ngữ này áp dụng cho tờ và văn bản xúc giác.</skos:scopeNote>
      <skos:prefLabel xml:lang="da">enkeltsidet</skos:prefLabel>
      <rdakit:toolkitLabel xml:lang="da">enkeltsidet</rdakit:toolkitLabel>
      <skos:definition xml:lang="da">Layout der anvender den ene side af et ark.</skos:definition>
      <rdakit:toolkitDefinition xml:lang="da">Layout der anvender den ene side af et ark.</rdakit:toolkitDefinition>
      <skos:scopeNote xml:lang="da">Denne term anvendes til ark og taktil tekst.</skos:scopeNote>
      <skos:prefLabel xml:lang="fr">simple face</skos:prefLabel>
      <rdakit:toolkitLabel xml:lang="fr">simple face</rdakit:toolkitLabel>
      <skos:definition xml:lang="fr">Disposition qui utilise un seul côté d’une feuille.</skos:definition>
      <rdakit:toolkitDefinition xml:lang="fr">Disposition qui utilise un seul côté d’une feuille.</rdakit:toolkitDefinition>
      <skos:scopeNote xml:lang="fr">Ce terme s’applique aux feuilles et au texte tactile.</skos:scopeNote>
      <skos:prefLabel xml:lang="no">enkeltsidig</skos:prefLabel>
      <rdakit:toolkitLabel xml:lang="no">enkeltsidig</rdakit:toolkitLabel>
      <skos:definition xml:lang="no">Et oppsett som bruker bare den ene siden av et ark.</skos:definition>
      <rdakit:toolkitDefinition xml:lang="no">Et oppsett som bruker bare den ene siden av et ark.</rdakit:toolkitDefinition>
      <skos:scopeNote xml:lang="no">Dette begrepet gjelder ark og taktil tekst.</skos:scopeNote>
    </skos:Concept>
<!-- Concept: vertical score  -->
    <skos:Concept rdf:about="http://rdaregistry.info/termList/layout/1016" xml:lang="en">
      <skos:inScheme rdf:resource="http://rdaregistry.info/termList/layout"/>
      <reg:status rdf:resource="http://metadataregistry.org/uri/RegStatus/1001"/>
      <reg:identifier rdf:resource="http://metadataregistry.org/concepts/8449"/>
      <skos:prefLabel xml:lang="en">vertical score</skos:prefLabel>
      <rdakit:toolkitLabel xml:lang="en">vertical score</rdakit:toolkitLabel>
      <skos:definition xml:lang="en">A layout consisting of musical parts that are combined and written as chords.</skos:definition>
      <rdakit:toolkitDefinition xml:lang="en">A layout consisting of musical parts that are combined and written as chords.</rdakit:toolkitDefinition>
      <skos:scopeNote xml:lang="en">This term applies to tactile music resources.</skos:scopeNote>
      <skos:prefLabel xml:lang="it">partitura verticale</skos:prefLabel>
      <rdakit:toolkitLabel xml:lang="it">partitura verticale</rdakit:toolkitLabel>
      <skos:prefLabel xml:lang="de">vertical score</skos:prefLabel>
      <rdakit:toolkitLabel xml:lang="de">vertical score</rdakit:toolkitLabel>
      <skos:definition xml:lang="de">Ein Layout, bei dem mehrere Stimmen kombiniert und als Akkord geschrieben werden.</skos:definition>
      <rdakit:toolkitDefinition xml:lang="de">Ein Layout, bei dem mehrere Stimmen kombiniert und als Akkord geschrieben werden.</rdakit:toolkitDefinition>
      <skos:scopeNote xml:lang="de">Dieser Terminus trifft auf taktile Musikressourcen zu.</skos:scopeNote>
      <skos:prefLabel xml:lang="fi">vertikaalinen partituuri</skos:prefLabel>
      <rdakit:toolkitLabel xml:lang="fi">vertikaalinen partituuri</rdakit:toolkitLabel>
      <skos:definition xml:lang="fi">Layout, joka koostuu nuottistemmoista, jotka on yhdistetty ja merkitty sointuina.</skos:definition>
      <rdakit:toolkitDefinition xml:lang="fi">Layout, joka koostuu nuottistemmoista, jotka on yhdistetty ja merkitty sointuina.</rdakit:toolkitDefinition>
      <skos:scopeNote xml:lang="fi">Termi koskee taktiileja musiikkiaineistoja.</skos:scopeNote>
      <skos:prefLabel xml:lang="vi">bảng tổng phổ dọc</skos:prefLabel>
      <rdakit:toolkitLabel xml:lang="vi">bảng tổng phổ dọc</rdakit:toolkitLabel>
      <skos:definition xml:lang="vi">Sắp đặt gồm có các phần âm nhạc được kết hợp và viết như là hợp âm.</skos:definition>
      <rdakit:toolkitDefinition xml:lang="vi">Sắp đặt gồm có các phần âm nhạc được kết hợp và viết như là hợp âm.</rdakit:toolkitDefinition>
      <skos:scopeNote xml:lang="vi">Thuật ngữ này áp dụng cho tài nguyên âm nhạc xúc giác.</skos:scopeNote>
      <skos:prefLabel xml:lang="da">vertikalt partitur</skos:prefLabel>
      <rdakit:toolkitLabel xml:lang="da">vertikalt partitur</rdakit:toolkitLabel>
      <skos:definition xml:lang="da">Layout bestående af musikstemmer der er kombineret og skrevet som akkorder.</skos:definition>
      <rdakit:toolkitDefinition xml:lang="da">Layout bestående af musikstemmer der er kombineret og skrevet som akkorder.</rdakit:toolkitDefinition>
      <skos:scopeNote xml:lang="da">Denne term anvendes til taktile musik-ressourcer.</skos:scopeNote>
      <skos:prefLabel xml:lang="fr">partition verticale</skos:prefLabel>
      <rdakit:toolkitLabel xml:lang="fr">partition verticale</rdakit:toolkitLabel>
      <skos:definition xml:lang="fr">Disposition qui consiste en parties musicales combinées ensemble et écrites sous forme d’accords.</skos:definition>
      <rdakit:toolkitDefinition xml:lang="fr">Disposition qui consiste en parties musicales combinées ensemble et écrites sous forme d’accords.</rdakit:toolkitDefinition>
      <skos:scopeNote xml:lang="fr">Ce terme s’applique aux ressources de musique tactile.</skos:scopeNote>
      <skos:prefLabel xml:lang="no">vertikalt partitur</skos:prefLabel>
      <rdakit:toolkitLabel xml:lang="no">vertikalt partitur</rdakit:toolkitLabel>
      <skos:definition xml:lang="no">Et oppsett som består av musikalske stemmer som kombineres og skrives som akkorder.</skos:definition>
      <rdakit:toolkitDefinition xml:lang="no">Et oppsett som består av musikalske stemmer som kombineres og skrives som akkorder.</rdakit:toolkitDefinition>
      <skos:scopeNote xml:lang="no">Dette begrepet gjelder taktile musikkressurser.</skos:scopeNote>
    </skos:Concept>

<!-- Status properties used in this document  -->
    <skos:Concept rdf:about="http://metadataregistry.org/uri/RegStatus/1001">
        <skos:prefLabel xml:lang="en">Published</skos:prefLabel>
    </skos:Concept>

</rdf:RDF>
