<?xml version="1.0" encoding = "UTF-8"?>
<rdf:RDF
    xmlns:dc="http://purl.org/dc/elements/1.1/"
    xmlns:rdakit="http://metadataregistry.org/uri/profile/rdakit/"
    xmlns:rdf="http://www.w3.org/1999/02/22-rdf-syntax-ns#"
    xmlns:reg="http://metadataregistry.org/uri/profile/regap/"
    xmlns:owl="http://www.w3.org/2002/07/owl#"
    xmlns:skos="http://www.w3.org/2004/02/skos/core#">

<owl:Ontology rdf:about="http://rdaregistry.info/termList/noteMove" />
<!-- Scheme: RDA Form of Notated Movement -->
    <skos:ConceptScheme rdf:about="http://rdaregistry.info/termList/noteMove">
        <dc:title>RDA Form of Notated Movement</dc:title>
    </skos:ConceptScheme>

<!-- Concept: action stroke dance notation  -->
    <skos:Concept rdf:about="http://rdaregistry.info/termList/noteMove/1009" xml:lang="en">
      <skos:inScheme rdf:resource="http://rdaregistry.info/termList/noteMove"/>
      <reg:status rdf:resource="http://metadataregistry.org/uri/RegStatus/1001"/>
      <reg:identifier rdf:resource="http://metadataregistry.org/concepts/1035"/>
      <skos:prefLabel xml:lang="en">action stroke dance notation</skos:prefLabel>
      <skos:definition xml:lang="en">A form of notated movement using abstract symbols to represent body and limb positions and movements.</skos:definition>
      <skos:prefLabel xml:lang="de">Action Stroke Dance Notation</skos:prefLabel>
      <skos:definition xml:lang="de">Eine Form der Bewegungsnotation, die abstrakte Symbole verwendet, um die Positionen des Körpers und der Gliedmaßen und die Bewegungen darzustellen. Sie wird auf getrennten vertikalen Linien erfasst, die die Arme, Beine und den Körper darstellen.</skos:definition>
      <skos:definition xml:lang="fr">Forme de notation du mouvement qui utilise des symboles abstraits pour représenter les positions et les mouvements du corps et des membres.</skos:definition>
      <skos:prefLabel xml:lang="es">notación de movimientos para danza</skos:prefLabel>
      <skos:prefLabel xml:lang="zh">动作分解舞谱</skos:prefLabel>
      <rdakit:toolkitLabel xml:lang="zh">动作分解舞谱</rdakit:toolkitLabel>
      <rdakit:toolkitLabel xml:lang="en">action stroke dance notation</rdakit:toolkitLabel>
      <skos:definition xml:lang="zh">一种用抽象的符号表示身体和四肢位置及运动的动作谱形式。它在不同的垂直谱线上分别记录上肢、下肢和躯干的表现。</skos:definition>
      <rdakit:toolkitDefinition xml:lang="zh">一种用抽象的符号表示身体和四肢位置及运动的动作谱形式。它在不同的垂直谱线上分别记录上肢、下肢和躯干的表现。</rdakit:toolkitDefinition>
      <rdakit:toolkitDefinition xml:lang="en">A form of notated movement using abstract symbols to represent body and limb positions and movements.</rdakit:toolkitDefinition>
      <rdakit:toolkitDefinition xml:lang="fr">Forme de notation du mouvement qui utilise des symboles abstraits pour représenter les positions et les mouvements du corps et des membres.</rdakit:toolkitDefinition>
      <rdakit:toolkitLabel xml:lang="es">notación de movimientos para danza</rdakit:toolkitLabel>
      <skos:definition xml:lang="es">Forma de movimiento notado que utiliza símbolos abstractos para representar las posiciones y los movimientos del cuerpo y las extremidades. Se registra en un pentagrama vertical que representa los brazos, las piernas y el tronco.</skos:definition>
      <rdakit:toolkitDefinition xml:lang="es">Forma de movimiento notado que utiliza símbolos abstractos para representar las posiciones y los movimientos del cuerpo y las extremidades. Se registra en un pentagrama vertical que representa los brazos, las piernas y el tronco.</rdakit:toolkitDefinition>
      <skos:scopeNote xml:lang="en">It is recorded on separate vertical staffs representing the arms, legs, and trunk.</skos:scopeNote>
      <skos:prefLabel xml:lang="nl">Action Stroke Dance-notatie</skos:prefLabel>
      <rdakit:toolkitLabel xml:lang="nl">Action Stroke Dance-notatie</rdakit:toolkitLabel>
      <skos:definition xml:lang="nl">Een vorm van bewegingsnotatie waarbij abstracte symbolen gebruikt worden om posities en bewegingen voor te stellen van lichaam en ledematen. Deze is vastgelegd op aparte verticale balken voor armen, benen en romp.</skos:definition>
      <rdakit:toolkitDefinition xml:lang="nl">Een vorm van bewegingsnotatie waarbij abstracte symbolen gebruikt worden om posities en bewegingen voor te stellen van lichaam en ledematen. Deze is vastgelegd op aparte verticale balken voor armen, benen en romp.</rdakit:toolkitDefinition>
      <rdakit:toolkitLabel xml:lang="de">Action Stroke Dance Notation</rdakit:toolkitLabel>
      <rdakit:toolkitDefinition xml:lang="de">Eine Form der Bewegungsnotation, die abstrakte Symbole verwendet, um die Positionen des Körpers und der Gliedmaßen und die Bewegungen darzustellen. Sie wird auf getrennten vertikalen Linien erfasst, die die Arme, Beine und den Körper darstellen.</rdakit:toolkitDefinition>
      <skos:prefLabel xml:lang="it">Notazione coreografica Action Stroke</skos:prefLabel>
      <rdakit:toolkitLabel xml:lang="it">Notazione coreografica Action Stroke</rdakit:toolkitLabel>
      <skos:prefLabel xml:lang="fi">action stroke dance-notaatio</skos:prefLabel>
      <rdakit:toolkitLabel xml:lang="fi">action stroke dance-notaatio</rdakit:toolkitLabel>
      <skos:scopeNote xml:lang="de">Sie wird auf getrennten vertikalen Linien erfasst, die die Arme, Beine und den Körper darstellen.</skos:scopeNote>
      <skos:prefLabel xml:lang="vi">ký hiệu nhẩy theo nhịp hành động</skos:prefLabel>
      <rdakit:toolkitLabel xml:lang="vi">ký hiệu nhẩy theo nhịp hành động</rdakit:toolkitLabel>
      <skos:definition xml:lang="vi">Hình thái của động thái ký hiệu sử dụng ký hiệu trừu tượng để biểu diễn thân thể và vị trí và chuyển động tay chân.</skos:definition>
      <rdakit:toolkitDefinition xml:lang="vi">Hình thái của động thái ký hiệu sử dụng ký hiệu trừu tượng để biểu diễn thân thể và vị trí và chuyển động tay chân.</rdakit:toolkitDefinition>
      <skos:scopeNote xml:lang="vi">Nó được ghi trong các khuông nhạc dọc riêng rẽ biểu diễn tay, chân, thân hình.</skos:scopeNote>
      <skos:prefLabel xml:lang="da">action stroke-dansenotation</skos:prefLabel>
      <rdakit:toolkitLabel xml:lang="da">action stroke-dansenotation</rdakit:toolkitLabel>
      <skos:definition xml:lang="da">Form for bevægelsesnotation, der anvender abstrakte symboler til at repræsentere en krops og lemmers stillinger og bevægelser.</skos:definition>
      <rdakit:toolkitDefinition xml:lang="da">Form for bevægelsesnotation, der anvender abstrakte symboler til at repræsentere en krops og lemmers stillinger og bevægelser.</rdakit:toolkitDefinition>
      <skos:scopeNote xml:lang="da">Registreres på separate lodrette nodesystemer, der repræsenterer arme, ben og krop.</skos:scopeNote>
      <skos:prefLabel xml:lang="ca">notació de dansa per traços d’acció</skos:prefLabel>
      <rdakit:toolkitLabel xml:lang="ca">notació de dansa per traços d’acció</rdakit:toolkitLabel>
      <skos:definition xml:lang="ca">Forma de notació del moviment que usa símbols abstractes per representar les posicions i els moviments del cos i les extremitats.</skos:definition>
      <rdakit:toolkitDefinition xml:lang="ca">Forma de notació del moviment que usa símbols abstractes per representar les posicions i els moviments del cos i les extremitats.</rdakit:toolkitDefinition>
      <skos:scopeNote xml:lang="ca">S’enregistra en pentagrames verticals separats que representen els braços, les cames i el tronc.</skos:scopeNote>
      <skos:definition xml:lang="fi">Tanssinotaatio, jossa kehon ja raajojen asentoja ja liikkeitä esitetään abstrakteilla symboleilla.</skos:definition>
      <rdakit:toolkitDefinition xml:lang="fi">Tanssinotaatio, jossa kehon ja raajojen asentoja ja liikkeitä esitetään abstrakteilla symboleilla.</rdakit:toolkitDefinition>
      <skos:scopeNote xml:lang="fi">Käsiä, jalkoja ja kehoa kuvaavat symbolit merkitään erillisille pystysuorille viivoille.</skos:scopeNote>
      <skos:prefLabel xml:lang="fr">notation de la danse par traits d’action</skos:prefLabel>
      <rdakit:toolkitLabel xml:lang="fr">notation de la danse par traits d’action</rdakit:toolkitLabel>
      <skos:scopeNote xml:lang="fr">Cette notation utilise des portées verticales distinctes représentant les bras, les jambes et le tronc.</skos:scopeNote>
      <skos:prefLabel xml:lang="no">action stroke-dansenotasjon</skos:prefLabel>
      <rdakit:toolkitLabel xml:lang="no">action stroke-dansenotasjon</rdakit:toolkitLabel>
      <skos:definition xml:lang="no">En form for bevegelsesnotasjon som bruker abstrakte symboler for å representere kroppens og lemmenes posisjoner og bevegelser.</skos:definition>
      <rdakit:toolkitDefinition xml:lang="no">En form for bevegelsesnotasjon som bruker abstrakte symboler for å representere kroppens og lemmenes posisjoner og bevegelser.</rdakit:toolkitDefinition>
      <skos:scopeNote xml:lang="no">Dette registreres på adskilte, loddrette linjer som representerer armer, ben og torso.</skos:scopeNote>
    </skos:Concept>
<!-- Concept: Beauchamp-Feuillet notation  -->
    <skos:Concept rdf:about="http://rdaregistry.info/termList/noteMove/1008" xml:lang="en">
      <skos:inScheme rdf:resource="http://rdaregistry.info/termList/noteMove"/>
      <reg:status rdf:resource="http://metadataregistry.org/uri/RegStatus/1001"/>
      <reg:identifier rdf:resource="http://metadataregistry.org/concepts/1034"/>
      <skos:prefLabel xml:lang="en">Beauchamp-Feuillet notation</skos:prefLabel>
      <skos:definition xml:lang="en">A form of notated movement using abstract symbols to represent movements of the feet during an associated passage of music.</skos:definition>
      <skos:prefLabel xml:lang="de">Beauchamp-Feuillet-Notation</skos:prefLabel>
      <skos:definition xml:lang="de">Eine Form der Bewegungsnotation, die abstrakte Symbole verwendet, um die Bewegungen der Füße während einer damit in Verbindung stehenden Musikpassage darzustellen. Sie wird auf einer Spur erfasst, die den Weg des Tänzers auf dem Fußboden nachzeichnet.</skos:definition>
      <skos:prefLabel xml:lang="fr">notation Beauchamp-Feuillet</skos:prefLabel>
      <skos:definition xml:lang="fr">Forme de notation du mouvement qui utilise des symboles abstraits pour représenter les mouvements des pieds pendant un passage de musique auxquels ils sont associés.</skos:definition>
      <skos:prefLabel xml:lang="es">notación Beauchamp-Feuillet</skos:prefLabel>
      <skos:definition xml:lang="es">Forma de movimiento notado que utiliza símbolos abstractos para representar los movimientos del pie durante un pasaje asociado de música. Es registrado en un dibujo de pista que traza el camino del bailarín a lo largo del piso.</skos:definition>
      <skos:prefLabel xml:lang="zh">博尚-傅叶舞谱</skos:prefLabel>
      <rdakit:toolkitLabel xml:lang="zh">博尚-傅叶舞谱</rdakit:toolkitLabel>
      <rdakit:toolkitLabel xml:lang="en">Beauchamp-Feuillet notation</rdakit:toolkitLabel>
      <skos:definition xml:lang="zh">一种用抽象的符号表示与一段音乐相关的脚步运动的动作谱形式。它记录舞者在地面上的足迹或跨越的轨迹。</skos:definition>
      <rdakit:toolkitDefinition xml:lang="zh">一种用抽象的符号表示与一段音乐相关的脚步运动的动作谱形式。它记录舞者在地面上的足迹或跨越的轨迹。</rdakit:toolkitDefinition>
      <rdakit:toolkitDefinition xml:lang="en">A form of notated movement using abstract symbols to represent movements of the feet during an associated passage of music.</rdakit:toolkitDefinition>
      <rdakit:toolkitLabel xml:lang="fr">notation Beauchamp-Feuillet</rdakit:toolkitLabel>
      <rdakit:toolkitDefinition xml:lang="fr">Forme de notation du mouvement qui utilise des symboles abstraits pour représenter les mouvements des pieds pendant un passage de musique auxquels ils sont associés.</rdakit:toolkitDefinition>
      <rdakit:toolkitLabel xml:lang="es">notación Beauchamp-Feuillet</rdakit:toolkitLabel>
      <rdakit:toolkitDefinition xml:lang="es">Forma de movimiento notado que utiliza símbolos abstractos para representar los movimientos del pie durante un pasaje asociado de música. Es registrado en un dibujo de pista que traza el camino del bailarín a lo largo del piso.</rdakit:toolkitDefinition>
      <skos:scopeNote xml:lang="en">It is recorded on a track drawing that traces the path of the dancer across the floor.</skos:scopeNote>
      <skos:prefLabel xml:lang="nl">Beauchamp-Feuillet notatie</skos:prefLabel>
      <rdakit:toolkitLabel xml:lang="nl">Beauchamp-Feuillet notatie</rdakit:toolkitLabel>
      <skos:definition xml:lang="nl">Een vorm van bewegingsnotatie waarbij abstracte symbolen gebruikt worden om de bewegingen van de voeten voor te stellen gedurende een bijpassend stuk muziek. Deze is vastgelegd in een tekening die het spoor van de danser volgt over de vloer.</skos:definition>
      <rdakit:toolkitDefinition xml:lang="nl">Een vorm van bewegingsnotatie waarbij abstracte symbolen gebruikt worden om de bewegingen van de voeten voor te stellen gedurende een bijpassend stuk muziek. Deze is vastgelegd in een tekening die het spoor van de danser volgt over de vloer.</rdakit:toolkitDefinition>
      <rdakit:toolkitLabel xml:lang="de">Beauchamp-Feuillet-Notation</rdakit:toolkitLabel>
      <rdakit:toolkitDefinition xml:lang="de">Eine Form der Bewegungsnotation, die abstrakte Symbole verwendet, um die Bewegungen der Füße während einer damit in Verbindung stehenden Musikpassage darzustellen. Sie wird auf einer Spur erfasst, die den Weg des Tänzers auf dem Fußboden nachzeichnet.</rdakit:toolkitDefinition>
      <skos:prefLabel xml:lang="it">Notazione Beauchamp-Feuillet</skos:prefLabel>
      <rdakit:toolkitLabel xml:lang="it">Notazione Beauchamp-Feuillet</rdakit:toolkitLabel>
      <skos:prefLabel xml:lang="fi">Beauchamp-Feuillet-notaatio</skos:prefLabel>
      <rdakit:toolkitLabel xml:lang="fi">Beauchamp-Feuillet-notaatio</rdakit:toolkitLabel>
      <skos:prefLabel xml:lang="sv">Feuilletnotation</skos:prefLabel>
      <rdakit:toolkitLabel xml:lang="sv">Feuilletnotation</rdakit:toolkitLabel>
      <skos:scopeNote xml:lang="de">Sie wird auf einer Spur erfasst, die den Weg des Tänzers auf dem Fußboden nachzeichnet.</skos:scopeNote>
      <skos:prefLabel xml:lang="vi">ký hiệu Beauchamp-feuillet</skos:prefLabel>
      <rdakit:toolkitLabel xml:lang="vi">ký hiệu Beauchamp-feuillet</rdakit:toolkitLabel>
      <skos:definition xml:lang="vi">Hình thái của động thái ký hiệu sử dụng ký hiệu trừu tượng để trình bày chuyển động của chân với các đoạn âm nhạc.</skos:definition>
      <rdakit:toolkitDefinition xml:lang="vi">Hình thái của động thái ký hiệu sử dụng ký hiệu trừu tượng để trình bày chuyển động của chân với các đoạn âm nhạc.</rdakit:toolkitDefinition>
      <skos:scopeNote xml:lang="vi">Nó được ghi trên các rãnh ghi lại các bước của người múa trên sàn.</skos:scopeNote>
      <skos:prefLabel xml:lang="da">Beauchamp-Feuillet-notation</skos:prefLabel>
      <rdakit:toolkitLabel xml:lang="da">Beauchamp-Feuillet-notation</rdakit:toolkitLabel>
      <skos:definition xml:lang="da">Bevægelsesnotationsform, der anvender abstrakte symboler til at repræsentere føddernes bevægelse i forbindelse med et stykke musik.</skos:definition>
      <rdakit:toolkitDefinition xml:lang="da">Bevægelsesnotationsform, der anvender abstrakte symboler til at repræsentere føddernes bevægelse i forbindelse med et stykke musik.</rdakit:toolkitDefinition>
      <skos:scopeNote xml:lang="da">Registreres på en tegning, hvor en dansers vej hen over gulvet noteres.</skos:scopeNote>
      <skos:prefLabel xml:lang="ca">notació Beauchamp-Feuillet</skos:prefLabel>
      <rdakit:toolkitLabel xml:lang="ca">notació Beauchamp-Feuillet</rdakit:toolkitLabel>
      <skos:definition xml:lang="ca">Forma de notació del moviment que usa símbols abstractes per representar els moviments dels peus durant un passatge de música associat.</skos:definition>
      <rdakit:toolkitDefinition xml:lang="ca">Forma de notació del moviment que usa símbols abstractes per representar els moviments dels peus durant un passatge de música associat.</rdakit:toolkitDefinition>
      <skos:scopeNote xml:lang="ca">S’enregistra en un dibuix de la pista que traça el recorregut del ballarí sobre el terra.</skos:scopeNote>
      <skos:definition xml:lang="fi">Tanssinotaatio, jossa abstraktit symbolit esittävät jalkojen liikkeitä yhdistettynä samaan aikaan esitettävän musiikin kanssa.</skos:definition>
      <rdakit:toolkitDefinition xml:lang="fi">Tanssinotaatio, jossa abstraktit symbolit esittävät jalkojen liikkeitä yhdistettynä samaan aikaan esitettävän musiikin kanssa.</rdakit:toolkitDefinition>
      <skos:scopeNote xml:lang="fi">Notaatio merkitään piirroksilla, jotka seuraavat lattian ylittävän tanssijan liikerataa.</skos:scopeNote>
      <skos:scopeNote xml:lang="fr">Cette notation utilise un dessin montrant le parcours du danseur sur le plancher.</skos:scopeNote>
      <skos:prefLabel xml:lang="no">Beauchamp-Feuillet-notasjon</skos:prefLabel>
      <rdakit:toolkitLabel xml:lang="no">Beauchamp-Feuillet-notasjon</rdakit:toolkitLabel>
      <skos:definition xml:lang="no">En form for bevegelsesnotasjon som bruker abstrakte symboler for å representere føttenes bevegelser under et tilknyttet musikkstykke.</skos:definition>
      <rdakit:toolkitDefinition xml:lang="no">En form for bevegelsesnotasjon som bruker abstrakte symboler for å representere føttenes bevegelser under et tilknyttet musikkstykke.</rdakit:toolkitDefinition>
      <skos:scopeNote xml:lang="no">Dette registreres på en tegning som følger danserens spor over gulvet.</skos:scopeNote>
    </skos:Concept>
<!-- Concept: Benesh movement notation  -->
    <skos:Concept rdf:about="http://rdaregistry.info/termList/noteMove/1007" xml:lang="en">
      <skos:inScheme rdf:resource="http://rdaregistry.info/termList/noteMove"/>
      <reg:status rdf:resource="http://metadataregistry.org/uri/RegStatus/1001"/>
      <reg:identifier rdf:resource="http://metadataregistry.org/concepts/1033"/>
      <skos:prefLabel xml:lang="en">Benesh movement notation</skos:prefLabel>
      <skos:definition xml:lang="en">A form of notated movement using abstract symbols to represent body and limb positions as seen from the back.</skos:definition>
      <skos:definition xml:lang="de">Eine Form der Bewegungsnotation, die abstrakte Symbole verwendet, um die Positionen des Körpers und der Gliedmaßen darzustellen, wie sie von hinten zu sehen sind. Sie wird auf fünfzeiligen horizontalen Notenlinien erfasst, die den Körper darstellen.</skos:definition>
      <skos:prefLabel xml:lang="de">Choreologie</skos:prefLabel>
      <skos:prefLabel xml:lang="fr">notation Benesh</skos:prefLabel>
      <skos:definition xml:lang="fr">Forme de notation du mouvement qui utilise des symboles abstraits pour représenter les positions du corps et des membres vus de dos.</skos:definition>
      <skos:prefLabel xml:lang="es">notación de movimientos Benesh</skos:prefLabel>
      <skos:definition xml:lang="es">Forma de movimiento notado que utiliza símbolos abstractos para representar posiciones del cuerpo y miembros vistos desde atrás. Es registrado en un pentagrama horizontal de cinco líneas que representa el cuerpo.</skos:definition>
      <skos:prefLabel xml:lang="zh">班尼斯动作谱</skos:prefLabel>
      <rdakit:toolkitLabel xml:lang="zh">班尼斯动作谱</rdakit:toolkitLabel>
      <rdakit:toolkitLabel xml:lang="en">Benesh movement notation</rdakit:toolkitLabel>
      <skos:definition xml:lang="zh">一种用抽象的符号表示从背后所看到的身体和四肢位置的动作谱形式。它在五条水平谱线上记录身体的表现。</skos:definition>
      <rdakit:toolkitDefinition xml:lang="zh">一种用抽象的符号表示从背后所看到的身体和四肢位置的动作谱形式。它在五条水平谱线上记录身体的表现。</rdakit:toolkitDefinition>
      <rdakit:toolkitDefinition xml:lang="en">A form of notated movement using abstract symbols to represent body and limb positions as seen from the back.</rdakit:toolkitDefinition>
      <rdakit:toolkitLabel xml:lang="fr">notation Benesh</rdakit:toolkitLabel>
      <rdakit:toolkitDefinition xml:lang="fr">Forme de notation du mouvement qui utilise des symboles abstraits pour représenter les positions du corps et des membres vus de dos.</rdakit:toolkitDefinition>
      <rdakit:toolkitLabel xml:lang="es">notación de movimientos Benesh</rdakit:toolkitLabel>
      <rdakit:toolkitDefinition xml:lang="es">Forma de movimiento notado que utiliza símbolos abstractos para representar posiciones del cuerpo y miembros vistos desde atrás. Es registrado en un pentagrama horizontal de cinco líneas que representa el cuerpo.</rdakit:toolkitDefinition>
      <skos:scopeNote xml:lang="en">It is recorded on a five-line horizontal staff that represents the body.</skos:scopeNote>
      <skos:prefLabel xml:lang="nl">Benesh bewegingsnotatie</skos:prefLabel>
      <skos:altLabel xml:lang="nl">Choreologie</skos:altLabel>
      <rdakit:toolkitLabel xml:lang="nl">Benesh bewegingsnotatie</rdakit:toolkitLabel>
      <skos:definition xml:lang="nl">Een vorm van bewegingsnotatie waarbij abstracte symbolen gebruikt worden om de posities van lichaam en ledematen voor te stellen gezien vanaf de rug. Deze is vastgelegd op een horizontale balk van vijf lijntjes, die het lichaam voorstelt.</skos:definition>
      <rdakit:toolkitDefinition xml:lang="nl">Een vorm van bewegingsnotatie waarbij abstracte symbolen gebruikt worden om de posities van lichaam en ledematen voor te stellen gezien vanaf de rug. Deze is vastgelegd op een horizontale balk van vijf lijntjes, die het lichaam voorstelt.</rdakit:toolkitDefinition>
      <rdakit:toolkitLabel xml:lang="de">Choreologie</rdakit:toolkitLabel>
      <rdakit:toolkitDefinition xml:lang="de">Eine Form der Bewegungsnotation, die abstrakte Symbole verwendet, um die Positionen des Körpers und der Gliedmaßen darzustellen, wie sie von hinten zu sehen sind. Sie wird auf fünfzeiligen horizontalen Notenlinien erfasst, die den Körper darstellen.</rdakit:toolkitDefinition>
      <skos:prefLabel xml:lang="it">Notazione Benesh</skos:prefLabel>
      <rdakit:toolkitLabel xml:lang="it">Notazione Benesh</rdakit:toolkitLabel>
      <skos:prefLabel xml:lang="fi">Benesh-liikenotaatio</skos:prefLabel>
      <rdakit:toolkitLabel xml:lang="fi">Benesh-liikenotaatio</rdakit:toolkitLabel>
      <skos:prefLabel xml:lang="sv">Beneshnotation</skos:prefLabel>
      <rdakit:toolkitLabel xml:lang="sv">Beneshnotation</rdakit:toolkitLabel>
      <skos:scopeNote xml:lang="de">Sie wird auf fünfzeiligen horizontalen Notenlinien erfasst, die den Körper darstellen.</skos:scopeNote>
      <skos:prefLabel xml:lang="vi">ký hiệu chuyển động Benesh</skos:prefLabel>
      <rdakit:toolkitLabel xml:lang="vi">ký hiệu chuyển động Benesh</rdakit:toolkitLabel>
      <skos:definition xml:lang="vi">Hình thái của động thái ký hiệu sử dụng ký hiệu trừu tượng để biểu diễn thân thể và vị trí tay chân được nhìn từ phía sau.</skos:definition>
      <rdakit:toolkitDefinition xml:lang="vi">Hình thái của động thái ký hiệu sử dụng ký hiệu trừu tượng để biểu diễn thân thể và vị trí tay chân được nhìn từ phía sau.</rdakit:toolkitDefinition>
      <skos:scopeNote xml:lang="vi">Nố được ghi trên khuông nhạc ngang biểu diễn thân thể.</skos:scopeNote>
      <skos:prefLabel xml:lang="da">Beneshs bevægelsesnotation</skos:prefLabel>
      <rdakit:toolkitLabel xml:lang="da">Beneshs bevægelsesnotation</rdakit:toolkitLabel>
      <skos:definition xml:lang="da">Bevægelsesnotationsform, der anvender abstrakte symboler til at repræsentere en krops og lemmers stillinger set bagfra.</skos:definition>
      <rdakit:toolkitDefinition xml:lang="da">Bevægelsesnotationsform, der anvender abstrakte symboler til at repræsentere en krops og lemmers stillinger set bagfra.</rdakit:toolkitDefinition>
      <skos:scopeNote xml:lang="da">Registreres i et femlinjet vandret nodesystem, der repræsenterer kroppen.</skos:scopeNote>
      <skos:prefLabel xml:lang="ca">notació de moviment Benesh</skos:prefLabel>
      <rdakit:toolkitLabel xml:lang="ca">notació de moviment Benesh</rdakit:toolkitLabel>
      <skos:definition xml:lang="ca">Forma de notació del moviment que usa símbols abstractes per representar les posicions del cos i les extremitats tal com es veuen des de darrere.</skos:definition>
      <rdakit:toolkitDefinition xml:lang="ca">Forma de notació del moviment que usa símbols abstractes per representar les posicions del cos i les extremitats tal com es veuen des de darrere.</rdakit:toolkitDefinition>
      <skos:scopeNote xml:lang="ca">S’enregistra en un pentagrama horitzontal de cinc línies que representa el cos.</skos:scopeNote>
      <skos:definition xml:lang="fi">Tanssinotaatio, jossa abstrakteilla symboleilla esitetään kehon ja raajojen asentoja takaapäin nähtynä.</skos:definition>
      <rdakit:toolkitDefinition xml:lang="fi">Tanssinotaatio, jossa abstrakteilla symboleilla esitetään kehon ja raajojen asentoja takaapäin nähtynä.</rdakit:toolkitDefinition>
      <skos:scopeNote xml:lang="fi">Notaatio merkitään kehoa esittävälle viisiriviselle horisontaaliselle linjastolle.</skos:scopeNote>
      <skos:scopeNote xml:lang="fr">Cette notation utilise une portée horizontale de cinq lignes qui représente le corps.</skos:scopeNote>
      <skos:prefLabel xml:lang="no">Benesh-notasjon</skos:prefLabel>
      <rdakit:toolkitLabel xml:lang="no">Benesh-notasjon</rdakit:toolkitLabel>
      <skos:definition xml:lang="no">En form for bevegelsesnotasjon som bruker abstrakte symboler for å representere kroppens og lemmenes posisjoner sett bakfra.</skos:definition>
      <rdakit:toolkitDefinition xml:lang="no">En form for bevegelsesnotasjon som bruker abstrakte symboler for å representere kroppens og lemmenes posisjoner sett bakfra.</rdakit:toolkitDefinition>
      <skos:scopeNote xml:lang="no">Dette registreres på en vannrett stav med fem linjer som representerer kroppen.</skos:scopeNote>
    </skos:Concept>
<!-- Concept: DanceWriting  -->
    <skos:Concept rdf:about="http://rdaregistry.info/termList/noteMove/1006" xml:lang="en">
      <skos:inScheme rdf:resource="http://rdaregistry.info/termList/noteMove"/>
      <reg:status rdf:resource="http://metadataregistry.org/uri/RegStatus/1001"/>
      <reg:identifier rdf:resource="http://metadataregistry.org/concepts/1032"/>
      <skos:prefLabel xml:lang="en">DanceWriting</skos:prefLabel>
      <skos:definition xml:lang="en">A form of notated movement using figurative and abstract symbols to represent body and limb positions and movements.</skos:definition>
      <skos:definition xml:lang="de">Eine Form der Bewegungsnotation, die figurative und abstrakte Symbole verwendet, um die Positionen des Körpers und der Gliedmaßen und die Bewegungen darzustellen. Sie wird auf fünfzeiligen horizontalen Notenlinien erfasst, die den Körper darstellen.</skos:definition>
      <skos:prefLabel xml:lang="de">Sutton Dance-Writing</skos:prefLabel>
      <skos:prefLabel xml:lang="fr">DanceWriting</skos:prefLabel>
      <skos:definition xml:lang="fr">Forme de notation du mouvement qui utilise des symboles figuratifs et abstraits pour représenter les positions et les mouvements du corps et des membres.</skos:definition>
      <skos:prefLabel xml:lang="es">DanceWriting</skos:prefLabel>
      <skos:definition xml:lang="es">Forma de movimiento notado que utiliza símbolos figurativos y abstractos para representar posiciones y movimientos del cuerpo y las extremidades. Es registrado en un pentagrama horizontal de cinco líneas que representa el cuerpo.</skos:definition>
      <skos:prefLabel xml:lang="zh">[萨顿] 舞谱</skos:prefLabel>
      <rdakit:toolkitLabel xml:lang="zh">[萨顿] 舞谱</rdakit:toolkitLabel>
      <rdakit:toolkitLabel xml:lang="en">DanceWriting</rdakit:toolkitLabel>
      <skos:definition xml:lang="zh">一种用形象的和抽象的符号表示身体和四肢位置及运动的动作谱形式。它在水平方向的五条谱线上记录身体的表现。</skos:definition>
      <rdakit:toolkitDefinition xml:lang="zh">一种用形象的和抽象的符号表示身体和四肢位置及运动的动作谱形式。它在水平方向的五条谱线上记录身体的表现。</rdakit:toolkitDefinition>
      <rdakit:toolkitDefinition xml:lang="en">A form of notated movement using figurative and abstract symbols to represent body and limb positions and movements.</rdakit:toolkitDefinition>
      <rdakit:toolkitLabel xml:lang="fr">DanceWriting</rdakit:toolkitLabel>
      <rdakit:toolkitDefinition xml:lang="fr">Forme de notation du mouvement qui utilise des symboles figuratifs et abstraits pour représenter les positions et les mouvements du corps et des membres.</rdakit:toolkitDefinition>
      <rdakit:toolkitLabel xml:lang="es">DanceWriting</rdakit:toolkitLabel>
      <rdakit:toolkitDefinition xml:lang="es">Forma de movimiento notado que utiliza símbolos figurativos y abstractos para representar posiciones y movimientos del cuerpo y las extremidades. Es registrado en un pentagrama horizontal de cinco líneas que representa el cuerpo.</rdakit:toolkitDefinition>
      <skos:scopeNote xml:lang="en">It is recorded on a five-line horizontal staff that represents the body.</skos:scopeNote>
      <skos:prefLabel xml:lang="nl">DanceWriting</skos:prefLabel>
      <rdakit:toolkitLabel xml:lang="nl">DanceWriting</rdakit:toolkitLabel>
      <skos:definition xml:lang="nl">Een vorm van bewegingsnotatie waarbij figuratieve en abstracte symbolen gebruikt worden om posities en bewegingen voor te stellen van lichaam en ledematen. Deze is vastgelegd op een horizontale balk van vijf lijntjes, die het lichaam voorstelt.</skos:definition>
      <rdakit:toolkitDefinition xml:lang="nl">Een vorm van bewegingsnotatie waarbij figuratieve en abstracte symbolen gebruikt worden om posities en bewegingen voor te stellen van lichaam en ledematen. Deze is vastgelegd op een horizontale balk van vijf lijntjes, die het lichaam voorstelt.</rdakit:toolkitDefinition>
      <rdakit:toolkitLabel xml:lang="de">Sutton Dance-Writing</rdakit:toolkitLabel>
      <rdakit:toolkitDefinition xml:lang="de">Eine Form der Bewegungsnotation, die figurative und abstrakte Symbole verwendet, um die Positionen des Körpers und der Gliedmaßen und die Bewegungen darzustellen. Sie wird auf fünfzeiligen horizontalen Notenlinien erfasst, die den Körper darstellen.</rdakit:toolkitDefinition>
      <skos:prefLabel xml:lang="it">DanceWriting</skos:prefLabel>
      <rdakit:toolkitLabel xml:lang="it">DanceWriting</rdakit:toolkitLabel>
      <skos:prefLabel xml:lang="fi">DanceWriting</skos:prefLabel>
      <rdakit:toolkitLabel xml:lang="fi">DanceWriting</rdakit:toolkitLabel>
      <skos:scopeNote xml:lang="de">Sie wird auf fünfzeiligen horizontalen Notenlinien erfasst, die den Körper darstellen.</skos:scopeNote>
      <skos:prefLabel xml:lang="vi">DanceWriting</skos:prefLabel>
      <rdakit:toolkitLabel xml:lang="vi">DanceWriting</rdakit:toolkitLabel>
      <skos:definition xml:lang="vi">Hình thái của động thái ký hiệu sử dụng ký hiệutượng hình và trừu tượng đểbiểu diễncho các vị trívà chuyển động củacơ thể và chân tay.</skos:definition>
      <rdakit:toolkitDefinition xml:lang="vi">Hình thái của động thái ký hiệu sử dụng ký hiệutượng hình và trừu tượng đểbiểu diễncho các vị trívà chuyển động củacơ thể và chân tay.</rdakit:toolkitDefinition>
      <skos:scopeNote xml:lang="vi">Nóp được ghi trên khuông nhạc ngang năm dòng biểu diễn thân thể.</skos:scopeNote>
      <skos:prefLabel xml:lang="da">Dansenotation</skos:prefLabel>
      <rdakit:toolkitLabel xml:lang="da">Dansenotation</rdakit:toolkitLabel>
      <skos:definition xml:lang="da">Bevægelsesnotationsform, der anvender figurative og abstrakte symboler til at repræsentere en krops og lemmers stillinger og bevægelser.</skos:definition>
      <rdakit:toolkitDefinition xml:lang="da">Bevægelsesnotationsform, der anvender figurative og abstrakte symboler til at repræsentere en krops og lemmers stillinger og bevægelser.</rdakit:toolkitDefinition>
      <skos:scopeNote xml:lang="da">Registreres i et femlinjet vandret nodesystem, der repræsenterer kroppen.</skos:scopeNote>
      <skos:prefLabel xml:lang="ca">DanceWriting</skos:prefLabel>
      <rdakit:toolkitLabel xml:lang="ca">DanceWriting</rdakit:toolkitLabel>
      <skos:definition xml:lang="ca">Forma de notació del moviment que usa símbols figuratius i abstractes per representat les posicions i els moviments del cos i les extremitats.</skos:definition>
      <rdakit:toolkitDefinition xml:lang="ca">Forma de notació del moviment que usa símbols figuratius i abstractes per representat les posicions i els moviments del cos i les extremitats.</rdakit:toolkitDefinition>
      <skos:scopeNote xml:lang="ca">S’enregistra en un pentagrama horitzontal de cinc línies que representa el cos.</skos:scopeNote>
      <skos:definition xml:lang="fi">Tanssinotaatio, jossa esittävin ja abstraktein symbolein esitetään kehon ja raajojen asentoja ja liikkeitä.</skos:definition>
      <rdakit:toolkitDefinition xml:lang="fi">Tanssinotaatio, jossa esittävin ja abstraktein symbolein esitetään kehon ja raajojen asentoja ja liikkeitä.</rdakit:toolkitDefinition>
      <skos:scopeNote xml:lang="fi">Notaatio merkitään kehoa esittävälle viisiriviselle horisontaaliselle linjastolle.</skos:scopeNote>
      <skos:scopeNote xml:lang="fr">Cette notation utilise une portée horizontale de cinq lignes qui représente le corps.</skos:scopeNote>
      <skos:prefLabel xml:lang="no">dansenotasjon</skos:prefLabel>
      <rdakit:toolkitLabel xml:lang="no">dansenotasjon</rdakit:toolkitLabel>
      <skos:definition xml:lang="no">En form for bevegelsesnotasjon som bruker figurative og abstrakte symboler for å representere kroppens og lemmenes posisjoner og bevegelser.</skos:definition>
      <rdakit:toolkitDefinition xml:lang="no">En form for bevegelsesnotasjon som bruker figurative og abstrakte symboler for å representere kroppens og lemmenes posisjoner og bevegelser.</rdakit:toolkitDefinition>
      <skos:scopeNote xml:lang="no">Dette registreres på en vannrett stav med fem linjer som representerer kroppen.</skos:scopeNote>
    </skos:Concept>
<!-- Concept: Eshkol-Wachman movement notation  -->
    <skos:Concept rdf:about="http://rdaregistry.info/termList/noteMove/1005" xml:lang="en">
      <skos:inScheme rdf:resource="http://rdaregistry.info/termList/noteMove"/>
      <reg:status rdf:resource="http://metadataregistry.org/uri/RegStatus/1001"/>
      <reg:identifier rdf:resource="http://metadataregistry.org/concepts/1031"/>
      <skos:prefLabel xml:lang="en">Eshkol-Wachman movement notation</skos:prefLabel>
      <skos:definition xml:lang="en">A form of notated movement using a spherical coordinate system to denote body and limb positions.</skos:definition>
      <skos:prefLabel xml:lang="de">Eshkol-Wachmann-Notation</skos:prefLabel>
      <skos:definition xml:lang="de">Eine Form der Bewegungsnotation, die ein sphärisches Koordinatensystem verwendet, um die Positionen des Körpers und der Gliedmaßen anzuzeigen. Sie wird auf einem Gitternetz erfasst, das den Körper darstellt.</skos:definition>
      <skos:prefLabel xml:lang="fr">notation Eshkol-Wachman</skos:prefLabel>
      <skos:definition xml:lang="fr">Forme de notation du mouvement qui utilise un système sphérique de coordonnées pour représenter les positions du corps et des membres.</skos:definition>
      <skos:prefLabel xml:lang="es">notación de movimientos Eshkol-Wachman</skos:prefLabel>
      <skos:definition xml:lang="es">Forma de movimiento notado que utiliza un sistema esférico coordinado para denotar las posiciones del cuerpo y las extremidades. Es registrado en una rejilla que representa el cuerpo.</skos:definition>
      <skos:prefLabel xml:lang="zh">埃什科尔-瓦克曼动作谱</skos:prefLabel>
      <rdakit:toolkitLabel xml:lang="zh">埃什科尔-瓦克曼动作谱</rdakit:toolkitLabel>
      <rdakit:toolkitLabel xml:lang="en">Eshkol-Wachman movement notation</rdakit:toolkitLabel>
      <skos:definition xml:lang="zh">一种用球面坐标体系指出身体和四肢位置的动作谱形式。它在一个网格上记录身体的表现。</skos:definition>
      <rdakit:toolkitDefinition xml:lang="zh">一种用球面坐标体系指出身体和四肢位置的动作谱形式。它在一个网格上记录身体的表现。</rdakit:toolkitDefinition>
      <rdakit:toolkitDefinition xml:lang="en">A form of notated movement using a spherical coordinate system to denote body and limb positions.</rdakit:toolkitDefinition>
      <rdakit:toolkitLabel xml:lang="fr">notation Eshkol-Wachman</rdakit:toolkitLabel>
      <rdakit:toolkitDefinition xml:lang="fr">Forme de notation du mouvement qui utilise un système sphérique de coordonnées pour représenter les positions du corps et des membres.</rdakit:toolkitDefinition>
      <rdakit:toolkitLabel xml:lang="es">notación de movimientos Eshkol-Wachman</rdakit:toolkitLabel>
      <rdakit:toolkitDefinition xml:lang="es">Forma de movimiento notado que utiliza un sistema esférico coordinado para denotar las posiciones del cuerpo y las extremidades. Es registrado en una rejilla que representa el cuerpo.</rdakit:toolkitDefinition>
      <skos:scopeNote xml:lang="en">It is recorded on a grid that represents the body.</skos:scopeNote>
      <skos:prefLabel xml:lang="nl">Eshkol-Wachman bewegingsnotatie</skos:prefLabel>
      <rdakit:toolkitLabel xml:lang="nl">Eshkol-Wachman bewegingsnotatie</rdakit:toolkitLabel>
      <skos:definition xml:lang="nl">Een vorm van bewegingsnotatie waarbij een bolvormig coördinatensysteem gebruikt wordt om de positie van lichaam en ledematen voor te stellen. Deze is vastgelegd op een raster dat het lichaam voorstelt.</skos:definition>
      <rdakit:toolkitDefinition xml:lang="nl">Een vorm van bewegingsnotatie waarbij een bolvormig coördinatensysteem gebruikt wordt om de positie van lichaam en ledematen voor te stellen. Deze is vastgelegd op een raster dat het lichaam voorstelt.</rdakit:toolkitDefinition>
      <rdakit:toolkitLabel xml:lang="de">Eshkol-Wachmann-Notation</rdakit:toolkitLabel>
      <rdakit:toolkitDefinition xml:lang="de">Eine Form der Bewegungsnotation, die ein sphärisches Koordinatensystem verwendet, um die Positionen des Körpers und der Gliedmaßen anzuzeigen. Sie wird auf einem Gitternetz erfasst, das den Körper darstellt.</rdakit:toolkitDefinition>
      <skos:prefLabel xml:lang="it">Notazione di movimento Eshkol-Wachman</skos:prefLabel>
      <rdakit:toolkitLabel xml:lang="it">Notazione di movimento Eshkol-Wachman</rdakit:toolkitLabel>
      <skos:prefLabel xml:lang="fi">Eshkol-Wachman -liikenotaatio</skos:prefLabel>
      <rdakit:toolkitLabel xml:lang="fi">Eshkol-Wachman -liikenotaatio</rdakit:toolkitLabel>
      <skos:prefLabel xml:lang="sv">Eshkol-Wachmnnotation</skos:prefLabel>
      <rdakit:toolkitLabel xml:lang="sv">Eshkol-Wachmnnotation</rdakit:toolkitLabel>
      <skos:scopeNote xml:lang="de">Sie wird auf einem Gitternetz erfasst, das den Körper darstellt.</skos:scopeNote>
      <skos:prefLabel xml:lang="vi">ký hiệu chuyển động Eshkol-wachman</skos:prefLabel>
      <rdakit:toolkitLabel xml:lang="vi">ký hiệu chuyển động Eshkol-wachman</rdakit:toolkitLabel>
      <skos:definition xml:lang="vi">Hình thái của động thái ký hiệusử dụng một hệ thống phối hợp hình cầu để biểu thị các vị trícủacơ thể và chân tay.</skos:definition>
      <rdakit:toolkitDefinition xml:lang="vi">Hình thái của động thái ký hiệusử dụng một hệ thống phối hợp hình cầu để biểu thị các vị trícủacơ thể và chân tay.</rdakit:toolkitDefinition>
      <skos:scopeNote xml:lang="vi">Nó được ghi trên lướikẻ ô biểu diễncơ thể.</skos:scopeNote>
      <skos:prefLabel xml:lang="da">Eshkol-Wachman-bevægelsesnotation</skos:prefLabel>
      <rdakit:toolkitLabel xml:lang="da">Eshkol-Wachman-bevægelsesnotation</rdakit:toolkitLabel>
      <skos:definition xml:lang="da">Bevægelsesnotationsform, der anvender et kugleformet koordinatsystem til at angive en krops og lemmers stillinger.</skos:definition>
      <rdakit:toolkitDefinition xml:lang="da">Bevægelsesnotationsform, der anvender et kugleformet koordinatsystem til at angive en krops og lemmers stillinger.</rdakit:toolkitDefinition>
      <skos:scopeNote xml:lang="da">Registreres i et gradnet, der repræsenterer kroppen.</skos:scopeNote>
      <skos:prefLabel xml:lang="ca">notació de moviment Eshkol-Wachman</skos:prefLabel>
      <rdakit:toolkitLabel xml:lang="ca">notació de moviment Eshkol-Wachman</rdakit:toolkitLabel>
      <skos:definition xml:lang="ca">Forma de notació del moviment que usa un sistema esfèric de coordenades per representar les posicions del cos i les extremitats.</skos:definition>
      <rdakit:toolkitDefinition xml:lang="ca">Forma de notació del moviment que usa un sistema esfèric de coordenades per representar les posicions del cos i les extremitats.</rdakit:toolkitDefinition>
      <skos:scopeNote xml:lang="ca">S’enregistra sobre una quadrícula que representa el cos.</skos:scopeNote>
      <skos:definition xml:lang="fi">Liikenotaatio, jossa käytetään pallokoordinaatistoa ilmaisemaan kehon ja raajojen asentoa.</skos:definition>
      <rdakit:toolkitDefinition xml:lang="fi">Liikenotaatio, jossa käytetään pallokoordinaatistoa ilmaisemaan kehon ja raajojen asentoa.</rdakit:toolkitDefinition>
      <skos:scopeNote xml:lang="fi">Notaatio merkitään kehoa esittävään ruudukkoon.</skos:scopeNote>
      <skos:scopeNote xml:lang="fr">Cette notation utilise une grille qui représente le corps.</skos:scopeNote>
      <skos:prefLabel xml:lang="no">Eshkol-Wachman-notasjon</skos:prefLabel>
      <rdakit:toolkitLabel xml:lang="no">Eshkol-Wachman-notasjon</rdakit:toolkitLabel>
      <skos:definition xml:lang="no">En form for bevegelsesnotasjon som bruker et kuleformet koordinatsystem for å betegne kroppens og lemmenes posisjoner og bevegelser.</skos:definition>
      <rdakit:toolkitDefinition xml:lang="no">En form for bevegelsesnotasjon som bruker et kuleformet koordinatsystem for å betegne kroppens og lemmenes posisjoner og bevegelser.</rdakit:toolkitDefinition>
      <skos:scopeNote xml:lang="no">Det er gjengitt på et nett som representerer kroppen.</skos:scopeNote>
    </skos:Concept>
<!-- Concept: game play notation  -->
    <skos:Concept rdf:about="http://rdaregistry.info/termList/noteMove/1004" xml:lang="en">
      <skos:inScheme rdf:resource="http://rdaregistry.info/termList/noteMove"/>
      <reg:status rdf:resource="http://metadataregistry.org/uri/RegStatus/1001"/>
      <reg:identifier rdf:resource="http://metadataregistry.org/concepts/1030"/>
      <skos:prefLabel xml:lang="en">game play notation</skos:prefLabel>
      <skos:definition xml:lang="en">A form of notated movement for recording the position of players or pieces during the course of a game.</skos:definition>
      <skos:prefLabel xml:lang="de">Spielnotation</skos:prefLabel>
      <skos:definition xml:lang="de">Eine Form der Bewegungsnotation, die taktische Bewegungen während eines Spiels wie zum Beispiel Schach aufzeichnet.</skos:definition>
      <skos:prefLabel xml:lang="fr">notation de jeu</skos:prefLabel>
      <skos:definition xml:lang="fr">Forme de notation du mouvement servant à enregistrer la position des joueurs ou des pièces pendant le déroulement d’un jeu.</skos:definition>
      <skos:prefLabel xml:lang="es">notación de jugabilidad</skos:prefLabel>
      <skos:prefLabel xml:lang="zh">游戏谱</skos:prefLabel>
      <rdakit:toolkitLabel xml:lang="zh">游戏谱</rdakit:toolkitLabel>
      <rdakit:toolkitLabel xml:lang="en">game play notation</rdakit:toolkitLabel>
      <skos:definition xml:lang="zh">在诸如下棋的游戏过程中记录战术步骤的动作谱形式。</skos:definition>
      <rdakit:toolkitDefinition xml:lang="zh">在诸如下棋的游戏过程中记录战术步骤的动作谱形式。</rdakit:toolkitDefinition>
      <rdakit:toolkitDefinition xml:lang="en">A form of notated movement for recording the position of players or pieces during the course of a game.</rdakit:toolkitDefinition>
      <rdakit:toolkitLabel xml:lang="fr">notation de jeu</rdakit:toolkitLabel>
      <rdakit:toolkitDefinition xml:lang="fr">Forme de notation du mouvement servant à enregistrer la position des joueurs ou des pièces pendant le déroulement d’un jeu.</rdakit:toolkitDefinition>
      <rdakit:toolkitLabel xml:lang="es">notación de jugabilidad</rdakit:toolkitLabel>
      <skos:definition xml:lang="es">Forma de movimiento notado que registra los movimientos tácticos durante el curso de un juego, como el ajedrez.</skos:definition>
      <rdakit:toolkitDefinition xml:lang="es">Forma de movimiento notado que registra los movimientos tácticos durante el curso de un juego, como el ajedrez.</rdakit:toolkitDefinition>
      <skos:prefLabel xml:lang="nl">Spelnotatie</skos:prefLabel>
      <skos:altLabel xml:lang="nl">Speldiagrammen</skos:altLabel>
      <rdakit:toolkitLabel xml:lang="nl">Spelnotatie</rdakit:toolkitLabel>
      <skos:definition xml:lang="nl">Een vorm van bewegingsnotatie waarbij tactische zetten bijgehouden worden gedurende het verloop van een spel, zoals schaken.</skos:definition>
      <rdakit:toolkitDefinition xml:lang="nl">Een vorm van bewegingsnotatie waarbij tactische zetten bijgehouden worden gedurende het verloop van een spel, zoals schaken.</rdakit:toolkitDefinition>
      <rdakit:toolkitLabel xml:lang="de">Spielnotation</rdakit:toolkitLabel>
      <rdakit:toolkitDefinition xml:lang="de">Eine Form der Bewegungsnotation, die taktische Bewegungen während eines Spiels wie zum Beispiel Schach aufzeichnet.</rdakit:toolkitDefinition>
      <skos:prefLabel xml:lang="it">Notazione di gioco</skos:prefLabel>
      <rdakit:toolkitLabel xml:lang="it">Notazione di gioco</rdakit:toolkitLabel>
      <skos:prefLabel xml:lang="fi">pelinotaatio</skos:prefLabel>
      <rdakit:toolkitLabel xml:lang="fi">pelinotaatio</rdakit:toolkitLabel>
      <skos:prefLabel xml:lang="sv">spelnotation</skos:prefLabel>
      <rdakit:toolkitLabel xml:lang="sv">spelnotation</rdakit:toolkitLabel>
      <skos:prefLabel xml:lang="vi">ký hiệu chơi trò chơi</skos:prefLabel>
      <rdakit:toolkitLabel xml:lang="vi">ký hiệu chơi trò chơi</rdakit:toolkitLabel>
      <skos:definition xml:lang="vi">Hình thái của động thái ký hiệu để ghi lại vị trí của người chơi hoặc tiến trình của trò chơi.</skos:definition>
      <rdakit:toolkitDefinition xml:lang="vi">Hình thái của động thái ký hiệu để ghi lại vị trí của người chơi hoặc tiến trình của trò chơi.</rdakit:toolkitDefinition>
      <skos:prefLabel xml:lang="da">spillenotation</skos:prefLabel>
      <rdakit:toolkitLabel xml:lang="da">spillenotation</rdakit:toolkitLabel>
      <skos:definition xml:lang="da">Form for bevægelsesnotation, der registrerer taktile bevægelser i løbet af et spil.</skos:definition>
      <rdakit:toolkitDefinition xml:lang="da">Form for bevægelsesnotation, der registrerer taktile bevægelser i løbet af et spil.</rdakit:toolkitDefinition>
      <skos:prefLabel xml:lang="ca">notació de joc</skos:prefLabel>
      <rdakit:toolkitLabel xml:lang="ca">notació de joc</rdakit:toolkitLabel>
      <skos:definition xml:lang="ca">Forma de notació del moviment que enregistra la posició dels jugadors o de les peces en el desenvolupament d’un joc.</skos:definition>
      <rdakit:toolkitDefinition xml:lang="ca">Forma de notació del moviment que enregistra la posició dels jugadors o de les peces en el desenvolupament d’un joc.</rdakit:toolkitDefinition>
      <skos:definition xml:lang="fi">Liikenotaatio pelaajien tai pelinappuloiden asemien tallentamiseksi pelin aikana.</skos:definition>
      <rdakit:toolkitDefinition xml:lang="fi">Liikenotaatio pelaajien tai pelinappuloiden asemien tallentamiseksi pelin aikana.</rdakit:toolkitDefinition>
      <skos:prefLabel xml:lang="no">spillnotasjon</skos:prefLabel>
      <rdakit:toolkitLabel xml:lang="no">spillnotasjon</rdakit:toolkitLabel>
      <skos:definition xml:lang="no">En form for bevegelsesnotasjon for å registrere plasseringen av spillere eller brikker i løpet av spillet.</skos:definition>
      <rdakit:toolkitDefinition xml:lang="no">En form for bevegelsesnotasjon for å registrere plasseringen av spillere eller brikker i løpet av spillet.</rdakit:toolkitDefinition>
    </skos:Concept>
<!-- Concept: Kinetography Laban  -->
    <skos:Concept rdf:about="http://rdaregistry.info/termList/noteMove/1010" xml:lang="en">
      <skos:inScheme rdf:resource="http://rdaregistry.info/termList/noteMove"/>
      <reg:status rdf:resource="http://metadataregistry.org/uri/RegStatus/1001"/>
      <reg:identifier rdf:resource="http://metadataregistry.org/concepts/5924"/>
      <skos:prefLabel xml:lang="en">Kinetography Laban</skos:prefLabel>
      <skos:definition xml:lang="en">A form of notated movement using abstract symbols on a vertical three-line staff to represent movement of the body and limbs as seen from the back, developed in Europe in the middle of the 20th century.</skos:definition>
      <skos:prefLabel xml:lang="de">Kinetography Laban</skos:prefLabel>
      <skos:definition xml:lang="de">Eine Form der Bewegungsnotation, die abstrakte Symbole verwendet, um die Positionen des Körpers und der Gliedmaßen darzustellen, wie sie von hinten zu sehen sind. Sie wird auf vertikalen dreizeiligen Notenlinien erfasst, die den Körper darstellen. Ähnlich wie Labanotation.</skos:definition>
      <skos:prefLabel xml:lang="fr">Cinétographie Laban</skos:prefLabel>
      <skos:definition xml:lang="fr">Forme de notation du mouvement qui utilise des symboles abstraits sur une portée verticale de trois lignes pour représenter les mouvements du corps et des membres vus de dos et qui a été développée en Europe au milieu du 20e siècle.</skos:definition>
      <skos:prefLabel xml:lang="es">Kinetografía Laban</skos:prefLabel>
      <skos:definition xml:lang="es">Forma de movimiento notado que utiliza símbolos abstractos para representar el movimiento del cuerpo y extremidades vistos desde atrás. Se registra en un pentagrama vertical de tres líneas que representa el cuerpo. Similar a la Labanotación.</skos:definition>
      <skos:prefLabel xml:lang="zh">拉班书面舞谱</skos:prefLabel>
      <rdakit:toolkitLabel xml:lang="zh">拉班书面舞谱</rdakit:toolkitLabel>
      <rdakit:toolkitLabel xml:lang="en">Kinetography Laban</rdakit:toolkitLabel>
      <skos:note xml:lang="zh">与拉班舞谱类似。</skos:note>
      <skos:definition xml:lang="zh">一种用抽象的符号表示从背后所看到的身体和四肢运动的动作谱形式。它在垂直的三条谱线上记录身体的表现，与拉班舞谱类似。</skos:definition>
      <rdakit:toolkitDefinition xml:lang="zh">一种用抽象的符号表示从背后所看到的身体和四肢运动的动作谱形式。它在垂直的三条谱线上记录身体的表现，与拉班舞谱类似。</rdakit:toolkitDefinition>
      <rdakit:toolkitDefinition xml:lang="en">A form of notated movement using abstract symbols on a vertical three-line staff to represent movement of the body and limbs as seen from the back, developed in Europe in the middle of the 20th century.</rdakit:toolkitDefinition>
      <skos:scopeNote xml:lang="zh">与拉班舞谱类似。</skos:scopeNote>
      <rdakit:toolkitLabel xml:lang="fr">Cinétographie Laban</rdakit:toolkitLabel>
      <rdakit:toolkitDefinition xml:lang="fr">Forme de notation du mouvement qui utilise des symboles abstraits sur une portée verticale de trois lignes pour représenter les mouvements du corps et des membres vus de dos et qui a été développée en Europe au milieu du 20e siècle.</rdakit:toolkitDefinition>
      <rdakit:toolkitLabel xml:lang="es">Kinetografía Laban</rdakit:toolkitLabel>
      <rdakit:toolkitDefinition xml:lang="es">Forma de movimiento notado que utiliza símbolos abstractos para representar el movimiento del cuerpo y extremidades vistos desde atrás. Se registra en un pentagrama vertical de tres líneas que representa el cuerpo. Similar a la Labanotación.</rdakit:toolkitDefinition>
      <skos:scopeNote xml:lang="en">Kineography Laban is now harmonized with, while remaining distinct from, Labanotation.</skos:scopeNote>
	    <skos:related rdf:resource="http://rdaregistry.info/termList/noteMove/1002"/>
      <skos:prefLabel xml:lang="nl">Kinetography Laban</skos:prefLabel>
      <rdakit:toolkitLabel xml:lang="nl">Kinetography Laban</rdakit:toolkitLabel>
      <skos:definition xml:lang="nl">Een vorm van bewegingsnotatie waarbij abstracte symbolen gebruikt worden om bewegingen voor te stellen van lichaam en ledematen vanaf de rug. Deze is vastgelegd op een verticale balk van drie lijntjes, die het lichaam voorstelt. Vergelijkbaar met Labanotation.</skos:definition>
      <rdakit:toolkitDefinition xml:lang="nl">Een vorm van bewegingsnotatie waarbij abstracte symbolen gebruikt worden om bewegingen voor te stellen van lichaam en ledematen vanaf de rug. Deze is vastgelegd op een verticale balk van drie lijntjes, die het lichaam voorstelt. Vergelijkbaar met Labanotation.</rdakit:toolkitDefinition>
      <rdakit:toolkitLabel xml:lang="de">Kinetography Laban</rdakit:toolkitLabel>
      <rdakit:toolkitDefinition xml:lang="de">Eine Form der Bewegungsnotation, die abstrakte Symbole verwendet, um die Positionen des Körpers und der Gliedmaßen darzustellen, wie sie von hinten zu sehen sind. Sie wird auf vertikalen dreizeiligen Notenlinien erfasst, die den Körper darstellen. Ähnlich wie Labanotation.</rdakit:toolkitDefinition>
      <skos:prefLabel xml:lang="it">Cinetografia Laban</skos:prefLabel>
      <rdakit:toolkitLabel xml:lang="it">Cinetografia Laban</rdakit:toolkitLabel>
      <skos:prefLabel xml:lang="fi">Kinetography Laban -notaatio</skos:prefLabel>
      <rdakit:toolkitLabel xml:lang="fi">Kinetography Laban -notaatio</rdakit:toolkitLabel>
      <skos:scopeNote xml:lang="de">Kinetografie Laban ist nun der Labanotation angeglichen, bleibt jedoch unterscheidbar.</skos:scopeNote>
      <skos:prefLabel xml:lang="vi">Kinetography laban</skos:prefLabel>
      <rdakit:toolkitLabel xml:lang="vi">Kinetography laban</rdakit:toolkitLabel>
      <skos:definition xml:lang="vi">Hình tháicủađộng thái ký hiệusử dụngký hiệutrừu tượngtrên khuông nhạc dọc ba đườngđểbiểu diễn chuyển độngcủa cơ thể và chân tay khi nhìn từ phía sau, được phát triển ở Hoa Kỳ và Vương quốc Anh vào giữa thế kỷ 20.</skos:definition>
      <rdakit:toolkitDefinition xml:lang="vi">Hình tháicủađộng thái ký hiệusử dụngký hiệutrừu tượngtrên khuông nhạc dọc ba đườngđểbiểu diễn chuyển độngcủa cơ thể và chân tay khi nhìn từ phía sau, được phát triển ở Hoa Kỳ và Vương quốc Anh vào giữa thế kỷ 20.</rdakit:toolkitDefinition>
      <skos:scopeNote xml:lang="vi">Kinetography Laban hiện nay được hài hoà với, trong khi vẫn giữ khác biệt với, Labanotation.</skos:scopeNote>
      <skos:prefLabel xml:lang="da">Kinetography Laban</skos:prefLabel>
      <rdakit:toolkitLabel xml:lang="da">Kinetography Laban</rdakit:toolkitLabel>
      <skos:definition xml:lang="da">Bevægelsesnotationsform, der anvender abstrakte symboler til at repræsentere en krops og lemmers bevægelser set bagfra, udviklet i Europa i midten af 1900-talet.</skos:definition>
      <rdakit:toolkitDefinition xml:lang="da">Bevægelsesnotationsform, der anvender abstrakte symboler til at repræsentere en krops og lemmers bevægelser set bagfra, udviklet i Europa i midten af 1900-talet.</rdakit:toolkitDefinition>
      <skos:scopeNote xml:lang="da">Kinetography Laban er nu harmoniseret med, imens den bliver distinkt fra, Labanotation.</skos:scopeNote>
      <skos:prefLabel xml:lang="ca">cinetografia Laban</skos:prefLabel>
      <rdakit:toolkitLabel xml:lang="ca">cinetografia Laban</rdakit:toolkitLabel>
      <skos:definition xml:lang="ca">Forma de notació del moviment que usa símbols abstractes en un pentagrama vertical de tres línies per representar el moviment del cos i les extremitats vistos des del darrere, desenvolupada a Europa a mitjans del segle XX.</skos:definition>
      <rdakit:toolkitDefinition xml:lang="ca">Forma de notació del moviment que usa símbols abstractes en un pentagrama vertical de tres línies per representar el moviment del cos i les extremitats vistos des del darrere, desenvolupada a Europa a mitjans del segle XX.</rdakit:toolkitDefinition>
      <skos:scopeNote xml:lang="ca">La cinetografia Laban actualment està harmonitzada amb la notació Laban, encara que continua sent diferent.</skos:scopeNote>
      <skos:definition xml:lang="fi">Tanssinotaatio, jossa abstrakteilla symboleilla merkitään pystysuoralle kolmiriviselle viivastolle kehon ja raajojen liikkeitä takaapäin nähtynä. Kehitetty Euroopassa 1900-luvun keskivaiheilla.</skos:definition>
      <rdakit:toolkitDefinition xml:lang="fi">Tanssinotaatio, jossa abstrakteilla symboleilla merkitään pystysuoralle kolmiriviselle viivastolle kehon ja raajojen liikkeitä takaapäin nähtynä. Kehitetty Euroopassa 1900-luvun keskivaiheilla.</rdakit:toolkitDefinition>
      <skos:scopeNote xml:lang="fi">Kineography Laban-notaatio on harmonisoitu Laban -notaation kanssa, joskin on erillinen siitä.</skos:scopeNote>
      <skos:scopeNote xml:lang="fr">La Cinétographie Laban est maintenant harmonisée avec la Labanotation dont elle demeure cependant distincte.</skos:scopeNote>
      <skos:prefLabel xml:lang="no">Kinetografi Laban</skos:prefLabel>
      <rdakit:toolkitLabel xml:lang="no">Kinetografi Laban</rdakit:toolkitLabel>
      <skos:definition xml:lang="no">En form for bevegelsesnotasjon som bruker abstrakte symboler på en stav med tre linjer for å representere kroppens og lemmenes bevegelse sett bakfra. Utviklet i Europa på midten av 1900-tallet.</skos:definition>
      <rdakit:toolkitDefinition xml:lang="no">En form for bevegelsesnotasjon som bruker abstrakte symboler på en stav med tre linjer for å representere kroppens og lemmenes bevegelse sett bakfra. Utviklet i Europa på midten av 1900-tallet.</rdakit:toolkitDefinition>
      <skos:scopeNote xml:lang="no">Kinetografi Laban er nå harmonisert med, men adskilt fra, Labanotasjon.</skos:scopeNote>
    </skos:Concept>
<!-- Concept: Labanotation  -->
    <skos:Concept rdf:about="http://rdaregistry.info/termList/noteMove/1002" xml:lang="en">
      <skos:inScheme rdf:resource="http://rdaregistry.info/termList/noteMove"/>
      <reg:status rdf:resource="http://metadataregistry.org/uri/RegStatus/1001"/>
      <reg:identifier rdf:resource="http://metadataregistry.org/concepts/1028"/>
      <skos:prefLabel xml:lang="en">Labanotation</skos:prefLabel>
      <skos:definition xml:lang="en">A form of notated movement using abstract symbols on a vertical three-line staff to represent movement of the body and limbs as seen from the back, developed in the United States and the United Kingdom in the middle of the 20th century.</skos:definition>
      <skos:prefLabel xml:lang="de">Labanotation</skos:prefLabel>
      <skos:definition xml:lang="de">Eine Form der Bewegungsnotation, die abstrakte Symbole verwendet, um die Positionen des Körpers und der Gliedmaßen darzustellen, wie sie von hinten zu sehen sind. Sie wird auf vertikalen dreizeiligen Notenlinien erfasst, die den Körper darstellen. Ähnlich wie Kinetografie Laban.</skos:definition>
      <skos:prefLabel xml:lang="fr">Labanotation</skos:prefLabel>
      <skos:definition xml:lang="fr">Forme de notation du mouvement qui utilise des symboles abstraits sur une portée verticale de trois lignes pour représenter les mouvements du corps et des membres vus de dos et qui a été développée aux États-Unis et au Royaume-Uni au milieu du 20e siècle.</skos:definition>
      <skos:prefLabel xml:lang="es">Labanotación</skos:prefLabel>
      <skos:definition xml:lang="es">Forma de movimiento notado que utiliza símbolos abstractos para representar el movimiento del cuerpo y extremidades vistos desde atrás. Se registra en un pentagrama vertical de tres líneas que representa el cuerpo. Similar a la Kinetografía Laban.</skos:definition>
      <skos:prefLabel xml:lang="zh">拉班舞谱</skos:prefLabel>
      <rdakit:toolkitLabel xml:lang="zh">拉班舞谱</rdakit:toolkitLabel>
      <rdakit:toolkitLabel xml:lang="en">Labanotation</rdakit:toolkitLabel>
      <skos:note xml:lang="zh">与拉班书面舞谱类似。</skos:note>
      <skos:definition xml:lang="zh">一种用抽象的符号表示从背后所看到的身体和四肢运动的动作谱形式。它在垂直的三条谱线上记录身体的表现，与拉班书面舞谱类似。</skos:definition>
      <rdakit:toolkitDefinition xml:lang="zh">一种用抽象的符号表示从背后所看到的身体和四肢运动的动作谱形式。它在垂直的三条谱线上记录身体的表现，与拉班书面舞谱类似。</rdakit:toolkitDefinition>
      <rdakit:toolkitDefinition xml:lang="en">A form of notated movement using abstract symbols on a vertical three-line staff to represent movement of the body and limbs as seen from the back, developed in the United States and the United Kingdom in the middle of the 20th century.</rdakit:toolkitDefinition>
      <skos:scopeNote xml:lang="zh">与拉班书面舞谱类似。</skos:scopeNote>
      <rdakit:toolkitLabel xml:lang="fr">Labanotation</rdakit:toolkitLabel>
      <rdakit:toolkitDefinition xml:lang="fr">Forme de notation du mouvement qui utilise des symboles abstraits sur une portée verticale de trois lignes pour représenter les mouvements du corps et des membres vus de dos et qui a été développée aux États-Unis et au Royaume-Uni au milieu du 20e siècle.</rdakit:toolkitDefinition>
      <rdakit:toolkitLabel xml:lang="es">Labanotación</rdakit:toolkitLabel>
      <rdakit:toolkitDefinition xml:lang="es">Forma de movimiento notado que utiliza símbolos abstractos para representar el movimiento del cuerpo y extremidades vistos desde atrás. Se registra en un pentagrama vertical de tres líneas que representa el cuerpo. Similar a la Kinetografía Laban.</rdakit:toolkitDefinition>
      <skos:scopeNote xml:lang="en">Labanotation is now harmonized with, while remaining distinct from, Kineography Laban.</skos:scopeNote>
	    <skos:related rdf:resource="http://rdaregistry.info/termList/noteMove/1010"/>
      <skos:prefLabel xml:lang="nl">Labannotatie</skos:prefLabel>
      <skos:altLabel xml:lang="nl">Labanotatie</skos:altLabel>
      <rdakit:toolkitLabel xml:lang="nl">Labannotatie</rdakit:toolkitLabel>
      <skos:definition xml:lang="nl">Een vorm van bewegingsnotatie waarbij abstracte symbolen gebruikt worden om beweging voor te stellen van lichaam en ledematen gezien vanaf de rug. Deze is vastgelegd op een verticale balk van drie lijntjes, die het lichaam voorstelt. Gebaseerd op Kinetography Laban.</skos:definition>
      <rdakit:toolkitDefinition xml:lang="nl">Een vorm van bewegingsnotatie waarbij abstracte symbolen gebruikt worden om beweging voor te stellen van lichaam en ledematen gezien vanaf de rug. Deze is vastgelegd op een verticale balk van drie lijntjes, die het lichaam voorstelt. Gebaseerd op Kinetography Laban.</rdakit:toolkitDefinition>
      <rdakit:toolkitLabel xml:lang="de">Labanotation</rdakit:toolkitLabel>
      <rdakit:toolkitDefinition xml:lang="de">Eine Form der Bewegungsnotation, die abstrakte Symbole verwendet, um die Positionen des Körpers und der Gliedmaßen darzustellen, wie sie von hinten zu sehen sind. Sie wird auf vertikalen dreizeiligen Notenlinien erfasst, die den Körper darstellen. Ähnlich wie Kinetografie Laban.</rdakit:toolkitDefinition>
      <skos:prefLabel xml:lang="it">Notazione Laban</skos:prefLabel>
      <rdakit:toolkitLabel xml:lang="it">Notazione Laban</rdakit:toolkitLabel>
      <skos:prefLabel xml:lang="fi">Laban-notaatio</skos:prefLabel>
      <rdakit:toolkitLabel xml:lang="fi">Laban-notaatio</rdakit:toolkitLabel>
      <skos:prefLabel xml:lang="sv">labanotation</skos:prefLabel>
      <rdakit:toolkitLabel xml:lang="sv">labanotation</rdakit:toolkitLabel>
      <skos:scopeNote xml:lang="de">Labanotation ist nun der Kinetografie Laban angegelichen, bleibt jedoch unterscheidbar.</skos:scopeNote>
      <skos:prefLabel xml:lang="vi">Labanotation</skos:prefLabel>
      <rdakit:toolkitLabel xml:lang="vi">Labanotation</rdakit:toolkitLabel>
      <skos:definition xml:lang="vi">Hình tháicủađộng thái ký hiệusử dụngký hiệutrừu tượngtrên khuông nhạc dọc ba đườngđểbiểu diễn chuyển độngcủa cơ thể và chân tay khi nhìn từ phía sau, được phát triển ở Hoa Kỳ và Vương quốc Anh vào giữa thế kỷ 20.</skos:definition>
      <rdakit:toolkitDefinition xml:lang="vi">Hình tháicủađộng thái ký hiệusử dụngký hiệutrừu tượngtrên khuông nhạc dọc ba đườngđểbiểu diễn chuyển độngcủa cơ thể và chân tay khi nhìn từ phía sau, được phát triển ở Hoa Kỳ và Vương quốc Anh vào giữa thế kỷ 20.</rdakit:toolkitDefinition>
      <skos:scopeNote xml:lang="vi">Labanotation hiện nay được hài hoà với, trong khi vẫn giữ khác biệt với, Kinetography Laban</skos:scopeNote>
      <skos:prefLabel xml:lang="da">labanotation</skos:prefLabel>
      <rdakit:toolkitLabel xml:lang="da">labanotation</rdakit:toolkitLabel>
      <skos:definition xml:lang="da">Bevægelsesnotationsform, der anvender abstrakte symboler til at repræsentere en krops og lemmers bevægelser set bagfra, udviklet i USA og Storbritannien i midten af 1900-talet.</skos:definition>
      <rdakit:toolkitDefinition xml:lang="da">Bevægelsesnotationsform, der anvender abstrakte symboler til at repræsentere en krops og lemmers bevægelser set bagfra, udviklet i USA og Storbritannien i midten af 1900-talet.</rdakit:toolkitDefinition>
      <skos:scopeNote xml:lang="da">Labanotation er nu harmoniseret med, imens den bliver distinkt fra, Kinetography Laban.</skos:scopeNote>
      <skos:prefLabel xml:lang="ca">notació Laban</skos:prefLabel>
      <rdakit:toolkitLabel xml:lang="ca">notació Laban</rdakit:toolkitLabel>
      <skos:definition xml:lang="ca">Forma de notació del moviment que usa símbols abstractes en un pentagrama vertical de tres línies per representar el moviment del cos i les extremitats vistos des del darrere, desenvolupada als Estats Units i al Regne Unit a mitjans del segle XX.</skos:definition>
      <rdakit:toolkitDefinition xml:lang="ca">Forma de notació del moviment que usa símbols abstractes en un pentagrama vertical de tres línies per representar el moviment del cos i les extremitats vistos des del darrere, desenvolupada als Estats Units i al Regne Unit a mitjans del segle XX.</rdakit:toolkitDefinition>
      <skos:scopeNote xml:lang="ca">La notació Laban actualment està harmonitzada amb la cinetografia Laban, encara que continua sent diferent.</skos:scopeNote>
      <skos:definition xml:lang="fi">Tanssinotaatio, jossa abstrakteilla symboleilla esitetään kehon ja raajojen asentoja takaapäin nähtynä. Notaatio merkitään pystysuoralle kolmiriviselle viivastolle. Kehitetty Yhdysvalloissa ja Iso-Britanniassa 1900-luvun keskivaiheilla.</skos:definition>
      <rdakit:toolkitDefinition xml:lang="fi">Tanssinotaatio, jossa abstrakteilla symboleilla esitetään kehon ja raajojen asentoja takaapäin nähtynä. Notaatio merkitään pystysuoralle kolmiriviselle viivastolle. Kehitetty Yhdysvalloissa ja Iso-Britanniassa 1900-luvun keskivaiheilla.</rdakit:toolkitDefinition>
      <skos:scopeNote xml:lang="fi">Laban-notaatio on harmonisoitu Kineography Laban -notaation kanssa, joskin on erillinen siitä.</skos:scopeNote>
      <skos:scopeNote xml:lang="fr">La Labanotation est maintenant harmonisée avec la Cinétographie Laban dont elle demeure cependant distincte.</skos:scopeNote>
      <skos:prefLabel xml:lang="no">Labanotasjon</skos:prefLabel>
      <rdakit:toolkitLabel xml:lang="no">Labanotasjon</rdakit:toolkitLabel>
      <skos:definition xml:lang="no">En form for bevegelsesnotasjon som bruker abstrakte symboler på en stav med tre linjer for å representere kroppens og lemmenes bevegelse sett bakfra. Utviklet i USA og Storbritannia på midten av 1900-tallet.</skos:definition>
      <rdakit:toolkitDefinition xml:lang="no">En form for bevegelsesnotasjon som bruker abstrakte symboler på en stav med tre linjer for å representere kroppens og lemmenes bevegelse sett bakfra. Utviklet i USA og Storbritannia på midten av 1900-tallet.</rdakit:toolkitDefinition>
      <skos:scopeNote xml:lang="no">Labanotasjon er nå harmonisert med, men adskilt fra, Kinetografi Laban.</skos:scopeNote>
    </skos:Concept>
<!-- Concept: Stepanov dance notation  -->
    <skos:Concept rdf:about="http://rdaregistry.info/termList/noteMove/1001" xml:lang="en">
      <skos:inScheme rdf:resource="http://rdaregistry.info/termList/noteMove"/>
      <reg:status rdf:resource="http://metadataregistry.org/uri/RegStatus/1001"/>
      <reg:identifier rdf:resource="http://metadataregistry.org/concepts/1027"/>
      <skos:prefLabel xml:lang="en">Stepanov dance notation</skos:prefLabel>
      <skos:definition xml:lang="en">A form of notated movement for dance using musical notation to represent movements by single parts of the body.</skos:definition>
      <skos:prefLabel xml:lang="de">Notation nach Stepanov</skos:prefLabel>
      <skos:definition xml:lang="de">Eine Form der Bewegungsnotation für Tanz, die Musiknoten verwendet, um die Bewegungen der einzelnen Teile des Körpers darzustellen. Sie wird auf horizontalen neunzeiligen Notenlinien erfasst, die den Körper darstellen.</skos:definition>
      <skos:prefLabel xml:lang="fr">notation Stepanov</skos:prefLabel>
      <skos:definition xml:lang="fr">Forme de notation du mouvement pour la danse qui utilise la notation musicale pour représenter les mouvements des parties individuelles du corps.</skos:definition>
      <skos:prefLabel xml:lang="es">notación Stepanov para danza</skos:prefLabel>
      <skos:definition xml:lang="es">Forma de movimiento notado para danza que utiliza notación musical para representar movimientos de partes individuales del cuerpo. Es registrado en un pentagrama horizontal de nueve líneas que representa el cuerpo.</skos:definition>
      <skos:prefLabel xml:lang="zh">斯捷潘诺夫舞谱</skos:prefLabel>
      <rdakit:toolkitLabel xml:lang="zh">斯捷潘诺夫舞谱</rdakit:toolkitLabel>
      <rdakit:toolkitLabel xml:lang="en">Stepanov dance notation</rdakit:toolkitLabel>
      <skos:definition xml:lang="zh">一种用乐谱表示身体各部分运动的动作谱形式。它在水平方向的九条谱线上记录身体的表现。</skos:definition>
      <rdakit:toolkitDefinition xml:lang="zh">一种用乐谱表示身体各部分运动的动作谱形式。它在水平方向的九条谱线上记录身体的表现。</rdakit:toolkitDefinition>
      <rdakit:toolkitDefinition xml:lang="en">A form of notated movement for dance using musical notation to represent movements by single parts of the body.</rdakit:toolkitDefinition>
      <rdakit:toolkitLabel xml:lang="fr">notation Stepanov</rdakit:toolkitLabel>
      <rdakit:toolkitDefinition xml:lang="fr">Forme de notation du mouvement pour la danse qui utilise la notation musicale pour représenter les mouvements des parties individuelles du corps.</rdakit:toolkitDefinition>
      <rdakit:toolkitLabel xml:lang="es">notación Stepanov para danza</rdakit:toolkitLabel>
      <rdakit:toolkitDefinition xml:lang="es">Forma de movimiento notado para danza que utiliza notación musical para representar movimientos de partes individuales del cuerpo. Es registrado en un pentagrama horizontal de nueve líneas que representa el cuerpo.</rdakit:toolkitDefinition>
      <skos:scopeNote xml:lang="en">It is recorded on a horizontal nine-line staff that represents the body.</skos:scopeNote>
      <skos:prefLabel xml:lang="nl">Stepanov dansnotatie</skos:prefLabel>
      <rdakit:toolkitLabel xml:lang="nl">Stepanov dansnotatie</rdakit:toolkitLabel>
      <skos:definition xml:lang="nl">Een vorm van bewegingsnotatie voor dans waarbij muzieknotatie gebruikt wordt om bewegingen voor te stellen per lichaamsdeel. Deze is vastgelegd op een horizontale balk van negen lijntjes, die het lichaam voorstelt.</skos:definition>
      <rdakit:toolkitDefinition xml:lang="nl">Een vorm van bewegingsnotatie voor dans waarbij muzieknotatie gebruikt wordt om bewegingen voor te stellen per lichaamsdeel. Deze is vastgelegd op een horizontale balk van negen lijntjes, die het lichaam voorstelt.</rdakit:toolkitDefinition>
      <rdakit:toolkitLabel xml:lang="de">Notation nach Stepanov</rdakit:toolkitLabel>
      <rdakit:toolkitDefinition xml:lang="de">Eine Form der Bewegungsnotation für Tanz, die Musiknoten verwendet, um die Bewegungen der einzelnen Teile des Körpers darzustellen. Sie wird auf horizontalen neunzeiligen Notenlinien erfasst, die den Körper darstellen.</rdakit:toolkitDefinition>
      <skos:prefLabel xml:lang="it">Notazione coreografica Stepanov</skos:prefLabel>
      <rdakit:toolkitLabel xml:lang="it">Notazione coreografica Stepanov</rdakit:toolkitLabel>
      <skos:prefLabel xml:lang="fi">Stepanov-tanssinotaatio</skos:prefLabel>
      <rdakit:toolkitLabel xml:lang="fi">Stepanov-tanssinotaatio</rdakit:toolkitLabel>
      <skos:scopeNote xml:lang="de">Sie wird auf horizontalen neunzeiligen Notenlinien erfasst, die den Körper darstellen.</skos:scopeNote>
      <skos:prefLabel xml:lang="vi">ký hiệu điệu nhẩy Stepanov</skos:prefLabel>
      <rdakit:toolkitLabel xml:lang="vi">ký hiệu điệu nhẩy Stepanov</rdakit:toolkitLabel>
      <skos:definition xml:lang="vi">Hình thái của động thái ký hiệucho điệu nhảyđược ghisử dụng ký hiệu âm nhạcbiểu diễncác bộ phậnđơn lẻcủa cơ thể.</skos:definition>
      <rdakit:toolkitDefinition xml:lang="vi">Hình thái của động thái ký hiệucho điệu nhảyđược ghisử dụng ký hiệu âm nhạcbiểu diễncác bộ phậnđơn lẻcủa cơ thể.</rdakit:toolkitDefinition>
      <skos:scopeNote xml:lang="vi">Nó được ghi lại trênkhuông nhạcchín đường nằm ngangbiểu diễncơ thể.</skos:scopeNote>
      <skos:prefLabel xml:lang="da">Stepanov-dansenotation</skos:prefLabel>
      <rdakit:toolkitLabel xml:lang="da">Stepanov-dansenotation</rdakit:toolkitLabel>
      <skos:definition xml:lang="da">Form for bevægelsesnotation der anvender musiknotation til at repræsentere bevægelser for kroppens forskellige dele.</skos:definition>
      <rdakit:toolkitDefinition xml:lang="da">Form for bevægelsesnotation der anvender musiknotation til at repræsentere bevægelser for kroppens forskellige dele.</rdakit:toolkitDefinition>
      <skos:scopeNote xml:lang="da">Registreres i et ni-linjet vandret nodesystem, der repræsenterer kroppen.</skos:scopeNote>
      <skos:prefLabel xml:lang="ca">notació Stepanov</skos:prefLabel>
      <rdakit:toolkitLabel xml:lang="ca">notació Stepanov</rdakit:toolkitLabel>
      <skos:definition xml:lang="ca">Forma de notació del moviment per a la dansa que usa la notació musical per representar els moviments de les parts individuals del cos.</skos:definition>
      <rdakit:toolkitDefinition xml:lang="ca">Forma de notació del moviment per a la dansa que usa la notació musical per representar els moviments de les parts individuals del cos.</rdakit:toolkitDefinition>
      <skos:scopeNote xml:lang="ca">S’enregistra en un pentagrama horitzontal de nou línies que representa el cos.</skos:scopeNote>
      <skos:definition xml:lang="fi">Tanssinotaatio, jossa musiikkinotaatiota käytetään esittämään kehon yksittäisten osien liikettä.</skos:definition>
      <rdakit:toolkitDefinition xml:lang="fi">Tanssinotaatio, jossa musiikkinotaatiota käytetään esittämään kehon yksittäisten osien liikettä.</rdakit:toolkitDefinition>
      <skos:scopeNote xml:lang="fi">Notaatio merkitään yhdeksänriviselle vaakasuoralle viivastolle.</skos:scopeNote>
      <skos:scopeNote xml:lang="fr">Cette notation utilise une portée horizontale de neuf lignes qui représente le corps.</skos:scopeNote>
      <skos:prefLabel xml:lang="no">Stepanov-dansenotasjon</skos:prefLabel>
      <rdakit:toolkitLabel xml:lang="no">Stepanov-dansenotasjon</rdakit:toolkitLabel>
      <skos:definition xml:lang="no">En form for bevegelsesnotasjon for dans som bruker musikalsk notasjon for å representere de enkelte kroppsdelenes bevegelser.</skos:definition>
      <rdakit:toolkitDefinition xml:lang="no">En form for bevegelsesnotasjon for dans som bruker musikalsk notasjon for å representere de enkelte kroppsdelenes bevegelser.</rdakit:toolkitDefinition>
      <skos:scopeNote xml:lang="no">Dette registreres på en vannrett stav med ni linjer som representerer kroppen.</skos:scopeNote>
    </skos:Concept>

<!-- Status properties used in this document  -->
    <skos:Concept rdf:about="http://metadataregistry.org/uri/RegStatus/1001">
        <skos:prefLabel xml:lang="en">Published</skos:prefLabel>
    </skos:Concept>

</rdf:RDF>
