<?xml version="1.0" encoding = "UTF-8"?>
<rdf:RDF
    xmlns:dc="http://purl.org/dc/elements/1.1/"
    xmlns:rdakit="http://metadataregistry.org/uri/profile/rdakit/"
    xmlns:rdf="http://www.w3.org/1999/02/22-rdf-syntax-ns#"
    xmlns:reg="http://metadataregistry.org/uri/profile/regap/"
    xmlns:owl="http://www.w3.org/2002/07/owl#"
    xmlns:skos="http://www.w3.org/2004/02/skos/core#">

<owl:Ontology rdf:about="http://rdaregistry.info/termList/presFormat" />
<!-- Scheme: RDA Presentation Format -->
    <skos:ConceptScheme rdf:about="http://rdaregistry.info/termList/presFormat">
        <dc:title>RDA Presentation Format</dc:title>
    </skos:ConceptScheme>

<!-- Concept: 3D  -->
    <skos:Concept rdf:about="http://rdaregistry.info/termList/presFormat/1012" xml:lang="en">
      <skos:inScheme rdf:resource="http://rdaregistry.info/termList/presFormat"/>
      <reg:status rdf:resource="http://metadataregistry.org/uri/RegStatus/1001"/>
      <reg:identifier rdf:resource="http://metadataregistry.org/concepts/898"/>
      <skos:prefLabel xml:lang="en">3D</skos:prefLabel>
      <rdakit:toolkitLabel xml:lang="en">3D</rdakit:toolkitLabel>
      <skos:definition xml:lang="en">A presentation format of a motion picture film that gives the illusion of three dimensions.</skos:definition>
      <rdakit:toolkitDefinition xml:lang="en">A presentation format of a motion picture film that gives the illusion of three dimensions.</rdakit:toolkitDefinition>
      <skos:prefLabel xml:lang="de">3D</skos:prefLabel>
      <rdakit:toolkitLabel xml:lang="de">3D</rdakit:toolkitLabel>
      <skos:definition xml:lang="de">Ein Wiedergabeformat eines Films, das die Illusion von drei Dimensionen vermittelt.</skos:definition>
      <rdakit:toolkitDefinition xml:lang="de">Ein Wiedergabeformat eines Films, das die Illusion von drei Dimensionen vermittelt.</rdakit:toolkitDefinition>
      <skos:prefLabel xml:lang="fi">3D</skos:prefLabel>
      <rdakit:toolkitLabel xml:lang="fi">3D</rdakit:toolkitLabel>
      <skos:definition xml:lang="fi">Elokuvafilmin esitysformaatti, joka luo kolmiulotteisuuden vaikutelman.</skos:definition>
      <rdakit:toolkitDefinition xml:lang="fi">Elokuvafilmin esitysformaatti, joka luo kolmiulotteisuuden vaikutelman.</rdakit:toolkitDefinition>
      <skos:prefLabel xml:lang="da">3D</skos:prefLabel>
      <rdakit:toolkitLabel xml:lang="da">3D</rdakit:toolkitLabel>
      <skos:definition xml:lang="da">Præsentationsformat til film, der giver illusionen af tre dimensioner.</skos:definition>
      <rdakit:toolkitDefinition xml:lang="da">Præsentationsformat til film, der giver illusionen af tre dimensioner.</rdakit:toolkitDefinition>
      <skos:prefLabel xml:lang="ca">3D</skos:prefLabel>
      <rdakit:toolkitLabel xml:lang="ca">3D</rdakit:toolkitLabel>
      <skos:definition xml:lang="ca">Format de presentació d'una pel·lícula cinematogràfica que dóna la il·lusió de tres dimensions.</skos:definition>
      <rdakit:toolkitDefinition xml:lang="ca">Format de presentació d'una pel·lícula cinematogràfica que dóna la il·lusió de tres dimensions.</rdakit:toolkitDefinition>
      <skos:prefLabel xml:lang="vi">3D</skos:prefLabel>
      <rdakit:toolkitLabel xml:lang="vi">3D</rdakit:toolkitLabel>
      <skos:definition xml:lang="vi">Định dạng trình bày của phim điện ảnh tạo ảo giác ba chiều.</skos:definition>
      <rdakit:toolkitDefinition xml:lang="vi">Định dạng trình bày của phim điện ảnh tạo ảo giác ba chiều.</rdakit:toolkitDefinition>
      <skos:prefLabel xml:lang="fr">3D</skos:prefLabel>
      <rdakit:toolkitLabel xml:lang="fr">3D</rdakit:toolkitLabel>
      <skos:definition xml:lang="fr">Format de projection d’un film cinématographique qui donne l’illusion des trois dimensions.</skos:definition>
      <rdakit:toolkitDefinition xml:lang="fr">Format de projection d’un film cinématographique qui donne l’illusion des trois dimensions.</rdakit:toolkitDefinition>
    </skos:Concept>
<!-- Concept: Cinemiracle  -->
    <skos:Concept rdf:about="http://rdaregistry.info/termList/presFormat/1002" xml:lang="en">
      <skos:inScheme rdf:resource="http://rdaregistry.info/termList/presFormat"/>
      <reg:status rdf:resource="http://metadataregistry.org/uri/RegStatus/1001"/>
      <reg:identifier rdf:resource="http://metadataregistry.org/concepts/888"/>
      <skos:prefLabel xml:lang="en">Cinemiracle</skos:prefLabel>
      <rdakit:toolkitLabel xml:lang="en">Cinemiracle</rdakit:toolkitLabel>
      <skos:definition xml:lang="en">A presentation format of a motion picture film that presents an aspect ratio of 2.59:1 using three synchronized projectors.</skos:definition>
      <rdakit:toolkitDefinition xml:lang="en">A presentation format of a motion picture film that presents an aspect ratio of 2.59:1 using three synchronized projectors.</rdakit:toolkitDefinition>
      <skos:prefLabel xml:lang="de">Cinemiracle</skos:prefLabel>
      <rdakit:toolkitLabel xml:lang="de">Cinemiracle</rdakit:toolkitLabel>
      <skos:definition xml:lang="de">Ein Wiedergabeformat eines Films, das ein Bildformat von 2.59:1 darstellt, für das drei synchron laufende Projektoren verwendet werden.</skos:definition>
      <rdakit:toolkitDefinition xml:lang="de">Ein Wiedergabeformat eines Films, das ein Bildformat von 2.59:1 darstellt, für das drei synchron laufende Projektoren verwendet werden.</rdakit:toolkitDefinition>
      <skos:prefLabel xml:lang="fi">Cinemiracle</skos:prefLabel>
      <rdakit:toolkitLabel xml:lang="fi">Cinemiracle</rdakit:toolkitLabel>
      <skos:definition xml:lang="fi">Elokuvafilmin esitysformaatti, jonka kuvasuhde on 2.59:1 ja joka käyttää kolmea synkronoitua projektoria.</skos:definition>
      <rdakit:toolkitDefinition xml:lang="fi">Elokuvafilmin esitysformaatti, jonka kuvasuhde on 2.59:1 ja joka käyttää kolmea synkronoitua projektoria.</rdakit:toolkitDefinition>
      <skos:prefLabel xml:lang="da">Cinemiracle</skos:prefLabel>
      <rdakit:toolkitLabel xml:lang="da">Cinemiracle</rdakit:toolkitLabel>
      <skos:definition xml:lang="da">Præsentationsformat til film, som har et billedformat på op til 2.59:1, og som oprindelig anvendte tre synkroniserede projektorer.</skos:definition>
      <rdakit:toolkitDefinition xml:lang="da">Præsentationsformat til film, som har et billedformat på op til 2.59:1, og som oprindelig anvendte tre synkroniserede projektorer.</rdakit:toolkitDefinition>
      <skos:prefLabel xml:lang="ca">Cinemiracle</skos:prefLabel>
      <rdakit:toolkitLabel xml:lang="ca">Cinemiracle</rdakit:toolkitLabel>
      <skos:definition xml:lang="ca">Format de presentació d'una pel·lícula cinematogràfica que presenta una relació d'aspecte de 2,59:1 que usa tres projectors sincronitzats.</skos:definition>
      <rdakit:toolkitDefinition xml:lang="ca">Format de presentació d'una pel·lícula cinematogràfica que presenta una relació d'aspecte de 2,59:1 que usa tres projectors sincronitzats.</rdakit:toolkitDefinition>
      <skos:prefLabel xml:lang="vi">màn ảnh khá rộng</skos:prefLabel>
      <rdakit:toolkitLabel xml:lang="vi">màn ảnh khá rộng</rdakit:toolkitLabel>
      <skos:definition xml:lang="vi">Định dạng trình bày của phim điện ảnh trình bày tỷ lệ bề ngoài lên tới 2,59:1, sử dụng nguyên gốc ba máy chiếu đồng bộ.</skos:definition>
      <rdakit:toolkitDefinition xml:lang="vi">Định dạng trình bày của phim điện ảnh trình bày tỷ lệ bề ngoài lên tới 2,59:1, sử dụng nguyên gốc ba máy chiếu đồng bộ.</rdakit:toolkitDefinition>
      <skos:prefLabel xml:lang="fr">Cinémiracle</skos:prefLabel>
      <rdakit:toolkitLabel xml:lang="fr">Cinémiracle</rdakit:toolkitLabel>
      <skos:definition xml:lang="fr">Format de projection d’un film cinématographique qui produit un format d’image de 2,59:1 au moyen de trois projecteurs synchronisés.</skos:definition>
      <rdakit:toolkitDefinition xml:lang="fr">Format de projection d’un film cinématographique qui produit un format d’image de 2,59:1 au moyen de trois projecteurs synchronisés.</rdakit:toolkitDefinition>
    </skos:Concept>
<!-- Concept: Cinerama  -->
    <skos:Concept rdf:about="http://rdaregistry.info/termList/presFormat/1001" xml:lang="en">
      <skos:inScheme rdf:resource="http://rdaregistry.info/termList/presFormat"/>
      <reg:status rdf:resource="http://metadataregistry.org/uri/RegStatus/1001"/>
      <reg:identifier rdf:resource="http://metadataregistry.org/concepts/887"/>
      <skos:prefLabel xml:lang="en">Cinerama</skos:prefLabel>
      <rdakit:toolkitLabel xml:lang="en">Cinerama</rdakit:toolkitLabel>
      <skos:definition xml:lang="en">A presentation format of a motion picture film that presents an aspect ratio of up to 2.76:1, originally using three synchronized projectors.</skos:definition>
      <rdakit:toolkitDefinition xml:lang="en">A presentation format of a motion picture film that presents an aspect ratio of up to 2.76:1, originally using three synchronized projectors.</rdakit:toolkitDefinition>
      <skos:prefLabel xml:lang="de">Cinerama</skos:prefLabel>
      <rdakit:toolkitLabel xml:lang="de">Cinerama</rdakit:toolkitLabel>
      <skos:definition xml:lang="de">Ein Wiedergabeformat eines Films, das ein Bildformat von bis zu 2,76:1 darstellt, für das eigentlich drei synchron laufende Projektoren verwendet werden.</skos:definition>
      <rdakit:toolkitDefinition xml:lang="de">Ein Wiedergabeformat eines Films, das ein Bildformat von bis zu 2,76:1 darstellt, für das eigentlich drei synchron laufende Projektoren verwendet werden.</rdakit:toolkitDefinition>
      <skos:prefLabel xml:lang="fi">Cinerama</skos:prefLabel>
      <rdakit:toolkitLabel xml:lang="fi">Cinerama</rdakit:toolkitLabel>
      <skos:definition xml:lang="fi">Elokuvafilmin esitysformaatti, jonka kuvasuhde on enintään 2.76:1 ja joka käyttää alun perin kolmea synkronoitua projektoria.</skos:definition>
      <rdakit:toolkitDefinition xml:lang="fi">Elokuvafilmin esitysformaatti, jonka kuvasuhde on enintään 2.76:1 ja joka käyttää alun perin kolmea synkronoitua projektoria.</rdakit:toolkitDefinition>
      <skos:prefLabel xml:lang="da">Cinerama</skos:prefLabel>
      <rdakit:toolkitLabel xml:lang="da">Cinerama</rdakit:toolkitLabel>
      <skos:definition xml:lang="da">Præsentationsformat til film, som har et billedformat på op til 2.76:1, og som oprindelig anvendte tre synkroniserede projektorer.</skos:definition>
      <rdakit:toolkitDefinition xml:lang="da">Præsentationsformat til film, som har et billedformat på op til 2.76:1, og som oprindelig anvendte tre synkroniserede projektorer.</rdakit:toolkitDefinition>
      <skos:prefLabel xml:lang="ca">Cinerama</skos:prefLabel>
      <rdakit:toolkitLabel xml:lang="ca">Cinerama</rdakit:toolkitLabel>
      <skos:definition xml:lang="ca">Format de presentació d'una pel·lícula cinematogràfica que presenta una relació d'aspecte fins a 2,76:1, originalment usant tres projectors sincronitzats.</skos:definition>
      <rdakit:toolkitDefinition xml:lang="ca">Format de presentació d'una pel·lícula cinematogràfica que presenta una relació d'aspecte fins a 2,76:1, originalment usant tres projectors sincronitzats.</rdakit:toolkitDefinition>
      <skos:prefLabel xml:lang="vi">màn ảnh cực rộng</skos:prefLabel>
      <rdakit:toolkitLabel xml:lang="vi">màn ảnh cực rộng</rdakit:toolkitLabel>
      <skos:definition xml:lang="vi">Định dạng trình bày của phim điện ảnh trình bày tỷ lệ bề ngoài lên tới 2,78:1, sử dụng nguyên gốc ba máy chiếu đồng bộ.</skos:definition>
      <rdakit:toolkitDefinition xml:lang="vi">Định dạng trình bày của phim điện ảnh trình bày tỷ lệ bề ngoài lên tới 2,78:1, sử dụng nguyên gốc ba máy chiếu đồng bộ.</rdakit:toolkitDefinition>
      <skos:prefLabel xml:lang="fr">Cinérama</skos:prefLabel>
      <rdakit:toolkitLabel xml:lang="fr">Cinérama</rdakit:toolkitLabel>
      <skos:definition xml:lang="fr">Format de projection d’un film cinématographique qui produit un format d’image allant jusqu’à 2,76:1, à l'origine au moyen de trois projecteurs synchronisés.</skos:definition>
      <rdakit:toolkitDefinition xml:lang="fr">Format de projection d’un film cinématographique qui produit un format d’image allant jusqu’à 2,76:1, à l'origine au moyen de trois projecteurs synchronisés.</rdakit:toolkitDefinition>
    </skos:Concept>
<!-- Concept: Circarama  -->
    <skos:Concept rdf:about="http://rdaregistry.info/termList/presFormat/1003" xml:lang="en">
      <skos:inScheme rdf:resource="http://rdaregistry.info/termList/presFormat"/>
      <reg:status rdf:resource="http://metadataregistry.org/uri/RegStatus/1001"/>
      <reg:identifier rdf:resource="http://metadataregistry.org/concepts/889"/>
      <skos:prefLabel xml:lang="en">Circarama</skos:prefLabel>
      <skos:altLabel xml:lang="en">Circle-Vision</skos:altLabel>
      <rdakit:toolkitLabel xml:lang="en">Circarama</rdakit:toolkitLabel>
      <skos:definition xml:lang="en">A presentation format of a motion picture film that uses nine projectors for screens arranged in a circle.</skos:definition>
      <rdakit:toolkitDefinition xml:lang="en">A presentation format of a motion picture film that uses nine projectors for screens arranged in a circle.</rdakit:toolkitDefinition>
      <skos:prefLabel xml:lang="de">Circarama</skos:prefLabel>
      <rdakit:toolkitLabel xml:lang="de">Circarama</rdakit:toolkitLabel>
      <skos:definition xml:lang="de">Ein Wiedergabeformat eines Films, das für Leinwände, die im Kreis angeordnet sind, neun Projektoren verwendet.</skos:definition>
      <rdakit:toolkitDefinition xml:lang="de">Ein Wiedergabeformat eines Films, das für Leinwände, die im Kreis angeordnet sind, neun Projektoren verwendet.</rdakit:toolkitDefinition>
      <skos:prefLabel xml:lang="fi">Circarama</skos:prefLabel>
      <rdakit:toolkitLabel xml:lang="fi">Circarama</rdakit:toolkitLabel>
      <skos:definition xml:lang="fi">Elokuvafilmin esitysformaatti, joka käyttää yhdeksää projektoria ympyrään asetelluille kankaille.</skos:definition>
      <rdakit:toolkitDefinition xml:lang="fi">Elokuvafilmin esitysformaatti, joka käyttää yhdeksää projektoria ympyrään asetelluille kankaille.</rdakit:toolkitDefinition>
      <skos:prefLabel xml:lang="da">Circarama</skos:prefLabel>
      <skos:altLabel xml:lang="da">Circle-Vision</skos:altLabel>
      <rdakit:toolkitLabel xml:lang="da">Circarama</rdakit:toolkitLabel>
      <skos:definition xml:lang="da">Præsentationsformat til film, der anvender ni projektorer til skærmbilleder arrangeret i en cirkel.</skos:definition>
      <rdakit:toolkitDefinition xml:lang="da">Præsentationsformat til film, der anvender ni projektorer til skærmbilleder arrangeret i en cirkel.</rdakit:toolkitDefinition>
      <skos:prefLabel xml:lang="ca">Circarama</skos:prefLabel>
      <skos:altLabel xml:lang="ca">Circle-Vision</skos:altLabel>
      <rdakit:toolkitLabel xml:lang="ca">Circarama</rdakit:toolkitLabel>
      <skos:definition xml:lang="ca">Format de presentació d'una pel·lícula cinematogràfica que usa nou projectors per a pantalles disposades en un cercle.</skos:definition>
      <rdakit:toolkitDefinition xml:lang="ca">Format de presentació d'una pel·lícula cinematogràfica que usa nou projectors per a pantalles disposades en un cercle.</rdakit:toolkitDefinition>
      <skos:prefLabel xml:lang="vi">màn ảnh vòng tròn</skos:prefLabel>
      <skos:altLabel xml:lang="vi">Ảo cảnh vòng</skos:altLabel>
      <rdakit:toolkitLabel xml:lang="vi">màn ảnh vòng tròn</rdakit:toolkitLabel>
      <skos:definition xml:lang="vi">Định dạng trình bày của phim điện ảnh sử dụng chín máy chiếu cho các màn ảnh được bố trí trong hình tròn.</skos:definition>
      <rdakit:toolkitDefinition xml:lang="vi">Định dạng trình bày của phim điện ảnh sử dụng chín máy chiếu cho các màn ảnh được bố trí trong hình tròn.</rdakit:toolkitDefinition>
      <skos:prefLabel xml:lang="fr">Circarama</skos:prefLabel>
      <skos:altLabel xml:lang="fr">Circle-Vision</skos:altLabel>
      <rdakit:toolkitLabel xml:lang="fr">Circarama</rdakit:toolkitLabel>
      <skos:definition xml:lang="fr">Format de projection d’un film cinématographique qui utilise neuf projecteurs et des écrans agencés en cercle.</skos:definition>
      <rdakit:toolkitDefinition xml:lang="fr">Format de projection d’un film cinématographique qui utilise neuf projecteurs et des écrans agencés en cercle.</rdakit:toolkitDefinition>
    </skos:Concept>
<!-- Concept: IMAX  -->
    <skos:Concept rdf:about="http://rdaregistry.info/termList/presFormat/1004" xml:lang="en">
      <skos:inScheme rdf:resource="http://rdaregistry.info/termList/presFormat"/>
      <reg:status rdf:resource="http://metadataregistry.org/uri/RegStatus/1001"/>
      <reg:identifier rdf:resource="http://metadataregistry.org/concepts/890"/>
      <skos:prefLabel xml:lang="en">IMAX</skos:prefLabel>
      <rdakit:toolkitLabel xml:lang="en">IMAX</rdakit:toolkitLabel>
      <skos:definition xml:lang="en">A presentation format of a motion picture film that projects images of far greater size and resolution than conventional film systems.</skos:definition>
      <rdakit:toolkitDefinition xml:lang="en">A presentation format of a motion picture film that projects images of far greater size and resolution than conventional film systems.</rdakit:toolkitDefinition>
      <skos:prefLabel xml:lang="de">IMAX</skos:prefLabel>
      <rdakit:toolkitLabel xml:lang="de">IMAX</rdakit:toolkitLabel>
      <skos:definition xml:lang="de">Ein Wiedergabeformat eines Films, das Bilder deutlich größer und in deutlich besserer Auflösung zeigt als herkömmliche Filmsysteme.</skos:definition>
      <rdakit:toolkitDefinition xml:lang="de">Ein Wiedergabeformat eines Films, das Bilder deutlich größer und in deutlich besserer Auflösung zeigt als herkömmliche Filmsysteme.</rdakit:toolkitDefinition>
      <skos:prefLabel xml:lang="fi">IMAX</skos:prefLabel>
      <rdakit:toolkitLabel xml:lang="fi">IMAX</rdakit:toolkitLabel>
      <skos:definition xml:lang="fi">Elokuvafilmin esitysformaatti, joka heijastaa tavanomaisia filmijärjestelmiä paljon suurempikokoisia ja -resoluutioisia kuvia.</skos:definition>
      <rdakit:toolkitDefinition xml:lang="fi">Elokuvafilmin esitysformaatti, joka heijastaa tavanomaisia filmijärjestelmiä paljon suurempikokoisia ja -resoluutioisia kuvia.</rdakit:toolkitDefinition>
      <skos:prefLabel xml:lang="da">IMAX</skos:prefLabel>
      <rdakit:toolkitLabel xml:lang="da">IMAX</rdakit:toolkitLabel>
      <skos:definition xml:lang="da">Præsentationsformat til film, der projekterer billeder af langt større størrelse og opløsning end konventionelle filmsystemer.</skos:definition>
      <rdakit:toolkitDefinition xml:lang="da">Præsentationsformat til film, der projekterer billeder af langt større størrelse og opløsning end konventionelle filmsystemer.</rdakit:toolkitDefinition>
      <skos:prefLabel xml:lang="ca">IMAX</skos:prefLabel>
      <rdakit:toolkitLabel xml:lang="ca">IMAX</rdakit:toolkitLabel>
      <skos:definition xml:lang="ca">Format de presentació d'una pel·lícula cinematogràfica que projecta imatges molt més grans de mida i resolució que els sistemes convencionals de pel·lícula.</skos:definition>
      <rdakit:toolkitDefinition xml:lang="ca">Format de presentació d'una pel·lícula cinematogràfica que projecta imatges molt més grans de mida i resolució que els sistemes convencionals de pel·lícula.</rdakit:toolkitDefinition>
      <skos:prefLabel xml:lang="vi">IMAX</skos:prefLabel>
      <rdakit:toolkitLabel xml:lang="vi">IMAX</rdakit:toolkitLabel>
      <skos:definition xml:lang="vi">Định dạng trình bày của phim điện ảnh chiếu hình ảnh với khổ và độ phân giải lớn hơn nhiều so với hệ thống phim thông thường.</skos:definition>
      <rdakit:toolkitDefinition xml:lang="vi">Định dạng trình bày của phim điện ảnh chiếu hình ảnh với khổ và độ phân giải lớn hơn nhiều so với hệ thống phim thông thường.</rdakit:toolkitDefinition>
      <skos:prefLabel xml:lang="fr">IMAX</skos:prefLabel>
      <rdakit:toolkitLabel xml:lang="fr">IMAX</rdakit:toolkitLabel>
      <skos:definition xml:lang="fr">Format de projection d’un film cinématographique qui produit des images de taille et de résolution largement supérieures à celles des systèmes conventionnels.</skos:definition>
      <rdakit:toolkitDefinition xml:lang="fr">Format de projection d’un film cinématographique qui produit des images de taille et de résolution largement supérieures à celles des systèmes conventionnels.</rdakit:toolkitDefinition>
    </skos:Concept>
<!-- Concept: multiprojector  -->
    <skos:Concept rdf:about="http://rdaregistry.info/termList/presFormat/1005" xml:lang="en">
      <skos:inScheme rdf:resource="http://rdaregistry.info/termList/presFormat"/>
      <reg:status rdf:resource="http://metadataregistry.org/uri/RegStatus/1001"/>
      <reg:identifier rdf:resource="http://metadataregistry.org/concepts/891"/>
      <skos:prefLabel xml:lang="en">multiprojector</skos:prefLabel>
      <rdakit:toolkitLabel xml:lang="en">multiprojector</rdakit:toolkitLabel>
      <skos:definition xml:lang="en">A presentation format of a motion picture film using multiple synchronized projectors.</skos:definition>
      <rdakit:toolkitDefinition xml:lang="en">A presentation format of a motion picture film using multiple synchronized projectors.</rdakit:toolkitDefinition>
      <skos:prefLabel xml:lang="de">Multiprojektion</skos:prefLabel>
      <rdakit:toolkitLabel xml:lang="de">Multiprojektion</rdakit:toolkitLabel>
      <skos:definition xml:lang="de">Ein Wiedergabeformat eines Films, das mehrere synchron laufende Projektoren verwendet.</skos:definition>
      <rdakit:toolkitDefinition xml:lang="de">Ein Wiedergabeformat eines Films, das mehrere synchron laufende Projektoren verwendet.</rdakit:toolkitDefinition>
      <skos:prefLabel xml:lang="fi">multiprojektori</skos:prefLabel>
      <rdakit:toolkitLabel xml:lang="fi">multiprojektori</rdakit:toolkitLabel>
      <skos:definition xml:lang="fi">Elokuvafilmin esitysformaatti, joka käyttää useampia synkronoituja projektoreita.</skos:definition>
      <rdakit:toolkitDefinition xml:lang="fi">Elokuvafilmin esitysformaatti, joka käyttää useampia synkronoituja projektoreita.</rdakit:toolkitDefinition>
      <skos:definition xml:lang="da">Præsentationsformat til film, der anvender flere synkroniserede projektorer.</skos:definition>
      <rdakit:toolkitDefinition xml:lang="da">Præsentationsformat til film, der anvender flere synkroniserede projektorer.</rdakit:toolkitDefinition>
      <skos:prefLabel xml:lang="ca">multiprojector</skos:prefLabel>
      <rdakit:toolkitLabel xml:lang="ca">multiprojector</rdakit:toolkitLabel>
      <skos:definition xml:lang="ca">Format de presentació d'una pel·lícula cinematogràfica que usa múltiples projectors sincronitzats.</skos:definition>
      <rdakit:toolkitDefinition xml:lang="ca">Format de presentació d'una pel·lícula cinematogràfica que usa múltiples projectors sincronitzats.</rdakit:toolkitDefinition>
      <skos:prefLabel xml:lang="vi">đa máy chiếu</skos:prefLabel>
      <rdakit:toolkitLabel xml:lang="vi">đa máy chiếu</rdakit:toolkitLabel>
      <skos:definition xml:lang="vi">Định dạng trình bày của phim điện ảnh sử dụng nhiều máy chiếu đồng bộ.</skos:definition>
      <rdakit:toolkitDefinition xml:lang="vi">Định dạng trình bày của phim điện ảnh sử dụng nhiều máy chiếu đồng bộ.</rdakit:toolkitDefinition>
      <skos:prefLabel xml:lang="fr">multiprojecteurs</skos:prefLabel>
      <rdakit:toolkitLabel xml:lang="fr">multiprojecteurs</rdakit:toolkitLabel>
      <skos:definition xml:lang="fr">Format de projection d’un film cinématographique qui utilise plusieurs projecteurs synchronisés.</skos:definition>
      <rdakit:toolkitDefinition xml:lang="fr">Format de projection d’un film cinématographique qui utilise plusieurs projecteurs synchronisés.</rdakit:toolkitDefinition>
    </skos:Concept>
<!-- Concept: multiscreen  -->
    <skos:Concept rdf:about="http://rdaregistry.info/termList/presFormat/1006" xml:lang="en">
      <skos:inScheme rdf:resource="http://rdaregistry.info/termList/presFormat"/>
      <reg:status rdf:resource="http://metadataregistry.org/uri/RegStatus/1001"/>
      <reg:identifier rdf:resource="http://metadataregistry.org/concepts/892"/>
      <skos:prefLabel xml:lang="en">multiscreen</skos:prefLabel>
      <rdakit:toolkitLabel xml:lang="en">multiscreen</rdakit:toolkitLabel>
      <skos:definition xml:lang="en">A presentation format of a motion picture film using multiple screens.</skos:definition>
      <rdakit:toolkitDefinition xml:lang="en">A presentation format of a motion picture film using multiple screens.</rdakit:toolkitDefinition>
      <skos:prefLabel xml:lang="de">Multiscreen</skos:prefLabel>
      <rdakit:toolkitLabel xml:lang="de">Multiscreen</rdakit:toolkitLabel>
      <skos:definition xml:lang="de">Ein Wiedergabeformat eines Films, das mehrere Bildschirme verwendet.</skos:definition>
      <rdakit:toolkitDefinition xml:lang="de">Ein Wiedergabeformat eines Films, das mehrere Bildschirme verwendet.</rdakit:toolkitDefinition>
      <skos:prefLabel xml:lang="fi">monikangas</skos:prefLabel>
      <rdakit:toolkitLabel xml:lang="fi">monikangas</rdakit:toolkitLabel>
      <skos:definition xml:lang="fi">Elokuvafilmin esitysformaatti, joka käyttää useampia kankaita.</skos:definition>
      <rdakit:toolkitDefinition xml:lang="fi">Elokuvafilmin esitysformaatti, joka käyttää useampia kankaita.</rdakit:toolkitDefinition>
      <skos:definition xml:lang="da">Præsentationsformat til film, der anvender flere skærmbilleder.</skos:definition>
      <rdakit:toolkitDefinition xml:lang="da">Præsentationsformat til film, der anvender flere skærmbilleder.</rdakit:toolkitDefinition>
      <skos:prefLabel xml:lang="ca">multicinema</skos:prefLabel>
      <rdakit:toolkitLabel xml:lang="ca">multicinema</rdakit:toolkitLabel>
      <skos:definition xml:lang="ca">Format de presentació d'una pel·lícula cinematogràfica que usa diverses pantalles.</skos:definition>
      <rdakit:toolkitDefinition xml:lang="ca">Format de presentació d'una pel·lícula cinematogràfica que usa diverses pantalles.</rdakit:toolkitDefinition>
      <skos:prefLabel xml:lang="vi">nhiều màn ảnh</skos:prefLabel>
      <rdakit:toolkitLabel xml:lang="vi">nhiều màn ảnh</rdakit:toolkitLabel>
      <skos:definition xml:lang="vi">Định dạng trình bày của phim điện ảnh dùng nhiều màn ảnh.</skos:definition>
      <rdakit:toolkitDefinition xml:lang="vi">Định dạng trình bày của phim điện ảnh dùng nhiều màn ảnh.</rdakit:toolkitDefinition>
      <skos:prefLabel xml:lang="fr">multiécrans</skos:prefLabel>
      <rdakit:toolkitLabel xml:lang="fr">multiécrans</rdakit:toolkitLabel>
      <skos:definition xml:lang="fr">Format de projection d’un film cinématographique qui utilise plusieurs écrans.</skos:definition>
      <rdakit:toolkitDefinition xml:lang="fr">Format de projection d’un film cinématographique qui utilise plusieurs écrans.</rdakit:toolkitDefinition>
    </skos:Concept>
<!-- Concept: Panavision  -->
    <skos:Concept rdf:about="http://rdaregistry.info/termList/presFormat/1007" xml:lang="en">
      <skos:inScheme rdf:resource="http://rdaregistry.info/termList/presFormat"/>
      <reg:status rdf:resource="http://metadataregistry.org/uri/RegStatus/1001"/>
      <reg:identifier rdf:resource="http://metadataregistry.org/concepts/893"/>
      <skos:prefLabel xml:lang="en">Panavision</skos:prefLabel>
      <rdakit:toolkitLabel xml:lang="en">Panavision</rdakit:toolkitLabel>
      <skos:definition xml:lang="en">A presentation format of a motion picture film that presents a wide-screen aspect ratio using Panavision anamorphic lenses.</skos:definition>
      <rdakit:toolkitDefinition xml:lang="en">A presentation format of a motion picture film that presents a wide-screen aspect ratio using Panavision anamorphic lenses.</rdakit:toolkitDefinition>
      <skos:prefLabel xml:lang="de">Panavision</skos:prefLabel>
      <rdakit:toolkitLabel xml:lang="de">Panavision</rdakit:toolkitLabel>
      <skos:definition xml:lang="de">Ein Wiedergabeformat eines Films, das ein Breitband-Bildformat darstellt, das durch die Verwendung eines Anamorphot-Objektivs von Panavision entsteht.</skos:definition>
      <rdakit:toolkitDefinition xml:lang="de">Ein Wiedergabeformat eines Films, das ein Breitband-Bildformat darstellt, das durch die Verwendung eines Anamorphot-Objektivs von Panavision entsteht.</rdakit:toolkitDefinition>
      <skos:prefLabel xml:lang="fi">Panavision</skos:prefLabel>
      <rdakit:toolkitLabel xml:lang="fi">Panavision</rdakit:toolkitLabel>
      <skos:definition xml:lang="fi">Elokuvafilmin esitysformaatti, joka esittää kuvan laajakangaskuvasuhteessa käyttäen Panavisionin anamorfisia linssejä.</skos:definition>
      <rdakit:toolkitDefinition xml:lang="fi">Elokuvafilmin esitysformaatti, joka esittää kuvan laajakangaskuvasuhteessa käyttäen Panavisionin anamorfisia linssejä.</rdakit:toolkitDefinition>
      <skos:prefLabel xml:lang="da">Panavision</skos:prefLabel>
      <rdakit:toolkitLabel xml:lang="da">Panavision</rdakit:toolkitLabel>
      <skos:definition xml:lang="da">Præsentationsformat til film, der præsenterer er bredbåndsformat forhold ved anvendelse af Panavision anamorfe linser.</skos:definition>
      <rdakit:toolkitDefinition xml:lang="da">Præsentationsformat til film, der præsenterer er bredbåndsformat forhold ved anvendelse af Panavision anamorfe linser.</rdakit:toolkitDefinition>
      <skos:prefLabel xml:lang="ca">Panavision</skos:prefLabel>
      <rdakit:toolkitLabel xml:lang="ca">Panavision</rdakit:toolkitLabel>
      <skos:definition xml:lang="ca">Format de presentació d'una pel·lícula cinematogràfica que presenta una relació d'aspecte de pantalla panoràmica que usa lents anamòrfiques de Panavision.</skos:definition>
      <rdakit:toolkitDefinition xml:lang="ca">Format de presentació d'una pel·lícula cinematogràfica que presenta una relació d'aspecte de pantalla panoràmica que usa lents anamòrfiques de Panavision.</rdakit:toolkitDefinition>
      <skos:prefLabel xml:lang="vi">Panavision</skos:prefLabel>
      <rdakit:toolkitLabel xml:lang="vi">Panavision</rdakit:toolkitLabel>
      <skos:definition xml:lang="vi">Định dạng trình bày của phim điện ảnh trình bày tỷ lệ bề ngoài màn ảnh rộng sử dụng các thấu kính anamorphic Panavision</skos:definition>
      <rdakit:toolkitDefinition xml:lang="vi">Định dạng trình bày của phim điện ảnh trình bày tỷ lệ bề ngoài màn ảnh rộng sử dụng các thấu kính anamorphic Panavision</rdakit:toolkitDefinition>
      <skos:prefLabel xml:lang="fr">Panavision</skos:prefLabel>
      <rdakit:toolkitLabel xml:lang="fr">Panavision</rdakit:toolkitLabel>
      <skos:definition xml:lang="fr">Format de projection d’un film cinématographique qui produit un format d’image pour écran large au moyen d’objectifs anamorphiques Panavision.</skos:definition>
      <rdakit:toolkitDefinition xml:lang="fr">Format de projection d’un film cinématographique qui produit un format d’image pour écran large au moyen d’objectifs anamorphiques Panavision.</rdakit:toolkitDefinition>
    </skos:Concept>
<!-- Concept: standard silent aperture  -->
    <skos:Concept rdf:about="http://rdaregistry.info/termList/presFormat/1008" xml:lang="en">
      <skos:inScheme rdf:resource="http://rdaregistry.info/termList/presFormat"/>
      <reg:status rdf:resource="http://metadataregistry.org/uri/RegStatus/1001"/>
      <reg:identifier rdf:resource="http://metadataregistry.org/concepts/894"/>
      <skos:prefLabel xml:lang="en">standard silent aperture</skos:prefLabel>
      <rdakit:toolkitLabel xml:lang="en">standard silent aperture</rdakit:toolkitLabel>
      <skos:definition xml:lang="en">A presentation format of a motion picture film that uses a standard projector aperture for silent film.</skos:definition>
      <rdakit:toolkitDefinition xml:lang="en">A presentation format of a motion picture film that uses a standard projector aperture for silent film.</rdakit:toolkitDefinition>
      <skos:prefLabel xml:lang="de">standard silent aperture</skos:prefLabel>
      <rdakit:toolkitLabel xml:lang="de">standard silent aperture</rdakit:toolkitLabel>
      <skos:definition xml:lang="de">Ein Wiedergabeformat eines Films, das eine Standardprojektorapertur für einen Stummfilm verwendet.</skos:definition>
      <rdakit:toolkitDefinition xml:lang="de">Ein Wiedergabeformat eines Films, das eine Standardprojektorapertur für einen Stummfilm verwendet.</rdakit:toolkitDefinition>
      <skos:prefLabel xml:lang="fi">standardimykkäfilmin kuvakoko</skos:prefLabel>
      <rdakit:toolkitLabel xml:lang="fi">standardimykkäfilmin kuvakoko</rdakit:toolkitLabel>
      <skos:definition xml:lang="fi">Elokuvafilmin esitysformaatti, joka käyttää mykkäfilmin standardiprojektoriaukkoa.</skos:definition>
      <rdakit:toolkitDefinition xml:lang="fi">Elokuvafilmin esitysformaatti, joka käyttää mykkäfilmin standardiprojektoriaukkoa.</rdakit:toolkitDefinition>
      <skos:definition xml:lang="da">Præsentationsformat til  film, der anvender standard projektoråbning til stumfilm.</skos:definition>
      <rdakit:toolkitDefinition xml:lang="da">Præsentationsformat til  film, der anvender standard projektoråbning til stumfilm.</rdakit:toolkitDefinition>
      <skos:prefLabel xml:lang="ca">format mut estàndard</skos:prefLabel>
      <rdakit:toolkitLabel xml:lang="ca">format mut estàndard</rdakit:toolkitLabel>
      <skos:definition xml:lang="ca">Format de presentació d'una pel·lícula cinematogràfica que usa un format de projector estàndard per a una pel·lícula muda.</skos:definition>
      <rdakit:toolkitDefinition xml:lang="ca">Format de presentació d'una pel·lícula cinematogràfica que usa un format de projector estàndard per a una pel·lícula muda.</rdakit:toolkitDefinition>
      <skos:prefLabel xml:lang="vi">kẽ hở câm chuẩn</skos:prefLabel>
      <rdakit:toolkitLabel xml:lang="vi">kẽ hở câm chuẩn</rdakit:toolkitLabel>
      <skos:definition xml:lang="vi">Định dạng trình bày của phim điện ảnh sử dụng kẽ hở máy chiếu chuẩn cho phim câm.</skos:definition>
      <rdakit:toolkitDefinition xml:lang="vi">Định dạng trình bày của phim điện ảnh sử dụng kẽ hở máy chiếu chuẩn cho phim câm.</rdakit:toolkitDefinition>
      <skos:prefLabel xml:lang="fr">format standard muet</skos:prefLabel>
      <rdakit:toolkitLabel xml:lang="fr">format standard muet</rdakit:toolkitLabel>
      <skos:definition xml:lang="fr">Format de projection d’un film cinématographique qui utilise une fenêtre de projection standard pour films muets.</skos:definition>
      <rdakit:toolkitDefinition xml:lang="fr">Format de projection d’un film cinématographique qui utilise une fenêtre de projection standard pour films muets.</rdakit:toolkitDefinition>
    </skos:Concept>
<!-- Concept: standard sound aperture  -->
    <skos:Concept rdf:about="http://rdaregistry.info/termList/presFormat/1009" xml:lang="en">
      <skos:inScheme rdf:resource="http://rdaregistry.info/termList/presFormat"/>
      <reg:status rdf:resource="http://metadataregistry.org/uri/RegStatus/1001"/>
      <reg:identifier rdf:resource="http://metadataregistry.org/concepts/895"/>
      <skos:prefLabel xml:lang="en">standard sound aperture</skos:prefLabel>
      <rdakit:toolkitLabel xml:lang="en">standard sound aperture</rdakit:toolkitLabel>
      <skos:definition xml:lang="en">A presentation format of a motion picture film that uses a standard projector aperture for film with a sound-track.</skos:definition>
      <rdakit:toolkitDefinition xml:lang="en">A presentation format of a motion picture film that uses a standard projector aperture for film with a sound-track.</rdakit:toolkitDefinition>
      <skos:prefLabel xml:lang="de">standard sound aperture</skos:prefLabel>
      <rdakit:toolkitLabel xml:lang="de">standard sound aperture</rdakit:toolkitLabel>
      <skos:definition xml:lang="de">Ein Wiedergabeformat eines Films, das eine Standardprojektorapertur für einen Film mit einer Tonspur verwendet.</skos:definition>
      <rdakit:toolkitDefinition xml:lang="de">Ein Wiedergabeformat eines Films, das eine Standardprojektorapertur für einen Film mit einer Tonspur verwendet.</rdakit:toolkitDefinition>
      <skos:prefLabel xml:lang="fi">standardiäänifilmin kuvakoko</skos:prefLabel>
      <rdakit:toolkitLabel xml:lang="fi">standardiäänifilmin kuvakoko</rdakit:toolkitLabel>
      <skos:definition xml:lang="fi">Elokuvafilmin esitysformaatti, joka käyttää ääniraidallisen elokuvan standardiprojektoriaukkoa.</skos:definition>
      <rdakit:toolkitDefinition xml:lang="fi">Elokuvafilmin esitysformaatti, joka käyttää ääniraidallisen elokuvan standardiprojektoriaukkoa.</rdakit:toolkitDefinition>
      <skos:definition xml:lang="da">Præsentationsformat til film, der anvender en standard projektoråbning til en film med lydspor.</skos:definition>
      <rdakit:toolkitDefinition xml:lang="da">Præsentationsformat til film, der anvender en standard projektoråbning til en film med lydspor.</rdakit:toolkitDefinition>
      <skos:prefLabel xml:lang="ca">format àudio estàndard</skos:prefLabel>
      <rdakit:toolkitLabel xml:lang="ca">format àudio estàndard</rdakit:toolkitLabel>
      <skos:definition xml:lang="ca">Format de presentació d'una pel·lícula cinematogràficaque usa un format de projector estàndard per a una pel·lícula amb una banda sonora.</skos:definition>
      <rdakit:toolkitDefinition xml:lang="ca">Format de presentació d'una pel·lícula cinematogràficaque usa un format de projector estàndard per a una pel·lícula amb una banda sonora.</rdakit:toolkitDefinition>
      <skos:prefLabel xml:lang="vi">kẽ hở tiếng chuẩn</skos:prefLabel>
      <rdakit:toolkitLabel xml:lang="vi">kẽ hở tiếng chuẩn</rdakit:toolkitLabel>
      <skos:definition xml:lang="vi">Định dạng trình bày của phim điện ảnh sử dụng kẽ hở máy chiếu chuẩn cho phim với rãnh âm thanh.</skos:definition>
      <rdakit:toolkitDefinition xml:lang="vi">Định dạng trình bày của phim điện ảnh sử dụng kẽ hở máy chiếu chuẩn cho phim với rãnh âm thanh.</rdakit:toolkitDefinition>
      <skos:prefLabel xml:lang="fr">format standard sonore</skos:prefLabel>
      <rdakit:toolkitLabel xml:lang="fr">format standard sonore</rdakit:toolkitLabel>
      <skos:definition xml:lang="fr">Format de projection d’un film cinématographique qui utilise une fenêtre de projection standard pour films avec bande sonore.</skos:definition>
      <rdakit:toolkitDefinition xml:lang="fr">Format de projection d’un film cinématographique qui utilise une fenêtre de projection standard pour films avec bande sonore.</rdakit:toolkitDefinition>
    </skos:Concept>
<!-- Concept: stereoscopic  -->
    <skos:Concept rdf:about="http://rdaregistry.info/termList/presFormat/1010" xml:lang="en">
      <skos:inScheme rdf:resource="http://rdaregistry.info/termList/presFormat"/>
      <reg:status rdf:resource="http://metadataregistry.org/uri/RegStatus/1001"/>
      <reg:identifier rdf:resource="http://metadataregistry.org/concepts/896"/>
      <skos:prefLabel xml:lang="en">stereoscopic</skos:prefLabel>
      <rdakit:toolkitLabel xml:lang="en">stereoscopic</rdakit:toolkitLabel>
      <skos:definition xml:lang="en">A presentation format of a motion picture film that gives the illusion of three dimensions by using stereoscopic images.</skos:definition>
      <rdakit:toolkitDefinition xml:lang="en">A presentation format of a motion picture film that gives the illusion of three dimensions by using stereoscopic images.</rdakit:toolkitDefinition>
      <skos:prefLabel xml:lang="de">Stereoskop</skos:prefLabel>
      <rdakit:toolkitLabel xml:lang="de">Stereoskop</rdakit:toolkitLabel>
      <skos:definition xml:lang="de">Ein Wiedergabeformat eines Films, das die Illusion von drei Dimensionen mit stereoskopischen Bildern vermittelt.</skos:definition>
      <rdakit:toolkitDefinition xml:lang="de">Ein Wiedergabeformat eines Films, das die Illusion von drei Dimensionen mit stereoskopischen Bildern vermittelt.</rdakit:toolkitDefinition>
      <skos:prefLabel xml:lang="fi">stereoskooppinen</skos:prefLabel>
      <rdakit:toolkitLabel xml:lang="fi">stereoskooppinen</rdakit:toolkitLabel>
      <skos:definition xml:lang="fi">Elokuvafilmin esitysformaatti, joka luo kolmiulotteisuuden vaikutelman käyttämällä stereoskooppisia kuvia.</skos:definition>
      <rdakit:toolkitDefinition xml:lang="fi">Elokuvafilmin esitysformaatti, joka luo kolmiulotteisuuden vaikutelman käyttämällä stereoskooppisia kuvia.</rdakit:toolkitDefinition>
      <skos:prefLabel xml:lang="da">stereoskopisk</skos:prefLabel>
      <rdakit:toolkitLabel xml:lang="da">stereoskopisk</rdakit:toolkitLabel>
      <skos:definition xml:lang="da">Præsentationsfamt til film, der giver illusionen af tre dimensioner ved hjælp af stereoskopiske billeder.</skos:definition>
      <rdakit:toolkitDefinition xml:lang="da">Præsentationsfamt til film, der giver illusionen af tre dimensioner ved hjælp af stereoskopiske billeder.</rdakit:toolkitDefinition>
      <skos:prefLabel xml:lang="ca">estereoscòpic</skos:prefLabel>
      <rdakit:toolkitLabel xml:lang="ca">estereoscòpic</rdakit:toolkitLabel>
      <skos:definition xml:lang="ca">Format de presentació d'una pel·lícula cinematogràfica que dóna la il·lusió de tres dimensions usant imatges estereoscòpiques.</skos:definition>
      <rdakit:toolkitDefinition xml:lang="ca">Format de presentació d'una pel·lícula cinematogràfica que dóna la il·lusió de tres dimensions usant imatges estereoscòpiques.</rdakit:toolkitDefinition>
      <skos:prefLabel xml:lang="vi">lập thể</skos:prefLabel>
      <rdakit:toolkitLabel xml:lang="vi">lập thể</rdakit:toolkitLabel>
      <skos:definition xml:lang="vi">Định dạng trình bày của phim điện ảnh tạo ảo giác ba chiều bằng cách dùng hình ảnh lập thể.</skos:definition>
      <rdakit:toolkitDefinition xml:lang="vi">Định dạng trình bày của phim điện ảnh tạo ảo giác ba chiều bằng cách dùng hình ảnh lập thể.</rdakit:toolkitDefinition>
      <skos:prefLabel xml:lang="fr">procédé stéréoscopique</skos:prefLabel>
      <rdakit:toolkitLabel xml:lang="fr">procédé stéréoscopique</rdakit:toolkitLabel>
      <skos:definition xml:lang="fr">Format de projection d’un film cinématographique qui donne l’illusion des trois dimensions au moyen d’images stéréoscopiques.</skos:definition>
      <rdakit:toolkitDefinition xml:lang="fr">Format de projection d’un film cinématographique qui donne l’illusion des trois dimensions au moyen d’images stéréoscopiques.</rdakit:toolkitDefinition>
    </skos:Concept>
<!-- Concept: Techniscope  -->
    <skos:Concept rdf:about="http://rdaregistry.info/termList/presFormat/1011" xml:lang="en">
      <skos:inScheme rdf:resource="http://rdaregistry.info/termList/presFormat"/>
      <reg:status rdf:resource="http://metadataregistry.org/uri/RegStatus/1001"/>
      <reg:identifier rdf:resource="http://metadataregistry.org/concepts/897"/>
      <skos:prefLabel xml:lang="en">Techniscope</skos:prefLabel>
      <rdakit:toolkitLabel xml:lang="en">Techniscope</rdakit:toolkitLabel>
      <skos:definition xml:lang="en">A presentation format of a motion picture film that presents an aspect ratio of 2.33:1 using 35 mm film.</skos:definition>
      <rdakit:toolkitDefinition xml:lang="en">A presentation format of a motion picture film that presents an aspect ratio of 2.33:1 using 35 mm film.</rdakit:toolkitDefinition>
      <skos:prefLabel xml:lang="de">Techniscope</skos:prefLabel>
      <rdakit:toolkitLabel xml:lang="de">Techniscope</rdakit:toolkitLabel>
      <skos:definition xml:lang="de">Ein Wiedergabeformat eines Films, das ein Bildformat von 2,33:1 mit einem 35 mm Film darstellt.</skos:definition>
      <rdakit:toolkitDefinition xml:lang="de">Ein Wiedergabeformat eines Films, das ein Bildformat von 2,33:1 mit einem 35 mm Film darstellt.</rdakit:toolkitDefinition>
      <skos:prefLabel xml:lang="fi">techniscope</skos:prefLabel>
      <rdakit:toolkitLabel xml:lang="fi">techniscope</rdakit:toolkitLabel>
      <skos:definition xml:lang="fi">Elokuvafilmin esitysformaatti, jonka kuvasuhde on 2.33:1 käyttäen 35 mm:n filmiä.</skos:definition>
      <rdakit:toolkitDefinition xml:lang="fi">Elokuvafilmin esitysformaatti, jonka kuvasuhde on 2.33:1 käyttäen 35 mm:n filmiä.</rdakit:toolkitDefinition>
      <skos:prefLabel xml:lang="da">Techniscope</skos:prefLabel>
      <rdakit:toolkitLabel xml:lang="da">Techniscope</rdakit:toolkitLabel>
      <skos:definition xml:lang="da">Præsentationsformat til film, der præsenterer et billedforhold på 2.33:1 ved anvendelse af 35 mm film.</skos:definition>
      <rdakit:toolkitDefinition xml:lang="da">Præsentationsformat til film, der præsenterer et billedforhold på 2.33:1 ved anvendelse af 35 mm film.</rdakit:toolkitDefinition>
      <skos:prefLabel xml:lang="ca">Techniscope</skos:prefLabel>
      <rdakit:toolkitLabel xml:lang="ca">Techniscope</rdakit:toolkitLabel>
      <skos:definition xml:lang="ca">Format de presentació d'una pel·lícula cinematogràfica que presenta una relació d'aspecte de 2,33:1 usant una pel·lícula de 35 mm.</skos:definition>
      <rdakit:toolkitDefinition xml:lang="ca">Format de presentació d'una pel·lícula cinematogràfica que presenta una relació d'aspecte de 2,33:1 usant una pel·lícula de 35 mm.</rdakit:toolkitDefinition>
      <skos:prefLabel xml:lang="vi">Techniscope</skos:prefLabel>
      <rdakit:toolkitLabel xml:lang="vi">Techniscope</rdakit:toolkitLabel>
      <skos:definition xml:lang="vi">Định dạng trình bày của phim điện ảnh trình bày tỷ lệ bề ngoài là 2,33:1 dùng phim 35 mm.</skos:definition>
      <rdakit:toolkitDefinition xml:lang="vi">Định dạng trình bày của phim điện ảnh trình bày tỷ lệ bề ngoài là 2,33:1 dùng phim 35 mm.</rdakit:toolkitDefinition>
      <skos:prefLabel xml:lang="fr">Techniscope</skos:prefLabel>
      <rdakit:toolkitLabel xml:lang="fr">Techniscope</rdakit:toolkitLabel>
      <skos:definition xml:lang="fr">Format de projection d’un film cinématographique qui produit un format d’image de 2,33:1 sur film 35 mm.</skos:definition>
      <rdakit:toolkitDefinition xml:lang="fr">Format de projection d’un film cinématographique qui produit un format d’image de 2,33:1 sur film 35 mm.</rdakit:toolkitDefinition>
    </skos:Concept>

<!-- Status properties used in this document  -->
    <skos:Concept rdf:about="http://metadataregistry.org/uri/RegStatus/1001">
        <skos:prefLabel xml:lang="en">Published</skos:prefLabel>
    </skos:Concept>

</rdf:RDF>
