<?xml version="1.0" encoding = "UTF-8"?>
<rdf:RDF
    xmlns:dc="http://purl.org/dc/elements/1.1/"
    xmlns:rdakit="http://metadataregistry.org/uri/profile/rdakit/"
    xmlns:rdf="http://www.w3.org/1999/02/22-rdf-syntax-ns#"
    xmlns:reg="http://metadataregistry.org/uri/profile/regap/"
    xmlns:owl="http://www.w3.org/2002/07/owl#"
    xmlns:skos="http://www.w3.org/2004/02/skos/core#">

<owl:Ontology rdf:about="http://rdaregistry.info/termList/RDAContentType" />
<!-- Scheme: RDA Content Type -->
    <skos:ConceptScheme rdf:about="http://rdaregistry.info/termList/RDAContentType">
        <dc:title>RDA Content Type</dc:title>
    </skos:ConceptScheme>

<!-- Concept: cartographic dataset  -->
    <skos:Concept rdf:about="http://rdaregistry.info/termList/RDAContentType/1001" xml:lang="en">
      <skos:inScheme rdf:resource="http://rdaregistry.info/termList/RDAContentType"/>
      <reg:status rdf:resource="http://metadataregistry.org/uri/RegStatus/1001"/>
      <reg:identifier rdf:resource="http://metadataregistry.org/concepts/510"/>
      <skos:prefLabel xml:lang="en">cartographic dataset</skos:prefLabel>
      <skos:definition xml:lang="en">A content type consisting of cartographic content expressed through a digitally encoded dataset intended to be processed by a computer.</skos:definition>
      <skos:prefLabel xml:lang="de">Kartografischer Datensatz</skos:prefLabel>
      <skos:definition xml:lang="de">Ein Inhaltstyp, der aus kartografischem Inhalt besteht, der über einen digital kodierten Datenbestand ausgedrückt wird, der für die Verarbeitung durch einen Computer konzipiert ist.</skos:definition>
      <skos:scopeNote xml:lang="en">A cartographic dataset excludes cartographic data intended to be perceived in the form of an image or three-dimensional form.</skos:scopeNote>
	    <skos:related rdf:resource="http://rdaregistry.info/termList/RDAContentType/1003"/>
	    <skos:related rdf:resource="http://rdaregistry.info/termList/RDAContentType/1004"/>
	    <skos:related rdf:resource="http://rdaregistry.info/termList/RDAContentType/1005"/>
	    <skos:related rdf:resource="http://rdaregistry.info/termList/RDAContentType/1006"/>
	    <skos:related rdf:resource="http://rdaregistry.info/termList/RDAContentType/1002"/>
	    <skos:related rdf:resource="http://rdaregistry.info/termList/RDAContentType/1007"/>
      <skos:prefLabel xml:lang="fr">données cartographiques</skos:prefLabel>
      <skos:definition xml:lang="fr">Type de contenu qui consiste en contenu cartographique exprimé au moyen de données encodées numériquement en vue d’un traitement par ordinateur.</skos:definition>
      <skos:prefLabel xml:lang="es">conjunto de datos cartográficos</skos:prefLabel>
      <skos:definition xml:lang="es">Contenido cartográfico expresado mediante un conjunto de datos codificados digitalmente para ser procesados por un computador.</skos:definition>
      <rdakit:toolkitLabel xml:lang="en">cartographic dataset</rdakit:toolkitLabel>
      <rdakit:toolkitLabel xml:lang="fr">données cartographiques</rdakit:toolkitLabel>
      <rdakit:toolkitDefinition xml:lang="en">A content type consisting of cartographic content expressed through a digitally encoded dataset intended to be processed by a computer.</rdakit:toolkitDefinition>
      <rdakit:toolkitDefinition xml:lang="fr">Type de contenu qui consiste en contenu cartographique exprimé au moyen de données encodées numériquement en vue d’un traitement par ordinateur.</rdakit:toolkitDefinition>
      <rdakit:toolkitLabel xml:lang="de">Kartografischer Datensatz</rdakit:toolkitLabel>
      <rdakit:toolkitDefinition xml:lang="de">Ein Inhaltstyp, der aus kartografischem Inhalt besteht, der über einen digital kodierten Datenbestand ausgedrückt wird, der für die Verarbeitung durch einen Computer konzipiert ist.</rdakit:toolkitDefinition>
      <rdakit:toolkitLabel xml:lang="es">conjunto de datos cartográficos</rdakit:toolkitLabel>
      <rdakit:toolkitDefinition xml:lang="es">Contenido cartográfico expresado mediante un conjunto de datos codificados digitalmente para ser procesados por un computador.</rdakit:toolkitDefinition>
      <skos:prefLabel xml:lang="zh">地图数据集</skos:prefLabel>
      <rdakit:toolkitLabel xml:lang="zh">地图数据集</rdakit:toolkitLabel>
      <skos:definition xml:lang="zh">经计算机处理的、以数字编码数据集所表达的地图内容。</skos:definition>
      <rdakit:toolkitDefinition xml:lang="zh">经计算机处理的、以数字编码数据集所表达的地图内容。</rdakit:toolkitDefinition>
      <skos:scopeNote xml:lang="es">No incluye datos cartográficos destinados a ser percibidos en forma de una imagen o forma tridimensional.</skos:scopeNote>
      <skos:prefLabel xml:lang="nl">cartografische dataset</skos:prefLabel>
      <rdakit:toolkitLabel xml:lang="nl">cartografische dataset</rdakit:toolkitLabel>
      <skos:definition xml:lang="nl">Cartografische content uitgedrukt door een digitaal gecodeerde dataset bedoeld om verwerkt te worden door een computer.</skos:definition>
      <rdakit:toolkitDefinition xml:lang="nl">Cartografische content uitgedrukt door een digitaal gecodeerde dataset bedoeld om verwerkt te worden door een computer.</rdakit:toolkitDefinition>
      <skos:prefLabel xml:lang="it">dataset cartografico</skos:prefLabel>
      <rdakit:toolkitLabel xml:lang="it">dataset cartografico</rdakit:toolkitLabel>
      <skos:definition xml:lang="it">Contenuto cartografico espresso mediante un dataset codificato in forma digitale e destinato a essere elaborato mediante un computer.</skos:definition>
      <rdakit:toolkitDefinition xml:lang="it">Contenuto cartografico espresso mediante un dataset codificato in forma digitale e destinato a essere elaborato mediante un computer.</rdakit:toolkitDefinition>
      <skos:prefLabel xml:lang="fi">kartografinen data</skos:prefLabel>
      <rdakit:toolkitLabel xml:lang="fi">kartografinen data</rdakit:toolkitLabel>
      <skos:definition xml:lang="fi">Digitaalisesti koodattuna datana esitetty kartografinen sisältö, joka on tarkoitettu tietokoneen käsiteltäväksi.</skos:definition>
      <rdakit:toolkitDefinition xml:lang="fi">Digitaalisesti koodattuna datana esitetty kartografinen sisältö, joka on tarkoitettu tietokoneen käsiteltäväksi.</rdakit:toolkitDefinition>
      <skos:prefLabel xml:lang="he">קבוצת נתונים קרטוגרפיים</skos:prefLabel>
      <rdakit:toolkitLabel xml:lang="he">קבוצת נתונים קרטוגרפיים</rdakit:toolkitLabel>
      <skos:definition xml:lang="he">סוג תוכן המכיל תוכן קרטוגרפי אשר קיבל את ביטויו באמצעות קבוצת נתונים דיגיטליים, ומיועד לעיבוד על ידי מחשב.</skos:definition>
      <rdakit:toolkitDefinition xml:lang="he">סוג תוכן המכיל תוכן קרטוגרפי אשר קיבל את ביטויו באמצעות קבוצת נתונים דיגיטליים, ומיועד לעיבוד על ידי מחשב.</rdakit:toolkitDefinition>
      <skos:scopeNote xml:lang="he">לא כולל נתונים קרטוגרפיים המיועדים לצפייה כתמונה או כצורה תלת-ממדית.</skos:scopeNote>
      <skos:prefLabel xml:lang="ar">مجموعة بيانات خرائطية</skos:prefLabel>
      <skos:prefLabel xml:lang="sv">kartografiskt dataset</skos:prefLabel>
      <rdakit:toolkitLabel xml:lang="sv">kartografiskt dataset</rdakit:toolkitLabel>
      <skos:prefLabel xml:lang="vi">bộ dữ liệu bản đồ</skos:prefLabel>
      <rdakit:toolkitLabel xml:lang="vi">bộ dữ liệu bản đồ</rdakit:toolkitLabel>
      <skos:definition xml:lang="vi">Loại nội dung gồm có nội dung bản đồ được biểu hiện qua bộ dữ liệu mã hoá kỹ thuật số để xử lý bằng máy tính.</skos:definition>
      <rdakit:toolkitDefinition xml:lang="vi">Loại nội dung gồm có nội dung bản đồ được biểu hiện qua bộ dữ liệu mã hoá kỹ thuật số để xử lý bằng máy tính.</rdakit:toolkitDefinition>
      <skos:scopeNote xml:lang="vi">Bộ dữ liệu bản đồ không bao gồm nội dung bản đồ để nhận biết dưới hình thái của hình ảnh hoặc thình thái ba chiều.</skos:scopeNote>
      <skos:scopeNote xml:lang="de">Ein kartografischer Datensatz beinhaltet keine kartografischen Daten, die in Form eines Bildes oder einer dreidimensionalen Form wahrgenommen werden sollen.</skos:scopeNote>
      <skos:prefLabel xml:lang="da">kartografisk datasæt</skos:prefLabel>
      <rdakit:toolkitLabel xml:lang="da">kartografisk datasæt</rdakit:toolkitLabel>
      <skos:definition xml:lang="da">Indholdstype der består af kartografisk indhold udtrykt gennem et digitalt kodet datasæt mhp. at blive behandlet af en computer.</skos:definition>
      <rdakit:toolkitDefinition xml:lang="da">Indholdstype der består af kartografisk indhold udtrykt gennem et digitalt kodet datasæt mhp. at blive behandlet af en computer.</rdakit:toolkitDefinition>
      <skos:scopeNote xml:lang="da">Kartografisk datasæt omfatter ikke kartografiske data mhp. at fornemmes som et billede eller i tredimensional form.</skos:scopeNote>
      <skos:scopeNote xml:lang="fi">Kartografinen datasetti ei sisällä kartta-aineistoa, joka on tarkoitettu  tarkasteltavaksi kuvana tai kolmiulotteisena muotona.</skos:scopeNote>
      <skos:scopeNote xml:lang="fr">Ne comprend pas les données cartographiques destinées à être perçues sous la forme d’une image ou d’une forme tridimensionnelle.</skos:scopeNote>
      <skos:prefLabel xml:lang="no">kartografisk datasett</skos:prefLabel>
      <rdakit:toolkitLabel xml:lang="no">kartografisk datasett</rdakit:toolkitLabel>
      <skos:definition xml:lang="no">En innholdstype som består av kartografisk innhold uttrykt gjennom et digitalt kodet datasett som skal behandles av en datamaskin.</skos:definition>
      <rdakit:toolkitDefinition xml:lang="no">En innholdstype som består av kartografisk innhold uttrykt gjennom et digitalt kodet datasett som skal behandles av en datamaskin.</rdakit:toolkitDefinition>
      <skos:scopeNote xml:lang="no">Et kartografisk datasett utelukker kartografiske data som skal oppfattes som et bilde eller en tredimensjonal form.</skos:scopeNote>
    </skos:Concept>
<!-- Concept: cartographic image  -->
    <skos:Concept rdf:about="http://rdaregistry.info/termList/RDAContentType/1002" xml:lang="en">
      <skos:inScheme rdf:resource="http://rdaregistry.info/termList/RDAContentType"/>
      <reg:status rdf:resource="http://metadataregistry.org/uri/RegStatus/1001"/>
      <reg:identifier rdf:resource="http://metadataregistry.org/concepts/511"/>
      <skos:prefLabel xml:lang="en">cartographic image</skos:prefLabel>
      <skos:definition xml:lang="en">A content type consisting of cartographic content expressed through line, shape, shading, etc., intended to be perceived visually as a still image or images in two dimensions.</skos:definition>
      <skos:prefLabel xml:lang="de">Kartografisches Bild</skos:prefLabel>
      <skos:definition xml:lang="de">Ein Inhaltstyp, der aus kartografischem Inhalt besteht, der durch Linie, Form, Schattierung usw. ausgedrückt wird und konzipiert ist, um visuell zweidimensional als unbewegtes Bild oder Bilder wahrgenommen zu werden.</skos:definition>
      <skos:scopeNote xml:lang="en">Maps, views, atlases, remote-sensing images, etc., are included.</skos:scopeNote>
	    <skos:related rdf:resource="http://rdaregistry.info/termList/RDAContentType/1014"/>
      <skos:prefLabel xml:lang="fr">image cartographique</skos:prefLabel>
      <skos:definition xml:lang="fr">Type de contenu qui consiste en contenu cartographique exprimé au moyen de lignes, de contours, d’estompage, etc. destinés à être perçus visuellement comme une ou plusieurs images fixes en deux dimensions.</skos:definition>
      <skos:scopeNote xml:lang="fr">Comprend les cartes, les vues, les atlas, les images de télédétection, etc.</skos:scopeNote>
      <skos:scopeNote xml:lang="de">Dazu gehören Karten, Ansichten, Atlanten, Fernerkundungsbilder usw.</skos:scopeNote>
      <skos:prefLabel xml:lang="es">imagen cartográfica</skos:prefLabel>
      <skos:definition xml:lang="es">Contenido cartográfico expresado mediante líneas, forma, sombreado, etc., pensado para ser percibido visualmente como una imagen fija o imágenes en dos dimensiones.</skos:definition>
      <skos:scopeNote xml:lang="es">Incluye mapas, visores, atlas, imágenes de detección remota, etc.</skos:scopeNote>
      <rdakit:toolkitLabel xml:lang="en">cartographic image</rdakit:toolkitLabel>
      <rdakit:toolkitLabel xml:lang="fr">image cartographique</rdakit:toolkitLabel>
      <rdakit:toolkitDefinition xml:lang="en">A content type consisting of cartographic content expressed through line, shape, shading, etc., intended to be perceived visually as a still image or images in two dimensions.</rdakit:toolkitDefinition>
      <rdakit:toolkitDefinition xml:lang="fr">Type de contenu qui consiste en contenu cartographique exprimé au moyen de lignes, de contours, d’estompage, etc. destinés à être perçus visuellement comme une ou plusieurs images fixes en deux dimensions.</rdakit:toolkitDefinition>
      <rdakit:toolkitLabel xml:lang="de">Kartografisches Bild</rdakit:toolkitLabel>
      <rdakit:toolkitDefinition xml:lang="de">Ein Inhaltstyp, der aus kartografischem Inhalt besteht, der durch Linie, Form, Schattierung usw. ausgedrückt wird und konzipiert ist, um visuell zweidimensional als unbewegtes Bild oder Bilder wahrgenommen zu werden.</rdakit:toolkitDefinition>
      <rdakit:toolkitLabel xml:lang="es">imagen cartográfica</rdakit:toolkitLabel>
      <rdakit:toolkitDefinition xml:lang="es">Contenido cartográfico expresado mediante líneas, forma, sombreado, etc., pensado para ser percibido visualmente como una imagen fija o imágenes en dos dimensiones.</rdakit:toolkitDefinition>
      <skos:prefLabel xml:lang="zh">地图图像</skos:prefLabel>
      <rdakit:toolkitLabel xml:lang="zh">地图图像</rdakit:toolkitLabel>
      <skos:definition xml:lang="zh">以线条、形状、阴影等表达的，旨在作为一个或多个二维静态图像通过视觉感知的地图内容。</skos:definition>
      <rdakit:toolkitDefinition xml:lang="zh">以线条、形状、阴影等表达的，旨在作为一个或多个二维静态图像通过视觉感知的地图内容。</rdakit:toolkitDefinition>
      <skos:scopeNote xml:lang="zh">包括地图、视图、地图集、遥感图像等。</skos:scopeNote>
      <skos:prefLabel xml:lang="nl">cartografische afbeelding</skos:prefLabel>
      <rdakit:toolkitLabel xml:lang="nl">cartografische afbeelding</rdakit:toolkitLabel>
      <skos:definition xml:lang="nl">Cartografische content uitgedrukt door lijnen, vormen, schaduw etc., bedoeld om visueel waar te nemen als een stilstaand beeld of beelden in twee dimensies.</skos:definition>
      <rdakit:toolkitDefinition xml:lang="nl">Cartografische content uitgedrukt door lijnen, vormen, schaduw etc., bedoeld om visueel waar te nemen als een stilstaand beeld of beelden in twee dimensies.</rdakit:toolkitDefinition>
      <skos:prefLabel xml:lang="it">immagine cartografica</skos:prefLabel>
      <rdakit:toolkitLabel xml:lang="it">immagine cartografica</rdakit:toolkitLabel>
      <skos:definition xml:lang="it">Contenuto cartografico espresso mediante linee, forme, ombreggiature, etc. percepibili con la vista come un'immagine fissa o in due dimensioni.</skos:definition>
      <rdakit:toolkitDefinition xml:lang="it">Contenuto cartografico espresso mediante linee, forme, ombreggiature, etc. percepibili con la vista come un'immagine fissa o in due dimensioni.</rdakit:toolkitDefinition>
      <skos:scopeNote xml:lang="it">Include carte geografiche, vedute, atlanti, immagini aeree, etc.</skos:scopeNote>
      <skos:prefLabel xml:lang="fi">kartografinen kuva</skos:prefLabel>
      <rdakit:toolkitLabel xml:lang="fi">kartografinen kuva</rdakit:toolkitLabel>
      <skos:definition xml:lang="fi">Viivana, muotona, varjostuksena tms. esitetty kartografinen sisältö, joka on tarkoitettu katsottavaksi kaksiulotteisena stillkuvana tai -kuvina.</skos:definition>
      <rdakit:toolkitDefinition xml:lang="fi">Viivana, muotona, varjostuksena tms. esitetty kartografinen sisältö, joka on tarkoitettu katsottavaksi kaksiulotteisena stillkuvana tai -kuvina.</rdakit:toolkitDefinition>
      <skos:scopeNote xml:lang="fi">Esimerkiksi kartat, näkymäkartat, kartastot, kaukokartoituskuvat jne.</skos:scopeNote>
      <skos:prefLabel xml:lang="he">תמונה קרטוגרפית</skos:prefLabel>
      <rdakit:toolkitLabel xml:lang="he">תמונה קרטוגרפית</rdakit:toolkitLabel>
      <skos:definition xml:lang="he">סוג תוכן המכיל תוכן קרטוגרפי אשר קיבל את ביטויו באמצעות קווים, צורות, גיוון צבעים וכד', ומיועד לצפייה כתמונה (או תמונות) דו-ממדית.</skos:definition>
      <rdakit:toolkitDefinition xml:lang="he">סוג תוכן המכיל תוכן קרטוגרפי אשר קיבל את ביטויו באמצעות קווים, צורות, גיוון צבעים וכד', ומיועד לצפייה כתמונה (או תמונות) דו-ממדית.</rdakit:toolkitDefinition>
      <skos:scopeNote xml:lang="he">כולל מפות, תצפיות, אטלסים, תמונת חִּישת רחק, וכו'.</skos:scopeNote>
      <skos:prefLabel xml:lang="ar">صورة خرائطية</skos:prefLabel>
      <skos:prefLabel xml:lang="sv">kartografisk bild</skos:prefLabel>
      <rdakit:toolkitLabel xml:lang="sv">kartografisk bild</rdakit:toolkitLabel>
      <skos:prefLabel xml:lang="vi">hình ảnh bản đồ</skos:prefLabel>
      <rdakit:toolkitLabel xml:lang="vi">hình ảnh bản đồ</rdakit:toolkitLabel>
      <skos:definition xml:lang="vi">Loại nội dung gồn có nội dung bản đồ được biểu hiện qua đường nét, hình dạng, hình bóng v.v... để nhận biết bằng thị giác như là hình ảnh tĩnh hoặc hình ảnh hai chiều.</skos:definition>
      <rdakit:toolkitDefinition xml:lang="vi">Loại nội dung gồn có nội dung bản đồ được biểu hiện qua đường nét, hình dạng, hình bóng v.v... để nhận biết bằng thị giác như là hình ảnh tĩnh hoặc hình ảnh hai chiều.</rdakit:toolkitDefinition>
      <skos:scopeNote xml:lang="vi">Bản đồ, quang cảnh, hình ảnh cảm nhận từ xa, v.v..., được bao gồm</skos:scopeNote>
      <skos:prefLabel xml:lang="da">kartografisk indhold</skos:prefLabel>
      <rdakit:toolkitLabel xml:lang="da">kartografisk indhold</rdakit:toolkitLabel>
      <skos:definition xml:lang="da">Indholdstype der består af kartografisk indhold udtrykt som en linje, figur, skravering etc. mhp. at blive opfattet visuelt som et eller flere todimensionale billeder.</skos:definition>
      <rdakit:toolkitDefinition xml:lang="da">Indholdstype der består af kartografisk indhold udtrykt som en linje, figur, skravering etc. mhp. at blive opfattet visuelt som et eller flere todimensionale billeder.</rdakit:toolkitDefinition>
      <skos:scopeNote xml:lang="da">Kort, perspektiver, atlasser, remote-sensing billeder etc. er omfattet.</skos:scopeNote>
      <skos:prefLabel xml:lang="no">kartografisk bilde</skos:prefLabel>
      <rdakit:toolkitLabel xml:lang="no">kartografisk bilde</rdakit:toolkitLabel>
      <skos:definition xml:lang="no">En innholdstype som består av kartografisk innhold uttrykt gjennom linjer, former, skyggelegging etc., som skal oppfattes visuelt som ett eller flere stillbilder i to dimensjoner.</skos:definition>
      <rdakit:toolkitDefinition xml:lang="no">En innholdstype som består av kartografisk innhold uttrykt gjennom linjer, former, skyggelegging etc., som skal oppfattes visuelt som ett eller flere stillbilder i to dimensjoner.</rdakit:toolkitDefinition>
      <skos:scopeNote xml:lang="no">Kart, projeksjoner, atlas, fjernanalysebilder, etc. er inkludert.</skos:scopeNote>
    </skos:Concept>
<!-- Concept: cartographic moving image  -->
    <skos:Concept rdf:about="http://rdaregistry.info/termList/RDAContentType/1003" xml:lang="en">
      <skos:inScheme rdf:resource="http://rdaregistry.info/termList/RDAContentType"/>
      <reg:status rdf:resource="http://metadataregistry.org/uri/RegStatus/1001"/>
      <reg:identifier rdf:resource="http://metadataregistry.org/concepts/512"/>
      <skos:prefLabel xml:lang="en">cartographic moving image</skos:prefLabel>
      <skos:definition xml:lang="en">A content type consisting of cartographic content expressed through images intended to be perceived as moving, in two dimensions.</skos:definition>
      <skos:prefLabel xml:lang="de">Kartografisches bewegtes Bild</skos:prefLabel>
      <skos:definition xml:lang="de">Ein Inhaltstyp, der aus kartografischem Inhalt besteht, der durch Bilder ausgedrückt wird und konzipiert ist, um als zweidimensionale Bewegung wahrgenommen zu werden.</skos:definition>
      <skos:scopeNote xml:lang="en">Satellite images of the Earth or other celestial bodies in motion are included.</skos:scopeNote>
	    <skos:related rdf:resource="http://rdaregistry.info/termList/RDAContentType/1023"/>
      <skos:scopeNote xml:lang="de">Dazu gehören Satellitenbilder der Erde oder anderer Himmelskörper, die in Bewegung sind.</skos:scopeNote>
      <skos:prefLabel xml:lang="fr">image cartographique animée</skos:prefLabel>
      <skos:definition xml:lang="fr">Type de contenu qui consiste en contenu cartographique exprimé au moyen d’images destinées à être perçues comme animées en deux dimensions.</skos:definition>
      <skos:scopeNote xml:lang="fr">Comprend les images satellite de la Terre ou d’autres corps célestes en mouvement.</skos:scopeNote>
      <skos:prefLabel xml:lang="es">imagen cartográfica en movimiento</skos:prefLabel>
      <skos:definition xml:lang="es">Contenido cartográfico expresado mediante imágenes proyectadas para ser percibidas en movimiento, en dos dimensiones.</skos:definition>
      <skos:scopeNote xml:lang="es">Incluye imágenes de satélite de la Tierra u otros cuerpos celestes en movimiento.</skos:scopeNote>
      <rdakit:toolkitLabel xml:lang="en">cartographic moving image</rdakit:toolkitLabel>
      <rdakit:toolkitLabel xml:lang="fr">image cartographique animée</rdakit:toolkitLabel>
      <rdakit:toolkitDefinition xml:lang="en">A content type consisting of cartographic content expressed through images intended to be perceived as moving, in two dimensions.</rdakit:toolkitDefinition>
      <rdakit:toolkitDefinition xml:lang="fr">Type de contenu qui consiste en contenu cartographique exprimé au moyen d’images destinées à être perçues comme animées en deux dimensions.</rdakit:toolkitDefinition>
      <rdakit:toolkitLabel xml:lang="de">Kartografisches bewegtes Bild</rdakit:toolkitLabel>
      <rdakit:toolkitDefinition xml:lang="de">Ein Inhaltstyp, der aus kartografischem Inhalt besteht, der durch Bilder ausgedrückt wird und konzipiert ist, um als zweidimensionale Bewegung wahrgenommen zu werden.</rdakit:toolkitDefinition>
      <rdakit:toolkitLabel xml:lang="es">imagen cartográfica en movimiento</rdakit:toolkitLabel>
      <rdakit:toolkitDefinition xml:lang="es">Contenido cartográfico expresado mediante imágenes proyectadas para ser percibidas en movimiento, en dos dimensiones.</rdakit:toolkitDefinition>
      <skos:prefLabel xml:lang="zh">地图的动态图像</skos:prefLabel>
      <rdakit:toolkitLabel xml:lang="zh">地图的动态图像</rdakit:toolkitLabel>
      <skos:definition xml:lang="zh">以图像表达的，旨在作为二维动态图像感知的地图内容。</skos:definition>
      <rdakit:toolkitDefinition xml:lang="zh">以图像表达的，旨在作为二维动态图像感知的地图内容。</rdakit:toolkitDefinition>
      <skos:scopeNote xml:lang="zh">包括运动中的地球或其他天体的卫星图像。</skos:scopeNote>
	    <skos:related rdf:resource="http://rdaregistry.info/termList/RDAContentType/1022"/>
      <skos:prefLabel xml:lang="nl">cartografisch bewegend beeld</skos:prefLabel>
      <rdakit:toolkitLabel xml:lang="nl">cartografisch bewegend beeld</rdakit:toolkitLabel>
      <skos:definition xml:lang="nl">Cartografische content uitgedrukt door beelden bedoeld om waar te nemen als bewegend in twee dimensies.</skos:definition>
      <rdakit:toolkitDefinition xml:lang="nl">Cartografische content uitgedrukt door beelden bedoeld om waar te nemen als bewegend in twee dimensies.</rdakit:toolkitDefinition>
      <skos:prefLabel xml:lang="it">immagine in movimento cartografica</skos:prefLabel>
      <rdakit:toolkitLabel xml:lang="it">immagine in movimento cartografica</rdakit:toolkitLabel>
      <skos:definition xml:lang="it">Contenuto cartografico espresso mediante immagini percepibili come in movimento, in due dimensioni.</skos:definition>
      <rdakit:toolkitDefinition xml:lang="it">Contenuto cartografico espresso mediante immagini percepibili come in movimento, in due dimensioni.</rdakit:toolkitDefinition>
      <skos:scopeNote xml:lang="it">Include le immagini di telerilevamento della Terra e di altri corpi celesti in movimento.</skos:scopeNote>
      <skos:prefLabel xml:lang="fi">kartografinen liikkuva kuva</skos:prefLabel>
      <rdakit:toolkitLabel xml:lang="fi">kartografinen liikkuva kuva</rdakit:toolkitLabel>
      <skos:definition xml:lang="fi">Kaksiulotteisena liikkuvana kuvana esitetty kartografinen sisältö.</skos:definition>
      <rdakit:toolkitDefinition xml:lang="fi">Kaksiulotteisena liikkuvana kuvana esitetty kartografinen sisältö.</rdakit:toolkitDefinition>
      <skos:scopeNote xml:lang="fi">Esimerkiksi liikkuvat satelliittikuvat maasta tai muista taivaankappaleista.</skos:scopeNote>
      <skos:prefLabel xml:lang="he">תמונת-נוע קרטוגרפית</skos:prefLabel>
      <rdakit:toolkitLabel xml:lang="he">תמונת-נוע קרטוגרפית</rdakit:toolkitLabel>
      <skos:definition xml:lang="he">סוג תוכן המכיל תוכן קרטוגרפי אשר קיבל את ביטויו באמצעות תמונות נעות, דו-ממדיות.</skos:definition>
      <rdakit:toolkitDefinition xml:lang="he">סוג תוכן המכיל תוכן קרטוגרפי אשר קיבל את ביטויו באמצעות תמונות נעות, דו-ממדיות.</rdakit:toolkitDefinition>
      <skos:scopeNote xml:lang="he">כולל תמונות לווין של כדור הארץ או של גופים שמימיים אחרים בתנועה.</skos:scopeNote>
      <skos:prefLabel xml:lang="ar">صورة متحركة خرائطية</skos:prefLabel>
      <skos:prefLabel xml:lang="sv">kartografisk rörlig bild</skos:prefLabel>
      <rdakit:toolkitLabel xml:lang="sv">kartografisk rörlig bild</rdakit:toolkitLabel>
      <skos:prefLabel xml:lang="vi">hình ảnh động bản đồ</skos:prefLabel>
      <rdakit:toolkitLabel xml:lang="vi">hình ảnh động bản đồ</rdakit:toolkitLabel>
      <skos:definition xml:lang="vi">Loại nội dung gồm có nội dung bản đồ được biểu hiện qua hình ảnh để nhận biết như là hình ảnh động hai chiều.</skos:definition>
      <rdakit:toolkitDefinition xml:lang="vi">Loại nội dung gồm có nội dung bản đồ được biểu hiện qua hình ảnh để nhận biết như là hình ảnh động hai chiều.</rdakit:toolkitDefinition>
      <skos:scopeNote xml:lang="vi">Hình ảnh vệ tinh về chuyển động của trái đất và các thiên thể khác được bao gồm.</skos:scopeNote>
      <skos:prefLabel xml:lang="da">levende kartografisk billede</skos:prefLabel>
      <rdakit:toolkitLabel xml:lang="da">levende kartografisk billede</rdakit:toolkitLabel>
      <skos:definition xml:lang="da">Indholdstype der består af kartografisk indhold udtrykt gennem billeder mhp. at blive opfattet som værende i bevægelse, i to dimensioner.</skos:definition>
      <rdakit:toolkitDefinition xml:lang="da">Indholdstype der består af kartografisk indhold udtrykt gennem billeder mhp. at blive opfattet som værende i bevægelse, i to dimensioner.</rdakit:toolkitDefinition>
      <skos:scopeNote xml:lang="da">Satellitbilleder af Jorden og andre himmellegemer i bevægelse er omfattet.</skos:scopeNote>
      <skos:prefLabel xml:lang="no">kartografisk levende bilde</skos:prefLabel>
      <rdakit:toolkitLabel xml:lang="no">kartografisk levende bilde</rdakit:toolkitLabel>
      <skos:definition xml:lang="no">En innholdstype som består av kartografisk innhold uttrykt gjennom levende bilder som skal oppfattes todimensjonalt.</skos:definition>
      <rdakit:toolkitDefinition xml:lang="no">En innholdstype som består av kartografisk innhold uttrykt gjennom levende bilder som skal oppfattes todimensjonalt.</rdakit:toolkitDefinition>
      <skos:scopeNote xml:lang="no">Satellittbilder av Jorden eller andre himmellegemer i bevegelse er inkludert.</skos:scopeNote>
    </skos:Concept>
<!-- Concept: cartographic tactile image  -->
    <skos:Concept rdf:about="http://rdaregistry.info/termList/RDAContentType/1004" xml:lang="en">
      <skos:inScheme rdf:resource="http://rdaregistry.info/termList/RDAContentType"/>
      <reg:status rdf:resource="http://metadataregistry.org/uri/RegStatus/1001"/>
      <reg:identifier rdf:resource="http://metadataregistry.org/concepts/513"/>
      <skos:prefLabel xml:lang="en">cartographic tactile image</skos:prefLabel>
      <skos:definition xml:lang="en">A content type consisting of cartographic content expressed through line, shape, and/or other forms, intended to be perceived through touch as a still image in two dimensions.</skos:definition>
      <skos:prefLabel xml:lang="de">Kartografisches taktiles Bild</skos:prefLabel>
      <skos:definition xml:lang="de">Ein Inhaltstyp, der aus kartografischem Inhalt besteht, der durch Linie, Form und/oder andere Gestaltungen ausgedrückt wird und konzipiert ist, um über den Tastsinn zweidimensional als unbewegtes Bild wahrgenommen zu werden.</skos:definition>
	    <skos:related rdf:resource="http://rdaregistry.info/termList/RDAContentType/1001"/>
      <skos:prefLabel xml:lang="fr">image cartographique tactile</skos:prefLabel>
      <skos:definition xml:lang="fr">Type de contenu qui consiste en contenu cartographique exprimé au moyen de lignes, de contours et/ou d’autres formes destinés à être perçus au toucher comme une image fixe en deux dimensions.</skos:definition>
      <skos:prefLabel xml:lang="es">imagen cartográfica táctil</skos:prefLabel>
      <skos:definition xml:lang="es">Contenido cartográfico expresado mediante líneas, forma, y/u otras formas, pensado para ser percibido mediante el tacto como imagen fija en dos dimensiones.</skos:definition>
      <rdakit:toolkitLabel xml:lang="en">cartographic tactile image</rdakit:toolkitLabel>
      <rdakit:toolkitLabel xml:lang="fr">image cartographique tactile</rdakit:toolkitLabel>
      <rdakit:toolkitDefinition xml:lang="en">A content type consisting of cartographic content expressed through line, shape, and/or other forms, intended to be perceived through touch as a still image in two dimensions.</rdakit:toolkitDefinition>
      <rdakit:toolkitDefinition xml:lang="fr">Type de contenu qui consiste en contenu cartographique exprimé au moyen de lignes, de contours et/ou d’autres formes destinés à être perçus au toucher comme une image fixe en deux dimensions.</rdakit:toolkitDefinition>
      <rdakit:toolkitLabel xml:lang="de">Kartografisches taktiles Bild</rdakit:toolkitLabel>
      <rdakit:toolkitDefinition xml:lang="de">Ein Inhaltstyp, der aus kartografischem Inhalt besteht, der durch Linie, Form und/oder andere Gestaltungen ausgedrückt wird und konzipiert ist, um über den Tastsinn zweidimensional als unbewegtes Bild wahrgenommen zu werden.</rdakit:toolkitDefinition>
      <rdakit:toolkitLabel xml:lang="es">imagen cartográfica táctil</rdakit:toolkitLabel>
      <rdakit:toolkitDefinition xml:lang="es">Contenido cartográfico expresado mediante líneas, forma, y/u otras formas, pensado para ser percibido mediante el tacto como imagen fija en dos dimensiones.</rdakit:toolkitDefinition>
      <skos:prefLabel xml:lang="zh">地图的触摸图像</skos:prefLabel>
      <rdakit:toolkitLabel xml:lang="zh">地图的触摸图像</rdakit:toolkitLabel>
      <skos:definition xml:lang="zh">以线条、形状和/或其他形式表达的，旨在作为二维静态图像通过触觉感知的地图内容。</skos:definition>
      <rdakit:toolkitDefinition xml:lang="zh">以线条、形状和/或其他形式表达的，旨在作为二维静态图像通过触觉感知的地图内容。</rdakit:toolkitDefinition>
      <skos:prefLabel xml:lang="nl">cartografische tactiele afbeelding</skos:prefLabel>
      <rdakit:toolkitLabel xml:lang="nl">cartografische tactiele afbeelding</rdakit:toolkitLabel>
      <skos:definition xml:lang="nl">Cartografische content uitgedrukt door lijnen, vormen etc., bedoeld om waar te nemen door aanraking als een stilstaand beeld in twee dimensies.</skos:definition>
      <rdakit:toolkitDefinition xml:lang="nl">Cartografische content uitgedrukt door lijnen, vormen etc., bedoeld om waar te nemen door aanraking als een stilstaand beeld in twee dimensies.</rdakit:toolkitDefinition>
      <skos:prefLabel xml:lang="it">immagine tattile cartografica</skos:prefLabel>
      <rdakit:toolkitLabel xml:lang="it">immagine tattile cartografica</rdakit:toolkitLabel>
      <skos:definition xml:lang="it">Contenuto cartografico mediante linee, figure e/o altre forme, percepibili mediante il tatto come immagini fisse in due dimensioni.</skos:definition>
      <rdakit:toolkitDefinition xml:lang="it">Contenuto cartografico mediante linee, figure e/o altre forme, percepibili mediante il tatto come immagini fisse in due dimensioni.</rdakit:toolkitDefinition>
      <skos:prefLabel xml:lang="fi">kartografinen taktiili kuva</skos:prefLabel>
      <rdakit:toolkitLabel xml:lang="fi">kartografinen taktiili kuva</rdakit:toolkitLabel>
      <skos:definition xml:lang="fi">Viivoina, muotoina tms. esitetty kartografinen sisältö, joka on tarkoitettu kosketeltavaksi kaksiulotteisena stillkuvana tai -kuvina.</skos:definition>
      <rdakit:toolkitDefinition xml:lang="fi">Viivoina, muotoina tms. esitetty kartografinen sisältö, joka on tarkoitettu kosketeltavaksi kaksiulotteisena stillkuvana tai -kuvina.</rdakit:toolkitDefinition>
      <skos:prefLabel xml:lang="he">תמונה קרטוגרפית מישושית</skos:prefLabel>
      <rdakit:toolkitLabel xml:lang="he">תמונה קרטוגרפית מישושית</rdakit:toolkitLabel>
      <skos:definition xml:lang="he">סוג תוכן המכיל תוכן קרטוגרפי אשר קיבל את ביטויו באמצעות קווים, צורות וכד', ומיועד למישוש כתמונה (או תמונות) דו-ממדית.</skos:definition>
      <rdakit:toolkitDefinition xml:lang="he">סוג תוכן המכיל תוכן קרטוגרפי אשר קיבל את ביטויו באמצעות קווים, צורות וכד', ומיועד למישוש כתמונה (או תמונות) דו-ממדית.</rdakit:toolkitDefinition>
      <skos:prefLabel xml:lang="ar">صورة لمسية خرائطية</skos:prefLabel>
      <skos:prefLabel xml:lang="sv">kartografisk taktil bild</skos:prefLabel>
      <rdakit:toolkitLabel xml:lang="sv">kartografisk taktil bild</rdakit:toolkitLabel>
      <skos:prefLabel xml:lang="vi">hình ảnh xúc giác bản đồ</skos:prefLabel>
      <rdakit:toolkitLabel xml:lang="vi">hình ảnh xúc giác bản đồ</rdakit:toolkitLabel>
      <skos:definition xml:lang="vi">Loại nội dung gồm có nội dung bản đồ được biểu hiện qua đường nét, hình dạng, và/hoặc hình thái khác, để nhận biết qua xúc giác như là hình ảnh tĩnh hai chiều.</skos:definition>
      <rdakit:toolkitDefinition xml:lang="vi">Loại nội dung gồm có nội dung bản đồ được biểu hiện qua đường nét, hình dạng, và/hoặc hình thái khác, để nhận biết qua xúc giác như là hình ảnh tĩnh hai chiều.</rdakit:toolkitDefinition>
      <skos:prefLabel xml:lang="da">taktilt kartografisk billede</skos:prefLabel>
      <rdakit:toolkitLabel xml:lang="da">taktilt kartografisk billede</rdakit:toolkitLabel>
      <skos:definition xml:lang="da">Indholdstyper der består af kartografisk indhold udtrykt som en linje, figur og/eller andre former mhp. at blive opfattet ved berøring som et todimensionalt billede.</skos:definition>
      <rdakit:toolkitDefinition xml:lang="da">Indholdstyper der består af kartografisk indhold udtrykt som en linje, figur og/eller andre former mhp. at blive opfattet ved berøring som et todimensionalt billede.</rdakit:toolkitDefinition>
      <skos:prefLabel xml:lang="no">kartografisk taktilt bilde</skos:prefLabel>
      <rdakit:toolkitLabel xml:lang="no">kartografisk taktilt bilde</rdakit:toolkitLabel>
      <skos:definition xml:lang="no">En innholdstype som består av kartografisk innhold uttrykt gjennom linjer og/eller andre former, som skal oppfattes gjennom berøring som et stillbilde i to dimensjoner.</skos:definition>
      <rdakit:toolkitDefinition xml:lang="no">En innholdstype som består av kartografisk innhold uttrykt gjennom linjer og/eller andre former, som skal oppfattes gjennom berøring som et stillbilde i to dimensjoner.</rdakit:toolkitDefinition>
    </skos:Concept>
<!-- Concept: cartographic tactile three-dimensional form  -->
    <skos:Concept rdf:about="http://rdaregistry.info/termList/RDAContentType/1005" xml:lang="en">
      <skos:inScheme rdf:resource="http://rdaregistry.info/termList/RDAContentType"/>
      <reg:status rdf:resource="http://metadataregistry.org/uri/RegStatus/1001"/>
      <reg:identifier rdf:resource="http://metadataregistry.org/concepts/514"/>
      <skos:prefLabel xml:lang="en">cartographic tactile three-dimensional form</skos:prefLabel>
      <skos:definition xml:lang="en">A content type consisting of cartographic content expressed through a form or forms intended to be perceived through touch as a three-dimensional form or forms.</skos:definition>
      <skos:prefLabel xml:lang="de">Kartografische taktile dreidimensionale Form</skos:prefLabel>
      <skos:definition xml:lang="de">Ein Inhaltstyp, der aus kartografischem Inhalt besteht, der durch eine Form oder mehrere Formen ausgedrückt wird, und konzipiert ist, um über den Tastsinn als dreidimensionale Form oder Formen wahrgenommen zu werden.</skos:definition>
	    <skos:related rdf:resource="http://rdaregistry.info/termList/RDAContentType/1001"/>
      <skos:prefLabel xml:lang="fr">forme cartographique tridimensionnelle tactile</skos:prefLabel>
      <skos:definition xml:lang="fr">Type de contenu qui consiste en contenu cartographique exprimé au moyen d’une ou plusieurs formes destinées à être perçues au toucher comme une ou plusieurs formes tridimensionnelles.</skos:definition>
      <skos:prefLabel xml:lang="es">forma cartográfica táctil tridimensional</skos:prefLabel>
      <skos:definition xml:lang="es">Contenido cartográfico expresado mediante una forma o formas pensadas para ser percibidas mediante el tacto como una forma o formas tridimensionales.</skos:definition>
      <rdakit:toolkitLabel xml:lang="en">cartographic tactile three-dimensional form</rdakit:toolkitLabel>
      <rdakit:toolkitLabel xml:lang="fr">forme cartographique tridimensionnelle tactile</rdakit:toolkitLabel>
      <rdakit:toolkitDefinition xml:lang="en">A content type consisting of cartographic content expressed through a form or forms intended to be perceived through touch as a three-dimensional form or forms.</rdakit:toolkitDefinition>
      <rdakit:toolkitDefinition xml:lang="fr">Type de contenu qui consiste en contenu cartographique exprimé au moyen d’une ou plusieurs formes destinées à être perçues au toucher comme une ou plusieurs formes tridimensionnelles.</rdakit:toolkitDefinition>
      <rdakit:toolkitLabel xml:lang="de">Kartografische taktile dreidimensionale Form</rdakit:toolkitLabel>
      <rdakit:toolkitDefinition xml:lang="de">Ein Inhaltstyp, der aus kartografischem Inhalt besteht, der durch eine Form oder mehrere Formen ausgedrückt wird, und konzipiert ist, um über den Tastsinn als dreidimensionale Form oder Formen wahrgenommen zu werden.</rdakit:toolkitDefinition>
      <rdakit:toolkitLabel xml:lang="es">forma cartográfica táctil tridimensional</rdakit:toolkitLabel>
      <rdakit:toolkitDefinition xml:lang="es">Contenido cartográfico expresado mediante una forma o formas pensadas para ser percibidas mediante el tacto como una forma o formas tridimensionales.</rdakit:toolkitDefinition>
      <skos:prefLabel xml:lang="zh">地图的触摸三维形式</skos:prefLabel>
      <rdakit:toolkitLabel xml:lang="zh">地图的触摸三维形式</rdakit:toolkitLabel>
      <skos:definition xml:lang="zh">以一种或多种形式表达的，旨在作为一个或多个三维形式通过触觉感知的地图内容。</skos:definition>
      <rdakit:toolkitDefinition xml:lang="zh">以一种或多种形式表达的，旨在作为一个或多个三维形式通过触觉感知的地图内容。</rdakit:toolkitDefinition>
      <skos:prefLabel xml:lang="nl">cartografische tactiele driedimensionale vorm</skos:prefLabel>
      <rdakit:toolkitLabel xml:lang="nl">cartografische tactiele driedimensionale vorm</rdakit:toolkitLabel>
      <skos:definition xml:lang="nl">Cartografische content uitgedrukt door een vorm of vormen bedoeld om waar te nemen door aanraking als een driedimensionale vorm of vormen.</skos:definition>
      <rdakit:toolkitDefinition xml:lang="nl">Cartografische content uitgedrukt door een vorm of vormen bedoeld om waar te nemen door aanraking als een driedimensionale vorm of vormen.</rdakit:toolkitDefinition>
      <skos:prefLabel xml:lang="it">forma tridimensionale tattile cartografica</skos:prefLabel>
      <rdakit:toolkitLabel xml:lang="it">forma tridimensionale tattile cartografica</rdakit:toolkitLabel>
      <skos:definition xml:lang="it">Contenuto cartografico espresso mediante una o più forme percepibili mediante il tatto come forme tridimensionali.</skos:definition>
      <rdakit:toolkitDefinition xml:lang="it">Contenuto cartografico espresso mediante una o più forme percepibili mediante il tatto come forme tridimensionali.</rdakit:toolkitDefinition>
      <skos:scopeNote xml:lang="it">Include dati numerici, ambientali, etc. utilizzati da applicazioni software per calcolare medie, correlazioni, etc. o per produrre modelli, etc. ma normalmente non visualizzati nella loro forma grezza.</skos:scopeNote>
      <skos:prefLabel xml:lang="fi">kartografinen taktiili kolmiulotteinen muoto</skos:prefLabel>
      <rdakit:toolkitLabel xml:lang="fi">kartografinen taktiili kolmiulotteinen muoto</rdakit:toolkitLabel>
      <skos:definition xml:lang="fi">Muotona tai muotoina esitetty kartografinen sisältö, joka on tarkoitettu kosketeltavaksi kolmiulotteiseksi muodoksi.</skos:definition>
      <rdakit:toolkitDefinition xml:lang="fi">Muotona tai muotoina esitetty kartografinen sisältö, joka on tarkoitettu kosketeltavaksi kolmiulotteiseksi muodoksi.</rdakit:toolkitDefinition>
      <skos:prefLabel xml:lang="he">צורה קרטוגרפית מישושית תלת-ממדית</skos:prefLabel>
      <rdakit:toolkitLabel xml:lang="he">צורה קרטוגרפית מישושית תלת-ממדית</rdakit:toolkitLabel>
      <skos:definition xml:lang="he">סוג תוכן המכיל תוכן קרטוגרפי אשר קיבל את ביטויו באמצעות צורה או צורות וכד', ומיועד לתפיסה עלי ידי מישוש כצורה תלת-ממדי.</skos:definition>
      <rdakit:toolkitDefinition xml:lang="he">סוג תוכן המכיל תוכן קרטוגרפי אשר קיבל את ביטויו באמצעות צורה או צורות וכד', ומיועד לתפיסה עלי ידי מישוש כצורה תלת-ממדי.</rdakit:toolkitDefinition>
      <skos:prefLabel xml:lang="ar">شكل خرائطي لمسي ثلاثي الأبعاد</skos:prefLabel>
      <skos:prefLabel xml:lang="sv">kartografisk taktil tredimensionell form</skos:prefLabel>
      <rdakit:toolkitLabel xml:lang="sv">kartografisk taktil tredimensionell form</rdakit:toolkitLabel>
      <skos:prefLabel xml:lang="vi">hình thái ba chiều xúc giác bản đồ</skos:prefLabel>
      <rdakit:toolkitLabel xml:lang="vi">hình thái ba chiều xúc giác bản đồ</rdakit:toolkitLabel>
      <skos:definition xml:lang="vi">Loại nội dung gồm có nội dung bản đồ được biểu hiện qua một hoặc nhiều hình thái để nhận biết bằng xúc giác như một hoặc nhiều hình thái ba chiều.</skos:definition>
      <rdakit:toolkitDefinition xml:lang="vi">Loại nội dung gồm có nội dung bản đồ được biểu hiện qua một hoặc nhiều hình thái để nhận biết bằng xúc giác như một hoặc nhiều hình thái ba chiều.</rdakit:toolkitDefinition>
      <skos:prefLabel xml:lang="da">taktil kartografisk tredimensional form</skos:prefLabel>
      <rdakit:toolkitLabel xml:lang="da">taktil kartografisk tredimensional form</rdakit:toolkitLabel>
      <skos:definition xml:lang="da">Indholdstype der består af kartografisk indhold udtrykt som en eller flere former mhp. at blive opfattet ved berøring som en eller flere tredimensionale former.</skos:definition>
      <rdakit:toolkitDefinition xml:lang="da">Indholdstype der består af kartografisk indhold udtrykt som en eller flere former mhp. at blive opfattet ved berøring som en eller flere tredimensionale former.</rdakit:toolkitDefinition>
      <skos:prefLabel xml:lang="no">kartografisk taktil tredimensjonal form</skos:prefLabel>
      <rdakit:toolkitLabel xml:lang="no">kartografisk taktil tredimensjonal form</rdakit:toolkitLabel>
      <skos:definition xml:lang="no">En innholdstype som består av kartografisk innhold uttrykt gjennom én eller flere former, som skal oppfattes gjennom berøring som én eller flere tredimensjonale former.</skos:definition>
      <rdakit:toolkitDefinition xml:lang="no">En innholdstype som består av kartografisk innhold uttrykt gjennom én eller flere former, som skal oppfattes gjennom berøring som én eller flere tredimensjonale former.</rdakit:toolkitDefinition>
    </skos:Concept>
<!-- Concept: cartographic three-dimensional form  -->
    <skos:Concept rdf:about="http://rdaregistry.info/termList/RDAContentType/1006" xml:lang="en">
      <skos:inScheme rdf:resource="http://rdaregistry.info/termList/RDAContentType"/>
      <reg:status rdf:resource="http://metadataregistry.org/uri/RegStatus/1001"/>
      <reg:identifier rdf:resource="http://metadataregistry.org/concepts/515"/>
      <skos:prefLabel xml:lang="en">cartographic three-dimensional form</skos:prefLabel>
      <skos:definition xml:lang="en">A content type consisting of cartographic content expressed through a form or forms intended to be perceived visually in three-dimensions.</skos:definition>
      <skos:prefLabel xml:lang="de">Kartografische dreidimensionale Form</skos:prefLabel>
      <skos:definition xml:lang="de">Ein Inhaltstyp, der aus kartografischem Inhalt besteht, der durch eine Form oder mehrere Formen ausgedrückt wird, und konzipiert ist, um visuell dreidimensional wahrgenommen zu werden.</skos:definition>
      <skos:scopeNote xml:lang="en">Globes, relief models, etc., are included.</skos:scopeNote>
	    <skos:related rdf:resource="http://rdaregistry.info/termList/RDAContentType/1019"/>
	    <skos:related rdf:resource="http://rdaregistry.info/termList/RDAContentType/1021"/>
      <skos:scopeNote xml:lang="de">Dazu gehören Globen, Reliefmodelle usw.</skos:scopeNote>
      <skos:prefLabel xml:lang="fr">forme cartographique tridimensionnelle</skos:prefLabel>
      <skos:definition xml:lang="fr">Type de contenu qui consiste en contenu cartographique exprimé au moyen d’une ou plusieurs formes destinées à être perçues visuellement en trois dimensions.</skos:definition>
      <skos:scopeNote xml:lang="fr">Comprend les globes, les modèles en relief, etc.</skos:scopeNote>
      <skos:prefLabel xml:lang="es">forma cartográfica tridimensional</skos:prefLabel>
      <skos:definition xml:lang="es">Contenido cartográfico expresado mediante una forma o formas pensadas para ser percibidas visualmente en tres dimensiones.</skos:definition>
      <skos:scopeNote xml:lang="es">Incluye globos, modelos en relieve, etc.</skos:scopeNote>
      <rdakit:toolkitLabel xml:lang="en">cartographic three-dimensional form</rdakit:toolkitLabel>
      <rdakit:toolkitLabel xml:lang="fr">forme cartographique tridimensionnelle</rdakit:toolkitLabel>
      <rdakit:toolkitDefinition xml:lang="en">A content type consisting of cartographic content expressed through a form or forms intended to be perceived visually in three-dimensions.</rdakit:toolkitDefinition>
      <rdakit:toolkitDefinition xml:lang="fr">Type de contenu qui consiste en contenu cartographique exprimé au moyen d’une ou plusieurs formes destinées à être perçues visuellement en trois dimensions.</rdakit:toolkitDefinition>
      <rdakit:toolkitLabel xml:lang="de">Kartografische dreidimensionale Form</rdakit:toolkitLabel>
      <rdakit:toolkitDefinition xml:lang="de">Ein Inhaltstyp, der aus kartografischem Inhalt besteht, der durch eine Form oder mehrere Formen ausgedrückt wird, und konzipiert ist, um visuell dreidimensional wahrgenommen zu werden.</rdakit:toolkitDefinition>
      <rdakit:toolkitLabel xml:lang="es">forma cartográfica tridimensional</rdakit:toolkitLabel>
      <rdakit:toolkitDefinition xml:lang="es">Contenido cartográfico expresado mediante una forma o formas pensadas para ser percibidas visualmente en tres dimensiones.</rdakit:toolkitDefinition>
      <skos:prefLabel xml:lang="zh">地图的三维形式</skos:prefLabel>
      <rdakit:toolkitLabel xml:lang="zh">地图的三维形式</rdakit:toolkitLabel>
      <skos:definition xml:lang="zh">以一种或多种形式表达的，旨在通过视觉感知的三维地图内容。</skos:definition>
      <rdakit:toolkitDefinition xml:lang="zh">以一种或多种形式表达的，旨在通过视觉感知的三维地图内容。</rdakit:toolkitDefinition>
      <skos:scopeNote xml:lang="zh">包括球仪、地形模型等。</skos:scopeNote>
	    <skos:broader rdf:resource="http://rdaregistry.info/termList/RDAContentType/1021"/>
      <skos:prefLabel xml:lang="nl">cartografische driedimensionale vorm</skos:prefLabel>
      <rdakit:toolkitLabel xml:lang="nl">cartografische driedimensionale vorm</rdakit:toolkitLabel>
      <skos:definition xml:lang="nl">Cartografische content uitgedrukt door een vorm of vormen bedoeld om visueel waar te nemen in drie dimensies.</skos:definition>
      <rdakit:toolkitDefinition xml:lang="nl">Cartografische content uitgedrukt door een vorm of vormen bedoeld om visueel waar te nemen in drie dimensies.</rdakit:toolkitDefinition>
      <skos:prefLabel xml:lang="it">forma tridimensionale cartografica</skos:prefLabel>
      <rdakit:toolkitLabel xml:lang="it">forma tridimensionale cartografica</rdakit:toolkitLabel>
      <skos:definition xml:lang="it">Contenuto cartografico espresso mediante una o più forme in tre dimensioni percepibili con la vista.</skos:definition>
      <rdakit:toolkitDefinition xml:lang="it">Contenuto cartografico espresso mediante una o più forme in tre dimensioni percepibili con la vista.</rdakit:toolkitDefinition>
      <skos:scopeNote xml:lang="it">Include globi, modelli a rilievo, etc.</skos:scopeNote>
      <skos:prefLabel xml:lang="fi">kartografinen kolmiulotteinen muoto</skos:prefLabel>
      <rdakit:toolkitLabel xml:lang="fi">kartografinen kolmiulotteinen muoto</rdakit:toolkitLabel>
      <skos:definition xml:lang="fi">Muotona tai muotoina esitetty kartografinen sisältö, joka on tarkoitettu katsottavaksi kolmiulotteisena.</skos:definition>
      <rdakit:toolkitDefinition xml:lang="fi">Muotona tai muotoina esitetty kartografinen sisältö, joka on tarkoitettu katsottavaksi kolmiulotteisena.</rdakit:toolkitDefinition>
      <skos:scopeNote xml:lang="fi">Esimerkiksi karttapallot, pienoismallit jne.</skos:scopeNote>
      <skos:prefLabel xml:lang="he">צורה קרטוגרפית תלת-ממדית</skos:prefLabel>
      <rdakit:toolkitLabel xml:lang="he">צורה קרטוגרפית תלת-ממדית</rdakit:toolkitLabel>
      <skos:definition xml:lang="he">סוג תוכן המכיל תוכן קרטוגרפי אשר קיבל את ביטויו באמצעות צורה או צורות וכד', ומיועד לצפייה כאובייקט תלת-ממדי.</skos:definition>
      <rdakit:toolkitDefinition xml:lang="he">סוג תוכן המכיל תוכן קרטוגרפי אשר קיבל את ביטויו באמצעות צורה או צורות וכד', ומיועד לצפייה כאובייקט תלת-ממדי.</rdakit:toolkitDefinition>
      <skos:scopeNote xml:lang="he">כולל גְלוֹּבּוס, מוֹדֶל תבְלִּיטִּי וכד'.</skos:scopeNote>
      <skos:prefLabel xml:lang="ar">شكل خرائطي ثلاثي الأبعاد</skos:prefLabel>
      <skos:prefLabel xml:lang="sv">kartografisk tredimensionell form</skos:prefLabel>
      <rdakit:toolkitLabel xml:lang="sv">kartografisk tredimensionell form</rdakit:toolkitLabel>
      <skos:prefLabel xml:lang="vi">hình thái ba chiều bản đồ</skos:prefLabel>
      <rdakit:toolkitLabel xml:lang="vi">hình thái ba chiều bản đồ</rdakit:toolkitLabel>
      <skos:definition xml:lang="vi">Loại nội dung gồm có nội dung bản đồ được biểu hiện qua một hoặc nhiều hình thái để nhận biết bằng thị giác ở ba chiều.</skos:definition>
      <rdakit:toolkitDefinition xml:lang="vi">Loại nội dung gồm có nội dung bản đồ được biểu hiện qua một hoặc nhiều hình thái để nhận biết bằng thị giác ở ba chiều.</rdakit:toolkitDefinition>
      <skos:scopeNote xml:lang="vi">Quả địa cầu, mô hình địa hình, v.v..., được bao gồm</skos:scopeNote>
      <skos:prefLabel xml:lang="da">kartografisk tredimensional form</skos:prefLabel>
      <rdakit:toolkitLabel xml:lang="da">kartografisk tredimensional form</rdakit:toolkitLabel>
      <skos:definition xml:lang="da">Indholdstype der består af kartografisk indhold udtrykt som en eller flere former mhp. at blive opfattet visuelt i tre dimensioner.</skos:definition>
      <rdakit:toolkitDefinition xml:lang="da">Indholdstype der består af kartografisk indhold udtrykt som en eller flere former mhp. at blive opfattet visuelt i tre dimensioner.</rdakit:toolkitDefinition>
      <skos:scopeNote xml:lang="da">Glober, reliefmodeller etc. er omfattet.</skos:scopeNote>
      <skos:prefLabel xml:lang="no">kartografisk tredimensjonal form</skos:prefLabel>
      <rdakit:toolkitLabel xml:lang="no">kartografisk tredimensjonal form</rdakit:toolkitLabel>
      <skos:definition xml:lang="no">En innholdstype som består av kartografisk innhold uttrykt gjennom én eller flere former, som skal oppfattes visuelt i tre dimensjoner.</skos:definition>
      <rdakit:toolkitDefinition xml:lang="no">En innholdstype som består av kartografisk innhold uttrykt gjennom én eller flere former, som skal oppfattes visuelt i tre dimensjoner.</rdakit:toolkitDefinition>
      <skos:scopeNote xml:lang="no">Globuser, relieffmodeller etc. er inkludert.</skos:scopeNote>
    </skos:Concept>
<!-- Concept: computer dataset  -->
    <skos:Concept rdf:about="http://rdaregistry.info/termList/RDAContentType/1007" xml:lang="en">
      <skos:inScheme rdf:resource="http://rdaregistry.info/termList/RDAContentType"/>
      <reg:status rdf:resource="http://metadataregistry.org/uri/RegStatus/1001"/>
      <reg:identifier rdf:resource="http://metadataregistry.org/concepts/516"/>
      <skos:prefLabel xml:lang="en">computer dataset</skos:prefLabel>
      <skos:definition xml:lang="en">A content type consisting of content expressed through a digitally encoded dataset intended to be processed by a computer.</skos:definition>
      <skos:prefLabel xml:lang="de">Computerdaten</skos:prefLabel>
      <skos:scopeNote xml:lang="de">Dazu gehören numerische Daten, Umweltdaten usw., die von Anwendersoftware verwendet werden, um Durchschnittsmengen, Korrelationen usw. zu berechnen oder um Modelle usw. zu erstellen, normalerweise aber nicht als Rohdaten präsentiert werden.</skos:scopeNote>
      <skos:definition xml:lang="de">Ein Inhaltstyp, der aus Inhalt besteht, der über einen digital kodierten Datensatz ausgedrückt wird, der für die Verarbeitung durch einen Computer konzipiert ist.</skos:definition>
      <skos:scopeNote xml:lang="en">Numeric data, environmental data, etc., used by applications software to calculate averages, correlations, etc., or to produce models, etc., but not normally displayed in its raw form, are included.</skos:scopeNote>
      <skos:scopeNote xml:lang="en">For data intended to be perceived in an audible form, see performed music, sounds, and spoken word.</skos:scopeNote>
      <skos:scopeNote xml:lang="en">For cartographic data, see cartographic dataset.</skos:scopeNote>
	    <skos:related rdf:resource="http://rdaregistry.info/termList/RDAContentType/1001"/>
	    <skos:related rdf:resource="http://rdaregistry.info/termList/RDAContentType/1009"/>
	    <skos:related rdf:resource="http://rdaregistry.info/termList/RDAContentType/1010"/>
	    <skos:related rdf:resource="http://rdaregistry.info/termList/RDAContentType/1014"/>
	    <skos:related rdf:resource="http://rdaregistry.info/termList/RDAContentType/1020"/>
	    <skos:related rdf:resource="http://rdaregistry.info/termList/RDAContentType/1023"/>
	    <skos:related rdf:resource="http://rdaregistry.info/termList/RDAContentType/1022"/>
	    <skos:related rdf:resource="http://rdaregistry.info/termList/RDAContentType/1021"/>
	    <skos:related rdf:resource="http://rdaregistry.info/termList/RDAContentType/1013"/>
	    <skos:related rdf:resource="http://rdaregistry.info/termList/RDAContentType/1012"/>
	    <skos:related rdf:resource="http://rdaregistry.info/termList/RDAContentType/1011"/>
      <skos:prefLabel xml:lang="fr">données informatiques</skos:prefLabel>
      <skos:definition xml:lang="fr">Type de contenu qui consiste en contenu exprimé au moyen de données encodées numériquement, en vue d’un traitement par ordinateur.</skos:definition>
      <skos:scopeNote xml:lang="fr">Comprend les données numériques, les données sur l’environnement, etc. utilisées par des logiciels d’application pour calculer des moyennes, des corrélations, etc. ou pour produire des modèles, etc. mais qui, normalement, ne sont pas affichées sous leur forme brute. Ne comprend pas les données destinées à être perçues visuellement sous forme de notation, d’image ou de forme tridimensionnelle.</skos:scopeNote>
      <skos:prefLabel xml:lang="es">conjunto de datos para computadora</skos:prefLabel>
      <skos:definition xml:lang="es">Contenido expresado mediante un conjunto de datos codificado digitalmente pensado para ser procesado por una computadora.</skos:definition>
      <skos:scopeNote xml:lang="es">Incluye datos numéricos, datos ambientales, etc., utilizados por aplicaciones informáticas para calcular promedios, correlaciones, etc., o para producir modelos, etc., pero que no están desplegados normalmente en su estado original.</skos:scopeNote>
      <rdakit:toolkitLabel xml:lang="en">computer dataset</rdakit:toolkitLabel>
      <rdakit:toolkitLabel xml:lang="fr">données informatiques</rdakit:toolkitLabel>
      <rdakit:toolkitDefinition xml:lang="en">A content type consisting of content expressed through a digitally encoded dataset intended to be processed by a computer.</rdakit:toolkitDefinition>
      <rdakit:toolkitDefinition xml:lang="fr">Type de contenu qui consiste en contenu exprimé au moyen de données encodées numériquement, en vue d’un traitement par ordinateur.</rdakit:toolkitDefinition>
      <rdakit:toolkitLabel xml:lang="de">Computerdaten</rdakit:toolkitLabel>
      <rdakit:toolkitDefinition xml:lang="de">Ein Inhaltstyp, der aus Inhalt besteht, der über einen digital kodierten Datensatz ausgedrückt wird, der für die Verarbeitung durch einen Computer konzipiert ist.</rdakit:toolkitDefinition>
      <rdakit:toolkitLabel xml:lang="es">conjunto de datos para computadora</rdakit:toolkitLabel>
      <rdakit:toolkitDefinition xml:lang="es">Contenido expresado mediante un conjunto de datos codificado digitalmente pensado para ser procesado por una computadora.</rdakit:toolkitDefinition>
      <skos:prefLabel xml:lang="zh">计算机数据集</skos:prefLabel>
      <rdakit:toolkitLabel xml:lang="zh">计算机数据集</rdakit:toolkitLabel>
      <skos:definition xml:lang="zh">经计算机处理的、以数字编码数据集表达的内容。</skos:definition>
      <rdakit:toolkitDefinition xml:lang="zh">经计算机处理的、以数字编码数据集表达的内容。</rdakit:toolkitDefinition>
      <skos:scopeNote xml:lang="zh">包括通过应用软件计算平均值、相互关系等的数字数据、环境数据等，或通常以非原始状态显示的产品模型等。</skos:scopeNote>
      <skos:prefLabel xml:lang="nl">computerdataset</skos:prefLabel>
      <rdakit:toolkitLabel xml:lang="nl">computerdataset</rdakit:toolkitLabel>
      <skos:definition xml:lang="nl">Content uitgedrukt door een digitaal gecodeerde dataset bedoeld om verwerkt te worden door een computer.</skos:definition>
      <rdakit:toolkitDefinition xml:lang="nl">Content uitgedrukt door een digitaal gecodeerde dataset bedoeld om verwerkt te worden door een computer.</rdakit:toolkitDefinition>
      <skos:prefLabel xml:lang="it">dataset per computer</skos:prefLabel>
      <rdakit:toolkitLabel xml:lang="it">dataset per computer</rdakit:toolkitLabel>
      <skos:definition xml:lang="it">Contenuto espresso mediante un dataset codificato in modo digitale e destinato a essere elaborato mediante un computer.</skos:definition>
      <rdakit:toolkitDefinition xml:lang="it">Contenuto espresso mediante un dataset codificato in modo digitale e destinato a essere elaborato mediante un computer.</rdakit:toolkitDefinition>
      <skos:prefLabel xml:lang="fi">digitaalinen data</skos:prefLabel>
      <rdakit:toolkitLabel xml:lang="fi">digitaalinen data</rdakit:toolkitLabel>
      <skos:definition xml:lang="fi">Tietokoneen käsiteltäväksi tarkoitettu digitaalinen sisältö.</skos:definition>
      <rdakit:toolkitDefinition xml:lang="fi">Tietokoneen käsiteltäväksi tarkoitettu digitaalinen sisältö.</rdakit:toolkitDefinition>
      <skos:scopeNote xml:lang="fi">Esimerkiksi numeerinen data, ympäristödata jne., jota ohjelmistot käyttävät keskiarvojen, korrelaatioiden jne. laskemiseen tai mallien tms. tuottamiseen, mutta jota tavallisesti ei esitetä sellaisenaan raakamateriaalina. Ei sisällä dataa, joka on tarkoitettu tarkasteltavaksi visuaalisesti notaation, kuvan tai kolmiulotteisessa muodossa.</skos:scopeNote>
      <skos:prefLabel xml:lang="he">קבוצת נתונים למחשב</skos:prefLabel>
      <rdakit:toolkitLabel xml:lang="he">קבוצת נתונים למחשב</rdakit:toolkitLabel>
      <skos:definition xml:lang="he">סוג תוכן המכיל תוכן שקיבל את ביטויו באמצעות קבוצת נתונים דיגיטליים המיועדת לעיבוד על ידי מחשב.</skos:definition>
      <rdakit:toolkitDefinition xml:lang="he">סוג תוכן המכיל תוכן שקיבל את ביטויו באמצעות קבוצת נתונים דיגיטליים המיועדת לעיבוד על ידי מחשב.</rdakit:toolkitDefinition>
      <skos:scopeNote xml:lang="he">כולל נתונים ספרתיים, נתונים סביבתיים וכיוצ&quot;ב המשמשים יישומים לחישוב ממוצעים, מתאמים וכו', או כדי להפיק מודלים, וכו'. בדרך כלל נתונים אלו אינם מוצגים בצורתם הגולמית.</skos:scopeNote>
      <skos:prefLabel xml:lang="ar">مجموعة بيانات حاسوبية</skos:prefLabel>
      <skos:prefLabel xml:lang="vi">bộ dữ liệu máy tính</skos:prefLabel>
      <rdakit:toolkitLabel xml:lang="vi">bộ dữ liệu máy tính</rdakit:toolkitLabel>
      <skos:definition xml:lang="vi">Loại nội dung gồm có nội dung được biểu hiện qua bộ dữ liệu mã hoá kỹ thuật số để xử lý bằng máy tính.</skos:definition>
      <rdakit:toolkitDefinition xml:lang="vi">Loại nội dung gồm có nội dung được biểu hiện qua bộ dữ liệu mã hoá kỹ thuật số để xử lý bằng máy tính.</rdakit:toolkitDefinition>
      <skos:scopeNote xml:lang="vi">Dữ liệu bằng số, dữ liệu môi trường, v.v..., được sử dụng bằng phần mềm ứng dụng để tính trung bình, tương quan, v.v..., hoặc tạo mô hình, v.v... nhưng thường không hiển thị dưới dạng thô, được bao gồm</skos:scopeNote>
      <skos:prefLabel xml:lang="da">computerdataset</skos:prefLabel>
      <rdakit:toolkitLabel xml:lang="da">computerdataset</rdakit:toolkitLabel>
      <skos:definition xml:lang="da">Indholdstype der består af indhold udtrykt gennem et digitalt kodet datasæt skabt til at blive behandlet af en computer.</skos:definition>
      <rdakit:toolkitDefinition xml:lang="da">Indholdstype der består af indhold udtrykt gennem et digitalt kodet datasæt skabt til at blive behandlet af en computer.</rdakit:toolkitDefinition>
      <skos:scopeNote xml:lang="da">Numeriske data, miljødata etc., der anvendes af applikationssoftware til at beregne gennemsnit, korrelationer etc., eller til at fremstille modeller etc., men som normalt ikke vises i rå form er omfattet. Data der er beregnet til at blive opfattet visuelt i form af en notation, et billede, eller en tredimensional form er ikke omfattet.</skos:scopeNote>
      <skos:prefLabel xml:lang="no">datasett</skos:prefLabel>
      <rdakit:toolkitLabel xml:lang="no">datasett</rdakit:toolkitLabel>
      <skos:definition xml:lang="no">En innholdstype som består av innhold uttrykt gjennom et digitalt kodet datasett som skal behandles av en datamaskin.</skos:definition>
      <rdakit:toolkitDefinition xml:lang="no">En innholdstype som består av innhold uttrykt gjennom et digitalt kodet datasett som skal behandles av en datamaskin.</rdakit:toolkitDefinition>
      <skos:scopeNote xml:lang="no">Numeriske data, miljødata etc. som programmer bruker til å beregne gjennomsnitt, korrelasjoner etc. eller til å lage modeller etc., men som vanligvis ikke vises i sin ubehandlede form, er inkludert. Utelukker data som skal oppfattes visuelt som notasjon, bilde eller tredimensjonal form. Se framført musikk, lyder og tale for data som er ment for å oppfattes i hørbar form. Se kartografisk datasett for kartografiske data.</skos:scopeNote>
    </skos:Concept>
<!-- Concept: computer program  -->
    <skos:Concept rdf:about="http://rdaregistry.info/termList/RDAContentType/1008" xml:lang="en">
      <skos:inScheme rdf:resource="http://rdaregistry.info/termList/RDAContentType"/>
      <reg:status rdf:resource="http://metadataregistry.org/uri/RegStatus/1001"/>
      <reg:identifier rdf:resource="http://metadataregistry.org/concepts/517"/>
      <skos:prefLabel xml:lang="en">computer program</skos:prefLabel>
      <skos:definition xml:lang="en">A content type consisting of content expressed through digitally encoded instructions intended to be processed and performed by a computer.</skos:definition>
      <skos:prefLabel xml:lang="de">Computerprogramm</skos:prefLabel>
      <skos:definition xml:lang="de">Ein Inhaltstyp, der aus Inhalt besteht, der durch digital kodierte Anweisungen ausgedrückt wird und für Verarbeitung und Ausführung mit Hilfe eines Computers konzipiert ist.</skos:definition>
      <skos:scopeNote xml:lang="en">Operating systems, applications software, etc., are included.</skos:scopeNote>
      <skos:scopeNote xml:lang="de">Dazu gehören Betriebssysteme, Anwendersoftware usw.</skos:scopeNote>
      <skos:prefLabel xml:lang="fr">programme informatique</skos:prefLabel>
      <skos:definition xml:lang="fr">Type de contenu qui consiste en contenu exprimé au moyen d’instructions encodées numériquement, en vue d’un traitement et d’une exécution par ordinateur.</skos:definition>
      <skos:scopeNote xml:lang="fr">Comprend les systèmes d’exploitation, les logiciels d’application, etc.</skos:scopeNote>
      <skos:prefLabel xml:lang="es">programa para computadora</skos:prefLabel>
      <skos:definition xml:lang="es">Contenido expresado mediante instrucciones codificadas digitalmente pensadas para ser procesadas y ejecutadas por una computadora.</skos:definition>
      <skos:scopeNote xml:lang="es">Incluye sistemas operativos, aplicaciones, programas informáticos, etc.</skos:scopeNote>
      <rdakit:toolkitLabel xml:lang="en">computer program</rdakit:toolkitLabel>
      <rdakit:toolkitLabel xml:lang="fr">programme informatique</rdakit:toolkitLabel>
      <rdakit:toolkitDefinition xml:lang="en">A content type consisting of content expressed through digitally encoded instructions intended to be processed and performed by a computer.</rdakit:toolkitDefinition>
      <rdakit:toolkitDefinition xml:lang="fr">Type de contenu qui consiste en contenu exprimé au moyen d’instructions encodées numériquement, en vue d’un traitement et d’une exécution par ordinateur.</rdakit:toolkitDefinition>
      <rdakit:toolkitLabel xml:lang="de">Computerprogramm</rdakit:toolkitLabel>
      <rdakit:toolkitDefinition xml:lang="de">Ein Inhaltstyp, der aus Inhalt besteht, der durch digital kodierte Anweisungen ausgedrückt wird und für Verarbeitung und Ausführung mit Hilfe eines Computers konzipiert ist.</rdakit:toolkitDefinition>
      <rdakit:toolkitLabel xml:lang="es">programa para computadora</rdakit:toolkitLabel>
      <rdakit:toolkitDefinition xml:lang="es">Contenido expresado mediante instrucciones codificadas digitalmente pensadas para ser procesadas y ejecutadas por una computadora.</rdakit:toolkitDefinition>
      <skos:prefLabel xml:lang="zh">计算机程序</skos:prefLabel>
      <rdakit:toolkitLabel xml:lang="zh">计算机程序</rdakit:toolkitLabel>
      <skos:definition xml:lang="zh">经计算机处理和操作的，以数字编码指令表达的内容。</skos:definition>
      <rdakit:toolkitDefinition xml:lang="zh">经计算机处理和操作的，以数字编码指令表达的内容。</rdakit:toolkitDefinition>
      <skos:scopeNote xml:lang="zh">包括操作系统、应用软件等。</skos:scopeNote>
      <skos:prefLabel xml:lang="nl">computerprogramma</skos:prefLabel>
      <rdakit:toolkitLabel xml:lang="nl">computerprogramma</rdakit:toolkitLabel>
      <skos:definition xml:lang="nl">Content uitgedrukt door digitaal gecodeerde instructies bedoeld om verwerkt en uitgevoerd te worden door een computer.</skos:definition>
      <rdakit:toolkitDefinition xml:lang="nl">Content uitgedrukt door digitaal gecodeerde instructies bedoeld om verwerkt en uitgevoerd te worden door een computer.</rdakit:toolkitDefinition>
      <skos:prefLabel xml:lang="it">programma per computer</skos:prefLabel>
      <rdakit:toolkitLabel xml:lang="it">programma per computer</rdakit:toolkitLabel>
      <skos:definition xml:lang="it">Contenuto espresso mediante istruzioni codificate in modo digitale, elaborate ed eseguite da un computer.</skos:definition>
      <rdakit:toolkitDefinition xml:lang="it">Contenuto espresso mediante istruzioni codificate in modo digitale, elaborate ed eseguite da un computer.</rdakit:toolkitDefinition>
      <skos:scopeNote xml:lang="it">Include sistemi operativi, applicazioni software, etc.</skos:scopeNote>
      <skos:prefLabel xml:lang="fi">tietokoneohjelma</skos:prefLabel>
      <rdakit:toolkitLabel xml:lang="fi">tietokoneohjelma</rdakit:toolkitLabel>
      <skos:definition xml:lang="fi">Tietokoneen käsiteltäväksi ja suoritettavaksi tarkoitettu (digitaalisesti koodattu) ohjelma.</skos:definition>
      <rdakit:toolkitDefinition xml:lang="fi">Tietokoneen käsiteltäväksi ja suoritettavaksi tarkoitettu (digitaalisesti koodattu) ohjelma.</rdakit:toolkitDefinition>
      <skos:scopeNote xml:lang="fi">Esimerkiksi käyttöjärjestelmät, sovellusohjelmat jne.</skos:scopeNote>
      <skos:prefLabel xml:lang="he">תוכנת מחשב</skos:prefLabel>
      <rdakit:toolkitLabel xml:lang="he">תוכנת מחשב</rdakit:toolkitLabel>
      <skos:definition xml:lang="he">סוג תוכן המכיל תוכן שקיבל את ביטויו באמצעות הוראות מקודדות המיועדות לעיבוד וביצוע על ידי מחשב.</skos:definition>
      <rdakit:toolkitDefinition xml:lang="he">סוג תוכן המכיל תוכן שקיבל את ביטויו באמצעות הוראות מקודדות המיועדות לעיבוד וביצוע על ידי מחשב.</rdakit:toolkitDefinition>
      <skos:scopeNote xml:lang="he">כולל תוכנות הפעלה, תוכנות יישומיות וכו'.</skos:scopeNote>
      <skos:prefLabel xml:lang="ar">برنامج حاسوبي</skos:prefLabel>
      <skos:prefLabel xml:lang="sv">datorprogram</skos:prefLabel>
      <rdakit:toolkitLabel xml:lang="sv">datorprogram</rdakit:toolkitLabel>
      <skos:prefLabel xml:lang="vi">chương trình máy tính</skos:prefLabel>
      <rdakit:toolkitLabel xml:lang="vi">chương trình máy tính</rdakit:toolkitLabel>
      <skos:definition xml:lang="vi">Loại nội dung được biểu hiện qua các lệnh mã hoá kỹ thuật số để xử lý và hoạt động bằng máy tính.</skos:definition>
      <rdakit:toolkitDefinition xml:lang="vi">Loại nội dung được biểu hiện qua các lệnh mã hoá kỹ thuật số để xử lý và hoạt động bằng máy tính.</rdakit:toolkitDefinition>
      <skos:scopeNote xml:lang="vi">Hệ điều hành, phần mềm ứng dụng, v.v...,được bao gồm</skos:scopeNote>
      <skos:prefLabel xml:lang="da">computerprogram</skos:prefLabel>
      <rdakit:toolkitLabel xml:lang="da">computerprogram</rdakit:toolkitLabel>
      <skos:definition xml:lang="da">Indholdstype der består af indhold udtrykt gennem digitalt kodede instruktioner beregnet til at blive behandlet og udført af en computer.</skos:definition>
      <rdakit:toolkitDefinition xml:lang="da">Indholdstype der består af indhold udtrykt gennem digitalt kodede instruktioner beregnet til at blive behandlet og udført af en computer.</rdakit:toolkitDefinition>
      <skos:scopeNote xml:lang="da">Operativsystemer, applikationssoftware etc. er omfattet.</skos:scopeNote>
      <skos:prefLabel xml:lang="no">dataprogram</skos:prefLabel>
      <rdakit:toolkitLabel xml:lang="no">dataprogram</rdakit:toolkitLabel>
      <skos:definition xml:lang="no">En innholdstype som består av innhold uttrykt gjennom digitalt kodede instruksjoner som skal behandles og utføres av en datamaskin.</skos:definition>
      <rdakit:toolkitDefinition xml:lang="no">En innholdstype som består av innhold uttrykt gjennom digitalt kodede instruksjoner som skal behandles og utføres av en datamaskin.</rdakit:toolkitDefinition>
      <skos:scopeNote xml:lang="no">Operativsystemer, dataprogrammer etc. er inkludert.</skos:scopeNote>
    </skos:Concept>
<!-- Concept: notated movement  -->
    <skos:Concept rdf:about="http://rdaregistry.info/termList/RDAContentType/1009" xml:lang="en">
      <skos:inScheme rdf:resource="http://rdaregistry.info/termList/RDAContentType"/>
      <reg:status rdf:resource="http://metadataregistry.org/uri/RegStatus/1001"/>
      <reg:identifier rdf:resource="http://metadataregistry.org/concepts/518"/>
      <skos:prefLabel xml:lang="en">notated movement</skos:prefLabel>
      <skos:definition xml:lang="en">A content type consisting of content expressed through a form of notation for movement intended to be perceived visually.</skos:definition>
      <skos:scopeNote xml:lang="en">All forms of movement notation other than those intended to be perceived through touch are included.</skos:scopeNote>
      <skos:prefLabel xml:lang="de">Bewegungsnotation</skos:prefLabel>
      <skos:scopeNote xml:lang="de">Dazu gehören alle Formen der Bewegungsnotation, außer denjenigen, die konzipiert sind, um über den Tastsinn wahrgenommen zu werden.</skos:scopeNote>
      <skos:definition xml:lang="de">Ein Inhaltstyp, der aus Inhalt besteht, der durch eine Notationsform für Bewegung ausgedrückt wird und konzipiert ist, um visuell wahrgenommen zu werden.</skos:definition>
	    <skos:related rdf:resource="http://rdaregistry.info/termList/RDAContentType/1007"/>
	    <skos:related rdf:resource="http://rdaregistry.info/termList/RDAContentType/1017"/>
      <skos:prefLabel xml:lang="fr">mouvement noté</skos:prefLabel>
      <skos:definition xml:lang="fr">Type de contenu qui consiste en contenu exprimé au moyen d’une forme de notation du mouvement destinée à être perçue visuellement.</skos:definition>
      <skos:scopeNote xml:lang="fr">Comprend toutes les formes de notation du mouvement différentes de celles destinées à être perçues au toucher.</skos:scopeNote>
      <skos:prefLabel xml:lang="es">notación de movimientos</skos:prefLabel>
      <skos:definition xml:lang="es">Contenido expresado mediante una forma de notación para movimiento pensado para ser percibido visualmente.</skos:definition>
      <skos:scopeNote xml:lang="es">Incluye todas las formas de notación de movimientos diferentes de aquellas proyectadas para ser percibidas mediante el tacto.</skos:scopeNote>
      <rdakit:toolkitLabel xml:lang="en">notated movement</rdakit:toolkitLabel>
      <rdakit:toolkitLabel xml:lang="fr">mouvement noté</rdakit:toolkitLabel>
      <rdakit:toolkitDefinition xml:lang="en">A content type consisting of content expressed through a form of notation for movement intended to be perceived visually.</rdakit:toolkitDefinition>
      <rdakit:toolkitDefinition xml:lang="fr">Type de contenu qui consiste en contenu exprimé au moyen d’une forme de notation du mouvement destinée à être perçue visuellement.</rdakit:toolkitDefinition>
      <rdakit:toolkitLabel xml:lang="de">Bewegungsnotation</rdakit:toolkitLabel>
      <rdakit:toolkitDefinition xml:lang="de">Ein Inhaltstyp, der aus Inhalt besteht, der durch eine Notationsform für Bewegung ausgedrückt wird und konzipiert ist, um visuell wahrgenommen zu werden.</rdakit:toolkitDefinition>
      <rdakit:toolkitLabel xml:lang="es">notación de movimientos</rdakit:toolkitLabel>
      <rdakit:toolkitDefinition xml:lang="es">Contenido expresado mediante una forma de notación para movimiento pensado para ser percibido visualmente.</rdakit:toolkitDefinition>
      <skos:prefLabel xml:lang="zh">动作谱</skos:prefLabel>
      <rdakit:toolkitLabel xml:lang="zh">动作谱</rdakit:toolkitLabel>
      <skos:definition xml:lang="zh">以动作标记法表达的，旨在通过视觉感知的内容。</skos:definition>
      <rdakit:toolkitDefinition xml:lang="zh">以动作标记法表达的，旨在通过视觉感知的内容。</rdakit:toolkitDefinition>
      <skos:scopeNote xml:lang="zh">包括所有类型的动作标记法，但以触觉感知的形式除外。</skos:scopeNote>
      <skos:prefLabel xml:lang="nl">bewegingsnotatie</skos:prefLabel>
      <rdakit:toolkitLabel xml:lang="nl">bewegingsnotatie</rdakit:toolkitLabel>
      <skos:definition xml:lang="nl">Content uitgedrukt door een vorm van bewegingsnotatie bedoeld om visueel waar te nemen.</skos:definition>
      <rdakit:toolkitDefinition xml:lang="nl">Content uitgedrukt door een vorm van bewegingsnotatie bedoeld om visueel waar te nemen.</rdakit:toolkitDefinition>
      <skos:prefLabel xml:lang="it">movimento notato</skos:prefLabel>
      <rdakit:toolkitLabel xml:lang="it">movimento notato</rdakit:toolkitLabel>
      <skos:definition xml:lang="it">Contenuto espresso mediante una forma di notazione del movimento percepibile con la vista.</skos:definition>
      <rdakit:toolkitDefinition xml:lang="it">Contenuto espresso mediante una forma di notazione del movimento percepibile con la vista.</rdakit:toolkitDefinition>
      <skos:scopeNote xml:lang="it">Include tutte le forme di notazione del movimento diverse da quelle percepibili mediante il tatto.</skos:scopeNote>
      <skos:prefLabel xml:lang="fi">liikenotaatio</skos:prefLabel>
      <rdakit:toolkitLabel xml:lang="fi">liikenotaatio</rdakit:toolkitLabel>
      <skos:definition xml:lang="fi">Liikettä kuvailevan merkkijärjestelmän avulla esitetty sisältö, joka on tarkoitettu katsottavaksi.</skos:definition>
      <rdakit:toolkitDefinition xml:lang="fi">Liikettä kuvailevan merkkijärjestelmän avulla esitetty sisältö, joka on tarkoitettu katsottavaksi.</rdakit:toolkitDefinition>
      <skos:scopeNote xml:lang="fi">Sisältää kaikki muut kuin kosketeltavassa muodossa olevat liikenotaatiot.</skos:scopeNote>
      <skos:prefLabel xml:lang="he">תווי תנועה</skos:prefLabel>
      <rdakit:toolkitLabel xml:lang="he">תווי תנועה</rdakit:toolkitLabel>
      <skos:definition xml:lang="he">סוג תוכן המכיל תוכן שקיבל את ביטויו באמצעות תווים המייצגים תנועה המיועדים לצפייה.</skos:definition>
      <rdakit:toolkitDefinition xml:lang="he">סוג תוכן המכיל תוכן שקיבל את ביטויו באמצעות תווים המייצגים תנועה המיועדים לצפייה.</rdakit:toolkitDefinition>
      <skos:scopeNote xml:lang="he">כולל כל סוגי תווי התנועה, למעט אלה המיועדים לתפיסה על ידי מישוש.</skos:scopeNote>
      <skos:prefLabel xml:lang="ar">حركة مدونة (مرمزة)</skos:prefLabel>
      <skos:prefLabel xml:lang="vi">động thái ký hiệu</skos:prefLabel>
      <rdakit:toolkitLabel xml:lang="vi">động thái ký hiệu</rdakit:toolkitLabel>
      <skos:definition xml:lang="vi">Loại nội dung được biểu hiện qua hình thái ký hiệu cho động thái để nhận biết bằng thị giác.</skos:definition>
      <rdakit:toolkitDefinition xml:lang="vi">Loại nội dung được biểu hiện qua hình thái ký hiệu cho động thái để nhận biết bằng thị giác.</rdakit:toolkitDefinition>
      <skos:scopeNote xml:lang="vi">Tất cả các hình thái của ký hiệu động thái khác với để nhận biết bằng xúc giác được bao gồm</skos:scopeNote>
      <skos:prefLabel xml:lang="da">noteret bevægelse</skos:prefLabel>
      <rdakit:toolkitLabel xml:lang="da">noteret bevægelse</rdakit:toolkitLabel>
      <skos:definition xml:lang="da">Indholdstype der består af indhold udtrykt via en bevægelsesnotationsform, beregnet til visuel opfattelse.</skos:definition>
      <rdakit:toolkitDefinition xml:lang="da">Indholdstype der består af indhold udtrykt via en bevægelsesnotationsform, beregnet til visuel opfattelse.</rdakit:toolkitDefinition>
      <skos:scopeNote xml:lang="da">Alle former for bevægelsesnotation, bortset fra dem der er beregnet til at opfattes ved berøring er omfattet.</skos:scopeNote>
      <skos:prefLabel xml:lang="no">bevegelsesnotasjon</skos:prefLabel>
      <rdakit:toolkitLabel xml:lang="no">bevegelsesnotasjon</rdakit:toolkitLabel>
      <skos:definition xml:lang="no">En innholdstype som består av innhold uttrykt ved hjelp av en form for bevegelsesnotasjon som er ment å oppfattes visuelt.</skos:definition>
      <rdakit:toolkitDefinition xml:lang="no">En innholdstype som består av innhold uttrykt ved hjelp av en form for bevegelsesnotasjon som er ment å oppfattes visuelt.</rdakit:toolkitDefinition>
      <skos:scopeNote xml:lang="no">Alle former for bevegelsesnotasjon bortsett fra de som er ment å oppfattes gjennom berøring, er inkludert.</skos:scopeNote>
    </skos:Concept>
<!-- Concept: notated music  -->
    <skos:Concept rdf:about="http://rdaregistry.info/termList/RDAContentType/1010" xml:lang="en">
      <skos:inScheme rdf:resource="http://rdaregistry.info/termList/RDAContentType"/>
      <reg:status rdf:resource="http://metadataregistry.org/uri/RegStatus/1001"/>
      <reg:identifier rdf:resource="http://metadataregistry.org/concepts/519"/>
      <skos:prefLabel xml:lang="en">notated music</skos:prefLabel>
      <skos:definition xml:lang="en">A content type consisting of content expressed through a form of musical notation intended to be perceived visually.</skos:definition>
      <skos:scopeNote xml:lang="en">All forms of music notation other than those intended to be perceived through touch are included.</skos:scopeNote>
      <skos:prefLabel xml:lang="de">Noten</skos:prefLabel>
      <skos:scopeNote xml:lang="de">Dazu gehören alle Formen von Musiknotation, außer denjenigen, die konzipiert sind, um über den Tastsinn wahrgenommen zu werden.</skos:scopeNote>
      <skos:definition xml:lang="de">Ein Inhaltstyp, der aus Inhalt besteht, der durch eine Notationsform für Musik ausgedrückt wird und konzipiert ist, um visuell wahrgenommen zu werden.</skos:definition>
	    <skos:related rdf:resource="http://rdaregistry.info/termList/RDAContentType/1007"/>
	    <skos:related rdf:resource="http://rdaregistry.info/termList/RDAContentType/1016"/>
      <skos:prefLabel xml:lang="fr">musique notée</skos:prefLabel>
      <skos:definition xml:lang="fr">Type de contenu qui consiste en contenu exprimé au moyen d’une forme de notation musicale destinée à être perçue visuellement.</skos:definition>
      <skos:scopeNote xml:lang="fr">Comprend toutes les formes de notation musicale différentes de celles destinées à être perçues au toucher.</skos:scopeNote>
      <skos:prefLabel xml:lang="es">música notada</skos:prefLabel>
      <skos:definition xml:lang="es">Contenido expresado mediante una forma de notación musical pensado para ser percibido visualmente.</skos:definition>
      <skos:scopeNote xml:lang="es">Incluye todas las formas de notación musical diferentes de las pensadas para ser percibidas mediante el tacto.</skos:scopeNote>
      <rdakit:toolkitLabel xml:lang="en">notated music</rdakit:toolkitLabel>
      <rdakit:toolkitLabel xml:lang="fr">musique notée</rdakit:toolkitLabel>
      <rdakit:toolkitDefinition xml:lang="en">A content type consisting of content expressed through a form of musical notation intended to be perceived visually.</rdakit:toolkitDefinition>
      <rdakit:toolkitDefinition xml:lang="fr">Type de contenu qui consiste en contenu exprimé au moyen d’une forme de notation musicale destinée à être perçue visuellement.</rdakit:toolkitDefinition>
      <rdakit:toolkitLabel xml:lang="de">Noten</rdakit:toolkitLabel>
      <rdakit:toolkitDefinition xml:lang="de">Ein Inhaltstyp, der aus Inhalt besteht, der durch eine Notationsform für Musik ausgedrückt wird und konzipiert ist, um visuell wahrgenommen zu werden.</rdakit:toolkitDefinition>
      <rdakit:toolkitLabel xml:lang="es">música notada</rdakit:toolkitLabel>
      <rdakit:toolkitDefinition xml:lang="es">Contenido expresado mediante una forma de notación musical pensado para ser percibido visualmente.</rdakit:toolkitDefinition>
      <skos:prefLabel xml:lang="zh">乐谱</skos:prefLabel>
      <rdakit:toolkitLabel xml:lang="zh">乐谱</rdakit:toolkitLabel>
      <skos:definition xml:lang="zh">以音符形式表达的，旨在通过视觉感知的内容。</skos:definition>
      <rdakit:toolkitDefinition xml:lang="zh">以音符形式表达的，旨在通过视觉感知的内容。</rdakit:toolkitDefinition>
      <skos:scopeNote xml:lang="zh">。包括所有类型的音符形式，但以触觉感知的形式除外。</skos:scopeNote>
      <skos:prefLabel xml:lang="nl">muzieknotatie</skos:prefLabel>
      <rdakit:toolkitLabel xml:lang="nl">muzieknotatie</rdakit:toolkitLabel>
      <skos:definition xml:lang="nl">Content uitgedrukt door een vorm van muzieknotatie bedoeld om visueel waar te nemen.</skos:definition>
      <rdakit:toolkitDefinition xml:lang="nl">Content uitgedrukt door een vorm van muzieknotatie bedoeld om visueel waar te nemen.</rdakit:toolkitDefinition>
      <skos:prefLabel xml:lang="it">musica notata</skos:prefLabel>
      <rdakit:toolkitLabel xml:lang="it">musica notata</rdakit:toolkitLabel>
      <skos:definition xml:lang="it">Contenuto espresso mediante una forma di notazione musicale percepibile mediante la vista.</skos:definition>
      <rdakit:toolkitDefinition xml:lang="it">Contenuto espresso mediante una forma di notazione musicale percepibile mediante la vista.</rdakit:toolkitDefinition>
      <skos:scopeNote xml:lang="it">Include tutte le forme di notazione musicale diverse da quelle percepibili mediante il tatto.</skos:scopeNote>
      <skos:prefLabel xml:lang="fi">nuottikirjoitus</skos:prefLabel>
      <rdakit:toolkitLabel xml:lang="fi">nuottikirjoitus</rdakit:toolkitLabel>
      <skos:definition xml:lang="fi">Musiikkinotaationa esitetty sisältö, joka on tarkoitettu katsottavaksi.</skos:definition>
      <rdakit:toolkitDefinition xml:lang="fi">Musiikkinotaationa esitetty sisältö, joka on tarkoitettu katsottavaksi.</rdakit:toolkitDefinition>
      <skos:scopeNote xml:lang="fi">Sisältää kaikki muut kuin kosketeltavassa muodossa olevat musiikkinotaatiot.</skos:scopeNote>
      <skos:prefLabel xml:lang="he">תווי מוסיקה</skos:prefLabel>
      <rdakit:toolkitLabel xml:lang="he">תווי מוסיקה</rdakit:toolkitLabel>
      <skos:definition xml:lang="he">סוג תוכן המכיל תוכן שקיבל את ביטויו באמצעות תווי מוסיקה, המיועדים לצפייה.</skos:definition>
      <rdakit:toolkitDefinition xml:lang="he">סוג תוכן המכיל תוכן שקיבל את ביטויו באמצעות תווי מוסיקה, המיועדים לצפייה.</rdakit:toolkitDefinition>
      <skos:scopeNote xml:lang="he">כולל כל סוגי תווי המוסיקה, למעט אלו המיועדים לתפיסה על ידי מישוש.</skos:scopeNote>
      <skos:prefLabel xml:lang="ar">موسيقى مدونة</skos:prefLabel>
      <skos:prefLabel xml:lang="vi">âm nhạc ký hiệu</skos:prefLabel>
      <rdakit:toolkitLabel xml:lang="vi">âm nhạc ký hiệu</rdakit:toolkitLabel>
      <skos:definition xml:lang="vi">Loại nội dung được biểu hiện qua một hình thái ký hiệu âm nhạc để cảm nhận bằng thị giác.</skos:definition>
      <rdakit:toolkitDefinition xml:lang="vi">Loại nội dung được biểu hiện qua một hình thái ký hiệu âm nhạc để cảm nhận bằng thị giác.</rdakit:toolkitDefinition>
      <skos:scopeNote xml:lang="vi">Tất cả các hình thái ký hiệu âm nhạc khác với hình thái để cảm nhận bằng xúc giác được bao gồm</skos:scopeNote>
      <skos:prefLabel xml:lang="da">noteret musik</skos:prefLabel>
      <rdakit:toolkitLabel xml:lang="da">noteret musik</rdakit:toolkitLabel>
      <skos:definition xml:lang="da">Indholdstype der består af indhold udtrykt i musikalsk notationsform beregnet til visuel opfattelse.</skos:definition>
      <rdakit:toolkitDefinition xml:lang="da">Indholdstype der består af indhold udtrykt i musikalsk notationsform beregnet til visuel opfattelse.</rdakit:toolkitDefinition>
      <skos:scopeNote xml:lang="da">Alle former for musikalsk notation, bortset fra dem der er beregnet til at opfattes ved berøring er omfattet.</skos:scopeNote>
      <skos:prefLabel xml:lang="no">nedskrevet musikk</skos:prefLabel>
      <rdakit:toolkitLabel xml:lang="no">nedskrevet musikk</rdakit:toolkitLabel>
      <skos:definition xml:lang="no">En innholdstype som består av innhold uttrykt ved hjelp av en form for musikknotasjon som er ment å oppfattes visuelt.</skos:definition>
      <rdakit:toolkitDefinition xml:lang="no">En innholdstype som består av innhold uttrykt ved hjelp av en form for musikknotasjon som er ment å oppfattes visuelt.</rdakit:toolkitDefinition>
      <skos:scopeNote xml:lang="no">Alle former for musikknotasjon bortsett fra de som er ment å oppfattes gjennom berøring, er inkludert.</skos:scopeNote>
    </skos:Concept>
<!-- Concept: performed music  -->
    <skos:Concept rdf:about="http://rdaregistry.info/termList/RDAContentType/1011" xml:lang="en">
      <skos:inScheme rdf:resource="http://rdaregistry.info/termList/RDAContentType"/>
      <reg:status rdf:resource="http://metadataregistry.org/uri/RegStatus/1001"/>
      <reg:identifier rdf:resource="http://metadataregistry.org/concepts/520"/>
      <skos:prefLabel xml:lang="en">performed music</skos:prefLabel>
      <skos:definition xml:lang="en">A content type consisting of content expressed through music in an audible form.</skos:definition>
      <skos:scopeNote xml:lang="en">Recorded performances of music, computer-generated music, etc. are included.</skos:scopeNote>
      <skos:prefLabel xml:lang="de">Aufgeführte Musik</skos:prefLabel>
      <skos:scopeNote xml:lang="de">Dazu gehören aufgezeichnete Musikaufführungen, computer-generierte Musik usw.</skos:scopeNote>
      <skos:definition xml:lang="de">Ein Inhaltstyp, der aus Inhalt besteht, der durch Musik in hörbarer Form ausgedrückt wird.</skos:definition>
	    <skos:related rdf:resource="http://rdaregistry.info/termList/RDAContentType/1007"/>
      <skos:prefLabel xml:lang="fr">musique exécutée</skos:prefLabel>
      <skos:definition xml:lang="fr">Type de contenu qui consiste en contenu exprimé au moyen de musique sous une forme audible.</skos:definition>
      <skos:scopeNote xml:lang="fr">Comprend les prestations musicales enregistrées, la musique créée par ordinateur, etc.</skos:scopeNote>
      <skos:prefLabel xml:lang="es">música interpretada</skos:prefLabel>
      <skos:definition xml:lang="es">Contenido expresado mediante música en una forma audible.</skos:definition>
      <skos:scopeNote xml:lang="es">Incluye interpretación de música grabada, música generada por computadora, etc.</skos:scopeNote>
      <rdakit:toolkitLabel xml:lang="en">performed music</rdakit:toolkitLabel>
      <rdakit:toolkitLabel xml:lang="fr">musique exécutée</rdakit:toolkitLabel>
      <rdakit:toolkitDefinition xml:lang="en">A content type consisting of content expressed through music in an audible form.</rdakit:toolkitDefinition>
      <rdakit:toolkitDefinition xml:lang="fr">Type de contenu qui consiste en contenu exprimé au moyen de musique sous une forme audible.</rdakit:toolkitDefinition>
      <rdakit:toolkitLabel xml:lang="de">Aufgeführte Musik</rdakit:toolkitLabel>
      <rdakit:toolkitDefinition xml:lang="de">Ein Inhaltstyp, der aus Inhalt besteht, der durch Musik in hörbarer Form ausgedrückt wird.</rdakit:toolkitDefinition>
      <rdakit:toolkitLabel xml:lang="es">música interpretada</rdakit:toolkitLabel>
      <rdakit:toolkitDefinition xml:lang="es">Contenido expresado mediante música en una forma audible.</rdakit:toolkitDefinition>
      <skos:prefLabel xml:lang="zh">表演音乐</skos:prefLabel>
      <rdakit:toolkitLabel xml:lang="zh">表演音乐</rdakit:toolkitLabel>
      <skos:definition xml:lang="zh">以可听见形式的音乐表达的内容。</skos:definition>
      <rdakit:toolkitDefinition xml:lang="zh">以可听见形式的音乐表达的内容。</rdakit:toolkitDefinition>
      <skos:scopeNote xml:lang="zh">包括录制的音乐表演、计算机生成的音乐等。</skos:scopeNote>
      <skos:prefLabel xml:lang="nl">uitgevoerde muziek</skos:prefLabel>
      <rdakit:toolkitLabel xml:lang="nl">uitgevoerde muziek</rdakit:toolkitLabel>
      <skos:definition xml:lang="nl">Content uitgedrukt door muziek in een hoorbare vorm.</skos:definition>
      <rdakit:toolkitDefinition xml:lang="nl">Content uitgedrukt door muziek in een hoorbare vorm.</rdakit:toolkitDefinition>
      <skos:prefLabel xml:lang="it">musica interpretata</skos:prefLabel>
      <rdakit:toolkitLabel xml:lang="it">musica interpretata</rdakit:toolkitLabel>
      <skos:definition xml:lang="it">Contenuto espresso mediante la musica in forma sonora.</skos:definition>
      <rdakit:toolkitDefinition xml:lang="it">Contenuto espresso mediante la musica in forma sonora.</rdakit:toolkitDefinition>
      <skos:scopeNote xml:lang="it">Include interpretazioni registrate di musica, musica generata con il computer.</skos:scopeNote>
      <skos:prefLabel xml:lang="fi">esitetty musiikki</skos:prefLabel>
      <rdakit:toolkitLabel xml:lang="fi">esitetty musiikki</rdakit:toolkitLabel>
      <skos:definition xml:lang="fi">Kuunneltavaksi tarkoitettu musiikki.</skos:definition>
      <rdakit:toolkitDefinition xml:lang="fi">Kuunneltavaksi tarkoitettu musiikki.</rdakit:toolkitDefinition>
      <skos:scopeNote xml:lang="fi">Sisältää esim. musiikkiesitysten tallennukset, tietokoneella tuotetun musiikin jne.</skos:scopeNote>
      <skos:prefLabel xml:lang="he">ביצוע מוסיקלי</skos:prefLabel>
      <rdakit:toolkitLabel xml:lang="he">ביצוע מוסיקלי</rdakit:toolkitLabel>
      <skos:definition xml:lang="he">סוג תוכן המכיל תוכן שקיבל את ביטויו באמצעות מוסיקה מושמעת.</skos:definition>
      <rdakit:toolkitDefinition xml:lang="he">סוג תוכן המכיל תוכן שקיבל את ביטויו באמצעות מוסיקה מושמעת.</rdakit:toolkitDefinition>
      <skos:scopeNote xml:lang="he">כולל הקלטות של ביצועים מוסיקליים, מוסיקה שנוצרה באמצעות מחשב, וכיוצ&quot;ב.</skos:scopeNote>
      <skos:prefLabel xml:lang="ar">موسيقى مؤداة</skos:prefLabel>
      <skos:prefLabel xml:lang="sv">framförd musik</skos:prefLabel>
      <rdakit:toolkitLabel xml:lang="sv">framförd musik</rdakit:toolkitLabel>
      <skos:prefLabel xml:lang="vi">âm nhạc biểu diễn</skos:prefLabel>
      <rdakit:toolkitLabel xml:lang="vi">âm nhạc biểu diễn</rdakit:toolkitLabel>
      <skos:definition xml:lang="vi">Loại nội dung được biểu hiện qua âm nhạc dưới hình thái thính giác.</skos:definition>
      <rdakit:toolkitDefinition xml:lang="vi">Loại nội dung được biểu hiện qua âm nhạc dưới hình thái thính giác.</rdakit:toolkitDefinition>
      <skos:scopeNote xml:lang="vi">Biểu diễn ghi âm âm nhạc, âm nhạc do máy tính tạo ra, v.v..., được bao gồm</skos:scopeNote>
      <skos:prefLabel xml:lang="da">opført musik</skos:prefLabel>
      <rdakit:toolkitLabel xml:lang="da">opført musik</rdakit:toolkitLabel>
      <skos:definition xml:lang="da">Indholdstyper der består af indhold udtrykt gennem musik i hørbar form. Inkl.</skos:definition>
      <rdakit:toolkitDefinition xml:lang="da">Indholdstyper der består af indhold udtrykt gennem musik i hørbar form. Inkl.</rdakit:toolkitDefinition>
      <skos:scopeNote xml:lang="da">Optagne/indspillede opførelser af musik, computergenereret musik etc. er omfattet.</skos:scopeNote>
      <skos:prefLabel xml:lang="no">framført musikk</skos:prefLabel>
      <rdakit:toolkitLabel xml:lang="no">framført musikk</rdakit:toolkitLabel>
      <skos:definition xml:lang="no">En innholdstype som består av innhold uttrykt gjennom musikk i hørbar form.</skos:definition>
      <rdakit:toolkitDefinition xml:lang="no">En innholdstype som består av innhold uttrykt gjennom musikk i hørbar form.</rdakit:toolkitDefinition>
      <skos:scopeNote xml:lang="no">Opptak av framføringer av musikk, datagenerert musikk, etc. er inkludert.</skos:scopeNote>
    </skos:Concept>
<!-- Concept: sounds  -->
    <skos:Concept rdf:about="http://rdaregistry.info/termList/RDAContentType/1012" xml:lang="en">
      <skos:inScheme rdf:resource="http://rdaregistry.info/termList/RDAContentType"/>
      <reg:status rdf:resource="http://metadataregistry.org/uri/RegStatus/1001"/>
      <reg:identifier rdf:resource="http://metadataregistry.org/concepts/521"/>
      <skos:prefLabel xml:lang="en">sounds</skos:prefLabel>
      <skos:definition xml:lang="en">A content type consisting of content other than language or music, expressed in an audible form.</skos:definition>
      <skos:scopeNote xml:lang="en">Natural sounds, artificially produced sounds, etc., are included.</skos:scopeNote>
      <skos:prefLabel xml:lang="de">Geräusche</skos:prefLabel>
      <skos:scopeNote xml:lang="de">Dazu gehören natürliche Geräusche, künstlich erzeugte Geräusche usw.</skos:scopeNote>
      <skos:definition xml:lang="de">Ein Inhaltstyp, der aus Inhalt (außer Sprache oder Musik) besteht, der in einer hörbaren Form ausgedrückt wird.</skos:definition>
	    <skos:related rdf:resource="http://rdaregistry.info/termList/RDAContentType/1007"/>
      <skos:prefLabel xml:lang="fr">sons</skos:prefLabel>
      <skos:definition xml:lang="fr">Type de contenu qui consiste en contenu, différent du langage ou de la musique, exprimé sous une forme audible.</skos:definition>
      <skos:scopeNote xml:lang="fr">Comprend les sons naturels, les sons artificiellement produits, etc.</skos:scopeNote>
      <skos:prefLabel xml:lang="es">sonidos</skos:prefLabel>
      <skos:definition xml:lang="es">Contenido diferente del lenguaje o la música, expresado en forma audible.</skos:definition>
      <skos:scopeNote xml:lang="es">Incluye sonidos naturales, sonidos producidos artificialmente, etc.</skos:scopeNote>
      <rdakit:toolkitLabel xml:lang="en">sounds</rdakit:toolkitLabel>
      <rdakit:toolkitLabel xml:lang="fr">sons</rdakit:toolkitLabel>
      <rdakit:toolkitDefinition xml:lang="en">A content type consisting of content other than language or music, expressed in an audible form.</rdakit:toolkitDefinition>
      <rdakit:toolkitDefinition xml:lang="fr">Type de contenu qui consiste en contenu, différent du langage ou de la musique, exprimé sous une forme audible.</rdakit:toolkitDefinition>
      <rdakit:toolkitLabel xml:lang="de">Geräusche</rdakit:toolkitLabel>
      <rdakit:toolkitDefinition xml:lang="de">Ein Inhaltstyp, der aus Inhalt (außer Sprache oder Musik) besteht, der in einer hörbaren Form ausgedrückt wird.</rdakit:toolkitDefinition>
      <rdakit:toolkitLabel xml:lang="es">sonidos</rdakit:toolkitLabel>
      <rdakit:toolkitDefinition xml:lang="es">Contenido diferente del lenguaje o la música, expresado en forma audible.</rdakit:toolkitDefinition>
      <skos:prefLabel xml:lang="zh">声音</skos:prefLabel>
      <rdakit:toolkitLabel xml:lang="zh">声音</rdakit:toolkitLabel>
      <skos:definition xml:lang="zh">除语言或音乐之外的、以可听见形式表达的内容。</skos:definition>
      <rdakit:toolkitDefinition xml:lang="zh">除语言或音乐之外的、以可听见形式表达的内容。</rdakit:toolkitDefinition>
      <skos:scopeNote xml:lang="zh">包括自然的声音、人工制造的声音等。</skos:scopeNote>
      <skos:prefLabel xml:lang="nl">geluiden</skos:prefLabel>
      <rdakit:toolkitLabel xml:lang="nl">geluiden</rdakit:toolkitLabel>
      <skos:definition xml:lang="nl">Content anders dan taal of muziek, uitgedrukt in een hoorbare vorm.</skos:definition>
      <rdakit:toolkitDefinition xml:lang="nl">Content anders dan taal of muziek, uitgedrukt in een hoorbare vorm.</rdakit:toolkitDefinition>
      <skos:prefLabel xml:lang="it">suoni</skos:prefLabel>
      <rdakit:toolkitLabel xml:lang="it">suoni</rdakit:toolkitLabel>
      <skos:definition xml:lang="it">Contenuto diverso dalla lingua o dalla musica, espresso in forma sonora.</skos:definition>
      <rdakit:toolkitDefinition xml:lang="it">Contenuto diverso dalla lingua o dalla musica, espresso in forma sonora.</rdakit:toolkitDefinition>
      <skos:scopeNote xml:lang="it">Include suoni naturali, suoni prodotti artificialmente, etc.</skos:scopeNote>
      <skos:prefLabel xml:lang="fi">ääni</skos:prefLabel>
      <rdakit:toolkitLabel xml:lang="fi">ääni</rdakit:toolkitLabel>
      <skos:definition xml:lang="fi">Kuunneltavaksi tarkoitettu muu äänisisältö kuin puhe tai musiikki.</skos:definition>
      <rdakit:toolkitDefinition xml:lang="fi">Kuunneltavaksi tarkoitettu muu äänisisältö kuin puhe tai musiikki.</rdakit:toolkitDefinition>
      <skos:scopeNote xml:lang="fi">Sisältää esim. luonnonäänet, keinotekoisesti tuotetut äänet jne.</skos:scopeNote>
      <skos:prefLabel xml:lang="he">קולות</skos:prefLabel>
      <rdakit:toolkitLabel xml:lang="he">קולות</rdakit:toolkitLabel>
      <skos:definition xml:lang="he">סוג תוכן המכיל תוכן שקיבל את ביטויו באמצעות קולות הניתנות לשמיעה, למעט שפה ומוסיקה.</skos:definition>
      <rdakit:toolkitDefinition xml:lang="he">סוג תוכן המכיל תוכן שקיבל את ביטויו באמצעות קולות הניתנות לשמיעה, למעט שפה ומוסיקה.</rdakit:toolkitDefinition>
      <skos:scopeNote xml:lang="he">כולל קולות טבעיים, קולות שהופקו בצורה מלאכותית וכיוצ&quot;ב.</skos:scopeNote>
      <skos:prefLabel xml:lang="ar">أصوات</skos:prefLabel>
      <skos:prefLabel xml:lang="sv">ljud (utom tal och musik)</skos:prefLabel>
      <rdakit:toolkitLabel xml:lang="sv">ljud (utom tal och musik)</rdakit:toolkitLabel>
      <skos:prefLabel xml:lang="vi">âm thanh</skos:prefLabel>
      <rdakit:toolkitLabel xml:lang="vi">âm thanh</rdakit:toolkitLabel>
      <skos:definition xml:lang="vi">Loại nội dung khác với ngôn ngữ hoặc âm nhạc, được biểu hiện trong một hình thái có thể nghe được.</skos:definition>
      <rdakit:toolkitDefinition xml:lang="vi">Loại nội dung khác với ngôn ngữ hoặc âm nhạc, được biểu hiện trong một hình thái có thể nghe được.</rdakit:toolkitDefinition>
      <skos:scopeNote xml:lang="vi">Âm thanh tự nhiên, âm thanh nhân tạo, v.v..., được bao gồm</skos:scopeNote>
      <skos:prefLabel xml:lang="da">lyde</skos:prefLabel>
      <rdakit:toolkitLabel xml:lang="da">lyde</rdakit:toolkitLabel>
      <skos:definition xml:lang="da">Indholdstype der består af indhold ud over tale eller musik, udtrykt i hørbar form.</skos:definition>
      <rdakit:toolkitDefinition xml:lang="da">Indholdstype der består af indhold ud over tale eller musik, udtrykt i hørbar form.</rdakit:toolkitDefinition>
      <skos:scopeNote xml:lang="da">Naturlige lyde, kunstigt fremstillede lyde etc. er omfattet.</skos:scopeNote>
      <skos:prefLabel xml:lang="no">lyder</skos:prefLabel>
      <rdakit:toolkitLabel xml:lang="no">lyder</rdakit:toolkitLabel>
      <skos:definition xml:lang="no">En innholdstype som består av annet innhold enn tale eller musikk, uttrykt i en hørbar form.</skos:definition>
      <rdakit:toolkitDefinition xml:lang="no">En innholdstype som består av annet innhold enn tale eller musikk, uttrykt i en hørbar form.</rdakit:toolkitDefinition>
      <skos:scopeNote xml:lang="no">Lyder fra naturen, kunstig produserte lyder, etc. er inkludert.</skos:scopeNote>
    </skos:Concept>
<!-- Concept: spoken word  -->
    <skos:Concept rdf:about="http://rdaregistry.info/termList/RDAContentType/1013" xml:lang="en">
      <skos:inScheme rdf:resource="http://rdaregistry.info/termList/RDAContentType"/>
      <reg:status rdf:resource="http://metadataregistry.org/uri/RegStatus/1001"/>
      <reg:identifier rdf:resource="http://metadataregistry.org/concepts/522"/>
      <skos:prefLabel xml:lang="en">spoken word</skos:prefLabel>
      <skos:definition xml:lang="en">A content type consisting of content expressed through language in an audible form.</skos:definition>
      <skos:scopeNote xml:lang="en">Recorded readings, recitations, speeches, interviews, oral histories, etc., computer-generated speech, etc., are included.</skos:scopeNote>
      <skos:prefLabel xml:lang="de">Gesprochenes Wort</skos:prefLabel>
      <skos:scopeNote xml:lang="de">Dazu gehören Lesungen, Rezitationen, Reden, Interviews, mündliche Geschichte, usw., computer-erzeugte Sprache usw.</skos:scopeNote>
      <skos:definition xml:lang="de">Ein Inhaltstyp, der aus Inhalt besteht, der durch Sprache in einer hörbaren Form ausgedrückt wird.</skos:definition>
	    <skos:related rdf:resource="http://rdaregistry.info/termList/RDAContentType/1007"/>
      <skos:prefLabel xml:lang="fr">parole énoncée</skos:prefLabel>
      <skos:definition xml:lang="fr">Type de contenu qui consiste en contenu exprimé au moyen du langage sous une forme audible.</skos:definition>
      <skos:prefLabel xml:lang="es">palabra hablada</skos:prefLabel>
      <skos:definition xml:lang="es">Contenido expresado mediante lenguaje en una forma audible.</skos:definition>
      <skos:scopeNote xml:lang="es">Incluye lecturas grabadas, recitales, discursos, entrevistas, historias orales, etc., discursos generado por computadora, etc.</skos:scopeNote>
      <rdakit:toolkitLabel xml:lang="en">spoken word</rdakit:toolkitLabel>
      <rdakit:toolkitLabel xml:lang="fr">parole énoncée</rdakit:toolkitLabel>
      <rdakit:toolkitDefinition xml:lang="en">A content type consisting of content expressed through language in an audible form.</rdakit:toolkitDefinition>
      <rdakit:toolkitDefinition xml:lang="fr">Type de contenu qui consiste en contenu exprimé au moyen du langage sous une forme audible.</rdakit:toolkitDefinition>
      <rdakit:toolkitLabel xml:lang="de">Gesprochenes Wort</rdakit:toolkitLabel>
      <rdakit:toolkitDefinition xml:lang="de">Ein Inhaltstyp, der aus Inhalt besteht, der durch Sprache in einer hörbaren Form ausgedrückt wird.</rdakit:toolkitDefinition>
      <rdakit:toolkitLabel xml:lang="es">palabra hablada</rdakit:toolkitLabel>
      <rdakit:toolkitDefinition xml:lang="es">Contenido expresado mediante lenguaje en una forma audible.</rdakit:toolkitDefinition>
      <skos:prefLabel xml:lang="zh">口头表述</skos:prefLabel>
      <rdakit:toolkitLabel xml:lang="zh">口头表述</rdakit:toolkitLabel>
      <skos:definition xml:lang="zh">以可听见形式的语言表达的内容。</skos:definition>
      <rdakit:toolkitDefinition xml:lang="zh">以可听见形式的语言表达的内容。</rdakit:toolkitDefinition>
      <skos:scopeNote xml:lang="zh">包括录制的朗读、背诵、演讲、采访、口述史等、计算机生成的演说等。</skos:scopeNote>
      <skos:prefLabel xml:lang="nl">gesproken woord</skos:prefLabel>
      <rdakit:toolkitLabel xml:lang="nl">gesproken woord</rdakit:toolkitLabel>
      <skos:definition xml:lang="nl">Content uitgedrukt door taal in een hoorbare vorm.</skos:definition>
      <rdakit:toolkitDefinition xml:lang="nl">Content uitgedrukt door taal in een hoorbare vorm.</rdakit:toolkitDefinition>
      <skos:prefLabel xml:lang="it">parlato</skos:prefLabel>
      <rdakit:toolkitLabel xml:lang="it">parlato</rdakit:toolkitLabel>
      <skos:definition xml:lang="it">Contenuto espresso mediante la lingua in forma sonora.</skos:definition>
      <rdakit:toolkitDefinition xml:lang="it">Contenuto espresso mediante la lingua in forma sonora.</rdakit:toolkitDefinition>
      <skos:scopeNote xml:lang="it">Include letture, recitazioni, discorsi, interviste, storie orali etc. registrate, linguaggio generato dal computer, etc.</skos:scopeNote>
      <skos:prefLabel xml:lang="fi">puhe</skos:prefLabel>
      <rdakit:toolkitLabel xml:lang="fi">puhe</rdakit:toolkitLabel>
      <skos:definition xml:lang="fi">Kuunneltavaksi tarkoitettu kielellinen sisältö.</skos:definition>
      <rdakit:toolkitDefinition xml:lang="fi">Kuunneltavaksi tarkoitettu kielellinen sisältö.</rdakit:toolkitDefinition>
      <skos:scopeNote xml:lang="fi">Sisältä esim. puheäänitteet, runonlausunnat, puheet, haastattelut, suulliset tarinat, tietokoneella tuotetun puheen jne</skos:scopeNote>
      <skos:prefLabel xml:lang="he">מילה מדוברת</skos:prefLabel>
      <rdakit:toolkitLabel xml:lang="he">מילה מדוברת</rdakit:toolkitLabel>
      <skos:definition xml:lang="he">סוג תוכן המכיל תוכן שקיבל את ביטויו באמצעות שפה שניתנת לשמיעה.</skos:definition>
      <rdakit:toolkitDefinition xml:lang="he">סוג תוכן המכיל תוכן שקיבל את ביטויו באמצעות שפה שניתנת לשמיעה.</rdakit:toolkitDefinition>
      <skos:scopeNote xml:lang="he">כולל קריאות מוקלטות, דקלומים, נאומים, ראיונות, היסטוריה אורלית, וכו', דיבור שנוצר באמצעות מחשב וכיוצ&quot;ב.</skos:scopeNote>
      <skos:prefLabel xml:lang="ar">كلمة منطوقة</skos:prefLabel>
      <skos:prefLabel xml:lang="sv">tal</skos:prefLabel>
      <rdakit:toolkitLabel xml:lang="sv">tal</rdakit:toolkitLabel>
      <skos:prefLabel xml:lang="vi">từ nói</skos:prefLabel>
      <rdakit:toolkitLabel xml:lang="vi">từ nói</rdakit:toolkitLabel>
      <skos:definition xml:lang="vi">Loại nội dung biểu hiện qua ngôn ngữ trong hình thái có thể nghe được.</skos:definition>
      <rdakit:toolkitDefinition xml:lang="vi">Loại nội dung biểu hiện qua ngôn ngữ trong hình thái có thể nghe được.</rdakit:toolkitDefinition>
      <skos:scopeNote xml:lang="vi">Bản ghi âm, kể lại, bài nói, phỏng vấn, lịch sử truyền miệng, v.v..., bài nói do máy tính sinh ra, v.v.., được bao gồm</skos:scopeNote>
      <skos:prefLabel xml:lang="da">talt ord</skos:prefLabel>
      <rdakit:toolkitLabel xml:lang="da">talt ord</rdakit:toolkitLabel>
      <skos:definition xml:lang="da">Indholdstype der består af indhold udtrykt gennem sprog i hørbar form.</skos:definition>
      <rdakit:toolkitDefinition xml:lang="da">Indholdstype der består af indhold udtrykt gennem sprog i hørbar form.</rdakit:toolkitDefinition>
      <skos:scopeNote xml:lang="da">Optagne oplæsninger, recitationer, taler, interviews, mundtlige historier etc., computergenereret tale etc. er omfattet.</skos:scopeNote>
      <skos:prefLabel xml:lang="no">tale</skos:prefLabel>
      <rdakit:toolkitLabel xml:lang="no">tale</rdakit:toolkitLabel>
      <skos:definition xml:lang="no">En innholdstype som består av innhold uttrykt gjennom språk i hørbar form.</skos:definition>
      <rdakit:toolkitDefinition xml:lang="no">En innholdstype som består av innhold uttrykt gjennom språk i hørbar form.</rdakit:toolkitDefinition>
      <skos:scopeNote xml:lang="no">Innlest tekst, resitasjoner, taler, intervjuer, muntlige fortellinger etc., datagenerert tale, etc. er inkludert.</skos:scopeNote>
    </skos:Concept>
<!-- Concept: still image  -->
    <skos:Concept rdf:about="http://rdaregistry.info/termList/RDAContentType/1014" xml:lang="en">
      <skos:inScheme rdf:resource="http://rdaregistry.info/termList/RDAContentType"/>
      <reg:status rdf:resource="http://metadataregistry.org/uri/RegStatus/1001"/>
      <reg:identifier rdf:resource="http://metadataregistry.org/concepts/523"/>
      <skos:prefLabel xml:lang="en">still image</skos:prefLabel>
      <skos:definition xml:lang="en">A content type consisting of content expressed through line, shape, shading, etc., intended to be perceived visually as a still image or images in two dimensions.</skos:definition>
      <skos:scopeNote xml:lang="en">Drawings, paintings, diagrams, photographic images known as stills, etc., are included.</skos:scopeNote>
      <skos:prefLabel xml:lang="de">Unbewegtes Bild</skos:prefLabel>
      <skos:scopeNote xml:lang="de">Dazu gehören Zeichnungen, Gemälde, Diagramme, Fotografien (einzelne) usw.</skos:scopeNote>
      <skos:definition xml:lang="de">Ein Inhaltstyp, der aus Inhalt besteht, der durch Linie, Form, Schattierung usw. ausgedrückt wird und konzipiert ist, um visuell zweidimensional als unbewegtes Bild oder Bilder wahrgenommen zu werden.</skos:definition>
      <skos:scopeNote xml:lang="en">For cartographic content intended to be perceived as a two-dimensional image, see cartographic image.</skos:scopeNote>
      <skos:scopeNote xml:lang="en">For images intended to be perceived through touch, see tactile image.</skos:scopeNote>
	    <skos:related rdf:resource="http://rdaregistry.info/termList/RDAContentType/1007"/>
	    <skos:related rdf:resource="http://rdaregistry.info/termList/RDAContentType/1002"/>
	    <skos:related rdf:resource="http://rdaregistry.info/termList/RDAContentType/1015"/>
      <skos:prefLabel xml:lang="fr">image fixe</skos:prefLabel>
      <skos:definition xml:lang="fr">Type de contenu qui consiste en contenu exprimé au moyen de lignes, de contours, d’estompage, etc. destinés à être perçus visuellement comme une ou plusieurs images fixes en deux dimensions.</skos:definition>
      <skos:scopeNote xml:lang="fr">Comprend les dessins, les peintures, les diagrammes, les images photographiques fixes, etc.</skos:scopeNote>
      <skos:prefLabel xml:lang="es">imagen fija</skos:prefLabel>
      <skos:definition xml:lang="es">Contenido expresado mediante líneas, forma, sombreado, etc., pensado para ser percibido visualmente como una imagen fija o imágenes en dos dimensiones.</skos:definition>
      <rdakit:toolkitLabel xml:lang="en">still image</rdakit:toolkitLabel>
      <rdakit:toolkitLabel xml:lang="fr">image fixe</rdakit:toolkitLabel>
      <rdakit:toolkitDefinition xml:lang="en">A content type consisting of content expressed through line, shape, shading, etc., intended to be perceived visually as a still image or images in two dimensions.</rdakit:toolkitDefinition>
      <rdakit:toolkitDefinition xml:lang="fr">Type de contenu qui consiste en contenu exprimé au moyen de lignes, de contours, d’estompage, etc. destinés à être perçus visuellement comme une ou plusieurs images fixes en deux dimensions.</rdakit:toolkitDefinition>
      <rdakit:toolkitLabel xml:lang="de">Unbewegtes Bild</rdakit:toolkitLabel>
      <rdakit:toolkitDefinition xml:lang="de">Ein Inhaltstyp, der aus Inhalt besteht, der durch Linie, Form, Schattierung usw. ausgedrückt wird und konzipiert ist, um visuell zweidimensional als unbewegtes Bild oder Bilder wahrgenommen zu werden.</rdakit:toolkitDefinition>
      <rdakit:toolkitLabel xml:lang="es">imagen fija</rdakit:toolkitLabel>
      <rdakit:toolkitDefinition xml:lang="es">Contenido expresado mediante líneas, forma, sombreado, etc., pensado para ser percibido visualmente como una imagen fija o imágenes en dos dimensiones.</rdakit:toolkitDefinition>
      <skos:prefLabel xml:lang="zh">静态图像</skos:prefLabel>
      <rdakit:toolkitLabel xml:lang="zh">静态图像</rdakit:toolkitLabel>
      <skos:definition xml:lang="zh">以线条、形状、阴影等表达的，旨在通过视觉感知的一种或多种二维静态图像内容。</skos:definition>
      <rdakit:toolkitDefinition xml:lang="zh">以线条、形状、阴影等表达的，旨在通过视觉感知的一种或多种二维静态图像内容。</rdakit:toolkitDefinition>
      <skos:scopeNote xml:lang="zh">包括绘图、绘画、线图、摄影图像（静态）等。</skos:scopeNote>
      <skos:scopeNote xml:lang="es">Incluye dibujos, pinturas, diagramas, imágenes fotográficas (fijas), etc.</skos:scopeNote>
      <skos:prefLabel xml:lang="nl">niet-bewegend beeld</skos:prefLabel>
      <rdakit:toolkitLabel xml:lang="nl">niet-bewegend beeld</rdakit:toolkitLabel>
      <skos:definition xml:lang="nl">Content uitgedrukt door lijnen, vormen, schaduw etc., bedoeld om visueel waar te nemen als een stilstaand beeld of beelden in twee dimensies.</skos:definition>
      <rdakit:toolkitDefinition xml:lang="nl">Content uitgedrukt door lijnen, vormen, schaduw etc., bedoeld om visueel waar te nemen als een stilstaand beeld of beelden in twee dimensies.</rdakit:toolkitDefinition>
      <skos:prefLabel xml:lang="it">immagine fissa</skos:prefLabel>
      <rdakit:toolkitLabel xml:lang="it">immagine fissa</rdakit:toolkitLabel>
      <skos:definition xml:lang="it">Contenuto espresso mediante linea, figura, ombreggiatura, etc., percepibile mediante la vista in due dimensioni.</skos:definition>
      <rdakit:toolkitDefinition xml:lang="it">Contenuto espresso mediante linea, figura, ombreggiatura, etc., percepibile mediante la vista in due dimensioni.</rdakit:toolkitDefinition>
      <skos:scopeNote xml:lang="it">Include disegni, pitture, diagrammi, immagini fotografiche (fisse), etc.</skos:scopeNote>
      <skos:prefLabel xml:lang="fi">stillkuva</skos:prefLabel>
      <rdakit:toolkitLabel xml:lang="fi">stillkuva</rdakit:toolkitLabel>
      <skos:definition xml:lang="fi">Viivoina, muotoina, varjostuksina jne. esitetty sisältö, joka on tarkoitettu katsottavaksi kaksiulotteisena stillkuvana tai -kuvina.</skos:definition>
      <rdakit:toolkitDefinition xml:lang="fi">Viivoina, muotoina, varjostuksina jne. esitetty sisältö, joka on tarkoitettu katsottavaksi kaksiulotteisena stillkuvana tai -kuvina.</rdakit:toolkitDefinition>
      <skos:scopeNote xml:lang="fi">Esimerkiksi piirrokset, maalaukset, diagrammit, valokuvat jne.</skos:scopeNote>
      <skos:prefLabel xml:lang="he">תמונה</skos:prefLabel>
      <rdakit:toolkitLabel xml:lang="he">תמונה</rdakit:toolkitLabel>
      <skos:definition xml:lang="he">סוג תוכן המכיל תוכן אשר קיבל את ביטויו באמצעות קווים, צורות, גיוון צבעים וכד', ומיועד לצפייה כתמונה (או תמונות) דו-ממדית.</skos:definition>
      <rdakit:toolkitDefinition xml:lang="he">סוג תוכן המכיל תוכן אשר קיבל את ביטויו באמצעות קווים, צורות, גיוון צבעים וכד', ומיועד לצפייה כתמונה (או תמונות) דו-ממדית.</rdakit:toolkitDefinition>
      <skos:scopeNote xml:lang="he">כולל רישומים, ציורים, דיאגראמות, תצלומים וכו'.</skos:scopeNote>
      <skos:prefLabel xml:lang="ar">صورة ساكنة</skos:prefLabel>
      <skos:prefLabel xml:lang="sv">stillbild</skos:prefLabel>
      <rdakit:toolkitLabel xml:lang="sv">stillbild</rdakit:toolkitLabel>
      <skos:prefLabel xml:lang="vi">hình ảnh tĩnh</skos:prefLabel>
      <rdakit:toolkitLabel xml:lang="vi">hình ảnh tĩnh</rdakit:toolkitLabel>
      <skos:definition xml:lang="vi">Loại nội dung được biểu hiện qua đường nét, hình dạng, hình bóng, v.v... để nhận biết bằng thị giác như là hình ảnh tĩnh trong ở hai chiều.</skos:definition>
      <rdakit:toolkitDefinition xml:lang="vi">Loại nội dung được biểu hiện qua đường nét, hình dạng, hình bóng, v.v... để nhận biết bằng thị giác như là hình ảnh tĩnh trong ở hai chiều.</rdakit:toolkitDefinition>
      <skos:scopeNote xml:lang="vi">Bản vẽ, đồ hoạ, đồ hình, ảnh chụp được biết tới như là hình ảnh tĩnh được bao gồm</skos:scopeNote>
      <skos:prefLabel xml:lang="da">fast billede</skos:prefLabel>
      <rdakit:toolkitLabel xml:lang="da">fast billede</rdakit:toolkitLabel>
      <skos:definition xml:lang="da">Indholdstype der består af indhold udtrykt som en linje, en figur, en skravering etc. mhp. at blive opfattet visuelt i to dimensioner.</skos:definition>
      <rdakit:toolkitDefinition xml:lang="da">Indholdstype der består af indhold udtrykt som en linje, en figur, en skravering etc. mhp. at blive opfattet visuelt i to dimensioner.</rdakit:toolkitDefinition>
      <skos:scopeNote xml:lang="da">Tegninger, malerier, diagrammer, fotografiske billeder (stillbilleder) etc. er omfattet.</skos:scopeNote>
      <skos:prefLabel xml:lang="no">stillbilde</skos:prefLabel>
      <rdakit:toolkitLabel xml:lang="no">stillbilde</rdakit:toolkitLabel>
      <skos:definition xml:lang="no">En innholdstype som består av innhold uttrykt gjennom linjer, former, skyggelegging etc., som skal oppfattes visuelt som ett eller flere stillbilder i to dimensjoner.</skos:definition>
      <rdakit:toolkitDefinition xml:lang="no">En innholdstype som består av innhold uttrykt gjennom linjer, former, skyggelegging etc., som skal oppfattes visuelt som ett eller flere stillbilder i to dimensjoner.</rdakit:toolkitDefinition>
      <skos:scopeNote xml:lang="no">Tegninger, malerier, diagrammer, fotografiske stillbilder etc. er inkludert. For kartografisk innhold som skal oppfattes som et todimensjonalt levende bilde, se kartografisk bilde. For bilder som skal oppfattes gjennom berøring, se taktilt bilde.</skos:scopeNote>
    </skos:Concept>
<!-- Concept: tactile image  -->
    <skos:Concept rdf:about="http://rdaregistry.info/termList/RDAContentType/1015" xml:lang="en">
      <skos:inScheme rdf:resource="http://rdaregistry.info/termList/RDAContentType"/>
      <reg:status rdf:resource="http://metadataregistry.org/uri/RegStatus/1001"/>
      <reg:identifier rdf:resource="http://metadataregistry.org/concepts/524"/>
      <skos:prefLabel xml:lang="en">tactile image</skos:prefLabel>
      <skos:definition xml:lang="en">A content type consisting of content expressed through line, shape, and/or other forms, intended to be perceived through touch as a still image in two dimensions.</skos:definition>
      <skos:prefLabel xml:lang="de">Taktiles Bild</skos:prefLabel>
      <skos:definition xml:lang="de">Ein Inhaltstyp, der aus Inhalt besteht, der durch Linie, Form und/oder andere Gestaltung ausgedrückt wird und konzipiert ist, um über den Tastsinn zweidimensional als unbewegtes Bild oder Bilder wahrgenommen zu werden.</skos:definition>
	    <skos:related rdf:resource="http://rdaregistry.info/termList/RDAContentType/1014"/>
      <skos:prefLabel xml:lang="fr">image tactile</skos:prefLabel>
      <skos:definition xml:lang="fr">Type de contenu qui consiste en contenu exprimé au moyen de lignes, de contours et/ou d’autres formes destinés à être perçus au toucher comme une image fixe en deux dimensions.</skos:definition>
      <skos:prefLabel xml:lang="es">imagen táctil</skos:prefLabel>
      <skos:definition xml:lang="es">Contenido expresado mediante líneas, forma, y/u otras formas, destinadas para ser percibidas mediante el tacto como imagen fija en dos dimensiones.</skos:definition>
      <rdakit:toolkitLabel xml:lang="en">tactile image</rdakit:toolkitLabel>
      <rdakit:toolkitLabel xml:lang="fr">image tactile</rdakit:toolkitLabel>
      <rdakit:toolkitDefinition xml:lang="en">A content type consisting of content expressed through line, shape, and/or other forms, intended to be perceived through touch as a still image in two dimensions.</rdakit:toolkitDefinition>
      <rdakit:toolkitDefinition xml:lang="fr">Type de contenu qui consiste en contenu exprimé au moyen de lignes, de contours et/ou d’autres formes destinés à être perçus au toucher comme une image fixe en deux dimensions.</rdakit:toolkitDefinition>
      <rdakit:toolkitLabel xml:lang="de">Taktiles Bild</rdakit:toolkitLabel>
      <rdakit:toolkitDefinition xml:lang="de">Ein Inhaltstyp, der aus Inhalt besteht, der durch Linie, Form und/oder andere Gestaltung ausgedrückt wird und konzipiert ist, um über den Tastsinn zweidimensional als unbewegtes Bild oder Bilder wahrgenommen zu werden.</rdakit:toolkitDefinition>
      <rdakit:toolkitLabel xml:lang="es">imagen táctil</rdakit:toolkitLabel>
      <rdakit:toolkitDefinition xml:lang="es">Contenido expresado mediante líneas, forma, y/u otras formas, destinadas para ser percibidas mediante el tacto como imagen fija en dos dimensiones.</rdakit:toolkitDefinition>
      <skos:prefLabel xml:lang="zh">触摸图像</skos:prefLabel>
      <rdakit:toolkitLabel xml:lang="zh">触摸图像</rdakit:toolkitLabel>
      <skos:definition xml:lang="zh">以线条、形状和/或其他形式表达的、旨在通过触觉感知的二维静态图像内容。</skos:definition>
      <rdakit:toolkitDefinition xml:lang="zh">以线条、形状和/或其他形式表达的、旨在通过触觉感知的二维静态图像内容。</rdakit:toolkitDefinition>
      <skos:prefLabel xml:lang="nl">tactiele afbeelding</skos:prefLabel>
      <rdakit:toolkitLabel xml:lang="nl">tactiele afbeelding</rdakit:toolkitLabel>
      <skos:definition xml:lang="nl">Content uitgedrukt door lijnen, vormen etc., bedoeld om waar te nemen door aanraking als een stilstaand beeld in twee dimensies.</skos:definition>
      <rdakit:toolkitDefinition xml:lang="nl">Content uitgedrukt door lijnen, vormen etc., bedoeld om waar te nemen door aanraking als een stilstaand beeld in twee dimensies.</rdakit:toolkitDefinition>
      <skos:prefLabel xml:lang="it">immagine tattile</skos:prefLabel>
      <rdakit:toolkitLabel xml:lang="it">immagine tattile</rdakit:toolkitLabel>
      <skos:definition xml:lang="it">Contenuto espresso mediante linea, figura e/o altre forme, percepibile mediante il tatto come immagine fissa bidimensionale.</skos:definition>
      <rdakit:toolkitDefinition xml:lang="it">Contenuto espresso mediante linea, figura e/o altre forme, percepibile mediante il tatto come immagine fissa bidimensionale.</rdakit:toolkitDefinition>
      <skos:prefLabel xml:lang="fi">taktiili kuva</skos:prefLabel>
      <rdakit:toolkitLabel xml:lang="fi">taktiili kuva</rdakit:toolkitLabel>
      <skos:definition xml:lang="fi">Viivoina, muotoina jne. esitetty sisältö, joka on tarkoitettu kosketeltavaksi kaksiulotteiseksi stillkuvaksi tai -kuviksi.</skos:definition>
      <rdakit:toolkitDefinition xml:lang="fi">Viivoina, muotoina jne. esitetty sisältö, joka on tarkoitettu kosketeltavaksi kaksiulotteiseksi stillkuvaksi tai -kuviksi.</rdakit:toolkitDefinition>
      <skos:prefLabel xml:lang="he">תמונה מישושית</skos:prefLabel>
      <rdakit:toolkitLabel xml:lang="he">תמונה מישושית</rdakit:toolkitLabel>
      <skos:definition xml:lang="he">סוג תוכן המכיל תוכן אשר קיבל את ביטויו באמצעות קווים, צורות וכד', ומיועד לתפיסה על ידי מישוש כתמונה דו-ממדית.</skos:definition>
      <rdakit:toolkitDefinition xml:lang="he">סוג תוכן המכיל תוכן אשר קיבל את ביטויו באמצעות קווים, צורות וכד', ומיועד לתפיסה על ידי מישוש כתמונה דו-ממדית.</rdakit:toolkitDefinition>
      <skos:prefLabel xml:lang="ar">صورة لمسية</skos:prefLabel>
      <skos:prefLabel xml:lang="sv">taktil bild</skos:prefLabel>
      <rdakit:toolkitLabel xml:lang="sv">taktil bild</rdakit:toolkitLabel>
      <skos:prefLabel xml:lang="vi">hình ảnh xúc giác</skos:prefLabel>
      <rdakit:toolkitLabel xml:lang="vi">hình ảnh xúc giác</rdakit:toolkitLabel>
      <skos:definition xml:lang="vi">Loại nội dung được biểu hiện qua đường nét, hình dạng, và/hoặc hình thái khác, để nhận biết qua xúc giác như là hình ảnh tĩnh ở hai chiều.</skos:definition>
      <rdakit:toolkitDefinition xml:lang="vi">Loại nội dung được biểu hiện qua đường nét, hình dạng, và/hoặc hình thái khác, để nhận biết qua xúc giác như là hình ảnh tĩnh ở hai chiều.</rdakit:toolkitDefinition>
      <skos:prefLabel xml:lang="da">taktilt billede</skos:prefLabel>
      <rdakit:toolkitLabel xml:lang="da">taktilt billede</rdakit:toolkitLabel>
      <skos:definition xml:lang="da">Indholdstype der består af indhold udtrykt som en linje, en figur og/eller andre former mhp. at blive opfattet ved berøring som et fast todimensionelt billede.</skos:definition>
      <rdakit:toolkitDefinition xml:lang="da">Indholdstype der består af indhold udtrykt som en linje, en figur og/eller andre former mhp. at blive opfattet ved berøring som et fast todimensionelt billede.</rdakit:toolkitDefinition>
      <skos:prefLabel xml:lang="no">taktilt bilde</skos:prefLabel>
      <rdakit:toolkitLabel xml:lang="no">taktilt bilde</rdakit:toolkitLabel>
      <skos:definition xml:lang="no">En innholdstype som består av innhold uttrykt gjennom linjer og/eller andre former, som skal oppfattes gjennom berøring som et stillbilde i to dimensjoner.</skos:definition>
      <rdakit:toolkitDefinition xml:lang="no">En innholdstype som består av innhold uttrykt gjennom linjer og/eller andre former, som skal oppfattes gjennom berøring som et stillbilde i to dimensjoner.</rdakit:toolkitDefinition>
    </skos:Concept>
<!-- Concept: tactile notated movement  -->
    <skos:Concept rdf:about="http://rdaregistry.info/termList/RDAContentType/1017" xml:lang="en">
      <skos:inScheme rdf:resource="http://rdaregistry.info/termList/RDAContentType"/>
      <reg:status rdf:resource="http://metadataregistry.org/uri/RegStatus/1001"/>
      <reg:identifier rdf:resource="http://metadataregistry.org/concepts/526"/>
      <skos:prefLabel xml:lang="en">tactile notated movement</skos:prefLabel>
      <skos:definition xml:lang="en">A content type consisting of content expressed through a form of notation for movement intended to be perceived through touch.</skos:definition>
      <skos:prefLabel xml:lang="de">Taktile Bewegungsnotation</skos:prefLabel>
      <skos:definition xml:lang="de">Ein Inhaltstyp, der aus Inhalt besteht, der durch eine Notationsform für Bewegung ausgedrückt wird und konzipiert ist, um über den Tastsinn wahrgenommen zu werden.</skos:definition>
	    <skos:related rdf:resource="http://rdaregistry.info/termList/RDAContentType/1009"/>
      <skos:prefLabel xml:lang="fr">mouvement noté tactile</skos:prefLabel>
      <skos:definition xml:lang="fr">Type de contenu qui consiste en contenu exprimé au moyen d’une forme de notation du mouvement destinée à être perçue au toucher.</skos:definition>
      <skos:prefLabel xml:lang="es">movimiento notado táctil</skos:prefLabel>
      <skos:definition xml:lang="es">Contenido expresado mediante una forma de notación para movimiento pensado para ser percibido mediante el tacto.</skos:definition>
      <rdakit:toolkitLabel xml:lang="en">tactile notated movement</rdakit:toolkitLabel>
      <rdakit:toolkitLabel xml:lang="fr">mouvement noté tactile</rdakit:toolkitLabel>
      <rdakit:toolkitDefinition xml:lang="en">A content type consisting of content expressed through a form of notation for movement intended to be perceived through touch.</rdakit:toolkitDefinition>
      <rdakit:toolkitDefinition xml:lang="fr">Type de contenu qui consiste en contenu exprimé au moyen d’une forme de notation du mouvement destinée à être perçue au toucher.</rdakit:toolkitDefinition>
      <rdakit:toolkitLabel xml:lang="de">Taktile Bewegungsnotation</rdakit:toolkitLabel>
      <rdakit:toolkitDefinition xml:lang="de">Ein Inhaltstyp, der aus Inhalt besteht, der durch eine Notationsform für Bewegung ausgedrückt wird und konzipiert ist, um über den Tastsinn wahrgenommen zu werden.</rdakit:toolkitDefinition>
      <rdakit:toolkitLabel xml:lang="es">movimiento notado táctil</rdakit:toolkitLabel>
      <rdakit:toolkitDefinition xml:lang="es">Contenido expresado mediante una forma de notación para movimiento pensado para ser percibido mediante el tacto.</rdakit:toolkitDefinition>
      <skos:prefLabel xml:lang="zh">触摸动作谱</skos:prefLabel>
      <rdakit:toolkitLabel xml:lang="zh">触摸动作谱</rdakit:toolkitLabel>
      <skos:definition xml:lang="zh">以动作记谱形式表达的、旨在通过触觉感知的内容。</skos:definition>
      <rdakit:toolkitDefinition xml:lang="zh">以动作记谱形式表达的、旨在通过触觉感知的内容。</rdakit:toolkitDefinition>
      <skos:prefLabel xml:lang="nl">tactiele beschreven beweging</skos:prefLabel>
      <skos:altLabel xml:lang="nl">tactiele bewegingsnotatie</skos:altLabel>
      <rdakit:toolkitLabel xml:lang="nl">tactiele beschreven beweging</rdakit:toolkitLabel>
      <skos:definition xml:lang="nl">Content uitgedrukt door een vorm van bewegingsnotatie bedoeld om waar te nemen door aanraking.</skos:definition>
      <rdakit:toolkitDefinition xml:lang="nl">Content uitgedrukt door een vorm van bewegingsnotatie bedoeld om waar te nemen door aanraking.</rdakit:toolkitDefinition>
      <skos:prefLabel xml:lang="it">movimento notato tattile</skos:prefLabel>
      <rdakit:toolkitLabel xml:lang="it">movimento notato tattile</rdakit:toolkitLabel>
      <skos:definition xml:lang="it">Contenuto espresso mediante una forma di notazione per il movimento percepibile mediante il tatto.</skos:definition>
      <rdakit:toolkitDefinition xml:lang="it">Contenuto espresso mediante una forma di notazione per il movimento percepibile mediante il tatto.</rdakit:toolkitDefinition>
      <skos:prefLabel xml:lang="fi">taktiili liikenotaatio</skos:prefLabel>
      <rdakit:toolkitLabel xml:lang="fi">taktiili liikenotaatio</rdakit:toolkitLabel>
      <skos:definition xml:lang="fi">Liikettä kuvailevan merkkijärjestelmän avulla esitetty sisältö, joka on tarkoitettu kosketeltavaksi.</skos:definition>
      <rdakit:toolkitDefinition xml:lang="fi">Liikettä kuvailevan merkkijärjestelmän avulla esitetty sisältö, joka on tarkoitettu kosketeltavaksi.</rdakit:toolkitDefinition>
      <skos:prefLabel xml:lang="he">תווי מוסיקה מישושיים</skos:prefLabel>
      <rdakit:toolkitLabel xml:lang="he">תווי מוסיקה מישושיים</rdakit:toolkitLabel>
      <skos:definition xml:lang="he">סוג תוכן המכיל תוכן שקיבל את ביטויו באמצעות תווי מוסיקה, המיועדים לתפיסה על ידי מישוש.</skos:definition>
      <rdakit:toolkitDefinition xml:lang="he">סוג תוכן המכיל תוכן שקיבל את ביטויו באמצעות תווי מוסיקה, המיועדים לתפיסה על ידי מישוש.</rdakit:toolkitDefinition>
      <skos:prefLabel xml:lang="ar">حركة مدونة لمسية</skos:prefLabel>
      <skos:prefLabel xml:lang="vi">động thái ký hiệu xúc giác</skos:prefLabel>
      <rdakit:toolkitLabel xml:lang="vi">động thái ký hiệu xúc giác</rdakit:toolkitLabel>
      <skos:definition xml:lang="vi">Loại nội dung được biểu hiện qua hình thái của ký hiệu cho động thái nhằm mục đích nhận biết qua xúc giác.</skos:definition>
      <rdakit:toolkitDefinition xml:lang="vi">Loại nội dung được biểu hiện qua hình thái của ký hiệu cho động thái nhằm mục đích nhận biết qua xúc giác.</rdakit:toolkitDefinition>
      <skos:prefLabel xml:lang="da">taktil noteret bevægelse</skos:prefLabel>
      <rdakit:toolkitLabel xml:lang="da">taktil noteret bevægelse</rdakit:toolkitLabel>
      <skos:definition xml:lang="da">Indholdstype der består af indhold udtrykt vha. en form for bevægelsesnotation, beregnet til at opfattes ved berøring.</skos:definition>
      <rdakit:toolkitDefinition xml:lang="da">Indholdstype der består af indhold udtrykt vha. en form for bevægelsesnotation, beregnet til at opfattes ved berøring.</rdakit:toolkitDefinition>
      <skos:prefLabel xml:lang="no">taktil bevegelsesnotasjon</skos:prefLabel>
      <rdakit:toolkitLabel xml:lang="no">taktil bevegelsesnotasjon</rdakit:toolkitLabel>
      <skos:definition xml:lang="no">En innholdstype som består av innhold uttrykt ved hjelp av en form for bevegelsesnotasjon som er ment å oppfattes gjennom berøring.</skos:definition>
      <rdakit:toolkitDefinition xml:lang="no">En innholdstype som består av innhold uttrykt ved hjelp av en form for bevegelsesnotasjon som er ment å oppfattes gjennom berøring.</rdakit:toolkitDefinition>
    </skos:Concept>
<!-- Concept: tactile notated music  -->
    <skos:Concept rdf:about="http://rdaregistry.info/termList/RDAContentType/1016" xml:lang="en">
      <skos:inScheme rdf:resource="http://rdaregistry.info/termList/RDAContentType"/>
      <reg:status rdf:resource="http://metadataregistry.org/uri/RegStatus/1001"/>
      <reg:identifier rdf:resource="http://metadataregistry.org/concepts/525"/>
      <skos:prefLabel xml:lang="en">tactile notated music</skos:prefLabel>
      <skos:definition xml:lang="en">A content type consisting of content expressed through a form of musical notation intended to be perceived through touch.</skos:definition>
      <skos:scopeNote xml:lang="en">Braille music and other tactile forms of musical notation are included.</skos:scopeNote>
      <skos:prefLabel xml:lang="de">Taktile Noten</skos:prefLabel>
      <skos:scopeNote xml:lang="de">Dazu gehören Braille-Musik und andere taktile Formen von Noten.</skos:scopeNote>
      <skos:definition xml:lang="de">Ein Inhaltstyp, der aus Inhalt besteht, der durch eine Notationsform für Musik ausgedrückt wird und konzipiert ist, um über den Tastsinn wahrgenommen zu werden.</skos:definition>
	    <skos:related rdf:resource="http://rdaregistry.info/termList/RDAContentType/1010"/>
      <skos:prefLabel xml:lang="fr">musique notée tactile</skos:prefLabel>
      <skos:definition xml:lang="fr">Type de contenu qui consiste en contenu exprimé au moyen d’une forme de notation musicale destinée à être perçue au toucher.</skos:definition>
      <skos:scopeNote xml:lang="fr">Comprend la musique en braille et les autres formes tactiles de notation musicale.</skos:scopeNote>
      <skos:prefLabel xml:lang="es">música notada táctil</skos:prefLabel>
      <skos:definition xml:lang="es">Contenido expresado mediante una forma de notación musical pensada para ser percibida mediante el tacto.</skos:definition>
      <skos:scopeNote xml:lang="es">Incluye música en braille y otras formas táctiles de notación músical.</skos:scopeNote>
      <rdakit:toolkitLabel xml:lang="en">tactile notated music</rdakit:toolkitLabel>
      <rdakit:toolkitLabel xml:lang="fr">musique notée tactile</rdakit:toolkitLabel>
      <rdakit:toolkitDefinition xml:lang="en">A content type consisting of content expressed through a form of musical notation intended to be perceived through touch.</rdakit:toolkitDefinition>
      <rdakit:toolkitDefinition xml:lang="fr">Type de contenu qui consiste en contenu exprimé au moyen d’une forme de notation musicale destinée à être perçue au toucher.</rdakit:toolkitDefinition>
      <rdakit:toolkitLabel xml:lang="de">Taktile Noten</rdakit:toolkitLabel>
      <rdakit:toolkitDefinition xml:lang="de">Ein Inhaltstyp, der aus Inhalt besteht, der durch eine Notationsform für Musik ausgedrückt wird und konzipiert ist, um über den Tastsinn wahrgenommen zu werden.</rdakit:toolkitDefinition>
      <rdakit:toolkitLabel xml:lang="es">música notada táctil</rdakit:toolkitLabel>
      <rdakit:toolkitDefinition xml:lang="es">Contenido expresado mediante una forma de notación musical pensada para ser percibida mediante el tacto.</rdakit:toolkitDefinition>
      <skos:prefLabel xml:lang="zh">触摸乐谱</skos:prefLabel>
      <rdakit:toolkitLabel xml:lang="zh">触摸乐谱</rdakit:toolkitLabel>
      <skos:definition xml:lang="zh">以音乐标记法表达的、旨在通过触觉感知的内容。</skos:definition>
      <rdakit:toolkitDefinition xml:lang="zh">以音乐标记法表达的、旨在通过触觉感知的内容。</rdakit:toolkitDefinition>
      <skos:scopeNote xml:lang="zh">包括布莱叶盲文乐谱和其他触摸形式的音乐标记法。</skos:scopeNote>
      <skos:prefLabel xml:lang="nl">tactiele muzieknotatie</skos:prefLabel>
      <rdakit:toolkitLabel xml:lang="nl">tactiele muzieknotatie</rdakit:toolkitLabel>
      <skos:definition xml:lang="nl">Content uitgedrukt door een vorm van muzieknotatie bedoeld om waar te nemen door aanraking.</skos:definition>
      <rdakit:toolkitDefinition xml:lang="nl">Content uitgedrukt door een vorm van muzieknotatie bedoeld om waar te nemen door aanraking.</rdakit:toolkitDefinition>
      <skos:prefLabel xml:lang="it">musica notata tattile</skos:prefLabel>
      <rdakit:toolkitLabel xml:lang="it">musica notata tattile</rdakit:toolkitLabel>
      <skos:definition xml:lang="it">Contenuto espresso mediante una forma di notazione musicale percepibile mediante il tatto.</skos:definition>
      <rdakit:toolkitDefinition xml:lang="it">Contenuto espresso mediante una forma di notazione musicale percepibile mediante il tatto.</rdakit:toolkitDefinition>
      <skos:scopeNote xml:lang="it">Comprende la musica braille e altre forme di notazione musicale tattili.</skos:scopeNote>
      <skos:prefLabel xml:lang="fi">taktiili nuottikirjoitus</skos:prefLabel>
      <rdakit:toolkitLabel xml:lang="fi">taktiili nuottikirjoitus</rdakit:toolkitLabel>
      <skos:definition xml:lang="fi">Musiikkinotaationa esitetty sisältö, joka on tarkoitettu kosketeltavaksi.</skos:definition>
      <rdakit:toolkitDefinition xml:lang="fi">Musiikkinotaationa esitetty sisältö, joka on tarkoitettu kosketeltavaksi.</rdakit:toolkitDefinition>
      <skos:scopeNote xml:lang="fi">Esimerkiksi pistenuottikirjoitus ja muut taktiilit nuottikirjoitukset.</skos:scopeNote>
      <skos:prefLabel xml:lang="he">תווי תנועה מישושיים</skos:prefLabel>
      <rdakit:toolkitLabel xml:lang="he">תווי תנועה מישושיים</rdakit:toolkitLabel>
      <skos:definition xml:lang="he">סוג תוכן המכיל תוכן שקבל את ביטויו באמצעות תווים המייצגים תנועה, המיועדים לתפיסה על ידי מישוש.</skos:definition>
      <rdakit:toolkitDefinition xml:lang="he">סוג תוכן המכיל תוכן שקבל את ביטויו באמצעות תווים המייצגים תנועה, המיועדים לתפיסה על ידי מישוש.</rdakit:toolkitDefinition>
      <skos:scopeNote xml:lang="he">כולל תווי מוסיקה בברייל וצורות אחרות של תווי מוסיקה למישוש.</skos:scopeNote>
      <skos:prefLabel xml:lang="ar">موسيقى مدونة لمسية</skos:prefLabel>
      <skos:prefLabel xml:lang="vi">âm nhạc ký hiệu xúc giác</skos:prefLabel>
      <rdakit:toolkitLabel xml:lang="vi">âm nhạc ký hiệu xúc giác</rdakit:toolkitLabel>
      <skos:definition xml:lang="vi">Loại nội dung được biểu hiện qua hình thái của ký hiệu âm nhạc để nhận biết qua xúc giác.</skos:definition>
      <rdakit:toolkitDefinition xml:lang="vi">Loại nội dung được biểu hiện qua hình thái của ký hiệu âm nhạc để nhận biết qua xúc giác.</rdakit:toolkitDefinition>
      <skos:scopeNote xml:lang="vi">Âm nhạc chữ braille và các hình thái xúc giác khác của ký hiệu âm nhạc được bao gồm</skos:scopeNote>
      <skos:prefLabel xml:lang="da">taktil noteret musik</skos:prefLabel>
      <rdakit:toolkitLabel xml:lang="da">taktil noteret musik</rdakit:toolkitLabel>
      <skos:definition xml:lang="da">Indholdstype der består af indhold udtrykt som en musikalsk notationsform, beregnet til at opfattes ved berøring.</skos:definition>
      <rdakit:toolkitDefinition xml:lang="da">Indholdstype der består af indhold udtrykt som en musikalsk notationsform, beregnet til at opfattes ved berøring.</rdakit:toolkitDefinition>
      <skos:scopeNote xml:lang="da">Braillemusik og andre taktile former for musiknotation er omfattet.</skos:scopeNote>
      <skos:prefLabel xml:lang="no">taktil musikknotasjon</skos:prefLabel>
      <rdakit:toolkitLabel xml:lang="no">taktil musikknotasjon</rdakit:toolkitLabel>
      <skos:definition xml:lang="no">En innholdstype som består av innhold uttrykt ved hjelp av en form for musikknotasjon som er ment å oppfattes gjennom berøring.</skos:definition>
      <rdakit:toolkitDefinition xml:lang="no">En innholdstype som består av innhold uttrykt ved hjelp av en form for musikknotasjon som er ment å oppfattes gjennom berøring.</rdakit:toolkitDefinition>
      <skos:scopeNote xml:lang="no">Punktskrift og andre taktile former for musikknotasjon er inkludert.</skos:scopeNote>
    </skos:Concept>
<!-- Concept: tactile text  -->
    <skos:Concept rdf:about="http://rdaregistry.info/termList/RDAContentType/1018" xml:lang="en">
      <skos:inScheme rdf:resource="http://rdaregistry.info/termList/RDAContentType"/>
      <reg:status rdf:resource="http://metadataregistry.org/uri/RegStatus/1001"/>
      <reg:identifier rdf:resource="http://metadataregistry.org/concepts/527"/>
      <skos:prefLabel xml:lang="en">tactile text</skos:prefLabel>
      <skos:definition xml:lang="en">A content type consisting of content expressed through a form of notation for language intended to be perceived through touch.</skos:definition>
      <skos:scopeNote xml:lang="en">Braille text and other tactile forms of language notation are included.</skos:scopeNote>
      <skos:prefLabel xml:lang="de">Taktiler Text</skos:prefLabel>
      <skos:definition xml:lang="de">Ein Inhaltstyp, der aus Inhalt besteht, der durch eine Notationsform für Sprache ausgedrückt wird und konzipiert ist, um über den Tastsinn wahrgenommen zu werden.</skos:definition>
      <skos:scopeNote xml:lang="de">Dazu gehören Braille-Texte und andere taktile Formen sprachlicher Notation.</skos:scopeNote>
	    <skos:related rdf:resource="http://rdaregistry.info/termList/RDAContentType/1020"/>
      <skos:prefLabel xml:lang="fr">texte tactile</skos:prefLabel>
      <skos:definition xml:lang="fr">Type de contenu qui consiste en contenu exprimé au moyen d’une forme de notation du langage destinée à être perçue au toucher.</skos:definition>
      <skos:scopeNote xml:lang="fr">Comprend les textes en braille et les autres formes tactiles de notation du langage.</skos:scopeNote>
      <skos:prefLabel xml:lang="es">texto táctil</skos:prefLabel>
      <skos:definition xml:lang="es">Contenido expresado mediante una forma de notación de lenguaje pensado para ser percibido mediante el tacto.</skos:definition>
      <skos:scopeNote xml:lang="es">Incluye textos en braille y otras formas táctiles del lenguaje de notación.</skos:scopeNote>
      <rdakit:toolkitLabel xml:lang="en">tactile text</rdakit:toolkitLabel>
      <rdakit:toolkitLabel xml:lang="fr">texte tactile</rdakit:toolkitLabel>
      <rdakit:toolkitDefinition xml:lang="en">A content type consisting of content expressed through a form of notation for language intended to be perceived through touch.</rdakit:toolkitDefinition>
      <rdakit:toolkitDefinition xml:lang="fr">Type de contenu qui consiste en contenu exprimé au moyen d’une forme de notation du langage destinée à être perçue au toucher.</rdakit:toolkitDefinition>
      <rdakit:toolkitLabel xml:lang="de">Taktiler Text</rdakit:toolkitLabel>
      <rdakit:toolkitDefinition xml:lang="de">Ein Inhaltstyp, der aus Inhalt besteht, der durch eine Notationsform für Sprache ausgedrückt wird und konzipiert ist, um über den Tastsinn wahrgenommen zu werden.</rdakit:toolkitDefinition>
      <rdakit:toolkitLabel xml:lang="es">texto táctil</rdakit:toolkitLabel>
      <rdakit:toolkitDefinition xml:lang="es">Contenido expresado mediante una forma de notación de lenguaje pensado para ser percibido mediante el tacto.</rdakit:toolkitDefinition>
      <skos:prefLabel xml:lang="zh">触摸文本</skos:prefLabel>
      <rdakit:toolkitLabel xml:lang="zh">触摸文本</rdakit:toolkitLabel>
      <skos:definition xml:lang="zh">以语言标记法表达的、旨在通过触觉感知的内容。</skos:definition>
      <rdakit:toolkitDefinition xml:lang="zh">以语言标记法表达的、旨在通过触觉感知的内容。</rdakit:toolkitDefinition>
      <skos:scopeNote xml:lang="zh">包括布莱叶盲文和其他触摸形式的语言符号（见触摸文本）。</skos:scopeNote>
      <skos:prefLabel xml:lang="nl">tactiele tekst</skos:prefLabel>
      <rdakit:toolkitLabel xml:lang="nl">tactiele tekst</rdakit:toolkitLabel>
      <skos:definition xml:lang="nl">Content uitgedrukt door een vorm van notatie van taal bedoeld om waar te nemen door aanraking.</skos:definition>
      <rdakit:toolkitDefinition xml:lang="nl">Content uitgedrukt door een vorm van notatie van taal bedoeld om waar te nemen door aanraking.</rdakit:toolkitDefinition>
      <skos:prefLabel xml:lang="it">testo tattile</skos:prefLabel>
      <rdakit:toolkitLabel xml:lang="it">testo tattile</rdakit:toolkitLabel>
      <skos:definition xml:lang="it">Contenuto espresso mediante una forma di notazione linguistica percepibile mediante il tatto.</skos:definition>
      <rdakit:toolkitDefinition xml:lang="it">Contenuto espresso mediante una forma di notazione linguistica percepibile mediante il tatto.</rdakit:toolkitDefinition>
      <skos:scopeNote xml:lang="it">Comprende il testo braille e altre forme di notazione linguistica tattili.</skos:scopeNote>
      <skos:prefLabel xml:lang="fi">taktiili teksti</skos:prefLabel>
      <rdakit:toolkitLabel xml:lang="fi">taktiili teksti</rdakit:toolkitLabel>
      <skos:definition xml:lang="fi">Kielen merkkijärjestelmällä esitetty sisältö, joka on tarkoitettu kosketeltavaksi.</skos:definition>
      <rdakit:toolkitDefinition xml:lang="fi">Kielen merkkijärjestelmällä esitetty sisältö, joka on tarkoitettu kosketeltavaksi.</rdakit:toolkitDefinition>
      <skos:scopeNote xml:lang="fi">Esimerkiksi pistekirjoitus ja muut taktiilit tekstinkirjoitusmuodot.</skos:scopeNote>
      <skos:prefLabel xml:lang="he">טקסט מישושי</skos:prefLabel>
      <rdakit:toolkitLabel xml:lang="he">טקסט מישושי</rdakit:toolkitLabel>
      <skos:definition xml:lang="he">סוג תוכן המכיל תוכן שקיבל את ביטויו באמצעות סימנים המייצגים שפה ומיועדים לתפיסה על ידי מישוש.</skos:definition>
      <rdakit:toolkitDefinition xml:lang="he">סוג תוכן המכיל תוכן שקיבל את ביטויו באמצעות סימנים המייצגים שפה ומיועדים לתפיסה על ידי מישוש.</rdakit:toolkitDefinition>
      <skos:scopeNote xml:lang="he">כולל טקסט בברייל וצורות אחרות של סימני שפה למישוש.</skos:scopeNote>
      <skos:prefLabel xml:lang="ar">نص لمسي</skos:prefLabel>
      <skos:prefLabel xml:lang="sv">taktil text</skos:prefLabel>
      <rdakit:toolkitLabel xml:lang="sv">taktil text</rdakit:toolkitLabel>
      <skos:prefLabel xml:lang="vi">văn bản xúc giác</skos:prefLabel>
      <rdakit:toolkitLabel xml:lang="vi">văn bản xúc giác</rdakit:toolkitLabel>
      <skos:definition xml:lang="vi">Loại nội dung được biểu hiện qua hình thái của ký hiệu ngôn ngữ để nhận biết bằng xúc giác.</skos:definition>
      <rdakit:toolkitDefinition xml:lang="vi">Loại nội dung được biểu hiện qua hình thái của ký hiệu ngôn ngữ để nhận biết bằng xúc giác.</rdakit:toolkitDefinition>
      <skos:scopeNote xml:lang="vi">Văn bản chữ Braille và các hình thái xúc giác khác của ký hiệu ngôn ngữ được bao gồm</skos:scopeNote>
      <skos:prefLabel xml:lang="da">taktil tekst</skos:prefLabel>
      <rdakit:toolkitLabel xml:lang="da">taktil tekst</rdakit:toolkitLabel>
      <skos:definition xml:lang="da">Indholdstype der består af indhold udtrykt vha. en sprognotationsform, beregnet til at opfattes ved berøring.</skos:definition>
      <rdakit:toolkitDefinition xml:lang="da">Indholdstype der består af indhold udtrykt vha. en sprognotationsform, beregnet til at opfattes ved berøring.</rdakit:toolkitDefinition>
      <skos:scopeNote xml:lang="da">Brailletekst og andre taktile sprognotationsformer er omfattet.</skos:scopeNote>
      <skos:prefLabel xml:lang="no">taktil tekst</skos:prefLabel>
      <rdakit:toolkitLabel xml:lang="no">taktil tekst</rdakit:toolkitLabel>
      <skos:definition xml:lang="no">En innholdstype som består av innhold uttrykt ved hjelp av en form for språkbasert tegnsystem som er ment å oppfattes gjennom berøring.</skos:definition>
      <rdakit:toolkitDefinition xml:lang="no">En innholdstype som består av innhold uttrykt ved hjelp av en form for språkbasert tegnsystem som er ment å oppfattes gjennom berøring.</rdakit:toolkitDefinition>
      <skos:scopeNote xml:lang="no">Punktskrift og andre taktile former for språknotasjon er inkludert.</skos:scopeNote>
    </skos:Concept>
<!-- Concept: tactile three-dimensional form  -->
    <skos:Concept rdf:about="http://rdaregistry.info/termList/RDAContentType/1019" xml:lang="en">
      <skos:inScheme rdf:resource="http://rdaregistry.info/termList/RDAContentType"/>
      <reg:status rdf:resource="http://metadataregistry.org/uri/RegStatus/1001"/>
      <reg:identifier rdf:resource="http://metadataregistry.org/concepts/528"/>
      <skos:prefLabel xml:lang="en">tactile three-dimensional form</skos:prefLabel>
      <skos:definition xml:lang="en">A content type consisting of content expressed through a form or forms intended to be perceived through touch as a three-dimensional form or forms.</skos:definition>
      <skos:prefLabel xml:lang="de">Taktile dreidimensionale Form</skos:prefLabel>
      <skos:definition xml:lang="de">Ein Inhaltstyp, der aus Inhalt besteht, der durch eine Form bzw. Formen ausgedrückt wird und konzipiert ist, um über den Tastsinn als dreidimensionale Form oder Formen wahrgenommen zu werden.</skos:definition>
	    <skos:related rdf:resource="http://rdaregistry.info/termList/RDAContentType/1021"/>
	    <skos:related rdf:resource="http://rdaregistry.info/termList/RDAContentType/1006"/>
      <skos:prefLabel xml:lang="fr">forme tridimensionnelle tactile</skos:prefLabel>
      <skos:definition xml:lang="fr">Type de contenu qui consiste en contenu exprimé au moyen d’une ou plusieurs formes destinées à être perçues au toucher comme une ou plusieurs formes tridimensionnelles.</skos:definition>
      <skos:prefLabel xml:lang="es">forma tridimensional táctil</skos:prefLabel>
      <skos:definition xml:lang="es">Contenido expresado mediante una forma o formas pensadas para ser percibidas mediante el tacto como forma o formas tridimensionales.</skos:definition>
      <rdakit:toolkitLabel xml:lang="en">tactile three-dimensional form</rdakit:toolkitLabel>
      <rdakit:toolkitLabel xml:lang="fr">forme tridimensionnelle tactile</rdakit:toolkitLabel>
      <rdakit:toolkitDefinition xml:lang="en">A content type consisting of content expressed through a form or forms intended to be perceived through touch as a three-dimensional form or forms.</rdakit:toolkitDefinition>
      <rdakit:toolkitDefinition xml:lang="fr">Type de contenu qui consiste en contenu exprimé au moyen d’une ou plusieurs formes destinées à être perçues au toucher comme une ou plusieurs formes tridimensionnelles.</rdakit:toolkitDefinition>
      <rdakit:toolkitLabel xml:lang="de">Taktile dreidimensionale Form</rdakit:toolkitLabel>
      <rdakit:toolkitDefinition xml:lang="de">Ein Inhaltstyp, der aus Inhalt besteht, der durch eine Form bzw. Formen ausgedrückt wird und konzipiert ist, um über den Tastsinn als dreidimensionale Form oder Formen wahrgenommen zu werden.</rdakit:toolkitDefinition>
      <rdakit:toolkitLabel xml:lang="es">forma tridimensional táctil</rdakit:toolkitLabel>
      <rdakit:toolkitDefinition xml:lang="es">Contenido expresado mediante una forma o formas pensadas para ser percibidas mediante el tacto como forma o formas tridimensionales.</rdakit:toolkitDefinition>
      <skos:prefLabel xml:lang="zh">触摸三维形式</skos:prefLabel>
      <rdakit:toolkitLabel xml:lang="zh">触摸三维形式</rdakit:toolkitLabel>
      <skos:definition xml:lang="zh">以一个或多个三维形式表达的、旨在通过触觉感知的内容。</skos:definition>
      <rdakit:toolkitDefinition xml:lang="zh">以一个或多个三维形式表达的、旨在通过触觉感知的内容。</rdakit:toolkitDefinition>
      <skos:prefLabel xml:lang="nl">tactiele driedimensionale vorm</skos:prefLabel>
      <rdakit:toolkitLabel xml:lang="nl">tactiele driedimensionale vorm</rdakit:toolkitLabel>
      <skos:definition xml:lang="nl">Content uitgedrukt door een vorm of vormen bedoeld om waar te nemen door aanraking als een driedimensionale vorm of vormen.</skos:definition>
      <rdakit:toolkitDefinition xml:lang="nl">Content uitgedrukt door een vorm of vormen bedoeld om waar te nemen door aanraking als een driedimensionale vorm of vormen.</rdakit:toolkitDefinition>
      <skos:prefLabel xml:lang="it">forma tridimensionale tattile</skos:prefLabel>
      <rdakit:toolkitLabel xml:lang="it">forma tridimensionale tattile</rdakit:toolkitLabel>
      <skos:definition xml:lang="it">Contenuto espresso mediante una o più forme percepibili mediante il tatto come forme tridimensionali.</skos:definition>
      <rdakit:toolkitDefinition xml:lang="it">Contenuto espresso mediante una o più forme percepibili mediante il tatto come forme tridimensionali.</rdakit:toolkitDefinition>
      <skos:prefLabel xml:lang="fi">taktiili kolmiulotteinen muoto</skos:prefLabel>
      <rdakit:toolkitLabel xml:lang="fi">taktiili kolmiulotteinen muoto</rdakit:toolkitLabel>
      <skos:definition xml:lang="fi">Muotona tai muotoina esitetty sisältö, joka on tarkoitettu kosketeltavaksi kolmiulotteiseksi muodoksi.</skos:definition>
      <rdakit:toolkitDefinition xml:lang="fi">Muotona tai muotoina esitetty sisältö, joka on tarkoitettu kosketeltavaksi kolmiulotteiseksi muodoksi.</rdakit:toolkitDefinition>
      <skos:prefLabel xml:lang="he">צורה תלת-ממדית מישושית</skos:prefLabel>
      <rdakit:toolkitLabel xml:lang="he">צורה תלת-ממדית מישושית</rdakit:toolkitLabel>
      <skos:definition xml:lang="he">סוג תוכן המכיל תוכן אשר קיבל את ביטויו באמצעות צורה או צורות ומיועדות לתפיסה על ידי מישוש כצורה תלת-ממדית.</skos:definition>
      <rdakit:toolkitDefinition xml:lang="he">סוג תוכן המכיל תוכן אשר קיבל את ביטויו באמצעות צורה או צורות ומיועדות לתפיסה על ידי מישוש כצורה תלת-ממדית.</rdakit:toolkitDefinition>
      <skos:prefLabel xml:lang="ar">شكل لمسي ثلاثي الأبعاد</skos:prefLabel>
      <skos:prefLabel xml:lang="sv">taktil tredimensionell form</skos:prefLabel>
      <rdakit:toolkitLabel xml:lang="sv">taktil tredimensionell form</rdakit:toolkitLabel>
      <skos:prefLabel xml:lang="vi">hình thái ba chiều xúc giác</skos:prefLabel>
      <rdakit:toolkitLabel xml:lang="vi">hình thái ba chiều xúc giác</rdakit:toolkitLabel>
      <skos:definition xml:lang="vi">Loại nội dung được biểu hiện qua một hoặc nhiều hình thái để nhận biết qua xúc giác như là một hoặc nhiều hình thái ba chiều.</skos:definition>
      <rdakit:toolkitDefinition xml:lang="vi">Loại nội dung được biểu hiện qua một hoặc nhiều hình thái để nhận biết qua xúc giác như là một hoặc nhiều hình thái ba chiều.</rdakit:toolkitDefinition>
      <skos:prefLabel xml:lang="da">taktil tredimensional form</skos:prefLabel>
      <rdakit:toolkitLabel xml:lang="da">taktil tredimensional form</rdakit:toolkitLabel>
      <skos:definition xml:lang="da">Indholdstype der består af indhold udtrykt som en eller flere former mhp. at blive opfattet ved berøring som en eller flere tredimensionelle former.</skos:definition>
      <rdakit:toolkitDefinition xml:lang="da">Indholdstype der består af indhold udtrykt som en eller flere former mhp. at blive opfattet ved berøring som en eller flere tredimensionelle former.</rdakit:toolkitDefinition>
      <skos:prefLabel xml:lang="no">taktil tredimensjonal form</skos:prefLabel>
      <rdakit:toolkitLabel xml:lang="no">taktil tredimensjonal form</rdakit:toolkitLabel>
      <skos:definition xml:lang="no">En innholdstype som består av innhold uttrykt gjennom én eller flere former, som skal oppfattes gjennom berøring som én eller flere tredimensjonale former.</skos:definition>
      <rdakit:toolkitDefinition xml:lang="no">En innholdstype som består av innhold uttrykt gjennom én eller flere former, som skal oppfattes gjennom berøring som én eller flere tredimensjonale former.</rdakit:toolkitDefinition>
    </skos:Concept>
<!-- Concept: text  -->
    <skos:Concept rdf:about="http://rdaregistry.info/termList/RDAContentType/1020" xml:lang="en">
      <skos:inScheme rdf:resource="http://rdaregistry.info/termList/RDAContentType"/>
      <reg:status rdf:resource="http://metadataregistry.org/uri/RegStatus/1001"/>
      <reg:identifier rdf:resource="http://metadataregistry.org/concepts/529"/>
      <skos:prefLabel xml:lang="en">text</skos:prefLabel>
      <skos:definition xml:lang="en">A content type consisting of content expressed through a form of notation for language intended to be perceived visually.</skos:definition>
      <skos:scopeNote xml:lang="en">All forms of language notation other than those intended to be perceived through touch are included.</skos:scopeNote>
      <skos:prefLabel xml:lang="de">Text</skos:prefLabel>
      <skos:definition xml:lang="de">Ein Inhaltstyp, der aus Inhalt besteht, der durch eine Notationsform für Sprache ausgedrückt wird und für die visuelle Wahrnehmung konzipiert ist.</skos:definition>
      <skos:scopeNote xml:lang="de">Dazu gehören alle Formen von Notationen für Sprache, die nicht über den Tastsinn wahrgenommen werden sollen.</skos:scopeNote>
	    <skos:related rdf:resource="http://rdaregistry.info/termList/RDAContentType/1007"/>
	    <skos:related rdf:resource="http://rdaregistry.info/termList/RDAContentType/1018"/>
      <skos:prefLabel xml:lang="fr">texte</skos:prefLabel>
      <skos:definition xml:lang="fr">Type de contenu qui consiste en contenu exprimé au moyen d’une forme de notation du langage destinée à être perçue visuellement.</skos:definition>
      <skos:scopeNote xml:lang="fr">Comprend toutes les formes de notation du langage différentes de celles destinées à être perçues au toucher.</skos:scopeNote>
      <skos:prefLabel xml:lang="es">texto</skos:prefLabel>
      <skos:definition xml:lang="es">Contenido expresado mediante una forma de notación de lenguaje pensado para ser percibido visualmente.</skos:definition>
      <skos:scopeNote xml:lang="es">Incluye todas las formas de lenguaje de notación diferente de aquellos pensados para ser percibidos mediante el tacto.</skos:scopeNote>
      <rdakit:toolkitLabel xml:lang="en">text</rdakit:toolkitLabel>
      <rdakit:toolkitLabel xml:lang="fr">texte</rdakit:toolkitLabel>
      <rdakit:toolkitDefinition xml:lang="en">A content type consisting of content expressed through a form of notation for language intended to be perceived visually.</rdakit:toolkitDefinition>
      <rdakit:toolkitDefinition xml:lang="fr">Type de contenu qui consiste en contenu exprimé au moyen d’une forme de notation du langage destinée à être perçue visuellement.</rdakit:toolkitDefinition>
      <rdakit:toolkitLabel xml:lang="de">Text</rdakit:toolkitLabel>
      <rdakit:toolkitDefinition xml:lang="de">Ein Inhaltstyp, der aus Inhalt besteht, der durch eine Notationsform für Sprache ausgedrückt wird und für die visuelle Wahrnehmung konzipiert ist.</rdakit:toolkitDefinition>
      <rdakit:toolkitLabel xml:lang="es">texto</rdakit:toolkitLabel>
      <rdakit:toolkitDefinition xml:lang="es">Contenido expresado mediante una forma de notación de lenguaje pensado para ser percibido visualmente.</rdakit:toolkitDefinition>
      <skos:prefLabel xml:lang="zh">文本</skos:prefLabel>
      <rdakit:toolkitLabel xml:lang="zh">文本</rdakit:toolkitLabel>
      <skos:definition xml:lang="zh">以视觉感知的语言符号形式表达的内容。</skos:definition>
      <rdakit:toolkitDefinition xml:lang="zh">以视觉感知的语言符号形式表达的内容。</rdakit:toolkitDefinition>
      <skos:scopeNote xml:lang="zh">包括除触觉感知之外的所有语言符号形式。</skos:scopeNote>
      <skos:prefLabel xml:lang="nl">tekst</skos:prefLabel>
      <rdakit:toolkitLabel xml:lang="nl">tekst</rdakit:toolkitLabel>
      <skos:definition xml:lang="nl">Content uitgedrukt door een vorm van notatie van taal bedoeld om visueel waar te nemen.</skos:definition>
      <rdakit:toolkitDefinition xml:lang="nl">Content uitgedrukt door een vorm van notatie van taal bedoeld om visueel waar te nemen.</rdakit:toolkitDefinition>
      <skos:prefLabel xml:lang="it">testo</skos:prefLabel>
      <rdakit:toolkitLabel xml:lang="it">testo</rdakit:toolkitLabel>
      <skos:definition xml:lang="it">Contenuto espresso mediante una forma di notazione linguistica percepibile con la vista.</skos:definition>
      <rdakit:toolkitDefinition xml:lang="it">Contenuto espresso mediante una forma di notazione linguistica percepibile con la vista.</rdakit:toolkitDefinition>
      <skos:scopeNote xml:lang="it">Include tutte le forme di notazione linguistica diverse da quelle percepibili mediante il tatto.</skos:scopeNote>
      <skos:prefLabel xml:lang="fi">teksti</skos:prefLabel>
      <rdakit:toolkitLabel xml:lang="fi">teksti</rdakit:toolkitLabel>
      <skos:definition xml:lang="fi">Kielen merkkijärjestelmällä esitetty sisältö, joka on tarkoitettu katsottavaksi.</skos:definition>
      <rdakit:toolkitDefinition xml:lang="fi">Kielen merkkijärjestelmällä esitetty sisältö, joka on tarkoitettu katsottavaksi.</rdakit:toolkitDefinition>
      <skos:scopeNote xml:lang="fi">Sisältää kaikki muut kielen merkkijärjestelmät, paitsi kosketeltavaksi tarkoitetun tekstin.</skos:scopeNote>
      <skos:prefLabel xml:lang="he">טקסט</skos:prefLabel>
      <rdakit:toolkitLabel xml:lang="he">טקסט</rdakit:toolkitLabel>
      <skos:definition xml:lang="he">סוג תוכן המכיל תוכן שקיבל את ביטויו באמצעות סימנים המייצגים שפה ומיועדים לצפייה.</skos:definition>
      <rdakit:toolkitDefinition xml:lang="he">סוג תוכן המכיל תוכן שקיבל את ביטויו באמצעות סימנים המייצגים שפה ומיועדים לצפייה.</rdakit:toolkitDefinition>
      <skos:scopeNote xml:lang="he">כולל כל סוגי הסימנים המייצגים שפה, למעט אלו המיועדים לתפיסה על ידי מישוש.</skos:scopeNote>
      <skos:prefLabel xml:lang="ar">نص</skos:prefLabel>
      <skos:prefLabel xml:lang="sv">text</skos:prefLabel>
      <rdakit:toolkitLabel xml:lang="sv">text</rdakit:toolkitLabel>
      <skos:prefLabel xml:lang="vi">văn bản</skos:prefLabel>
      <rdakit:toolkitLabel xml:lang="vi">văn bản</rdakit:toolkitLabel>
      <skos:definition xml:lang="vi">Loại nội dung được biểu hiện qua hình thái của ký hiệu ngôn ngữ để nhận biết bằng thị giác.</skos:definition>
      <rdakit:toolkitDefinition xml:lang="vi">Loại nội dung được biểu hiện qua hình thái của ký hiệu ngôn ngữ để nhận biết bằng thị giác.</rdakit:toolkitDefinition>
      <skos:scopeNote xml:lang="vi">Tất cả các hình thái của ký hiệu ngôn ngữ khác với hình thái để nhận biết bằng xúc giácđược bao gồm</skos:scopeNote>
      <skos:prefLabel xml:lang="da">tekst</skos:prefLabel>
      <rdakit:toolkitLabel xml:lang="da">tekst</rdakit:toolkitLabel>
      <skos:definition xml:lang="da">Indholdstype der består af indhold udtrykt vha. en sprognotationsform, beregnet til at blive opfattet visuelt.</skos:definition>
      <rdakit:toolkitDefinition xml:lang="da">Indholdstype der består af indhold udtrykt vha. en sprognotationsform, beregnet til at blive opfattet visuelt.</rdakit:toolkitDefinition>
      <skos:scopeNote xml:lang="da">Alle sprognotationsformer, bortset fra dem der er beregnet til at opfattes ved berøring er omfattet.</skos:scopeNote>
      <skos:prefLabel xml:lang="no">tekst</skos:prefLabel>
      <rdakit:toolkitLabel xml:lang="no">tekst</rdakit:toolkitLabel>
      <skos:definition xml:lang="no">En innholdstype som består av innhold uttrykt ved hjelp av en form for språknotasjon som er ment å oppfattes visuelt.</skos:definition>
      <rdakit:toolkitDefinition xml:lang="no">En innholdstype som består av innhold uttrykt ved hjelp av en form for språknotasjon som er ment å oppfattes visuelt.</rdakit:toolkitDefinition>
      <skos:scopeNote xml:lang="no">Alle former for språknotasjon bortsett fra de som er ment å oppfattes gjennom berøring, er inkludert.</skos:scopeNote>
    </skos:Concept>
<!-- Concept: three-dimensional form  -->
    <skos:Concept rdf:about="http://rdaregistry.info/termList/RDAContentType/1021" xml:lang="en">
      <skos:inScheme rdf:resource="http://rdaregistry.info/termList/RDAContentType"/>
      <reg:status rdf:resource="http://metadataregistry.org/uri/RegStatus/1001"/>
      <reg:identifier rdf:resource="http://metadataregistry.org/concepts/530"/>
      <skos:prefLabel xml:lang="en">three-dimensional form</skos:prefLabel>
      <skos:definition xml:lang="en">A content type consisting of content expressed through a form or forms intended to be perceived visually in three-dimensions.</skos:definition>
      <skos:scopeNote xml:lang="en">Sculptures, models, naturally occurring objects and specimens, holograms, etc., are included.</skos:scopeNote>
      <skos:prefLabel xml:lang="de">Dreidimensionale Form</skos:prefLabel>
      <skos:scopeNote xml:lang="de">Dazu gehören Skulpturen, Modelle, natürlich vorkommende Gegenstände und Proben, Hologramme usw.</skos:scopeNote>
      <skos:definition xml:lang="de">Ein Inhaltstyp, der aus Inhalt besteht, der durch eine Form bzw. Formen dargestellt wird und konzipiert ist, um visuell dreidimensional wahrgenommen zu werden.</skos:definition>
	    <skos:related rdf:resource="http://rdaregistry.info/termList/RDAContentType/1019"/>
	    <skos:related rdf:resource="http://rdaregistry.info/termList/RDAContentType/1007"/>
      <skos:prefLabel xml:lang="fr">forme tridimensionnelle</skos:prefLabel>
      <skos:definition xml:lang="fr">Type de contenu qui consiste en contenu exprimé au moyen d’une ou plusieurs formes destinées à être perçues visuellement en trois dimensions.</skos:definition>
      <skos:scopeNote xml:lang="fr">Comprend les sculptures, les maquettes, les objets et spécimens naturels, les hologrammes, etc. Ne comprend pas le contenu cartographique destiné à être perçu comme une forme tridimensionnelle. Ne comprend pas les formes tridimensionnelles destinées à être perçues au toucher.</skos:scopeNote>
      <skos:prefLabel xml:lang="es">forma tridimensional</skos:prefLabel>
      <skos:definition xml:lang="es">Contenido expresado mediante una forma o formas pensadas para ser percibidas visualmente en tres dimensiones.</skos:definition>
      <skos:scopeNote xml:lang="es">Incluye esculturas, modelos, objetos y especímenes que ocurren naturalmente, hologramas, etc.</skos:scopeNote>
      <rdakit:toolkitLabel xml:lang="en">three-dimensional form</rdakit:toolkitLabel>
      <rdakit:toolkitLabel xml:lang="fr">forme tridimensionnelle</rdakit:toolkitLabel>
      <rdakit:toolkitDefinition xml:lang="en">A content type consisting of content expressed through a form or forms intended to be perceived visually in three-dimensions.</rdakit:toolkitDefinition>
      <rdakit:toolkitDefinition xml:lang="fr">Type de contenu qui consiste en contenu exprimé au moyen d’une ou plusieurs formes destinées à être perçues visuellement en trois dimensions.</rdakit:toolkitDefinition>
      <rdakit:toolkitLabel xml:lang="de">Dreidimensionale Form</rdakit:toolkitLabel>
      <rdakit:toolkitDefinition xml:lang="de">Ein Inhaltstyp, der aus Inhalt besteht, der durch eine Form bzw. Formen dargestellt wird und konzipiert ist, um visuell dreidimensional wahrgenommen zu werden.</rdakit:toolkitDefinition>
      <rdakit:toolkitLabel xml:lang="es">forma tridimensional</rdakit:toolkitLabel>
      <rdakit:toolkitDefinition xml:lang="es">Contenido expresado mediante una forma o formas pensadas para ser percibidas visualmente en tres dimensiones.</rdakit:toolkitDefinition>
      <skos:prefLabel xml:lang="zh">三维形式</skos:prefLabel>
      <rdakit:toolkitLabel xml:lang="zh">三维形式</rdakit:toolkitLabel>
      <skos:definition xml:lang="zh">以视觉感知的一个或多个三维形式表达的内容。</skos:definition>
      <rdakit:toolkitDefinition xml:lang="zh">以视觉感知的一个或多个三维形式表达的内容。</rdakit:toolkitDefinition>
      <skos:scopeNote xml:lang="zh">包括雕塑、模型、自然物体和标本、全息图等。</skos:scopeNote>
	    <skos:narrower rdf:resource="http://rdaregistry.info/termList/RDAContentType/1006"/>
      <skos:prefLabel xml:lang="nl">driedimensionale vorm</skos:prefLabel>
      <rdakit:toolkitLabel xml:lang="nl">driedimensionale vorm</rdakit:toolkitLabel>
      <skos:definition xml:lang="nl">Content uitgedrukt door een vorm of vormen bedoeld om visueel waar te nemen in drie dimensies.</skos:definition>
      <rdakit:toolkitDefinition xml:lang="nl">Content uitgedrukt door een vorm of vormen bedoeld om visueel waar te nemen in drie dimensies.</rdakit:toolkitDefinition>
      <skos:prefLabel xml:lang="it">forma tridimensionale</skos:prefLabel>
      <rdakit:toolkitLabel xml:lang="it">forma tridimensionale</rdakit:toolkitLabel>
      <skos:definition xml:lang="it">Contenuto espresso mediante una o più forme percepibili con la vista in tre dimensioni.</skos:definition>
      <rdakit:toolkitDefinition xml:lang="it">Contenuto espresso mediante una o più forme percepibili con la vista in tre dimensioni.</rdakit:toolkitDefinition>
      <skos:scopeNote xml:lang="it">Include sculture, modelli, reperti ed esemplari naturali, ologrammi, etc.</skos:scopeNote>
      <skos:prefLabel xml:lang="fi">kolmiulotteinen muoto</skos:prefLabel>
      <rdakit:toolkitLabel xml:lang="fi">kolmiulotteinen muoto</rdakit:toolkitLabel>
      <skos:definition xml:lang="fi">Muotona tai muotoina esitetty sisältö, joka on tarkoitettu katsottavaksi kolmiulotteisena.</skos:definition>
      <rdakit:toolkitDefinition xml:lang="fi">Muotona tai muotoina esitetty sisältö, joka on tarkoitettu katsottavaksi kolmiulotteisena.</rdakit:toolkitDefinition>
      <skos:scopeNote xml:lang="fi">Esimerkiksi veistokset, mallit, luonnonesineet, hologrammit jne. Ei sisällä kosketeltavaksi tarkoitettuja kolmiulotteisia muotoja.</skos:scopeNote>
      <skos:prefLabel xml:lang="he">צורה תלת-ממדית</skos:prefLabel>
      <rdakit:toolkitLabel xml:lang="he">צורה תלת-ממדית</rdakit:toolkitLabel>
      <skos:definition xml:lang="he">סוג תוכן המכיל תוכן אשר קיבל את ביטויו באמצעות צורה או צורות המיועדות לצפייה תלת-ממדית.</skos:definition>
      <rdakit:toolkitDefinition xml:lang="he">סוג תוכן המכיל תוכן אשר קיבל את ביטויו באמצעות צורה או צורות המיועדות לצפייה תלת-ממדית.</rdakit:toolkitDefinition>
      <skos:scopeNote xml:lang="he">כולל פסלים, דגמים, אובייקטים ודגימות טבעיים, הוֹלוֹגְרָמות וכיוצ&quot;ב.</skos:scopeNote>
      <skos:prefLabel xml:lang="ar">شكل ثلاثي الأبعاد</skos:prefLabel>
      <skos:prefLabel xml:lang="sv">tredimensionell form</skos:prefLabel>
      <rdakit:toolkitLabel xml:lang="sv">tredimensionell form</rdakit:toolkitLabel>
      <skos:prefLabel xml:lang="vi">hình thái ba chiều</skos:prefLabel>
      <rdakit:toolkitLabel xml:lang="vi">hình thái ba chiều</rdakit:toolkitLabel>
      <skos:definition xml:lang="vi">Loại nội dung được biểu hiện qua một hoặc nhiều hình thái để nhận biết qua thị giác ở ba chiều.</skos:definition>
      <rdakit:toolkitDefinition xml:lang="vi">Loại nội dung được biểu hiện qua một hoặc nhiều hình thái để nhận biết qua thị giác ở ba chiều.</rdakit:toolkitDefinition>
      <skos:scopeNote xml:lang="vi">Điêu khắc, mô hình, vật thể và mẫu vật xuất hiện tự nhiên, tạo ảnh ba chiều, v.v..., được bao gồm</skos:scopeNote>
      <skos:prefLabel xml:lang="da">tredimensional form</skos:prefLabel>
      <rdakit:toolkitLabel xml:lang="da">tredimensional form</rdakit:toolkitLabel>
      <skos:definition xml:lang="da">Indholdstype der består av indhold udtrykt gennem en eller flere former mhp. at blive opfattet visuelt i tre dimensioner.</skos:definition>
      <rdakit:toolkitDefinition xml:lang="da">Indholdstype der består av indhold udtrykt gennem en eller flere former mhp. at blive opfattet visuelt i tre dimensioner.</rdakit:toolkitDefinition>
      <skos:scopeNote xml:lang="da">Skulpturer, modeller, naturligt forekommende genstande og prøveemner, hologrammer etc. er omfattet. Kartografisk indhold, der er beregnet til at blive opfattet som en tredimensional form er ikke omfattet. Tredimensionale former, der er beregnet til at blive opfattet ved berøring er ikke omfattet.</skos:scopeNote>
      <skos:prefLabel xml:lang="no">tredimensjonal form</skos:prefLabel>
      <rdakit:toolkitLabel xml:lang="no">tredimensjonal form</rdakit:toolkitLabel>
      <skos:definition xml:lang="no">En innholdstype som består av innhold uttrykt gjennom én eller flere former, som skal oppfattes visuelt i tre dimensjoner.</skos:definition>
      <rdakit:toolkitDefinition xml:lang="no">En innholdstype som består av innhold uttrykt gjennom én eller flere former, som skal oppfattes visuelt i tre dimensjoner.</rdakit:toolkitDefinition>
      <skos:scopeNote xml:lang="no">Skulpturer, modeller, naturobjekter og eksemplarer, hologrammer, etc. er inkludert. Kartografisk innhold som er ment for å oppfattes som en tredimensjonal form, er ikke inkludert. Tredimensjonale former som er ment for å oppfattes gjennom berøring, er ikke inkludert.</skos:scopeNote>
    </skos:Concept>
<!-- Concept: three-dimensional moving image  -->
    <skos:Concept rdf:about="http://rdaregistry.info/termList/RDAContentType/1022" xml:lang="en">
      <skos:inScheme rdf:resource="http://rdaregistry.info/termList/RDAContentType"/>
      <reg:status rdf:resource="http://metadataregistry.org/uri/RegStatus/1001"/>
      <reg:identifier rdf:resource="http://metadataregistry.org/concepts/531"/>
      <skos:prefLabel xml:lang="en">three-dimensional moving image</skos:prefLabel>
      <skos:definition xml:lang="en">A content type consisting of content expressed through images intended to be perceived to be moving, and in three dimensions.</skos:definition>
      <skos:scopeNote xml:lang="en">3-D motion pictures using live action and/or animation; stereoscopic, known as S-3D, video games; etc., are included. Three-dimensional moving images may or may not be accompanied by sound.</skos:scopeNote>
      <skos:prefLabel xml:lang="de">Dreidimensionales bewegtes Bild</skos:prefLabel>
      <skos:scopeNote xml:lang="de">Dazu gehören 3D-Filme (natürliche und/oder animierte), stereoskopische (S-3D) Videospiele usw.</skos:scopeNote>
      <skos:definition xml:lang="de">Ein Inhaltstyp, der aus Inhalt besteht, der durch Bilder dargestellt wird und konzipiert ist, um als dreidimensionale Bewegung wahrgenommen zu werden.</skos:definition>
      <skos:scopeNote xml:lang="en">Three-dimensional moving images may or may not be accompanied by sound.</skos:scopeNote>
	    <skos:related rdf:resource="http://rdaregistry.info/termList/RDAContentType/1007"/>
	    <skos:related rdf:resource="http://rdaregistry.info/termList/RDAContentType/1003"/>
      <skos:prefLabel xml:lang="fr">image animée tridimensionnelle</skos:prefLabel>
      <skos:definition xml:lang="fr">Type de contenu qui consiste en contenu exprimé au moyen d’images destinées à être perçues comme animées et en trois dimensions.</skos:definition>
      <skos:scopeNote xml:lang="fr">Comprend les films en 3D utlisant la prise de vue en direct et/ou l’animation, les jeux vidéo en 3D stéréoscopique, également appelée 3DS, etc. Les images animées tridimensionnelles peuvent ou non être accompagnées de son.</skos:scopeNote>
      <skos:prefLabel xml:lang="es">Imagen móvil tridimensional</skos:prefLabel>
      <skos:definition xml:lang="es">Contenido expresado mediante imágenes pensadas para ser percibidas en movimiento en tres dimensiones.</skos:definition>
      <skos:scopeNote xml:lang="es">Incluye películas cinematográficas tridimensionales (que utilizan acción en vivo y/o animación), videojuegos tridimensionales, etc. Las imágenes en movimiento tridimensionales podrían o no estar acompañadas de sonido..</skos:scopeNote>
      <rdakit:toolkitLabel xml:lang="en">three-dimensional moving image</rdakit:toolkitLabel>
      <rdakit:toolkitLabel xml:lang="fr">image animée tridimensionnelle</rdakit:toolkitLabel>
      <rdakit:toolkitDefinition xml:lang="en">A content type consisting of content expressed through images intended to be perceived to be moving, and in three dimensions.</rdakit:toolkitDefinition>
      <rdakit:toolkitDefinition xml:lang="fr">Type de contenu qui consiste en contenu exprimé au moyen d’images destinées à être perçues comme animées et en trois dimensions.</rdakit:toolkitDefinition>
      <rdakit:toolkitLabel xml:lang="de">Dreidimensionales bewegtes Bild</rdakit:toolkitLabel>
      <rdakit:toolkitDefinition xml:lang="de">Ein Inhaltstyp, der aus Inhalt besteht, der durch Bilder dargestellt wird und konzipiert ist, um als dreidimensionale Bewegung wahrgenommen zu werden.</rdakit:toolkitDefinition>
      <rdakit:toolkitLabel xml:lang="es">Imagen móvil tridimensional</rdakit:toolkitLabel>
      <rdakit:toolkitDefinition xml:lang="es">Contenido expresado mediante imágenes pensadas para ser percibidas en movimiento en tres dimensiones.</rdakit:toolkitDefinition>
      <skos:prefLabel xml:lang="zh">三维动态图像</skos:prefLabel>
      <rdakit:toolkitLabel xml:lang="zh">三维动态图像</rdakit:toolkitLabel>
      <skos:definition xml:lang="zh">以三维动态图像表达的、旨在通过动态感知的内容。</skos:definition>
      <rdakit:toolkitDefinition xml:lang="zh">以三维动态图像表达的、旨在通过动态感知的内容。</rdakit:toolkitDefinition>
      <skos:scopeNote xml:lang="zh">包括3-D电影（用真人表演和/或动画模拟）、3-D视频游戏等。三维动态图像有无伴声均可。</skos:scopeNote>
	    <skos:related rdf:resource="http://rdaregistry.info/termList/RDAContentType/1023"/>
      <skos:prefLabel xml:lang="nl">driedimensionaal bewegend beeld</skos:prefLabel>
      <rdakit:toolkitLabel xml:lang="nl">driedimensionaal bewegend beeld</rdakit:toolkitLabel>
      <skos:definition xml:lang="nl">Content uitgedrukt door beelden bedoeld om bewegend waar te nemen en in drie dimensies.</skos:definition>
      <rdakit:toolkitDefinition xml:lang="nl">Content uitgedrukt door beelden bedoeld om bewegend waar te nemen en in drie dimensies.</rdakit:toolkitDefinition>
      <skos:prefLabel xml:lang="it">immagine in movimento tridimensionale</skos:prefLabel>
      <rdakit:toolkitLabel xml:lang="it">immagine in movimento tridimensionale</rdakit:toolkitLabel>
      <skos:definition xml:lang="it">Contenuto espresso mediante immagini percepibili come in movimento, in tre dimensioni.</skos:definition>
      <rdakit:toolkitDefinition xml:lang="it">Contenuto espresso mediante immagini percepibili come in movimento, in tre dimensioni.</rdakit:toolkitDefinition>
      <skos:scopeNote xml:lang="it">Include film 3D (che utilizzano riprese dal vivo e/o animazioni), video giochi 3D, etc. Le immagini in movimento tridimensionali possono o meno essere accompagnate dal suono.</skos:scopeNote>
      <skos:prefLabel xml:lang="fi">kolmiulotteinen liikkuva kuva</skos:prefLabel>
      <rdakit:toolkitLabel xml:lang="fi">kolmiulotteinen liikkuva kuva</rdakit:toolkitLabel>
      <skos:definition xml:lang="fi">Kolmiulotteisena liikkuvana kuvana esitetty sisältö.</skos:definition>
      <rdakit:toolkitDefinition xml:lang="fi">Kolmiulotteisena liikkuvana kuvana esitetty sisältö.</rdakit:toolkitDefinition>
      <skos:scopeNote xml:lang="fi">Elävää kuvaa ja/tai animaatiota sisältävät 3-D -elokuvat.</skos:scopeNote>
      <skos:prefLabel xml:lang="he">תמונת-נוע תלת-ממדית</skos:prefLabel>
      <rdakit:toolkitLabel xml:lang="he">תמונת-נוע תלת-ממדית</rdakit:toolkitLabel>
      <skos:definition xml:lang="he">סוג תוכן המכיל תוכן אשר קיבל את ביטויו באמצעות תמונות נעות המיועדות לצפייה בתלת-ממד.</skos:definition>
      <rdakit:toolkitDefinition xml:lang="he">סוג תוכן המכיל תוכן אשר קיבל את ביטויו באמצעות תמונות נעות המיועדות לצפייה בתלת-ממד.</rdakit:toolkitDefinition>
      <skos:scopeNote xml:lang="he">כולל סרטים בתלת-ממד (בפעולה חיה ו/או בהנפשה), משחקי וידאו בתלת-ממד וכיוצ&quot;ב. כל אלו בליווי קול או בלי קול.</skos:scopeNote>
      <skos:prefLabel xml:lang="ar">صورة متحركة ثلاثية الأبعاد</skos:prefLabel>
      <skos:prefLabel xml:lang="sv">tredimensionell rörlig bild</skos:prefLabel>
      <rdakit:toolkitLabel xml:lang="sv">tredimensionell rörlig bild</rdakit:toolkitLabel>
      <skos:prefLabel xml:lang="vi">hình ảnh động ba chiều</skos:prefLabel>
      <rdakit:toolkitLabel xml:lang="vi">hình ảnh động ba chiều</rdakit:toolkitLabel>
      <skos:definition xml:lang="vi">Loại nội dung được biểu hiện qua hình ảnh để nhận biết chuyển động, và ở ba chiều.</skos:definition>
      <rdakit:toolkitDefinition xml:lang="vi">Loại nội dung được biểu hiện qua hình ảnh để nhận biết chuyển động, và ở ba chiều.</rdakit:toolkitDefinition>
      <skos:scopeNote xml:lang="vi">Phim điện ảnh 3-D dùng hoạt động trực tiếp và/hoặc hoạt hoạ, lập thể, được biết tới như là S-3D, trò chơi video được bao gồm. Hình ảnh động ba chiều có thể kèm theo âm thanh hoặc không.</skos:scopeNote>
      <skos:prefLabel xml:lang="da">tredimensionalt levende billede</skos:prefLabel>
      <rdakit:toolkitLabel xml:lang="da">tredimensionalt levende billede</rdakit:toolkitLabel>
      <skos:definition xml:lang="da">Indholdstype der består af indhold udtrykt gennem billeder mhp. at blive opfattet som værende i bevægelse og i tre dimensioner.</skos:definition>
      <rdakit:toolkitDefinition xml:lang="da">Indholdstype der består af indhold udtrykt gennem billeder mhp. at blive opfattet som værende i bevægelse og i tre dimensioner.</rdakit:toolkitDefinition>
      <skos:scopeNote xml:lang="da">Levende 3D-billeder, der bruger realfilm eller animation; stereoskopiske billeder kendt som S-3D, videospil etc. er omfattet.</skos:scopeNote>
      <skos:prefLabel xml:lang="no">tredimensjonalt levende bilde</skos:prefLabel>
      <rdakit:toolkitLabel xml:lang="no">tredimensjonalt levende bilde</rdakit:toolkitLabel>
      <skos:definition xml:lang="no">En innholdstype som består av innhold uttrykt gjennom levende bilder som skal oppfattes tredimensjonalt.</skos:definition>
      <rdakit:toolkitDefinition xml:lang="no">En innholdstype som består av innhold uttrykt gjennom levende bilder som skal oppfattes tredimensjonalt.</rdakit:toolkitDefinition>
      <skos:scopeNote xml:lang="no">Spillefilm og/eller animert film i 3D, videospill i 3D, etc. er inkludert. Tredimensjonale levende bilder kan være ledsaget av lyd. </skos:scopeNote>
    </skos:Concept>
<!-- Concept: two-dimensional moving image  -->
    <skos:Concept rdf:about="http://rdaregistry.info/termList/RDAContentType/1023" xml:lang="en">
      <skos:inScheme rdf:resource="http://rdaregistry.info/termList/RDAContentType"/>
      <reg:status rdf:resource="http://metadataregistry.org/uri/RegStatus/1001"/>
      <reg:identifier rdf:resource="http://metadataregistry.org/concepts/532"/>
      <skos:prefLabel xml:lang="en">two-dimensional moving image</skos:prefLabel>
      <skos:definition xml:lang="en">A content type consisting of content expressed through images intended to be perceived to be moving, and in two dimensions.</skos:definition>
      <skos:scopeNote xml:lang="en">Motion pictures using live action and/or animation, film and video recordings of performances, events, etc., other than those intended to be perceived in three dimensions, are included. Moving images may or may not be accompanied by sound.</skos:scopeNote>
      <skos:prefLabel xml:lang="de">Zweidimensionales bewegtes Bild</skos:prefLabel>
      <skos:scopeNote xml:lang="de">Dazu gehören Filme (natürliche und/oder animierte), Film- und Videoaufnahmen von Aufführungen, Ereignissen usw., die nicht dafür konzipiert sind, dreidimensional wahrgenommen zu werden. Es kann sich um bewegte Bilder mit oder ohne Ton handeln.</skos:scopeNote>
      <skos:definition xml:lang="de">Ein Inhaltstyp, der aus Inhalt besteht, der durch Bilder dargestellt wird und konzipiert ist, um als zweidimensionale Bewegung wahrgenommen zu werden.</skos:definition>
	    <skos:related rdf:resource="http://rdaregistry.info/termList/RDAContentType/1007"/>
	    <skos:related rdf:resource="http://rdaregistry.info/termList/RDAContentType/1003"/>
      <skos:prefLabel xml:lang="fr">image animée bidimensionnelle</skos:prefLabel>
      <skos:definition xml:lang="fr">Type de contenu qui consiste en contenu exprimé au moyen d’images destinées à être perçues comme animées et en deux dimensions.</skos:definition>
      <skos:scopeNote xml:lang="fr">Comprend les films utilisant la prise de vue en direct et/ou l’animation, les enregistrements sur film ou vidéo de spectacles, d’événements, etc., les jeux vidéo, etc., différents de ceux destinés à être perçus en trois dimensions. Les images animées peuvent ou non être accompagnées de son.</skos:scopeNote>
      <skos:prefLabel xml:lang="es">imagen en movimiento bidimensional</skos:prefLabel>
      <skos:definition xml:lang="es">Contenido expresado mediante imágenes pensadas para ser percibidas en movimiento en dos dimensiones.</skos:definition>
      <skos:scopeNote xml:lang="es">Incluye películas (utilizando acción en vivo y/o animación), grabaciones en película o video de interepretaciones, eventos,etc., diferentes de los pensados para ser percibidos en tres dimensiones. Imágenes en movimiento pueden estar o no acompañadas por sonido.</skos:scopeNote>
      <rdakit:toolkitLabel xml:lang="en">two-dimensional moving image</rdakit:toolkitLabel>
      <rdakit:toolkitLabel xml:lang="fr">image animée bidimensionnelle</rdakit:toolkitLabel>
      <rdakit:toolkitDefinition xml:lang="en">A content type consisting of content expressed through images intended to be perceived to be moving, and in two dimensions.</rdakit:toolkitDefinition>
      <rdakit:toolkitDefinition xml:lang="fr">Type de contenu qui consiste en contenu exprimé au moyen d’images destinées à être perçues comme animées et en deux dimensions.</rdakit:toolkitDefinition>
      <rdakit:toolkitLabel xml:lang="de">Zweidimensionales bewegtes Bild</rdakit:toolkitLabel>
      <rdakit:toolkitDefinition xml:lang="de">Ein Inhaltstyp, der aus Inhalt besteht, der durch Bilder dargestellt wird und konzipiert ist, um als zweidimensionale Bewegung wahrgenommen zu werden.</rdakit:toolkitDefinition>
      <rdakit:toolkitLabel xml:lang="es">imagen en movimiento bidimensional</rdakit:toolkitLabel>
      <rdakit:toolkitDefinition xml:lang="es">Contenido expresado mediante imágenes pensadas para ser percibidas en movimiento en dos dimensiones.</rdakit:toolkitDefinition>
      <skos:prefLabel xml:lang="zh">二维动态图像</skos:prefLabel>
      <rdakit:toolkitLabel xml:lang="zh">二维动态图像</rdakit:toolkitLabel>
      <skos:definition xml:lang="zh">以二维图像表达的、旨在通过动态感知的内容。</skos:definition>
      <rdakit:toolkitDefinition xml:lang="zh">以二维图像表达的、旨在通过动态感知的内容。</rdakit:toolkitDefinition>
      <skos:scopeNote xml:lang="zh">包括电影（用真人表演和/或动画模拟），表演、事件等的摄影或录像，但三维动态图像除外（见三维动态图像Three-Dimensional Moving Image）。动态图像有无伴声均可。</skos:scopeNote>
      <skos:scopeNote xml:lang="es">Incluye películas cinematográficas (que utilizan acción en vivo y/o animación), grabaciones en película y video de interpretaciones, eventos, etc., videojuegos, etc., (excepto aquellas pensadas para ser percibidas en tres dimensiones).</skos:scopeNote>
	    <skos:related rdf:resource="http://rdaregistry.info/termList/RDAContentType/1022"/>
      <skos:prefLabel xml:lang="nl">tweedimensionaal bewegend beeld</skos:prefLabel>
      <rdakit:toolkitLabel xml:lang="nl">tweedimensionaal bewegend beeld</rdakit:toolkitLabel>
      <skos:definition xml:lang="nl">Content uitgedrukt door beelden bedoeld om bewegend waar te nemen en in twee dimensies.</skos:definition>
      <rdakit:toolkitDefinition xml:lang="nl">Content uitgedrukt door beelden bedoeld om bewegend waar te nemen en in twee dimensies.</rdakit:toolkitDefinition>
      <skos:prefLabel xml:lang="it">immagine in movimento bidimensionale</skos:prefLabel>
      <rdakit:toolkitLabel xml:lang="it">immagine in movimento bidimensionale</rdakit:toolkitLabel>
      <skos:definition xml:lang="it">Contenuto espresso mediante immagini percepibili come in movimento, in due dimensioni.</skos:definition>
      <rdakit:toolkitDefinition xml:lang="it">Contenuto espresso mediante immagini percepibili come in movimento, in due dimensioni.</rdakit:toolkitDefinition>
      <skos:scopeNote xml:lang="it">Include film (che utilizzano riprese dal vivo e/o animazioni), registrazioni su pellicola o video di esecuzioni, eventi, etc., video giochi, etc. diversi da quelli percepibili in tre dimensioni. Le immagini in movimento possono o meno essere accompagnate dal suono.</skos:scopeNote>
      <skos:prefLabel xml:lang="fi">kaksiulotteinen liikkuva kuva</skos:prefLabel>
      <rdakit:toolkitLabel xml:lang="fi">kaksiulotteinen liikkuva kuva</rdakit:toolkitLabel>
      <skos:definition xml:lang="fi">Kaksiulotteisena liikkuvana kuvana esitetty sisältö.</skos:definition>
      <rdakit:toolkitDefinition xml:lang="fi">Kaksiulotteisena liikkuvana kuvana esitetty sisältö.</rdakit:toolkitDefinition>
      <skos:scopeNote xml:lang="fi">Esimerkiksi kaksiulotteiset elokuvat (näytellyt tai piirretyt), esitysten ja tapahtumien jne. filmi- ja videotallenteet. Liikkuvaan kuvaan voi liittyä ääntä.</skos:scopeNote>
      <skos:prefLabel xml:lang="he">תמונת-נוע דו-ממדית</skos:prefLabel>
      <rdakit:toolkitLabel xml:lang="he">תמונת-נוע דו-ממדית</rdakit:toolkitLabel>
      <skos:definition xml:lang="he">סוג תוכן המכיל תוכן אשר קיבל את ביטויו באמצעות תמונות נעות, המיועדות לצפייה בדו-ממד.</skos:definition>
      <rdakit:toolkitDefinition xml:lang="he">סוג תוכן המכיל תוכן אשר קיבל את ביטויו באמצעות תמונות נעות, המיועדות לצפייה בדו-ממד.</rdakit:toolkitDefinition>
      <skos:scopeNote xml:lang="he">כולל סרטים (בפעולה חיה ו/או בהנפשה), הקלטות וידיאו של ביצועים, הצגות אירועים וכו', משחקי וידאו וכיוצ&quot;ב, למעט אלו בתלת-ממד. כל אלו בליווי קול או בלי קול.</skos:scopeNote>
      <skos:prefLabel xml:lang="ar">صورة متحركة ثنائية الأبعاد</skos:prefLabel>
      <skos:prefLabel xml:lang="sv">tvådimensionell rörlig bild</skos:prefLabel>
      <rdakit:toolkitLabel xml:lang="sv">tvådimensionell rörlig bild</rdakit:toolkitLabel>
      <skos:prefLabel xml:lang="vi">hình ảnh động hai chiều</skos:prefLabel>
      <rdakit:toolkitLabel xml:lang="vi">hình ảnh động hai chiều</rdakit:toolkitLabel>
      <skos:definition xml:lang="vi">Loại nội dung được biểu hiện qua hình ảnh để nhận biết chuyển động, và ở hai chiều.</skos:definition>
      <rdakit:toolkitDefinition xml:lang="vi">Loại nội dung được biểu hiện qua hình ảnh để nhận biết chuyển động, và ở hai chiều.</rdakit:toolkitDefinition>
      <skos:scopeNote xml:lang="vi">Phim điện ảnh dùng hoạt động trực tiếp và/hoặc hoạt hoạ, phim và video ghi lại cuộc biểu diễn, sự kiện, v.v..., khác với các loại để nhận biết ở trạng thái ba chiều,được bao gồm, Hình ảnh động có thể kèm theo âm thanh hoặc không.</skos:scopeNote>
      <skos:prefLabel xml:lang="da">todimensionalt levende billede</skos:prefLabel>
      <rdakit:toolkitLabel xml:lang="da">todimensionalt levende billede</rdakit:toolkitLabel>
      <skos:definition xml:lang="da">Indholdstype der består af indhold udtrykt gennem billeder beregnet til at blive opfattet som værende i bevægelse og i to dimensioner.</skos:definition>
      <rdakit:toolkitDefinition xml:lang="da">Indholdstype der består af indhold udtrykt gennem billeder beregnet til at blive opfattet som værende i bevægelse og i to dimensioner.</rdakit:toolkitDefinition>
      <skos:scopeNote xml:lang="da">Levende billeder der bruger realfilm og/eller animation, film- og videooptagelser af shows, events etc. bortset fra dem, der er beregnet til at blive opfattet i 3D er omfattet. Levende billeder kan være ledsaget af lyd.</skos:scopeNote>
      <skos:prefLabel xml:lang="no">todimensjonalt levende bilde</skos:prefLabel>
      <rdakit:toolkitLabel xml:lang="no">todimensjonalt levende bilde</rdakit:toolkitLabel>
      <skos:definition xml:lang="no">En innholdstype som består av innhold uttrykt gjennom levende bilder som skal oppfattes todimensjonalt.</skos:definition>
      <rdakit:toolkitDefinition xml:lang="no">En innholdstype som består av innhold uttrykt gjennom levende bilder som skal oppfattes todimensjonalt.</rdakit:toolkitDefinition>
      <skos:scopeNote xml:lang="no">Spillefilm, film og videoopptak av forestillinger, hendelser, etc. med unntak av de som skal oppfattes tredimensjonalt, er inkludert. Levende bilder kan være ledsaget av lyd.</skos:scopeNote>
    </skos:Concept>

<!-- Status properties used in this document  -->
    <skos:Concept rdf:about="http://metadataregistry.org/uri/RegStatus/1001">
        <skos:prefLabel xml:lang="en">Published</skos:prefLabel>
    </skos:Concept>

</rdf:RDF>
