<?xml version="1.0" encoding = "UTF-8"?>
<rdf:RDF
    xmlns:dc="http://purl.org/dc/elements/1.1/"
    xmlns:rdakit="http://metadataregistry.org/uri/profile/rdakit/"
    xmlns:rdf="http://www.w3.org/1999/02/22-rdf-syntax-ns#"
    xmlns:reg="http://metadataregistry.org/uri/profile/regap/"
    xmlns:owl="http://www.w3.org/2002/07/owl#"
    xmlns:skos="http://www.w3.org/2004/02/skos/core#">

<owl:Ontology rdf:about="http://rdaregistry.info/termList/RDACarrierEU" />
<!-- Scheme: RDA Carrier Extent Unit -->
    <skos:ConceptScheme rdf:about="http://rdaregistry.info/termList/RDACarrierEU">
        <dc:title>RDA Carrier Extent Unit</dc:title>
    </skos:ConceptScheme>

<!-- Concept: activity card  -->
    <skos:Concept rdf:about="http://rdaregistry.info/termList/RDACarrierEU/1001" xml:lang="en">
      <skos:inScheme rdf:resource="http://rdaregistry.info/termList/RDACarrierEU"/>
      <reg:status rdf:resource="http://metadataregistry.org/uri/RegStatus/1001"/>
      <reg:identifier rdf:resource="http://metadataregistry.org/concepts/8623"/>
      <skos:prefLabel xml:lang="en">activity card</skos:prefLabel>
      <rdakit:toolkitLabel xml:lang="en">activity card</rdakit:toolkitLabel>
      <skos:definition xml:lang="en">A unit of extent that is a card printed with words, numerals, and/or pictures to be used by an individual or a group as a basis for performing a specific activity.</skos:definition>
      <rdakit:toolkitDefinition xml:lang="en">A unit of extent that is a card printed with words, numerals, and/or pictures to be used by an individual or a group as a basis for performing a specific activity.</rdakit:toolkitDefinition>
      <skos:scopeNote xml:lang="en">This term applies to still images. The cards are usually issued in sets.</skos:scopeNote>
	    <skos:related rdf:resource="http://rdaregistry.info/termList/RDACarrierEU/1039"/>
      <skos:prefLabel xml:lang="ca">fitxa d’activitat</skos:prefLabel>
      <rdakit:toolkitLabel xml:lang="ca">fitxa d’activitat</rdakit:toolkitLabel>
      <skos:definition xml:lang="ca">Unitat d’extensió que és una fitxa impresa amb paraules, xifres i/o imatges, que pot usar un individu o un grup com a base d’una activitat concreta.</skos:definition>
      <rdakit:toolkitDefinition xml:lang="ca">Unitat d’extensió que és una fitxa impresa amb paraules, xifres i/o imatges, que pot usar un individu o un grup com a base d’una activitat concreta.</rdakit:toolkitDefinition>
      <skos:scopeNote xml:lang="ca">Aquest terme s’aplica a imatges fixes. Les fitxes normalment es publiquen en conjunts.</skos:scopeNote>
      <skos:prefLabel xml:lang="vi">quân bài hoạt động</skos:prefLabel>
      <rdakit:toolkitLabel xml:lang="vi">quân bài hoạt động</rdakit:toolkitLabel>
      <skos:definition xml:lang="vi">Đơn vị của quy mô là quân bài in các từ, chữ số, và/hoặc ảnh được dùng vởi một người hoặc nhóm như là điểm xuất phát để tiến hành một hoạt động cụ thể.</skos:definition>
      <rdakit:toolkitDefinition xml:lang="vi">Đơn vị của quy mô là quân bài in các từ, chữ số, và/hoặc ảnh được dùng vởi một người hoặc nhóm như là điểm xuất phát để tiến hành một hoạt động cụ thể.</rdakit:toolkitDefinition>
      <skos:scopeNote xml:lang="vi">Thuật ngữ này áp dụng cho hình ảnh tĩnh. Quân bài này luôn được công bố theo bộ.</skos:scopeNote>
      <skos:prefLabel xml:lang="de">Spielkarte</skos:prefLabel>
      <rdakit:toolkitLabel xml:lang="de">Spielkarte</rdakit:toolkitLabel>
      <skos:definition xml:lang="de">Eine Einheit für den Umfang einer Karte, die mit Wörtern, Zahlen und/oder Bildern bedruckt ist, und von einer Person oder einer Gruppe als Grundlage für die Durchführung einer spezifischen Aktivität verwendet wird.</skos:definition>
      <rdakit:toolkitDefinition xml:lang="de">Eine Einheit für den Umfang einer Karte, die mit Wörtern, Zahlen und/oder Bildern bedruckt ist, und von einer Person oder einer Gruppe als Grundlage für die Durchführung einer spezifischen Aktivität verwendet wird.</rdakit:toolkitDefinition>
      <skos:scopeNote xml:lang="de">Dieser Terminus trifft auf unbewegte Bilder zu. Erscheint normalerweise in Sets.</skos:scopeNote>
      <skos:prefLabel xml:lang="fi">toimintakortti</skos:prefLabel>
      <rdakit:toolkitLabel xml:lang="fi">toimintakortti</rdakit:toolkitLabel>
      <skos:definition xml:lang="fi">Laajuuden yksikkö, kortti, johon on painettu sanoja, numeroita, tai/ja kuvia, ja jota käytetään tietyn toiminnan toteuttamisessa.</skos:definition>
      <rdakit:toolkitDefinition xml:lang="fi">Laajuuden yksikkö, kortti, johon on painettu sanoja, numeroita, tai/ja kuvia, ja jota käytetään tietyn toiminnan toteuttamisessa.</rdakit:toolkitDefinition>
      <skos:scopeNote xml:lang="fi">Termi koskee stillkuvia. Kortit julkaistaan yleensä sarjoina.</skos:scopeNote>
      <skos:altLabel xml:lang="da">aktivitetskort</skos:altLabel>
      <rdakit:toolkitLabel xml:lang="da">aktivitetskort</rdakit:toolkitLabel>
      <skos:definition xml:lang="da">Enhed, der består af et kort med påtrykte ord, tal og/eller billeder til brug for en enkelt person eller en gruppe som grundlag for at udføre en bestemt aktivitet. Normalt udgivet i sæt.</skos:definition>
      <rdakit:toolkitDefinition xml:lang="da">Enhed, der består af et kort med påtrykte ord, tal og/eller billeder til brug for en enkelt person eller en gruppe som grundlag for at udføre en bestemt aktivitet. Normalt udgivet i sæt.</rdakit:toolkitDefinition>
      <skos:scopeNote xml:lang="da">Denne term anvendes for faste billeder. Kortene er normalt udgivet i sæt.</skos:scopeNote>
      <skos:prefLabel xml:lang="fr">carte d’activité</skos:prefLabel>
      <rdakit:toolkitLabel xml:lang="fr">carte d’activité</rdakit:toolkitLabel>
      <skos:definition xml:lang="fr">Unité d’importance matérielle qui consiste en une carte sur laquelle sont imprimés des mots, des chiffres et/ou des images et destinée à être utilisée par une personne ou un groupe comme support à l’exécution d’une activité donnée.</skos:definition>
      <rdakit:toolkitDefinition xml:lang="fr">Unité d’importance matérielle qui consiste en une carte sur laquelle sont imprimés des mots, des chiffres et/ou des images et destinée à être utilisée par une personne ou un groupe comme support à l’exécution d’une activité donnée.</rdakit:toolkitDefinition>
      <skos:scopeNote xml:lang="fr">Ce terme s’applique aux ressources cartographiques et aux formes tridimensionnelles.</skos:scopeNote>
      <skos:prefLabel xml:lang="no">aktivitetskort</skos:prefLabel>
      <rdakit:toolkitLabel xml:lang="no">aktivitetskort</rdakit:toolkitLabel>
      <skos:definition xml:lang="no">En omfangsenhet i form av et kort med trykte ord, tall og/eller bilder, ment for bruk av enkeltpersoner eller grupper som utgangspunkt for å utføre en bestemt aktivitet.</skos:definition>
      <rdakit:toolkitDefinition xml:lang="no">En omfangsenhet i form av et kort med trykte ord, tall og/eller bilder, ment for bruk av enkeltpersoner eller grupper som utgangspunkt for å utføre en bestemt aktivitet.</rdakit:toolkitDefinition>
      <skos:scopeNote xml:lang="no">Dette begrepet gjelder stillbilder. Kortene utgis vanligvis som sett.</skos:scopeNote>
    </skos:Concept>
<!-- Concept: atlas  -->
    <skos:Concept rdf:about="http://rdaregistry.info/termList/RDACarrierEU/1002" xml:lang="en">
      <skos:inScheme rdf:resource="http://rdaregistry.info/termList/RDACarrierEU"/>
      <reg:status rdf:resource="http://metadataregistry.org/uri/RegStatus/1001"/>
      <reg:identifier rdf:resource="http://metadataregistry.org/concepts/8624"/>
      <skos:prefLabel xml:lang="en">atlas</skos:prefLabel>
      <rdakit:toolkitLabel xml:lang="en">atlas</rdakit:toolkitLabel>
      <skos:definition xml:lang="en">A unit of extent that is a volume of maps or other cartographic content with or without descriptive text.</skos:definition>
      <rdakit:toolkitDefinition xml:lang="en">A unit of extent that is a volume of maps or other cartographic content with or without descriptive text.</rdakit:toolkitDefinition>
      <skos:scopeNote xml:lang="en">This term applies to cartographic resources.</skos:scopeNote>
      <skos:prefLabel xml:lang="ca">atles</skos:prefLabel>
      <rdakit:toolkitLabel xml:lang="ca">atles</rdakit:toolkitLabel>
      <skos:definition xml:lang="ca">Unitat d’extensió que és un volum de mapes o de qualsevol altre contingut cartogràfic amb o sense text descriptiu.</skos:definition>
      <rdakit:toolkitDefinition xml:lang="ca">Unitat d’extensió que és un volum de mapes o de qualsevol altre contingut cartogràfic amb o sense text descriptiu.</rdakit:toolkitDefinition>
      <skos:scopeNote xml:lang="ca">Aquest terme s’aplica a recursos cartogràfics.</skos:scopeNote>
      <skos:prefLabel xml:lang="vi">tập bản đồ</skos:prefLabel>
      <rdakit:toolkitLabel xml:lang="vi">tập bản đồ</rdakit:toolkitLabel>
      <skos:definition xml:lang="vi">Đơn vị của quy mô là tập các bản đồ hoặc nội dung đồ hình khác, có hoặc không văn bản mô tả.</skos:definition>
      <rdakit:toolkitDefinition xml:lang="vi">Đơn vị của quy mô là tập các bản đồ hoặc nội dung đồ hình khác, có hoặc không văn bản mô tả.</rdakit:toolkitDefinition>
      <skos:scopeNote xml:lang="vi">Thuật ngữ này áp dụng cho tài nguyên bản đồ.</skos:scopeNote>
      <skos:prefLabel xml:lang="de">Atlas</skos:prefLabel>
      <rdakit:toolkitLabel xml:lang="de">Atlas</rdakit:toolkitLabel>
      <skos:definition xml:lang="de">Eine Einheit für den Umfang eines Bandes von Karten oder sonstigen kartografischen Inhalten mit oder ohne beschreibenden Text.</skos:definition>
      <rdakit:toolkitDefinition xml:lang="de">Eine Einheit für den Umfang eines Bandes von Karten oder sonstigen kartografischen Inhalten mit oder ohne beschreibenden Text.</rdakit:toolkitDefinition>
      <skos:scopeNote xml:lang="de">Dieser Terminus trifft auf kartografische Ressource zu.</skos:scopeNote>
      <skos:prefLabel xml:lang="fi">kartasto</skos:prefLabel>
      <rdakit:toolkitLabel xml:lang="fi">kartasto</rdakit:toolkitLabel>
      <skos:definition xml:lang="fi">Laajuuden yksikkö, karttakirja tai muu karttakokonaisuus, selittävän tekstin kanssa tai ilman.</skos:definition>
      <rdakit:toolkitDefinition xml:lang="fi">Laajuuden yksikkö, karttakirja tai muu karttakokonaisuus, selittävän tekstin kanssa tai ilman.</rdakit:toolkitDefinition>
      <skos:scopeNote xml:lang="fi">Termi koskee kartografisia aineistoja.</skos:scopeNote>
      <skos:altLabel xml:lang="da">atlas</skos:altLabel>
      <rdakit:toolkitLabel xml:lang="da">atlas</rdakit:toolkitLabel>
      <skos:definition xml:lang="da">Enhed, der består af et bind med kort eller andet kartografisk indhold med eller uden beskrivende tekst.</skos:definition>
      <rdakit:toolkitDefinition xml:lang="da">Enhed, der består af et bind med kort eller andet kartografisk indhold med eller uden beskrivende tekst.</rdakit:toolkitDefinition>
      <skos:scopeNote xml:lang="da">Denne term anvendes for kartografiske ressourcer.</skos:scopeNote>
      <skos:prefLabel xml:lang="fr">atlas</skos:prefLabel>
      <rdakit:toolkitLabel xml:lang="fr">atlas</rdakit:toolkitLabel>
      <skos:definition xml:lang="fr">Unité d’importance matérielle qui consiste en un volume de cartes ou d’autre contenu cartographique avec ou sans texte descriptif.</skos:definition>
      <rdakit:toolkitDefinition xml:lang="fr">Unité d’importance matérielle qui consiste en un volume de cartes ou d’autre contenu cartographique avec ou sans texte descriptif.</rdakit:toolkitDefinition>
      <skos:prefLabel xml:lang="no">atlas</skos:prefLabel>
      <rdakit:toolkitLabel xml:lang="no">atlas</rdakit:toolkitLabel>
      <skos:definition xml:lang="no">En omfangsenhet som består av et bind med kart eller annet kartografisk innhold med eller uten beskrivende tekst.</skos:definition>
      <rdakit:toolkitDefinition xml:lang="no">En omfangsenhet som består av et bind med kart eller annet kartografisk innhold med eller uten beskrivende tekst.</rdakit:toolkitDefinition>
      <skos:scopeNote xml:lang="no">Dette begrepet gjelder kartografiske ressurser.</skos:scopeNote>
    </skos:Concept>
<!-- Concept: case  -->
    <skos:Concept rdf:about="http://rdaregistry.info/termList/RDACarrierEU/1003" xml:lang="en">
      <skos:inScheme rdf:resource="http://rdaregistry.info/termList/RDACarrierEU"/>
      <reg:status rdf:resource="http://metadataregistry.org/uri/RegStatus/1001"/>
      <reg:identifier rdf:resource="http://metadataregistry.org/concepts/8625"/>
      <skos:prefLabel xml:lang="en">case</skos:prefLabel>
      <rdakit:toolkitLabel xml:lang="en">case</rdakit:toolkitLabel>
      <skos:definition xml:lang="en">A unit of extent consisting of a box containing bound or unbound resources.</skos:definition>
      <rdakit:toolkitDefinition xml:lang="en">A unit of extent consisting of a box containing bound or unbound resources.</rdakit:toolkitDefinition>
      <skos:prefLabel xml:lang="ca">capsa</skos:prefLabel>
      <rdakit:toolkitLabel xml:lang="ca">capsa</rdakit:toolkitLabel>
      <skos:definition xml:lang="ca">Unitat d’extensió que consisteix en un estoig que conté recursos relligats o sense relligar.</skos:definition>
      <rdakit:toolkitDefinition xml:lang="ca">Unitat d’extensió que consisteix en un estoig que conté recursos relligats o sense relligar.</rdakit:toolkitDefinition>
      <skos:prefLabel xml:lang="vi">hộp đựng</skos:prefLabel>
      <rdakit:toolkitLabel xml:lang="vi">hộp đựng</rdakit:toolkitLabel>
      <skos:definition xml:lang="vi">Đơn vị của quy mô là Hộp để đựng nguồn lực đóng bìa hoặc không đóng bìa.</skos:definition>
      <rdakit:toolkitDefinition xml:lang="vi">Đơn vị của quy mô là Hộp để đựng nguồn lực đóng bìa hoặc không đóng bìa.</rdakit:toolkitDefinition>
      <skos:prefLabel xml:lang="de">Kiste</skos:prefLabel>
      <rdakit:toolkitLabel xml:lang="de">Kiste</rdakit:toolkitLabel>
      <skos:definition xml:lang="de">Eine Einheit für den Umfang, der aus einer Schachtel besteht, die gebundene oder ungebundene Ressourcen enthält.</skos:definition>
      <rdakit:toolkitDefinition xml:lang="de">Eine Einheit für den Umfang, der aus einer Schachtel besteht, die gebundene oder ungebundene Ressourcen enthält.</rdakit:toolkitDefinition>
      <skos:prefLabel xml:lang="fi">kotelo</skos:prefLabel>
      <rdakit:toolkitLabel xml:lang="fi">kotelo</rdakit:toolkitLabel>
      <skos:definition xml:lang="fi">Laajuuden yksikkö, muodostuu sidottuja tai sitomattomia aineistoja sisältävästä laatikosta.</skos:definition>
      <rdakit:toolkitDefinition xml:lang="fi">Laajuuden yksikkö, muodostuu sidottuja tai sitomattomia aineistoja sisältävästä laatikosta.</rdakit:toolkitDefinition>
      <skos:altLabel xml:lang="da">opbevaringsudstyr</skos:altLabel>
      <rdakit:toolkitLabel xml:lang="da">opbevaringsudstyr</rdakit:toolkitLabel>
      <skos:definition xml:lang="da">Enhed, der består af en kasse eller æske, der indeholder indbundne eller ikke-indbundne ressourcer.</skos:definition>
      <rdakit:toolkitDefinition xml:lang="da">Enhed, der består af en kasse eller æske, der indeholder indbundne eller ikke-indbundne ressourcer.</rdakit:toolkitDefinition>
      <skos:prefLabel xml:lang="fr">emboîtage</skos:prefLabel>
      <rdakit:toolkitLabel xml:lang="fr">emboîtage</rdakit:toolkitLabel>
      <skos:definition xml:lang="fr">Unité d’importance matérielle qui consiste en une boîte contenant des ressources reliées ou non reliées.</skos:definition>
      <rdakit:toolkitDefinition xml:lang="fr">Unité d’importance matérielle qui consiste en une boîte contenant des ressources reliées ou non reliées.</rdakit:toolkitDefinition>
      <skos:scopeNote xml:lang="fr">Ce terme s’applique aux images fixes.</skos:scopeNote>
      <skos:prefLabel xml:lang="no">eske</skos:prefLabel>
      <rdakit:toolkitLabel xml:lang="no">eske</rdakit:toolkitLabel>
      <skos:definition xml:lang="no">En omfangsenhet. Består av en boks som inneholder innbundne eller uinnbundne ressurser.</skos:definition>
      <rdakit:toolkitDefinition xml:lang="no">En omfangsenhet. Består av en boks som inneholder innbundne eller uinnbundne ressurser.</rdakit:toolkitDefinition>
    </skos:Concept>
<!-- Concept: chart  -->
    <skos:Concept rdf:about="http://rdaregistry.info/termList/RDACarrierEU/1004" xml:lang="en">
      <skos:inScheme rdf:resource="http://rdaregistry.info/termList/RDACarrierEU"/>
      <reg:status rdf:resource="http://metadataregistry.org/uri/RegStatus/1001"/>
      <reg:identifier rdf:resource="http://metadataregistry.org/concepts/8626"/>
      <skos:prefLabel xml:lang="en">chart</skos:prefLabel>
      <rdakit:toolkitLabel xml:lang="en">chart</rdakit:toolkitLabel>
      <skos:definition xml:lang="en">A unit of extent consisting of a two-dimensional representation of data in graphic or tabular form.</skos:definition>
      <rdakit:toolkitDefinition xml:lang="en">A unit of extent consisting of a two-dimensional representation of data in graphic or tabular form.</rdakit:toolkitDefinition>
      <skos:scopeNote xml:lang="en">This term applies to still images.</skos:scopeNote>
      <skos:prefLabel xml:lang="ca">diagrama</skos:prefLabel>
      <rdakit:toolkitLabel xml:lang="ca">diagrama</rdakit:toolkitLabel>
      <skos:definition xml:lang="ca">Unitat d'extensió que consisteix en una representació bidimensional de dades en una forma gràfica o tabular.</skos:definition>
      <rdakit:toolkitDefinition xml:lang="ca">Unitat d'extensió que consisteix en una representació bidimensional de dades en una forma gràfica o tabular.</rdakit:toolkitDefinition>
      <skos:scopeNote xml:lang="ca">Aquest terme s'aplica a imatges fixes.</skos:scopeNote>
      <skos:prefLabel xml:lang="vi">đồ thị</skos:prefLabel>
      <rdakit:toolkitLabel xml:lang="vi">đồ thị</rdakit:toolkitLabel>
      <skos:definition xml:lang="vi">Đơn vị của quy mô gồm có Trình bày hai chiều của dữ liệu dưới hình thái đồ hình hoặc bảng biểu.</skos:definition>
      <rdakit:toolkitDefinition xml:lang="vi">Đơn vị của quy mô gồm có Trình bày hai chiều của dữ liệu dưới hình thái đồ hình hoặc bảng biểu.</rdakit:toolkitDefinition>
      <skos:scopeNote xml:lang="vi">Thuật ngữ này áp dụng cho hình ảnh tĩnh.</skos:scopeNote>
      <skos:prefLabel xml:lang="de">Schaubild</skos:prefLabel>
      <rdakit:toolkitLabel xml:lang="de">Schaubild</rdakit:toolkitLabel>
      <skos:definition xml:lang="de">Eine Einheit für den Umfang, bestehend aus einer zweidimensionale Darstellung der Daten in grafischer oder tabellarischer Form.</skos:definition>
      <rdakit:toolkitDefinition xml:lang="de">Eine Einheit für den Umfang, bestehend aus einer zweidimensionale Darstellung der Daten in grafischer oder tabellarischer Form.</rdakit:toolkitDefinition>
      <skos:scopeNote xml:lang="de">Dieser Terminus trifft auf unbewegte Bilder zu.</skos:scopeNote>
      <skos:prefLabel xml:lang="fi">taulukko</skos:prefLabel>
      <rdakit:toolkitLabel xml:lang="fi">taulukko</rdakit:toolkitLabel>
      <skos:definition xml:lang="fi">Kaksiulotteinen tiedon esitystapa joko graafisessa muodossa tai taulukkona.</skos:definition>
      <rdakit:toolkitDefinition xml:lang="fi">Kaksiulotteinen tiedon esitystapa joko graafisessa muodossa tai taulukkona.</rdakit:toolkitDefinition>
      <skos:scopeNote xml:lang="fi">Termi koskee stillkuvia.</skos:scopeNote>
      <skos:altLabel xml:lang="da">diagram</skos:altLabel>
      <rdakit:toolkitLabel xml:lang="da">diagram</rdakit:toolkitLabel>
      <skos:definition xml:lang="da">Enhed, der består af en todimensionel gengivelse af data i grafisk eller tabelform</skos:definition>
      <rdakit:toolkitDefinition xml:lang="da">Enhed, der består af en todimensionel gengivelse af data i grafisk eller tabelform</rdakit:toolkitDefinition>
      <skos:scopeNote xml:lang="da">Denne term anvendes for faste billeder.</skos:scopeNote>
      <skos:prefLabel xml:lang="fr">diagramme</skos:prefLabel>
      <rdakit:toolkitLabel xml:lang="fr">diagramme</rdakit:toolkitLabel>
      <skos:definition xml:lang="fr">Unité d’importance matérielle qui consiste en une représentation bidimensionnelle de données sous forme d’un graphique ou d’un tableau.</skos:definition>
      <rdakit:toolkitDefinition xml:lang="fr">Unité d’importance matérielle qui consiste en une représentation bidimensionnelle de données sous forme d’un graphique ou d’un tableau.</rdakit:toolkitDefinition>
      <skos:prefLabel xml:lang="no">plansje</skos:prefLabel>
      <rdakit:toolkitLabel xml:lang="no">plansje</rdakit:toolkitLabel>
      <skos:definition xml:lang="no">En omfangsenhet som består av en todimensjonal fremstilling av data i grafisk form eller tabellform.</skos:definition>
      <rdakit:toolkitDefinition xml:lang="no">En omfangsenhet som består av en todimensjonal fremstilling av data i grafisk form eller tabellform.</rdakit:toolkitDefinition>
      <skos:scopeNote xml:lang="no">Dette begrepet gjelder stillbilder.</skos:scopeNote>
    </skos:Concept>
<!-- Concept: coin  -->
    <skos:Concept rdf:about="http://rdaregistry.info/termList/RDACarrierEU/1005" xml:lang="en">
      <skos:inScheme rdf:resource="http://rdaregistry.info/termList/RDACarrierEU"/>
      <reg:status rdf:resource="http://metadataregistry.org/uri/RegStatus/1001"/>
      <reg:identifier rdf:resource="http://metadataregistry.org/concepts/8627"/>
      <skos:prefLabel xml:lang="en">coin</skos:prefLabel>
      <rdakit:toolkitLabel xml:lang="en">coin</rdakit:toolkitLabel>
      <skos:definition xml:lang="en">A unit of extent consisting of a piece of metal stamped by government authority for use as money.</skos:definition>
      <rdakit:toolkitDefinition xml:lang="en">A unit of extent consisting of a piece of metal stamped by government authority for use as money.</rdakit:toolkitDefinition>
      <skos:scopeNote xml:lang="en">This term applies to three-dimensional forms.</skos:scopeNote>
      <skos:prefLabel xml:lang="ca">moneda</skos:prefLabel>
      <rdakit:toolkitLabel xml:lang="ca">moneda</rdakit:toolkitLabel>
      <skos:definition xml:lang="ca">Unitat d’extensió que consisteix en una peça de metall estampada per l’autoritat del govern perquè s’usi com a diner.</skos:definition>
      <rdakit:toolkitDefinition xml:lang="ca">Unitat d’extensió que consisteix en una peça de metall estampada per l’autoritat del govern perquè s’usi com a diner.</rdakit:toolkitDefinition>
      <skos:scopeNote xml:lang="ca">Aquest terme s'aplica a formes tridimensionals.</skos:scopeNote>
      <skos:prefLabel xml:lang="vi">đồng xu</skos:prefLabel>
      <rdakit:toolkitLabel xml:lang="vi">đồng xu</rdakit:toolkitLabel>
      <skos:definition xml:lang="vi">Đơn vị của quy mô là gồm có miếng kim loại được cơ quan thẩm quyền của chính phủ in dấu để sử dụng như tiền.</skos:definition>
      <rdakit:toolkitDefinition xml:lang="vi">Đơn vị của quy mô là gồm có miếng kim loại được cơ quan thẩm quyền của chính phủ in dấu để sử dụng như tiền.</rdakit:toolkitDefinition>
      <skos:scopeNote xml:lang="vi">Thuật ngữ này áp dụng cho hình thái ba chiều.</skos:scopeNote>
      <skos:prefLabel xml:lang="de">Münze</skos:prefLabel>
      <rdakit:toolkitLabel xml:lang="de">Münze</rdakit:toolkitLabel>
      <skos:definition xml:lang="de">Eine Einheit für den Umfang, bestehend aus einem Stück Metall, das von einer staatlichen Behörde zur Verwendung als Geld geprägt wurde.</skos:definition>
      <rdakit:toolkitDefinition xml:lang="de">Eine Einheit für den Umfang, bestehend aus einem Stück Metall, das von einer staatlichen Behörde zur Verwendung als Geld geprägt wurde.</rdakit:toolkitDefinition>
      <skos:scopeNote xml:lang="de">Dieser Terminus trifft auf dreidimensionale Formen zu.</skos:scopeNote>
      <skos:prefLabel xml:lang="fi">metalliraha</skos:prefLabel>
      <rdakit:toolkitLabel xml:lang="fi">metalliraha</rdakit:toolkitLabel>
      <skos:definition xml:lang="fi">Laajuuden yksikkö, rahana käytetty metallikappale, jossa on virallisen tahon kuten valtion, hallitsijan tms. leima.</skos:definition>
      <rdakit:toolkitDefinition xml:lang="fi">Laajuuden yksikkö, rahana käytetty metallikappale, jossa on virallisen tahon kuten valtion, hallitsijan tms. leima.</rdakit:toolkitDefinition>
      <skos:scopeNote xml:lang="fi">Termi koskee kolmiulotteisia muotoja.</skos:scopeNote>
      <skos:altLabel xml:lang="da">mønt</skos:altLabel>
      <rdakit:toolkitLabel xml:lang="da">mønt</rdakit:toolkitLabel>
      <skos:definition xml:lang="da">Enhed, der består af et stykke metal, der er præget af staten mhp. at blive brugt som penge.</skos:definition>
      <rdakit:toolkitDefinition xml:lang="da">Enhed, der består af et stykke metal, der er præget af staten mhp. at blive brugt som penge.</rdakit:toolkitDefinition>
      <skos:scopeNote xml:lang="da">Denne term anvendes for tredimensionelle former.</skos:scopeNote>
      <skos:prefLabel xml:lang="fr">monnaie</skos:prefLabel>
      <rdakit:toolkitLabel xml:lang="fr">monnaie</rdakit:toolkitLabel>
      <skos:definition xml:lang="fr">Unité d’importance matérielle qui consiste en une pièce de métal frappée par une autorité gouvernementale pour usage monétaire.</skos:definition>
      <rdakit:toolkitDefinition xml:lang="fr">Unité d’importance matérielle qui consiste en une pièce de métal frappée par une autorité gouvernementale pour usage monétaire.</rdakit:toolkitDefinition>
      <skos:scopeNote xml:lang="fr">Ce terme s’applique aux images fixes.</skos:scopeNote>
      <skos:prefLabel xml:lang="no">mynt</skos:prefLabel>
      <rdakit:toolkitLabel xml:lang="no">mynt</rdakit:toolkitLabel>
      <skos:definition xml:lang="no">En omfangsenhet som består av et metallstykke som er preget av offentlige myndigheter og brukes som penger.</skos:definition>
      <rdakit:toolkitDefinition xml:lang="no">En omfangsenhet som består av et metallstykke som er preget av offentlige myndigheter og brukes som penger.</rdakit:toolkitDefinition>
      <skos:scopeNote xml:lang="no">Dette begrepet gjelder tredimensjonale former.</skos:scopeNote>
    </skos:Concept>
<!-- Concept: collage  -->
    <skos:Concept rdf:about="http://rdaregistry.info/termList/RDACarrierEU/1006" xml:lang="en">
      <skos:inScheme rdf:resource="http://rdaregistry.info/termList/RDACarrierEU"/>
      <reg:status rdf:resource="http://metadataregistry.org/uri/RegStatus/1001"/>
      <reg:identifier rdf:resource="http://metadataregistry.org/concepts/8628"/>
      <skos:prefLabel xml:lang="en">collage</skos:prefLabel>
      <rdakit:toolkitLabel xml:lang="en">collage</rdakit:toolkitLabel>
      <skos:definition xml:lang="en">A unit of extent consisting of a work in two dimensions or very low relief that was made by affixing paper, fabrics, photographs, or other materials onto a flat surface.</skos:definition>
      <rdakit:toolkitDefinition xml:lang="en">A unit of extent consisting of a work in two dimensions or very low relief that was made by affixing paper, fabrics, photographs, or other materials onto a flat surface.</rdakit:toolkitDefinition>
      <skos:scopeNote xml:lang="en">This term applies to still images.</skos:scopeNote>
      <skos:prefLabel xml:lang="ca">collage</skos:prefLabel>
      <rdakit:toolkitLabel xml:lang="ca">collage</rdakit:toolkitLabel>
      <skos:definition xml:lang="ca">Unitat d’extensió que consisteix en una obra en dues dimensions o d’un relleu molt baix, feta a base d’enganxar paper, tela, fotografies o altres materials en una superfície plana.</skos:definition>
      <rdakit:toolkitDefinition xml:lang="ca">Unitat d’extensió que consisteix en una obra en dues dimensions o d’un relleu molt baix, feta a base d’enganxar paper, tela, fotografies o altres materials en una superfície plana.</rdakit:toolkitDefinition>
      <skos:scopeNote xml:lang="ca">Aquest terme s'aplica a imatges fixes.</skos:scopeNote>
      <skos:prefLabel xml:lang="vi">hình cắt dán</skos:prefLabel>
      <rdakit:toolkitLabel xml:lang="vi">hình cắt dán</rdakit:toolkitLabel>
      <skos:definition xml:lang="vi">Đơn vị của quy mô gồm có tác phẩm hai chiều hoặc chạm nổi rất thấp được tạo ra bằng cách dán giấy, vải, bức ảnh, hoặc vật liệu khác trên bề mặt phẳng.</skos:definition>
      <rdakit:toolkitDefinition xml:lang="vi">Đơn vị của quy mô gồm có tác phẩm hai chiều hoặc chạm nổi rất thấp được tạo ra bằng cách dán giấy, vải, bức ảnh, hoặc vật liệu khác trên bề mặt phẳng.</rdakit:toolkitDefinition>
      <skos:scopeNote xml:lang="vi">Thuật ngữ này áp dụng cho hình ảnh tĩnh.</skos:scopeNote>
      <skos:prefLabel xml:lang="de">Collage</skos:prefLabel>
      <rdakit:toolkitLabel xml:lang="de">Collage</rdakit:toolkitLabel>
      <skos:definition xml:lang="de">Eine Einheit für den Umfang, bestehend aus einem zweidimensionalen oder sehr flachen reliefartigen Werk, das durch Befestigung von Papier, Stoff, Fotografien oder sonstigen Materialien auf einer ebenen Oberfläche gemacht ist.</skos:definition>
      <rdakit:toolkitDefinition xml:lang="de">Eine Einheit für den Umfang, bestehend aus einem zweidimensionalen oder sehr flachen reliefartigen Werk, das durch Befestigung von Papier, Stoff, Fotografien oder sonstigen Materialien auf einer ebenen Oberfläche gemacht ist.</rdakit:toolkitDefinition>
      <skos:scopeNote xml:lang="de">Dieser Terminus trifft auf unbewegte Bilder zu.</skos:scopeNote>
      <skos:prefLabel xml:lang="fi">kollaasi</skos:prefLabel>
      <rdakit:toolkitLabel xml:lang="fi">kollaasi</rdakit:toolkitLabel>
      <skos:definition xml:lang="fi">Laajuuden yksikkö, koostuu kaksiulotteisesta tai hyvin matalasta kohokuvasta, joka on tehty liimaamalla yhteen paperia, kangasta, valokuvia tai muita materiaaleja tasaiselle pinnalle.</skos:definition>
      <rdakit:toolkitDefinition xml:lang="fi">Laajuuden yksikkö, koostuu kaksiulotteisesta tai hyvin matalasta kohokuvasta, joka on tehty liimaamalla yhteen paperia, kangasta, valokuvia tai muita materiaaleja tasaiselle pinnalle.</rdakit:toolkitDefinition>
      <skos:scopeNote xml:lang="fi">Termi koskee stillkuvia.</skos:scopeNote>
      <skos:altLabel xml:lang="da">collage</skos:altLabel>
      <rdakit:toolkitLabel xml:lang="da">collage</rdakit:toolkitLabel>
      <skos:definition xml:lang="da">Enhed, der består af et todimensionelt værk eller et værk i meget flad relief, der er fremstillet ved, at papir, stof, fotos eller andre materialer er fæstnet på en flad overflade.</skos:definition>
      <rdakit:toolkitDefinition xml:lang="da">Enhed, der består af et todimensionelt værk eller et værk i meget flad relief, der er fremstillet ved, at papir, stof, fotos eller andre materialer er fæstnet på en flad overflade.</rdakit:toolkitDefinition>
      <skos:scopeNote xml:lang="da">Denne term anvendes for faste billeder.</skos:scopeNote>
      <skos:prefLabel xml:lang="fr">collage</skos:prefLabel>
      <rdakit:toolkitLabel xml:lang="fr">collage</rdakit:toolkitLabel>
      <skos:definition xml:lang="fr">Unité d’importance matérielle qui consiste en une œuvre bidimensionnelle ou à très bas relief réalisée par l’apposition de papier, de tissus, de photographies ou d’autres matériaux sur une surface plane.</skos:definition>
      <rdakit:toolkitDefinition xml:lang="fr">Unité d’importance matérielle qui consiste en une œuvre bidimensionnelle ou à très bas relief réalisée par l’apposition de papier, de tissus, de photographies ou d’autres matériaux sur une surface plane.</rdakit:toolkitDefinition>
      <skos:prefLabel xml:lang="no">collage</skos:prefLabel>
      <rdakit:toolkitLabel xml:lang="no">collage</rdakit:toolkitLabel>
      <skos:definition xml:lang="no">En omfangsenhet som består av et verk i to dimensjoner eller med svært lav relieff, laget ved å feste papir, tekstiler, fotografier eller andre materialer på et flatt underlag.</skos:definition>
      <rdakit:toolkitDefinition xml:lang="no">En omfangsenhet som består av et verk i to dimensjoner eller med svært lav relieff, laget ved å feste papir, tekstiler, fotografier eller andre materialer på et flatt underlag.</rdakit:toolkitDefinition>
      <skos:scopeNote xml:lang="no">Dette begrepet gjelder stillbilder.</skos:scopeNote>
    </skos:Concept>
<!-- Concept: column  -->
    <skos:Concept rdf:about="http://rdaregistry.info/termList/RDACarrierEU/1007" xml:lang="en">
      <skos:inScheme rdf:resource="http://rdaregistry.info/termList/RDACarrierEU"/>
      <reg:status rdf:resource="http://metadataregistry.org/uri/RegStatus/1001"/>
      <reg:identifier rdf:resource="http://metadataregistry.org/concepts/8629"/>
      <skos:prefLabel xml:lang="en">column</skos:prefLabel>
      <rdakit:toolkitLabel xml:lang="en">column</rdakit:toolkitLabel>
      <skos:definition xml:lang="en">A unit of extent consisting of one of two or more vertical sections of text appearing on the same page or leaf.</skos:definition>
      <rdakit:toolkitDefinition xml:lang="en">A unit of extent consisting of one of two or more vertical sections of text appearing on the same page or leaf.</rdakit:toolkitDefinition>
      <skos:prefLabel xml:lang="ca">columna</skos:prefLabel>
      <rdakit:toolkitLabel xml:lang="ca">columna</rdakit:toolkitLabel>
      <skos:definition xml:lang="ca">Unitat d’extensió que consisteix en una, dues o més seccions verticals de text que figuren a la mateixa pàgina o al mateix full.</skos:definition>
      <rdakit:toolkitDefinition xml:lang="ca">Unitat d’extensió que consisteix en una, dues o més seccions verticals de text que figuren a la mateixa pàgina o al mateix full.</rdakit:toolkitDefinition>
      <skos:prefLabel xml:lang="vi">cột</skos:prefLabel>
      <rdakit:toolkitLabel xml:lang="vi">cột</rdakit:toolkitLabel>
      <skos:definition xml:lang="vi">Đơn vị của quy mô gồm có một của hai hoặc nhiều hơn đoan văn bản xuất hiện trên cùng trang hoặc tờ.</skos:definition>
      <rdakit:toolkitDefinition xml:lang="vi">Đơn vị của quy mô gồm có một của hai hoặc nhiều hơn đoan văn bản xuất hiện trên cùng trang hoặc tờ.</rdakit:toolkitDefinition>
      <skos:prefLabel xml:lang="de">Spalte</skos:prefLabel>
      <rdakit:toolkitLabel xml:lang="de">Spalte</rdakit:toolkitLabel>
      <skos:definition xml:lang="de">Eine Einheit für den Umfang, bestehend aus einem oder zwei vertikal angeordneten Textabschnitten, die auf derselben Seite oder demselben Blatt erscheinen.</skos:definition>
      <rdakit:toolkitDefinition xml:lang="de">Eine Einheit für den Umfang, bestehend aus einem oder zwei vertikal angeordneten Textabschnitten, die auf derselben Seite oder demselben Blatt erscheinen.</rdakit:toolkitDefinition>
      <skos:prefLabel xml:lang="fi">palsta</skos:prefLabel>
      <rdakit:toolkitLabel xml:lang="fi">palsta</rdakit:toolkitLabel>
      <skos:definition xml:lang="fi">Laajuuden yksikkö, kahdelle tai useammalle pystysuoralle saman sivun osalle jaetun tekstin yksi pystysuora osa.</skos:definition>
      <rdakit:toolkitDefinition xml:lang="fi">Laajuuden yksikkö, kahdelle tai useammalle pystysuoralle saman sivun osalle jaetun tekstin yksi pystysuora osa.</rdakit:toolkitDefinition>
      <skos:altLabel xml:lang="da">spalte</skos:altLabel>
      <rdakit:toolkitLabel xml:lang="da">spalte</rdakit:toolkitLabel>
      <skos:definition xml:lang="da">Enhed, der består af en af to eller flere lodrette tekstsektioner på samme side eller blad.</skos:definition>
      <rdakit:toolkitDefinition xml:lang="da">Enhed, der består af en af to eller flere lodrette tekstsektioner på samme side eller blad.</rdakit:toolkitDefinition>
      <skos:prefLabel xml:lang="fr">colonne</skos:prefLabel>
      <rdakit:toolkitLabel xml:lang="fr">colonne</rdakit:toolkitLabel>
      <skos:definition xml:lang="fr">Unité d’importance matérielle qui consiste en l’une de deux ou plusieurs sections verticales de texte figurant sur la même page ou le même feuillet.</skos:definition>
      <rdakit:toolkitDefinition xml:lang="fr">Unité d’importance matérielle qui consiste en l’une de deux ou plusieurs sections verticales de texte figurant sur la même page ou le même feuillet.</rdakit:toolkitDefinition>
      <skos:scopeNote xml:lang="fr">Ce terme s’applique aux images fixes.</skos:scopeNote>
      <skos:prefLabel xml:lang="no">spalte</skos:prefLabel>
      <rdakit:toolkitLabel xml:lang="no">spalte</rdakit:toolkitLabel>
      <skos:definition xml:lang="no">En omfangsenhet. Består av to eller flere loddrette tekstseksjoner på samme side eller blad.</skos:definition>
      <rdakit:toolkitDefinition xml:lang="no">En omfangsenhet. Består av to eller flere loddrette tekstseksjoner på samme side eller blad.</rdakit:toolkitDefinition>
    </skos:Concept>
<!-- Concept: diagram  -->
    <skos:Concept rdf:about="http://rdaregistry.info/termList/RDACarrierEU/1008" xml:lang="en">
      <skos:inScheme rdf:resource="http://rdaregistry.info/termList/RDACarrierEU"/>
      <reg:status rdf:resource="http://metadataregistry.org/uri/RegStatus/1001"/>
      <reg:identifier rdf:resource="http://metadataregistry.org/concepts/8630"/>
      <skos:prefLabel xml:lang="en">diagram</skos:prefLabel>
      <rdakit:toolkitLabel xml:lang="en">diagram</rdakit:toolkitLabel>
      <skos:definition xml:lang="en">A unit of extent that is a geographic representation of numeric data, or of the course or results of an action or process.</skos:definition>
      <rdakit:toolkitDefinition xml:lang="en">A unit of extent that is a geographic representation of numeric data, or of the course or results of an action or process.</rdakit:toolkitDefinition>
      <skos:scopeNote xml:lang="en">This term applies to cartographic resources. The term is sometimes also applied to maps characterized by much simplified, or schematic, representation.</skos:scopeNote>
      <skos:prefLabel xml:lang="ca">diagrama</skos:prefLabel>
      <rdakit:toolkitLabel xml:lang="ca">diagrama</rdakit:toolkitLabel>
      <skos:definition xml:lang="ca">Unitat d’extensió que és una representació geogràfica de dades numèriques, o del curs o els resultats d’una acció o un procés.</skos:definition>
      <rdakit:toolkitDefinition xml:lang="ca">Unitat d’extensió que és una representació geogràfica de dades numèriques, o del curs o els resultats d’una acció o un procés.</rdakit:toolkitDefinition>
      <skos:scopeNote xml:lang="ca">Aquest terme s'aplica a recursos cartogràfics. El terme també s’aplica de vegades a mapes que es caracteritzen per una representació molt esquemàtica o simplificada.</skos:scopeNote>
      <skos:prefLabel xml:lang="vi">biểu đồ</skos:prefLabel>
      <rdakit:toolkitLabel xml:lang="vi">biểu đồ</rdakit:toolkitLabel>
      <skos:definition xml:lang="vi">Đơn vị của quy mô là trình bày địa lý của dữ liệu số, hoặc của tiến trình hoặc kết quả của hoạt động hoặc quá trình.</skos:definition>
      <rdakit:toolkitDefinition xml:lang="vi">Đơn vị của quy mô là trình bày địa lý của dữ liệu số, hoặc của tiến trình hoặc kết quả của hoạt động hoặc quá trình.</rdakit:toolkitDefinition>
      <skos:scopeNote xml:lang="vi">Thuật ngữ này áp dụng cho tài nguyên bản đồ. Thuật ngữ này cũng đôi khi áp dụng cho bản đồ được đặc trưng bởi trình bày đơn giản hoá, hoặc dưới dạng giản đồ.</skos:scopeNote>
      <skos:prefLabel xml:lang="de">Diagramm</skos:prefLabel>
      <rdakit:toolkitLabel xml:lang="de">Diagramm</rdakit:toolkitLabel>
      <skos:definition xml:lang="de">Eine Einheit für den Umfang, bestehend aus einer geografischen Darstellung numerischer Daten bzw. dem Verlauf oder den Ergebnissen einer Tätigkeit oder eines Prozesses.</skos:definition>
      <rdakit:toolkitDefinition xml:lang="de">Eine Einheit für den Umfang, bestehend aus einer geografischen Darstellung numerischer Daten bzw. dem Verlauf oder den Ergebnissen einer Tätigkeit oder eines Prozesses.</rdakit:toolkitDefinition>
      <skos:scopeNote xml:lang="de">Dieser Terminus trifft auf kartografische Ressourcen zu. Der Terminus wird manchmal auch für Karten verwendet, die durch sehr vereinfachte oder schematische Darstellung charakterisiert sind.</skos:scopeNote>
      <skos:prefLabel xml:lang="fi">diagrammi</skos:prefLabel>
      <rdakit:toolkitLabel xml:lang="fi">diagrammi</rdakit:toolkitLabel>
      <skos:definition xml:lang="fi">Laajuuden yksikkö, kartta-aineisto, joka on numeerisen tiedon tai jonkin tapahtuman tai prosessin etenemisen tai vaikutusten maantieteellinen esitysmuoto.</skos:definition>
      <rdakit:toolkitDefinition xml:lang="fi">Laajuuden yksikkö, kartta-aineisto, joka on numeerisen tiedon tai jonkin tapahtuman tai prosessin etenemisen tai vaikutusten maantieteellinen esitysmuoto.</rdakit:toolkitDefinition>
      <skos:scopeNote xml:lang="fi">Termi koskee kartografisia aineistoja. Termiä käytetään toisinaan myös karttoihin, jotka ovat luonteeltaan erittäin yksinkertaisia tai yleisluontoisia.</skos:scopeNote>
      <skos:altLabel xml:lang="da">diagram</skos:altLabel>
      <rdakit:toolkitLabel xml:lang="da">diagram</rdakit:toolkitLabel>
      <skos:definition xml:lang="da">Enhed, der geografisk præsenterer numeriske data, forløbet eller resultaterne af en handling eller proces.</skos:definition>
      <rdakit:toolkitDefinition xml:lang="da">Enhed, der geografisk præsenterer numeriske data, forløbet eller resultaterne af en handling eller proces.</rdakit:toolkitDefinition>
      <skos:scopeNote xml:lang="da">Denne term anvendes for kartografiske ressourcer. Termen anvendes også sommetider om kort, der er karakteriseret ved en meget simplificeret eller skematisk repræsentation.</skos:scopeNote>
      <skos:prefLabel xml:lang="fr">diagramme</skos:prefLabel>
      <rdakit:toolkitLabel xml:lang="fr">diagramme</rdakit:toolkitLabel>
      <skos:definition xml:lang="fr">Unité d’importance matérielle qui consiste en une représentation géographique de données numériques, ou du déroulement ou des résultats d’une action ou d’un processus.</skos:definition>
      <rdakit:toolkitDefinition xml:lang="fr">Unité d’importance matérielle qui consiste en une représentation géographique de données numériques, ou du déroulement ou des résultats d’une action ou d’un processus.</rdakit:toolkitDefinition>
      <skos:scopeNote xml:lang="fr">Ce terme s’applique aux images fixes.</skos:scopeNote>
      <skos:prefLabel xml:lang="no">diagram</skos:prefLabel>
      <rdakit:toolkitLabel xml:lang="no">diagram</rdakit:toolkitLabel>
      <skos:definition xml:lang="no">En omfangsenhet som er en geografisk framstilling av numeriske data, eller av gangen i eller resultatet av en handling eller prosess.</skos:definition>
      <rdakit:toolkitDefinition xml:lang="no">En omfangsenhet som er en geografisk framstilling av numeriske data, eller av gangen i eller resultatet av en handling eller prosess.</rdakit:toolkitDefinition>
      <skos:scopeNote xml:lang="no">Dette begrepet gjelder kartografiske ressurser. Begrepet kan også brukes på kart med en kraftig forenklet eller skjematisk gjengivelse.</skos:scopeNote>
    </skos:Concept>
<!-- Concept: diorama  -->
    <skos:Concept rdf:about="http://rdaregistry.info/termList/RDACarrierEU/1009" xml:lang="en">
      <skos:inScheme rdf:resource="http://rdaregistry.info/termList/RDACarrierEU"/>
      <reg:status rdf:resource="http://metadataregistry.org/uri/RegStatus/1001"/>
      <reg:identifier rdf:resource="http://metadataregistry.org/concepts/8631"/>
      <skos:prefLabel xml:lang="en">diorama</skos:prefLabel>
      <rdakit:toolkitLabel xml:lang="en">diorama</rdakit:toolkitLabel>
      <skos:definition xml:lang="en">A unit of extent consisting of a three-dimensional representation of a scene created by placing objects, figures, etc., in front of a two-dimensional painted background.</skos:definition>
      <rdakit:toolkitDefinition xml:lang="en">A unit of extent consisting of a three-dimensional representation of a scene created by placing objects, figures, etc., in front of a two-dimensional painted background.</rdakit:toolkitDefinition>
      <skos:scopeNote xml:lang="en">This term applies to three-dimensional forms.</skos:scopeNote>
      <skos:prefLabel xml:lang="ca">diorama</skos:prefLabel>
      <rdakit:toolkitLabel xml:lang="ca">diorama</rdakit:toolkitLabel>
      <skos:definition xml:lang="ca">Unitat d’extensió que consisteix en una representació tridimensional d’una escena creada mitjançant la col·locació d’objectes, de figures, etc., davant d’un decorat de fons, pintat i bidimensional.</skos:definition>
      <rdakit:toolkitDefinition xml:lang="ca">Unitat d’extensió que consisteix en una representació tridimensional d’una escena creada mitjançant la col·locació d’objectes, de figures, etc., davant d’un decorat de fons, pintat i bidimensional.</rdakit:toolkitDefinition>
      <skos:scopeNote xml:lang="ca">Aquest terme s'aplica a formes tridimensionals.</skos:scopeNote>
      <skos:prefLabel xml:lang="vi">cảnh tầm sâu</skos:prefLabel>
      <rdakit:toolkitLabel xml:lang="vi">cảnh tầm sâu</rdakit:toolkitLabel>
      <skos:definition xml:lang="vi">Đơn vị của quy mô gồm có Trình bày ba chiều của quang cảnh được tao ra bằng cách sắp đặt đối tượng, vật thể, vv..., trước hậu cảnh hội hoạ hai chiều.</skos:definition>
      <rdakit:toolkitDefinition xml:lang="vi">Đơn vị của quy mô gồm có Trình bày ba chiều của quang cảnh được tao ra bằng cách sắp đặt đối tượng, vật thể, vv..., trước hậu cảnh hội hoạ hai chiều.</rdakit:toolkitDefinition>
      <skos:scopeNote xml:lang="vi">Thuật ngữ này áp dụng cho hình thái ba chiều.</skos:scopeNote>
      <skos:prefLabel xml:lang="de">Diorama</skos:prefLabel>
      <rdakit:toolkitLabel xml:lang="de">Diorama</rdakit:toolkitLabel>
      <skos:definition xml:lang="de">Eine Einheit für den Umfang, bestehend aus einer dreidimensionalen Darstellung einer Szene, die durch das Platzieren von Objekten, Figuren usw. vor einem zweidimensionalen gezeichneten Hintergrund geschaffen wird.</skos:definition>
      <rdakit:toolkitDefinition xml:lang="de">Eine Einheit für den Umfang, bestehend aus einer dreidimensionalen Darstellung einer Szene, die durch das Platzieren von Objekten, Figuren usw. vor einem zweidimensionalen gezeichneten Hintergrund geschaffen wird.</rdakit:toolkitDefinition>
      <skos:scopeNote xml:lang="de">Dieser Terminus trifft auf dreidimensionale Formen zu.</skos:scopeNote>
      <skos:prefLabel xml:lang="fi">dioraama</skos:prefLabel>
      <rdakit:toolkitLabel xml:lang="fi">dioraama</rdakit:toolkitLabel>
      <skos:definition xml:lang="fi">Laajuuden yksikkö, kolmiulotteinen maisemamalli tai asetelma, jossa kaksiulotteisen maalatun taustan eteen on aseteltu esineitä, hahmoja tms.</skos:definition>
      <rdakit:toolkitDefinition xml:lang="fi">Laajuuden yksikkö, kolmiulotteinen maisemamalli tai asetelma, jossa kaksiulotteisen maalatun taustan eteen on aseteltu esineitä, hahmoja tms.</rdakit:toolkitDefinition>
      <skos:scopeNote xml:lang="fi">Termi koskee kolmiulotteisia muotoja.</skos:scopeNote>
      <skos:altLabel xml:lang="da">diorama</skos:altLabel>
      <rdakit:toolkitLabel xml:lang="da">diorama</rdakit:toolkitLabel>
      <skos:definition xml:lang="da">Enhed, der består af en tredimensionel repræsentation, der der gengiver en scene, der er skabt, ved at genstande, figurer etc. er placeret foran en todimensionel malet baggrund.</skos:definition>
      <rdakit:toolkitDefinition xml:lang="da">Enhed, der består af en tredimensionel repræsentation, der der gengiver en scene, der er skabt, ved at genstande, figurer etc. er placeret foran en todimensionel malet baggrund.</rdakit:toolkitDefinition>
      <skos:scopeNote xml:lang="da">Denne term anvendes for tredimensionelle former.</skos:scopeNote>
      <skos:prefLabel xml:lang="fr">diorama</skos:prefLabel>
      <rdakit:toolkitLabel xml:lang="fr">diorama</rdakit:toolkitLabel>
      <skos:definition xml:lang="fr">Unité d’importance matérielle qui consiste en une représentation tridimensionnelle d’une scène créée par la disposition d’objets, de personnages, etc. devant un fond bidimensionnel peint.</skos:definition>
      <rdakit:toolkitDefinition xml:lang="fr">Unité d’importance matérielle qui consiste en une représentation tridimensionnelle d’une scène créée par la disposition d’objets, de personnages, etc. devant un fond bidimensionnel peint.</rdakit:toolkitDefinition>
      <skos:scopeNote xml:lang="fr">Ce terme s’applique aux images fixes.</skos:scopeNote>
      <skos:prefLabel xml:lang="no">diorama</skos:prefLabel>
      <rdakit:toolkitLabel xml:lang="no">diorama</rdakit:toolkitLabel>
      <skos:definition xml:lang="no">En omfangsenhet i tredimensjonal form som består av en tredimensjonal representasjon av et motiv skapt ved å plassere gjenstander, figutrer, etc. foran en todimensjonal, malt bakgrunn.</skos:definition>
      <rdakit:toolkitDefinition xml:lang="no">En omfangsenhet i tredimensjonal form som består av en tredimensjonal representasjon av et motiv skapt ved å plassere gjenstander, figutrer, etc. foran en todimensjonal, malt bakgrunn.</rdakit:toolkitDefinition>
      <skos:scopeNote xml:lang="no">Dette begrepet gjelder tredimensjonale former.</skos:scopeNote>
    </skos:Concept>
<!-- Concept: drawing  -->
    <skos:Concept rdf:about="http://rdaregistry.info/termList/RDACarrierEU/1010" xml:lang="en">
      <skos:inScheme rdf:resource="http://rdaregistry.info/termList/RDACarrierEU"/>
      <reg:status rdf:resource="http://metadataregistry.org/uri/RegStatus/1001"/>
      <reg:identifier rdf:resource="http://metadataregistry.org/concepts/8632"/>
      <skos:prefLabel xml:lang="en">drawing</skos:prefLabel>
      <rdakit:toolkitLabel xml:lang="en">drawing</rdakit:toolkitLabel>
      <skos:definition xml:lang="en">A unit of extent consisting of a visual work produced by drawing, which is the application of lines on a surface, often paper, by using a pencil, pen, chalk, or some other tracing instrument to focus on the delineation of form rather than the application of color.</skos:definition>
      <rdakit:toolkitDefinition xml:lang="en">A unit of extent consisting of a visual work produced by drawing, which is the application of lines on a surface, often paper, by using a pencil, pen, chalk, or some other tracing instrument to focus on the delineation of form rather than the application of color.</rdakit:toolkitDefinition>
      <skos:scopeNote xml:lang="en">This term applies to still images. This term is often defined broadly to refer to computer-generated images as well.</skos:scopeNote>
      <skos:prefLabel xml:lang="ca">dibuix</skos:prefLabel>
      <rdakit:toolkitLabel xml:lang="ca">dibuix</rdakit:toolkitLabel>
      <skos:definition xml:lang="ca">Unitat d’extensió que consisteix en una obra visual produïda mitjançant un dibuix, que és l’aplicació de línies sobre una superfície, sovint paper, amb un llapis, una ploma, un guix o qualsevol altre instrument, i que se centra en el traçat de formes més que en l’aplicació de color.</skos:definition>
      <rdakit:toolkitDefinition xml:lang="ca">Unitat d’extensió que consisteix en una obra visual produïda mitjançant un dibuix, que és l’aplicació de línies sobre una superfície, sovint paper, amb un llapis, una ploma, un guix o qualsevol altre instrument, i que se centra en el traçat de formes més que en l’aplicació de color.</rdakit:toolkitDefinition>
      <skos:scopeNote xml:lang="ca">Aquest terme s'aplica a imatges fixes. Aquest terme sovint es defineix més àmpliament per fer referència també a les imatges generades per ordinador.</skos:scopeNote>
      <skos:prefLabel xml:lang="vi">bản vẽ</skos:prefLabel>
      <rdakit:toolkitLabel xml:lang="vi">bản vẽ</rdakit:toolkitLabel>
      <skos:definition xml:lang="vi">Đơn vị của quy mô gồm có tác phẩm thị giác được sản xuất bằng cách vẽ, nghĩa là áp dụng các đường trên bề mặt, thường là giấy, bằng cách dùng bút chì, bút, phấn, hoặc các dụng cụ kẻ đường khác để tập trung vào mô tả hình thể hơn là áp dụng màu sắc.</skos:definition>
      <rdakit:toolkitDefinition xml:lang="vi">Đơn vị của quy mô gồm có tác phẩm thị giác được sản xuất bằng cách vẽ, nghĩa là áp dụng các đường trên bề mặt, thường là giấy, bằng cách dùng bút chì, bút, phấn, hoặc các dụng cụ kẻ đường khác để tập trung vào mô tả hình thể hơn là áp dụng màu sắc.</rdakit:toolkitDefinition>
      <skos:scopeNote xml:lang="vi">Thuật ngữ này áp dụng cho hình ảnh tĩnh.</skos:scopeNote>
      <skos:prefLabel xml:lang="de">Zeichnung</skos:prefLabel>
      <rdakit:toolkitLabel xml:lang="de">Zeichnung</rdakit:toolkitLabel>
      <skos:definition xml:lang="de">Eine Einheit für den Umfang, bestehend aus einem visuellen Werk, das durch Zeichnen, d. h. Aufbringen von Linien auf eine Oberfläche, häufig Papier, unter Verwendung eines Bleistifts, eines Zeichenstifts, Kohle oder eines anderen Spuren hinterlassenden Instruments erstellt wird. Dabei liegt der Fokus auf der Darstellung der Form und weniger auf der Anwendung von Farbe.</skos:definition>
      <rdakit:toolkitDefinition xml:lang="de">Eine Einheit für den Umfang, bestehend aus einem visuellen Werk, das durch Zeichnen, d. h. Aufbringen von Linien auf eine Oberfläche, häufig Papier, unter Verwendung eines Bleistifts, eines Zeichenstifts, Kohle oder eines anderen Spuren hinterlassenden Instruments erstellt wird. Dabei liegt der Fokus auf der Darstellung der Form und weniger auf der Anwendung von Farbe.</rdakit:toolkitDefinition>
      <skos:scopeNote xml:lang="de">Dieser Terminus trifft auf unbewegte Bilder zu. Dieser Terminus wird häufig breit definiert, damit er sich ebenso auf computer-generierte Bilder beziehen kann.</skos:scopeNote>
      <skos:prefLabel xml:lang="fi">piirustus</skos:prefLabel>
      <rdakit:toolkitLabel xml:lang="fi">piirustus</rdakit:toolkitLabel>
      <skos:definition xml:lang="fi">Laajuuden yksikkö, piirtämällä tehty liikkumaton kuva pohjamateriaalille, usein paperille, käyttäen kynää, hiiltä, liitua tai puuta piirustusvälinettä ja korostaen muotoa ennemmin kuin värejä.</skos:definition>
      <rdakit:toolkitDefinition xml:lang="fi">Laajuuden yksikkö, piirtämällä tehty liikkumaton kuva pohjamateriaalille, usein paperille, käyttäen kynää, hiiltä, liitua tai puuta piirustusvälinettä ja korostaen muotoa ennemmin kuin värejä.</rdakit:toolkitDefinition>
      <skos:scopeNote xml:lang="fi">Termi koskee stillkuvia. Termiä käytetään usein laajemmassa merkityksessä myös tietokoneella tuotettuihin kuviin.</skos:scopeNote>
      <skos:altLabel xml:lang="da">tegning</skos:altLabel>
      <rdakit:toolkitLabel xml:lang="da">tegning</rdakit:toolkitLabel>
      <skos:definition xml:lang="da">Enhed, der består af et visuelt værk fremstillet ved tegning, dvs. påføring af linjer på en overflade, ofte papir, vha. blyant, kuglepen, kridt eller et andet tegneværktøj med fokus på afbildning af form snarere end påføring af farve.</skos:definition>
      <rdakit:toolkitDefinition xml:lang="da">Enhed, der består af et visuelt værk fremstillet ved tegning, dvs. påføring af linjer på en overflade, ofte papir, vha. blyant, kuglepen, kridt eller et andet tegneværktøj med fokus på afbildning af form snarere end påføring af farve.</rdakit:toolkitDefinition>
      <skos:scopeNote xml:lang="da">Denne term anvendes for faste billeder.Termen defineres ofte bredt, så den også refererer til computergenererede billeder.</skos:scopeNote>
      <skos:prefLabel xml:lang="fr">dessin</skos:prefLabel>
      <rdakit:toolkitLabel xml:lang="fr">dessin</rdakit:toolkitLabel>
      <skos:definition xml:lang="fr">Unité d’importance matérielle qui consiste en une œuvre visuelle produite par dessin, qui est l’application de traits sur une surface, souvent du papier, à l’aide d’un crayon, d’un stylo, d’une plume, d’une craie ou d’un autre instrument traceur pour se concentrer sur la délimitation de la forme plutôt que sur l’application de couleur.</skos:definition>
      <rdakit:toolkitDefinition xml:lang="fr">Unité d’importance matérielle qui consiste en une œuvre visuelle produite par dessin, qui est l’application de traits sur une surface, souvent du papier, à l’aide d’un crayon, d’un stylo, d’une plume, d’une craie ou d’un autre instrument traceur pour se concentrer sur la délimitation de la forme plutôt que sur l’application de couleur.</rdakit:toolkitDefinition>
      <skos:scopeNote xml:lang="fr">Ce terme s’applique aux ressources cartographiques.</skos:scopeNote>
      <skos:prefLabel xml:lang="no">tegning</skos:prefLabel>
      <rdakit:toolkitLabel xml:lang="no">tegning</rdakit:toolkitLabel>
      <skos:definition xml:lang="no">En omfangsenhet som består av et verk produsert ved å tegne, som er å plassere linjer på en overflate, ofte av papir, ved å bruke blyant, penn, kritt eller andre hjelpemidler, for å fokusere på avbildning av form framfor fargelegging.</skos:definition>
      <rdakit:toolkitDefinition xml:lang="no">En omfangsenhet som består av et verk produsert ved å tegne, som er å plassere linjer på en overflate, ofte av papir, ved å bruke blyant, penn, kritt eller andre hjelpemidler, for å fokusere på avbildning av form framfor fargelegging.</rdakit:toolkitDefinition>
      <skos:scopeNote xml:lang="no">Dette begrepet gjelder stillbilder. Denne termen defineres ofte bredt, for også å omfatte digitalt genererte bilder.</skos:scopeNote>
    </skos:Concept>
<!-- Concept: exhibit  -->
    <skos:Concept rdf:about="http://rdaregistry.info/termList/RDACarrierEU/1011" xml:lang="en">
      <skos:inScheme rdf:resource="http://rdaregistry.info/termList/RDACarrierEU"/>
      <reg:status rdf:resource="http://metadataregistry.org/uri/RegStatus/1001"/>
      <reg:identifier rdf:resource="http://metadataregistry.org/concepts/8633"/>
      <skos:prefLabel xml:lang="en">exhibit</skos:prefLabel>
      <rdakit:toolkitLabel xml:lang="en">exhibit</rdakit:toolkitLabel>
      <skos:definition xml:lang="en">A unit of extent consisting of objects on display, along with the display environment of cases, labels, etc.</skos:definition>
      <rdakit:toolkitDefinition xml:lang="en">A unit of extent consisting of objects on display, along with the display environment of cases, labels, etc.</rdakit:toolkitDefinition>
      <skos:scopeNote xml:lang="en">This term applies to three-dimensional forms.</skos:scopeNote>
      <skos:prefLabel xml:lang="ca">objecte d’exposició</skos:prefLabel>
      <rdakit:toolkitLabel xml:lang="ca">objecte d’exposició</rdakit:toolkitLabel>
      <skos:definition xml:lang="ca">Unitat d’extensió que consisteix en objectes en exposició, juntament amb l’entorn de l’exposició (capses, etiquetes, etc.).</skos:definition>
      <rdakit:toolkitDefinition xml:lang="ca">Unitat d’extensió que consisteix en objectes en exposició, juntament amb l’entorn de l’exposició (capses, etiquetes, etc.).</rdakit:toolkitDefinition>
      <skos:scopeNote xml:lang="ca">Aquest terme s'aplica a formes tridimensionals.</skos:scopeNote>
      <skos:prefLabel xml:lang="vi">triển lãm</skos:prefLabel>
      <rdakit:toolkitLabel xml:lang="vi">triển lãm</rdakit:toolkitLabel>
      <skos:definition xml:lang="vi">Đơn vị của quy mô gồm có vật thể được trưng bày, cùng với mội trường trưng bày như tủ, nhãn, v.v...</skos:definition>
      <rdakit:toolkitDefinition xml:lang="vi">Đơn vị của quy mô gồm có vật thể được trưng bày, cùng với mội trường trưng bày như tủ, nhãn, v.v...</rdakit:toolkitDefinition>
      <skos:scopeNote xml:lang="vi">Thuật ngữ này áp dụng cho hình thái ba chiều.</skos:scopeNote>
      <skos:prefLabel xml:lang="de">Ausstellungsstück</skos:prefLabel>
      <rdakit:toolkitLabel xml:lang="de">Ausstellungsstück</rdakit:toolkitLabel>
      <skos:definition xml:lang="de">Eine Einheit für den Umfang, die aus ausgestellten Gegenständen mit dem Ausstellungsumfeld (Kisten, Labels usw.) besteht.</skos:definition>
      <rdakit:toolkitDefinition xml:lang="de">Eine Einheit für den Umfang, die aus ausgestellten Gegenständen mit dem Ausstellungsumfeld (Kisten, Labels usw.) besteht.</rdakit:toolkitDefinition>
      <skos:scopeNote xml:lang="de">Dieser Terminus trifft auf dreidimensionale Formen zu.</skos:scopeNote>
      <skos:prefLabel xml:lang="fi">näyttelyesine</skos:prefLabel>
      <rdakit:toolkitLabel xml:lang="fi">näyttelyesine</rdakit:toolkitLabel>
      <skos:definition xml:lang="fi">Laajuuden yksikkö, esine joka on esillä näyttelynomaisessa ympäristössä mukaan lukien kotelo, etiketti tms.</skos:definition>
      <rdakit:toolkitDefinition xml:lang="fi">Laajuuden yksikkö, esine joka on esillä näyttelynomaisessa ympäristössä mukaan lukien kotelo, etiketti tms.</rdakit:toolkitDefinition>
      <skos:scopeNote xml:lang="fi">Termi koskee kolmiulotteisia muotoja.</skos:scopeNote>
      <skos:altLabel xml:lang="da">udstilling</skos:altLabel>
      <rdakit:toolkitLabel xml:lang="da">udstilling</rdakit:toolkitLabel>
      <skos:definition xml:lang="da">Enhed, der består af udstillede genstande samt udstillingsmiljø af beholdere, etiketter etc.</skos:definition>
      <rdakit:toolkitDefinition xml:lang="da">Enhed, der består af udstillede genstande samt udstillingsmiljø af beholdere, etiketter etc.</rdakit:toolkitDefinition>
      <skos:scopeNote xml:lang="da">Denne term anvendes for tredimensionelle former.</skos:scopeNote>
      <skos:prefLabel xml:lang="fr">objet exposé</skos:prefLabel>
      <rdakit:toolkitLabel xml:lang="fr">objet exposé</rdakit:toolkitLabel>
      <skos:definition xml:lang="fr">Unité d’importance matérielle qui consiste en objets en exposition accompagnés de l’environnement d’exposition comprenant les vitrines, les étiquettes, etc.</skos:definition>
      <rdakit:toolkitDefinition xml:lang="fr">Unité d’importance matérielle qui consiste en objets en exposition accompagnés de l’environnement d’exposition comprenant les vitrines, les étiquettes, etc.</rdakit:toolkitDefinition>
      <skos:prefLabel xml:lang="no">utstillingsgjenstand</skos:prefLabel>
      <rdakit:toolkitLabel xml:lang="no">utstillingsgjenstand</rdakit:toolkitLabel>
      <skos:definition xml:lang="no">En omfangsenhet som består av gjenstander som vises fram, sammen med utstillingsomgivelser som esker, etiketter etc.</skos:definition>
      <rdakit:toolkitDefinition xml:lang="no">En omfangsenhet som består av gjenstander som vises fram, sammen med utstillingsomgivelser som esker, etiketter etc.</rdakit:toolkitDefinition>
      <skos:scopeNote xml:lang="no">Dette begrepet gjelder tredimensjonale former.</skos:scopeNote>
    </skos:Concept>
<!-- Concept: flash card  -->
    <skos:Concept rdf:about="http://rdaregistry.info/termList/RDACarrierEU/1012" xml:lang="en">
      <skos:inScheme rdf:resource="http://rdaregistry.info/termList/RDACarrierEU"/>
      <reg:status rdf:resource="http://metadataregistry.org/uri/RegStatus/1001"/>
      <reg:identifier rdf:resource="http://metadataregistry.org/concepts/8634"/>
      <skos:prefLabel xml:lang="en">flash card</skos:prefLabel>
      <skos:altLabel xml:lang="en">electronic flash card</skos:altLabel>
      <rdakit:toolkitLabel xml:lang="en">flash card</rdakit:toolkitLabel>
      <skos:definition xml:lang="en">A unit of extent consisting of a card, or digital representation of a card, carrying words, numerals, pictures, etc., designed for rapid display as an aid to learning.</skos:definition>
      <rdakit:toolkitDefinition xml:lang="en">A unit of extent consisting of a card, or digital representation of a card, carrying words, numerals, pictures, etc., designed for rapid display as an aid to learning.</rdakit:toolkitDefinition>
      <skos:scopeNote xml:lang="en">This term applies to still images.</skos:scopeNote>
      <skos:prefLabel xml:lang="ca">fitxa de pregunta ràpida</skos:prefLabel>
      <rdakit:toolkitLabel xml:lang="ca">fitxa de pregunta ràpida</rdakit:toolkitLabel>
      <skos:definition xml:lang="ca">Unitat d’extensió que consisteix en una fitxa, o en una representació digital d’una fitxa, que porta paraules, xifres, imatges, etc., concebuda per a una visualització ràpida com una ajuda a l’aprenentatge.</skos:definition>
      <rdakit:toolkitDefinition xml:lang="ca">Unitat d’extensió que consisteix en una fitxa, o en una representació digital d’una fitxa, que porta paraules, xifres, imatges, etc., concebuda per a una visualització ràpida com una ajuda a l’aprenentatge.</rdakit:toolkitDefinition>
      <skos:scopeNote xml:lang="ca">Aquest terme s'aplica a imatges fixes.</skos:scopeNote>
      <skos:prefLabel xml:lang="vi">quân bài nháy</skos:prefLabel>
      <skos:altLabel xml:lang="vi">quân bài nháy điện tử</skos:altLabel>
      <rdakit:toolkitLabel xml:lang="vi">quân bài nháy</rdakit:toolkitLabel>
      <skos:definition xml:lang="vi">Đơn vị của quy mô bao gồm Quân bài hoặc vật liệu cản quang khác có in từ, chữ số, hoặc ảnh và được thiết kế để hiện hình nhanh khi trợ giúp học tập.</skos:definition>
      <rdakit:toolkitDefinition xml:lang="vi">Đơn vị của quy mô bao gồm Quân bài hoặc vật liệu cản quang khác có in từ, chữ số, hoặc ảnh và được thiết kế để hiện hình nhanh khi trợ giúp học tập.</rdakit:toolkitDefinition>
      <skos:scopeNote xml:lang="vi">Thuật ngữ này áp dụng cho hình ảnh tĩnh.</skos:scopeNote>
      <skos:prefLabel xml:lang="de">Lernkarte</skos:prefLabel>
      <rdakit:toolkitLabel xml:lang="de">Lernkarte</rdakit:toolkitLabel>
      <skos:definition xml:lang="de">Eine Einheit für den Umfang, bestehend aus einer Karte (oder der digitalen Repräsentation einer Karte), die Wörter, Zahlen, Bilder usw. enthält und für eine schnelle Anzeige als Lernhilfe konzipiert ist.</skos:definition>
      <rdakit:toolkitDefinition xml:lang="de">Eine Einheit für den Umfang, bestehend aus einer Karte (oder der digitalen Repräsentation einer Karte), die Wörter, Zahlen, Bilder usw. enthält und für eine schnelle Anzeige als Lernhilfe konzipiert ist.</rdakit:toolkitDefinition>
      <skos:scopeNote xml:lang="de">Dieser Terminus trifft auf unbewegten Bilder zu.</skos:scopeNote>
      <skos:prefLabel xml:lang="fi">opetuskortti</skos:prefLabel>
      <rdakit:toolkitLabel xml:lang="fi">opetuskortti</rdakit:toolkitLabel>
      <skos:definition xml:lang="fi">Laajuuden yksikkö, kuvakortti (fyysinen tai digitaalinen), joka sisältää sanoja, numeroita, kuvia jne., suunniteltu näytettäväksi nopeasti opetuksen apuvälineinä.</skos:definition>
      <rdakit:toolkitDefinition xml:lang="fi">Laajuuden yksikkö, kuvakortti (fyysinen tai digitaalinen), joka sisältää sanoja, numeroita, kuvia jne., suunniteltu näytettäväksi nopeasti opetuksen apuvälineinä.</rdakit:toolkitDefinition>
      <skos:scopeNote xml:lang="fi">Termi koskee stillkuvia.</skos:scopeNote>
      <skos:altLabel xml:lang="da">flashcard</skos:altLabel>
      <rdakit:toolkitLabel xml:lang="da">flashcard</rdakit:toolkitLabel>
      <skos:definition xml:lang="da">Enhed, der består af et kort, eller en digital gengivelse af et kort, med ord, tal, billeder etc., beregnet til hurtig fremvisning som et læringshjælpemiddel.</skos:definition>
      <rdakit:toolkitDefinition xml:lang="da">Enhed, der består af et kort, eller en digital gengivelse af et kort, med ord, tal, billeder etc., beregnet til hurtig fremvisning som et læringshjælpemiddel.</rdakit:toolkitDefinition>
      <skos:scopeNote xml:lang="da">Denne term anvendes til faste billeder.</skos:scopeNote>
      <skos:prefLabel xml:lang="fr">carte éclair</skos:prefLabel>
      <skos:altLabel xml:lang="fr">carte éclair électronique</skos:altLabel>
      <rdakit:toolkitLabel xml:lang="fr">carte éclair</rdakit:toolkitLabel>
      <skos:definition xml:lang="fr">Unité d’importance matérielle qui consiste en une carte, ou en une représentation numérique d’une carte, sur laquelle figurent des mots, des chiffres ou des images, etc. et conçue pour un affichage rapide comme moyen d’apprentissage.</skos:definition>
      <rdakit:toolkitDefinition xml:lang="fr">Unité d’importance matérielle qui consiste en une carte, ou en une représentation numérique d’une carte, sur laquelle figurent des mots, des chiffres ou des images, etc. et conçue pour un affichage rapide comme moyen d’apprentissage.</rdakit:toolkitDefinition>
      <skos:scopeNote xml:lang="fr">Ce terme s’applique aux ressources cartographiques.</skos:scopeNote>
      <skos:prefLabel xml:lang="no">billed-/ord-/symbolkort</skos:prefLabel>
      <skos:altLabel xml:lang="no">elektronisk billed-/ord-/symbolkort</skos:altLabel>
      <rdakit:toolkitLabel xml:lang="no">billed-/ord-/symbolkort</rdakit:toolkitLabel>
      <skos:definition xml:lang="no">En omfangsenhet som består av et kort (eller en digital framstilling av et kort) der det er gjengitt ord, tall eller bilder som i læreøyemed bare skal vises et kort øyeblikk.</skos:definition>
      <rdakit:toolkitDefinition xml:lang="no">En omfangsenhet som består av et kort (eller en digital framstilling av et kort) der det er gjengitt ord, tall eller bilder som i læreøyemed bare skal vises et kort øyeblikk.</rdakit:toolkitDefinition>
      <skos:scopeNote xml:lang="no">Dette begrepet gjelder stillbilder.</skos:scopeNote>
    </skos:Concept>
<!-- Concept: folded sheet  -->
    <skos:Concept rdf:about="http://rdaregistry.info/termList/RDACarrierEU/1013" xml:lang="en">
      <skos:inScheme rdf:resource="http://rdaregistry.info/termList/RDACarrierEU"/>
      <reg:status rdf:resource="http://metadataregistry.org/uri/RegStatus/1001"/>
      <reg:identifier rdf:resource="http://metadataregistry.org/concepts/8635"/>
      <skos:prefLabel xml:lang="en">folded sheet</skos:prefLabel>
      <rdakit:toolkitLabel xml:lang="en">folded sheet</rdakit:toolkitLabel>
      <skos:definition xml:lang="en">A unit of extent consisting of a sheet designed to be read in pages when folded.</skos:definition>
      <rdakit:toolkitDefinition xml:lang="en">A unit of extent consisting of a sheet designed to be read in pages when folded.</rdakit:toolkitDefinition>
      <skos:prefLabel xml:lang="ca">full plegat</skos:prefLabel>
      <rdakit:toolkitLabel xml:lang="ca">full plegat</rdakit:toolkitLabel>
      <skos:definition xml:lang="ca">Unitat d'extensió consistent en un full concebut per ser llegit en pàgines quan està plegat.</skos:definition>
      <rdakit:toolkitDefinition xml:lang="ca">Unitat d'extensió consistent en un full concebut per ser llegit en pàgines quan està plegat.</rdakit:toolkitDefinition>
      <skos:prefLabel xml:lang="vi">tờ gấp</skos:prefLabel>
      <rdakit:toolkitLabel xml:lang="vi">tờ gấp</rdakit:toolkitLabel>
      <skos:definition xml:lang="vi">Đơn vị của quy mô gồm có tờ được thiết kế để đọc trong trang khi gấp.</skos:definition>
      <rdakit:toolkitDefinition xml:lang="vi">Đơn vị của quy mô gồm có tờ được thiết kế để đọc trong trang khi gấp.</rdakit:toolkitDefinition>
      <skos:prefLabel xml:lang="de">Gefaltetes Blatt</skos:prefLabel>
      <rdakit:toolkitLabel xml:lang="de">Gefaltetes Blatt</rdakit:toolkitLabel>
      <skos:definition xml:lang="de">Eine Einheit für den Umfang, bestehend aus einem Blatt, der so angeordnet ist, dass er nach dem Falten die richtige Seitenreihenfolge hat.</skos:definition>
      <rdakit:toolkitDefinition xml:lang="de">Eine Einheit für den Umfang, bestehend aus einem Blatt, der so angeordnet ist, dass er nach dem Falten die richtige Seitenreihenfolge hat.</rdakit:toolkitDefinition>
      <skos:prefLabel xml:lang="fi">taitettu lehti</skos:prefLabel>
      <rdakit:toolkitLabel xml:lang="fi">taitettu lehti</rdakit:toolkitLabel>
      <skos:definition xml:lang="fi">Laajuuden yksikkö joka koostuu arkista, jota on tarkoitus lukea sivuiksi taiteltuna.</skos:definition>
      <rdakit:toolkitDefinition xml:lang="fi">Laajuuden yksikkö joka koostuu arkista, jota on tarkoitus lukea sivuiksi taiteltuna.</rdakit:toolkitDefinition>
      <skos:altLabel xml:lang="da">foldet ark</skos:altLabel>
      <rdakit:toolkitLabel xml:lang="da">foldet ark</rdakit:toolkitLabel>
      <skos:definition xml:lang="da">Enhed, der består af et ark skabt til at blive læst som sider, når det er foldet.</skos:definition>
      <rdakit:toolkitDefinition xml:lang="da">Enhed, der består af et ark skabt til at blive læst som sider, når det er foldet.</rdakit:toolkitDefinition>
      <skos:prefLabel xml:lang="fr">feuille pliée</skos:prefLabel>
      <rdakit:toolkitLabel xml:lang="fr">feuille pliée</rdakit:toolkitLabel>
      <skos:definition xml:lang="fr">Unité d’importance matérielle qui consiste en une feuille conçue pour former des pages lorsqu’elle est pliée.</skos:definition>
      <rdakit:toolkitDefinition xml:lang="fr">Unité d’importance matérielle qui consiste en une feuille conçue pour former des pages lorsqu’elle est pliée.</rdakit:toolkitDefinition>
      <skos:scopeNote xml:lang="fr">Ce terme s’applique aux formes tridimensionnelles.</skos:scopeNote>
      <skos:prefLabel xml:lang="no">foldet ark</skos:prefLabel>
      <rdakit:toolkitLabel xml:lang="no">foldet ark</rdakit:toolkitLabel>
      <skos:definition xml:lang="no">En omfangsenhet som består av et ark laget for å leses som sider når det er brettet.</skos:definition>
      <rdakit:toolkitDefinition xml:lang="no">En omfangsenhet som består av et ark laget for å leses som sider når det er brettet.</rdakit:toolkitDefinition>
    </skos:Concept>
<!-- Concept: game  -->
    <skos:Concept rdf:about="http://rdaregistry.info/termList/RDACarrierEU/1014" xml:lang="en">
      <skos:inScheme rdf:resource="http://rdaregistry.info/termList/RDACarrierEU"/>
      <reg:status rdf:resource="http://metadataregistry.org/uri/RegStatus/1001"/>
      <reg:identifier rdf:resource="http://metadataregistry.org/concepts/8636"/>
      <skos:prefLabel xml:lang="en">game</skos:prefLabel>
      <rdakit:toolkitLabel xml:lang="en">game</rdakit:toolkitLabel>
      <skos:definition xml:lang="en">A unit of extent consisting of a set of objects designed for manipulation according to prescribed or implicit rules for education, entertainment, or therapy.</skos:definition>
      <rdakit:toolkitDefinition xml:lang="en">A unit of extent consisting of a set of objects designed for manipulation according to prescribed or implicit rules for education, entertainment, or therapy.</rdakit:toolkitDefinition>
      <skos:scopeNote xml:lang="en">This term applies to three-dimensional forms.</skos:scopeNote>
	    <skos:related rdf:resource="http://rdaregistry.info/termList/RDACarrierEU/1039"/>
      <skos:prefLabel xml:lang="ca">joc</skos:prefLabel>
      <rdakit:toolkitLabel xml:lang="ca">joc</rdakit:toolkitLabel>
      <skos:definition xml:lang="ca">Unitat d’extensió que consisteix en un conjunt d’objectes dissenyat per ser manipulat d’acord amb unes regles prescrites o implícites amb una finalitat educativa, d’entreteniment o de teràpia.</skos:definition>
      <rdakit:toolkitDefinition xml:lang="ca">Unitat d’extensió que consisteix en un conjunt d’objectes dissenyat per ser manipulat d’acord amb unes regles prescrites o implícites amb una finalitat educativa, d’entreteniment o de teràpia.</rdakit:toolkitDefinition>
      <skos:scopeNote xml:lang="ca">Aquest terme s'aplica a formes tridimensionals.</skos:scopeNote>
      <skos:prefLabel xml:lang="vi">trò chơi</skos:prefLabel>
      <rdakit:toolkitLabel xml:lang="vi">trò chơi</rdakit:toolkitLabel>
      <skos:definition xml:lang="vi">Đơn vị của quy mô gồm có bộ các vật thể được thiết kế để thao tác theo luật chơi hoặc ngầm hiểu cho giáo dục, giải trí, hoặc trị liệu.</skos:definition>
      <rdakit:toolkitDefinition xml:lang="vi">Đơn vị của quy mô gồm có bộ các vật thể được thiết kế để thao tác theo luật chơi hoặc ngầm hiểu cho giáo dục, giải trí, hoặc trị liệu.</rdakit:toolkitDefinition>
      <skos:scopeNote xml:lang="vi">Thuật ngữ này áp dụng cho hình thái ba chiều.</skos:scopeNote>
      <skos:prefLabel xml:lang="de">Spiel</skos:prefLabel>
      <rdakit:toolkitLabel xml:lang="de">Spiel</rdakit:toolkitLabel>
      <skos:definition xml:lang="de">Eine Einheit für den Umfang, bestehend aus einem Satz von Gegenständen, der für die Bedienung nach vorgeschriebenen oder impliziten Regeln für Unterricht, Unterhaltung oder Therapie konzipiert ist.</skos:definition>
      <rdakit:toolkitDefinition xml:lang="de">Eine Einheit für den Umfang, bestehend aus einem Satz von Gegenständen, der für die Bedienung nach vorgeschriebenen oder impliziten Regeln für Unterricht, Unterhaltung oder Therapie konzipiert ist.</rdakit:toolkitDefinition>
      <skos:scopeNote xml:lang="de">Dieser Terminus trifft auf dreidimensionale Formen zu.</skos:scopeNote>
      <skos:prefLabel xml:lang="fi">peli</skos:prefLabel>
      <rdakit:toolkitLabel xml:lang="fi">peli</rdakit:toolkitLabel>
      <skos:definition xml:lang="fi">Laajuuden yksikkö, kolmiulotteisia objekteja sisältävä kokonaisuus, jota on tarkoitettu käytettäväksi sovittujen sääntöjen mukaisesti leikeissä opetuksessa, huviksi tai terapiassa.</skos:definition>
      <rdakit:toolkitDefinition xml:lang="fi">Laajuuden yksikkö, kolmiulotteisia objekteja sisältävä kokonaisuus, jota on tarkoitettu käytettäväksi sovittujen sääntöjen mukaisesti leikeissä opetuksessa, huviksi tai terapiassa.</rdakit:toolkitDefinition>
      <skos:scopeNote xml:lang="fi">Termi koskee kolmiulotteisia muotoja.</skos:scopeNote>
      <skos:altLabel xml:lang="da">spil</skos:altLabel>
      <rdakit:toolkitLabel xml:lang="da">spil</rdakit:toolkitLabel>
      <skos:definition xml:lang="da">Enhed, der består af genstande, beregnet til at kunne manipuleres iht. foreskrevne eller implicitte regler, til undervisnings-, underholdnings- eller terapibrug.</skos:definition>
      <rdakit:toolkitDefinition xml:lang="da">Enhed, der består af genstande, beregnet til at kunne manipuleres iht. foreskrevne eller implicitte regler, til undervisnings-, underholdnings- eller terapibrug.</rdakit:toolkitDefinition>
      <skos:scopeNote xml:lang="da">Denne term anvendes for tredimensionelle former.</skos:scopeNote>
      <skos:prefLabel xml:lang="fr">jeu</skos:prefLabel>
      <rdakit:toolkitLabel xml:lang="fr">jeu</rdakit:toolkitLabel>
      <skos:definition xml:lang="fr">Unité d’importance matérielle qui consiste en un ensemble d’objets conçus pour être manipulés selon des règles prescrites ou implicites à des fins éducatives, de divertissement ou thérapeutiques.</skos:definition>
      <rdakit:toolkitDefinition xml:lang="fr">Unité d’importance matérielle qui consiste en un ensemble d’objets conçus pour être manipulés selon des règles prescrites ou implicites à des fins éducatives, de divertissement ou thérapeutiques.</rdakit:toolkitDefinition>
      <skos:scopeNote xml:lang="fr">Ce terme s’applique aux ressources cartographiques.</skos:scopeNote>
      <skos:prefLabel xml:lang="no">spill</skos:prefLabel>
      <rdakit:toolkitLabel xml:lang="no">spill</rdakit:toolkitLabel>
      <skos:definition xml:lang="no">En omfangsenhet som består av et sett objekter som håndteres ifølge fastsatte regler. Brukes innen opplæring, underholdning eller terapi.</skos:definition>
      <rdakit:toolkitDefinition xml:lang="no">En omfangsenhet som består av et sett objekter som håndteres ifølge fastsatte regler. Brukes innen opplæring, underholdning eller terapi.</rdakit:toolkitDefinition>
      <skos:scopeNote xml:lang="no">Dette begrepet gjelder tredimensjonale former.</skos:scopeNote>
    </skos:Concept>
<!-- Concept: globe  -->
    <skos:Concept rdf:about="http://rdaregistry.info/termList/RDACarrierEU/1015" xml:lang="en">
      <skos:inScheme rdf:resource="http://rdaregistry.info/termList/RDACarrierEU"/>
      <reg:status rdf:resource="http://metadataregistry.org/uri/RegStatus/1001"/>
      <reg:identifier rdf:resource="http://metadataregistry.org/concepts/8637"/>
      <skos:prefLabel xml:lang="en">globe</skos:prefLabel>
      <rdakit:toolkitLabel xml:lang="en">globe</rdakit:toolkitLabel>
      <skos:definition xml:lang="en">A unit of extent that is a depiction of the Earth or other celestial body, real or imaginary, on the surface of a sphere.</skos:definition>
      <rdakit:toolkitDefinition xml:lang="en">A unit of extent that is a depiction of the Earth or other celestial body, real or imaginary, on the surface of a sphere.</rdakit:toolkitDefinition>
      <skos:scopeNote xml:lang="en">This term applies to cartographic resources.</skos:scopeNote>
      <skos:prefLabel xml:lang="ca">globus</skos:prefLabel>
      <rdakit:toolkitLabel xml:lang="ca">globus</rdakit:toolkitLabel>
      <skos:definition xml:lang="ca">Unitat d’extensió que és una representació de la Terra o d’un altre cos celeste, real o imaginari, sobre la superfície d’una esfera.</skos:definition>
      <rdakit:toolkitDefinition xml:lang="ca">Unitat d’extensió que és una representació de la Terra o d’un altre cos celeste, real o imaginari, sobre la superfície d’una esfera.</rdakit:toolkitDefinition>
      <skos:scopeNote xml:lang="ca">Aquest terme s'aplica a recursos cartogràfics.</skos:scopeNote>
      <skos:prefLabel xml:lang="vi">quả địa cầu</skos:prefLabel>
      <rdakit:toolkitLabel xml:lang="vi">quả địa cầu</rdakit:toolkitLabel>
      <skos:definition xml:lang="vi">Đơn vị của quy mô là mô tả của Trái đất hoặc vật thể vũ trụ khác, thực hoặc tưởng tượng, trên bề mặt của hình cầu.</skos:definition>
      <rdakit:toolkitDefinition xml:lang="vi">Đơn vị của quy mô là mô tả của Trái đất hoặc vật thể vũ trụ khác, thực hoặc tưởng tượng, trên bề mặt của hình cầu.</rdakit:toolkitDefinition>
      <skos:scopeNote xml:lang="vi">Thuật ngữ này áp dụng cho tài nguyên bản đồ.</skos:scopeNote>
      <skos:prefLabel xml:lang="de">Globus</skos:prefLabel>
      <rdakit:toolkitLabel xml:lang="de">Globus</rdakit:toolkitLabel>
      <skos:definition xml:lang="de">Eine Einheit für den Umfang, der eine Darstellung der Erde oder eines anderen Himmelskörpers (real oder imaginär) auf der Oberfläche einer Kugel ist.</skos:definition>
      <rdakit:toolkitDefinition xml:lang="de">Eine Einheit für den Umfang, der eine Darstellung der Erde oder eines anderen Himmelskörpers (real oder imaginär) auf der Oberfläche einer Kugel ist.</rdakit:toolkitDefinition>
      <skos:scopeNote xml:lang="de">Dieser Terminus trifft auf kartografische Ressourcen zu.</skos:scopeNote>
      <skos:prefLabel xml:lang="fi">karttapallo</skos:prefLabel>
      <rdakit:toolkitLabel xml:lang="fi">karttapallo</rdakit:toolkitLabel>
      <skos:definition xml:lang="fi">Laajuuden yksikkö, kartta-aineisto, joka kuvaa maapalloa tai muita taivaankappaleita (oikeita tai kuvitteellisia) pallon pinnalla.</skos:definition>
      <rdakit:toolkitDefinition xml:lang="fi">Laajuuden yksikkö, kartta-aineisto, joka kuvaa maapalloa tai muita taivaankappaleita (oikeita tai kuvitteellisia) pallon pinnalla.</rdakit:toolkitDefinition>
      <skos:scopeNote xml:lang="fi">Termi koskee kartografisia aineistoja.</skos:scopeNote>
      <skos:altLabel xml:lang="da">globus</skos:altLabel>
      <rdakit:toolkitLabel xml:lang="da">globus</rdakit:toolkitLabel>
      <skos:definition xml:lang="da">Enhed, der skildrer jorden eller et andet himmellegeme (ægte eller opdigtet) på en kugleformet overflade.</skos:definition>
      <rdakit:toolkitDefinition xml:lang="da">Enhed, der skildrer jorden eller et andet himmellegeme (ægte eller opdigtet) på en kugleformet overflade.</rdakit:toolkitDefinition>
      <skos:scopeNote xml:lang="da">Denne term anvendes for kartografiske ressourcer.</skos:scopeNote>
      <skos:prefLabel xml:lang="fr">globe</skos:prefLabel>
      <rdakit:toolkitLabel xml:lang="fr">globe</rdakit:toolkitLabel>
      <skos:definition xml:lang="fr">Unité d’importance matérielle qui consiste en une représentation de la Terre ou d’un autre corps céleste, réel ou imaginaire, sur la surface d’une sphère.</skos:definition>
      <rdakit:toolkitDefinition xml:lang="fr">Unité d’importance matérielle qui consiste en une représentation de la Terre ou d’un autre corps céleste, réel ou imaginaire, sur la surface d’une sphère.</rdakit:toolkitDefinition>
      <skos:scopeNote xml:lang="fr">Ce terme s’applique aux formes tridimensionnelles.</skos:scopeNote>
      <skos:prefLabel xml:lang="no">globus</skos:prefLabel>
      <rdakit:toolkitLabel xml:lang="no">globus</rdakit:toolkitLabel>
      <skos:definition xml:lang="no">En omfangsenhet som er en avbildning av Jorden eller andre himmellegemer (virkelige eller imaginære) på overflaten av en kule.</skos:definition>
      <rdakit:toolkitDefinition xml:lang="no">En omfangsenhet som er en avbildning av Jorden eller andre himmellegemer (virkelige eller imaginære) på overflaten av en kule.</rdakit:toolkitDefinition>
      <skos:scopeNote xml:lang="no">Dette begrepet gjelder kartografiske ressurser.</skos:scopeNote>
    </skos:Concept>
<!-- Concept: icon  -->
    <skos:Concept rdf:about="http://rdaregistry.info/termList/RDACarrierEU/1016" xml:lang="en">
      <skos:inScheme rdf:resource="http://rdaregistry.info/termList/RDACarrierEU"/>
      <reg:status rdf:resource="http://metadataregistry.org/uri/RegStatus/1001"/>
      <reg:identifier rdf:resource="http://metadataregistry.org/concepts/8638"/>
      <skos:prefLabel xml:lang="en">icon</skos:prefLabel>
      <rdakit:toolkitLabel xml:lang="en">icon</rdakit:toolkitLabel>
      <skos:definition xml:lang="en">A unit of extent consisting of an image that portrays a sacred entity and that is itself regarded as sacred.</skos:definition>
      <rdakit:toolkitDefinition xml:lang="en">A unit of extent consisting of an image that portrays a sacred entity and that is itself regarded as sacred.</rdakit:toolkitDefinition>
      <skos:scopeNote xml:lang="en">This term applies to still images. Most commonly it comprises tempera on panel, but it may be in any two-dimensional or relief medium, including fresco.</skos:scopeNote>
      <skos:prefLabel xml:lang="ca">icona</skos:prefLabel>
      <rdakit:toolkitLabel xml:lang="ca">icona</rdakit:toolkitLabel>
      <skos:definition xml:lang="ca">Unitat d’extensió que consisteix en una imatge que representa una entitat sagrada i que ella mateixa és considerada sagrada.</skos:definition>
      <rdakit:toolkitDefinition xml:lang="ca">Unitat d’extensió que consisteix en una imatge que representa una entitat sagrada i que ella mateixa és considerada sagrada.</rdakit:toolkitDefinition>
      <skos:scopeNote xml:lang="ca">Aquest terme s'aplica a imatges fixes. Habitualment és una pintura al tremp sobre un plafó, però pot estar en qualsevol suport bidimensional o en relleu, inclòs un fresc.</skos:scopeNote>
      <skos:prefLabel xml:lang="vi">hình tượng</skos:prefLabel>
      <rdakit:toolkitLabel xml:lang="vi">hình tượng</rdakit:toolkitLabel>
      <skos:definition xml:lang="vi">Đơn vị của quy mô bao gồm hình ảnh mô tả thực thể linh thiêng và tự nó được xem là linh thiêng.</skos:definition>
      <rdakit:toolkitDefinition xml:lang="vi">Đơn vị của quy mô bao gồm hình ảnh mô tả thực thể linh thiêng và tự nó được xem là linh thiêng.</rdakit:toolkitDefinition>
      <skos:scopeNote xml:lang="vi">Thuật ngữ này áp dụng cho hình ảnh tĩnh. Thông thường nhất nó bao gồm màu keo trên ô vải nhưng cũng có thể trong phương tiện hai chiều hoặc vật thay thế khác bao gồm cả bích hoạ.</skos:scopeNote>
      <skos:prefLabel xml:lang="de">Ikone</skos:prefLabel>
      <rdakit:toolkitLabel xml:lang="de">Ikone</rdakit:toolkitLabel>
      <skos:definition xml:lang="de">Eine Einheit für den Umfang, bestehend aus einem Bild, das eine heilige Entität porträtiert, und das selbst als heilig angesehen wird.</skos:definition>
      <rdakit:toolkitDefinition xml:lang="de">Eine Einheit für den Umfang, bestehend aus einem Bild, das eine heilige Entität porträtiert, und das selbst als heilig angesehen wird.</rdakit:toolkitDefinition>
      <skos:scopeNote xml:lang="de">Dieser Terminus trifft auf unbewegte Bilde zu. Besteht zumeist aus Temperafarbe auf einem Brett, aber sie kann auch in einem zweidimensionalen oder reliefartigen Medium einschließlich Fresko sein.</skos:scopeNote>
      <skos:prefLabel xml:lang="fi">ikoni</skos:prefLabel>
      <rdakit:toolkitLabel xml:lang="fi">ikoni</rdakit:toolkitLabel>
      <skos:definition xml:lang="fi">Laajuuden yksikkö, kuva joka esittää pyhää entiteettiä ja jota itseään pidetään pyhänä.</skos:definition>
      <rdakit:toolkitDefinition xml:lang="fi">Laajuuden yksikkö, kuva joka esittää pyhää entiteettiä ja jota itseään pidetään pyhänä.</rdakit:toolkitDefinition>
      <skos:scopeNote xml:lang="fi">Termi koskee stillkuvia. Yleensä temperamaalaus puupohjalle, mutta voi olla missä tahansa kaksiulotteisessa muodossa tai reliefi, myös fresko.</skos:scopeNote>
      <skos:altLabel xml:lang="da">ikon</skos:altLabel>
      <rdakit:toolkitLabel xml:lang="da">ikon</rdakit:toolkitLabel>
      <skos:definition xml:lang="da">Enhed, der består af et billede, der skildrer en hellig entitet, og som i sig selv betragtes som hellig.</skos:definition>
      <rdakit:toolkitDefinition xml:lang="da">Enhed, der består af et billede, der skildrer en hellig entitet, og som i sig selv betragtes som hellig.</rdakit:toolkitDefinition>
      <skos:scopeNote xml:lang="da">Denne term anvendes for faste billeder. Består normalt af temperafarve på en plade, men kan være i ethvert todimensionelt eller reliefmedium, inkl. fresko.</skos:scopeNote>
      <skos:prefLabel xml:lang="fr">icône</skos:prefLabel>
      <rdakit:toolkitLabel xml:lang="fr">icône</rdakit:toolkitLabel>
      <skos:definition xml:lang="fr">Unité d’importance matérielle qui consiste en une image représentant une entité sacrée et qui est elle-même considérée comme sacrée.</skos:definition>
      <rdakit:toolkitDefinition xml:lang="fr">Unité d’importance matérielle qui consiste en une image représentant une entité sacrée et qui est elle-même considérée comme sacrée.</rdakit:toolkitDefinition>
      <skos:prefLabel xml:lang="no">ikon</skos:prefLabel>
      <rdakit:toolkitLabel xml:lang="no">ikon</rdakit:toolkitLabel>
      <skos:definition xml:lang="no">En omfangsenhet som består av et bilde som framstiller en hellig enhet og som i seg selv anses som hellig.</skos:definition>
      <rdakit:toolkitDefinition xml:lang="no">En omfangsenhet som består av et bilde som framstiller en hellig enhet og som i seg selv anses som hellig.</rdakit:toolkitDefinition>
      <skos:scopeNote xml:lang="no">Dette begrepet gjelder stillbilder. Vanligvis temperamaleri, men kan også være i et todimensjonalt medium eller relieff. Inkluderer også fresko.</skos:scopeNote>
    </skos:Concept>
<!-- Concept: jigsaw puzzle  -->
    <skos:Concept rdf:about="http://rdaregistry.info/termList/RDACarrierEU/1017" xml:lang="en">
      <skos:inScheme rdf:resource="http://rdaregistry.info/termList/RDACarrierEU"/>
      <reg:status rdf:resource="http://metadataregistry.org/uri/RegStatus/1001"/>
      <reg:identifier rdf:resource="http://metadataregistry.org/concepts/8639"/>
      <skos:prefLabel xml:lang="en">jigsaw puzzle</skos:prefLabel>
      <rdakit:toolkitLabel xml:lang="en">jigsaw puzzle</rdakit:toolkitLabel>
      <skos:definition xml:lang="en">A unit of extent consisting of a picture usually on pasteboard or wood, which has been cut into interlocking shapes intended to be re-assembled.</skos:definition>
      <rdakit:toolkitDefinition xml:lang="en">A unit of extent consisting of a picture usually on pasteboard or wood, which has been cut into interlocking shapes intended to be re-assembled.</rdakit:toolkitDefinition>
      <skos:scopeNote xml:lang="en">This term applies to three-dimensional forms.</skos:scopeNote>
      <skos:prefLabel xml:lang="ca">trencaclosques</skos:prefLabel>
      <rdakit:toolkitLabel xml:lang="ca">trencaclosques</rdakit:toolkitLabel>
      <skos:definition xml:lang="ca">Unitat d’extensió que consisteix en una imatge, normalment sobre cartró o fusta, que ha estat tallada en formes entrellaçades concebudes perquè es rejuntin.</skos:definition>
      <rdakit:toolkitDefinition xml:lang="ca">Unitat d’extensió que consisteix en una imatge, normalment sobre cartró o fusta, que ha estat tallada en formes entrellaçades concebudes perquè es rejuntin.</rdakit:toolkitDefinition>
      <skos:scopeNote xml:lang="ca">Aquest terme s'aplica a formes tridimensionals.</skos:scopeNote>
      <skos:prefLabel xml:lang="vi">trò chơi lắp hình</skos:prefLabel>
      <rdakit:toolkitLabel xml:lang="vi">trò chơi lắp hình</rdakit:toolkitLabel>
      <skos:definition xml:lang="vi">Đơn vị của quy mô gồm có một bức hoạ thường trên bìa cứng hoặc gỗ đã được cắt thành các hình dành cho lắp ráp lại.</skos:definition>
      <rdakit:toolkitDefinition xml:lang="vi">Đơn vị của quy mô gồm có một bức hoạ thường trên bìa cứng hoặc gỗ đã được cắt thành các hình dành cho lắp ráp lại.</rdakit:toolkitDefinition>
      <skos:scopeNote xml:lang="vi">Thuật ngữ này áp dụng cho hình thái ba chiều.</skos:scopeNote>
      <skos:prefLabel xml:lang="de">Puzzle</skos:prefLabel>
      <rdakit:toolkitLabel xml:lang="de">Puzzle</rdakit:toolkitLabel>
      <skos:definition xml:lang="de">Eine Einheit für den Umfang, bestehend aus einem Bild, normalerweise auf Karton oder Holz, das in ineinander greifende Formen geschnitten wurde und dazu konzipiert ist, wieder zusammengefügt zu werden.</skos:definition>
      <rdakit:toolkitDefinition xml:lang="de">Eine Einheit für den Umfang, bestehend aus einem Bild, normalerweise auf Karton oder Holz, das in ineinander greifende Formen geschnitten wurde und dazu konzipiert ist, wieder zusammengefügt zu werden.</rdakit:toolkitDefinition>
      <skos:scopeNote xml:lang="de">Dieser Terminus trifft auf dreidimensionale Formen zu.</skos:scopeNote>
      <skos:prefLabel xml:lang="fi">palapeli</skos:prefLabel>
      <rdakit:toolkitLabel xml:lang="fi">palapeli</rdakit:toolkitLabel>
      <skos:definition xml:lang="fi">Laajuuden yksikkö, yleensä pahvista tai puusta erimuotoisiksi paloiksi leikattuja kolmiulotteisia muotoja, joista muodostuu koottava kuva.</skos:definition>
      <rdakit:toolkitDefinition xml:lang="fi">Laajuuden yksikkö, yleensä pahvista tai puusta erimuotoisiksi paloiksi leikattuja kolmiulotteisia muotoja, joista muodostuu koottava kuva.</rdakit:toolkitDefinition>
      <skos:scopeNote xml:lang="fi">Termi koskee kolmiulotteisia muotoja.</skos:scopeNote>
      <skos:altLabel xml:lang="da">puslespil</skos:altLabel>
      <rdakit:toolkitLabel xml:lang="da">puslespil</rdakit:toolkitLabel>
      <skos:definition xml:lang="da">Enhed, der består af et billede, normalt på pap eller træ, der er skåret ud i mindre stykker, der griber ind i hinanden, når de samles igen.</skos:definition>
      <rdakit:toolkitDefinition xml:lang="da">Enhed, der består af et billede, normalt på pap eller træ, der er skåret ud i mindre stykker, der griber ind i hinanden, når de samles igen.</rdakit:toolkitDefinition>
      <skos:scopeNote xml:lang="da">Denne term anvendes for tredimensionelle former.</skos:scopeNote>
      <skos:prefLabel xml:lang="fr">puzzle</skos:prefLabel>
      <rdakit:toolkitLabel xml:lang="fr">puzzle</rdakit:toolkitLabel>
      <skos:definition xml:lang="fr">Unité d’importance matérielle qui consiste en une image, généralement sur carton ou sur bois, qui a été taillée en des formes qui s’emboîtent les unes dans les autres et qui sont destinées à être réassemblées.</skos:definition>
      <rdakit:toolkitDefinition xml:lang="fr">Unité d’importance matérielle qui consiste en une image, généralement sur carton ou sur bois, qui a été taillée en des formes qui s’emboîtent les unes dans les autres et qui sont destinées à être réassemblées.</rdakit:toolkitDefinition>
      <skos:scopeNote xml:lang="fr">Ce terme s’applique aux images fixes.</skos:scopeNote>
      <skos:prefLabel xml:lang="no">puslespill</skos:prefLabel>
      <rdakit:toolkitLabel xml:lang="no">puslespill</rdakit:toolkitLabel>
      <skos:definition xml:lang="no">En omfangsenhet som består av et bilde, vanligvis på en plate av tre eller papp, kuttet opp i biter som passer sammen og er ment for å settes sammen igjen.</skos:definition>
      <rdakit:toolkitDefinition xml:lang="no">En omfangsenhet som består av et bilde, vanligvis på en plate av tre eller papp, kuttet opp i biter som passer sammen og er ment for å settes sammen igjen.</rdakit:toolkitDefinition>
      <skos:scopeNote xml:lang="no">Dette begrepet gjelder tredimensjonale former.</skos:scopeNote>
    </skos:Concept>
<!-- Concept: leaf  -->
    <skos:Concept rdf:about="http://rdaregistry.info/termList/RDACarrierEU/1018" xml:lang="en">
      <skos:inScheme rdf:resource="http://rdaregistry.info/termList/RDACarrierEU"/>
      <reg:status rdf:resource="http://metadataregistry.org/uri/RegStatus/1001"/>
      <reg:identifier rdf:resource="http://metadataregistry.org/concepts/8640"/>
      <skos:prefLabel xml:lang="en">leaf</skos:prefLabel>
      <rdakit:toolkitLabel xml:lang="en">leaf</rdakit:toolkitLabel>
      <skos:definition xml:lang="en">A unit of extent consisting of a single bound or fastened sheet as a subunit of a volume; each leaf consists of two pages, one on each side, either or both of which may be blank.</skos:definition>
      <rdakit:toolkitDefinition xml:lang="en">A unit of extent consisting of a single bound or fastened sheet as a subunit of a volume; each leaf consists of two pages, one on each side, either or both of which may be blank.</rdakit:toolkitDefinition>
      <skos:prefLabel xml:lang="ca">full</skos:prefLabel>
      <rdakit:toolkitLabel xml:lang="ca">full</rdakit:toolkitLabel>
      <skos:definition xml:lang="ca">Unitat d’extensió que consisteix en un sol full lligat o subjectat com una subunitat d’un volum; cada full consisteix en dues pàgines, una en cada cara, cada una de les quals pot estar en blanc.</skos:definition>
      <rdakit:toolkitDefinition xml:lang="ca">Unitat d’extensió que consisteix en un sol full lligat o subjectat com una subunitat d’un volum; cada full consisteix en dues pàgines, una en cada cara, cada una de les quals pot estar en blanc.</rdakit:toolkitDefinition>
      <skos:prefLabel xml:lang="vi">tờ</skos:prefLabel>
      <rdakit:toolkitLabel xml:lang="vi">tờ</rdakit:toolkitLabel>
      <skos:definition xml:lang="vi">Đơn vị của quy mô gồm có tờ đơn hoặc được đóng lại như là tiểu đơn vị của tập, mỗi tờ có hai trang, mỗi trang ở một mặt, một hoặc cả hai trang có thể để trống.</skos:definition>
      <rdakit:toolkitDefinition xml:lang="vi">Đơn vị của quy mô gồm có tờ đơn hoặc được đóng lại như là tiểu đơn vị của tập, mỗi tờ có hai trang, mỗi trang ở một mặt, một hoặc cả hai trang có thể để trống.</rdakit:toolkitDefinition>
      <skos:prefLabel xml:lang="de">Blatt</skos:prefLabel>
      <rdakit:toolkitLabel xml:lang="de">Blatt</rdakit:toolkitLabel>
      <skos:definition xml:lang="de">Eine Einheit für den Umfang, bestehend aus einem einzelnen gebundenen oder befestigten Bogen als Untereinheit eines Bandes. Jedes Blatt besteht aus zwei Seiten, auf jeder Seite eine, die auch leer sein können.</skos:definition>
      <rdakit:toolkitDefinition xml:lang="de">Eine Einheit für den Umfang, bestehend aus einem einzelnen gebundenen oder befestigten Bogen als Untereinheit eines Bandes. Jedes Blatt besteht aus zwei Seiten, auf jeder Seite eine, die auch leer sein können.</rdakit:toolkitDefinition>
      <skos:prefLabel xml:lang="fi">lehti</skos:prefLabel>
      <rdakit:toolkitLabel xml:lang="fi">lehti</rdakit:toolkitLabel>
      <skos:definition xml:lang="fi">Laajuuden yksikkö, yksittäinen arkki, joka muodostaa sidotun tai nidotun niteen alayksikön.</skos:definition>
      <rdakit:toolkitDefinition xml:lang="fi">Laajuuden yksikkö, yksittäinen arkki, joka muodostaa sidotun tai nidotun niteen alayksikön.</rdakit:toolkitDefinition>
      <skos:altLabel xml:lang="da">blad</skos:altLabel>
      <rdakit:toolkitLabel xml:lang="da">blad</rdakit:toolkitLabel>
      <skos:definition xml:lang="da">Enhed, der består af et enkelt indbundet eller fæstnet ark som underenhed til et bind; hvert blad består af to sider, en til højre og en til venstre, hvoraf en eller begge kan være tomme.</skos:definition>
      <rdakit:toolkitDefinition xml:lang="da">Enhed, der består af et enkelt indbundet eller fæstnet ark som underenhed til et bind; hvert blad består af to sider, en til højre og en til venstre, hvoraf en eller begge kan være tomme.</rdakit:toolkitDefinition>
      <skos:prefLabel xml:lang="fr">feuillet</skos:prefLabel>
      <rdakit:toolkitLabel xml:lang="fr">feuillet</rdakit:toolkitLabel>
      <skos:definition xml:lang="fr">Unité d’importance matérielle qui consiste en une seule feuille reliée ou attachée en tant que sous-unité d’un volume ; chaque feuillet comprend deux pages, une de chaque côté, dont l’une ou les deux peuvent être blanches.</skos:definition>
      <rdakit:toolkitDefinition xml:lang="fr">Unité d’importance matérielle qui consiste en une seule feuille reliée ou attachée en tant que sous-unité d’un volume ; chaque feuillet comprend deux pages, une de chaque côté, dont l’une ou les deux peuvent être blanches.</rdakit:toolkitDefinition>
      <skos:scopeNote xml:lang="fr">Ce terme s’applique aux formes tridimensionnelles.</skos:scopeNote>
      <skos:prefLabel xml:lang="no">blad</skos:prefLabel>
      <rdakit:toolkitLabel xml:lang="no">blad</rdakit:toolkitLabel>
      <skos:definition xml:lang="no">En omfangsenhet. Består av et enkelt eller festet ark som er en del av et bind. Hvert blad består av to sider, der den ene eller begge kan være blanke.</skos:definition>
      <rdakit:toolkitDefinition xml:lang="no">En omfangsenhet. Består av et enkelt eller festet ark som er en del av et bind. Hvert blad består av to sider, der den ene eller begge kan være blanke.</rdakit:toolkitDefinition>
    </skos:Concept>
<!-- Concept: map  -->
    <skos:Concept rdf:about="http://rdaregistry.info/termList/RDACarrierEU/1019" xml:lang="en">
      <skos:inScheme rdf:resource="http://rdaregistry.info/termList/RDACarrierEU"/>
      <reg:status rdf:resource="http://metadataregistry.org/uri/RegStatus/1001"/>
      <reg:identifier rdf:resource="http://metadataregistry.org/concepts/8641"/>
      <skos:prefLabel xml:lang="en">map</skos:prefLabel>
      <rdakit:toolkitLabel xml:lang="en">map</rdakit:toolkitLabel>
      <skos:definition xml:lang="en">A unit of extent consisting of a representation, normally to scale and on a two-dimensional medium, of a selection of material or abstract features on, or in relation to, the surface of Earth, another celestial body, or an imaginary place.</skos:definition>
      <rdakit:toolkitDefinition xml:lang="en">A unit of extent consisting of a representation, normally to scale and on a two-dimensional medium, of a selection of material or abstract features on, or in relation to, the surface of Earth, another celestial body, or an imaginary place.</rdakit:toolkitDefinition>
      <skos:scopeNote xml:lang="en">This term applies to cartographic resources.</skos:scopeNote>
      <skos:prefLabel xml:lang="ca">mapa</skos:prefLabel>
      <rdakit:toolkitLabel xml:lang="ca">mapa</rdakit:toolkitLabel>
      <skos:definition xml:lang="ca">Unitat d’extensió que consisteix en una representació, normalment a escala i en un suport bidimensional, d’una selecció de característiques materials o abstractes de la superfície de la Terra, o en relació amb ella, d’un altre cos celeste, o d’un lloc imaginari.</skos:definition>
      <rdakit:toolkitDefinition xml:lang="ca">Unitat d’extensió que consisteix en una representació, normalment a escala i en un suport bidimensional, d’una selecció de característiques materials o abstractes de la superfície de la Terra, o en relació amb ella, d’un altre cos celeste, o d’un lloc imaginari.</rdakit:toolkitDefinition>
      <skos:scopeNote xml:lang="ca">Aquest terme s'aplica a recursos cartogràfics.</skos:scopeNote>
      <skos:prefLabel xml:lang="vi">bản đồ</skos:prefLabel>
      <rdakit:toolkitLabel xml:lang="vi">bản đồ</rdakit:toolkitLabel>
      <skos:definition xml:lang="vi">Đơn vị của quy mô gồm có trình bày, thường theo tỷ lệ và bằng phương tiện hai chiều, của một lựa chọn của đặc tính vật chất hoặc trừu tượng về, hoặc liên quan tới, bề mặt trái đất, thiên thể khác, hoặc một địa điểm tưởng tượng.</skos:definition>
      <rdakit:toolkitDefinition xml:lang="vi">Đơn vị của quy mô gồm có trình bày, thường theo tỷ lệ và bằng phương tiện hai chiều, của một lựa chọn của đặc tính vật chất hoặc trừu tượng về, hoặc liên quan tới, bề mặt trái đất, thiên thể khác, hoặc một địa điểm tưởng tượng.</rdakit:toolkitDefinition>
      <skos:scopeNote xml:lang="vi">Thuật ngữ này áp dụng cho tài nguyên bản đồ.</skos:scopeNote>
      <skos:prefLabel xml:lang="de">Karte</skos:prefLabel>
      <skos:altLabel xml:lang="de">Plan (Kartografie)</skos:altLabel>
      <rdakit:toolkitLabel xml:lang="de">Karte</rdakit:toolkitLabel>
      <skos:definition xml:lang="de">Eine Einheit für den Umfang, bestehend aus einer Darstellung einer Auswahl von Material oder von abstrakten Besonderheiten auf oder in Verbindung mit der Erdoberfläche, einem anderen Himmelskörper oder einem imaginären Ort; normalerweise maßstabsgerecht und auf einem zweidimensionalen Medium.</skos:definition>
      <rdakit:toolkitDefinition xml:lang="de">Eine Einheit für den Umfang, bestehend aus einer Darstellung einer Auswahl von Material oder von abstrakten Besonderheiten auf oder in Verbindung mit der Erdoberfläche, einem anderen Himmelskörper oder einem imaginären Ort; normalerweise maßstabsgerecht und auf einem zweidimensionalen Medium.</rdakit:toolkitDefinition>
      <skos:scopeNote xml:lang="de">Dieser Terminus trifft auf kartografische Ressourcen zu.</skos:scopeNote>
      <skos:prefLabel xml:lang="fi">kartta</skos:prefLabel>
      <rdakit:toolkitLabel xml:lang="fi">kartta</rdakit:toolkitLabel>
      <skos:definition xml:lang="fi">Laajuuden yksikkö, yleensä mittakaavassa ja kaksiulotteisena esitetty kartta, joka on maan tai muun tähtitaivaan kappaleen tai kuvitteellisen paikan pinnan kuvaus kokonaisuudessaan tai osittain.</skos:definition>
      <rdakit:toolkitDefinition xml:lang="fi">Laajuuden yksikkö, yleensä mittakaavassa ja kaksiulotteisena esitetty kartta, joka on maan tai muun tähtitaivaan kappaleen tai kuvitteellisen paikan pinnan kuvaus kokonaisuudessaan tai osittain.</rdakit:toolkitDefinition>
      <skos:scopeNote xml:lang="fi">Termi koskee kartografisia aineistoja.</skos:scopeNote>
      <skos:altLabel xml:lang="da">kort</skos:altLabel>
      <rdakit:toolkitLabel xml:lang="da">kort</rdakit:toolkitLabel>
      <skos:definition xml:lang="da">Enhed, der er en repræsentation, normalt i korrekt målestoksforhold, af et todimensionelt medium eller et materialeudvalg eller abstrakte træk på eller i forbindelse med Jordens overflade eller overfladen på et andet himmellegeme eller et opdigtet sted.</skos:definition>
      <rdakit:toolkitDefinition xml:lang="da">Enhed, der er en repræsentation, normalt i korrekt målestoksforhold, af et todimensionelt medium eller et materialeudvalg eller abstrakte træk på eller i forbindelse med Jordens overflade eller overfladen på et andet himmellegeme eller et opdigtet sted.</rdakit:toolkitDefinition>
      <skos:scopeNote xml:lang="da">Denne term anvendes for kartografiske ressourcer.</skos:scopeNote>
      <skos:prefLabel xml:lang="fr">carte</skos:prefLabel>
      <skos:altLabel xml:lang="fr">plan (cartographie)</skos:altLabel>
      <rdakit:toolkitLabel xml:lang="fr">carte</rdakit:toolkitLabel>
      <skos:definition xml:lang="fr">Unité d’importance matérielle qui consiste en une représentation, normalement à l’échelle et sur un support bidimensionnel, d’une sélection de caractéristiques matérielles ou conventionnelles de la surface de la Terre, d’un autre corps céleste ou d’un lieu imaginaire, ou bien en relation avec elle.</skos:definition>
      <rdakit:toolkitDefinition xml:lang="fr">Unité d’importance matérielle qui consiste en une représentation, normalement à l’échelle et sur un support bidimensionnel, d’une sélection de caractéristiques matérielles ou conventionnelles de la surface de la Terre, d’un autre corps céleste ou d’un lieu imaginaire, ou bien en relation avec elle.</rdakit:toolkitDefinition>
      <skos:scopeNote xml:lang="fr">Ce terme s’applique aux ressources cartographiques. Comprend une vue à vol d’oiseau, un panorama, un dessin panoramique, une perspective à ras du sol, etc.</skos:scopeNote>
      <skos:prefLabel xml:lang="no">kart</skos:prefLabel>
      <rdakit:toolkitLabel xml:lang="no">kart</rdakit:toolkitLabel>
      <skos:definition xml:lang="no">En omfangsenhet som består av en framstilling, som regel skalatro og i et todimensjonalt medium, av et utvalg fysiske eller abstrakte elementer på eller i forhold til jordoverflaten, andre himmellegemer, eller et oppdiktet sted.</skos:definition>
      <rdakit:toolkitDefinition xml:lang="no">En omfangsenhet som består av en framstilling, som regel skalatro og i et todimensjonalt medium, av et utvalg fysiske eller abstrakte elementer på eller i forhold til jordoverflaten, andre himmellegemer, eller et oppdiktet sted.</rdakit:toolkitDefinition>
      <skos:scopeNote xml:lang="no">Dette begrepet gjelder kartografiske ressurser.</skos:scopeNote>
    </skos:Concept>
<!-- Concept: medal  -->
    <skos:Concept rdf:about="http://rdaregistry.info/termList/RDACarrierEU/1020" xml:lang="en">
      <skos:inScheme rdf:resource="http://rdaregistry.info/termList/RDACarrierEU"/>
      <reg:status rdf:resource="http://metadataregistry.org/uri/RegStatus/1001"/>
      <reg:identifier rdf:resource="http://metadataregistry.org/concepts/8642"/>
      <skos:prefLabel xml:lang="en">medal</skos:prefLabel>
      <rdakit:toolkitLabel xml:lang="en">medal</rdakit:toolkitLabel>
      <skos:definition xml:lang="en">A unit of extent consisting of a small piece of metal, bearing a relief design on one or both sides and having a commemorative purpose; not used as a medium of exchange.</skos:definition>
      <rdakit:toolkitDefinition xml:lang="en">A unit of extent consisting of a small piece of metal, bearing a relief design on one or both sides and having a commemorative purpose; not used as a medium of exchange.</rdakit:toolkitDefinition>
      <skos:scopeNote xml:lang="en">This term applies to three-dimensional forms.</skos:scopeNote>
      <skos:prefLabel xml:lang="ca">medalla</skos:prefLabel>
      <rdakit:toolkitLabel xml:lang="ca">medalla</rdakit:toolkitLabel>
      <skos:definition xml:lang="ca">Unitat d’extensió que consisteix en una peça petita de metall, que porta un disseny en relleu a una cara o a totes dues i que té un propòsit commemoratiu; no s’usa com a mitjà d’intercanvi.</skos:definition>
      <rdakit:toolkitDefinition xml:lang="ca">Unitat d’extensió que consisteix en una peça petita de metall, que porta un disseny en relleu a una cara o a totes dues i que té un propòsit commemoratiu; no s’usa com a mitjà d’intercanvi.</rdakit:toolkitDefinition>
      <skos:scopeNote xml:lang="ca">Aquest terme s'aplica a formes tridimensionals.</skos:scopeNote>
      <skos:prefLabel xml:lang="vi">huân chương</skos:prefLabel>
      <rdakit:toolkitLabel xml:lang="vi">huân chương</rdakit:toolkitLabel>
      <skos:definition xml:lang="vi">Đơn vị của quy môgồmcómột mảnh kim loạinhỏ, mang một thiết kếnổi bậttrên một hoặc cả haimặtvớimục đích kỷ niệm; không sử dụng như mộtphương tiện trao đổi.</skos:definition>
      <rdakit:toolkitDefinition xml:lang="vi">Đơn vị của quy môgồmcómột mảnh kim loạinhỏ, mang một thiết kếnổi bậttrên một hoặc cả haimặtvớimục đích kỷ niệm; không sử dụng như mộtphương tiện trao đổi.</rdakit:toolkitDefinition>
      <skos:scopeNote xml:lang="vi">Thuật ngữ này áp dụng cho hình thái ba chiều.</skos:scopeNote>
      <skos:prefLabel xml:lang="de">Medaille</skos:prefLabel>
      <rdakit:toolkitLabel xml:lang="de">Medaille</rdakit:toolkitLabel>
      <skos:definition xml:lang="de">Eine Einheit für den Umfang, bestehend aus einem kleinen Stück Metall, das auf einer oder beiden Seiten ein Relief trägt und einen Erinnerungszweck hat; wird nicht als Zahlungsmittel verwendet.</skos:definition>
      <rdakit:toolkitDefinition xml:lang="de">Eine Einheit für den Umfang, bestehend aus einem kleinen Stück Metall, das auf einer oder beiden Seiten ein Relief trägt und einen Erinnerungszweck hat; wird nicht als Zahlungsmittel verwendet.</rdakit:toolkitDefinition>
      <skos:scopeNote xml:lang="de">Dieser Terminus trifft auf dreidimensionale Formen zu.</skos:scopeNote>
      <skos:prefLabel xml:lang="fi">kunniamerkki</skos:prefLabel>
      <rdakit:toolkitLabel xml:lang="fi">kunniamerkki</rdakit:toolkitLabel>
      <skos:definition xml:lang="fi">Laajuuden yksikkö, pienestä metallinpalasta muodostuva kolmiulotteinen esine, jossa on kohokuvio toisella tai molemmilla puolilla ja jolla on muistotarkoitus.</skos:definition>
      <rdakit:toolkitDefinition xml:lang="fi">Laajuuden yksikkö, pienestä metallinpalasta muodostuva kolmiulotteinen esine, jossa on kohokuvio toisella tai molemmilla puolilla ja jolla on muistotarkoitus.</rdakit:toolkitDefinition>
      <skos:altLabel xml:lang="da">medalje</skos:altLabel>
      <rdakit:toolkitLabel xml:lang="da">medalje</rdakit:toolkitLabel>
      <skos:definition xml:lang="da">Enhed, der består af et lille stykke metal med et reliefdesign på en eller begge sider, der har et erindringsformål; ikke brugt som betalingsmiddel.</skos:definition>
      <rdakit:toolkitDefinition xml:lang="da">Enhed, der består af et lille stykke metal med et reliefdesign på en eller begge sider, der har et erindringsformål; ikke brugt som betalingsmiddel.</rdakit:toolkitDefinition>
      <skos:scopeNote xml:lang="da">Denne term anvendes for tredimensionelle former.</skos:scopeNote>
      <skos:prefLabel xml:lang="fr">médaille</skos:prefLabel>
      <rdakit:toolkitLabel xml:lang="fr">médaille</rdakit:toolkitLabel>
      <skos:definition xml:lang="fr">Unité d’importance matérielle qui consiste en une petite pièce de métal présentant un motif en relief sur l’un ou les deux côtés et ayant une fonction commémorative ; n’est pas utilisée comme moyen d’échange.</skos:definition>
      <rdakit:toolkitDefinition xml:lang="fr">Unité d’importance matérielle qui consiste en une petite pièce de métal présentant un motif en relief sur l’un ou les deux côtés et ayant une fonction commémorative ; n’est pas utilisée comme moyen d’échange.</rdakit:toolkitDefinition>
      <skos:scopeNote xml:lang="fr">Ce terme s’applique aux images fixes.</skos:scopeNote>
      <skos:prefLabel xml:lang="no">medalje</skos:prefLabel>
      <rdakit:toolkitLabel xml:lang="no">medalje</rdakit:toolkitLabel>
      <skos:definition xml:lang="no">En omfangsenhet som består av et lite stykke metall med design i relieff på én eller begge sider, os som brukes til minneformål, ikke som byttemiddel.</skos:definition>
      <rdakit:toolkitDefinition xml:lang="no">En omfangsenhet som består av et lite stykke metall med design i relieff på én eller begge sider, os som brukes til minneformål, ikke som byttemiddel.</rdakit:toolkitDefinition>
      <skos:scopeNote xml:lang="no">Dette begrepet gjelder tredimensjonale former.</skos:scopeNote>
    </skos:Concept>
<!-- Concept: mock-up  -->
    <skos:Concept rdf:about="http://rdaregistry.info/termList/RDACarrierEU/1021" xml:lang="en">
      <skos:inScheme rdf:resource="http://rdaregistry.info/termList/RDACarrierEU"/>
      <reg:status rdf:resource="http://metadataregistry.org/uri/RegStatus/1001"/>
      <reg:identifier rdf:resource="http://metadataregistry.org/concepts/8643"/>
      <skos:prefLabel xml:lang="en">mock-up</skos:prefLabel>
      <rdakit:toolkitLabel xml:lang="en">mock-up</rdakit:toolkitLabel>
      <skos:definition xml:lang="en">A unit of extent consisting of a physical representation of a device or process that may be modified for training or analysis to emphasize a particular part or function.</skos:definition>
      <rdakit:toolkitDefinition xml:lang="en">A unit of extent consisting of a physical representation of a device or process that may be modified for training or analysis to emphasize a particular part or function.</rdakit:toolkitDefinition>
      <skos:scopeNote xml:lang="en">This term applies to three-dimensional forms.</skos:scopeNote>
      <skos:prefLabel xml:lang="ca">model</skos:prefLabel>
      <rdakit:toolkitLabel xml:lang="ca">model</rdakit:toolkitLabel>
      <skos:definition xml:lang="ca">Unitat d’extensió que consisteix en la representació física d’un aparell o un procés que pot ser modificat de cara a la formació o a l’anàlisi per remarcar-ne una part o una funció concreta.</skos:definition>
      <rdakit:toolkitDefinition xml:lang="ca">Unitat d’extensió que consisteix en la representació física d’un aparell o un procés que pot ser modificat de cara a la formació o a l’anàlisi per remarcar-ne una part o una funció concreta.</rdakit:toolkitDefinition>
      <skos:scopeNote xml:lang="ca">Aquest terme s'aplica a formes tridimensionals.</skos:scopeNote>
      <skos:prefLabel xml:lang="vi">mẫu hình</skos:prefLabel>
      <rdakit:toolkitLabel xml:lang="vi">mẫu hình</rdakit:toolkitLabel>
      <skos:definition xml:lang="vi">Đơn vị của quy mô gồm có trình bày vật lý của thiết bị hoặc quá trình có thể được sửa đổi để đào tạo hoặc phân tích để nhấn mạnh phần phần hoặc chức năng riêng lẻ.</skos:definition>
      <rdakit:toolkitDefinition xml:lang="vi">Đơn vị của quy mô gồm có trình bày vật lý của thiết bị hoặc quá trình có thể được sửa đổi để đào tạo hoặc phân tích để nhấn mạnh phần phần hoặc chức năng riêng lẻ.</rdakit:toolkitDefinition>
      <skos:scopeNote xml:lang="vi">Thuật ngữ này áp dụng cho hình thái ba chiều.</skos:scopeNote>
      <skos:prefLabel xml:lang="de">Nachbildung</skos:prefLabel>
      <rdakit:toolkitLabel xml:lang="de">Nachbildung</rdakit:toolkitLabel>
      <skos:definition xml:lang="de">Eine Einheit für den Umfang, bestehend aus einer physischen Darstellung eines Gerätes oder eines Prozesses, das/der zur Übung oder zur Analyse modifiziert werden kann, um einen bestimmten Teil oder eine Funktion herauszustellen.</skos:definition>
      <rdakit:toolkitDefinition xml:lang="de">Eine Einheit für den Umfang, bestehend aus einer physischen Darstellung eines Gerätes oder eines Prozesses, das/der zur Übung oder zur Analyse modifiziert werden kann, um einen bestimmten Teil oder eine Funktion herauszustellen.</rdakit:toolkitDefinition>
      <skos:scopeNote xml:lang="de">Dieser Terminus trifft auf dreidimensionale Formen zu.</skos:scopeNote>
      <skos:prefLabel xml:lang="fi">mallikappale</skos:prefLabel>
      <rdakit:toolkitLabel xml:lang="fi">mallikappale</rdakit:toolkitLabel>
      <skos:definition xml:lang="fi">Laajuuden yksikkö, laitetta tai prosessia kuvaava kappale, jota voidaan muokata koulutus- tai analyysitarkoituksessa tietyn osan tai toiminnon korostamiseksi.</skos:definition>
      <rdakit:toolkitDefinition xml:lang="fi">Laajuuden yksikkö, laitetta tai prosessia kuvaava kappale, jota voidaan muokata koulutus- tai analyysitarkoituksessa tietyn osan tai toiminnon korostamiseksi.</rdakit:toolkitDefinition>
      <skos:scopeNote xml:lang="fi">Termi koskee kolmiulotteisia muotoja.</skos:scopeNote>
      <skos:altLabel xml:lang="da">mockup</skos:altLabel>
      <rdakit:toolkitLabel xml:lang="da">mockup</rdakit:toolkitLabel>
      <skos:definition xml:lang="da">Enhed, der repræsenterer en anordning eller proces og som kan ændres til øvelses- eller analysebrug for at fremhæve en særlig del eller funktion.</skos:definition>
      <rdakit:toolkitDefinition xml:lang="da">Enhed, der repræsenterer en anordning eller proces og som kan ændres til øvelses- eller analysebrug for at fremhæve en særlig del eller funktion.</rdakit:toolkitDefinition>
      <skos:scopeNote xml:lang="da">Denne term anvendes for tredimensionelle former.</skos:scopeNote>
      <skos:prefLabel xml:lang="fr">maquette grandeur nature</skos:prefLabel>
      <skos:altLabel xml:lang="fr">maquette en vraie grandeur</skos:altLabel>
      <rdakit:toolkitLabel xml:lang="fr">maquette grandeur nature</rdakit:toolkitLabel>
      <skos:definition xml:lang="fr">Unité d’importance matérielle qui consiste en une représentation physique d’un dispositif ou d’un processus, qui peut être modifiée pour des besoins de formation ou d’analyse afin de mettre l’accent sur une partie ou une fonction spécifiques.</skos:definition>
      <rdakit:toolkitDefinition xml:lang="fr">Unité d’importance matérielle qui consiste en une représentation physique d’un dispositif ou d’un processus, qui peut être modifiée pour des besoins de formation ou d’analyse afin de mettre l’accent sur une partie ou une fonction spécifiques.</rdakit:toolkitDefinition>
      <skos:altLabel xml:lang="fr">maquette grandeur réelle</skos:altLabel>
      <skos:prefLabel xml:lang="no">øvelsesmodell</skos:prefLabel>
      <rdakit:toolkitLabel xml:lang="no">øvelsesmodell</rdakit:toolkitLabel>
      <skos:definition xml:lang="no">En omfangsenhet som består av en fysisk framstilling av en innretning, mekanisme eller prosess som kan modifiseres for opplæring eller analyse med sikte på å legge vekt på en bestemt del eller funksjon.</skos:definition>
      <rdakit:toolkitDefinition xml:lang="no">En omfangsenhet som består av en fysisk framstilling av en innretning, mekanisme eller prosess som kan modifiseres for opplæring eller analyse med sikte på å legge vekt på en bestemt del eller funksjon.</rdakit:toolkitDefinition>
      <skos:scopeNote xml:lang="no">Dette begrepet gjelder tredimensjonale former.</skos:scopeNote>
    </skos:Concept>
<!-- Concept: model  -->
    <skos:Concept rdf:about="http://rdaregistry.info/termList/RDACarrierEU/1022" xml:lang="en">
      <skos:inScheme rdf:resource="http://rdaregistry.info/termList/RDACarrierEU"/>
      <reg:status rdf:resource="http://metadataregistry.org/uri/RegStatus/1001"/>
      <reg:identifier rdf:resource="http://metadataregistry.org/concepts/8644"/>
      <skos:prefLabel xml:lang="en">model</skos:prefLabel>
      <rdakit:toolkitLabel xml:lang="en">model</rdakit:toolkitLabel>
      <skos:definition xml:lang="en">A unit of extent consisting of a three-dimensional representation of a real or imagined object.</skos:definition>
      <rdakit:toolkitDefinition xml:lang="en">A unit of extent consisting of a three-dimensional representation of a real or imagined object.</rdakit:toolkitDefinition>
      <skos:scopeNote xml:lang="en">This term applies to cartographic resources and three-dimensional forms.</skos:scopeNote>
	    <skos:related rdf:resource="http://rdaregistry.info/termList/RDACarrierEU/1039"/>
      <skos:prefLabel xml:lang="ca">maqueta</skos:prefLabel>
      <rdakit:toolkitLabel xml:lang="ca">maqueta</rdakit:toolkitLabel>
      <skos:definition xml:lang="ca">Unitat d’extensió que consisteix en una representació tridimensional d’un objecte real o imaginat.</skos:definition>
      <rdakit:toolkitDefinition xml:lang="ca">Unitat d’extensió que consisteix en una representació tridimensional d’un objecte real o imaginat.</rdakit:toolkitDefinition>
      <skos:scopeNote xml:lang="ca">Aquest terme s'aplica a recursos cartogràfics i formes tridimensionals.</skos:scopeNote>
      <skos:prefLabel xml:lang="vi">mô hình</skos:prefLabel>
      <rdakit:toolkitLabel xml:lang="vi">mô hình</rdakit:toolkitLabel>
      <skos:definition xml:lang="vi">Đơn vị của quy mô gồm có trình bày ba chiều của vật thể thực hoặc tưởng tượng.</skos:definition>
      <rdakit:toolkitDefinition xml:lang="vi">Đơn vị của quy mô gồm có trình bày ba chiều của vật thể thực hoặc tưởng tượng.</rdakit:toolkitDefinition>
      <skos:scopeNote xml:lang="vi">Thuật ngữ này áp dụng cho tài nguyên bản đồ và hình thái ba chiều.</skos:scopeNote>
      <skos:prefLabel xml:lang="de">Modell</skos:prefLabel>
      <rdakit:toolkitLabel xml:lang="de">Modell</rdakit:toolkitLabel>
      <skos:definition xml:lang="de">Eine Einheit für den Umfang, bestehend aus einer dreidimensionalen Darstellung eines realen oder imaginären Objekts.</skos:definition>
      <rdakit:toolkitDefinition xml:lang="de">Eine Einheit für den Umfang, bestehend aus einer dreidimensionalen Darstellung eines realen oder imaginären Objekts.</rdakit:toolkitDefinition>
      <skos:scopeNote xml:lang="de">Dieser Terminus trifft auf kartografische Ressourcen und dreidimensionale Formen zu.</skos:scopeNote>
      <skos:prefLabel xml:lang="fi">malli</skos:prefLabel>
      <rdakit:toolkitLabel xml:lang="fi">malli</rdakit:toolkitLabel>
      <skos:definition xml:lang="fi">Laajuuden yksikkö, kolmiulotteinen esine, joka kuvaa todellista tai kuvitteellista objektia.</skos:definition>
      <rdakit:toolkitDefinition xml:lang="fi">Laajuuden yksikkö, kolmiulotteinen esine, joka kuvaa todellista tai kuvitteellista objektia.</rdakit:toolkitDefinition>
      <skos:scopeNote xml:lang="fi">Termi koskee kartografisia aineistoja ja kolmiulotteisia muotoja.</skos:scopeNote>
      <skos:altLabel xml:lang="da">model</skos:altLabel>
      <rdakit:toolkitLabel xml:lang="da">model</rdakit:toolkitLabel>
      <skos:definition xml:lang="da">Enhed, der repræsenterer en virkelig eller opdigtet genstand, normalt i mindre målestok.</skos:definition>
      <rdakit:toolkitDefinition xml:lang="da">Enhed, der repræsenterer en virkelig eller opdigtet genstand, normalt i mindre målestok.</rdakit:toolkitDefinition>
      <skos:scopeNote xml:lang="da">Denne term anvendes for kartografiske ressourcer og tredimensionelle former.</skos:scopeNote>
      <skos:prefLabel xml:lang="fr">maquette</skos:prefLabel>
      <rdakit:toolkitLabel xml:lang="fr">maquette</rdakit:toolkitLabel>
      <skos:definition xml:lang="fr">Unité d’importance matérielle qui consiste en une représentation tridimensionnelle d’un objet réel ou imaginaire.</skos:definition>
      <rdakit:toolkitDefinition xml:lang="fr">Unité d’importance matérielle qui consiste en une représentation tridimensionnelle d’un objet réel ou imaginaire.</rdakit:toolkitDefinition>
      <skos:prefLabel xml:lang="no">modell</skos:prefLabel>
      <rdakit:toolkitLabel xml:lang="no">modell</rdakit:toolkitLabel>
      <skos:definition xml:lang="no">En omfangsenhet som består av en tredimensjonal fremstilling av et virkelig eller innbilt objekt.</skos:definition>
      <rdakit:toolkitDefinition xml:lang="no">En omfangsenhet som består av en tredimensjonal fremstilling av et virkelig eller innbilt objekt.</rdakit:toolkitDefinition>
      <skos:scopeNote xml:lang="no">Denne begrepet gjelder kartografiske ressurser og tredimensjonale former.</skos:scopeNote>
    </skos:Concept>
<!-- Concept: page  -->
    <skos:Concept rdf:about="http://rdaregistry.info/termList/RDACarrierEU/1023" xml:lang="en">
      <skos:inScheme rdf:resource="http://rdaregistry.info/termList/RDACarrierEU"/>
      <reg:status rdf:resource="http://metadataregistry.org/uri/RegStatus/1001"/>
      <reg:identifier rdf:resource="http://metadataregistry.org/concepts/8645"/>
      <skos:prefLabel xml:lang="en">page</skos:prefLabel>
      <rdakit:toolkitLabel xml:lang="en">page</rdakit:toolkitLabel>
      <skos:definition xml:lang="en">A unit of extent consisting of a single side of a leaf.</skos:definition>
      <rdakit:toolkitDefinition xml:lang="en">A unit of extent consisting of a single side of a leaf.</rdakit:toolkitDefinition>
      <skos:prefLabel xml:lang="ca">pàgina</skos:prefLabel>
      <rdakit:toolkitLabel xml:lang="ca">pàgina</rdakit:toolkitLabel>
      <skos:definition xml:lang="ca">Unitat d’extensió que consisteix en una cara d’un full.</skos:definition>
      <rdakit:toolkitDefinition xml:lang="ca">Unitat d’extensió que consisteix en una cara d’un full.</rdakit:toolkitDefinition>
      <skos:prefLabel xml:lang="vi">trang</skos:prefLabel>
      <rdakit:toolkitLabel xml:lang="vi">trang</rdakit:toolkitLabel>
      <skos:definition xml:lang="vi">Đơn vị của quy mô gồm có một mặt đơn của tờ.</skos:definition>
      <rdakit:toolkitDefinition xml:lang="vi">Đơn vị của quy mô gồm có một mặt đơn của tờ.</rdakit:toolkitDefinition>
      <skos:prefLabel xml:lang="de">Seite</skos:prefLabel>
      <rdakit:toolkitLabel xml:lang="de">Seite</rdakit:toolkitLabel>
      <skos:definition xml:lang="de">Eine Einheit für den Umfang, bestehend aus einer einzelnen Seite eines Blattes.</skos:definition>
      <rdakit:toolkitDefinition xml:lang="de">Eine Einheit für den Umfang, bestehend aus einer einzelnen Seite eines Blattes.</rdakit:toolkitDefinition>
      <skos:prefLabel xml:lang="fi">sivu</skos:prefLabel>
      <rdakit:toolkitLabel xml:lang="fi">sivu</rdakit:toolkitLabel>
      <skos:definition xml:lang="fi">Laajuuden yksikkö, muodostuu lehden yhdestä puolesta.</skos:definition>
      <rdakit:toolkitDefinition xml:lang="fi">Laajuuden yksikkö, muodostuu lehden yhdestä puolesta.</rdakit:toolkitDefinition>
      <skos:altLabel xml:lang="da">side</skos:altLabel>
      <rdakit:toolkitLabel xml:lang="da">side</rdakit:toolkitLabel>
      <skos:definition xml:lang="da">Enhed, der består af en enkelt side af et blad.</skos:definition>
      <rdakit:toolkitDefinition xml:lang="da">Enhed, der består af en enkelt side af et blad.</rdakit:toolkitDefinition>
      <skos:prefLabel xml:lang="fr">page</skos:prefLabel>
      <rdakit:toolkitLabel xml:lang="fr">page</rdakit:toolkitLabel>
      <skos:definition xml:lang="fr">Unité d’importance matérielle qui consiste en un seul côté d’un feuillet.</skos:definition>
      <rdakit:toolkitDefinition xml:lang="fr">Unité d’importance matérielle qui consiste en un seul côté d’un feuillet.</rdakit:toolkitDefinition>
      <skos:prefLabel xml:lang="no">side</skos:prefLabel>
      <rdakit:toolkitLabel xml:lang="no">side</rdakit:toolkitLabel>
      <skos:definition xml:lang="no">En omfangsenhet som betegner den ene siden av et blad.</skos:definition>
      <rdakit:toolkitDefinition xml:lang="no">En omfangsenhet som betegner den ene siden av et blad.</rdakit:toolkitDefinition>
    </skos:Concept>
<!-- Concept: painting  -->
    <skos:Concept rdf:about="http://rdaregistry.info/termList/RDACarrierEU/1024" xml:lang="en">
      <skos:inScheme rdf:resource="http://rdaregistry.info/termList/RDACarrierEU"/>
      <reg:status rdf:resource="http://metadataregistry.org/uri/RegStatus/1001"/>
      <reg:identifier rdf:resource="http://metadataregistry.org/concepts/8646"/>
      <skos:prefLabel xml:lang="en">painting</skos:prefLabel>
      <rdakit:toolkitLabel xml:lang="en">painting</rdakit:toolkitLabel>
      <skos:definition xml:lang="en">A unit of extent consisting of an item in which images are formed primarily by the direct application of pigment suspended in a medium, arranged in masses of colour onto a generally two-dimensional surface.</skos:definition>
      <rdakit:toolkitDefinition xml:lang="en">A unit of extent consisting of an item in which images are formed primarily by the direct application of pigment suspended in a medium, arranged in masses of colour onto a generally two-dimensional surface.</rdakit:toolkitDefinition>
      <skos:scopeNote xml:lang="en">This term applies to still images.</skos:scopeNote>
      <skos:prefLabel xml:lang="ca">pintura</skos:prefLabel>
      <rdakit:toolkitLabel xml:lang="ca">pintura</rdakit:toolkitLabel>
      <skos:definition xml:lang="ca">Unitat d’extensió consisteix en un ítem en el qual les imatges es formen principalment per mitjà de l’aplicació directa de pigments suspesos en una substància i que s’arrangen en masses de color sobre una superfície que, en general, és bidimensional.</skos:definition>
      <rdakit:toolkitDefinition xml:lang="ca">Unitat d’extensió consisteix en un ítem en el qual les imatges es formen principalment per mitjà de l’aplicació directa de pigments suspesos en una substància i que s’arrangen en masses de color sobre una superfície que, en general, és bidimensional.</rdakit:toolkitDefinition>
      <skos:scopeNote xml:lang="ca">Aquest terme s'aplica a imatges fixes</skos:scopeNote>
      <skos:prefLabel xml:lang="vi">bức hoạ</skos:prefLabel>
      <rdakit:toolkitLabel xml:lang="vi">bức hoạ</rdakit:toolkitLabel>
      <skos:definition xml:lang="vi">Đơn vị của quy môgồm cómộtbảntrong đó hình ảnh được hình thành chủ yếu bởi các ứng dụng trực tiếp củacácsắc tốđược gántrong một phương tiện, sắp xếp theo khối lượng của màu sắc lên, nói chung,một bề mặt hai chiều.</skos:definition>
      <rdakit:toolkitDefinition xml:lang="vi">Đơn vị của quy môgồm cómộtbảntrong đó hình ảnh được hình thành chủ yếu bởi các ứng dụng trực tiếp củacácsắc tốđược gántrong một phương tiện, sắp xếp theo khối lượng của màu sắc lên, nói chung,một bề mặt hai chiều.</rdakit:toolkitDefinition>
      <skos:scopeNote xml:lang="vi">Thuật ngữ này áp dụng cho hình ảnh tĩnh.</skos:scopeNote>
      <skos:prefLabel xml:lang="de">Gemälde</skos:prefLabel>
      <rdakit:toolkitLabel xml:lang="de">Gemälde</rdakit:toolkitLabel>
      <skos:definition xml:lang="de">Eine Einheit für den Umfang, bestehend aus einem Objekt, bei dem Bilder in erster Linie durch direktes Auftragen von Pigment dargestellt werden, das in ein Medium eingebracht ist und in Farbmengen auf einer im Allgemeinen zweidimensionalen Oberfläche angeordnet wird.</skos:definition>
      <rdakit:toolkitDefinition xml:lang="de">Eine Einheit für den Umfang, bestehend aus einem Objekt, bei dem Bilder in erster Linie durch direktes Auftragen von Pigment dargestellt werden, das in ein Medium eingebracht ist und in Farbmengen auf einer im Allgemeinen zweidimensionalen Oberfläche angeordnet wird.</rdakit:toolkitDefinition>
      <skos:scopeNote xml:lang="de">Dieser Terminus trifft auf unbewegte Bilder zu.</skos:scopeNote>
      <skos:prefLabel xml:lang="fi">maalaus</skos:prefLabel>
      <rdakit:toolkitLabel xml:lang="fi">maalaus</rdakit:toolkitLabel>
      <skos:definition xml:lang="fi">Laajuuden yksikkö, liikkumaton kuva, joka on tehty useimmiten maalaamalla väriaineita suoraan alustalle, yleensä kaksiulotteiselle pinnalle.</skos:definition>
      <rdakit:toolkitDefinition xml:lang="fi">Laajuuden yksikkö, liikkumaton kuva, joka on tehty useimmiten maalaamalla väriaineita suoraan alustalle, yleensä kaksiulotteiselle pinnalle.</rdakit:toolkitDefinition>
      <skos:scopeNote xml:lang="fi">Termi koskee stillkuvia.</skos:scopeNote>
      <skos:altLabel xml:lang="da">maleri</skos:altLabel>
      <rdakit:toolkitLabel xml:lang="da">maleri</rdakit:toolkitLabel>
      <skos:definition xml:lang="da">Enhed, der består af et eksemplar, hvori billeder er dannet primært ved direkte påføring af pigment, der er opslæmmet og arrangeret i flader af farve på en almindeligvis todimensionel overflade.</skos:definition>
      <rdakit:toolkitDefinition xml:lang="da">Enhed, der består af et eksemplar, hvori billeder er dannet primært ved direkte påføring af pigment, der er opslæmmet og arrangeret i flader af farve på en almindeligvis todimensionel overflade.</rdakit:toolkitDefinition>
      <skos:scopeNote xml:lang="da">Denne term anvendes for faste billeder.</skos:scopeNote>
      <skos:prefLabel xml:lang="fr">peinture</skos:prefLabel>
      <rdakit:toolkitLabel xml:lang="fr">peinture</rdakit:toolkitLabel>
      <skos:definition xml:lang="fr">Unité d’importance matérielle qui consiste en un item dans lequel les images sont principalement formées par l’application directe d’un pigment en suspension dans un médium, arrangées en masses de couleur sur une surface généralement bidimensionnelle.</skos:definition>
      <rdakit:toolkitDefinition xml:lang="fr">Unité d’importance matérielle qui consiste en un item dans lequel les images sont principalement formées par l’application directe d’un pigment en suspension dans un médium, arrangées en masses de couleur sur une surface généralement bidimensionnelle.</rdakit:toolkitDefinition>
      <skos:prefLabel xml:lang="no">maleri</skos:prefLabel>
      <rdakit:toolkitLabel xml:lang="no">maleri</rdakit:toolkitLabel>
      <skos:definition xml:lang="no">En omfangsenhet som består av et eksemplar der bilder hovedsakelig skapes gjennom direkte påføring av pigment i et medium, ordnet i områder av farge på en vanligvis todimensjonal overflate.</skos:definition>
      <rdakit:toolkitDefinition xml:lang="no">En omfangsenhet som består av et eksemplar der bilder hovedsakelig skapes gjennom direkte påføring av pigment i et medium, ordnet i områder av farge på en vanligvis todimensjonal overflate.</rdakit:toolkitDefinition>
      <skos:scopeNote xml:lang="no">Dette begrepet gjelder stillbilder.</skos:scopeNote>
    </skos:Concept>
<!-- Concept: photograph  -->
    <skos:Concept rdf:about="http://rdaregistry.info/termList/RDACarrierEU/1025" xml:lang="en">
      <skos:inScheme rdf:resource="http://rdaregistry.info/termList/RDACarrierEU"/>
      <reg:status rdf:resource="http://metadataregistry.org/uri/RegStatus/1001"/>
      <reg:identifier rdf:resource="http://metadataregistry.org/concepts/8647"/>
      <skos:prefLabel xml:lang="en">photograph</skos:prefLabel>
      <rdakit:toolkitLabel xml:lang="en">photograph</rdakit:toolkitLabel>
      <skos:definition xml:lang="en">A unit of extent consisting of an image captured by a lens and carried on the surface of a sheet.</skos:definition>
      <rdakit:toolkitDefinition xml:lang="en">A unit of extent consisting of an image captured by a lens and carried on the surface of a sheet.</rdakit:toolkitDefinition>
      <skos:prefLabel xml:lang="ca">fotografia</skos:prefLabel>
      <rdakit:toolkitLabel xml:lang="ca">fotografia</rdakit:toolkitLabel>
      <skos:definition xml:lang="ca">Unitat d'extensió consistent en una imatge capturada amb una lent i traslladada sobre la superfície d'un full.</skos:definition>
      <rdakit:toolkitDefinition xml:lang="ca">Unitat d'extensió consistent en una imatge capturada amb una lent i traslladada sobre la superfície d'un full.</rdakit:toolkitDefinition>
      <skos:prefLabel xml:lang="vi">bức ảnh</skos:prefLabel>
      <rdakit:toolkitLabel xml:lang="vi">bức ảnh</rdakit:toolkitLabel>
      <skos:definition xml:lang="vi">Đơn vị của quy mô gồm có hình ảnh được thu nạp bởi ống kính và được chứa trên bề mặt của tờ.</skos:definition>
      <rdakit:toolkitDefinition xml:lang="vi">Đơn vị của quy mô gồm có hình ảnh được thu nạp bởi ống kính và được chứa trên bề mặt của tờ.</rdakit:toolkitDefinition>
      <skos:prefLabel xml:lang="de">Fotografie</skos:prefLabel>
      <rdakit:toolkitLabel xml:lang="de">Fotografie</rdakit:toolkitLabel>
      <skos:definition xml:lang="de">Eine Einheit für den Umfang bestehend aus einem Bild, das mit einer Linse aufgenommen wurde und auf die Oberfläche eines Blattes übertragen wurde.</skos:definition>
      <rdakit:toolkitDefinition xml:lang="de">Eine Einheit für den Umfang bestehend aus einem Bild, das mit einer Linse aufgenommen wurde und auf die Oberfläche eines Blattes übertragen wurde.</rdakit:toolkitDefinition>
      <skos:prefLabel xml:lang="fi">valokuva</skos:prefLabel>
      <rdakit:toolkitLabel xml:lang="fi">valokuva</rdakit:toolkitLabel>
      <skos:definition xml:lang="fi">Laajuuden yksikkö, linssillä otettu kuva joka on siirretty arkin pinnalle.</skos:definition>
      <rdakit:toolkitDefinition xml:lang="fi">Laajuuden yksikkö, linssillä otettu kuva joka on siirretty arkin pinnalle.</rdakit:toolkitDefinition>
      <skos:altLabel xml:lang="da">foto</skos:altLabel>
      <rdakit:toolkitLabel xml:lang="da">foto</rdakit:toolkitLabel>
      <skos:definition xml:lang="da">Enhed, der består af et billede fanget af en linse og overført til overfladen af et ark.</skos:definition>
      <rdakit:toolkitDefinition xml:lang="da">Enhed, der består af et billede fanget af en linse og overført til overfladen af et ark.</rdakit:toolkitDefinition>
      <skos:prefLabel xml:lang="fr">photographie</skos:prefLabel>
      <rdakit:toolkitLabel xml:lang="fr">photographie</rdakit:toolkitLabel>
      <skos:definition xml:lang="fr">Unité d’importance matérielle qui consiste en une image captée par une lentille et transférée sur la surface d’une feuille.</skos:definition>
      <rdakit:toolkitDefinition xml:lang="fr">Unité d’importance matérielle qui consiste en une image captée par une lentille et transférée sur la surface d’une feuille.</rdakit:toolkitDefinition>
      <skos:prefLabel xml:lang="no">fotografi</skos:prefLabel>
      <rdakit:toolkitLabel xml:lang="no">fotografi</rdakit:toolkitLabel>
      <skos:definition xml:lang="no">En omfangsenhet som består av et bilde som er tatt ved hjelp av et objektiv og som vises på overflaten av et ark.</skos:definition>
      <rdakit:toolkitDefinition xml:lang="no">En omfangsenhet som består av et bilde som er tatt ved hjelp av et objektiv og som vises på overflaten av et ark.</rdakit:toolkitDefinition>
    </skos:Concept>
<!-- Concept: picture  -->
    <skos:Concept rdf:about="http://rdaregistry.info/termList/RDACarrierEU/1026" xml:lang="en">
      <skos:inScheme rdf:resource="http://rdaregistry.info/termList/RDACarrierEU"/>
      <reg:status rdf:resource="http://metadataregistry.org/uri/RegStatus/1001"/>
      <reg:identifier rdf:resource="http://metadataregistry.org/concepts/8648"/>
      <skos:prefLabel xml:lang="en">picture</skos:prefLabel>
      <rdakit:toolkitLabel xml:lang="en">picture</rdakit:toolkitLabel>
      <skos:definition xml:lang="en">A unit of extent consisting of two-dimensional representations.</skos:definition>
      <rdakit:toolkitDefinition xml:lang="en">A unit of extent consisting of two-dimensional representations.</rdakit:toolkitDefinition>
      <skos:scopeNote xml:lang="en">This term applies to still images.</skos:scopeNote>
      <skos:prefLabel xml:lang="ca">làmina</skos:prefLabel>
      <rdakit:toolkitLabel xml:lang="ca">làmina</rdakit:toolkitLabel>
      <skos:definition xml:lang="ca">Unitat d’extensió que consisteix en representacions bidimensionals.</skos:definition>
      <rdakit:toolkitDefinition xml:lang="ca">Unitat d’extensió que consisteix en representacions bidimensionals.</rdakit:toolkitDefinition>
      <skos:scopeNote xml:lang="ca">Aquest terme s'aplica a imatges fixes</skos:scopeNote>
      <skos:prefLabel xml:lang="vi">bức tranh</skos:prefLabel>
      <rdakit:toolkitLabel xml:lang="vi">bức tranh</rdakit:toolkitLabel>
      <skos:definition xml:lang="vi">Đơn vị của quy mô gồm có các trình bày hai chiều.</skos:definition>
      <rdakit:toolkitDefinition xml:lang="vi">Đơn vị của quy mô gồm có các trình bày hai chiều.</rdakit:toolkitDefinition>
      <skos:scopeNote xml:lang="vi">Thuật ngữ này áp dụng cho hình ảnh tĩnh.</skos:scopeNote>
      <skos:prefLabel xml:lang="de">Bild</skos:prefLabel>
      <rdakit:toolkitLabel xml:lang="de">Bild</rdakit:toolkitLabel>
      <skos:definition xml:lang="de">Eine Einheit für den Umfang der aus zweidimensionalen Darstellungen besteht.</skos:definition>
      <rdakit:toolkitDefinition xml:lang="de">Eine Einheit für den Umfang der aus zweidimensionalen Darstellungen besteht.</rdakit:toolkitDefinition>
      <skos:scopeNote xml:lang="de">Dieser Terminus trifft auf unbewegte Bilder zu.</skos:scopeNote>
      <skos:prefLabel xml:lang="fi">kuva</skos:prefLabel>
      <rdakit:toolkitLabel xml:lang="fi">kuva</rdakit:toolkitLabel>
      <skos:definition xml:lang="fi">Laajuuden yksikkö, kaksiulotteinen liikkumaton kuva.</skos:definition>
      <rdakit:toolkitDefinition xml:lang="fi">Laajuuden yksikkö, kaksiulotteinen liikkumaton kuva.</rdakit:toolkitDefinition>
      <skos:scopeNote xml:lang="fi">Termi koskee stillkuvia.</skos:scopeNote>
      <skos:altLabel xml:lang="da">billede</skos:altLabel>
      <rdakit:toolkitLabel xml:lang="da">billede</rdakit:toolkitLabel>
      <skos:definition xml:lang="da">Enhed, der består af todimensionelle repræsentationer.</skos:definition>
      <rdakit:toolkitDefinition xml:lang="da">Enhed, der består af todimensionelle repræsentationer.</rdakit:toolkitDefinition>
      <skos:scopeNote xml:lang="da">Denne term anvendes til faste billeder.</skos:scopeNote>
      <skos:prefLabel xml:lang="fr">image</skos:prefLabel>
      <rdakit:toolkitLabel xml:lang="fr">image</rdakit:toolkitLabel>
      <skos:definition xml:lang="fr">Unité d’importance matérielle qui consiste en représentations bidimensionnelles.</skos:definition>
      <rdakit:toolkitDefinition xml:lang="fr">Unité d’importance matérielle qui consiste en représentations bidimensionnelles.</rdakit:toolkitDefinition>
      <skos:prefLabel xml:lang="no">bilde</skos:prefLabel>
      <rdakit:toolkitLabel xml:lang="no">bilde</rdakit:toolkitLabel>
      <skos:definition xml:lang="no">En omfangsenhet som består av todimensjonale fremstillinger.</skos:definition>
      <rdakit:toolkitDefinition xml:lang="no">En omfangsenhet som består av todimensjonale fremstillinger.</rdakit:toolkitDefinition>
      <skos:scopeNote xml:lang="no">Dette begrepet gjelder stillbilder.</skos:scopeNote>
    </skos:Concept>
<!-- Concept: portfolio  -->
    <skos:Concept rdf:about="http://rdaregistry.info/termList/RDACarrierEU/1027" xml:lang="en">
      <skos:inScheme rdf:resource="http://rdaregistry.info/termList/RDACarrierEU"/>
      <reg:status rdf:resource="http://metadataregistry.org/uri/RegStatus/1001"/>
      <reg:identifier rdf:resource="http://metadataregistry.org/concepts/8649"/>
      <skos:prefLabel xml:lang="en">portfolio</skos:prefLabel>
      <rdakit:toolkitLabel xml:lang="en">portfolio</rdakit:toolkitLabel>
      <skos:definition xml:lang="en">A unit of extent that is a container for holding loose materials, usually consisting of two covers joined together at the back.</skos:definition>
      <rdakit:toolkitDefinition xml:lang="en">A unit of extent that is a container for holding loose materials, usually consisting of two covers joined together at the back.</rdakit:toolkitDefinition>
      <skos:prefLabel xml:lang="ca">carpeta</skos:prefLabel>
      <rdakit:toolkitLabel xml:lang="ca">carpeta</rdakit:toolkitLabel>
      <skos:definition xml:lang="ca">Unitat d’extensió que és un contenidor per allotjar materials solts, normalment consisteix en dues cobertes unides pel llom.</skos:definition>
      <rdakit:toolkitDefinition xml:lang="ca">Unitat d’extensió que és un contenidor per allotjar materials solts, normalment consisteix en dues cobertes unides pel llom.</rdakit:toolkitDefinition>
      <skos:prefLabel xml:lang="vi">cặp đựng</skos:prefLabel>
      <rdakit:toolkitLabel xml:lang="vi">cặp đựng</rdakit:toolkitLabel>
      <skos:definition xml:lang="vi">Đơn vị của quy mô là vỏ chứa để đựng các tài liệu rời thường gồm có hai bìa nối với nhau ở gáy.</skos:definition>
      <rdakit:toolkitDefinition xml:lang="vi">Đơn vị của quy mô là vỏ chứa để đựng các tài liệu rời thường gồm có hai bìa nối với nhau ở gáy.</rdakit:toolkitDefinition>
      <skos:prefLabel xml:lang="de">Mappe</skos:prefLabel>
      <rdakit:toolkitLabel xml:lang="de">Mappe</rdakit:toolkitLabel>
      <skos:definition xml:lang="de">Eine Einheit für den Umfang, die ein Behältnis zum Zusammenhalten von losen Materialien ist, das normalerweise aus zwei Deckblättern besteht, die an der Rückseite verbunden sind.</skos:definition>
      <rdakit:toolkitDefinition xml:lang="de">Eine Einheit für den Umfang, die ein Behältnis zum Zusammenhalten von losen Materialien ist, das normalerweise aus zwei Deckblättern besteht, die an der Rückseite verbunden sind.</rdakit:toolkitDefinition>
      <skos:prefLabel xml:lang="fi">kansio</skos:prefLabel>
      <rdakit:toolkitLabel xml:lang="fi">kansio</rdakit:toolkitLabel>
      <skos:definition xml:lang="fi">Laajuuden yksikkö, joka on kotelo irrallisen aineiston säilyttämiseen. Koostuu yleensä kahdesta kannesta jotka on liitetty takana yhteen.</skos:definition>
      <rdakit:toolkitDefinition xml:lang="fi">Laajuuden yksikkö, joka on kotelo irrallisen aineiston säilyttämiseen. Koostuu yleensä kahdesta kannesta jotka on liitetty takana yhteen.</rdakit:toolkitDefinition>
      <skos:altLabel xml:lang="da">portfolio</skos:altLabel>
      <rdakit:toolkitLabel xml:lang="da">portfolio</rdakit:toolkitLabel>
      <skos:definition xml:lang="da">Enhed til samling af løse materialer, normalt bestående af to omslag, der er samlet på bagsiden.</skos:definition>
      <rdakit:toolkitDefinition xml:lang="da">Enhed til samling af løse materialer, normalt bestående af to omslag, der er samlet på bagsiden.</rdakit:toolkitDefinition>
      <skos:prefLabel xml:lang="fr">portfolio</skos:prefLabel>
      <rdakit:toolkitLabel xml:lang="fr">portfolio</rdakit:toolkitLabel>
      <skos:definition xml:lang="fr">Unité d’importance matérielle qui consiste en un conteneur servant à maintenir du matériel non relié, constitué habituellement de deux couvertures réunies au dos.</skos:definition>
      <rdakit:toolkitDefinition xml:lang="fr">Unité d’importance matérielle qui consiste en un conteneur servant à maintenir du matériel non relié, constitué habituellement de deux couvertures réunies au dos.</rdakit:toolkitDefinition>
      <skos:prefLabel xml:lang="no">mappe</skos:prefLabel>
      <rdakit:toolkitLabel xml:lang="no">mappe</rdakit:toolkitLabel>
      <skos:definition xml:lang="no">En omfangsenhet som består av en beholder for oppbevaring av løst materiale. Består vanligvis av to permer som henger sammen i ryggen.</skos:definition>
      <rdakit:toolkitDefinition xml:lang="no">En omfangsenhet som består av en beholder for oppbevaring av løst materiale. Består vanligvis av to permer som henger sammen i ryggen.</rdakit:toolkitDefinition>
    </skos:Concept>
<!-- Concept: postcard  -->
    <skos:Concept rdf:about="http://rdaregistry.info/termList/RDACarrierEU/1028" xml:lang="en">
      <skos:inScheme rdf:resource="http://rdaregistry.info/termList/RDACarrierEU"/>
      <reg:status rdf:resource="http://metadataregistry.org/uri/RegStatus/1001"/>
      <reg:identifier rdf:resource="http://metadataregistry.org/concepts/8650"/>
      <skos:prefLabel xml:lang="en">postcard</skos:prefLabel>
      <rdakit:toolkitLabel xml:lang="en">postcard</rdakit:toolkitLabel>
      <skos:definition xml:lang="en">A unit of extent of consisting of a card on which a message may be written or printed for mailing without an envelope.</skos:definition>
      <rdakit:toolkitDefinition xml:lang="en">A unit of extent of consisting of a card on which a message may be written or printed for mailing without an envelope.</rdakit:toolkitDefinition>
      <skos:scopeNote xml:lang="en">This term applies to still images.</skos:scopeNote>
      <skos:prefLabel xml:lang="ca">postal</skos:prefLabel>
      <rdakit:toolkitLabel xml:lang="ca">postal</rdakit:toolkitLabel>
      <skos:definition xml:lang="ca">Unitat d’extensió que consisteix en una targeta en la qual es pot escriure o imprimir un missatge per enviar-lo per correu sense sobre.</skos:definition>
      <rdakit:toolkitDefinition xml:lang="ca">Unitat d’extensió que consisteix en una targeta en la qual es pot escriure o imprimir un missatge per enviar-lo per correu sense sobre.</rdakit:toolkitDefinition>
      <skos:scopeNote xml:lang="ca">Aquest terme s'aplica a imatges fixes</skos:scopeNote>
      <skos:prefLabel xml:lang="vi">bưu thiếp</skos:prefLabel>
      <rdakit:toolkitLabel xml:lang="vi">bưu thiếp</rdakit:toolkitLabel>
      <skos:definition xml:lang="vi">Đơn vị của quy mô gồm có tấm bìa trên đó thông báo được viết hoặc in để gửi thư mà không cần phong bì.</skos:definition>
      <rdakit:toolkitDefinition xml:lang="vi">Đơn vị của quy mô gồm có tấm bìa trên đó thông báo được viết hoặc in để gửi thư mà không cần phong bì.</rdakit:toolkitDefinition>
      <skos:scopeNote xml:lang="vi">Thuật ngữ này áp dụng cho hình ảnh tĩnh.</skos:scopeNote>
      <skos:prefLabel xml:lang="de">Postkarte</skos:prefLabel>
      <rdakit:toolkitLabel xml:lang="de">Postkarte</rdakit:toolkitLabel>
      <skos:definition xml:lang="de">Eine Einheit für den Umfang, bestehend aus einer Karte, auf die eine Nachricht geschrieben oder gedruckt sein kann, zum Postversand ohne Umschlag.</skos:definition>
      <rdakit:toolkitDefinition xml:lang="de">Eine Einheit für den Umfang, bestehend aus einer Karte, auf die eine Nachricht geschrieben oder gedruckt sein kann, zum Postversand ohne Umschlag.</rdakit:toolkitDefinition>
      <skos:scopeNote xml:lang="de">Dieser Terminus trifft auf unbewegte Bilder zu.</skos:scopeNote>
      <skos:prefLabel xml:lang="fi">postikortti</skos:prefLabel>
      <rdakit:toolkitLabel xml:lang="fi">postikortti</rdakit:toolkitLabel>
      <skos:definition xml:lang="fi">Laajuuden yksikkö, kortti, johon voi kirjoittaa tai painaa viestin ja lähettää postitse ilman kirjekuorta.</skos:definition>
      <rdakit:toolkitDefinition xml:lang="fi">Laajuuden yksikkö, kortti, johon voi kirjoittaa tai painaa viestin ja lähettää postitse ilman kirjekuorta.</rdakit:toolkitDefinition>
      <skos:scopeNote xml:lang="fi">Termi koskee stillkuvia.</skos:scopeNote>
      <skos:altLabel xml:lang="da">postkort</skos:altLabel>
      <rdakit:toolkitLabel xml:lang="da">postkort</rdakit:toolkitLabel>
      <skos:definition xml:lang="da">Enhed, der består af et kort, hvorpå en besked kan skrives eller trykkes, og som kan sendes uden kuvert.</skos:definition>
      <rdakit:toolkitDefinition xml:lang="da">Enhed, der består af et kort, hvorpå en besked kan skrives eller trykkes, og som kan sendes uden kuvert.</rdakit:toolkitDefinition>
      <skos:scopeNote xml:lang="da">Denne term anvendes for faste billeder.</skos:scopeNote>
      <skos:prefLabel xml:lang="fr">carte postale</skos:prefLabel>
      <rdakit:toolkitLabel xml:lang="fr">carte postale</rdakit:toolkitLabel>
      <skos:definition xml:lang="fr">Unité d’importance matérielle qui consiste en une carte sur laquelle un message peut être écrit ou imprimé pour envoi sans enveloppe.</skos:definition>
      <rdakit:toolkitDefinition xml:lang="fr">Unité d’importance matérielle qui consiste en une carte sur laquelle un message peut être écrit ou imprimé pour envoi sans enveloppe.</rdakit:toolkitDefinition>
      <skos:prefLabel xml:lang="no">postkort</skos:prefLabel>
      <rdakit:toolkitLabel xml:lang="no">postkort</rdakit:toolkitLabel>
      <skos:definition xml:lang="no">En omfangsenhet som består av et kort det kan skrives en melding på, og som kan sendes i posten uten konvolutt.</skos:definition>
      <rdakit:toolkitDefinition xml:lang="no">En omfangsenhet som består av et kort det kan skrives en melding på, og som kan sendes i posten uten konvolutt.</rdakit:toolkitDefinition>
      <skos:scopeNote xml:lang="no">Dette begrepet gjelder stillbilder.</skos:scopeNote>
    </skos:Concept>
<!-- Concept: poster  -->
    <skos:Concept rdf:about="http://rdaregistry.info/termList/RDACarrierEU/1029" xml:lang="en">
      <skos:inScheme rdf:resource="http://rdaregistry.info/termList/RDACarrierEU"/>
      <reg:status rdf:resource="http://metadataregistry.org/uri/RegStatus/1001"/>
      <reg:identifier rdf:resource="http://metadataregistry.org/concepts/8651"/>
      <skos:prefLabel xml:lang="en">poster</skos:prefLabel>
      <rdakit:toolkitLabel xml:lang="en">poster</rdakit:toolkitLabel>
      <skos:definition xml:lang="en">A unit of extent consisting of a notice, usually decorative or pictorial, intended to be posted to advertise, promote, or publicize an activity, cause, product, or service; also, a decorative, mass-produced print intended for hanging.</skos:definition>
      <rdakit:toolkitDefinition xml:lang="en">A unit of extent consisting of a notice, usually decorative or pictorial, intended to be posted to advertise, promote, or publicize an activity, cause, product, or service; also, a decorative, mass-produced print intended for hanging.</rdakit:toolkitDefinition>
      <skos:scopeNote xml:lang="en">This term applies to still images.</skos:scopeNote>
      <skos:prefLabel xml:lang="ca">cartell</skos:prefLabel>
      <rdakit:toolkitLabel xml:lang="ca">cartell</rdakit:toolkitLabel>
      <skos:definition xml:lang="ca">Unitat d’extensió que consisteix en una notícia, normalment decorativa o il·lustrada, concebuda per fer-la pública amb l’objectiu d’anunciar, de promoure o de difondre una activitat, una causa, un producte o un servei; també fa referència a un imprès decoratiu, produït en massa i concebut per penjar-lo.</skos:definition>
      <rdakit:toolkitDefinition xml:lang="ca">Unitat d’extensió que consisteix en una notícia, normalment decorativa o il·lustrada, concebuda per fer-la pública amb l’objectiu d’anunciar, de promoure o de difondre una activitat, una causa, un producte o un servei; també fa referència a un imprès decoratiu, produït en massa i concebut per penjar-lo.</rdakit:toolkitDefinition>
      <skos:scopeNote xml:lang="ca">Aquest terme s'aplica a imatges fixes.</skos:scopeNote>
      <skos:prefLabel xml:lang="vi">áp phích</skos:prefLabel>
      <rdakit:toolkitLabel xml:lang="vi">áp phích</rdakit:toolkitLabel>
      <skos:definition xml:lang="vi">Đơn vị của quy mô gồm cóthông báo, thườngcótrang trí hoặc tranh ảnh, dự định để đăng quảng cáo, quảng bá, hoặc công bố công khai một hoạt động, nguyêncớ, sản phẩm hoặc dịch vụ; cũnglà bảnin sản xuất hàng loạtcótrang tríđểtreo.</skos:definition>
      <rdakit:toolkitDefinition xml:lang="vi">Đơn vị của quy mô gồm cóthông báo, thườngcótrang trí hoặc tranh ảnh, dự định để đăng quảng cáo, quảng bá, hoặc công bố công khai một hoạt động, nguyêncớ, sản phẩm hoặc dịch vụ; cũnglà bảnin sản xuất hàng loạtcótrang tríđểtreo.</rdakit:toolkitDefinition>
      <skos:scopeNote xml:lang="vi">Thuật ngữ này áp dụng cho hình ảnh tĩnh.</skos:scopeNote>
      <skos:prefLabel xml:lang="de">Plakat</skos:prefLabel>
      <rdakit:toolkitLabel xml:lang="de">Plakat</rdakit:toolkitLabel>
      <skos:definition xml:lang="de">Eine Einheit für den Umfang, bestehend aus einer normalerweise dekorativen oder bildlichen Ankündigung, die dazu gedacht ist, bekannt gemacht zu werden, um für eine Aktivität, eine Sache, ein Produkt oder eine Dienstleistung zu werben, zu annoncieren, zu fördern oder zu propagieren. Auch eine dekorative, massen-hergestellte Druckgrafik, die zum Aufhängen gedacht ist.</skos:definition>
      <rdakit:toolkitDefinition xml:lang="de">Eine Einheit für den Umfang, bestehend aus einer normalerweise dekorativen oder bildlichen Ankündigung, die dazu gedacht ist, bekannt gemacht zu werden, um für eine Aktivität, eine Sache, ein Produkt oder eine Dienstleistung zu werben, zu annoncieren, zu fördern oder zu propagieren. Auch eine dekorative, massen-hergestellte Druckgrafik, die zum Aufhängen gedacht ist.</rdakit:toolkitDefinition>
      <skos:scopeNote xml:lang="de">Dieser Terminus trifft auf unbewegte Bilder zu.</skos:scopeNote>
      <skos:prefLabel xml:lang="fi">juliste</skos:prefLabel>
      <rdakit:toolkitLabel xml:lang="fi">juliste</rdakit:toolkitLabel>
      <skos:definition xml:lang="fi">Laajuuden yksikkö, liikkumaton kuva, joka sisältää ilmoituksen, yleensä koristeellinen tai kuvitettu, tarkoituksenaan mainostaa, edistää tai tiedottaa jostakin toiminnasta, tapahtumasta, tuotteesta tai palvelusta.</skos:definition>
      <rdakit:toolkitDefinition xml:lang="fi">Laajuuden yksikkö, liikkumaton kuva, joka sisältää ilmoituksen, yleensä koristeellinen tai kuvitettu, tarkoituksenaan mainostaa, edistää tai tiedottaa jostakin toiminnasta, tapahtumasta, tuotteesta tai palvelusta.</rdakit:toolkitDefinition>
      <skos:altLabel xml:lang="da">plakat</skos:altLabel>
      <rdakit:toolkitLabel xml:lang="da">plakat</rdakit:toolkitLabel>
      <skos:definition xml:lang="da">Enhed, der består af en notits, normalt dekorativ eller billedlig, beregnet til opsætning som reklame, støtte eller offentliggørelse af en aktivitet, en sag, et produkt eller en service; også et dekorativt, massefremstillet tryk beregnet til ophængning.</skos:definition>
      <rdakit:toolkitDefinition xml:lang="da">Enhed, der består af en notits, normalt dekorativ eller billedlig, beregnet til opsætning som reklame, støtte eller offentliggørelse af en aktivitet, en sag, et produkt eller en service; også et dekorativt, massefremstillet tryk beregnet til ophængning.</rdakit:toolkitDefinition>
      <skos:scopeNote xml:lang="da">Denne term anvendes for faste billeder.</skos:scopeNote>
      <skos:prefLabel xml:lang="fr">affiche</skos:prefLabel>
      <rdakit:toolkitLabel xml:lang="fr">affiche</rdakit:toolkitLabel>
      <skos:definition xml:lang="fr">Unité d’importance matérielle qui consiste en une annonce, généralement décorative ou illustrée, destinée à être affichée pour annoncer, promouvoir ou publiciser une activité, une cause, un produit ou un service ; aussi, un imprimé décoratif produit en série et destiné à être accroché.</skos:definition>
      <rdakit:toolkitDefinition xml:lang="fr">Unité d’importance matérielle qui consiste en une annonce, généralement décorative ou illustrée, destinée à être affichée pour annoncer, promouvoir ou publiciser une activité, une cause, un produit ou un service ; aussi, un imprimé décoratif produit en série et destiné à être accroché.</rdakit:toolkitDefinition>
      <skos:prefLabel xml:lang="no">plakat</skos:prefLabel>
      <rdakit:toolkitLabel xml:lang="no">plakat</rdakit:toolkitLabel>
      <skos:definition xml:lang="no">En omfangsenhet som består av en melding, som regel med bilde(r) eller dekorasjon, ment for å henges opp for å annonsere, promotere eller kunngjøre en aktivitet eller sak, et produkt eller en tjeneste. Kan også være et dekorativt, masseprodusert trykk ment for å henges opp.</skos:definition>
      <rdakit:toolkitDefinition xml:lang="no">En omfangsenhet som består av en melding, som regel med bilde(r) eller dekorasjon, ment for å henges opp for å annonsere, promotere eller kunngjøre en aktivitet eller sak, et produkt eller en tjeneste. Kan også være et dekorativt, masseprodusert trykk ment for å henges opp.</rdakit:toolkitDefinition>
      <skos:scopeNote xml:lang="no">Dette begrepet gjelder stillbilder.</skos:scopeNote>
    </skos:Concept>
<!-- Concept: print  -->
    <skos:Concept rdf:about="http://rdaregistry.info/termList/RDACarrierEU/1030" xml:lang="en">
      <skos:inScheme rdf:resource="http://rdaregistry.info/termList/RDACarrierEU"/>
      <reg:status rdf:resource="http://metadataregistry.org/uri/RegStatus/1001"/>
      <reg:identifier rdf:resource="http://metadataregistry.org/concepts/8652"/>
      <skos:prefLabel xml:lang="en">print</skos:prefLabel>
      <rdakit:toolkitLabel xml:lang="en">print</rdakit:toolkitLabel>
      <skos:definition xml:lang="en">A unit of extent consisting of a pictorial work produced by transferring an image by means of a matrix such as a plate, block, or screen, using any of various printing processes.</skos:definition>
      <rdakit:toolkitDefinition xml:lang="en">A unit of extent consisting of a pictorial work produced by transferring an image by means of a matrix such as a plate, block, or screen, using any of various printing processes.</rdakit:toolkitDefinition>
      <skos:scopeNote xml:lang="en">This term applies to still images.</skos:scopeNote>
      <skos:prefLabel xml:lang="ca">estampa</skos:prefLabel>
      <rdakit:toolkitLabel xml:lang="ca">estampa</rdakit:toolkitLabel>
      <skos:definition xml:lang="ca">Unitat d’extensió que consisteix en una obra visual produïda per la transferència d’una imatge per mitjà d’una matriu com ara una placa, un clixé, una impressió serigràfica, usant qualsevol dels diversos processos d’impressió.</skos:definition>
      <rdakit:toolkitDefinition xml:lang="ca">Unitat d’extensió que consisteix en una obra visual produïda per la transferència d’una imatge per mitjà d’una matriu com ara una placa, un clixé, una impressió serigràfica, usant qualsevol dels diversos processos d’impressió.</rdakit:toolkitDefinition>
      <skos:scopeNote xml:lang="ca">Aquest terme s'aplica a imatges fixes.</skos:scopeNote>
      <skos:prefLabel xml:lang="vi">bản in</skos:prefLabel>
      <rdakit:toolkitLabel xml:lang="vi">bản in</rdakit:toolkitLabel>
      <skos:definition xml:lang="vi">Đơn vị của quy mô lgồm có tác phẩm tranh được sản xuất bằng cách chuyển hình ảnh theo phương pháp ma trận như là bát chữ, bản khắc, hoặc màn hình, sử dụng quá trình in bất kỳ.</skos:definition>
      <rdakit:toolkitDefinition xml:lang="vi">Đơn vị của quy mô lgồm có tác phẩm tranh được sản xuất bằng cách chuyển hình ảnh theo phương pháp ma trận như là bát chữ, bản khắc, hoặc màn hình, sử dụng quá trình in bất kỳ.</rdakit:toolkitDefinition>
      <skos:scopeNote xml:lang="vi">Thuật ngữ này áp dụng cho hình ảnh tĩnh.</skos:scopeNote>
      <skos:prefLabel xml:lang="de">Druckgrafik</skos:prefLabel>
      <rdakit:toolkitLabel xml:lang="de">Druckgrafik</rdakit:toolkitLabel>
      <skos:definition xml:lang="de">Eine Einheit für den Umfang, bestehend aus einem bildhaften Werk, das durch Übertragung eines Bildes mittels einer Matrix, zum Beispiel einer Platte, einem Block oder einem Bildschirm, unter Verwendung von beliebigen Druckprozessen erstellt wird.</skos:definition>
      <rdakit:toolkitDefinition xml:lang="de">Eine Einheit für den Umfang, bestehend aus einem bildhaften Werk, das durch Übertragung eines Bildes mittels einer Matrix, zum Beispiel einer Platte, einem Block oder einem Bildschirm, unter Verwendung von beliebigen Druckprozessen erstellt wird.</rdakit:toolkitDefinition>
      <skos:scopeNote xml:lang="de">Dieser Terminus trifft auf unbewegte Bilder zu.</skos:scopeNote>
      <skos:prefLabel xml:lang="fi">painokuva</skos:prefLabel>
      <rdakit:toolkitLabel xml:lang="fi">painokuva</rdakit:toolkitLabel>
      <skos:definition xml:lang="fi">Laajuuden yksikkö, liikkumaton kuva, joka on valmistettu siirtämällä kuva esimerkiksi painolevyn, kuvaruudun tai muun matriisin kautta käyttäen mitä tahansa monista painomenetelmistä.</skos:definition>
      <rdakit:toolkitDefinition xml:lang="fi">Laajuuden yksikkö, liikkumaton kuva, joka on valmistettu siirtämällä kuva esimerkiksi painolevyn, kuvaruudun tai muun matriisin kautta käyttäen mitä tahansa monista painomenetelmistä.</rdakit:toolkitDefinition>
      <skos:scopeNote xml:lang="fi">Termi koskee stillkuvia.</skos:scopeNote>
      <skos:altLabel xml:lang="da">tryk</skos:altLabel>
      <rdakit:toolkitLabel xml:lang="da">tryk</rdakit:toolkitLabel>
      <skos:definition xml:lang="da">Enhed, der består af et billedværk, der er fremstillet ved at overføre et billede vha. en matrice, såsom en plade, blok eller skærm med brug af forskellige trykkeprocesser.</skos:definition>
      <rdakit:toolkitDefinition xml:lang="da">Enhed, der består af et billedværk, der er fremstillet ved at overføre et billede vha. en matrice, såsom en plade, blok eller skærm med brug af forskellige trykkeprocesser.</rdakit:toolkitDefinition>
      <skos:scopeNote xml:lang="da">Denne term anvendes for faste billeder.</skos:scopeNote>
      <skos:prefLabel xml:lang="fr">estampe</skos:prefLabel>
      <rdakit:toolkitLabel xml:lang="fr">estampe</rdakit:toolkitLabel>
      <skos:definition xml:lang="fr">Unité d’importance matérielle qui consiste en une œuvre visuelle produite par le transfert d’une image au moyen d’une matrice telle qu’une plaque, une planche ou un écran, selon différents procédés d’impression.</skos:definition>
      <rdakit:toolkitDefinition xml:lang="fr">Unité d’importance matérielle qui consiste en une œuvre visuelle produite par le transfert d’une image au moyen d’une matrice telle qu’une plaque, une planche ou un écran, selon différents procédés d’impression.</rdakit:toolkitDefinition>
      <skos:prefLabel xml:lang="no">trykk</skos:prefLabel>
      <rdakit:toolkitLabel xml:lang="no">trykk</rdakit:toolkitLabel>
      <skos:definition xml:lang="no">En omfangsenhet som består av et verk i bildeform, produsert ved å overføre et bilde ved hjelp av en matrise som en trykkeplate eller sjablong, med en av mange ulike trykkeprosesser.</skos:definition>
      <rdakit:toolkitDefinition xml:lang="no">En omfangsenhet som består av et verk i bildeform, produsert ved å overføre et bilde ved hjelp av en matrise som en trykkeplate eller sjablong, med en av mange ulike trykkeprosesser.</rdakit:toolkitDefinition>
      <skos:scopeNote xml:lang="no">Dette begrepet gjelder stillbilder.</skos:scopeNote>
    </skos:Concept>
<!-- Concept: profile  -->
    <skos:Concept rdf:about="http://rdaregistry.info/termList/RDACarrierEU/1031" xml:lang="en">
      <skos:inScheme rdf:resource="http://rdaregistry.info/termList/RDACarrierEU"/>
      <reg:status rdf:resource="http://metadataregistry.org/uri/RegStatus/1001"/>
      <reg:identifier rdf:resource="http://metadataregistry.org/concepts/8653"/>
      <skos:prefLabel xml:lang="en">profile</skos:prefLabel>
      <rdakit:toolkitLabel xml:lang="en">profile</rdakit:toolkitLabel>
      <skos:definition xml:lang="en">A unit of extent that is a scale representation of the intersection of a vertical surface, which may or may not be a plane, with the surface of the ground, or of the intersection of such a vertical surface with that of a conceptual three-dimensional model representing phenomena having a continuous distribution.</skos:definition>
      <rdakit:toolkitDefinition xml:lang="en">A unit of extent that is a scale representation of the intersection of a vertical surface, which may or may not be a plane, with the surface of the ground, or of the intersection of such a vertical surface with that of a conceptual three-dimensional model representing phenomena having a continuous distribution.</rdakit:toolkitDefinition>
      <skos:scopeNote xml:lang="en">This term applies to cartographic resources.</skos:scopeNote>
      <skos:prefLabel xml:lang="ca">perfil</skos:prefLabel>
      <rdakit:toolkitLabel xml:lang="ca">perfil</rdakit:toolkitLabel>
      <skos:definition xml:lang="ca">Unitat d’extensió que és una representació a escala de la intersecció d’una superfície vertical (que pot ser plana o no) amb la superfície del sòl, o de la intersecció d’una superfície vertical d’aquest tipus amb la d’un model conceptual tridimensional que representa fenòmens que tenen una distribució contínua.</skos:definition>
      <rdakit:toolkitDefinition xml:lang="ca">Unitat d’extensió que és una representació a escala de la intersecció d’una superfície vertical (que pot ser plana o no) amb la superfície del sòl, o de la intersecció d’una superfície vertical d’aquest tipus amb la d’un model conceptual tridimensional que representa fenòmens que tenen una distribució contínua.</rdakit:toolkitDefinition>
      <skos:scopeNote xml:lang="ca">Aquest terme s’aplica a recursos cartogràfics.</skos:scopeNote>
      <skos:prefLabel xml:lang="vi">trắc diện</skos:prefLabel>
      <rdakit:toolkitLabel xml:lang="vi">trắc diện</rdakit:toolkitLabel>
      <skos:definition xml:lang="vi">Đơn vị của quy mô là trình bày tỷ lệ của chỗ giao nhau của một mặt đứng, có thể hoặc không là mặt phẳng, với mặt đất, hoặc chỗ giao nhau mặt đứng như vậy với mô hình ba chiều dựa trên khái niệm trình bày hiện tượng phân bố liên tục.</skos:definition>
      <rdakit:toolkitDefinition xml:lang="vi">Đơn vị của quy mô là trình bày tỷ lệ của chỗ giao nhau của một mặt đứng, có thể hoặc không là mặt phẳng, với mặt đất, hoặc chỗ giao nhau mặt đứng như vậy với mô hình ba chiều dựa trên khái niệm trình bày hiện tượng phân bố liên tục.</rdakit:toolkitDefinition>
      <skos:scopeNote xml:lang="vi">Thuật ngữ này áp dụng cho tài nguyên bản đồ.</skos:scopeNote>
      <skos:prefLabel xml:lang="de">Profil</skos:prefLabel>
      <rdakit:toolkitLabel xml:lang="de">Profil</rdakit:toolkitLabel>
      <skos:definition xml:lang="de">Eine Einheit für den Umfang einer maßstabsgetreuen Repräsentation der Schnittpunkte einer vertikalen Oberfläche (die eine Ebene sein kann oder nicht) mit der Erdoberfläche oder der Schnittpunkte einer solchen vertikalen Oberfläche mit der eines konzeptionellen dreidimensionalen Modells, welches Phänomene repräsentiert, die eine kontinuierliche Verbreitung haben.</skos:definition>
      <rdakit:toolkitDefinition xml:lang="de">Eine Einheit für den Umfang einer maßstabsgetreuen Repräsentation der Schnittpunkte einer vertikalen Oberfläche (die eine Ebene sein kann oder nicht) mit der Erdoberfläche oder der Schnittpunkte einer solchen vertikalen Oberfläche mit der eines konzeptionellen dreidimensionalen Modells, welches Phänomene repräsentiert, die eine kontinuierliche Verbreitung haben.</rdakit:toolkitDefinition>
      <skos:scopeNote xml:lang="de">Dieser Terminus trifft auf kartografische Ressourcen zu.</skos:scopeNote>
      <skos:prefLabel xml:lang="fi">poikkileikkaus</skos:prefLabel>
      <rdakit:toolkitLabel xml:lang="fi">poikkileikkaus</rdakit:toolkitLabel>
      <skos:definition xml:lang="fi">Laajuuden yksikkö, mittakaavassa oleva kartta-aineisto, joka on pystysuoran pinnan leikkauspisteen esitys mittakaavassa, joka voi olla yhdensuuntainen maanpinnan kanssa, tai tällaisen pystysuoran pinnan leikkaus kolmiulotteinen malli, joka edustaa jatkuvasti jakautuvia ilmiöitä.</skos:definition>
      <rdakit:toolkitDefinition xml:lang="fi">Laajuuden yksikkö, mittakaavassa oleva kartta-aineisto, joka on pystysuoran pinnan leikkauspisteen esitys mittakaavassa, joka voi olla yhdensuuntainen maanpinnan kanssa, tai tällaisen pystysuoran pinnan leikkaus kolmiulotteinen malli, joka edustaa jatkuvasti jakautuvia ilmiöitä.</rdakit:toolkitDefinition>
      <skos:scopeNote xml:lang="fi">Termi koskee kartografisia aineistoja.</skos:scopeNote>
      <skos:altLabel xml:lang="da">profil</skos:altLabel>
      <rdakit:toolkitLabel xml:lang="da">profil</rdakit:toolkitLabel>
      <skos:definition xml:lang="da">Enhed, der i korrekt målestoksforhold repræsenterer:  skæringspunktet mellem en lodret overflade (der kan være, men ikke nødvendigvis er, plan) og jordens overflade, eller skæringspunktet mellem en sådan lodret overflade og en konceptuel tredimensionel model, der repræsenterer fænomener med kontinuert fordeling.</skos:definition>
      <rdakit:toolkitDefinition xml:lang="da">Enhed, der i korrekt målestoksforhold repræsenterer:  skæringspunktet mellem en lodret overflade (der kan være, men ikke nødvendigvis er, plan) og jordens overflade, eller skæringspunktet mellem en sådan lodret overflade og en konceptuel tredimensionel model, der repræsenterer fænomener med kontinuert fordeling.</rdakit:toolkitDefinition>
      <skos:scopeNote xml:lang="da">Denne term anvendes for kartografiske ressourcer.</skos:scopeNote>
      <skos:prefLabel xml:lang="fr">profil du relief</skos:prefLabel>
      <rdakit:toolkitLabel xml:lang="fr">profil du relief</rdakit:toolkitLabel>
      <skos:definition xml:lang="fr">Unité d’importance matérielle qui consiste en une représentation à l’échelle de l’intersection d’une surface verticale, qui peut être plane ou non, avec la surface du sol ou de l’intersection d’une surface verticale de ce type avec celle d’un modèle conceptuel tridimensionnel représentant des phénomènes à distribution continue.</skos:definition>
      <rdakit:toolkitDefinition xml:lang="fr">Unité d’importance matérielle qui consiste en une représentation à l’échelle de l’intersection d’une surface verticale, qui peut être plane ou non, avec la surface du sol ou de l’intersection d’une surface verticale de ce type avec celle d’un modèle conceptuel tridimensionnel représentant des phénomènes à distribution continue.</rdakit:toolkitDefinition>
      <skos:prefLabel xml:lang="no">profil</skos:prefLabel>
      <rdakit:toolkitLabel xml:lang="no">profil</rdakit:toolkitLabel>
      <skos:definition xml:lang="no">En omfangsenhet som er en framstilling i målestokk av skjæringspunktet mellom en loddrett overflate, som kan være flat eller ikke, og bakken, eller av skjæringspunktet mellom en slik loddrett overflate og en tredimensjonal konseptuell modell som representerer fenomener med kontinuerlig distribusjon.</skos:definition>
      <rdakit:toolkitDefinition xml:lang="no">En omfangsenhet som er en framstilling i målestokk av skjæringspunktet mellom en loddrett overflate, som kan være flat eller ikke, og bakken, eller av skjæringspunktet mellom en slik loddrett overflate og en tredimensjonal konseptuell modell som representerer fenomener med kontinuerlig distribusjon.</rdakit:toolkitDefinition>
      <skos:scopeNote xml:lang="no">Dette begrepet gjelder kartografiske ressurser.</skos:scopeNote>
    </skos:Concept>
<!-- Concept: radiograph  -->
    <skos:Concept rdf:about="http://rdaregistry.info/termList/RDACarrierEU/1032" xml:lang="en">
      <skos:inScheme rdf:resource="http://rdaregistry.info/termList/RDACarrierEU"/>
      <reg:status rdf:resource="http://metadataregistry.org/uri/RegStatus/1001"/>
      <reg:identifier rdf:resource="http://metadataregistry.org/concepts/8654"/>
      <skos:prefLabel xml:lang="en">radiograph</skos:prefLabel>
      <rdakit:toolkitLabel xml:lang="en">radiograph</rdakit:toolkitLabel>
      <skos:definition xml:lang="en">A unit of extent that is a photograph produced by the passage of radiation, such as X rays, gamma rays, or neutrons, through an opaque object.</skos:definition>
      <rdakit:toolkitDefinition xml:lang="en">A unit of extent that is a photograph produced by the passage of radiation, such as X rays, gamma rays, or neutrons, through an opaque object.</rdakit:toolkitDefinition>
      <skos:prefLabel xml:lang="ca">radiografia</skos:prefLabel>
      <rdakit:toolkitLabel xml:lang="ca">radiografia</rdakit:toolkitLabel>
      <skos:definition xml:lang="ca">Unitat d’extensió que és una fotografia produïda pel pas de radiacions, com ara raigs X, raigs gamma o neutrons, a través d’un objecte opac.</skos:definition>
      <rdakit:toolkitDefinition xml:lang="ca">Unitat d’extensió que és una fotografia produïda pel pas de radiacions, com ara raigs X, raigs gamma o neutrons, a través d’un objecte opac.</rdakit:toolkitDefinition>
      <skos:prefLabel xml:lang="vi">hình chụp bằng phóng xạ</skos:prefLabel>
      <rdakit:toolkitLabel xml:lang="vi">hình chụp bằng phóng xạ</rdakit:toolkitLabel>
      <skos:definition xml:lang="vi">Đơn vị của quy mô là Ảnh được tạo ra bằng cách cho phóng xạ, như tia X, tia gamma, hoặc neutron, đi qua một vật thể cản quang.</skos:definition>
      <rdakit:toolkitDefinition xml:lang="vi">Đơn vị của quy mô là Ảnh được tạo ra bằng cách cho phóng xạ, như tia X, tia gamma, hoặc neutron, đi qua một vật thể cản quang.</rdakit:toolkitDefinition>
      <skos:prefLabel xml:lang="de">Röntgenbild</skos:prefLabel>
      <rdakit:toolkitLabel xml:lang="de">Röntgenbild</rdakit:toolkitLabel>
      <skos:definition xml:lang="de">Eine Einheit für den Umfang, bestehend aus einer Fotografie, die durch den Durchtritt von Strahlung wie zum Beispiel Röntgenstrahlen, Gammastrahlen oder Neutronen durch ein lichtundurchlässiges Objekt erzeugt wird.</skos:definition>
      <rdakit:toolkitDefinition xml:lang="de">Eine Einheit für den Umfang, bestehend aus einer Fotografie, die durch den Durchtritt von Strahlung wie zum Beispiel Röntgenstrahlen, Gammastrahlen oder Neutronen durch ein lichtundurchlässiges Objekt erzeugt wird.</rdakit:toolkitDefinition>
      <skos:prefLabel xml:lang="fi">röntgenkuva</skos:prefLabel>
      <rdakit:toolkitLabel xml:lang="fi">röntgenkuva</rdakit:toolkitLabel>
      <skos:definition xml:lang="fi">Laajuuden yksikkö, stillkuva, joka perustuu säteilyn - esimerkiksi röntgen-, gamma- tai neutronisäteilyn - läpäisyyn läpinäkymättömän kohteen läpi.</skos:definition>
      <rdakit:toolkitDefinition xml:lang="fi">Laajuuden yksikkö, stillkuva, joka perustuu säteilyn - esimerkiksi röntgen-, gamma- tai neutronisäteilyn - läpäisyyn läpinäkymättömän kohteen läpi.</rdakit:toolkitDefinition>
      <skos:altLabel xml:lang="da">røntgenbillede</skos:altLabel>
      <rdakit:toolkitLabel xml:lang="da">røntgenbillede</rdakit:toolkitLabel>
      <skos:definition xml:lang="da">Enhed, der består af et fotografi, der er fremstillet ved at sende radioaktiv stråling, såsom røntgenstråler, gammastråler eller neutroner, gennem et uigennemsigtigt objekt.</skos:definition>
      <rdakit:toolkitDefinition xml:lang="da">Enhed, der består af et fotografi, der er fremstillet ved at sende radioaktiv stråling, såsom røntgenstråler, gammastråler eller neutroner, gennem et uigennemsigtigt objekt.</rdakit:toolkitDefinition>
      <skos:prefLabel xml:lang="fr">radiographie</skos:prefLabel>
      <rdakit:toolkitLabel xml:lang="fr">radiographie</rdakit:toolkitLabel>
      <skos:definition xml:lang="fr">Unité d’importance matérielle qui consiste en une photographie produite par le passage de radiations, telles que des rayons X, des rayons gamma ou des neutrons, à travers un objet visuellement opaque.</skos:definition>
      <rdakit:toolkitDefinition xml:lang="fr">Unité d’importance matérielle qui consiste en une photographie produite par le passage de radiations, telles que des rayons X, des rayons gamma ou des neutrons, à travers un objet visuellement opaque.</rdakit:toolkitDefinition>
      <skos:prefLabel xml:lang="no">radiogram</skos:prefLabel>
      <rdakit:toolkitLabel xml:lang="no">radiogram</rdakit:toolkitLabel>
      <skos:definition xml:lang="no">En omfangsenhet som er et fotografi produsert ved å slippe stråling, for eksempel røntgenstråler, gammastråler eller nøytroner gjennom en ugjennomskinnelig gjenstand.</skos:definition>
      <rdakit:toolkitDefinition xml:lang="no">En omfangsenhet som er et fotografi produsert ved å slippe stråling, for eksempel røntgenstråler, gammastråler eller nøytroner gjennom en ugjennomskinnelig gjenstand.</rdakit:toolkitDefinition>
    </skos:Concept>
<!-- Concept: remote-sensing image  -->
    <skos:Concept rdf:about="http://rdaregistry.info/termList/RDACarrierEU/1033" xml:lang="en">
      <skos:inScheme rdf:resource="http://rdaregistry.info/termList/RDACarrierEU"/>
      <reg:status rdf:resource="http://metadataregistry.org/uri/RegStatus/1001"/>
      <reg:identifier rdf:resource="http://metadataregistry.org/concepts/8655"/>
      <skos:prefLabel xml:lang="en">remote-sensing image</skos:prefLabel>
      <rdakit:toolkitLabel xml:lang="en">remote-sensing image</rdakit:toolkitLabel>
      <skos:definition xml:lang="en">A unit of extent that is a pictorial product of any remote-sensing instrument that detects and measures reflected and/or emitted electromagnetic radiation from a distance and reflected underwater sound waves in the case of sonar.</skos:definition>
      <rdakit:toolkitDefinition xml:lang="en">A unit of extent that is a pictorial product of any remote-sensing instrument that detects and measures reflected and/or emitted electromagnetic radiation from a distance and reflected underwater sound waves in the case of sonar.</rdakit:toolkitDefinition>
      <skos:scopeNote xml:lang="en">This term applies to cartographic resources.</skos:scopeNote>
      <skos:prefLabel xml:lang="ca">imatge de teledetecció</skos:prefLabel>
      <rdakit:toolkitLabel xml:lang="ca">imatge de teledetecció</rdakit:toolkitLabel>
      <skos:definition xml:lang="ca">Unitat d’extensió que és un producte il·lustrat de qualsevol instrument de teledetecció que detecta i mesura una radiació electromagnètica reflectida i/o emesa des d’una distància i reflectida en ones sonores sota l’aigua en el cas del sonar.</skos:definition>
      <rdakit:toolkitDefinition xml:lang="ca">Unitat d’extensió que és un producte il·lustrat de qualsevol instrument de teledetecció que detecta i mesura una radiació electromagnètica reflectida i/o emesa des d’una distància i reflectida en ones sonores sota l’aigua en el cas del sonar.</rdakit:toolkitDefinition>
      <skos:scopeNote xml:lang="ca">Aquest terme s’aplica a recursos cartogràfics.</skos:scopeNote>
      <skos:prefLabel xml:lang="vi">hình ảnh cảm nhận từ xa</skos:prefLabel>
      <rdakit:toolkitLabel xml:lang="vi">hình ảnh cảm nhận từ xa</rdakit:toolkitLabel>
      <skos:definition xml:lang="vi">Đơn vị của quy mô là tài nguyên bản đồ là sản phẩm tranh ảnh của công cụ cảm nhận từ xa bất kỳ, được nhận biết và đo lường qua bức xạ quang từ với khoảng cách xa và phản chiếu sóng âm dưới mặt nước trong trường hợp định vị vật dưới mặt nước.</skos:definition>
      <rdakit:toolkitDefinition xml:lang="vi">Đơn vị của quy mô là tài nguyên bản đồ là sản phẩm tranh ảnh của công cụ cảm nhận từ xa bất kỳ, được nhận biết và đo lường qua bức xạ quang từ với khoảng cách xa và phản chiếu sóng âm dưới mặt nước trong trường hợp định vị vật dưới mặt nước.</rdakit:toolkitDefinition>
      <skos:scopeNote xml:lang="vi">Thuật ngữ này áp dụng cho tài nguyên bản đồ.</skos:scopeNote>
      <skos:prefLabel xml:lang="de">Fernerkundungsbild</skos:prefLabel>
      <rdakit:toolkitLabel xml:lang="de">Fernerkundungsbild</rdakit:toolkitLabel>
      <skos:definition xml:lang="de">Eine Einheit für den Umfang, bestehend aus einem bildlichen Produkt eines Fernerkundungsinstruments, das reflektierte und/oder emittierte elektromagnetische Strahlung aus der Distanz entdeckt und misst sowie im Falle eines Sonars Schallwellen unter Wasser reflektiert.</skos:definition>
      <rdakit:toolkitDefinition xml:lang="de">Eine Einheit für den Umfang, bestehend aus einem bildlichen Produkt eines Fernerkundungsinstruments, das reflektierte und/oder emittierte elektromagnetische Strahlung aus der Distanz entdeckt und misst sowie im Falle eines Sonars Schallwellen unter Wasser reflektiert.</rdakit:toolkitDefinition>
      <skos:scopeNote xml:lang="de">Dieser Terminus trifft auf kartografische Ressourcen zu.</skos:scopeNote>
      <skos:prefLabel xml:lang="fi">kaukokartoituskuva</skos:prefLabel>
      <rdakit:toolkitLabel xml:lang="fi">kaukokartoituskuva</rdakit:toolkitLabel>
      <skos:definition xml:lang="fi">Laajuuden yksikkö, kartta-aineisto, joka perustuu kaukokartoitusmittalaitteen etäältä havaitsemaan ja mittaamaan heijastuneeseen ja/tai säteilleeseen elektromagneettiseen säteilyyn tai, kaikuluotaimen ollessa kyseessä, heijastuneisiin vedenalaisiin ääniaaltoihin.</skos:definition>
      <rdakit:toolkitDefinition xml:lang="fi">Laajuuden yksikkö, kartta-aineisto, joka perustuu kaukokartoitusmittalaitteen etäältä havaitsemaan ja mittaamaan heijastuneeseen ja/tai säteilleeseen elektromagneettiseen säteilyyn tai, kaikuluotaimen ollessa kyseessä, heijastuneisiin vedenalaisiin ääniaaltoihin.</rdakit:toolkitDefinition>
      <skos:scopeNote xml:lang="fi">Termi koskee kartografisia aineistoja.</skos:scopeNote>
      <skos:altLabel xml:lang="da">remote-sensing kort</skos:altLabel>
      <rdakit:toolkitLabel xml:lang="da">remote-sensing kort</rdakit:toolkitLabel>
      <skos:definition xml:lang="da">Enhed, der er et billedligt produkt, skabt ved, at et remote-sensing- / fjerndetektionsinstrument detekterer og måler reflekteret og/eller udledt elektromagnetisk stråling på afstand, eller reflekterede undervandslydbølger, hvis der er tale om en sonar.</skos:definition>
      <rdakit:toolkitDefinition xml:lang="da">Enhed, der er et billedligt produkt, skabt ved, at et remote-sensing- / fjerndetektionsinstrument detekterer og måler reflekteret og/eller udledt elektromagnetisk stråling på afstand, eller reflekterede undervandslydbølger, hvis der er tale om en sonar.</rdakit:toolkitDefinition>
      <skos:scopeNote xml:lang="da">Denne term anvendes for kartografiske ressourcer.</skos:scopeNote>
      <skos:prefLabel xml:lang="fr">image de télédétection</skos:prefLabel>
      <rdakit:toolkitLabel xml:lang="fr">image de télédétection</rdakit:toolkitLabel>
      <skos:definition xml:lang="fr">Unité d’importance matérielle qui consiste en un produit image de tout instrument qui détecte et mesure d’une certaine distance la radiation électromagnétique reflétée et/ou émise et les ondes sonores reflétées sous l’eau dans le cas du sonar.</skos:definition>
      <rdakit:toolkitDefinition xml:lang="fr">Unité d’importance matérielle qui consiste en un produit image de tout instrument qui détecte et mesure d’une certaine distance la radiation électromagnétique reflétée et/ou émise et les ondes sonores reflétées sous l’eau dans le cas du sonar.</rdakit:toolkitDefinition>
      <skos:prefLabel xml:lang="no">fjernanalysebilde</skos:prefLabel>
      <rdakit:toolkitLabel xml:lang="no">fjernanalysebilde</rdakit:toolkitLabel>
      <skos:definition xml:lang="no">En omfangsenhet som er et produkt i bildeform fra et instrument for fjernanalyse som registrerer og måler reflektert og/eller utstrålt elektromagnetisk stråling på avstand, eller, for ekkolodd, reflekterte lydbølger under vann.</skos:definition>
      <rdakit:toolkitDefinition xml:lang="no">En omfangsenhet som er et produkt i bildeform fra et instrument for fjernanalyse som registrerer og måler reflektert og/eller utstrålt elektromagnetisk stråling på avstand, eller, for ekkolodd, reflekterte lydbølger under vann.</rdakit:toolkitDefinition>
      <skos:scopeNote xml:lang="no">Dette begrepet gjelder kartografiske ressurser.</skos:scopeNote>
    </skos:Concept>
<!-- Concept: sculpture  -->
    <skos:Concept rdf:about="http://rdaregistry.info/termList/RDACarrierEU/1034" xml:lang="en">
      <skos:inScheme rdf:resource="http://rdaregistry.info/termList/RDACarrierEU"/>
      <reg:status rdf:resource="http://metadataregistry.org/uri/RegStatus/1001"/>
      <reg:identifier rdf:resource="http://metadataregistry.org/concepts/8656"/>
      <skos:prefLabel xml:lang="en">sculpture</skos:prefLabel>
      <rdakit:toolkitLabel xml:lang="en">sculpture</rdakit:toolkitLabel>
      <skos:definition xml:lang="en">A unit of extent consisting of a physical representation, usually of art, in which an image or form is produced in relief, in intaglio, or in the round.</skos:definition>
      <rdakit:toolkitDefinition xml:lang="en">A unit of extent consisting of a physical representation, usually of art, in which an image or form is produced in relief, in intaglio, or in the round.</rdakit:toolkitDefinition>
      <skos:scopeNote xml:lang="en">This term applies to three-dimensional forms.</skos:scopeNote>
      <skos:prefLabel xml:lang="ca">escultura</skos:prefLabel>
      <rdakit:toolkitLabel xml:lang="ca">escultura</rdakit:toolkitLabel>
      <skos:definition xml:lang="ca">Unitat d’extensió que consisteix en una representació física, normalment d’art, en la qual les imatges o les formes es produeixen en relleu, gravades al buit o de forma estatuària o aïllada.</skos:definition>
      <rdakit:toolkitDefinition xml:lang="ca">Unitat d’extensió que consisteix en una representació física, normalment d’art, en la qual les imatges o les formes es produeixen en relleu, gravades al buit o de forma estatuària o aïllada.</rdakit:toolkitDefinition>
      <skos:scopeNote xml:lang="ca">Aquest terme s'aplica a formes tridimensionals.</skos:scopeNote>
      <skos:prefLabel xml:lang="vi">điêu khắc</skos:prefLabel>
      <rdakit:toolkitLabel xml:lang="vi">điêu khắc</rdakit:toolkitLabel>
      <skos:definition xml:lang="vi">Đơn vịcủa quy mô gồm cótrình bày vật lý, thường là nghệ thuật, trong đó hình ảnhhoặcđịnh dạngđượctạo rabằng vật thay thế,chạm chim,hoặc vòngtròn.</skos:definition>
      <rdakit:toolkitDefinition xml:lang="vi">Đơn vịcủa quy mô gồm cótrình bày vật lý, thường là nghệ thuật, trong đó hình ảnhhoặcđịnh dạngđượctạo rabằng vật thay thế,chạm chim,hoặc vòngtròn.</rdakit:toolkitDefinition>
      <skos:scopeNote xml:lang="vi">Thuật ngữ này áp dụng cho hình thái ba chiều.</skos:scopeNote>
      <skos:prefLabel xml:lang="de">Skulptur</skos:prefLabel>
      <rdakit:toolkitLabel xml:lang="de">Skulptur</rdakit:toolkitLabel>
      <skos:definition xml:lang="de">Eine Einheit für den Umfang, bestehend aus einer physischen Darstellung, normalerweise in der Kunst, bei der Bilder und Formen als Relief, als Intaglio oder in Rundumansicht erzeugt werden.</skos:definition>
      <rdakit:toolkitDefinition xml:lang="de">Eine Einheit für den Umfang, bestehend aus einer physischen Darstellung, normalerweise in der Kunst, bei der Bilder und Formen als Relief, als Intaglio oder in Rundumansicht erzeugt werden.</rdakit:toolkitDefinition>
      <skos:scopeNote xml:lang="de">Dieser Terminus trifft auf dreidimensionale Formen zu.</skos:scopeNote>
      <skos:prefLabel xml:lang="fi">veistos</skos:prefLabel>
      <rdakit:toolkitLabel xml:lang="fi">veistos</rdakit:toolkitLabel>
      <skos:definition xml:lang="fi">Laajuuden yksikkö, kolmiulotteinen fyysinen yleensä taiteen ilmaisumuoto jossa kuva ja muoto on tehty kohokuvana (pintareliefi tai upotettu reliefi) tai joka puolelta katsottavana muotona.</skos:definition>
      <rdakit:toolkitDefinition xml:lang="fi">Laajuuden yksikkö, kolmiulotteinen fyysinen yleensä taiteen ilmaisumuoto jossa kuva ja muoto on tehty kohokuvana (pintareliefi tai upotettu reliefi) tai joka puolelta katsottavana muotona.</rdakit:toolkitDefinition>
      <skos:scopeNote xml:lang="fi">Termi koskee kolmiulotteisia muotoja.</skos:scopeNote>
      <skos:altLabel xml:lang="da">skulptur</skos:altLabel>
      <rdakit:toolkitLabel xml:lang="da">skulptur</rdakit:toolkitLabel>
      <skos:definition xml:lang="da">Enhed, der består af fysiske repræsentationer, normalt som kunst, hvor billeder og former fremstilles i relief, dybtryk eller i fri figur.</skos:definition>
      <rdakit:toolkitDefinition xml:lang="da">Enhed, der består af fysiske repræsentationer, normalt som kunst, hvor billeder og former fremstilles i relief, dybtryk eller i fri figur.</rdakit:toolkitDefinition>
      <skos:scopeNote xml:lang="da">Denne term anvendes for tredimensionelle former.</skos:scopeNote>
      <skos:prefLabel xml:lang="fr">sculpture</skos:prefLabel>
      <rdakit:toolkitLabel xml:lang="fr">sculpture</rdakit:toolkitLabel>
      <skos:definition xml:lang="fr">Unité d’importance matérielle qui consiste en une représentation physique, généralement d’art, dans laquelle une image ou une forme est produite en relief, en creux ou en ronde-bosse.</skos:definition>
      <rdakit:toolkitDefinition xml:lang="fr">Unité d’importance matérielle qui consiste en une représentation physique, généralement d’art, dans laquelle une image ou une forme est produite en relief, en creux ou en ronde-bosse.</rdakit:toolkitDefinition>
      <skos:prefLabel xml:lang="no">skulptur</skos:prefLabel>
      <rdakit:toolkitLabel xml:lang="no">skulptur</rdakit:toolkitLabel>
      <skos:definition xml:lang="no">En omfangsenhet som består av en fysisk framstilling, som regel i form av kunst, der en avbildning eller figur produseres som relieff, utskjæring eller friskulptur.</skos:definition>
      <rdakit:toolkitDefinition xml:lang="no">En omfangsenhet som består av en fysisk framstilling, som regel i form av kunst, der en avbildning eller figur produseres som relieff, utskjæring eller friskulptur.</rdakit:toolkitDefinition>
      <skos:scopeNote xml:lang="no">Dette begrepet gjelder tredimensjonale former.</skos:scopeNote>
    </skos:Concept>
<!-- Concept: section  -->
    <skos:Concept rdf:about="http://rdaregistry.info/termList/RDACarrierEU/1035" xml:lang="en">
      <skos:inScheme rdf:resource="http://rdaregistry.info/termList/RDACarrierEU"/>
      <reg:status rdf:resource="http://metadataregistry.org/uri/RegStatus/1001"/>
      <reg:identifier rdf:resource="http://metadataregistry.org/concepts/8657"/>
      <skos:prefLabel xml:lang="en">section</skos:prefLabel>
      <skos:altLabel xml:lang="en">map section</skos:altLabel>
      <rdakit:toolkitLabel xml:lang="en">section</rdakit:toolkitLabel>
      <skos:definition xml:lang="en">A unit of extent that is a scale representation of a vertical surface, commonly a plane, displaying both the profile where it intersects the surface of a celestial body, or some conceptual model, and the underlying structures along the plane of intersection.</skos:definition>
      <rdakit:toolkitDefinition xml:lang="en">A unit of extent that is a scale representation of a vertical surface, commonly a plane, displaying both the profile where it intersects the surface of a celestial body, or some conceptual model, and the underlying structures along the plane of intersection.</rdakit:toolkitDefinition>
      <skos:scopeNote xml:lang="en">This term applies to cartographic resources.</skos:scopeNote>
      <skos:prefLabel xml:lang="ca">secció</skos:prefLabel>
      <skos:altLabel xml:lang="ca">secció de mapa</skos:altLabel>
      <rdakit:toolkitLabel xml:lang="ca">secció</rdakit:toolkitLabel>
      <skos:definition xml:lang="ca">Unitat d’extensió que és una representació a escala d’una superfície vertical, generalment un pla, que mostra tant el perfil que interseca la superfície d’un cos celeste o d’algun model conceptual, com les estructures que queden per sota del pla de la intersecció.</skos:definition>
      <rdakit:toolkitDefinition xml:lang="ca">Unitat d’extensió que és una representació a escala d’una superfície vertical, generalment un pla, que mostra tant el perfil que interseca la superfície d’un cos celeste o d’algun model conceptual, com les estructures que queden per sota del pla de la intersecció.</rdakit:toolkitDefinition>
      <skos:scopeNote xml:lang="ca">Aquest terme s’aplica a recursos cartogràfics.</skos:scopeNote>
      <skos:prefLabel xml:lang="vi">mặt cắt</skos:prefLabel>
      <skos:altLabel xml:lang="vi">trắc diện bản đồ</skos:altLabel>
      <rdakit:toolkitLabel xml:lang="vi">mặt cắt</rdakit:toolkitLabel>
      <skos:definition xml:lang="vi">Đơn vị của quy mô là trình bày tỷ lệ mặt đứng, thường là mặt phẳng thể hiện cả hai mặt nghiêng phân cắt bề mặt của thiên thể, hoặc mô hình khái niệm nào đó, và nằm dưới cấu trúc dọc theo mặt phẳng cắt ngang.</skos:definition>
      <rdakit:toolkitDefinition xml:lang="vi">Đơn vị của quy mô là trình bày tỷ lệ mặt đứng, thường là mặt phẳng thể hiện cả hai mặt nghiêng phân cắt bề mặt của thiên thể, hoặc mô hình khái niệm nào đó, và nằm dưới cấu trúc dọc theo mặt phẳng cắt ngang.</rdakit:toolkitDefinition>
      <skos:scopeNote xml:lang="vi">Thuật ngữ này áp dụng cho tài nguyên bản đồ.</skos:scopeNote>
      <skos:prefLabel xml:lang="de">Schnitt</skos:prefLabel>
      <rdakit:toolkitLabel xml:lang="de">Schnitt</rdakit:toolkitLabel>
      <skos:definition xml:lang="de">Eine Einheit für den Umfang einer maßstabsgetreuen Darstellung einer vertikalen Oberfläche (normalerweise eine Ebene), die sowohl das Profil anzeigt, wo es die Oberfläche eines Himmelskörpers oder eines konzeptionellen Modells schneidet, als auch die darunter liegenden Strukturen entlang der Schnittebene.</skos:definition>
      <rdakit:toolkitDefinition xml:lang="de">Eine Einheit für den Umfang einer maßstabsgetreuen Darstellung einer vertikalen Oberfläche (normalerweise eine Ebene), die sowohl das Profil anzeigt, wo es die Oberfläche eines Himmelskörpers oder eines konzeptionellen Modells schneidet, als auch die darunter liegenden Strukturen entlang der Schnittebene.</rdakit:toolkitDefinition>
      <skos:scopeNote xml:lang="de">Dieser Terminus trifft auf kartografische Ressourcen zu.</skos:scopeNote>
      <skos:prefLabel xml:lang="fi">poikkileikkauskartta</skos:prefLabel>
      <rdakit:toolkitLabel xml:lang="fi">poikkileikkauskartta</rdakit:toolkitLabel>
      <skos:definition xml:lang="fi">Laajuuden yksikkö, mittakaavassa oleva kartta-aineisto, joka kuvaa pystysuoran pinnan leikkauskohtaa maaperän pinnan kanssa tai jatkuvaa ilmiötä kuvaavan käsitteellisen kolmiulotteisen mallin kanssa.</skos:definition>
      <rdakit:toolkitDefinition xml:lang="fi">Laajuuden yksikkö, mittakaavassa oleva kartta-aineisto, joka kuvaa pystysuoran pinnan leikkauskohtaa maaperän pinnan kanssa tai jatkuvaa ilmiötä kuvaavan käsitteellisen kolmiulotteisen mallin kanssa.</rdakit:toolkitDefinition>
      <skos:altLabel xml:lang="da">snit</skos:altLabel>
      <rdakit:toolkitLabel xml:lang="da">snit</rdakit:toolkitLabel>
      <skos:definition xml:lang="da">Enhed, der er en repræsentation i korrekt målestoksforhold af en lodret overflade (normalt et plan), der viser både profilen, hvor den skærer et himmellegemes overflade eller en konceptmodel, og de underliggende strukturer langs skæringspunktsplanet.</skos:definition>
      <rdakit:toolkitDefinition xml:lang="da">Enhed, der er en repræsentation i korrekt målestoksforhold af en lodret overflade (normalt et plan), der viser både profilen, hvor den skærer et himmellegemes overflade eller en konceptmodel, og de underliggende strukturer langs skæringspunktsplanet.</rdakit:toolkitDefinition>
      <skos:scopeNote xml:lang="da">Denne term anvendes for kartografiske ressourcer.</skos:scopeNote>
      <skos:prefLabel xml:lang="fr">coupe de terrain</skos:prefLabel>
      <skos:altLabel xml:lang="fr">coupe (cartographie)</skos:altLabel>
      <rdakit:toolkitLabel xml:lang="fr">coupe de terrain</rdakit:toolkitLabel>
      <skos:definition xml:lang="fr">Unité d’importance matérielle qui consiste en une représentation à l’échelle d’une surface verticale, généralement plane, montrant à la fois le profil du relief à son intersection avec la surface d’un corps céleste ou d’un modèle conceptuel, ainsi que les structures sous-jacentes au plan de l’intersection.</skos:definition>
      <rdakit:toolkitDefinition xml:lang="fr">Unité d’importance matérielle qui consiste en une représentation à l’échelle d’une surface verticale, généralement plane, montrant à la fois le profil du relief à son intersection avec la surface d’un corps céleste ou d’un modèle conceptuel, ainsi que les structures sous-jacentes au plan de l’intersection.</rdakit:toolkitDefinition>
      <skos:prefLabel xml:lang="no">tverrsnitt</skos:prefLabel>
      <skos:altLabel xml:lang="no">kartutsnitt</skos:altLabel>
      <rdakit:toolkitLabel xml:lang="no">tverrsnitt</rdakit:toolkitLabel>
      <skos:definition xml:lang="no">En omfangsenhet som er en framstilling i målestokk av en loddrett overflate (som regel et plan), som viser både profilen der flaten skjærer overflaten til et himmellegeme, eller en konseptuell modell, og underliggende strukturer langs skjæringsplanet.</skos:definition>
      <rdakit:toolkitDefinition xml:lang="no">En omfangsenhet som er en framstilling i målestokk av en loddrett overflate (som regel et plan), som viser både profilen der flaten skjærer overflaten til et himmellegeme, eller en konseptuell modell, og underliggende strukturer langs skjæringsplanet.</rdakit:toolkitDefinition>
      <skos:scopeNote xml:lang="no">Dette begrepet gjelder kartografiske ressurser.</skos:scopeNote>
    </skos:Concept>
<!-- Concept: specimen  -->
    <skos:Concept rdf:about="http://rdaregistry.info/termList/RDACarrierEU/1036" xml:lang="en">
      <skos:inScheme rdf:resource="http://rdaregistry.info/termList/RDACarrierEU"/>
      <reg:status rdf:resource="http://metadataregistry.org/uri/RegStatus/1001"/>
      <reg:identifier rdf:resource="http://metadataregistry.org/concepts/8658"/>
      <skos:prefLabel xml:lang="en">specimen</skos:prefLabel>
      <rdakit:toolkitLabel xml:lang="en">specimen</rdakit:toolkitLabel>
      <skos:definition xml:lang="en">A unit of extent consisting of an individual unit or sample chosen to represent a larger population or aggregation.</skos:definition>
      <rdakit:toolkitDefinition xml:lang="en">A unit of extent consisting of an individual unit or sample chosen to represent a larger population or aggregation.</rdakit:toolkitDefinition>
      <skos:scopeNote xml:lang="en">This term applies to three-dimensional forms.</skos:scopeNote>
      <skos:prefLabel xml:lang="ca">espècimen</skos:prefLabel>
      <rdakit:toolkitLabel xml:lang="ca">espècimen</rdakit:toolkitLabel>
      <skos:definition xml:lang="ca">Unitat d’extensió que consisteix en una unitat o una mostra individual triada per representar una població o un conjunt més ampli.</skos:definition>
      <rdakit:toolkitDefinition xml:lang="ca">Unitat d’extensió que consisteix en una unitat o una mostra individual triada per representar una població o un conjunt més ampli.</rdakit:toolkitDefinition>
      <skos:scopeNote xml:lang="ca">Aquest terme s'aplica a formes tridimensionals.</skos:scopeNote>
      <skos:prefLabel xml:lang="vi">mẫu vật</skos:prefLabel>
      <rdakit:toolkitLabel xml:lang="vi">mẫu vật</rdakit:toolkitLabel>
      <skos:definition xml:lang="vi">Đơn vị của quy môgồmcómột đơn vịhoặc mẫucáthể được chọn để trình bày một nhóm hoặc tập hợp lớn hơn.</skos:definition>
      <rdakit:toolkitDefinition xml:lang="vi">Đơn vị của quy môgồmcómột đơn vịhoặc mẫucáthể được chọn để trình bày một nhóm hoặc tập hợp lớn hơn.</rdakit:toolkitDefinition>
      <skos:scopeNote xml:lang="vi">Thuật ngữ này áp dụng cho hình thái ba chiều.</skos:scopeNote>
      <skos:prefLabel xml:lang="de">Muster</skos:prefLabel>
      <rdakit:toolkitLabel xml:lang="de">Muster</rdakit:toolkitLabel>
      <skos:definition xml:lang="de">Eine Einheit für den Umfang, bestehend aus einer einzelnen Einheit oder einem Beispiel, das ausgewählt wurde, um einen größeren Bestand oder eine Aggregation zu repräsentieren.</skos:definition>
      <rdakit:toolkitDefinition xml:lang="de">Eine Einheit für den Umfang, bestehend aus einer einzelnen Einheit oder einem Beispiel, das ausgewählt wurde, um einen größeren Bestand oder eine Aggregation zu repräsentieren.</rdakit:toolkitDefinition>
      <skos:scopeNote xml:lang="de">Dieser Terminus trifft auf dreidimensionale Formen zu.</skos:scopeNote>
      <skos:prefLabel xml:lang="fi">näyte</skos:prefLabel>
      <rdakit:toolkitLabel xml:lang="fi">näyte</rdakit:toolkitLabel>
      <skos:definition xml:lang="fi">Laajuuden yksikkö, joka muodostuu yksittäisestä yksiköstä tai mallikappaleesta, joka on valittu edustamaan suurempaa kokonaismäärää.</skos:definition>
      <rdakit:toolkitDefinition xml:lang="fi">Laajuuden yksikkö, joka muodostuu yksittäisestä yksiköstä tai mallikappaleesta, joka on valittu edustamaan suurempaa kokonaismäärää.</rdakit:toolkitDefinition>
      <skos:scopeNote xml:lang="fi">Termi koskee kolmiulotteisia muotoja.</skos:scopeNote>
      <skos:altLabel xml:lang="da">prøveemne</skos:altLabel>
      <rdakit:toolkitLabel xml:lang="da">prøveemne</rdakit:toolkitLabel>
      <skos:definition xml:lang="da">Enhed, der består af en enkelt enhed eller en prøve, der er valgt til at repræsentere en større bestand eller samling.</skos:definition>
      <rdakit:toolkitDefinition xml:lang="da">Enhed, der består af en enkelt enhed eller en prøve, der er valgt til at repræsentere en større bestand eller samling.</rdakit:toolkitDefinition>
      <skos:scopeNote xml:lang="da">Denne term anvendes for tredimensionelle former.</skos:scopeNote>
      <skos:prefLabel xml:lang="fr">spécimen</skos:prefLabel>
      <rdakit:toolkitLabel xml:lang="fr">spécimen</rdakit:toolkitLabel>
      <skos:definition xml:lang="fr">Unité d’importance matérielle qui consiste en une unité ou en un échantillon individuel choisi pour représenter une population ou une agrégation plus importante.</skos:definition>
      <rdakit:toolkitDefinition xml:lang="fr">Unité d’importance matérielle qui consiste en une unité ou en un échantillon individuel choisi pour représenter une population ou une agrégation plus importante.</rdakit:toolkitDefinition>
      <skos:prefLabel xml:lang="no">prøve</skos:prefLabel>
      <rdakit:toolkitLabel xml:lang="no">prøve</rdakit:toolkitLabel>
      <skos:definition xml:lang="no">En omfangsenhet som består av en enkeltenhet eller et utvalg som er valgt for å representere en større populasjon eller samling.</skos:definition>
      <rdakit:toolkitDefinition xml:lang="no">En omfangsenhet som består av en enkeltenhet eller et utvalg som er valgt for å representere en større populasjon eller samling.</rdakit:toolkitDefinition>
      <skos:scopeNote xml:lang="no">Dette begrepet gjelder tredimensjonale former.</skos:scopeNote>
    </skos:Concept>
<!-- Concept: study print  -->
    <skos:Concept rdf:about="http://rdaregistry.info/termList/RDACarrierEU/1037" xml:lang="en">
      <skos:inScheme rdf:resource="http://rdaregistry.info/termList/RDACarrierEU"/>
      <reg:status rdf:resource="http://metadataregistry.org/uri/RegStatus/1001"/>
      <reg:identifier rdf:resource="http://metadataregistry.org/concepts/8659"/>
      <skos:prefLabel xml:lang="en">study print</skos:prefLabel>
      <rdakit:toolkitLabel xml:lang="en">study print</rdakit:toolkitLabel>
      <skos:definition xml:lang="en">A unit of extent consisting of an image sometimes accompanied by text and used for education.</skos:definition>
      <rdakit:toolkitDefinition xml:lang="en">A unit of extent consisting of an image sometimes accompanied by text and used for education.</rdakit:toolkitDefinition>
      <skos:prefLabel xml:lang="ca">làmina didáctica</skos:prefLabel>
      <rdakit:toolkitLabel xml:lang="ca">làmina didáctica</rdakit:toolkitLabel>
      <skos:definition xml:lang="ca">Unitat d’extensió que consisteix en una imatge a vegades acompanyada de text i amb una finalitat educativa.</skos:definition>
      <rdakit:toolkitDefinition xml:lang="ca">Unitat d’extensió que consisteix en una imatge a vegades acompanyada de text i amb una finalitat educativa.</rdakit:toolkitDefinition>
      <skos:prefLabel xml:lang="vi">bản in học tập</skos:prefLabel>
      <rdakit:toolkitLabel xml:lang="vi">bản in học tập</rdakit:toolkitLabel>
      <skos:definition xml:lang="vi">Đơn vị của quy mô gồm có hình ảnh đôi khi kèm theo văn bản được dùng cho giáo dục.</skos:definition>
      <rdakit:toolkitDefinition xml:lang="vi">Đơn vị của quy mô gồm có hình ảnh đôi khi kèm theo văn bản được dùng cho giáo dục.</rdakit:toolkitDefinition>
      <skos:prefLabel xml:lang="de">Studiendruck</skos:prefLabel>
      <rdakit:toolkitLabel xml:lang="de">Studiendruck</rdakit:toolkitLabel>
      <skos:definition xml:lang="de">Eine Einheit für den Umfang, bestehend aus einem Bild, manchmal begleitet von einem Text, die für die Ausbildung verwendet wird.</skos:definition>
      <rdakit:toolkitDefinition xml:lang="de">Eine Einheit für den Umfang, bestehend aus einem Bild, manchmal begleitet von einem Text, die für die Ausbildung verwendet wird.</rdakit:toolkitDefinition>
      <skos:prefLabel xml:lang="fi">opetuskuva</skos:prefLabel>
      <rdakit:toolkitLabel xml:lang="fi">opetuskuva</rdakit:toolkitLabel>
      <skos:definition xml:lang="fi">Laajuuden yksikkö, kuva jonka ohessa voi olla tekstiä ja jota käytetään opetustarkoitukseen.</skos:definition>
      <rdakit:toolkitDefinition xml:lang="fi">Laajuuden yksikkö, kuva jonka ohessa voi olla tekstiä ja jota käytetään opetustarkoitukseen.</rdakit:toolkitDefinition>
      <skos:altLabel xml:lang="da">studietryk</skos:altLabel>
      <rdakit:toolkitLabel xml:lang="da">studietryk</rdakit:toolkitLabel>
      <skos:definition xml:lang="da">Enhed, der består af et billede som kan være ledsaget af tekst og anvendes til uddannelse.</skos:definition>
      <rdakit:toolkitDefinition xml:lang="da">Enhed, der består af et billede som kan være ledsaget af tekst og anvendes til uddannelse.</rdakit:toolkitDefinition>
      <skos:prefLabel xml:lang="fr">image didactique</skos:prefLabel>
      <rdakit:toolkitLabel xml:lang="fr">image didactique</rdakit:toolkitLabel>
      <skos:definition xml:lang="fr">Unité d’importance matérielle qui consiste en une image parfois accompagnée de texte et utilisée à des fins éducatives.</skos:definition>
      <rdakit:toolkitDefinition xml:lang="fr">Unité d’importance matérielle qui consiste en une image parfois accompagnée de texte et utilisée à des fins éducatives.</rdakit:toolkitDefinition>
      <skos:prefLabel xml:lang="no">studietrykk</skos:prefLabel>
      <rdakit:toolkitLabel xml:lang="no">studietrykk</rdakit:toolkitLabel>
      <skos:definition xml:lang="no">En omfangsenhet som består av et bilde som kan være ledsaget av tekst, og som brukes til undervisningsformål.</skos:definition>
      <rdakit:toolkitDefinition xml:lang="no">En omfangsenhet som består av et bilde som kan være ledsaget av tekst, og som brukes til undervisningsformål.</rdakit:toolkitDefinition>
    </skos:Concept>
<!-- Concept: technical drawing  -->
    <skos:Concept rdf:about="http://rdaregistry.info/termList/RDACarrierEU/1038" xml:lang="en">
      <skos:inScheme rdf:resource="http://rdaregistry.info/termList/RDACarrierEU"/>
      <reg:status rdf:resource="http://metadataregistry.org/uri/RegStatus/1001"/>
      <reg:identifier rdf:resource="http://metadataregistry.org/concepts/8660"/>
      <skos:prefLabel xml:lang="en">technical drawing</skos:prefLabel>
      <rdakit:toolkitLabel xml:lang="en">technical drawing</rdakit:toolkitLabel>
      <skos:definition xml:lang="en">A unit of extent consisting of a cross section, detail, diagram, elevation, perspective, plan, working plan, etc., made for use in an engineering or other technical context.</skos:definition>
      <rdakit:toolkitDefinition xml:lang="en">A unit of extent consisting of a cross section, detail, diagram, elevation, perspective, plan, working plan, etc., made for use in an engineering or other technical context.</rdakit:toolkitDefinition>
      <skos:scopeNote xml:lang="en">This term applies to still images.</skos:scopeNote>
      <skos:prefLabel xml:lang="ca">dibuix lineal</skos:prefLabel>
      <rdakit:toolkitLabel xml:lang="ca">dibuix lineal</rdakit:toolkitLabel>
      <skos:definition xml:lang="ca">Unitat d’extensió que consisteix en una secció transversal, un detall, un diagrama, un alçat, una perspectiva, una planta, un plànol de treball, etc., usat en enginyeria o en qualsevol altre context tècnic.</skos:definition>
      <rdakit:toolkitDefinition xml:lang="ca">Unitat d’extensió que consisteix en una secció transversal, un detall, un diagrama, un alçat, una perspectiva, una planta, un plànol de treball, etc., usat en enginyeria o en qualsevol altre context tècnic.</rdakit:toolkitDefinition>
      <skos:scopeNote xml:lang="ca">Aquest terme s'aplica a imatges fixes.</skos:scopeNote>
      <skos:prefLabel xml:lang="vi">bản vẽ kỹ thuật</skos:prefLabel>
      <rdakit:toolkitLabel xml:lang="vi">bản vẽ kỹ thuật</rdakit:toolkitLabel>
      <skos:definition xml:lang="vi">Đơn vị của quy mô là mặt cắt chéo, chi tiết, bản đồ, mặt chiếu, phối cảnh, mặt bằng, mặt bằng làm việc v.v... được tạo ra trong bối cảnh công trình hoặc kỹ thuật.</skos:definition>
      <rdakit:toolkitDefinition xml:lang="vi">Đơn vị của quy mô là mặt cắt chéo, chi tiết, bản đồ, mặt chiếu, phối cảnh, mặt bằng, mặt bằng làm việc v.v... được tạo ra trong bối cảnh công trình hoặc kỹ thuật.</rdakit:toolkitDefinition>
      <skos:scopeNote xml:lang="vi">Thuật ngữ này áp dụng cho hình ảnh tĩnh.</skos:scopeNote>
      <skos:prefLabel xml:lang="de">Technische Zeichnung</skos:prefLabel>
      <rdakit:toolkitLabel xml:lang="de">Technische Zeichnung</rdakit:toolkitLabel>
      <skos:definition xml:lang="de">Eine Einheit für den Umfang, bestehend aus einem Querschnitt, einem Detail, einem Diagramm, einem Aufriss, einer Ansicht, einem Plan, einem Arbeitsplan usw., der/die für die Verwendung in einem technischen oder anderen fachlichen Zusammenhang gemacht wurde.</skos:definition>
      <rdakit:toolkitDefinition xml:lang="de">Eine Einheit für den Umfang, bestehend aus einem Querschnitt, einem Detail, einem Diagramm, einem Aufriss, einer Ansicht, einem Plan, einem Arbeitsplan usw., der/die für die Verwendung in einem technischen oder anderen fachlichen Zusammenhang gemacht wurde.</rdakit:toolkitDefinition>
      <skos:scopeNote xml:lang="de">Dieser Terminus trifft auf unbewegte Bilder zu.</skos:scopeNote>
      <skos:prefLabel xml:lang="fi">tekninen piirustus</skos:prefLabel>
      <rdakit:toolkitLabel xml:lang="fi">tekninen piirustus</rdakit:toolkitLabel>
      <skos:definition xml:lang="fi">Laajuuden yksikkö, liikkumaton kuva, joka muodostuu poikkileikkauksesta, yksityiskohdista, kaavioista, julkisivupiirustuksesta, perspektiivistä, pohjapiirroksesta, työpiirustuksesta tms. Käytetään rakentamisessa ja muissa teknisissä yhteyksissä.</skos:definition>
      <rdakit:toolkitDefinition xml:lang="fi">Laajuuden yksikkö, liikkumaton kuva, joka muodostuu poikkileikkauksesta, yksityiskohdista, kaavioista, julkisivupiirustuksesta, perspektiivistä, pohjapiirroksesta, työpiirustuksesta tms. Käytetään rakentamisessa ja muissa teknisissä yhteyksissä.</rdakit:toolkitDefinition>
      <skos:scopeNote xml:lang="fi">Termi koskee stillkuvia.</skos:scopeNote>
      <skos:altLabel xml:lang="da">teknisk tegning</skos:altLabel>
      <rdakit:toolkitLabel xml:lang="da">teknisk tegning</rdakit:toolkitLabel>
      <skos:definition xml:lang="da">Enhed, der består af et tværsnit, en detalje, et diagram, en kote, et perspektiv, en plan, en arbejdsplan etc., beregnet til anvendelse i maskin- eller anden teknisk kontekst.</skos:definition>
      <rdakit:toolkitDefinition xml:lang="da">Enhed, der består af et tværsnit, en detalje, et diagram, en kote, et perspektiv, en plan, en arbejdsplan etc., beregnet til anvendelse i maskin- eller anden teknisk kontekst.</rdakit:toolkitDefinition>
      <skos:scopeNote xml:lang="da">Denne term anvendes tor faste billeder.</skos:scopeNote>
      <skos:prefLabel xml:lang="fr">dessin industriel</skos:prefLabel>
      <rdakit:toolkitLabel xml:lang="fr">dessin industriel</rdakit:toolkitLabel>
      <skos:definition xml:lang="fr">Unité d’importance matérielle qui consiste en une coupe transversale, en un détail, en un diagramme, en une coupe verticale, en une perspective, en un plan, en un plan de fonctionnement, etc. pour une utilisation en ingénierie ou dans un autre contexte technique.</skos:definition>
      <rdakit:toolkitDefinition xml:lang="fr">Unité d’importance matérielle qui consiste en une coupe transversale, en un détail, en un diagramme, en une coupe verticale, en une perspective, en un plan, en un plan de fonctionnement, etc. pour une utilisation en ingénierie ou dans un autre contexte technique.</rdakit:toolkitDefinition>
      <skos:prefLabel xml:lang="no">teknisk tegning</skos:prefLabel>
      <rdakit:toolkitLabel xml:lang="no">teknisk tegning</rdakit:toolkitLabel>
      <skos:definition xml:lang="no">En omfangsenhet som består av tverrsnitt, detaljer, diagram, vertikalprojeksjon, perspektivtegning, plan, arbeidsplan etc., laget for bruk i en konstruksjon eller annen teknisk sammenheng.</skos:definition>
      <rdakit:toolkitDefinition xml:lang="no">En omfangsenhet som består av tverrsnitt, detaljer, diagram, vertikalprojeksjon, perspektivtegning, plan, arbeidsplan etc., laget for bruk i en konstruksjon eller annen teknisk sammenheng.</rdakit:toolkitDefinition>
      <skos:scopeNote xml:lang="no">Dette begrepet gjelder stillbilder.</skos:scopeNote>
    </skos:Concept>
<!-- Concept: toy  -->
    <skos:Concept rdf:about="http://rdaregistry.info/termList/RDACarrierEU/1039" xml:lang="en">
      <skos:inScheme rdf:resource="http://rdaregistry.info/termList/RDACarrierEU"/>
      <reg:status rdf:resource="http://metadataregistry.org/uri/RegStatus/1001"/>
      <reg:identifier rdf:resource="http://metadataregistry.org/concepts/8661"/>
      <skos:prefLabel xml:lang="en">toy</skos:prefLabel>
      <rdakit:toolkitLabel xml:lang="en">toy</rdakit:toolkitLabel>
      <skos:definition xml:lang="en">A unit of extent consisting of an object designed for education, entertainment, or stimulation through play.</skos:definition>
      <rdakit:toolkitDefinition xml:lang="en">A unit of extent consisting of an object designed for education, entertainment, or stimulation through play.</rdakit:toolkitDefinition>
      <skos:scopeNote xml:lang="en">This term applies to three-dimensional forms.</skos:scopeNote>
	    <skos:related rdf:resource="http://rdaregistry.info/termList/RDACarrierEU/1001"/>
	    <skos:related rdf:resource="http://rdaregistry.info/termList/RDACarrierEU/1014"/>
	    <skos:related rdf:resource="http://rdaregistry.info/termList/RDACarrierEU/1022"/>
      <skos:prefLabel xml:lang="ca">joguina</skos:prefLabel>
      <rdakit:toolkitLabel xml:lang="ca">joguina</rdakit:toolkitLabel>
      <skos:definition xml:lang="ca">Unitat d’extensió que consisteix en un objecte concebut amb finalitat educativa, d’entreteniment o de motivació per mitjà del joc.</skos:definition>
      <rdakit:toolkitDefinition xml:lang="ca">Unitat d’extensió que consisteix en un objecte concebut amb finalitat educativa, d’entreteniment o de motivació per mitjà del joc.</rdakit:toolkitDefinition>
      <skos:scopeNote xml:lang="ca">Aquest terme s'aplica a formes tridimensionals.</skos:scopeNote>
      <skos:prefLabel xml:lang="vi">đồ chơi</skos:prefLabel>
      <rdakit:toolkitLabel xml:lang="vi">đồ chơi</rdakit:toolkitLabel>
      <skos:definition xml:lang="vi">Đơn vị của quy mô là vật thể được thiết kế cho giáo dục, giải trí, hoặc kích thích qua chơi.</skos:definition>
      <rdakit:toolkitDefinition xml:lang="vi">Đơn vị của quy mô là vật thể được thiết kế cho giáo dục, giải trí, hoặc kích thích qua chơi.</rdakit:toolkitDefinition>
      <skos:scopeNote xml:lang="vi">Thuật ngữ này áp dụng cho hình thái ba chiều.</skos:scopeNote>
      <skos:prefLabel xml:lang="de">Spielzeug</skos:prefLabel>
      <rdakit:toolkitLabel xml:lang="de">Spielzeug</rdakit:toolkitLabel>
      <skos:definition xml:lang="de">Eine Einheit für den Umfang, bestehend aus einem Gegenstand, der für die spielerische Bildung, Unterhaltung oder Stimulation konzipiert ist.</skos:definition>
      <rdakit:toolkitDefinition xml:lang="de">Eine Einheit für den Umfang, bestehend aus einem Gegenstand, der für die spielerische Bildung, Unterhaltung oder Stimulation konzipiert ist.</rdakit:toolkitDefinition>
      <skos:scopeNote xml:lang="de">Dieser Terminus trifft auf dreidimensionale Formen zu.</skos:scopeNote>
      <skos:prefLabel xml:lang="fi">lelu</skos:prefLabel>
      <rdakit:toolkitLabel xml:lang="fi">lelu</rdakit:toolkitLabel>
      <skos:definition xml:lang="fi">Laajuuden yksikkö, objekti, joka on suunniteltu opetusta, huvia tai leikkiä varten.</skos:definition>
      <rdakit:toolkitDefinition xml:lang="fi">Laajuuden yksikkö, objekti, joka on suunniteltu opetusta, huvia tai leikkiä varten.</rdakit:toolkitDefinition>
      <skos:scopeNote xml:lang="fi">Termi koskee kolmiulotteisia muotoja.</skos:scopeNote>
      <skos:altLabel xml:lang="da">legetøj</skos:altLabel>
      <rdakit:toolkitLabel xml:lang="da">legetøj</rdakit:toolkitLabel>
      <skos:definition xml:lang="da">Enhed, der består af en genstand, der er skabt til undervisnings-, underholdnings- eller stimuleringsbrug gennem leg.</skos:definition>
      <rdakit:toolkitDefinition xml:lang="da">Enhed, der består af en genstand, der er skabt til undervisnings-, underholdnings- eller stimuleringsbrug gennem leg.</rdakit:toolkitDefinition>
      <skos:scopeNote xml:lang="da">Denne term anvendes for tredimensionelle former.</skos:scopeNote>
      <skos:prefLabel xml:lang="fr">jouet</skos:prefLabel>
      <rdakit:toolkitLabel xml:lang="fr">jouet</rdakit:toolkitLabel>
      <skos:definition xml:lang="fr">Unité d’importance matérielle qui consiste en un objet conçu à des fins éducatives, de divertissement ou de stimulation par le jeu.</skos:definition>
      <rdakit:toolkitDefinition xml:lang="fr">Unité d’importance matérielle qui consiste en un objet conçu à des fins éducatives, de divertissement ou de stimulation par le jeu.</rdakit:toolkitDefinition>
      <skos:prefLabel xml:lang="no">leke</skos:prefLabel>
      <rdakit:toolkitLabel xml:lang="no">leke</rdakit:toolkitLabel>
      <skos:definition xml:lang="no">En omfangsenhet som består av en gjenstand som er laget for å lekes med og som har som mål å stimulere, underholde eller opplyse brukeren.</skos:definition>
      <rdakit:toolkitDefinition xml:lang="no">En omfangsenhet som består av en gjenstand som er laget for å lekes med og som har som mål å stimulere, underholde eller opplyse brukeren.</rdakit:toolkitDefinition>
      <skos:scopeNote xml:lang="no">Dette begrepet gjelder tredimensjonale former.</skos:scopeNote>
    </skos:Concept>
<!-- Concept: view  -->
    <skos:Concept rdf:about="http://rdaregistry.info/termList/RDACarrierEU/1040" xml:lang="en">
      <skos:inScheme rdf:resource="http://rdaregistry.info/termList/RDACarrierEU"/>
      <reg:status rdf:resource="http://metadataregistry.org/uri/RegStatus/1001"/>
      <reg:identifier rdf:resource="http://metadataregistry.org/concepts/8662"/>
      <skos:prefLabel xml:lang="en">view</skos:prefLabel>
      <rdakit:toolkitLabel xml:lang="en">view</rdakit:toolkitLabel>
      <skos:definition xml:lang="en">A unit of extent that is a perspective representation of the landscape in which detail is shown as if projected on an oblique plane.</skos:definition>
      <rdakit:toolkitDefinition xml:lang="en">A unit of extent that is a perspective representation of the landscape in which detail is shown as if projected on an oblique plane.</rdakit:toolkitDefinition>
      <skos:scopeNote xml:lang="en">This term applies to cartographic resources. A bird’s-eye view, panorama, panoramic drawing, worm’s-eye view, etc., are included.</skos:scopeNote>
      <skos:prefLabel xml:lang="ca">vista</skos:prefLabel>
      <rdakit:toolkitLabel xml:lang="ca">vista</rdakit:toolkitLabel>
      <skos:definition xml:lang="ca">Unitat d’extensió que és una representació amb perspectiva d’un paisatge en la qual es mostra el detall com si es projectés en un pla oblic.</skos:definition>
      <rdakit:toolkitDefinition xml:lang="ca">Unitat d’extensió que és una representació amb perspectiva d’un paisatge en la qual es mostra el detall com si es projectés en un pla oblic.</rdakit:toolkitDefinition>
      <skos:scopeNote xml:lang="ca">Aquest terme s’aplica a recursos cartogràfics. Inclou una vista a vol d’ocell, una panoràmica, un dibuix panoràmic, una vista des d’un pla inferior, etc.</skos:scopeNote>
      <skos:prefLabel xml:lang="vi">quang cảnh</skos:prefLabel>
      <rdakit:toolkitLabel xml:lang="vi">quang cảnh</rdakit:toolkitLabel>
      <skos:definition xml:lang="vi">Đơn vị của quy mô là trình bày phối cảnh của cảnh quan trong đó chi tiết được hiển thị như thể được chiếu trên một mặt xiên.</skos:definition>
      <rdakit:toolkitDefinition xml:lang="vi">Đơn vị của quy mô là trình bày phối cảnh của cảnh quan trong đó chi tiết được hiển thị như thể được chiếu trên một mặt xiên.</rdakit:toolkitDefinition>
      <skos:scopeNote xml:lang="vi">Thuật ngữ này áp dụng cho tài nguyên bản đồ. Quang cảnh nhìn từ trên xuống, toàn cảnh, vẽ toàn cảnh, quang cảnh nhìn từ dưới lên, được bao gồm.</skos:scopeNote>
      <skos:prefLabel xml:lang="de">Ansicht</skos:prefLabel>
      <rdakit:toolkitLabel xml:lang="de">Ansicht</rdakit:toolkitLabel>
      <skos:definition xml:lang="de">Eine Einheit für den Umfang einer perspektivische Darstellung der Landschaft, in der Einzelheiten wie auf eine schräge Ebene projiziert dargestellt sind.</skos:definition>
      <rdakit:toolkitDefinition xml:lang="de">Eine Einheit für den Umfang einer perspektivische Darstellung der Landschaft, in der Einzelheiten wie auf eine schräge Ebene projiziert dargestellt sind.</rdakit:toolkitDefinition>
      <skos:scopeNote xml:lang="de">Dieser Terminus trifft auf kartografische Ressource zu. Dazu gehört die Vogelperspektive, das Panorama, die Panorama-Zeichnung, die Froschperspektive usw.</skos:scopeNote>
      <skos:prefLabel xml:lang="fi">näkymäkartta</skos:prefLabel>
      <rdakit:toolkitLabel xml:lang="fi">näkymäkartta</rdakit:toolkitLabel>
      <skos:definition xml:lang="fi">Laajuuden yksikkö, perspektiivinäkymänä esitetty kartta-aineisto, jossa yksityiskohdat on esitetty kuin ne näkyisivät vinolta tasolta katsottuna.</skos:definition>
      <rdakit:toolkitDefinition xml:lang="fi">Laajuuden yksikkö, perspektiivinäkymänä esitetty kartta-aineisto, jossa yksityiskohdat on esitetty kuin ne näkyisivät vinolta tasolta katsottuna.</rdakit:toolkitDefinition>
      <skos:scopeNote xml:lang="fi">Termi koskee kartta-aineistoja. Sisältää mm. lintuperspektiivi, panoraama, panoraamapiirustus, sammakkoperspektiivi.</skos:scopeNote>
      <skos:altLabel xml:lang="da">perspektiv</skos:altLabel>
      <rdakit:toolkitLabel xml:lang="da">perspektiv</rdakit:toolkitLabel>
      <skos:definition xml:lang="da">Enhed, der er en perspektivisk repræsentation af landskabet, hvor en detalje vises, som om den bliver projiceret op på et skråt plan.</skos:definition>
      <rdakit:toolkitDefinition xml:lang="da">Enhed, der er en perspektivisk repræsentation af landskabet, hvor en detalje vises, som om den bliver projiceret op på et skråt plan.</rdakit:toolkitDefinition>
      <skos:scopeNote xml:lang="da">Denne term anvendes for kartografiske ressourcer. Et fugleperspektiv, et panorama, en panoramategning, et frøperspektiv er omfattet.</skos:scopeNote>
      <skos:prefLabel xml:lang="fr">vue</skos:prefLabel>
      <rdakit:toolkitLabel xml:lang="fr">vue</rdakit:toolkitLabel>
      <skos:definition xml:lang="fr">Unité d’importance matérielle qui consiste en une représentation en perspective du paysage dans laquelle les détails sont montrés en projection sur un plan oblique.</skos:definition>
      <rdakit:toolkitDefinition xml:lang="fr">Unité d’importance matérielle qui consiste en une représentation en perspective du paysage dans laquelle les détails sont montrés en projection sur un plan oblique.</rdakit:toolkitDefinition>
      <skos:prefLabel xml:lang="no">perspektiv</skos:prefLabel>
      <rdakit:toolkitLabel xml:lang="no">perspektiv</rdakit:toolkitLabel>
      <skos:definition xml:lang="no">En omfangsenhet som er en geografisk fremstilling av landskapet, der detaljene vises som om de er projisert på et skrått plan.</skos:definition>
      <rdakit:toolkitDefinition xml:lang="no">En omfangsenhet som er en geografisk fremstilling av landskapet, der detaljene vises som om de er projisert på et skrått plan.</rdakit:toolkitDefinition>
      <skos:scopeNote xml:lang="no">Dette begrepet gjelder kartografiske ressurser. Fugleperspektiv, panorama, panoramisk tegning, froskeperspektiv, etc. er inkludert.</skos:scopeNote>
    </skos:Concept>
<!-- Concept: wall chart  -->
    <skos:Concept rdf:about="http://rdaregistry.info/termList/RDACarrierEU/1041" xml:lang="en">
      <skos:inScheme rdf:resource="http://rdaregistry.info/termList/RDACarrierEU"/>
      <reg:status rdf:resource="http://metadataregistry.org/uri/RegStatus/1001"/>
      <reg:identifier rdf:resource="http://metadataregistry.org/concepts/8663"/>
      <skos:prefLabel xml:lang="en">wall chart</skos:prefLabel>
      <rdakit:toolkitLabel xml:lang="en">wall chart</rdakit:toolkitLabel>
      <skos:definition xml:lang="en">A unit of extent consisting of a tabular or graphic representation of data appropriate for display on a wall.</skos:definition>
      <rdakit:toolkitDefinition xml:lang="en">A unit of extent consisting of a tabular or graphic representation of data appropriate for display on a wall.</rdakit:toolkitDefinition>
      <skos:scopeNote xml:lang="en">This term applies to still images.</skos:scopeNote>
      <skos:prefLabel xml:lang="ca">panel mural</skos:prefLabel>
      <rdakit:toolkitLabel xml:lang="ca">panel mural</rdakit:toolkitLabel>
      <skos:definition xml:lang="ca">Unitat d’extensió que consisteix en una representació de les dades en forma tabular o gràfica i apropiada perquè es visualitzi en una paret.</skos:definition>
      <rdakit:toolkitDefinition xml:lang="ca">Unitat d’extensió que consisteix en una representació de les dades en forma tabular o gràfica i apropiada perquè es visualitzi en una paret.</rdakit:toolkitDefinition>
      <skos:scopeNote xml:lang="ca">Aquest terme s'aplica a imatges fixes.</skos:scopeNote>
      <skos:prefLabel xml:lang="vi">biểu đồ tường</skos:prefLabel>
      <rdakit:toolkitLabel xml:lang="vi">biểu đồ tường</rdakit:toolkitLabel>
      <skos:definition xml:lang="vi">Đơn vịcủa quy mô gồm cóhìnhảnhtĩnhbao gồm một bảng hoặctrình bàyđồ hoạ của dữ liệu thích hợp để hiển thị trên tường.</skos:definition>
      <rdakit:toolkitDefinition xml:lang="vi">Đơn vịcủa quy mô gồm cóhìnhảnhtĩnhbao gồm một bảng hoặctrình bàyđồ hoạ của dữ liệu thích hợp để hiển thị trên tường.</rdakit:toolkitDefinition>
      <skos:scopeNote xml:lang="vi">Thuật ngữ này áp dụng cho hình ảnh tĩnh.</skos:scopeNote>
      <skos:prefLabel xml:lang="de">Schautafel</skos:prefLabel>
      <rdakit:toolkitLabel xml:lang="de">Schautafel</rdakit:toolkitLabel>
      <skos:definition xml:lang="de">Eine Einheit für den Umfang, bestehend aus einer tabellarischen oder grafischen Repräsentation von Daten, die für die Anzeige an einer Wand geeignet ist.</skos:definition>
      <rdakit:toolkitDefinition xml:lang="de">Eine Einheit für den Umfang, bestehend aus einer tabellarischen oder grafischen Repräsentation von Daten, die für die Anzeige an einer Wand geeignet ist.</rdakit:toolkitDefinition>
      <skos:scopeNote xml:lang="de">Dieser Terminus trifft auf unbewegte Bilder zu.</skos:scopeNote>
      <skos:prefLabel xml:lang="fi">opetustaulu</skos:prefLabel>
      <rdakit:toolkitLabel xml:lang="fi">opetustaulu</rdakit:toolkitLabel>
      <skos:definition xml:lang="fi">Laajuuden yksikkö, liikkumaton kuva joka koostuu taulukkona tai muuna grafiikkana esitetystä datasta ja joka voidaan ripustaa seinälle.</skos:definition>
      <rdakit:toolkitDefinition xml:lang="fi">Laajuuden yksikkö, liikkumaton kuva joka koostuu taulukkona tai muuna grafiikkana esitetystä datasta ja joka voidaan ripustaa seinälle.</rdakit:toolkitDefinition>
      <skos:scopeNote xml:lang="fi">Termi koskee stillkuvia.</skos:scopeNote>
      <skos:altLabel xml:lang="da">vægplanche</skos:altLabel>
      <rdakit:toolkitLabel xml:lang="da">vægplanche</rdakit:toolkitLabel>
      <skos:definition xml:lang="da">Enhed, der består af en tabelbaseret eller grafisk repræsentation af data, der egner sig til at blive hængt op på en væg.</skos:definition>
      <rdakit:toolkitDefinition xml:lang="da">Enhed, der består af en tabelbaseret eller grafisk repræsentation af data, der egner sig til at blive hængt op på en væg.</rdakit:toolkitDefinition>
      <skos:scopeNote xml:lang="da">Denne term anvendes for faste billeder.</skos:scopeNote>
      <skos:prefLabel xml:lang="fr">panneau mural</skos:prefLabel>
      <rdakit:toolkitLabel xml:lang="fr">panneau mural</rdakit:toolkitLabel>
      <skos:definition xml:lang="fr">Unité d’importance matérielle qui consiste en une représentation de données, sous la forme de tableaux ou de graphiques, appropriée pour l’affichage mural.</skos:definition>
      <rdakit:toolkitDefinition xml:lang="fr">Unité d’importance matérielle qui consiste en une représentation de données, sous la forme de tableaux ou de graphiques, appropriée pour l’affichage mural.</rdakit:toolkitDefinition>
      <skos:prefLabel xml:lang="no">veggplansje</skos:prefLabel>
      <rdakit:toolkitLabel xml:lang="no">veggplansje</rdakit:toolkitLabel>
      <skos:definition xml:lang="no">En omfangsenhet som består av en representasjon av data i grafisk form eller tabellform egnet for visning på vegg.</skos:definition>
      <rdakit:toolkitDefinition xml:lang="no">En omfangsenhet som består av en representasjon av data i grafisk form eller tabellform egnet for visning på vegg.</rdakit:toolkitDefinition>
      <skos:scopeNote xml:lang="no">Dette begrepet gjelder stillbilder.</skos:scopeNote>
    </skos:Concept>

<!-- Status properties used in this document  -->
    <skos:Concept rdf:about="http://metadataregistry.org/uri/RegStatus/1001">
        <skos:prefLabel xml:lang="en">Published</skos:prefLabel>
    </skos:Concept>

</rdf:RDF>
