<?xml version="1.0" encoding = "UTF-8"?>
<rdf:RDF
    xmlns:dc="http://purl.org/dc/elements/1.1/"
    xmlns:rdakit="http://metadataregistry.org/uri/profile/rdakit/"
    xmlns:rdf="http://www.w3.org/1999/02/22-rdf-syntax-ns#"
    xmlns:reg="http://metadataregistry.org/uri/profile/regap/"
    xmlns:owl="http://www.w3.org/2002/07/owl#"
    xmlns:skos="http://www.w3.org/2004/02/skos/core#">

<owl:Ontology rdf:about="http://rdaregistry.info/termList/RDAGeneration" />
<!-- Scheme: RDA Generation -->
    <skos:ConceptScheme rdf:about="http://rdaregistry.info/termList/RDAGeneration">
        <dc:title>RDA Generation</dc:title>
    </skos:ConceptScheme>

<!-- Concept: derivative master  -->
    <skos:Concept rdf:about="http://rdaregistry.info/termList/RDAGeneration/1001" xml:lang="en">
      <skos:inScheme rdf:resource="http://rdaregistry.info/termList/RDAGeneration"/>
      <reg:status rdf:resource="http://metadataregistry.org/uri/RegStatus/1001"/>
      <reg:identifier rdf:resource="http://metadataregistry.org/concepts/8418"/>
      <skos:prefLabel xml:lang="en">derivative master</skos:prefLabel>
      <rdakit:toolkitLabel xml:lang="en">derivative master</rdakit:toolkitLabel>
      <skos:definition xml:lang="en">A generation that is derived from the master.</skos:definition>
      <rdakit:toolkitDefinition xml:lang="en">A generation that is derived from the master.</rdakit:toolkitDefinition>
      <skos:scopeNote xml:lang="en">This term applies to digital resources.</skos:scopeNote>
	    <skos:related rdf:resource="http://rdaregistry.info/termList/RDAGeneration/1005"/>
      <skos:prefLabel xml:lang="de">Derivative Master</skos:prefLabel>
      <rdakit:toolkitLabel xml:lang="de">Derivative Master</rdakit:toolkitLabel>
      <skos:definition xml:lang="de">Eine Kopiengeneration die vom Master abgeleitet ist.</skos:definition>
      <rdakit:toolkitDefinition xml:lang="de">Eine Kopiengeneration die vom Master abgeleitet ist.</rdakit:toolkitDefinition>
      <skos:scopeNote xml:lang="de">Dieser Terminus bezieht sich auf digitalen Ressourcen.</skos:scopeNote>
      <skos:prefLabel xml:lang="vi">bản gốc dẫn xuất</skos:prefLabel>
      <rdakit:toolkitLabel xml:lang="vi">bản gốc dẫn xuất</rdakit:toolkitLabel>
      <skos:definition xml:lang="vi">Thế hệ bắt nguồn từ bản gốc.</skos:definition>
      <rdakit:toolkitDefinition xml:lang="vi">Thế hệ bắt nguồn từ bản gốc.</rdakit:toolkitDefinition>
      <skos:scopeNote xml:lang="vi">Thuật ngữ này áp dụng cho tài nguyên số.</skos:scopeNote>
      <skos:prefLabel xml:lang="fi">johdannaismaster</skos:prefLabel>
      <rdakit:toolkitLabel xml:lang="fi">johdannaismaster</rdakit:toolkitLabel>
      <skos:definition xml:lang="fi">Alkuperäisen tallenteen ja siihen perustuvan kopion välinen suhde.</skos:definition>
      <rdakit:toolkitDefinition xml:lang="fi">Alkuperäisen tallenteen ja siihen perustuvan kopion välinen suhde.</rdakit:toolkitDefinition>
      <skos:scopeNote xml:lang="fi">Termi koskee digitaalista aineistoa.</skos:scopeNote>
      <skos:prefLabel xml:lang="da">afledt master</skos:prefLabel>
      <rdakit:toolkitLabel xml:lang="da">afledt master</rdakit:toolkitLabel>
      <skos:definition xml:lang="da">Generation af digital ressource, der er afledt fra masteren.</skos:definition>
      <rdakit:toolkitDefinition xml:lang="da">Generation af digital ressource, der er afledt fra masteren.</rdakit:toolkitDefinition>
      <skos:scopeNote xml:lang="da">Denne term anvendes for digitale ressourcer.</skos:scopeNote>
      <skos:prefLabel xml:lang="fr">matrice de dérivation</skos:prefLabel>
      <rdakit:toolkitLabel xml:lang="fr">matrice de dérivation</rdakit:toolkitLabel>
      <skos:definition xml:lang="fr">Génération qui est dérivée de la matrice.</skos:definition>
      <rdakit:toolkitDefinition xml:lang="fr">Génération qui est dérivée de la matrice.</rdakit:toolkitDefinition>
      <skos:scopeNote xml:lang="fr">Ce terme s’applique aux ressources numériques.</skos:scopeNote>
      <skos:prefLabel xml:lang="no">avledet master</skos:prefLabel>
      <rdakit:toolkitLabel xml:lang="no">avledet master</rdakit:toolkitLabel>
      <skos:definition xml:lang="no">En generasjon som er avledet fra masteren.</skos:definition>
      <rdakit:toolkitDefinition xml:lang="no">En generasjon som er avledet fra masteren.</rdakit:toolkitDefinition>
      <skos:scopeNote xml:lang="no">Dette begrepet gjelder digitale ressurser.</skos:scopeNote>
    </skos:Concept>
<!-- Concept: disc master  -->
    <skos:Concept rdf:about="http://rdaregistry.info/termList/RDAGeneration/1002" xml:lang="en">
      <skos:inScheme rdf:resource="http://rdaregistry.info/termList/RDAGeneration"/>
      <reg:status rdf:resource="http://metadataregistry.org/uri/RegStatus/1001"/>
      <reg:identifier rdf:resource="http://metadataregistry.org/concepts/8419"/>
      <skos:prefLabel xml:lang="en">disc master</skos:prefLabel>
      <rdakit:toolkitLabel xml:lang="en">disc master</rdakit:toolkitLabel>
      <skos:definition xml:lang="en">A generation that is a negative metal copy of a recording cut typically onto a lacquer-coated disc by means of a disc lathe; the lacquer original is destroyed in the process.</skos:definition>
      <rdakit:toolkitDefinition xml:lang="en">A generation that is a negative metal copy of a recording cut typically onto a lacquer-coated disc by means of a disc lathe; the lacquer original is destroyed in the process.</rdakit:toolkitDefinition>
      <skos:scopeNote xml:lang="en">This term applies to audio resources.</skos:scopeNote>
      <skos:prefLabel xml:lang="de">Disk-Master</skos:prefLabel>
      <rdakit:toolkitLabel xml:lang="de">Disk-Master</rdakit:toolkitLabel>
      <skos:definition xml:lang="de">Eine Kopiengeneration für eine negative Metallkopie eines Aufnahme-Schnitts mithilfe einer Drehmaschine (typischerweise) auf einer mit Lack beschichteten Platte. Das Lack-Original wird bei diesem Vorgang zerstört.</skos:definition>
      <rdakit:toolkitDefinition xml:lang="de">Eine Kopiengeneration für eine negative Metallkopie eines Aufnahme-Schnitts mithilfe einer Drehmaschine (typischerweise) auf einer mit Lack beschichteten Platte. Das Lack-Original wird bei diesem Vorgang zerstört.</rdakit:toolkitDefinition>
      <skos:scopeNote xml:lang="de">Dieser Terminus bezieht sich auf Audioressourcen.</skos:scopeNote>
      <skos:prefLabel xml:lang="vi">đĩa chủ</skos:prefLabel>
      <rdakit:toolkitLabel xml:lang="vi">đĩa chủ</rdakit:toolkitLabel>
      <skos:definition xml:lang="vi">Thế hệlà bản sao kim loại củabản ghiâmthường được chiếuvàomột đĩabọclaquer bằng phương tiệnchuyên dụng;nguyêngốc laquer bị phá huỷ trong quá trình này.</skos:definition>
      <rdakit:toolkitDefinition xml:lang="vi">Thế hệlà bản sao kim loại củabản ghiâmthường được chiếuvàomột đĩabọclaquer bằng phương tiệnchuyên dụng;nguyêngốc laquer bị phá huỷ trong quá trình này.</rdakit:toolkitDefinition>
      <skos:scopeNote xml:lang="vi">Thuật ngữ này áp dụng cho tài nguyên audio.</skos:scopeNote>
      <skos:prefLabel xml:lang="fi">originaalilevy</skos:prefLabel>
      <rdakit:toolkitLabel xml:lang="fi">originaalilevy</rdakit:toolkitLabel>
      <skos:definition xml:lang="fi">Äänitteen sukupolven määrite tallenteen negatiiviselle metallikopiolle, joka on kaiverrettu lakkapäällysteiselle levylle levysorvin avulla.</skos:definition>
      <rdakit:toolkitDefinition xml:lang="fi">Äänitteen sukupolven määrite tallenteen negatiiviselle metallikopiolle, joka on kaiverrettu lakkapäällysteiselle levylle levysorvin avulla.</rdakit:toolkitDefinition>
      <skos:prefLabel xml:lang="da">disc master</skos:prefLabel>
      <rdakit:toolkitLabel xml:lang="da">disc master</rdakit:toolkitLabel>
      <skos:definition xml:lang="da">Generation, der består af en negativ metalkopi af en optagelse, der (typisk) er skåret på en lakbelagt disc vha. en discdrejebænk; lakoriginalen ødelægges under processen.</skos:definition>
      <rdakit:toolkitDefinition xml:lang="da">Generation, der består af en negativ metalkopi af en optagelse, der (typisk) er skåret på en lakbelagt disc vha. en discdrejebænk; lakoriginalen ødelægges under processen.</rdakit:toolkitDefinition>
      <skos:scopeNote xml:lang="da">Denne term anvendes for lydressourcer.</skos:scopeNote>
      <skos:prefLabel xml:lang="fr">père</skos:prefLabel>
      <rdakit:toolkitLabel xml:lang="fr">père</rdakit:toolkitLabel>
      <skos:definition xml:lang="fr">Génération qui consiste en une copie négative en métal, généralement gravée à l’aide d’un tour à graver sur un disque enduit de laque ; le processus détruit l’original en laque.</skos:definition>
      <rdakit:toolkitDefinition xml:lang="fr">Génération qui consiste en une copie négative en métal, généralement gravée à l’aide d’un tour à graver sur un disque enduit de laque ; le processus détruit l’original en laque.</rdakit:toolkitDefinition>
      <skos:scopeNote xml:lang="fr">Ce terme s’applique aux ressources audio.</skos:scopeNote>
      <skos:prefLabel xml:lang="no">platemaster</skos:prefLabel>
      <rdakit:toolkitLabel xml:lang="no">platemaster</rdakit:toolkitLabel>
      <skos:definition xml:lang="no">En generasjon som består av en negativ metallkopi av et opptak som vanligvis er gravert inn i en plate dekket med skjellakk. Lakkoriginalen blir ødelagt i denne produksjonsprosessen.</skos:definition>
      <rdakit:toolkitDefinition xml:lang="no">En generasjon som består av en negativ metallkopi av et opptak som vanligvis er gravert inn i en plate dekket med skjellakk. Lakkoriginalen blir ødelagt i denne produksjonsprosessen.</rdakit:toolkitDefinition>
      <skos:scopeNote xml:lang="no">Dette begrepet gjelder lydressurser.</skos:scopeNote>
    </skos:Concept>
<!-- Concept: duplicate  -->
    <skos:Concept rdf:about="http://rdaregistry.info/termList/RDAGeneration/1003" xml:lang="en">
      <skos:inScheme rdf:resource="http://rdaregistry.info/termList/RDAGeneration"/>
      <reg:status rdf:resource="http://metadataregistry.org/uri/RegStatus/1001"/>
      <reg:identifier rdf:resource="http://metadataregistry.org/concepts/8420"/>
      <skos:prefLabel xml:lang="en">duplicate</skos:prefLabel>
      <skos:altLabel xml:lang="en">duplicate negative</skos:altLabel>
      <rdakit:toolkitLabel xml:lang="en">duplicate</rdakit:toolkitLabel>
      <skos:definition xml:lang="en">A generation that is a reproduction, usually with negative polarity, of the original picture or sound track, where a duplicate negative is made from a master positive, which in turn was made from an earlier negative.</skos:definition>
      <rdakit:toolkitDefinition xml:lang="en">A generation that is a reproduction, usually with negative polarity, of the original picture or sound track, where a duplicate negative is made from a master positive, which in turn was made from an earlier negative.</rdakit:toolkitDefinition>
      <skos:scopeNote xml:lang="en">This term applies to motion picture resources.</skos:scopeNote>
      <skos:prefLabel xml:lang="de">Duplikat</skos:prefLabel>
      <rdakit:toolkitLabel xml:lang="de">Duplikat</rdakit:toolkitLabel>
      <skos:definition xml:lang="de">Eine Kopiengeneration für eine Reproduktion (meist mit einer negativen Polarität) der ursprünglichen Bild- oder Tonspur, bei der ein Duplikatnegativ anhand des Masterpositivs erstellt wurde, welches wiederum aus einem früheren Negativ hergestellt wurde.</skos:definition>
      <rdakit:toolkitDefinition xml:lang="de">Eine Kopiengeneration für eine Reproduktion (meist mit einer negativen Polarität) der ursprünglichen Bild- oder Tonspur, bei der ein Duplikatnegativ anhand des Masterpositivs erstellt wurde, welches wiederum aus einem früheren Negativ hergestellt wurde.</rdakit:toolkitDefinition>
      <skos:scopeNote xml:lang="de">Dieser Terminus bezieht sich auf Filme.</skos:scopeNote>
      <skos:prefLabel xml:lang="vi">bản sao</skos:prefLabel>
      <skos:altLabel xml:lang="vi">bản sao âm</skos:altLabel>
      <rdakit:toolkitLabel xml:lang="vi">bản sao</rdakit:toolkitLabel>
      <skos:definition xml:lang="vi">Thế hệ là bản sao, luôn luôn với phân cực âm, của bức tranh hoặc rãnh âm thanh nguyên gốc, nơi bản sao chép được tạo ra từ bản gốc dương được tạo ra từ bản âm trước nữa.</skos:definition>
      <rdakit:toolkitDefinition xml:lang="vi">Thế hệ là bản sao, luôn luôn với phân cực âm, của bức tranh hoặc rãnh âm thanh nguyên gốc, nơi bản sao chép được tạo ra từ bản gốc dương được tạo ra từ bản âm trước nữa.</rdakit:toolkitDefinition>
      <skos:scopeNote xml:lang="vi">Thuật ngữ này áp dụng cho tài nguyên phim điện ảnh.</skos:scopeNote>
      <skos:prefLabel xml:lang="fi">duplikaatti</skos:prefLabel>
      <rdakit:toolkitLabel xml:lang="fi">duplikaatti</rdakit:toolkitLabel>
      <skos:definition xml:lang="fi">Sukupolven määrite, joka on alkuperäisen kuvan tai ääniraidan jäljitelmä, tavallisesti negatiivisella polariteetilla, jossa negatiivinen duplikaatti on valmistettu master-positiivista, joka vuorostaan on valmistettu aiemmasta negatiivista.</skos:definition>
      <rdakit:toolkitDefinition xml:lang="fi">Sukupolven määrite, joka on alkuperäisen kuvan tai ääniraidan jäljitelmä, tavallisesti negatiivisella polariteetilla, jossa negatiivinen duplikaatti on valmistettu master-positiivista, joka vuorostaan on valmistettu aiemmasta negatiivista.</rdakit:toolkitDefinition>
      <skos:scopeNote xml:lang="fi">Termi koskee elokuvia.</skos:scopeNote>
      <skos:prefLabel xml:lang="da">duplikat</skos:prefLabel>
      <rdakit:toolkitLabel xml:lang="da">duplikat</rdakit:toolkitLabel>
      <skos:scopeNote xml:lang="da">Denne term anvendes for ressourcer med levende billeder.</skos:scopeNote>
      <skos:prefLabel xml:lang="fr">internégatif</skos:prefLabel>
      <skos:altLabel xml:lang="fr">contretype négatif</skos:altLabel>
      <rdakit:toolkitLabel xml:lang="fr">internégatif</rdakit:toolkitLabel>
      <skos:definition xml:lang="fr">Génération qui consiste en une reproduction, habituellement de polarité négative, de la piste visuelle ou sonore originale, où une copie négative est produite à partir d’un interpositif qui a lui-même été produit à partir d’un négatif antérieur.</skos:definition>
      <rdakit:toolkitDefinition xml:lang="fr">Génération qui consiste en une reproduction, habituellement de polarité négative, de la piste visuelle ou sonore originale, où une copie négative est produite à partir d’un interpositif qui a lui-même été produit à partir d’un négatif antérieur.</rdakit:toolkitDefinition>
      <skos:scopeNote xml:lang="fr">Ce terme s’applique aux ressources filmiques.</skos:scopeNote>
      <skos:altLabel xml:lang="fr">négatif intermédiaire</skos:altLabel>
      <skos:altLabel xml:lang="fr">contretype</skos:altLabel>
      <skos:prefLabel xml:lang="no">duplikat</skos:prefLabel>
      <skos:altLabel xml:lang="no">duplikatnegativ</skos:altLabel>
      <rdakit:toolkitLabel xml:lang="no">duplikat</rdakit:toolkitLabel>
      <skos:definition xml:lang="no">En generasjon som er en reproduksjon, vanligvis med negativ polaritet, av det opprinnelige bildet eller lydsporet, der et duplikatnegativ lages fra et masterpositiv, som igjen ble laget fra et tidligere negativ.</skos:definition>
      <rdakit:toolkitDefinition xml:lang="no">En generasjon som er en reproduksjon, vanligvis med negativ polaritet, av det opprinnelige bildet eller lydsporet, der et duplikatnegativ lages fra et masterpositiv, som igjen ble laget fra et tidligere negativ.</rdakit:toolkitDefinition>
      <skos:scopeNote xml:lang="no">Dette begrepet gjelder spillefilmressurser.</skos:scopeNote>
    </skos:Concept>
<!-- Concept: first generation  -->
    <skos:Concept rdf:about="http://rdaregistry.info/termList/RDAGeneration/1004" xml:lang="en">
      <skos:inScheme rdf:resource="http://rdaregistry.info/termList/RDAGeneration"/>
      <reg:status rdf:resource="http://metadataregistry.org/uri/RegStatus/1001"/>
      <reg:identifier rdf:resource="http://metadataregistry.org/concepts/8421"/>
      <skos:prefLabel xml:lang="en">first generation</skos:prefLabel>
      <skos:altLabel xml:lang="en">first-generation master</skos:altLabel>
      <rdakit:toolkitLabel xml:lang="en">first generation</rdakit:toolkitLabel>
      <skos:definition xml:lang="en">A generation that is the original camera film or videotape used to record the production.</skos:definition>
      <rdakit:toolkitDefinition xml:lang="en">A generation that is the original camera film or videotape used to record the production.</rdakit:toolkitDefinition>
      <skos:scopeNote xml:lang="en">This term applies to microform and video resources.</skos:scopeNote>
      <skos:prefLabel xml:lang="de">Erste Generation</skos:prefLabel>
      <skos:altLabel xml:lang="de">Master der ersten Generation</skos:altLabel>
      <rdakit:toolkitLabel xml:lang="de">Erste Generation</rdakit:toolkitLabel>
      <skos:definition xml:lang="de">Eine Kopiengeneration für den ursprünglichen Kamerafilm oder das ursprüngliche Videoband, welcher/welches für die Aufnahme der Produktion verwendet wurde.</skos:definition>
      <rdakit:toolkitDefinition xml:lang="de">Eine Kopiengeneration für den ursprünglichen Kamerafilm oder das ursprüngliche Videoband, welcher/welches für die Aufnahme der Produktion verwendet wurde.</rdakit:toolkitDefinition>
      <skos:scopeNote xml:lang="de">Dieser Terminus bezieht sich auf Mikroform- und Videoressourcen.</skos:scopeNote>
      <skos:altLabel xml:lang="de">Bestandserhaltungsmaster</skos:altLabel>
      <skos:prefLabel xml:lang="vi">thế hệ thứ nhất</skos:prefLabel>
      <skos:altLabel xml:lang="vi">thế hệ thứ nhất chủ</skos:altLabel>
      <rdakit:toolkitLabel xml:lang="vi">thế hệ thứ nhất</rdakit:toolkitLabel>
      <skos:definition xml:lang="vi">Thế hệlà phim máy ảnh hoặc băng video nguyên gốc được dùng để ghi tác phẩm</skos:definition>
      <rdakit:toolkitDefinition xml:lang="vi">Thế hệlà phim máy ảnh hoặc băng video nguyên gốc được dùng để ghi tác phẩm</rdakit:toolkitDefinition>
      <skos:scopeNote xml:lang="vi">Thuật ngữ này áp dụng cho tài nguyên vi dạng và video.</skos:scopeNote>
      <skos:prefLabel xml:lang="fi">ensimmäinen sukupolvi</skos:prefLabel>
      <skos:altLabel xml:lang="fi">ensimmäisen sukupolven masteri</skos:altLabel>
      <rdakit:toolkitLabel xml:lang="fi">ensimmäinen sukupolvi</rdakit:toolkitLabel>
      <skos:definition xml:lang="fi">Sukupolven määrite alkuperäiselle kamerafilmille tai videonauhalle, jolle aineisto on kuvattu.</skos:definition>
      <rdakit:toolkitDefinition xml:lang="fi">Sukupolven määrite alkuperäiselle kamerafilmille tai videonauhalle, jolle aineisto on kuvattu.</rdakit:toolkitDefinition>
      <skos:scopeNote xml:lang="fi">Termi koskee mikromuotoista aineistoa ja videoaineistoa.</skos:scopeNote>
      <skos:prefLabel xml:lang="da">førstegeneration</skos:prefLabel>
      <skos:altLabel xml:lang="da">førstegeneration master</skos:altLabel>
      <rdakit:toolkitLabel xml:lang="da">førstegeneration</rdakit:toolkitLabel>
      <skos:definition xml:lang="da">Generation, der består af den originale kamerafilm eller videobånd anvendt for at indspille produktionen.</skos:definition>
      <rdakit:toolkitDefinition xml:lang="da">Generation, der består af den originale kamerafilm eller videobånd anvendt for at indspille produktionen.</rdakit:toolkitDefinition>
      <skos:scopeNote xml:lang="da">Denne term anvendes for mikroform- og videoressourcer.</skos:scopeNote>
      <skos:prefLabel xml:lang="fr">première génération</skos:prefLabel>
      <rdakit:toolkitLabel xml:lang="fr">première génération</rdakit:toolkitLabel>
      <skos:definition xml:lang="fr">Génération qui consiste en la pellicule photographique ou en la bande vidéo originale utilisée pour enregistrer la production.</skos:definition>
      <rdakit:toolkitDefinition xml:lang="fr">Génération qui consiste en la pellicule photographique ou en la bande vidéo originale utilisée pour enregistrer la production.</rdakit:toolkitDefinition>
      <skos:scopeNote xml:lang="fr">Ce terme s’applique aux ressources sur microformes et aux ressources vidéo.</skos:scopeNote>
      <skos:prefLabel xml:lang="no">første generasjon</skos:prefLabel>
      <skos:altLabel xml:lang="no">førstegenerasjons master</skos:altLabel>
      <rdakit:toolkitLabel xml:lang="no">første generasjon</rdakit:toolkitLabel>
      <skos:definition xml:lang="no">En generasjon som er den opprinnelige kamerafilmen eller det opprinnelige videobåndet som ble brukt ved innspilling av produksjonen.</skos:definition>
      <rdakit:toolkitDefinition xml:lang="no">En generasjon som er den opprinnelige kamerafilmen eller det opprinnelige videobåndet som ble brukt ved innspilling av produksjonen.</rdakit:toolkitDefinition>
      <skos:scopeNote xml:lang="no">Dette begrepet gjelder mikroform- og videoressurser.</skos:scopeNote>
    </skos:Concept>
<!-- Concept: master  -->
    <skos:Concept rdf:about="http://rdaregistry.info/termList/RDAGeneration/1005" xml:lang="en">
      <skos:inScheme rdf:resource="http://rdaregistry.info/termList/RDAGeneration"/>
      <reg:status rdf:resource="http://metadataregistry.org/uri/RegStatus/1001"/>
      <reg:identifier rdf:resource="http://metadataregistry.org/concepts/8422"/>
      <skos:prefLabel xml:lang="en">master</skos:prefLabel>
      <rdakit:toolkitLabel xml:lang="en">master</rdakit:toolkitLabel>
      <skos:definition xml:lang="en">A generation that is created from the process of digitization at the highest resolution and often used to make derivative copies.</skos:definition>
      <rdakit:toolkitDefinition xml:lang="en">A generation that is created from the process of digitization at the highest resolution and often used to make derivative copies.</rdakit:toolkitDefinition>
      <skos:scopeNote xml:lang="en">This term applies to digital resources.</skos:scopeNote>
	    <skos:related rdf:resource="http://rdaregistry.info/termList/RDAGeneration/1009"/>
	    <skos:related rdf:resource="http://rdaregistry.info/termList/RDAGeneration/1001"/>
      <skos:prefLabel xml:lang="de">Master</skos:prefLabel>
      <rdakit:toolkitLabel xml:lang="de">Master</rdakit:toolkitLabel>
      <skos:definition xml:lang="de">Eine Kopiengeneration die beim Digitalisierungsprozess mit der höchsten Auflösung erzeugt wird und häufig verwendet wird, um davon abgeleitete Kopien zu machen.</skos:definition>
      <rdakit:toolkitDefinition xml:lang="de">Eine Kopiengeneration die beim Digitalisierungsprozess mit der höchsten Auflösung erzeugt wird und häufig verwendet wird, um davon abgeleitete Kopien zu machen.</rdakit:toolkitDefinition>
      <skos:scopeNote xml:lang="de">Dieser Terminus bezieht sich auf digitalen Ressourcen.</skos:scopeNote>
      <skos:prefLabel xml:lang="vi">chủ</skos:prefLabel>
      <rdakit:toolkitLabel xml:lang="vi">chủ</rdakit:toolkitLabel>
      <skos:definition xml:lang="vi">Thế hệ được sáng tạo từ quá trình số hoá ở độ phân giải cao và thường dùng để tạo các bản dẫn xuất</skos:definition>
      <rdakit:toolkitDefinition xml:lang="vi">Thế hệ được sáng tạo từ quá trình số hoá ở độ phân giải cao và thường dùng để tạo các bản dẫn xuất</rdakit:toolkitDefinition>
      <skos:scopeNote xml:lang="vi">Thuật ngữ này áp dụng cho tài nguyên số.</skos:scopeNote>
      <skos:prefLabel xml:lang="fi">masterkopio</skos:prefLabel>
      <rdakit:toolkitLabel xml:lang="fi">masterkopio</rdakit:toolkitLabel>
      <skos:definition xml:lang="fi">Sukupolven määrite digitaaliselle aineistolle, joka on luotu digitoimalla suurimmalla mahdollisella resoluutiolla ja jota usein käytetään kopioiden valmistamiseen.</skos:definition>
      <rdakit:toolkitDefinition xml:lang="fi">Sukupolven määrite digitaaliselle aineistolle, joka on luotu digitoimalla suurimmalla mahdollisella resoluutiolla ja jota usein käytetään kopioiden valmistamiseen.</rdakit:toolkitDefinition>
      <skos:scopeNote xml:lang="fi">Termi koskee digitaalista aineistoa.</skos:scopeNote>
      <skos:prefLabel xml:lang="da">master</skos:prefLabel>
      <rdakit:toolkitLabel xml:lang="da">master</rdakit:toolkitLabel>
      <skos:definition xml:lang="da">Generation af en digital ressource, der er skabt ved en digitaliseringsproces ved højeste opløsning og ofte anvendt til at lave afledte kopier.</skos:definition>
      <rdakit:toolkitDefinition xml:lang="da">Generation af en digital ressource, der er skabt ved en digitaliseringsproces ved højeste opløsning og ofte anvendt til at lave afledte kopier.</rdakit:toolkitDefinition>
      <skos:scopeNote xml:lang="da">Denne term anvendes for digitale ressourcer.</skos:scopeNote>
      <skos:prefLabel xml:lang="fr">matrice</skos:prefLabel>
      <rdakit:toolkitLabel xml:lang="fr">matrice</rdakit:toolkitLabel>
      <skos:definition xml:lang="fr">Génération qui est créée à la suite du processus de numérisation à la résolution maximale et souvent utilisée pour créer des copies dérivées.</skos:definition>
      <rdakit:toolkitDefinition xml:lang="fr">Génération qui est créée à la suite du processus de numérisation à la résolution maximale et souvent utilisée pour créer des copies dérivées.</rdakit:toolkitDefinition>
      <skos:scopeNote xml:lang="fr">Ce terme s’applique aux ressources numériques.</skos:scopeNote>
      <skos:prefLabel xml:lang="no">master</skos:prefLabel>
      <rdakit:toolkitLabel xml:lang="no">master</rdakit:toolkitLabel>
      <skos:definition xml:lang="no">En generasjon som skapes i digitaliseringsprosessen ved høyeste oppløsning og som ofte brukes til å lage avledede kopier.</skos:definition>
      <rdakit:toolkitDefinition xml:lang="no">En generasjon som skapes i digitaliseringsprosessen ved høyeste oppløsning og som ofte brukes til å lage avledede kopier.</rdakit:toolkitDefinition>
      <skos:scopeNote xml:lang="no">Dette begrepet gjelder digitale ressurser.</skos:scopeNote>
    </skos:Concept>
<!-- Concept: master positive  -->
    <skos:Concept rdf:about="http://rdaregistry.info/termList/RDAGeneration/1012" xml:lang="en">
      <skos:inScheme rdf:resource="http://rdaregistry.info/termList/RDAGeneration"/>
      <reg:status rdf:resource="http://metadataregistry.org/uri/RegStatus/1001"/>
      <reg:identifier rdf:resource="http://metadataregistry.org/concepts/8429"/>
      <skos:prefLabel xml:lang="en">master positive</skos:prefLabel>
      <rdakit:toolkitLabel xml:lang="en">master positive</rdakit:toolkitLabel>
      <skos:definition xml:lang="en">A generation that is a positive print made from an earlier generation negative film and used for the preparation of duplicate negatives rather than projection.</skos:definition>
      <rdakit:toolkitDefinition xml:lang="en">A generation that is a positive print made from an earlier generation negative film and used for the preparation of duplicate negatives rather than projection.</rdakit:toolkitDefinition>
      <skos:scopeNote xml:lang="en">This term applies to motion picture resources.</skos:scopeNote>
      <skos:prefLabel xml:lang="de">Masterpositiv</skos:prefLabel>
      <rdakit:toolkitLabel xml:lang="de">Masterpositiv</rdakit:toolkitLabel>
      <skos:definition xml:lang="de">Eine Kopiengeneration für einen Positivdruck, der aus einer früheren Negativdruckgeneration erstellt wird und anstelle von Projektionen verwendet wird, um Duplikatnegative zu erstellen.</skos:definition>
      <rdakit:toolkitDefinition xml:lang="de">Eine Kopiengeneration für einen Positivdruck, der aus einer früheren Negativdruckgeneration erstellt wird und anstelle von Projektionen verwendet wird, um Duplikatnegative zu erstellen.</rdakit:toolkitDefinition>
      <skos:scopeNote xml:lang="de">Dieser Terminus bezieht sich auf Filme.</skos:scopeNote>
      <skos:prefLabel xml:lang="vi">bản chủ dương</skos:prefLabel>
      <rdakit:toolkitLabel xml:lang="vi">bản chủ dương</rdakit:toolkitLabel>
      <skos:definition xml:lang="vi">Thế hệ là bản in dương được tạo ra từ phim thế hệ âm trước nữa và dùng để chuẩn bị cho các bản âm nhân sao hơn là để chiếu.</skos:definition>
      <rdakit:toolkitDefinition xml:lang="vi">Thế hệ là bản in dương được tạo ra từ phim thế hệ âm trước nữa và dùng để chuẩn bị cho các bản âm nhân sao hơn là để chiếu.</rdakit:toolkitDefinition>
      <skos:scopeNote xml:lang="vi">Thuật ngữ này áp dụng cho tài nguyên phim điện ảnh.</skos:scopeNote>
      <skos:prefLabel xml:lang="fi">master-positiivi</skos:prefLabel>
      <rdakit:toolkitLabel xml:lang="fi">master-positiivi</rdakit:toolkitLabel>
      <skos:definition xml:lang="fi">Sukupolven määrite, joka on aikaisemman sukupolven negatiivifilmistä valmistettu positiivivedos, ja jota käytetään negatiivikopioiden valmistamiseksi kuvien sijaan.</skos:definition>
      <rdakit:toolkitDefinition xml:lang="fi">Sukupolven määrite, joka on aikaisemman sukupolven negatiivifilmistä valmistettu positiivivedos, ja jota käytetään negatiivikopioiden valmistamiseksi kuvien sijaan.</rdakit:toolkitDefinition>
      <skos:scopeNote xml:lang="fi">Termi koskee elokuvia.</skos:scopeNote>
      <skos:prefLabel xml:lang="da">positiv master</skos:prefLabel>
      <rdakit:toolkitLabel xml:lang="da">positiv master</rdakit:toolkitLabel>
      <skos:definition xml:lang="da">Generation, der består af et positivt tryk skabt af en tidligere generation negativ film og der bruges til fremstilling af duplikat negativer frem for projektion.</skos:definition>
      <rdakit:toolkitDefinition xml:lang="da">Generation, der består af et positivt tryk skabt af en tidligere generation negativ film og der bruges til fremstilling af duplikat negativer frem for projektion.</rdakit:toolkitDefinition>
      <skos:scopeNote xml:lang="da">Denne term anvendes for ressourcer med levende billeder.</skos:scopeNote>
      <skos:prefLabel xml:lang="fr">interpositif</skos:prefLabel>
      <skos:altLabel xml:lang="fr">contretype positif</skos:altLabel>
      <rdakit:toolkitLabel xml:lang="fr">interpositif</rdakit:toolkitLabel>
      <skos:definition xml:lang="fr">Génération qui consiste en une copie positive produite à partir d’un négatif d’une génération antérieure et qui est utilisée pour préparer des internégatifs plutôt que pour la projection.</skos:definition>
      <rdakit:toolkitDefinition xml:lang="fr">Génération qui consiste en une copie positive produite à partir d’un négatif d’une génération antérieure et qui est utilisée pour préparer des internégatifs plutôt que pour la projection.</rdakit:toolkitDefinition>
      <skos:scopeNote xml:lang="fr">Ce terme s’applique aux ressources filmiques.</skos:scopeNote>
      <skos:altLabel xml:lang="fr">positif intermédiaire</skos:altLabel>
      <skos:prefLabel xml:lang="no">masterpositiv</skos:prefLabel>
      <rdakit:toolkitLabel xml:lang="no">masterpositiv</rdakit:toolkitLabel>
      <skos:definition xml:lang="no">En generasjon som er en positiv kopi laget av en tidligere generasjon med negativ film og som brukes til å klargjøre dupliserte negativer, ikke til fremvisning.</skos:definition>
      <rdakit:toolkitDefinition xml:lang="no">En generasjon som er en positiv kopi laget av en tidligere generasjon med negativ film og som brukes til å klargjøre dupliserte negativer, ikke til fremvisning.</rdakit:toolkitDefinition>
      <skos:scopeNote xml:lang="no">Dette begrepet gjelder spillefilmressurser.</skos:scopeNote>
    </skos:Concept>
<!-- Concept: master tape  -->
    <skos:Concept rdf:about="http://rdaregistry.info/termList/RDAGeneration/1006" xml:lang="en">
      <skos:inScheme rdf:resource="http://rdaregistry.info/termList/RDAGeneration"/>
      <reg:status rdf:resource="http://metadataregistry.org/uri/RegStatus/1001"/>
      <reg:identifier rdf:resource="http://metadataregistry.org/concepts/8423"/>
      <skos:prefLabel xml:lang="en">master tape</skos:prefLabel>
      <rdakit:toolkitLabel xml:lang="en">master tape</rdakit:toolkitLabel>
      <skos:definition xml:lang="en">A generation that is the original recorded version of a tape from which copies can be made.</skos:definition>
      <rdakit:toolkitDefinition xml:lang="en">A generation that is the original recorded version of a tape from which copies can be made.</rdakit:toolkitDefinition>
      <skos:scopeNote xml:lang="en">This term applies to audio resources.</skos:scopeNote>
      <skos:prefLabel xml:lang="de">Masterband</skos:prefLabel>
      <rdakit:toolkitLabel xml:lang="de">Masterband</rdakit:toolkitLabel>
      <skos:definition xml:lang="de">Eine Kopiengeneration für eine original aufgezeichnete Version eines Bandes, von dem Kopien gemacht werden können.</skos:definition>
      <rdakit:toolkitDefinition xml:lang="de">Eine Kopiengeneration für eine original aufgezeichnete Version eines Bandes, von dem Kopien gemacht werden können.</rdakit:toolkitDefinition>
      <skos:scopeNote xml:lang="de">Dieser Terminus bezieht sich auf Audioressourcen.</skos:scopeNote>
      <skos:prefLabel xml:lang="vi">băng chủ</skos:prefLabel>
      <rdakit:toolkitLabel xml:lang="vi">băng chủ</rdakit:toolkitLabel>
      <skos:definition xml:lang="vi">Thế hệlà phiên bản được ghi nguyên gốc của băng mà từ đó các bản sao có thể được tạo ra.</skos:definition>
      <rdakit:toolkitDefinition xml:lang="vi">Thế hệlà phiên bản được ghi nguyên gốc của băng mà từ đó các bản sao có thể được tạo ra.</rdakit:toolkitDefinition>
      <skos:scopeNote xml:lang="vi">Thuật ngữ này áp dụng cho tài nguyên audio.</skos:scopeNote>
      <skos:prefLabel xml:lang="fi">masternauha</skos:prefLabel>
      <rdakit:toolkitLabel xml:lang="fi">masternauha</rdakit:toolkitLabel>
      <skos:definition xml:lang="fi">Äänitteen sukupolven määrite nauhan alkuperäiselle äänitysversiolle, josta voidaan tehdä kopioita.</skos:definition>
      <rdakit:toolkitDefinition xml:lang="fi">Äänitteen sukupolven määrite nauhan alkuperäiselle äänitysversiolle, josta voidaan tehdä kopioita.</rdakit:toolkitDefinition>
      <skos:scopeNote xml:lang="fi">Termi koskee äänitteitä.</skos:scopeNote>
      <skos:prefLabel xml:lang="da">masterbånd</skos:prefLabel>
      <rdakit:toolkitLabel xml:lang="da">masterbånd</rdakit:toolkitLabel>
      <skos:definition xml:lang="da">Generation, der består af den oprindeligt indspillede version af et bånd, hvorfra kopier kan laves.</skos:definition>
      <rdakit:toolkitDefinition xml:lang="da">Generation, der består af den oprindeligt indspillede version af et bånd, hvorfra kopier kan laves.</rdakit:toolkitDefinition>
      <skos:scopeNote xml:lang="da">Denne term anvendes for lydressourcer.</skos:scopeNote>
      <skos:prefLabel xml:lang="fr">bande maîtresse</skos:prefLabel>
      <rdakit:toolkitLabel xml:lang="fr">bande maîtresse</rdakit:toolkitLabel>
      <skos:definition xml:lang="fr">Génération qui consiste en la version originale d’un enregistrement sur bande magnétique à partir de laquelle des copies peuvent être effectuées.</skos:definition>
      <rdakit:toolkitDefinition xml:lang="fr">Génération qui consiste en la version originale d’un enregistrement sur bande magnétique à partir de laquelle des copies peuvent être effectuées.</rdakit:toolkitDefinition>
      <skos:scopeNote xml:lang="fr">Ce terme s’applique aux ressources audio.</skos:scopeNote>
      <skos:prefLabel xml:lang="no">masterbånd</skos:prefLabel>
      <rdakit:toolkitLabel xml:lang="no">masterbånd</rdakit:toolkitLabel>
      <skos:definition xml:lang="no">En generasjon som er originalinnspillingen på bånd og som det kan lages kopier av.</skos:definition>
      <rdakit:toolkitDefinition xml:lang="no">En generasjon som er originalinnspillingen på bånd og som det kan lages kopier av.</rdakit:toolkitDefinition>
      <skos:scopeNote xml:lang="no">Dette begrepet gjelder lydressurser.</skos:scopeNote>
    </skos:Concept>
<!-- Concept: mixed generation  -->
    <skos:Concept rdf:about="http://rdaregistry.info/termList/RDAGeneration/1007" xml:lang="en">
      <skos:inScheme rdf:resource="http://rdaregistry.info/termList/RDAGeneration"/>
      <reg:status rdf:resource="http://metadataregistry.org/uri/RegStatus/1001"/>
      <reg:identifier rdf:resource="http://metadataregistry.org/concepts/8424"/>
      <skos:prefLabel xml:lang="en">mixed generation</skos:prefLabel>
      <rdakit:toolkitLabel xml:lang="en">mixed generation</rdakit:toolkitLabel>
      <skos:definition xml:lang="en">A generation that is a combination of generations for which it is not possible to assign more precise terms.</skos:definition>
      <rdakit:toolkitDefinition xml:lang="en">A generation that is a combination of generations for which it is not possible to assign more precise terms.</rdakit:toolkitDefinition>
      <skos:prefLabel xml:lang="de">Gemischte Generation</skos:prefLabel>
      <rdakit:toolkitLabel xml:lang="de">Gemischte Generation</rdakit:toolkitLabel>
      <skos:definition xml:lang="de">Eine Kopiengeneration für eine Kombination von Filmgenerationen, für die es nicht möglich ist, einen präziseren Terminus zu vergeben.</skos:definition>
      <rdakit:toolkitDefinition xml:lang="de">Eine Kopiengeneration für eine Kombination von Filmgenerationen, für die es nicht möglich ist, einen präziseren Terminus zu vergeben.</rdakit:toolkitDefinition>
      <skos:prefLabel xml:lang="vi">thế hệ hỗn hợp</skos:prefLabel>
      <rdakit:toolkitLabel xml:lang="vi">thế hệ hỗn hợp</rdakit:toolkitLabel>
      <skos:definition xml:lang="vi">Thế hệ là tổ hợp của các thế hệ mà không thể gán các thuật ngữ chính xác hơn.</skos:definition>
      <rdakit:toolkitDefinition xml:lang="vi">Thế hệ là tổ hợp của các thế hệ mà không thể gán các thuật ngữ chính xác hơn.</rdakit:toolkitDefinition>
      <skos:prefLabel xml:lang="fi">sukupolvien yhdistelmä</skos:prefLabel>
      <rdakit:toolkitLabel xml:lang="fi">sukupolvien yhdistelmä</rdakit:toolkitLabel>
      <skos:definition xml:lang="fi">Sukupolven määrite aineistolle, joka on eri sukupolvien yhdistelmä ja jota ei tästä syystä voida kuvata täsmällisemmällä termillä.</skos:definition>
      <rdakit:toolkitDefinition xml:lang="fi">Sukupolven määrite aineistolle, joka on eri sukupolvien yhdistelmä ja jota ei tästä syystä voida kuvata täsmällisemmällä termillä.</rdakit:toolkitDefinition>
      <skos:prefLabel xml:lang="da">blandet generation</skos:prefLabel>
      <rdakit:toolkitLabel xml:lang="da">blandet generation</rdakit:toolkitLabel>
      <skos:definition xml:lang="da">Generation, der består af en kombination af generationer af film, for hvilke det ikke er muligt at angive mere præcise termer.</skos:definition>
      <rdakit:toolkitDefinition xml:lang="da">Generation, der består af en kombination af generationer af film, for hvilke det ikke er muligt at angive mere præcise termer.</rdakit:toolkitDefinition>
      <skos:prefLabel xml:lang="fr">génération mixte</skos:prefLabel>
      <rdakit:toolkitLabel xml:lang="fr">génération mixte</rdakit:toolkitLabel>
      <skos:definition xml:lang="fr">Génération qui consiste en une combinaison de générations pour laquelle il n’est pas possible d’attribuer des termes plus précis.</skos:definition>
      <rdakit:toolkitDefinition xml:lang="fr">Génération qui consiste en une combinaison de générations pour laquelle il n’est pas possible d’attribuer des termes plus précis.</rdakit:toolkitDefinition>
      <skos:prefLabel xml:lang="no">blandet generasjon</skos:prefLabel>
      <rdakit:toolkitLabel xml:lang="no">blandet generasjon</rdakit:toolkitLabel>
      <skos:definition xml:lang="no">En generasjon som består av en kombinasjon av generasjoner som det det ikke er mulig å gi en mer presis betegnelse.</skos:definition>
      <rdakit:toolkitDefinition xml:lang="no">En generasjon som består av en kombinasjon av generasjoner som det det ikke er mulig å gi en mer presis betegnelse.</rdakit:toolkitDefinition>
    </skos:Concept>
<!-- Concept: mother  -->
    <skos:Concept rdf:about="http://rdaregistry.info/termList/RDAGeneration/1008" xml:lang="en">
      <skos:inScheme rdf:resource="http://rdaregistry.info/termList/RDAGeneration"/>
      <reg:status rdf:resource="http://metadataregistry.org/uri/RegStatus/1001"/>
      <reg:identifier rdf:resource="http://metadataregistry.org/concepts/8425"/>
      <skos:prefLabel xml:lang="en">mother</skos:prefLabel>
      <rdakit:toolkitLabel xml:lang="en">mother</rdakit:toolkitLabel>
      <skos:definition xml:lang="en">A generation that is a positive metal copy of a disc master used to create one or more stampers.</skos:definition>
      <rdakit:toolkitDefinition xml:lang="en">A generation that is a positive metal copy of a disc master used to create one or more stampers.</rdakit:toolkitDefinition>
      <skos:scopeNote xml:lang="en">This term applies to audio resources.</skos:scopeNote>
      <skos:prefLabel xml:lang="de">Mutterband</skos:prefLabel>
      <rdakit:toolkitLabel xml:lang="de">Mutterband</rdakit:toolkitLabel>
      <skos:definition xml:lang="de">Eine Kopiengeneration für eine positive Metallkopie eines Disk-Masters, die verwendet wird, um ein oder mehrere Matrizen zu erstellen.</skos:definition>
      <rdakit:toolkitDefinition xml:lang="de">Eine Kopiengeneration für eine positive Metallkopie eines Disk-Masters, die verwendet wird, um ein oder mehrere Matrizen zu erstellen.</rdakit:toolkitDefinition>
      <skos:scopeNote xml:lang="de">Dieser Terminus bezieht sich auf Audioressourcen.</skos:scopeNote>
      <skos:prefLabel xml:lang="vi">mẹ</skos:prefLabel>
      <rdakit:toolkitLabel xml:lang="vi">mẹ</rdakit:toolkitLabel>
      <skos:definition xml:lang="vi">Thế hệ là bản sao kim loại dương của đĩa gốc được dùng để tao ra một hoặc nhiều hơn dấu khắc.</skos:definition>
      <rdakit:toolkitDefinition xml:lang="vi">Thế hệ là bản sao kim loại dương của đĩa gốc được dùng để tao ra một hoặc nhiều hơn dấu khắc.</rdakit:toolkitDefinition>
      <skos:scopeNote xml:lang="vi">Thuật ngữ này áp dụng cho tài nguyên audio.</skos:scopeNote>
      <skos:prefLabel xml:lang="fi">äitiö</skos:prefLabel>
      <rdakit:toolkitLabel xml:lang="fi">äitiö</rdakit:toolkitLabel>
      <skos:definition xml:lang="fi">Äänitteen sukupolven määrite originaalilevyn positiiviselle metallikopiolle, jota on käytetty yhden tai useamman isiön tuottamiseen.</skos:definition>
      <rdakit:toolkitDefinition xml:lang="fi">Äänitteen sukupolven määrite originaalilevyn positiiviselle metallikopiolle, jota on käytetty yhden tai useamman isiön tuottamiseen.</rdakit:toolkitDefinition>
      <skos:scopeNote xml:lang="fi">Termi koskee äänitteitä.</skos:scopeNote>
      <skos:prefLabel xml:lang="da">matrice</skos:prefLabel>
      <rdakit:toolkitLabel xml:lang="da">matrice</rdakit:toolkitLabel>
      <skos:definition xml:lang="da">Generation, der består af en positiv metalkopi af en discmaster, der anvendes til at skabe en eller flere patricer.</skos:definition>
      <rdakit:toolkitDefinition xml:lang="da">Generation, der består af en positiv metalkopi af en discmaster, der anvendes til at skabe en eller flere patricer.</rdakit:toolkitDefinition>
      <skos:scopeNote xml:lang="da">Denne term anvendes for lydressourcer.</skos:scopeNote>
      <skos:prefLabel xml:lang="fr">mère</skos:prefLabel>
      <rdakit:toolkitLabel xml:lang="fr">mère</rdakit:toolkitLabel>
      <skos:definition xml:lang="fr">Génération qui consiste en une copie positive en métal d’un disque père utilisée pour créer une ou plusieurs matrices de pressage.</skos:definition>
      <rdakit:toolkitDefinition xml:lang="fr">Génération qui consiste en une copie positive en métal d’un disque père utilisée pour créer une ou plusieurs matrices de pressage.</rdakit:toolkitDefinition>
      <skos:scopeNote xml:lang="fr">Ce terme s’applique aux ressources audio.</skos:scopeNote>
      <skos:prefLabel xml:lang="no">mor</skos:prefLabel>
      <rdakit:toolkitLabel xml:lang="no">mor</rdakit:toolkitLabel>
      <skos:definition xml:lang="no">En generasjon som består av en positiv metallkopi av en platemaster brukt for å lage en eller flere matriser.</skos:definition>
      <rdakit:toolkitDefinition xml:lang="no">En generasjon som består av en positiv metallkopi av en platemaster brukt for å lage en eller flere matriser.</rdakit:toolkitDefinition>
      <skos:scopeNote xml:lang="no">Dette begrepet gjelder lydressurser.</skos:scopeNote>
    </skos:Concept>
<!-- Concept: original  -->
    <skos:Concept rdf:about="http://rdaregistry.info/termList/RDAGeneration/1009" xml:lang="en">
      <skos:inScheme rdf:resource="http://rdaregistry.info/termList/RDAGeneration"/>
      <reg:status rdf:resource="http://metadataregistry.org/uri/RegStatus/1001"/>
      <reg:identifier rdf:resource="http://metadataregistry.org/concepts/8426"/>
      <skos:prefLabel xml:lang="en">original</skos:prefLabel>
      <rdakit:toolkitLabel xml:lang="en">original</rdakit:toolkitLabel>
      <skos:definition xml:lang="en">A generation that is the first of a resource created digitally.</skos:definition>
      <rdakit:toolkitDefinition xml:lang="en">A generation that is the first of a resource created digitally.</rdakit:toolkitDefinition>
      <skos:scopeNote xml:lang="en">This term applies to digital resources.</skos:scopeNote>
	    <skos:related rdf:resource="http://rdaregistry.info/termList/RDAGeneration/1005"/>
      <skos:prefLabel xml:lang="de">Original</skos:prefLabel>
      <rdakit:toolkitLabel xml:lang="de">Original</rdakit:toolkitLabel>
      <skos:definition xml:lang="de">Eine Kopiengeneration für eine erste, digital hergestellte Ressource.</skos:definition>
      <rdakit:toolkitDefinition xml:lang="de">Eine Kopiengeneration für eine erste, digital hergestellte Ressource.</rdakit:toolkitDefinition>
      <skos:scopeNote xml:lang="de">Dieser Terminus bezieht sich auf digitalen Ressourcen.</skos:scopeNote>
      <skos:prefLabel xml:lang="vi">gốc</skos:prefLabel>
      <rdakit:toolkitLabel xml:lang="vi">gốc</rdakit:toolkitLabel>
      <skos:definition xml:lang="vi">Thế hệ là đầu tiên của tài nguyên được tạo ra theo kỹ thuật số</skos:definition>
      <rdakit:toolkitDefinition xml:lang="vi">Thế hệ là đầu tiên của tài nguyên được tạo ra theo kỹ thuật số</rdakit:toolkitDefinition>
      <skos:scopeNote xml:lang="vi">Thuật ngữ này áp dụng cho tài nguyên số.</skos:scopeNote>
      <skos:prefLabel xml:lang="fi">originaali</skos:prefLabel>
      <rdakit:toolkitLabel xml:lang="fi">originaali</rdakit:toolkitLabel>
      <skos:definition xml:lang="fi">Sukupolven määrite digitaaliselle aineistolle, joka on digitaalisesti luodun aineiston ensimmäinen versio.</skos:definition>
      <rdakit:toolkitDefinition xml:lang="fi">Sukupolven määrite digitaaliselle aineistolle, joka on digitaalisesti luodun aineiston ensimmäinen versio.</rdakit:toolkitDefinition>
      <skos:scopeNote xml:lang="fi">Termi koskee digitaalista aineistoa.</skos:scopeNote>
      <skos:prefLabel xml:lang="da">original</skos:prefLabel>
      <rdakit:toolkitLabel xml:lang="da">original</rdakit:toolkitLabel>
      <skos:definition xml:lang="da">Generation, der er den første af en digitalt skabt ressource.</skos:definition>
      <rdakit:toolkitDefinition xml:lang="da">Generation, der er den første af en digitalt skabt ressource.</rdakit:toolkitDefinition>
      <skos:scopeNote xml:lang="da">Denne term anvendes for digitale ressourcer.</skos:scopeNote>
      <skos:prefLabel xml:lang="fr">original</skos:prefLabel>
      <rdakit:toolkitLabel xml:lang="fr">original</rdakit:toolkitLabel>
      <skos:definition xml:lang="fr">Génération qui est la première d’une ressource créée numériquement.</skos:definition>
      <rdakit:toolkitDefinition xml:lang="fr">Génération qui est la première d’une ressource créée numériquement.</rdakit:toolkitDefinition>
      <skos:scopeNote xml:lang="fr">Ce terme s’applique aux ressources numériques.</skos:scopeNote>
      <skos:prefLabel xml:lang="no">original</skos:prefLabel>
      <rdakit:toolkitLabel xml:lang="no">original</rdakit:toolkitLabel>
      <skos:definition xml:lang="no">Den første generasjonen av en ressurs som er skapt digitalt.</skos:definition>
      <rdakit:toolkitDefinition xml:lang="no">Den første generasjonen av en ressurs som er skapt digitalt.</rdakit:toolkitDefinition>
      <skos:scopeNote xml:lang="no">Dette begrepet gjelder digitale ressurser.</skos:scopeNote>
    </skos:Concept>
<!-- Concept: original negative  -->
    <skos:Concept rdf:about="http://rdaregistry.info/termList/RDAGeneration/1013" xml:lang="en">
      <skos:inScheme rdf:resource="http://rdaregistry.info/termList/RDAGeneration"/>
      <reg:status rdf:resource="http://metadataregistry.org/uri/RegStatus/1001"/>
      <reg:identifier rdf:resource="http://metadataregistry.org/concepts/8430"/>
      <skos:prefLabel xml:lang="en">original negative</skos:prefLabel>
      <rdakit:toolkitLabel xml:lang="en">original negative</rdakit:toolkitLabel>
      <skos:definition xml:lang="en">A generation usually of negative polarity for film exposed in a camera and thus of better quality than any subsequent generation or derivative.</skos:definition>
      <rdakit:toolkitDefinition xml:lang="en">A generation usually of negative polarity for film exposed in a camera and thus of better quality than any subsequent generation or derivative.</rdakit:toolkitDefinition>
      <skos:scopeNote xml:lang="en">This term applies to motion picture resources.</skos:scopeNote>
      <skos:prefLabel xml:lang="de">Originalnegativ</skos:prefLabel>
      <rdakit:toolkitLabel xml:lang="de">Originalnegativ</rdakit:toolkitLabel>
      <skos:definition xml:lang="de">Eine Kopiengeneration für Filme (normalerweise mit negativer Polarität), die in einer Kamera belichtet werden und deshalb von besserer Qualität sind, als jede nachfolgende Kopiengeneration oder Derivat.</skos:definition>
      <rdakit:toolkitDefinition xml:lang="de">Eine Kopiengeneration für Filme (normalerweise mit negativer Polarität), die in einer Kamera belichtet werden und deshalb von besserer Qualität sind, als jede nachfolgende Kopiengeneration oder Derivat.</rdakit:toolkitDefinition>
      <skos:scopeNote xml:lang="de">Dieser Terminus bezieht sich auf Filme.</skos:scopeNote>
      <skos:prefLabel xml:lang="vi">bản gốc âm</skos:prefLabel>
      <rdakit:toolkitLabel xml:lang="vi">bản gốc âm</rdakit:toolkitLabel>
      <skos:definition xml:lang="vi">Thế hệ thường là phân cực âm của phim được phơi sáng trong máy ảnh và như vậy có chất lượng tốt hơn so với thế hệ hoặc dẫn xuất tiếp sau.</skos:definition>
      <rdakit:toolkitDefinition xml:lang="vi">Thế hệ thường là phân cực âm của phim được phơi sáng trong máy ảnh và như vậy có chất lượng tốt hơn so với thế hệ hoặc dẫn xuất tiếp sau.</rdakit:toolkitDefinition>
      <skos:scopeNote xml:lang="vi">Thuật ngữ này áp dụng cho tài nguyên phim điện ảnh.</skos:scopeNote>
      <skos:prefLabel xml:lang="fi">alkuperäinen negatiivi</skos:prefLabel>
      <rdakit:toolkitLabel xml:lang="fi">alkuperäinen negatiivi</rdakit:toolkitLabel>
      <skos:definition xml:lang="fi">Negatiivisen polariteetin filmi, joka on valotettu kamerassa ja joka siksi yleensä on parempilaatuinen kuin seuraava sukupolvi tai johdannainen.</skos:definition>
      <rdakit:toolkitDefinition xml:lang="fi">Negatiivisen polariteetin filmi, joka on valotettu kamerassa ja joka siksi yleensä on parempilaatuinen kuin seuraava sukupolvi tai johdannainen.</rdakit:toolkitDefinition>
      <skos:scopeNote xml:lang="fi">Termi koskee elokuvia.</skos:scopeNote>
      <skos:prefLabel xml:lang="da">original negativ</skos:prefLabel>
      <rdakit:toolkitLabel xml:lang="da">original negativ</rdakit:toolkitLabel>
      <skos:definition xml:lang="da">Generation af film, normalt med negativ polaritet eksponeret i et kamera og dermed af bedre kvalitet end nogen efterfølgende generation eller derivat.</skos:definition>
      <rdakit:toolkitDefinition xml:lang="da">Generation af film, normalt med negativ polaritet eksponeret i et kamera og dermed af bedre kvalitet end nogen efterfølgende generation eller derivat.</rdakit:toolkitDefinition>
      <skos:scopeNote xml:lang="da">Denne term anvendes for ressourcer med levende billeder.</skos:scopeNote>
      <skos:prefLabel xml:lang="fr">négatif original</skos:prefLabel>
      <rdakit:toolkitLabel xml:lang="fr">négatif original</rdakit:toolkitLabel>
      <skos:definition xml:lang="fr">Génération habituellement de polarité négative d’un film qui a été exposé dans une caméra et est par conséquent de meilleure qualité que toute génération subséquente ou tout dérivé.</skos:definition>
      <rdakit:toolkitDefinition xml:lang="fr">Génération habituellement de polarité négative d’un film qui a été exposé dans une caméra et est par conséquent de meilleure qualité que toute génération subséquente ou tout dérivé.</rdakit:toolkitDefinition>
      <skos:scopeNote xml:lang="fr">Ce terme s’applique aux ressources filmiques.</skos:scopeNote>
      <skos:prefLabel xml:lang="no">originalnegativ</skos:prefLabel>
      <rdakit:toolkitLabel xml:lang="no">originalnegativ</rdakit:toolkitLabel>
      <skos:definition xml:lang="no">En generasjon som vanligvis har negativ polaritet, for film eksponert i et kamera og dermed av høyere kvalitet enn noen påfølgende generasjon eller noe derivat.</skos:definition>
      <rdakit:toolkitDefinition xml:lang="no">En generasjon som vanligvis har negativ polaritet, for film eksponert i et kamera og dermed av høyere kvalitet enn noen påfølgende generasjon eller noe derivat.</rdakit:toolkitDefinition>
      <skos:scopeNote xml:lang="no">Dette begrepet gjelder spillefilmressurser.</skos:scopeNote>
    </skos:Concept>
<!-- Concept: printing master  -->
    <skos:Concept rdf:about="http://rdaregistry.info/termList/RDAGeneration/1010" xml:lang="en">
      <skos:inScheme rdf:resource="http://rdaregistry.info/termList/RDAGeneration"/>
      <reg:status rdf:resource="http://metadataregistry.org/uri/RegStatus/1001"/>
      <reg:identifier rdf:resource="http://metadataregistry.org/concepts/8427"/>
      <skos:prefLabel xml:lang="en">printing master</skos:prefLabel>
      <skos:altLabel xml:lang="en">copying master</skos:altLabel>
      <rdakit:toolkitLabel xml:lang="en">printing master</rdakit:toolkitLabel>
      <skos:definition xml:lang="en">A generation that is used to produce subsequent generations of microforms.</skos:definition>
      <rdakit:toolkitDefinition xml:lang="en">A generation that is used to produce subsequent generations of microforms.</rdakit:toolkitDefinition>
      <skos:prefLabel xml:lang="de">Druckmaster</skos:prefLabel>
      <skos:altLabel xml:lang="de">Kopiermaster</skos:altLabel>
      <rdakit:toolkitLabel xml:lang="de">Druckmaster</rdakit:toolkitLabel>
      <skos:definition xml:lang="de">Eine Kopiengeneration die verwendet wird, um spätere Generationen von Mikroformen zu erstellen.</skos:definition>
      <rdakit:toolkitDefinition xml:lang="de">Eine Kopiengeneration die verwendet wird, um spätere Generationen von Mikroformen zu erstellen.</rdakit:toolkitDefinition>
      <skos:altLabel xml:lang="de">Dupe neg</skos:altLabel>
      <skos:altLabel xml:lang="de">Sub-Master</skos:altLabel>
      <skos:prefLabel xml:lang="vi">bản in chủ</skos:prefLabel>
      <skos:altLabel xml:lang="vi">bản sao chủ</skos:altLabel>
      <rdakit:toolkitLabel xml:lang="vi">bản in chủ</rdakit:toolkitLabel>
      <skos:definition xml:lang="vi">Thế hệ dùng để sản xuất các thế hệ tiếp sau của vi dạng.</skos:definition>
      <rdakit:toolkitDefinition xml:lang="vi">Thế hệ dùng để sản xuất các thế hệ tiếp sau của vi dạng.</rdakit:toolkitDefinition>
      <skos:prefLabel xml:lang="fi">painomaster</skos:prefLabel>
      <rdakit:toolkitLabel xml:lang="fi">painomaster</rdakit:toolkitLabel>
      <skos:definition xml:lang="fi">Sukupolven määrite mikromuotoiselle aineistolle, jota käytetään seuraavien sukupolvien mikromuotoisten aineistojen valmistamiseen.</skos:definition>
      <rdakit:toolkitDefinition xml:lang="fi">Sukupolven määrite mikromuotoiselle aineistolle, jota käytetään seuraavien sukupolvien mikromuotoisten aineistojen valmistamiseen.</rdakit:toolkitDefinition>
      <skos:prefLabel xml:lang="da">trykmaster</skos:prefLabel>
      <skos:altLabel xml:lang="da">kopimaster</skos:altLabel>
      <rdakit:toolkitLabel xml:lang="da">trykmaster</rdakit:toolkitLabel>
      <skos:definition xml:lang="da">Generation, der anvendes til at fremstille efterfølgende generationer af mikroformer.</skos:definition>
      <rdakit:toolkitDefinition xml:lang="da">Generation, der anvendes til at fremstille efterfølgende generationer af mikroformer.</rdakit:toolkitDefinition>
      <skos:prefLabel xml:lang="fr">matrice de tirage</skos:prefLabel>
      <rdakit:toolkitLabel xml:lang="fr">matrice de tirage</rdakit:toolkitLabel>
      <skos:definition xml:lang="fr">Génération utilisée pour produire des générations subséquentes de microformes.</skos:definition>
      <rdakit:toolkitDefinition xml:lang="fr">Génération utilisée pour produire des générations subséquentes de microformes.</rdakit:toolkitDefinition>
      <skos:prefLabel xml:lang="no">trykkemaster</skos:prefLabel>
      <skos:altLabel xml:lang="no">kopimaster</skos:altLabel>
      <rdakit:toolkitLabel xml:lang="no">trykkemaster</rdakit:toolkitLabel>
      <skos:definition xml:lang="no">En generasjon som brukes som brukes til å produsere påfølgende generasjoner av mikroformer.</skos:definition>
      <rdakit:toolkitDefinition xml:lang="no">En generasjon som brukes som brukes til å produsere påfølgende generasjoner av mikroformer.</rdakit:toolkitDefinition>
    </skos:Concept>
<!-- Concept: reference print  -->
    <skos:Concept rdf:about="http://rdaregistry.info/termList/RDAGeneration/1011" xml:lang="en">
      <skos:inScheme rdf:resource="http://rdaregistry.info/termList/RDAGeneration"/>
      <reg:status rdf:resource="http://metadataregistry.org/uri/RegStatus/1001"/>
      <reg:identifier rdf:resource="http://metadataregistry.org/concepts/8428"/>
      <skos:prefLabel xml:lang="en">reference print</skos:prefLabel>
      <rdakit:toolkitLabel xml:lang="en">reference print</rdakit:toolkitLabel>
      <skos:definition xml:lang="en">A generation that is a release print approved by the producer and director of a film.</skos:definition>
      <rdakit:toolkitDefinition xml:lang="en">A generation that is a release print approved by the producer and director of a film.</rdakit:toolkitDefinition>
      <skos:scopeNote xml:lang="en">This term applies to motion picture resources.</skos:scopeNote>
      <skos:prefLabel xml:lang="de">Referenzabzug</skos:prefLabel>
      <rdakit:toolkitLabel xml:lang="de">Referenzabzug</rdakit:toolkitLabel>
      <skos:definition xml:lang="de">Eine Kopiengeneration für eine Druckfreigabe, die vom Produzenten und Regisseur eines Films genehmigt wurde.</skos:definition>
      <rdakit:toolkitDefinition xml:lang="de">Eine Kopiengeneration für eine Druckfreigabe, die vom Produzenten und Regisseur eines Films genehmigt wurde.</rdakit:toolkitDefinition>
      <skos:scopeNote xml:lang="de">Dieser Terminus bezieht sich auf Filme.</skos:scopeNote>
      <skos:prefLabel xml:lang="vi">bản in tham chiếu</skos:prefLabel>
      <rdakit:toolkitLabel xml:lang="vi">bản in tham chiếu</rdakit:toolkitLabel>
      <skos:definition xml:lang="vi">Thế hệ là bản in công bố được nhà sản xuất và đạo diễn phim chấp nhận.</skos:definition>
      <rdakit:toolkitDefinition xml:lang="vi">Thế hệ là bản in công bố được nhà sản xuất và đạo diễn phim chấp nhận.</rdakit:toolkitDefinition>
      <skos:scopeNote xml:lang="vi">Thuật ngữ này áp dụng cho tài nguyên phim điện ảnh.</skos:scopeNote>
      <skos:prefLabel xml:lang="fi">koevedos</skos:prefLabel>
      <rdakit:toolkitLabel xml:lang="fi">koevedos</rdakit:toolkitLabel>
      <skos:definition xml:lang="fi">Sukupolven määrite, joka on elokuvan tuottajan ja ohjaajan hyväksymä koevedos.</skos:definition>
      <rdakit:toolkitDefinition xml:lang="fi">Sukupolven määrite, joka on elokuvan tuottajan ja ohjaajan hyväksymä koevedos.</rdakit:toolkitDefinition>
      <skos:scopeNote xml:lang="fi">Termi koskee elokuvia.</skos:scopeNote>
      <skos:prefLabel xml:lang="da">udgivelse</skos:prefLabel>
      <rdakit:toolkitLabel xml:lang="da">udgivelse</rdakit:toolkitLabel>
      <skos:definition xml:lang="da">Generation, der består af en frigivet udgivelse, som er godkendt af producenten og direktøren for en film.</skos:definition>
      <rdakit:toolkitDefinition xml:lang="da">Generation, der består af en frigivet udgivelse, som er godkendt af producenten og direktøren for en film.</rdakit:toolkitDefinition>
      <skos:scopeNote xml:lang="da">Denne term anvendes for ressourcer med levende billeder.</skos:scopeNote>
      <skos:prefLabel xml:lang="fr">copie de référence</skos:prefLabel>
      <rdakit:toolkitLabel xml:lang="fr">copie de référence</rdakit:toolkitLabel>
      <skos:definition xml:lang="fr">Génération qui consiste en une copie d’exploitation approuvée par le producteur et le réalisateur d’un film.</skos:definition>
      <rdakit:toolkitDefinition xml:lang="fr">Génération qui consiste en une copie d’exploitation approuvée par le producteur et le réalisateur d’un film.</rdakit:toolkitDefinition>
      <skos:scopeNote xml:lang="fr">Ce terme s’applique aux ressources filmiques.</skos:scopeNote>
      <skos:prefLabel xml:lang="no">referansekopi</skos:prefLabel>
      <rdakit:toolkitLabel xml:lang="no">referansekopi</rdakit:toolkitLabel>
      <skos:definition xml:lang="no">En generasjon som er en kopi for utgivelse som er godkjent av produsenten og regissøren av en film.</skos:definition>
      <rdakit:toolkitDefinition xml:lang="no">En generasjon som er en kopi for utgivelse som er godkjent av produsenten og regissøren av en film.</rdakit:toolkitDefinition>
      <skos:scopeNote xml:lang="no">Dette begrepet gjelder spillefilmressurser.</skos:scopeNote>
    </skos:Concept>
<!-- Concept: service copy  -->
    <skos:Concept rdf:about="http://rdaregistry.info/termList/RDAGeneration/1014" xml:lang="en">
      <skos:inScheme rdf:resource="http://rdaregistry.info/termList/RDAGeneration"/>
      <reg:status rdf:resource="http://metadataregistry.org/uri/RegStatus/1001"/>
      <reg:identifier rdf:resource="http://metadataregistry.org/concepts/8431"/>
      <skos:prefLabel xml:lang="en">service copy</skos:prefLabel>
      <skos:altLabel xml:lang="en">reference copy</skos:altLabel>
      <rdakit:toolkitLabel xml:lang="en">service copy</rdakit:toolkitLabel>
      <skos:definition xml:lang="en">A generation that is intended primarily for use.</skos:definition>
      <rdakit:toolkitDefinition xml:lang="en">A generation that is intended primarily for use.</rdakit:toolkitDefinition>
      <skos:prefLabel xml:lang="de">Arbeitskopie</skos:prefLabel>
      <skos:altLabel xml:lang="de">Referenzexemplar</skos:altLabel>
      <rdakit:toolkitLabel xml:lang="de">Arbeitskopie</rdakit:toolkitLabel>
      <skos:definition xml:lang="de">Eine Kopiengeneration die in erster Linie für die Benutzung gedacht ist.</skos:definition>
      <rdakit:toolkitDefinition xml:lang="de">Eine Kopiengeneration die in erster Linie für die Benutzung gedacht ist.</rdakit:toolkitDefinition>
      <skos:altLabel xml:lang="de">Arbeitsexemplar</skos:altLabel>
      <skos:prefLabel xml:lang="vi">bản sao phục vụ</skos:prefLabel>
      <skos:altLabel xml:lang="vi">bản sao tham chiếu</skos:altLabel>
      <rdakit:toolkitLabel xml:lang="vi">bản sao phục vụ</rdakit:toolkitLabel>
      <skos:definition xml:lang="vi">Thế hệ chủ yếu dành để sử dụng.</skos:definition>
      <rdakit:toolkitDefinition xml:lang="vi">Thế hệ chủ yếu dành để sử dụng.</rdakit:toolkitDefinition>
      <skos:prefLabel xml:lang="fi">käyttökopio</skos:prefLabel>
      <rdakit:toolkitLabel xml:lang="fi">käyttökopio</rdakit:toolkitLabel>
      <skos:definition xml:lang="fi">Sukupolven määrite aineistolle, joka on pääasiallisesti tarkoitettu käyttöön.</skos:definition>
      <rdakit:toolkitDefinition xml:lang="fi">Sukupolven määrite aineistolle, joka on pääasiallisesti tarkoitettu käyttöön.</rdakit:toolkitDefinition>
      <skos:prefLabel xml:lang="da">servicekopi</skos:prefLabel>
      <skos:altLabel xml:lang="da">referencekopi</skos:altLabel>
      <rdakit:toolkitLabel xml:lang="da">servicekopi</rdakit:toolkitLabel>
      <skos:definition xml:lang="da">Generation der primært er beregnet til brug.</skos:definition>
      <rdakit:toolkitDefinition xml:lang="da">Generation der primært er beregnet til brug.</rdakit:toolkitDefinition>
      <skos:prefLabel xml:lang="fr">copie de consultation</skos:prefLabel>
      <skos:altLabel xml:lang="fr">copie d’utilisation</skos:altLabel>
      <rdakit:toolkitLabel xml:lang="fr">copie de consultation</rdakit:toolkitLabel>
      <skos:definition xml:lang="fr">Génération qui est prévue principalement pour l’utilisation.</skos:definition>
      <rdakit:toolkitDefinition xml:lang="fr">Génération qui est prévue principalement pour l’utilisation.</rdakit:toolkitDefinition>
      <skos:prefLabel xml:lang="no">brukseksemplar</skos:prefLabel>
      <skos:altLabel xml:lang="no">referanseeksemplar</skos:altLabel>
      <rdakit:toolkitLabel xml:lang="no">brukseksemplar</rdakit:toolkitLabel>
      <skos:definition xml:lang="no">En generasjon som primært er ment for bruk.</skos:definition>
      <rdakit:toolkitDefinition xml:lang="no">En generasjon som primært er ment for bruk.</rdakit:toolkitDefinition>
    </skos:Concept>
<!-- Concept: stamper  -->
    <skos:Concept rdf:about="http://rdaregistry.info/termList/RDAGeneration/1015" xml:lang="en">
      <skos:inScheme rdf:resource="http://rdaregistry.info/termList/RDAGeneration"/>
      <reg:status rdf:resource="http://metadataregistry.org/uri/RegStatus/1001"/>
      <reg:identifier rdf:resource="http://metadataregistry.org/concepts/8432"/>
      <skos:prefLabel xml:lang="en">stamper</skos:prefLabel>
      <rdakit:toolkitLabel xml:lang="en">stamper</rdakit:toolkitLabel>
      <skos:definition xml:lang="en">A generation that is a hard metal negative copy of a disc master that can be mounted within a press and used to impress the groove pattern in a production run of discs.</skos:definition>
      <rdakit:toolkitDefinition xml:lang="en">A generation that is a hard metal negative copy of a disc master that can be mounted within a press and used to impress the groove pattern in a production run of discs.</rdakit:toolkitDefinition>
      <skos:scopeNote xml:lang="en">This term applies to audio resources.</skos:scopeNote>
      <skos:prefLabel xml:lang="de">Matrize</skos:prefLabel>
      <rdakit:toolkitLabel xml:lang="de">Matrize</rdakit:toolkitLabel>
      <skos:definition xml:lang="de">Eine Kopiengeneration die aus einer negativen Hartmetallkopie eines Disk-Masters besteht, die in eine Presse montiert und verwendet werden kann, um das Rillenmuster in einem Disk-Fertigungslauf zu prägen.</skos:definition>
      <rdakit:toolkitDefinition xml:lang="de">Eine Kopiengeneration die aus einer negativen Hartmetallkopie eines Disk-Masters besteht, die in eine Presse montiert und verwendet werden kann, um das Rillenmuster in einem Disk-Fertigungslauf zu prägen.</rdakit:toolkitDefinition>
      <skos:scopeNote xml:lang="de">Dieser Terminus bezieht sich auf Audioressourcen.</skos:scopeNote>
      <skos:prefLabel xml:lang="vi">dấu khắc</skos:prefLabel>
      <rdakit:toolkitLabel xml:lang="vi">dấu khắc</rdakit:toolkitLabel>
      <skos:definition xml:lang="vi">Thế hệ là bản kim loại âm của đĩa chủ có thể tạo khung bên trong máy ép và dùng để tạo ra mẫu đường rãnh của sản phẩm đĩa.</skos:definition>
      <rdakit:toolkitDefinition xml:lang="vi">Thế hệ là bản kim loại âm của đĩa chủ có thể tạo khung bên trong máy ép và dùng để tạo ra mẫu đường rãnh của sản phẩm đĩa.</rdakit:toolkitDefinition>
      <skos:scopeNote xml:lang="vi">Thuật ngữ này áp dụng cho tài nguyên audio.</skos:scopeNote>
      <skos:prefLabel xml:lang="fi">isiö</skos:prefLabel>
      <rdakit:toolkitLabel xml:lang="fi">isiö</rdakit:toolkitLabel>
      <skos:definition xml:lang="fi">Äänitteen sukupolven määrite originaalilevyn kovametalliselle negatiivikopiolle, joka voidaan asentaa puristimeen ja käyttää urakuvion painamiseen levyjen tuotantoerän valmistuksessa.</skos:definition>
      <rdakit:toolkitDefinition xml:lang="fi">Äänitteen sukupolven määrite originaalilevyn kovametalliselle negatiivikopiolle, joka voidaan asentaa puristimeen ja käyttää urakuvion painamiseen levyjen tuotantoerän valmistuksessa.</rdakit:toolkitDefinition>
      <skos:scopeNote xml:lang="fi">Termi koskee äänitteitä.</skos:scopeNote>
      <skos:prefLabel xml:lang="da">patrice</skos:prefLabel>
      <rdakit:toolkitLabel xml:lang="da">patrice</rdakit:toolkitLabel>
      <skos:definition xml:lang="da">Generation, der består af en negativ hårdmetalkopi af en discmaster, der kan sættes i en presse og bruges til at præge rillemønsteret i en produktionskørsel af discs.</skos:definition>
      <rdakit:toolkitDefinition xml:lang="da">Generation, der består af en negativ hårdmetalkopi af en discmaster, der kan sættes i en presse og bruges til at præge rillemønsteret i en produktionskørsel af discs.</rdakit:toolkitDefinition>
      <skos:scopeNote xml:lang="da">Denne term anvendes for lydressourcer.</skos:scopeNote>
      <skos:prefLabel xml:lang="fr">matrice de pressage</skos:prefLabel>
      <rdakit:toolkitLabel xml:lang="fr">matrice de pressage</rdakit:toolkitLabel>
      <skos:definition xml:lang="fr">Génération qui consiste en une copie négative en métal dur d’un disque père qui peut être montée sur une presse et utilisée pour imprimer le dessin des sillons sur les disques produits lors d’un même tirage.</skos:definition>
      <rdakit:toolkitDefinition xml:lang="fr">Génération qui consiste en une copie négative en métal dur d’un disque père qui peut être montée sur une presse et utilisée pour imprimer le dessin des sillons sur les disques produits lors d’un même tirage.</rdakit:toolkitDefinition>
      <skos:scopeNote xml:lang="fr">Ce terme s’applique aux ressources audio.</skos:scopeNote>
      <skos:prefLabel xml:lang="no">matrise</skos:prefLabel>
      <rdakit:toolkitLabel xml:lang="no">matrise</rdakit:toolkitLabel>
      <skos:definition xml:lang="no">En generasjon som består av en hard, negativ metallkopi av en platemaster som kan monteres i en presse og brukes til å trykke rillemønsteret i et produksjonsopplag av plater.</skos:definition>
      <rdakit:toolkitDefinition xml:lang="no">En generasjon som består av en hard, negativ metallkopi av en platemaster som kan monteres i en presse og brukes til å trykke rillemønsteret i et produksjonsopplag av plater.</rdakit:toolkitDefinition>
      <skos:scopeNote xml:lang="no">Dette begrepet gjelder lydressurser.</skos:scopeNote>
    </skos:Concept>
<!-- Concept: tape duplication master  -->
    <skos:Concept rdf:about="http://rdaregistry.info/termList/RDAGeneration/1016" xml:lang="en">
      <skos:inScheme rdf:resource="http://rdaregistry.info/termList/RDAGeneration"/>
      <reg:status rdf:resource="http://metadataregistry.org/uri/RegStatus/1001"/>
      <reg:identifier rdf:resource="http://metadataregistry.org/concepts/8433"/>
      <skos:prefLabel xml:lang="en">tape duplication master</skos:prefLabel>
      <rdakit:toolkitLabel xml:lang="en">tape duplication master</rdakit:toolkitLabel>
      <skos:definition xml:lang="en">A generation that is a tape copy, usually a first generation copy of the master, used for creating multiple copies of the content.</skos:definition>
      <rdakit:toolkitDefinition xml:lang="en">A generation that is a tape copy, usually a first generation copy of the master, used for creating multiple copies of the content.</rdakit:toolkitDefinition>
      <skos:scopeNote xml:lang="en">This term applies to audio resources.</skos:scopeNote>
      <skos:prefLabel xml:lang="de">Bandvervielfältigungsmaster</skos:prefLabel>
      <rdakit:toolkitLabel xml:lang="de">Bandvervielfältigungsmaster</rdakit:toolkitLabel>
      <skos:definition xml:lang="de">Eine Kopiengeneration für eine Bandkopie (üblicherweise einer Kopie der ersten Generation vom Master), die verwendet wird, um mehrfache Kopien des Inhalts zu erstellen (z. B. für Kompaktkassetten).</skos:definition>
      <rdakit:toolkitDefinition xml:lang="de">Eine Kopiengeneration für eine Bandkopie (üblicherweise einer Kopie der ersten Generation vom Master), die verwendet wird, um mehrfache Kopien des Inhalts zu erstellen (z. B. für Kompaktkassetten).</rdakit:toolkitDefinition>
      <skos:scopeNote xml:lang="de">Dieser Terminus bezieht sich auf Audioressourcen.</skos:scopeNote>
      <skos:prefLabel xml:lang="vi">băng sao chủ</skos:prefLabel>
      <rdakit:toolkitLabel xml:lang="vi">băng sao chủ</rdakit:toolkitLabel>
      <skos:definition xml:lang="vi">Thế hệ là bản sao băng, thường là bản sao thế hệ thứ nhất của băng chủ, dùng để tạo ra nhiều bản sao của nội dung.</skos:definition>
      <rdakit:toolkitDefinition xml:lang="vi">Thế hệ là bản sao băng, thường là bản sao thế hệ thứ nhất của băng chủ, dùng để tạo ra nhiều bản sao của nội dung.</rdakit:toolkitDefinition>
      <skos:scopeNote xml:lang="vi">Thuật ngữ này áp dụng cho tài nguyên audio.</skos:scopeNote>
      <skos:prefLabel xml:lang="fi">kopiomasternauha</skos:prefLabel>
      <rdakit:toolkitLabel xml:lang="fi">kopiomasternauha</rdakit:toolkitLabel>
      <skos:definition xml:lang="fi">Äänitteen sukupolven määrite nauhakopiolle, yleensä originaalin ensimmäisen sukupolven kopiolle, jota käytetään massakopioidenvalmistamiseen.</skos:definition>
      <rdakit:toolkitDefinition xml:lang="fi">Äänitteen sukupolven määrite nauhakopiolle, yleensä originaalin ensimmäisen sukupolven kopiolle, jota käytetään massakopioidenvalmistamiseen.</rdakit:toolkitDefinition>
      <skos:scopeNote xml:lang="fi">Termi koskee äänitteitä.</skos:scopeNote>
      <skos:prefLabel xml:lang="da">båndkopieringsmaster</skos:prefLabel>
      <rdakit:toolkitLabel xml:lang="da">båndkopieringsmaster</rdakit:toolkitLabel>
      <skos:definition xml:lang="da">Generation, der består af en båndkopi, normalt en førstegenerationskopi af masteren, der anvendes til at skabe flere kopier af indholdet.</skos:definition>
      <rdakit:toolkitDefinition xml:lang="da">Generation, der består af en båndkopi, normalt en førstegenerationskopi af masteren, der anvendes til at skabe flere kopier af indholdet.</rdakit:toolkitDefinition>
      <skos:scopeNote xml:lang="da">Denne term anvendes for lydressourcer.</skos:scopeNote>
      <skos:prefLabel xml:lang="fr">matrice de duplication de bande</skos:prefLabel>
      <rdakit:toolkitLabel xml:lang="fr">matrice de duplication de bande</rdakit:toolkitLabel>
      <skos:definition xml:lang="fr">Génération qui consiste en une copie sur bande magnétique, généralement une copie de première génération de la bande maîtresse, utilisée pour créer de multiples copies du contenu.</skos:definition>
      <rdakit:toolkitDefinition xml:lang="fr">Génération qui consiste en une copie sur bande magnétique, généralement une copie de première génération de la bande maîtresse, utilisée pour créer de multiples copies du contenu.</rdakit:toolkitDefinition>
      <skos:scopeNote xml:lang="fr">Ce terme s’applique aux ressources audio.</skos:scopeNote>
      <skos:prefLabel xml:lang="no">lydbåndmaster for mangfoldiggjøring</skos:prefLabel>
      <rdakit:toolkitLabel xml:lang="no">lydbåndmaster for mangfoldiggjøring</rdakit:toolkitLabel>
      <skos:definition xml:lang="no">En generasjon som er en lydbåndkopi, vanligvis en førstegenerasjons kopi av en master, som brukes for å lage flere kopier av innholdet.</skos:definition>
      <rdakit:toolkitDefinition xml:lang="no">En generasjon som er en lydbåndkopi, vanligvis en førstegenerasjons kopi av en master, som brukes for å lage flere kopier av innholdet.</rdakit:toolkitDefinition>
      <skos:scopeNote xml:lang="no">Dette begrepet gjelder lydressurser.</skos:scopeNote>
    </skos:Concept>
<!-- Concept: test pressing  -->
    <skos:Concept rdf:about="http://rdaregistry.info/termList/RDAGeneration/1017" xml:lang="en">
      <skos:inScheme rdf:resource="http://rdaregistry.info/termList/RDAGeneration"/>
      <reg:status rdf:resource="http://metadataregistry.org/uri/RegStatus/1001"/>
      <reg:identifier rdf:resource="http://metadataregistry.org/concepts/8434"/>
      <skos:prefLabel xml:lang="en">test pressing</skos:prefLabel>
      <rdakit:toolkitLabel xml:lang="en">test pressing</rdakit:toolkitLabel>
      <skos:definition xml:lang="en">A generation that is one of a short run of pressings used to check for any flaws before running a full pressing.</skos:definition>
      <rdakit:toolkitDefinition xml:lang="en">A generation that is one of a short run of pressings used to check for any flaws before running a full pressing.</rdakit:toolkitDefinition>
      <skos:scopeNote xml:lang="en">This term applies to audio resources. Initial pressings sent out to reviewers, DJs, etc., are excluded.</skos:scopeNote>
      <skos:prefLabel xml:lang="de">Testpressung</skos:prefLabel>
      <rdakit:toolkitLabel xml:lang="de">Testpressung</rdakit:toolkitLabel>
      <skos:definition xml:lang="de">Eine Kopiengeneration die aus einem kurzen Presslauf besteht, der verwendet wird, um vor dem Lauf einer vollständigen Pressung nach Fehlern zu suchen.</skos:definition>
      <rdakit:toolkitDefinition xml:lang="de">Eine Kopiengeneration die aus einem kurzen Presslauf besteht, der verwendet wird, um vor dem Lauf einer vollständigen Pressung nach Fehlern zu suchen.</rdakit:toolkitDefinition>
      <skos:scopeNote xml:lang="de">Dieser Terminus bezieht sich auf Audioressourcen. Erstpressungen, die an Kritiker, DJs usw. geschickt werden, sind hiervon ausgeschlossen.</skos:scopeNote>
      <skos:prefLabel xml:lang="vi">xử lý thử nghiệm</skos:prefLabel>
      <rdakit:toolkitLabel xml:lang="vi">xử lý thử nghiệm</rdakit:toolkitLabel>
      <skos:definition xml:lang="vi">Thế hệ là mộtđoạn ngắn của xử lý tạm thời được dùng để kiểm tra lỗi bất kỳ trước khi xử lý toàn bộ.</skos:definition>
      <rdakit:toolkitDefinition xml:lang="vi">Thế hệ là mộtđoạn ngắn của xử lý tạm thời được dùng để kiểm tra lỗi bất kỳ trước khi xử lý toàn bộ.</rdakit:toolkitDefinition>
      <skos:scopeNote xml:lang="vi">Thuật ngữ này áp dụng cho tài nguyên audio. Bản ban đầu gửi chi người duyệt, D.J, v.v..., không được bao gồm.</skos:scopeNote>
      <skos:prefLabel xml:lang="fi">koepainos</skos:prefLabel>
      <rdakit:toolkitLabel xml:lang="fi">koepainos</rdakit:toolkitLabel>
      <skos:definition xml:lang="fi">Sukupolven määrite äänitteen painoserälle, joka tehdään virheiden tarkistamiseksi ennen täyden painoksen valmistamista.</skos:definition>
      <rdakit:toolkitDefinition xml:lang="fi">Sukupolven määrite äänitteen painoserälle, joka tehdään virheiden tarkistamiseksi ennen täyden painoksen valmistamista.</rdakit:toolkitDefinition>
      <skos:scopeNote xml:lang="fi">Termi koskee äänitteitä. Se ei sisällä arvostelijoille, DJ:lle tms. lähetettyä esipainosta.</skos:scopeNote>
      <skos:prefLabel xml:lang="da">prøvepresning</skos:prefLabel>
      <rdakit:toolkitLabel xml:lang="da">prøvepresning</rdakit:toolkitLabel>
      <skos:definition xml:lang="da">Generation, der består af en eller flere kørsler af presninger, der anvendes til at tjekke for fejl, før der produceres.</skos:definition>
      <rdakit:toolkitDefinition xml:lang="da">Generation, der består af en eller flere kørsler af presninger, der anvendes til at tjekke for fejl, før der produceres.</rdakit:toolkitDefinition>
      <skos:scopeNote xml:lang="da">Denne term anvendes for lydressourcer. Første presninger, der sendes ud til anmeldere, DJs er ikke omfattet.</skos:scopeNote>
      <skos:prefLabel xml:lang="fr">disque-épreuve</skos:prefLabel>
      <rdakit:toolkitLabel xml:lang="fr">disque-épreuve</rdakit:toolkitLabel>
      <skos:definition xml:lang="fr">Génération qui consiste en une copie faisant partie d’un très petit tirage produit pour détecter les éventuels défauts avant la production en grand nombre.</skos:definition>
      <rdakit:toolkitDefinition xml:lang="fr">Génération qui consiste en une copie faisant partie d’un très petit tirage produit pour détecter les éventuels défauts avant la production en grand nombre.</rdakit:toolkitDefinition>
      <skos:scopeNote xml:lang="fr">Ce terme s’applique aux ressources audio. Ne comprend pas les copies initiales envoyées aux critiques, aux disc jockeys, etc.</skos:scopeNote>
      <skos:prefLabel xml:lang="no">testpressing</skos:prefLabel>
      <rdakit:toolkitLabel xml:lang="no">testpressing</rdakit:toolkitLabel>
      <skos:definition xml:lang="no">En generasjon som er fra et lite opplag av trykksom brukes for å sjekke feil før den endelige trykkingen.</skos:definition>
      <rdakit:toolkitDefinition xml:lang="no">En generasjon som er fra et lite opplag av trykksom brukes for å sjekke feil før den endelige trykkingen.</rdakit:toolkitDefinition>
      <skos:scopeNote xml:lang="no">Dette begrepet gjelder lydressurser. Det første trykket som blir sendt til anmeldere, DJ-er, etc., er ikke inkludert.</skos:scopeNote>
    </skos:Concept>
<!-- Concept: viewing copy  -->
    <skos:Concept rdf:about="http://rdaregistry.info/termList/RDAGeneration/1018" xml:lang="en">
      <skos:inScheme rdf:resource="http://rdaregistry.info/termList/RDAGeneration"/>
      <reg:status rdf:resource="http://metadataregistry.org/uri/RegStatus/1001"/>
      <reg:identifier rdf:resource="http://metadataregistry.org/concepts/8435"/>
      <skos:prefLabel xml:lang="en">viewing copy</skos:prefLabel>
      <rdakit:toolkitLabel xml:lang="en">viewing copy</rdakit:toolkitLabel>
      <skos:definition xml:lang="en">A generation that is a copy that may be viewed by researchers.</skos:definition>
      <rdakit:toolkitDefinition xml:lang="en">A generation that is a copy that may be viewed by researchers.</rdakit:toolkitDefinition>
      <skos:scopeNote xml:lang="en">This term applies to motion picture resources.</skos:scopeNote>
      <skos:prefLabel xml:lang="de">Vorführkopie</skos:prefLabel>
      <rdakit:toolkitLabel xml:lang="de">Vorführkopie</rdakit:toolkitLabel>
      <skos:definition xml:lang="de">Eine Kopiengeneration die zu wissenschaftlichen Zwecken vorgeführt werden kann.</skos:definition>
      <rdakit:toolkitDefinition xml:lang="de">Eine Kopiengeneration die zu wissenschaftlichen Zwecken vorgeführt werden kann.</rdakit:toolkitDefinition>
      <skos:scopeNote xml:lang="de">Dieser Terminus bezieht sich auf Filme.</skos:scopeNote>
      <skos:prefLabel xml:lang="vi">bản xem lại</skos:prefLabel>
      <rdakit:toolkitLabel xml:lang="vi">bản xem lại</rdakit:toolkitLabel>
      <skos:definition xml:lang="vi">Thế hệ là bản sao có thể được xem lại bởi các nhà nghiên cứu</skos:definition>
      <rdakit:toolkitDefinition xml:lang="vi">Thế hệ là bản sao có thể được xem lại bởi các nhà nghiên cứu</rdakit:toolkitDefinition>
      <skos:scopeNote xml:lang="vi">Thuật ngữ này áp dụng cho tài nguyên phim điện ảnh.</skos:scopeNote>
      <skos:prefLabel xml:lang="fi">katselukopio</skos:prefLabel>
      <rdakit:toolkitLabel xml:lang="fi">katselukopio</rdakit:toolkitLabel>
      <skos:definition xml:lang="fi">Sukupolven määrite aineistolle, joka on tutkimuskäyttöön tehty kopio.</skos:definition>
      <rdakit:toolkitDefinition xml:lang="fi">Sukupolven määrite aineistolle, joka on tutkimuskäyttöön tehty kopio.</rdakit:toolkitDefinition>
      <skos:scopeNote xml:lang="fi">Termi koskee elokuvia.</skos:scopeNote>
      <skos:prefLabel xml:lang="da">fremvisningskopi</skos:prefLabel>
      <rdakit:toolkitLabel xml:lang="da">fremvisningskopi</rdakit:toolkitLabel>
      <skos:definition xml:lang="da">Generation, der består af en kopi, der må anvendes af forskere.</skos:definition>
      <rdakit:toolkitDefinition xml:lang="da">Generation, der består af en kopi, der må anvendes af forskere.</rdakit:toolkitDefinition>
      <skos:scopeNote xml:lang="da">Denne term anvendes for ressourcer med levende billeder.</skos:scopeNote>
      <skos:prefLabel xml:lang="fr">copie de visionnement</skos:prefLabel>
      <rdakit:toolkitLabel xml:lang="fr">copie de visionnement</rdakit:toolkitLabel>
      <skos:definition xml:lang="fr">Génération qui consiste en une copie qui peut être visionnée par les chercheurs.</skos:definition>
      <rdakit:toolkitDefinition xml:lang="fr">Génération qui consiste en une copie qui peut être visionnée par les chercheurs.</rdakit:toolkitDefinition>
      <skos:scopeNote xml:lang="fr">Ce terme s’applique aux ressources filmiques.</skos:scopeNote>
      <skos:prefLabel xml:lang="no">visningseksemplar</skos:prefLabel>
      <rdakit:toolkitLabel xml:lang="no">visningseksemplar</rdakit:toolkitLabel>
      <skos:definition xml:lang="no">En generasjon som er en kopi som kan brukes av forskere.</skos:definition>
      <rdakit:toolkitDefinition xml:lang="no">En generasjon som er en kopi som kan brukes av forskere.</rdakit:toolkitDefinition>
      <skos:scopeNote xml:lang="no">Dette begrepet gjelder spillefilmressurser.</skos:scopeNote>
    </skos:Concept>

<!-- Status properties used in this document  -->
    <skos:Concept rdf:about="http://metadataregistry.org/uri/RegStatus/1001">
        <skos:prefLabel xml:lang="en">Published</skos:prefLabel>
    </skos:Concept>

</rdf:RDF>
