<?xml version="1.0" encoding = "UTF-8"?>
<rdf:RDF
    xmlns:dc="http://purl.org/dc/elements/1.1/"
    xmlns:rdakit="http://metadataregistry.org/uri/profile/rdakit/"
    xmlns:rdf="http://www.w3.org/1999/02/22-rdf-syntax-ns#"
    xmlns:reg="http://metadataregistry.org/uri/profile/regap/"
    xmlns:owl="http://www.w3.org/2002/07/owl#"
    xmlns:skos="http://www.w3.org/2004/02/skos/core#">

<owl:Ontology rdf:about="http://rdaregistry.info/termList/RDATerms" />
<!-- Scheme: RDA Terms -->
    <skos:ConceptScheme rdf:about="http://rdaregistry.info/termList/RDATerms">
        <dc:title>RDA Terms</dc:title>
    </skos:ConceptScheme>

<!-- Concept: access point  -->
    <skos:Concept rdf:about="http://rdaregistry.info/termList/RDATerms/1001" xml:lang="en">
      <skos:inScheme rdf:resource="http://rdaregistry.info/termList/RDATerms"/>
      <reg:status rdf:resource="http://metadataregistry.org/uri/RegStatus/1001"/>
      <reg:identifier rdf:resource="http://metadataregistry.org/concepts/8516"/>
      <skos:prefLabel xml:lang="en">access point</skos:prefLabel>
      <rdakit:toolkitLabel xml:lang="en">access point</rdakit:toolkitLabel>
      <skos:definition xml:lang="en">A name, term, code, etc., representing a specific entity.</skos:definition>
      <rdakit:toolkitDefinition xml:lang="en">A name, term, code, etc., representing a specific entity.</rdakit:toolkitDefinition>
	    <skos:narrower rdf:resource="http://rdaregistry.info/termList/RDATerms/1012"/>
	    <skos:narrower rdf:resource="http://rdaregistry.info/termList/RDATerms/1102"/>
      <skos:prefLabel xml:lang="it">punto d'accesso</skos:prefLabel>
      <rdakit:toolkitLabel xml:lang="it">punto d'accesso</rdakit:toolkitLabel>
      <skos:definition xml:lang="it">Nome, termine, codice, etc. che rappresenta un'entità specifica.</skos:definition>
      <rdakit:toolkitDefinition xml:lang="it">Nome, termine, codice, etc. che rappresenta un'entità specifica.</rdakit:toolkitDefinition>
      <skos:prefLabel xml:lang="fr">point d’accès</skos:prefLabel>
      <rdakit:toolkitLabel xml:lang="fr">point d’accès</rdakit:toolkitLabel>
      <skos:definition xml:lang="fr">Nom, terme, code, etc. représentant une entité spécifique.</skos:definition>
      <rdakit:toolkitDefinition xml:lang="fr">Nom, terme, code, etc. représentant une entité spécifique.</rdakit:toolkitDefinition>
      <skos:prefLabel xml:lang="es">punto de acceso</skos:prefLabel>
      <rdakit:toolkitLabel xml:lang="es">punto de acceso</rdakit:toolkitLabel>
      <skos:definition xml:lang="es">Nombre, término, código, etc., bajo el cual podrá encontrarse información que pertenece a una entidad específica.</skos:definition>
      <rdakit:toolkitDefinition xml:lang="es">Nombre, término, código, etc., bajo el cual podrá encontrarse información que pertenece a una entidad específica.</rdakit:toolkitDefinition>
      <skos:prefLabel xml:lang="de">Sucheinstieg</skos:prefLabel>
      <rdakit:toolkitLabel xml:lang="de">Sucheinstieg</rdakit:toolkitLabel>
      <skos:definition xml:lang="de">Ein Name, ein Terminus, ein Code usw., der eine bestimmte Entität repräsentiert.</skos:definition>
      <rdakit:toolkitDefinition xml:lang="de">Ein Name, ein Terminus, ein Code usw., der eine bestimmte Entität repräsentiert.</rdakit:toolkitDefinition>
      <skos:prefLabel xml:lang="fi">hakutieto</skos:prefLabel>
      <rdakit:toolkitLabel xml:lang="fi">hakutieto</rdakit:toolkitLabel>
      <skos:definition xml:lang="fi">Nimi, termi, koodi tms., joka edustaa tiettyä entiteettiä.</skos:definition>
      <rdakit:toolkitDefinition xml:lang="fi">Nimi, termi, koodi tms., joka edustaa tiettyä entiteettiä.</rdakit:toolkitDefinition>
      <skos:prefLabel xml:lang="da">søgeindgang</skos:prefLabel>
      <rdakit:toolkitLabel xml:lang="da">søgeindgang</rdakit:toolkitLabel>
      <skos:definition xml:lang="da">Navn, term, kode etc., der repræsenterer en bestemt entitet.</skos:definition>
      <rdakit:toolkitDefinition xml:lang="da">Navn, term, kode etc., der repræsenterer en bestemt entitet.</rdakit:toolkitDefinition>
      <skos:prefLabel xml:lang="ca">punt d’accés</skos:prefLabel>
      <rdakit:toolkitLabel xml:lang="ca">punt d’accés</rdakit:toolkitLabel>
      <skos:definition xml:lang="ca">Nom, terme, codi, etc., que representa una entitat concreta.</skos:definition>
      <rdakit:toolkitDefinition xml:lang="ca">Nom, terme, codi, etc., que representa una entitat concreta.</rdakit:toolkitDefinition>
      <skos:prefLabel xml:lang="vi">Điểm truy cập</skos:prefLabel>
      <rdakit:toolkitLabel xml:lang="vi">Điểm truy cập</rdakit:toolkitLabel>
      <skos:definition xml:lang="vi">Tên, thuật ngữ, mã, vv...trình bày một thực thể cụ thể.</skos:definition>
      <rdakit:toolkitDefinition xml:lang="vi">Tên, thuật ngữ, mã, vv...trình bày một thực thể cụ thể.</rdakit:toolkitDefinition>
      <skos:prefLabel xml:lang="no">søkeinngang</skos:prefLabel>
      <rdakit:toolkitLabel xml:lang="no">søkeinngang</rdakit:toolkitLabel>
      <skos:definition xml:lang="no">Et navn, et begrep, en kode, etc. som representerer en bestemt entitet.</skos:definition>
      <rdakit:toolkitDefinition xml:lang="no">Et navn, et begrep, en kode, etc. som representerer en bestemt entitet.</rdakit:toolkitDefinition>
    </skos:Concept>
<!-- Concept: accessible labels  -->
    <skos:Concept rdf:about="http://rdaregistry.info/termList/RDATerms/1002" xml:lang="en">
      <skos:inScheme rdf:resource="http://rdaregistry.info/termList/RDATerms"/>
      <reg:status rdf:resource="http://metadataregistry.org/uri/RegStatus/1001"/>
      <reg:identifier rdf:resource="http://metadataregistry.org/concepts/8517"/>
      <skos:prefLabel xml:lang="en">accessible labels</skos:prefLabel>
      <rdakit:toolkitLabel xml:lang="en">accessible labels</rdakit:toolkitLabel>
      <skos:definition xml:lang="en">An accessible tactile language text that is attached to a tactile image, map or diagram.</skos:definition>
      <rdakit:toolkitDefinition xml:lang="en">An accessible tactile language text that is attached to a tactile image, map or diagram.</rdakit:toolkitDefinition>
      <skos:prefLabel xml:lang="it">etichette accessibili</skos:prefLabel>
      <rdakit:toolkitLabel xml:lang="it">etichette accessibili</rdakit:toolkitLabel>
      <skos:definition xml:lang="it">Testo linguistico accessibile al tatto, presente su un'immagine, carta geografica o diagramma tattile.</skos:definition>
      <rdakit:toolkitDefinition xml:lang="it">Testo linguistico accessibile al tatto, presente su un'immagine, carta geografica o diagramma tattile.</rdakit:toolkitDefinition>
      <skos:prefLabel xml:lang="de">Barrierefreie Labels</skos:prefLabel>
      <rdakit:toolkitLabel xml:lang="de">Barrierefreie Labels</rdakit:toolkitLabel>
      <skos:definition xml:lang="de">Ein barrierefreier, taktiler Text, der einem taktilen Bild, einer taktilen Karte oder einem taktilen Diagramm beigelegt ist.</skos:definition>
      <rdakit:toolkitDefinition xml:lang="de">Ein barrierefreier, taktiler Text, der einem taktilen Bild, einer taktilen Karte oder einem taktilen Diagramm beigelegt ist.</rdakit:toolkitDefinition>
      <skos:prefLabel xml:lang="fi">kuvaseloste</skos:prefLabel>
      <rdakit:toolkitLabel xml:lang="fi">kuvaseloste</rdakit:toolkitLabel>
      <skos:definition xml:lang="fi">Tuntoaistiin perustuva teksti joka on liitetty tai toimitetaan yhdessä kosketukseen perustuvan kuvan, kartan tai kaavion kanssa.</skos:definition>
      <rdakit:toolkitDefinition xml:lang="fi">Tuntoaistiin perustuva teksti joka on liitetty tai toimitetaan yhdessä kosketukseen perustuvan kuvan, kartan tai kaavion kanssa.</rdakit:toolkitDefinition>
      <skos:prefLabel xml:lang="da">etiketter om tilgængelighed</skos:prefLabel>
      <rdakit:toolkitLabel xml:lang="da">etiketter om tilgængelighed</rdakit:toolkitLabel>
      <skos:definition xml:lang="da">Tilgængelig taktil tekst, fastgjort på et taktilt billede, kort eller diagram.</skos:definition>
      <rdakit:toolkitDefinition xml:lang="da">Tilgængelig taktil tekst, fastgjort på et taktilt billede, kort eller diagram.</rdakit:toolkitDefinition>
      <skos:prefLabel xml:lang="ca">etiquetes accessibles</skos:prefLabel>
      <rdakit:toolkitLabel xml:lang="ca">etiquetes accessibles</rdakit:toolkitLabel>
      <skos:definition xml:lang="ca">Text accessible en llenguatge tàctil que acompanya una imatge, un mapa o un diagrama tàctil.</skos:definition>
      <rdakit:toolkitDefinition xml:lang="ca">Text accessible en llenguatge tàctil que acompanya una imatge, un mapa o un diagrama tàctil.</rdakit:toolkitDefinition>
      <skos:prefLabel xml:lang="fr">étiquettes accessibles</skos:prefLabel>
      <rdakit:toolkitLabel xml:lang="fr">étiquettes accessibles</rdakit:toolkitLabel>
      <skos:definition xml:lang="fr">Texte accessible en langage tactile rattaché à une image, une carte ou un diagramme tactile.</skos:definition>
      <rdakit:toolkitDefinition xml:lang="fr">Texte accessible en langage tactile rattaché à une image, une carte ou un diagramme tactile.</rdakit:toolkitDefinition>
      <skos:prefLabel xml:lang="vi">Nhãn truy cập</skos:prefLabel>
      <rdakit:toolkitLabel xml:lang="vi">Nhãn truy cập</rdakit:toolkitLabel>
      <skos:definition xml:lang="vi">Văn bản ngôn ngữ xúc giác truy cập được gắn vào hình ảnh, bản đồ hoặc biểu đồ xúc giác.</skos:definition>
      <rdakit:toolkitDefinition xml:lang="vi">Văn bản ngôn ngữ xúc giác truy cập được gắn vào hình ảnh, bản đồ hoặc biểu đồ xúc giác.</rdakit:toolkitDefinition>
      <skos:prefLabel xml:lang="no">tilrettelagte etiketter</skos:prefLabel>
      <rdakit:toolkitLabel xml:lang="no">tilrettelagte etiketter</rdakit:toolkitLabel>
      <skos:definition xml:lang="no">En tilgjengelig taktil tekst som er tilknyttet et taktilt bilde, kart eller diagram.</skos:definition>
      <rdakit:toolkitDefinition xml:lang="no">En tilgjengelig taktil tekst som er tilknyttet et taktilt bilde, kart eller diagram.</rdakit:toolkitDefinition>
    </skos:Concept>
<!-- Concept: adaptation  -->
    <skos:Concept rdf:about="http://rdaregistry.info/termList/RDATerms/1003" xml:lang="en">
      <skos:inScheme rdf:resource="http://rdaregistry.info/termList/RDATerms"/>
      <reg:status rdf:resource="http://metadataregistry.org/uri/RegStatus/1001"/>
      <reg:identifier rdf:resource="http://metadataregistry.org/concepts/8518"/>
      <skos:prefLabel xml:lang="en">adaptation</skos:prefLabel>
      <rdakit:toolkitLabel xml:lang="en">adaptation</rdakit:toolkitLabel>
      <skos:definition xml:lang="en">A new derivative work created by revision of a previously existing work that substantially changes the nature and content of that work.</skos:definition>
      <rdakit:toolkitDefinition xml:lang="en">A new derivative work created by revision of a previously existing work that substantially changes the nature and content of that work.</rdakit:toolkitDefinition>
      <skos:scopeNote xml:lang="en">In the case of a musical work, a derivative work described as freely transcribed, based on, etc.; a revision incorporating new material; a paraphrase of various works by, or in the general style of, another composer; revisions in which the harmony or musical style of the original has been changed; performances involving substantial creative responsibility for adaptation, improvisation, etc., on the part of the performer or performers; or any other distinct alteration of another musical work, are included.</skos:scopeNote>
	    <skos:related rdf:resource="http://rdaregistry.info/termList/RDATerms/1008"/>
      <skos:prefLabel xml:lang="it">adattamento</skos:prefLabel>
      <rdakit:toolkitLabel xml:lang="it">adattamento</rdakit:toolkitLabel>
      <skos:definition xml:lang="it">Nuova opera derivata, nata dalla revisione di un'opera preesistente, che ne modifica sostanzialmente natura e contenuto.</skos:definition>
      <rdakit:toolkitDefinition xml:lang="it">Nuova opera derivata, nata dalla revisione di un'opera preesistente, che ne modifica sostanzialmente natura e contenuto.</rdakit:toolkitDefinition>
      <skos:prefLabel xml:lang="fr">adaptation</skos:prefLabel>
      <rdakit:toolkitLabel xml:lang="fr">adaptation</rdakit:toolkitLabel>
      <skos:definition xml:lang="fr">Nouvelle œuvre dérivée créée par la révision d’une œuvre préexistante qui change considérablement la nature et le contenu de cette œuvre.</skos:definition>
      <rdakit:toolkitDefinition xml:lang="fr">Nouvelle œuvre dérivée créée par la révision d’une œuvre préexistante qui change considérablement la nature et le contenu de cette œuvre.</rdakit:toolkitDefinition>
      <skos:prefLabel xml:lang="de">Bearbeitung</skos:prefLabel>
      <rdakit:toolkitLabel xml:lang="de">Bearbeitung</rdakit:toolkitLabel>
      <skos:definition xml:lang="de">Ein neues abgeleitetes Werk, das durch die Überarbeitung eines zuvor existierenden Werks geschaffen wird, das die Art und den Inhalt dieses Werks substanziell ändert.</skos:definition>
      <rdakit:toolkitDefinition xml:lang="de">Ein neues abgeleitetes Werk, das durch die Überarbeitung eines zuvor existierenden Werks geschaffen wird, das die Art und den Inhalt dieses Werks substanziell ändert.</rdakit:toolkitDefinition>
      <skos:scopeNote xml:lang="de">Im Fall eines Musikwerks ein abgeleitetes Werk, das als frei transkribiert, basierend auf usw. beschrieben wird; eine Überarbeitung, die neues Material enthält; eine Paraphrase verschiedener Werke von oder im allgemeinen Stil eines anderen Komponisten; Überarbeitungen, in denen die Harmonie oder der Musikstil des Originals geändert ist; Aufführungen, die substanzielle schöpferische Verantwortung für die Bearbeitung, Improvisation usw. auf Seiten des oder der Aufführenden haben; oder jede andere deutliche Veränderung eines anderen Musikwerks.</skos:scopeNote>
      <skos:prefLabel xml:lang="fi">mukaelma</skos:prefLabel>
      <rdakit:toolkitLabel xml:lang="fi">mukaelma</rdakit:toolkitLabel>
      <skos:definition xml:lang="fi">Uusi johdannaisteos, joka on luotu muokkaamalla varhaisempaa teosta siten, että tämän luonne ja sisältö ovat muuttuneet olennaisesti.</skos:definition>
      <rdakit:toolkitDefinition xml:lang="fi">Uusi johdannaisteos, joka on luotu muokkaamalla varhaisempaa teosta siten, että tämän luonne ja sisältö ovat muuttuneet olennaisesti.</rdakit:toolkitDefinition>
      <skos:scopeNote xml:lang="fi">Musiikkiteosten yhteydessä: johdannaisteos, jota luonnehditaan seuraavasti: “vapaasti transkriboitu”, “perustuu [johonkin]” tms.</skos:scopeNote>
      <skos:prefLabel xml:lang="da">bearbejdelse</skos:prefLabel>
      <rdakit:toolkitLabel xml:lang="da">bearbejdelse</rdakit:toolkitLabel>
      <skos:definition xml:lang="da">Nyt afledt værk skabt ved omarbejdelse af et tidligere eksisterende værk, der ændrer dette værks oprindelige natur og indhold betydeligt.</skos:definition>
      <rdakit:toolkitDefinition xml:lang="da">Nyt afledt værk skabt ved omarbejdelse af et tidligere eksisterende værk, der ændrer dette værks oprindelige natur og indhold betydeligt.</rdakit:toolkitDefinition>
      <skos:scopeNote xml:lang="da">Hvis der er tale om et musikværk: et afledt værk, der beskrives som frit omskrevet, baseret på etc.; en revision, der indarbejder nyt materiale; en parafrase af flere værker af en anden komponist eller i dennes generelle stil; revisioner, hvori originalens harmonisering eller musikalske stil er ændret; opførelser, der medfører væsentligt kreativt ansvar for bearbejdelse, improvisation etc. for udøveren/udøverne; eller enhver anden markant ændring af et andet musikværk er omfattet.</skos:scopeNote>
      <skos:prefLabel xml:lang="ca">adaptació</skos:prefLabel>
      <rdakit:toolkitLabel xml:lang="ca">adaptació</rdakit:toolkitLabel>
      <skos:definition xml:lang="ca">Obra derivada nova creada a partir de la revisió d’una obra que existia prèviament i que en canvia substancialment la natura i el contingut.</skos:definition>
      <rdakit:toolkitDefinition xml:lang="ca">Obra derivada nova creada a partir de la revisió d’una obra que existia prèviament i que en canvia substancialment la natura i el contingut.</rdakit:toolkitDefinition>
      <skos:scopeNote xml:lang="ca">Inclou, en el cas d’una obra musical, una obra derivada que es descriu com a transcrita lliurement, basada en, etc.; una revisió que incorpora material nou; una paràfrasi de diverses obres d’un altre compositor, o en el seu estil general; revisions en les quals s’ha canviat l’harmonia o l’estil musical de l’original; interpretacions que suposen una responsabilitat creativa substancial d’adaptació, d’improvisació, etc., de part de l’intèrpret o els intèrprets; o qualsevol altra alteració distinta d’una altra obra musical.</skos:scopeNote>
      <skos:scopeNote xml:lang="fr">Dans le cas d’une œuvre musicale, comprend une œuvre dérivée décrite comme librement transcrite, basée sur, etc. ; une révision incorporant un nouveau matériau ; une paraphrase d’œuvres diverses ou dans le style général d’un autre compositeur ; les révisions dans lesquelles l’harmonie ou le style musical de l’original a été modifié ; les prestations impliquant de la part du ou des interprètes une importante responsabilité de création en matière d’adaptation, d’improvisation, etc. ; ou toute autre modification notable d’une autre œuvre musicale.</skos:scopeNote>
      <skos:prefLabel xml:lang="vi">Phóng tác</skos:prefLabel>
      <rdakit:toolkitLabel xml:lang="vi">Phóng tác</rdakit:toolkitLabel>
      <skos:definition xml:lang="vi">Tác phẩm dẫn xuất mới được sáng tạo bằng cách sửa đổi tác phẩm đã có từ trước với sự thay đổi lớn về bản chất và nội dung của tác phẩm đó.</skos:definition>
      <rdakit:toolkitDefinition xml:lang="vi">Tác phẩm dẫn xuất mới được sáng tạo bằng cách sửa đổi tác phẩm đã có từ trước với sự thay đổi lớn về bản chất và nội dung của tác phẩm đó.</rdakit:toolkitDefinition>
      <skos:scopeNote xml:lang="vi">Trong trường hợp tác phẩm âm nhạc, tác phẩm dẫn xuất được mô tả như là được chuyển biên, dựa trên, v.v...; sửa đổi kết hợp tài liệu mới; diễn giải tác phẩm khác bởi, hoặc với phong cách chung của, người soạn khác; sửa đổi với hoà âm và phong cách âm nhạc của nguyên gốc bị thay đổi; biểu diễn với trách nhiệm sáng tạo lớn đối với phóng tác, tức hứng, v.v..., về bè của người biểu diễn hoặc những người biểu diễn; hoặc bất kỳ sự lựa chọn riêng biệt khác của tác phẩm âm nhạc, được bao gồm.</skos:scopeNote>
      <skos:prefLabel xml:lang="no">bearbeidelse</skos:prefLabel>
      <rdakit:toolkitLabel xml:lang="no">bearbeidelse</rdakit:toolkitLabel>
      <skos:definition xml:lang="no">Et nytt avledet eller bearbeidet verk skapt ved revidering av et allerede eksisterende verk, som vesentlig forandrer dette verkets natur og innhold.</skos:definition>
      <rdakit:toolkitDefinition xml:lang="no">Et nytt avledet eller bearbeidet verk skapt ved revidering av et allerede eksisterende verk, som vesentlig forandrer dette verkets natur og innhold.</rdakit:toolkitDefinition>
      <skos:scopeNote xml:lang="no">For musikalske verk gjelder dette avledede eller bearbeidede verk beskrevet som fritt omskrevet, basert på etc., en revisjon som omfatter nytt materiale, en omskrivning av ulike verk av, eller i samme stil som, en annen komponist, revisjoner der originalens harmonikk eller musikalske stil er endret, framføringer der utøveren eller utøverne har omfattende kreativt ansvar for bearbeidelse, improvisasjon etc., eller enhver annen tydelig endring av et musikalsk verk.</skos:scopeNote>
    </skos:Concept>
<!-- Concept: added title page  -->
    <skos:Concept rdf:about="http://rdaregistry.info/termList/RDATerms/1004" xml:lang="en">
      <skos:inScheme rdf:resource="http://rdaregistry.info/termList/RDATerms"/>
      <reg:status rdf:resource="http://metadataregistry.org/uri/RegStatus/1001"/>
      <reg:identifier rdf:resource="http://metadataregistry.org/concepts/8519"/>
      <skos:prefLabel xml:lang="en">added title page</skos:prefLabel>
      <rdakit:toolkitLabel xml:lang="en">added title page</rdakit:toolkitLabel>
      <skos:definition xml:lang="en">A title page preceding or following the title page chosen as the preferred source of information.</skos:definition>
      <rdakit:toolkitDefinition xml:lang="en">A title page preceding or following the title page chosen as the preferred source of information.</rdakit:toolkitDefinition>
      <skos:scopeNote xml:lang="en">An added title page may be more general or equally general. A series title page is an example of a more general title page; a title page is another language is an example of an equally general title page.</skos:scopeNote>
	    <skos:related rdf:resource="http://rdaregistry.info/termList/RDATerms/1095"/>
	    <skos:related rdf:resource="http://rdaregistry.info/termList/RDATerms/1082"/>
      <skos:prefLabel xml:lang="it">frontespizio aggiunto</skos:prefLabel>
      <rdakit:toolkitLabel xml:lang="it">frontespizio aggiunto</rdakit:toolkitLabel>
      <skos:definition xml:lang="it">Frontespizio che precede o segue il frontespizio scelto come fonte d'informazione preferita.</skos:definition>
      <rdakit:toolkitDefinition xml:lang="it">Frontespizio che precede o segue il frontespizio scelto come fonte d'informazione preferita.</rdakit:toolkitDefinition>
      <skos:scopeNote xml:lang="it">Può essere di livello superiore (per esempio, un frontespizio della serie) o dello stesso livello (per esempio, un frontespizio in un'altra lingua).</skos:scopeNote>
      <skos:prefLabel xml:lang="de">Zusätzliche Titelseite</skos:prefLabel>
      <rdakit:toolkitLabel xml:lang="de">Zusätzliche Titelseite</rdakit:toolkitLabel>
      <skos:definition xml:lang="de">Eine Titelseite vor oder hinter der Titelseite, die als bevorzugte Informationsquelle gewählt wurde.</skos:definition>
      <rdakit:toolkitDefinition xml:lang="de">Eine Titelseite vor oder hinter der Titelseite, die als bevorzugte Informationsquelle gewählt wurde.</rdakit:toolkitDefinition>
      <skos:scopeNote xml:lang="de">Sie kann allgemeiner (z. B. eine Titelseite der Reihe) oder gleichermaßen allgemein (z. B. eine Titelseite in einer anderen Sprache) sein.</skos:scopeNote>
      <skos:prefLabel xml:lang="fi">lisätty nimiösivu</skos:prefLabel>
      <rdakit:toolkitLabel xml:lang="fi">lisätty nimiösivu</rdakit:toolkitLabel>
      <skos:definition xml:lang="fi">Nimiösivu, joka edeltää tai seuraa nimiösivua, joka on valittu ensisijaiseksi tiedonlähteeksi.</skos:definition>
      <rdakit:toolkitDefinition xml:lang="fi">Nimiösivu, joka edeltää tai seuraa nimiösivua, joka on valittu ensisijaiseksi tiedonlähteeksi.</rdakit:toolkitDefinition>
      <skos:scopeNote xml:lang="fi">Lisätty nimiösivu voi olla yleisempi tai yhtä yleinen. Esim. sarjan nimiösivu on esimerkki yleisemmästä nimiösivusta.</skos:scopeNote>
      <skos:prefLabel xml:lang="da">ekstra titelside</skos:prefLabel>
      <rdakit:toolkitLabel xml:lang="da">ekstra titelside</rdakit:toolkitLabel>
      <skos:definition xml:lang="da">Titelside, der kommer før eller efter den titelside, der er valgt som foretrukken kilde til oplysninger.</skos:definition>
      <rdakit:toolkitDefinition xml:lang="da">Titelside, der kommer før eller efter den titelside, der er valgt som foretrukken kilde til oplysninger.</rdakit:toolkitDefinition>
      <skos:scopeNote xml:lang="da">En ekstra titelside kan være mere generel eller lige så generel. En serietitelside er et eksempel på en mere generell titelside; en titelside på et andet sprog er et eksempel på en lige så generel titelside.</skos:scopeNote>
      <skos:prefLabel xml:lang="ca">portada addicional</skos:prefLabel>
      <rdakit:toolkitLabel xml:lang="ca">portada addicional</rdakit:toolkitLabel>
      <skos:definition xml:lang="ca">Portada que precedeix o segueix la portada triada com la font preferida d’informació.</skos:definition>
      <rdakit:toolkitDefinition xml:lang="ca">Portada que precedeix o segueix la portada triada com la font preferida d’informació.</rdakit:toolkitDefinition>
      <skos:scopeNote xml:lang="ca">Una portada addicional pot ser més general o igualment general. Una portada de col·lecció és un exemple d'una portada més general; una portada en una altra llengua és un exemple d'una portada igualment general.</skos:scopeNote>
      <skos:prefLabel xml:lang="fr">page de titre supplémentaire</skos:prefLabel>
      <rdakit:toolkitLabel xml:lang="fr">page de titre supplémentaire</rdakit:toolkitLabel>
      <skos:definition xml:lang="fr">Page de titre précédant ou suivant la page de titre choisie comme source d’information privilégiée.</skos:definition>
      <rdakit:toolkitDefinition xml:lang="fr">Page de titre précédant ou suivant la page de titre choisie comme source d’information privilégiée.</rdakit:toolkitDefinition>
      <skos:scopeNote xml:lang="fr">Une page de titre supplémentaire peut être plus générale ou tout aussi générale. Une page de titre de collection est un exemple de page plus générale ; une page de titre dans une autre langue est un exemple de page tout aussi générale.</skos:scopeNote>
      <skos:prefLabel xml:lang="vi">Trang nhan đề phụ</skos:prefLabel>
      <rdakit:toolkitLabel xml:lang="vi">Trang nhan đề phụ</rdakit:toolkitLabel>
      <skos:definition xml:lang="vi">Trang nhan đề ở trước hoặc sau trang nhan đề được lựa chọn như là nguồn lấy thông tin ưu tiên.</skos:definition>
      <rdakit:toolkitDefinition xml:lang="vi">Trang nhan đề ở trước hoặc sau trang nhan đề được lựa chọn như là nguồn lấy thông tin ưu tiên.</rdakit:toolkitDefinition>
      <skos:scopeNote xml:lang="vi">Trang nhan đề phụ có thể tổng quát hơn. Trang nhan đề tùng thư là một ví dụ của trang nhan đề tổng quát hơn; trang nhan đề trong ngôn ngữ khác là ví dụ của trang nhan đề ngang bằng.</skos:scopeNote>
      <skos:prefLabel xml:lang="no">ekstra tittelside</skos:prefLabel>
      <rdakit:toolkitLabel xml:lang="no">ekstra tittelside</rdakit:toolkitLabel>
      <skos:definition xml:lang="no">En tittelside foran eller etter den tittelsiden som er valgt som foretrukket informasjonskilde.</skos:definition>
      <rdakit:toolkitDefinition xml:lang="no">En tittelside foran eller etter den tittelsiden som er valgt som foretrukket informasjonskilde.</rdakit:toolkitDefinition>
      <skos:scopeNote xml:lang="no">En ekstra tittelside kan være mer generell eller like generell. En tittelside for serie er et eksempel på en mer generell tittelside, mens en tittelside på et annet språk er et eksempel på en like generell tittelside.</skos:scopeNote>
    </skos:Concept>
<!-- Concept: alternative title  -->
    <skos:Concept rdf:about="http://rdaregistry.info/termList/RDATerms/1005" xml:lang="en">
      <skos:inScheme rdf:resource="http://rdaregistry.info/termList/RDATerms"/>
      <reg:status rdf:resource="http://metadataregistry.org/uri/RegStatus/1001"/>
      <reg:identifier rdf:resource="http://metadataregistry.org/concepts/8520"/>
      <skos:prefLabel xml:lang="en">alternative title</skos:prefLabel>
      <rdakit:toolkitLabel xml:lang="en">alternative title</rdakit:toolkitLabel>
      <skos:definition xml:lang="en">A second part of a title proper that consists of two parts, each of which has the form of an independent title, joined by a word such as &quot;or&quot; or its equivalent in another language.</skos:definition>
      <rdakit:toolkitDefinition xml:lang="en">A second part of a title proper that consists of two parts, each of which has the form of an independent title, joined by a word such as &quot;or&quot; or its equivalent in another language.</rdakit:toolkitDefinition>
      <skos:prefLabel xml:lang="it">titolo alternativo</skos:prefLabel>
      <rdakit:toolkitLabel xml:lang="it">titolo alternativo</rdakit:toolkitLabel>
      <skos:definition xml:lang="it">Seconda parte di un titolo proprio che consiste di due parti (ciascuna delle quali ha la forma di un titolo indipendente), unite da una congiunzione come o o da un suo equivalente in altra lingua.</skos:definition>
      <rdakit:toolkitDefinition xml:lang="it">Seconda parte di un titolo proprio che consiste di due parti (ciascuna delle quali ha la forma di un titolo indipendente), unite da una congiunzione come o o da un suo equivalente in altra lingua.</rdakit:toolkitDefinition>
      <skos:prefLabel xml:lang="fr">titre alternatif</skos:prefLabel>
      <rdakit:toolkitLabel xml:lang="fr">titre alternatif</rdakit:toolkitLabel>
      <skos:definition xml:lang="fr">Seconde partie d’un titre propre composé de deux parties dont chacune se présente comme un titre indépendant et qui sont reliées par un mot tel que « ou » ou son équivalent dans une autre langue.</skos:definition>
      <rdakit:toolkitDefinition xml:lang="fr">Seconde partie d’un titre propre composé de deux parties dont chacune se présente comme un titre indépendant et qui sont reliées par un mot tel que « ou » ou son équivalent dans une autre langue.</rdakit:toolkitDefinition>
      <skos:prefLabel xml:lang="es">título alternativo</skos:prefLabel>
      <rdakit:toolkitLabel xml:lang="es">título alternativo</rdakit:toolkitLabel>
      <skos:definition xml:lang="es">Segunda parte de un título propiamente dicho que consiste en dos partes (cada una de las cuales tiene la forma de un título independiente), unida mediante una palabra tal como &quot;o&quot; o su equivalente en otra lengua.</skos:definition>
      <rdakit:toolkitDefinition xml:lang="es">Segunda parte de un título propiamente dicho que consiste en dos partes (cada una de las cuales tiene la forma de un título independiente), unida mediante una palabra tal como &quot;o&quot; o su equivalente en otra lengua.</rdakit:toolkitDefinition>
      <skos:prefLabel xml:lang="de">Alternativtitel</skos:prefLabel>
      <rdakit:toolkitLabel xml:lang="de">Alternativtitel</rdakit:toolkitLabel>
      <skos:definition xml:lang="de">Der zweite Teil eines Haupttitels, der aus zwei Teilen besteht (von denen jeder die Form eines unabhängigen Titels hat), die mit einem Wort wie „oder“ oder dessen Entsprechung in einer anderen Sprache verbunden sind.</skos:definition>
      <rdakit:toolkitDefinition xml:lang="de">Der zweite Teil eines Haupttitels, der aus zwei Teilen besteht (von denen jeder die Form eines unabhängigen Titels hat), die mit einem Wort wie „oder“ oder dessen Entsprechung in einer anderen Sprache verbunden sind.</rdakit:toolkitDefinition>
      <skos:prefLabel xml:lang="fi">vaihtoehtoinen nimeke</skos:prefLabel>
      <rdakit:toolkitLabel xml:lang="fi">vaihtoehtoinen nimeke</rdakit:toolkitLabel>
      <skos:definition xml:lang="fi">Kahdesta osasta koostuvan päänimekkeen jälkimmäinen osa, joka on myös muodoltaan itsenäinen. Osia yhdistää sana ”tai”, ”eli” tai vastaava muunkielinen sana.</skos:definition>
      <rdakit:toolkitDefinition xml:lang="fi">Kahdesta osasta koostuvan päänimekkeen jälkimmäinen osa, joka on myös muodoltaan itsenäinen. Osia yhdistää sana ”tai”, ”eli” tai vastaava muunkielinen sana.</rdakit:toolkitDefinition>
      <skos:prefLabel xml:lang="da">alternativ titel</skos:prefLabel>
      <rdakit:toolkitLabel xml:lang="da">alternativ titel</rdakit:toolkitLabel>
      <skos:definition xml:lang="da">Anden del af en hovedtitel, bestående af to selvstændige titler, der forbindes af et ord som fx  ’eller’ eller et tilsvarende ord på et andet sprog.</skos:definition>
      <rdakit:toolkitDefinition xml:lang="da">Anden del af en hovedtitel, bestående af to selvstændige titler, der forbindes af et ord som fx  ’eller’ eller et tilsvarende ord på et andet sprog.</rdakit:toolkitDefinition>
      <skos:prefLabel xml:lang="ca">títol alternatiu</skos:prefLabel>
      <rdakit:toolkitLabel xml:lang="ca">títol alternatiu</rdakit:toolkitLabel>
      <skos:definition xml:lang="ca">Segona part d’un títol propi que consisteix en dues parts, cada una de les quals té la forma d’un títol independent, unides per una paraula com ara “o” o el seu equivalent en una altra llengua.</skos:definition>
      <rdakit:toolkitDefinition xml:lang="ca">Segona part d’un títol propi que consisteix en dues parts, cada una de les quals té la forma d’un títol independent, unides per una paraula com ara “o” o el seu equivalent en una altra llengua.</rdakit:toolkitDefinition>
      <skos:prefLabel xml:lang="vi">nhan đề lựa chọn</skos:prefLabel>
      <rdakit:toolkitLabel xml:lang="vi">nhan đề lựa chọn</rdakit:toolkitLabel>
      <skos:definition xml:lang="vi">Phần thứ hai của nhan đề hợp thức chứa hai phần, mỗi phần có hình thái của nhan đề độc lập, được nối bằng từ như “or” hoặc tương đương trong ngôn ngữ khác</skos:definition>
      <rdakit:toolkitDefinition xml:lang="vi">Phần thứ hai của nhan đề hợp thức chứa hai phần, mỗi phần có hình thái của nhan đề độc lập, được nối bằng từ như “or” hoặc tương đương trong ngôn ngữ khác</rdakit:toolkitDefinition>
      <skos:prefLabel xml:lang="no">alternativ tittel</skos:prefLabel>
      <rdakit:toolkitLabel xml:lang="no">alternativ tittel</rdakit:toolkitLabel>
      <skos:definition xml:lang="no">Annen del av en hovedtittel som består av to deler hvor begge kan betraktes som uavhengige titler, og som er knyttet til hverandre med ordet “eller” eller tilsvarende ord på et annet språk.</skos:definition>
      <rdakit:toolkitDefinition xml:lang="no">Annen del av en hovedtittel som består av to deler hvor begge kan betraktes som uavhengige titler, og som er knyttet til hverandre med ordet “eller” eller tilsvarende ord på et annet språk.</rdakit:toolkitDefinition>
    </skos:Concept>
<!-- Concept: analytical description  -->
    <skos:Concept rdf:about="http://rdaregistry.info/termList/RDATerms/1006" xml:lang="en">
      <skos:inScheme rdf:resource="http://rdaregistry.info/termList/RDATerms"/>
      <reg:status rdf:resource="http://metadataregistry.org/uri/RegStatus/1001"/>
      <reg:identifier rdf:resource="http://metadataregistry.org/concepts/8521"/>
      <skos:prefLabel xml:lang="en">analytical description</skos:prefLabel>
      <rdakit:toolkitLabel xml:lang="en">analytical description</rdakit:toolkitLabel>
      <skos:definition xml:lang="en">A description that describes a part of a larger manifestation.</skos:definition>
      <rdakit:toolkitDefinition xml:lang="en">A description that describes a part of a larger manifestation.</rdakit:toolkitDefinition>
      <skos:scopeNote xml:lang="en">Analytical description includes a description for a single volume of a three-volume biography, a single map forming part of a map series, etc.</skos:scopeNote>
      <skos:prefLabel xml:lang="it">descrizione analitica</skos:prefLabel>
      <rdakit:toolkitLabel xml:lang="it">descrizione analitica</rdakit:toolkitLabel>
      <skos:definition xml:lang="it">Descrizione di una parte di una risorsa più ampia</skos:definition>
      <rdakit:toolkitDefinition xml:lang="it">Descrizione di una parte di una risorsa più ampia</rdakit:toolkitDefinition>
      <skos:prefLabel xml:lang="fr">description analytique</skos:prefLabel>
      <rdakit:toolkitLabel xml:lang="fr">description analytique</rdakit:toolkitLabel>
      <skos:definition xml:lang="fr">Description d’une partie d’une manifestation plus vaste.</skos:definition>
      <rdakit:toolkitDefinition xml:lang="fr">Description d’une partie d’une manifestation plus vaste.</rdakit:toolkitDefinition>
      <skos:prefLabel xml:lang="es">descripción analítica</skos:prefLabel>
      <rdakit:toolkitLabel xml:lang="es">descripción analítica</rdakit:toolkitLabel>
      <skos:definition xml:lang="es">Descripción que describe una parte de un recurso mayor.</skos:definition>
      <rdakit:toolkitDefinition xml:lang="es">Descripción que describe una parte de un recurso mayor.</rdakit:toolkitDefinition>
      <skos:prefLabel xml:lang="de">Analytische Beschreibung</skos:prefLabel>
      <rdakit:toolkitLabel xml:lang="de">Analytische Beschreibung</rdakit:toolkitLabel>
      <skos:definition xml:lang="de">Eine Beschreibung, die einen Teil einer größeren Manifestation beschreibt.</skos:definition>
      <rdakit:toolkitDefinition xml:lang="de">Eine Beschreibung, die einen Teil einer größeren Manifestation beschreibt.</rdakit:toolkitDefinition>
      <skos:scopeNote xml:lang="de">Zur analytischen Beschreibung zählt die Beschreibung eines Einzelbandes einer dreibändigen Biografie, eine einzelne Karte als Teil eines Kartensatzes usw.</skos:scopeNote>
      <skos:prefLabel xml:lang="fi">analyyttinen kuvailu</skos:prefLabel>
      <rdakit:toolkitLabel xml:lang="fi">analyyttinen kuvailu</rdakit:toolkitLabel>
      <skos:definition xml:lang="fi">Kuvailu, joka kuvailee laajemman manifestaation yksittäisen osan.</skos:definition>
      <rdakit:toolkitDefinition xml:lang="fi">Kuvailu, joka kuvailee laajemman manifestaation yksittäisen osan.</rdakit:toolkitDefinition>
      <skos:scopeNote xml:lang="fi">Esim. kolmiosaisen elämäkerran yhden osan kuvailu, karttasarjan yksittäisen kartan kuvailu.</skos:scopeNote>
      <skos:prefLabel xml:lang="da">analytisk beskrivelse</skos:prefLabel>
      <rdakit:toolkitLabel xml:lang="da">analytisk beskrivelse</rdakit:toolkitLabel>
      <skos:definition xml:lang="da">Beskrivelse af en del af en større manifestation.</skos:definition>
      <rdakit:toolkitDefinition xml:lang="da">Beskrivelse af en del af en større manifestation.</rdakit:toolkitDefinition>
      <skos:scopeNote xml:lang="da">Analytisk beskrivelse omfatter en beskrivelse af et enkelt bind af en trebindsbiografi, et enkelt kort, der er en del af en kortserie etc.</skos:scopeNote>
      <skos:prefLabel xml:lang="ca">descripció analítica</skos:prefLabel>
      <rdakit:toolkitLabel xml:lang="ca">descripció analítica</rdakit:toolkitLabel>
      <skos:definition xml:lang="ca">Descripció que descriu una part d’una manifestació més gran.</skos:definition>
      <rdakit:toolkitDefinition xml:lang="ca">Descripció que descriu una part d’una manifestació més gran.</rdakit:toolkitDefinition>
      <skos:scopeNote xml:lang="ca">La descripció analítica inclou una descripció per a un volum sol d’una biografia en tres volums, un mapa sol que forma part d’una sèrie de mapes, etc.</skos:scopeNote>
      <skos:scopeNote xml:lang="fr">Comprend une description d’un volume isolé d’une biographie en trois volumes, une carte isolée d’une série cartographique, etc.</skos:scopeNote>
      <skos:prefLabel xml:lang="vi">mô tả phân tích</skos:prefLabel>
      <rdakit:toolkitLabel xml:lang="vi">mô tả phân tích</rdakit:toolkitLabel>
      <skos:definition xml:lang="vi">Mô tả mô tả phần của biểu thị lớn hơn.</skos:definition>
      <rdakit:toolkitDefinition xml:lang="vi">Mô tả mô tả phần của biểu thị lớn hơn.</rdakit:toolkitDefinition>
      <skos:scopeNote xml:lang="vi">Mô tả phân tích bao gồm mô tả một tập đơn lẻ của bộ tiểu sử ba tập, một bản đồ đơn lẻ tạo thành phần của một tùng thư bản đồ, v.v...</skos:scopeNote>
      <skos:prefLabel xml:lang="no">analytisk beskrivelse</skos:prefLabel>
      <rdakit:toolkitLabel xml:lang="no">analytisk beskrivelse</rdakit:toolkitLabel>
      <skos:definition xml:lang="no">En beskrivelse som beskriver en del av en større manifestasjon.</skos:definition>
      <rdakit:toolkitDefinition xml:lang="no">En beskrivelse som beskriver en del av en større manifestasjon.</rdakit:toolkitDefinition>
      <skos:scopeNote xml:lang="no">Analytisk beskrivelse inkluderer en beskrivelse av et enkeltbind i en trebinds biografi, et enkeltkart som er del av en kartserie, etc.</skos:scopeNote>
    </skos:Concept>
<!-- Concept: archival resource  -->
    <skos:Concept rdf:about="http://rdaregistry.info/termList/RDATerms/1007" xml:lang="en">
      <skos:inScheme rdf:resource="http://rdaregistry.info/termList/RDATerms"/>
      <reg:status rdf:resource="http://metadataregistry.org/uri/RegStatus/1001"/>
      <reg:identifier rdf:resource="http://metadataregistry.org/concepts/8522"/>
      <skos:prefLabel xml:lang="en">archival resource</skos:prefLabel>
      <rdakit:toolkitLabel xml:lang="en">archival resource</rdakit:toolkitLabel>
      <skos:definition xml:lang="en">A document or documents organically created, accumulated, or used by an agent in the course of the conduct of affairs and preserved because of their continuing value.</skos:definition>
      <rdakit:toolkitDefinition xml:lang="en">A document or documents organically created, accumulated, or used by an agent in the course of the conduct of affairs and preserved because of their continuing value.</rdakit:toolkitDefinition>
      <skos:scopeNote xml:lang="en">The resource may be an aggregation of documents or it may be a discrete item. It may also be a collection acquired and assembled by an archival repository, individual, or other institution, that does not share a common provenance or origin but that reflects some common characteristic, for example, a particular subject, theme, or form.</skos:scopeNote>
      <skos:prefLabel xml:lang="it">risorsa archivistica</skos:prefLabel>
      <rdakit:toolkitLabel xml:lang="it">risorsa archivistica</rdakit:toolkitLabel>
      <skos:definition xml:lang="it">Documento o documenti creati, accumulati e/o utilizzati organicamente da una persona, famiglia, ente nella conduzione delle proprie attività e conservati per il loro valore permanente.</skos:definition>
      <rdakit:toolkitDefinition xml:lang="it">Documento o documenti creati, accumulati e/o utilizzati organicamente da una persona, famiglia, ente nella conduzione delle proprie attività e conservati per il loro valore permanente.</rdakit:toolkitDefinition>
      <skos:scopeNote xml:lang="it">Questa risorsa può essere un'aggregazione di documenti o può essere un item distinto. Può essere anche una collezione acquisita e assemblata da un archivio, individuo o altra istituzione, che non ha una provenienza o un'origine comune ma condivide qualche caratteristica comune, per esempio, un soggetto, un tema o una forma particolari.</skos:scopeNote>
      <skos:prefLabel xml:lang="fr">ressource archivistique</skos:prefLabel>
      <rdakit:toolkitLabel xml:lang="fr">ressource archivistique</rdakit:toolkitLabel>
      <skos:definition xml:lang="fr">Document ou ensemble de documents organiquement créé, accumulé ou utilisé par un agent au cours de son activité et préservé en raison de sa valeur permanente.</skos:definition>
      <rdakit:toolkitDefinition xml:lang="fr">Document ou ensemble de documents organiquement créé, accumulé ou utilisé par un agent au cours de son activité et préservé en raison de sa valeur permanente.</rdakit:toolkitDefinition>
      <skos:scopeNote xml:lang="fr">La ressource peut être aussi bien une agrégation de documents qu’un item isolé. Elle peut être également une collection acquise et rassemblée par un dépôt d’archives, un particulier ou une autre institution, qui n’a ni provenance ni origine communes mais qui présente des caractéristiques communes, comme un sujet, un thème ou une forme spécifiques.</skos:scopeNote>
      <skos:prefLabel xml:lang="es">recurso archivítico</skos:prefLabel>
      <rdakit:toolkitLabel xml:lang="es">recurso archivítico</rdakit:toolkitLabel>
      <skos:definition xml:lang="es">Documento o documentos creados orgánicamente, acumulados y/o usados por una persona, familia o entidad corporativa en el curso de la gestión de sus asuntos; y preservada debido a su valor duradero.</skos:definition>
      <rdakit:toolkitDefinition xml:lang="es">Documento o documentos creados orgánicamente, acumulados y/o usados por una persona, familia o entidad corporativa en el curso de la gestión de sus asuntos; y preservada debido a su valor duradero.</rdakit:toolkitDefinition>
      <skos:scopeNote xml:lang="es">Este recurso puede ser una agregación de documentos o puede ser un ítem separado. También puede ser una colección adquirida y reunida por un repositorio de archivo, un individuo u otra institución, que no comparte un origen o procedencia común pero que refleja alguna característica común, por ejemplo, un tema, una materia o una forma determinadas.</skos:scopeNote>
      <skos:prefLabel xml:lang="de">Archivalische Ressource</skos:prefLabel>
      <rdakit:toolkitLabel xml:lang="de">Archivalische Ressource</rdakit:toolkitLabel>
      <skos:definition xml:lang="de">Ein Dokument oder Dokumente, das/die organisch gewachsen und angefallen ist/sind und/oder von einem Akteur bei der Abwicklung von Geschäften benutzt und aufgrund ihres dauerhaften Wertes aufbewahrt werden.</skos:definition>
      <rdakit:toolkitDefinition xml:lang="de">Ein Dokument oder Dokumente, das/die organisch gewachsen und angefallen ist/sind und/oder von einem Akteur bei der Abwicklung von Geschäften benutzt und aufgrund ihres dauerhaften Wertes aufbewahrt werden.</rdakit:toolkitDefinition>
      <skos:scopeNote xml:lang="de">Diese Ressource kann eine Aggregation von Dokumenten oder ein einzelnes Objekt sein. Es kann sich auch um eine Sammlung handeln, die von einem Archivrepository, einem Individuum oder einer anderen Institution erworben und gesammelt wurde, wobei die (einzelnen Bestandteile) keine gemeinsame Herkunft oder Ursprung, aber eine gemeinsame Eigenschaft haben, z. B. ein bestimmtes Fachgebiet, ein Thema oder eine Form.</skos:scopeNote>
      <skos:prefLabel xml:lang="fi">arkistoaineisto</skos:prefLabel>
      <rdakit:toolkitLabel xml:lang="fi">arkistoaineisto</rdakit:toolkitLabel>
      <skos:definition xml:lang="fi">Asiakirja tai asiakirjoja, joita toimija on luonut, kartuttanut tai käyttänyt toimintansa aikana ja jotka on säilytetty niiden pysyvän arvon vuoksi.</skos:definition>
      <rdakit:toolkitDefinition xml:lang="fi">Asiakirja tai asiakirjoja, joita toimija on luonut, kartuttanut tai käyttänyt toimintansa aikana ja jotka on säilytetty niiden pysyvän arvon vuoksi.</rdakit:toolkitDefinition>
      <skos:scopeNote xml:lang="fi">Aineisto voi olla asiakirjojen kokoelma tai yksittäinen asiakirja. Se voi olla myös arkiston, henkilön tai muun laitoksen hankkima ja koostama kokoelma, jolla ei ole yhteistä alkuperää mutta jolla on jokin yhteinen luonteenpiirre kuten aihe, teema tai muoto.</skos:scopeNote>
      <skos:prefLabel xml:lang="da">arkivressource</skos:prefLabel>
      <rdakit:toolkitLabel xml:lang="da">arkivressource</rdakit:toolkitLabel>
      <skos:definition xml:lang="da">Et eller flere dokumenter, der oprindelig er skabt, samlet, eller anvendt af en agent i forbindelse med dens anliggender, og som er bevaret pga. deres værdi.</skos:definition>
      <rdakit:toolkitDefinition xml:lang="da">Et eller flere dokumenter, der oprindelig er skabt, samlet, eller anvendt af en agent i forbindelse med dens anliggender, og som er bevaret pga. deres værdi.</rdakit:toolkitDefinition>
      <skos:scopeNote xml:lang="da">Ressourcen kan være en sammenlægning af dokumenter eller et separat eksemplar. Det kan også være en samling, der er erhvervet eller samlet af et arkivdepot, en enkeltperson eller en anden institution, og som ikke har fælles proveniens eller oprindelse men dog visse fælles træk, fx et bestemt emne eller tema eller en bestemt form.</skos:scopeNote>
      <skos:prefLabel xml:lang="ca">recurs arxivístic</skos:prefLabel>
      <rdakit:toolkitLabel xml:lang="ca">recurs arxivístic</rdakit:toolkitLabel>
      <skos:definition xml:lang="ca">Document o conjunt de documents creat orgànicament, acumulat o usat per un agent en el curs de la seva activitat i preservat pel seu valor durador.</skos:definition>
      <rdakit:toolkitDefinition xml:lang="ca">Document o conjunt de documents creat orgànicament, acumulat o usat per un agent en el curs de la seva activitat i preservat pel seu valor durador.</rdakit:toolkitDefinition>
      <skos:scopeNote xml:lang="ca">El recurs pot ser un agregat de documents o un document sol. També pot ser una col·lecció adquirida i aplegada per un dipòsit d’arxiu, un individu o qualsevol altra institució, i que no té una provinença o un origen comú, però que té algunes característiques comunes, com ara una matèria, un tema o una forma concreta.</skos:scopeNote>
      <skos:prefLabel xml:lang="vi">tài nguyên lưu trữ</skos:prefLabel>
      <rdakit:toolkitLabel xml:lang="vi">tài nguyên lưu trữ</rdakit:toolkitLabel>
      <skos:definition xml:lang="vi">Một hoặc nhiều tài liệu được sáng tạo một cách hữu cơ, được tích luỹ, và/hoặc sử dụng bởi một cá nhân, gia đình, hoặc tập thể trong khi quản lý sự vụ và lưu giữ vì giá trị tiếp tục của chúng.</skos:definition>
      <rdakit:toolkitDefinition xml:lang="vi">Một hoặc nhiều tài liệu được sáng tạo một cách hữu cơ, được tích luỹ, và/hoặc sử dụng bởi một cá nhân, gia đình, hoặc tập thể trong khi quản lý sự vụ và lưu giữ vì giá trị tiếp tục của chúng.</rdakit:toolkitDefinition>
      <skos:scopeNote xml:lang="vi">Tài nguyên này có thể là tập hợp các tài liệu hoặc có thể là một bản riêng biệt. Cũng có thể là bộ sưu tập được bổ sung và thu thập bởi một kho lưu trữ, cá nhân, hoặc cơ quan khác, không chia sẻ lai lịch hoặc nguồn gốc nhưng phản ánh đặc tính chung nào đó, ví dụ, chủ đề, đề tài, hoặc hình thái riêng biệt</skos:scopeNote>
      <skos:prefLabel xml:lang="no">arkivressurs</skos:prefLabel>
      <rdakit:toolkitLabel xml:lang="no">arkivressurs</rdakit:toolkitLabel>
      <skos:definition xml:lang="no">Ett eller flere dokumenter som er skapt, samlet, eller brukt av en agent i sitt virke og bevart fordi de fortsatt har verdi.</skos:definition>
      <rdakit:toolkitDefinition xml:lang="no">Ett eller flere dokumenter som er skapt, samlet, eller brukt av en agent i sitt virke og bevart fordi de fortsatt har verdi.</rdakit:toolkitDefinition>
      <skos:scopeNote xml:lang="no">Ressursen kan bestå av en samling av dokumenter eller ett enkelt eksemplar. Den kan også være anskaffet og samlet av et arkiv, en enkeltperson eller en annen institusjon uten felles opprinnelse, men som gjenspeiler én eller annen felles egenskap, for eksempel et bestemt emne eller tema eller en bestemt form.</skos:scopeNote>
    </skos:Concept>
<!-- Concept: arrangement  -->
    <skos:Concept rdf:about="http://rdaregistry.info/termList/RDATerms/1008" xml:lang="en">
      <skos:inScheme rdf:resource="http://rdaregistry.info/termList/RDATerms"/>
      <reg:status rdf:resource="http://metadataregistry.org/uri/RegStatus/1001"/>
      <reg:identifier rdf:resource="http://metadataregistry.org/concepts/8523"/>
      <skos:prefLabel xml:lang="en">arrangement</skos:prefLabel>
      <rdakit:toolkitLabel xml:lang="en">arrangement</rdakit:toolkitLabel>
      <skos:definition xml:lang="en">An expression of a musical work resulting either from a change in the medium of performance, or from a simplification or other modification of the work with or without a change in medium of performance.</skos:definition>
      <rdakit:toolkitDefinition xml:lang="en">An expression of a musical work resulting either from a change in the medium of performance, or from a simplification or other modification of the work with or without a change in medium of performance.</rdakit:toolkitDefinition>
	    <skos:related rdf:resource="http://rdaregistry.info/termList/RDATerms/1003"/>
      <skos:definition xml:lang="it">Espressione di un'opera musicale che risulta da (a) un cambiamento nel mezzo d’interpretazione o (b) una semplificazione o altra modifica dell'opera, con o senza cambiamento del mezzo d’interpretazione.</skos:definition>
      <rdakit:toolkitDefinition xml:lang="it">Espressione di un'opera musicale che risulta da (a) un cambiamento nel mezzo d’interpretazione o (b) una semplificazione o altra modifica dell'opera, con o senza cambiamento del mezzo d’interpretazione.</rdakit:toolkitDefinition>
      <skos:prefLabel xml:lang="de">Arrangement</skos:prefLabel>
      <rdakit:toolkitLabel xml:lang="de">Arrangement</rdakit:toolkitLabel>
      <skos:definition xml:lang="de">Eine Expression eines Musikwerks, das aus (a) einer Änderung der Besetzung oder (b) einer Vereinfachung oder sonstigen Modifizierung des Werks mit oder ohne Änderung der Besetzung resultiert.</skos:definition>
      <rdakit:toolkitDefinition xml:lang="de">Eine Expression eines Musikwerks, das aus (a) einer Änderung der Besetzung oder (b) einer Vereinfachung oder sonstigen Modifizierung des Werks mit oder ohne Änderung der Besetzung resultiert.</rdakit:toolkitDefinition>
      <skos:prefLabel xml:lang="fi">sovitus</skos:prefLabel>
      <rdakit:toolkitLabel xml:lang="fi">sovitus</rdakit:toolkitLabel>
      <skos:definition xml:lang="fi">Musiikkiteoksen ekspressio, joka on joko seurausta muutoksesta esityskokoonpanossa tai teoksen yksinkertaistamisesta tai muusta muuntamisesta, jolloin esityskokoonpano voi muuttua tai pysyä samana.</skos:definition>
      <rdakit:toolkitDefinition xml:lang="fi">Musiikkiteoksen ekspressio, joka on joko seurausta muutoksesta esityskokoonpanossa tai teoksen yksinkertaistamisesta tai muusta muuntamisesta, jolloin esityskokoonpano voi muuttua tai pysyä samana.</rdakit:toolkitDefinition>
      <skos:prefLabel xml:lang="da">arrangement</skos:prefLabel>
      <rdakit:toolkitLabel xml:lang="da">arrangement</rdakit:toolkitLabel>
      <skos:definition xml:lang="da">Et udtryk af et musikværk, der er resultatet af enten en ændring i besætning, eller en forenkling eller anden modificering af værket, med eller uden ændring i besætning.</skos:definition>
      <rdakit:toolkitDefinition xml:lang="da">Et udtryk af et musikværk, der er resultatet af enten en ændring i besætning, eller en forenkling eller anden modificering af værket, med eller uden ændring i besætning.</rdakit:toolkitDefinition>
      <skos:prefLabel xml:lang="ca">arranjament</skos:prefLabel>
      <rdakit:toolkitLabel xml:lang="ca">arranjament</rdakit:toolkitLabel>
      <skos:definition xml:lang="ca">Expressió d’una obra musical que és el resultat o bé d'un un canvi en el repartiment d’execució, o una simplificació o qualsevol altra modificació de l’obra, amb o sense un canvi en el repartiment de l’execució.</skos:definition>
      <rdakit:toolkitDefinition xml:lang="ca">Expressió d’una obra musical que és el resultat o bé d'un un canvi en el repartiment d’execució, o una simplificació o qualsevol altra modificació de l’obra, amb o sense un canvi en el repartiment de l’execució.</rdakit:toolkitDefinition>
      <skos:prefLabel xml:lang="fr">arrangement</skos:prefLabel>
      <rdakit:toolkitLabel xml:lang="fr">arrangement</rdakit:toolkitLabel>
      <skos:definition xml:lang="fr">Expression d’une œuvre musicale résultant soit d’un changement dans la distribution d’exécution soit d’une simplification ou d’une autre modification de l’œuvre, avec ou sans changement dans la distribution d’exécution.</skos:definition>
      <rdakit:toolkitDefinition xml:lang="fr">Expression d’une œuvre musicale résultant soit d’un changement dans la distribution d’exécution soit d’une simplification ou d’une autre modification de l’œuvre, avec ou sans changement dans la distribution d’exécution.</rdakit:toolkitDefinition>
      <skos:prefLabel xml:lang="vi">cải biên</skos:prefLabel>
      <rdakit:toolkitLabel xml:lang="vi">cải biên</rdakit:toolkitLabel>
      <skos:definition xml:lang="vi">Biểu hiện của tác phẩm âm nhạc sinh ra từ thay đổi về phương tiện biểu diễn, hoặc đơn giản hoá hoặc sửa đổi khác cúa tác phẩm, với có hoặc không thay đổi phương tiện biểu diễn.</skos:definition>
      <rdakit:toolkitDefinition xml:lang="vi">Biểu hiện của tác phẩm âm nhạc sinh ra từ thay đổi về phương tiện biểu diễn, hoặc đơn giản hoá hoặc sửa đổi khác cúa tác phẩm, với có hoặc không thay đổi phương tiện biểu diễn.</rdakit:toolkitDefinition>
      <skos:prefLabel xml:lang="no">arrangement</skos:prefLabel>
      <rdakit:toolkitLabel xml:lang="no">arrangement</rdakit:toolkitLabel>
      <skos:definition xml:lang="no">Et uttrykk av et musikalsk verk som resultat av enten en endring av mediet for framføring eller en forenkling eller annen endring av verket, med eller uten endring av framføringsmediet.</skos:definition>
      <rdakit:toolkitDefinition xml:lang="no">Et uttrykk av et musikalsk verk som resultat av enten en endring av mediet for framføring eller en forenkling eller annen endring av verket, med eller uten endring av framføringsmediet.</rdakit:toolkitDefinition>
    </skos:Concept>
<!-- Concept: audio description  -->
    <skos:Concept rdf:about="http://rdaregistry.info/termList/RDATerms/1009" xml:lang="en">
      <skos:inScheme rdf:resource="http://rdaregistry.info/termList/RDATerms"/>
      <reg:status rdf:resource="http://metadataregistry.org/uri/RegStatus/1001"/>
      <reg:identifier rdf:resource="http://metadataregistry.org/concepts/8524"/>
      <skos:prefLabel xml:lang="en">audio description</skos:prefLabel>
      <skos:altLabel xml:lang="en">audio captioning</skos:altLabel>
      <rdakit:toolkitLabel xml:lang="en">audio description</rdakit:toolkitLabel>
      <skos:definition xml:lang="en">A narrative text, read out loud by a human being or by voice synthesis, that succinctly explains visual details not apparent from the audio element of the expression.</skos:definition>
      <rdakit:toolkitDefinition xml:lang="en">A narrative text, read out loud by a human being or by voice synthesis, that succinctly explains visual details not apparent from the audio element of the expression.</rdakit:toolkitDefinition>
      <skos:prefLabel xml:lang="it">descrizione audio</skos:prefLabel>
      <skos:altLabel xml:lang="it">intitolazione audio</skos:altLabel>
      <rdakit:toolkitLabel xml:lang="it">descrizione audio</rdakit:toolkitLabel>
      <skos:definition xml:lang="it">Testo narrativo, letto ad alta voce da un essere umano o da una voce sintetica, che spiega in sintesi i dettagli visivi non evidenti dall'elemento audio della risorsa.</skos:definition>
      <rdakit:toolkitDefinition xml:lang="it">Testo narrativo, letto ad alta voce da un essere umano o da una voce sintetica, che spiega in sintesi i dettagli visivi non evidenti dall'elemento audio della risorsa.</rdakit:toolkitDefinition>
      <skos:prefLabel xml:lang="fr">description audio</skos:prefLabel>
      <rdakit:toolkitLabel xml:lang="fr">description audio</rdakit:toolkitLabel>
      <skos:definition xml:lang="fr">Texte descriptif, lu à haute voix par un être humain ou par une voix de synthèse, qui explique succinctement des détails visuels dont l’élément audio de l’expression ne rend pas compte.</skos:definition>
      <rdakit:toolkitDefinition xml:lang="fr">Texte descriptif, lu à haute voix par un être humain ou par une voix de synthèse, qui explique succinctement des détails visuels dont l’élément audio de l’expression ne rend pas compte.</rdakit:toolkitDefinition>
      <skos:prefLabel xml:lang="de">Audiodeskription</skos:prefLabel>
      <skos:altLabel xml:lang="de">Audio-Erzählung</skos:altLabel>
      <rdakit:toolkitLabel xml:lang="de">Audiodeskription</rdakit:toolkitLabel>
      <skos:definition xml:lang="de">Eine Erzählung, die von einer Person oder durch eine synthetische Stimme laut gelesen wird, und die kurz und bündig visuelle Details erklärt, die aus dem Audio-Element der Expression nicht ersichtlich sind.</skos:definition>
      <rdakit:toolkitDefinition xml:lang="de">Eine Erzählung, die von einer Person oder durch eine synthetische Stimme laut gelesen wird, und die kurz und bündig visuelle Details erklärt, die aus dem Audio-Element der Expression nicht ersichtlich sind.</rdakit:toolkitDefinition>
      <skos:altLabel xml:lang="de">Videobeschreibung</skos:altLabel>
      <skos:altLabel xml:lang="de">beschreibendes Video</skos:altLabel>
      <skos:altLabel xml:lang="de">Audio-Untertitel</skos:altLabel>
      <skos:prefLabel xml:lang="fi">ääniselostus</skos:prefLabel>
      <rdakit:toolkitLabel xml:lang="fi">ääniselostus</rdakit:toolkitLabel>
      <skos:definition xml:lang="fi">Ihmisen tai äänisyntetisaattorin ääneen lukema kerronnallinen teksti, jossa selostetaan kohteen visuaalisia yksityiskohtia, jotka eivät muuten ilmene kohteen ääniaineksesta.</skos:definition>
      <rdakit:toolkitDefinition xml:lang="fi">Ihmisen tai äänisyntetisaattorin ääneen lukema kerronnallinen teksti, jossa selostetaan kohteen visuaalisia yksityiskohtia, jotka eivät muuten ilmene kohteen ääniaineksesta.</rdakit:toolkitDefinition>
      <skos:prefLabel xml:lang="da">synstolkning</skos:prefLabel>
      <rdakit:toolkitLabel xml:lang="da">synstolkning</rdakit:toolkitLabel>
      <skos:definition xml:lang="da">Fortællende tekst, der læses højt af et menneske eller via talesyntese, der kortfattet forklarer visuelle detaljer, der ikke tydeliggøres af udtrykkets lydelement.</skos:definition>
      <rdakit:toolkitDefinition xml:lang="da">Fortællende tekst, der læses højt af et menneske eller via talesyntese, der kortfattet forklarer visuelle detaljer, der ikke tydeliggøres af udtrykkets lydelement.</rdakit:toolkitDefinition>
      <skos:prefLabel xml:lang="ca">audiodescripció</skos:prefLabel>
      <skos:altLabel xml:lang="ca">subtitulat àudio</skos:altLabel>
      <rdakit:toolkitLabel xml:lang="ca">audiodescripció</rdakit:toolkitLabel>
      <skos:definition xml:lang="ca">Text narratiu, llegit en veu alta per un ésser humà o per un sintetitzador de parla, que explica succintament els detalls visuals que no són evidents a partir de l’element àudio de l'expressió.</skos:definition>
      <rdakit:toolkitDefinition xml:lang="ca">Text narratiu, llegit en veu alta per un ésser humà o per un sintetitzador de parla, que explica succintament els detalls visuals que no són evidents a partir de l’element àudio de l'expressió.</rdakit:toolkitDefinition>
      <skos:altLabel xml:lang="fr">audiodescription</skos:altLabel>
      <skos:altLabel xml:lang="fr">description narrative</skos:altLabel>
      <skos:altLabel xml:lang="fr">description vidéo</skos:altLabel>
      <skos:altLabel xml:lang="fr">vidéo descriptive</skos:altLabel>
      <skos:altLabel xml:lang="fr">vidéodescription</skos:altLabel>
      <skos:prefLabel xml:lang="vi">mô tả audio</skos:prefLabel>
      <rdakit:toolkitLabel xml:lang="vi">mô tả audio</rdakit:toolkitLabel>
      <skos:definition xml:lang="vi">Văn bản kể chuyện, được đọc to bởi con người hoặc bởi thiết bị tạo giọng nói, giải thích ngắn gọn các chi tiết thị giác không hiện ra từ yếu tố audeo của biểu hiện.</skos:definition>
      <rdakit:toolkitDefinition xml:lang="vi">Văn bản kể chuyện, được đọc to bởi con người hoặc bởi thiết bị tạo giọng nói, giải thích ngắn gọn các chi tiết thị giác không hiện ra từ yếu tố audeo của biểu hiện.</rdakit:toolkitDefinition>
      <skos:prefLabel xml:lang="no">lydbeskrivelse</skos:prefLabel>
      <rdakit:toolkitLabel xml:lang="no">lydbeskrivelse</rdakit:toolkitLabel>
      <skos:definition xml:lang="no">En fortellende tekst som enten leses høyt av et menneske eller genereres gjennom talesyntese, og som gir en kortfattet forklaring av visuelle detaljer som ikke fremkommer fra uttrykkets lydelement.</skos:definition>
      <rdakit:toolkitDefinition xml:lang="no">En fortellende tekst som enten leses høyt av et menneske eller genereres gjennom talesyntese, og som gir en kortfattet forklaring av visuelle detaljer som ikke fremkommer fra uttrykkets lydelement.</rdakit:toolkitDefinition>
    </skos:Concept>
<!-- Concept: audio recording  -->
    <skos:Concept rdf:about="http://rdaregistry.info/termList/RDATerms/1010" xml:lang="en">
      <skos:inScheme rdf:resource="http://rdaregistry.info/termList/RDATerms"/>
      <reg:status rdf:resource="http://metadataregistry.org/uri/RegStatus/1001"/>
      <reg:identifier rdf:resource="http://metadataregistry.org/concepts/8525"/>
      <skos:prefLabel xml:lang="en">audio recording</skos:prefLabel>
      <rdakit:toolkitLabel xml:lang="en">audio recording</rdakit:toolkitLabel>
      <skos:definition xml:lang="en">A recording on which sound vibrations have been registered by mechanical or electrical means so that the sound may be reproduced.</skos:definition>
      <rdakit:toolkitDefinition xml:lang="en">A recording on which sound vibrations have been registered by mechanical or electrical means so that the sound may be reproduced.</rdakit:toolkitDefinition>
      <skos:prefLabel xml:lang="it">registrazione audio</skos:prefLabel>
      <rdakit:toolkitLabel xml:lang="it">registrazione audio</rdakit:toolkitLabel>
      <skos:definition xml:lang="it">Registrazione in cui le vibrazioni sonore sono state registrate per mezzo di strumenti meccanici o elettrici in modo che il suono possa essere riprodotto.</skos:definition>
      <rdakit:toolkitDefinition xml:lang="it">Registrazione in cui le vibrazioni sonore sono state registrate per mezzo di strumenti meccanici o elettrici in modo che il suono possa essere riprodotto.</rdakit:toolkitDefinition>
      <skos:prefLabel xml:lang="de">Audioaufnahme</skos:prefLabel>
      <rdakit:toolkitLabel xml:lang="de">Audioaufnahme</rdakit:toolkitLabel>
      <skos:definition xml:lang="de">Eine Aufnahme, bei der Tonvibrationen durch mechanische oder elektrische Mittel registriert werden, so dass der Ton reproduziert werden kann.</skos:definition>
      <rdakit:toolkitDefinition xml:lang="de">Eine Aufnahme, bei der Tonvibrationen durch mechanische oder elektrische Mittel registriert werden, so dass der Ton reproduziert werden kann.</rdakit:toolkitDefinition>
      <skos:prefLabel xml:lang="fi">äänite</skos:prefLabel>
      <rdakit:toolkitLabel xml:lang="fi">äänite</rdakit:toolkitLabel>
      <skos:definition xml:lang="fi">Tallenne, johon äänivärähtelyt on rekisteröity mekaanisin tai sähköisin menetelmin siten, että ääni voidaan toistaa.</skos:definition>
      <rdakit:toolkitDefinition xml:lang="fi">Tallenne, johon äänivärähtelyt on rekisteröity mekaanisin tai sähköisin menetelmin siten, että ääni voidaan toistaa.</rdakit:toolkitDefinition>
      <skos:prefLabel xml:lang="da">lydoptagelse</skos:prefLabel>
      <rdakit:toolkitLabel xml:lang="da">lydoptagelse</rdakit:toolkitLabel>
      <skos:definition xml:lang="da">Optagelse, hvorpå lydvibrationer er registreret ad mekanisk eller elektronisk vej, så lyden kan gengives.</skos:definition>
      <rdakit:toolkitDefinition xml:lang="da">Optagelse, hvorpå lydvibrationer er registreret ad mekanisk eller elektronisk vej, så lyden kan gengives.</rdakit:toolkitDefinition>
      <skos:prefLabel xml:lang="ca">enregistrament àudio</skos:prefLabel>
      <rdakit:toolkitLabel xml:lang="ca">enregistrament àudio</rdakit:toolkitLabel>
      <skos:definition xml:lang="ca">Enregistrament sobre el qual s’han enregistrat vibracions sonores de manera mecànica o elèctrica per tal que el so es pugui reproduir.</skos:definition>
      <rdakit:toolkitDefinition xml:lang="ca">Enregistrament sobre el qual s’han enregistrat vibracions sonores de manera mecànica o elèctrica per tal que el so es pugui reproduir.</rdakit:toolkitDefinition>
      <skos:prefLabel xml:lang="fr">enregistrement audio</skos:prefLabel>
      <rdakit:toolkitLabel xml:lang="fr">enregistrement audio</rdakit:toolkitLabel>
      <skos:definition xml:lang="fr">Enregistrement sur lequel des vibrations sonores ont été enregistrées par un moyen mécanique ou électrique de façon à pouvoir reproduire le son.</skos:definition>
      <rdakit:toolkitDefinition xml:lang="fr">Enregistrement sur lequel des vibrations sonores ont été enregistrées par un moyen mécanique ou électrique de façon à pouvoir reproduire le son.</rdakit:toolkitDefinition>
      <skos:prefLabel xml:lang="vi">bản ghi audio</skos:prefLabel>
      <rdakit:toolkitLabel xml:lang="vi">bản ghi audio</rdakit:toolkitLabel>
      <skos:definition xml:lang="vi">Bản ghi trong đó rung động âm thanh được bảo toàn bằng các phương cách cơ học hoặc điện tử để có thể tái tạo.</skos:definition>
      <rdakit:toolkitDefinition xml:lang="vi">Bản ghi trong đó rung động âm thanh được bảo toàn bằng các phương cách cơ học hoặc điện tử để có thể tái tạo.</rdakit:toolkitDefinition>
      <skos:prefLabel xml:lang="no">lydopptak</skos:prefLabel>
      <rdakit:toolkitLabel xml:lang="no">lydopptak</rdakit:toolkitLabel>
      <skos:definition xml:lang="no">Et opptak der lydvibrasjoner er blitt registrert ved mekaniske eller elektriske hjelpemidler, slik at lyden kan reproduseres.</skos:definition>
      <rdakit:toolkitDefinition xml:lang="no">Et opptak der lydvibrasjoner er blitt registrert ved mekaniske eller elektriske hjelpemidler, slik at lyden kan reproduseres.</rdakit:toolkitDefinition>
    </skos:Concept>
<!-- Concept: audiotape  -->
    <skos:Concept rdf:about="http://rdaregistry.info/termList/RDATerms/1011" xml:lang="en">
      <skos:inScheme rdf:resource="http://rdaregistry.info/termList/RDATerms"/>
      <reg:status rdf:resource="http://metadataregistry.org/uri/RegStatus/1001"/>
      <reg:identifier rdf:resource="http://metadataregistry.org/concepts/8526"/>
      <skos:prefLabel xml:lang="en">audiotape</skos:prefLabel>
      <rdakit:toolkitLabel xml:lang="en">audiotape</rdakit:toolkitLabel>
      <skos:definition xml:lang="en">A length of magnetic tape on which are recorded electrical signals that can be converted to sound using audio playback equipment.</skos:definition>
      <rdakit:toolkitDefinition xml:lang="en">A length of magnetic tape on which are recorded electrical signals that can be converted to sound using audio playback equipment.</rdakit:toolkitDefinition>
      <skos:prefLabel xml:lang="it">nastro audio</skos:prefLabel>
      <rdakit:toolkitLabel xml:lang="it">nastro audio</rdakit:toolkitLabel>
      <skos:definition xml:lang="it">Striscia di nastro magnetico sulla quale sono registrati segnali elettrici che possono essere convertiti in suono utilizzando un’attrezzatura per la riproduzione audio.</skos:definition>
      <rdakit:toolkitDefinition xml:lang="it">Striscia di nastro magnetico sulla quale sono registrati segnali elettrici che possono essere convertiti in suono utilizzando un’attrezzatura per la riproduzione audio.</rdakit:toolkitDefinition>
      <skos:prefLabel xml:lang="fr">bande audio</skos:prefLabel>
      <rdakit:toolkitLabel xml:lang="fr">bande audio</rdakit:toolkitLabel>
      <skos:definition xml:lang="fr">Métrage de bande magnétique sur laquelle sont enregistrés des signaux électriques qui peuvent être convertis en sons à l’aide d’un appareil de lecture audio.</skos:definition>
      <rdakit:toolkitDefinition xml:lang="fr">Métrage de bande magnétique sur laquelle sont enregistrés des signaux électriques qui peuvent être convertis en sons à l’aide d’un appareil de lecture audio.</rdakit:toolkitDefinition>
      <skos:prefLabel xml:lang="de">Tonband</skos:prefLabel>
      <rdakit:toolkitLabel xml:lang="de">Tonband</rdakit:toolkitLabel>
      <skos:definition xml:lang="de">Ein Stück Magnetband, auf dem elektrische Signale aufgezeichnet sind, die mithilfe eines Audio-Wiedergabegeräts in Ton umgewandelt werden können.</skos:definition>
      <rdakit:toolkitDefinition xml:lang="de">Ein Stück Magnetband, auf dem elektrische Signale aufgezeichnet sind, die mithilfe eines Audio-Wiedergabegeräts in Ton umgewandelt werden können.</rdakit:toolkitDefinition>
      <skos:prefLabel xml:lang="fi">ääninauha</skos:prefLabel>
      <rdakit:toolkitLabel xml:lang="fi">ääninauha</rdakit:toolkitLabel>
      <skos:definition xml:lang="fi">Magneettinauha, jolle on tallennettu sähkösignaaleja, jotka voidaan muuntaa ääneksi äänentoistolaitteistolla.</skos:definition>
      <rdakit:toolkitDefinition xml:lang="fi">Magneettinauha, jolle on tallennettu sähkösignaaleja, jotka voidaan muuntaa ääneksi äänentoistolaitteistolla.</rdakit:toolkitDefinition>
      <skos:prefLabel xml:lang="da">lydbånd</skos:prefLabel>
      <rdakit:toolkitLabel xml:lang="da">lydbånd</rdakit:toolkitLabel>
      <skos:definition xml:lang="da">Et stykke magnetbånd, hvorpå elektriske signaler er optaget, der kan omdannes til lyd vha. lydafspiller.</skos:definition>
      <rdakit:toolkitDefinition xml:lang="da">Et stykke magnetbånd, hvorpå elektriske signaler er optaget, der kan omdannes til lyd vha. lydafspiller.</rdakit:toolkitDefinition>
      <skos:prefLabel xml:lang="ca">cinta àudio</skos:prefLabel>
      <rdakit:toolkitLabel xml:lang="ca">cinta àudio</rdakit:toolkitLabel>
      <skos:definition xml:lang="ca">Tira de cinta magnètica sobre la qual s’enregistren senyals elèctrics que es poden convertir en sons usant un equipament de reproducció àudio.</skos:definition>
      <rdakit:toolkitDefinition xml:lang="ca">Tira de cinta magnètica sobre la qual s’enregistren senyals elèctrics que es poden convertir en sons usant un equipament de reproducció àudio.</rdakit:toolkitDefinition>
      <skos:prefLabel xml:lang="vi">băng audio</skos:prefLabel>
      <rdakit:toolkitLabel xml:lang="vi">băng audio</rdakit:toolkitLabel>
      <skos:definition xml:lang="vi">Băng từ dài trên đó ghi tín hiệu điện tử có thể chuyển thành âm thanh khi dùng thiết bị phát lại audio.</skos:definition>
      <rdakit:toolkitDefinition xml:lang="vi">Băng từ dài trên đó ghi tín hiệu điện tử có thể chuyển thành âm thanh khi dùng thiết bị phát lại audio.</rdakit:toolkitDefinition>
      <skos:prefLabel xml:lang="no">lydbånd</skos:prefLabel>
      <rdakit:toolkitLabel xml:lang="no">lydbånd</rdakit:toolkitLabel>
      <skos:definition xml:lang="no">Et stykke magnetbånd der det kan lagres elektriske signaler som kan konverteres til lyd ved hjelp av lydavspillingsutstyr.</skos:definition>
      <rdakit:toolkitDefinition xml:lang="no">Et stykke magnetbånd der det kan lagres elektriske signaler som kan konverteres til lyd ved hjelp av lydavspillingsutstyr.</rdakit:toolkitDefinition>
    </skos:Concept>
<!-- Concept: authorized access point  -->
    <skos:Concept rdf:about="http://rdaregistry.info/termList/RDATerms/1012" xml:lang="en">
      <skos:inScheme rdf:resource="http://rdaregistry.info/termList/RDATerms"/>
      <reg:status rdf:resource="http://metadataregistry.org/uri/RegStatus/1001"/>
      <reg:identifier rdf:resource="http://metadataregistry.org/concepts/8527"/>
      <skos:prefLabel xml:lang="en">authorized access point</skos:prefLabel>
      <rdakit:toolkitLabel xml:lang="en">authorized access point</rdakit:toolkitLabel>
      <skos:definition xml:lang="en">A standardized access point representing an entity.</skos:definition>
      <rdakit:toolkitDefinition xml:lang="en">A standardized access point representing an entity.</rdakit:toolkitDefinition>
	    <skos:broader rdf:resource="http://rdaregistry.info/termList/RDATerms/1001"/>
      <skos:prefLabel xml:lang="it">punto d'accesso autorizzato</skos:prefLabel>
      <rdakit:toolkitLabel xml:lang="it">punto d'accesso autorizzato</rdakit:toolkitLabel>
      <skos:definition xml:lang="it">Punto d'accesso standardizzato che rappresenta un'entità.</skos:definition>
      <rdakit:toolkitDefinition xml:lang="it">Punto d'accesso standardizzato che rappresenta un'entità.</rdakit:toolkitDefinition>
      <skos:prefLabel xml:lang="fr">point d’accès autorisé</skos:prefLabel>
      <rdakit:toolkitLabel xml:lang="fr">point d’accès autorisé</rdakit:toolkitLabel>
      <skos:definition xml:lang="fr">Point d’accès normalisé représentant une entité.</skos:definition>
      <rdakit:toolkitDefinition xml:lang="fr">Point d’accès normalisé représentant une entité.</rdakit:toolkitDefinition>
      <skos:prefLabel xml:lang="es">punto de acceso autorizado</skos:prefLabel>
      <rdakit:toolkitLabel xml:lang="es">punto de acceso autorizado</rdakit:toolkitLabel>
      <skos:definition xml:lang="es">Punto de acceso normalizado que representa una entidad.</skos:definition>
      <rdakit:toolkitDefinition xml:lang="es">Punto de acceso normalizado que representa una entidad.</rdakit:toolkitDefinition>
      <skos:prefLabel xml:lang="fi">auktorisoitu hakutieto</skos:prefLabel>
      <rdakit:toolkitLabel xml:lang="fi">auktorisoitu hakutieto</rdakit:toolkitLabel>
      <skos:definition xml:lang="fi">Entiteetin vahvistettu hakutieto.</skos:definition>
      <rdakit:toolkitDefinition xml:lang="fi">Entiteetin vahvistettu hakutieto.</rdakit:toolkitDefinition>
      <skos:prefLabel xml:lang="de">Normierter Sucheinstieg</skos:prefLabel>
      <rdakit:toolkitLabel xml:lang="de">Normierter Sucheinstieg</rdakit:toolkitLabel>
      <skos:definition xml:lang="de">Ein standardisierter Sucheinstieg, der eine Entität repräsentiert.</skos:definition>
      <rdakit:toolkitDefinition xml:lang="de">Ein standardisierter Sucheinstieg, der eine Entität repräsentiert.</rdakit:toolkitDefinition>
      <skos:prefLabel xml:lang="da">autoriseret søgeindgang</skos:prefLabel>
      <rdakit:toolkitLabel xml:lang="da">autoriseret søgeindgang</rdakit:toolkitLabel>
      <skos:definition xml:lang="da">Den standardiserede søgeindgang, der repræsenterer en entitet.</skos:definition>
      <rdakit:toolkitDefinition xml:lang="da">Den standardiserede søgeindgang, der repræsenterer en entitet.</rdakit:toolkitDefinition>
      <skos:prefLabel xml:lang="ca">punt d’accés autoritzat</skos:prefLabel>
      <rdakit:toolkitLabel xml:lang="ca">punt d’accés autoritzat</rdakit:toolkitLabel>
      <skos:definition xml:lang="ca">Punt d’accés normalitzat que representa una entitat.</skos:definition>
      <rdakit:toolkitDefinition xml:lang="ca">Punt d’accés normalitzat que representa una entitat.</rdakit:toolkitDefinition>
      <skos:prefLabel xml:lang="vi">điểm truy cập được phép</skos:prefLabel>
      <rdakit:toolkitLabel xml:lang="vi">điểm truy cập được phép</rdakit:toolkitLabel>
      <skos:definition xml:lang="vi">Điểm truy cập được chuẩn hoá trình bày một thực thể.</skos:definition>
      <rdakit:toolkitDefinition xml:lang="vi">Điểm truy cập được chuẩn hoá trình bày một thực thể.</rdakit:toolkitDefinition>
      <skos:prefLabel xml:lang="no">autorisert søkeinngang</skos:prefLabel>
      <rdakit:toolkitLabel xml:lang="no">autorisert søkeinngang</rdakit:toolkitLabel>
      <skos:definition xml:lang="no">En autorisert søkeinngang som representerer en entitet.</skos:definition>
      <rdakit:toolkitDefinition xml:lang="no">En autorisert søkeinngang som representerer en entitet.</rdakit:toolkitDefinition>
    </skos:Concept>
<!-- Concept: binding  -->
    <skos:Concept rdf:about="http://rdaregistry.info/termList/RDATerms/1013" xml:lang="en">
      <skos:inScheme rdf:resource="http://rdaregistry.info/termList/RDATerms"/>
      <reg:status rdf:resource="http://metadataregistry.org/uri/RegStatus/1001"/>
      <reg:identifier rdf:resource="http://metadataregistry.org/concepts/8528"/>
      <skos:prefLabel xml:lang="en">binding</skos:prefLabel>
      <rdakit:toolkitLabel xml:lang="en">binding</rdakit:toolkitLabel>
      <skos:definition xml:lang="en">An outer cover affixed to a gathering of one or more sheets.</skos:definition>
      <rdakit:toolkitDefinition xml:lang="en">An outer cover affixed to a gathering of one or more sheets.</rdakit:toolkitDefinition>
      <skos:prefLabel xml:lang="it">legatura</skos:prefLabel>
      <rdakit:toolkitLabel xml:lang="it">legatura</rdakit:toolkitLabel>
      <skos:definition xml:lang="it">Copertura esterna apposta a un fascicolo di uno o più fogli.</skos:definition>
      <rdakit:toolkitDefinition xml:lang="it">Copertura esterna apposta a un fascicolo di uno o più fogli.</rdakit:toolkitDefinition>
      <skos:prefLabel xml:lang="fr">reliure</skos:prefLabel>
      <rdakit:toolkitLabel xml:lang="fr">reliure</rdakit:toolkitLabel>
      <skos:definition xml:lang="fr">Couverture extérieure fixée à un assemblage d’une ou plusieurs feuilles.</skos:definition>
      <rdakit:toolkitDefinition xml:lang="fr">Couverture extérieure fixée à un assemblage d’une ou plusieurs feuilles.</rdakit:toolkitDefinition>
      <skos:prefLabel xml:lang="de">Einband</skos:prefLabel>
      <rdakit:toolkitLabel xml:lang="de">Einband</rdakit:toolkitLabel>
      <skos:definition xml:lang="de">Eine äußere Hülle, die um eine Lage von einem oder mehreren Blättern angebracht ist.</skos:definition>
      <rdakit:toolkitDefinition xml:lang="de">Eine äußere Hülle, die um eine Lage von einem oder mehreren Blättern angebracht ist.</rdakit:toolkitDefinition>
      <skos:prefLabel xml:lang="fi">sidos</skos:prefLabel>
      <rdakit:toolkitLabel xml:lang="fi">sidos</rdakit:toolkitLabel>
      <skos:definition xml:lang="fi">Ulkoinen kansi ja siihen kiinnitetyt yksi tai useampi painoarkki.</skos:definition>
      <rdakit:toolkitDefinition xml:lang="fi">Ulkoinen kansi ja siihen kiinnitetyt yksi tai useampi painoarkki.</rdakit:toolkitDefinition>
      <skos:prefLabel xml:lang="da">indbindning</skos:prefLabel>
      <rdakit:toolkitLabel xml:lang="da">indbindning</rdakit:toolkitLabel>
      <skos:definition xml:lang="da">Omslag, der er fæstnet til en samling af et eller flere ark.</skos:definition>
      <rdakit:toolkitDefinition xml:lang="da">Omslag, der er fæstnet til en samling af et eller flere ark.</rdakit:toolkitDefinition>
      <skos:prefLabel xml:lang="ca">enquadernació</skos:prefLabel>
      <rdakit:toolkitLabel xml:lang="ca">enquadernació</rdakit:toolkitLabel>
      <skos:definition xml:lang="ca">Coberta exterior enganxada a un quadern d’un o més fulls.</skos:definition>
      <rdakit:toolkitDefinition xml:lang="ca">Coberta exterior enganxada a un quadern d’un o més fulls.</rdakit:toolkitDefinition>
      <skos:prefLabel xml:lang="vi">đóng bìa</skos:prefLabel>
      <rdakit:toolkitLabel xml:lang="vi">đóng bìa</rdakit:toolkitLabel>
      <skos:definition xml:lang="vi">Bìa ngoài được đóng vào một tập hợp của một hoặc nhiều tờ.</skos:definition>
      <rdakit:toolkitDefinition xml:lang="vi">Bìa ngoài được đóng vào một tập hợp của một hoặc nhiều tờ.</rdakit:toolkitDefinition>
      <skos:prefLabel xml:lang="no">innbinding</skos:prefLabel>
      <rdakit:toolkitLabel xml:lang="no">innbinding</rdakit:toolkitLabel>
      <skos:definition xml:lang="no">Et omslag festet til en samling av ett eller flere ark.</skos:definition>
      <rdakit:toolkitDefinition xml:lang="no">Et omslag festet til en samling av ett eller flere ark.</rdakit:toolkitDefinition>
    </skos:Concept>
<!-- Concept: caption title  -->
    <skos:Concept rdf:about="http://rdaregistry.info/termList/RDATerms/1014" xml:lang="en">
      <skos:inScheme rdf:resource="http://rdaregistry.info/termList/RDATerms"/>
      <reg:status rdf:resource="http://metadataregistry.org/uri/RegStatus/1001"/>
      <reg:identifier rdf:resource="http://metadataregistry.org/concepts/8529"/>
      <skos:prefLabel xml:lang="en">caption title</skos:prefLabel>
      <rdakit:toolkitLabel xml:lang="en">caption title</rdakit:toolkitLabel>
      <skos:definition xml:lang="en">A title given at the beginning of the first page of the text or, for notated music, at the top of the first page.</skos:definition>
      <rdakit:toolkitDefinition xml:lang="en">A title given at the beginning of the first page of the text or, for notated music, at the top of the first page.</rdakit:toolkitDefinition>
      <skos:prefLabel xml:lang="it">intitolazione</skos:prefLabel>
      <rdakit:toolkitLabel xml:lang="it">intitolazione</rdakit:toolkitLabel>
      <skos:definition xml:lang="it">Titolo che figura all'inizio della prima pagina di testo o, per la musica notata, alla sommità della prima pagina.</skos:definition>
      <rdakit:toolkitDefinition xml:lang="it">Titolo che figura all'inizio della prima pagina di testo o, per la musica notata, alla sommità della prima pagina.</rdakit:toolkitDefinition>
      <skos:prefLabel xml:lang="de">Kopftitel</skos:prefLabel>
      <rdakit:toolkitLabel xml:lang="de">Kopftitel</rdakit:toolkitLabel>
      <skos:definition xml:lang="de">Ein Titel, der am Anfang der ersten Seite des Texts oder bei Noten oben auf der ersten Seite des Stücks aufgeführt ist.</skos:definition>
      <rdakit:toolkitDefinition xml:lang="de">Ein Titel, der am Anfang der ersten Seite des Texts oder bei Noten oben auf der ersten Seite des Stücks aufgeführt ist.</rdakit:toolkitDefinition>
      <skos:prefLabel xml:lang="fi">otsikkonimeke</skos:prefLabel>
      <rdakit:toolkitLabel xml:lang="fi">otsikkonimeke</rdakit:toolkitLabel>
      <skos:definition xml:lang="fi">Nimeke, joka esiintyy tekstin ensimmäisen sivun alussa, nuottijulkaisuissa ensimmäisen sivun yläosassa.</skos:definition>
      <rdakit:toolkitDefinition xml:lang="fi">Nimeke, joka esiintyy tekstin ensimmäisen sivun alussa, nuottijulkaisuissa ensimmäisen sivun yläosassa.</rdakit:toolkitDefinition>
      <skos:prefLabel xml:lang="da">overskrifttitel</skos:prefLabel>
      <rdakit:toolkitLabel xml:lang="da">overskrifttitel</rdakit:toolkitLabel>
      <skos:definition xml:lang="da">Titel angivet ved begyndelsen af en teksts første side eller ved toppen af første side af noteret musik.</skos:definition>
      <rdakit:toolkitDefinition xml:lang="da">Titel angivet ved begyndelsen af en teksts første side eller ved toppen af første side af noteret musik.</rdakit:toolkitDefinition>
      <skos:prefLabel xml:lang="ca">títol inicial</skos:prefLabel>
      <rdakit:toolkitLabel xml:lang="ca">títol inicial</rdakit:toolkitLabel>
      <skos:definition xml:lang="ca">Títol donat al començament de la primera pàgina del text o, en el cas de la música notada, al capdamunt de la primera pàgina.</skos:definition>
      <rdakit:toolkitDefinition xml:lang="ca">Títol donat al començament de la primera pàgina del text o, en el cas de la música notada, al capdamunt de la primera pàgina.</rdakit:toolkitDefinition>
      <skos:prefLabel xml:lang="fr">titre de départ</skos:prefLabel>
      <rdakit:toolkitLabel xml:lang="fr">titre de départ</rdakit:toolkitLabel>
      <skos:definition xml:lang="fr">Titre donné au début de la première page du texte ou, pour la musique notée, en haut de la première page de musique.</skos:definition>
      <rdakit:toolkitDefinition xml:lang="fr">Titre donné au début de la première page du texte ou, pour la musique notée, en haut de la première page de musique.</rdakit:toolkitDefinition>
      <skos:prefLabel xml:lang="vi">nhan đề đầu đề</skos:prefLabel>
      <rdakit:toolkitLabel xml:lang="vi">nhan đề đầu đề</rdakit:toolkitLabel>
      <skos:definition xml:lang="vi">Nhan đề ở đầu trang đầu tiên của văn bản hoặc, đối với âm nhạc ghi, ở đầu của trang đầu tiên.</skos:definition>
      <rdakit:toolkitDefinition xml:lang="vi">Nhan đề ở đầu trang đầu tiên của văn bản hoặc, đối với âm nhạc ghi, ở đầu của trang đầu tiên.</rdakit:toolkitDefinition>
      <skos:prefLabel xml:lang="no">spisstittel</skos:prefLabel>
      <rdakit:toolkitLabel xml:lang="no">spisstittel</rdakit:toolkitLabel>
      <skos:definition xml:lang="no">En tittel som er oppgitt ved begynnelsen av den første siden av teksten, eller øverst på den første siden for musikknotasjon.</skos:definition>
      <rdakit:toolkitDefinition xml:lang="no">En tittel som er oppgitt ved begynnelsen av den første siden av teksten, eller øverst på den første siden for musikknotasjon.</rdakit:toolkitDefinition>
    </skos:Concept>
<!-- Concept: captioning  -->
    <skos:Concept rdf:about="http://rdaregistry.info/termList/RDATerms/1015" xml:lang="en">
      <skos:inScheme rdf:resource="http://rdaregistry.info/termList/RDATerms"/>
      <reg:status rdf:resource="http://metadataregistry.org/uri/RegStatus/1001"/>
      <reg:identifier rdf:resource="http://metadataregistry.org/concepts/8530"/>
      <skos:prefLabel xml:lang="en">captioning</skos:prefLabel>
      <rdakit:toolkitLabel xml:lang="en">captioning</rdakit:toolkitLabel>
      <skos:definition xml:lang="en">A text representing speech and other audible information that is displayed on screen in the written language of the audio element of the expression.</skos:definition>
      <rdakit:toolkitDefinition xml:lang="en">A text representing speech and other audible information that is displayed on screen in the written language of the audio element of the expression.</rdakit:toolkitDefinition>
      <skos:scopeNote xml:lang="en">This is usually found as closed captions that are encoded and must be decoded, that is,  switched on, to be made visible. There are also open captions which are always visible and cannot be turned off. Excludes subtitles in a language different from the spoken content.</skos:scopeNote>
      <skos:prefLabel xml:lang="it">didascalia</skos:prefLabel>
      <rdakit:toolkitLabel xml:lang="it">didascalia</rdakit:toolkitLabel>
      <skos:definition xml:lang="it">Testo che rappresenta il parlato e altre informazioni in forma sonora e che è visualizzato sullo schermo nella lingua dell'elemento audio della risorsa.</skos:definition>
      <rdakit:toolkitDefinition xml:lang="it">Testo che rappresenta il parlato e altre informazioni in forma sonora e che è visualizzato sullo schermo nella lingua dell'elemento audio della risorsa.</rdakit:toolkitDefinition>
      <skos:scopeNote xml:lang="it">Solitamente presente come &quot;didascalia nascosta&quot; codificata che deve essere decodificata (o attivata) per essere resa visibile. Esistono anche le &quot;didascalie in chiaro&quot; che sono sempre visibili e che non possono essere disattivate. Sono esclusi i sottotitoli in lingue diverse dal contenuto parlato.</skos:scopeNote>
      <skos:prefLabel xml:lang="de">Untertitel für Hörgeschädigte</skos:prefLabel>
      <rdakit:toolkitLabel xml:lang="de">Untertitel für Hörgeschädigte</rdakit:toolkitLabel>
      <skos:definition xml:lang="de">Ein Text, der Sprach- und sonstige hörbare Informationen darstellt, die auf dem Bildschirm in der geschriebenen Sprache des Audio-Elements der Expression angezeigt werden.</skos:definition>
      <rdakit:toolkitDefinition xml:lang="de">Ein Text, der Sprach- und sonstige hörbare Informationen darstellt, die auf dem Bildschirm in der geschriebenen Sprache des Audio-Elements der Expression angezeigt werden.</rdakit:toolkitDefinition>
      <skos:scopeNote xml:lang="de">In der Regel gefunden als „geschlossene Untertitel für Hörgeschädigte“, die kodiert sind und dekodiert (eingeschaltet) werden müssen, um sichtbar zu werden. Es gibt auch „offene Untertitel für Hörgeschädigte“, die immer sichtbar sind und nicht ausgeschaltet werden können. Ausgenommen sind Untertitel in einer anderen Sprache als der des gesprochenen Inhalts.</skos:scopeNote>
      <skos:prefLabel xml:lang="fi">ohjelmatekstitys</skos:prefLabel>
      <rdakit:toolkitLabel xml:lang="fi">ohjelmatekstitys</rdakit:toolkitLabel>
      <skos:definition xml:lang="fi">Ruudulla näkyvä teksti, joka toistaa kirjoitettuna ekspressiossa kuultavan puheen ja muun kuunneltavan informaation.</skos:definition>
      <rdakit:toolkitDefinition xml:lang="fi">Ruudulla näkyvä teksti, joka toistaa kirjoitettuna ekspressiossa kuultavan puheen ja muun kuunneltavan informaation.</rdakit:toolkitDefinition>
      <skos:scopeNote xml:lang="fi">Tavallisesti tämä on ohjelmaan piilotettu kuvateksti, joka on koodattu ja dekoodattava eli kytkettävä päälle tullakseen näkyville. Avoin tekstitys on aina näkyvillä eikä sitä voi kytkeä pois.</skos:scopeNote>
      <skos:prefLabel xml:lang="da">tekstning</skos:prefLabel>
      <rdakit:toolkitLabel xml:lang="da">tekstning</rdakit:toolkitLabel>
      <skos:definition xml:lang="da">Tekst som gengiver tale og anden lydinformation. Teksten vises på skærmen som et skriftligt udtryk af udtrykkets lydelementer</skos:definition>
      <rdakit:toolkitDefinition xml:lang="da">Tekst som gengiver tale og anden lydinformation. Teksten vises på skærmen som et skriftligt udtryk af udtrykkets lydelementer</rdakit:toolkitDefinition>
      <skos:scopeNote xml:lang="da">Teksten forekommer sædvanligvis som skjult information, som skal aktiveres for  at blive synlig. Teksten forekommer også i versioner, hvor den altid er synlig og ikke kan skjules. Undertekster på et andet sprog end det talte i lydgengivelsen er ikke inkluderet.</skos:scopeNote>
      <skos:prefLabel xml:lang="ca">subtitulació per a persones sordes</skos:prefLabel>
      <rdakit:toolkitLabel xml:lang="ca">subtitulació per a persones sordes</rdakit:toolkitLabel>
      <skos:definition xml:lang="ca">Text que representa el discurs i altres informacions audibles, que es visualitza a la pantalla en la llengua escrita de l’element àudio de l'expressió.</skos:definition>
      <rdakit:toolkitDefinition xml:lang="ca">Text que representa el discurs i altres informacions audibles, que es visualitza a la pantalla en la llengua escrita de l’element àudio de l'expressió.</rdakit:toolkitDefinition>
      <skos:scopeNote xml:lang="ca">Normalment es presenta en la forma de subtítols codificats, que s’han de descodificar, és a dir, activar, perquè siguin visibles. També hi ha subtítols oberts que sempre són visibles i no es poden desactivar. S’exclouen els subtítols en una llengua diferent del contingut parlat.</skos:scopeNote>
      <skos:prefLabel xml:lang="fr">sous-titrage pour malentendants</skos:prefLabel>
      <rdakit:toolkitLabel xml:lang="fr">sous-titrage pour malentendants</rdakit:toolkitLabel>
      <skos:definition xml:lang="fr">Texte représentant du langage parlé et d’autres informations audibles et qui est affiché à l’écran dans la langue écrite de l’élément audio de l’expression.</skos:definition>
      <rdakit:toolkitDefinition xml:lang="fr">Texte représentant du langage parlé et d’autres informations audibles et qui est affiché à l’écran dans la langue écrite de l’élément audio de l’expression.</rdakit:toolkitDefinition>
      <skos:scopeNote xml:lang="fr">Généralement présenté comme un sous-titre codé qui doit être décodé, c’est-à-dire activé, pour être visible. Il existe aussi des sous-titres visibles qui sont toujours visibles et ne peuvent être désactivés. Ne comprend pas les sous-titres dans une langue différente du contenu parlé.</skos:scopeNote>
      <skos:prefLabel xml:lang="vi">thuyết minh</skos:prefLabel>
      <rdakit:toolkitLabel xml:lang="vi">thuyết minh</rdakit:toolkitLabel>
      <skos:definition xml:lang="vi">Văn bản trình bày bài nói hoặc thông tin có thể nghe được khác được hiển thị trên nàm hình bằng ngôn ngữ viết của yếu tố audio của biểu hiện.</skos:definition>
      <rdakit:toolkitDefinition xml:lang="vi">Văn bản trình bày bài nói hoặc thông tin có thể nghe được khác được hiển thị trên nàm hình bằng ngôn ngữ viết của yếu tố audio của biểu hiện.</rdakit:toolkitDefinition>
      <skos:scopeNote xml:lang="vi">Thường được tìn thấy như là bản thu nạp kín được mã hoá và phải giải mã, nghĩa là, thay đổi sang có thể nhìn được. Cũng có bản thu nạp mở luôn luôn nhìn thấy được và không thể tắt. Không bao gồm nhan đề phụ bằng ngôn ngữ khác với nội dung nói.</skos:scopeNote>
      <skos:prefLabel xml:lang="no">teksting</skos:prefLabel>
      <rdakit:toolkitLabel xml:lang="no">teksting</rdakit:toolkitLabel>
      <skos:definition xml:lang="no">En tekst som gjengir tale og annen hørbar informasjon og som vises på skjermen på skriftspråket for uttrykkets lydelement.</skos:definition>
      <rdakit:toolkitDefinition xml:lang="no">En tekst som gjengir tale og annen hørbar informasjon og som vises på skjermen på skriftspråket for uttrykkets lydelement.</rdakit:toolkitDefinition>
      <skos:scopeNote xml:lang="no">Tekstingen kan være kodet, og må da dekodes, dvs. slås på, for å vises. Det finnes også teksting som alltid vises og ikke kan slås av. Undertekster på et annet språk enn taleinnholdet er ikke inkludert.</skos:scopeNote>
    </skos:Concept>
<!-- Concept: carrier  -->
    <skos:Concept rdf:about="http://rdaregistry.info/termList/RDATerms/1016" xml:lang="en">
      <skos:inScheme rdf:resource="http://rdaregistry.info/termList/RDATerms"/>
      <reg:status rdf:resource="http://metadataregistry.org/uri/RegStatus/1001"/>
      <reg:identifier rdf:resource="http://metadataregistry.org/concepts/8531"/>
      <skos:prefLabel xml:lang="en">carrier</skos:prefLabel>
      <rdakit:toolkitLabel xml:lang="en">carrier</rdakit:toolkitLabel>
      <skos:definition xml:lang="en">A physical medium in which data, sound, images, etc., are stored.</skos:definition>
      <rdakit:toolkitDefinition xml:lang="en">A physical medium in which data, sound, images, etc., are stored.</rdakit:toolkitDefinition>
      <skos:scopeNote xml:lang="en">For certain types of manifestations, the carrier may consist of a storage medium  sometimes encased in a plastic, metal, etc., housing that is an integral part of the manifestation.</skos:scopeNote>
	    <skos:related rdf:resource="http://rdaregistry.info/termList/RDATerms/1086"/>
	    <skos:related rdf:resource="http://rdaregistry.info/termList/RDATerms/1058"/>
	    <skos:related rdf:resource="http://rdaregistry.info/termList/RDATerms/1026"/>
      <skos:prefLabel xml:lang="it">supporto</skos:prefLabel>
      <rdakit:toolkitLabel xml:lang="it">supporto</rdakit:toolkitLabel>
      <skos:definition xml:lang="it">Mezzo fisico in cui si memorizzano dati, suoni, immagini, etc.</skos:definition>
      <rdakit:toolkitDefinition xml:lang="it">Mezzo fisico in cui si memorizzano dati, suoni, immagini, etc.</rdakit:toolkitDefinition>
      <skos:scopeNote xml:lang="it">Per alcuni tipi di risorsa, il supporto può consistere in un mezzo di memorizzazione (per esempio, nastro, pellicola) talvolta rivestito da una custodia di plastica, di metallo, etc. (per esempio, cassette, cartucce) che è parte integrante della risorsa.</skos:scopeNote>
      <skos:prefLabel xml:lang="fr">support matériel</skos:prefLabel>
      <rdakit:toolkitLabel xml:lang="fr">support matériel</rdakit:toolkitLabel>
      <skos:definition xml:lang="fr">Support physique sur lequel des données, du son, des images, etc. sont emmagasinés.</skos:definition>
      <rdakit:toolkitDefinition xml:lang="fr">Support physique sur lequel des données, du son, des images, etc. sont emmagasinés.</rdakit:toolkitDefinition>
      <skos:scopeNote xml:lang="fr">Pour certains types de manifestations, le support matériel peut consister en un support de stockage parfois intégré dans un contenant en plastique, en métal, etc. qui fait partie intégrante de la manifestation.</skos:scopeNote>
      <skos:prefLabel xml:lang="de">Datenträger</skos:prefLabel>
      <rdakit:toolkitLabel xml:lang="de">Datenträger</rdakit:toolkitLabel>
      <skos:definition xml:lang="de">Ein physisches Medium, auf dem Daten, Ton, Bilder usw. gespeichert sind.</skos:definition>
      <rdakit:toolkitDefinition xml:lang="de">Ein physisches Medium, auf dem Daten, Ton, Bilder usw. gespeichert sind.</rdakit:toolkitDefinition>
      <skos:scopeNote xml:lang="de">Für bestimmte Arten von Manifestationen kann der Datenträger aus einem Speichermedium bestehen, das manchmal von einem Kunststoff-, einem Metallgehäuse o. Ä. umhüllt ist, das ein integraler Bestandteil der Manifestation ist.</skos:scopeNote>
      <skos:prefLabel xml:lang="fi">tallenne</skos:prefLabel>
      <rdakit:toolkitLabel xml:lang="fi">tallenne</rdakit:toolkitLabel>
      <skos:definition xml:lang="fi">Fyysinen väline, jolle dataa, ääntä, kuvia tms. on tallennettu.</skos:definition>
      <rdakit:toolkitDefinition xml:lang="fi">Fyysinen väline, jolle dataa, ääntä, kuvia tms. on tallennettu.</rdakit:toolkitDefinition>
      <skos:scopeNote xml:lang="fi">Tietyntyyppisissä manifestaatioissa tallenne voi sisältää tallennusvälineen, joka voi olla pakattu muoviseen, metalliseen tms. kuoreen, joka on kiinteä osa aineistoa.</skos:scopeNote>
      <skos:prefLabel xml:lang="da">bærer</skos:prefLabel>
      <rdakit:toolkitLabel xml:lang="da">bærer</rdakit:toolkitLabel>
      <skos:definition xml:lang="da">Fysisk medie, på hvilket data, lyd, billeder etc. er lagret.</skos:definition>
      <rdakit:toolkitDefinition xml:lang="da">Fysisk medie, på hvilket data, lyd, billeder etc. er lagret.</rdakit:toolkitDefinition>
      <skos:scopeNote xml:lang="da">I nogle tilfælde vil bæreren bestå af et lagringsmedie samt et opbevaringsudstyr, som er en integreret del af ressourcen.</skos:scopeNote>
      <skos:prefLabel xml:lang="ca">suport físic</skos:prefLabel>
      <rdakit:toolkitLabel xml:lang="ca">suport físic</rdakit:toolkitLabel>
      <skos:definition xml:lang="ca">Base física en la qual s’emmagatzemen les dades, el so, les imatges, etc.</skos:definition>
      <rdakit:toolkitDefinition xml:lang="ca">Base física en la qual s’emmagatzemen les dades, el so, les imatges, etc.</rdakit:toolkitDefinition>
      <skos:scopeNote xml:lang="ca">En el cas d’alguns tipus de manifestacions, el suport físic pot consistir en el suport d’emmagatzematge que de vegades va encapsat en un embolcall de plàstic, metall, etc., que és una part integrant de la manifestació.</skos:scopeNote>
      <skos:prefLabel xml:lang="vi">vật mang tin</skos:prefLabel>
      <rdakit:toolkitLabel xml:lang="vi">vật mang tin</rdakit:toolkitLabel>
      <skos:definition xml:lang="vi">Phương tiện vật lý trong đó dữ liệu, âm thanh, hình ảnh. v.v... được lưu giữ.</skos:definition>
      <rdakit:toolkitDefinition xml:lang="vi">Phương tiện vật lý trong đó dữ liệu, âm thanh, hình ảnh. v.v... được lưu giữ.</rdakit:toolkitDefinition>
      <skos:scopeNote xml:lang="vi">Đối với một số loại của biểu thị, vật mang tin có thể gồm có phương tiện lưu giữ đôi khi được đựng trong vật chứa chất deo, kim loại, v.v... là bộ phận cấu thành của biểu thị.</skos:scopeNote>
      <skos:prefLabel xml:lang="no">bærer</skos:prefLabel>
      <rdakit:toolkitLabel xml:lang="no">bærer</rdakit:toolkitLabel>
      <skos:definition xml:lang="no">Et fysisk medium som data, lyd, bilder, etc. er lagret på.</skos:definition>
      <rdakit:toolkitDefinition xml:lang="no">Et fysisk medium som data, lyd, bilder, etc. er lagret på.</rdakit:toolkitDefinition>
      <skos:scopeNote xml:lang="no">For enkelte typer manifestasjoner kan bæreren bestå av et lagringsmedium som kan være omsluttet av plast, metall, etc. som en integrert del av manifestasjonen.</skos:scopeNote>
    </skos:Concept>
<!-- Concept: cartographic content  -->
    <skos:Concept rdf:about="http://rdaregistry.info/termList/RDATerms/1017" xml:lang="en">
      <skos:inScheme rdf:resource="http://rdaregistry.info/termList/RDATerms"/>
      <reg:status rdf:resource="http://metadataregistry.org/uri/RegStatus/1001"/>
      <reg:identifier rdf:resource="http://metadataregistry.org/concepts/8532"/>
      <skos:prefLabel xml:lang="en">cartographic content</skos:prefLabel>
      <rdakit:toolkitLabel xml:lang="en">cartographic content</rdakit:toolkitLabel>
      <skos:definition xml:lang="en">A content that represents the whole or part of the Earth, any celestial body, or imaginary place at any scale.</skos:definition>
      <rdakit:toolkitDefinition xml:lang="en">A content that represents the whole or part of the Earth, any celestial body, or imaginary place at any scale.</rdakit:toolkitDefinition>
      <skos:prefLabel xml:lang="it">contenuto cartografico</skos:prefLabel>
      <rdakit:toolkitLabel xml:lang="it">contenuto cartografico</rdakit:toolkitLabel>
      <skos:definition xml:lang="it">Contenuto che rappresenta per intero o in parte la Terra, qualsiasi corpo celeste o luogo immaginario in qualunque scala.</skos:definition>
      <rdakit:toolkitDefinition xml:lang="it">Contenuto che rappresenta per intero o in parte la Terra, qualsiasi corpo celeste o luogo immaginario in qualunque scala.</rdakit:toolkitDefinition>
      <skos:prefLabel xml:lang="fr">contenu cartographique</skos:prefLabel>
      <rdakit:toolkitLabel xml:lang="fr">contenu cartographique</rdakit:toolkitLabel>
      <skos:definition xml:lang="fr">Contenu qui représente la totalité ou une partie de la Terre, de tout corps céleste ou d’un lieu imaginaire à n’importe quelle échelle.</skos:definition>
      <rdakit:toolkitDefinition xml:lang="fr">Contenu qui représente la totalité ou une partie de la Terre, de tout corps céleste ou d’un lieu imaginaire à n’importe quelle échelle.</rdakit:toolkitDefinition>
      <skos:prefLabel xml:lang="es">contenido cartográfico</skos:prefLabel>
      <rdakit:toolkitLabel xml:lang="es">contenido cartográfico</rdakit:toolkitLabel>
      <skos:definition xml:lang="es">Contenido que representa a toda o una parte de la Tierra, a los cuerpos celestes o lugares ficticios en cualquier escala.</skos:definition>
      <rdakit:toolkitDefinition xml:lang="es">Contenido que representa a toda o una parte de la Tierra, a los cuerpos celestes o lugares ficticios en cualquier escala.</rdakit:toolkitDefinition>
      <skos:prefLabel xml:lang="de">Kartografischer Inhalt</skos:prefLabel>
      <rdakit:toolkitLabel xml:lang="de">Kartografischer Inhalt</rdakit:toolkitLabel>
      <skos:definition xml:lang="de">Ein Inhalt, der die ganze Erde oder Teile davon, einen Himmelskörper oder einen imaginären Ort in einem beliebigen Maßstab darstellt.</skos:definition>
      <rdakit:toolkitDefinition xml:lang="de">Ein Inhalt, der die ganze Erde oder Teile davon, einen Himmelskörper oder einen imaginären Ort in einem beliebigen Maßstab darstellt.</rdakit:toolkitDefinition>
      <skos:prefLabel xml:lang="fi">kartografinen sisältö</skos:prefLabel>
      <rdakit:toolkitLabel xml:lang="fi">kartografinen sisältö</rdakit:toolkitLabel>
      <skos:definition xml:lang="fi">Sisältö, joka esittää maapalloa tai sen osaa, taivaankappaleita tai kuvitteellista paikkaa missä tahansa mittakaavassa.</skos:definition>
      <rdakit:toolkitDefinition xml:lang="fi">Sisältö, joka esittää maapalloa tai sen osaa, taivaankappaleita tai kuvitteellista paikkaa missä tahansa mittakaavassa.</rdakit:toolkitDefinition>
      <skos:prefLabel xml:lang="da">kartografisk indhold</skos:prefLabel>
      <rdakit:toolkitLabel xml:lang="da">kartografisk indhold</rdakit:toolkitLabel>
      <skos:definition xml:lang="da">Indhold, der repræsenterer hele eller dele af jorden, et himmellegeme eller et imaginært sted i ethvert målestoksforhold.</skos:definition>
      <rdakit:toolkitDefinition xml:lang="da">Indhold, der repræsenterer hele eller dele af jorden, et himmellegeme eller et imaginært sted i ethvert målestoksforhold.</rdakit:toolkitDefinition>
      <skos:prefLabel xml:lang="ca">contingut cartogràfic</skos:prefLabel>
      <rdakit:toolkitLabel xml:lang="ca">contingut cartogràfic</rdakit:toolkitLabel>
      <skos:definition xml:lang="ca">Contingut que representa la totalitat o una part de la Terra, de qualsevol cos celeste o d’un lloc imaginari a qualsevol escala.</skos:definition>
      <rdakit:toolkitDefinition xml:lang="ca">Contingut que representa la totalitat o una part de la Terra, de qualsevol cos celeste o d’un lloc imaginari a qualsevol escala.</rdakit:toolkitDefinition>
      <skos:prefLabel xml:lang="vi">nội dung bản đồ</skos:prefLabel>
      <rdakit:toolkitLabel xml:lang="vi">nội dung bản đồ</rdakit:toolkitLabel>
      <skos:definition xml:lang="vi">Nội dung trình bày toàn bộ hoặc phần của trái đất, thiên thể bất kỳ, hoặc địa điểm tưởng tượng với tỷ lệ bất kỳ.</skos:definition>
      <rdakit:toolkitDefinition xml:lang="vi">Nội dung trình bày toàn bộ hoặc phần của trái đất, thiên thể bất kỳ, hoặc địa điểm tưởng tượng với tỷ lệ bất kỳ.</rdakit:toolkitDefinition>
      <skos:prefLabel xml:lang="no">kartografisk innhold</skos:prefLabel>
      <rdakit:toolkitLabel xml:lang="no">kartografisk innhold</rdakit:toolkitLabel>
      <skos:definition xml:lang="no">Innhold i en eller annen målestokk som gjengir hele eller deler av Jorden, et himmellegeme eller et fiktivt sted.</skos:definition>
      <rdakit:toolkitDefinition xml:lang="no">Innhold i en eller annen målestokk som gjengir hele eller deler av Jorden, et himmellegeme eller et fiktivt sted.</rdakit:toolkitDefinition>
    </skos:Concept>
<!-- Concept: citation title of a legal work  -->
    <skos:Concept rdf:about="http://rdaregistry.info/termList/RDATerms/1018" xml:lang="en">
      <skos:inScheme rdf:resource="http://rdaregistry.info/termList/RDATerms"/>
      <reg:status rdf:resource="http://metadataregistry.org/uri/RegStatus/1001"/>
      <reg:identifier rdf:resource="http://metadataregistry.org/concepts/8533"/>
      <skos:prefLabel xml:lang="en">citation title of a legal work</skos:prefLabel>
      <rdakit:toolkitLabel xml:lang="en">citation title of a legal work</rdakit:toolkitLabel>
      <skos:definition xml:lang="en">A title of a legal work used for the citation of the work either in the text of the work or in legal literature.</skos:definition>
      <rdakit:toolkitDefinition xml:lang="en">A title of a legal work used for the citation of the work either in the text of the work or in legal literature.</rdakit:toolkitDefinition>
      <skos:prefLabel xml:lang="it">titolo di citazione di un'opera giuridica</skos:prefLabel>
      <rdakit:toolkitLabel xml:lang="it">titolo di citazione di un'opera giuridica</rdakit:toolkitLabel>
      <skos:definition xml:lang="it">Titolo di un'opera giuridica utilizzato per la citazione dell'opera nel testo dell'opera stessa o nella letteratura giuridica.</skos:definition>
      <rdakit:toolkitDefinition xml:lang="it">Titolo di un'opera giuridica utilizzato per la citazione dell'opera nel testo dell'opera stessa o nella letteratura giuridica.</rdakit:toolkitDefinition>
      <skos:prefLabel xml:lang="fr">titre de référence d’une œuvre juridique</skos:prefLabel>
      <rdakit:toolkitLabel xml:lang="fr">titre de référence d’une œuvre juridique</rdakit:toolkitLabel>
      <skos:definition xml:lang="fr">Titre d’une œuvre juridique utilisé pour faire référence à l’œuvre, que ce soit dans le texte même de l’œuvre ou dans la littérature juridique.</skos:definition>
      <rdakit:toolkitDefinition xml:lang="fr">Titre d’une œuvre juridique utilisé pour faire référence à l’œuvre, que ce soit dans le texte même de l’œuvre ou dans la littérature juridique.</rdakit:toolkitDefinition>
      <skos:prefLabel xml:lang="es">título de citación de una obra jurídica</skos:prefLabel>
      <rdakit:toolkitLabel xml:lang="es">título de citación de una obra jurídica</rdakit:toolkitLabel>
      <skos:definition xml:lang="es">Un título de una obra jurídica usado para citar la obra ya sea en el texto de la obra o en la literatura jurídica.</skos:definition>
      <rdakit:toolkitDefinition xml:lang="es">Un título de una obra jurídica usado para citar la obra ya sea en el texto de la obra o en la literatura jurídica.</rdakit:toolkitDefinition>
      <skos:prefLabel xml:lang="de">Zitiertitel eines juristischen Werks</skos:prefLabel>
      <rdakit:toolkitLabel xml:lang="de">Zitiertitel eines juristischen Werks</rdakit:toolkitLabel>
      <skos:definition xml:lang="de">Ein Titel eines juristischen Werks, das zum Zitieren des Werks entweder im Text des Werks oder in der juristischen Literatur verwendet wird.</skos:definition>
      <rdakit:toolkitDefinition xml:lang="de">Ein Titel eines juristischen Werks, das zum Zitieren des Werks entweder im Text des Werks oder in der juristischen Literatur verwendet wird.</rdakit:toolkitDefinition>
      <skos:prefLabel xml:lang="fi">juridisen teoksen viittausnimeke</skos:prefLabel>
      <rdakit:toolkitLabel xml:lang="fi">juridisen teoksen viittausnimeke</rdakit:toolkitLabel>
      <skos:definition xml:lang="fi">Juridisen teoksen nimeke jolla teokseen viitataan joko teoksessa itsessään tai muussa juridisessa kirjallisuudessa.</skos:definition>
      <rdakit:toolkitDefinition xml:lang="fi">Juridisen teoksen nimeke jolla teokseen viitataan joko teoksessa itsessään tai muussa juridisessa kirjallisuudessa.</rdakit:toolkitDefinition>
      <skos:prefLabel xml:lang="da">henvisningstitel for juridiks værk</skos:prefLabel>
      <rdakit:toolkitLabel xml:lang="da">henvisningstitel for juridiks værk</rdakit:toolkitLabel>
      <skos:definition xml:lang="da">Titel på et juridisk værk, der anvendes til at henvise til værket enten i værkets tekst eller i juridisk litteratur.</skos:definition>
      <rdakit:toolkitDefinition xml:lang="da">Titel på et juridisk værk, der anvendes til at henvise til værket enten i værkets tekst eller i juridisk litteratur.</rdakit:toolkitDefinition>
      <skos:prefLabel xml:lang="ca">títol de citació d’una obra jurídica</skos:prefLabel>
      <rdakit:toolkitLabel xml:lang="ca">títol de citació d’una obra jurídica</rdakit:toolkitLabel>
      <skos:definition xml:lang="ca">Títol d’una obra jurídica usat per a la citació de l’obra ja sigui en el text de l’obra o en la bibliografia jurídica.</skos:definition>
      <rdakit:toolkitDefinition xml:lang="ca">Títol d’una obra jurídica usat per a la citació de l’obra ja sigui en el text de l’obra o en la bibliografia jurídica.</rdakit:toolkitDefinition>
      <skos:prefLabel xml:lang="vi">nhan đề trích dẫn của tác phẩm luật pháp</skos:prefLabel>
      <rdakit:toolkitLabel xml:lang="vi">nhan đề trích dẫn của tác phẩm luật pháp</rdakit:toolkitLabel>
      <skos:definition xml:lang="vi">Nhan đề của tác phẩm luật pháp được dùng để trích dẫn tác phẩm đó cả trong văn bản của tác phẩm đó hoặc trong tài liệu luật pháp.</skos:definition>
      <rdakit:toolkitDefinition xml:lang="vi">Nhan đề của tác phẩm luật pháp được dùng để trích dẫn tác phẩm đó cả trong văn bản của tác phẩm đó hoặc trong tài liệu luật pháp.</rdakit:toolkitDefinition>
      <skos:prefLabel xml:lang="no">siteringstittel på et juridisk verk</skos:prefLabel>
      <rdakit:toolkitLabel xml:lang="no">siteringstittel på et juridisk verk</rdakit:toolkitLabel>
      <skos:definition xml:lang="no">En tittel på et juridisk verk brukt for å henvise til verket, enten i verkets tekst eller i juridisk litteratur.</skos:definition>
      <rdakit:toolkitDefinition xml:lang="no">En tittel på et juridisk verk brukt for å henvise til verket, enten i verkets tekst eller i juridisk litteratur.</rdakit:toolkitDefinition>
    </skos:Concept>
<!-- Concept: collection  -->
    <skos:Concept rdf:about="http://rdaregistry.info/termList/RDATerms/1019" xml:lang="en">
      <skos:inScheme rdf:resource="http://rdaregistry.info/termList/RDATerms"/>
      <reg:status rdf:resource="http://metadataregistry.org/uri/RegStatus/1001"/>
      <reg:identifier rdf:resource="http://metadataregistry.org/concepts/8534"/>
      <skos:prefLabel xml:lang="en">collection</skos:prefLabel>
      <rdakit:toolkitLabel xml:lang="en">collection</rdakit:toolkitLabel>
      <skos:definition xml:lang="en">A group of resources assembled by an agent from a variety of sources.</skos:definition>
      <rdakit:toolkitDefinition xml:lang="en">A group of resources assembled by an agent from a variety of sources.</rdakit:toolkitDefinition>
      <skos:prefLabel xml:lang="it">collezione</skos:prefLabel>
      <rdakit:toolkitLabel xml:lang="it">collezione</rdakit:toolkitLabel>
      <skos:definition xml:lang="it">Gruppo di risorse riunite da una persona, famiglia o ente attingendo a una varietà di fonti.</skos:definition>
      <rdakit:toolkitDefinition xml:lang="it">Gruppo di risorse riunite da una persona, famiglia o ente attingendo a una varietà di fonti.</rdakit:toolkitDefinition>
      <skos:prefLabel xml:lang="fr">collection</skos:prefLabel>
      <rdakit:toolkitLabel xml:lang="fr">collection</rdakit:toolkitLabel>
      <skos:definition xml:lang="fr">Groupe de ressources d’origine variée rassemblées par un agent.</skos:definition>
      <rdakit:toolkitDefinition xml:lang="fr">Groupe de ressources d’origine variée rassemblées par un agent.</rdakit:toolkitDefinition>
      <skos:prefLabel xml:lang="es">colección</skos:prefLabel>
      <rdakit:toolkitLabel xml:lang="es">colección</rdakit:toolkitLabel>
      <skos:definition xml:lang="es">Grupo de recursos reunido, por una persona, familia o entidad corporativa, a partir de una variedad de fuentes.</skos:definition>
      <rdakit:toolkitDefinition xml:lang="es">Grupo de recursos reunido, por una persona, familia o entidad corporativa, a partir de una variedad de fuentes.</rdakit:toolkitDefinition>
      <skos:prefLabel xml:lang="de">Sammlung</skos:prefLabel>
      <rdakit:toolkitLabel xml:lang="de">Sammlung</rdakit:toolkitLabel>
      <skos:definition xml:lang="de">Eine Gruppe von Ressourcen, die von einem Akteur aus einer Vielzahl von Quellen zusammengetragen ist.</skos:definition>
      <rdakit:toolkitDefinition xml:lang="de">Eine Gruppe von Ressourcen, die von einem Akteur aus einer Vielzahl von Quellen zusammengetragen ist.</rdakit:toolkitDefinition>
      <skos:prefLabel xml:lang="fi">kokoelma</skos:prefLabel>
      <rdakit:toolkitLabel xml:lang="fi">kokoelma</rdakit:toolkitLabel>
      <skos:definition xml:lang="fi">Toimijan useasta lähteestä kokoama aineistoryhmä.</skos:definition>
      <rdakit:toolkitDefinition xml:lang="fi">Toimijan useasta lähteestä kokoama aineistoryhmä.</rdakit:toolkitDefinition>
      <skos:prefLabel xml:lang="da">samling</skos:prefLabel>
      <rdakit:toolkitLabel xml:lang="da">samling</rdakit:toolkitLabel>
      <skos:definition xml:lang="da">Gruppe af ressourcer samlet af en person, familie eller korporation fra forskellige kilder.</skos:definition>
      <rdakit:toolkitDefinition xml:lang="da">Gruppe af ressourcer samlet af en person, familie eller korporation fra forskellige kilder.</rdakit:toolkitDefinition>
      <skos:prefLabel xml:lang="ca">col·lecció</skos:prefLabel>
      <skos:altLabel xml:lang="ca">col·lecció arxivística</skos:altLabel>
      <rdakit:toolkitLabel xml:lang="ca">col·lecció</rdakit:toolkitLabel>
      <skos:definition xml:lang="ca">Grup de recursos aplegats per un agent a partir d’una diversitat de fonts.</skos:definition>
      <rdakit:toolkitDefinition xml:lang="ca">Grup de recursos aplegats per un agent a partir d’una diversitat de fonts.</rdakit:toolkitDefinition>
      <skos:prefLabel xml:lang="vi">bộ sưu tập</skos:prefLabel>
      <rdakit:toolkitLabel xml:lang="vi">bộ sưu tập</rdakit:toolkitLabel>
      <skos:definition xml:lang="vi">Nhóm tài nguyên do cá nhân, gia đình, hoặc tập thể thu thập từ các nguồn khác nhau.</skos:definition>
      <rdakit:toolkitDefinition xml:lang="vi">Nhóm tài nguyên do cá nhân, gia đình, hoặc tập thể thu thập từ các nguồn khác nhau.</rdakit:toolkitDefinition>
      <skos:prefLabel xml:lang="no">samling</skos:prefLabel>
      <rdakit:toolkitLabel xml:lang="no">samling</rdakit:toolkitLabel>
      <skos:definition xml:lang="no">En gruppe ressurser fra flere kilder samlet av en agent.</skos:definition>
      <rdakit:toolkitDefinition xml:lang="no">En gruppe ressurser fra flere kilder samlet av en agent.</rdakit:toolkitDefinition>
    </skos:Concept>
<!-- Concept: collective title  -->
    <skos:Concept rdf:about="http://rdaregistry.info/termList/RDATerms/1020" xml:lang="en">
      <skos:inScheme rdf:resource="http://rdaregistry.info/termList/RDATerms"/>
      <reg:status rdf:resource="http://metadataregistry.org/uri/RegStatus/1001"/>
      <reg:identifier rdf:resource="http://metadataregistry.org/concepts/8535"/>
      <skos:prefLabel xml:lang="en">collective title</skos:prefLabel>
      <rdakit:toolkitLabel xml:lang="en">collective title</rdakit:toolkitLabel>
      <skos:definition xml:lang="en">An inclusive title used either as a title proper for a manifestation containing separately titled individual contents, or as a preferred title for a compilation of two or more works.</skos:definition>
      <rdakit:toolkitDefinition xml:lang="en">An inclusive title used either as a title proper for a manifestation containing separately titled individual contents, or as a preferred title for a compilation of two or more works.</rdakit:toolkitDefinition>
	    <skos:narrower rdf:resource="http://rdaregistry.info/termList/RDATerms/1027"/>
      <skos:prefLabel xml:lang="it">titolo collettivo</skos:prefLabel>
      <rdakit:toolkitLabel xml:lang="it">titolo collettivo</rdakit:toolkitLabel>
      <skos:definition xml:lang="it">Titolo proprio che è un titolo comprensivo di una risorsa che contiene più parti componenti intitolate distintamente.</skos:definition>
      <rdakit:toolkitDefinition xml:lang="it">Titolo proprio che è un titolo comprensivo di una risorsa che contiene più parti componenti intitolate distintamente.</rdakit:toolkitDefinition>
      <skos:prefLabel xml:lang="fr">titre collectif</skos:prefLabel>
      <rdakit:toolkitLabel xml:lang="fr">titre collectif</rdakit:toolkitLabel>
      <skos:definition xml:lang="fr">Titre global utilisé soit comme titre propre d’une manifestation ayant des contenus individuels titrés séparément, soit comme titre privilégié d’une compilation de deux ou plusieurs œuvres.</skos:definition>
      <rdakit:toolkitDefinition xml:lang="fr">Titre global utilisé soit comme titre propre d’une manifestation ayant des contenus individuels titrés séparément, soit comme titre privilégié d’une compilation de deux ou plusieurs œuvres.</rdakit:toolkitDefinition>
      <skos:prefLabel xml:lang="es">título colectivo</skos:prefLabel>
      <rdakit:toolkitLabel xml:lang="es">título colectivo</rdakit:toolkitLabel>
      <skos:definition xml:lang="es">Título inclusivo usado ya sea como el título propiamente dicho para un recurso que tiene contenido individual titulado separadamente, o como el título preferido para una compilación de dos o más obra.</skos:definition>
      <rdakit:toolkitDefinition xml:lang="es">Título inclusivo usado ya sea como el título propiamente dicho para un recurso que tiene contenido individual titulado separadamente, o como el título preferido para una compilación de dos o más obra.</rdakit:toolkitDefinition>
      <skos:prefLabel xml:lang="de">Übergeordneter Titel</skos:prefLabel>
      <rdakit:toolkitLabel xml:lang="de">Übergeordneter Titel</rdakit:toolkitLabel>
      <skos:definition xml:lang="de">Ein umfassender Titel, der entweder als Haupttitel für eine Manifestation die separat betitelte einzelne Inhalte enthält, oder als bevorzugter Titel für eine Zusammenstellung von mehreren Werken verwendet wird.</skos:definition>
      <rdakit:toolkitDefinition xml:lang="de">Ein umfassender Titel, der entweder als Haupttitel für eine Manifestation die separat betitelte einzelne Inhalte enthält, oder als bevorzugter Titel für eine Zusammenstellung von mehreren Werken verwendet wird.</rdakit:toolkitDefinition>
      <skos:prefLabel xml:lang="fi">kokoava nimeke</skos:prefLabel>
      <rdakit:toolkitLabel xml:lang="fi">kokoava nimeke</rdakit:toolkitLabel>
      <skos:definition xml:lang="fi">Kattava nimeke jota käytetään joko useasta osakohteesta koostuvan manifestaation päänimekkeenä tai useasta teoksesta koostuvan kokoelman päänimekkeenä.</skos:definition>
      <rdakit:toolkitDefinition xml:lang="fi">Kattava nimeke jota käytetään joko useasta osakohteesta koostuvan manifestaation päänimekkeenä tai useasta teoksesta koostuvan kokoelman päänimekkeenä.</rdakit:toolkitDefinition>
      <skos:prefLabel xml:lang="da">fællestitel</skos:prefLabel>
      <rdakit:toolkitLabel xml:lang="da">fællestitel</rdakit:toolkitLabel>
      <skos:definition xml:lang="da">Titel, der anvendes enten som hovedtitel for en manifestation, der indeholder individuelle dele med separate titler, eller som den foretrukne titel for en kompilation af to eller flere værker.</skos:definition>
      <rdakit:toolkitDefinition xml:lang="da">Titel, der anvendes enten som hovedtitel for en manifestation, der indeholder individuelle dele med separate titler, eller som den foretrukne titel for en kompilation af to eller flere værker.</rdakit:toolkitDefinition>
      <skos:prefLabel xml:lang="ca">títol col·lectiu</skos:prefLabel>
      <rdakit:toolkitLabel xml:lang="ca">títol col·lectiu</rdakit:toolkitLabel>
      <skos:definition xml:lang="ca">Títol inclusiu usat o bé com a títol propi d’una manifestació que inclou continguts individuals titulats separadament, o bé com un títol preferit d’una compilació de dues o més obres.</skos:definition>
      <rdakit:toolkitDefinition xml:lang="ca">Títol inclusiu usat o bé com a títol propi d’una manifestació que inclou continguts individuals titulats separadament, o bé com un títol preferit d’una compilació de dues o més obres.</rdakit:toolkitDefinition>
      <skos:prefLabel xml:lang="vi">nhan đề tập hợp</skos:prefLabel>
      <rdakit:toolkitLabel xml:lang="vi">nhan đề tập hợp</rdakit:toolkitLabel>
      <skos:definition xml:lang="vi">Nhan đề bao gồm được dùng hoặc như là nhan đề hợp thức cho một biểu thị chứa các nội dung riêng được đặt tên tách biệt, hoặc như là nhan đề ưu tiên cho sưu tập hai hoặc nhiều hơn tác phẩm.</skos:definition>
      <rdakit:toolkitDefinition xml:lang="vi">Nhan đề bao gồm được dùng hoặc như là nhan đề hợp thức cho một biểu thị chứa các nội dung riêng được đặt tên tách biệt, hoặc như là nhan đề ưu tiên cho sưu tập hai hoặc nhiều hơn tác phẩm.</rdakit:toolkitDefinition>
      <skos:prefLabel xml:lang="no">fellestittel</skos:prefLabel>
      <rdakit:toolkitLabel xml:lang="no">fellestittel</rdakit:toolkitLabel>
      <skos:definition xml:lang="no">En inkluderende tittel som brukes enten som hovedtittel på en manifestasjon som inneholder innholdselementer med egne titler, eller som foretrukket tittel på en samling av to eller flere verk.</skos:definition>
      <rdakit:toolkitDefinition xml:lang="no">En inkluderende tittel som brukes enten som hovedtittel på en manifestasjon som inneholder innholdselementer med egne titler, eller som foretrukket tittel på en samling av to eller flere verk.</rdakit:toolkitDefinition>
    </skos:Concept>
<!-- Concept: component part  -->
    <skos:Concept rdf:about="http://rdaregistry.info/termList/RDATerms/1021" xml:lang="en">
      <skos:inScheme rdf:resource="http://rdaregistry.info/termList/RDATerms"/>
      <reg:status rdf:resource="http://metadataregistry.org/uri/RegStatus/1001"/>
      <reg:identifier rdf:resource="http://metadataregistry.org/concepts/8536"/>
      <skos:prefLabel xml:lang="en">component part</skos:prefLabel>
      <rdakit:toolkitLabel xml:lang="en">component part</rdakit:toolkitLabel>
      <skos:definition xml:lang="en">A discrete unit of intellectual content within a larger resource.</skos:definition>
      <rdakit:toolkitDefinition xml:lang="en">A discrete unit of intellectual content within a larger resource.</rdakit:toolkitDefinition>
      <skos:prefLabel xml:lang="de">Bestandteil</skos:prefLabel>
      <rdakit:toolkitLabel xml:lang="de">Bestandteil</rdakit:toolkitLabel>
      <skos:definition xml:lang="de">Eine einzelne Einheit von intellektuellem Inhalt innerhalb einer größeren Ressource.</skos:definition>
      <rdakit:toolkitDefinition xml:lang="de">Eine einzelne Einheit von intellektuellem Inhalt innerhalb einer größeren Ressource.</rdakit:toolkitDefinition>
      <skos:prefLabel xml:lang="fi">osakohde</skos:prefLabel>
      <rdakit:toolkitLabel xml:lang="fi">osakohde</rdakit:toolkitLabel>
      <skos:definition xml:lang="fi">Erillinen tiedollinen sisältö suuremmassa aineistossa.</skos:definition>
      <rdakit:toolkitDefinition xml:lang="fi">Erillinen tiedollinen sisältö suuremmassa aineistossa.</rdakit:toolkitDefinition>
      <skos:prefLabel xml:lang="da">del</skos:prefLabel>
      <rdakit:toolkitLabel xml:lang="da">del</rdakit:toolkitLabel>
      <skos:definition xml:lang="da">Særskilt enhed af intellektuelt indhold i en større ressource.</skos:definition>
      <rdakit:toolkitDefinition xml:lang="da">Særskilt enhed af intellektuelt indhold i en større ressource.</rdakit:toolkitDefinition>
      <skos:prefLabel xml:lang="ca">part component</skos:prefLabel>
      <rdakit:toolkitLabel xml:lang="ca">part component</rdakit:toolkitLabel>
      <skos:definition xml:lang="ca">Unitat discreta de contingut intel·lectual dins d’un recurs més ampli.</skos:definition>
      <rdakit:toolkitDefinition xml:lang="ca">Unitat discreta de contingut intel·lectual dins d’un recurs més ampli.</rdakit:toolkitDefinition>
      <skos:prefLabel xml:lang="fr">partie composante</skos:prefLabel>
      <rdakit:toolkitLabel xml:lang="fr">partie composante</rdakit:toolkitLabel>
      <skos:definition xml:lang="fr">Unité distincte de contenu intellectuel au sein d’une ressource plus vaste.</skos:definition>
      <rdakit:toolkitDefinition xml:lang="fr">Unité distincte de contenu intellectuel au sein d’une ressource plus vaste.</rdakit:toolkitDefinition>
      <skos:prefLabel xml:lang="vi">phần cấu thành</skos:prefLabel>
      <rdakit:toolkitLabel xml:lang="vi">phần cấu thành</rdakit:toolkitLabel>
      <skos:definition xml:lang="vi">Đơn vị riêng biệt của nội dung trí tuệ bên trong một tài nguyên lớn hơn.</skos:definition>
      <rdakit:toolkitDefinition xml:lang="vi">Đơn vị riêng biệt của nội dung trí tuệ bên trong một tài nguyên lớn hơn.</rdakit:toolkitDefinition>
      <skos:prefLabel xml:lang="no">avgrenset del</skos:prefLabel>
      <rdakit:toolkitLabel xml:lang="no">avgrenset del</rdakit:toolkitLabel>
      <skos:definition xml:lang="no">En avgrenset, intellektuell enhet innen en mer omfattende ressurs.</skos:definition>
      <rdakit:toolkitDefinition xml:lang="no">En avgrenset, intellektuell enhet innen en mer omfattende ressurs.</rdakit:toolkitDefinition>
    </skos:Concept>
<!-- Concept: composite description  -->
    <skos:Concept rdf:about="http://rdaregistry.info/termList/RDATerms/1022" xml:lang="en">
      <skos:inScheme rdf:resource="http://rdaregistry.info/termList/RDATerms"/>
      <reg:status rdf:resource="http://metadataregistry.org/uri/RegStatus/1001"/>
      <reg:identifier rdf:resource="http://metadataregistry.org/concepts/8537"/>
      <skos:prefLabel xml:lang="en">composite description</skos:prefLabel>
      <rdakit:toolkitLabel xml:lang="en">composite description</rdakit:toolkitLabel>
      <skos:definition xml:lang="en">A description that combines one or more elements identifying a work and/or expression embodied in a manifestation with a description of the manifestation.</skos:definition>
      <rdakit:toolkitDefinition xml:lang="en">A description that combines one or more elements identifying a work and/or expression embodied in a manifestation with a description of the manifestation.</rdakit:toolkitDefinition>
      <skos:prefLabel xml:lang="it">descrizione composita</skos:prefLabel>
      <rdakit:toolkitLabel xml:lang="it">descrizione composita</rdakit:toolkitLabel>
      <skos:definition xml:lang="it">Descrizione che combina la descrizione di una manifestazione con uno o più elementi che identificano l'opera e/o l'espressione materializzate in quella manifestazione.</skos:definition>
      <rdakit:toolkitDefinition xml:lang="it">Descrizione che combina la descrizione di una manifestazione con uno o più elementi che identificano l'opera e/o l'espressione materializzate in quella manifestazione.</rdakit:toolkitDefinition>
      <skos:prefLabel xml:lang="fr">description composite</skos:prefLabel>
      <rdakit:toolkitLabel xml:lang="fr">description composite</rdakit:toolkitLabel>
      <skos:definition xml:lang="fr">Description qui combine un ou plusieurs éléments identifiant une œuvre et/ou une expression matérialisée dans une manifestation avec une description de la manifestation.</skos:definition>
      <rdakit:toolkitDefinition xml:lang="fr">Description qui combine un ou plusieurs éléments identifiant une œuvre et/ou une expression matérialisée dans une manifestation avec une description de la manifestation.</rdakit:toolkitDefinition>
      <skos:prefLabel xml:lang="es">descripción compuesta</skos:prefLabel>
      <rdakit:toolkitLabel xml:lang="es">descripción compuesta</rdakit:toolkitLabel>
      <skos:definition xml:lang="es">Descripción que combina uno o más elementos que identifican una obra y/o expresión materializada en una manifestación con una descripción de una manifestación.</skos:definition>
      <rdakit:toolkitDefinition xml:lang="es">Descripción que combina uno o más elementos que identifican una obra y/o expresión materializada en una manifestación con una descripción de una manifestación.</rdakit:toolkitDefinition>
      <skos:prefLabel xml:lang="de">Zusammengesetzte Beschreibung</skos:prefLabel>
      <rdakit:toolkitLabel xml:lang="de">Zusammengesetzte Beschreibung</rdakit:toolkitLabel>
      <skos:definition xml:lang="de">Eine Beschreibung, die ein Element oder mehrere Elemente, das/die ein Werk und/oder eine Expression identifiziert/identifizieren, das/die in einer Manifestation verkörpert ist/sind, mit einer Beschreibung der Manifestation kombiniert.</skos:definition>
      <rdakit:toolkitDefinition xml:lang="de">Eine Beschreibung, die ein Element oder mehrere Elemente, das/die ein Werk und/oder eine Expression identifiziert/identifizieren, das/die in einer Manifestation verkörpert ist/sind, mit einer Beschreibung der Manifestation kombiniert.</rdakit:toolkitDefinition>
      <skos:prefLabel xml:lang="fi">yhdistelmäkuvailu</skos:prefLabel>
      <rdakit:toolkitLabel xml:lang="fi">yhdistelmäkuvailu</rdakit:toolkitLabel>
      <skos:definition xml:lang="fi">Yhdistelmäkuvailulla laaditaan kokonaisuus, joka sisältää yhden tai useampia teosta ja/tai ekspressiota identifioivia elementtejä sekä niiden manifestaation kuvailun.</skos:definition>
      <rdakit:toolkitDefinition xml:lang="fi">Yhdistelmäkuvailulla laaditaan kokonaisuus, joka sisältää yhden tai useampia teosta ja/tai ekspressiota identifioivia elementtejä sekä niiden manifestaation kuvailun.</rdakit:toolkitDefinition>
      <skos:prefLabel xml:lang="da">sammensat beskrivelse</skos:prefLabel>
      <rdakit:toolkitLabel xml:lang="da">sammensat beskrivelse</rdakit:toolkitLabel>
      <skos:definition xml:lang="da">Beskrivelse af en manifestation der samtidig indeholder et eller flere elementer, der identificerer det værk og/eller det udtryk, der er indeholdt i manifestationen.</skos:definition>
      <rdakit:toolkitDefinition xml:lang="da">Beskrivelse af en manifestation der samtidig indeholder et eller flere elementer, der identificerer det værk og/eller det udtryk, der er indeholdt i manifestationen.</rdakit:toolkitDefinition>
      <skos:prefLabel xml:lang="ca">descripció composta</skos:prefLabel>
      <rdakit:toolkitLabel xml:lang="ca">descripció composta</rdakit:toolkitLabel>
      <skos:definition xml:lang="ca">Descripció que combina un o més elements que identifiquen una obra i/o una expressió materialitzada en una manifestació amb una descripció de la manifestació.</skos:definition>
      <rdakit:toolkitDefinition xml:lang="ca">Descripció que combina un o més elements que identifiquen una obra i/o una expressió materialitzada en una manifestació amb una descripció de la manifestació.</rdakit:toolkitDefinition>
      <skos:prefLabel xml:lang="vi">mô tả hỗn hợp</skos:prefLabel>
      <rdakit:toolkitLabel xml:lang="vi">mô tả hỗn hợp</rdakit:toolkitLabel>
      <skos:definition xml:lang="vi">Mô tả kết hợp một hoặc nhiều hơn yếu tố nhận dạng một tác phẩm và/hoặc biểu hiện được thể hiện trong một biểu thị với một mô tả của biểu thị.</skos:definition>
      <rdakit:toolkitDefinition xml:lang="vi">Mô tả kết hợp một hoặc nhiều hơn yếu tố nhận dạng một tác phẩm và/hoặc biểu hiện được thể hiện trong một biểu thị với một mô tả của biểu thị.</rdakit:toolkitDefinition>
      <skos:prefLabel xml:lang="no">sammensatt beskrivelse</skos:prefLabel>
      <rdakit:toolkitLabel xml:lang="no">sammensatt beskrivelse</rdakit:toolkitLabel>
      <skos:definition xml:lang="no">En beskrivelse som kombinerer ett eller flere elementer som identifiserer et verk og/eller et uttrykk innbefattet i en manifestasjon med en beskrivelse av manifestasjonen.</skos:definition>
      <rdakit:toolkitDefinition xml:lang="no">En beskrivelse som kombinerer ett eller flere elementer som identifiserer et verk og/eller et uttrykk innbefattet i en manifestasjon med en beskrivelse av manifestasjonen.</rdakit:toolkitDefinition>
    </skos:Concept>
<!-- Concept: compound surname  -->
    <skos:Concept rdf:about="http://rdaregistry.info/termList/RDATerms/1023" xml:lang="en">
      <skos:inScheme rdf:resource="http://rdaregistry.info/termList/RDATerms"/>
      <reg:status rdf:resource="http://metadataregistry.org/uri/RegStatus/1001"/>
      <reg:identifier rdf:resource="http://metadataregistry.org/concepts/8538"/>
      <skos:prefLabel xml:lang="en">compound surname</skos:prefLabel>
      <rdakit:toolkitLabel xml:lang="en">compound surname</rdakit:toolkitLabel>
      <skos:definition xml:lang="en">A surname consisting of two or more proper names, sometimes connected by a hyphen, or conjunction, and/or preposition.</skos:definition>
      <rdakit:toolkitDefinition xml:lang="en">A surname consisting of two or more proper names, sometimes connected by a hyphen, or conjunction, and/or preposition.</rdakit:toolkitDefinition>
      <skos:prefLabel xml:lang="it">cognome composto</skos:prefLabel>
      <rdakit:toolkitLabel xml:lang="it">cognome composto</rdakit:toolkitLabel>
      <skos:definition xml:lang="it">Cognome che consiste di due o più nomi propri, talvolta connessi da un trattino o una congiunzione e/o una preposizione.</skos:definition>
      <rdakit:toolkitDefinition xml:lang="it">Cognome che consiste di due o più nomi propri, talvolta connessi da un trattino o una congiunzione e/o una preposizione.</rdakit:toolkitDefinition>
      <skos:prefLabel xml:lang="fr">nom de famille composé</skos:prefLabel>
      <rdakit:toolkitLabel xml:lang="fr">nom de famille composé</rdakit:toolkitLabel>
      <skos:definition xml:lang="fr">Nom de famille constitué de deux ou plusieurs noms propres parfois reliés par un trait d’union, une conjonction et/ou une préposition.</skos:definition>
      <rdakit:toolkitDefinition xml:lang="fr">Nom de famille constitué de deux ou plusieurs noms propres parfois reliés par un trait d’union, une conjonction et/ou une préposition.</rdakit:toolkitDefinition>
      <skos:prefLabel xml:lang="de">Zusammengesetzter Nachname</skos:prefLabel>
      <rdakit:toolkitLabel xml:lang="de">Zusammengesetzter Nachname</rdakit:toolkitLabel>
      <skos:definition xml:lang="de">Ein Nachname, der aus mehreren Eigennamen besteht, die manchmal mit einem Bindestrich oder einer Konjunktion und/oder einer Präposition verbunden sind.</skos:definition>
      <rdakit:toolkitDefinition xml:lang="de">Ein Nachname, der aus mehreren Eigennamen besteht, die manchmal mit einem Bindestrich oder einer Konjunktion und/oder einer Präposition verbunden sind.</rdakit:toolkitDefinition>
      <skos:prefLabel xml:lang="fi">moniosainen sukunimi</skos:prefLabel>
      <rdakit:toolkitLabel xml:lang="fi">moniosainen sukunimi</rdakit:toolkitLabel>
      <skos:definition xml:lang="fi">Sukunimi, joka koostuu kahdesta tai useammasta nimestä. Nimiä voi yhdistää yhdysmerkki, konjunktio ja/tai prepositio.</skos:definition>
      <rdakit:toolkitDefinition xml:lang="fi">Sukunimi, joka koostuu kahdesta tai useammasta nimestä. Nimiä voi yhdistää yhdysmerkki, konjunktio ja/tai prepositio.</rdakit:toolkitDefinition>
      <skos:prefLabel xml:lang="da">sammensat efternavn</skos:prefLabel>
      <rdakit:toolkitLabel xml:lang="da">sammensat efternavn</rdakit:toolkitLabel>
      <skos:definition xml:lang="da">Efternavn, der består af to eller flere egennavne, nogle gange forbundet af en bindestreg, et bindeord og/eller et forholdsord.</skos:definition>
      <rdakit:toolkitDefinition xml:lang="da">Efternavn, der består af to eller flere egennavne, nogle gange forbundet af en bindestreg, et bindeord og/eller et forholdsord.</rdakit:toolkitDefinition>
      <skos:prefLabel xml:lang="ca">cognom compost</skos:prefLabel>
      <rdakit:toolkitLabel xml:lang="ca">cognom compost</rdakit:toolkitLabel>
      <skos:definition xml:lang="ca">Cognom que consisteix en dos o més noms propis, de vegades connectats amb un guionet, una conjunció i/o una preposició.</skos:definition>
      <rdakit:toolkitDefinition xml:lang="ca">Cognom que consisteix en dos o més noms propis, de vegades connectats amb un guionet, una conjunció i/o una preposició.</rdakit:toolkitDefinition>
      <skos:prefLabel xml:lang="vi">họ phức hợp</skos:prefLabel>
      <rdakit:toolkitLabel xml:lang="vi">họ phức hợp</rdakit:toolkitLabel>
      <skos:definition xml:lang="vi">Họ chứa hai hoặc nhiều tên riêng, đôi khi nối bằng gạch nối, hoặc liên từ, và/hoặc giới từ.</skos:definition>
      <rdakit:toolkitDefinition xml:lang="vi">Họ chứa hai hoặc nhiều tên riêng, đôi khi nối bằng gạch nối, hoặc liên từ, và/hoặc giới từ.</rdakit:toolkitDefinition>
      <skos:prefLabel xml:lang="no">sammensatt etternavn</skos:prefLabel>
      <rdakit:toolkitLabel xml:lang="no">sammensatt etternavn</rdakit:toolkitLabel>
      <skos:definition xml:lang="no">Et etternavn som består av to eller flere egennavn, noen ganger forbundet med en bindestrek, konjunksjon og/eller preposisjon.</skos:definition>
      <rdakit:toolkitDefinition xml:lang="no">Et etternavn som består av to eller flere egennavn, noen ganger forbundet med en bindestrek, konjunksjon og/eller preposisjon.</rdakit:toolkitDefinition>
    </skos:Concept>
<!-- Concept: comprehensive description  -->
    <skos:Concept rdf:about="http://rdaregistry.info/termList/RDATerms/1024" xml:lang="en">
      <skos:inScheme rdf:resource="http://rdaregistry.info/termList/RDATerms"/>
      <reg:status rdf:resource="http://metadataregistry.org/uri/RegStatus/1001"/>
      <reg:identifier rdf:resource="http://metadataregistry.org/concepts/8539"/>
      <skos:prefLabel xml:lang="en">comprehensive description</skos:prefLabel>
      <rdakit:toolkitLabel xml:lang="en">comprehensive description</rdakit:toolkitLabel>
      <skos:definition xml:lang="en">A description that describes the manifestation as a whole.</skos:definition>
      <rdakit:toolkitDefinition xml:lang="en">A description that describes the manifestation as a whole.</rdakit:toolkitDefinition>
      <skos:scopeNote xml:lang="en">A description for a map, a periodical, a collection of posters assembled by a library, or a kit consisting of a filmstrip, an audiotape, and a teacher’s manual, are included.</skos:scopeNote>
      <skos:prefLabel xml:lang="it">descrizione comprensiva</skos:prefLabel>
      <rdakit:toolkitLabel xml:lang="it">descrizione comprensiva</rdakit:toolkitLabel>
      <skos:definition xml:lang="it">Descrizione che rappresenta la risorsa nel suo insieme</skos:definition>
      <rdakit:toolkitDefinition xml:lang="it">Descrizione che rappresenta la risorsa nel suo insieme</rdakit:toolkitDefinition>
      <skos:prefLabel xml:lang="fr">description globale</skos:prefLabel>
      <rdakit:toolkitLabel xml:lang="fr">description globale</rdakit:toolkitLabel>
      <skos:definition xml:lang="fr">Description qui décrit la manifestation dans son ensemble</skos:definition>
      <rdakit:toolkitDefinition xml:lang="fr">Description qui décrit la manifestation dans son ensemble</rdakit:toolkitDefinition>
      <skos:prefLabel xml:lang="es">descripción integral</skos:prefLabel>
      <rdakit:toolkitLabel xml:lang="es">descripción integral</rdakit:toolkitLabel>
      <skos:definition xml:lang="es">Descripción en la que se describe al recurso como un todo.</skos:definition>
      <rdakit:toolkitDefinition xml:lang="es">Descripción en la que se describe al recurso como un todo.</rdakit:toolkitDefinition>
      <skos:prefLabel xml:lang="de">Umfassende Beschreibung</skos:prefLabel>
      <rdakit:toolkitLabel xml:lang="de">Umfassende Beschreibung</rdakit:toolkitLabel>
      <skos:definition xml:lang="de">Eine Beschreibung, die eine Manifestation als Ganzes beschreibt.</skos:definition>
      <rdakit:toolkitDefinition xml:lang="de">Eine Beschreibung, die eine Manifestation als Ganzes beschreibt.</rdakit:toolkitDefinition>
      <skos:scopeNote xml:lang="de">Dazu gehört eine Beschreibung einer Karte, einer Zeitschrift, einer Sammlung von Plakaten einer Bibliothek oder eine Medienkombination, die aus einem Filmstreifen, einem Tonband und einem Lehrerhandbuch besteht.</skos:scopeNote>
      <skos:prefLabel xml:lang="fi">kokonaisuuden kuvailu</skos:prefLabel>
      <rdakit:toolkitLabel xml:lang="fi">kokonaisuuden kuvailu</rdakit:toolkitLabel>
      <skos:definition xml:lang="fi">Manifestaation kuvailun kuvailu.</skos:definition>
      <rdakit:toolkitDefinition xml:lang="fi">Manifestaation kuvailun kuvailu.</rdakit:toolkitDefinition>
      <skos:scopeNote xml:lang="fi">Esim. kartan, aikakausjulkaisun, kirjaston julistekokoelman tai rainasta, äänikasetista ja opettajan oppaasta muodostuvan koosteen kuvailu.</skos:scopeNote>
      <skos:prefLabel xml:lang="da">helhedsbeskrivelse</skos:prefLabel>
      <rdakit:toolkitLabel xml:lang="da">helhedsbeskrivelse</rdakit:toolkitLabel>
      <skos:definition xml:lang="da">Beskrivelse, der beskriver manifestationen som helhed.</skos:definition>
      <rdakit:toolkitDefinition xml:lang="da">Beskrivelse, der beskriver manifestationen som helhed.</rdakit:toolkitDefinition>
      <skos:scopeNote xml:lang="da">Beskrivelse af et kort, et tidsskrift, en plakatsamling, der er sat sammen af et bibliotek, et sæt, der består af en filmstrip, et lydbånd og en undervisningsvejledning er omfattet.</skos:scopeNote>
      <skos:prefLabel xml:lang="ca">descripció completa</skos:prefLabel>
      <rdakit:toolkitLabel xml:lang="ca">descripció completa</rdakit:toolkitLabel>
      <skos:definition xml:lang="ca">Descripció que descriu la manifestació com un tot.</skos:definition>
      <rdakit:toolkitDefinition xml:lang="ca">Descripció que descriu la manifestació com un tot.</rdakit:toolkitDefinition>
      <skos:scopeNote xml:lang="ca">Inclou una descripció d'un mapa, un periòdic, una col·lecció de cartells aplegada per una biblioteca, un document compost que consisteix en una filmina, una cinta àudio i un manual del mestre.</skos:scopeNote>
      <skos:scopeNote xml:lang="fr">Comprend une description d’une carte, d’un périodique, d’une collection d’affiches rassemblée par une bibliothèque ou d’une ressource multimédia multisupport comprenant un film fixe, une bande audio et un manuel de l’enseignant.</skos:scopeNote>
      <skos:prefLabel xml:lang="vi">mô tả tổng hợp</skos:prefLabel>
      <rdakit:toolkitLabel xml:lang="vi">mô tả tổng hợp</rdakit:toolkitLabel>
      <skos:definition xml:lang="vi">Mô tả toàn bộ biểu thị.</skos:definition>
      <rdakit:toolkitDefinition xml:lang="vi">Mô tả toàn bộ biểu thị.</rdakit:toolkitDefinition>
      <skos:scopeNote xml:lang="vi">Mô tả bản đồ, ấn phẩm định kỳ, bộ sưu tập áp phích do thư viện thu thập, phim đèn chiếu, băng audio, cẩm nang giáo viện, được bao gồm.</skos:scopeNote>
      <skos:prefLabel xml:lang="no">samlet beskrivelse</skos:prefLabel>
      <rdakit:toolkitLabel xml:lang="no">samlet beskrivelse</rdakit:toolkitLabel>
      <skos:definition xml:lang="no">En beskrivelse som beskriver manifestasjonen som helhet.</skos:definition>
      <rdakit:toolkitDefinition xml:lang="no">En beskrivelse som beskriver manifestasjonen som helhet.</rdakit:toolkitDefinition>
      <skos:scopeNote xml:lang="no">En beskrivelse av et kart, et periodikum, en plakatsamling i biblioteket, eller et kombinert dokument bestående av en filmremse, et lydbånd og en lærerveiledning, er inkludert.</skos:scopeNote>
    </skos:Concept>
<!-- Concept: conference  -->
    <skos:Concept rdf:about="http://rdaregistry.info/termList/RDATerms/1025" xml:lang="en">
      <skos:inScheme rdf:resource="http://rdaregistry.info/termList/RDATerms"/>
      <reg:status rdf:resource="http://metadataregistry.org/uri/RegStatus/1001"/>
      <reg:identifier rdf:resource="http://metadataregistry.org/concepts/8540"/>
      <skos:prefLabel xml:lang="en">conference</skos:prefLabel>
      <rdakit:toolkitLabel xml:lang="en">conference</rdakit:toolkitLabel>
      <skos:definition xml:lang="en">A meeting of individuals or representatives of various bodies for the purpose of discussing and/or acting on topics of common interest or a meeting of representatives of a corporate body that constitutes its legislative or governing body.</skos:definition>
      <rdakit:toolkitDefinition xml:lang="en">A meeting of individuals or representatives of various bodies for the purpose of discussing and/or acting on topics of common interest or a meeting of representatives of a corporate body that constitutes its legislative or governing body.</rdakit:toolkitDefinition>
      <skos:prefLabel xml:lang="it">conferenza</skos:prefLabel>
      <rdakit:toolkitLabel xml:lang="it">conferenza</rdakit:toolkitLabel>
      <skos:definition xml:lang="it">Incontro di persone o rappresentanti di vari enti per discutere e/o agire su temi di comune interesse o incontro dei rappresentanti di un ente che ne costituisce l'organo legislativo o di governo.</skos:definition>
      <rdakit:toolkitDefinition xml:lang="it">Incontro di persone o rappresentanti di vari enti per discutere e/o agire su temi di comune interesse o incontro dei rappresentanti di un ente che ne costituisce l'organo legislativo o di governo.</rdakit:toolkitDefinition>
      <skos:prefLabel xml:lang="de">Konferenz</skos:prefLabel>
      <rdakit:toolkitLabel xml:lang="de">Konferenz</rdakit:toolkitLabel>
      <skos:definition xml:lang="de">Eine Tagung von Personen oder Vertretern verschiedener Gruppen zum Zwecke der Diskussion und/oder Behandlung von Themen von gemeinsamem Interesse oder eine Tagung von Vertretern einer Körperschaft, die deren direktives oder ausführendes Gremium darstellt.</skos:definition>
      <rdakit:toolkitDefinition xml:lang="de">Eine Tagung von Personen oder Vertretern verschiedener Gruppen zum Zwecke der Diskussion und/oder Behandlung von Themen von gemeinsamem Interesse oder eine Tagung von Vertretern einer Körperschaft, die deren direktives oder ausführendes Gremium darstellt.</rdakit:toolkitDefinition>
      <skos:prefLabel xml:lang="fi">konferenssi</skos:prefLabel>
      <rdakit:toolkitLabel xml:lang="fi">konferenssi</rdakit:toolkitLabel>
      <skos:definition xml:lang="fi">Tilaisuus, johon yksilöt tai yhteisöjen edustajat kokoontuvat keskustelemaan ja/tai toimimaan yhteisesti kiinnostavan aiheen puolesta, tai yhteisön lakiasäätävän tai hallinnollisen elimen kokoontuminen.</skos:definition>
      <rdakit:toolkitDefinition xml:lang="fi">Tilaisuus, johon yksilöt tai yhteisöjen edustajat kokoontuvat keskustelemaan ja/tai toimimaan yhteisesti kiinnostavan aiheen puolesta, tai yhteisön lakiasäätävän tai hallinnollisen elimen kokoontuminen.</rdakit:toolkitDefinition>
      <skos:prefLabel xml:lang="da">konference</skos:prefLabel>
      <rdakit:toolkitLabel xml:lang="da">konference</rdakit:toolkitLabel>
      <skos:definition xml:lang="da">Møde mellem enkeltpersoner eller repræsentanter for forskellige institutioner med det formål at diskutere og/eller gøre noget ved emner af fælles interesse, eller møde mellem repræsentanter for en korporation, der udgør den juridisk ansvarlige eller styrende forsamling.</skos:definition>
      <rdakit:toolkitDefinition xml:lang="da">Møde mellem enkeltpersoner eller repræsentanter for forskellige institutioner med det formål at diskutere og/eller gøre noget ved emner af fælles interesse, eller møde mellem repræsentanter for en korporation, der udgør den juridisk ansvarlige eller styrende forsamling.</rdakit:toolkitDefinition>
      <skos:prefLabel xml:lang="ca">congrés</skos:prefLabel>
      <rdakit:toolkitLabel xml:lang="ca">congrés</rdakit:toolkitLabel>
      <skos:definition xml:lang="ca">Reunió d’individus o de representants de diverses entitats amb la finalitat de discutir i/o d’actuar sobre temes d’interès comú, o una reunió de representants d’una entitat corporativa que constitueix el seu òrgan legislatiu o de govern.</skos:definition>
      <rdakit:toolkitDefinition xml:lang="ca">Reunió d’individus o de representants de diverses entitats amb la finalitat de discutir i/o d’actuar sobre temes d’interès comú, o una reunió de representants d’una entitat corporativa que constitueix el seu òrgan legislatiu o de govern.</rdakit:toolkitDefinition>
      <skos:prefLabel xml:lang="fr">congrès</skos:prefLabel>
      <rdakit:toolkitLabel xml:lang="fr">congrès</rdakit:toolkitLabel>
      <skos:definition xml:lang="fr">Réunion de particuliers ou de représentants de diverses collectivités dans le but de discuter et/ou d’agir sur des sujets d’intérêt général ou réunion des représentants d’une collectivité, qui constitue son corps législatif ou administratif.</skos:definition>
      <rdakit:toolkitDefinition xml:lang="fr">Réunion de particuliers ou de représentants de diverses collectivités dans le but de discuter et/ou d’agir sur des sujets d’intérêt général ou réunion des représentants d’une collectivité, qui constitue son corps législatif ou administratif.</rdakit:toolkitDefinition>
      <skos:prefLabel xml:lang="vi">hội nghị</skos:prefLabel>
      <rdakit:toolkitLabel xml:lang="vi">hội nghị</rdakit:toolkitLabel>
      <skos:definition xml:lang="vi">Cuộc họp của các cá nhân hoặc đại diện của các cơ quan khác nhau nhằm mục đích thảo luận và/hoặc hoạt động về các đề tài được quan tâm chung hoặc Cuộc họp của đại diện của một tập thể thiết lập cơ quan pháp luật và cai trị.</skos:definition>
      <rdakit:toolkitDefinition xml:lang="vi">Cuộc họp của các cá nhân hoặc đại diện của các cơ quan khác nhau nhằm mục đích thảo luận và/hoặc hoạt động về các đề tài được quan tâm chung hoặc Cuộc họp của đại diện của một tập thể thiết lập cơ quan pháp luật và cai trị.</rdakit:toolkitDefinition>
      <skos:prefLabel xml:lang="no">konferanse</skos:prefLabel>
      <rdakit:toolkitLabel xml:lang="no">konferanse</rdakit:toolkitLabel>
      <skos:definition xml:lang="no">Et møte mellom enkeltpersoner eller representanter for ulike organer for å diskutere og/eller handle i forhold til emner av felles interesse, eller et møte mellom representanter for en korporasjon som utgjør korporasjonens lovgivende eller styrende organ.</skos:definition>
      <rdakit:toolkitDefinition xml:lang="no">Et møte mellom enkeltpersoner eller representanter for ulike organer for å diskutere og/eller handle i forhold til emner av felles interesse, eller et møte mellom representanter for en korporasjon som utgjør korporasjonens lovgivende eller styrende organ.</rdakit:toolkitDefinition>
    </skos:Concept>
<!-- Concept: container  -->
    <skos:Concept rdf:about="http://rdaregistry.info/termList/RDATerms/1026" xml:lang="en">
      <skos:inScheme rdf:resource="http://rdaregistry.info/termList/RDATerms"/>
      <reg:status rdf:resource="http://metadataregistry.org/uri/RegStatus/1001"/>
      <reg:identifier rdf:resource="http://metadataregistry.org/concepts/8541"/>
      <skos:prefLabel xml:lang="en">container</skos:prefLabel>
      <rdakit:toolkitLabel xml:lang="en">container</rdakit:toolkitLabel>
      <skos:definition xml:lang="en">A housing that is physically separable from the carrier being housed.</skos:definition>
      <rdakit:toolkitDefinition xml:lang="en">A housing that is physically separable from the carrier being housed.</rdakit:toolkitDefinition>
      <skos:scopeNote xml:lang="en">A container includes a box for a disc or videocassette, a sleeve for a videodisc, etc.; an insert visible through the housing is part of the container.</skos:scopeNote>
	    <skos:related rdf:resource="http://rdaregistry.info/termList/RDATerms/1016"/>
	    <skos:related rdf:resource="http://rdaregistry.info/termList/RDATerms/1058"/>
	    <skos:related rdf:resource="http://rdaregistry.info/termList/RDATerms/1086"/>
	    <skos:narrower rdf:resource="http://rdaregistry.info/termList/RDATerms/1054"/>
      <skos:prefLabel xml:lang="it">contenitore</skos:prefLabel>
      <rdakit:toolkitLabel xml:lang="it">contenitore</rdakit:toolkitLabel>
      <skos:definition xml:lang="it">Custodia della risorsa, che ne è fisicamente separabile.</skos:definition>
      <rdakit:toolkitDefinition xml:lang="it">Custodia della risorsa, che ne è fisicamente separabile.</rdakit:toolkitDefinition>
      <skos:prefLabel xml:lang="fr">conteneur</skos:prefLabel>
      <rdakit:toolkitLabel xml:lang="fr">conteneur</rdakit:toolkitLabel>
      <skos:definition xml:lang="fr">Contenant qui est physiquement séparable du support matériel qu’il contient.</skos:definition>
      <rdakit:toolkitDefinition xml:lang="fr">Contenant qui est physiquement séparable du support matériel qu’il contient.</rdakit:toolkitDefinition>
      <skos:prefLabel xml:lang="de">Behältnis</skos:prefLabel>
      <rdakit:toolkitLabel xml:lang="de">Behältnis</rdakit:toolkitLabel>
      <skos:definition xml:lang="de">Ein Gehäuse, das von dem darin aufbewahrten Datenträger physisch trennbar ist.</skos:definition>
      <rdakit:toolkitDefinition xml:lang="de">Ein Gehäuse, das von dem darin aufbewahrten Datenträger physisch trennbar ist.</rdakit:toolkitDefinition>
      <skos:scopeNote xml:lang="de">Zum Behältnis gehört eine Schachtel für eine Disk oder eine Videokassette, eine Hülle für eine Videodisk usw. Eine Beilage, die durch das Gehäuse hindurch sichtbar ist, ist Teil des Behältnisses.</skos:scopeNote>
      <skos:prefLabel xml:lang="fi">kotelo</skos:prefLabel>
      <rdakit:toolkitLabel xml:lang="fi">kotelo</rdakit:toolkitLabel>
      <skos:definition xml:lang="fi">Aineiston säilyttämiseen tarkoitettu kotelo, josta säilytettävä tallenne on fyysisesti erotettavissa.</skos:definition>
      <rdakit:toolkitDefinition xml:lang="fi">Aineiston säilyttämiseen tarkoitettu kotelo, josta säilytettävä tallenne on fyysisesti erotettavissa.</rdakit:toolkitDefinition>
      <skos:scopeNote xml:lang="fi">Kotelo käsittää CD-levyn tai videokasetin kotelon, videolevyn suojuksen jne.</skos:scopeNote>
      <skos:prefLabel xml:lang="da">opbevaringsudstyr</skos:prefLabel>
      <rdakit:toolkitLabel xml:lang="da">opbevaringsudstyr</rdakit:toolkitLabel>
      <skos:definition xml:lang="da">Indpakning, der typisk kan adskilles fra den bærer, den indeholder</skos:definition>
      <rdakit:toolkitDefinition xml:lang="da">Indpakning, der typisk kan adskilles fra den bærer, den indeholder</rdakit:toolkitDefinition>
      <skos:scopeNote xml:lang="da">Et opbevaringsudstyr omfatter en kasse eller æske til en disc eller et videobånd, et hylster til en videodisc, etc.; et indstik der er synligt gennem indpakningen er en del af opbevaringsudstyret.</skos:scopeNote>
      <skos:prefLabel xml:lang="ca">contenidor</skos:prefLabel>
      <rdakit:toolkitLabel xml:lang="ca">contenidor</rdakit:toolkitLabel>
      <skos:definition xml:lang="ca">Embolcall que està separat físicament del suport físic que conté.</skos:definition>
      <rdakit:toolkitDefinition xml:lang="ca">Embolcall que està separat físicament del suport físic que conté.</rdakit:toolkitDefinition>
      <skos:scopeNote xml:lang="ca">Un contenidor inclou una capsa d’un disc o una videocasset, una funda d’un videodisc, etc.; un encartament visible a través de l'embolcall que és part del contenidor.</skos:scopeNote>
      <skos:scopeNote xml:lang="fr">Comprend un boîtier de disque ou de cassette vidéo, une pochette de vidéodisque, etc. ; une insertion visible à travers le contenant fait partie du conteneur.</skos:scopeNote>
      <skos:prefLabel xml:lang="vi">vỏ chứa</skos:prefLabel>
      <rdakit:toolkitLabel xml:lang="vi">vỏ chứa</rdakit:toolkitLabel>
      <skos:definition xml:lang="vi">Vỏ bọc phân cách về vật lý với tài nguyên được chứa.</skos:definition>
      <rdakit:toolkitDefinition xml:lang="vi">Vỏ bọc phân cách về vật lý với tài nguyên được chứa.</rdakit:toolkitDefinition>
      <skos:scopeNote xml:lang="vi">Vỏ chức bao gồm hộp đựng đĩa hoặc videocasset, vỏ đĩa video, v.v..., bộ phận chèn có thể nhìn thấy quavỏ bọclà phần củavỏchứa</skos:scopeNote>
      <skos:prefLabel xml:lang="no">beholder</skos:prefLabel>
      <rdakit:toolkitLabel xml:lang="no">beholder</rdakit:toolkitLabel>
      <skos:definition xml:lang="no">En beholder som kan skilles fysisk fra bæreren i beholderen.</skos:definition>
      <rdakit:toolkitDefinition xml:lang="no">En beholder som kan skilles fysisk fra bæreren i beholderen.</rdakit:toolkitDefinition>
      <skos:scopeNote xml:lang="no">En beholder kan være et plateomslag eller omslag for videokassett, en boks, etc. Et innlegg som er synlig gjennom beholderen, er en del av beholderen.</skos:scopeNote>
    </skos:Concept>
<!-- Concept: conventional collective title  -->
    <skos:Concept rdf:about="http://rdaregistry.info/termList/RDATerms/1027" xml:lang="en">
      <skos:inScheme rdf:resource="http://rdaregistry.info/termList/RDATerms"/>
      <reg:status rdf:resource="http://metadataregistry.org/uri/RegStatus/1001"/>
      <reg:identifier rdf:resource="http://metadataregistry.org/concepts/8542"/>
      <skos:prefLabel xml:lang="en">conventional collective title</skos:prefLabel>
      <rdakit:toolkitLabel xml:lang="en">conventional collective title</rdakit:toolkitLabel>
      <skos:definition xml:lang="en">A title used as a preferred title for a compilation containing two or more works by one agent, or two or more parts of a work.</skos:definition>
      <rdakit:toolkitDefinition xml:lang="en">A title used as a preferred title for a compilation containing two or more works by one agent, or two or more parts of a work.</rdakit:toolkitDefinition>
	    <skos:broader rdf:resource="http://rdaregistry.info/termList/RDATerms/1020"/>
      <skos:prefLabel xml:lang="it">titolo collettivo convenzionale</skos:prefLabel>
      <rdakit:toolkitLabel xml:lang="it">titolo collettivo convenzionale</rdakit:toolkitLabel>
      <skos:definition xml:lang="it">Titolo utilizzato come titolo preferito per una compilazione che contiene due o più opere di una persona, famiglia o ente, o due o più parti di un'opera.</skos:definition>
      <rdakit:toolkitDefinition xml:lang="it">Titolo utilizzato come titolo preferito per una compilazione che contiene due o più opere di una persona, famiglia o ente, o due o più parti di un'opera.</rdakit:toolkitDefinition>
      <skos:prefLabel xml:lang="fr">titre collectif conventionnel</skos:prefLabel>
      <rdakit:toolkitLabel xml:lang="fr">titre collectif conventionnel</rdakit:toolkitLabel>
      <skos:definition xml:lang="fr">Titre utilisé comme titre privilégié pour une compilation contenant deux ou plusieurs œuvres d’un même agent ou deux ou plusieurs parties d’une œuvre.</skos:definition>
      <rdakit:toolkitDefinition xml:lang="fr">Titre utilisé comme titre privilégié pour une compilation contenant deux ou plusieurs œuvres d’un même agent ou deux ou plusieurs parties d’une œuvre.</rdakit:toolkitDefinition>
      <skos:prefLabel xml:lang="de">Formaltitel</skos:prefLabel>
      <rdakit:toolkitLabel xml:lang="de">Formaltitel</rdakit:toolkitLabel>
      <skos:definition xml:lang="de">Ein Titel, der als bevorzugter Titel für eine Zusammenstellung verwendet wird, die aus mehreren Werken oder mehreren Teilen eines Werks (z. B. Werke, Lyrik, Auswahl) eines Akteurs besteht.</skos:definition>
      <rdakit:toolkitDefinition xml:lang="de">Ein Titel, der als bevorzugter Titel für eine Zusammenstellung verwendet wird, die aus mehreren Werken oder mehreren Teilen eines Werks (z. B. Werke, Lyrik, Auswahl) eines Akteurs besteht.</rdakit:toolkitDefinition>
      <skos:prefLabel xml:lang="fi">vakiintunut kokoava nimeke</skos:prefLabel>
      <rdakit:toolkitLabel xml:lang="fi">vakiintunut kokoava nimeke</rdakit:toolkitLabel>
      <skos:definition xml:lang="fi">Nimeke, jota käytetään ensisijaisena nimekkeenä kokoelmasta, joka sisältää kahden tai useamman toimijan teoksia, tai kaksi tai useamman osan teoksesta.</skos:definition>
      <rdakit:toolkitDefinition xml:lang="fi">Nimeke, jota käytetään ensisijaisena nimekkeenä kokoelmasta, joka sisältää kahden tai useamman toimijan teoksia, tai kaksi tai useamman osan teoksesta.</rdakit:toolkitDefinition>
      <skos:prefLabel xml:lang="da">konventionel fællestitel</skos:prefLabel>
      <rdakit:toolkitLabel xml:lang="da">konventionel fællestitel</rdakit:toolkitLabel>
      <skos:definition xml:lang="da">Titel, der anvendes som foretrukken titel for en samling, der indeholder to eller flere værker af en agent, eller to eller flere dele af et værk.</skos:definition>
      <rdakit:toolkitDefinition xml:lang="da">Titel, der anvendes som foretrukken titel for en samling, der indeholder to eller flere værker af en agent, eller to eller flere dele af et værk.</rdakit:toolkitDefinition>
      <skos:prefLabel xml:lang="ca">títol col·lectiu convencional</skos:prefLabel>
      <rdakit:toolkitLabel xml:lang="ca">títol col·lectiu convencional</rdakit:toolkitLabel>
      <skos:definition xml:lang="ca">Títol usat com a títol preferit d’una compilació que inclou dues o més obres d'un agent, o dues o més parts d’una obra.</skos:definition>
      <rdakit:toolkitDefinition xml:lang="ca">Títol usat com a títol preferit d’una compilació que inclou dues o més obres d'un agent, o dues o més parts d’una obra.</rdakit:toolkitDefinition>
      <skos:prefLabel xml:lang="vi">nhan đề tập hợp quy ước</skos:prefLabel>
      <rdakit:toolkitLabel xml:lang="vi">nhan đề tập hợp quy ước</rdakit:toolkitLabel>
      <skos:definition xml:lang="vi">Nhan đề được dùng như nhan đề ưu tiên của tổ hợp chứa hai hoặc nhiều hơn tác phẩm bởi một tác nhân, hoặc hai hoặc nhiều hơn phần của tác phẩm.</skos:definition>
      <rdakit:toolkitDefinition xml:lang="vi">Nhan đề được dùng như nhan đề ưu tiên của tổ hợp chứa hai hoặc nhiều hơn tác phẩm bởi một tác nhân, hoặc hai hoặc nhiều hơn phần của tác phẩm.</rdakit:toolkitDefinition>
      <skos:prefLabel xml:lang="no">konvensjonell fellestittel</skos:prefLabel>
      <rdakit:toolkitLabel xml:lang="no">konvensjonell fellestittel</rdakit:toolkitLabel>
      <skos:definition xml:lang="no">En tittel brukt som foretrukket tittel på en samling som inneholder to eller flere verk av én agent, eller to eller flere deler av et verk.</skos:definition>
      <rdakit:toolkitDefinition xml:lang="no">En tittel brukt som foretrukket tittel på en samling som inneholder to eller flere verk av én agent, eller to eller flere deler av et verk.</rdakit:toolkitDefinition>
    </skos:Concept>
<!-- Concept: conventional name  -->
    <skos:Concept rdf:about="http://rdaregistry.info/termList/RDATerms/1028" xml:lang="en">
      <skos:inScheme rdf:resource="http://rdaregistry.info/termList/RDATerms"/>
      <reg:status rdf:resource="http://metadataregistry.org/uri/RegStatus/1001"/>
      <reg:identifier rdf:resource="http://metadataregistry.org/concepts/8543"/>
      <skos:prefLabel xml:lang="en">conventional name</skos:prefLabel>
      <rdakit:toolkitLabel xml:lang="en">conventional name</rdakit:toolkitLabel>
      <skos:definition xml:lang="en">A name, other than the real or official name, by which a corporate body has come to be known.</skos:definition>
      <rdakit:toolkitDefinition xml:lang="en">A name, other than the real or official name, by which a corporate body has come to be known.</rdakit:toolkitDefinition>
      <skos:prefLabel xml:lang="it">nome convenzionale</skos:prefLabel>
      <rdakit:toolkitLabel xml:lang="it">nome convenzionale</rdakit:toolkitLabel>
      <skos:definition xml:lang="it">Nome, diverso dal nome reale o ufficiale, con cui un ente è conosciuto.</skos:definition>
      <rdakit:toolkitDefinition xml:lang="it">Nome, diverso dal nome reale o ufficiale, con cui un ente è conosciuto.</rdakit:toolkitDefinition>
      <skos:prefLabel xml:lang="fr">nom conventionnel</skos:prefLabel>
      <rdakit:toolkitLabel xml:lang="fr">nom conventionnel</rdakit:toolkitLabel>
      <skos:definition xml:lang="fr">Nom, autre que le nom réel ou officiel, sous lequel une collectivité en est venue à être connue.</skos:definition>
      <rdakit:toolkitDefinition xml:lang="fr">Nom, autre que le nom réel ou officiel, sous lequel une collectivité en est venue à être connue.</rdakit:toolkitDefinition>
      <skos:prefLabel xml:lang="es">nombre convencional</skos:prefLabel>
      <rdakit:toolkitLabel xml:lang="es">nombre convencional</rdakit:toolkitLabel>
      <skos:definition xml:lang="es">Nombre, diferente al nombre verdadero u oficial, mediante el cual llega a ser conocida una entidad corporativa, un lugar o un objeto.</skos:definition>
      <rdakit:toolkitDefinition xml:lang="es">Nombre, diferente al nombre verdadero u oficial, mediante el cual llega a ser conocida una entidad corporativa, un lugar o un objeto.</rdakit:toolkitDefinition>
      <skos:prefLabel xml:lang="de">Gebräuchlicher Name</skos:prefLabel>
      <rdakit:toolkitLabel xml:lang="de">Gebräuchlicher Name</rdakit:toolkitLabel>
      <skos:definition xml:lang="de">Ein anderer als der wirkliche oder offizielle Name, durch den eine Körperschaft bekannt geworden ist.</skos:definition>
      <rdakit:toolkitDefinition xml:lang="de">Ein anderer als der wirkliche oder offizielle Name, durch den eine Körperschaft bekannt geworden ist.</rdakit:toolkitDefinition>
      <skos:prefLabel xml:lang="fi">vakiintunut nimi</skos:prefLabel>
      <rdakit:toolkitLabel xml:lang="fi">vakiintunut nimi</rdakit:toolkitLabel>
      <skos:definition xml:lang="fi">Muu kuin todellinen tai virallinen nimi, jolla yhteisö yleisesti tunnetaan. A name, other than the real or official name, by which a corporate body has come to be known.</skos:definition>
      <rdakit:toolkitDefinition xml:lang="fi">Muu kuin todellinen tai virallinen nimi, jolla yhteisö yleisesti tunnetaan. A name, other than the real or official name, by which a corporate body has come to be known.</rdakit:toolkitDefinition>
      <skos:prefLabel xml:lang="da">konventionelt navn</skos:prefLabel>
      <rdakit:toolkitLabel xml:lang="da">konventionelt navn</rdakit:toolkitLabel>
      <skos:definition xml:lang="da">Navn, som en korporation er blevet kendt under, men som ikke er korporationens egentlige eller officielle navn.</skos:definition>
      <rdakit:toolkitDefinition xml:lang="da">Navn, som en korporation er blevet kendt under, men som ikke er korporationens egentlige eller officielle navn.</rdakit:toolkitDefinition>
      <skos:prefLabel xml:lang="ca">nom convencional</skos:prefLabel>
      <rdakit:toolkitLabel xml:lang="ca">nom convencional</rdakit:toolkitLabel>
      <skos:definition xml:lang="ca">Nom, diferent del nom real o de l’oficial, pel qual una entitat corporativa ha esdevingut coneguda.</skos:definition>
      <rdakit:toolkitDefinition xml:lang="ca">Nom, diferent del nom real o de l’oficial, pel qual una entitat corporativa ha esdevingut coneguda.</rdakit:toolkitDefinition>
      <skos:prefLabel xml:lang="vi">tên quy ước</skos:prefLabel>
      <rdakit:toolkitLabel xml:lang="vi">tên quy ước</rdakit:toolkitLabel>
      <skos:definition xml:lang="vi">Tên, khác với tên thật hoặc chính thức, mà một tập thể, địa điểm, hoặc sự vật được biết tới.</skos:definition>
      <rdakit:toolkitDefinition xml:lang="vi">Tên, khác với tên thật hoặc chính thức, mà một tập thể, địa điểm, hoặc sự vật được biết tới.</rdakit:toolkitDefinition>
      <skos:prefLabel xml:lang="no">konvensjonelt navn</skos:prefLabel>
      <rdakit:toolkitLabel xml:lang="no">konvensjonelt navn</rdakit:toolkitLabel>
      <skos:definition xml:lang="no">Et navn som ikke er det reelle eller offisielle, som en korporasjon er blitt alminnelig kjent under.</skos:definition>
      <rdakit:toolkitDefinition xml:lang="no">Et navn som ikke er det reelle eller offisielle, som en korporasjon er blitt alminnelig kjent under.</rdakit:toolkitDefinition>
    </skos:Concept>
<!-- Concept: core  -->
    <skos:Concept rdf:about="http://rdaregistry.info/termList/RDATerms/1029" xml:lang="en">
      <skos:inScheme rdf:resource="http://rdaregistry.info/termList/RDATerms"/>
      <reg:status rdf:resource="http://metadataregistry.org/uri/RegStatus/1001"/>
      <reg:identifier rdf:resource="http://metadataregistry.org/concepts/8544"/>
      <skos:prefLabel xml:lang="en">core</skos:prefLabel>
      <rdakit:toolkitLabel xml:lang="en">core</rdakit:toolkitLabel>
      <skos:definition xml:lang="en">An indication that an RDA element, element sub-type, or sub-element is required to support specified user tasks according to the FRBR assessment of the value of each attribute and relationship.</skos:definition>
      <rdakit:toolkitDefinition xml:lang="en">An indication that an RDA element, element sub-type, or sub-element is required to support specified user tasks according to the FRBR assessment of the value of each attribute and relationship.</rdakit:toolkitDefinition>
      <skos:prefLabel xml:lang="de">Kernelement</skos:prefLabel>
      <rdakit:toolkitLabel xml:lang="de">Kernelement</rdakit:toolkitLabel>
      <skos:definition xml:lang="de">Ein Hinweis darauf, dass ein RDA Element, ein Untertyp eines Elements oder ein Unterelement erforderlich ist, um spezifische Benutzeranforderungen zu unterstützen. Grundlage hierfür ist die FRBR-Einschätzung des Werts jedes Merkmals und jeder Beziehung.</skos:definition>
      <rdakit:toolkitDefinition xml:lang="de">Ein Hinweis darauf, dass ein RDA Element, ein Untertyp eines Elements oder ein Unterelement erforderlich ist, um spezifische Benutzeranforderungen zu unterstützen. Grundlage hierfür ist die FRBR-Einschätzung des Werts jedes Merkmals und jeder Beziehung.</rdakit:toolkitDefinition>
      <skos:prefLabel xml:lang="fi">ydin</skos:prefLabel>
      <rdakit:toolkitLabel xml:lang="fi">ydin</rdakit:toolkitLabel>
      <skos:definition xml:lang="fi">An indication that an RDA element, element sub-type, or sub-element is required to support specified user tasks according to the FRBR assessment of the value of each attribute and relationship.</skos:definition>
      <rdakit:toolkitDefinition xml:lang="fi">An indication that an RDA element, element sub-type, or sub-element is required to support specified user tasks according to the FRBR assessment of the value of each attribute and relationship.</rdakit:toolkitDefinition>
      <skos:prefLabel xml:lang="da">core</skos:prefLabel>
      <rdakit:toolkitLabel xml:lang="da">core</rdakit:toolkitLabel>
      <skos:definition xml:lang="da">Angivelse af, at et RDA-element, et undertype af et element eller et underelement heraf er påkrævet for at understøtte et specifikt brugerbehov i henhold til vurderingen i FRBR af værdien af de enkelte attributter og relationer.</skos:definition>
      <rdakit:toolkitDefinition xml:lang="da">Angivelse af, at et RDA-element, et undertype af et element eller et underelement heraf er påkrævet for at understøtte et specifikt brugerbehov i henhold til vurderingen i FRBR af værdien af de enkelte attributter og relationer.</rdakit:toolkitDefinition>
      <skos:prefLabel xml:lang="ca">bàsic</skos:prefLabel>
      <rdakit:toolkitLabel xml:lang="ca">bàsic</rdakit:toolkitLabel>
      <skos:definition xml:lang="ca">Indicació que un element RDA, un subtipus d'element o un subelement es requereix per donar suport específic a les tasques de l'usuari d’acord amb la valoració que els FRBR fan de cada atribut i relació.</skos:definition>
      <rdakit:toolkitDefinition xml:lang="ca">Indicació que un element RDA, un subtipus d'element o un subelement es requereix per donar suport específic a les tasques de l'usuari d’acord amb la valoració que els FRBR fan de cada atribut i relació.</rdakit:toolkitDefinition>
      <skos:prefLabel xml:lang="fr">fondamental</skos:prefLabel>
      <rdakit:toolkitLabel xml:lang="fr">fondamental</rdakit:toolkitLabel>
      <skos:definition xml:lang="fr">Mention indiquant qu’un élément, un sous-type d’élément ou un sous-élément RDA est requis dans l’accomplissement de tâches de l’utilisateur spécifiques en fonction du degré de pertinence que les FRBR accordent à chaque attribut et à chaque relation.</skos:definition>
      <rdakit:toolkitDefinition xml:lang="fr">Mention indiquant qu’un élément, un sous-type d’élément ou un sous-élément RDA est requis dans l’accomplissement de tâches de l’utilisateur spécifiques en fonction du degré de pertinence que les FRBR accordent à chaque attribut et à chaque relation.</rdakit:toolkitDefinition>
      <skos:prefLabel xml:lang="vi">cốt lõi</skos:prefLabel>
      <rdakit:toolkitLabel xml:lang="vi">cốt lõi</rdakit:toolkitLabel>
      <skos:definition xml:lang="vi">Dấu hiệu chỉ ra một yếu tố, tiểu loại yếu tố, hoặc tiểu yếu tố RDA được yêu cầu để hỗ trợ nhiệm vụ người dùng chuyên biệt theo đánh giá FRBR về giá trị của mỗi thuộc tính và mối quan hệ.</skos:definition>
      <rdakit:toolkitDefinition xml:lang="vi">Dấu hiệu chỉ ra một yếu tố, tiểu loại yếu tố, hoặc tiểu yếu tố RDA được yêu cầu để hỗ trợ nhiệm vụ người dùng chuyên biệt theo đánh giá FRBR về giá trị của mỗi thuộc tính và mối quan hệ.</rdakit:toolkitDefinition>
      <skos:prefLabel xml:lang="no">kjerne</skos:prefLabel>
      <rdakit:toolkitLabel xml:lang="no">kjerne</rdakit:toolkitLabel>
      <skos:definition xml:lang="no">En betegnelse som angir at et RDA-element, en undertype av element eller et underelement er nødvendig for å støtte bestemte brukeroppgaver i henhold til FRBR-vurderingen av verdien av hvert attributt og hver relasjon.</skos:definition>
      <rdakit:toolkitDefinition xml:lang="no">En betegnelse som angir at et RDA-element, en undertype av element eller et underelement er nødvendig for å støtte bestemte brukeroppgaver i henhold til FRBR-vurderingen av verdien av hvert attributt og hver relasjon.</rdakit:toolkitDefinition>
    </skos:Concept>
<!-- Concept: cover  -->
    <skos:Concept rdf:about="http://rdaregistry.info/termList/RDATerms/1030" xml:lang="en">
      <skos:inScheme rdf:resource="http://rdaregistry.info/termList/RDATerms"/>
      <reg:status rdf:resource="http://metadataregistry.org/uri/RegStatus/1001"/>
      <reg:identifier rdf:resource="http://metadataregistry.org/concepts/8545"/>
      <skos:prefLabel xml:lang="en">cover</skos:prefLabel>
      <rdakit:toolkitLabel xml:lang="en">cover</rdakit:toolkitLabel>
      <skos:definition xml:lang="en">An outer protective material attached to a volume, consisting of both sides of the front and back panels and the spine to which they are joined.</skos:definition>
      <rdakit:toolkitDefinition xml:lang="en">An outer protective material attached to a volume, consisting of both sides of the front and back panels and the spine to which they are joined.</rdakit:toolkitDefinition>
      <skos:prefLabel xml:lang="it">copertina</skos:prefLabel>
      <rdakit:toolkitLabel xml:lang="it">copertina</rdakit:toolkitLabel>
      <skos:definition xml:lang="it">Materiale protettivo esterno attaccato a un volume, che consiste di entrambi i lati delle coperture anteriore e posteriore e del dorso al quale esse sono unite.</skos:definition>
      <rdakit:toolkitDefinition xml:lang="it">Materiale protettivo esterno attaccato a un volume, che consiste di entrambi i lati delle coperture anteriore e posteriore e del dorso al quale esse sono unite.</rdakit:toolkitDefinition>
      <skos:prefLabel xml:lang="fr">couverture</skos:prefLabel>
      <rdakit:toolkitLabel xml:lang="fr">couverture</rdakit:toolkitLabel>
      <skos:definition xml:lang="fr">Matériau de protection externe fixé à un volume, constitué des deux faces des plats avant et arrière en plus du dos auquel ils sont liés.</skos:definition>
      <rdakit:toolkitDefinition xml:lang="fr">Matériau de protection externe fixé à un volume, constitué des deux faces des plats avant et arrière en plus du dos auquel ils sont liés.</rdakit:toolkitDefinition>
      <skos:prefLabel xml:lang="es">cubierta</skos:prefLabel>
      <rdakit:toolkitLabel xml:lang="es">cubierta</rdakit:toolkitLabel>
      <skos:definition xml:lang="es">Envoltura protectora de un volumen, que consiste en de una hoja que cubre la parte frontal, el lomo del volumen y la parte posterior.</skos:definition>
      <rdakit:toolkitDefinition xml:lang="es">Envoltura protectora de un volumen, que consiste en de una hoja que cubre la parte frontal, el lomo del volumen y la parte posterior.</rdakit:toolkitDefinition>
      <skos:prefLabel xml:lang="de">Einbanddecke</skos:prefLabel>
      <skos:altLabel xml:lang="de">Bucheinband</skos:altLabel>
      <rdakit:toolkitLabel xml:lang="de">Einbanddecke</rdakit:toolkitLabel>
      <skos:definition xml:lang="de">Ein äußeres Schutzmaterial, das einem Band beigefügt wird. Es besteht aus einem Vorder- und Hinterdeckel und ist durch einen Buchrücken verbunden.</skos:definition>
      <rdakit:toolkitDefinition xml:lang="de">Ein äußeres Schutzmaterial, das einem Band beigefügt wird. Es besteht aus einem Vorder- und Hinterdeckel und ist durch einen Buchrücken verbunden.</rdakit:toolkitDefinition>
      <skos:altLabel xml:lang="de">Buchdecke</skos:altLabel>
      <skos:altLabel xml:lang="de">Cover</skos:altLabel>
      <skos:prefLabel xml:lang="fi">kannet</skos:prefLabel>
      <rdakit:toolkitLabel xml:lang="fi">kannet</rdakit:toolkitLabel>
      <skos:definition xml:lang="fi">Nidokseen liitetty päällysmateriaali, joka muodostuu sekä etu- ja takakannesta että selkämyksestä joka liittää nämä yhteen.</skos:definition>
      <rdakit:toolkitDefinition xml:lang="fi">Nidokseen liitetty päällysmateriaali, joka muodostuu sekä etu- ja takakannesta että selkämyksestä joka liittää nämä yhteen.</rdakit:toolkitDefinition>
      <skos:prefLabel xml:lang="da">omslag</skos:prefLabel>
      <rdakit:toolkitLabel xml:lang="da">omslag</rdakit:toolkitLabel>
      <skos:definition xml:lang="da">Ydre beskyttende materiale, der omslutter et bind, og som består af forside, ryg og bagside.</skos:definition>
      <rdakit:toolkitDefinition xml:lang="da">Ydre beskyttende materiale, der omslutter et bind, og som består af forside, ryg og bagside.</rdakit:toolkitDefinition>
      <skos:prefLabel xml:lang="ca">coberta</skos:prefLabel>
      <rdakit:toolkitLabel xml:lang="ca">coberta</rdakit:toolkitLabel>
      <skos:definition xml:lang="ca">Material protector exterior lligat a un volum, que consisteix en les dues cares de les tapes anterior i posterior i el llom al qual van unides.</skos:definition>
      <rdakit:toolkitDefinition xml:lang="ca">Material protector exterior lligat a un volum, que consisteix en les dues cares de les tapes anterior i posterior i el llom al qual van unides.</rdakit:toolkitDefinition>
      <skos:prefLabel xml:lang="vi">bìa</skos:prefLabel>
      <rdakit:toolkitLabel xml:lang="vi">bìa</rdakit:toolkitLabel>
      <skos:definition xml:lang="vi">Vật liệu bao bọc bên ngoài gắn với tập, bao gồm cả mặt trước, mặt sau và gáy của tập đó.</skos:definition>
      <rdakit:toolkitDefinition xml:lang="vi">Vật liệu bao bọc bên ngoài gắn với tập, bao gồm cả mặt trước, mặt sau và gáy của tập đó.</rdakit:toolkitDefinition>
      <skos:prefLabel xml:lang="no">omslag</skos:prefLabel>
      <rdakit:toolkitLabel xml:lang="no">omslag</rdakit:toolkitLabel>
      <skos:definition xml:lang="no">Et ytre beskyttende materialet rundt et bind. Består av for- og bakside og ryggen som forener bindet.</skos:definition>
      <rdakit:toolkitDefinition xml:lang="no">Et ytre beskyttende materialet rundt et bind. Består av for- og bakside og ryggen som forener bindet.</rdakit:toolkitDefinition>
    </skos:Concept>
<!-- Concept: dataset  -->
    <skos:Concept rdf:about="http://rdaregistry.info/termList/RDATerms/1031" xml:lang="en">
      <skos:inScheme rdf:resource="http://rdaregistry.info/termList/RDATerms"/>
      <reg:status rdf:resource="http://metadataregistry.org/uri/RegStatus/1001"/>
      <reg:identifier rdf:resource="http://metadataregistry.org/concepts/8546"/>
      <skos:prefLabel xml:lang="en">dataset</skos:prefLabel>
      <rdakit:toolkitLabel xml:lang="en">dataset</rdakit:toolkitLabel>
      <skos:definition xml:lang="en">A collection of factual information presented in a structured form.</skos:definition>
      <rdakit:toolkitDefinition xml:lang="en">A collection of factual information presented in a structured form.</rdakit:toolkitDefinition>
      <skos:prefLabel xml:lang="it">dataset</skos:prefLabel>
      <rdakit:toolkitLabel xml:lang="it">dataset</rdakit:toolkitLabel>
      <skos:definition xml:lang="it">Informazione fattuale presentata in forma strutturata.</skos:definition>
      <rdakit:toolkitDefinition xml:lang="it">Informazione fattuale presentata in forma strutturata.</rdakit:toolkitDefinition>
      <skos:prefLabel xml:lang="fr">ensemble de données</skos:prefLabel>
      <rdakit:toolkitLabel xml:lang="fr">ensemble de données</rdakit:toolkitLabel>
      <skos:definition xml:lang="fr">Assemblage d’informations factuelles présentées sous une forme structurée.</skos:definition>
      <rdakit:toolkitDefinition xml:lang="fr">Assemblage d’informations factuelles présentées sous une forme structurée.</rdakit:toolkitDefinition>
      <skos:prefLabel xml:lang="de">Datensatz</skos:prefLabel>
      <rdakit:toolkitLabel xml:lang="de">Datensatz</rdakit:toolkitLabel>
      <skos:definition xml:lang="de">Eine Sammlung von Sachinformationen, die in einer strukturierten Form präsentiert werden.</skos:definition>
      <rdakit:toolkitDefinition xml:lang="de">Eine Sammlung von Sachinformationen, die in einer strukturierten Form präsentiert werden.</rdakit:toolkitDefinition>
      <skos:prefLabel xml:lang="fi">tietoaineisto</skos:prefLabel>
      <rdakit:toolkitLabel xml:lang="fi">tietoaineisto</rdakit:toolkitLabel>
      <skos:definition xml:lang="fi">Strukturoidussa muodossa esitetty tietosisältö.</skos:definition>
      <rdakit:toolkitDefinition xml:lang="fi">Strukturoidussa muodossa esitetty tietosisältö.</rdakit:toolkitDefinition>
      <skos:prefLabel xml:lang="da">datasæt</skos:prefLabel>
      <rdakit:toolkitLabel xml:lang="da">datasæt</rdakit:toolkitLabel>
      <skos:definition xml:lang="da">Samling af faktuelle oplysninger præsenteret i struktureret form.</skos:definition>
      <rdakit:toolkitDefinition xml:lang="da">Samling af faktuelle oplysninger præsenteret i struktureret form.</rdakit:toolkitDefinition>
      <skos:prefLabel xml:lang="ca">conjunt de dades</skos:prefLabel>
      <rdakit:toolkitLabel xml:lang="ca">conjunt de dades</rdakit:toolkitLabel>
      <skos:definition xml:lang="ca">Col·lecció d'informació factual presentada de forma estructurada.</skos:definition>
      <rdakit:toolkitDefinition xml:lang="ca">Col·lecció d'informació factual presentada de forma estructurada.</rdakit:toolkitDefinition>
      <skos:prefLabel xml:lang="vi">bộ dữ liệu</skos:prefLabel>
      <rdakit:toolkitLabel xml:lang="vi">bộ dữ liệu</rdakit:toolkitLabel>
      <skos:definition xml:lang="vi">Sưu tập thông tin thực tế được trình bày dưới một hình thái có cấu trúc.</skos:definition>
      <rdakit:toolkitDefinition xml:lang="vi">Sưu tập thông tin thực tế được trình bày dưới một hình thái có cấu trúc.</rdakit:toolkitDefinition>
      <skos:prefLabel xml:lang="no">datasett</skos:prefLabel>
      <rdakit:toolkitLabel xml:lang="no">datasett</rdakit:toolkitLabel>
      <skos:definition xml:lang="no">En samling med faktainformasjon presentert i en strukturert form.</skos:definition>
      <rdakit:toolkitDefinition xml:lang="no">En samling med faktainformasjon presentert i en strukturert form.</rdakit:toolkitDefinition>
    </skos:Concept>
<!-- Concept: date of a treaty  -->
    <skos:Concept rdf:about="http://rdaregistry.info/termList/RDATerms/1032" xml:lang="en">
      <skos:inScheme rdf:resource="http://rdaregistry.info/termList/RDATerms"/>
      <reg:status rdf:resource="http://metadataregistry.org/uri/RegStatus/1001"/>
      <reg:identifier rdf:resource="http://metadataregistry.org/concepts/8547"/>
      <skos:prefLabel xml:lang="en">date of a treaty</skos:prefLabel>
      <rdakit:toolkitLabel xml:lang="en">date of a treaty</rdakit:toolkitLabel>
      <skos:definition xml:lang="en">An earliest date a treaty or a protocol to a treaty was adopted by an international intergovernmental body or by an international conference, was opened for signing, was formally signed, was ratified, was proclaimed, etc.</skos:definition>
      <rdakit:toolkitDefinition xml:lang="en">An earliest date a treaty or a protocol to a treaty was adopted by an international intergovernmental body or by an international conference, was opened for signing, was formally signed, was ratified, was proclaimed, etc.</rdakit:toolkitDefinition>
      <skos:prefLabel xml:lang="it">data di un trattato</skos:prefLabel>
      <rdakit:toolkitLabel xml:lang="it">data di un trattato</rdakit:toolkitLabel>
      <skos:definition xml:lang="it">La prima data in cui un trattato o il protocollo di un trattato è stato adottato da un ente intergovernativo internazionale o da una conferenza internazionale, è stato aperto alla firma, ratificato, proclamato, etc.</skos:definition>
      <rdakit:toolkitDefinition xml:lang="it">La prima data in cui un trattato o il protocollo di un trattato è stato adottato da un ente intergovernativo internazionale o da una conferenza internazionale, è stato aperto alla firma, ratificato, proclamato, etc.</rdakit:toolkitDefinition>
      <skos:prefLabel xml:lang="fr">date d’un traité</skos:prefLabel>
      <rdakit:toolkitLabel xml:lang="fr">date d’un traité</rdakit:toolkitLabel>
      <skos:definition xml:lang="fr">Date la plus ancienne où un traité ou un protocole d’un traité a été adopté par une organisation internationale intergouvernementale ou par une conférence internationale, a été ouvert à la signature, a été signé officiellement, a été ratifié, a été proclamé, etc.</skos:definition>
      <rdakit:toolkitDefinition xml:lang="fr">Date la plus ancienne où un traité ou un protocole d’un traité a été adopté par une organisation internationale intergouvernementale ou par une conférence internationale, a été ouvert à la signature, a été signé officiellement, a été ratifié, a été proclamé, etc.</rdakit:toolkitDefinition>
      <skos:prefLabel xml:lang="de">Datum eines Abkommens</skos:prefLabel>
      <rdakit:toolkitLabel xml:lang="de">Datum eines Abkommens</rdakit:toolkitLabel>
      <skos:definition xml:lang="de">Das früheste Datum, an dem ein Abkommen oder ein Protokoll zu einem Abkommen von einer internationalen, zwischenstaatlichen Körperschaft oder einer internationalen Konferenz für die Unterzeichnung geöffnet, förmlich unterzeichnet, ratifiziert, öffentlich bekanntgegeben usw. wurde.</skos:definition>
      <rdakit:toolkitDefinition xml:lang="de">Das früheste Datum, an dem ein Abkommen oder ein Protokoll zu einem Abkommen von einer internationalen, zwischenstaatlichen Körperschaft oder einer internationalen Konferenz für die Unterzeichnung geöffnet, förmlich unterzeichnet, ratifiziert, öffentlich bekanntgegeben usw. wurde.</rdakit:toolkitDefinition>
      <skos:prefLabel xml:lang="fi">valtiosopimuksen ajankohta</skos:prefLabel>
      <rdakit:toolkitLabel xml:lang="fi">valtiosopimuksen ajankohta</rdakit:toolkitLabel>
      <skos:definition xml:lang="fi">Varhaisin ajankohta jolloin valtiosopimus tai siihen liittyvä pöytäkirja on kansainvälisen hallitusten välisen yhteisön toimesta hyväksytty, virallisesti allekirjoitettu, ratifioitu jne.</skos:definition>
      <rdakit:toolkitDefinition xml:lang="fi">Varhaisin ajankohta jolloin valtiosopimus tai siihen liittyvä pöytäkirja on kansainvälisen hallitusten välisen yhteisön toimesta hyväksytty, virallisesti allekirjoitettu, ratifioitu jne.</rdakit:toolkitDefinition>
      <skos:prefLabel xml:lang="da">traktatdato</skos:prefLabel>
      <rdakit:toolkitLabel xml:lang="da">traktatdato</rdakit:toolkitLabel>
      <skos:definition xml:lang="da">Den tidligste dato, en traktat eller traktatprotokol blev vedtaget af en international mellemstatslig instans eller en international konference, blev åbnet for underskrivelse, formelt blev underskrevet, blev ratificeret, blev bekendtgjort etc.</skos:definition>
      <rdakit:toolkitDefinition xml:lang="da">Den tidligste dato, en traktat eller traktatprotokol blev vedtaget af en international mellemstatslig instans eller en international konference, blev åbnet for underskrivelse, formelt blev underskrevet, blev ratificeret, blev bekendtgjort etc.</rdakit:toolkitDefinition>
      <skos:prefLabel xml:lang="ca">data d’un tractat</skos:prefLabel>
      <rdakit:toolkitLabel xml:lang="ca">data d’un tractat</rdakit:toolkitLabel>
      <skos:definition xml:lang="ca">Data més antiga en què un tractat o un protocol d’un tractat ha estat adoptat per una organització internacional intergovernamental, o per una conferència internacional, s’ha presentat per a la signatura, s’ha signat formalment, ha estat ratificat, proclamat, etc.</skos:definition>
      <rdakit:toolkitDefinition xml:lang="ca">Data més antiga en què un tractat o un protocol d’un tractat ha estat adoptat per una organització internacional intergovernamental, o per una conferència internacional, s’ha presentat per a la signatura, s’ha signat formalment, ha estat ratificat, proclamat, etc.</rdakit:toolkitDefinition>
      <skos:prefLabel xml:lang="vi">ngày của hiệp ước</skos:prefLabel>
      <rdakit:toolkitLabel xml:lang="vi">ngày của hiệp ước</rdakit:toolkitLabel>
      <skos:definition xml:lang="vi">Ngày sớm nhất của hiệp ước hoặc nghị định thư của hiệp ước được thông qua bởi một tổ chức liên chính phủ quốc tế hoặc bởi một hội nghị quốc tế, được mở để ký, được ký chính thức, được phê chuẩn, được công bố, v.v...</skos:definition>
      <rdakit:toolkitDefinition xml:lang="vi">Ngày sớm nhất của hiệp ước hoặc nghị định thư của hiệp ước được thông qua bởi một tổ chức liên chính phủ quốc tế hoặc bởi một hội nghị quốc tế, được mở để ký, được ký chính thức, được phê chuẩn, được công bố, v.v...</rdakit:toolkitDefinition>
      <skos:prefLabel xml:lang="no">tidspunkt for traktat</skos:prefLabel>
      <rdakit:toolkitLabel xml:lang="no">tidspunkt for traktat</rdakit:toolkitLabel>
      <skos:definition xml:lang="no">Det tidligste tidspunkt for når en traktat eller en protokoll ble antatt av en internasjonal mellomstatlig organisasjon eller av en internasjonal konferanse, ble lagt fram for signering, ble formelt undertegnet, ble ratifisert, ble proklamert, etc.</skos:definition>
      <rdakit:toolkitDefinition xml:lang="no">Det tidligste tidspunkt for når en traktat eller en protokoll ble antatt av en internasjonal mellomstatlig organisasjon eller av en internasjonal konferanse, ble lagt fram for signering, ble formelt undertegnet, ble ratifisert, ble proklamert, etc.</rdakit:toolkitDefinition>
    </skos:Concept>
<!-- Concept: date of promulgation of a law, etc.  -->
    <skos:Concept rdf:about="http://rdaregistry.info/termList/RDATerms/1033" xml:lang="en">
      <skos:inScheme rdf:resource="http://rdaregistry.info/termList/RDATerms"/>
      <reg:status rdf:resource="http://metadataregistry.org/uri/RegStatus/1001"/>
      <reg:identifier rdf:resource="http://metadataregistry.org/concepts/8548"/>
      <skos:prefLabel xml:lang="en">date of promulgation of a law, etc.</skos:prefLabel>
      <rdakit:toolkitLabel xml:lang="en">date of promulgation of a law, etc.</rdakit:toolkitLabel>
      <skos:definition xml:lang="en">A year a law, etc., was promulgated or brought into force.</skos:definition>
      <rdakit:toolkitDefinition xml:lang="en">A year a law, etc., was promulgated or brought into force.</rdakit:toolkitDefinition>
      <skos:prefLabel xml:lang="it">data di promulgazione di una legge</skos:prefLabel>
      <rdakit:toolkitLabel xml:lang="it">data di promulgazione di una legge</rdakit:toolkitLabel>
      <skos:definition xml:lang="it">Anno in cui una legge è stata promulgata o è entrata in vigore.</skos:definition>
      <rdakit:toolkitDefinition xml:lang="it">Anno in cui una legge è stata promulgata o è entrata in vigore.</rdakit:toolkitDefinition>
      <skos:prefLabel xml:lang="fr">date de promulgation d’une loi, etc.</skos:prefLabel>
      <rdakit:toolkitLabel xml:lang="fr">date de promulgation d’une loi, etc.</rdakit:toolkitLabel>
      <skos:definition xml:lang="fr">Année où une loi, etc. a été promulguée ou est entrée en vigueur.</skos:definition>
      <rdakit:toolkitDefinition xml:lang="fr">Année où une loi, etc. a été promulguée ou est entrée en vigueur.</rdakit:toolkitDefinition>
      <skos:prefLabel xml:lang="de">Verkündungsdatum eines Gesetzes usw.</skos:prefLabel>
      <rdakit:toolkitLabel xml:lang="de">Verkündungsdatum eines Gesetzes usw.</rdakit:toolkitLabel>
      <skos:definition xml:lang="de">Ein Jahr, in dem ein Gesetz usw. verkündet oder in Kraft gesetzt wurde.</skos:definition>
      <rdakit:toolkitDefinition xml:lang="de">Ein Jahr, in dem ein Gesetz usw. verkündet oder in Kraft gesetzt wurde.</rdakit:toolkitDefinition>
      <skos:prefLabel xml:lang="fi">lain jne. voimaantulon ajankohta</skos:prefLabel>
      <rdakit:toolkitLabel xml:lang="fi">lain jne. voimaantulon ajankohta</rdakit:toolkitLabel>
      <skos:definition xml:lang="fi">Vuosi jolloin laki jne. hyväksyttiin tai se astui voimaan.</skos:definition>
      <rdakit:toolkitDefinition xml:lang="fi">Vuosi jolloin laki jne. hyväksyttiin tai se astui voimaan.</rdakit:toolkitDefinition>
      <skos:prefLabel xml:lang="da">år for kundgørelse af lov etc.</skos:prefLabel>
      <rdakit:toolkitLabel xml:lang="da">år for kundgørelse af lov etc.</rdakit:toolkitLabel>
      <skos:definition xml:lang="da">År eller dato, hvor en lov etc. blev bekendtgjort eller trådte i kraft.</skos:definition>
      <rdakit:toolkitDefinition xml:lang="da">År eller dato, hvor en lov etc. blev bekendtgjort eller trådte i kraft.</rdakit:toolkitDefinition>
      <skos:prefLabel xml:lang="ca">data de promulgació d’una llei, etc.</skos:prefLabel>
      <rdakit:toolkitLabel xml:lang="ca">data de promulgació d’una llei, etc.</rdakit:toolkitLabel>
      <skos:definition xml:lang="ca">Any en què una llei, etc., s’ha promulgat o ha entrat en vigor.</skos:definition>
      <rdakit:toolkitDefinition xml:lang="ca">Any en què una llei, etc., s’ha promulgat o ha entrat en vigor.</rdakit:toolkitDefinition>
      <skos:prefLabel xml:lang="vi">ngày ban hành luật, v.v...</skos:prefLabel>
      <rdakit:toolkitLabel xml:lang="vi">ngày ban hành luật, v.v...</rdakit:toolkitLabel>
      <skos:definition xml:lang="vi">Năm một luật, v.v... được ban hành hoặc có hiệu lực.</skos:definition>
      <rdakit:toolkitDefinition xml:lang="vi">Năm một luật, v.v... được ban hành hoặc có hiệu lực.</rdakit:toolkitDefinition>
      <skos:prefLabel xml:lang="no">tidspunkt for kunngjøring av en lov etc.</skos:prefLabel>
      <rdakit:toolkitLabel xml:lang="no">tidspunkt for kunngjøring av en lov etc.</rdakit:toolkitLabel>
      <skos:definition xml:lang="no">Et tidspunkt da en lov etc. ble kunngjort eller trådte i kraft.</skos:definition>
      <rdakit:toolkitDefinition xml:lang="no">Et tidspunkt da en lov etc. ble kunngjort eller trådte i kraft.</rdakit:toolkitDefinition>
    </skos:Concept>
<!-- Concept: description  -->
    <skos:Concept rdf:about="http://rdaregistry.info/termList/RDATerms/1035" xml:lang="en">
      <skos:inScheme rdf:resource="http://rdaregistry.info/termList/RDATerms"/>
      <reg:status rdf:resource="http://metadataregistry.org/uri/RegStatus/1001"/>
      <reg:identifier rdf:resource="http://metadataregistry.org/concepts/8550"/>
      <skos:prefLabel xml:lang="en">description</skos:prefLabel>
      <rdakit:toolkitLabel xml:lang="en">description</rdakit:toolkitLabel>
      <skos:definition xml:lang="en">A set of data recording and identifying an entity.</skos:definition>
      <rdakit:toolkitDefinition xml:lang="en">A set of data recording and identifying an entity.</rdakit:toolkitDefinition>
      <skos:prefLabel xml:lang="it">descrizione</skos:prefLabel>
      <rdakit:toolkitLabel xml:lang="it">descrizione</rdakit:toolkitLabel>
      <skos:definition xml:lang="it">Insieme di dati che registrano e identificano un'entità.</skos:definition>
      <rdakit:toolkitDefinition xml:lang="it">Insieme di dati che registrano e identificano un'entità.</rdakit:toolkitDefinition>
      <skos:prefLabel xml:lang="fr">description</skos:prefLabel>
      <rdakit:toolkitLabel xml:lang="fr">description</rdakit:toolkitLabel>
      <skos:definition xml:lang="fr">Ensemble de données enregistrant et identifiant une entité.</skos:definition>
      <rdakit:toolkitDefinition xml:lang="fr">Ensemble de données enregistrant et identifiant une entité.</rdakit:toolkitDefinition>
      <skos:prefLabel xml:lang="es">descripción</skos:prefLabel>
      <rdakit:toolkitLabel xml:lang="es">descripción</rdakit:toolkitLabel>
      <skos:definition xml:lang="es">Conjunto de datos que registran e identifican a una entidad.</skos:definition>
      <rdakit:toolkitDefinition xml:lang="es">Conjunto de datos que registran e identifican a una entidad.</rdakit:toolkitDefinition>
      <skos:prefLabel xml:lang="de">Beschreibung</skos:prefLabel>
      <rdakit:toolkitLabel xml:lang="de">Beschreibung</rdakit:toolkitLabel>
      <skos:definition xml:lang="de">Ein Satz von Daten, der eine Entität erfasst und identifiziert.</skos:definition>
      <rdakit:toolkitDefinition xml:lang="de">Ein Satz von Daten, der eine Entität erfasst und identifiziert.</rdakit:toolkitDefinition>
      <skos:prefLabel xml:lang="fi">kuvailu</skos:prefLabel>
      <rdakit:toolkitLabel xml:lang="fi">kuvailu</rdakit:toolkitLabel>
      <skos:definition xml:lang="fi">Tietoaineisto, joka rekisteröi ja identifioi entiteetin.</skos:definition>
      <rdakit:toolkitDefinition xml:lang="fi">Tietoaineisto, joka rekisteröi ja identifioi entiteetin.</rdakit:toolkitDefinition>
      <skos:prefLabel xml:lang="da">beskrivelse</skos:prefLabel>
      <rdakit:toolkitLabel xml:lang="da">beskrivelse</rdakit:toolkitLabel>
      <skos:definition xml:lang="da">Sæt af oplysninger, der beskriver og identificerer en entitet.</skos:definition>
      <rdakit:toolkitDefinition xml:lang="da">Sæt af oplysninger, der beskriver og identificerer en entitet.</rdakit:toolkitDefinition>
      <skos:prefLabel xml:lang="ca">descripció</skos:prefLabel>
      <rdakit:toolkitLabel xml:lang="ca">descripció</rdakit:toolkitLabel>
      <skos:definition xml:lang="ca">Conjunt de dades que enregistren i identifiquen una entitat.</skos:definition>
      <rdakit:toolkitDefinition xml:lang="ca">Conjunt de dades que enregistren i identifiquen una entitat.</rdakit:toolkitDefinition>
      <skos:prefLabel xml:lang="vi">mô tả</skos:prefLabel>
      <rdakit:toolkitLabel xml:lang="vi">mô tả</rdakit:toolkitLabel>
      <skos:definition xml:lang="vi">Tập hợp dữ liệu ghi và nhận dạng một thực thể.</skos:definition>
      <rdakit:toolkitDefinition xml:lang="vi">Tập hợp dữ liệu ghi và nhận dạng một thực thể.</rdakit:toolkitDefinition>
      <skos:prefLabel xml:lang="no">beskrivelse</skos:prefLabel>
      <rdakit:toolkitLabel xml:lang="no">beskrivelse</rdakit:toolkitLabel>
      <skos:definition xml:lang="no">Et sett med data som gjengir og identifiserer en entitet.</skos:definition>
      <rdakit:toolkitDefinition xml:lang="no">Et sett med data som gjengir og identifiserer en entitet.</rdakit:toolkitDefinition>
    </skos:Concept>
<!-- Concept: designation  -->
    <skos:Concept rdf:about="http://rdaregistry.info/termList/RDATerms/1034" xml:lang="en">
      <skos:inScheme rdf:resource="http://rdaregistry.info/termList/RDATerms"/>
      <reg:status rdf:resource="http://metadataregistry.org/uri/RegStatus/1001"/>
      <reg:identifier rdf:resource="http://metadataregistry.org/concepts/8549"/>
      <skos:prefLabel xml:lang="en">designation</skos:prefLabel>
      <rdakit:toolkitLabel xml:lang="en">designation</rdakit:toolkitLabel>
      <skos:definition xml:lang="en">A word or phrase that describes an aspect of an entity.</skos:definition>
      <rdakit:toolkitDefinition xml:lang="en">A word or phrase that describes an aspect of an entity.</rdakit:toolkitDefinition>
      <skos:prefLabel xml:lang="de">Bezeichnung</skos:prefLabel>
      <rdakit:toolkitLabel xml:lang="de">Bezeichnung</rdakit:toolkitLabel>
      <skos:definition xml:lang="de">Ein Wort oder eine Phrase, die einen Aspekt einer Entität beschreibt.</skos:definition>
      <rdakit:toolkitDefinition xml:lang="de">Ein Wort oder eine Phrase, die einen Aspekt einer Entität beschreibt.</rdakit:toolkitDefinition>
      <skos:prefLabel xml:lang="fi">määrite</skos:prefLabel>
      <rdakit:toolkitLabel xml:lang="fi">määrite</rdakit:toolkitLabel>
      <skos:definition xml:lang="fi">Sana tai lause, joka kuvaa kokonaisuuden osaa.</skos:definition>
      <rdakit:toolkitDefinition xml:lang="fi">Sana tai lause, joka kuvaa kokonaisuuden osaa.</rdakit:toolkitDefinition>
      <skos:prefLabel xml:lang="da">betegnelse</skos:prefLabel>
      <rdakit:toolkitLabel xml:lang="da">betegnelse</rdakit:toolkitLabel>
      <skos:definition xml:lang="da">Ord eller frase der beskriver et aspekt af en entitet.</skos:definition>
      <rdakit:toolkitDefinition xml:lang="da">Ord eller frase der beskriver et aspekt af en entitet.</rdakit:toolkitDefinition>
      <skos:prefLabel xml:lang="ca">designació</skos:prefLabel>
      <rdakit:toolkitLabel xml:lang="ca">designació</rdakit:toolkitLabel>
      <skos:definition xml:lang="ca">Paraula o frase que descriu un aspecte d'una entitat.</skos:definition>
      <rdakit:toolkitDefinition xml:lang="ca">Paraula o frase que descriu un aspecte d'una entitat.</rdakit:toolkitDefinition>
      <skos:prefLabel xml:lang="fr">désignation</skos:prefLabel>
      <rdakit:toolkitLabel xml:lang="fr">désignation</rdakit:toolkitLabel>
      <skos:definition xml:lang="fr">Mot ou expression qui décrit un aspect d’une entitié.</skos:definition>
      <rdakit:toolkitDefinition xml:lang="fr">Mot ou expression qui décrit un aspect d’une entitié.</rdakit:toolkitDefinition>
      <skos:prefLabel xml:lang="vi">định danh</skos:prefLabel>
      <rdakit:toolkitLabel xml:lang="vi">định danh</rdakit:toolkitLabel>
      <skos:definition xml:lang="vi">Từ hoặc cụm từ mô tả một khía cạnh của thực thể.</skos:definition>
      <rdakit:toolkitDefinition xml:lang="vi">Từ hoặc cụm từ mô tả một khía cạnh của thực thể.</rdakit:toolkitDefinition>
      <skos:prefLabel xml:lang="no">betegnelse</skos:prefLabel>
      <rdakit:toolkitLabel xml:lang="no">betegnelse</rdakit:toolkitLabel>
      <skos:definition xml:lang="no">Et ord eller uttrykk som beskriver et aspekt ved en entitet.</skos:definition>
      <rdakit:toolkitDefinition xml:lang="no">Et ord eller uttrykk som beskriver et aspekt ved en entitet.</rdakit:toolkitDefinition>
    </skos:Concept>
<!-- Concept: devised title  -->
    <skos:Concept rdf:about="http://rdaregistry.info/termList/RDATerms/1036" xml:lang="en">
      <skos:inScheme rdf:resource="http://rdaregistry.info/termList/RDATerms"/>
      <reg:status rdf:resource="http://metadataregistry.org/uri/RegStatus/1001"/>
      <reg:identifier rdf:resource="http://metadataregistry.org/concepts/8551"/>
      <skos:prefLabel xml:lang="en">devised title</skos:prefLabel>
      <rdakit:toolkitLabel xml:lang="en">devised title</rdakit:toolkitLabel>
      <skos:definition xml:lang="en">A title proper created by an agency preparing a description of a manifestation that bears no title itself and has no title associated with it that can be found in accompanying material, a published description of the manifestation, a reference source, etc.</skos:definition>
      <rdakit:toolkitDefinition xml:lang="en">A title proper created by an agency preparing a description of a manifestation that bears no title itself and has no title associated with it that can be found in accompanying material, a published description of the manifestation, a reference source, etc.</rdakit:toolkitDefinition>
      <skos:prefLabel xml:lang="it">titolo escogitato</skos:prefLabel>
      <rdakit:toolkitLabel xml:lang="it">titolo escogitato</rdakit:toolkitLabel>
      <skos:definition xml:lang="it">Titolo proprio creato da un'agenzia che redige una descrizione di una risorsa che non reca alcun titolo e non ha un titolo associato reperibile in altre fonti.</skos:definition>
      <rdakit:toolkitDefinition xml:lang="it">Titolo proprio creato da un'agenzia che redige una descrizione di una risorsa che non reca alcun titolo e non ha un titolo associato reperibile in altre fonti.</rdakit:toolkitDefinition>
      <skos:prefLabel xml:lang="fr">titre forgé</skos:prefLabel>
      <rdakit:toolkitLabel xml:lang="fr">titre forgé</rdakit:toolkitLabel>
      <skos:definition xml:lang="fr">Titre propre créé par une agence préparant une description d’une manifestation qui ne porte par elle-même aucun titre et n’a pas de titre qu’il soit possible de trouver à lui associer dans le matériel d’accompagnement, une description publiée de la manifestation, une source de référence, etc.</skos:definition>
      <rdakit:toolkitDefinition xml:lang="fr">Titre propre créé par une agence préparant une description d’une manifestation qui ne porte par elle-même aucun titre et n’a pas de titre qu’il soit possible de trouver à lui associer dans le matériel d’accompagnement, une description publiée de la manifestation, une source de référence, etc.</rdakit:toolkitDefinition>
      <skos:prefLabel xml:lang="de">Fingierter Titel</skos:prefLabel>
      <rdakit:toolkitLabel xml:lang="de">Fingierter Titel</rdakit:toolkitLabel>
      <skos:definition xml:lang="de">Ein Haupttitel, der von einer Agentur erzeugt wurde, die die Beschreibung für einer Manifestation erstellt, die selbst keinen Titel hat und die mit keinem Titel in Verbindung steht, der in anderen Quellen (z. B. Begleitmaterial, einer veröffentlichten Beschreibung der Manifestation oder einem Nachschlagewerk) gefunden werden kann.</skos:definition>
      <rdakit:toolkitDefinition xml:lang="de">Ein Haupttitel, der von einer Agentur erzeugt wurde, die die Beschreibung für einer Manifestation erstellt, die selbst keinen Titel hat und die mit keinem Titel in Verbindung steht, der in anderen Quellen (z. B. Begleitmaterial, einer veröffentlichten Beschreibung der Manifestation oder einem Nachschlagewerk) gefunden werden kann.</rdakit:toolkitDefinition>
      <skos:prefLabel xml:lang="fi">sepitetty nimeke</skos:prefLabel>
      <rdakit:toolkitLabel xml:lang="fi">sepitetty nimeke</rdakit:toolkitLabel>
      <skos:definition xml:lang="fi">Kuvailevan yhteisön muodostama nimeke silloin kun manifestaatiossa ei ole nimekettä, eikä sellaista voida löytää muista lähteistä kuten liiteaineistosta, aineiston julkaistusta kuvailusta tai tietolähteistä.</skos:definition>
      <rdakit:toolkitDefinition xml:lang="fi">Kuvailevan yhteisön muodostama nimeke silloin kun manifestaatiossa ei ole nimekettä, eikä sellaista voida löytää muista lähteistä kuten liiteaineistosta, aineiston julkaistusta kuvailusta tai tietolähteistä.</rdakit:toolkitDefinition>
      <skos:prefLabel xml:lang="da">konstrueret titel</skos:prefLabel>
      <rdakit:toolkitLabel xml:lang="da">konstrueret titel</rdakit:toolkitLabel>
      <skos:definition xml:lang="da">Hovedtitel skabt af en institution, der udformer beskrivelsen af en manifestation uden titel, og for hvilken der ikke kan findes en titel i ledsagende materiale; en offentliggjort beskrivelse af manifestationen; en henvisningskilde etc.</skos:definition>
      <rdakit:toolkitDefinition xml:lang="da">Hovedtitel skabt af en institution, der udformer beskrivelsen af en manifestation uden titel, og for hvilken der ikke kan findes en titel i ledsagende materiale; en offentliggjort beskrivelse af manifestationen; en henvisningskilde etc.</rdakit:toolkitDefinition>
      <skos:prefLabel xml:lang="ca">títol inventat</skos:prefLabel>
      <rdakit:toolkitLabel xml:lang="ca">títol inventat</rdakit:toolkitLabel>
      <skos:definition xml:lang="ca">Títol propi creat per una agència que prepara una descripció d’una manifestació que no porta títol i que tampoc no té un títol associat que es pugui trobar en el material d’acompanyament, en una descripció publicada de la manifestació, en una font de referència, etc.</skos:definition>
      <rdakit:toolkitDefinition xml:lang="ca">Títol propi creat per una agència que prepara una descripció d’una manifestació que no porta títol i que tampoc no té un títol associat que es pugui trobar en el material d’acompanyament, en una descripció publicada de la manifestació, en una font de referència, etc.</rdakit:toolkitDefinition>
      <skos:altLabel xml:lang="fr">titre factice</skos:altLabel>
      <skos:prefLabel xml:lang="vi">nhan đề tự đặt</skos:prefLabel>
      <rdakit:toolkitLabel xml:lang="vi">nhan đề tự đặt</rdakit:toolkitLabel>
      <skos:definition xml:lang="vi">Nhan đề hợp thức do một tác nhân tạo ra để mô tả một biểu hiện không có nhan đề và không có nhan đề liên quan với nó có thể tìm thấy trong tài liệu kèm theo, mô tả xuất bản của tài nguyên đó, nguồn tham khảo, v.v...</skos:definition>
      <rdakit:toolkitDefinition xml:lang="vi">Nhan đề hợp thức do một tác nhân tạo ra để mô tả một biểu hiện không có nhan đề và không có nhan đề liên quan với nó có thể tìm thấy trong tài liệu kèm theo, mô tả xuất bản của tài nguyên đó, nguồn tham khảo, v.v...</rdakit:toolkitDefinition>
      <skos:prefLabel xml:lang="no">tilføyd tittel</skos:prefLabel>
      <rdakit:toolkitLabel xml:lang="no">tilføyd tittel</rdakit:toolkitLabel>
      <skos:definition xml:lang="no">En hovedtittel utformet av institusjonen som registrerer en beskrivelse av en manifestasjon som er uten tittel i seg selv og som ikke kan knyttes til en tittel som finnes i andre kilder som medfølgende materiale, en utgitt beskrivelse av manifestasjonen, et referanseverk, etc.</skos:definition>
      <rdakit:toolkitDefinition xml:lang="no">En hovedtittel utformet av institusjonen som registrerer en beskrivelse av en manifestasjon som er uten tittel i seg selv og som ikke kan knyttes til en tittel som finnes i andre kilder som medfølgende materiale, en utgitt beskrivelse av manifestasjonen, et referanseverk, etc.</rdakit:toolkitDefinition>
    </skos:Concept>
<!-- Concept: digital resource  -->
    <skos:Concept rdf:about="http://rdaregistry.info/termList/RDATerms/1037" xml:lang="en">
      <skos:inScheme rdf:resource="http://rdaregistry.info/termList/RDATerms"/>
      <reg:status rdf:resource="http://metadataregistry.org/uri/RegStatus/1001"/>
      <reg:identifier rdf:resource="http://metadataregistry.org/concepts/8552"/>
      <skos:prefLabel xml:lang="en">digital resource</skos:prefLabel>
      <rdakit:toolkitLabel xml:lang="en">digital resource</rdakit:toolkitLabel>
      <skos:definition xml:lang="en">A resource, consisting of data and/or one or more programs, encoded for manipulation by a computerized device.</skos:definition>
      <rdakit:toolkitDefinition xml:lang="en">A resource, consisting of data and/or one or more programs, encoded for manipulation by a computerized device.</rdakit:toolkitDefinition>
      <skos:scopeNote xml:lang="en">The resource may require the use of a peripheral device directly connected to a computerized device, an application program, and/or a connection to a computer network.</skos:scopeNote>
      <skos:prefLabel xml:lang="it">risorsa digitale</skos:prefLabel>
      <rdakit:toolkitLabel xml:lang="it">risorsa digitale</rdakit:toolkitLabel>
      <skos:definition xml:lang="it">Risorsa (dati e/o programmi) codificata per la manipolazione mediante un dispositivo computerizzato.</skos:definition>
      <rdakit:toolkitDefinition xml:lang="it">Risorsa (dati e/o programmi) codificata per la manipolazione mediante un dispositivo computerizzato.</rdakit:toolkitDefinition>
      <skos:scopeNote xml:lang="it">La risorsa può richiedere una periferica direttamente connessa al dispositivo computerizzato (per esempio, un lettore CD-ROM), un'applicazione (per esempio, un programma di riproduzione, di visualizzazione di immagini) e/o la connessione a una rete di computer (per esempio, internet).</skos:scopeNote>
      <skos:prefLabel xml:lang="fr">ressource numérique</skos:prefLabel>
      <rdakit:toolkitLabel xml:lang="fr">ressource numérique</rdakit:toolkitLabel>
      <skos:definition xml:lang="fr">Ressource qui consiste en données et/ou en un ou plusieurs programmes, encodée en vue d’un traitement par un dispositif informatisé.</skos:definition>
      <rdakit:toolkitDefinition xml:lang="fr">Ressource qui consiste en données et/ou en un ou plusieurs programmes, encodée en vue d’un traitement par un dispositif informatisé.</rdakit:toolkitDefinition>
      <skos:scopeNote xml:lang="fr">La ressource peut requérir l’utilisation d’un système périphérique directement connecté à un dispositif informatisé, un programme d’application et/ou une connexion à un réseau d’ordinateurs.</skos:scopeNote>
      <skos:prefLabel xml:lang="es">recurso digital</skos:prefLabel>
      <rdakit:toolkitLabel xml:lang="es">recurso digital</rdakit:toolkitLabel>
      <skos:definition xml:lang="es">Recurso (datos y/o programa(s)) codificado para su manipulación por un aparato computerizado.</skos:definition>
      <rdakit:toolkitDefinition xml:lang="es">Recurso (datos y/o programa(s)) codificado para su manipulación por un aparato computerizado.</rdakit:toolkitDefinition>
      <skos:scopeNote xml:lang="es">El recurso puede requerir el uso de aparatos periféricos conectados directamente a un aparato computerizado (p.ej., una unidad de CD-ROM), un programa de aplicaciones (p.ej., un reproductor de un medio o un visualizador de imagen), y/o una conexión a una red de computadoras (p.ej., internet).</skos:scopeNote>
      <skos:prefLabel xml:lang="de">Digitale Ressource</skos:prefLabel>
      <skos:altLabel xml:lang="de">Datei</skos:altLabel>
      <rdakit:toolkitLabel xml:lang="de">Digitale Ressource</rdakit:toolkitLabel>
      <skos:definition xml:lang="de">Eine Ressource (Daten und/oder Programm(e)), die zur Bedienung mit einem computerbasierten Gerät kodiert ist.</skos:definition>
      <rdakit:toolkitDefinition xml:lang="de">Eine Ressource (Daten und/oder Programm(e)), die zur Bedienung mit einem computerbasierten Gerät kodiert ist.</rdakit:toolkitDefinition>
      <skos:scopeNote xml:lang="de">Es kann notwendig sein, dass für die Verwendung der Ressource ein Peripheriegerät erforderlich ist, das direkt mit dem Rechner verbunden ist, ein Anwendungsprogramm und/oder eine Verbindung zu einem Computernetz.</skos:scopeNote>
      <skos:prefLabel xml:lang="fi">digitaalinen aineisto</skos:prefLabel>
      <rdakit:toolkitLabel xml:lang="fi">digitaalinen aineisto</rdakit:toolkitLabel>
      <skos:definition xml:lang="fi">Aineisto joka koostuu tietosisällöstä ja/tai ohjelmasta/ohjelmista, ja joka on koodattu käytettäväksi tietokoneella.</skos:definition>
      <rdakit:toolkitDefinition xml:lang="fi">Aineisto joka koostuu tietosisällöstä ja/tai ohjelmasta/ohjelmista, ja joka on koodattu käytettäväksi tietokoneella.</rdakit:toolkitDefinition>
      <skos:scopeNote xml:lang="fi">Aineiston käyttö saattaa edellyttää oheislaitetta joka on suoraan kytkettynä tietokoneeseen, sovellusohjelmaa ja/tai yhteyttä tietoverkkoon.</skos:scopeNote>
      <skos:prefLabel xml:lang="da">digital ressource</skos:prefLabel>
      <rdakit:toolkitLabel xml:lang="da">digital ressource</rdakit:toolkitLabel>
      <skos:definition xml:lang="da">Ressource, der består af data og/eller et eller flere programmer, der er kodet til at blive behandlet af en computer.</skos:definition>
      <rdakit:toolkitDefinition xml:lang="da">Ressource, der består af data og/eller et eller flere programmer, der er kodet til at blive behandlet af en computer.</rdakit:toolkitDefinition>
      <skos:scopeNote xml:lang="da">Ressourcen kan kræve brug af udstyr forbundet med en computer, et applikationsprogram og/eller en forbindelse til et computernetværk.</skos:scopeNote>
      <skos:prefLabel xml:lang="ca">recurs digital</skos:prefLabel>
      <rdakit:toolkitLabel xml:lang="ca">recurs digital</rdakit:toolkitLabel>
      <skos:definition xml:lang="ca">Recurs que consisteix en dades i/o un o més programes codificat perquè pugui ser manipulat per un aparell informàtic.</skos:definition>
      <rdakit:toolkitDefinition xml:lang="ca">Recurs que consisteix en dades i/o un o més programes codificat perquè pugui ser manipulat per un aparell informàtic.</rdakit:toolkitDefinition>
      <skos:scopeNote xml:lang="ca">El recurs pot requerir l’ús d’un aparell perifèric connectat directament a un aparell informàtic, d’un programa d’aplicació i/o d’una connexió a una xarxa d’ordinadors.</skos:scopeNote>
      <skos:prefLabel xml:lang="vi">tài nguyên số</skos:prefLabel>
      <rdakit:toolkitLabel xml:lang="vi">tài nguyên số</rdakit:toolkitLabel>
      <skos:definition xml:lang="vi">Tài nguyên gồm có dữ liệu và/hoặc một hoặc nhiều hơn chương trình được mã hoá để thao tác bằng thiết bị tin học hoá.</skos:definition>
      <rdakit:toolkitDefinition xml:lang="vi">Tài nguyên gồm có dữ liệu và/hoặc một hoặc nhiều hơn chương trình được mã hoá để thao tác bằng thiết bị tin học hoá.</rdakit:toolkitDefinition>
      <skos:scopeNote xml:lang="vi">Tài nguyên này có thể yêu cầu sử dụng thiết bị ngoại vi trực tiếp nối với thiết bị tin học hoá, chương trình ứng dụng, và/hoặc nối với mạng máy tính.</skos:scopeNote>
      <skos:prefLabel xml:lang="no">digital ressurs</skos:prefLabel>
      <rdakit:toolkitLabel xml:lang="no">digital ressurs</rdakit:toolkitLabel>
      <skos:definition xml:lang="no">En ressurs som består av data og/eller ett eller flere programmer, kodet for behandling av en datamaskin.</skos:definition>
      <rdakit:toolkitDefinition xml:lang="no">En ressurs som består av data og/eller ett eller flere programmer, kodet for behandling av en datamaskin.</rdakit:toolkitDefinition>
      <skos:scopeNote xml:lang="no">Ressursen kan kreve bruk av en ekstern enhet koblet direkte til en datamaskin, et dataprogram og/eller en kobling til et datanettverk.</skos:scopeNote>
    </skos:Concept>
<!-- Concept: distinctive title  -->
    <skos:Concept rdf:about="http://rdaregistry.info/termList/RDATerms/1038" xml:lang="en">
      <skos:inScheme rdf:resource="http://rdaregistry.info/termList/RDATerms"/>
      <reg:status rdf:resource="http://metadataregistry.org/uri/RegStatus/1001"/>
      <reg:identifier rdf:resource="http://metadataregistry.org/concepts/8553"/>
      <skos:prefLabel xml:lang="en">distinctive title</skos:prefLabel>
      <rdakit:toolkitLabel xml:lang="en">distinctive title</rdakit:toolkitLabel>
      <skos:definition xml:lang="en">A title of a musical work that is not just a form or musical genre, a tempo indication, a number of performers, or a type of liturgical text.</skos:definition>
      <rdakit:toolkitDefinition xml:lang="en">A title of a musical work that is not just a form or musical genre, a tempo indication, a number of performers, or a type of liturgical text.</rdakit:toolkitDefinition>
      <skos:prefLabel xml:lang="it">titolo distintivo</skos:prefLabel>
      <rdakit:toolkitLabel xml:lang="it">titolo distintivo</rdakit:toolkitLabel>
      <skos:definition xml:lang="it">Nel contesto delle opere musicali, titolo che non enuncia una forma o un genere musicale, un'indicazione di tempo, un numero di interpreti o un tipo di testo liturgico.</skos:definition>
      <rdakit:toolkitDefinition xml:lang="it">Nel contesto delle opere musicali, titolo che non enuncia una forma o un genere musicale, un'indicazione di tempo, un numero di interpreti o un tipo di testo liturgico.</rdakit:toolkitDefinition>
      <skos:prefLabel xml:lang="fr">titre distinctif</skos:prefLabel>
      <rdakit:toolkitLabel xml:lang="fr">titre distinctif</rdakit:toolkitLabel>
      <skos:definition xml:lang="fr">Titre d’une œuvre musicale qui n’est pas simplement une forme ou un genre musical, une indication de tempo, un nombre d’interprètes ou un type de texte liturgique.</skos:definition>
      <rdakit:toolkitDefinition xml:lang="fr">Titre d’une œuvre musicale qui n’est pas simplement une forme ou un genre musical, une indication de tempo, un nombre d’interprètes ou un type de texte liturgique.</rdakit:toolkitDefinition>
      <skos:prefLabel xml:lang="es">título distintivo</skos:prefLabel>
      <rdakit:toolkitLabel xml:lang="es">título distintivo</rdakit:toolkitLabel>
      <skos:definition xml:lang="es">En el contexto de las obras musicales, un título que no constituye solamente una forma o género musical, una indicación de tiempo, un número de interprétes o un tipo de texto litúrgico.</skos:definition>
      <rdakit:toolkitDefinition xml:lang="es">En el contexto de las obras musicales, un título que no constituye solamente una forma o género musical, una indicación de tiempo, un número de interprétes o un tipo de texto litúrgico.</rdakit:toolkitDefinition>
      <skos:prefLabel xml:lang="de">Spezifischer Titel</skos:prefLabel>
      <rdakit:toolkitLabel xml:lang="de">Spezifischer Titel</rdakit:toolkitLabel>
      <skos:definition xml:lang="de">Ein Titel eines Musikwerks, der nicht nur aus einer Form oder einem musikalischen Genre, einer Tempoangabe, einer Reihe von Ausführenden oder einer Form von liturgischem Text besteht.</skos:definition>
      <rdakit:toolkitDefinition xml:lang="de">Ein Titel eines Musikwerks, der nicht nur aus einer Form oder einem musikalischen Genre, einer Tempoangabe, einer Reihe von Ausführenden oder einer Form von liturgischem Text besteht.</rdakit:toolkitDefinition>
      <skos:prefLabel xml:lang="fi">erottuva nimeke</skos:prefLabel>
      <rdakit:toolkitLabel xml:lang="fi">erottuva nimeke</rdakit:toolkitLabel>
      <skos:definition xml:lang="fi">Musiikkiteosten kontekstissa nimeke, joka on muutakin kuin vain muoto tai musiikinlaji, tempomerkintä, esittäjien lukumäärä tai liturgisen teoksen tyyppi.</skos:definition>
      <rdakit:toolkitDefinition xml:lang="fi">Musiikkiteosten kontekstissa nimeke, joka on muutakin kuin vain muoto tai musiikinlaji, tempomerkintä, esittäjien lukumäärä tai liturgisen teoksen tyyppi.</rdakit:toolkitDefinition>
      <skos:prefLabel xml:lang="da">prægnant titel</skos:prefLabel>
      <rdakit:toolkitLabel xml:lang="da">prægnant titel</rdakit:toolkitLabel>
      <skos:definition xml:lang="da">Titel på et musikværk, der ikke bare er en formbetegnelse eller en musikgenre, en angivelse af tempo, et antal udøvere eller en slags liturgisk tekst.</skos:definition>
      <rdakit:toolkitDefinition xml:lang="da">Titel på et musikværk, der ikke bare er en formbetegnelse eller en musikgenre, en angivelse af tempo, et antal udøvere eller en slags liturgisk tekst.</rdakit:toolkitDefinition>
      <skos:prefLabel xml:lang="ca">títol distintiu</skos:prefLabel>
      <rdakit:toolkitLabel xml:lang="ca">títol distintiu</rdakit:toolkitLabel>
      <skos:definition xml:lang="ca">Títol d'una obra musical que no és simplement una forma o un gènere musical, una indicació de tempo, un nombre d’intèrprets o un tipus de text litúrgic.</skos:definition>
      <rdakit:toolkitDefinition xml:lang="ca">Títol d'una obra musical que no és simplement una forma o un gènere musical, una indicació de tempo, un nombre d’intèrprets o un tipus de text litúrgic.</rdakit:toolkitDefinition>
      <skos:prefLabel xml:lang="vi">nhan đề phân biệt</skos:prefLabel>
      <rdakit:toolkitLabel xml:lang="vi">nhan đề phân biệt</rdakit:toolkitLabel>
      <skos:definition xml:lang="vi">Nhan đề của tác phẩm âm nhạc không chỉ là định dạng hoặc thể loại âm nhạc, biểu thị nhịp độ, số lượng người biểu diễn, hoặc loại văn bản nghi thức tế lễ.</skos:definition>
      <rdakit:toolkitDefinition xml:lang="vi">Nhan đề của tác phẩm âm nhạc không chỉ là định dạng hoặc thể loại âm nhạc, biểu thị nhịp độ, số lượng người biểu diễn, hoặc loại văn bản nghi thức tế lễ.</rdakit:toolkitDefinition>
      <skos:prefLabel xml:lang="no">gjenkjennelig tittel</skos:prefLabel>
      <rdakit:toolkitLabel xml:lang="no">gjenkjennelig tittel</rdakit:toolkitLabel>
      <skos:definition xml:lang="no">En tittel for et musikalsk verk som ikke bare er en form eller musikalsk sjanger, indikasjon på tempo, antall utøvere eller en type liturgisk tekst.</skos:definition>
      <rdakit:toolkitDefinition xml:lang="no">En tittel for et musikalsk verk som ikke bare er en form eller musikalsk sjanger, indikasjon på tempo, antall utøvere eller en type liturgisk tekst.</rdakit:toolkitDefinition>
    </skos:Concept>
<!-- Concept: double leaf  -->
    <skos:Concept rdf:about="http://rdaregistry.info/termList/RDATerms/1039" xml:lang="en">
      <skos:inScheme rdf:resource="http://rdaregistry.info/termList/RDATerms"/>
      <reg:status rdf:resource="http://metadataregistry.org/uri/RegStatus/1001"/>
      <reg:identifier rdf:resource="http://metadataregistry.org/concepts/8554"/>
      <skos:prefLabel xml:lang="en">double leaf</skos:prefLabel>
      <rdakit:toolkitLabel xml:lang="en">double leaf</rdakit:toolkitLabel>
      <skos:definition xml:lang="en">A leaf of double size relative to the rest of a manifestation or item, folded in half at the fore-edge or top edge, with the fold uncut and no printing inside the fold, and typically bound at the inner margin.</skos:definition>
      <rdakit:toolkitDefinition xml:lang="en">A leaf of double size relative to the rest of a manifestation or item, folded in half at the fore-edge or top edge, with the fold uncut and no printing inside the fold, and typically bound at the inner margin.</rdakit:toolkitDefinition>
      <skos:prefLabel xml:lang="it">foglio piegato</skos:prefLabel>
      <rdakit:toolkitLabel xml:lang="it">foglio piegato</rdakit:toolkitLabel>
      <skos:definition xml:lang="it">Un foglio di dimensioni doppie che presenta una piega sul bordo anteriore o sul bordo superiore della risorsa.</skos:definition>
      <rdakit:toolkitDefinition xml:lang="it">Un foglio di dimensioni doppie che presenta una piega sul bordo anteriore o sul bordo superiore della risorsa.</rdakit:toolkitDefinition>
      <skos:prefLabel xml:lang="fr">feuillet double</skos:prefLabel>
      <rdakit:toolkitLabel xml:lang="fr">feuillet double</rdakit:toolkitLabel>
      <skos:definition xml:lang="fr">Feuillet de taille double par rapport au reste d’une manifestation ou d’un item, plié en deux au niveau de la tranche latérale ou supérieure, dont le pli n’est pas coupé ni imprimé sur son côté intérieur, et généralement relié à la marge intérieure.</skos:definition>
      <rdakit:toolkitDefinition xml:lang="fr">Feuillet de taille double par rapport au reste d’une manifestation ou d’un item, plié en deux au niveau de la tranche latérale ou supérieure, dont le pli n’est pas coupé ni imprimé sur son côté intérieur, et généralement relié à la marge intérieure.</rdakit:toolkitDefinition>
      <skos:prefLabel xml:lang="de">Faltblatt</skos:prefLabel>
      <skos:altLabel xml:lang="de">Doppelblatt</skos:altLabel>
      <rdakit:toolkitLabel xml:lang="de">Faltblatt</rdakit:toolkitLabel>
      <skos:definition xml:lang="de">Ein Blatt von doppelter Größe gegenüber dem Rest der Manifestation, das an der Vorderkante oder an der oberen Kante in der Mitte gefaltet wird, die Knickkante wird nicht aufgeschnitten und ist innen nicht bedruckt und wird typischerweise im inneren Seitenrand zusammengebunden.</skos:definition>
      <rdakit:toolkitDefinition xml:lang="de">Ein Blatt von doppelter Größe gegenüber dem Rest der Manifestation, das an der Vorderkante oder an der oberen Kante in der Mitte gefaltet wird, die Knickkante wird nicht aufgeschnitten und ist innen nicht bedruckt und wird typischerweise im inneren Seitenrand zusammengebunden.</rdakit:toolkitDefinition>
      <skos:prefLabel xml:lang="fi">kaksoislehti</skos:prefLabel>
      <rdakit:toolkitLabel xml:lang="fi">kaksoislehti</rdakit:toolkitLabel>
      <skos:definition xml:lang="fi">Kaksi kertaa muun aineiston kokoinen lehti, joka on taitettu kahtia etureunasta tai yläreunasta. Taite on leikkaamaton eikä sen sisällä ole painettua sisältöä, ja se on sidottu tavallisesti sisäreunasta.</skos:definition>
      <rdakit:toolkitDefinition xml:lang="fi">Kaksi kertaa muun aineiston kokoinen lehti, joka on taitettu kahtia etureunasta tai yläreunasta. Taite on leikkaamaton eikä sen sisällä ole painettua sisältöä, ja se on sidottu tavallisesti sisäreunasta.</rdakit:toolkitDefinition>
      <skos:prefLabel xml:lang="da">dobbeltblad</skos:prefLabel>
      <rdakit:toolkitLabel xml:lang="da">dobbeltblad</rdakit:toolkitLabel>
      <skos:definition xml:lang="da">Blad i dobbelt størrelse i forhold til resten af ressourcen, foldet én gang ved forsnittet eller oversnittet, med folden uopskåret og uden tryk på foldens inderside; typisk bundet ved indermarginen.</skos:definition>
      <rdakit:toolkitDefinition xml:lang="da">Blad i dobbelt størrelse i forhold til resten af ressourcen, foldet én gang ved forsnittet eller oversnittet, med folden uopskåret og uden tryk på foldens inderside; typisk bundet ved indermarginen.</rdakit:toolkitDefinition>
      <skos:prefLabel xml:lang="ca">full doble</skos:prefLabel>
      <rdakit:toolkitLabel xml:lang="ca">full doble</rdakit:toolkitLabel>
      <skos:definition xml:lang="ca">Full de mida doble en relació a la resta d'una manifestació o d'un ítem, plegat per la meitat pel marge lateral o superior amb el plec sense tallar i sense imprimir a l'interior del plec, i en general enquadernat pel marge interior.</skos:definition>
      <rdakit:toolkitDefinition xml:lang="ca">Full de mida doble en relació a la resta d'una manifestació o d'un ítem, plegat per la meitat pel marge lateral o superior amb el plec sense tallar i sense imprimir a l'interior del plec, i en general enquadernat pel marge interior.</rdakit:toolkitDefinition>
      <skos:prefLabel xml:lang="vi">tờ kép</skos:prefLabel>
      <rdakit:toolkitLabel xml:lang="vi">tờ kép</rdakit:toolkitLabel>
      <skos:definition xml:lang="vi">Tờ cỡ gấp đôi so với phần còn lại của biểu thị hoặc bản, được gấp thành đôi ở rìa trước hoặc rìa trên, với chỗ gấp không cắt và không in bên trong, và giới hạn ở lề trong.</skos:definition>
      <rdakit:toolkitDefinition xml:lang="vi">Tờ cỡ gấp đôi so với phần còn lại của biểu thị hoặc bản, được gấp thành đôi ở rìa trước hoặc rìa trên, với chỗ gấp không cắt và không in bên trong, và giới hạn ở lề trong.</rdakit:toolkitDefinition>
      <skos:prefLabel xml:lang="no">dobbeltblad</skos:prefLabel>
      <rdakit:toolkitLabel xml:lang="no">dobbeltblad</rdakit:toolkitLabel>
      <skos:definition xml:lang="no">Et blad i dobbel størrelse i forhold til resten av manifestasjonen eller eksemplaret, brettet i to langs yttermarg eller overkant, med ubeskåret brett og uten noe trykt på innsiden av bretten, vanligvis innbundet langs innermargen.</skos:definition>
      <rdakit:toolkitDefinition xml:lang="no">Et blad i dobbel størrelse i forhold til resten av manifestasjonen eller eksemplaret, brettet i to langs yttermarg eller overkant, med ubeskåret brett og uten noe trykt på innsiden av bretten, vanligvis innbundet langs innermargen.</rdakit:toolkitDefinition>
    </skos:Concept>
<!-- Concept: early printed resource  -->
    <skos:Concept rdf:about="http://rdaregistry.info/termList/RDATerms/1040" xml:lang="en">
      <skos:inScheme rdf:resource="http://rdaregistry.info/termList/RDATerms"/>
      <reg:status rdf:resource="http://metadataregistry.org/uri/RegStatus/1001"/>
      <reg:identifier rdf:resource="http://metadataregistry.org/concepts/8555"/>
      <skos:prefLabel xml:lang="en">early printed resource</skos:prefLabel>
      <rdakit:toolkitLabel xml:lang="en">early printed resource</rdakit:toolkitLabel>
      <skos:definition xml:lang="en">A manifestation manufactured using a hand-press method, before the advent of machine printing in the nineteenth century.</skos:definition>
      <skos:prefLabel xml:lang="it">risorsa antiche a stampa</skos:prefLabel>
      <rdakit:toolkitLabel xml:lang="it">risorsa antiche a stampa</rdakit:toolkitLabel>
      <skos:definition xml:lang="it">Materiali prodotti prima dell'introduzione della stampa meccanica, approssimativamente tra il 1825 e il 1830.</skos:definition>
      <rdakit:toolkitDefinition xml:lang="it">Materiali prodotti prima dell'introduzione della stampa meccanica, approssimativamente tra il 1825 e il 1830.</rdakit:toolkitDefinition>
      <rdakit:toolkitDefinition xml:lang="en">A manifestation manufactured using a hand-press method, before the advent of machine printing in the nineteenth century.</rdakit:toolkitDefinition>
      <skos:prefLabel xml:lang="de">Alte Drucke</skos:prefLabel>
      <rdakit:toolkitLabel xml:lang="de">Alte Drucke</rdakit:toolkitLabel>
      <skos:definition xml:lang="de">Eine Manifestation, die vor der Einführung des Maschinendrucks (circa 1825 - 1830) mit einer Handpresse hergestellt wurde.</skos:definition>
      <rdakit:toolkitDefinition xml:lang="de">Eine Manifestation, die vor der Einführung des Maschinendrucks (circa 1825 - 1830) mit einer Handpresse hergestellt wurde.</rdakit:toolkitDefinition>
      <skos:prefLabel xml:lang="fi">vanhat painetut aineistot</skos:prefLabel>
      <rdakit:toolkitLabel xml:lang="fi">vanhat painetut aineistot</rdakit:toolkitLabel>
      <skos:definition xml:lang="fi">Manifestaatio, joka on valmistettu käsipainomenetelmällä ennen painokoneen yleistymistä 1800-luvulla.</skos:definition>
      <rdakit:toolkitDefinition xml:lang="fi">Manifestaatio, joka on valmistettu käsipainomenetelmällä ennen painokoneen yleistymistä 1800-luvulla.</rdakit:toolkitDefinition>
      <skos:prefLabel xml:lang="da">tidlige tryk</skos:prefLabel>
      <rdakit:toolkitLabel xml:lang="da">tidlige tryk</rdakit:toolkitLabel>
      <skos:definition xml:lang="da">Manifestation fremstillet vha. en håndpressemetode, før maskintrykkeri gjorde sit indtog i 1800-tallet.</skos:definition>
      <rdakit:toolkitDefinition xml:lang="da">Manifestation fremstillet vha. en håndpressemetode, før maskintrykkeri gjorde sit indtog i 1800-tallet.</rdakit:toolkitDefinition>
      <skos:prefLabel xml:lang="ca">recursos impresos antics</skos:prefLabel>
      <rdakit:toolkitLabel xml:lang="ca">recursos impresos antics</rdakit:toolkitLabel>
      <skos:definition xml:lang="ca">Manifestació fabricada usant un mètode d'impremta manual anterior a l’aparició de la impremta industrial del segle XIX.</skos:definition>
      <rdakit:toolkitDefinition xml:lang="ca">Manifestació fabricada usant un mètode d'impremta manual anterior a l’aparició de la impremta industrial del segle XIX.</rdakit:toolkitDefinition>
      <skos:prefLabel xml:lang="fr">ressource imprimée ancienne</skos:prefLabel>
      <rdakit:toolkitLabel xml:lang="fr">ressource imprimée ancienne</rdakit:toolkitLabel>
      <skos:definition xml:lang="fr">Manifestation fabriquée à l’aide d’un procédé d’impression manuel, avant l’apparition de l’imprimerie mécanisée au dix-neuvième siècle.</skos:definition>
      <rdakit:toolkitDefinition xml:lang="fr">Manifestation fabriquée à l’aide d’un procédé d’impression manuel, avant l’apparition de l’imprimerie mécanisée au dix-neuvième siècle.</rdakit:toolkitDefinition>
      <skos:prefLabel xml:lang="vi">tài nguyên in đầu</skos:prefLabel>
      <rdakit:toolkitLabel xml:lang="vi">tài nguyên in đầu</rdakit:toolkitLabel>
      <skos:definition xml:lang="vi">Tài liệu được chế tạo sử dụng phương pháp in ấn bằng tay, trước khi in máy xuất hiện trong thế kỷ mười chín.</skos:definition>
      <rdakit:toolkitDefinition xml:lang="vi">Tài liệu được chế tạo sử dụng phương pháp in ấn bằng tay, trước khi in máy xuất hiện trong thế kỷ mười chín.</rdakit:toolkitDefinition>
      <skos:prefLabel xml:lang="no">tidligere, trykt ressurs</skos:prefLabel>
      <rdakit:toolkitLabel xml:lang="no">tidligere, trykt ressurs</rdakit:toolkitLabel>
      <skos:definition xml:lang="no">En manifestasjon som er trykt for hånd før maskintrykking kom i bruk rundt 1825-1830.</skos:definition>
      <rdakit:toolkitDefinition xml:lang="no">En manifestasjon som er trykt for hånd før maskintrykking kom i bruk rundt 1825-1830.</rdakit:toolkitDefinition>
    </skos:Concept>
<!-- Concept: element  -->
    <skos:Concept rdf:about="http://rdaregistry.info/termList/RDATerms/1041" xml:lang="en">
      <skos:inScheme rdf:resource="http://rdaregistry.info/termList/RDATerms"/>
      <reg:status rdf:resource="http://metadataregistry.org/uri/RegStatus/1001"/>
      <reg:identifier rdf:resource="http://metadataregistry.org/concepts/8556"/>
      <skos:prefLabel xml:lang="en">element</skos:prefLabel>
      <rdakit:toolkitLabel xml:lang="en">element</rdakit:toolkitLabel>
      <skos:definition xml:lang="en">A word, character, or group of words and/or characters representing a distinct unit of bibliographic information.</skos:definition>
      <rdakit:toolkitDefinition xml:lang="en">A word, character, or group of words and/or characters representing a distinct unit of bibliographic information.</rdakit:toolkitDefinition>
      <skos:prefLabel xml:lang="it">elemento</skos:prefLabel>
      <rdakit:toolkitLabel xml:lang="it">elemento</rdakit:toolkitLabel>
      <skos:definition xml:lang="it">Parola, carattere o serie di parole e/o caratteri che rappresentano un'unità distinta d'informazione bibliografica.</skos:definition>
      <rdakit:toolkitDefinition xml:lang="it">Parola, carattere o serie di parole e/o caratteri che rappresentano un'unità distinta d'informazione bibliografica.</rdakit:toolkitDefinition>
      <skos:prefLabel xml:lang="fr">élément</skos:prefLabel>
      <rdakit:toolkitLabel xml:lang="fr">élément</rdakit:toolkitLabel>
      <skos:definition xml:lang="fr">Mot, caractère ou groupe de mots et/ou de caractères représentant une unité distincte d’information bibliographique.</skos:definition>
      <rdakit:toolkitDefinition xml:lang="fr">Mot, caractère ou groupe de mots et/ou de caractères représentant une unité distincte d’information bibliographique.</rdakit:toolkitDefinition>
      <skos:prefLabel xml:lang="fi">elementti</skos:prefLabel>
      <rdakit:toolkitLabel xml:lang="fi">elementti</rdakit:toolkitLabel>
      <skos:definition xml:lang="fi">Sana, merkki tai sana - ja/tai merkkiryhmä, joka on bibliografisten tietojen erillinen yksikkö.</skos:definition>
      <rdakit:toolkitDefinition xml:lang="fi">Sana, merkki tai sana - ja/tai merkkiryhmä, joka on bibliografisten tietojen erillinen yksikkö.</rdakit:toolkitDefinition>
      <skos:prefLabel xml:lang="de">Element</skos:prefLabel>
      <rdakit:toolkitLabel xml:lang="de">Element</rdakit:toolkitLabel>
      <skos:definition xml:lang="de">Ein Wort, ein Zeichen oder eine Gruppe von Wörtern und/oder Zeichen, das/die eine eindeutige Einheit bibliografischer Information repräsentiert.</skos:definition>
      <rdakit:toolkitDefinition xml:lang="de">Ein Wort, ein Zeichen oder eine Gruppe von Wörtern und/oder Zeichen, das/die eine eindeutige Einheit bibliografischer Information repräsentiert.</rdakit:toolkitDefinition>
      <skos:prefLabel xml:lang="da">element</skos:prefLabel>
      <rdakit:toolkitLabel xml:lang="da">element</rdakit:toolkitLabel>
      <skos:definition xml:lang="da">Ord, tegn eller gruppe af ord og/eller tegn, der repræsenterer en distinkt bibliografisk oplysning.</skos:definition>
      <rdakit:toolkitDefinition xml:lang="da">Ord, tegn eller gruppe af ord og/eller tegn, der repræsenterer en distinkt bibliografisk oplysning.</rdakit:toolkitDefinition>
      <skos:prefLabel xml:lang="ca">element</skos:prefLabel>
      <rdakit:toolkitLabel xml:lang="ca">element</rdakit:toolkitLabel>
      <skos:definition xml:lang="ca">Paraula, caràcter o grup de paraules i/o de caràcters que representa una unitat distinta d’informació bibliogràfica.</skos:definition>
      <rdakit:toolkitDefinition xml:lang="ca">Paraula, caràcter o grup de paraules i/o de caràcters que representa una unitat distinta d’informació bibliogràfica.</rdakit:toolkitDefinition>
      <skos:prefLabel xml:lang="vi">yếu tố</skos:prefLabel>
      <rdakit:toolkitLabel xml:lang="vi">yếu tố</rdakit:toolkitLabel>
      <skos:definition xml:lang="vi">Từ, ký tự, hoặc nhóm từ và/hoặc ký tự trình bày một đơn vị riêng biệt của thông tin thư mục.</skos:definition>
      <rdakit:toolkitDefinition xml:lang="vi">Từ, ký tự, hoặc nhóm từ và/hoặc ký tự trình bày một đơn vị riêng biệt của thông tin thư mục.</rdakit:toolkitDefinition>
      <skos:prefLabel xml:lang="no">element</skos:prefLabel>
      <rdakit:toolkitLabel xml:lang="no">element</rdakit:toolkitLabel>
      <skos:definition xml:lang="no">Et ord, et tegn eller gruppe av ord og/eller tegn som utgjør en enkelt enhet av bibliografisk informasjon.</skos:definition>
      <rdakit:toolkitDefinition xml:lang="no">Et ord, et tegn eller gruppe av ord og/eller tegn som utgjør en enkelt enhet av bibliografisk informasjon.</rdakit:toolkitDefinition>
    </skos:Concept>
<!-- Concept: explanatory reference  -->
    <skos:Concept rdf:about="http://rdaregistry.info/termList/RDATerms/1042" xml:lang="en">
      <skos:inScheme rdf:resource="http://rdaregistry.info/termList/RDATerms"/>
      <reg:status rdf:resource="http://metadataregistry.org/uri/RegStatus/1001"/>
      <reg:identifier rdf:resource="http://metadataregistry.org/concepts/8557"/>
      <skos:prefLabel xml:lang="en">explanatory reference</skos:prefLabel>
      <rdakit:toolkitLabel xml:lang="en">explanatory reference</rdakit:toolkitLabel>
      <skos:definition xml:lang="en">An elaborated see reference or see also reference that explains the circumstances under which the authorized access points involved should be consulted.</skos:definition>
      <rdakit:toolkitDefinition xml:lang="en">An elaborated see reference or see also reference that explains the circumstances under which the authorized access points involved should be consulted.</rdakit:toolkitDefinition>
      <skos:prefLabel xml:lang="it">rinvio esplicativo</skos:prefLabel>
      <rdakit:toolkitLabel xml:lang="it">rinvio esplicativo</rdakit:toolkitLabel>
      <skos:definition xml:lang="it">Un rinviovedi o vedi anche redatto per spiegare i casi per i quali dovrebbero essere consultati i rispettivi punti d'accesso autorizzati.</skos:definition>
      <rdakit:toolkitDefinition xml:lang="it">Un rinviovedi o vedi anche redatto per spiegare i casi per i quali dovrebbero essere consultati i rispettivi punti d'accesso autorizzati.</rdakit:toolkitDefinition>
      <skos:prefLabel xml:lang="de">Erläuternde Verweisung</skos:prefLabel>
      <rdakit:toolkitLabel xml:lang="de">Erläuternde Verweisung</rdakit:toolkitLabel>
      <skos:definition xml:lang="de">Eine erweiterte &quot;Siehe&quot;- oder &quot;Siehe-auch&quot;-Verweisung, die die Fälle erläutert, in denen die betreffenden normierten Sucheinstiege hinzugezogen werden sollten.</skos:definition>
      <rdakit:toolkitDefinition xml:lang="de">Eine erweiterte &quot;Siehe&quot;- oder &quot;Siehe-auch&quot;-Verweisung, die die Fälle erläutert, in denen die betreffenden normierten Sucheinstiege hinzugezogen werden sollten.</rdakit:toolkitDefinition>
      <skos:prefLabel xml:lang="fi">selittävä viittaus</skos:prefLabel>
      <rdakit:toolkitLabel xml:lang="fi">selittävä viittaus</rdakit:toolkitLabel>
      <skos:definition xml:lang="fi">Katso tai katso myös -viittaus, joka ilmaisee, milloin tulee kääntyä auktorisoitujen hakutietojen puoleen.</skos:definition>
      <rdakit:toolkitDefinition xml:lang="fi">Katso tai katso myös -viittaus, joka ilmaisee, milloin tulee kääntyä auktorisoitujen hakutietojen puoleen.</rdakit:toolkitDefinition>
      <skos:prefLabel xml:lang="da">forklarende henvisning</skos:prefLabel>
      <rdakit:toolkitLabel xml:lang="da">forklarende henvisning</rdakit:toolkitLabel>
      <skos:definition xml:lang="da">Uddybende se- eller se også-henvisning, der forklarer de forhold, under hvilke de involverede autoriserede søgeindgange bør konsulteres.</skos:definition>
      <rdakit:toolkitDefinition xml:lang="da">Uddybende se- eller se også-henvisning, der forklarer de forhold, under hvilke de involverede autoriserede søgeindgange bør konsulteres.</rdakit:toolkitDefinition>
      <skos:prefLabel xml:lang="ca">referència explicativa</skos:prefLabel>
      <rdakit:toolkitLabel xml:lang="ca">referència explicativa</rdakit:toolkitLabel>
      <skos:definition xml:lang="ca">Referència detallada de vegeu o de vegeu també que explica les circumstàncies en les quals cal consultar els punts d’accés autoritzats en qüestió.</skos:definition>
      <rdakit:toolkitDefinition xml:lang="ca">Referència detallada de vegeu o de vegeu també que explica les circumstàncies en les quals cal consultar els punts d’accés autoritzats en qüestió.</rdakit:toolkitDefinition>
      <skos:prefLabel xml:lang="fr">renvoi justificatif</skos:prefLabel>
      <rdakit:toolkitLabel xml:lang="fr">renvoi justificatif</rdakit:toolkitLabel>
      <skos:definition xml:lang="fr">Renvoi voir ou renvoi voir aussi détaillé qui explique dans quelles circonstances il faut consulter les points d’accès autorisés concernés.</skos:definition>
      <rdakit:toolkitDefinition xml:lang="fr">Renvoi voir ou renvoi voir aussi détaillé qui explique dans quelles circonstances il faut consulter les points d’accès autorisés concernés.</rdakit:toolkitDefinition>
      <skos:prefLabel xml:lang="vi">tra cứu giải thích</skos:prefLabel>
      <rdakit:toolkitLabel xml:lang="vi">tra cứu giải thích</rdakit:toolkitLabel>
      <skos:definition xml:lang="vi">Tham chiếu xem hoặc cũng xem giải thích tình huống mà một điểm truy cập được phép có liên quan phải được tra cứu.</skos:definition>
      <rdakit:toolkitDefinition xml:lang="vi">Tham chiếu xem hoặc cũng xem giải thích tình huống mà một điểm truy cập được phép có liên quan phải được tra cứu.</rdakit:toolkitDefinition>
      <skos:prefLabel xml:lang="no">forklarende henvisning</skos:prefLabel>
      <rdakit:toolkitLabel xml:lang="no">forklarende henvisning</rdakit:toolkitLabel>
      <skos:definition xml:lang="no">En utførlig se- eller se også-henvisning som forklarer når de aktuelle autoriserte søkeinngangene bør konsulteres.</skos:definition>
      <rdakit:toolkitDefinition xml:lang="no">En utførlig se- eller se også-henvisning som forklarer når de aktuelle autoriserte søkeinngangene bør konsulteres.</rdakit:toolkitDefinition>
    </skos:Concept>
<!-- Concept: finding aid  -->
    <skos:Concept rdf:about="http://rdaregistry.info/termList/RDATerms/1043" xml:lang="en">
      <skos:inScheme rdf:resource="http://rdaregistry.info/termList/RDATerms"/>
      <reg:status rdf:resource="http://metadataregistry.org/uri/RegStatus/1001"/>
      <reg:identifier rdf:resource="http://metadataregistry.org/concepts/8558"/>
      <skos:prefLabel xml:lang="en">finding aid</skos:prefLabel>
      <rdakit:toolkitLabel xml:lang="en">finding aid</rdakit:toolkitLabel>
      <skos:definition xml:lang="en">A descriptive tool providing access to a resource.</skos:definition>
      <rdakit:toolkitDefinition xml:lang="en">A descriptive tool providing access to a resource.</rdakit:toolkitDefinition>
      <skos:prefLabel xml:lang="it">aiuto alla ricerca</skos:prefLabel>
      <rdakit:toolkitLabel xml:lang="it">aiuto alla ricerca</rdakit:toolkitLabel>
      <skos:definition xml:lang="it">Strumento descrittivo che fornisce accesso a una risorsa.</skos:definition>
      <rdakit:toolkitDefinition xml:lang="it">Strumento descrittivo che fornisce accesso a una risorsa.</rdakit:toolkitDefinition>
      <skos:prefLabel xml:lang="de">Fundstellennachweis</skos:prefLabel>
      <rdakit:toolkitLabel xml:lang="de">Fundstellennachweis</rdakit:toolkitLabel>
      <skos:definition xml:lang="de">Eine Orientierungshilfe, die Zugang zu einer Ressource bietet.</skos:definition>
      <rdakit:toolkitDefinition xml:lang="de">Eine Orientierungshilfe, die Zugang zu einer Ressource bietet.</rdakit:toolkitDefinition>
      <skos:prefLabel xml:lang="fi">hakemisto</skos:prefLabel>
      <rdakit:toolkitLabel xml:lang="fi">hakemisto</rdakit:toolkitLabel>
      <skos:definition xml:lang="fi">Kuvaileva väline joka tarjoaa pääsyn aineistoon.</skos:definition>
      <rdakit:toolkitDefinition xml:lang="fi">Kuvaileva väline joka tarjoaa pääsyn aineistoon.</rdakit:toolkitDefinition>
      <skos:prefLabel xml:lang="da">vejledning</skos:prefLabel>
      <rdakit:toolkitLabel xml:lang="da">vejledning</rdakit:toolkitLabel>
      <skos:definition xml:lang="da">Beskrivende værktøj, der giver adgang til en ressource.</skos:definition>
      <rdakit:toolkitDefinition xml:lang="da">Beskrivende værktøj, der giver adgang til en ressource.</rdakit:toolkitDefinition>
      <skos:prefLabel xml:lang="ca">instrument de descripció</skos:prefLabel>
      <rdakit:toolkitLabel xml:lang="ca">instrument de descripció</rdakit:toolkitLabel>
      <skos:definition xml:lang="ca">Eina descriptiva que proporciona accés a un recurs.</skos:definition>
      <rdakit:toolkitDefinition xml:lang="ca">Eina descriptiva que proporciona accés a un recurs.</rdakit:toolkitDefinition>
      <skos:prefLabel xml:lang="fr">instrument de recherche</skos:prefLabel>
      <rdakit:toolkitLabel xml:lang="fr">instrument de recherche</rdakit:toolkitLabel>
      <skos:definition xml:lang="fr">Instrument descriptif fournissant l’accès à une ressource.</skos:definition>
      <rdakit:toolkitDefinition xml:lang="fr">Instrument descriptif fournissant l’accès à une ressource.</rdakit:toolkitDefinition>
      <skos:prefLabel xml:lang="vi">hỗ trợ tìm kiếm</skos:prefLabel>
      <rdakit:toolkitLabel xml:lang="vi">hỗ trợ tìm kiếm</rdakit:toolkitLabel>
      <skos:definition xml:lang="vi">Công cụ mô tả cung cấp truy cập tới một tài nguyên.</skos:definition>
      <rdakit:toolkitDefinition xml:lang="vi">Công cụ mô tả cung cấp truy cập tới một tài nguyên.</rdakit:toolkitDefinition>
      <skos:prefLabel xml:lang="no">veiledning</skos:prefLabel>
      <rdakit:toolkitLabel xml:lang="no">veiledning</rdakit:toolkitLabel>
      <skos:definition xml:lang="no">Et beskrivende verktøy som gir tilgang til en ressurs.</skos:definition>
      <rdakit:toolkitDefinition xml:lang="no">Et beskrivende verktøy som gir tilgang til en ressurs.</rdakit:toolkitDefinition>
    </skos:Concept>
<!-- Concept: formally presented  -->
    <skos:Concept rdf:about="http://rdaregistry.info/termList/RDATerms/1044" xml:lang="en">
      <skos:inScheme rdf:resource="http://rdaregistry.info/termList/RDATerms"/>
      <reg:status rdf:resource="http://metadataregistry.org/uri/RegStatus/1001"/>
      <reg:identifier rdf:resource="http://metadataregistry.org/concepts/8559"/>
      <skos:prefLabel xml:lang="en">formally presented</skos:prefLabel>
      <rdakit:toolkitLabel xml:lang="en">formally presented</rdakit:toolkitLabel>
      <skos:definition xml:lang="en">An element appearing in isolation, as opposed to appearing embedded in text, and in a prominent location.</skos:definition>
      <rdakit:toolkitDefinition xml:lang="en">An element appearing in isolation, as opposed to appearing embedded in text, and in a prominent location.</rdakit:toolkitDefinition>
      <skos:prefLabel xml:lang="de">Förmlich präsentierten</skos:prefLabel>
      <rdakit:toolkitLabel xml:lang="de">Förmlich präsentierten</rdakit:toolkitLabel>
      <skos:definition xml:lang="de">Ein Element, das an exponierter Stelle einzeln aufgeführt wird, im Gegensatz zur Aufführung im Text.</skos:definition>
      <rdakit:toolkitDefinition xml:lang="de">Ein Element, das an exponierter Stelle einzeln aufgeführt wird, im Gegensatz zur Aufführung im Text.</rdakit:toolkitDefinition>
      <skos:prefLabel xml:lang="fi">muodollisesti esitetty</skos:prefLabel>
      <rdakit:toolkitLabel xml:lang="fi">muodollisesti esitetty</rdakit:toolkitLabel>
      <skos:definition xml:lang="fi">Esiintyy muualla kuin itse tekstissä, arvovaltaisessa lähteessä.</skos:definition>
      <rdakit:toolkitDefinition xml:lang="fi">Esiintyy muualla kuin itse tekstissä, arvovaltaisessa lähteessä.</rdakit:toolkitDefinition>
      <skos:prefLabel xml:lang="da">formelt præsenteret</skos:prefLabel>
      <rdakit:toolkitLabel xml:lang="da">formelt præsenteret</rdakit:toolkitLabel>
      <skos:definition xml:lang="da">Element der optræder isoleret på fremtrædende plads, i modsætning til i løbende tekst.</skos:definition>
      <rdakit:toolkitDefinition xml:lang="da">Element der optræder isoleret på fremtrædende plads, i modsætning til i løbende tekst.</rdakit:toolkitDefinition>
      <skos:prefLabel xml:lang="ca">presentat formalment</skos:prefLabel>
      <rdakit:toolkitLabel xml:lang="ca">presentat formalment</rdakit:toolkitLabel>
      <skos:definition xml:lang="ca">Element presentat separadament, per oposició a la presentació inserida en el text, i en un lloc destacat.</skos:definition>
      <rdakit:toolkitDefinition xml:lang="ca">Element presentat separadament, per oposició a la presentació inserida en el text, i en un lloc destacat.</rdakit:toolkitDefinition>
      <skos:prefLabel xml:lang="fr">présenté de façon formelle</skos:prefLabel>
      <rdakit:toolkitLabel xml:lang="fr">présenté de façon formelle</rdakit:toolkitLabel>
      <skos:definition xml:lang="fr">Élément présenté isolément plutôt qu’intégré dans du texte, et à un endroit mis en évidence.</skos:definition>
      <rdakit:toolkitDefinition xml:lang="fr">Élément présenté isolément plutôt qu’intégré dans du texte, et à un endroit mis en évidence.</rdakit:toolkitDefinition>
      <skos:prefLabel xml:lang="vi">thể hiện chính thức</skos:prefLabel>
      <rdakit:toolkitLabel xml:lang="vi">thể hiện chính thức</rdakit:toolkitLabel>
      <skos:definition xml:lang="vi">Yếu tố xuất hiện riêng biệt, ngược với xuất hiện nhúng trong văn bản, và ở vị trí nổi bật.</skos:definition>
      <rdakit:toolkitDefinition xml:lang="vi">Yếu tố xuất hiện riêng biệt, ngược với xuất hiện nhúng trong văn bản, và ở vị trí nổi bật.</rdakit:toolkitDefinition>
      <skos:prefLabel xml:lang="no">formell angivelse</skos:prefLabel>
      <rdakit:toolkitLabel xml:lang="no">formell angivelse</rdakit:toolkitLabel>
      <skos:definition xml:lang="no">Et element som finnes alene og på fremtredende plass, ikke i en løpende tekst.</skos:definition>
      <rdakit:toolkitDefinition xml:lang="no">Et element som finnes alene og på fremtredende plass, ikke i en løpende tekst.</rdakit:toolkitDefinition>
    </skos:Concept>
<!-- Concept: gathering  -->
    <skos:Concept rdf:about="http://rdaregistry.info/termList/RDATerms/1045" xml:lang="en">
      <skos:inScheme rdf:resource="http://rdaregistry.info/termList/RDATerms"/>
      <reg:status rdf:resource="http://metadataregistry.org/uri/RegStatus/1001"/>
      <reg:identifier rdf:resource="http://metadataregistry.org/concepts/8560"/>
      <skos:prefLabel xml:lang="en">gathering</skos:prefLabel>
      <rdakit:toolkitLabel xml:lang="en">gathering</rdakit:toolkitLabel>
      <skos:definition xml:lang="en">A pair or pairs of leaves that together form a distinctive unit for binding purposes.</skos:definition>
      <rdakit:toolkitDefinition xml:lang="en">A pair or pairs of leaves that together form a distinctive unit for binding purposes.</rdakit:toolkitDefinition>
      <skos:scopeNote xml:lang="en">A gathering may consist of a folded sheet, a fraction of a folded sheet, or several folded sheets tucked inside one another.</skos:scopeNote>
      <skos:prefLabel xml:lang="it">fascicolo</skos:prefLabel>
      <rdakit:toolkitLabel xml:lang="it">fascicolo</rdakit:toolkitLabel>
      <skos:definition xml:lang="it">Uno o più coppie di carte – costituite da un foglio piegato, una parte di foglio piegata o numerosi fogli piegati inseriti l'uno nell'altro – che formano insieme un'unità distinta per la legatura.</skos:definition>
      <rdakit:toolkitDefinition xml:lang="it">Uno o più coppie di carte – costituite da un foglio piegato, una parte di foglio piegata o numerosi fogli piegati inseriti l'uno nell'altro – che formano insieme un'unità distinta per la legatura.</rdakit:toolkitDefinition>
      <skos:prefLabel xml:lang="de">Lage</skos:prefLabel>
      <rdakit:toolkitLabel xml:lang="de">Lage</rdakit:toolkitLabel>
      <skos:definition xml:lang="de">Ein Paar oder mehrere Paare von Blättern, die zusammen eine spezifische Einheit für Buchbinderzwecke bilden.</skos:definition>
      <rdakit:toolkitDefinition xml:lang="de">Ein Paar oder mehrere Paare von Blättern, die zusammen eine spezifische Einheit für Buchbinderzwecke bilden.</rdakit:toolkitDefinition>
      <skos:scopeNote xml:lang="de">Eine Lage kann aus einem gefalteten Bogen, einem Teil eines gefalteten Bogens oder mehreren gefalteten Bogen, die einander gesteckt sind, bestehen.</skos:scopeNote>
      <skos:prefLabel xml:lang="fi">arkkivihko</skos:prefLabel>
      <rdakit:toolkitLabel xml:lang="fi">arkkivihko</rdakit:toolkitLabel>
      <skos:definition xml:lang="fi">Yksi tai useampi lehtipari joista yhdessä muodostuu erillinen kirjan sidoksen perusyksikkö.</skos:definition>
      <rdakit:toolkitDefinition xml:lang="fi">Yksi tai useampi lehtipari joista yhdessä muodostuu erillinen kirjan sidoksen perusyksikkö.</rdakit:toolkitDefinition>
      <skos:scopeNote xml:lang="fi">Arkkivihko voi olla koottu taitetusta painoarkista, taitetun painoarkin osasta tai useasta sisäkkäin sijoitetusta painoarkista.</skos:scopeNote>
      <skos:prefLabel xml:lang="da">læg</skos:prefLabel>
      <rdakit:toolkitLabel xml:lang="da">læg</rdakit:toolkitLabel>
      <skos:definition xml:lang="da">Et eller flere sæt af ark, som tilsammen udgør en distinkt enhed til indbindingsformål.</skos:definition>
      <rdakit:toolkitDefinition xml:lang="da">Et eller flere sæt af ark, som tilsammen udgør en distinkt enhed til indbindingsformål.</rdakit:toolkitDefinition>
      <skos:scopeNote xml:lang="da">Et læg kan bestå af et foldet ark, en brøkdel af et foldet ark eller flere foldede ark, der er stukket ind i hinanden.</skos:scopeNote>
      <skos:prefLabel xml:lang="ca">quadern</skos:prefLabel>
      <rdakit:toolkitLabel xml:lang="ca">quadern</rdakit:toolkitLabel>
      <skos:definition xml:lang="ca">Un o més parells de fulls que conjuntament formen una unitat distintiva amb la finalitat de l’enquadernació.</skos:definition>
      <rdakit:toolkitDefinition xml:lang="ca">Un o més parells de fulls que conjuntament formen una unitat distintiva amb la finalitat de l’enquadernació.</rdakit:toolkitDefinition>
      <skos:scopeNote xml:lang="ca">Un quadern pot consistir d’un full plegat, d’una fracció de full plegat, o de diversos fulls plegats inserits els uns en els altres</skos:scopeNote>
      <skos:prefLabel xml:lang="fr">cahier</skos:prefLabel>
      <rdakit:toolkitLabel xml:lang="fr">cahier</rdakit:toolkitLabel>
      <skos:definition xml:lang="fr">Une ou plusieurs paires de feuillets qui, ensemble, forment une unité distincte aux fins de reliure.</skos:definition>
      <rdakit:toolkitDefinition xml:lang="fr">Une ou plusieurs paires de feuillets qui, ensemble, forment une unité distincte aux fins de reliure.</rdakit:toolkitDefinition>
      <skos:scopeNote xml:lang="fr">Un cahier peut consister en une feuille pliée, en une fraction d’une feuille pliée ou en plusieurs feuilles pliées insérées les unes dans les autres.</skos:scopeNote>
      <skos:prefLabel xml:lang="vi">tay sách</skos:prefLabel>
      <rdakit:toolkitLabel xml:lang="vi">tay sách</rdakit:toolkitLabel>
      <skos:definition xml:lang="vi">Một cặp hoặc các cặp tờ in kết hợp với nhau tạo ra một đơn vị phân biệt cho mục đích đóng bìa.</skos:definition>
      <rdakit:toolkitDefinition xml:lang="vi">Một cặp hoặc các cặp tờ in kết hợp với nhau tạo ra một đơn vị phân biệt cho mục đích đóng bìa.</rdakit:toolkitDefinition>
      <skos:scopeNote xml:lang="vi">Taysách có thể gồm có tờ gấp, phần của tờ gấp, hoặc một vài tờ gấp được lồng vào nhau.</skos:scopeNote>
      <skos:prefLabel xml:lang="no">legg</skos:prefLabel>
      <rdakit:toolkitLabel xml:lang="no">legg</rdakit:toolkitLabel>
      <skos:definition xml:lang="no">Ett eller flere par blad som sammen danner en enhet for innbinding.</skos:definition>
      <rdakit:toolkitDefinition xml:lang="no">Ett eller flere par blad som sammen danner en enhet for innbinding.</rdakit:toolkitDefinition>
      <skos:scopeNote xml:lang="no">Det kan bestå av et foldet ark, en del av et foldet ark eller flere foldete ark lagt inni hverandre.</skos:scopeNote>
    </skos:Concept>
<!-- Concept: government  -->
    <skos:Concept rdf:about="http://rdaregistry.info/termList/RDATerms/1046" xml:lang="en">
      <skos:inScheme rdf:resource="http://rdaregistry.info/termList/RDATerms"/>
      <reg:status rdf:resource="http://metadataregistry.org/uri/RegStatus/1001"/>
      <reg:identifier rdf:resource="http://metadataregistry.org/concepts/8561"/>
      <skos:prefLabel xml:lang="en">government</skos:prefLabel>
      <rdakit:toolkitLabel xml:lang="en">government</rdakit:toolkitLabel>
      <skos:definition xml:lang="en">A totality of executive, legislative, and judicial corporate bodies exercising the powers of a jurisdiction.</skos:definition>
      <rdakit:toolkitDefinition xml:lang="en">A totality of executive, legislative, and judicial corporate bodies exercising the powers of a jurisdiction.</rdakit:toolkitDefinition>
      <skos:prefLabel xml:lang="it">governo</skos:prefLabel>
      <rdakit:toolkitLabel xml:lang="it">governo</rdakit:toolkitLabel>
      <skos:definition xml:lang="it">Insieme degli organi (esecutivi, legislativi e giudiziari) che esercitano i poteri di una giurisdizione.</skos:definition>
      <rdakit:toolkitDefinition xml:lang="it">Insieme degli organi (esecutivi, legislativi e giudiziari) che esercitano i poteri di una giurisdizione.</rdakit:toolkitDefinition>
      <skos:prefLabel xml:lang="fr">gouvernement</skos:prefLabel>
      <rdakit:toolkitLabel xml:lang="fr">gouvernement</rdakit:toolkitLabel>
      <skos:definition xml:lang="fr">Ensemble des collectivités exécutives, législatives et judiciaires exerçant les pouvoirs d’une juridiction.</skos:definition>
      <rdakit:toolkitDefinition xml:lang="fr">Ensemble des collectivités exécutives, législatives et judiciaires exerçant les pouvoirs d’une juridiction.</rdakit:toolkitDefinition>
      <skos:prefLabel xml:lang="de">Gebietskörperschaft</skos:prefLabel>
      <rdakit:toolkitLabel xml:lang="de">Gebietskörperschaft</rdakit:toolkitLabel>
      <skos:definition xml:lang="de">Eine Gesamtheit der Körperschaften (Exekutive, Legistlative und Judikative), die staatliche Macht ausüben.</skos:definition>
      <rdakit:toolkitDefinition xml:lang="de">Eine Gesamtheit der Körperschaften (Exekutive, Legistlative und Judikative), die staatliche Macht ausüben.</rdakit:toolkitDefinition>
      <skos:prefLabel xml:lang="fi">hallintoviranomaiset</skos:prefLabel>
      <rdakit:toolkitLabel xml:lang="fi">hallintoviranomaiset</rdakit:toolkitLabel>
      <skos:definition xml:lang="fi">Toimivaltaa harjoittavat  toimeenpanevat , lainsäädännölliset  ja oikeuselimet.</skos:definition>
      <rdakit:toolkitDefinition xml:lang="fi">Toimivaltaa harjoittavat  toimeenpanevat , lainsäädännölliset  ja oikeuselimet.</rdakit:toolkitDefinition>
      <skos:prefLabel xml:lang="da">myndigheder</skos:prefLabel>
      <rdakit:toolkitLabel xml:lang="da">myndigheder</rdakit:toolkitLabel>
      <skos:definition xml:lang="da">Helheden af udøvende, lovgivende og dømmende korporationer, der varetager en jurisdiktions magtbeføjelser.</skos:definition>
      <rdakit:toolkitDefinition xml:lang="da">Helheden af udøvende, lovgivende og dømmende korporationer, der varetager en jurisdiktions magtbeføjelser.</rdakit:toolkitDefinition>
      <skos:prefLabel xml:lang="ca">govern</skos:prefLabel>
      <rdakit:toolkitLabel xml:lang="ca">govern</rdakit:toolkitLabel>
      <skos:definition xml:lang="ca">Conjunt de les entitats corporatives executives, legislatives i judicials que exerceixen els poders d’una jurisdicció.</skos:definition>
      <rdakit:toolkitDefinition xml:lang="ca">Conjunt de les entitats corporatives executives, legislatives i judicials que exerceixen els poders d’una jurisdicció.</rdakit:toolkitDefinition>
      <skos:prefLabel xml:lang="vi">chính quyền</skos:prefLabel>
      <rdakit:toolkitLabel xml:lang="vi">chính quyền</rdakit:toolkitLabel>
      <skos:definition xml:lang="vi">Tất cả các tập thể hành pháp, lập pháp, tư pháp thực thi quyền lực của một khu vực pháp quyền.</skos:definition>
      <rdakit:toolkitDefinition xml:lang="vi">Tất cả các tập thể hành pháp, lập pháp, tư pháp thực thi quyền lực của một khu vực pháp quyền.</rdakit:toolkitDefinition>
      <skos:prefLabel xml:lang="no">offentlige myndigheter</skos:prefLabel>
      <rdakit:toolkitLabel xml:lang="no">offentlige myndigheter</rdakit:toolkitLabel>
      <skos:definition xml:lang="no">De samlede utøvende, lovgivende og dømmende korporasjoner som utøver makt i en jurisdiksjon.</skos:definition>
      <rdakit:toolkitDefinition xml:lang="no">De samlede utøvende, lovgivende og dømmende korporasjoner som utøver makt i en jurisdiksjon.</rdakit:toolkitDefinition>
    </skos:Concept>
<!-- Concept: harmony  -->
    <skos:Concept rdf:about="http://rdaregistry.info/termList/RDATerms/1047" xml:lang="en">
      <skos:inScheme rdf:resource="http://rdaregistry.info/termList/RDATerms"/>
      <reg:status rdf:resource="http://metadataregistry.org/uri/RegStatus/1001"/>
      <reg:identifier rdf:resource="http://metadataregistry.org/concepts/8562"/>
      <skos:prefLabel xml:lang="en">harmony</skos:prefLabel>
      <rdakit:toolkitLabel xml:lang="en">harmony</rdakit:toolkitLabel>
      <skos:definition xml:lang="en">An arrangement of passages of the Bible on the same topic into parallel columns so that similarities and differences may be compared readily, or an interweaving of such passages into a continuous text.</skos:definition>
      <rdakit:toolkitDefinition xml:lang="en">An arrangement of passages of the Bible on the same topic into parallel columns so that similarities and differences may be compared readily, or an interweaving of such passages into a continuous text.</rdakit:toolkitDefinition>
      <skos:prefLabel xml:lang="it">sinossi</skos:prefLabel>
      <rdakit:toolkitLabel xml:lang="it">sinossi</rdakit:toolkitLabel>
      <skos:prefLabel xml:lang="fr">harmonie</skos:prefLabel>
      <rdakit:toolkitLabel xml:lang="fr">harmonie</rdakit:toolkitLabel>
      <skos:prefLabel xml:lang="de">Synopse</skos:prefLabel>
      <rdakit:toolkitLabel xml:lang="de">Synopse</rdakit:toolkitLabel>
      <skos:definition xml:lang="de">Eine Anordnung von Passagen der Bibel zum selben Thema in parallelen Spalten, so dass Gemeinsamkeiten und Unterschiede leicht verglichen werden können oder eine Einbindung solcher Passagen in einen fortlaufenden Text.</skos:definition>
      <rdakit:toolkitDefinition xml:lang="de">Eine Anordnung von Passagen der Bibel zum selben Thema in parallelen Spalten, so dass Gemeinsamkeiten und Unterschiede leicht verglichen werden können oder eine Einbindung solcher Passagen in einen fortlaufenden Text.</rdakit:toolkitDefinition>
      <skos:prefLabel xml:lang="fi">harmonia</skos:prefLabel>
      <rdakit:toolkitLabel xml:lang="fi">harmonia</rdakit:toolkitLabel>
      <skos:definition xml:lang="fi">Raamatun samaan aiheeseen liittyvien katkelmien esittäminen rinnakkain niin, että yhtäläisyyksiä ja eroja voi verrata, tai tällaisten katkelmien esitys yhtenäisenä tekstinä.</skos:definition>
      <rdakit:toolkitDefinition xml:lang="fi">Raamatun samaan aiheeseen liittyvien katkelmien esittäminen rinnakkain niin, että yhtäläisyyksiä ja eroja voi verrata, tai tällaisten katkelmien esitys yhtenäisenä tekstinä.</rdakit:toolkitDefinition>
      <skos:prefLabel xml:lang="da">konkordans</skos:prefLabel>
      <rdakit:toolkitLabel xml:lang="da">konkordans</rdakit:toolkitLabel>
      <skos:definition xml:lang="da">Opsætning af tekststykker i Bibelen, der vedrører samme emne, i parallelle spalter, så ligheder og forskelle nemt kan sammenlignes, eller sammenfletning af sådanne tekststykker til en fortløbende tekst.</skos:definition>
      <rdakit:toolkitDefinition xml:lang="da">Opsætning af tekststykker i Bibelen, der vedrører samme emne, i parallelle spalter, så ligheder og forskelle nemt kan sammenlignes, eller sammenfletning af sådanne tekststykker til en fortløbende tekst.</rdakit:toolkitDefinition>
      <skos:prefLabel xml:lang="ca">harmonia</skos:prefLabel>
      <rdakit:toolkitLabel xml:lang="ca">harmonia</rdakit:toolkitLabel>
      <skos:definition xml:lang="ca">Disposició dels passatges de la Bíblia sobre el mateix tema en columnes paral·leles de manera que es puguin comparar ràpidament les semblances i les diferències, o un entrellaçat d’aquests passatges en un text continu.</skos:definition>
      <rdakit:toolkitDefinition xml:lang="ca">Disposició dels passatges de la Bíblia sobre el mateix tema en columnes paral·leles de manera que es puguin comparar ràpidament les semblances i les diferències, o un entrellaçat d’aquests passatges en un text continu.</rdakit:toolkitDefinition>
      <skos:definition xml:lang="fr">Présentation des passages de la Bible portant sur le même sujet en colonnes paralèlles de sorte que les similitudes et les différences peuvent être facilement comparées, ou imbrication de ces mêmes passages dans un texte en continu.</skos:definition>
      <rdakit:toolkitDefinition xml:lang="fr">Présentation des passages de la Bible portant sur le même sujet en colonnes paralèlles de sorte que les similitudes et les différences peuvent être facilement comparées, ou imbrication de ces mêmes passages dans un texte en continu.</rdakit:toolkitDefinition>
      <skos:prefLabel xml:lang="vi">hài hoà</skos:prefLabel>
      <rdakit:toolkitLabel xml:lang="vi">hài hoà</rdakit:toolkitLabel>
      <skos:definition xml:lang="vi">Sắp xếp các đoạn của Kinh thánh về cùng chủ đề vào các cột song song để sự giống nhau và khác nhau có thể dễ dàng so sánh, hoặc liên kết các đoạn như vậy thành văn bản liên tục.</skos:definition>
      <rdakit:toolkitDefinition xml:lang="vi">Sắp xếp các đoạn của Kinh thánh về cùng chủ đề vào các cột song song để sự giống nhau và khác nhau có thể dễ dàng so sánh, hoặc liên kết các đoạn như vậy thành văn bản liên tục.</rdakit:toolkitDefinition>
      <skos:prefLabel xml:lang="no">evangelieharmoni</skos:prefLabel>
      <rdakit:toolkitLabel xml:lang="no">evangelieharmoni</rdakit:toolkitLabel>
      <skos:definition xml:lang="no">Et oppsett av bibelpassasjer om samme emne i parallelle spalter slik at likheter og forskjeller enkelt kan sammenliknes, eller en sammenstilling av slike passasjer i en kontinuerlig tekst.</skos:definition>
      <rdakit:toolkitDefinition xml:lang="no">Et oppsett av bibelpassasjer om samme emne i parallelle spalter slik at likheter og forskjeller enkelt kan sammenliknes, eller en sammenstilling av slike passasjer i en kontinuerlig tekst.</rdakit:toolkitDefinition>
    </skos:Concept>
<!-- Concept: hierarchical description  -->
    <skos:Concept rdf:about="http://rdaregistry.info/termList/RDATerms/1048" xml:lang="en">
      <skos:inScheme rdf:resource="http://rdaregistry.info/termList/RDATerms"/>
      <reg:status rdf:resource="http://metadataregistry.org/uri/RegStatus/1001"/>
      <reg:identifier rdf:resource="http://metadataregistry.org/concepts/8563"/>
      <skos:prefLabel xml:lang="en">hierarchical description</skos:prefLabel>
      <rdakit:toolkitLabel xml:lang="en">hierarchical description</rdakit:toolkitLabel>
      <skos:definition xml:lang="en">A description that combines a comprehensive description of the whole manifestation with analytical descriptions of one or more of its parts.</skos:definition>
      <rdakit:toolkitDefinition xml:lang="en">A description that combines a comprehensive description of the whole manifestation with analytical descriptions of one or more of its parts.</rdakit:toolkitDefinition>
      <skos:prefLabel xml:lang="it">descrizione gerarchica</skos:prefLabel>
      <rdakit:toolkitLabel xml:lang="it">descrizione gerarchica</rdakit:toolkitLabel>
      <skos:definition xml:lang="it">Descrizione che combina la descrizione comprensiva dell'intera risorsa con le descrizioni analitiche di una o più parti di essa.</skos:definition>
      <rdakit:toolkitDefinition xml:lang="it">Descrizione che combina la descrizione comprensiva dell'intera risorsa con le descrizioni analitiche di una o più parti di essa.</rdakit:toolkitDefinition>
      <skos:prefLabel xml:lang="fr">description hiérarchisée</skos:prefLabel>
      <rdakit:toolkitLabel xml:lang="fr">description hiérarchisée</rdakit:toolkitLabel>
      <skos:definition xml:lang="fr">Description combinant une description globale de la manifestation dans son ensemble et des descriptions analytiques d’une ou plusieurs de ses parties.</skos:definition>
      <rdakit:toolkitDefinition xml:lang="fr">Description combinant une description globale de la manifestation dans son ensemble et des descriptions analytiques d’une ou plusieurs de ses parties.</rdakit:toolkitDefinition>
      <skos:prefLabel xml:lang="es">descripción jerárquica</skos:prefLabel>
      <rdakit:toolkitLabel xml:lang="es">descripción jerárquica</rdakit:toolkitLabel>
      <skos:definition xml:lang="es">Descripción que combina una descripción integral del recurso completo con descripciones analíticas de una o más de sus partes.</skos:definition>
      <rdakit:toolkitDefinition xml:lang="es">Descripción que combina una descripción integral del recurso completo con descripciones analíticas de una o más de sus partes.</rdakit:toolkitDefinition>
      <skos:prefLabel xml:lang="de">Hierarchische Beschreibung</skos:prefLabel>
      <rdakit:toolkitLabel xml:lang="de">Hierarchische Beschreibung</rdakit:toolkitLabel>
      <skos:definition xml:lang="de">Eine Beschreibung, die eine umfassende Beschreibung der ganzen Manifestation mit den analytischen Beschreibungen von einem oder von mehreren ihrer Teile enthält.</skos:definition>
      <rdakit:toolkitDefinition xml:lang="de">Eine Beschreibung, die eine umfassende Beschreibung der ganzen Manifestation mit den analytischen Beschreibungen von einem oder von mehreren ihrer Teile enthält.</rdakit:toolkitDefinition>
      <skos:prefLabel xml:lang="fi">hierarkkinen kuvailu</skos:prefLabel>
      <rdakit:toolkitLabel xml:lang="fi">hierarkkinen kuvailu</rdakit:toolkitLabel>
      <skos:definition xml:lang="fi">Manifestaatiokonaisuuden ja manifestaation yhden tai useamman osan analyyttisen kuvailun yhdistäminen.</skos:definition>
      <rdakit:toolkitDefinition xml:lang="fi">Manifestaatiokonaisuuden ja manifestaation yhden tai useamman osan analyyttisen kuvailun yhdistäminen.</rdakit:toolkitDefinition>
      <skos:prefLabel xml:lang="da">hierarkisk beskrivelse</skos:prefLabel>
      <rdakit:toolkitLabel xml:lang="da">hierarkisk beskrivelse</rdakit:toolkitLabel>
      <skos:definition xml:lang="da">Beskrivelse, der kombinerer en omfattende beskrivelse af hele ressourcen med analytiske beskrivelser af en eller flere af dens dele.</skos:definition>
      <rdakit:toolkitDefinition xml:lang="da">Beskrivelse, der kombinerer en omfattende beskrivelse af hele ressourcen med analytiske beskrivelser af en eller flere af dens dele.</rdakit:toolkitDefinition>
      <skos:prefLabel xml:lang="ca">descripció jeràrquica</skos:prefLabel>
      <rdakit:toolkitLabel xml:lang="ca">descripció jeràrquica</rdakit:toolkitLabel>
      <skos:definition xml:lang="ca">Descripció que combina una descripció completa de tota la manifestació amb descripcions analítiques d’una o més de les seves parts.</skos:definition>
      <rdakit:toolkitDefinition xml:lang="ca">Descripció que combina una descripció completa de tota la manifestació amb descripcions analítiques d’una o més de les seves parts.</rdakit:toolkitDefinition>
      <skos:prefLabel xml:lang="vi">mô tả theo thứ bậc</skos:prefLabel>
      <rdakit:toolkitLabel xml:lang="vi">mô tả theo thứ bậc</rdakit:toolkitLabel>
      <skos:definition xml:lang="vi">Mô tả kết hợp mô tả tổng hợp của toàn bộ tài nguyên với mô tả phân tích của một hoặc nhiều hơn phần của nó.</skos:definition>
      <rdakit:toolkitDefinition xml:lang="vi">Mô tả kết hợp mô tả tổng hợp của toàn bộ tài nguyên với mô tả phân tích của một hoặc nhiều hơn phần của nó.</rdakit:toolkitDefinition>
      <skos:prefLabel xml:lang="no">hierarkisk beskrivelse</skos:prefLabel>
      <rdakit:toolkitLabel xml:lang="no">hierarkisk beskrivelse</rdakit:toolkitLabel>
      <skos:definition xml:lang="no">En beskrivelse som kombinerer en omfattende beskrivelse av hele manifestasjonen med analytiske beskrivelser av én eller flere av manifestasjonens deler.</skos:definition>
      <rdakit:toolkitDefinition xml:lang="no">En beskrivelse som kombinerer en omfattende beskrivelse av hele manifestasjonen med analytiske beskrivelser av én eller flere av manifestasjonens deler.</rdakit:toolkitDefinition>
    </skos:Concept>
<!-- Concept: identifiable subject system  -->
    <skos:Concept rdf:about="http://rdaregistry.info/termList/RDATerms/1049" xml:lang="en">
      <skos:inScheme rdf:resource="http://rdaregistry.info/termList/RDATerms"/>
      <reg:status rdf:resource="http://metadataregistry.org/uri/RegStatus/1001"/>
      <reg:identifier rdf:resource="http://metadataregistry.org/concepts/8564"/>
      <skos:prefLabel xml:lang="en">identifiable subject system</skos:prefLabel>
      <rdakit:toolkitLabel xml:lang="en">identifiable subject system</rdakit:toolkitLabel>
      <skos:definition xml:lang="en">A standard for subject access points and/or classification numbers used in determining the names or terms, other identifying attributes, and relationships representing what a work is about.</skos:definition>
      <rdakit:toolkitDefinition xml:lang="en">A standard for subject access points and/or classification numbers used in determining the names or terms, other identifying attributes, and relationships representing what a work is about.</rdakit:toolkitDefinition>
      <skos:scopeNote xml:lang="en">An identifiable subject system includes rules for application of terms, systematic combination of terminology such as pre- or post-coordination, and guidelines on cardinality and depth of assignment.</skos:scopeNote>
      <skos:prefLabel xml:lang="fi">aihetta identifioiva käsitejärjestelmä</skos:prefLabel>
      <rdakit:toolkitLabel xml:lang="fi">aihetta identifioiva käsitejärjestelmä</rdakit:toolkitLabel>
      <skos:definition xml:lang="fi">Järjestelmä, jota kuvaileva yhteisö käyttää aiheeseen liittyvien hakutietojen ja/tai luokituskaavion luokkien merkitsemiseen.</skos:definition>
      <rdakit:toolkitDefinition xml:lang="fi">Järjestelmä, jota kuvaileva yhteisö käyttää aiheeseen liittyvien hakutietojen ja/tai luokituskaavion luokkien merkitsemiseen.</rdakit:toolkitDefinition>
      <skos:scopeNote xml:lang="fi">Sitä voidaan käyttää määrittämään terminologiaa, muita identifioivia attribuutteja ja teoksen aihetta. Se voi myös sisältää termien soveltamista ja yhdistämistä koskevia ohjeita (esim. etuliite) ja suosituksia periaatteista ja tarkkuuden tasosta.</skos:scopeNote>
      <skos:prefLabel xml:lang="de">Belegbares Inhaltserschließungssystem</skos:prefLabel>
      <rdakit:toolkitLabel xml:lang="de">Belegbares Inhaltserschließungssystem</rdakit:toolkitLabel>
      <skos:definition xml:lang="de">Ein Standard für Themensucheinstiege und/oder Notationen, der verwendet wird, um die Benennungen, Termini oder sonstige identifizierbare Merkmale und Beziehungen zu bestimmen, die das Thema eines Werks repräsentieren.</skos:definition>
      <rdakit:toolkitDefinition xml:lang="de">Ein Standard für Themensucheinstiege und/oder Notationen, der verwendet wird, um die Benennungen, Termini oder sonstige identifizierbare Merkmale und Beziehungen zu bestimmen, die das Thema eines Werks repräsentieren.</rdakit:toolkitDefinition>
      <skos:scopeNote xml:lang="de">Ein belegbares Inhaltserschließungssystem beinhaltet Regeln zur Anwendung von Termini, systematische Kombinationen von Terminologie (z. B. Prä- oder Postkoordination) und Richtlinien zur Kardinalität und zur Tiefe der Vergabe.</skos:scopeNote>
      <skos:prefLabel xml:lang="da">identificerbart emnesystem</skos:prefLabel>
      <rdakit:toolkitLabel xml:lang="da">identificerbart emnesystem</rdakit:toolkitLabel>
      <skos:definition xml:lang="da">Standard for emnesøgeindgange og/eller klassifikationstal, der anvendes til at fastlægge navne eller termer, andre identificerende attributter og relationer, der angiver, hvad et værk handler om.</skos:definition>
      <rdakit:toolkitDefinition xml:lang="da">Standard for emnesøgeindgange og/eller klassifikationstal, der anvendes til at fastlægge navne eller termer, andre identificerende attributter og relationer, der angiver, hvad et værk handler om.</rdakit:toolkitDefinition>
      <skos:scopeNote xml:lang="da">Et identificerbart emnesystem omfatter regler for brug af termer, systematisk terminologikombination, som fx præ- eller postkoordingering, samt vejledning om tildelning.</skos:scopeNote>
      <skos:prefLabel xml:lang="ca">sistema de matèries identificable</skos:prefLabel>
      <rdakit:toolkitLabel xml:lang="ca">sistema de matèries identificable</rdakit:toolkitLabel>
      <skos:definition xml:lang="ca">Estàndard de punts d’accés de matèries i/o de números de classificació usat per determinar els noms o els termes, els altres atributs identificadors i les relacions que representen de què tracta una obra.</skos:definition>
      <rdakit:toolkitDefinition xml:lang="ca">Estàndard de punts d’accés de matèries i/o de números de classificació usat per determinar els noms o els termes, els altres atributs identificadors i les relacions que representen de què tracta una obra.</rdakit:toolkitDefinition>
      <skos:scopeNote xml:lang="ca">Un sistema de matèries identificable inclou regles per a l’aplicació dels termes, la combinació sistemàtica de terminologia com ara la precoordinació o la postcoordinació, i les directrius sobre la cardinalitat i la profunditat de l’assignació.</skos:scopeNote>
      <skos:prefLabel xml:lang="fr">système d’analyse documentaire identifiable</skos:prefLabel>
      <rdakit:toolkitLabel xml:lang="fr">système d’analyse documentaire identifiable</rdakit:toolkitLabel>
      <skos:definition xml:lang="fr">Norme applicable aux points d’accès matière et/ou aux indices de classification, utilisée pour déterminer les noms ou les termes, les autres attributs d’identification ainsi que les relations représentant ce dont traite une œuvre.</skos:definition>
      <rdakit:toolkitDefinition xml:lang="fr">Norme applicable aux points d’accès matière et/ou aux indices de classification, utilisée pour déterminer les noms ou les termes, les autres attributs d’identification ainsi que les relations représentant ce dont traite une œuvre.</rdakit:toolkitDefinition>
      <skos:scopeNote xml:lang="fr">Un système d’analyse documentaire identifiable comprend des règles d’application des termes, la combinaison systématique de la terminologie, telles la précoordination ou la postcoordination, ainsi que des lignes directrices sur la cardinalité et la profondeur de l’attribution.</skos:scopeNote>
      <skos:prefLabel xml:lang="vi">hệ thống chủ đề nhận dạng</skos:prefLabel>
      <rdakit:toolkitLabel xml:lang="vi">hệ thống chủ đề nhận dạng</rdakit:toolkitLabel>
      <skos:definition xml:lang="vi">Một chuẩn của điểm truy cập chủ đề và/hoặc chỉ số phân loại được một cơ quan sử dụng để tạo lập dữ liệu. Nó có thể được sử dụng để xác định tên hoặc thuật ngữ, các thuộc tính nhận dạng khác, và mối quan hệ trình bày tác phẩm nói về cái gì.</skos:definition>
      <rdakit:toolkitDefinition xml:lang="vi">Một chuẩn của điểm truy cập chủ đề và/hoặc chỉ số phân loại được một cơ quan sử dụng để tạo lập dữ liệu. Nó có thể được sử dụng để xác định tên hoặc thuật ngữ, các thuộc tính nhận dạng khác, và mối quan hệ trình bày tác phẩm nói về cái gì.</rdakit:toolkitDefinition>
      <skos:scopeNote xml:lang="vi">hệ thống chủ đề nhận dạng có thể cũng bao gồm các quy tắc để áp dụng thuật ngữ, kết hợp có hệ thống các thuật ngữ (ví dụ, tiền kết hợp và hậu kết hợp), và chỉ dẫn về số các yếu tố và độ sâu trong xử lý.</skos:scopeNote>
      <skos:prefLabel xml:lang="no">identifiserbart emnesystem</skos:prefLabel>
      <rdakit:toolkitLabel xml:lang="no">identifiserbart emnesystem</rdakit:toolkitLabel>
      <skos:definition xml:lang="no">En standard for emneinnførsler og/eller klassifikasjonsnumre som brukes for å bestemme navn eller termer, andre identifiserende attributter/egenskaper og relasjoner som representerer verkets innhold.</skos:definition>
      <rdakit:toolkitDefinition xml:lang="no">En standard for emneinnførsler og/eller klassifikasjonsnumre som brukes for å bestemme navn eller termer, andre identifiserende attributter/egenskaper og relasjoner som representerer verkets innhold.</rdakit:toolkitDefinition>
      <skos:scopeNote xml:lang="no">Et identifiserbart emnesystem kan også omfatte regler for bruk av termene, systematisk kombinasjon av terminologi (f.eks. pre- eller postkoordinering) og retningslinjer for sammenhengen mellom to grupper data og grad av spesifisitet.</skos:scopeNote>
    </skos:Concept>
<!-- Concept: image description  -->
    <skos:Concept rdf:about="http://rdaregistry.info/termList/RDATerms/1050" xml:lang="en">
      <skos:inScheme rdf:resource="http://rdaregistry.info/termList/RDATerms"/>
      <reg:status rdf:resource="http://metadataregistry.org/uri/RegStatus/1001"/>
      <reg:identifier rdf:resource="http://metadataregistry.org/concepts/8565"/>
      <skos:prefLabel xml:lang="en">image description</skos:prefLabel>
      <rdakit:toolkitLabel xml:lang="en">image description</rdakit:toolkitLabel>
      <skos:definition xml:lang="en">A descriptive audio or tactile language text that is attached to, or supplied with, a tactile image, map or diagram.</skos:definition>
      <rdakit:toolkitDefinition xml:lang="en">A descriptive audio or tactile language text that is attached to, or supplied with, a tactile image, map or diagram.</rdakit:toolkitDefinition>
      <skos:prefLabel xml:lang="it">descrizione dell'immagine</skos:prefLabel>
      <rdakit:toolkitLabel xml:lang="it">descrizione dell'immagine</rdakit:toolkitLabel>
      <skos:definition xml:lang="it">Testo descrittivo audio o in linguaggio tattile allegato o fornito insieme a un'immagine, una carta geografica o un diagramma tattile.</skos:definition>
      <rdakit:toolkitDefinition xml:lang="it">Testo descrittivo audio o in linguaggio tattile allegato o fornito insieme a un'immagine, una carta geografica o un diagramma tattile.</rdakit:toolkitDefinition>
      <skos:prefLabel xml:lang="fr">description d’image</skos:prefLabel>
      <rdakit:toolkitLabel xml:lang="fr">description d’image</rdakit:toolkitLabel>
      <skos:definition xml:lang="fr">Texte descriptif audio ou tactile qui est joint à, ou fourni avec, une image, une carte ou un diagramme tactiles.</skos:definition>
      <rdakit:toolkitDefinition xml:lang="fr">Texte descriptif audio ou tactile qui est joint à, ou fourni avec, une image, une carte ou un diagramme tactiles.</rdakit:toolkitDefinition>
      <skos:prefLabel xml:lang="de">Bildbeschreibung</skos:prefLabel>
      <rdakit:toolkitLabel xml:lang="de">Bildbeschreibung</rdakit:toolkitLabel>
      <skos:definition xml:lang="de">Ein beschreibender hörbarer oder taktiler Text, der einem taktilen Bild, einer taktilen Karte oder einem taktilen Diagramm beigefügt ist oder damit geliefert wird.</skos:definition>
      <rdakit:toolkitDefinition xml:lang="de">Ein beschreibender hörbarer oder taktiler Text, der einem taktilen Bild, einer taktilen Karte oder einem taktilen Diagramm beigefügt ist oder damit geliefert wird.</rdakit:toolkitDefinition>
      <skos:prefLabel xml:lang="fi">kuvaselostus</skos:prefLabel>
      <rdakit:toolkitLabel xml:lang="fi">kuvaselostus</rdakit:toolkitLabel>
      <skos:definition xml:lang="fi">Kuvaileva kuunneltava tai tuntoaistilla havaittava teksti joka liittyy tai toimitetaan yhdessä taktiilin kuvan, kartan tai diagrammin kanssa.</skos:definition>
      <rdakit:toolkitDefinition xml:lang="fi">Kuvaileva kuunneltava tai tuntoaistilla havaittava teksti joka liittyy tai toimitetaan yhdessä taktiilin kuvan, kartan tai diagrammin kanssa.</rdakit:toolkitDefinition>
      <skos:prefLabel xml:lang="da">billedbeskrivelse</skos:prefLabel>
      <rdakit:toolkitLabel xml:lang="da">billedbeskrivelse</rdakit:toolkitLabel>
      <skos:definition xml:lang="da">Beskrivende lyd- eller taktil tekst, der sidder på, eller leveres med, et taktilt billede, kort eller diagram.</skos:definition>
      <rdakit:toolkitDefinition xml:lang="da">Beskrivende lyd- eller taktil tekst, der sidder på, eller leveres med, et taktilt billede, kort eller diagram.</rdakit:toolkitDefinition>
      <skos:prefLabel xml:lang="ca">descripció d’imatge</skos:prefLabel>
      <rdakit:toolkitLabel xml:lang="ca">descripció d’imatge</rdakit:toolkitLabel>
      <skos:definition xml:lang="ca">Text descriptiu àudio o tàctil que va lligat a, o es proporciona amb, una imatge, un mapa o un diagrama tàctils.</skos:definition>
      <rdakit:toolkitDefinition xml:lang="ca">Text descriptiu àudio o tàctil que va lligat a, o es proporciona amb, una imatge, un mapa o un diagrama tàctils.</rdakit:toolkitDefinition>
      <skos:prefLabel xml:lang="vi">mô tả hình ảnh</skos:prefLabel>
      <rdakit:toolkitLabel xml:lang="vi">mô tả hình ảnh</rdakit:toolkitLabel>
      <skos:definition xml:lang="vi">Mô tả audio hoặc văn bản ngôn ngữ xúc giác gắn liền với, hoặc được cung cấp cùng với, hình ảnh xúc giác, bản đồ hoặc đồ hình.</skos:definition>
      <rdakit:toolkitDefinition xml:lang="vi">Mô tả audio hoặc văn bản ngôn ngữ xúc giác gắn liền với, hoặc được cung cấp cùng với, hình ảnh xúc giác, bản đồ hoặc đồ hình.</rdakit:toolkitDefinition>
      <skos:prefLabel xml:lang="no">beskrivelse av bilde</skos:prefLabel>
      <rdakit:toolkitLabel xml:lang="no">beskrivelse av bilde</rdakit:toolkitLabel>
      <skos:definition xml:lang="no">En beskrivende lyd eller taktil, språklig tekst som er tilknyttet, eller supplert med, et taktilt bilde, kart eller diagram.</skos:definition>
      <rdakit:toolkitDefinition xml:lang="no">En beskrivende lyd eller taktil, språklig tekst som er tilknyttet, eller supplert med, et taktilt bilde, kart eller diagram.</rdakit:toolkitDefinition>
    </skos:Concept>
<!-- Concept: international intergovernmental body  -->
    <skos:Concept rdf:about="http://rdaregistry.info/termList/RDATerms/1051" xml:lang="en">
      <skos:inScheme rdf:resource="http://rdaregistry.info/termList/RDATerms"/>
      <reg:status rdf:resource="http://metadataregistry.org/uri/RegStatus/1001"/>
      <reg:identifier rdf:resource="http://metadataregistry.org/concepts/8566"/>
      <skos:prefLabel xml:lang="en">international intergovernmental body</skos:prefLabel>
      <rdakit:toolkitLabel xml:lang="en">international intergovernmental body</rdakit:toolkitLabel>
      <skos:definition xml:lang="en">An international body created by intergovernmental action.</skos:definition>
      <rdakit:toolkitDefinition xml:lang="en">An international body created by intergovernmental action.</rdakit:toolkitDefinition>
      <skos:prefLabel xml:lang="it">ente intergovernativo internazionale</skos:prefLabel>
      <rdakit:toolkitLabel xml:lang="it">ente intergovernativo internazionale</rdakit:toolkitLabel>
      <skos:definition xml:lang="it">Un ente internazionale creato per iniziativa intergovernativa.</skos:definition>
      <rdakit:toolkitDefinition xml:lang="it">Un ente internazionale creato per iniziativa intergovernativa.</rdakit:toolkitDefinition>
      <skos:prefLabel xml:lang="de">Internationale zwischenstaatliche Körperschaft</skos:prefLabel>
      <rdakit:toolkitLabel xml:lang="de">Internationale zwischenstaatliche Körperschaft</rdakit:toolkitLabel>
      <skos:definition xml:lang="de">Eine internationale Körperschaft, die durch zwischenstaatliches Handeln ins Leben gerufen wird.</skos:definition>
      <rdakit:toolkitDefinition xml:lang="de">Eine internationale Körperschaft, die durch zwischenstaatliches Handeln ins Leben gerufen wird.</rdakit:toolkitDefinition>
      <skos:prefLabel xml:lang="fi">kansainvälinen hallitustenvälinen yhteisö</skos:prefLabel>
      <rdakit:toolkitLabel xml:lang="fi">kansainvälinen hallitustenvälinen yhteisö</rdakit:toolkitLabel>
      <skos:definition xml:lang="fi">Hallitustenvälisen toiminnan tuloksena syntynyt kansainvälinen yhteisö.</skos:definition>
      <rdakit:toolkitDefinition xml:lang="fi">Hallitustenvälisen toiminnan tuloksena syntynyt kansainvälinen yhteisö.</rdakit:toolkitDefinition>
      <skos:prefLabel xml:lang="da">internationalt mellemstatsligt organ</skos:prefLabel>
      <rdakit:toolkitLabel xml:lang="da">internationalt mellemstatsligt organ</rdakit:toolkitLabel>
      <skos:definition xml:lang="da">Internationalt organ skabt ved en mellemstatslig handling.</skos:definition>
      <rdakit:toolkitDefinition xml:lang="da">Internationalt organ skabt ved en mellemstatslig handling.</rdakit:toolkitDefinition>
      <skos:prefLabel xml:lang="ca">organització internacional intergovernamental</skos:prefLabel>
      <rdakit:toolkitLabel xml:lang="ca">organització internacional intergovernamental</rdakit:toolkitLabel>
      <skos:definition xml:lang="ca">Entitat internacional creada per decisió intergovernamental.</skos:definition>
      <rdakit:toolkitDefinition xml:lang="ca">Entitat internacional creada per decisió intergovernamental.</rdakit:toolkitDefinition>
      <skos:prefLabel xml:lang="fr">organisation internationale intergouvernementale</skos:prefLabel>
      <rdakit:toolkitLabel xml:lang="fr">organisation internationale intergouvernementale</rdakit:toolkitLabel>
      <skos:definition xml:lang="fr">Organisation internationale créée par décision intergouvernementale.</skos:definition>
      <rdakit:toolkitDefinition xml:lang="fr">Organisation internationale créée par décision intergouvernementale.</rdakit:toolkitDefinition>
      <skos:prefLabel xml:lang="vi">cơ quan liên chính phủ quốc tế</skos:prefLabel>
      <rdakit:toolkitLabel xml:lang="vi">cơ quan liên chính phủ quốc tế</rdakit:toolkitLabel>
      <skos:definition xml:lang="vi">Cơ quan quốc tế được tạo ra theo hoạt động liên chính phủ.</skos:definition>
      <rdakit:toolkitDefinition xml:lang="vi">Cơ quan quốc tế được tạo ra theo hoạt động liên chính phủ.</rdakit:toolkitDefinition>
      <skos:prefLabel xml:lang="no">internasjonal, mellomstatlig organisasjon</skos:prefLabel>
      <rdakit:toolkitLabel xml:lang="no">internasjonal, mellomstatlig organisasjon</rdakit:toolkitLabel>
      <skos:definition xml:lang="no">Et internasjonalt organ opprettet på initiativ av flere stater.</skos:definition>
      <rdakit:toolkitDefinition xml:lang="no">Et internasjonalt organ opprettet på initiativ av flere stater.</rdakit:toolkitDefinition>
    </skos:Concept>
<!-- Concept: issue  -->
    <skos:Concept rdf:about="http://rdaregistry.info/termList/RDATerms/1052" xml:lang="en">
      <skos:inScheme rdf:resource="http://rdaregistry.info/termList/RDATerms"/>
      <reg:status rdf:resource="http://metadataregistry.org/uri/RegStatus/1001"/>
      <reg:identifier rdf:resource="http://metadataregistry.org/concepts/8567"/>
      <skos:prefLabel xml:lang="en">issue</skos:prefLabel>
      <rdakit:toolkitLabel xml:lang="en">issue</rdakit:toolkitLabel>
      <skos:definition xml:lang="en">A successive part of a serial.</skos:definition>
      <rdakit:toolkitDefinition xml:lang="en">A successive part of a serial.</rdakit:toolkitDefinition>
	    <skos:related rdf:resource="http://rdaregistry.info/termList/RDATerms/1065"/>
      <skos:prefLabel xml:lang="de">Ausgabe</skos:prefLabel>
      <rdakit:toolkitLabel xml:lang="de">Ausgabe</rdakit:toolkitLabel>
      <skos:definition xml:lang="de">Einer von aufeinander folgenden Teilen einer fortlaufenden Ressource.</skos:definition>
      <rdakit:toolkitDefinition xml:lang="de">Einer von aufeinander folgenden Teilen einer fortlaufenden Ressource.</rdakit:toolkitDefinition>
      <skos:prefLabel xml:lang="fi">sarjan osa</skos:prefLabel>
      <rdakit:toolkitLabel xml:lang="fi">sarjan osa</rdakit:toolkitLabel>
      <skos:definition xml:lang="fi">Yksi sarjan peräkkäisistä osista.</skos:definition>
      <rdakit:toolkitDefinition xml:lang="fi">Yksi sarjan peräkkäisistä osista.</rdakit:toolkitDefinition>
      <skos:prefLabel xml:lang="da">nummer</skos:prefLabel>
      <rdakit:toolkitLabel xml:lang="da">nummer</rdakit:toolkitLabel>
      <skos:definition xml:lang="da">En successiv del af et periodikum.</skos:definition>
      <rdakit:toolkitDefinition xml:lang="da">En successiv del af et periodikum.</rdakit:toolkitDefinition>
      <skos:prefLabel xml:lang="ca">número</skos:prefLabel>
      <rdakit:toolkitLabel xml:lang="ca">número</rdakit:toolkitLabel>
      <skos:definition xml:lang="ca">Una de les parts successives d’una publicació en sèrie.</skos:definition>
      <rdakit:toolkitDefinition xml:lang="ca">Una de les parts successives d’una publicació en sèrie.</rdakit:toolkitDefinition>
      <skos:prefLabel xml:lang="fr">livraison</skos:prefLabel>
      <rdakit:toolkitLabel xml:lang="fr">livraison</rdakit:toolkitLabel>
      <skos:definition xml:lang="fr">Partie successive d’une publication en série.</skos:definition>
      <rdakit:toolkitDefinition xml:lang="fr">Partie successive d’une publication en série.</rdakit:toolkitDefinition>
      <skos:prefLabel xml:lang="vi">số</skos:prefLabel>
      <rdakit:toolkitLabel xml:lang="vi">số</rdakit:toolkitLabel>
      <skos:definition xml:lang="vi">Một phần kế tiếp của một ấm phẩm nhiều kỳ.</skos:definition>
      <rdakit:toolkitDefinition xml:lang="vi">Một phần kế tiếp của một ấm phẩm nhiều kỳ.</rdakit:toolkitDefinition>
      <skos:prefLabel xml:lang="no">hefte</skos:prefLabel>
      <rdakit:toolkitLabel xml:lang="no">hefte</rdakit:toolkitLabel>
      <skos:definition xml:lang="no">En påfølgende del av et periodikum.</skos:definition>
      <rdakit:toolkitDefinition xml:lang="no">En påfølgende del av et periodikum.</rdakit:toolkitDefinition>
    </skos:Concept>
<!-- Concept: iteration  -->
    <skos:Concept rdf:about="http://rdaregistry.info/termList/RDATerms/1053" xml:lang="en">
      <skos:inScheme rdf:resource="http://rdaregistry.info/termList/RDATerms"/>
      <reg:status rdf:resource="http://metadataregistry.org/uri/RegStatus/1001"/>
      <reg:identifier rdf:resource="http://metadataregistry.org/concepts/8568"/>
      <skos:prefLabel xml:lang="en">iteration</skos:prefLabel>
      <rdakit:toolkitLabel xml:lang="en">iteration</rdakit:toolkitLabel>
      <skos:definition xml:lang="en">An instance of an integrating resource, either as first released or after it has been updated.</skos:definition>
      <rdakit:toolkitDefinition xml:lang="en">An instance of an integrating resource, either as first released or after it has been updated.</rdakit:toolkitDefinition>
      <skos:prefLabel xml:lang="it">iterazione</skos:prefLabel>
      <rdakit:toolkitLabel xml:lang="it">iterazione</rdakit:toolkitLabel>
      <skos:definition xml:lang="it">Istanza di una risorsa integrativa, così come rilasciata la prima volta o dopo un aggiornamento.</skos:definition>
      <rdakit:toolkitDefinition xml:lang="it">Istanza di una risorsa integrativa, così come rilasciata la prima volta o dopo un aggiornamento.</rdakit:toolkitDefinition>
      <skos:prefLabel xml:lang="fr">itération</skos:prefLabel>
      <rdakit:toolkitLabel xml:lang="fr">itération</rdakit:toolkitLabel>
      <skos:definition xml:lang="fr">Instance d’une ressource intégratrice, soit lors de sa première mise à disposition soit après une mise à jour.</skos:definition>
      <rdakit:toolkitDefinition xml:lang="fr">Instance d’une ressource intégratrice, soit lors de sa première mise à disposition soit après une mise à jour.</rdakit:toolkitDefinition>
      <skos:prefLabel xml:lang="de">Iteration</skos:prefLabel>
      <rdakit:toolkitLabel xml:lang="de">Iteration</rdakit:toolkitLabel>
      <skos:definition xml:lang="de">Eine Instanz einer integrierenden Ressource, entweder so wie sie ursprünglich erschienen ist oder nachdem sie aktualisiert wurde.</skos:definition>
      <rdakit:toolkitDefinition xml:lang="de">Eine Instanz einer integrierenden Ressource, entweder so wie sie ursprünglich erschienen ist oder nachdem sie aktualisiert wurde.</rdakit:toolkitDefinition>
      <skos:prefLabel xml:lang="fi">iteraatio</skos:prefLabel>
      <rdakit:toolkitLabel xml:lang="fi">iteraatio</rdakit:toolkitLabel>
      <skos:definition xml:lang="fi">Yksi päivittyvän aineiston versio, joko julkaistaessa se ensi kertaa tai päivityksen jälkeen.</skos:definition>
      <rdakit:toolkitDefinition xml:lang="fi">Yksi päivittyvän aineiston versio, joko julkaistaessa se ensi kertaa tai päivityksen jälkeen.</rdakit:toolkitDefinition>
      <skos:prefLabel xml:lang="da">iteration</skos:prefLabel>
      <rdakit:toolkitLabel xml:lang="da">iteration</rdakit:toolkitLabel>
      <skos:definition xml:lang="da">En forekomst af en integrerende ressource, enten som den først er udgivet, eller efterfølgende opdateret.</skos:definition>
      <rdakit:toolkitDefinition xml:lang="da">En forekomst af en integrerende ressource, enten som den først er udgivet, eller efterfølgende opdateret.</rdakit:toolkitDefinition>
      <skos:prefLabel xml:lang="ca">iteració</skos:prefLabel>
      <rdakit:toolkitLabel xml:lang="ca">iteració</rdakit:toolkitLabel>
      <skos:definition xml:lang="ca">Ocurrència d’un recurs integrant, o bé com a primera emissió o després d’una actualització.</skos:definition>
      <rdakit:toolkitDefinition xml:lang="ca">Ocurrència d’un recurs integrant, o bé com a primera emissió o després d’una actualització.</rdakit:toolkitDefinition>
      <skos:prefLabel xml:lang="vi">lần lặp</skos:prefLabel>
      <rdakit:toolkitLabel xml:lang="vi">lần lặp</rdakit:toolkitLabel>
      <skos:definition xml:lang="vi">Trường hợp của một tài nguyên tích hợp, hoặc là lưu hành lần đầu hoặc là sau khi cập nhật.</skos:definition>
      <rdakit:toolkitDefinition xml:lang="vi">Trường hợp của một tài nguyên tích hợp, hoặc là lưu hành lần đầu hoặc là sau khi cập nhật.</rdakit:toolkitDefinition>
      <skos:prefLabel xml:lang="no">versjon (integrerende ressurs)</skos:prefLabel>
      <rdakit:toolkitLabel xml:lang="no">versjon (integrerende ressurs)</rdakit:toolkitLabel>
      <skos:definition xml:lang="no">En &quot;utgave&quot; av en integrerende ressurs, enten som den først ble utgitt, eller etter at den er blitt oppdatert.</skos:definition>
      <rdakit:toolkitDefinition xml:lang="no">En &quot;utgave&quot; av en integrerende ressurs, enten som den først ble utgitt, eller etter at den er blitt oppdatert.</rdakit:toolkitDefinition>
    </skos:Concept>
<!-- Concept: jacket  -->
    <skos:Concept rdf:about="http://rdaregistry.info/termList/RDATerms/1054" xml:lang="en">
      <skos:inScheme rdf:resource="http://rdaregistry.info/termList/RDATerms"/>
      <reg:status rdf:resource="http://metadataregistry.org/uri/RegStatus/1001"/>
      <reg:identifier rdf:resource="http://metadataregistry.org/concepts/8569"/>
      <skos:prefLabel xml:lang="en">jacket</skos:prefLabel>
      <skos:altLabel xml:lang="en">book jacket</skos:altLabel>
      <rdakit:toolkitLabel xml:lang="en">jacket</rdakit:toolkitLabel>
      <skos:definition xml:lang="en">A detachable, protective wrapping of a volume, issued as part of a manifestation by a publisher, etc.</skos:definition>
      <rdakit:toolkitDefinition xml:lang="en">A detachable, protective wrapping of a volume, issued as part of a manifestation by a publisher, etc.</rdakit:toolkitDefinition>
	    <skos:broader rdf:resource="http://rdaregistry.info/termList/RDATerms/1026"/>
      <skos:prefLabel xml:lang="it">sovraccoperta</skos:prefLabel>
      <rdakit:toolkitLabel xml:lang="it">sovraccoperta</rdakit:toolkitLabel>
      <skos:definition xml:lang="it">La copertura protettiva e staccabile di un volume, pubblicata come parte della risorsa da un editore.</skos:definition>
      <rdakit:toolkitDefinition xml:lang="it">La copertura protettiva e staccabile di un volume, pubblicata come parte della risorsa da un editore.</rdakit:toolkitDefinition>
      <skos:prefLabel xml:lang="fr">jaquette</skos:prefLabel>
      <skos:altLabel xml:lang="fr">couvre-livre</skos:altLabel>
      <rdakit:toolkitLabel xml:lang="fr">jaquette</rdakit:toolkitLabel>
      <skos:definition xml:lang="fr">Chemise de protection amovible d’un volume, distribuée comme faisant partie intégrante d’une manifestation par un éditeur, etc.</skos:definition>
      <rdakit:toolkitDefinition xml:lang="fr">Chemise de protection amovible d’un volume, distribuée comme faisant partie intégrante d’une manifestation par un éditeur, etc.</rdakit:toolkitDefinition>
      <skos:prefLabel xml:lang="de">Schutzumschlag</skos:prefLabel>
      <skos:altLabel xml:lang="de">Buchumschlag</skos:altLabel>
      <rdakit:toolkitLabel xml:lang="de">Schutzumschlag</rdakit:toolkitLabel>
      <skos:definition xml:lang="de">Die abnehmbare, schützende Hülle eines Bandes, der als Teil der Manifestation vom Verlag usw. herausgegeben wird.</skos:definition>
      <rdakit:toolkitDefinition xml:lang="de">Die abnehmbare, schützende Hülle eines Bandes, der als Teil der Manifestation vom Verlag usw. herausgegeben wird.</rdakit:toolkitDefinition>
      <skos:altLabel xml:lang="de">Schmutzumschlag</skos:altLabel>
      <skos:prefLabel xml:lang="fi">irtopäällys</skos:prefLabel>
      <rdakit:toolkitLabel xml:lang="fi">irtopäällys</rdakit:toolkitLabel>
      <skos:definition xml:lang="fi">Niteen irrotettava suojaava kääre, joka julkaistaan manifestaation osana.</skos:definition>
      <rdakit:toolkitDefinition xml:lang="fi">Niteen irrotettava suojaava kääre, joka julkaistaan manifestaation osana.</rdakit:toolkitDefinition>
      <skos:prefLabel xml:lang="da">smudsomslag</skos:prefLabel>
      <rdakit:toolkitLabel xml:lang="da">smudsomslag</rdakit:toolkitLabel>
      <skos:definition xml:lang="da">Aftageligt, beskyttende omslag til et bind, leveret af en udgiver etc. som en del af manfestationen.</skos:definition>
      <rdakit:toolkitDefinition xml:lang="da">Aftageligt, beskyttende omslag til et bind, leveret af en udgiver etc. som en del af manfestationen.</rdakit:toolkitDefinition>
      <skos:prefLabel xml:lang="ca">sobrecoberta</skos:prefLabel>
      <rdakit:toolkitLabel xml:lang="ca">sobrecoberta</rdakit:toolkitLabel>
      <skos:definition xml:lang="ca">Embolcall separable i protector d’un volum, publicat com a part d’una manifestació per un editor, etc.</skos:definition>
      <rdakit:toolkitDefinition xml:lang="ca">Embolcall separable i protector d’un volum, publicat com a part d’una manifestació per un editor, etc.</rdakit:toolkitDefinition>
      <skos:prefLabel xml:lang="vi">áo sách</skos:prefLabel>
      <rdakit:toolkitLabel xml:lang="vi">áo sách</rdakit:toolkitLabel>
      <skos:definition xml:lang="vi">Vật bao bọc bảo vệ, có thể tháo rời của tập tài liệu, được nhà xuất bản, v.v... công bố như là phần của biểu thị.</skos:definition>
      <rdakit:toolkitDefinition xml:lang="vi">Vật bao bọc bảo vệ, có thể tháo rời của tập tài liệu, được nhà xuất bản, v.v... công bố như là phần của biểu thị.</rdakit:toolkitDefinition>
      <skos:prefLabel xml:lang="no">løst omslag</skos:prefLabel>
      <skos:altLabel xml:lang="no">bokomslag</skos:altLabel>
      <rdakit:toolkitLabel xml:lang="no">løst omslag</rdakit:toolkitLabel>
      <skos:definition xml:lang="no">Et løst og beskyttende blad rundt en bok, utgitt som en del av en manifestasjon.</skos:definition>
      <rdakit:toolkitDefinition xml:lang="no">Et løst og beskyttende blad rundt en bok, utgitt som en del av en manifestasjon.</rdakit:toolkitDefinition>
    </skos:Concept>
<!-- Concept: logical unit  -->
    <skos:Concept rdf:about="http://rdaregistry.info/termList/RDATerms/1055" xml:lang="en">
      <skos:inScheme rdf:resource="http://rdaregistry.info/termList/RDATerms"/>
      <reg:status rdf:resource="http://metadataregistry.org/uri/RegStatus/1001"/>
      <reg:identifier rdf:resource="http://metadataregistry.org/concepts/8570"/>
      <skos:prefLabel xml:lang="en">logical unit</skos:prefLabel>
      <rdakit:toolkitLabel xml:lang="en">logical unit</rdakit:toolkitLabel>
      <skos:definition xml:lang="en">A constituent of an intangible manifestation.</skos:definition>
      <rdakit:toolkitDefinition xml:lang="en">A constituent of an intangible manifestation.</rdakit:toolkitDefinition>
      <skos:scopeNote xml:lang="en">A digital file is included.</skos:scopeNote>
      <skos:prefLabel xml:lang="it">unità logica</skos:prefLabel>
      <rdakit:toolkitLabel xml:lang="it">unità logica</rdakit:toolkitLabel>
      <skos:definition xml:lang="it">Componente di una risorsa intangibile.</skos:definition>
      <rdakit:toolkitDefinition xml:lang="it">Componente di una risorsa intangibile.</rdakit:toolkitDefinition>
      <skos:prefLabel xml:lang="fr">unité logique</skos:prefLabel>
      <rdakit:toolkitLabel xml:lang="fr">unité logique</rdakit:toolkitLabel>
      <skos:definition xml:lang="fr">Partie constituante d’une manifestation immatérielle.</skos:definition>
      <rdakit:toolkitDefinition xml:lang="fr">Partie constituante d’une manifestation immatérielle.</rdakit:toolkitDefinition>
      <skos:prefLabel xml:lang="es">unidad lógica</skos:prefLabel>
      <rdakit:toolkitLabel xml:lang="es">unidad lógica</rdakit:toolkitLabel>
      <skos:definition xml:lang="es">Componente de un recurso intangible, tal como un archivo digital.</skos:definition>
      <rdakit:toolkitDefinition xml:lang="es">Componente de un recurso intangible, tal como un archivo digital.</rdakit:toolkitDefinition>
      <skos:prefLabel xml:lang="de">Logische Einheit</skos:prefLabel>
      <rdakit:toolkitLabel xml:lang="de">Logische Einheit</rdakit:toolkitLabel>
      <skos:definition xml:lang="de">Ein Bestandteil einer nicht anfassbaren Einheit.</skos:definition>
      <rdakit:toolkitDefinition xml:lang="de">Ein Bestandteil einer nicht anfassbaren Einheit.</rdakit:toolkitDefinition>
      <skos:scopeNote xml:lang="de">Dazu gehört eine Datei.</skos:scopeNote>
      <skos:prefLabel xml:lang="fi">looginen kokonaisuus</skos:prefLabel>
      <rdakit:toolkitLabel xml:lang="fi">looginen kokonaisuus</rdakit:toolkitLabel>
      <skos:definition xml:lang="fi">Aineettoman manifestaation rakenneosa.</skos:definition>
      <rdakit:toolkitDefinition xml:lang="fi">Aineettoman manifestaation rakenneosa.</rdakit:toolkitDefinition>
      <skos:scopeNote xml:lang="fi">Käsittää myös digitaalisen tiedoston.</skos:scopeNote>
      <skos:prefLabel xml:lang="da">logisk enhed</skos:prefLabel>
      <rdakit:toolkitLabel xml:lang="da">logisk enhed</rdakit:toolkitLabel>
      <skos:definition xml:lang="da">Del af en ikke-fysisk ressource.</skos:definition>
      <rdakit:toolkitDefinition xml:lang="da">Del af en ikke-fysisk ressource.</rdakit:toolkitDefinition>
      <skos:scopeNote xml:lang="da">En digital fil er omfattet.</skos:scopeNote>
      <skos:prefLabel xml:lang="ca">unitat lògica</skos:prefLabel>
      <rdakit:toolkitLabel xml:lang="ca">unitat lògica</rdakit:toolkitLabel>
      <skos:definition xml:lang="ca">Component d’un recurs intangible.</skos:definition>
      <rdakit:toolkitDefinition xml:lang="ca">Component d’un recurs intangible.</rdakit:toolkitDefinition>
      <skos:scopeNote xml:lang="ca">Inclou un fitxer digital.</skos:scopeNote>
      <skos:scopeNote xml:lang="fr">Comprend un fichier numérique.</skos:scopeNote>
      <skos:prefLabel xml:lang="vi">đơn vị logic</skos:prefLabel>
      <rdakit:toolkitLabel xml:lang="vi">đơn vị logic</rdakit:toolkitLabel>
      <skos:definition xml:lang="vi">Thành phần của một biểu thị không sờ thấy được.</skos:definition>
      <rdakit:toolkitDefinition xml:lang="vi">Thành phần của một biểu thị không sờ thấy được.</rdakit:toolkitDefinition>
      <skos:scopeNote xml:lang="vi">Tệp số được bao gồm.</skos:scopeNote>
      <skos:prefLabel xml:lang="no">logisk enhet</skos:prefLabel>
      <rdakit:toolkitLabel xml:lang="no">logisk enhet</rdakit:toolkitLabel>
      <skos:definition xml:lang="no">En bestanddel av en uhåndgripelig manifestasjon.</skos:definition>
      <rdakit:toolkitDefinition xml:lang="no">En bestanddel av en uhåndgripelig manifestasjon.</rdakit:toolkitDefinition>
      <skos:scopeNote xml:lang="no">En digtal fil er inkludert.</skos:scopeNote>
    </skos:Concept>
<!-- Concept: main series  -->
    <skos:Concept rdf:about="http://rdaregistry.info/termList/RDATerms/1056" xml:lang="en">
      <skos:inScheme rdf:resource="http://rdaregistry.info/termList/RDATerms"/>
      <reg:status rdf:resource="http://metadataregistry.org/uri/RegStatus/1001"/>
      <reg:identifier rdf:resource="http://metadataregistry.org/concepts/8571"/>
      <skos:prefLabel xml:lang="en">main series</skos:prefLabel>
      <rdakit:toolkitLabel xml:lang="en">main series</rdakit:toolkitLabel>
      <skos:definition xml:lang="en">A series that contains one or more subseries.</skos:definition>
      <rdakit:toolkitDefinition xml:lang="en">A series that contains one or more subseries.</rdakit:toolkitDefinition>
      <skos:prefLabel xml:lang="it">serie principale</skos:prefLabel>
      <rdakit:toolkitLabel xml:lang="it">serie principale</rdakit:toolkitLabel>
      <skos:definition xml:lang="it">Serie che contiene una o più sottoserie.</skos:definition>
      <rdakit:toolkitDefinition xml:lang="it">Serie che contiene una o più sottoserie.</rdakit:toolkitDefinition>
      <skos:prefLabel xml:lang="es">serie principal</skos:prefLabel>
      <rdakit:toolkitLabel xml:lang="es">serie principal</rdakit:toolkitLabel>
      <skos:definition xml:lang="es">Una serie que contiene una o más subseries.</skos:definition>
      <rdakit:toolkitDefinition xml:lang="es">Una serie que contiene una o más subseries.</rdakit:toolkitDefinition>
      <skos:prefLabel xml:lang="de">Hauptreihe</skos:prefLabel>
      <rdakit:toolkitLabel xml:lang="de">Hauptreihe</rdakit:toolkitLabel>
      <skos:definition xml:lang="de">Eine Reihe, die eine oder mehrere Unterreihen enthält.</skos:definition>
      <rdakit:toolkitDefinition xml:lang="de">Eine Reihe, die eine oder mehrere Unterreihen enthält.</rdakit:toolkitDefinition>
      <skos:prefLabel xml:lang="fi">pääsarja</skos:prefLabel>
      <rdakit:toolkitLabel xml:lang="fi">pääsarja</rdakit:toolkitLabel>
      <skos:definition xml:lang="fi">Sarja, joka sisältää yhden tai useampia alasarjoja.</skos:definition>
      <rdakit:toolkitDefinition xml:lang="fi">Sarja, joka sisältää yhden tai useampia alasarjoja.</rdakit:toolkitDefinition>
      <skos:prefLabel xml:lang="da">hovedserie</skos:prefLabel>
      <rdakit:toolkitLabel xml:lang="da">hovedserie</rdakit:toolkitLabel>
      <skos:definition xml:lang="da">Serie, der indeholder en eller flere underserier.</skos:definition>
      <rdakit:toolkitDefinition xml:lang="da">Serie, der indeholder en eller flere underserier.</rdakit:toolkitDefinition>
      <skos:prefLabel xml:lang="ca">col·lecció principal</skos:prefLabel>
      <rdakit:toolkitLabel xml:lang="ca">col·lecció principal</rdakit:toolkitLabel>
      <skos:definition xml:lang="ca">Col·lecció que conté una o més subcol·leccions.</skos:definition>
      <rdakit:toolkitDefinition xml:lang="ca">Col·lecció que conté una o més subcol·leccions.</rdakit:toolkitDefinition>
      <skos:prefLabel xml:lang="fr">collection principale</skos:prefLabel>
      <rdakit:toolkitLabel xml:lang="fr">collection principale</rdakit:toolkitLabel>
      <skos:definition xml:lang="fr">Collection qui contient une ou plusieurs sous-collections.</skos:definition>
      <rdakit:toolkitDefinition xml:lang="fr">Collection qui contient une ou plusieurs sous-collections.</rdakit:toolkitDefinition>
      <skos:prefLabel xml:lang="vi">tùng thư chính</skos:prefLabel>
      <rdakit:toolkitLabel xml:lang="vi">tùng thư chính</rdakit:toolkitLabel>
      <skos:definition xml:lang="vi">Tùng thư chứa một hoặc nhiều hơn tiểu tùng thư.</skos:definition>
      <rdakit:toolkitDefinition xml:lang="vi">Tùng thư chứa một hoặc nhiều hơn tiểu tùng thư.</rdakit:toolkitDefinition>
      <skos:prefLabel xml:lang="no">hovedserie</skos:prefLabel>
      <rdakit:toolkitLabel xml:lang="no">hovedserie</rdakit:toolkitLabel>
      <skos:definition xml:lang="no">En serie som består av en eller flere underserier.</skos:definition>
      <rdakit:toolkitDefinition xml:lang="no">En serie som består av en eller flere underserier.</rdakit:toolkitDefinition>
    </skos:Concept>
<!-- Concept: map series  -->
    <skos:Concept rdf:about="http://rdaregistry.info/termList/RDATerms/1057" xml:lang="en">
      <skos:inScheme rdf:resource="http://rdaregistry.info/termList/RDATerms"/>
      <reg:status rdf:resource="http://metadataregistry.org/uri/RegStatus/1001"/>
      <reg:identifier rdf:resource="http://metadataregistry.org/concepts/8572"/>
      <skos:prefLabel xml:lang="en">map series</skos:prefLabel>
      <rdakit:toolkitLabel xml:lang="en">map series</rdakit:toolkitLabel>
      <skos:definition xml:lang="en">A number of related but physically separate and bibliographically distinct cartographic units intended to form a single group, collectively identified by any commonly occurring unifying characteristic or combination of characteristics.</skos:definition>
      <rdakit:toolkitDefinition xml:lang="en">A number of related but physically separate and bibliographically distinct cartographic units intended to form a single group, collectively identified by any commonly occurring unifying characteristic or combination of characteristics.</rdakit:toolkitDefinition>
      <skos:prefLabel xml:lang="it">serie di carte geografiche</skos:prefLabel>
      <rdakit:toolkitLabel xml:lang="it">serie di carte geografiche</rdakit:toolkitLabel>
      <skos:definition xml:lang="it">Numero di unità cartografiche correlate ma fisicamente separate e bibliograficamente distinte, destinate a formare un gruppo unico.</skos:definition>
      <rdakit:toolkitDefinition xml:lang="it">Numero di unità cartografiche correlate ma fisicamente separate e bibliograficamente distinte, destinate a formare un gruppo unico.</rdakit:toolkitDefinition>
      <skos:prefLabel xml:lang="fr">série cartographique</skos:prefLabel>
      <rdakit:toolkitLabel xml:lang="fr">série cartographique</rdakit:toolkitLabel>
      <skos:definition xml:lang="fr">Unités cartographiques en relation mais physiquement et bibliographiquement distinctes, destinées à former un ensemble unique et identifiées de façon collective par toute caractéristique ou combinaison de caractéristiques communes et unifiantes.</skos:definition>
      <rdakit:toolkitDefinition xml:lang="fr">Unités cartographiques en relation mais physiquement et bibliographiquement distinctes, destinées à former un ensemble unique et identifiées de façon collective par toute caractéristique ou combinaison de caractéristiques communes et unifiantes.</rdakit:toolkitDefinition>
      <skos:prefLabel xml:lang="es">serie cartográfica</skos:prefLabel>
      <rdakit:toolkitLabel xml:lang="es">serie cartográfica</rdakit:toolkitLabel>
      <skos:definition xml:lang="es">Un número de unidades cartográficas relacionadas pero físicamente separadas y bibliográficamente distintas, pensadas para formar un solo grupo individual.</skos:definition>
      <rdakit:toolkitDefinition xml:lang="es">Un número de unidades cartográficas relacionadas pero físicamente separadas y bibliográficamente distintas, pensadas para formar un solo grupo individual.</rdakit:toolkitDefinition>
      <skos:scopeNote xml:lang="es">En su tratamiento bibliográfico, el grupo se identifica colectivamente mediante una característica común unificadora o a través de una combinación de características, incluyendo una designación común (p.ej., un título colectivo, un número o una combinación de ambos); un sistema de identificación de hojas (incluyendo los sistemas de numeración sucesiva o cronológica); la escala; el editor; especificaciones cartográficas; formato uniforme; etc.</skos:scopeNote>
      <skos:prefLabel xml:lang="de">Kartenwerk</skos:prefLabel>
      <rdakit:toolkitLabel xml:lang="de">Kartenwerk</rdakit:toolkitLabel>
      <skos:definition xml:lang="de">Eine Reihe von miteinander in Beziehung stehenden, aber physisch voneinander getrennten und bibliografisch unterscheidbaren kartografischen Einheiten, die als einzelne Gruppe gedacht sind und gemeinsam identifiziert werden durch eine allgemein vorkommende vereinende Eigenschaft oder durch die Kombination von Eigenschaften einschließlich einer gemeinsamen Bezeichnung.</skos:definition>
      <rdakit:toolkitDefinition xml:lang="de">Eine Reihe von miteinander in Beziehung stehenden, aber physisch voneinander getrennten und bibliografisch unterscheidbaren kartografischen Einheiten, die als einzelne Gruppe gedacht sind und gemeinsam identifiziert werden durch eine allgemein vorkommende vereinende Eigenschaft oder durch die Kombination von Eigenschaften einschließlich einer gemeinsamen Bezeichnung.</rdakit:toolkitDefinition>
      <skos:prefLabel xml:lang="fi">karttasarja</skos:prefLabel>
      <rdakit:toolkitLabel xml:lang="fi">karttasarja</rdakit:toolkitLabel>
      <skos:definition xml:lang="fi">Joukko toisiinsa liittyviä, mutta fyysisesti erillisiä ja bibliografisesti itsenäisesti käsiteltäviä karttoja, jotka muodostavat yhtenäisen ryhmän. Karttasarjan osilla on yhteisiä tunnusmerkkejä.</skos:definition>
      <rdakit:toolkitDefinition xml:lang="fi">Joukko toisiinsa liittyviä, mutta fyysisesti erillisiä ja bibliografisesti itsenäisesti käsiteltäviä karttoja, jotka muodostavat yhtenäisen ryhmän. Karttasarjan osilla on yhteisiä tunnusmerkkejä.</rdakit:toolkitDefinition>
      <skos:prefLabel xml:lang="da">kortserie</skos:prefLabel>
      <rdakit:toolkitLabel xml:lang="da">kortserie</rdakit:toolkitLabel>
      <skos:definition xml:lang="da">Et antal relaterede, men fysisk separate og bibliografisk distinkte kartografiske enheder beregnet til at udgøre en enkelt gruppe, samlet identificeret ved enhver forekommende egenskab eller kombination af egenskaber.</skos:definition>
      <rdakit:toolkitDefinition xml:lang="da">Et antal relaterede, men fysisk separate og bibliografisk distinkte kartografiske enheder beregnet til at udgøre en enkelt gruppe, samlet identificeret ved enhver forekommende egenskab eller kombination af egenskaber.</rdakit:toolkitDefinition>
      <skos:prefLabel xml:lang="ca">col·lecció de mapes</skos:prefLabel>
      <rdakit:toolkitLabel xml:lang="ca">col·lecció de mapes</rdakit:toolkitLabel>
      <skos:definition xml:lang="ca">Diverses unitats cartogràfiques relacionades però separades físicament i diferents bibliogràficament, concebudes perquè formin un sol grup, identificat col·lectivament per qualsevol característica comuna unificadora o per una combinació de característiques.</skos:definition>
      <rdakit:toolkitDefinition xml:lang="ca">Diverses unitats cartogràfiques relacionades però separades físicament i diferents bibliogràficament, concebudes perquè formin un sol grup, identificat col·lectivament per qualsevol característica comuna unificadora o per una combinació de característiques.</rdakit:toolkitDefinition>
      <skos:prefLabel xml:lang="vi">tùng thư bản đồ</skos:prefLabel>
      <rdakit:toolkitLabel xml:lang="vi">tùng thư bản đồ</rdakit:toolkitLabel>
      <skos:definition xml:lang="vi">Một số đơn vị đò bản riêng biệt về thư mục, có liên quan nhưng tách biệt về vật lý dùng để tạo thành một nhóm đơn lẻ, được nhận dạng tập thể bằng đặc trưng thống nhất xuất hiện chung hoặc tổ hợp các đặc trưng.</skos:definition>
      <rdakit:toolkitDefinition xml:lang="vi">Một số đơn vị đò bản riêng biệt về thư mục, có liên quan nhưng tách biệt về vật lý dùng để tạo thành một nhóm đơn lẻ, được nhận dạng tập thể bằng đặc trưng thống nhất xuất hiện chung hoặc tổ hợp các đặc trưng.</rdakit:toolkitDefinition>
      <skos:prefLabel xml:lang="no">kartserie</skos:prefLabel>
      <rdakit:toolkitLabel xml:lang="no">kartserie</rdakit:toolkitLabel>
      <skos:definition xml:lang="no">En serie med tilknyttede, men fysisk separate og bibliografisk adskilte kartografiske enheter som samlet er ment å utgjøre en gruppe, og som sammen identifiseres av en felles egenskap eller kombinasjon av egenskaper.</skos:definition>
      <rdakit:toolkitDefinition xml:lang="no">En serie med tilknyttede, men fysisk separate og bibliografisk adskilte kartografiske enheter som samlet er ment å utgjøre en gruppe, og som sammen identifiseres av en felles egenskap eller kombinasjon av egenskaper.</rdakit:toolkitDefinition>
    </skos:Concept>
<!-- Concept: media  -->
    <skos:Concept rdf:about="http://rdaregistry.info/termList/RDATerms/1058" xml:lang="en">
      <skos:inScheme rdf:resource="http://rdaregistry.info/termList/RDATerms"/>
      <reg:status rdf:resource="http://metadataregistry.org/uri/RegStatus/1001"/>
      <reg:identifier rdf:resource="http://metadataregistry.org/concepts/8573"/>
      <skos:prefLabel xml:lang="en">media</skos:prefLabel>
      <rdakit:toolkitLabel xml:lang="en">media</rdakit:toolkitLabel>
      <skos:definition xml:lang="en">A means used to convey information or artistic content.</skos:definition>
      <rdakit:toolkitDefinition xml:lang="en">A means used to convey information or artistic content.</rdakit:toolkitDefinition>
	    <skos:related rdf:resource="http://rdaregistry.info/termList/RDATerms/1016"/>
	    <skos:related rdf:resource="http://rdaregistry.info/termList/RDATerms/1086"/>
	    <skos:related rdf:resource="http://rdaregistry.info/termList/RDATerms/1026"/>
      <skos:prefLabel xml:lang="it">media</skos:prefLabel>
      <rdakit:toolkitLabel xml:lang="it">media</rdakit:toolkitLabel>
      <skos:definition xml:lang="it">Mezzi utilizzati per trasmettere le informazioni o il contenuto artistico.</skos:definition>
      <rdakit:toolkitDefinition xml:lang="it">Mezzi utilizzati per trasmettere le informazioni o il contenuto artistico.</rdakit:toolkitDefinition>
      <skos:prefLabel xml:lang="fr">média</skos:prefLabel>
      <rdakit:toolkitLabel xml:lang="fr">média</rdakit:toolkitLabel>
      <skos:definition xml:lang="fr">Moyen utilisé pour communiquer un contenu informatif ou artistique.</skos:definition>
      <rdakit:toolkitDefinition xml:lang="fr">Moyen utilisé pour communiquer un contenu informatif ou artistique.</rdakit:toolkitDefinition>
      <skos:prefLabel xml:lang="es">medios</skos:prefLabel>
      <rdakit:toolkitLabel xml:lang="es">medios</rdakit:toolkitLabel>
      <skos:definition xml:lang="es">Los medios utilizados para transmitir información o contenido artístico.</skos:definition>
      <rdakit:toolkitDefinition xml:lang="es">Los medios utilizados para transmitir información o contenido artístico.</rdakit:toolkitDefinition>
      <skos:prefLabel xml:lang="de">Medium</skos:prefLabel>
      <rdakit:toolkitLabel xml:lang="de">Medium</rdakit:toolkitLabel>
      <skos:definition xml:lang="de">Das Mittel, das verwendet wird, um die Information oder den künstlerischen Inhalt auszudrücken.</skos:definition>
      <rdakit:toolkitDefinition xml:lang="de">Das Mittel, das verwendet wird, um die Information oder den künstlerischen Inhalt auszudrücken.</rdakit:toolkitDefinition>
      <skos:prefLabel xml:lang="fi">viestin</skos:prefLabel>
      <rdakit:toolkitLabel xml:lang="fi">viestin</rdakit:toolkitLabel>
      <skos:definition xml:lang="fi">Tiedon tai taiteellisen sisällön välittämiseen käytetty väline.</skos:definition>
      <rdakit:toolkitDefinition xml:lang="fi">Tiedon tai taiteellisen sisällön välittämiseen käytetty väline.</rdakit:toolkitDefinition>
      <skos:prefLabel xml:lang="da">medie</skos:prefLabel>
      <rdakit:toolkitLabel xml:lang="da">medie</rdakit:toolkitLabel>
      <skos:definition xml:lang="da">Middel anvendt til at formidle information eller kunstnerisk indhold.</skos:definition>
      <rdakit:toolkitDefinition xml:lang="da">Middel anvendt til at formidle information eller kunstnerisk indhold.</rdakit:toolkitDefinition>
      <skos:prefLabel xml:lang="ca">suport</skos:prefLabel>
      <rdakit:toolkitLabel xml:lang="ca">suport</rdakit:toolkitLabel>
      <skos:definition xml:lang="ca">Mitjà usat per comunicar informació o contingut artístic.</skos:definition>
      <rdakit:toolkitDefinition xml:lang="ca">Mitjà usat per comunicar informació o contingut artístic.</rdakit:toolkitDefinition>
      <skos:prefLabel xml:lang="vi">phương tiện</skos:prefLabel>
      <rdakit:toolkitLabel xml:lang="vi">phương tiện</rdakit:toolkitLabel>
      <skos:definition xml:lang="vi">Cách thức dùng để chuyển tải thông tin hoặc nội dung nghệ thuật.</skos:definition>
      <rdakit:toolkitDefinition xml:lang="vi">Cách thức dùng để chuyển tải thông tin hoặc nội dung nghệ thuật.</rdakit:toolkitDefinition>
      <skos:prefLabel xml:lang="no">media</skos:prefLabel>
      <rdakit:toolkitLabel xml:lang="no">media</rdakit:toolkitLabel>
      <skos:definition xml:lang="no">Et middel som brukes til å overbringe informasjon eller kunstnerisk innhold.</skos:definition>
      <rdakit:toolkitDefinition xml:lang="no">Et middel som brukes til å overbringe informasjon eller kunstnerisk innhold.</rdakit:toolkitDefinition>
    </skos:Concept>
<!-- Concept: microfilm  -->
    <skos:Concept rdf:about="http://rdaregistry.info/termList/RDATerms/1059" xml:lang="en">
      <skos:inScheme rdf:resource="http://rdaregistry.info/termList/RDATerms"/>
      <reg:status rdf:resource="http://metadataregistry.org/uri/RegStatus/1001"/>
      <reg:identifier rdf:resource="http://metadataregistry.org/concepts/8574"/>
      <skos:prefLabel xml:lang="en">microfilm</skos:prefLabel>
      <rdakit:toolkitLabel xml:lang="en">microfilm</rdakit:toolkitLabel>
      <skos:definition xml:lang="en">A film bearing a number of microimages in linear array.</skos:definition>
      <rdakit:toolkitDefinition xml:lang="en">A film bearing a number of microimages in linear array.</rdakit:toolkitDefinition>
      <skos:prefLabel xml:lang="fr">microfilm</skos:prefLabel>
      <rdakit:toolkitLabel xml:lang="fr">microfilm</rdakit:toolkitLabel>
      <skos:definition xml:lang="fr">Film portant une série de micro-images disposées de façon linéaire.</skos:definition>
      <rdakit:toolkitDefinition xml:lang="fr">Film portant une série de micro-images disposées de façon linéaire.</rdakit:toolkitDefinition>
      <skos:prefLabel xml:lang="es">microfilme</skos:prefLabel>
      <rdakit:toolkitLabel xml:lang="es">microfilme</rdakit:toolkitLabel>
      <skos:definition xml:lang="es">Película que contiene un número de microimágenes en forma lineal.</skos:definition>
      <rdakit:toolkitDefinition xml:lang="es">Película que contiene un número de microimágenes en forma lineal.</rdakit:toolkitDefinition>
      <skos:prefLabel xml:lang="de">Mikrofilm</skos:prefLabel>
      <rdakit:toolkitLabel xml:lang="de">Mikrofilm</rdakit:toolkitLabel>
      <skos:definition xml:lang="de">Ein Film, der eine Reihe von Mikrobildern in einer linearen Anordnung trägt.</skos:definition>
      <rdakit:toolkitDefinition xml:lang="de">Ein Film, der eine Reihe von Mikrobildern in einer linearen Anordnung trägt.</rdakit:toolkitDefinition>
      <skos:prefLabel xml:lang="fi">mikrofilmi</skos:prefLabel>
      <rdakit:toolkitLabel xml:lang="fi">mikrofilmi</rdakit:toolkitLabel>
      <skos:definition xml:lang="fi">Filmi, jolla on mikrovalokuvia lineaarisessa järjestyksessä.</skos:definition>
      <rdakit:toolkitDefinition xml:lang="fi">Filmi, jolla on mikrovalokuvia lineaarisessa järjestyksessä.</rdakit:toolkitDefinition>
      <skos:prefLabel xml:lang="da">mikrofilm</skos:prefLabel>
      <rdakit:toolkitLabel xml:lang="da">mikrofilm</rdakit:toolkitLabel>
      <skos:definition xml:lang="da">Film med et antal mikrobilleder i lineær opsætning.</skos:definition>
      <rdakit:toolkitDefinition xml:lang="da">Film med et antal mikrobilleder i lineær opsætning.</rdakit:toolkitDefinition>
      <skos:prefLabel xml:lang="ca">microfilm</skos:prefLabel>
      <rdakit:toolkitLabel xml:lang="ca">microfilm</rdakit:toolkitLabel>
      <skos:definition xml:lang="ca">Pel·lícula que porta una sèrie de microimatges en una disposició lineal.</skos:definition>
      <rdakit:toolkitDefinition xml:lang="ca">Pel·lícula que porta una sèrie de microimatges en una disposició lineal.</rdakit:toolkitDefinition>
      <skos:prefLabel xml:lang="vi">vi phim</skos:prefLabel>
      <rdakit:toolkitLabel xml:lang="vi">vi phim</rdakit:toolkitLabel>
      <skos:definition xml:lang="vi">Phim chứa một số vi ảnh dạng mảng tuyến tính.</skos:definition>
      <rdakit:toolkitDefinition xml:lang="vi">Phim chứa một số vi ảnh dạng mảng tuyến tính.</rdakit:toolkitDefinition>
      <skos:prefLabel xml:lang="no">mikrofilm</skos:prefLabel>
      <rdakit:toolkitLabel xml:lang="no">mikrofilm</rdakit:toolkitLabel>
      <skos:definition xml:lang="no">Et stykke transparent film med en serie mikrofotografier på lineær rekke.</skos:definition>
      <rdakit:toolkitDefinition xml:lang="no">Et stykke transparent film med en serie mikrofotografier på lineær rekke.</rdakit:toolkitDefinition>
    </skos:Concept>
<!-- Concept: monograph  -->
    <skos:Concept rdf:about="http://rdaregistry.info/termList/RDATerms/1060" xml:lang="en">
      <skos:inScheme rdf:resource="http://rdaregistry.info/termList/RDATerms"/>
      <reg:status rdf:resource="http://metadataregistry.org/uri/RegStatus/1001"/>
      <reg:identifier rdf:resource="http://metadataregistry.org/concepts/8575"/>
      <skos:prefLabel xml:lang="en">monograph</skos:prefLabel>
      <rdakit:toolkitLabel xml:lang="en">monograph</rdakit:toolkitLabel>
      <skos:definition xml:lang="en">A resource that is complete in one part or intended to be completed within a finite number of parts.</skos:definition>
      <rdakit:toolkitDefinition xml:lang="en">A resource that is complete in one part or intended to be completed within a finite number of parts.</rdakit:toolkitDefinition>
      <skos:prefLabel xml:lang="it">monografia</skos:prefLabel>
      <rdakit:toolkitLabel xml:lang="it">monografia</rdakit:toolkitLabel>
      <skos:definition xml:lang="it">Risorsa completa in una sola parte o destinata a essere completata in un numero finito di parti.</skos:definition>
      <rdakit:toolkitDefinition xml:lang="it">Risorsa completa in una sola parte o destinata a essere completata in un numero finito di parti.</rdakit:toolkitDefinition>
      <skos:prefLabel xml:lang="fr">monographie</skos:prefLabel>
      <rdakit:toolkitLabel xml:lang="fr">monographie</rdakit:toolkitLabel>
      <skos:definition xml:lang="fr">Ressource complète en une seule partie ou destinée à être complète en un nombre limité de parties.</skos:definition>
      <rdakit:toolkitDefinition xml:lang="fr">Ressource complète en une seule partie ou destinée à être complète en un nombre limité de parties.</rdakit:toolkitDefinition>
      <skos:prefLabel xml:lang="es">monografía</skos:prefLabel>
      <rdakit:toolkitLabel xml:lang="es">monografía</rdakit:toolkitLabel>
      <skos:definition xml:lang="es">Recurso que está completo en una parte o que se tiene el propósito de completar con un número finito de partes.</skos:definition>
      <rdakit:toolkitDefinition xml:lang="es">Recurso que está completo en una parte o que se tiene el propósito de completar con un número finito de partes.</rdakit:toolkitDefinition>
      <skos:prefLabel xml:lang="de">Monografie</skos:prefLabel>
      <rdakit:toolkitLabel xml:lang="de">Monografie</rdakit:toolkitLabel>
      <skos:definition xml:lang="de">Eine Ressource, die in einem Teil abgeschlossen ist oder die innerhalb einer begrenzten Anzahl von Teilen abgeschlossen werden soll.</skos:definition>
      <rdakit:toolkitDefinition xml:lang="de">Eine Ressource, die in einem Teil abgeschlossen ist oder die innerhalb einer begrenzten Anzahl von Teilen abgeschlossen werden soll.</rdakit:toolkitDefinition>
      <skos:prefLabel xml:lang="fi">monografia</skos:prefLabel>
      <rdakit:toolkitLabel xml:lang="fi">monografia</rdakit:toolkitLabel>
      <skos:definition xml:lang="fi">Aineisto, joka ilmestyy vain yhtenä osana tai rajattuna määränä erillisiä osia.</skos:definition>
      <rdakit:toolkitDefinition xml:lang="fi">Aineisto, joka ilmestyy vain yhtenä osana tai rajattuna määränä erillisiä osia.</rdakit:toolkitDefinition>
      <skos:prefLabel xml:lang="da">monografi</skos:prefLabel>
      <rdakit:toolkitLabel xml:lang="da">monografi</rdakit:toolkitLabel>
      <skos:definition xml:lang="da">Ressource, der er komplet i én del eller vil blive afsluttet inden for et begrænset antal dele.</skos:definition>
      <rdakit:toolkitDefinition xml:lang="da">Ressource, der er komplet i én del eller vil blive afsluttet inden for et begrænset antal dele.</rdakit:toolkitDefinition>
      <skos:prefLabel xml:lang="ca">monografia</skos:prefLabel>
      <rdakit:toolkitLabel xml:lang="ca">monografia</rdakit:toolkitLabel>
      <skos:definition xml:lang="ca">Recurs que és complet en una part o que està previst que es completi en un nombre finit de parts.</skos:definition>
      <rdakit:toolkitDefinition xml:lang="ca">Recurs que és complet en una part o que està previst que es completi en un nombre finit de parts.</rdakit:toolkitDefinition>
      <skos:prefLabel xml:lang="vi">chuyên khảo</skos:prefLabel>
      <rdakit:toolkitLabel xml:lang="vi">chuyên khảo</rdakit:toolkitLabel>
      <skos:definition xml:lang="vi">Tài nguyên kết thúc chỉ có một phần hoặc dự định kết thúc với số lượng xác định các phần.</skos:definition>
      <rdakit:toolkitDefinition xml:lang="vi">Tài nguyên kết thúc chỉ có một phần hoặc dự định kết thúc với số lượng xác định các phần.</rdakit:toolkitDefinition>
      <skos:prefLabel xml:lang="no">monografi</skos:prefLabel>
      <rdakit:toolkitLabel xml:lang="no">monografi</rdakit:toolkitLabel>
      <skos:definition xml:lang="no">En ressurs som er avsluttet i én del eller planlagt avsluttet i et på forhånd fastsatt antall deler.</skos:definition>
      <rdakit:toolkitDefinition xml:lang="no">En ressurs som er avsluttet i én del eller planlagt avsluttet i et på forhånd fastsatt antall deler.</rdakit:toolkitDefinition>
    </skos:Concept>
<!-- Concept: multilevel description  -->
    <skos:Concept rdf:about="http://rdaregistry.info/termList/RDATerms/1061" xml:lang="en">
      <skos:inScheme rdf:resource="http://rdaregistry.info/termList/RDATerms"/>
      <reg:status rdf:resource="http://metadataregistry.org/uri/RegStatus/1001"/>
      <reg:identifier rdf:resource="http://metadataregistry.org/concepts/8576"/>
      <skos:prefLabel xml:lang="en">multilevel description</skos:prefLabel>
      <rdakit:toolkitLabel xml:lang="en">multilevel description</rdakit:toolkitLabel>
      <skos:definition xml:lang="en">A form of presentation, in an ISBD display, of descriptive data based on the division of information into two or more levels.</skos:definition>
      <rdakit:toolkitDefinition xml:lang="en">A form of presentation, in an ISBD display, of descriptive data based on the division of information into two or more levels.</rdakit:toolkitDefinition>
      <skos:scopeNote xml:lang="en">The first level contains information common to the whole or main resource. The second and subsequent levels contain information about an individual part.</skos:scopeNote>
      <skos:prefLabel xml:lang="it">descrizione a più livelli</skos:prefLabel>
      <rdakit:toolkitLabel xml:lang="it">descrizione a più livelli</rdakit:toolkitLabel>
      <skos:definition xml:lang="it">In una visualizzazione ISBD, la descrizione a più livelli è una forma di presentazione dei dati descrittivi basata sulla suddivisione delle informazioni descrittive su due o più livelli.</skos:definition>
      <rdakit:toolkitDefinition xml:lang="it">In una visualizzazione ISBD, la descrizione a più livelli è una forma di presentazione dei dati descrittivi basata sulla suddivisione delle informazioni descrittive su due o più livelli.</rdakit:toolkitDefinition>
      <skos:scopeNote xml:lang="it">Il primo livello contiene informazioni comuni a tutta la risorsa o a quella principale. Il secondo livello e quelli successivi contengono informazioni sulle parti singole.</skos:scopeNote>
      <skos:prefLabel xml:lang="fr">description à plusieurs niveaux</skos:prefLabel>
      <rdakit:toolkitLabel xml:lang="fr">description à plusieurs niveaux</rdakit:toolkitLabel>
      <skos:definition xml:lang="fr">Forme de présentation, dans un affichage ISBD, des données descriptives basée sur la répartition de l’information sur deux ou plusieurs niveaux.</skos:definition>
      <rdakit:toolkitDefinition xml:lang="fr">Forme de présentation, dans un affichage ISBD, des données descriptives basée sur la répartition de l’information sur deux ou plusieurs niveaux.</rdakit:toolkitDefinition>
      <skos:scopeNote xml:lang="fr">Le premier niveau contient l’information commune à l’ensemble de la ressource ou à la ressource principale. Le deuxième niveau et les niveaux suivants contiennent l’information sur la partie individuelle.</skos:scopeNote>
      <skos:prefLabel xml:lang="es">descripción multinivel</skos:prefLabel>
      <rdakit:toolkitLabel xml:lang="es">descripción multinivel</rdakit:toolkitLabel>
      <skos:definition xml:lang="es">En una muestra de ISBD, una descripción multinivel es una forma de presentación de datos descriptivos basados en la división de información descriptiva en dos o más niveles.</skos:definition>
      <rdakit:toolkitDefinition xml:lang="es">En una muestra de ISBD, una descripción multinivel es una forma de presentación de datos descriptivos basados en la división de información descriptiva en dos o más niveles.</rdakit:toolkitDefinition>
      <skos:scopeNote xml:lang="es">El primer nivel contiene información común al total o recurso principal. El segundo y niveles subsecuentes contienen información sobre la parte individual.</skos:scopeNote>
      <skos:prefLabel xml:lang="de">Multi-Level-Beschreibung</skos:prefLabel>
      <rdakit:toolkitLabel xml:lang="de">Multi-Level-Beschreibung</rdakit:toolkitLabel>
      <skos:definition xml:lang="de">Eine Form der Präsentation von beschreibenden Daten in einer ISBD-Anzeige, die die Gliederung der Informationen in zwei oder mehr Ebenen zugrunde legt.</skos:definition>
      <rdakit:toolkitDefinition xml:lang="de">Eine Form der Präsentation von beschreibenden Daten in einer ISBD-Anzeige, die die Gliederung der Informationen in zwei oder mehr Ebenen zugrunde legt.</rdakit:toolkitDefinition>
      <skos:scopeNote xml:lang="de">Die erste Ebene enthält Informationen, die zur gesamten Ressource oder Hauptressource gemeinsam gehören. Die zweite und nachfolgende Ebene enthält Informationen über einen einzelnen Teil.</skos:scopeNote>
      <skos:prefLabel xml:lang="fi">monitasoinen kuvailu</skos:prefLabel>
      <rdakit:toolkitLabel xml:lang="fi">monitasoinen kuvailu</rdakit:toolkitLabel>
      <skos:definition xml:lang="fi">ISBD-esitystapa, monitasoinen kuvailun menetelmä, joka perustuu tietojen jakamiseen kahdelle tai useammalle tasolle.</skos:definition>
      <rdakit:toolkitDefinition xml:lang="fi">ISBD-esitystapa, monitasoinen kuvailun menetelmä, joka perustuu tietojen jakamiseen kahdelle tai useammalle tasolle.</rdakit:toolkitDefinition>
      <skos:scopeNote xml:lang="fi">Ensimmäinen taso sisältää tietoja koko aineistosta tai pääaineistosta. Seuraava(t) taso(t) sisältävät tietoja yksittäisestä osasta.</skos:scopeNote>
      <skos:prefLabel xml:lang="da">beskrivelse på flere niveauer</skos:prefLabel>
      <rdakit:toolkitLabel xml:lang="da">beskrivelse på flere niveauer</rdakit:toolkitLabel>
      <skos:definition xml:lang="da">Præsentationsform i en ISBD-visning af beskrivende data med opdeling af oplysninger på to eller flere niveauer.</skos:definition>
      <rdakit:toolkitDefinition xml:lang="da">Præsentationsform i en ISBD-visning af beskrivende data med opdeling af oplysninger på to eller flere niveauer.</rdakit:toolkitDefinition>
      <skos:scopeNote xml:lang="da">Det første niveau indeholder oplysninger, der er fælles for helheden eller hovedressourcen. Det andet og evt. efterfølgende niveauer indeholder oplysninger om sektion eller individuel del.</skos:scopeNote>
      <skos:prefLabel xml:lang="ca">descripció en més d’un nivell</skos:prefLabel>
      <rdakit:toolkitLabel xml:lang="ca">descripció en més d’un nivell</rdakit:toolkitLabel>
      <skos:definition xml:lang="ca">Forma de presentació, en una visualització ISBD, de les dades descriptives que es basa en la divisió de la informació en dos o més nivells.</skos:definition>
      <rdakit:toolkitDefinition xml:lang="ca">Forma de presentació, en una visualització ISBD, de les dades descriptives que es basa en la divisió de la informació en dos o més nivells.</rdakit:toolkitDefinition>
      <skos:scopeNote xml:lang="ca">El primer nivell inclou informació comuna al conjunt o al recurs principal. El segon nivell i els següents inclouen informació sobre una part individual.</skos:scopeNote>
      <skos:prefLabel xml:lang="vi">mô tả theo nhiều mức</skos:prefLabel>
      <rdakit:toolkitLabel xml:lang="vi">mô tả theo nhiều mức</rdakit:toolkitLabel>
      <skos:definition xml:lang="vi">Hình thái trình bày, trong hiển thị ISBD, dữ liệu mô tả dựa trên phân chia thông tin thành hai hoặc hoặc nhiều hơn mức.</skos:definition>
      <rdakit:toolkitDefinition xml:lang="vi">Hình thái trình bày, trong hiển thị ISBD, dữ liệu mô tả dựa trên phân chia thông tin thành hai hoặc hoặc nhiều hơn mức.</rdakit:toolkitDefinition>
      <skos:scopeNote xml:lang="vi">Mức đầu tiên chứa thông tin chung về toàn bộ hoặc tài nguyên chính. Mức thứ hai và tiếp sau chứa thông tin về phần riêng lẻ.</skos:scopeNote>
      <skos:prefLabel xml:lang="no">flernivåbeskrivelse</skos:prefLabel>
      <rdakit:toolkitLabel xml:lang="no">flernivåbeskrivelse</rdakit:toolkitLabel>
      <skos:definition xml:lang="no">En form for presentasjon, i ISBD-visning, av deskriptive data basert på deling av informasjon på to eller flere nivåer.</skos:definition>
      <rdakit:toolkitDefinition xml:lang="no">En form for presentasjon, i ISBD-visning, av deskriptive data basert på deling av informasjon på to eller flere nivåer.</rdakit:toolkitDefinition>
      <skos:scopeNote xml:lang="no">Det første nivået inneholder informasjon som er felles for helheten eller hovedressursen. Det andre nivået og påfølgende nivåer inneholder informasjon om de enkelte delene.</skos:scopeNote>
    </skos:Concept>
<!-- Concept: name  -->
    <skos:Concept rdf:about="http://rdaregistry.info/termList/RDATerms/1062" xml:lang="en">
      <skos:inScheme rdf:resource="http://rdaregistry.info/termList/RDATerms"/>
      <reg:status rdf:resource="http://metadataregistry.org/uri/RegStatus/1001"/>
      <reg:identifier rdf:resource="http://metadataregistry.org/concepts/8577"/>
      <skos:prefLabel xml:lang="en">name</skos:prefLabel>
      <rdakit:toolkitLabel xml:lang="en">name</rdakit:toolkitLabel>
      <skos:definition xml:lang="en">A word, character, or group of words and/or characters by which an entity is known.</skos:definition>
      <rdakit:toolkitDefinition xml:lang="en">A word, character, or group of words and/or characters by which an entity is known.</rdakit:toolkitDefinition>
      <skos:prefLabel xml:lang="it">nome</skos:prefLabel>
      <rdakit:toolkitLabel xml:lang="it">nome</rdakit:toolkitLabel>
      <skos:definition xml:lang="it">Parola, carattere o serie di parole e/o caratteri con cui una persona, famiglia o ente è conosciuto.</skos:definition>
      <rdakit:toolkitDefinition xml:lang="it">Parola, carattere o serie di parole e/o caratteri con cui una persona, famiglia o ente è conosciuto.</rdakit:toolkitDefinition>
      <skos:prefLabel xml:lang="fr">nom</skos:prefLabel>
      <rdakit:toolkitLabel xml:lang="fr">nom</rdakit:toolkitLabel>
      <skos:definition xml:lang="fr">Mot, caractère ou groupe de mots et/ou de caractères sous lequel une entité est connue.</skos:definition>
      <rdakit:toolkitDefinition xml:lang="fr">Mot, caractère ou groupe de mots et/ou de caractères sous lequel une entité est connue.</rdakit:toolkitDefinition>
      <skos:prefLabel xml:lang="es">nombre</skos:prefLabel>
      <rdakit:toolkitLabel xml:lang="es">nombre</rdakit:toolkitLabel>
      <skos:definition xml:lang="es">Palabra, carácter o grupo de palabras y/o caracteres mediante el cual se conoce una entidad.</skos:definition>
      <rdakit:toolkitDefinition xml:lang="es">Palabra, carácter o grupo de palabras y/o caracteres mediante el cual se conoce una entidad.</rdakit:toolkitDefinition>
      <skos:prefLabel xml:lang="de">Name</skos:prefLabel>
      <rdakit:toolkitLabel xml:lang="de">Name</rdakit:toolkitLabel>
      <skos:definition xml:lang="de">Ein Wort, ein Zeichen oder eine Gruppe von Wörtern und/oder Zeichen, unter dem/der eine Entität bekannt ist.</skos:definition>
      <rdakit:toolkitDefinition xml:lang="de">Ein Wort, ein Zeichen oder eine Gruppe von Wörtern und/oder Zeichen, unter dem/der eine Entität bekannt ist.</rdakit:toolkitDefinition>
      <skos:prefLabel xml:lang="fi">nimi</skos:prefLabel>
      <rdakit:toolkitLabel xml:lang="fi">nimi</rdakit:toolkitLabel>
      <skos:definition xml:lang="fi">Sana, merkki tai sana- ja/tai merkkiyhdistelmä, jolla entiteetti tunnetaan.</skos:definition>
      <rdakit:toolkitDefinition xml:lang="fi">Sana, merkki tai sana- ja/tai merkkiyhdistelmä, jolla entiteetti tunnetaan.</rdakit:toolkitDefinition>
      <skos:prefLabel xml:lang="da">navn</skos:prefLabel>
      <rdakit:toolkitLabel xml:lang="da">navn</rdakit:toolkitLabel>
      <skos:definition xml:lang="da">Ord, tegn eller gruppe af ord og/eller tegn, som en person, familie eller korporation er kendt under.</skos:definition>
      <rdakit:toolkitDefinition xml:lang="da">Ord, tegn eller gruppe af ord og/eller tegn, som en person, familie eller korporation er kendt under.</rdakit:toolkitDefinition>
      <skos:prefLabel xml:lang="ca">nom</skos:prefLabel>
      <rdakit:toolkitLabel xml:lang="ca">nom</rdakit:toolkitLabel>
      <skos:definition xml:lang="ca">Paraula, caràcter o grup de paraules i/o de caràcters pel qual es coneix una entitat.</skos:definition>
      <rdakit:toolkitDefinition xml:lang="ca">Paraula, caràcter o grup de paraules i/o de caràcters pel qual es coneix una entitat.</rdakit:toolkitDefinition>
      <skos:prefLabel xml:lang="vi">tên</skos:prefLabel>
      <rdakit:toolkitLabel xml:lang="vi">tên</rdakit:toolkitLabel>
      <skos:definition xml:lang="vi">Từ, ký tự, hoặc nhóm từ và/hoặc ký tự mà theo đó một thực thể được biết đến.</skos:definition>
      <rdakit:toolkitDefinition xml:lang="vi">Từ, ký tự, hoặc nhóm từ và/hoặc ký tự mà theo đó một thực thể được biết đến.</rdakit:toolkitDefinition>
      <skos:prefLabel xml:lang="no">navn</skos:prefLabel>
      <rdakit:toolkitLabel xml:lang="no">navn</rdakit:toolkitLabel>
      <skos:definition xml:lang="no">Et ord, tegn eller grupper av ord og/eller tegn som en entitet er kjent under.</skos:definition>
      <rdakit:toolkitDefinition xml:lang="no">Et ord, tegn eller grupper av ord og/eller tegn som en entitet er kjent under.</rdakit:toolkitDefinition>
    </skos:Concept>
<!-- Concept: neat line  -->
    <skos:Concept rdf:about="http://rdaregistry.info/termList/RDATerms/1063" xml:lang="en">
      <skos:inScheme rdf:resource="http://rdaregistry.info/termList/RDATerms"/>
      <reg:status rdf:resource="http://metadataregistry.org/uri/RegStatus/1001"/>
      <reg:identifier rdf:resource="http://metadataregistry.org/concepts/8578"/>
      <skos:prefLabel xml:lang="en">neat line</skos:prefLabel>
      <rdakit:toolkitLabel xml:lang="en">neat line</rdakit:toolkitLabel>
      <skos:definition xml:lang="en">A line marking the outer edge of a map or chart, separating its detail from any border or margin.</skos:definition>
      <rdakit:toolkitDefinition xml:lang="en">A line marking the outer edge of a map or chart, separating its detail from any border or margin.</rdakit:toolkitDefinition>
      <skos:prefLabel xml:lang="de">Begrenzungslinie</skos:prefLabel>
      <rdakit:toolkitLabel xml:lang="de">Begrenzungslinie</rdakit:toolkitLabel>
      <skos:definition xml:lang="de">Eine Linie, welche die äußeren Grenzen einer Karte oder eines Charts markiert und deren/dessen Ausschnitt von einer Begrenzung oder dem Seitenrand trennt.</skos:definition>
      <rdakit:toolkitDefinition xml:lang="de">Eine Linie, welche die äußeren Grenzen einer Karte oder eines Charts markiert und deren/dessen Ausschnitt von einer Begrenzung oder dem Seitenrand trennt.</rdakit:toolkitDefinition>
      <skos:prefLabel xml:lang="fi">kartan reunaviiva</skos:prefLabel>
      <rdakit:toolkitLabel xml:lang="fi">kartan reunaviiva</rdakit:toolkitLabel>
      <skos:definition xml:lang="fi">Viiva, joka merkitsee kartan tai kaavion ulkoreunan erottaen sen yksityiskohdat reunuksesta tai marginaalista.</skos:definition>
      <rdakit:toolkitDefinition xml:lang="fi">Viiva, joka merkitsee kartan tai kaavion ulkoreunan erottaen sen yksityiskohdat reunuksesta tai marginaalista.</rdakit:toolkitDefinition>
      <skos:prefLabel xml:lang="da">indre kortramme</skos:prefLabel>
      <rdakit:toolkitLabel xml:lang="da">indre kortramme</rdakit:toolkitLabel>
      <skos:definition xml:lang="da">Linje, der markerer et korts eller en planches yderkant, og som adskiller kortets eller planchens detaljer fra enhver ramme eller margen.</skos:definition>
      <rdakit:toolkitDefinition xml:lang="da">Linje, der markerer et korts eller en planches yderkant, og som adskiller kortets eller planchens detaljer fra enhver ramme eller margen.</rdakit:toolkitDefinition>
      <skos:prefLabel xml:lang="ca">requadre</skos:prefLabel>
      <rdakit:toolkitLabel xml:lang="ca">requadre</rdakit:toolkitLabel>
      <skos:definition xml:lang="ca">Línia que marca el marge exterior d’un mapa o d’un plànol, separant així el detall del seu contingut de qualsevol vora o marge.</skos:definition>
      <rdakit:toolkitDefinition xml:lang="ca">Línia que marca el marge exterior d’un mapa o d’un plànol, separant així el detall del seu contingut de qualsevol vora o marge.</rdakit:toolkitDefinition>
      <skos:prefLabel xml:lang="fr">orle</skos:prefLabel>
      <rdakit:toolkitLabel xml:lang="fr">orle</rdakit:toolkitLabel>
      <skos:definition xml:lang="fr">Ligne marquant le pourtour extérieur d’une carte, y compris une carte de navigation, isolant ainsi le détail de son contenu de toute bordure ou marge.</skos:definition>
      <rdakit:toolkitDefinition xml:lang="fr">Ligne marquant le pourtour extérieur d’une carte, y compris une carte de navigation, isolant ainsi le détail de son contenu de toute bordure ou marge.</rdakit:toolkitDefinition>
      <skos:prefLabel xml:lang="vi">đường khung</skos:prefLabel>
      <rdakit:toolkitLabel xml:lang="vi">đường khung</rdakit:toolkitLabel>
      <skos:definition xml:lang="vi">Đường tạo ra lề ngoài của bản đồ hoặc biểu đồ, phân tách chi tiết của nó với đường viền hoặc lề bất kỳ.</skos:definition>
      <rdakit:toolkitDefinition xml:lang="vi">Đường tạo ra lề ngoài của bản đồ hoặc biểu đồ, phân tách chi tiết của nó với đường viền hoặc lề bất kỳ.</rdakit:toolkitDefinition>
      <skos:prefLabel xml:lang="no">inndelingsramme</skos:prefLabel>
      <rdakit:toolkitLabel xml:lang="no">inndelingsramme</rdakit:toolkitLabel>
      <skos:definition xml:lang="no">En linje som markerer ytterkanten av et kart eller en plansje, som skiller dets detaljer fra kanten eller margen.</skos:definition>
      <rdakit:toolkitDefinition xml:lang="no">En linje som markerer ytterkanten av et kart eller en plansje, som skiller dets detaljer fra kanten eller margen.</rdakit:toolkitDefinition>
    </skos:Concept>
<!-- Concept: non-self-describing manifestation  -->
    <skos:Concept rdf:about="http://rdaregistry.info/termList/RDATerms/1064" xml:lang="en">
      <skos:inScheme rdf:resource="http://rdaregistry.info/termList/RDATerms"/>
      <reg:status rdf:resource="http://metadataregistry.org/uri/RegStatus/1001"/>
      <reg:identifier rdf:resource="http://metadataregistry.org/concepts/8579"/>
      <skos:prefLabel xml:lang="en">non-self-describing manifestation</skos:prefLabel>
      <rdakit:toolkitLabel xml:lang="en">non-self-describing manifestation</rdakit:toolkitLabel>
      <skos:definition xml:lang="en">A manifestation that does not contain identifying information.</skos:definition>
      <rdakit:toolkitDefinition xml:lang="en">A manifestation that does not contain identifying information.</rdakit:toolkitDefinition>
      <skos:prefLabel xml:lang="de">Nicht selbstbeschreibende Manifestation</skos:prefLabel>
      <rdakit:toolkitLabel xml:lang="de">Nicht selbstbeschreibende Manifestation</rdakit:toolkitLabel>
      <skos:definition xml:lang="de">Eine Manifestation, die keine identifizierenden Informationen enthält.</skos:definition>
      <rdakit:toolkitDefinition xml:lang="de">Eine Manifestation, die keine identifizierenden Informationen enthält.</rdakit:toolkitDefinition>
      <skos:prefLabel xml:lang="fi">kuvailua tukematon manifestaatio</skos:prefLabel>
      <rdakit:toolkitLabel xml:lang="fi">kuvailua tukematon manifestaatio</rdakit:toolkitLabel>
      <skos:definition xml:lang="fi">Kuvailua tukematon manifestaatio, joka ei sisällä identifioivia tietoja.</skos:definition>
      <rdakit:toolkitDefinition xml:lang="fi">Kuvailua tukematon manifestaatio, joka ei sisällä identifioivia tietoja.</rdakit:toolkitDefinition>
      <skos:prefLabel xml:lang="da">ikke-selvbeskrivende manifestation</skos:prefLabel>
      <rdakit:toolkitLabel xml:lang="da">ikke-selvbeskrivende manifestation</rdakit:toolkitLabel>
      <skos:definition xml:lang="da">Manifestation uden identificerende oplysninger.</skos:definition>
      <rdakit:toolkitDefinition xml:lang="da">Manifestation uden identificerende oplysninger.</rdakit:toolkitDefinition>
      <skos:prefLabel xml:lang="ca">manifestació que no es descriu a ella mateixa</skos:prefLabel>
      <rdakit:toolkitLabel xml:lang="ca">manifestació que no es descriu a ella mateixa</rdakit:toolkitLabel>
      <skos:definition xml:lang="ca">Manifestació que no inclou informació identificadora.</skos:definition>
      <rdakit:toolkitDefinition xml:lang="ca">Manifestació que no inclou informació identificadora.</rdakit:toolkitDefinition>
      <skos:prefLabel xml:lang="fr">manifestation non autodescriptive</skos:prefLabel>
      <rdakit:toolkitLabel xml:lang="fr">manifestation non autodescriptive</rdakit:toolkitLabel>
      <skos:definition xml:lang="fr">Manifestation qui ne contient pas d’information d’identification.</skos:definition>
      <rdakit:toolkitDefinition xml:lang="fr">Manifestation qui ne contient pas d’information d’identification.</rdakit:toolkitDefinition>
      <skos:prefLabel xml:lang="vi">biểu thị không tự mô tả</skos:prefLabel>
      <rdakit:toolkitLabel xml:lang="vi">biểu thị không tự mô tả</rdakit:toolkitLabel>
      <skos:definition xml:lang="vi">Biểu thị không chứa thông tin nhận dạng.</skos:definition>
      <rdakit:toolkitDefinition xml:lang="vi">Biểu thị không chứa thông tin nhận dạng.</rdakit:toolkitDefinition>
      <skos:prefLabel xml:lang="no">ikke-selvbeskrivende manifestasjon</skos:prefLabel>
      <rdakit:toolkitLabel xml:lang="no">ikke-selvbeskrivende manifestasjon</rdakit:toolkitLabel>
      <skos:definition xml:lang="no">En manifestasjon som ikke inneholder identifiserende informasjon.</skos:definition>
      <rdakit:toolkitDefinition xml:lang="no">En manifestasjon som ikke inneholder identifiserende informasjon.</rdakit:toolkitDefinition>
    </skos:Concept>
<!-- Concept: part  -->
    <skos:Concept rdf:about="http://rdaregistry.info/termList/RDATerms/1065" xml:lang="en">
      <skos:inScheme rdf:resource="http://rdaregistry.info/termList/RDATerms"/>
      <reg:status rdf:resource="http://metadataregistry.org/uri/RegStatus/1001"/>
      <reg:identifier rdf:resource="http://metadataregistry.org/concepts/8580"/>
      <skos:prefLabel xml:lang="en">part</skos:prefLabel>
      <rdakit:toolkitLabel xml:lang="en">part</rdakit:toolkitLabel>
      <skos:definition xml:lang="en">A unit into which a resource has been permanently divided by a publisher, manufacturer, etc.</skos:definition>
      <rdakit:toolkitDefinition xml:lang="en">A unit into which a resource has been permanently divided by a publisher, manufacturer, etc.</rdakit:toolkitDefinition>
	    <skos:related rdf:resource="http://rdaregistry.info/termList/RDATerms/1052"/>
      <skos:prefLabel xml:lang="it">parte</skos:prefLabel>
      <rdakit:toolkitLabel xml:lang="it">parte</rdakit:toolkitLabel>
      <skos:prefLabel xml:lang="de">Teil</skos:prefLabel>
      <rdakit:toolkitLabel xml:lang="de">Teil</rdakit:toolkitLabel>
      <skos:definition xml:lang="de">Eine Einheit, in welcher die Ressource vom Verlag, Hersteller usw. unterteilt wurde.</skos:definition>
      <rdakit:toolkitDefinition xml:lang="de">Eine Einheit, in welcher die Ressource vom Verlag, Hersteller usw. unterteilt wurde.</rdakit:toolkitDefinition>
      <skos:prefLabel xml:lang="fi">osa</skos:prefLabel>
      <rdakit:toolkitLabel xml:lang="fi">osa</rdakit:toolkitLabel>
      <skos:definition xml:lang="fi">Yksikkö, johon kustantaja, valmistaja tms. on pysyvästi jakanut aineiston.</skos:definition>
      <rdakit:toolkitDefinition xml:lang="fi">Yksikkö, johon kustantaja, valmistaja tms. on pysyvästi jakanut aineiston.</rdakit:toolkitDefinition>
      <skos:prefLabel xml:lang="da">del</skos:prefLabel>
      <rdakit:toolkitLabel xml:lang="da">del</rdakit:toolkitLabel>
      <skos:definition xml:lang="da">Enhed, som en ressource er blevet permanent opdelt i af udgiveren, producenten etc.</skos:definition>
      <rdakit:toolkitDefinition xml:lang="da">Enhed, som en ressource er blevet permanent opdelt i af udgiveren, producenten etc.</rdakit:toolkitDefinition>
      <skos:prefLabel xml:lang="ca">part</skos:prefLabel>
      <rdakit:toolkitLabel xml:lang="ca">part</rdakit:toolkitLabel>
      <skos:definition xml:lang="ca">Unitat en què un editor, un fabricant, etc., divideix permanentment un recurs.</skos:definition>
      <rdakit:toolkitDefinition xml:lang="ca">Unitat en què un editor, un fabricant, etc., divideix permanentment un recurs.</rdakit:toolkitDefinition>
      <skos:prefLabel xml:lang="fr">partie</skos:prefLabel>
      <rdakit:toolkitLabel xml:lang="fr">partie</rdakit:toolkitLabel>
      <skos:definition xml:lang="fr">Une des unités entre lesquelles une ressource a été divisée de façon permanente par l’éditeur, le fabricant, etc.</skos:definition>
      <rdakit:toolkitDefinition xml:lang="fr">Une des unités entre lesquelles une ressource a été divisée de façon permanente par l’éditeur, le fabricant, etc.</rdakit:toolkitDefinition>
      <skos:prefLabel xml:lang="vi">phần</skos:prefLabel>
      <rdakit:toolkitLabel xml:lang="vi">phần</rdakit:toolkitLabel>
      <skos:definition xml:lang="vi">Đơn vị mà một tài nguyên được nhà xuất bản, nhà chế tạo, v.v... chia vĩnh cửu thành .</skos:definition>
      <rdakit:toolkitDefinition xml:lang="vi">Đơn vị mà một tài nguyên được nhà xuất bản, nhà chế tạo, v.v... chia vĩnh cửu thành .</rdakit:toolkitDefinition>
      <skos:prefLabel xml:lang="no">del</skos:prefLabel>
      <rdakit:toolkitLabel xml:lang="no">del</rdakit:toolkitLabel>
      <skos:definition xml:lang="no">En enhet som en ressurs er blitt permanent delt opp i av utgiver, tilvirker, etc.</skos:definition>
      <rdakit:toolkitDefinition xml:lang="no">En enhet som en ressurs er blitt permanent delt opp i av utgiver, tilvirker, etc.</rdakit:toolkitDefinition>
    </skos:Concept>
<!-- Concept: patronymic  -->
    <skos:Concept rdf:about="http://rdaregistry.info/termList/RDATerms/1066" xml:lang="en">
      <skos:inScheme rdf:resource="http://rdaregistry.info/termList/RDATerms"/>
      <reg:status rdf:resource="http://metadataregistry.org/uri/RegStatus/1001"/>
      <reg:identifier rdf:resource="http://metadataregistry.org/concepts/8581"/>
      <skos:prefLabel xml:lang="en">patronymic</skos:prefLabel>
      <rdakit:toolkitLabel xml:lang="en">patronymic</rdakit:toolkitLabel>
      <skos:definition xml:lang="en">A name derived from the given name of a father.</skos:definition>
      <rdakit:toolkitDefinition xml:lang="en">A name derived from the given name of a father.</rdakit:toolkitDefinition>
      <skos:prefLabel xml:lang="it">patronimico</skos:prefLabel>
      <rdakit:toolkitLabel xml:lang="it">patronimico</rdakit:toolkitLabel>
      <skos:definition xml:lang="it">Nome derivato dal nome proprio del padre.</skos:definition>
      <rdakit:toolkitDefinition xml:lang="it">Nome derivato dal nome proprio del padre.</rdakit:toolkitDefinition>
      <skos:prefLabel xml:lang="fr">patronyme</skos:prefLabel>
      <rdakit:toolkitLabel xml:lang="fr">patronyme</rdakit:toolkitLabel>
      <skos:definition xml:lang="fr">Nom formé à partir du prénom d’un père.</skos:definition>
      <rdakit:toolkitDefinition xml:lang="fr">Nom formé à partir du prénom d’un père.</rdakit:toolkitDefinition>
      <skos:prefLabel xml:lang="es">patronímico</skos:prefLabel>
      <rdakit:toolkitLabel xml:lang="es">patronímico</rdakit:toolkitLabel>
      <skos:definition xml:lang="es">Nombre derivado del nombre de pila de un padre.</skos:definition>
      <rdakit:toolkitDefinition xml:lang="es">Nombre derivado del nombre de pila de un padre.</rdakit:toolkitDefinition>
      <skos:prefLabel xml:lang="de">Patronym</skos:prefLabel>
      <rdakit:toolkitLabel xml:lang="de">Patronym</rdakit:toolkitLabel>
      <skos:definition xml:lang="de">Ein Name, der vom Vornamen eines Vaters abgeleitet ist.</skos:definition>
      <rdakit:toolkitDefinition xml:lang="de">Ein Name, der vom Vornamen eines Vaters abgeleitet ist.</rdakit:toolkitDefinition>
      <skos:prefLabel xml:lang="fi">patronyymi</skos:prefLabel>
      <rdakit:toolkitLabel xml:lang="fi">patronyymi</rdakit:toolkitLabel>
      <skos:definition xml:lang="fi">Isän etunimestä johdettu nimi.</skos:definition>
      <rdakit:toolkitDefinition xml:lang="fi">Isän etunimestä johdettu nimi.</rdakit:toolkitDefinition>
      <skos:prefLabel xml:lang="da">patronym</skos:prefLabel>
      <rdakit:toolkitLabel xml:lang="da">patronym</rdakit:toolkitLabel>
      <skos:definition xml:lang="da">Navn, der er afledt af en fars fornavn.</skos:definition>
      <rdakit:toolkitDefinition xml:lang="da">Navn, der er afledt af en fars fornavn.</rdakit:toolkitDefinition>
      <skos:prefLabel xml:lang="ca">patronímic</skos:prefLabel>
      <rdakit:toolkitLabel xml:lang="ca">patronímic</rdakit:toolkitLabel>
      <skos:definition xml:lang="ca">Nom derivat del nom de pila del pare.</skos:definition>
      <rdakit:toolkitDefinition xml:lang="ca">Nom derivat del nom de pila del pare.</rdakit:toolkitDefinition>
      <skos:prefLabel xml:lang="vi">tên đặt theo tên cha</skos:prefLabel>
      <rdakit:toolkitLabel xml:lang="vi">tên đặt theo tên cha</rdakit:toolkitLabel>
      <skos:definition xml:lang="vi">Tên bắt nguồn từ tên thánh của người cha.</skos:definition>
      <rdakit:toolkitDefinition xml:lang="vi">Tên bắt nguồn từ tên thánh của người cha.</rdakit:toolkitDefinition>
      <skos:prefLabel xml:lang="no">patronymikon</skos:prefLabel>
      <rdakit:toolkitLabel xml:lang="no">patronymikon</rdakit:toolkitLabel>
      <skos:definition xml:lang="no">Et navn avledet av fars fornavn.</skos:definition>
      <rdakit:toolkitDefinition xml:lang="no">Et navn avledet av fars fornavn.</rdakit:toolkitDefinition>
    </skos:Concept>
<!-- Concept: physical unit  -->
    <skos:Concept rdf:about="http://rdaregistry.info/termList/RDATerms/1067" xml:lang="en">
      <skos:inScheme rdf:resource="http://rdaregistry.info/termList/RDATerms"/>
      <reg:status rdf:resource="http://metadataregistry.org/uri/RegStatus/1001"/>
      <reg:identifier rdf:resource="http://metadataregistry.org/concepts/8582"/>
      <skos:prefLabel xml:lang="en">physical unit</skos:prefLabel>
      <rdakit:toolkitLabel xml:lang="en">physical unit</rdakit:toolkitLabel>
      <skos:definition xml:lang="en">A constituent of a tangible manifestation.</skos:definition>
      <rdakit:toolkitDefinition xml:lang="en">A constituent of a tangible manifestation.</rdakit:toolkitDefinition>
      <skos:scopeNote xml:lang="en">A physical unit includes a volume, audiocassette, or film reel.</skos:scopeNote>
      <skos:prefLabel xml:lang="it">unità fisica</skos:prefLabel>
      <rdakit:toolkitLabel xml:lang="it">unità fisica</rdakit:toolkitLabel>
      <skos:definition xml:lang="it">Componente di una risorsa tangibile.</skos:definition>
      <rdakit:toolkitDefinition xml:lang="it">Componente di una risorsa tangibile.</rdakit:toolkitDefinition>
      <skos:prefLabel xml:lang="fr">unité physique</skos:prefLabel>
      <rdakit:toolkitLabel xml:lang="fr">unité physique</rdakit:toolkitLabel>
      <skos:definition xml:lang="fr">Composant d’une manifestation matérielle.</skos:definition>
      <rdakit:toolkitDefinition xml:lang="fr">Composant d’une manifestation matérielle.</rdakit:toolkitDefinition>
      <skos:prefLabel xml:lang="de">Physische Einheit</skos:prefLabel>
      <rdakit:toolkitLabel xml:lang="de">Physische Einheit</rdakit:toolkitLabel>
      <skos:definition xml:lang="de">Ein Bestandteil einer materiellen Manifestation.</skos:definition>
      <rdakit:toolkitDefinition xml:lang="de">Ein Bestandteil einer materiellen Manifestation.</rdakit:toolkitDefinition>
      <skos:scopeNote xml:lang="de">Eine physische Einheit umfasst einen Band, eine Audiokassette oder einen Film.</skos:scopeNote>
      <skos:prefLabel xml:lang="fi">fyysinen yksikkö</skos:prefLabel>
      <rdakit:toolkitLabel xml:lang="fi">fyysinen yksikkö</rdakit:toolkitLabel>
      <skos:definition xml:lang="fi">Käsinkosketeltavan aineiston rakenneosa.</skos:definition>
      <rdakit:toolkitDefinition xml:lang="fi">Käsinkosketeltavan aineiston rakenneosa.</rdakit:toolkitDefinition>
      <skos:scopeNote xml:lang="fi">Fyysinen yksikkö käsittää niteen, äänikasetin tai filmikelan.</skos:scopeNote>
      <skos:prefLabel xml:lang="da">fysisk enhed</skos:prefLabel>
      <rdakit:toolkitLabel xml:lang="da">fysisk enhed</rdakit:toolkitLabel>
      <skos:definition xml:lang="da">Bestanddelaf en fysisk manifestation.</skos:definition>
      <rdakit:toolkitDefinition xml:lang="da">Bestanddelaf en fysisk manifestation.</rdakit:toolkitDefinition>
      <skos:scopeNote xml:lang="da">En fysisk ressource omfatter et bind, et audiokassettebånd eller en filmspole.</skos:scopeNote>
      <skos:prefLabel xml:lang="ca">unitat física</skos:prefLabel>
      <rdakit:toolkitLabel xml:lang="ca">unitat física</rdakit:toolkitLabel>
      <skos:definition xml:lang="ca">Component d’una manifestació tangible.</skos:definition>
      <rdakit:toolkitDefinition xml:lang="ca">Component d’una manifestació tangible.</rdakit:toolkitDefinition>
      <skos:scopeNote xml:lang="ca">Una unitat física inclou un volum, una casset àudio o una bobina de pel·lícula.</skos:scopeNote>
      <skos:scopeNote xml:lang="fr">Comprend un volume, une cassette audio ou une bobine de film.</skos:scopeNote>
      <skos:prefLabel xml:lang="vi">đơn vị vật lý</skos:prefLabel>
      <rdakit:toolkitLabel xml:lang="vi">đơn vị vật lý</rdakit:toolkitLabel>
      <skos:definition xml:lang="vi">Thành phần của một biểu thị hữu hình.</skos:definition>
      <rdakit:toolkitDefinition xml:lang="vi">Thành phần của một biểu thị hữu hình.</rdakit:toolkitDefinition>
      <skos:scopeNote xml:lang="vi">Đơn vị vật lý bao gồm tập, audiocassett, hoặc cuôn phim.</skos:scopeNote>
      <skos:prefLabel xml:lang="no">fysisk enhet</skos:prefLabel>
      <rdakit:toolkitLabel xml:lang="no">fysisk enhet</rdakit:toolkitLabel>
      <skos:definition xml:lang="no">En bestanddel av en håndgripelig manifestasjon.</skos:definition>
      <rdakit:toolkitDefinition xml:lang="no">En bestanddel av en håndgripelig manifestasjon.</rdakit:toolkitDefinition>
      <skos:scopeNote xml:lang="no">En fysisk enhet inkluderer et bind, en lydkassett eller en filmspole.</skos:scopeNote>
    </skos:Concept>
<!-- Concept: plate  -->
    <skos:Concept rdf:about="http://rdaregistry.info/termList/RDATerms/1068" xml:lang="en">
      <skos:inScheme rdf:resource="http://rdaregistry.info/termList/RDATerms"/>
      <reg:status rdf:resource="http://metadataregistry.org/uri/RegStatus/1001"/>
      <reg:identifier rdf:resource="http://metadataregistry.org/concepts/8583"/>
      <skos:prefLabel xml:lang="en">plate</skos:prefLabel>
      <rdakit:toolkitLabel xml:lang="en">plate</rdakit:toolkitLabel>
      <skos:definition xml:lang="en">A leaf, usually containing illustrative content, that does not form part of either the preliminary or the main sequence of pages or leaves.</skos:definition>
      <rdakit:toolkitDefinition xml:lang="en">A leaf, usually containing illustrative content, that does not form part of either the preliminary or the main sequence of pages or leaves.</rdakit:toolkitDefinition>
      <skos:prefLabel xml:lang="it">tavola</skos:prefLabel>
      <rdakit:toolkitLabel xml:lang="it">tavola</rdakit:toolkitLabel>
      <skos:definition xml:lang="it">Carta che presenta contenuto illustrativo, corredato o meno da testo esplicativo, che non fa parte delle parti preliminari né della sequenza principale delle pagine o carte.</skos:definition>
      <rdakit:toolkitDefinition xml:lang="it">Carta che presenta contenuto illustrativo, corredato o meno da testo esplicativo, che non fa parte delle parti preliminari né della sequenza principale delle pagine o carte.</rdakit:toolkitDefinition>
      <skos:prefLabel xml:lang="de">Bildtafel</skos:prefLabel>
      <rdakit:toolkitLabel xml:lang="de">Bildtafel</rdakit:toolkitLabel>
      <skos:definition xml:lang="de">Ein Blatt, das üblicherweise illustrierenden Inhalt enthält, und nicht Teil der vorangegangenen oder der Hauptsequenz der Seiten oder Blätter ist.</skos:definition>
      <rdakit:toolkitDefinition xml:lang="de">Ein Blatt, das üblicherweise illustrierenden Inhalt enthält, und nicht Teil der vorangegangenen oder der Hauptsequenz der Seiten oder Blätter ist.</rdakit:toolkitDefinition>
      <skos:prefLabel xml:lang="fi">kuvasivu</skos:prefLabel>
      <rdakit:toolkitLabel xml:lang="fi">kuvasivu</rdakit:toolkitLabel>
      <skos:definition xml:lang="fi">Yleensä kuvitusta sisältävä lehti, joka ei kuulu varsinaiseen sivunumerointiin tai sitä edeltäviin sivuihin tai lehtiin.</skos:definition>
      <rdakit:toolkitDefinition xml:lang="fi">Yleensä kuvitusta sisältävä lehti, joka ei kuulu varsinaiseen sivunumerointiin tai sitä edeltäviin sivuihin tai lehtiin.</rdakit:toolkitDefinition>
      <skos:prefLabel xml:lang="da">tavle</skos:prefLabel>
      <rdakit:toolkitLabel xml:lang="da">tavle</rdakit:toolkitLabel>
      <skos:definition xml:lang="da">Blad, der normalt indeholder illustrativt indhold, der ikke er en del af hverken den indledende sekvens eller hovedsekvensen af sider eller blade.</skos:definition>
      <rdakit:toolkitDefinition xml:lang="da">Blad, der normalt indeholder illustrativt indhold, der ikke er en del af hverken den indledende sekvens eller hovedsekvensen af sider eller blade.</rdakit:toolkitDefinition>
      <skos:prefLabel xml:lang="ca">làmina</skos:prefLabel>
      <rdakit:toolkitLabel xml:lang="ca">làmina</rdakit:toolkitLabel>
      <skos:definition xml:lang="ca">Full, normalment amb contingut il·lustratiu, que no forma part ni de les pàgines o els fulls preliminars ni de la seqüència principal de pàgines o fulls.</skos:definition>
      <rdakit:toolkitDefinition xml:lang="ca">Full, normalment amb contingut il·lustratiu, que no forma part ni de les pàgines o els fulls preliminars ni de la seqüència principal de pàgines o fulls.</rdakit:toolkitDefinition>
      <skos:prefLabel xml:lang="fr">planche</skos:prefLabel>
      <rdakit:toolkitLabel xml:lang="fr">planche</rdakit:toolkitLabel>
      <skos:definition xml:lang="fr">Feuillet comprenant généralement un contenu illustratif et qui ne fait partie ni de la séquence liminaire ni de la séquence principale de pages ou de feuillets.</skos:definition>
      <rdakit:toolkitDefinition xml:lang="fr">Feuillet comprenant généralement un contenu illustratif et qui ne fait partie ni de la séquence liminaire ni de la séquence principale de pages ou de feuillets.</rdakit:toolkitDefinition>
      <skos:prefLabel xml:lang="vi">Tờ minh hoạ</skos:prefLabel>
      <rdakit:toolkitLabel xml:lang="vi">Tờ minh hoạ</rdakit:toolkitLabel>
      <skos:definition xml:lang="vi">Tờ chứa nội dung minh hoạ, có văn bản giải thích hoặc không, không phải là phần của mở đầu hoặc các trang hoặc tờ chính.</skos:definition>
      <rdakit:toolkitDefinition xml:lang="vi">Tờ chứa nội dung minh hoạ, có văn bản giải thích hoặc không, không phải là phần của mở đầu hoặc các trang hoặc tờ chính.</rdakit:toolkitDefinition>
      <skos:prefLabel xml:lang="no">plansje</skos:prefLabel>
      <rdakit:toolkitLabel xml:lang="no">plansje</rdakit:toolkitLabel>
      <skos:definition xml:lang="no">Et blad som innholdsmessig  består av illustrasjonsmateriale med eller uten forklarende tekst, og som verken er innledende sekvens eller hovedsekvensen av sider eller blad.</skos:definition>
      <rdakit:toolkitDefinition xml:lang="no">Et blad som innholdsmessig  består av illustrasjonsmateriale med eller uten forklarende tekst, og som verken er innledende sekvens eller hovedsekvensen av sider eller blad.</rdakit:toolkitDefinition>
    </skos:Concept>
<!-- Concept: preferred name  -->
    <skos:Concept rdf:about="http://rdaregistry.info/termList/RDATerms/1069" xml:lang="en">
      <skos:inScheme rdf:resource="http://rdaregistry.info/termList/RDATerms"/>
      <reg:status rdf:resource="http://metadataregistry.org/uri/RegStatus/1001"/>
      <reg:identifier rdf:resource="http://metadataregistry.org/concepts/8584"/>
      <skos:prefLabel xml:lang="en">preferred name</skos:prefLabel>
      <rdakit:toolkitLabel xml:lang="en">preferred name</rdakit:toolkitLabel>
      <skos:definition xml:lang="en">A name or form of name chosen as the basis for an authorized access point representing an entity.</skos:definition>
      <rdakit:toolkitDefinition xml:lang="en">A name or form of name chosen as the basis for an authorized access point representing an entity.</rdakit:toolkitDefinition>
      <skos:prefLabel xml:lang="it">nome preferito</skos:prefLabel>
      <rdakit:toolkitLabel xml:lang="it">nome preferito</rdakit:toolkitLabel>
      <skos:definition xml:lang="it">Nome o forma del nome scelti come base per il punto d'accesso autorizzato che rappresenta un'entità.</skos:definition>
      <rdakit:toolkitDefinition xml:lang="it">Nome o forma del nome scelti come base per il punto d'accesso autorizzato che rappresenta un'entità.</rdakit:toolkitDefinition>
      <skos:prefLabel xml:lang="fr">nom privilégié</skos:prefLabel>
      <rdakit:toolkitLabel xml:lang="fr">nom privilégié</rdakit:toolkitLabel>
      <skos:definition xml:lang="fr">Nom ou forme de nom choisie comme élément de base d’un point d’accès autorisé représentant une entité.</skos:definition>
      <rdakit:toolkitDefinition xml:lang="fr">Nom ou forme de nom choisie comme élément de base d’un point d’accès autorisé représentant une entité.</rdakit:toolkitDefinition>
      <skos:prefLabel xml:lang="es">nombre preferido</skos:prefLabel>
      <rdakit:toolkitLabel xml:lang="es">nombre preferido</rdakit:toolkitLabel>
      <skos:definition xml:lang="es">El nombre o la forma del nombre elegida como base para el punto de acceso autorizado que representa una entidad.</skos:definition>
      <rdakit:toolkitDefinition xml:lang="es">El nombre o la forma del nombre elegida como base para el punto de acceso autorizado que representa una entidad.</rdakit:toolkitDefinition>
      <skos:prefLabel xml:lang="fi">ensisijainen nimi</skos:prefLabel>
      <rdakit:toolkitLabel xml:lang="fi">ensisijainen nimi</rdakit:toolkitLabel>
      <skos:definition xml:lang="fi">Nimi tai nimen muoto, joka on valittu entiteetin auktorisoidun hakutiedon perustaksi.</skos:definition>
      <rdakit:toolkitDefinition xml:lang="fi">Nimi tai nimen muoto, joka on valittu entiteetin auktorisoidun hakutiedon perustaksi.</rdakit:toolkitDefinition>
      <skos:prefLabel xml:lang="de">Bevorzugter Name</skos:prefLabel>
      <rdakit:toolkitLabel xml:lang="de">Bevorzugter Name</rdakit:toolkitLabel>
      <skos:definition xml:lang="de">Der Name oder die Namensform, der/die als Grundlage für den normierten Sucheinstieg gewählt wird, der eine Entität repräsentiert.</skos:definition>
      <rdakit:toolkitDefinition xml:lang="de">Der Name oder die Namensform, der/die als Grundlage für den normierten Sucheinstieg gewählt wird, der eine Entität repräsentiert.</rdakit:toolkitDefinition>
      <skos:prefLabel xml:lang="da">foretrukken navneform</skos:prefLabel>
      <rdakit:toolkitLabel xml:lang="da">foretrukken navneform</rdakit:toolkitLabel>
      <skos:definition xml:lang="da">Navn eller navneform, der er valgt som grundlag for en entitets autoriserede søgeindgang.</skos:definition>
      <rdakit:toolkitDefinition xml:lang="da">Navn eller navneform, der er valgt som grundlag for en entitets autoriserede søgeindgang.</rdakit:toolkitDefinition>
      <skos:prefLabel xml:lang="ca">nom preferit</skos:prefLabel>
      <rdakit:toolkitLabel xml:lang="ca">nom preferit</rdakit:toolkitLabel>
      <skos:definition xml:lang="ca">Nom o forma de nom triat com a base d'un punt d’accés autoritzat que representa una entitat.</skos:definition>
      <rdakit:toolkitDefinition xml:lang="ca">Nom o forma de nom triat com a base d'un punt d’accés autoritzat que representa una entitat.</rdakit:toolkitDefinition>
      <skos:prefLabel xml:lang="vi">tên ưu tiên</skos:prefLabel>
      <rdakit:toolkitLabel xml:lang="vi">tên ưu tiên</rdakit:toolkitLabel>
      <skos:definition xml:lang="vi">Tên hoặc hình thái của tên được lựa chọn như là cơ sở cho điểm truy cập được phép trình bày một thực thể.</skos:definition>
      <rdakit:toolkitDefinition xml:lang="vi">Tên hoặc hình thái của tên được lựa chọn như là cơ sở cho điểm truy cập được phép trình bày một thực thể.</rdakit:toolkitDefinition>
      <skos:prefLabel xml:lang="no">foretrukket navn</skos:prefLabel>
      <rdakit:toolkitLabel xml:lang="no">foretrukket navn</rdakit:toolkitLabel>
      <skos:definition xml:lang="no">Et navn eller en navneform som er valgt som utgangspunkt for en autorisert søkeinngang som representerer entiteten.</skos:definition>
      <rdakit:toolkitDefinition xml:lang="no">Et navn eller en navneform som er valgt som utgangspunkt for en autorisert søkeinngang som representerer entiteten.</rdakit:toolkitDefinition>
    </skos:Concept>
<!-- Concept: primary relationship  -->
    <skos:Concept rdf:about="http://rdaregistry.info/termList/RDATerms/1070" xml:lang="en">
      <skos:inScheme rdf:resource="http://rdaregistry.info/termList/RDATerms"/>
      <reg:status rdf:resource="http://metadataregistry.org/uri/RegStatus/1001"/>
      <reg:identifier rdf:resource="http://metadataregistry.org/concepts/8585"/>
      <skos:prefLabel xml:lang="en">primary relationship</skos:prefLabel>
      <rdakit:toolkitLabel xml:lang="en">primary relationship</rdakit:toolkitLabel>
      <skos:definition xml:lang="en">A relationship between a work, expression, manifestation, or item that is inherent in the FRBR definitions of those entities.</skos:definition>
      <rdakit:toolkitDefinition xml:lang="en">A relationship between a work, expression, manifestation, or item that is inherent in the FRBR definitions of those entities.</rdakit:toolkitDefinition>
      <skos:prefLabel xml:lang="de">Primärbeziehung</skos:prefLabel>
      <rdakit:toolkitLabel xml:lang="de">Primärbeziehung</rdakit:toolkitLabel>
      <skos:definition xml:lang="de">Eine Beziehung zwischen einem Werk, einer Expression, einer Manifestation und einem Exemplar, die in den FRBR-Definitionen dieser Entitäten enthalten ist.</skos:definition>
      <rdakit:toolkitDefinition xml:lang="de">Eine Beziehung zwischen einem Werk, einer Expression, einer Manifestation und einem Exemplar, die in den FRBR-Definitionen dieser Entitäten enthalten ist.</rdakit:toolkitDefinition>
      <skos:prefLabel xml:lang="fi">ensisijaiset suhteet</skos:prefLabel>
      <rdakit:toolkitLabel xml:lang="fi">ensisijaiset suhteet</rdakit:toolkitLabel>
      <skos:definition xml:lang="fi">Ensisijaiset suhteet vastaavat FRBR-mallissa määriteltyjä teoksen, ekspression, manifestaation ja kappaleen välisiä suhteita.</skos:definition>
      <rdakit:toolkitDefinition xml:lang="fi">Ensisijaiset suhteet vastaavat FRBR-mallissa määriteltyjä teoksen, ekspression, manifestaation ja kappaleen välisiä suhteita.</rdakit:toolkitDefinition>
      <skos:prefLabel xml:lang="da">primær relation</skos:prefLabel>
      <rdakit:toolkitLabel xml:lang="da">primær relation</rdakit:toolkitLabel>
      <skos:prefLabel xml:lang="ca">relacions principals</skos:prefLabel>
      <rdakit:toolkitLabel xml:lang="ca">relacions principals</rdakit:toolkitLabel>
      <skos:definition xml:lang="ca">Relació entre una obra, una expressió, una manifestació o un ítem que és inherent a les definicions d’aquestes entitats en el model FRBR.</skos:definition>
      <rdakit:toolkitDefinition xml:lang="ca">Relació entre una obra, una expressió, una manifestació o un ítem que és inherent a les definicions d’aquestes entitats en el model FRBR.</rdakit:toolkitDefinition>
      <skos:prefLabel xml:lang="fr">relation principale</skos:prefLabel>
      <rdakit:toolkitLabel xml:lang="fr">relation principale</rdakit:toolkitLabel>
      <skos:definition xml:lang="fr">Relation entre une œuvre, une expression, une manifestation ou un item qui est inhérente aux définitions de ces entités dans le modèle FRBR.</skos:definition>
      <rdakit:toolkitDefinition xml:lang="fr">Relation entre une œuvre, une expression, une manifestation ou un item qui est inhérente aux définitions de ces entités dans le modèle FRBR.</rdakit:toolkitDefinition>
      <skos:prefLabel xml:lang="vi">mối quan hệ nguyên sinh</skos:prefLabel>
      <rdakit:toolkitLabel xml:lang="vi">mối quan hệ nguyên sinh</rdakit:toolkitLabel>
      <skos:definition xml:lang="vi">Mối quan hệ giữa một tác phẩm, biểu hiện, biểu thị, và bản là cố hữu trong định nghĩa FRBR của các thực thể đó.</skos:definition>
      <rdakit:toolkitDefinition xml:lang="vi">Mối quan hệ giữa một tác phẩm, biểu hiện, biểu thị, và bản là cố hữu trong định nghĩa FRBR của các thực thể đó.</rdakit:toolkitDefinition>
      <skos:prefLabel xml:lang="no">primær relasjon</skos:prefLabel>
      <rdakit:toolkitLabel xml:lang="no">primær relasjon</rdakit:toolkitLabel>
      <skos:definition xml:lang="no">En relasjonen mellom et verk, et uttrykk, en manifestasjon eller et eksemplar som finnes i FRBRs definisjoner av disse entitetene.</skos:definition>
      <rdakit:toolkitDefinition xml:lang="no">En relasjonen mellom et verk, et uttrykk, en manifestasjon eller et eksemplar som finnes i FRBRs definisjoner av disse entitetene.</rdakit:toolkitDefinition>
    </skos:Concept>
<!-- Concept: protocol  -->
    <skos:Concept rdf:about="http://rdaregistry.info/termList/RDATerms/1071" xml:lang="en">
      <skos:inScheme rdf:resource="http://rdaregistry.info/termList/RDATerms"/>
      <reg:status rdf:resource="http://metadataregistry.org/uri/RegStatus/1001"/>
      <reg:identifier rdf:resource="http://metadataregistry.org/concepts/8586"/>
      <skos:prefLabel xml:lang="en">protocol</skos:prefLabel>
      <rdakit:toolkitLabel xml:lang="en">protocol</rdakit:toolkitLabel>
      <skos:definition xml:lang="en">A treaty amending and supplementing another treaty.</skos:definition>
      <rdakit:toolkitDefinition xml:lang="en">A treaty amending and supplementing another treaty.</rdakit:toolkitDefinition>
      <skos:prefLabel xml:lang="it">protocollo</skos:prefLabel>
      <rdakit:toolkitLabel xml:lang="it">protocollo</rdakit:toolkitLabel>
      <skos:definition xml:lang="it">Trattato che modifica e integra un altro trattato.</skos:definition>
      <rdakit:toolkitDefinition xml:lang="it">Trattato che modifica e integra un altro trattato.</rdakit:toolkitDefinition>
      <skos:prefLabel xml:lang="fr">protocole</skos:prefLabel>
      <rdakit:toolkitLabel xml:lang="fr">protocole</rdakit:toolkitLabel>
      <skos:definition xml:lang="fr">Traité amendant et complétant un autre traité.</skos:definition>
      <rdakit:toolkitDefinition xml:lang="fr">Traité amendant et complétant un autre traité.</rdakit:toolkitDefinition>
      <skos:prefLabel xml:lang="de">Protokoll</skos:prefLabel>
      <rdakit:toolkitLabel xml:lang="de">Protokoll</rdakit:toolkitLabel>
      <skos:definition xml:lang="de">Ein Abkommen, das ein anderes Abkommen verändert oder ergänzt.</skos:definition>
      <rdakit:toolkitDefinition xml:lang="de">Ein Abkommen, das ein anderes Abkommen verändert oder ergänzt.</rdakit:toolkitDefinition>
      <skos:prefLabel xml:lang="fi">pöytäkirja</skos:prefLabel>
      <rdakit:toolkitLabel xml:lang="fi">pöytäkirja</rdakit:toolkitLabel>
      <skos:definition xml:lang="fi">Valtiosopimus, joka muuttaa ja täydentää toista valtiosopimusta.</skos:definition>
      <rdakit:toolkitDefinition xml:lang="fi">Valtiosopimus, joka muuttaa ja täydentää toista valtiosopimusta.</rdakit:toolkitDefinition>
      <skos:prefLabel xml:lang="da">protokol</skos:prefLabel>
      <rdakit:toolkitLabel xml:lang="da">protokol</rdakit:toolkitLabel>
      <skos:definition xml:lang="da">Traktat, der ændrer eller supplerer en anden traktat.</skos:definition>
      <rdakit:toolkitDefinition xml:lang="da">Traktat, der ændrer eller supplerer en anden traktat.</rdakit:toolkitDefinition>
      <skos:prefLabel xml:lang="ca">protocol</skos:prefLabel>
      <rdakit:toolkitLabel xml:lang="ca">protocol</rdakit:toolkitLabel>
      <skos:definition xml:lang="ca">Tractat que esmena i complementa un altre tractat.</skos:definition>
      <rdakit:toolkitDefinition xml:lang="ca">Tractat que esmena i complementa un altre tractat.</rdakit:toolkitDefinition>
      <skos:prefLabel xml:lang="vi">nghị định thư</skos:prefLabel>
      <rdakit:toolkitLabel xml:lang="vi">nghị định thư</rdakit:toolkitLabel>
      <skos:definition xml:lang="vi">Một hiệp ước sửa đổi hoặc bổ sung cho hiệp ước khác.</skos:definition>
      <rdakit:toolkitDefinition xml:lang="vi">Một hiệp ước sửa đổi hoặc bổ sung cho hiệp ước khác.</rdakit:toolkitDefinition>
      <skos:prefLabel xml:lang="no">protokoll</skos:prefLabel>
      <rdakit:toolkitLabel xml:lang="no">protokoll</rdakit:toolkitLabel>
      <skos:definition xml:lang="no">En traktat som gjør tilføyelser til og endringer av en annen traktat.</skos:definition>
      <rdakit:toolkitDefinition xml:lang="no">En traktat som gjør tilføyelser til og endringer av en annen traktat.</rdakit:toolkitDefinition>
    </skos:Concept>
<!-- Concept: pseudonym  -->
    <skos:Concept rdf:about="http://rdaregistry.info/termList/RDATerms/1072" xml:lang="en">
      <skos:inScheme rdf:resource="http://rdaregistry.info/termList/RDATerms"/>
      <reg:status rdf:resource="http://metadataregistry.org/uri/RegStatus/1001"/>
      <reg:identifier rdf:resource="http://metadataregistry.org/concepts/8587"/>
      <skos:prefLabel xml:lang="en">pseudonym</skos:prefLabel>
      <rdakit:toolkitLabel xml:lang="en">pseudonym</rdakit:toolkitLabel>
      <skos:definition xml:lang="en">A name used by a person, either alone or in collaboration with others, that is not the person’s real name.</skos:definition>
      <rdakit:toolkitDefinition xml:lang="en">A name used by a person, either alone or in collaboration with others, that is not the person’s real name.</rdakit:toolkitDefinition>
      <skos:prefLabel xml:lang="it">pseudonimo</skos:prefLabel>
      <rdakit:toolkitLabel xml:lang="it">pseudonimo</rdakit:toolkitLabel>
      <skos:definition xml:lang="it">Nome utilizzato da una persona (da sola o in collaborazione con altri), diverso dal nome reale.</skos:definition>
      <rdakit:toolkitDefinition xml:lang="it">Nome utilizzato da una persona (da sola o in collaborazione con altri), diverso dal nome reale.</rdakit:toolkitDefinition>
      <skos:prefLabel xml:lang="fr">pseudonyme</skos:prefLabel>
      <rdakit:toolkitLabel xml:lang="fr">pseudonyme</rdakit:toolkitLabel>
      <skos:definition xml:lang="fr">Nom utilisé par une personne, seule ou en collaboration avec d’autres personnes, et qui n’est pas son nom véritable.</skos:definition>
      <rdakit:toolkitDefinition xml:lang="fr">Nom utilisé par une personne, seule ou en collaboration avec d’autres personnes, et qui n’est pas son nom véritable.</rdakit:toolkitDefinition>
      <skos:prefLabel xml:lang="es">seudónimo</skos:prefLabel>
      <rdakit:toolkitLabel xml:lang="es">seudónimo</rdakit:toolkitLabel>
      <skos:definition xml:lang="es">Un nombre utilizado por una persona (ya sea por sí sola o en colaboración con otros), que no es el nombre real de la persona.</skos:definition>
      <rdakit:toolkitDefinition xml:lang="es">Un nombre utilizado por una persona (ya sea por sí sola o en colaboración con otros), que no es el nombre real de la persona.</rdakit:toolkitDefinition>
      <skos:prefLabel xml:lang="de">Pseudonym</skos:prefLabel>
      <rdakit:toolkitLabel xml:lang="de">Pseudonym</rdakit:toolkitLabel>
      <skos:definition xml:lang="de">Ein Name, der von einer Person (entweder alleine oder zusammen mit anderen) verwendet wird, der nicht der reale Name der Person ist.</skos:definition>
      <rdakit:toolkitDefinition xml:lang="de">Ein Name, der von einer Person (entweder alleine oder zusammen mit anderen) verwendet wird, der nicht der reale Name der Person ist.</rdakit:toolkitDefinition>
      <skos:prefLabel xml:lang="fi">pseudonyymi</skos:prefLabel>
      <rdakit:toolkitLabel xml:lang="fi">pseudonyymi</rdakit:toolkitLabel>
      <skos:definition xml:lang="fi">Henkilön käyttämä nimi (yksin tai yhdessä yhden tai useamman muun henkilön kanssa), joka ei ole henkilön todellinen nimi.</skos:definition>
      <rdakit:toolkitDefinition xml:lang="fi">Henkilön käyttämä nimi (yksin tai yhdessä yhden tai useamman muun henkilön kanssa), joka ei ole henkilön todellinen nimi.</rdakit:toolkitDefinition>
      <skos:prefLabel xml:lang="da">pseudonym</skos:prefLabel>
      <rdakit:toolkitLabel xml:lang="da">pseudonym</rdakit:toolkitLabel>
      <skos:definition xml:lang="da">Navn anvendt af en person, enten alene eller sammen med andre, der ikke er personens rigtige navn.</skos:definition>
      <rdakit:toolkitDefinition xml:lang="da">Navn anvendt af en person, enten alene eller sammen med andre, der ikke er personens rigtige navn.</rdakit:toolkitDefinition>
      <skos:prefLabel xml:lang="ca">pseudònim</skos:prefLabel>
      <rdakit:toolkitLabel xml:lang="ca">pseudònim</rdakit:toolkitLabel>
      <skos:definition xml:lang="ca">Nom usat per una persona, sola o en col·laboració amb altres persones, i que no és el nom real de la persona.</skos:definition>
      <rdakit:toolkitDefinition xml:lang="ca">Nom usat per una persona, sola o en col·laboració amb altres persones, i que no és el nom real de la persona.</rdakit:toolkitDefinition>
      <skos:prefLabel xml:lang="vi">bút danh</skos:prefLabel>
      <rdakit:toolkitLabel xml:lang="vi">bút danh</rdakit:toolkitLabel>
      <skos:definition xml:lang="vi">Tên được dùng của một cá nhân, một mình hoặc cùng với những người khác, không phải tên thật của cá nhân đó.</skos:definition>
      <rdakit:toolkitDefinition xml:lang="vi">Tên được dùng của một cá nhân, một mình hoặc cùng với những người khác, không phải tên thật của cá nhân đó.</rdakit:toolkitDefinition>
      <skos:prefLabel xml:lang="no">pseudonym</skos:prefLabel>
      <rdakit:toolkitLabel xml:lang="no">pseudonym</rdakit:toolkitLabel>
      <skos:definition xml:lang="no">Et navn som blir brukt av en person, enten alene eller i samarbeid med andre, men som ikke er personens virkelige navn.</skos:definition>
      <rdakit:toolkitDefinition xml:lang="no">Et navn som blir brukt av en person, enten alene eller i samarbeid med andre, men som ikke er personens virkelige navn.</rdakit:toolkitDefinition>
    </skos:Concept>
<!-- Concept: reference  -->
    <skos:Concept rdf:about="http://rdaregistry.info/termList/RDATerms/1073" xml:lang="en">
      <skos:inScheme rdf:resource="http://rdaregistry.info/termList/RDATerms"/>
      <reg:status rdf:resource="http://metadataregistry.org/uri/RegStatus/1001"/>
      <reg:identifier rdf:resource="http://metadataregistry.org/concepts/8588"/>
      <skos:prefLabel xml:lang="en">reference</skos:prefLabel>
      <rdakit:toolkitLabel xml:lang="en">reference</rdakit:toolkitLabel>
      <skos:definition xml:lang="en">A direction from one access point to another.</skos:definition>
      <rdakit:toolkitDefinition xml:lang="en">A direction from one access point to another.</rdakit:toolkitDefinition>
      <skos:prefLabel xml:lang="it">rinvio</skos:prefLabel>
      <rdakit:toolkitLabel xml:lang="it">rinvio</rdakit:toolkitLabel>
      <skos:definition xml:lang="it">Rimando da un punto d'accesso a un altro.</skos:definition>
      <rdakit:toolkitDefinition xml:lang="it">Rimando da un punto d'accesso a un altro.</rdakit:toolkitDefinition>
      <skos:prefLabel xml:lang="de">Verweisung</skos:prefLabel>
      <rdakit:toolkitLabel xml:lang="de">Verweisung</rdakit:toolkitLabel>
      <skos:definition xml:lang="de">Ein Hinweis von einem Sucheinstieg auf einen anderen.</skos:definition>
      <rdakit:toolkitDefinition xml:lang="de">Ein Hinweis von einem Sucheinstieg auf einen anderen.</rdakit:toolkitDefinition>
      <skos:prefLabel xml:lang="fi">viittaus</skos:prefLabel>
      <rdakit:toolkitLabel xml:lang="fi">viittaus</rdakit:toolkitLabel>
      <skos:definition xml:lang="fi">Ohjaus hakutiedosta toiseen.</skos:definition>
      <rdakit:toolkitDefinition xml:lang="fi">Ohjaus hakutiedosta toiseen.</rdakit:toolkitDefinition>
      <skos:prefLabel xml:lang="da">henvisning</skos:prefLabel>
      <rdakit:toolkitLabel xml:lang="da">henvisning</rdakit:toolkitLabel>
      <skos:definition xml:lang="da">Reference fra én søgeindgang til en anden.</skos:definition>
      <rdakit:toolkitDefinition xml:lang="da">Reference fra én søgeindgang til en anden.</rdakit:toolkitDefinition>
      <skos:prefLabel xml:lang="ca">referència</skos:prefLabel>
      <rdakit:toolkitLabel xml:lang="ca">referència</rdakit:toolkitLabel>
      <skos:definition xml:lang="ca">Orientació d’un punt d’accés a un altre.</skos:definition>
      <rdakit:toolkitDefinition xml:lang="ca">Orientació d’un punt d’accés a un altre.</rdakit:toolkitDefinition>
      <skos:prefLabel xml:lang="fr">renvoi</skos:prefLabel>
      <rdakit:toolkitLabel xml:lang="fr">renvoi</rdakit:toolkitLabel>
      <skos:definition xml:lang="fr">Orientation d’un point d’accès vers un autre.</skos:definition>
      <rdakit:toolkitDefinition xml:lang="fr">Orientation d’un point d’accès vers un autre.</rdakit:toolkitDefinition>
      <skos:prefLabel xml:lang="vi">tra cứu</skos:prefLabel>
      <rdakit:toolkitLabel xml:lang="vi">tra cứu</rdakit:toolkitLabel>
      <skos:definition xml:lang="vi">Hướng dẫn từ một điểm truy cập tới điểm truy cập khác.</skos:definition>
      <rdakit:toolkitDefinition xml:lang="vi">Hướng dẫn từ một điểm truy cập tới điểm truy cập khác.</rdakit:toolkitDefinition>
      <skos:prefLabel xml:lang="no">henvisning</skos:prefLabel>
      <rdakit:toolkitLabel xml:lang="no">henvisning</rdakit:toolkitLabel>
      <skos:definition xml:lang="no">En peker fra en søkeinngang til en annen.</skos:definition>
      <rdakit:toolkitDefinition xml:lang="no">En peker fra en søkeinngang til en annen.</rdakit:toolkitDefinition>
    </skos:Concept>
<!-- Concept: reference source  -->
    <skos:Concept rdf:about="http://rdaregistry.info/termList/RDATerms/1074" xml:lang="en">
      <skos:inScheme rdf:resource="http://rdaregistry.info/termList/RDATerms"/>
      <reg:status rdf:resource="http://metadataregistry.org/uri/RegStatus/1001"/>
      <reg:identifier rdf:resource="http://metadataregistry.org/concepts/8589"/>
      <skos:prefLabel xml:lang="en">reference source</skos:prefLabel>
      <rdakit:toolkitLabel xml:lang="en">reference source</rdakit:toolkitLabel>
      <skos:definition xml:lang="en">A source from which authoritative information may be obtained.</skos:definition>
      <rdakit:toolkitDefinition xml:lang="en">A source from which authoritative information may be obtained.</rdakit:toolkitDefinition>
      <skos:scopeNote xml:lang="en">A reference source includes an authority file, a reference work, etc.</skos:scopeNote>
      <skos:prefLabel xml:lang="it">fonte di reference</skos:prefLabel>
      <rdakit:toolkitLabel xml:lang="it">fonte di reference</rdakit:toolkitLabel>
      <skos:definition xml:lang="it">Qualsiasi fonte da cui si possano ottenere informazioni autorevoli, compresi gli archivi di autorità, opere di consultazione, etc.</skos:definition>
      <rdakit:toolkitDefinition xml:lang="it">Qualsiasi fonte da cui si possano ottenere informazioni autorevoli, compresi gli archivi di autorità, opere di consultazione, etc.</rdakit:toolkitDefinition>
      <skos:prefLabel xml:lang="fr">source de référence</skos:prefLabel>
      <rdakit:toolkitLabel xml:lang="fr">source de référence</rdakit:toolkitLabel>
      <skos:definition xml:lang="fr">Source dans laquelle il est possible de puiser des informations faisant autorité.</skos:definition>
      <rdakit:toolkitDefinition xml:lang="fr">Source dans laquelle il est possible de puiser des informations faisant autorité.</rdakit:toolkitDefinition>
      <skos:prefLabel xml:lang="es">fuente de referencia</skos:prefLabel>
      <rdakit:toolkitLabel xml:lang="es">fuente de referencia</rdakit:toolkitLabel>
      <skos:definition xml:lang="es">Toda fuente de la cual se ha obtenido información autorizada.</skos:definition>
      <rdakit:toolkitDefinition xml:lang="es">Toda fuente de la cual se ha obtenido información autorizada.</rdakit:toolkitDefinition>
      <skos:scopeNote xml:lang="es">Incluye archivos de autoridad, fuentes de referencia, etc.</skos:scopeNote>
      <skos:prefLabel xml:lang="de">Nachschlagewerk</skos:prefLabel>
      <rdakit:toolkitLabel xml:lang="de">Nachschlagewerk</rdakit:toolkitLabel>
      <skos:definition xml:lang="de">Eine Quelle, aus der verlässliche Informationen bezogen werden können.</skos:definition>
      <rdakit:toolkitDefinition xml:lang="de">Eine Quelle, aus der verlässliche Informationen bezogen werden können.</rdakit:toolkitDefinition>
      <skos:scopeNote xml:lang="de">Dazu gehören Normdaten, Nachschlagewerke usw.</skos:scopeNote>
      <skos:prefLabel xml:lang="fi">tietolähde</skos:prefLabel>
      <rdakit:toolkitLabel xml:lang="fi">tietolähde</rdakit:toolkitLabel>
      <skos:definition xml:lang="fi">Mikä tahansa lähde, josta auktoritatiivinen tieto voidaan saada.</skos:definition>
      <rdakit:toolkitDefinition xml:lang="fi">Mikä tahansa lähde, josta auktoritatiivinen tieto voidaan saada.</rdakit:toolkitDefinition>
      <skos:scopeNote xml:lang="fi">Tietolähde käsittää auktoriteettitiedostot, tietosanakirjat jne.</skos:scopeNote>
      <skos:prefLabel xml:lang="da">kilde</skos:prefLabel>
      <rdakit:toolkitLabel xml:lang="da">kilde</rdakit:toolkitLabel>
      <skos:definition xml:lang="da">Kilde, hvorfra pålidelige oplysninger kan hentes.</skos:definition>
      <rdakit:toolkitDefinition xml:lang="da">Kilde, hvorfra pålidelige oplysninger kan hentes.</rdakit:toolkitDefinition>
      <skos:scopeNote xml:lang="da">En kilde omfatter autoritetsfiler, referenceværker etc.</skos:scopeNote>
      <skos:prefLabel xml:lang="ca">font de referència</skos:prefLabel>
      <rdakit:toolkitLabel xml:lang="ca">font de referència</rdakit:toolkitLabel>
      <skos:definition xml:lang="ca">Font a partir de la qual es pot obtenir informació autoritzada.</skos:definition>
      <rdakit:toolkitDefinition xml:lang="ca">Font a partir de la qual es pot obtenir informació autoritzada.</rdakit:toolkitDefinition>
      <skos:scopeNote xml:lang="ca">Una font de referència inclou un fitxer d’autoritat, una obra de referència, etc.</skos:scopeNote>
      <skos:scopeNote xml:lang="fr">Comprend un fichier d’autorité, un ouvrage de référence, etc.</skos:scopeNote>
      <skos:prefLabel xml:lang="vi">nguồn tra cứu</skos:prefLabel>
      <rdakit:toolkitLabel xml:lang="vi">nguồn tra cứu</rdakit:toolkitLabel>
      <skos:definition xml:lang="vi">Nguồn bất kỳ mà thông tin xác thực có thể được nhận,</skos:definition>
      <rdakit:toolkitDefinition xml:lang="vi">Nguồn bất kỳ mà thông tin xác thực có thể được nhận,</rdakit:toolkitDefinition>
      <skos:scopeNote xml:lang="vi">Nguồn tra cứu bao gồm các tệp chuẩn, tác phẩm tra cứu, v.v...</skos:scopeNote>
      <skos:prefLabel xml:lang="no">kilde for referanse</skos:prefLabel>
      <rdakit:toolkitLabel xml:lang="no">kilde for referanse</rdakit:toolkitLabel>
      <skos:definition xml:lang="no">En kilde hvor autoritativ informasjon kan hentes fra.</skos:definition>
      <rdakit:toolkitDefinition xml:lang="no">En kilde hvor autoritativ informasjon kan hentes fra.</rdakit:toolkitDefinition>
      <skos:scopeNote xml:lang="no">En kilde for referanse inkluderer autoritetsfiler, referanseverk etc.</skos:scopeNote>
    </skos:Concept>
<!-- Concept: related resource  -->
    <skos:Concept rdf:about="http://rdaregistry.info/termList/RDATerms/1107" xml:lang="en">
      <skos:inScheme rdf:resource="http://rdaregistry.info/termList/RDATerms"/>
      <reg:status rdf:resource="http://metadataregistry.org/uri/RegStatus/1001"/>
      <reg:identifier rdf:resource="http://metadataregistry.org/concepts/8622"/>
      <skos:prefLabel xml:lang="en">related resource</skos:prefLabel>
      <rdakit:toolkitLabel xml:lang="en">related resource</rdakit:toolkitLabel>
      <skos:definition xml:lang="en">A resource related to another resource.</skos:definition>
      <rdakit:toolkitDefinition xml:lang="en">A resource related to another resource.</rdakit:toolkitDefinition>
      <skos:prefLabel xml:lang="de">In Beziehung stehende Ressource</skos:prefLabel>
      <rdakit:toolkitLabel xml:lang="de">In Beziehung stehende Ressource</rdakit:toolkitLabel>
      <skos:definition xml:lang="de">Eine Ressource, die mit einer anderen Ressource in Beziehung steht.</skos:definition>
      <rdakit:toolkitDefinition xml:lang="de">Eine Ressource, die mit einer anderen Ressource in Beziehung steht.</rdakit:toolkitDefinition>
      <skos:prefLabel xml:lang="fi">liittyvä aineisto</skos:prefLabel>
      <rdakit:toolkitLabel xml:lang="fi">liittyvä aineisto</rdakit:toolkitLabel>
      <skos:definition xml:lang="fi">Aineisto, joka liittyy toiseen aineistoon.</skos:definition>
      <rdakit:toolkitDefinition xml:lang="fi">Aineisto, joka liittyy toiseen aineistoon.</rdakit:toolkitDefinition>
      <skos:prefLabel xml:lang="da">relateret ressource</skos:prefLabel>
      <rdakit:toolkitLabel xml:lang="da">relateret ressource</rdakit:toolkitLabel>
      <skos:definition xml:lang="da">En ressource relatert til en anden ressource.</skos:definition>
      <rdakit:toolkitDefinition xml:lang="da">En ressource relatert til en anden ressource.</rdakit:toolkitDefinition>
      <skos:prefLabel xml:lang="ca">recurs relacionat</skos:prefLabel>
      <rdakit:toolkitLabel xml:lang="ca">recurs relacionat</rdakit:toolkitLabel>
      <skos:definition xml:lang="ca">Recurs que es relaciona amb un altre recurs.</skos:definition>
      <rdakit:toolkitDefinition xml:lang="ca">Recurs que es relaciona amb un altre recurs.</rdakit:toolkitDefinition>
      <skos:prefLabel xml:lang="fr">ressource en relation</skos:prefLabel>
      <rdakit:toolkitLabel xml:lang="fr">ressource en relation</rdakit:toolkitLabel>
      <skos:definition xml:lang="fr">Ressource qui est en relation avec une autre ressource.</skos:definition>
      <rdakit:toolkitDefinition xml:lang="fr">Ressource qui est en relation avec une autre ressource.</rdakit:toolkitDefinition>
      <skos:prefLabel xml:lang="vi">tài nguyên có liên quan</skos:prefLabel>
      <rdakit:toolkitLabel xml:lang="vi">tài nguyên có liên quan</rdakit:toolkitLabel>
      <skos:definition xml:lang="vi">Tài nguyên có liên quan tới tài nguyên khác.</skos:definition>
      <rdakit:toolkitDefinition xml:lang="vi">Tài nguyên có liên quan tới tài nguyên khác.</rdakit:toolkitDefinition>
      <skos:prefLabel xml:lang="no">tilknyttet ressurs</skos:prefLabel>
      <rdakit:toolkitLabel xml:lang="no">tilknyttet ressurs</rdakit:toolkitLabel>
      <skos:definition xml:lang="no">En ressurs knyttet til en annen ressurs.</skos:definition>
      <rdakit:toolkitDefinition xml:lang="no">En ressurs knyttet til en annen ressurs.</rdakit:toolkitDefinition>
    </skos:Concept>
<!-- Concept: relationship designator  -->
    <skos:Concept rdf:about="http://rdaregistry.info/termList/RDATerms/1075" xml:lang="en">
      <skos:inScheme rdf:resource="http://rdaregistry.info/termList/RDATerms"/>
      <reg:status rdf:resource="http://metadataregistry.org/uri/RegStatus/1001"/>
      <reg:identifier rdf:resource="http://metadataregistry.org/concepts/8590"/>
      <skos:prefLabel xml:lang="en">relationship designator</skos:prefLabel>
      <rdakit:toolkitLabel xml:lang="en">relationship designator</rdakit:toolkitLabel>
      <skos:definition xml:lang="en">A designator that indicates the nature of a relationship between entities represented by authorized access points, descriptions, and/or identifiers.</skos:definition>
      <rdakit:toolkitDefinition xml:lang="en">A designator that indicates the nature of a relationship between entities represented by authorized access points, descriptions, and/or identifiers.</rdakit:toolkitDefinition>
      <skos:prefLabel xml:lang="it">designatore di relazione</skos:prefLabel>
      <rdakit:toolkitLabel xml:lang="it">designatore di relazione</rdakit:toolkitLabel>
      <skos:definition xml:lang="it">Designatore che indica la natura della relazione tra entità rappresentate da un punto d'accesso autorizzato, descrizioni e/o identificatori.</skos:definition>
      <rdakit:toolkitDefinition xml:lang="it">Designatore che indica la natura della relazione tra entità rappresentate da un punto d'accesso autorizzato, descrizioni e/o identificatori.</rdakit:toolkitDefinition>
      <skos:prefLabel xml:lang="fr">indicateur de relation</skos:prefLabel>
      <rdakit:toolkitLabel xml:lang="fr">indicateur de relation</rdakit:toolkitLabel>
      <skos:definition xml:lang="fr">Indicateur qui définit la nature d’une relation entre des entités représentées par des points d’accès autorisés, des descriptions et/ou des identifiants.</skos:definition>
      <rdakit:toolkitDefinition xml:lang="fr">Indicateur qui définit la nature d’une relation entre des entités représentées par des points d’accès autorisés, des descriptions et/ou des identifiants.</rdakit:toolkitDefinition>
      <skos:prefLabel xml:lang="es">designador de relación</skos:prefLabel>
      <rdakit:toolkitLabel xml:lang="es">designador de relación</rdakit:toolkitLabel>
      <skos:definition xml:lang="es">Designador que indica la naturaleza de la relación entre las entidades representadas mediante puntos de acceso autorizados, descriptores y/o identificadores.</skos:definition>
      <rdakit:toolkitDefinition xml:lang="es">Designador que indica la naturaleza de la relación entre las entidades representadas mediante puntos de acceso autorizados, descriptores y/o identificadores.</rdakit:toolkitDefinition>
      <skos:prefLabel xml:lang="de">Beziehungskennzeichnung</skos:prefLabel>
      <rdakit:toolkitLabel xml:lang="de">Beziehungskennzeichnung</rdakit:toolkitLabel>
      <skos:definition xml:lang="de">Eine Kennzeichnung für die Art der Beziehung zwischen Entitäten, die durch normierte Sucheinstiege, Beschreibungen und/oder Identifikatoren repräsentiert werden.</skos:definition>
      <rdakit:toolkitDefinition xml:lang="de">Eine Kennzeichnung für die Art der Beziehung zwischen Entitäten, die durch normierte Sucheinstiege, Beschreibungen und/oder Identifikatoren repräsentiert werden.</rdakit:toolkitDefinition>
      <skos:prefLabel xml:lang="fi">suhteen määrite</skos:prefLabel>
      <rdakit:toolkitLabel xml:lang="fi">suhteen määrite</rdakit:toolkitLabel>
      <skos:definition xml:lang="fi">Määrite, joka kertoo auktorisoitujen hakutietojen, kuvailun ja/tai tunnisteiden edustamien entiteettien välisen suhteen luonteen.</skos:definition>
      <rdakit:toolkitDefinition xml:lang="fi">Määrite, joka kertoo auktorisoitujen hakutietojen, kuvailun ja/tai tunnisteiden edustamien entiteettien välisen suhteen luonteen.</rdakit:toolkitDefinition>
      <skos:prefLabel xml:lang="da">relationsbetegnelse</skos:prefLabel>
      <rdakit:toolkitLabel xml:lang="da">relationsbetegnelse</rdakit:toolkitLabel>
      <skos:definition xml:lang="da">Betegnelse, der angiver arten af den relation mellem entiteter, der er repræsenteret af autoriserede søgeindgange, beskrivelser og/eller identifikatorer.</skos:definition>
      <rdakit:toolkitDefinition xml:lang="da">Betegnelse, der angiver arten af den relation mellem entiteter, der er repræsenteret af autoriserede søgeindgange, beskrivelser og/eller identifikatorer.</rdakit:toolkitDefinition>
      <skos:prefLabel xml:lang="ca">designador de relació</skos:prefLabel>
      <rdakit:toolkitLabel xml:lang="ca">designador de relació</rdakit:toolkitLabel>
      <skos:definition xml:lang="ca">Designador que indica la natura d'una relació entre les entitats representades per punts d’accés autoritzats, descripcions i/o identificadors.</skos:definition>
      <rdakit:toolkitDefinition xml:lang="ca">Designador que indica la natura d'una relació entre les entitats representades per punts d’accés autoritzats, descripcions i/o identificadors.</rdakit:toolkitDefinition>
      <skos:prefLabel xml:lang="vi">chỉ định mối quan hệ</skos:prefLabel>
      <rdakit:toolkitLabel xml:lang="vi">chỉ định mối quan hệ</rdakit:toolkitLabel>
      <skos:definition xml:lang="vi">Chỉ định mối quan hệ chỉ ra bản chất của mối quan hệ giữa các thực thể được trình bày bằng các điểm truy cập được phép, mô tả, và/hoặc chỉ số nhận dạng.</skos:definition>
      <rdakit:toolkitDefinition xml:lang="vi">Chỉ định mối quan hệ chỉ ra bản chất của mối quan hệ giữa các thực thể được trình bày bằng các điểm truy cập được phép, mô tả, và/hoặc chỉ số nhận dạng.</rdakit:toolkitDefinition>
      <skos:prefLabel xml:lang="no">relasjonsbetegnelse</skos:prefLabel>
      <rdakit:toolkitLabel xml:lang="no">relasjonsbetegnelse</rdakit:toolkitLabel>
      <skos:definition xml:lang="no">En betegnelse som angir tilknytningsformen mellom entiteter representert ved autoriserte søkeinnganger, beskrivelser og/eller identifikatorer.</skos:definition>
      <rdakit:toolkitDefinition xml:lang="no">En betegnelse som angir tilknytningsformen mellom entiteter representert ved autoriserte søkeinnganger, beskrivelser og/eller identifikatorer.</rdakit:toolkitDefinition>
    </skos:Concept>
<!-- Concept: reproduction  -->
    <skos:Concept rdf:about="http://rdaregistry.info/termList/RDATerms/1076" xml:lang="en">
      <skos:inScheme rdf:resource="http://rdaregistry.info/termList/RDATerms"/>
      <reg:status rdf:resource="http://metadataregistry.org/uri/RegStatus/1001"/>
      <reg:identifier rdf:resource="http://metadataregistry.org/concepts/8591"/>
      <skos:prefLabel xml:lang="en">reproduction</skos:prefLabel>
      <rdakit:toolkitLabel xml:lang="en">reproduction</rdakit:toolkitLabel>
      <skos:definition xml:lang="en">An exact copy of the content of a manifestation or item made by mechanical or electronic means.</skos:definition>
      <rdakit:toolkitDefinition xml:lang="en">An exact copy of the content of a manifestation or item made by mechanical or electronic means.</rdakit:toolkitDefinition>
      <skos:prefLabel xml:lang="it">riproduzione</skos:prefLabel>
      <rdakit:toolkitLabel xml:lang="it">riproduzione</rdakit:toolkitLabel>
      <skos:definition xml:lang="it">Copia esatta del contenuto di una risorsa ottenuta mediante mezzi meccanici o elettronici.</skos:definition>
      <rdakit:toolkitDefinition xml:lang="it">Copia esatta del contenuto di una risorsa ottenuta mediante mezzi meccanici o elettronici.</rdakit:toolkitDefinition>
      <skos:prefLabel xml:lang="fr">reproduction</skos:prefLabel>
      <rdakit:toolkitLabel xml:lang="fr">reproduction</rdakit:toolkitLabel>
      <skos:definition xml:lang="fr">Copie exacte du contenu d’une manifestation ou d’un item faite par un moyen mécanique ou électronique.</skos:definition>
      <skos:prefLabel xml:lang="es">reproducción</skos:prefLabel>
      <rdakit:toolkitLabel xml:lang="es">reproducción</rdakit:toolkitLabel>
      <skos:definition xml:lang="es">Copia exacta del contenido de un recurso, creada mediante medios mecánicos o electrónicos.</skos:definition>
      <rdakit:toolkitDefinition xml:lang="es">Copia exacta del contenido de un recurso, creada mediante medios mecánicos o electrónicos.</rdakit:toolkitDefinition>
      <skos:prefLabel xml:lang="de">Reproduktion</skos:prefLabel>
      <rdakit:toolkitLabel xml:lang="de">Reproduktion</rdakit:toolkitLabel>
      <skos:definition xml:lang="de">Eine exakte Kopie des Inhalts einer Manifestation, die mit mechanischen oder elektronischen Mitteln erstellt ist.</skos:definition>
      <rdakit:toolkitDefinition xml:lang="de">Eine exakte Kopie des Inhalts einer Manifestation, die mit mechanischen oder elektronischen Mitteln erstellt ist.</rdakit:toolkitDefinition>
      <skos:prefLabel xml:lang="fi">jäljenne</skos:prefLabel>
      <rdakit:toolkitLabel xml:lang="fi">jäljenne</rdakit:toolkitLabel>
      <skos:definition xml:lang="fi">Manifestaation tai kappaleen sisällön tarkka kopio, joka on tuotettu mekaanisilla tai elektronisilla välineillä.</skos:definition>
      <rdakit:toolkitDefinition xml:lang="fi">Manifestaation tai kappaleen sisällön tarkka kopio, joka on tuotettu mekaanisilla tai elektronisilla välineillä.</rdakit:toolkitDefinition>
      <skos:prefLabel xml:lang="da">reproduktion</skos:prefLabel>
      <rdakit:toolkitLabel xml:lang="da">reproduktion</rdakit:toolkitLabel>
      <skos:definition xml:lang="da">Nøjagtig kopi af en ressources indhold, fremstillet vha. mekaniske eller elektroniske midler.</skos:definition>
      <rdakit:toolkitDefinition xml:lang="da">Nøjagtig kopi af en ressources indhold, fremstillet vha. mekaniske eller elektroniske midler.</rdakit:toolkitDefinition>
      <skos:prefLabel xml:lang="ca">reproducció</skos:prefLabel>
      <rdakit:toolkitLabel xml:lang="ca">reproducció</rdakit:toolkitLabel>
      <skos:definition xml:lang="ca">Còpia exacta del contingut d’una manifestació o d'un ítem feta amb mitjans mecànics o electrònics.</skos:definition>
      <rdakit:toolkitDefinition xml:lang="ca">Còpia exacta del contingut d’una manifestació o d'un ítem feta amb mitjans mecànics o electrònics.</rdakit:toolkitDefinition>
      <rdakit:toolkitDefinition xml:lang="fr">Copie exacte du contenu d’une manifestation ou d’un item faite par un moyen mécanique ou électronique.</rdakit:toolkitDefinition>
      <skos:prefLabel xml:lang="vi">Nhân bản</skos:prefLabel>
      <rdakit:toolkitLabel xml:lang="vi">Nhân bản</rdakit:toolkitLabel>
      <skos:definition xml:lang="vi">Bản sao chính xác về nội dung của một tài nguyên được tạo ra bằng phương tiện cơ học hoặc điện tử.</skos:definition>
      <rdakit:toolkitDefinition xml:lang="vi">Bản sao chính xác về nội dung của một tài nguyên được tạo ra bằng phương tiện cơ học hoặc điện tử.</rdakit:toolkitDefinition>
      <skos:prefLabel xml:lang="no">reproduksjon</skos:prefLabel>
      <rdakit:toolkitLabel xml:lang="no">reproduksjon</rdakit:toolkitLabel>
      <skos:definition xml:lang="no">En tro kopi av innholdet til en manifestasjon eller et eksemplar, fremstilt mekanisk eller elektronisk.</skos:definition>
      <rdakit:toolkitDefinition xml:lang="no">En tro kopi av innholdet til en manifestasjon eller et eksemplar, fremstilt mekanisk eller elektronisk.</rdakit:toolkitDefinition>
    </skos:Concept>
<!-- Concept: resource  -->
    <skos:Concept rdf:about="http://rdaregistry.info/termList/RDATerms/1077" xml:lang="en">
      <skos:inScheme rdf:resource="http://rdaregistry.info/termList/RDATerms"/>
      <reg:status rdf:resource="http://metadataregistry.org/uri/RegStatus/1001"/>
      <reg:identifier rdf:resource="http://metadataregistry.org/concepts/8592"/>
      <skos:prefLabel xml:lang="en">resource</skos:prefLabel>
      <rdakit:toolkitLabel xml:lang="en">resource</rdakit:toolkitLabel>
      <skos:definition xml:lang="en">A work, expression, manifestation or item.</skos:definition>
      <rdakit:toolkitDefinition xml:lang="en">A work, expression, manifestation or item.</rdakit:toolkitDefinition>
      <skos:scopeNote xml:lang="en">A resource can be an individual entity, an aggregate, or a component of such an entity.  It can be a tangible or intangible entity.</skos:scopeNote>
      <skos:prefLabel xml:lang="it">risorsa</skos:prefLabel>
      <rdakit:toolkitLabel xml:lang="it">risorsa</rdakit:toolkitLabel>
      <skos:definition xml:lang="it">Opera, espressione, manifestazione o item.</skos:definition>
      <rdakit:toolkitDefinition xml:lang="it">Opera, espressione, manifestazione o item.</rdakit:toolkitDefinition>
      <skos:scopeNote xml:lang="it">Il termine include non solo un'entità individuale ma anche aggregati e componenti di tali entità (per esempio, tre fogli di carte geografiche, una diapositiva singola pubblicata come parte di un insieme di venti diapositive, l'articolo di un fascicolo di un giornale accademico). Può indicare un'entità tangibile (per esempio, un'audiocassetta) o un'entità intangibile (per esempio, un sito web).</skos:scopeNote>
      <skos:prefLabel xml:lang="fr">ressource</skos:prefLabel>
      <rdakit:toolkitLabel xml:lang="fr">ressource</rdakit:toolkitLabel>
      <skos:definition xml:lang="fr">Œuvre, expression, manifestation ou item.</skos:definition>
      <rdakit:toolkitDefinition xml:lang="fr">Œuvre, expression, manifestation ou item.</rdakit:toolkitDefinition>
      <skos:scopeNote xml:lang="fr">Une ressource peut être une entité individuelle, un agrégat ou une composante de ces entités. Il peut s’agir d’une entité matérielle ou immatérielle.</skos:scopeNote>
      <skos:prefLabel xml:lang="es">recurso</skos:prefLabel>
      <rdakit:toolkitLabel xml:lang="es">recurso</rdakit:toolkitLabel>
      <skos:definition xml:lang="es">Obra, expresión, manifestación o ítem.</skos:definition>
      <rdakit:toolkitDefinition xml:lang="es">Obra, expresión, manifestación o ítem.</rdakit:toolkitDefinition>
      <skos:scopeNote xml:lang="es">El término incluye no solamente a una entidad individual sino también a los agregados y los componentes de dichas entidades (p.ej., mapas de tres hojas; una diapositiva individual que forma parte de un conjunto de veinte; o un artículo de una entrega de una revista especializada). Puede referirse a una entidad tangible (p.ej., un audiocasete) o a una entidad intangible (p.ej., un sitio Web)</skos:scopeNote>
      <skos:prefLabel xml:lang="de">Ressource</skos:prefLabel>
      <rdakit:toolkitLabel xml:lang="de">Ressource</rdakit:toolkitLabel>
      <skos:definition xml:lang="de">Ein Werk, eine Expression, eine Manifestation oder ein Exemplar.</skos:definition>
      <rdakit:toolkitDefinition xml:lang="de">Ein Werk, eine Expression, eine Manifestation oder ein Exemplar.</rdakit:toolkitDefinition>
      <skos:scopeNote xml:lang="de">Eine Ressource kann eine individuelle Entität, ein Aggregat oder ein Bestandteil einer solcher Entität sein. Sie kann sich auf eine materielle Entität oder eine nicht anfassbare Entität beziehen.</skos:scopeNote>
      <skos:prefLabel xml:lang="fi">aineisto</skos:prefLabel>
      <rdakit:toolkitLabel xml:lang="fi">aineisto</rdakit:toolkitLabel>
      <skos:definition xml:lang="fi">Teos, ekspressio, manifestaatio tai kappale.</skos:definition>
      <rdakit:toolkitDefinition xml:lang="fi">Teos, ekspressio, manifestaatio tai kappale.</rdakit:toolkitDefinition>
      <skos:scopeNote xml:lang="fi">Termi aineisto voi viitata paitsi yksittäiseen entiteettiin myös aggregaatteihin ja entiteettien osiin. Se voi viitata joko käsin kosketeltavaan tai aineettomaan entiteettiin.</skos:scopeNote>
      <skos:prefLabel xml:lang="da">ressource</skos:prefLabel>
      <rdakit:toolkitLabel xml:lang="da">ressource</rdakit:toolkitLabel>
      <skos:definition xml:lang="da">Værk, udtryk, manifestation eller eksemplar.</skos:definition>
      <rdakit:toolkitDefinition xml:lang="da">Værk, udtryk, manifestation eller eksemplar.</rdakit:toolkitDefinition>
      <skos:scopeNote xml:lang="da">En ressource kan omfatte en individuel entitet, en samling, eller en komponent af en sådan entitet. Den kan være en fysisk eller ikke-fysisk entitet.</skos:scopeNote>
      <skos:prefLabel xml:lang="ca">recurs</skos:prefLabel>
      <rdakit:toolkitLabel xml:lang="ca">recurs</rdakit:toolkitLabel>
      <skos:definition xml:lang="ca">Obra, expressió, manifestació o ítem.</skos:definition>
      <rdakit:toolkitDefinition xml:lang="ca">Obra, expressió, manifestació o ítem.</rdakit:toolkitDefinition>
      <skos:scopeNote xml:lang="ca">Un recurs pot ser una entitat individual, un agregat o un component d’aquesta entitat. Pot ser una entitat tangible o intangible.</skos:scopeNote>
      <skos:prefLabel xml:lang="vi">tài nguyên</skos:prefLabel>
      <rdakit:toolkitLabel xml:lang="vi">tài nguyên</rdakit:toolkitLabel>
      <skos:definition xml:lang="vi">Tác phẩm, biểu hiện, biểu thị hoặc bản.</skos:definition>
      <rdakit:toolkitDefinition xml:lang="vi">Tác phẩm, biểu hiện, biểu thị hoặc bản.</rdakit:toolkitDefinition>
      <skos:scopeNote xml:lang="vi">Tài nguyên có thể là thực thể riêng lẻ, tập hợp, thành phần của thực thể. Nó có thể là thực thể hữu hình hoặc vô hình.</skos:scopeNote>
      <skos:prefLabel xml:lang="no">ressurs</skos:prefLabel>
      <rdakit:toolkitLabel xml:lang="no">ressurs</rdakit:toolkitLabel>
      <skos:definition xml:lang="no">Et verk, et uttrykk, en manifestasjon eller et eksemplar.</skos:definition>
      <rdakit:toolkitDefinition xml:lang="no">Et verk, et uttrykk, en manifestasjon eller et eksemplar.</rdakit:toolkitDefinition>
      <skos:scopeNote xml:lang="no">En ressurs kan være en enkeltstående entitet, en samling eller et element av en slik entitet. Entiteten kan være håndgripelig eller uhåndgripelig.</skos:scopeNote>
    </skos:Concept>
<!-- Concept: running title  -->
    <skos:Concept rdf:about="http://rdaregistry.info/termList/RDATerms/1078" xml:lang="en">
      <skos:inScheme rdf:resource="http://rdaregistry.info/termList/RDATerms"/>
      <reg:status rdf:resource="http://metadataregistry.org/uri/RegStatus/1001"/>
      <reg:identifier rdf:resource="http://metadataregistry.org/concepts/8593"/>
      <skos:prefLabel xml:lang="en">running title</skos:prefLabel>
      <rdakit:toolkitLabel xml:lang="en">running title</rdakit:toolkitLabel>
      <skos:definition xml:lang="en">A title, or abbreviated title, that is repeated at the head or foot of each page or leaf.</skos:definition>
      <rdakit:toolkitDefinition xml:lang="en">A title, or abbreviated title, that is repeated at the head or foot of each page or leaf.</rdakit:toolkitDefinition>
      <skos:prefLabel xml:lang="fr">titre courant</skos:prefLabel>
      <rdakit:toolkitLabel xml:lang="fr">titre courant</rdakit:toolkitLabel>
      <skos:definition xml:lang="fr">Titre, ou titre abrégé, répété en tête ou en pied de chaque page ou feuillet.</skos:definition>
      <rdakit:toolkitDefinition xml:lang="fr">Titre, ou titre abrégé, répété en tête ou en pied de chaque page ou feuillet.</rdakit:toolkitDefinition>
      <skos:prefLabel xml:lang="de">Kolumnentitel</skos:prefLabel>
      <rdakit:toolkitLabel xml:lang="de">Kolumnentitel</rdakit:toolkitLabel>
      <skos:definition xml:lang="de">Ein Titel oder ein Kurztitel, der in der Kopf- oder Fußzeile jeder Seite oder jedes Blattes wiederholt wird.</skos:definition>
      <rdakit:toolkitDefinition xml:lang="de">Ein Titel oder ein Kurztitel, der in der Kopf- oder Fußzeile jeder Seite oder jedes Blattes wiederholt wird.</rdakit:toolkitDefinition>
      <skos:prefLabel xml:lang="fi">juokseva nimeke</skos:prefLabel>
      <rdakit:toolkitLabel xml:lang="fi">juokseva nimeke</rdakit:toolkitLabel>
      <skos:definition xml:lang="fi">Nimeke tai lyhennetty nimeke, joka toistuu jokaisen sivun tai lehden ylä- tai alareunuksessa.</skos:definition>
      <rdakit:toolkitDefinition xml:lang="fi">Nimeke tai lyhennetty nimeke, joka toistuu jokaisen sivun tai lehden ylä- tai alareunuksessa.</rdakit:toolkitDefinition>
      <skos:prefLabel xml:lang="da">løbende klummetitel</skos:prefLabel>
      <rdakit:toolkitLabel xml:lang="da">løbende klummetitel</rdakit:toolkitLabel>
      <skos:definition xml:lang="da">Titel eller forkortet titel, der gentages i toppen eller bunden af hver side eller hvert blad.</skos:definition>
      <rdakit:toolkitDefinition xml:lang="da">Titel eller forkortet titel, der gentages i toppen eller bunden af hver side eller hvert blad.</rdakit:toolkitDefinition>
      <skos:prefLabel xml:lang="ca">llegenda de foli</skos:prefLabel>
      <rdakit:toolkitLabel xml:lang="ca">llegenda de foli</rdakit:toolkitLabel>
      <skos:definition xml:lang="ca">Títol, o títol abreujat, que es repeteix al capdamunt o al peu de cada pàgina o full.</skos:definition>
      <rdakit:toolkitDefinition xml:lang="ca">Títol, o títol abreujat, que es repeteix al capdamunt o al peu de cada pàgina o full.</rdakit:toolkitDefinition>
      <skos:prefLabel xml:lang="vi">nhan đề chạy</skos:prefLabel>
      <rdakit:toolkitLabel xml:lang="vi">nhan đề chạy</rdakit:toolkitLabel>
      <skos:definition xml:lang="vi">Nhan đề, hoặc nhan đề viết tắt được nhắc lại ở đầu hoặc cuối của mỗi trang hoặc tờ.</skos:definition>
      <rdakit:toolkitDefinition xml:lang="vi">Nhan đề, hoặc nhan đề viết tắt được nhắc lại ở đầu hoặc cuối của mỗi trang hoặc tờ.</rdakit:toolkitDefinition>
      <skos:prefLabel xml:lang="no">løpetittel</skos:prefLabel>
      <rdakit:toolkitLabel xml:lang="no">løpetittel</rdakit:toolkitLabel>
      <skos:definition xml:lang="no">En tittel eller forkortet tittel som er gjentatt øverst eller nederst på hver side eller blad.</skos:definition>
      <rdakit:toolkitDefinition xml:lang="no">En tittel eller forkortet tittel som er gjentatt øverst eller nederst på hver side eller blad.</rdakit:toolkitDefinition>
    </skos:Concept>
<!-- Concept: scroll  -->
    <skos:Concept rdf:about="http://rdaregistry.info/termList/RDATerms/1079" xml:lang="en">
      <skos:inScheme rdf:resource="http://rdaregistry.info/termList/RDATerms"/>
      <reg:status rdf:resource="http://metadataregistry.org/uri/RegStatus/1001"/>
      <reg:identifier rdf:resource="http://metadataregistry.org/concepts/8594"/>
      <skos:prefLabel xml:lang="en">scroll</skos:prefLabel>
      <rdakit:toolkitLabel xml:lang="en">scroll</rdakit:toolkitLabel>
      <skos:definition xml:lang="en">A single or composite sheet containing text and/or images, originally produced rolled, and intended to be unrolled a portion at a time for reading or viewing.</skos:definition>
      <rdakit:toolkitDefinition xml:lang="en">A single or composite sheet containing text and/or images, originally produced rolled, and intended to be unrolled a portion at a time for reading or viewing.</rdakit:toolkitDefinition>
      <skos:prefLabel xml:lang="de">Schriftrolle</skos:prefLabel>
      <rdakit:toolkitLabel xml:lang="de">Schriftrolle</rdakit:toolkitLabel>
      <skos:definition xml:lang="de">Ein Einzelblatt oder ein zusammengesetztes Blatt das Text und/oder Bilder beinhaltet, das ursprünglich eingerollt produziert wurde und zum Lesen oder Betrachten Stück für Stück abgerollt werden muss.</skos:definition>
      <rdakit:toolkitDefinition xml:lang="de">Ein Einzelblatt oder ein zusammengesetztes Blatt das Text und/oder Bilder beinhaltet, das ursprünglich eingerollt produziert wurde und zum Lesen oder Betrachten Stück für Stück abgerollt werden muss.</rdakit:toolkitDefinition>
      <skos:prefLabel xml:lang="fi">käärö</skos:prefLabel>
      <rdakit:toolkitLabel xml:lang="fi">käärö</rdakit:toolkitLabel>
      <skos:definition xml:lang="fi">Yksittäinen tai yhdistelty arkki, joka sisältää tekstiä ja/tai kuvia. Valmistettu alunperin rullattuna, ja tarkoitettu avattavaksi osa kerrallaan lukemista tai katselua varten.</skos:definition>
      <rdakit:toolkitDefinition xml:lang="fi">Yksittäinen tai yhdistelty arkki, joka sisältää tekstiä ja/tai kuvia. Valmistettu alunperin rullattuna, ja tarkoitettu avattavaksi osa kerrallaan lukemista tai katselua varten.</rdakit:toolkitDefinition>
      <skos:prefLabel xml:lang="da">skriftrulle</skos:prefLabel>
      <rdakit:toolkitLabel xml:lang="da">skriftrulle</rdakit:toolkitLabel>
      <skos:definition xml:lang="da">Enkelt eller sammensat ark, der indeholder tekst og/eller billeder, oprindeligt fremstillet som en rulle og beregnet til at blive rullet ud stykke for stykke for at blive læst eller set.</skos:definition>
      <rdakit:toolkitDefinition xml:lang="da">Enkelt eller sammensat ark, der indeholder tekst og/eller billeder, oprindeligt fremstillet som en rulle og beregnet til at blive rullet ud stykke for stykke for at blive læst eller set.</rdakit:toolkitDefinition>
      <skos:prefLabel xml:lang="ca">rotlle</skos:prefLabel>
      <rdakit:toolkitLabel xml:lang="ca">rotlle</rdakit:toolkitLabel>
      <skos:definition xml:lang="ca">Full sol o compost que conté text i/o imatges, que originalment va enrotllat i que està concebut perquè es desenrotlli una porció a mesura que es va llegint o visualitzant.</skos:definition>
      <rdakit:toolkitDefinition xml:lang="ca">Full sol o compost que conté text i/o imatges, que originalment va enrotllat i que està concebut perquè es desenrotlli una porció a mesura que es va llegint o visualitzant.</rdakit:toolkitDefinition>
      <skos:prefLabel xml:lang="fr">rouleau (feuille)</skos:prefLabel>
      <rdakit:toolkitLabel xml:lang="fr">rouleau (feuille)</rdakit:toolkitLabel>
      <skos:definition xml:lang="fr">Feuille simple ou composite contenant du texte et/ou des images, produite à l’origine sous forme enroulée et destinée à être déroulée une portion à la fois pour la lecture ou la consultation.</skos:definition>
      <rdakit:toolkitDefinition xml:lang="fr">Feuille simple ou composite contenant du texte et/ou des images, produite à l’origine sous forme enroulée et destinée à être déroulée une portion à la fois pour la lecture ou la consultation.</rdakit:toolkitDefinition>
      <skos:prefLabel xml:lang="vi">tờ cuộn</skos:prefLabel>
      <rdakit:toolkitLabel xml:lang="vi">tờ cuộn</rdakit:toolkitLabel>
      <skos:definition xml:lang="vi">Tờ đơn hoặc ghép có chứa văn bản và/hoặc hình ảnh, được sản xuất nguyên bản cuộn lại, và có ý định mở ra khi đọc hoặc xem.</skos:definition>
      <rdakit:toolkitDefinition xml:lang="vi">Tờ đơn hoặc ghép có chứa văn bản và/hoặc hình ảnh, được sản xuất nguyên bản cuộn lại, và có ý định mở ra khi đọc hoặc xem.</rdakit:toolkitDefinition>
      <skos:prefLabel xml:lang="no">bokrull</skos:prefLabel>
      <rdakit:toolkitLabel xml:lang="no">bokrull</rdakit:toolkitLabel>
      <skos:definition xml:lang="no">Et enkelt eller sammensatt ark som inneholder tekst og/eller bilder, opprinnelig produsert som ruller der et stykke kan rulles opp og leses eller vises om gangen.</skos:definition>
      <rdakit:toolkitDefinition xml:lang="no">Et enkelt eller sammensatt ark som inneholder tekst og/eller bilder, opprinnelig produsert som ruller der et stykke kan rulles opp og leses eller vises om gangen.</rdakit:toolkitDefinition>
    </skos:Concept>
<!-- Concept: section  -->
    <skos:Concept rdf:about="http://rdaregistry.info/termList/RDATerms/1106" xml:lang="en">
      <skos:inScheme rdf:resource="http://rdaregistry.info/termList/RDATerms"/>
      <reg:status rdf:resource="http://metadataregistry.org/uri/RegStatus/1001"/>
      <reg:identifier rdf:resource="http://metadataregistry.org/concepts/8621"/>
      <skos:prefLabel xml:lang="en">section</skos:prefLabel>
      <rdakit:toolkitLabel xml:lang="en">section</rdakit:toolkitLabel>
      <skos:definition xml:lang="en">A separately issued part of a manifestation, usually representing a particular subject category within the larger manifestation and identified by a designation that may be a topic, or an alphabetic or numeric designation, or a combination of these.</skos:definition>
      <rdakit:toolkitDefinition xml:lang="en">A separately issued part of a manifestation, usually representing a particular subject category within the larger manifestation and identified by a designation that may be a topic, or an alphabetic or numeric designation, or a combination of these.</rdakit:toolkitDefinition>
      <skos:prefLabel xml:lang="de">Untergliederung</skos:prefLabel>
      <rdakit:toolkitLabel xml:lang="de">Untergliederung</rdakit:toolkitLabel>
      <skos:definition xml:lang="de">Ein getrennt herausgegebener Teil einer Manifestation der normalerweise einen bestimmten Inhalt innerhalb der größeren Manifestation repräsentiert und durch eine Kennzeichnung identifiziert wird, die ein Thema oder eine alphanumerische Bezeichnung oder eine Kombination davon sein kann.</skos:definition>
      <rdakit:toolkitDefinition xml:lang="de">Ein getrennt herausgegebener Teil einer Manifestation der normalerweise einen bestimmten Inhalt innerhalb der größeren Manifestation repräsentiert und durch eine Kennzeichnung identifiziert wird, die ein Thema oder eine alphanumerische Bezeichnung oder eine Kombination davon sein kann.</rdakit:toolkitDefinition>
      <skos:prefLabel xml:lang="fi">lohko</skos:prefLabel>
      <rdakit:toolkitLabel xml:lang="fi">lohko</rdakit:toolkitLabel>
      <skos:definition xml:lang="fi">Erikseen julkaistu osa manifestaatiosta, joka yleensä kattaa tietyn aihealueen laajemmasta kokonaisuudesta ja joka on tunnistettavissa aiheen, aakkosellisen tai numeerisen järjestyksen mukaan tai näiden yhdistelmällä.</skos:definition>
      <rdakit:toolkitDefinition xml:lang="fi">Erikseen julkaistu osa manifestaatiosta, joka yleensä kattaa tietyn aihealueen laajemmasta kokonaisuudesta ja joka on tunnistettavissa aiheen, aakkosellisen tai numeerisen järjestyksen mukaan tai näiden yhdistelmällä.</rdakit:toolkitDefinition>
      <skos:prefLabel xml:lang="da">sektion</skos:prefLabel>
      <rdakit:toolkitLabel xml:lang="da">sektion</rdakit:toolkitLabel>
      <skos:definition xml:lang="da">Separat udgivet del af en ressource, der normalt repræsenterer en særlig emnekategori inden for en større ressource og identificeres ved en betegnelse, der kan være et tema, eller en alfabetisk eller numerisk betegnelse, eller en kombination af disse.</skos:definition>
      <rdakit:toolkitDefinition xml:lang="da">Separat udgivet del af en ressource, der normalt repræsenterer en særlig emnekategori inden for en større ressource og identificeres ved en betegnelse, der kan være et tema, eller en alfabetisk eller numerisk betegnelse, eller en kombination af disse.</rdakit:toolkitDefinition>
      <skos:prefLabel xml:lang="ca">secció</skos:prefLabel>
      <rdakit:toolkitLabel xml:lang="ca">secció</rdakit:toolkitLabel>
      <skos:definition xml:lang="ca">Part d’un recurs publicada separadament, que normalment representa una categoria temàtica concreta dins d’una manifestació més amplia, i que s’identifica amb una designació que pot ser temàtica, alfabètica o numèrica o una combinació de totes tres.</skos:definition>
      <rdakit:toolkitDefinition xml:lang="ca">Part d’un recurs publicada separadament, que normalment representa una categoria temàtica concreta dins d’una manifestació més amplia, i que s’identifica amb una designació que pot ser temàtica, alfabètica o numèrica o una combinació de totes tres.</rdakit:toolkitDefinition>
      <skos:prefLabel xml:lang="fr">section</skos:prefLabel>
      <rdakit:toolkitLabel xml:lang="fr">section</rdakit:toolkitLabel>
      <skos:definition xml:lang="fr">Partie d’une manifestation publiée séparément, traitant en général d’un domaine thématique particulier au sein de la manifestation plus vaste, identifiée par une désignation qui peut être thématique, alphabétique ou numérique ou être une combinaison de ces trois types.</skos:definition>
      <rdakit:toolkitDefinition xml:lang="fr">Partie d’une manifestation publiée séparément, traitant en général d’un domaine thématique particulier au sein de la manifestation plus vaste, identifiée par une désignation qui peut être thématique, alphabétique ou numérique ou être une combinaison de ces trois types.</rdakit:toolkitDefinition>
      <skos:prefLabel xml:lang="vi">phần</skos:prefLabel>
      <rdakit:toolkitLabel xml:lang="vi">phần</rdakit:toolkitLabel>
      <skos:definition xml:lang="vi">Một bộ phận được công bố tách biệt của một biểu thị, thường trình bày một loại chủ đề riêng bên trong tài nguyên lớn hơn đó và được nhận dạng bằng một định danh có thể là đề tài, hoặc một định danh chữ cái hoặc chữ số, hoặc tổ hợp cả hai.</skos:definition>
      <rdakit:toolkitDefinition xml:lang="vi">Một bộ phận được công bố tách biệt của một biểu thị, thường trình bày một loại chủ đề riêng bên trong tài nguyên lớn hơn đó và được nhận dạng bằng một định danh có thể là đề tài, hoặc một định danh chữ cái hoặc chữ số, hoặc tổ hợp cả hai.</rdakit:toolkitDefinition>
      <skos:prefLabel xml:lang="no">seksjon</skos:prefLabel>
      <rdakit:toolkitLabel xml:lang="no">seksjon</rdakit:toolkitLabel>
      <skos:definition xml:lang="no">En del av en manifestasjon som er utgitt alene og som vanligvis behandler et bestemt emneområde innenfor den mer omfattende manifestasjonen og har en betegnelse som kan være tematisk, alfabetisk eller numerisk eller en kombinasjon av disse.</skos:definition>
      <rdakit:toolkitDefinition xml:lang="no">En del av en manifestasjon som er utgitt alene og som vanligvis behandler et bestemt emneområde innenfor den mer omfattende manifestasjonen og har en betegnelse som kan være tematisk, alfabetisk eller numerisk eller en kombinasjon av disse.</rdakit:toolkitDefinition>
    </skos:Concept>
<!-- Concept: self-describing manifestation  -->
    <skos:Concept rdf:about="http://rdaregistry.info/termList/RDATerms/1080" xml:lang="en">
      <skos:inScheme rdf:resource="http://rdaregistry.info/termList/RDATerms"/>
      <reg:status rdf:resource="http://metadataregistry.org/uri/RegStatus/1001"/>
      <reg:identifier rdf:resource="http://metadataregistry.org/concepts/8595"/>
      <skos:prefLabel xml:lang="en">self-describing manifestation</skos:prefLabel>
      <rdakit:toolkitLabel xml:lang="en">self-describing manifestation</rdakit:toolkitLabel>
      <skos:definition xml:lang="en">A manifestation that contains identifying information.</skos:definition>
      <rdakit:toolkitDefinition xml:lang="en">A manifestation that contains identifying information.</rdakit:toolkitDefinition>
      <skos:prefLabel xml:lang="de">Selbstbeschreibende Manifestation</skos:prefLabel>
      <rdakit:toolkitLabel xml:lang="de">Selbstbeschreibende Manifestation</rdakit:toolkitLabel>
      <skos:definition xml:lang="de">Eine Manifestation, die identifizierende Informationen enthält.</skos:definition>
      <rdakit:toolkitDefinition xml:lang="de">Eine Manifestation, die identifizierende Informationen enthält.</rdakit:toolkitDefinition>
      <skos:prefLabel xml:lang="fi">kuvailua tukeva manifestaatio</skos:prefLabel>
      <rdakit:toolkitLabel xml:lang="fi">kuvailua tukeva manifestaatio</rdakit:toolkitLabel>
      <skos:definition xml:lang="fi">Tunnistamista tukevaa tietoa sisältävä manifestaatio.</skos:definition>
      <rdakit:toolkitDefinition xml:lang="fi">Tunnistamista tukevaa tietoa sisältävä manifestaatio.</rdakit:toolkitDefinition>
      <skos:prefLabel xml:lang="da">selvbeskrivende manifestation</skos:prefLabel>
      <rdakit:toolkitLabel xml:lang="da">selvbeskrivende manifestation</rdakit:toolkitLabel>
      <skos:definition xml:lang="da">Manifestation, der indeholder identificerende oplysninger.</skos:definition>
      <rdakit:toolkitDefinition xml:lang="da">Manifestation, der indeholder identificerende oplysninger.</rdakit:toolkitDefinition>
      <skos:prefLabel xml:lang="ca">manifestació que es descriu a ella mateixa</skos:prefLabel>
      <rdakit:toolkitLabel xml:lang="ca">manifestació que es descriu a ella mateixa</rdakit:toolkitLabel>
      <skos:definition xml:lang="ca">Manifestació que inclou informació identificadora.</skos:definition>
      <rdakit:toolkitDefinition xml:lang="ca">Manifestació que inclou informació identificadora.</rdakit:toolkitDefinition>
      <skos:prefLabel xml:lang="fr">manifestation autodescriptive</skos:prefLabel>
      <rdakit:toolkitLabel xml:lang="fr">manifestation autodescriptive</rdakit:toolkitLabel>
      <skos:definition xml:lang="fr">Manifestation qui contient de l’information d’identification.</skos:definition>
      <rdakit:toolkitDefinition xml:lang="fr">Manifestation qui contient de l’information d’identification.</rdakit:toolkitDefinition>
      <skos:prefLabel xml:lang="vi">biểu thị tự mô tả</skos:prefLabel>
      <rdakit:toolkitLabel xml:lang="vi">biểu thị tự mô tả</rdakit:toolkitLabel>
      <skos:definition xml:lang="vi">Biểu thị có chứa thông tin nhận dạng.</skos:definition>
      <rdakit:toolkitDefinition xml:lang="vi">Biểu thị có chứa thông tin nhận dạng.</rdakit:toolkitDefinition>
      <skos:prefLabel xml:lang="no">selvbeskrivende manifestasjon</skos:prefLabel>
      <rdakit:toolkitLabel xml:lang="no">selvbeskrivende manifestasjon</rdakit:toolkitLabel>
      <skos:definition xml:lang="no">En manifestasjon som inneholder identifiserende informasjon.</skos:definition>
      <rdakit:toolkitDefinition xml:lang="no">En manifestasjon som inneholder identifiserende informasjon.</rdakit:toolkitDefinition>
    </skos:Concept>
<!-- Concept: series  -->
    <skos:Concept rdf:about="http://rdaregistry.info/termList/RDATerms/1081" xml:lang="en">
      <skos:inScheme rdf:resource="http://rdaregistry.info/termList/RDATerms"/>
      <reg:status rdf:resource="http://metadataregistry.org/uri/RegStatus/1001"/>
      <reg:identifier rdf:resource="http://metadataregistry.org/concepts/8596"/>
      <skos:prefLabel xml:lang="en">series</skos:prefLabel>
      <rdakit:toolkitLabel xml:lang="en">series</rdakit:toolkitLabel>
      <skos:definition xml:lang="en">A group of separate manifestations related to one another by the fact that each manifestation bears, in addition to its own title proper, a collective title applying to the group as a whole with or without numbering or, a separately numbered sequence of volumes or issues within a series or serial.</skos:definition>
      <rdakit:toolkitDefinition xml:lang="en">A group of separate manifestations related to one another by the fact that each manifestation bears, in addition to its own title proper, a collective title applying to the group as a whole with or without numbering or, a separately numbered sequence of volumes or issues within a series or serial.</rdakit:toolkitDefinition>
      <skos:prefLabel xml:lang="it">serie</skos:prefLabel>
      <rdakit:toolkitLabel xml:lang="it">serie</rdakit:toolkitLabel>
      <skos:prefLabel xml:lang="es">serie</skos:prefLabel>
      <rdakit:toolkitLabel xml:lang="es">serie</rdakit:toolkitLabel>
      <skos:definition xml:lang="es">Grupo de recursos separados que estan relacionados entre si por el hecho de que cada recurso tiene, además de su título propiamente dicho, un título colectivo que se aplica al grupo como un todo. Los recursos individuales pueden estar o no numerados.</skos:definition>
      <rdakit:toolkitDefinition xml:lang="es">Grupo de recursos separados que estan relacionados entre si por el hecho de que cada recurso tiene, además de su título propiamente dicho, un título colectivo que se aplica al grupo como un todo. Los recursos individuales pueden estar o no numerados.</rdakit:toolkitDefinition>
      <skos:prefLabel xml:lang="de">Reihe</skos:prefLabel>
      <rdakit:toolkitLabel xml:lang="de">Reihe</rdakit:toolkitLabel>
      <skos:definition xml:lang="de">Eine Gruppe getrennter Manifestationen, die durch die Tatsache miteinander in Verbindung stehen, dass jede Manifestation zusätzlich zu ihrem eigenen Haupttitel einen übergeordneten Titel trägt, der zur Gruppe als Ganzes gehört. Die einzelnen Ressourcen können gezählt oder ungezählt sein. Oder aber eine getrennt gezählte Folge von Bänden oder Ausgaben innerhalb einer Reihe oder einer fortlaufenden Ressource.</skos:definition>
      <rdakit:toolkitDefinition xml:lang="de">Eine Gruppe getrennter Manifestationen, die durch die Tatsache miteinander in Verbindung stehen, dass jede Manifestation zusätzlich zu ihrem eigenen Haupttitel einen übergeordneten Titel trägt, der zur Gruppe als Ganzes gehört. Die einzelnen Ressourcen können gezählt oder ungezählt sein. Oder aber eine getrennt gezählte Folge von Bänden oder Ausgaben innerhalb einer Reihe oder einer fortlaufenden Ressource.</rdakit:toolkitDefinition>
      <skos:prefLabel xml:lang="fi">sarja</skos:prefLabel>
      <rdakit:toolkitLabel xml:lang="fi">sarja</rdakit:toolkitLabel>
      <skos:definition xml:lang="fi">Ryhmä erillisiä manifestaatioita, joilla on omien päänimekkeiden lisäksi koko ryhmälle yhteinen kokoava nimeke. Sarjaan sisältyvät aineistot voi olla numeroitu, tai sarjaan tai sarja-aineistoon voi sisältyvä erillinen osien numerointijakso.</skos:definition>
      <rdakit:toolkitDefinition xml:lang="fi">Ryhmä erillisiä manifestaatioita, joilla on omien päänimekkeiden lisäksi koko ryhmälle yhteinen kokoava nimeke. Sarjaan sisältyvät aineistot voi olla numeroitu, tai sarjaan tai sarja-aineistoon voi sisältyvä erillinen osien numerointijakso.</rdakit:toolkitDefinition>
      <skos:prefLabel xml:lang="da">serie</skos:prefLabel>
      <rdakit:toolkitLabel xml:lang="da">serie</rdakit:toolkitLabel>
      <skos:definition xml:lang="da">En gruppe af separate manifestationer relateret til hinanden ved, at hver manifestation, ud over sin egen hovedtitel, bærer en fællestitel, der gælder for gruppen som helhed med eller uden nummerering, eller et individuelt nummereret række af bind eller numre i en serie eller et periodikum.</skos:definition>
      <rdakit:toolkitDefinition xml:lang="da">En gruppe af separate manifestationer relateret til hinanden ved, at hver manifestation, ud over sin egen hovedtitel, bærer en fællestitel, der gælder for gruppen som helhed med eller uden nummerering, eller et individuelt nummereret række af bind eller numre i en serie eller et periodikum.</rdakit:toolkitDefinition>
      <skos:prefLabel xml:lang="vi">tùng thư</skos:prefLabel>
      <rdakit:toolkitLabel xml:lang="vi">tùng thư</rdakit:toolkitLabel>
      <skos:definition xml:lang="vi">Một nhóm biểu thị riêng biệt có lên quan với nhau bởi vì mỗi biểu thị mang, bên cạnh nhan đề hợp thức riêng, một nhan đề tập hợp được dùng cho cả nhóm có hoặc không đánh số hoặcChuỗi được đánh số riêng rẽ của các tập hoặc số bên trong một tùng thư hoặc ấn phẩm nhiều kỳ.</skos:definition>
      <rdakit:toolkitDefinition xml:lang="vi">Một nhóm biểu thị riêng biệt có lên quan với nhau bởi vì mỗi biểu thị mang, bên cạnh nhan đề hợp thức riêng, một nhan đề tập hợp được dùng cho cả nhóm có hoặc không đánh số hoặcChuỗi được đánh số riêng rẽ của các tập hoặc số bên trong một tùng thư hoặc ấn phẩm nhiều kỳ.</rdakit:toolkitDefinition>
      <skos:prefLabel xml:lang="no">serie</skos:prefLabel>
      <rdakit:toolkitLabel xml:lang="no">serie</rdakit:toolkitLabel>
      <skos:definition xml:lang="no">En rekke selvstendige manifestasjoner som er knyttet til hverandre ved at hver av dem foruten sin egen hovedtittel er utstyrt med en felles tittel som gjelder rekken som helhet, med eller uten nummerering, eller en særskilt nummerert rekke av bind eller hefter i en serie eller et periodikum.</skos:definition>
      <rdakit:toolkitDefinition xml:lang="no">En rekke selvstendige manifestasjoner som er knyttet til hverandre ved at hver av dem foruten sin egen hovedtittel er utstyrt med en felles tittel som gjelder rekken som helhet, med eller uten nummerering, eller en særskilt nummerert rekke av bind eller hefter i en serie eller et periodikum.</rdakit:toolkitDefinition>
    </skos:Concept>
<!-- Concept: series title page  -->
    <skos:Concept rdf:about="http://rdaregistry.info/termList/RDATerms/1082" xml:lang="en">
      <skos:inScheme rdf:resource="http://rdaregistry.info/termList/RDATerms"/>
      <reg:status rdf:resource="http://metadataregistry.org/uri/RegStatus/1001"/>
      <reg:identifier rdf:resource="http://metadataregistry.org/concepts/8597"/>
      <skos:prefLabel xml:lang="en">series title page</skos:prefLabel>
      <rdakit:toolkitLabel xml:lang="en">series title page</rdakit:toolkitLabel>
      <skos:definition xml:lang="en">An added title page bearing a series title proper and usually, though not necessarily, other information about a series such as statement of responsibility, numeric designation, data relating to publication, title of the manifestation within the series.</skos:definition>
      <rdakit:toolkitDefinition xml:lang="en">An added title page bearing a series title proper and usually, though not necessarily, other information about a series such as statement of responsibility, numeric designation, data relating to publication, title of the manifestation within the series.</rdakit:toolkitDefinition>
	    <skos:related rdf:resource="http://rdaregistry.info/termList/RDATerms/1004"/>
	    <skos:related rdf:resource="http://rdaregistry.info/termList/RDATerms/1095"/>
      <skos:prefLabel xml:lang="it">frontespizio della serie</skos:prefLabel>
      <rdakit:toolkitLabel xml:lang="it">frontespizio della serie</rdakit:toolkitLabel>
      <skos:definition xml:lang="it">Frontespizio aggiunto che presenta il titolo proprio della serie e solitamente, benché non necessariamente, altre informazioni sulla serie.</skos:definition>
      <rdakit:toolkitDefinition xml:lang="it">Frontespizio aggiunto che presenta il titolo proprio della serie e solitamente, benché non necessariamente, altre informazioni sulla serie.</rdakit:toolkitDefinition>
      <skos:prefLabel xml:lang="de">Titelseite der Reihe</skos:prefLabel>
      <rdakit:toolkitLabel xml:lang="de">Titelseite der Reihe</rdakit:toolkitLabel>
      <skos:definition xml:lang="de">Eine zusätzliche Titelseite mit dem Haupttitel der Reihe und meistens, aber nicht notwendigerweise, sonstigen Informationen über die Reihe (z. B. Verantwortlichkeitsangabe, numerische Bezeichnung, Erscheinungsdaten, Titel der Manifestation innerhalb der Reihe).</skos:definition>
      <rdakit:toolkitDefinition xml:lang="de">Eine zusätzliche Titelseite mit dem Haupttitel der Reihe und meistens, aber nicht notwendigerweise, sonstigen Informationen über die Reihe (z. B. Verantwortlichkeitsangabe, numerische Bezeichnung, Erscheinungsdaten, Titel der Manifestation innerhalb der Reihe).</rdakit:toolkitDefinition>
      <skos:prefLabel xml:lang="fi">sarjan nimiösivu</skos:prefLabel>
      <rdakit:toolkitLabel xml:lang="fi">sarjan nimiösivu</rdakit:toolkitLabel>
      <skos:definition xml:lang="fi">Lisätty nimiösivu, joka sisältää sarjan päänimekkeen ja usein, mutta ei välttämättä, muuta sarjaan liittyvää tietoa, esim. vastuullisuustiedon, numerointitiedon, julkaisutietoja, aineiston nimekkeen sarjassa.</skos:definition>
      <rdakit:toolkitDefinition xml:lang="fi">Lisätty nimiösivu, joka sisältää sarjan päänimekkeen ja usein, mutta ei välttämättä, muuta sarjaan liittyvää tietoa, esim. vastuullisuustiedon, numerointitiedon, julkaisutietoja, aineiston nimekkeen sarjassa.</rdakit:toolkitDefinition>
      <skos:prefLabel xml:lang="da">serietitelside</skos:prefLabel>
      <rdakit:toolkitLabel xml:lang="da">serietitelside</rdakit:toolkitLabel>
      <skos:definition xml:lang="da">Supplerende titelblad, der viser seriens hovedtitel og normalt, men ikke nødvendigvis, andre oplysninger om serien, som fx ophavsangivelse, numerisk betegnelse, data relateret til publicering, manifestationens titel i serien.</skos:definition>
      <rdakit:toolkitDefinition xml:lang="da">Supplerende titelblad, der viser seriens hovedtitel og normalt, men ikke nødvendigvis, andre oplysninger om serien, som fx ophavsangivelse, numerisk betegnelse, data relateret til publicering, manifestationens titel i serien.</rdakit:toolkitDefinition>
      <skos:prefLabel xml:lang="ca">portada de la col·lecció</skos:prefLabel>
      <rdakit:toolkitLabel xml:lang="ca">portada de la col·lecció</rdakit:toolkitLabel>
      <skos:definition xml:lang="ca">Portada addicional que porta un títol propi de la col·lecció i normalment, encara que no necessàriament, altra informació sobre una col·lecció, com ara la menció de responsabilitat, la designació numèrica, les dades relatives a la publicació, el títol de la manifestació dins de la col·lecció.</skos:definition>
      <rdakit:toolkitDefinition xml:lang="ca">Portada addicional que porta un títol propi de la col·lecció i normalment, encara que no necessàriament, altra informació sobre una col·lecció, com ara la menció de responsabilitat, la designació numèrica, les dades relatives a la publicació, el títol de la manifestació dins de la col·lecció.</rdakit:toolkitDefinition>
      <skos:prefLabel xml:lang="fr">page de titre de collection</skos:prefLabel>
      <rdakit:toolkitLabel xml:lang="fr">page de titre de collection</rdakit:toolkitLabel>
      <skos:definition xml:lang="fr">Page de titre supplémentaire portant un titre propre de collection et ordinairement, mais pas nécessairement, un supplément d’information sur la collection tel qu’une mention de responsabilité, une désignation numérique, des données relatives à la publication ou le titre de la manifestation à l’intérieur de la collection.</skos:definition>
      <rdakit:toolkitDefinition xml:lang="fr">Page de titre supplémentaire portant un titre propre de collection et ordinairement, mais pas nécessairement, un supplément d’information sur la collection tel qu’une mention de responsabilité, une désignation numérique, des données relatives à la publication ou le titre de la manifestation à l’intérieur de la collection.</rdakit:toolkitDefinition>
      <skos:prefLabel xml:lang="vi">trang nhan đề tùng thư</skos:prefLabel>
      <rdakit:toolkitLabel xml:lang="vi">trang nhan đề tùng thư</rdakit:toolkitLabel>
      <skos:definition xml:lang="vi">Trang nhan đề được thêm vào mang nhan đề hợp thức của tùng thư, mặc dù không nhất thiết, thông tin khác về tùng thư như thông tin trách nhiệm, định danh con số, dữ liệu liên quan tới xuất bản, nhan đề của tài nguyên bên trong tùng thư.</skos:definition>
      <rdakit:toolkitDefinition xml:lang="vi">Trang nhan đề được thêm vào mang nhan đề hợp thức của tùng thư, mặc dù không nhất thiết, thông tin khác về tùng thư như thông tin trách nhiệm, định danh con số, dữ liệu liên quan tới xuất bản, nhan đề của tài nguyên bên trong tùng thư.</rdakit:toolkitDefinition>
      <skos:prefLabel xml:lang="no">tittelside for serie</skos:prefLabel>
      <rdakit:toolkitLabel xml:lang="no">tittelside for serie</rdakit:toolkitLabel>
      <skos:definition xml:lang="no">En ekstra tittelside som inneholder seriens hovedtittel og vanligvis, men ikke nødvendigvis, annen informasjon om serien, for eksempel ansvarsangivelse, numerisk betegnelse, informasjon om utgivelsen eller tittel på manifestasjonen innen serien.</skos:definition>
      <rdakit:toolkitDefinition xml:lang="no">En ekstra tittelside som inneholder seriens hovedtittel og vanligvis, men ikke nødvendigvis, annen informasjon om serien, for eksempel ansvarsangivelse, numerisk betegnelse, informasjon om utgivelsen eller tittel på manifestasjonen innen serien.</rdakit:toolkitDefinition>
    </skos:Concept>
<!-- Concept: short title of a legal work  -->
    <skos:Concept rdf:about="http://rdaregistry.info/termList/RDATerms/1083" xml:lang="en">
      <skos:inScheme rdf:resource="http://rdaregistry.info/termList/RDATerms"/>
      <reg:status rdf:resource="http://metadataregistry.org/uri/RegStatus/1001"/>
      <reg:identifier rdf:resource="http://metadataregistry.org/concepts/8598"/>
      <skos:prefLabel xml:lang="en">short title of a legal work</skos:prefLabel>
      <rdakit:toolkitLabel xml:lang="en">short title of a legal work</rdakit:toolkitLabel>
      <skos:definition xml:lang="en">A title of a legal work that is given either in the text of the work or in legal literature and that succinctly names the work and often reflects how it is popularly known.</skos:definition>
      <rdakit:toolkitDefinition xml:lang="en">A title of a legal work that is given either in the text of the work or in legal literature and that succinctly names the work and often reflects how it is popularly known.</rdakit:toolkitDefinition>
      <skos:prefLabel xml:lang="fr">titre abrégé d’une œuvre juridique</skos:prefLabel>
      <rdakit:toolkitLabel xml:lang="fr">titre abrégé d’une œuvre juridique</rdakit:toolkitLabel>
      <skos:definition xml:lang="fr">Titre d’une œuvre juridique qui est donné dans le texte même de l’œuvre ou dans la littérature juridique et qui nomme succinctement l’œuvre et reflète souvent comment elle est couramment connue.</skos:definition>
      <rdakit:toolkitDefinition xml:lang="fr">Titre d’une œuvre juridique qui est donné dans le texte même de l’œuvre ou dans la littérature juridique et qui nomme succinctement l’œuvre et reflète souvent comment elle est couramment connue.</rdakit:toolkitDefinition>
      <skos:prefLabel xml:lang="de">Kurztitel eines juristischen Werks</skos:prefLabel>
      <rdakit:toolkitLabel xml:lang="de">Kurztitel eines juristischen Werks</rdakit:toolkitLabel>
      <skos:definition xml:lang="de">Ein Titel eines juristischen Werks, der entweder im Text des Werks oder in der juristischen Literatur genannt ist und der kurz und bündig das Werk benennt und häufig widerspiegelt, wie es allgemein bekannt ist.</skos:definition>
      <rdakit:toolkitDefinition xml:lang="de">Ein Titel eines juristischen Werks, der entweder im Text des Werks oder in der juristischen Literatur genannt ist und der kurz und bündig das Werk benennt und häufig widerspiegelt, wie es allgemein bekannt ist.</rdakit:toolkitDefinition>
      <skos:prefLabel xml:lang="fi">juridisen teoksen lyhennetty nimeke</skos:prefLabel>
      <rdakit:toolkitLabel xml:lang="fi">juridisen teoksen lyhennetty nimeke</rdakit:toolkitLabel>
      <skos:definition xml:lang="fi">Juridisen teoksen nimeke joka löytyy joko teoksessa itsessään tai juridisessa kirjallisuudessa. Se nimeää teoksen ytimekkäästi ja heijastaa sen yleisesti tunnettua nimimuotoa.</skos:definition>
      <rdakit:toolkitDefinition xml:lang="fi">Juridisen teoksen nimeke joka löytyy joko teoksessa itsessään tai juridisessa kirjallisuudessa. Se nimeää teoksen ytimekkäästi ja heijastaa sen yleisesti tunnettua nimimuotoa.</rdakit:toolkitDefinition>
      <skos:prefLabel xml:lang="da">kort titel på et juridisk værk</skos:prefLabel>
      <rdakit:toolkitLabel xml:lang="da">kort titel på et juridisk værk</rdakit:toolkitLabel>
      <skos:definition xml:lang="da">Titel på et juridisk værk, der er givet enten i værkets tekst eller i juridisk litteratur, og som koncist nævner værket og ofte afspejler, hvordan det almindeligvis omtales.</skos:definition>
      <rdakit:toolkitDefinition xml:lang="da">Titel på et juridisk værk, der er givet enten i værkets tekst eller i juridisk litteratur, og som koncist nævner værket og ofte afspejler, hvordan det almindeligvis omtales.</rdakit:toolkitDefinition>
      <skos:prefLabel xml:lang="ca">títol curt d’una obra jurídica</skos:prefLabel>
      <rdakit:toolkitLabel xml:lang="ca">títol curt d’una obra jurídica</rdakit:toolkitLabel>
      <skos:definition xml:lang="ca">Títol d’una obra jurídica que es dóna o bé en el text de l’obra o bé en la bibliografia jurídica, que dóna nom succintament a l’obra i que sovint reflecteix com se la coneix popularment.</skos:definition>
      <rdakit:toolkitDefinition xml:lang="ca">Títol d’una obra jurídica que es dóna o bé en el text de l’obra o bé en la bibliografia jurídica, que dóna nom succintament a l’obra i que sovint reflecteix com se la coneix popularment.</rdakit:toolkitDefinition>
      <skos:prefLabel xml:lang="vi">nhan đề ngắn của tác phẩm luật pháp</skos:prefLabel>
      <rdakit:toolkitLabel xml:lang="vi">nhan đề ngắn của tác phẩm luật pháp</rdakit:toolkitLabel>
      <skos:definition xml:lang="vi">Nhan đề của tác phẩm luật pháp nêu ra trong văn bản của tác phẩm hoặc trong tài liệu luật pháp đặt tên tóm tắt của tác phẩm và thường phản ánh cách mà tác phẩm đó được công chúng biết đến.</skos:definition>
      <rdakit:toolkitDefinition xml:lang="vi">Nhan đề của tác phẩm luật pháp nêu ra trong văn bản của tác phẩm hoặc trong tài liệu luật pháp đặt tên tóm tắt của tác phẩm và thường phản ánh cách mà tác phẩm đó được công chúng biết đến.</rdakit:toolkitDefinition>
      <skos:prefLabel xml:lang="no">korttittel på et juridisk verk</skos:prefLabel>
      <rdakit:toolkitLabel xml:lang="no">korttittel på et juridisk verk</rdakit:toolkitLabel>
      <skos:definition xml:lang="no">En tittel på et juridisk verk som enten er angitt i teksten for verket eller i juridisk litteratur og som kortfattet navngir verket og ofte gjenspeiler hvordan verket er alminnelig kjent.</skos:definition>
      <rdakit:toolkitDefinition xml:lang="no">En tittel på et juridisk verk som enten er angitt i teksten for verket eller i juridisk litteratur og som kortfattet navngir verket og ofte gjenspeiler hvordan verket er alminnelig kjent.</rdakit:toolkitDefinition>
    </skos:Concept>
<!-- Concept: sign language  -->
    <skos:Concept rdf:about="http://rdaregistry.info/termList/RDATerms/1084" xml:lang="en">
      <skos:inScheme rdf:resource="http://rdaregistry.info/termList/RDATerms"/>
      <reg:status rdf:resource="http://metadataregistry.org/uri/RegStatus/1001"/>
      <reg:identifier rdf:resource="http://metadataregistry.org/concepts/8599"/>
      <skos:prefLabel xml:lang="en">sign language</skos:prefLabel>
      <rdakit:toolkitLabel xml:lang="en">sign language</rdakit:toolkitLabel>
      <skos:definition xml:lang="en">A language that uses a system of manual, facial, and other body movements as the means of communication.</skos:definition>
      <rdakit:toolkitDefinition xml:lang="en">A language that uses a system of manual, facial, and other body movements as the means of communication.</rdakit:toolkitDefinition>
      <skos:prefLabel xml:lang="it">lingua dei segni</skos:prefLabel>
      <rdakit:toolkitLabel xml:lang="it">lingua dei segni</rdakit:toolkitLabel>
      <skos:definition xml:lang="it">Nel contesto del contenuto accessibile, una versione nella lingua dei segni del dialogo della risorsa visualizzato sullo schermo.</skos:definition>
      <rdakit:toolkitDefinition xml:lang="it">Nel contesto del contenuto accessibile, una versione nella lingua dei segni del dialogo della risorsa visualizzato sullo schermo.</rdakit:toolkitDefinition>
      <skos:prefLabel xml:lang="fr">langue des signes</skos:prefLabel>
      <rdakit:toolkitLabel xml:lang="fr">langue des signes</rdakit:toolkitLabel>
      <skos:definition xml:lang="fr">Langue qui utilise un système de mouvements des mains, du visage ou d’autres parties du corps comme moyen de communication.</skos:definition>
      <rdakit:toolkitDefinition xml:lang="fr">Langue qui utilise un système de mouvements des mains, du visage ou d’autres parties du corps comme moyen de communication.</rdakit:toolkitDefinition>
      <skos:prefLabel xml:lang="de">Gebärdensprache</skos:prefLabel>
      <rdakit:toolkitLabel xml:lang="de">Gebärdensprache</rdakit:toolkitLabel>
      <skos:definition xml:lang="de">Eine Sprache, die ein System von manuellen, Gesichts- und anderen Körperbewegungen als Kommunikationsmittel verwendet.</skos:definition>
      <rdakit:toolkitDefinition xml:lang="de">Eine Sprache, die ein System von manuellen, Gesichts- und anderen Körperbewegungen als Kommunikationsmittel verwendet.</rdakit:toolkitDefinition>
      <skos:prefLabel xml:lang="fi">viittomakieli</skos:prefLabel>
      <rdakit:toolkitLabel xml:lang="fi">viittomakieli</rdakit:toolkitLabel>
      <skos:definition xml:lang="fi">Kieli, joka käyttää käsien, kasvojen ja muiden kehonosien liikkeiden järjestelmää viestintävälineenä.</skos:definition>
      <rdakit:toolkitDefinition xml:lang="fi">Kieli, joka käyttää käsien, kasvojen ja muiden kehonosien liikkeiden järjestelmää viestintävälineenä.</rdakit:toolkitDefinition>
      <skos:prefLabel xml:lang="da">tegnsprog</skos:prefLabel>
      <rdakit:toolkitLabel xml:lang="da">tegnsprog</rdakit:toolkitLabel>
      <skos:definition xml:lang="da">Sprog som benytter et system af hånd-, ansigts- og andre kropsbevægelser til kommunikation.</skos:definition>
      <rdakit:toolkitDefinition xml:lang="da">Sprog som benytter et system af hånd-, ansigts- og andre kropsbevægelser til kommunikation.</rdakit:toolkitDefinition>
      <skos:prefLabel xml:lang="ca">llengua de signes</skos:prefLabel>
      <rdakit:toolkitLabel xml:lang="ca">llengua de signes</rdakit:toolkitLabel>
      <skos:definition xml:lang="ca">Llengua que usa un sistema de moviments manuals, facials i altres moviments corporals com a mitjans de comunicació.</skos:definition>
      <rdakit:toolkitDefinition xml:lang="ca">Llengua que usa un sistema de moviments manuals, facials i altres moviments corporals com a mitjans de comunicació.</rdakit:toolkitDefinition>
      <skos:prefLabel xml:lang="vi">ngôn ngữ cử chỉ</skos:prefLabel>
      <rdakit:toolkitLabel xml:lang="vi">ngôn ngữ cử chỉ</rdakit:toolkitLabel>
      <skos:definition xml:lang="vi">Ngôn ngữ dùng hệ thống bàn tay, mặt, và chuyển động thân thể khác như là phương tiện giao tiếp.</skos:definition>
      <rdakit:toolkitDefinition xml:lang="vi">Ngôn ngữ dùng hệ thống bàn tay, mặt, và chuyển động thân thể khác như là phương tiện giao tiếp.</rdakit:toolkitDefinition>
      <skos:prefLabel xml:lang="no">tegnspråk</skos:prefLabel>
      <rdakit:toolkitLabel xml:lang="no">tegnspråk</rdakit:toolkitLabel>
      <skos:definition xml:lang="no">Et språk som bruker et system med hånd-, ansikts- og kroppsbevegelser som kommunikasjonsmiddel.</skos:definition>
      <rdakit:toolkitDefinition xml:lang="no">Et språk som bruker et system med hånd-, ansikts- og kroppsbevegelser som kommunikasjonsmiddel.</rdakit:toolkitDefinition>
    </skos:Concept>
<!-- Concept: source of information  -->
    <skos:Concept rdf:about="http://rdaregistry.info/termList/RDATerms/1085" xml:lang="en">
      <skos:inScheme rdf:resource="http://rdaregistry.info/termList/RDATerms"/>
      <reg:status rdf:resource="http://metadataregistry.org/uri/RegStatus/1001"/>
      <reg:identifier rdf:resource="http://metadataregistry.org/concepts/8600"/>
      <skos:prefLabel xml:lang="en">source of information</skos:prefLabel>
      <rdakit:toolkitLabel xml:lang="en">source of information</rdakit:toolkitLabel>
      <skos:definition xml:lang="en">A source of data from which a description, or portion thereof, is prepared.</skos:definition>
      <rdakit:toolkitDefinition xml:lang="en">A source of data from which a description, or portion thereof, is prepared.</rdakit:toolkitDefinition>
      <skos:prefLabel xml:lang="it">fonte d'informazione</skos:prefLabel>
      <rdakit:toolkitLabel xml:lang="it">fonte d'informazione</rdakit:toolkitLabel>
      <skos:definition xml:lang="it">Fonte dei dati da cui si trae una descrizione (o una sua parte).</skos:definition>
      <rdakit:toolkitDefinition xml:lang="it">Fonte dei dati da cui si trae una descrizione (o una sua parte).</rdakit:toolkitDefinition>
      <skos:prefLabel xml:lang="es">fuente de información</skos:prefLabel>
      <rdakit:toolkitLabel xml:lang="es">fuente de información</rdakit:toolkitLabel>
      <skos:definition xml:lang="es">Fuente de los datos con los que se preparó una descripción (o una parte de ella).</skos:definition>
      <rdakit:toolkitDefinition xml:lang="es">Fuente de los datos con los que se preparó una descripción (o una parte de ella).</rdakit:toolkitDefinition>
      <skos:prefLabel xml:lang="de">Informationsquelle</skos:prefLabel>
      <rdakit:toolkitLabel xml:lang="de">Informationsquelle</rdakit:toolkitLabel>
      <skos:definition xml:lang="de">Eine Datenquelle, aus der eine Beschreibung (oder ein Teil davon) erstellt wird.</skos:definition>
      <rdakit:toolkitDefinition xml:lang="de">Eine Datenquelle, aus der eine Beschreibung (oder ein Teil davon) erstellt wird.</rdakit:toolkitDefinition>
      <skos:prefLabel xml:lang="fi">tiedonlähde</skos:prefLabel>
      <rdakit:toolkitLabel xml:lang="fi">tiedonlähde</rdakit:toolkitLabel>
      <skos:definition xml:lang="fi">Kuvailun tai kuvailun osan tietoja varten käytetty lähde.</skos:definition>
      <rdakit:toolkitDefinition xml:lang="fi">Kuvailun tai kuvailun osan tietoja varten käytetty lähde.</rdakit:toolkitDefinition>
      <skos:prefLabel xml:lang="da">kilde til oplysninger</skos:prefLabel>
      <rdakit:toolkitLabel xml:lang="da">kilde til oplysninger</rdakit:toolkitLabel>
      <skos:definition xml:lang="da">Kilde til data, hvorfra en beskrivelse (eller en del deraf) er udarbejdet.</skos:definition>
      <rdakit:toolkitDefinition xml:lang="da">Kilde til data, hvorfra en beskrivelse (eller en del deraf) er udarbejdet.</rdakit:toolkitDefinition>
      <skos:prefLabel xml:lang="ca">font d’informació</skos:prefLabel>
      <rdakit:toolkitLabel xml:lang="ca">font d’informació</rdakit:toolkitLabel>
      <skos:definition xml:lang="ca">Font de dades a partir de la qual es prepara una descripció o una part d’una descripció.</skos:definition>
      <rdakit:toolkitDefinition xml:lang="ca">Font de dades a partir de la qual es prepara una descripció o una part d’una descripció.</rdakit:toolkitDefinition>
      <skos:prefLabel xml:lang="fr">source d’information</skos:prefLabel>
      <rdakit:toolkitLabel xml:lang="fr">source d’information</rdakit:toolkitLabel>
      <skos:definition xml:lang="fr">Source de données servant à préparer une description ou une partie de description.</skos:definition>
      <rdakit:toolkitDefinition xml:lang="fr">Source de données servant à préparer une description ou une partie de description.</rdakit:toolkitDefinition>
      <skos:prefLabel xml:lang="vi">nguồn lấy thông tin</skos:prefLabel>
      <rdakit:toolkitLabel xml:lang="vi">nguồn lấy thông tin</rdakit:toolkitLabel>
      <skos:definition xml:lang="vi">Nguồn dữ liệu mà từ đó một mô tả (hoặc phần của mô tả) được chuẩn bị.</skos:definition>
      <rdakit:toolkitDefinition xml:lang="vi">Nguồn dữ liệu mà từ đó một mô tả (hoặc phần của mô tả) được chuẩn bị.</rdakit:toolkitDefinition>
      <skos:prefLabel xml:lang="no">informasjonskilde</skos:prefLabel>
      <rdakit:toolkitLabel xml:lang="no">informasjonskilde</rdakit:toolkitLabel>
      <skos:definition xml:lang="no">En informasjonskilde som en beskrivelse, eller deler av en beskrivelse, er basert på.</skos:definition>
      <rdakit:toolkitDefinition xml:lang="no">En informasjonskilde som en beskrivelse, eller deler av en beskrivelse, er basert på.</rdakit:toolkitDefinition>
    </skos:Concept>
<!-- Concept: storage medium  -->
    <skos:Concept rdf:about="http://rdaregistry.info/termList/RDATerms/1086" xml:lang="en">
      <skos:inScheme rdf:resource="http://rdaregistry.info/termList/RDATerms"/>
      <reg:status rdf:resource="http://metadataregistry.org/uri/RegStatus/1001"/>
      <reg:identifier rdf:resource="http://metadataregistry.org/concepts/8601"/>
      <skos:prefLabel xml:lang="en">storage medium</skos:prefLabel>
      <rdakit:toolkitLabel xml:lang="en">storage medium</rdakit:toolkitLabel>
      <skos:definition xml:lang="en">A physical material or substance on which information or artistic content is stored.</skos:definition>
      <rdakit:toolkitDefinition xml:lang="en">A physical material or substance on which information or artistic content is stored.</rdakit:toolkitDefinition>
	    <skos:related rdf:resource="http://rdaregistry.info/termList/RDATerms/1016"/>
	    <skos:related rdf:resource="http://rdaregistry.info/termList/RDATerms/1058"/>
	    <skos:related rdf:resource="http://rdaregistry.info/termList/RDATerms/1026"/>
      <skos:prefLabel xml:lang="it">mezzo di memorizzazione</skos:prefLabel>
      <rdakit:toolkitLabel xml:lang="it">mezzo di memorizzazione</rdakit:toolkitLabel>
      <skos:definition xml:lang="it">Materiale o sostanza fisica sul quale è memorizzata l'informazione o il contenuto artistico.</skos:definition>
      <rdakit:toolkitDefinition xml:lang="it">Materiale o sostanza fisica sul quale è memorizzata l'informazione o il contenuto artistico.</rdakit:toolkitDefinition>
      <skos:prefLabel xml:lang="de">Speichermedium</skos:prefLabel>
      <rdakit:toolkitLabel xml:lang="de">Speichermedium</rdakit:toolkitLabel>
      <skos:definition xml:lang="de">Ein physisches Material oder eine Substanz, auf dem/der Informationen oder künstlerischer Inhalt gespeichert sind/ist.</skos:definition>
      <rdakit:toolkitDefinition xml:lang="de">Ein physisches Material oder eine Substanz, auf dem/der Informationen oder künstlerischer Inhalt gespeichert sind/ist.</rdakit:toolkitDefinition>
      <skos:prefLabel xml:lang="fi">tallennusväline</skos:prefLabel>
      <rdakit:toolkitLabel xml:lang="fi">tallennusväline</rdakit:toolkitLabel>
      <skos:definition xml:lang="fi">Fyysinen materiaali, johon tiedollinen tai taiteellinen sisältö on tallennettu.</skos:definition>
      <rdakit:toolkitDefinition xml:lang="fi">Fyysinen materiaali, johon tiedollinen tai taiteellinen sisältö on tallennettu.</rdakit:toolkitDefinition>
      <skos:prefLabel xml:lang="da">lagringsmedie</skos:prefLabel>
      <rdakit:toolkitLabel xml:lang="da">lagringsmedie</rdakit:toolkitLabel>
      <skos:definition xml:lang="da">Fysisk materiale eller stof, hvorpå oplysninger eller kunstnerisk indhold lagres.</skos:definition>
      <rdakit:toolkitDefinition xml:lang="da">Fysisk materiale eller stof, hvorpå oplysninger eller kunstnerisk indhold lagres.</rdakit:toolkitDefinition>
      <skos:prefLabel xml:lang="ca">suport d’emmagatzematge</skos:prefLabel>
      <rdakit:toolkitLabel xml:lang="ca">suport d’emmagatzematge</rdakit:toolkitLabel>
      <skos:definition xml:lang="ca">Material físic o substància on s’emmagatzema la informació o el contingut artístic.</skos:definition>
      <rdakit:toolkitDefinition xml:lang="ca">Material físic o substància on s’emmagatzema la informació o el contingut artístic.</rdakit:toolkitDefinition>
      <skos:prefLabel xml:lang="fr">support de stockage</skos:prefLabel>
      <rdakit:toolkitLabel xml:lang="fr">support de stockage</rdakit:toolkitLabel>
      <skos:definition xml:lang="fr">Matériau ou substance physique sur laquelle sont emmagasinés de l’information ou un contenu artistique.</skos:definition>
      <rdakit:toolkitDefinition xml:lang="fr">Matériau ou substance physique sur laquelle sont emmagasinés de l’information ou un contenu artistique.</rdakit:toolkitDefinition>
      <skos:prefLabel xml:lang="vi">phương tiện lưu giữ</skos:prefLabel>
      <rdakit:toolkitLabel xml:lang="vi">phương tiện lưu giữ</rdakit:toolkitLabel>
      <skos:definition xml:lang="vi">Vật liệu hoặc vật chất mà thông tin hoặc nội dung nghệ thuật được chứa trong đó.</skos:definition>
      <rdakit:toolkitDefinition xml:lang="vi">Vật liệu hoặc vật chất mà thông tin hoặc nội dung nghệ thuật được chứa trong đó.</rdakit:toolkitDefinition>
      <skos:prefLabel xml:lang="no">lagringsmedium</skos:prefLabel>
      <rdakit:toolkitLabel xml:lang="no">lagringsmedium</rdakit:toolkitLabel>
      <skos:definition xml:lang="no">Et fysisk materiale eller substans der informasjon eller kunstnerisk innhold er lagret.</skos:definition>
      <rdakit:toolkitDefinition xml:lang="no">Et fysisk materiale eller substans der informasjon eller kunstnerisk innhold er lagret.</rdakit:toolkitDefinition>
    </skos:Concept>
<!-- Concept: structured description  -->
    <skos:Concept rdf:about="http://rdaregistry.info/termList/RDATerms/1087" xml:lang="en">
      <skos:inScheme rdf:resource="http://rdaregistry.info/termList/RDATerms"/>
      <reg:status rdf:resource="http://metadataregistry.org/uri/RegStatus/1001"/>
      <reg:identifier rdf:resource="http://metadataregistry.org/concepts/8602"/>
      <skos:prefLabel xml:lang="en">structured description</skos:prefLabel>
      <rdakit:toolkitLabel xml:lang="en">structured description</rdakit:toolkitLabel>
      <skos:definition xml:lang="en">A full or partial description of a related entity using the same data that would be recorded in RDA elements for a description of that related entity presented in an order specified by a recognized display standard.</skos:definition>
      <rdakit:toolkitDefinition xml:lang="en">A full or partial description of a related entity using the same data that would be recorded in RDA elements for a description of that related entity presented in an order specified by a recognized display standard.</rdakit:toolkitDefinition>
      <skos:prefLabel xml:lang="it">descrizione strutturata</skos:prefLabel>
      <rdakit:toolkitLabel xml:lang="it">descrizione strutturata</rdakit:toolkitLabel>
      <skos:definition xml:lang="it">Descrizione comprensiva o parziale di una risorsa che riflette la stessa struttura (cioè lo stesso ordine di elementi) della risorsa descritta.</skos:definition>
      <rdakit:toolkitDefinition xml:lang="it">Descrizione comprensiva o parziale di una risorsa che riflette la stessa struttura (cioè lo stesso ordine di elementi) della risorsa descritta.</rdakit:toolkitDefinition>
      <skos:prefLabel xml:lang="fr">description structurée</skos:prefLabel>
      <rdakit:toolkitLabel xml:lang="fr">description structurée</rdakit:toolkitLabel>
      <skos:definition xml:lang="fr">Description complète ou partielle d’une entité en relation rédigée en utilisant les mêmes données que celles qui seraient enregistrées dans des éléments RDA pour une description de cette entité en relation, présentées dans un ordre spécifié par une norme d’affichage reconnue.</skos:definition>
      <rdakit:toolkitDefinition xml:lang="fr">Description complète ou partielle d’une entité en relation rédigée en utilisant les mêmes données que celles qui seraient enregistrées dans des éléments RDA pour une description de cette entité en relation, présentées dans un ordre spécifié par une norme d’affichage reconnue.</rdakit:toolkitDefinition>
      <skos:prefLabel xml:lang="es">descripción estructurada</skos:prefLabel>
      <rdakit:toolkitLabel xml:lang="es">descripción estructurada</rdakit:toolkitLabel>
      <skos:definition xml:lang="es">Descripción completa o parcial de un recurso que utiliza la misma estructura (i.e., el mismo orden de elementos) que se usa en el recurso que se describe.</skos:definition>
      <rdakit:toolkitDefinition xml:lang="es">Descripción completa o parcial de un recurso que utiliza la misma estructura (i.e., el mismo orden de elementos) que se usa en el recurso que se describe.</rdakit:toolkitDefinition>
      <skos:prefLabel xml:lang="de">Strukturierten Beschreibung</skos:prefLabel>
      <rdakit:toolkitLabel xml:lang="de">Strukturierten Beschreibung</rdakit:toolkitLabel>
      <skos:definition xml:lang="de">Eine vollständige oder teilweise Beschreibung einer in Beziehung stehenden Entität, die dieselben Daten verwendet, die in RDA-Elementen für eine Beschreibung dieser in Beziehung stehenden Entität erfasst werden würden; die Reihenfolge, wie sie präsentiert werden, richtet sich nach einem anerkannten Anzeige-Standard.</skos:definition>
      <rdakit:toolkitDefinition xml:lang="de">Eine vollständige oder teilweise Beschreibung einer in Beziehung stehenden Entität, die dieselben Daten verwendet, die in RDA-Elementen für eine Beschreibung dieser in Beziehung stehenden Entität erfasst werden würden; die Reihenfolge, wie sie präsentiert werden, richtet sich nach einem anerkannten Anzeige-Standard.</rdakit:toolkitDefinition>
      <skos:prefLabel xml:lang="fi">rakenteistettu kuvailu</skos:prefLabel>
      <rdakit:toolkitLabel xml:lang="fi">rakenteistettu kuvailu</rdakit:toolkitLabel>
      <skos:definition xml:lang="fi">Täysi tai osittainen viittauksen kohteena olevan aineiston kuvailu, jossa käytetään samoja tietoja kuin käytettäisiin RDA-elementteinä viittauksen kohteena olevan aineiston kuvailussa näyttöstandardin määräämässä järjestyksessä.</skos:definition>
      <rdakit:toolkitDefinition xml:lang="fi">Täysi tai osittainen viittauksen kohteena olevan aineiston kuvailu, jossa käytetään samoja tietoja kuin käytettäisiin RDA-elementteinä viittauksen kohteena olevan aineiston kuvailussa näyttöstandardin määräämässä järjestyksessä.</rdakit:toolkitDefinition>
      <skos:prefLabel xml:lang="da">struktureret beskrivelse</skos:prefLabel>
      <rdakit:toolkitLabel xml:lang="da">struktureret beskrivelse</rdakit:toolkitLabel>
      <skos:definition xml:lang="da">Komplet eller delvis beskrivelse af en relateret entitet via brug af de samme data, som ville udgøre RDA-elementerne i beskrivelsen af en sådan relateret entitet og præsenteret i en rækkefølge specificeret af en anerkendt visningsstandard.</skos:definition>
      <rdakit:toolkitDefinition xml:lang="da">Komplet eller delvis beskrivelse af en relateret entitet via brug af de samme data, som ville udgøre RDA-elementerne i beskrivelsen af en sådan relateret entitet og præsenteret i en rækkefølge specificeret af en anerkendt visningsstandard.</rdakit:toolkitDefinition>
      <skos:prefLabel xml:lang="ca">descripció estructurada</skos:prefLabel>
      <rdakit:toolkitLabel xml:lang="ca">descripció estructurada</rdakit:toolkitLabel>
      <skos:definition xml:lang="ca">Descripció completa o parcial d’una entitat relacionada que usa les mateixes dades que s’enregistrarien com a elements RDA d’una descripció de l'entitat relacionada presentades en un ordre concret segons un estàndard de visualització reconegut.</skos:definition>
      <rdakit:toolkitDefinition xml:lang="ca">Descripció completa o parcial d’una entitat relacionada que usa les mateixes dades que s’enregistrarien com a elements RDA d’una descripció de l'entitat relacionada presentades en un ordre concret segons un estàndard de visualització reconegut.</rdakit:toolkitDefinition>
      <skos:prefLabel xml:lang="vi">mô tả có cấu trúc</skos:prefLabel>
      <rdakit:toolkitLabel xml:lang="vi">mô tả có cấu trúc</rdakit:toolkitLabel>
      <skos:definition xml:lang="vi">Mô tả đầy đủ hay một phần của thực thể có liên quan sử dụng cùng dữ liệu được ghi trong các yếu tố RDA để mô tả thực thể có liên quan đó được trình bày theo trật tự được chỉ ra bởi chuẩn hiện hình được nhận dạng.</skos:definition>
      <rdakit:toolkitDefinition xml:lang="vi">Mô tả đầy đủ hay một phần của thực thể có liên quan sử dụng cùng dữ liệu được ghi trong các yếu tố RDA để mô tả thực thể có liên quan đó được trình bày theo trật tự được chỉ ra bởi chuẩn hiện hình được nhận dạng.</rdakit:toolkitDefinition>
      <skos:prefLabel xml:lang="no">strukturert beskrivelse</skos:prefLabel>
      <rdakit:toolkitLabel xml:lang="no">strukturert beskrivelse</rdakit:toolkitLabel>
      <skos:definition xml:lang="no">En fullstendig eller delvis beskrivelse av en tilknyttet entitet som benytter samme data som ville være registrert i RDA-elementer for en beskrivelse av den tilknyttede entiteten, presentert i en rekkefølge angitt av et etablert standardformat.</skos:definition>
      <rdakit:toolkitDefinition xml:lang="no">En fullstendig eller delvis beskrivelse av en tilknyttet entitet som benytter samme data som ville være registrert i RDA-elementer for en beskrivelse av den tilknyttede entiteten, presentert i en rekkefølge angitt av et etablert standardformat.</rdakit:toolkitDefinition>
    </skos:Concept>
<!-- Concept: subject  -->
    <skos:Concept rdf:about="http://rdaregistry.info/termList/RDATerms/1088" xml:lang="en">
      <skos:inScheme rdf:resource="http://rdaregistry.info/termList/RDATerms"/>
      <reg:status rdf:resource="http://metadataregistry.org/uri/RegStatus/1001"/>
      <reg:identifier rdf:resource="http://metadataregistry.org/concepts/8603"/>
      <skos:prefLabel xml:lang="en">subject</skos:prefLabel>
      <rdakit:toolkitLabel xml:lang="en">subject</rdakit:toolkitLabel>
      <skos:definition xml:lang="en">A term, phrase, classification number, etc., that indicates what a work is about.</skos:definition>
      <rdakit:toolkitDefinition xml:lang="en">A term, phrase, classification number, etc., that indicates what a work is about.</rdakit:toolkitDefinition>
      <skos:prefLabel xml:lang="fi">aihe</skos:prefLabel>
      <rdakit:toolkitLabel xml:lang="fi">aihe</rdakit:toolkitLabel>
      <skos:definition xml:lang="fi">Termi, ilmaus, luokka tms., joka ilmaisee mitä aihetta teos käsittelee.</skos:definition>
      <rdakit:toolkitDefinition xml:lang="fi">Termi, ilmaus, luokka tms., joka ilmaisee mitä aihetta teos käsittelee.</rdakit:toolkitDefinition>
      <skos:prefLabel xml:lang="de">Thema</skos:prefLabel>
      <rdakit:toolkitLabel xml:lang="de">Thema</rdakit:toolkitLabel>
      <skos:definition xml:lang="de">Ein Terminus, eine Phrase, eine Notation usw., der/die angibt, wovon das Werk handelt.</skos:definition>
      <rdakit:toolkitDefinition xml:lang="de">Ein Terminus, eine Phrase, eine Notation usw., der/die angibt, wovon das Werk handelt.</rdakit:toolkitDefinition>
      <skos:prefLabel xml:lang="da">emne</skos:prefLabel>
      <rdakit:toolkitLabel xml:lang="da">emne</rdakit:toolkitLabel>
      <skos:definition xml:lang="da">Term, frase, klassifikation etc., der angiver, hvad et værk handler om.</skos:definition>
      <rdakit:toolkitDefinition xml:lang="da">Term, frase, klassifikation etc., der angiver, hvad et værk handler om.</rdakit:toolkitDefinition>
      <skos:prefLabel xml:lang="ca">matèria</skos:prefLabel>
      <rdakit:toolkitLabel xml:lang="ca">matèria</rdakit:toolkitLabel>
      <skos:definition xml:lang="ca">Terme, frase, número de classificació, etc., que indica de què tracta una obra.</skos:definition>
      <rdakit:toolkitDefinition xml:lang="ca">Terme, frase, número de classificació, etc., que indica de què tracta una obra.</rdakit:toolkitDefinition>
      <skos:prefLabel xml:lang="fr">sujet</skos:prefLabel>
      <rdakit:toolkitLabel xml:lang="fr">sujet</rdakit:toolkitLabel>
      <skos:definition xml:lang="fr">Terme, expression, indice de classification, etc. qui indique ce dont traite une œuvre.</skos:definition>
      <rdakit:toolkitDefinition xml:lang="fr">Terme, expression, indice de classification, etc. qui indique ce dont traite une œuvre.</rdakit:toolkitDefinition>
      <skos:prefLabel xml:lang="vi">chủ đề</skos:prefLabel>
      <rdakit:toolkitLabel xml:lang="vi">chủ đề</rdakit:toolkitLabel>
      <skos:definition xml:lang="vi">Thuật ngữ, cụm từ, ký hiệu phân loại, v.v... chỉ ra tác phẩm nói về cái gì.</skos:definition>
      <rdakit:toolkitDefinition xml:lang="vi">Thuật ngữ, cụm từ, ký hiệu phân loại, v.v... chỉ ra tác phẩm nói về cái gì.</rdakit:toolkitDefinition>
      <skos:prefLabel xml:lang="no">emne</skos:prefLabel>
      <rdakit:toolkitLabel xml:lang="no">emne</rdakit:toolkitLabel>
      <skos:definition xml:lang="no">Et ord, begrep, klassifikasjonsnummer, etc. som angir hva et verk handler om.</skos:definition>
      <rdakit:toolkitDefinition xml:lang="no">Et ord, begrep, klassifikasjonsnummer, etc. som angir hva et verk handler om.</rdakit:toolkitDefinition>
    </skos:Concept>
<!-- Concept: subordinate body  -->
    <skos:Concept rdf:about="http://rdaregistry.info/termList/RDATerms/1089" xml:lang="en">
      <skos:inScheme rdf:resource="http://rdaregistry.info/termList/RDATerms"/>
      <reg:status rdf:resource="http://metadataregistry.org/uri/RegStatus/1001"/>
      <reg:identifier rdf:resource="http://metadataregistry.org/concepts/8604"/>
      <skos:prefLabel xml:lang="en">subordinate body</skos:prefLabel>
      <rdakit:toolkitLabel xml:lang="en">subordinate body</rdakit:toolkitLabel>
      <skos:definition xml:lang="en">A corporate body that forms an integral part of a larger body in relation to which it holds an inferior hierarchical rank.</skos:definition>
      <rdakit:toolkitDefinition xml:lang="en">A corporate body that forms an integral part of a larger body in relation to which it holds an inferior hierarchical rank.</rdakit:toolkitDefinition>
      <skos:prefLabel xml:lang="it">ente subordinato</skos:prefLabel>
      <rdakit:toolkitLabel xml:lang="it">ente subordinato</rdakit:toolkitLabel>
      <skos:definition xml:lang="it">Ente che costituisce parte integrante di un ente più grande, rispetto al quale detiene un livello gerarchico inferiore.</skos:definition>
      <rdakit:toolkitDefinition xml:lang="it">Ente che costituisce parte integrante di un ente più grande, rispetto al quale detiene un livello gerarchico inferiore.</rdakit:toolkitDefinition>
      <skos:prefLabel xml:lang="fr">collectivité subordonnée</skos:prefLabel>
      <rdakit:toolkitLabel xml:lang="fr">collectivité subordonnée</rdakit:toolkitLabel>
      <skos:definition xml:lang="fr">Collectivité qui fait partie intégrante d’une collectivité plus vaste et qui, par rapport à celle-ci, occupe une position hiérarchique inférieure.</skos:definition>
      <rdakit:toolkitDefinition xml:lang="fr">Collectivité qui fait partie intégrante d’une collectivité plus vaste et qui, par rapport à celle-ci, occupe une position hiérarchique inférieure.</rdakit:toolkitDefinition>
      <skos:prefLabel xml:lang="de">Untergeordnete Körperschaft</skos:prefLabel>
      <rdakit:toolkitLabel xml:lang="de">Untergeordnete Körperschaft</rdakit:toolkitLabel>
      <skos:definition xml:lang="de">Eine Körperschaft, die einen integralen Bestandteil einer größeren Körperschaft darstellt und die in der Hierarchie unter dieser steht.</skos:definition>
      <rdakit:toolkitDefinition xml:lang="de">Eine Körperschaft, die einen integralen Bestandteil einer größeren Körperschaft darstellt und die in der Hierarchie unter dieser steht.</rdakit:toolkitDefinition>
      <skos:prefLabel xml:lang="fi">alayhteisö</skos:prefLabel>
      <rdakit:toolkitLabel xml:lang="fi">alayhteisö</rdakit:toolkitLabel>
      <skos:definition xml:lang="fi">Yhteisö, joka kuuluu laajempaan yhteisöön ja joka on sen alempi hierarkiataso.</skos:definition>
      <rdakit:toolkitDefinition xml:lang="fi">Yhteisö, joka kuuluu laajempaan yhteisöön ja joka on sen alempi hierarkiataso.</rdakit:toolkitDefinition>
      <skos:prefLabel xml:lang="da">underordnet korporation</skos:prefLabel>
      <rdakit:toolkitLabel xml:lang="da">underordnet korporation</rdakit:toolkitLabel>
      <skos:definition xml:lang="da">Korporation, der er en integreret del af en større korporation og er underlagt denne.</skos:definition>
      <rdakit:toolkitDefinition xml:lang="da">Korporation, der er en integreret del af en større korporation og er underlagt denne.</rdakit:toolkitDefinition>
      <skos:prefLabel xml:lang="ca">entitat subordinada</skos:prefLabel>
      <rdakit:toolkitLabel xml:lang="ca">entitat subordinada</rdakit:toolkitLabel>
      <skos:definition xml:lang="ca">Entitat corporativa que forma part integrant d’una entitat més gran, amb relació a la qual té una posició jeràrquica inferior.</skos:definition>
      <rdakit:toolkitDefinition xml:lang="ca">Entitat corporativa que forma part integrant d’una entitat més gran, amb relació a la qual té una posició jeràrquica inferior.</rdakit:toolkitDefinition>
      <skos:prefLabel xml:lang="vi">tập thể dưới cấp</skos:prefLabel>
      <rdakit:toolkitLabel xml:lang="vi">tập thể dưới cấp</rdakit:toolkitLabel>
      <skos:definition xml:lang="vi">Tập thể là một phần cấu thành của một tập thể lớn hơn, có thứ bậc thấp hơn.</skos:definition>
      <rdakit:toolkitDefinition xml:lang="vi">Tập thể là một phần cấu thành của một tập thể lớn hơn, có thứ bậc thấp hơn.</rdakit:toolkitDefinition>
      <skos:prefLabel xml:lang="no">underordnet organ</skos:prefLabel>
      <rdakit:toolkitLabel xml:lang="no">underordnet organ</rdakit:toolkitLabel>
      <skos:definition xml:lang="no">En korporasjon som er en integrert del av en større korporasjon og som har en lavere rang enn denne.</skos:definition>
      <rdakit:toolkitDefinition xml:lang="no">En korporasjon som er en integrert del av en større korporasjon og som har en lavere rang enn denne.</rdakit:toolkitDefinition>
    </skos:Concept>
<!-- Concept: subseries  -->
    <skos:Concept rdf:about="http://rdaregistry.info/termList/RDATerms/1090" xml:lang="en">
      <skos:inScheme rdf:resource="http://rdaregistry.info/termList/RDATerms"/>
      <reg:status rdf:resource="http://metadataregistry.org/uri/RegStatus/1001"/>
      <reg:identifier rdf:resource="http://metadataregistry.org/concepts/8605"/>
      <skos:prefLabel xml:lang="en">subseries</skos:prefLabel>
      <rdakit:toolkitLabel xml:lang="en">subseries</rdakit:toolkitLabel>
      <skos:definition xml:lang="en">A series within a series, that is, a series that always appears in conjunction with another, usually more comprehensive, series of which it forms a section. Its title may or may not be dependent on the title of the main series.</skos:definition>
      <rdakit:toolkitDefinition xml:lang="en">A series within a series, that is, a series that always appears in conjunction with another, usually more comprehensive, series of which it forms a section. Its title may or may not be dependent on the title of the main series.</rdakit:toolkitDefinition>
      <skos:prefLabel xml:lang="it">sottoserie</skos:prefLabel>
      <rdakit:toolkitLabel xml:lang="it">sottoserie</rdakit:toolkitLabel>
      <skos:definition xml:lang="it">Serie all'interno di una serie (cioè una serie che compare sempre insieme a un'altra serie, solitamente più ampia, di cui essa forma una sezione). Il suo titolo può essere o meno dipendente dal titolo della serie principale.</skos:definition>
      <rdakit:toolkitDefinition xml:lang="it">Serie all'interno di una serie (cioè una serie che compare sempre insieme a un'altra serie, solitamente più ampia, di cui essa forma una sezione). Il suo titolo può essere o meno dipendente dal titolo della serie principale.</rdakit:toolkitDefinition>
      <skos:prefLabel xml:lang="es">subserie</skos:prefLabel>
      <rdakit:toolkitLabel xml:lang="es">subserie</rdakit:toolkitLabel>
      <skos:definition xml:lang="es">Serie dentro de una serie (i.e., una serie que siempre aparece en conjunto con otra serie generalmente más amplia, de la cual aquella forma una sección). Su título puede o no dependiente del título de la serie principal.</skos:definition>
      <rdakit:toolkitDefinition xml:lang="es">Serie dentro de una serie (i.e., una serie que siempre aparece en conjunto con otra serie generalmente más amplia, de la cual aquella forma una sección). Su título puede o no dependiente del título de la serie principal.</rdakit:toolkitDefinition>
      <skos:prefLabel xml:lang="fi">alasarja</skos:prefLabel>
      <rdakit:toolkitLabel xml:lang="fi">alasarja</rdakit:toolkitLabel>
      <skos:definition xml:lang="fi">Sarja, joka ilmestyy toisen (pää)sarjan osana. Alasarjalla voi olla itsenäinen tai epäitsenäinen, pääsarjan nimekkeestä riippuvainen nimeke.</skos:definition>
      <rdakit:toolkitDefinition xml:lang="fi">Sarja, joka ilmestyy toisen (pää)sarjan osana. Alasarjalla voi olla itsenäinen tai epäitsenäinen, pääsarjan nimekkeestä riippuvainen nimeke.</rdakit:toolkitDefinition>
      <skos:prefLabel xml:lang="de">Unterreihe</skos:prefLabel>
      <rdakit:toolkitLabel xml:lang="de">Unterreihe</rdakit:toolkitLabel>
      <skos:definition xml:lang="de">Eine Reihe innerhalb einer Reihe (d. h. eine Reihe, die immer in Verbindung mit einer anderen normalerweise umfassenderen Reihe erscheint, von der sie eine Untergliederung darstellt). Ihr Titel kann von dem Titel der Hauptreihe abhängig sein oder auch nicht.</skos:definition>
      <rdakit:toolkitDefinition xml:lang="de">Eine Reihe innerhalb einer Reihe (d. h. eine Reihe, die immer in Verbindung mit einer anderen normalerweise umfassenderen Reihe erscheint, von der sie eine Untergliederung darstellt). Ihr Titel kann von dem Titel der Hauptreihe abhängig sein oder auch nicht.</rdakit:toolkitDefinition>
      <skos:prefLabel xml:lang="da">underserie</skos:prefLabel>
      <rdakit:toolkitLabel xml:lang="da">underserie</rdakit:toolkitLabel>
      <skos:definition xml:lang="da">Serie i en serie, dvs. en serie, der altid optræder sammen med en anden, normalt mere omfattende, serie og som den udgør en sektion af. Dens titel kan være afhængig af titlen på hovedserien.</skos:definition>
      <rdakit:toolkitDefinition xml:lang="da">Serie i en serie, dvs. en serie, der altid optræder sammen med en anden, normalt mere omfattende, serie og som den udgør en sektion af. Dens titel kan være afhængig af titlen på hovedserien.</rdakit:toolkitDefinition>
      <skos:prefLabel xml:lang="ca">subcol·lecció</skos:prefLabel>
      <rdakit:toolkitLabel xml:lang="ca">subcol·lecció</rdakit:toolkitLabel>
      <skos:definition xml:lang="ca">Col·lecció dins d’una col·lecció, és a dir, una col·lecció que sempre figura en conjunció amb una altra col·lecció, normalment més àmplia, de la qual forma una secció. El seu títol pot dependre, o no, del títol de la col·lecció principal.</skos:definition>
      <rdakit:toolkitDefinition xml:lang="ca">Col·lecció dins d’una col·lecció, és a dir, una col·lecció que sempre figura en conjunció amb una altra col·lecció, normalment més àmplia, de la qual forma una secció. El seu títol pot dependre, o no, del títol de la col·lecció principal.</rdakit:toolkitDefinition>
      <skos:prefLabel xml:lang="fr">sous-collection</skos:prefLabel>
      <rdakit:toolkitLabel xml:lang="fr">sous-collection</rdakit:toolkitLabel>
      <skos:definition xml:lang="fr">Collection faisant partie d’une collection, c’est-à-dire une collection qui apparaît toujours conjointement avec une autre collection, habituellement plus vaste, dont elle forme une section. Son titre peut ou non être dépendant de celui de la collection principale.</skos:definition>
      <rdakit:toolkitDefinition xml:lang="fr">Collection faisant partie d’une collection, c’est-à-dire une collection qui apparaît toujours conjointement avec une autre collection, habituellement plus vaste, dont elle forme une section. Son titre peut ou non être dépendant de celui de la collection principale.</rdakit:toolkitDefinition>
      <skos:prefLabel xml:lang="vi">tiểu tùng thư</skos:prefLabel>
      <rdakit:toolkitLabel xml:lang="vi">tiểu tùng thư</rdakit:toolkitLabel>
      <skos:definition xml:lang="vi">Tùng thư bên trong tùng thư, nghĩa là, tùng thư luôn xuất hiện cùng chung với tùng thư khác tổng hợp hơn, tùng thư mà nó tạo thành một bộ phận. Nhan đề có thể phụ thuộc vào nhan đề của tùng thư chính hoặc không.</skos:definition>
      <rdakit:toolkitDefinition xml:lang="vi">Tùng thư bên trong tùng thư, nghĩa là, tùng thư luôn xuất hiện cùng chung với tùng thư khác tổng hợp hơn, tùng thư mà nó tạo thành một bộ phận. Nhan đề có thể phụ thuộc vào nhan đề của tùng thư chính hoặc không.</rdakit:toolkitDefinition>
      <skos:prefLabel xml:lang="no">underserie</skos:prefLabel>
      <rdakit:toolkitLabel xml:lang="no">underserie</rdakit:toolkitLabel>
      <skos:definition xml:lang="no">En serie innen en serie, dvs. en serie som alltid opptrer i forbindelse med en annen, vanligvis mer omfattende, serie som den er en del av. Tittelen kan være avhengig eller uavhengig av hovedseriens tittel.</skos:definition>
      <rdakit:toolkitDefinition xml:lang="no">En serie innen en serie, dvs. en serie som alltid opptrer i forbindelse med en annen, vanligvis mer omfattende, serie som den er en del av. Tittelen kan være avhengig eller uavhengig av hovedseriens tittel.</rdakit:toolkitDefinition>
    </skos:Concept>
<!-- Concept: subtitle  -->
    <skos:Concept rdf:about="http://rdaregistry.info/termList/RDATerms/1091" xml:lang="en">
      <skos:inScheme rdf:resource="http://rdaregistry.info/termList/RDATerms"/>
      <reg:status rdf:resource="http://metadataregistry.org/uri/RegStatus/1001"/>
      <reg:identifier rdf:resource="http://metadataregistry.org/concepts/8606"/>
      <skos:prefLabel xml:lang="en">subtitle</skos:prefLabel>
      <rdakit:toolkitLabel xml:lang="en">subtitle</rdakit:toolkitLabel>
      <skos:definition xml:lang="en">A text displayed at the bottom of a moving image expression that is a translation or transcription of the dialogue or narrative.</skos:definition>
      <rdakit:toolkitDefinition xml:lang="en">A text displayed at the bottom of a moving image expression that is a translation or transcription of the dialogue or narrative.</rdakit:toolkitDefinition>
      <skos:prefLabel xml:lang="de">Untertitel</skos:prefLabel>
      <rdakit:toolkitLabel xml:lang="de">Untertitel</rdakit:toolkitLabel>
      <skos:definition xml:lang="de">Ein Text, der am unteren Rand eines Films angezeigt wird, der eine Übersetzung oder Transkription des Dialogs oder der Erzählung ist.</skos:definition>
      <rdakit:toolkitDefinition xml:lang="de">Ein Text, der am unteren Rand eines Films angezeigt wird, der eine Übersetzung oder Transkription des Dialogs oder der Erzählung ist.</rdakit:toolkitDefinition>
      <skos:prefLabel xml:lang="fi">tekstitys</skos:prefLabel>
      <rdakit:toolkitLabel xml:lang="fi">tekstitys</rdakit:toolkitLabel>
      <skos:definition xml:lang="fi">Liikkuvasta kuvasta koostuvan ekspression alalaidassa oleva teksti, joka on dialogin tai kerronnan käännös tai transkriptio.</skos:definition>
      <rdakit:toolkitDefinition xml:lang="fi">Liikkuvasta kuvasta koostuvan ekspression alalaidassa oleva teksti, joka on dialogin tai kerronnan käännös tai transkriptio.</rdakit:toolkitDefinition>
      <skos:prefLabel xml:lang="da">undertekster</skos:prefLabel>
      <rdakit:toolkitLabel xml:lang="da">undertekster</rdakit:toolkitLabel>
      <skos:definition xml:lang="da">Tekst, der fremvises nederst på et udtryk af levende billeder og som er en oversættelse af dialogen eller fortællingen.</skos:definition>
      <rdakit:toolkitDefinition xml:lang="da">Tekst, der fremvises nederst på et udtryk af levende billeder og som er en oversættelse af dialogen eller fortællingen.</rdakit:toolkitDefinition>
      <skos:prefLabel xml:lang="ca">subtítol</skos:prefLabel>
      <rdakit:toolkitLabel xml:lang="ca">subtítol</rdakit:toolkitLabel>
      <skos:definition xml:lang="ca">Text que es visualitza a la part inferior d'una expressió d'imatge en moviment que és una traducció o la transcripció del diàleg o narrativa.</skos:definition>
      <rdakit:toolkitDefinition xml:lang="ca">Text que es visualitza a la part inferior d'una expressió d'imatge en moviment que és una traducció o la transcripció del diàleg o narrativa.</rdakit:toolkitDefinition>
      <skos:prefLabel xml:lang="fr">sous-titre</skos:prefLabel>
      <rdakit:toolkitLabel xml:lang="fr">sous-titre</rdakit:toolkitLabel>
      <skos:definition xml:lang="fr">Texte affiché au bas d’une expression d’images animées et qui consiste en une traduction ou en une transcription des dialogues ou de la narration.</skos:definition>
      <rdakit:toolkitDefinition xml:lang="fr">Texte affiché au bas d’une expression d’images animées et qui consiste en une traduction ou en une transcription des dialogues ou de la narration.</rdakit:toolkitDefinition>
      <skos:prefLabel xml:lang="vi">phụ đề</skos:prefLabel>
      <rdakit:toolkitLabel xml:lang="vi">phụ đề</rdakit:toolkitLabel>
      <skos:definition xml:lang="vi">Văn bản hiện ra ở cuối biểu hiện hình ảnh động là bản dịch hoặc chuyển tự của đối thoại hoặc câu chuyện kể.</skos:definition>
      <rdakit:toolkitDefinition xml:lang="vi">Văn bản hiện ra ở cuối biểu hiện hình ảnh động là bản dịch hoặc chuyển tự của đối thoại hoặc câu chuyện kể.</rdakit:toolkitDefinition>
      <skos:prefLabel xml:lang="no">undertekst</skos:prefLabel>
      <rdakit:toolkitLabel xml:lang="no">undertekst</rdakit:toolkitLabel>
      <skos:definition xml:lang="no">En tekst som vises nederst på et uttrykk i form av levende bilder og som er en oversettelse eller omskrivning av dialogen eller historien.</skos:definition>
      <rdakit:toolkitDefinition xml:lang="no">En tekst som vises nederst på et uttrykk i form av levende bilder og som er en oversettelse eller omskrivning av dialogen eller historien.</rdakit:toolkitDefinition>
    </skos:Concept>
<!-- Concept: subunit  -->
    <skos:Concept rdf:about="http://rdaregistry.info/termList/RDATerms/1092" xml:lang="en">
      <skos:inScheme rdf:resource="http://rdaregistry.info/termList/RDATerms"/>
      <reg:status rdf:resource="http://metadataregistry.org/uri/RegStatus/1001"/>
      <reg:identifier rdf:resource="http://metadataregistry.org/concepts/8607"/>
      <skos:prefLabel xml:lang="en">subunit</skos:prefLabel>
      <rdakit:toolkitLabel xml:lang="en">subunit</rdakit:toolkitLabel>
      <skos:definition xml:lang="en">A physical or logical subdivision of a unit.</skos:definition>
      <rdakit:toolkitDefinition xml:lang="en">A physical or logical subdivision of a unit.</rdakit:toolkitDefinition>
      <skos:scopeNote xml:lang="en">A subunit includes a page of a volume, a frame of a microfiche, a record in a digital file, etc.</skos:scopeNote>
      <skos:prefLabel xml:lang="it">sottounità</skos:prefLabel>
      <rdakit:toolkitLabel xml:lang="it">sottounità</rdakit:toolkitLabel>
      <skos:definition xml:lang="it">Suddivisione fisica o logica di una unità.</skos:definition>
      <rdakit:toolkitDefinition xml:lang="it">Suddivisione fisica o logica di una unità.</rdakit:toolkitDefinition>
      <skos:prefLabel xml:lang="fr">sous-unité</skos:prefLabel>
      <rdakit:toolkitLabel xml:lang="fr">sous-unité</rdakit:toolkitLabel>
      <skos:definition xml:lang="fr">Subdivision physique ou logique d’une unité.</skos:definition>
      <rdakit:toolkitDefinition xml:lang="fr">Subdivision physique ou logique d’une unité.</rdakit:toolkitDefinition>
      <skos:prefLabel xml:lang="es">subunidad</skos:prefLabel>
      <rdakit:toolkitLabel xml:lang="es">subunidad</rdakit:toolkitLabel>
      <skos:definition xml:lang="es">Una subdivisión física o lógica de una unidad.</skos:definition>
      <rdakit:toolkitDefinition xml:lang="es">Una subdivisión física o lógica de una unidad.</rdakit:toolkitDefinition>
      <skos:prefLabel xml:lang="de">Untereinheit</skos:prefLabel>
      <rdakit:toolkitLabel xml:lang="de">Untereinheit</rdakit:toolkitLabel>
      <skos:definition xml:lang="de">Eine physische oder logische Untergliederung einer Einheit.</skos:definition>
      <rdakit:toolkitDefinition xml:lang="de">Eine physische oder logische Untergliederung einer Einheit.</rdakit:toolkitDefinition>
      <skos:scopeNote xml:lang="de">Dazu gehören eine Seite eines Bandes, ein Einzelbild auf einem Mikrofiche oder ein Datensatz in einer Datei.</skos:scopeNote>
      <skos:prefLabel xml:lang="fi">osayksikkö</skos:prefLabel>
      <rdakit:toolkitLabel xml:lang="fi">osayksikkö</rdakit:toolkitLabel>
      <skos:definition xml:lang="fi">Yksikön fyysinen tai looginen osajaotus.</skos:definition>
      <rdakit:toolkitDefinition xml:lang="fi">Yksikön fyysinen tai looginen osajaotus.</rdakit:toolkitDefinition>
      <skos:scopeNote xml:lang="fi">Esim. niteessä yksi sivu, mikrokortin ruutu, tiedoston tietue jne.</skos:scopeNote>
      <skos:prefLabel xml:lang="da">underenhed</skos:prefLabel>
      <rdakit:toolkitLabel xml:lang="da">underenhed</rdakit:toolkitLabel>
      <skos:definition xml:lang="da">Fysisk eller logisk del af en større enhed.</skos:definition>
      <rdakit:toolkitDefinition xml:lang="da">Fysisk eller logisk del af en større enhed.</rdakit:toolkitDefinition>
      <skos:scopeNote xml:lang="da">En underenhed omfatter en side af et bind, et mikrofichebillede, en post i en digital fil etc.</skos:scopeNote>
      <skos:prefLabel xml:lang="ca">subunitat</skos:prefLabel>
      <rdakit:toolkitLabel xml:lang="ca">subunitat</rdakit:toolkitLabel>
      <skos:definition xml:lang="ca">Subdivisió física o lògica d’una unitat.</skos:definition>
      <rdakit:toolkitDefinition xml:lang="ca">Subdivisió física o lògica d’una unitat.</rdakit:toolkitDefinition>
      <skos:scopeNote xml:lang="ca">Una subunitat inclou una pàgina d’un volum, un fotograma d’una microfitxa, un registre d’un fitxer digital, etc.</skos:scopeNote>
      <skos:scopeNote xml:lang="fr">Comprend une page d’un volume, une image d’une microfiche, un enregistrement dans un fichier numérique, etc.</skos:scopeNote>
      <skos:prefLabel xml:lang="vi">tiểu đơn vị</skos:prefLabel>
      <rdakit:toolkitLabel xml:lang="vi">tiểu đơn vị</rdakit:toolkitLabel>
      <skos:definition xml:lang="vi">Một chia nhỏ về vật lý hoặc logic của đơn vị.</skos:definition>
      <rdakit:toolkitDefinition xml:lang="vi">Một chia nhỏ về vật lý hoặc logic của đơn vị.</rdakit:toolkitDefinition>
      <skos:scopeNote xml:lang="vi">Tiểu đơn vị bao gồm trang của tập, khung hình của vi phiếu, biểu ghi trong tệp số, v.v...</skos:scopeNote>
      <skos:prefLabel xml:lang="no">underenhet</skos:prefLabel>
      <rdakit:toolkitLabel xml:lang="no">underenhet</rdakit:toolkitLabel>
      <skos:definition xml:lang="no">En fysisk eller logisk underinndeling av en enhet.</skos:definition>
      <rdakit:toolkitDefinition xml:lang="no">En fysisk eller logisk underinndeling av en enhet.</rdakit:toolkitDefinition>
      <skos:scopeNote xml:lang="no">En underenhet inkluderer en side i en bok, et bilde i en mikrofiche, en post i en digital fil, etc.</skos:scopeNote>
    </skos:Concept>
<!-- Concept: thematic index  -->
    <skos:Concept rdf:about="http://rdaregistry.info/termList/RDATerms/1093" xml:lang="en">
      <skos:inScheme rdf:resource="http://rdaregistry.info/termList/RDATerms"/>
      <reg:status rdf:resource="http://metadataregistry.org/uri/RegStatus/1001"/>
      <reg:identifier rdf:resource="http://metadataregistry.org/concepts/8608"/>
      <skos:prefLabel xml:lang="en">thematic index</skos:prefLabel>
      <rdakit:toolkitLabel xml:lang="en">thematic index</rdakit:toolkitLabel>
      <skos:definition xml:lang="en">A list of a composer’s works, usually arranged in chronological order or by categories, with the theme given for each composition or for each section of large compositions.</skos:definition>
      <rdakit:toolkitDefinition xml:lang="en">A list of a composer’s works, usually arranged in chronological order or by categories, with the theme given for each composition or for each section of large compositions.</rdakit:toolkitDefinition>
      <skos:prefLabel xml:lang="it">catalogo tematico</skos:prefLabel>
      <rdakit:toolkitLabel xml:lang="it">catalogo tematico</rdakit:toolkitLabel>
      <skos:definition xml:lang="it">Elenco delle opere di un compositore, solitamente ordinato in ordine cronologico o per categorie, con il tema per ciascuna composizione o per ciascuna sezione delle grandi composizioni.</skos:definition>
      <rdakit:toolkitDefinition xml:lang="it">Elenco delle opere di un compositore, solitamente ordinato in ordine cronologico o per categorie, con il tema per ciascuna composizione o per ciascuna sezione delle grandi composizioni.</rdakit:toolkitDefinition>
      <skos:prefLabel xml:lang="de">Werkverzeichnis</skos:prefLabel>
      <rdakit:toolkitLabel xml:lang="de">Werkverzeichnis</rdakit:toolkitLabel>
      <skos:definition xml:lang="de">Eine Liste von Werken eines Komponisten, die meist in chronologischer Reihenfolge oder nach Kategorien sortiert ist, mit Angabe des Themas für jede Komposition oder für jede Passage längerer Kompositionen.</skos:definition>
      <rdakit:toolkitDefinition xml:lang="de">Eine Liste von Werken eines Komponisten, die meist in chronologischer Reihenfolge oder nach Kategorien sortiert ist, mit Angabe des Themas für jede Komposition oder für jede Passage längerer Kompositionen.</rdakit:toolkitDefinition>
      <skos:prefLabel xml:lang="fi">temaattinen teosluettelo</skos:prefLabel>
      <rdakit:toolkitLabel xml:lang="fi">temaattinen teosluettelo</rdakit:toolkitLabel>
      <skos:definition xml:lang="fi">Luettelo säveltäjän teoksista, yleensä järjestetty aikajärjestykseen tai kategorioittain sisältäen teeman jokaisesta sävellyksestä tai laajan sävellyksen osasta.</skos:definition>
      <rdakit:toolkitDefinition xml:lang="fi">Luettelo säveltäjän teoksista, yleensä järjestetty aikajärjestykseen tai kategorioittain sisältäen teeman jokaisesta sävellyksestä tai laajan sävellyksen osasta.</rdakit:toolkitDefinition>
      <skos:prefLabel xml:lang="da">værkfortegnelse</skos:prefLabel>
      <rdakit:toolkitLabel xml:lang="da">værkfortegnelse</rdakit:toolkitLabel>
      <skos:definition xml:lang="da">Liste over en komponists værker, normalt arrangeret i kronologisk rækkefølge eller i kategorier med tema angivet for hver komposition eller for hver sektion af store kompositioner.</skos:definition>
      <rdakit:toolkitDefinition xml:lang="da">Liste over en komponists værker, normalt arrangeret i kronologisk rækkefølge eller i kategorier med tema angivet for hver komposition eller for hver sektion af store kompositioner.</rdakit:toolkitDefinition>
      <skos:prefLabel xml:lang="ca">índex temàtic</skos:prefLabel>
      <rdakit:toolkitLabel xml:lang="ca">índex temàtic</rdakit:toolkitLabel>
      <skos:definition xml:lang="ca">Llista de les obres d’un compositor, ordenades normalment per ordre cronològic o per categories, amb el tema de cada composició o, en el cas de composicions àmplies, de cada secció.</skos:definition>
      <rdakit:toolkitDefinition xml:lang="ca">Llista de les obres d’un compositor, ordenades normalment per ordre cronològic o per categories, amb el tema de cada composició o, en el cas de composicions àmplies, de cada secció.</rdakit:toolkitDefinition>
      <skos:prefLabel xml:lang="fr">catalogue thématique</skos:prefLabel>
      <rdakit:toolkitLabel xml:lang="fr">catalogue thématique</rdakit:toolkitLabel>
      <skos:definition xml:lang="fr">Liste des œuvres d’un compositeur, ordinairement classées par ordre chronologique ou par catégories, avec le thème de chaque composition ou de chaque section d’une composition dans le cas des compositions d’envergure.</skos:definition>
      <rdakit:toolkitDefinition xml:lang="fr">Liste des œuvres d’un compositeur, ordinairement classées par ordre chronologique ou par catégories, avec le thème de chaque composition ou de chaque section d’une composition dans le cas des compositions d’envergure.</rdakit:toolkitDefinition>
      <skos:prefLabel xml:lang="vi">chỉ mục chủ đề</skos:prefLabel>
      <rdakit:toolkitLabel xml:lang="vi">chỉ mục chủ đề</rdakit:toolkitLabel>
      <skos:definition xml:lang="vi">Danh mục các tác phẩm của một người sáng tác, thường được xếp theo trật tự biên niên hoặc theo loại hình, với chủ đề cho mỗi sáng tác hoặc cho mỗi mục của sáng tác lớn.</skos:definition>
      <rdakit:toolkitDefinition xml:lang="vi">Danh mục các tác phẩm của một người sáng tác, thường được xếp theo trật tự biên niên hoặc theo loại hình, với chủ đề cho mỗi sáng tác hoặc cho mỗi mục của sáng tác lớn.</rdakit:toolkitDefinition>
      <skos:prefLabel xml:lang="no">tematisk verkfortegnelse</skos:prefLabel>
      <rdakit:toolkitLabel xml:lang="no">tematisk verkfortegnelse</rdakit:toolkitLabel>
      <skos:definition xml:lang="no">En fortegnelse over en komponists verk, vanligvis ført opp i kronologisk orden eller etter kategorier, med temaet angitt for hver komposisjon eller hver seksjon av større komposisjoner.</skos:definition>
      <rdakit:toolkitDefinition xml:lang="no">En fortegnelse over en komponists verk, vanligvis ført opp i kronologisk orden eller etter kategorier, med temaet angitt for hver komposisjon eller hver seksjon av større komposisjoner.</rdakit:toolkitDefinition>
    </skos:Concept>
<!-- Concept: title frame  -->
    <skos:Concept rdf:about="http://rdaregistry.info/termList/RDATerms/1094" xml:lang="en">
      <skos:inScheme rdf:resource="http://rdaregistry.info/termList/RDATerms"/>
      <reg:status rdf:resource="http://metadataregistry.org/uri/RegStatus/1001"/>
      <reg:identifier rdf:resource="http://metadataregistry.org/concepts/8609"/>
      <skos:prefLabel xml:lang="en">title frame</skos:prefLabel>
      <rdakit:toolkitLabel xml:lang="en">title frame</rdakit:toolkitLabel>
      <skos:definition xml:lang="en">A frame or frames, usually found at the beginning of a manifestation produced on film, containing identifying textual information which is not part of the subject content of the work and which is used as a source of information in creating a description.</skos:definition>
      <rdakit:toolkitDefinition xml:lang="en">A frame or frames, usually found at the beginning of a manifestation produced on film, containing identifying textual information which is not part of the subject content of the work and which is used as a source of information in creating a description.</rdakit:toolkitDefinition>
      <skos:prefLabel xml:lang="it">fotogramma del titolo</skos:prefLabel>
      <rdakit:toolkitLabel xml:lang="it">fotogramma del titolo</rdakit:toolkitLabel>
      <skos:definition xml:lang="it">Uno o più fotogrammi, solitamente all'inizio di una risorsa prodotta su pellicola (film, filmina, etc.) che contengono informazioni testuali identificative, non comprese nel contenuto di soggetto della risorsa, e che sono utilizzati come fonte delle informazioni nella creazione della descrizione.</skos:definition>
      <rdakit:toolkitDefinition xml:lang="it">Uno o più fotogrammi, solitamente all'inizio di una risorsa prodotta su pellicola (film, filmina, etc.) che contengono informazioni testuali identificative, non comprese nel contenuto di soggetto della risorsa, e che sono utilizzati come fonte delle informazioni nella creazione della descrizione.</rdakit:toolkitDefinition>
      <skos:prefLabel xml:lang="de">Titelbildfeld</skos:prefLabel>
      <rdakit:toolkitLabel xml:lang="de">Titelbildfeld</rdakit:toolkitLabel>
      <skos:definition xml:lang="de">Ein Bildfeld oder Bildfelder, das/die normalerweise am Anfang einer Manifestation gefunden wird/werden, die auf Film produziert sind. Es/Sie enthält/enthalten identifizierende Textinformationen, die nicht Teil des inhaltlichen Themas eines Werks sind und das/die als Informationsquelle bei der Erstellung einer Beschreibung verwendet werden.</skos:definition>
      <rdakit:toolkitDefinition xml:lang="de">Ein Bildfeld oder Bildfelder, das/die normalerweise am Anfang einer Manifestation gefunden wird/werden, die auf Film produziert sind. Es/Sie enthält/enthalten identifizierende Textinformationen, die nicht Teil des inhaltlichen Themas eines Werks sind und das/die als Informationsquelle bei der Erstellung einer Beschreibung verwendet werden.</rdakit:toolkitDefinition>
      <skos:prefLabel xml:lang="fi">alku- ja/tai lopputekstit</skos:prefLabel>
      <rdakit:toolkitLabel xml:lang="fi">alku- ja/tai lopputekstit</rdakit:toolkitLabel>
      <skos:definition xml:lang="fi">Filmille tuotetunmanifestaation alussa tai lopussa esiintyvät kuvaruudut.Sisältävät teosta määrittävää, mutta teoksen aihesisältöön kuulumatonta tekstimuotoista tietoa, jota käytetään teoksen kuvailun lähteenä.</skos:definition>
      <rdakit:toolkitDefinition xml:lang="fi">Filmille tuotetunmanifestaation alussa tai lopussa esiintyvät kuvaruudut.Sisältävät teosta määrittävää, mutta teoksen aihesisältöön kuulumatonta tekstimuotoista tietoa, jota käytetään teoksen kuvailun lähteenä.</rdakit:toolkitDefinition>
      <skos:prefLabel xml:lang="da">titelbillede</skos:prefLabel>
      <rdakit:toolkitLabel xml:lang="da">titelbillede</rdakit:toolkitLabel>
      <skos:definition xml:lang="da">Et billede, eller flere billeder, normalt i begyndelsen af en filmmanifestation, der indeholder identificerende tekstoplysninger, der ikke er en del af værkets emneindhold, og som anvendes som kilde for oplysninger til at udforme en beskrivelse.</skos:definition>
      <rdakit:toolkitDefinition xml:lang="da">Et billede, eller flere billeder, normalt i begyndelsen af en filmmanifestation, der indeholder identificerende tekstoplysninger, der ikke er en del af værkets emneindhold, og som anvendes som kilde for oplysninger til at udforme en beskrivelse.</rdakit:toolkitDefinition>
      <skos:prefLabel xml:lang="ca">fotograma de títol</skos:prefLabel>
      <rdakit:toolkitLabel xml:lang="ca">fotograma de títol</rdakit:toolkitLabel>
      <skos:definition xml:lang="ca">Fotograma o fotogrames, normalment a l’inici d’una manifestació produïda sobre pel·lícula, que conté informació textual identificadora, que no forma part del contingut temàtic de l'obra i que s’usa com a font d’informació en crear una descripció.</skos:definition>
      <rdakit:toolkitDefinition xml:lang="ca">Fotograma o fotogrames, normalment a l’inici d’una manifestació produïda sobre pel·lícula, que conté informació textual identificadora, que no forma part del contingut temàtic de l'obra i que s’usa com a font d’informació en crear una descripció.</rdakit:toolkitDefinition>
      <skos:prefLabel xml:lang="fr">image du titre</skos:prefLabel>
      <rdakit:toolkitLabel xml:lang="fr">image du titre</rdakit:toolkitLabel>
      <skos:definition xml:lang="fr">Une ou plusieurs images trouvées ordinairement au début d’une manifestation produite sur film, contenant de l’information d’identification textuelle ne faisant pas partie du contenu thématique de l’œuvre et utilisées comme source d’information pour créer une description.</skos:definition>
      <rdakit:toolkitDefinition xml:lang="fr">Une ou plusieurs images trouvées ordinairement au début d’une manifestation produite sur film, contenant de l’information d’identification textuelle ne faisant pas partie du contenu thématique de l’œuvre et utilisées comme source d’information pour créer une description.</rdakit:toolkitDefinition>
      <skos:prefLabel xml:lang="vi">khung nhan đề</skos:prefLabel>
      <rdakit:toolkitLabel xml:lang="vi">khung nhan đề</rdakit:toolkitLabel>
      <skos:definition xml:lang="vi">Một hoặc nhiều khung, thường ở đầu của biểu thị được sản xuất trên phim chứa thông tin văn bản nhận dạng, không thuộc nội dung chủ đề của tài nguyên và được dùng như nguồn lấy thông tin để mô tả.</skos:definition>
      <rdakit:toolkitDefinition xml:lang="vi">Một hoặc nhiều khung, thường ở đầu của biểu thị được sản xuất trên phim chứa thông tin văn bản nhận dạng, không thuộc nội dung chủ đề của tài nguyên và được dùng như nguồn lấy thông tin để mô tả.</rdakit:toolkitDefinition>
      <skos:prefLabel xml:lang="no">tittelsekvens</skos:prefLabel>
      <rdakit:toolkitLabel xml:lang="no">tittelsekvens</rdakit:toolkitLabel>
      <skos:definition xml:lang="no">En rute eller sekvens med tekstinformasjon, som oftest i forkant eller starten av en manifestasjon produsert på film, som brukes for å beskrive/katalogisere verket utover filmens innhold eller handling.</skos:definition>
      <rdakit:toolkitDefinition xml:lang="no">En rute eller sekvens med tekstinformasjon, som oftest i forkant eller starten av en manifestasjon produsert på film, som brukes for å beskrive/katalogisere verket utover filmens innhold eller handling.</rdakit:toolkitDefinition>
    </skos:Concept>
<!-- Concept: title page  -->
    <skos:Concept rdf:about="http://rdaregistry.info/termList/RDATerms/1095" xml:lang="en">
      <skos:inScheme rdf:resource="http://rdaregistry.info/termList/RDATerms"/>
      <reg:status rdf:resource="http://metadataregistry.org/uri/RegStatus/1001"/>
      <reg:identifier rdf:resource="http://metadataregistry.org/concepts/8610"/>
      <skos:prefLabel xml:lang="en">title page</skos:prefLabel>
      <rdakit:toolkitLabel xml:lang="en">title page</rdakit:toolkitLabel>
      <skos:definition xml:lang="en">A page at the beginning of a manifestation bearing a title proper and usually, though not necessarily, a statement of responsibility and data relating to publication.</skos:definition>
      <rdakit:toolkitDefinition xml:lang="en">A page at the beginning of a manifestation bearing a title proper and usually, though not necessarily, a statement of responsibility and data relating to publication.</rdakit:toolkitDefinition>
      <skos:scopeNote xml:lang="en">Facing pages or pages on successive leaves containing this information with or without repetition are considered collectively as a title page.</skos:scopeNote>
	    <skos:related rdf:resource="http://rdaregistry.info/termList/RDATerms/1004"/>
	    <skos:related rdf:resource="http://rdaregistry.info/termList/RDATerms/1082"/>
      <skos:prefLabel xml:lang="it">frontespizio</skos:prefLabel>
      <rdakit:toolkitLabel xml:lang="it">frontespizio</rdakit:toolkitLabel>
      <skos:definition xml:lang="it">Pagina all'inizio di una risorsa che reca il titolo proprio e solitamente, benché non necessariamente, la formulazione di responsabilità e la data di pubblicazione.</skos:definition>
      <rdakit:toolkitDefinition xml:lang="it">Pagina all'inizio di una risorsa che reca il titolo proprio e solitamente, benché non necessariamente, la formulazione di responsabilità e la data di pubblicazione.</rdakit:toolkitDefinition>
      <skos:scopeNote xml:lang="it">Se queste informazioni sono date su due pagine a fronte o su pagine delle carte successive, con o senza ripetizioni, queste pagine si trattano nel loro insieme come frontespizio.</skos:scopeNote>
      <skos:prefLabel xml:lang="de">Titelseite</skos:prefLabel>
      <rdakit:toolkitLabel xml:lang="de">Titelseite</rdakit:toolkitLabel>
      <skos:definition xml:lang="de">Eine Seite am Anfang der Manifestation, die den Haupttitel und meistens, aber nicht notwendigerweise, die Verantwortlichkeitsangabe und das Erscheinungsdatum aufführt.</skos:definition>
      <rdakit:toolkitDefinition xml:lang="de">Eine Seite am Anfang der Manifestation, die den Haupttitel und meistens, aber nicht notwendigerweise, die Verantwortlichkeitsangabe und das Erscheinungsdatum aufführt.</rdakit:toolkitDefinition>
      <skos:scopeNote xml:lang="de">Wenn diese Informationen auf gegenüberliegenden Seiten oder Seiten auf folgenden Blättern stehen, mit oder ohne Wiederholung, sind diese Seiten zusammen als Titelseite zu behandeln.</skos:scopeNote>
      <skos:prefLabel xml:lang="fi">nimiösivu</skos:prefLabel>
      <rdakit:toolkitLabel xml:lang="fi">nimiösivu</rdakit:toolkitLabel>
      <skos:definition xml:lang="fi">Aineiston alussa oleva sivu, jossa on päänimeke ja usein, mutta ei välttämättä, vastuullisuustiedot sekä julkaisuun liittyvää tietoa.</skos:definition>
      <rdakit:toolkitDefinition xml:lang="fi">Aineiston alussa oleva sivu, jossa on päänimeke ja usein, mutta ei välttämättä, vastuullisuustiedot sekä julkaisuun liittyvää tietoa.</rdakit:toolkitDefinition>
      <skos:scopeNote xml:lang="fi">Jos nämä tiedot jakautuvat vastakkaisille sivuille tai seuraavilen lehtien sivuille (toistettuina tai ilman), katsotaan että nämä sivut yhdessä muodostavat nimiösivun.</skos:scopeNote>
      <skos:prefLabel xml:lang="da">titelside</skos:prefLabel>
      <rdakit:toolkitLabel xml:lang="da">titelside</rdakit:toolkitLabel>
      <skos:definition xml:lang="da">Side forrest i en manifestation, der indeholder hovedtitlen og normalt, men ikke nødvendigvis, ophavsangivelse samt oplysninger relateret til publicering.</skos:definition>
      <rdakit:toolkitDefinition xml:lang="da">Side forrest i en manifestation, der indeholder hovedtitlen og normalt, men ikke nødvendigvis, ophavsangivelse samt oplysninger relateret til publicering.</rdakit:toolkitDefinition>
      <skos:scopeNote xml:lang="da">Hvis disse oplysninger gives på modsatte sider eller sider på successive blade, med eller uden gentagelse, behandles disse samlet som titelside.</skos:scopeNote>
      <skos:prefLabel xml:lang="ca">portada</skos:prefLabel>
      <rdakit:toolkitLabel xml:lang="ca">portada</rdakit:toolkitLabel>
      <skos:definition xml:lang="ca">Pàgina a l’inici d’una manifestació que porta un títol propi i normalment, tot i que no necessàriament, una menció de responsabilitat i les dades relatives a la publicació.</skos:definition>
      <rdakit:toolkitDefinition xml:lang="ca">Pàgina a l’inici d’una manifestació que porta un títol propi i normalment, tot i que no necessàriament, una menció de responsabilitat i les dades relatives a la publicació.</rdakit:toolkitDefinition>
      <skos:scopeNote xml:lang="ca">Les pàgines encarades o les pàgines en fulls successius que contenen aquesta informació, amb o sense repetició, es tracten col·lectivament com a portada.</skos:scopeNote>
      <skos:prefLabel xml:lang="fr">page de titre</skos:prefLabel>
      <rdakit:toolkitLabel xml:lang="fr">page de titre</rdakit:toolkitLabel>
      <skos:definition xml:lang="fr">Page située au début d’une manifestation, portant un titre propre et ordinairement, mais pas nécessairement, une mention de responsabilité et des données relatives à la publication.</skos:definition>
      <rdakit:toolkitDefinition xml:lang="fr">Page située au début d’une manifestation, portant un titre propre et ordinairement, mais pas nécessairement, une mention de responsabilité et des données relatives à la publication.</rdakit:toolkitDefinition>
      <skos:scopeNote xml:lang="fr">Deux pages en regard ou des pages sur des feuillets successifs contenant ces informations, avec ou sans redondance, sont traitées collectivement comme une page de titre.</skos:scopeNote>
      <skos:prefLabel xml:lang="vi">trang nhan đề</skos:prefLabel>
      <rdakit:toolkitLabel xml:lang="vi">trang nhan đề</rdakit:toolkitLabel>
      <skos:definition xml:lang="vi">Trang ở đầu một biểu thị chứa nhan đề hợp thức và thường, mặc dù không nhất thiết, thông tin trách nhiệm và dữ liệu liên quan tới xuất bản.</skos:definition>
      <rdakit:toolkitDefinition xml:lang="vi">Trang ở đầu một biểu thị chứa nhan đề hợp thức và thường, mặc dù không nhất thiết, thông tin trách nhiệm và dữ liệu liên quan tới xuất bản.</rdakit:toolkitDefinition>
      <skos:scopeNote xml:lang="vi">Trang đối diện hoặc trang kế tiếp có chứ thông tin này, có hoặc không nhắc lại được xem tập thể như là trang nhan đề.</skos:scopeNote>
      <skos:prefLabel xml:lang="no">tittelside</skos:prefLabel>
      <rdakit:toolkitLabel xml:lang="no">tittelside</rdakit:toolkitLabel>
      <skos:definition xml:lang="no">En side i begynnelsen av en manifestasjon, som inneholder hovedtittel og som oftest, men ikke nødvendigvis, opplysninger om ansvarshavende og utgivelsesinformasjon.</skos:definition>
      <rdakit:toolkitDefinition xml:lang="no">En side i begynnelsen av en manifestasjon, som inneholder hovedtittel og som oftest, men ikke nødvendigvis, opplysninger om ansvarshavende og utgivelsesinformasjon.</rdakit:toolkitDefinition>
      <skos:scopeNote xml:lang="no">Hvis denne informasjonen er oppgitt på motstående sider eller på etterfølgende blader, med eller uten gjentagelse, betraktes disse sidene til sammen som tittelsiden.</skos:scopeNote>
    </skos:Concept>
<!-- Concept: title screen  -->
    <skos:Concept rdf:about="http://rdaregistry.info/termList/RDATerms/1096" xml:lang="en">
      <skos:inScheme rdf:resource="http://rdaregistry.info/termList/RDATerms"/>
      <reg:status rdf:resource="http://metadataregistry.org/uri/RegStatus/1001"/>
      <reg:identifier rdf:resource="http://metadataregistry.org/concepts/8611"/>
      <skos:prefLabel xml:lang="en">title screen</skos:prefLabel>
      <rdakit:toolkitLabel xml:lang="en">title screen</rdakit:toolkitLabel>
      <skos:definition xml:lang="en">A display of data about a digital manifestation that includes a title proper and usually, though not necessarily, a statement of responsibility and data relating to publication.</skos:definition>
      <rdakit:toolkitDefinition xml:lang="en">A display of data about a digital manifestation that includes a title proper and usually, though not necessarily, a statement of responsibility and data relating to publication.</rdakit:toolkitDefinition>
      <skos:prefLabel xml:lang="it">schermata del titolo</skos:prefLabel>
      <rdakit:toolkitLabel xml:lang="it">schermata del titolo</rdakit:toolkitLabel>
      <skos:definition xml:lang="it">Visualizzazione di dati su una risorsa digitale che include il titolo proprio e solitamente, benché non necessariamente, la formulazione di responsabilità e i dati sulla pubblicazione.</skos:definition>
      <rdakit:toolkitDefinition xml:lang="it">Visualizzazione di dati su una risorsa digitale che include il titolo proprio e solitamente, benché non necessariamente, la formulazione di responsabilità e i dati sulla pubblicazione.</rdakit:toolkitDefinition>
      <skos:prefLabel xml:lang="fr">écran-titre</skos:prefLabel>
      <rdakit:toolkitLabel xml:lang="fr">écran-titre</rdakit:toolkitLabel>
      <skos:definition xml:lang="fr">Affichage de données relatives à une manifestation numérique, comprenant un titre propre et ordinairement, mais pas nécessairement, une mention de responsabilité et des données relatives à la publication.</skos:definition>
      <rdakit:toolkitDefinition xml:lang="fr">Affichage de données relatives à une manifestation numérique, comprenant un titre propre et ordinairement, mais pas nécessairement, une mention de responsabilité et des données relatives à la publication.</rdakit:toolkitDefinition>
      <skos:prefLabel xml:lang="de">Titelbildschirm</skos:prefLabel>
      <rdakit:toolkitLabel xml:lang="de">Titelbildschirm</rdakit:toolkitLabel>
      <skos:definition xml:lang="de">Eine Darstellung von Daten über eine digitale Ressource, zu der der Haupttitel und meist, wenn auch nicht unbedingt, die Verantwortlichkeitsangabe und das Erscheinungsdatum gehören.</skos:definition>
      <rdakit:toolkitDefinition xml:lang="de">Eine Darstellung von Daten über eine digitale Ressource, zu der der Haupttitel und meist, wenn auch nicht unbedingt, die Verantwortlichkeitsangabe und das Erscheinungsdatum gehören.</rdakit:toolkitDefinition>
      <skos:prefLabel xml:lang="fi">nimiönäyttö</skos:prefLabel>
      <rdakit:toolkitLabel xml:lang="fi">nimiönäyttö</rdakit:toolkitLabel>
      <skos:definition xml:lang="fi">Digitaalisia aineistoja käsittävä tietonäyttö, joka sisältää nimekkeen, usein vastuullisuustietoja sekä muuta julkaisuun liittyvää informaatiota.</skos:definition>
      <rdakit:toolkitDefinition xml:lang="fi">Digitaalisia aineistoja käsittävä tietonäyttö, joka sisältää nimekkeen, usein vastuullisuustietoja sekä muuta julkaisuun liittyvää informaatiota.</rdakit:toolkitDefinition>
      <skos:prefLabel xml:lang="da">titelskærmbillede</skos:prefLabel>
      <rdakit:toolkitLabel xml:lang="da">titelskærmbillede</rdakit:toolkitLabel>
      <skos:definition xml:lang="da">Fremvisning af oplysninger om en digital ressource, der indeholder hovedtitlen og normalt, men ikke nødvendigvis, ophavsangivelse samt oplysninger relateret til publicering.</skos:definition>
      <rdakit:toolkitDefinition xml:lang="da">Fremvisning af oplysninger om en digital ressource, der indeholder hovedtitlen og normalt, men ikke nødvendigvis, ophavsangivelse samt oplysninger relateret til publicering.</rdakit:toolkitDefinition>
      <skos:prefLabel xml:lang="ca">pantalla de títol</skos:prefLabel>
      <rdakit:toolkitLabel xml:lang="ca">pantalla de títol</rdakit:toolkitLabel>
      <skos:definition xml:lang="ca">Visualització de dades sobre una manifestació digital que inclou un títol propi i normalment, tot i que no necessàriament, una menció de responsabilitat i les dades relatives a la publicació.</skos:definition>
      <rdakit:toolkitDefinition xml:lang="ca">Visualització de dades sobre una manifestació digital que inclou un títol propi i normalment, tot i que no necessàriament, una menció de responsabilitat i les dades relatives a la publicació.</rdakit:toolkitDefinition>
      <skos:prefLabel xml:lang="vi">màn ảnh nhan đề</skos:prefLabel>
      <rdakit:toolkitLabel xml:lang="vi">màn ảnh nhan đề</rdakit:toolkitLabel>
      <skos:definition xml:lang="vi">Hiển thị của dữ liệu về biểu thị số bao gồm nhan đề hợp thức và thường, mặc dù không nhất thiết, thông tin trách nhiệm và dữ liệu liên quan tới xuất bản.</skos:definition>
      <rdakit:toolkitDefinition xml:lang="vi">Hiển thị của dữ liệu về biểu thị số bao gồm nhan đề hợp thức và thường, mặc dù không nhất thiết, thông tin trách nhiệm và dữ liệu liên quan tới xuất bản.</rdakit:toolkitDefinition>
      <skos:prefLabel xml:lang="no">tittelskjermbilde</skos:prefLabel>
      <rdakit:toolkitLabel xml:lang="no">tittelskjermbilde</rdakit:toolkitLabel>
      <skos:definition xml:lang="no">En visning av data om en digital manifestasjon som omfatter hovedtittelen og som oftest, men ikke nødvendigvis, ansvarsangivelsen og opplysninger knyttet til utgivelse.</skos:definition>
      <rdakit:toolkitDefinition xml:lang="no">En visning av data om en digital manifestasjon som omfatter hovedtittelen og som oftest, men ikke nødvendigvis, ansvarsangivelsen og opplysninger knyttet til utgivelse.</rdakit:toolkitDefinition>
    </skos:Concept>
<!-- Concept: treaty  -->
    <skos:Concept rdf:about="http://rdaregistry.info/termList/RDATerms/1097" xml:lang="en">
      <skos:inScheme rdf:resource="http://rdaregistry.info/termList/RDATerms"/>
      <reg:status rdf:resource="http://metadataregistry.org/uri/RegStatus/1001"/>
      <reg:identifier rdf:resource="http://metadataregistry.org/concepts/8612"/>
      <skos:prefLabel xml:lang="en">treaty</skos:prefLabel>
      <rdakit:toolkitLabel xml:lang="en">treaty</rdakit:toolkitLabel>
      <skos:definition xml:lang="en">An international agreement concluded between states or international organizations in written form and governed by international law.</skos:definition>
      <rdakit:toolkitDefinition xml:lang="en">An international agreement concluded between states or international organizations in written form and governed by international law.</rdakit:toolkitDefinition>
      <skos:scopeNote xml:lang="en">A treaty may be designated by various other terms such as agreement, concordat, convention, charter, declaration, exchange of notes, memorandum of understanding, modus vivendi, or protocol.</skos:scopeNote>
      <skos:prefLabel xml:lang="it">trattato</skos:prefLabel>
      <rdakit:toolkitLabel xml:lang="it">trattato</rdakit:toolkitLabel>
      <skos:definition xml:lang="it">Accordo interazionale concluso tra stati od organizzazioni internazionali in forma scritta e governato dal diritto internazionale.</skos:definition>
      <rdakit:toolkitDefinition xml:lang="it">Accordo interazionale concluso tra stati od organizzazioni internazionali in forma scritta e governato dal diritto internazionale.</rdakit:toolkitDefinition>
      <skos:scopeNote xml:lang="it">Può essere designato da vari altri termini, come accordo, concordato, convenzione, statuto, dichiarazione, scambio di note, protocollo di intesa, modus vivendi, o protocollo.</skos:scopeNote>
      <skos:prefLabel xml:lang="fr">traité</skos:prefLabel>
      <rdakit:toolkitLabel xml:lang="fr">traité</rdakit:toolkitLabel>
      <skos:definition xml:lang="fr">Entente internationale sous forme écrite conclue entre des États ou des organisations internationales et régie par le droit international.</skos:definition>
      <rdakit:toolkitDefinition xml:lang="fr">Entente internationale sous forme écrite conclue entre des États ou des organisations internationales et régie par le droit international.</rdakit:toolkitDefinition>
      <skos:scopeNote xml:lang="fr">Un traité peut être désigné par une variété d’autres termes tels que accord, concordat, convention, charte, déclaration, échange de notes, entente, modus vivendi ou protocole.</skos:scopeNote>
      <skos:prefLabel xml:lang="de">Abkommen</skos:prefLabel>
      <rdakit:toolkitLabel xml:lang="de">Abkommen</rdakit:toolkitLabel>
      <skos:definition xml:lang="de">Eine internationale Vereinbarung, die zwischen Staaten oder internationalen Organisationen in schriftlicher Form, geregelt durch internationales Recht, abgeschlossen wurde.</skos:definition>
      <rdakit:toolkitDefinition xml:lang="de">Eine internationale Vereinbarung, die zwischen Staaten oder internationalen Organisationen in schriftlicher Form, geregelt durch internationales Recht, abgeschlossen wurde.</rdakit:toolkitDefinition>
      <skos:scopeNote xml:lang="de">Ein Abkommen kann mit verschiedenen anderen Termini wie zum Beispiel Vereinbarung, Konkordat, Konvention, Charta, Deklaration, Notenwechsel, Memorandum, Verfahrensweisen oder Protokoll bezeichnet werden.</skos:scopeNote>
      <skos:prefLabel xml:lang="fi">valtiosopimus</skos:prefLabel>
      <rdakit:toolkitLabel xml:lang="fi">valtiosopimus</rdakit:toolkitLabel>
      <skos:definition xml:lang="fi">Kansainvälinen valtioiden tai kansainvälisten järjestöjen välinen kirjallinen sopimus joka noudattaa kansainvälistä lakia.</skos:definition>
      <rdakit:toolkitDefinition xml:lang="fi">Kansainvälinen valtioiden tai kansainvälisten järjestöjen välinen kirjallinen sopimus joka noudattaa kansainvälistä lakia.</rdakit:toolkitDefinition>
      <skos:scopeNote xml:lang="fi">Valtiosopimukseen voidaan viitata muilla termeillä kuten sopimus, konkordaatti, yleissopimus, perustamissopimus, julistus, noottienvaihto, aiepöytäkirja, toistaiseksi sovittu järjestely, tai pöytäkirja.</skos:scopeNote>
      <skos:prefLabel xml:lang="da">traktat</skos:prefLabel>
      <rdakit:toolkitLabel xml:lang="da">traktat</rdakit:toolkitLabel>
      <skos:definition xml:lang="da">International aftale indgået mellem stater eller internationale organisationer i skreven form og underlagt international ret.</skos:definition>
      <rdakit:toolkitDefinition xml:lang="da">International aftale indgået mellem stater eller internationale organisationer i skreven form og underlagt international ret.</rdakit:toolkitDefinition>
      <skos:scopeNote xml:lang="da">En traktat kan benævnes med andre termer såsom aftale, konkordat, charter, konvention, deklaration, noteudveksling, hensigtserklæring, modus vivendi eller protokol.</skos:scopeNote>
      <skos:prefLabel xml:lang="ca">tractat</skos:prefLabel>
      <rdakit:toolkitLabel xml:lang="ca">tractat</rdakit:toolkitLabel>
      <skos:definition xml:lang="ca">Acord internacional signat entre estats o organitzacions internacionals en forma escrita i regit per la legislació internacional.</skos:definition>
      <rdakit:toolkitDefinition xml:lang="ca">Acord internacional signat entre estats o organitzacions internacionals en forma escrita i regit per la legislació internacional.</rdakit:toolkitDefinition>
      <skos:scopeNote xml:lang="ca">Un tractat es pot designar amb altres termes, com ara acord, concordat, convenció, estatut, declaració, modus vivendi o protocol.</skos:scopeNote>
      <skos:prefLabel xml:lang="vi">hiệp ước</skos:prefLabel>
      <rdakit:toolkitLabel xml:lang="vi">hiệp ước</rdakit:toolkitLabel>
      <skos:definition xml:lang="vi">Thoả thuận quốc tế được ký kết giữa các nhà nước hoặc tổ chức quốc tế bằng hình thái văn bản và quản lý bởi luật quốc tế.</skos:definition>
      <rdakit:toolkitDefinition xml:lang="vi">Thoả thuận quốc tế được ký kết giữa các nhà nước hoặc tổ chức quốc tế bằng hình thái văn bản và quản lý bởi luật quốc tế.</rdakit:toolkitDefinition>
      <skos:scopeNote xml:lang="vi">Hiệp ước có thể được định danh bởi các thuật ngữ khác như thoả thuận, giao ước, hiệp định, hiến chương, tuyên bố, công hàn, ghi nhớ, tạm ước, hoặc nghị định thư.</skos:scopeNote>
      <skos:prefLabel xml:lang="no">traktat</skos:prefLabel>
      <rdakit:toolkitLabel xml:lang="no">traktat</rdakit:toolkitLabel>
      <skos:definition xml:lang="no">En skriftlig, internasjonal avtale mellom stater eller internasjonale organisasjoner underlagt folkeretten.</skos:definition>
      <rdakit:toolkitDefinition xml:lang="no">En skriftlig, internasjonal avtale mellom stater eller internasjonale organisasjoner underlagt folkeretten.</rdakit:toolkitDefinition>
      <skos:scopeNote xml:lang="no">En traktat kan beskrives med andre termer som avtale, overenskomst, konvensjon, sjarter, kunngjøring, memorandum, foreløpig ordning eller protokoll.</skos:scopeNote>
    </skos:Concept>
<!-- Concept: type of composition  -->
    <skos:Concept rdf:about="http://rdaregistry.info/termList/RDATerms/1098" xml:lang="en">
      <skos:inScheme rdf:resource="http://rdaregistry.info/termList/RDATerms"/>
      <reg:status rdf:resource="http://metadataregistry.org/uri/RegStatus/1001"/>
      <reg:identifier rdf:resource="http://metadataregistry.org/concepts/8613"/>
      <skos:prefLabel xml:lang="en">type of composition</skos:prefLabel>
      <rdakit:toolkitLabel xml:lang="en">type of composition</rdakit:toolkitLabel>
      <skos:definition xml:lang="en">A form or genre or a generic term used frequently by different composers.</skos:definition>
      <rdakit:toolkitDefinition xml:lang="en">A form or genre or a generic term used frequently by different composers.</rdakit:toolkitDefinition>
      <skos:scopeNote xml:lang="en">Form or genre includes capriccio, chamber music, concerto, Magnificat, motion picture music, nocturne, opera, sacred music, suite, trio sonata. Generic term includes composition, movement, muziek, piece.</skos:scopeNote>
      <skos:prefLabel xml:lang="it">tipo di composizione</skos:prefLabel>
      <rdakit:toolkitLabel xml:lang="it">tipo di composizione</rdakit:toolkitLabel>
      <skos:definition xml:lang="it">Forma o genere (per esempio, capriccio, musica da camera, concerto, Magnificat, musica da film, notturno, opera musicale, musica sacra, suite, sonata a tre) o termine generico (per esempio, composizione, movimento, muziek, pezzo) utilizzati frequentemente da diversi compositori.</skos:definition>
      <rdakit:toolkitDefinition xml:lang="it">Forma o genere (per esempio, capriccio, musica da camera, concerto, Magnificat, musica da film, notturno, opera musicale, musica sacra, suite, sonata a tre) o termine generico (per esempio, composizione, movimento, muziek, pezzo) utilizzati frequentemente da diversi compositori.</rdakit:toolkitDefinition>
      <skos:prefLabel xml:lang="fr">type de composition</skos:prefLabel>
      <rdakit:toolkitLabel xml:lang="fr">type de composition</rdakit:toolkitLabel>
      <skos:definition xml:lang="fr">Forme ou genre, ou terme générique utilisé fréquemment par différents compositeurs.</skos:definition>
      <rdakit:toolkitDefinition xml:lang="fr">Forme ou genre, ou terme générique utilisé fréquemment par différents compositeurs.</rdakit:toolkitDefinition>
      <skos:prefLabel xml:lang="de">Kompositionsart</skos:prefLabel>
      <rdakit:toolkitLabel xml:lang="de">Kompositionsart</rdakit:toolkitLabel>
      <skos:definition xml:lang="de">Eine Form, ein Genre oder ein Gattungsbegriff, der häufig von verschiedenen Komponisten verwendet wird.</skos:definition>
      <rdakit:toolkitDefinition xml:lang="de">Eine Form, ein Genre oder ein Gattungsbegriff, der häufig von verschiedenen Komponisten verwendet wird.</rdakit:toolkitDefinition>
      <skos:scopeNote xml:lang="de">Zur Form oder zum Genre gehören Capriccio, Kammermusik, Konzert, Magnificat, Filmmusik, Nocturne, Oper, Kirchenmusik, Suite, Triosonate. Zum Gattungsbegriff gehört Komposition, Satz, Musik, Stück.</skos:scopeNote>
      <skos:prefLabel xml:lang="fi">sävellystyyppi</skos:prefLabel>
      <rdakit:toolkitLabel xml:lang="fi">sävellystyyppi</rdakit:toolkitLabel>
      <skos:definition xml:lang="fi">Muoto tai laji tai eri säveltäjien yleisesti käyttämä yleistermi.</skos:definition>
      <rdakit:toolkitDefinition xml:lang="fi">Muoto tai laji tai eri säveltäjien yleisesti käyttämä yleistermi.</rdakit:toolkitDefinition>
      <skos:scopeNote xml:lang="fi">Muoto tai laji esim. capriccio, kamarimusiikki, konsertto, Magnificat, elokuvamusiikki, nokturni, ooppera, hengellinen musiikki, sarja, triosonaatti.  Yleistermiin sisältyvät sävellys, osa, muziek, kappale.</skos:scopeNote>
      <skos:prefLabel xml:lang="da">kompositionstype</skos:prefLabel>
      <rdakit:toolkitLabel xml:lang="da">kompositionstype</rdakit:toolkitLabel>
      <skos:definition xml:lang="da">Form eller genre eller generisk term, der hyppigt anvendes af forskellige komponister.</skos:definition>
      <rdakit:toolkitDefinition xml:lang="da">Form eller genre eller generisk term, der hyppigt anvendes af forskellige komponister.</rdakit:toolkitDefinition>
      <skos:scopeNote xml:lang="da">Form eller genre omfatter capriccio, kammermusik, koncert, magnificat, spillefilmsmusik, nocturne, opera, kirkemusik, suite, triosonate. Generisk term omfatter kompostition, sats, stykke.</skos:scopeNote>
      <skos:prefLabel xml:lang="ca">gènere de composició musical</skos:prefLabel>
      <rdakit:toolkitLabel xml:lang="ca">gènere de composició musical</rdakit:toolkitLabel>
      <skos:definition xml:lang="ca">Forma o gènere o un terme genèric usat sovint per diferents compositors.</skos:definition>
      <rdakit:toolkitDefinition xml:lang="ca">Forma o gènere o un terme genèric usat sovint per diferents compositors.</rdakit:toolkitDefinition>
      <skos:scopeNote xml:lang="ca">Forma o gènere inclou capriccio, música de cambra, concerto, Magnificat, música de pel·lícula cinematogràfica, nocturn, òpera, música sacra, suite, sonates en trio. Terme genèric inclou composició, moviment, muziek, piece.</skos:scopeNote>
      <skos:scopeNote xml:lang="fr">Des exemples de formes ou de genres comprennent : capriccio, musique de chambre, concerto, Magnificat, musique de film, nocturne, opéra, musique sacrée, suite, sonate en trio. Des exemples de termes génériques comprennent : composition, mouvement, muziek, pièce.</skos:scopeNote>
      <skos:prefLabel xml:lang="vi">loại sáng tác</skos:prefLabel>
      <rdakit:toolkitLabel xml:lang="vi">loại sáng tác</rdakit:toolkitLabel>
      <skos:definition xml:lang="vi">Hình thái, thể loại, hoặc thuật ngữ chỉ loại được dùng thường xuyên của các nhà sáng tác khác nhau.</skos:definition>
      <rdakit:toolkitDefinition xml:lang="vi">Hình thái, thể loại, hoặc thuật ngữ chỉ loại được dùng thường xuyên của các nhà sáng tác khác nhau.</rdakit:toolkitDefinition>
      <skos:scopeNote xml:lang="vi">Hình thái của thể loại bao gồm capriccio, concerto, intermezzo, Magnificat, mass, movement, muziek, nocturne, requiem, Stuck, symphony, suite, Te Deum, trio sonata. Thuật ngữ thể loại bao gồm loại sáng tác, động thái, muziek, bản nhạc.</skos:scopeNote>
      <skos:prefLabel xml:lang="no">komposisjonstype</skos:prefLabel>
      <rdakit:toolkitLabel xml:lang="no">komposisjonstype</rdakit:toolkitLabel>
      <skos:definition xml:lang="no">En form eller en sjanger eller et generelt begrep som ofte brukes av ulike komponister.</skos:definition>
      <rdakit:toolkitDefinition xml:lang="no">En form eller en sjanger eller et generelt begrep som ofte brukes av ulike komponister.</rdakit:toolkitDefinition>
      <skos:scopeNote xml:lang="no">Sjanger eller form inkluderer capriccioer, konserter, intermesso, magnificat, messer, nokturne, rekviem, symfonier, suiter, Te Deum, trisonater. Generelle begreper inkluderer komposisjon, sats, muziek, stykke.</skos:scopeNote>
    </skos:Concept>
<!-- Concept: unit  -->
    <skos:Concept rdf:about="http://rdaregistry.info/termList/RDATerms/1099" xml:lang="en">
      <skos:inScheme rdf:resource="http://rdaregistry.info/termList/RDATerms"/>
      <reg:status rdf:resource="http://metadataregistry.org/uri/RegStatus/1001"/>
      <reg:identifier rdf:resource="http://metadataregistry.org/concepts/8614"/>
      <skos:prefLabel xml:lang="en">unit</skos:prefLabel>
      <rdakit:toolkitLabel xml:lang="en">unit</rdakit:toolkitLabel>
      <skos:definition xml:lang="en">A physical or logical constituent of a manifestation.</skos:definition>
      <rdakit:toolkitDefinition xml:lang="en">A physical or logical constituent of a manifestation.</rdakit:toolkitDefinition>
      <skos:scopeNote xml:lang="en">A unit includes a volume, audiocassette, film reel, a map, a digital file, etc.</skos:scopeNote>
      <skos:prefLabel xml:lang="it">unità</skos:prefLabel>
      <rdakit:toolkitLabel xml:lang="it">unità</rdakit:toolkitLabel>
      <skos:definition xml:lang="it">Componente fisica o logica di una risorsa.</skos:definition>
      <rdakit:toolkitDefinition xml:lang="it">Componente fisica o logica di una risorsa.</rdakit:toolkitDefinition>
      <skos:prefLabel xml:lang="fr">unité</skos:prefLabel>
      <rdakit:toolkitLabel xml:lang="fr">unité</rdakit:toolkitLabel>
      <skos:definition xml:lang="fr">Composant physique ou logique d’une manifestation.</skos:definition>
      <rdakit:toolkitDefinition xml:lang="fr">Composant physique ou logique d’une manifestation.</rdakit:toolkitDefinition>
      <skos:prefLabel xml:lang="es">unidad</skos:prefLabel>
      <rdakit:toolkitLabel xml:lang="es">unidad</rdakit:toolkitLabel>
      <skos:definition xml:lang="es">Un componente físico o lógico de un recurso.</skos:definition>
      <rdakit:toolkitDefinition xml:lang="es">Un componente físico o lógico de un recurso.</rdakit:toolkitDefinition>
      <skos:prefLabel xml:lang="de">Einheit</skos:prefLabel>
      <rdakit:toolkitLabel xml:lang="de">Einheit</rdakit:toolkitLabel>
      <skos:definition xml:lang="de">Ein physischer oder logischer Bestandteil einer Manifestation.</skos:definition>
      <rdakit:toolkitDefinition xml:lang="de">Ein physischer oder logischer Bestandteil einer Manifestation.</rdakit:toolkitDefinition>
      <skos:scopeNote xml:lang="de">Dazu gehören ein Band, eine Audiokassette, eine Filmspule, eine Karte, eine digitale Datei usw.</skos:scopeNote>
      <skos:prefLabel xml:lang="fi">yksikkö</skos:prefLabel>
      <rdakit:toolkitLabel xml:lang="fi">yksikkö</rdakit:toolkitLabel>
      <skos:definition xml:lang="fi">Manifestaation fyysinen tai looginen rakenneosa.</skos:definition>
      <rdakit:toolkitDefinition xml:lang="fi">Manifestaation fyysinen tai looginen rakenneosa.</rdakit:toolkitDefinition>
      <skos:scopeNote xml:lang="fi">Yksikkö voi olla esim. nide, äänikasetti, filmikela, kartta, tiedosto jne.</skos:scopeNote>
      <skos:prefLabel xml:lang="da">enhed</skos:prefLabel>
      <rdakit:toolkitLabel xml:lang="da">enhed</rdakit:toolkitLabel>
      <skos:definition xml:lang="da">Fysisk eller logisk bestanddel af en manifestation.</skos:definition>
      <rdakit:toolkitDefinition xml:lang="da">Fysisk eller logisk bestanddel af en manifestation.</rdakit:toolkitDefinition>
      <skos:scopeNote xml:lang="da">En enhed omfatter et bind, et kassettebånd, en filmspole, et kort, en digital fil.</skos:scopeNote>
      <skos:prefLabel xml:lang="ca">unitat</skos:prefLabel>
      <rdakit:toolkitLabel xml:lang="ca">unitat</rdakit:toolkitLabel>
      <skos:definition xml:lang="ca">Component físic o lògic d’una manifestació.</skos:definition>
      <rdakit:toolkitDefinition xml:lang="ca">Component físic o lògic d’una manifestació.</rdakit:toolkitDefinition>
      <skos:scopeNote xml:lang="ca">Una unitat inclou un volum, una casset àudio, una bobina de pel·lícula, un mapa, un fitxer digital, etc.</skos:scopeNote>
      <skos:scopeNote xml:lang="fr">Comprend un volume, une cassette audio, une bobine de film, une carte, un fichier numérique, etc.</skos:scopeNote>
      <skos:prefLabel xml:lang="vi">đơn vị</skos:prefLabel>
      <rdakit:toolkitLabel xml:lang="vi">đơn vị</rdakit:toolkitLabel>
      <skos:definition xml:lang="vi">Một thành phần vật lý hoặc logic của một biểu thị.</skos:definition>
      <rdakit:toolkitDefinition xml:lang="vi">Một thành phần vật lý hoặc logic của một biểu thị.</rdakit:toolkitDefinition>
      <skos:scopeNote xml:lang="vi">Đơn vị bao gồm một tập, audiocaset, cuộn phim, một bản đồ, một tệp số, v.v...</skos:scopeNote>
      <skos:prefLabel xml:lang="no">enhet</skos:prefLabel>
      <rdakit:toolkitLabel xml:lang="no">enhet</rdakit:toolkitLabel>
      <skos:definition xml:lang="no">En fysisk eller logisk bestanddel av en manifestasjon.</skos:definition>
      <rdakit:toolkitDefinition xml:lang="no">En fysisk eller logisk bestanddel av en manifestasjon.</rdakit:toolkitDefinition>
      <skos:scopeNote xml:lang="no">En enhet kan være et bind, en lydkassett, en filmrull, et kart, en digital fil, etc.</skos:scopeNote>
    </skos:Concept>
<!-- Concept: unstructured description  -->
    <skos:Concept rdf:about="http://rdaregistry.info/termList/RDATerms/1100" xml:lang="en">
      <skos:inScheme rdf:resource="http://rdaregistry.info/termList/RDATerms"/>
      <reg:status rdf:resource="http://metadataregistry.org/uri/RegStatus/1001"/>
      <reg:identifier rdf:resource="http://metadataregistry.org/concepts/8615"/>
      <skos:prefLabel xml:lang="en">unstructured description</skos:prefLabel>
      <rdakit:toolkitLabel xml:lang="en">unstructured description</rdakit:toolkitLabel>
      <skos:definition xml:lang="en">A full or partial description of an entity written as a phrase, sentence, paragraph, etc.</skos:definition>
      <rdakit:toolkitDefinition xml:lang="en">A full or partial description of an entity written as a phrase, sentence, paragraph, etc.</rdakit:toolkitDefinition>
      <skos:prefLabel xml:lang="it">descrizione non strutturata</skos:prefLabel>
      <rdakit:toolkitLabel xml:lang="it">descrizione non strutturata</rdakit:toolkitLabel>
      <skos:definition xml:lang="it">Descrizione comprensiva o parziale di una risorsa, redatta in forma di frase, paragrafo, etc.</skos:definition>
      <rdakit:toolkitDefinition xml:lang="it">Descrizione comprensiva o parziale di una risorsa, redatta in forma di frase, paragrafo, etc.</rdakit:toolkitDefinition>
      <skos:prefLabel xml:lang="fr">description non structurée</skos:prefLabel>
      <rdakit:toolkitLabel xml:lang="fr">description non structurée</rdakit:toolkitLabel>
      <skos:definition xml:lang="fr">Description complète ou partielle d’une entité rédigée sous la forme d’une expresion, d’une phrase, d’un paragraphe, etc.</skos:definition>
      <rdakit:toolkitDefinition xml:lang="fr">Description complète ou partielle d’une entité rédigée sous la forme d’une expresion, d’une phrase, d’un paragraphe, etc.</rdakit:toolkitDefinition>
      <skos:prefLabel xml:lang="es">descripción no estructurada</skos:prefLabel>
      <rdakit:toolkitLabel xml:lang="es">descripción no estructurada</rdakit:toolkitLabel>
      <skos:definition xml:lang="es">Descripción total o parcial de un recurso escrito ccomo una frase, parágrafo, etc.</skos:definition>
      <rdakit:toolkitDefinition xml:lang="es">Descripción total o parcial de un recurso escrito ccomo una frase, parágrafo, etc.</rdakit:toolkitDefinition>
      <skos:prefLabel xml:lang="de">Unstrukturierte Beschreibung</skos:prefLabel>
      <rdakit:toolkitLabel xml:lang="de">Unstrukturierte Beschreibung</rdakit:toolkitLabel>
      <skos:definition xml:lang="de">Eine vollständige oder teilweise Beschreibung einer Entität, die in Form eines Satzes oder Absatzes usw. geschrieben wird.</skos:definition>
      <rdakit:toolkitDefinition xml:lang="de">Eine vollständige oder teilweise Beschreibung einer Entität, die in Form eines Satzes oder Absatzes usw. geschrieben wird.</rdakit:toolkitDefinition>
      <skos:prefLabel xml:lang="fi">vapaamuotoinen kuvailu</skos:prefLabel>
      <rdakit:toolkitLabel xml:lang="fi">vapaamuotoinen kuvailu</rdakit:toolkitLabel>
      <skos:definition xml:lang="fi">Aineiston täydellinen tai osittainen kuvailu kirjoitettuna lausekkeena, lauseena, kappaleena tms.</skos:definition>
      <rdakit:toolkitDefinition xml:lang="fi">Aineiston täydellinen tai osittainen kuvailu kirjoitettuna lausekkeena, lauseena, kappaleena tms.</rdakit:toolkitDefinition>
      <skos:prefLabel xml:lang="da">ikke-struktureret beskrivelse</skos:prefLabel>
      <rdakit:toolkitLabel xml:lang="da">ikke-struktureret beskrivelse</rdakit:toolkitLabel>
      <skos:definition xml:lang="da">Komplet eller delvis beskrivelse af en ressource skrevet som en sætning, et afsnit etc.</skos:definition>
      <rdakit:toolkitDefinition xml:lang="da">Komplet eller delvis beskrivelse af en ressource skrevet som en sætning, et afsnit etc.</rdakit:toolkitDefinition>
      <skos:prefLabel xml:lang="ca">descripció no estructurada</skos:prefLabel>
      <rdakit:toolkitLabel xml:lang="ca">descripció no estructurada</rdakit:toolkitLabel>
      <skos:definition xml:lang="ca">Descripció completa o parcial d’una entitat escrita com una frase, un paràgraf, etc.</skos:definition>
      <rdakit:toolkitDefinition xml:lang="ca">Descripció completa o parcial d’una entitat escrita com una frase, un paràgraf, etc.</rdakit:toolkitDefinition>
      <skos:prefLabel xml:lang="vi">mô tả không cấu trúc</skos:prefLabel>
      <rdakit:toolkitLabel xml:lang="vi">mô tả không cấu trúc</rdakit:toolkitLabel>
      <skos:definition xml:lang="vi">Mô tả đầy đủ hoặc từng phần của một tài nguyên được viết dưới dạng câu hoặc đoạn, v.v...</skos:definition>
      <rdakit:toolkitDefinition xml:lang="vi">Mô tả đầy đủ hoặc từng phần của một tài nguyên được viết dưới dạng câu hoặc đoạn, v.v...</rdakit:toolkitDefinition>
      <skos:prefLabel xml:lang="no">ustrukturert beskrivelse</skos:prefLabel>
      <rdakit:toolkitLabel xml:lang="no">ustrukturert beskrivelse</rdakit:toolkitLabel>
      <skos:definition xml:lang="no">En fullstendig eller delvis beskrivelse av en entitet, skrevet som en frase, en setning eller et avsnitt.</skos:definition>
      <rdakit:toolkitDefinition xml:lang="no">En fullstendig eller delvis beskrivelse av en entitet, skrevet som en frase, en setning eller et avsnitt.</rdakit:toolkitDefinition>
    </skos:Concept>
<!-- Concept: updating loose-leaf  -->
    <skos:Concept rdf:about="http://rdaregistry.info/termList/RDATerms/1101" xml:lang="en">
      <skos:inScheme rdf:resource="http://rdaregistry.info/termList/RDATerms"/>
      <reg:status rdf:resource="http://metadataregistry.org/uri/RegStatus/1001"/>
      <reg:identifier rdf:resource="http://metadataregistry.org/concepts/8616"/>
      <skos:prefLabel xml:lang="en">updating loose-leaf</skos:prefLabel>
      <rdakit:toolkitLabel xml:lang="en">updating loose-leaf</rdakit:toolkitLabel>
      <skos:definition xml:lang="en">An integrating resource that consists of one or more base volumes updated by separate pages that are inserted, removed, and/or substituted.</skos:definition>
      <rdakit:toolkitDefinition xml:lang="en">An integrating resource that consists of one or more base volumes updated by separate pages that are inserted, removed, and/or substituted.</rdakit:toolkitDefinition>
      <skos:prefLabel xml:lang="it">aggiornamento a fogli mobili</skos:prefLabel>
      <rdakit:toolkitLabel xml:lang="it">aggiornamento a fogli mobili</rdakit:toolkitLabel>
      <skos:definition xml:lang="it">Risorsa integrativa costituita da uno o più volumi di base aggiornati mediante pagine fisicamente distinte inserite,rimosse e/o sostituite.</skos:definition>
      <rdakit:toolkitDefinition xml:lang="it">Risorsa integrativa costituita da uno o più volumi di base aggiornati mediante pagine fisicamente distinte inserite,rimosse e/o sostituite.</rdakit:toolkitDefinition>
      <skos:prefLabel xml:lang="de">Laufende Loseblattsammlung</skos:prefLabel>
      <rdakit:toolkitLabel xml:lang="de">Laufende Loseblattsammlung</rdakit:toolkitLabel>
      <skos:definition xml:lang="de">Eine integrierende Ressource, die aus einem oder mehreren Grundordnern besteht, die durch das Einfügen, Entfernen oder Ersetzen von einzelnen Seiten aktualisiert werden.</skos:definition>
      <rdakit:toolkitDefinition xml:lang="de">Eine integrierende Ressource, die aus einem oder mehreren Grundordnern besteht, die durch das Einfügen, Entfernen oder Ersetzen von einzelnen Seiten aktualisiert werden.</rdakit:toolkitDefinition>
      <skos:prefLabel xml:lang="fi">päivittyvät irtolehdet</skos:prefLabel>
      <rdakit:toolkitLabel xml:lang="fi">päivittyvät irtolehdet</rdakit:toolkitLabel>
      <skos:definition xml:lang="fi">Päivittyvä aineisto joka koostuu yhdestä tai useammasta niteestä, joita päivitetään lisäämällä, poistamalla ja/tai korvaamalla erillisiä sivuja.</skos:definition>
      <rdakit:toolkitDefinition xml:lang="fi">Päivittyvä aineisto joka koostuu yhdestä tai useammasta niteestä, joita päivitetään lisäämällä, poistamalla ja/tai korvaamalla erillisiä sivuja.</rdakit:toolkitDefinition>
      <skos:prefLabel xml:lang="da">opdaterende løsbladsværk</skos:prefLabel>
      <rdakit:toolkitLabel xml:lang="da">opdaterende løsbladsværk</rdakit:toolkitLabel>
      <skos:definition xml:lang="da">Integrerende ressource, der består af et eller flere basisbind, der opdateres med særskilte sider, der indsættes, fjernes og/eller erstattes.</skos:definition>
      <rdakit:toolkitDefinition xml:lang="da">Integrerende ressource, der består af et eller flere basisbind, der opdateres med særskilte sider, der indsættes, fjernes og/eller erstattes.</rdakit:toolkitDefinition>
      <skos:prefLabel xml:lang="ca">publicació en fulls actualitzables</skos:prefLabel>
      <rdakit:toolkitLabel xml:lang="ca">publicació en fulls actualitzables</rdakit:toolkitLabel>
      <skos:definition xml:lang="ca">Recurs integrant que consisteix en un o més volums bàsics que s’actualitzen a base de pàgines separades que s’insereixen i/o es retiren del volum i/o reemplacen pàgines existents.</skos:definition>
      <rdakit:toolkitDefinition xml:lang="ca">Recurs integrant que consisteix en un o més volums bàsics que s’actualitzen a base de pàgines separades que s’insereixen i/o es retiren del volum i/o reemplacen pàgines existents.</rdakit:toolkitDefinition>
      <skos:prefLabel xml:lang="fr">publication à feuillets mobiles à mise à jour</skos:prefLabel>
      <rdakit:toolkitLabel xml:lang="fr">publication à feuillets mobiles à mise à jour</rdakit:toolkitLabel>
      <skos:definition xml:lang="fr">Ressource intégratrice constituée d’un ou plusieurs volumes de base mis à jour par des pages distinctes qui sont insérées, retirées et/ou substituées.</skos:definition>
      <rdakit:toolkitDefinition xml:lang="fr">Ressource intégratrice constituée d’un ou plusieurs volumes de base mis à jour par des pages distinctes qui sont insérées, retirées et/ou substituées.</rdakit:toolkitDefinition>
      <skos:prefLabel xml:lang="vi">đóng tờ rời cập nhật</skos:prefLabel>
      <rdakit:toolkitLabel xml:lang="vi">đóng tờ rời cập nhật</rdakit:toolkitLabel>
      <skos:definition xml:lang="vi">Tài nguyên tích hợp bao gồm một hoặc nhiều tập lẻ được cập nhật bằng các trang riêng biệt chèn vào, bỏ đi và/hoặc thay thế</skos:definition>
      <rdakit:toolkitDefinition xml:lang="vi">Tài nguyên tích hợp bao gồm một hoặc nhiều tập lẻ được cập nhật bằng các trang riêng biệt chèn vào, bỏ đi và/hoặc thay thế</rdakit:toolkitDefinition>
      <skos:prefLabel xml:lang="no">oppdaterende løsbladpublikasjon</skos:prefLabel>
      <rdakit:toolkitLabel xml:lang="no">oppdaterende løsbladpublikasjon</rdakit:toolkitLabel>
      <skos:definition xml:lang="no">En integrerende ressurs som består av ett eller flere basisbind som oppdateres ved at enkeltsider settes inn, fjernes og/eller erstattes.</skos:definition>
      <rdakit:toolkitDefinition xml:lang="no">En integrerende ressurs som består av ett eller flere basisbind som oppdateres ved at enkeltsider settes inn, fjernes og/eller erstattes.</rdakit:toolkitDefinition>
    </skos:Concept>
<!-- Concept: variant access point  -->
    <skos:Concept rdf:about="http://rdaregistry.info/termList/RDATerms/1102" xml:lang="en">
      <skos:inScheme rdf:resource="http://rdaregistry.info/termList/RDATerms"/>
      <reg:status rdf:resource="http://metadataregistry.org/uri/RegStatus/1001"/>
      <reg:identifier rdf:resource="http://metadataregistry.org/concepts/8617"/>
      <skos:prefLabel xml:lang="en">variant access point</skos:prefLabel>
      <rdakit:toolkitLabel xml:lang="en">variant access point</rdakit:toolkitLabel>
      <skos:definition xml:lang="en">An alternative to an authorized access point representing an entity.</skos:definition>
      <rdakit:toolkitDefinition xml:lang="en">An alternative to an authorized access point representing an entity.</rdakit:toolkitDefinition>
	    <skos:broader rdf:resource="http://rdaregistry.info/termList/RDATerms/1001"/>
      <skos:prefLabel xml:lang="it">punto d'accesso variante</skos:prefLabel>
      <rdakit:toolkitLabel xml:lang="it">punto d'accesso variante</rdakit:toolkitLabel>
      <skos:definition xml:lang="it">Alternativa al punto d'accesso autorizzato che rappresenta un'entità.</skos:definition>
      <rdakit:toolkitDefinition xml:lang="it">Alternativa al punto d'accesso autorizzato che rappresenta un'entità.</rdakit:toolkitDefinition>
      <skos:prefLabel xml:lang="fr">variante de point d’accès</skos:prefLabel>
      <rdakit:toolkitLabel xml:lang="fr">variante de point d’accès</rdakit:toolkitLabel>
      <skos:definition xml:lang="fr">Autre forme d’un point d’accès autorisé représentant une entité.</skos:definition>
      <rdakit:toolkitDefinition xml:lang="fr">Autre forme d’un point d’accès autorisé représentant une entité.</rdakit:toolkitDefinition>
      <skos:prefLabel xml:lang="es">punto de acceso variante</skos:prefLabel>
      <rdakit:toolkitLabel xml:lang="es">punto de acceso variante</rdakit:toolkitLabel>
      <skos:definition xml:lang="es">Alternativa al punto de acceso autorizado que representa una entidad.</skos:definition>
      <rdakit:toolkitDefinition xml:lang="es">Alternativa al punto de acceso autorizado que representa una entidad.</rdakit:toolkitDefinition>
      <skos:prefLabel xml:lang="de">Zusätzlicher Sucheinstieg</skos:prefLabel>
      <rdakit:toolkitLabel xml:lang="de">Zusätzlicher Sucheinstieg</rdakit:toolkitLabel>
      <skos:definition xml:lang="de">Eine Alternative zum normierten Sucheinstieg, der eine Entität repräsentiert.</skos:definition>
      <rdakit:toolkitDefinition xml:lang="de">Eine Alternative zum normierten Sucheinstieg, der eine Entität repräsentiert.</rdakit:toolkitDefinition>
      <skos:prefLabel xml:lang="fi">varianttihakutieto</skos:prefLabel>
      <rdakit:toolkitLabel xml:lang="fi">varianttihakutieto</rdakit:toolkitLabel>
      <skos:definition xml:lang="fi">Entiteetin auktorisoidusta hakutiedosta poikkeava muoto.</skos:definition>
      <rdakit:toolkitDefinition xml:lang="fi">Entiteetin auktorisoidusta hakutiedosta poikkeava muoto.</rdakit:toolkitDefinition>
      <skos:prefLabel xml:lang="da">variantsøgeindgang</skos:prefLabel>
      <rdakit:toolkitLabel xml:lang="da">variantsøgeindgang</rdakit:toolkitLabel>
      <skos:definition xml:lang="da">Alternativ til den autoriserede søgeindgang, der repræsenterer en entitet.</skos:definition>
      <rdakit:toolkitDefinition xml:lang="da">Alternativ til den autoriserede søgeindgang, der repræsenterer en entitet.</rdakit:toolkitDefinition>
      <skos:prefLabel xml:lang="ca">variant de punt d’accés</skos:prefLabel>
      <rdakit:toolkitLabel xml:lang="ca">variant de punt d’accés</rdakit:toolkitLabel>
      <skos:definition xml:lang="ca">Alternativa a un punt d’accés autoritzat que representa una entitat.</skos:definition>
      <rdakit:toolkitDefinition xml:lang="ca">Alternativa a un punt d’accés autoritzat que representa una entitat.</rdakit:toolkitDefinition>
      <skos:prefLabel xml:lang="vi">điểm truy cập khác</skos:prefLabel>
      <rdakit:toolkitLabel xml:lang="vi">điểm truy cập khác</rdakit:toolkitLabel>
      <skos:definition xml:lang="vi">Một lựa chọn cho điểm truy cập được phép thể hiện một tiêu đề.</skos:definition>
      <rdakit:toolkitDefinition xml:lang="vi">Một lựa chọn cho điểm truy cập được phép thể hiện một tiêu đề.</rdakit:toolkitDefinition>
      <skos:prefLabel xml:lang="no">alternativ søkeinngang</skos:prefLabel>
      <rdakit:toolkitLabel xml:lang="no">alternativ søkeinngang</rdakit:toolkitLabel>
      <skos:definition xml:lang="no">Et alternativ til en autorisert søkeinngang som representerer en entitet.</skos:definition>
      <rdakit:toolkitDefinition xml:lang="no">Et alternativ til en autorisert søkeinngang som representerer en entitet.</rdakit:toolkitDefinition>
    </skos:Concept>
<!-- Concept: variant name  -->
    <skos:Concept rdf:about="http://rdaregistry.info/termList/RDATerms/1103" xml:lang="en">
      <skos:inScheme rdf:resource="http://rdaregistry.info/termList/RDATerms"/>
      <reg:status rdf:resource="http://metadataregistry.org/uri/RegStatus/1001"/>
      <reg:identifier rdf:resource="http://metadataregistry.org/concepts/8618"/>
      <skos:prefLabel xml:lang="en">variant name</skos:prefLabel>
      <rdakit:toolkitLabel xml:lang="en">variant name</rdakit:toolkitLabel>
      <skos:definition xml:lang="en">A name or form of name by which an entity is known that differs from the name or form of name chosen as a preferred name for that entity.</skos:definition>
      <rdakit:toolkitDefinition xml:lang="en">A name or form of name by which an entity is known that differs from the name or form of name chosen as a preferred name for that entity.</rdakit:toolkitDefinition>
      <skos:prefLabel xml:lang="it">nome variante</skos:prefLabel>
      <rdakit:toolkitLabel xml:lang="it">nome variante</rdakit:toolkitLabel>
      <skos:definition xml:lang="it">Nome o forma del nome con cui un'entità è conosciuta, diverso dal nome o dalla forma del nome scelti come nome preferito per quella entità.</skos:definition>
      <rdakit:toolkitDefinition xml:lang="it">Nome o forma del nome con cui un'entità è conosciuta, diverso dal nome o dalla forma del nome scelti come nome preferito per quella entità.</rdakit:toolkitDefinition>
      <skos:prefLabel xml:lang="fr">variante de nom</skos:prefLabel>
      <rdakit:toolkitLabel xml:lang="fr">variante de nom</rdakit:toolkitLabel>
      <skos:definition xml:lang="fr">Nom ou forme de nom sous laquelle une entité est connue et qui diffère du nom ou de la forme de nom choisie comme nom privilégié pour cette entité.</skos:definition>
      <rdakit:toolkitDefinition xml:lang="fr">Nom ou forme de nom sous laquelle une entité est connue et qui diffère du nom ou de la forme de nom choisie comme nom privilégié pour cette entité.</rdakit:toolkitDefinition>
      <skos:prefLabel xml:lang="es">variante del nombre</skos:prefLabel>
      <rdakit:toolkitLabel xml:lang="es">variante del nombre</rdakit:toolkitLabel>
      <skos:definition xml:lang="es">Nombre o una forma de un nombre mediante el cual se conoce a una entidad que difiere del nombre o forma del nombre escogido como el nombre preferido para esa entidad.</skos:definition>
      <rdakit:toolkitDefinition xml:lang="es">Nombre o una forma de un nombre mediante el cual se conoce a una entidad que difiere del nombre o forma del nombre escogido como el nombre preferido para esa entidad.</rdakit:toolkitDefinition>
      <skos:prefLabel xml:lang="de">Abweichender Name</skos:prefLabel>
      <rdakit:toolkitLabel xml:lang="de">Abweichender Name</rdakit:toolkitLabel>
      <skos:definition xml:lang="de">Ein Name oder eine Namensform, unter dem/der eine Enität bekannt ist, der/die sich von dem Namen oder der Namensform unterscheidet, der/die als bevorzugter Name für diese Entität gewählt wurde.</skos:definition>
      <rdakit:toolkitDefinition xml:lang="de">Ein Name oder eine Namensform, unter dem/der eine Enität bekannt ist, der/die sich von dem Namen oder der Namensform unterscheidet, der/die als bevorzugter Name für diese Entität gewählt wurde.</rdakit:toolkitDefinition>
      <skos:prefLabel xml:lang="fi">varianttinimi</skos:prefLabel>
      <rdakit:toolkitLabel xml:lang="fi">varianttinimi</rdakit:toolkitLabel>
      <skos:definition xml:lang="fi">Nimi tai nimen muoto, jolla entiteetti tunnetaan, mutta joka eroaa entiteetin ensisijaisesta nimestä.</skos:definition>
      <rdakit:toolkitDefinition xml:lang="fi">Nimi tai nimen muoto, jolla entiteetti tunnetaan, mutta joka eroaa entiteetin ensisijaisesta nimestä.</rdakit:toolkitDefinition>
      <skos:prefLabel xml:lang="da">variantnavn</skos:prefLabel>
      <rdakit:toolkitLabel xml:lang="da">variantnavn</rdakit:toolkitLabel>
      <skos:definition xml:lang="da">Navn eller form af navn, hvorunder enentitet er kendt, og som adskiller sig fra det navn eller den form af navn, der er valgt som det foretrukne navn for denne entitet.</skos:definition>
      <rdakit:toolkitDefinition xml:lang="da">Navn eller form af navn, hvorunder enentitet er kendt, og som adskiller sig fra det navn eller den form af navn, der er valgt som det foretrukne navn for denne entitet.</rdakit:toolkitDefinition>
      <skos:prefLabel xml:lang="ca">variant de nom</skos:prefLabel>
      <rdakit:toolkitLabel xml:lang="ca">variant de nom</rdakit:toolkitLabel>
      <skos:definition xml:lang="ca">Nom o forma de nom pel qual es coneix una entitat i que difereix del nom o de la forma de nom triat com a nom preferit d’aquesta entitat.</skos:definition>
      <rdakit:toolkitDefinition xml:lang="ca">Nom o forma de nom pel qual es coneix una entitat i que difereix del nom o de la forma de nom triat com a nom preferit d’aquesta entitat.</rdakit:toolkitDefinition>
      <skos:prefLabel xml:lang="vi">tên khác</skos:prefLabel>
      <rdakit:toolkitLabel xml:lang="vi">tên khác</rdakit:toolkitLabel>
      <skos:definition xml:lang="vi">Tên hoặc hình thái của tên mà theo đó một tiêu đề được biết tới nhưng khác với tên hoặc hình thái của tên được chọn là tên ưu tiên cho tiêu đề đó.</skos:definition>
      <rdakit:toolkitDefinition xml:lang="vi">Tên hoặc hình thái của tên mà theo đó một tiêu đề được biết tới nhưng khác với tên hoặc hình thái của tên được chọn là tên ưu tiên cho tiêu đề đó.</rdakit:toolkitDefinition>
      <skos:prefLabel xml:lang="no">variantform av navn</skos:prefLabel>
      <rdakit:toolkitLabel xml:lang="no">variantform av navn</rdakit:toolkitLabel>
      <skos:definition xml:lang="no">Et navn eller en navneform som en entitet er kjent under og som avviker fra navnet eller navneformen som er valgt som det foretrukne navnet.</skos:definition>
      <rdakit:toolkitDefinition xml:lang="no">Et navn eller en navneform som en entitet er kjent under og som avviker fra navnet eller navneformen som er valgt som det foretrukne navnet.</rdakit:toolkitDefinition>
    </skos:Concept>
<!-- Concept: video tape  -->
    <skos:Concept rdf:about="http://rdaregistry.info/termList/RDATerms/1104" xml:lang="en">
      <skos:inScheme rdf:resource="http://rdaregistry.info/termList/RDATerms"/>
      <reg:status rdf:resource="http://metadataregistry.org/uri/RegStatus/1001"/>
      <reg:identifier rdf:resource="http://metadataregistry.org/concepts/8619"/>
      <skos:prefLabel xml:lang="en">video tape</skos:prefLabel>
      <rdakit:toolkitLabel xml:lang="en">video tape</rdakit:toolkitLabel>
      <skos:definition xml:lang="en">A length of magnetic tape on which are recorded electrical signals that can be converted to images using video playback equipment.</skos:definition>
      <rdakit:toolkitDefinition xml:lang="en">A length of magnetic tape on which are recorded electrical signals that can be converted to images using video playback equipment.</rdakit:toolkitDefinition>
      <skos:prefLabel xml:lang="fr">bande vidéo</skos:prefLabel>
      <rdakit:toolkitLabel xml:lang="fr">bande vidéo</rdakit:toolkitLabel>
      <skos:definition xml:lang="fr">Métrage de bande magnétique sur laquelle sont enregistrés des signaux électriques qui peuvent être convertis en images à l’aide d’un appareil de lecture vidéo.</skos:definition>
      <rdakit:toolkitDefinition xml:lang="fr">Métrage de bande magnétique sur laquelle sont enregistrés des signaux électriques qui peuvent être convertis en images à l’aide d’un appareil de lecture vidéo.</rdakit:toolkitDefinition>
      <skos:prefLabel xml:lang="de">Videoband</skos:prefLabel>
      <rdakit:toolkitLabel xml:lang="de">Videoband</rdakit:toolkitLabel>
      <skos:definition xml:lang="de">Ein magnetisches Band, auf dem elektrische Signale aufgezeichnet sind, die mit Videowiedergabegeräten in Bilder umgewandelt werden können.</skos:definition>
      <rdakit:toolkitDefinition xml:lang="de">Ein magnetisches Band, auf dem elektrische Signale aufgezeichnet sind, die mit Videowiedergabegeräten in Bilder umgewandelt werden können.</rdakit:toolkitDefinition>
      <skos:prefLabel xml:lang="fi">videonauha</skos:prefLabel>
      <rdakit:toolkitLabel xml:lang="fi">videonauha</rdakit:toolkitLabel>
      <skos:definition xml:lang="fi">Magneettinauha, jolla on tallennettuna elektronisia signaaleja. Signaalit voidaan muuntaa kuviksi videoiden toistolaitteella.</skos:definition>
      <rdakit:toolkitDefinition xml:lang="fi">Magneettinauha, jolla on tallennettuna elektronisia signaaleja. Signaalit voidaan muuntaa kuviksi videoiden toistolaitteella.</rdakit:toolkitDefinition>
      <skos:prefLabel xml:lang="da">videobånd</skos:prefLabel>
      <rdakit:toolkitLabel xml:lang="da">videobånd</rdakit:toolkitLabel>
      <skos:definition xml:lang="da">Et stykke magnetbånd, hvorpå elektriske signaler er optaget, der kan omdannes til billeder vha. videoafspilningsudstyr.</skos:definition>
      <rdakit:toolkitDefinition xml:lang="da">Et stykke magnetbånd, hvorpå elektriske signaler er optaget, der kan omdannes til billeder vha. videoafspilningsudstyr.</rdakit:toolkitDefinition>
      <skos:prefLabel xml:lang="ca">cinta de vídeo</skos:prefLabel>
      <rdakit:toolkitLabel xml:lang="ca">cinta de vídeo</rdakit:toolkitLabel>
      <skos:definition xml:lang="ca">Tira de cinta magnètica en la qual hi ha enregistrats senyals elèctrics que es poden convertir en imatges usant un aparell de reproducció de vídeo.</skos:definition>
      <rdakit:toolkitDefinition xml:lang="ca">Tira de cinta magnètica en la qual hi ha enregistrats senyals elèctrics que es poden convertir en imatges usant un aparell de reproducció de vídeo.</rdakit:toolkitDefinition>
      <skos:prefLabel xml:lang="vi">băng video</skos:prefLabel>
      <rdakit:toolkitLabel xml:lang="vi">băng video</rdakit:toolkitLabel>
      <skos:definition xml:lang="vi">Băng từ dài trên đó ghi các tín hiệu điện tử có thể được chuyển thành hình ảnh bằng cách dùng thiết bị phát lại video.</skos:definition>
      <rdakit:toolkitDefinition xml:lang="vi">Băng từ dài trên đó ghi các tín hiệu điện tử có thể được chuyển thành hình ảnh bằng cách dùng thiết bị phát lại video.</rdakit:toolkitDefinition>
      <skos:prefLabel xml:lang="no">videobånd</skos:prefLabel>
      <rdakit:toolkitLabel xml:lang="no">videobånd</rdakit:toolkitLabel>
      <skos:definition xml:lang="no">Et stykke magnetbånd der det kan lagres elektriske signaler som kan konverteres til bilder ved hjelp av filmavspillingsutstyr.</skos:definition>
      <rdakit:toolkitDefinition xml:lang="no">Et stykke magnetbånd der det kan lagres elektriske signaler som kan konverteres til bilder ved hjelp av filmavspillingsutstyr.</rdakit:toolkitDefinition>
    </skos:Concept>
<!-- Concept: vocabulary encoding scheme  -->
    <skos:Concept rdf:about="http://rdaregistry.info/termList/RDATerms/1105" xml:lang="en">
      <skos:inScheme rdf:resource="http://rdaregistry.info/termList/RDATerms"/>
      <reg:status rdf:resource="http://metadataregistry.org/uri/RegStatus/1001"/>
      <reg:identifier rdf:resource="http://metadataregistry.org/concepts/8620"/>
      <skos:prefLabel xml:lang="en">vocabulary encoding scheme</skos:prefLabel>
      <rdakit:toolkitLabel xml:lang="en">vocabulary encoding scheme</rdakit:toolkitLabel>
      <skos:definition xml:lang="en">A named structured list of representations of controlled values for elements.</skos:definition>
      <rdakit:toolkitDefinition xml:lang="en">A named structured list of representations of controlled values for elements.</rdakit:toolkitDefinition>
      <skos:scopeNote xml:lang="en">A vocabulary encoding scheme includes an internal RDA list of terms or their corresponding value vocabularies with assigned URIs in the RDA Registry, an ISO code list, a standard terminology, etc.</skos:scopeNote>
      <skos:prefLabel xml:lang="it">schema di codifica di vocabolario</skos:prefLabel>
      <rdakit:toolkitLabel xml:lang="it">schema di codifica di vocabolario</rdakit:toolkitLabel>
      <skos:definition xml:lang="it">Una lista strutturata identificata di rappresentazioni di valori controllati per gli elementi (per es., le liste di termini incluse in RDA o i vocabolari di valori ad esse corrispondenti con gli URI assegnati nel RDA Registry, liste di codici ISO, terminologie standard).</skos:definition>
      <rdakit:toolkitDefinition xml:lang="it">Una lista strutturata identificata di rappresentazioni di valori controllati per gli elementi (per es., le liste di termini incluse in RDA o i vocabolari di valori ad esse corrispondenti con gli URI assegnati nel RDA Registry, liste di codici ISO, terminologie standard).</rdakit:toolkitDefinition>
      <skos:prefLabel xml:lang="fr">schéma d’encodage de vocabulaire</skos:prefLabel>
      <rdakit:toolkitLabel xml:lang="fr">schéma d’encodage de vocabulaire</rdakit:toolkitLabel>
      <skos:definition xml:lang="fr">Liste structurée et nommée de représentations de valeurs contrôlées pour les éléments.</skos:definition>
      <rdakit:toolkitDefinition xml:lang="fr">Liste structurée et nommée de représentations de valeurs contrôlées pour les éléments.</rdakit:toolkitDefinition>
      <skos:prefLabel xml:lang="de">Vokabularkodierungsschema</skos:prefLabel>
      <rdakit:toolkitLabel xml:lang="de">Vokabularkodierungsschema</rdakit:toolkitLabel>
      <skos:definition xml:lang="de">Eine benannte, strukturierte Liste der Repräsentationen von kontrollierten Werten für Elemente.</skos:definition>
      <rdakit:toolkitDefinition xml:lang="de">Eine benannte, strukturierte Liste der Repräsentationen von kontrollierten Werten für Elemente.</rdakit:toolkitDefinition>
      <skos:scopeNote xml:lang="de">Dazu gehören interne RDA-Listen von Termini oder den dazu korrespondierenden Vokabularen mit den zugewiesenen URIs in der RDA Registry, den ISO-Codelisten, der Standardterminologie usw.</skos:scopeNote>
      <skos:prefLabel xml:lang="fi">sanastoskeema</skos:prefLabel>
      <rdakit:toolkitLabel xml:lang="fi">sanastoskeema</rdakit:toolkitLabel>
      <skos:definition xml:lang="fi">Nimetty lista jossa on vakioituja arvoja eri tietoelementeille.</skos:definition>
      <rdakit:toolkitDefinition xml:lang="fi">Nimetty lista jossa on vakioituja arvoja eri tietoelementeille.</rdakit:toolkitDefinition>
      <skos:scopeNote xml:lang="fi">Esim. sisäinen RDA-termien sanasto ja termejä vastaavien vakioitujen arvojen URI-tunnisteet RDA Registryssä, ISO standardilistoilla tai muissa standardoiduissa sanastoissa, jne.</skos:scopeNote>
      <skos:prefLabel xml:lang="da">vokabularkodningsskema</skos:prefLabel>
      <rdakit:toolkitLabel xml:lang="da">vokabularkodningsskema</rdakit:toolkitLabel>
      <skos:definition xml:lang="da">Navngivet struktureret liste over repræsentationer af kontrollerede værdier for elementer.</skos:definition>
      <rdakit:toolkitDefinition xml:lang="da">Navngivet struktureret liste over repræsentationer af kontrollerede værdier for elementer.</rdakit:toolkitDefinition>
      <skos:scopeNote xml:lang="da">Et vokabularkodningsskema omfatter interne RDA-termlister eller deres tilsvarende værdivokabularer med tildelte URI’er i RDA-registret, ISO-kodelister, standardterminologier.</skos:scopeNote>
      <skos:prefLabel xml:lang="ca">esquema de codificació d'un vocabulari</skos:prefLabel>
      <rdakit:toolkitLabel xml:lang="ca">esquema de codificació d'un vocabulari</rdakit:toolkitLabel>
      <skos:definition xml:lang="ca">Llista estructurada i amb un nom de representacions de valors controlats d’elements.</skos:definition>
      <rdakit:toolkitDefinition xml:lang="ca">Llista estructurada i amb un nom de representacions de valors controlats d’elements.</rdakit:toolkitDefinition>
      <skos:scopeNote xml:lang="ca">Un esquema de codificació del vocabulari inclou una llista interna de termes d'RDA o els seus vocabularis dels valors corresponents amb URI assignats en l’RDA Registry, una llista de codis ISO, una terminologia normalitzada, etc.</skos:scopeNote>
      <skos:scopeNote xml:lang="fr">Comprend une liste de termes internes à RDA ou son vocabulaire de valeurs correspondant accompagné des URI qui leur ont été assignés dans le RDA Registry, un code ISO, une terminologie normalisée, etc.</skos:scopeNote>
      <skos:prefLabel xml:lang="vi">sơ đồ lập mã từ vựng</skos:prefLabel>
      <rdakit:toolkitLabel xml:lang="vi">sơ đồ lập mã từ vựng</rdakit:toolkitLabel>
      <skos:definition xml:lang="vi">Danh mục có cấu trúc được đặt tên của các thể hiện của giá trị được kiểm soát của các yếu tố.</skos:definition>
      <rdakit:toolkitDefinition xml:lang="vi">Danh mục có cấu trúc được đặt tên của các thể hiện của giá trị được kiểm soát của các yếu tố.</rdakit:toolkitDefinition>
      <skos:scopeNote xml:lang="vi">Sơ đồ lập mã từ vựng bao gồm danh mục nội bộ RDA của các thuật ngữ hoặc từ vựng giá trị tương ứng với các URI được gán trong Đăng ký RDA, danh mục mã ISO, thuật ngữ chuẩn, v.v...</skos:scopeNote>
      <skos:prefLabel xml:lang="no">kodeskjema for vokabular</skos:prefLabel>
      <rdakit:toolkitLabel xml:lang="no">kodeskjema for vokabular</rdakit:toolkitLabel>
      <skos:definition xml:lang="no">En navngitt, strukturert liste av kontrollerte verdier for elementer.</skos:definition>
      <rdakit:toolkitDefinition xml:lang="no">En navngitt, strukturert liste av kontrollerte verdier for elementer.</rdakit:toolkitDefinition>
      <skos:scopeNote xml:lang="no">En navngitt, strukturert liste av kontrollerte verdier for elementer (for eksempel interne RDA-lister over termer eller deres tilsvarende vokabularer over verdier med tildelte URI-er i RDA-registeret, ISO-kodelister, terminologistandarder).</skos:scopeNote>
    </skos:Concept>

<!-- Status properties used in this document  -->
    <skos:Concept rdf:about="http://metadataregistry.org/uri/RegStatus/1001">
        <skos:prefLabel xml:lang="en">Published</skos:prefLabel>
    </skos:Concept>

</rdf:RDF>
