<?xml version="1.0" encoding = "UTF-8"?>
<rdf:RDF
    xmlns:dc="http://purl.org/dc/elements/1.1/"
    xmlns:rdakit="http://metadataregistry.org/uri/profile/rdakit/"
    xmlns:rdf="http://www.w3.org/1999/02/22-rdf-syntax-ns#"
    xmlns:reg="http://metadataregistry.org/uri/profile/regap/"
    xmlns:owl="http://www.w3.org/2002/07/owl#"
    xmlns:skos="http://www.w3.org/2004/02/skos/core#">

<owl:Ontology rdf:about="http://rdaregistry.info/termList/videoFormat" />
<!-- Scheme: RDA Video Format -->
    <skos:ConceptScheme rdf:about="http://rdaregistry.info/termList/videoFormat">
        <dc:title>RDA Video Format</dc:title>
    </skos:ConceptScheme>

<!-- Concept: 8 mm  -->
    <skos:Concept rdf:about="http://rdaregistry.info/termList/videoFormat/1007" xml:lang="en">
      <skos:inScheme rdf:resource="http://rdaregistry.info/termList/videoFormat"/>
      <reg:status rdf:resource="http://metadataregistry.org/uri/RegStatus/1001"/>
      <reg:identifier rdf:resource="http://metadataregistry.org/concepts/905"/>
      <skos:prefLabel xml:lang="en">8 mm</skos:prefLabel>
      <rdakit:toolkitLabel xml:lang="en">8 mm</rdakit:toolkitLabel>
      <skos:definition xml:lang="en">A video format for analogue and digital tape that includes Video8, Hi-8, and Digital8 formats.</skos:definition>
      <rdakit:toolkitDefinition xml:lang="en">A video format for analogue and digital tape that includes Video8, Hi-8, and Digital8 formats.</rdakit:toolkitDefinition>
      <skos:prefLabel xml:lang="de">8 mm</skos:prefLabel>
      <rdakit:toolkitLabel xml:lang="de">8 mm</rdakit:toolkitLabel>
      <skos:definition xml:lang="de">Ein Videoformat für ein analoges und digitales Band, das die Formate Video8, Hi-8 und Digital8 umfasst.</skos:definition>
      <rdakit:toolkitDefinition xml:lang="de">Ein Videoformat für ein analoges und digitales Band, das die Formate Video8, Hi-8 und Digital8 umfasst.</rdakit:toolkitDefinition>
      <skos:prefLabel xml:lang="fi">8 mm</skos:prefLabel>
      <rdakit:toolkitLabel xml:lang="fi">8 mm</rdakit:toolkitLabel>
      <skos:definition xml:lang="fi">Analogisen ja digitaalisen nauhan videoformaatti, johon sisältyvät Video8, Hi-8 sekä Digital8 -formaatit.</skos:definition>
      <rdakit:toolkitDefinition xml:lang="fi">Analogisen ja digitaalisen nauhan videoformaatti, johon sisältyvät Video8, Hi-8 sekä Digital8 -formaatit.</rdakit:toolkitDefinition>
      <skos:prefLabel xml:lang="ca">8 mm</skos:prefLabel>
      <rdakit:toolkitLabel xml:lang="ca">8 mm</rdakit:toolkitLabel>
      <skos:definition xml:lang="ca">Format vídeo per a cinta analògica i digital que inclou els formats Video8, Hi-8, i Digital8.</skos:definition>
      <rdakit:toolkitDefinition xml:lang="ca">Format vídeo per a cinta analògica i digital que inclou els formats Video8, Hi-8, i Digital8.</rdakit:toolkitDefinition>
      <skos:prefLabel xml:lang="da">8 mm</skos:prefLabel>
      <rdakit:toolkitLabel xml:lang="da">8 mm</rdakit:toolkitLabel>
      <skos:definition xml:lang="da">Videoformat til analode og digitale bånd, inkl. Video8, Hi-8 og Digital8 formater.</skos:definition>
      <rdakit:toolkitDefinition xml:lang="da">Videoformat til analode og digitale bånd, inkl. Video8, Hi-8 og Digital8 formater.</rdakit:toolkitDefinition>
      <skos:prefLabel xml:lang="fr">8 mm</skos:prefLabel>
      <rdakit:toolkitLabel xml:lang="fr">8 mm</rdakit:toolkitLabel>
      <skos:definition xml:lang="fr">Format vidéo pour bande analogique ou numérique qui comprend les formats Video 8, Hi-8 et Digital8.</skos:definition>
      <rdakit:toolkitDefinition xml:lang="fr">Format vidéo pour bande analogique ou numérique qui comprend les formats Video 8, Hi-8 et Digital8.</rdakit:toolkitDefinition>
      <skos:prefLabel xml:lang="no">8 mm </skos:prefLabel>
      <rdakit:toolkitLabel xml:lang="no">8 mm </rdakit:toolkitLabel>
      <skos:definition xml:lang="no">Et videoformat for analoge og digitale videobånd, inkludert formatene Video8, Hi-8 og Digital8.</skos:definition>
      <rdakit:toolkitDefinition xml:lang="no">Et videoformat for analoge og digitale videobånd, inkludert formatene Video8, Hi-8 og Digital8.</rdakit:toolkitDefinition>
    </skos:Concept>
<!-- Concept: Betacam  -->
    <skos:Concept rdf:about="http://rdaregistry.info/termList/videoFormat/1002" xml:lang="en">
      <skos:inScheme rdf:resource="http://rdaregistry.info/termList/videoFormat"/>
      <reg:status rdf:resource="http://metadataregistry.org/uri/RegStatus/1001"/>
      <reg:identifier rdf:resource="http://metadataregistry.org/concepts/900"/>
      <skos:prefLabel xml:lang="en">Betacam</skos:prefLabel>
      <rdakit:toolkitLabel xml:lang="en">Betacam</rdakit:toolkitLabel>
      <skos:definition xml:lang="en">A video format for analogue tape developed for professional use by Sony in 1982.</skos:definition>
      <rdakit:toolkitDefinition xml:lang="en">A video format for analogue tape developed for professional use by Sony in 1982.</rdakit:toolkitDefinition>
      <skos:prefLabel xml:lang="de">Betacam</skos:prefLabel>
      <rdakit:toolkitLabel xml:lang="de">Betacam</rdakit:toolkitLabel>
      <skos:definition xml:lang="de">Ein Videoformat für ein analoges Band, das 1982 von Sony für den gewerblichen Gebrauch entwickelt wurde.</skos:definition>
      <rdakit:toolkitDefinition xml:lang="de">Ein Videoformat für ein analoges Band, das 1982 von Sony für den gewerblichen Gebrauch entwickelt wurde.</rdakit:toolkitDefinition>
      <skos:prefLabel xml:lang="fi">Betacam</skos:prefLabel>
      <rdakit:toolkitLabel xml:lang="fi">Betacam</rdakit:toolkitLabel>
      <skos:definition xml:lang="fi">Analogisen nauhan videoformaatti, jonka Sony kehitti ammattilaiskäyttöön vuonna 1982.</skos:definition>
      <rdakit:toolkitDefinition xml:lang="fi">Analogisen nauhan videoformaatti, jonka Sony kehitti ammattilaiskäyttöön vuonna 1982.</rdakit:toolkitDefinition>
      <skos:prefLabel xml:lang="ca">Betacam</skos:prefLabel>
      <rdakit:toolkitLabel xml:lang="ca">Betacam</rdakit:toolkitLabel>
      <skos:definition xml:lang="ca">Format vídeo per a cinta analògica desenvolupat per a ús professional per Sony el 1982.</skos:definition>
      <rdakit:toolkitDefinition xml:lang="ca">Format vídeo per a cinta analògica desenvolupat per a ús professional per Sony el 1982.</rdakit:toolkitDefinition>
      <skos:prefLabel xml:lang="da">Betacam</skos:prefLabel>
      <rdakit:toolkitLabel xml:lang="da">Betacam</rdakit:toolkitLabel>
      <skos:definition xml:lang="da">Videoformat til analogt bånd udviklet til professionel brug af Sony i 1975.</skos:definition>
      <rdakit:toolkitDefinition xml:lang="da">Videoformat til analogt bånd udviklet til professionel brug af Sony i 1975.</rdakit:toolkitDefinition>
      <skos:prefLabel xml:lang="fr">Betacam</skos:prefLabel>
      <rdakit:toolkitLabel xml:lang="fr">Betacam</rdakit:toolkitLabel>
      <skos:definition xml:lang="fr">Format vidéo pour bande analogique conçu pour un usage professionnel par Sony en 1982.</skos:definition>
      <rdakit:toolkitDefinition xml:lang="fr">Format vidéo pour bande analogique conçu pour un usage professionnel par Sony en 1982.</rdakit:toolkitDefinition>
      <skos:prefLabel xml:lang="no">Betacam</skos:prefLabel>
      <rdakit:toolkitLabel xml:lang="no">Betacam</rdakit:toolkitLabel>
      <skos:definition xml:lang="no">Et videoformat for analoge videobånd for profesjonell bruk, utviklet av Sony i 1982.</skos:definition>
      <rdakit:toolkitDefinition xml:lang="no">Et videoformat for analoge videobånd for profesjonell bruk, utviklet av Sony i 1982.</rdakit:toolkitDefinition>
    </skos:Concept>
<!-- Concept: Betacam SP  -->
    <skos:Concept rdf:about="http://rdaregistry.info/termList/videoFormat/1016" xml:lang="en">
      <skos:inScheme rdf:resource="http://rdaregistry.info/termList/videoFormat"/>
      <reg:status rdf:resource="http://metadataregistry.org/uri/RegStatus/1001"/>
      <reg:identifier rdf:resource="http://metadataregistry.org/concepts/1138"/>
      <skos:prefLabel xml:lang="en">Betacam SP</skos:prefLabel>
      <rdakit:toolkitLabel xml:lang="en">Betacam SP</rdakit:toolkitLabel>
      <skos:definition xml:lang="en">A video format for analogue tape based on the Betacam format that increases horizontal resolution to 340 lines.</skos:definition>
      <rdakit:toolkitDefinition xml:lang="en">A video format for analogue tape based on the Betacam format that increases horizontal resolution to 340 lines.</rdakit:toolkitDefinition>
      <skos:prefLabel xml:lang="de">Betacam SP</skos:prefLabel>
      <rdakit:toolkitLabel xml:lang="de">Betacam SP</rdakit:toolkitLabel>
      <skos:definition xml:lang="de">Ein Videoformat für ein analoges Band, basierend auf dem Betacam-Format, das die horizontale Auflösung auf 340 Zeilen erhöht.</skos:definition>
      <rdakit:toolkitDefinition xml:lang="de">Ein Videoformat für ein analoges Band, basierend auf dem Betacam-Format, das die horizontale Auflösung auf 340 Zeilen erhöht.</rdakit:toolkitDefinition>
      <skos:prefLabel xml:lang="fi">Betacam SP</skos:prefLabel>
      <rdakit:toolkitLabel xml:lang="fi">Betacam SP</rdakit:toolkitLabel>
      <skos:definition xml:lang="fi">Analogisen nauhan Betacam-formaattiin perustuva videoformaatti, joka nostaa horisontaalisen resoluution 340:een raitaan.</skos:definition>
      <rdakit:toolkitDefinition xml:lang="fi">Analogisen nauhan Betacam-formaattiin perustuva videoformaatti, joka nostaa horisontaalisen resoluution 340:een raitaan.</rdakit:toolkitDefinition>
      <skos:prefLabel xml:lang="ca">Betacam SP</skos:prefLabel>
      <rdakit:toolkitLabel xml:lang="ca">Betacam SP</rdakit:toolkitLabel>
      <skos:definition xml:lang="ca">Format vídeo per a cinta analògica basat en el format Betacam que incrementa la resolució horitzontal a 340 línies.</skos:definition>
      <rdakit:toolkitDefinition xml:lang="ca">Format vídeo per a cinta analògica basat en el format Betacam que incrementa la resolució horitzontal a 340 línies.</rdakit:toolkitDefinition>
      <skos:prefLabel xml:lang="da">Betacam SP</skos:prefLabel>
      <rdakit:toolkitLabel xml:lang="da">Betacam SP</rdakit:toolkitLabel>
      <skos:definition xml:lang="da">Videoformat til analoge bånd baseret på Betacan.formatet, der øger den horisontale opløsning på 340 linjer.</skos:definition>
      <rdakit:toolkitDefinition xml:lang="da">Videoformat til analoge bånd baseret på Betacan.formatet, der øger den horisontale opløsning på 340 linjer.</rdakit:toolkitDefinition>
      <skos:prefLabel xml:lang="fr">Betacam SP</skos:prefLabel>
      <rdakit:toolkitLabel xml:lang="fr">Betacam SP</rdakit:toolkitLabel>
      <skos:definition xml:lang="fr">Format vidéo pour bande analogique basé sur le format Betacam et qui augmente la résolution horizontale à 340 lignes.</skos:definition>
      <rdakit:toolkitDefinition xml:lang="fr">Format vidéo pour bande analogique basé sur le format Betacam et qui augmente la résolution horizontale à 340 lignes.</rdakit:toolkitDefinition>
      <skos:prefLabel xml:lang="no">Betacam SP</skos:prefLabel>
      <rdakit:toolkitLabel xml:lang="no">Betacam SP</rdakit:toolkitLabel>
      <skos:definition xml:lang="no">Et videoformat for analoge videobånd som er basert på Betacam-formatet og øker den horisontale oppløsningen til 340 linjer.</skos:definition>
      <rdakit:toolkitDefinition xml:lang="no">Et videoformat for analoge videobånd som er basert på Betacam-formatet og øker den horisontale oppløsningen til 340 linjer.</rdakit:toolkitDefinition>
    </skos:Concept>
<!-- Concept: Betamax  -->
    <skos:Concept rdf:about="http://rdaregistry.info/termList/videoFormat/1001" xml:lang="en">
      <skos:inScheme rdf:resource="http://rdaregistry.info/termList/videoFormat"/>
      <reg:status rdf:resource="http://metadataregistry.org/uri/RegStatus/1001"/>
      <reg:identifier rdf:resource="http://metadataregistry.org/concepts/899"/>
      <skos:prefLabel xml:lang="en">Betamax</skos:prefLabel>
      <skos:altLabel xml:lang="en">Beta</skos:altLabel>
      <rdakit:toolkitLabel xml:lang="en">Betamax</rdakit:toolkitLabel>
      <skos:definition xml:lang="en">A video format for analog tape developed for consumer use by Sony in 1975.</skos:definition>
      <rdakit:toolkitDefinition xml:lang="en">A video format for analog tape developed for consumer use by Sony in 1975.</rdakit:toolkitDefinition>
      <skos:prefLabel xml:lang="de">Beta</skos:prefLabel>
      <rdakit:toolkitLabel xml:lang="de">Beta</rdakit:toolkitLabel>
      <skos:definition xml:lang="de">Ein Videoformat für ein analoges Band, das 1975 von Sony für den privaten Gebrauch entwickelt wurde.</skos:definition>
      <rdakit:toolkitDefinition xml:lang="de">Ein Videoformat für ein analoges Band, das 1975 von Sony für den privaten Gebrauch entwickelt wurde.</rdakit:toolkitDefinition>
      <skos:prefLabel xml:lang="fi">Betamax</skos:prefLabel>
      <skos:altLabel xml:lang="fi">Beta</skos:altLabel>
      <rdakit:toolkitLabel xml:lang="fi">Betamax</rdakit:toolkitLabel>
      <skos:definition xml:lang="fi">Analogisen nauhan videoformaatti, jonka Sony kehitti kuluttajakäyttöön vuonna 1975.</skos:definition>
      <rdakit:toolkitDefinition xml:lang="fi">Analogisen nauhan videoformaatti, jonka Sony kehitti kuluttajakäyttöön vuonna 1975.</rdakit:toolkitDefinition>
      <skos:prefLabel xml:lang="ca">Betamax</skos:prefLabel>
      <skos:altLabel xml:lang="ca">Beta</skos:altLabel>
      <rdakit:toolkitLabel xml:lang="ca">Betamax</rdakit:toolkitLabel>
      <skos:definition xml:lang="ca">Format vídeo per a cinta analògica desenvolupat per a ús domèstic per Sony el 1975.</skos:definition>
      <rdakit:toolkitDefinition xml:lang="ca">Format vídeo per a cinta analògica desenvolupat per a ús domèstic per Sony el 1975.</rdakit:toolkitDefinition>
      <skos:prefLabel xml:lang="da">Betamax</skos:prefLabel>
      <rdakit:toolkitLabel xml:lang="da">Betamax</rdakit:toolkitLabel>
      <skos:definition xml:lang="da">Videoformat til analogt bånd udviklet til privat brug af Sony i 1975.</skos:definition>
      <rdakit:toolkitDefinition xml:lang="da">Videoformat til analogt bånd udviklet til privat brug af Sony i 1975.</rdakit:toolkitDefinition>
      <skos:prefLabel xml:lang="fr">Betamax</skos:prefLabel>
      <skos:altLabel xml:lang="fr">Beta</skos:altLabel>
      <rdakit:toolkitLabel xml:lang="fr">Betamax</rdakit:toolkitLabel>
      <skos:definition xml:lang="fr">Format vidéo pour bande analogique conçu pour un usage grand public par Sony en 1975.</skos:definition>
      <rdakit:toolkitDefinition xml:lang="fr">Format vidéo pour bande analogique conçu pour un usage grand public par Sony en 1975.</rdakit:toolkitDefinition>
      <skos:prefLabel xml:lang="no">Betamax</skos:prefLabel>
      <skos:altLabel xml:lang="no">Beta</skos:altLabel>
      <rdakit:toolkitLabel xml:lang="no">Betamax</rdakit:toolkitLabel>
      <skos:definition xml:lang="no">Et videoformat for analoge videobånd for hjemmebruk, utviklet av Sony i 1975.</skos:definition>
      <rdakit:toolkitDefinition xml:lang="no">Et videoformat for analoge videobånd for hjemmebruk, utviklet av Sony i 1975.</rdakit:toolkitDefinition>
    </skos:Concept>
<!-- Concept: CED  -->
    <skos:Concept rdf:about="http://rdaregistry.info/termList/videoFormat/1004" xml:lang="en">
      <skos:inScheme rdf:resource="http://rdaregistry.info/termList/videoFormat"/>
      <reg:status rdf:resource="http://metadataregistry.org/uri/RegStatus/1001"/>
      <reg:identifier rdf:resource="http://metadataregistry.org/concepts/902"/>
      <skos:prefLabel xml:lang="en">CED</skos:prefLabel>
      <skos:altLabel xml:lang="en">Capacitance Electronic Disc</skos:altLabel>
      <rdakit:toolkitLabel xml:lang="en">CED</rdakit:toolkitLabel>
      <skos:definition xml:lang="en">A video format for analogue disc.</skos:definition>
      <rdakit:toolkitDefinition xml:lang="en">A video format for analogue disc.</rdakit:toolkitDefinition>
      <skos:prefLabel xml:lang="de">CED</skos:prefLabel>
      <rdakit:toolkitLabel xml:lang="de">CED</rdakit:toolkitLabel>
      <skos:definition xml:lang="de">Ein Videoformat für eine analoge Platte.</skos:definition>
      <rdakit:toolkitDefinition xml:lang="de">Ein Videoformat für eine analoge Platte.</rdakit:toolkitDefinition>
      <skos:prefLabel xml:lang="fi">CED</skos:prefLabel>
      <rdakit:toolkitLabel xml:lang="fi">CED</rdakit:toolkitLabel>
      <skos:definition xml:lang="fi">Analogisen levyn videoformaatti.</skos:definition>
      <rdakit:toolkitDefinition xml:lang="fi">Analogisen levyn videoformaatti.</rdakit:toolkitDefinition>
      <skos:prefLabel xml:lang="ca">CED</skos:prefLabel>
      <skos:altLabel xml:lang="ca">Capacitance Electronic Disc</skos:altLabel>
      <rdakit:toolkitLabel xml:lang="ca">CED</rdakit:toolkitLabel>
      <skos:definition xml:lang="ca">Format vídeo per a disc analògic.</skos:definition>
      <rdakit:toolkitDefinition xml:lang="ca">Format vídeo per a disc analògic.</rdakit:toolkitDefinition>
      <skos:prefLabel xml:lang="da">CED</skos:prefLabel>
      <rdakit:toolkitLabel xml:lang="da">CED</rdakit:toolkitLabel>
      <skos:definition xml:lang="da">Videoformat til analog disk.</skos:definition>
      <rdakit:toolkitDefinition xml:lang="da">Videoformat til analog disk.</rdakit:toolkitDefinition>
      <skos:prefLabel xml:lang="fr">CED</skos:prefLabel>
      <skos:altLabel xml:lang="fr">vidéodisque à lecture capacitive</skos:altLabel>
      <rdakit:toolkitLabel xml:lang="fr">CED</rdakit:toolkitLabel>
      <skos:definition xml:lang="fr">Format vidéo pour disque analogique.</skos:definition>
      <rdakit:toolkitDefinition xml:lang="fr">Format vidéo pour disque analogique.</rdakit:toolkitDefinition>
      <skos:prefLabel xml:lang="no">CED</skos:prefLabel>
      <skos:altLabel xml:lang="no">Capacitance Electronic Disc</skos:altLabel>
      <rdakit:toolkitLabel xml:lang="no">CED</rdakit:toolkitLabel>
      <skos:definition xml:lang="no">Et videoformat for analoge plater.</skos:definition>
      <rdakit:toolkitDefinition xml:lang="no">Et videoformat for analoge plater.</rdakit:toolkitDefinition>
    </skos:Concept>
<!-- Concept: D-2  -->
    <skos:Concept rdf:about="http://rdaregistry.info/termList/videoFormat/1005" xml:lang="en">
      <skos:inScheme rdf:resource="http://rdaregistry.info/termList/videoFormat"/>
      <reg:status rdf:resource="http://metadataregistry.org/uri/RegStatus/1001"/>
      <reg:identifier rdf:resource="http://metadataregistry.org/concepts/903"/>
      <skos:prefLabel xml:lang="en">D-2</skos:prefLabel>
      <rdakit:toolkitLabel xml:lang="en">D-2</rdakit:toolkitLabel>
      <skos:definition xml:lang="en">A video format for analogue tape developed for professional use by Ampex in 1988.</skos:definition>
      <rdakit:toolkitDefinition xml:lang="en">A video format for analogue tape developed for professional use by Ampex in 1988.</rdakit:toolkitDefinition>
      <skos:prefLabel xml:lang="de">D-2</skos:prefLabel>
      <rdakit:toolkitLabel xml:lang="de">D-2</rdakit:toolkitLabel>
      <skos:definition xml:lang="de">Ein Videoformat für ein analoges Band, das 1988 von Ampex für den gewerblichen Gebrauch entwickelt wurde.</skos:definition>
      <rdakit:toolkitDefinition xml:lang="de">Ein Videoformat für ein analoges Band, das 1988 von Ampex für den gewerblichen Gebrauch entwickelt wurde.</rdakit:toolkitDefinition>
      <skos:prefLabel xml:lang="fi">D-2</skos:prefLabel>
      <rdakit:toolkitLabel xml:lang="fi">D-2</rdakit:toolkitLabel>
      <skos:definition xml:lang="fi">Analogisen nauhan videoformaatti, jonka Ampex kehitti ammattilaiskäyttöön vuonna 1988.</skos:definition>
      <rdakit:toolkitDefinition xml:lang="fi">Analogisen nauhan videoformaatti, jonka Ampex kehitti ammattilaiskäyttöön vuonna 1988.</rdakit:toolkitDefinition>
      <skos:prefLabel xml:lang="ca">D-2</skos:prefLabel>
      <rdakit:toolkitLabel xml:lang="ca">D-2</rdakit:toolkitLabel>
      <skos:definition xml:lang="ca">Format vídeo per a cinta analògica desenvolupat per a ús professional per Ampex el 1988.</skos:definition>
      <rdakit:toolkitDefinition xml:lang="ca">Format vídeo per a cinta analògica desenvolupat per a ús professional per Ampex el 1988.</rdakit:toolkitDefinition>
      <skos:prefLabel xml:lang="da">D-2</skos:prefLabel>
      <rdakit:toolkitLabel xml:lang="da">D-2</rdakit:toolkitLabel>
      <skos:definition xml:lang="da">Videoformat til analoge bånd udviklet til professionel brug af Ampex i 1998.</skos:definition>
      <rdakit:toolkitDefinition xml:lang="da">Videoformat til analoge bånd udviklet til professionel brug af Ampex i 1998.</rdakit:toolkitDefinition>
      <skos:prefLabel xml:lang="fr">D-2</skos:prefLabel>
      <rdakit:toolkitLabel xml:lang="fr">D-2</rdakit:toolkitLabel>
      <skos:definition xml:lang="fr">Format vidéo pour bande analogique conçu pour un usage professionnel par Ampex en 1988.</skos:definition>
      <rdakit:toolkitDefinition xml:lang="fr">Format vidéo pour bande analogique conçu pour un usage professionnel par Ampex en 1988.</rdakit:toolkitDefinition>
      <skos:prefLabel xml:lang="no">D-2</skos:prefLabel>
      <rdakit:toolkitLabel xml:lang="no">D-2</rdakit:toolkitLabel>
      <skos:definition xml:lang="no">Et videoformat for analoge videobånd utviklet av Ampex i 1988 for profesjonell bruk.</skos:definition>
      <rdakit:toolkitDefinition xml:lang="no">Et videoformat for analoge videobånd utviklet av Ampex i 1988 for profesjonell bruk.</rdakit:toolkitDefinition>
    </skos:Concept>
<!-- Concept: EIAJ  -->
    <skos:Concept rdf:about="http://rdaregistry.info/termList/videoFormat/1006" xml:lang="en">
      <skos:inScheme rdf:resource="http://rdaregistry.info/termList/videoFormat"/>
      <reg:status rdf:resource="http://metadataregistry.org/uri/RegStatus/1001"/>
      <reg:identifier rdf:resource="http://metadataregistry.org/concepts/904"/>
      <skos:prefLabel xml:lang="en">EIAJ</skos:prefLabel>
      <rdakit:toolkitLabel xml:lang="en">EIAJ</rdakit:toolkitLabel>
      <skos:definition xml:lang="en">A video format for analogue tape developed for professional use by the Electronic Industries Association of Japan in 1969.</skos:definition>
      <rdakit:toolkitDefinition xml:lang="en">A video format for analogue tape developed for professional use by the Electronic Industries Association of Japan in 1969.</rdakit:toolkitDefinition>
      <skos:prefLabel xml:lang="de">EIAJ</skos:prefLabel>
      <rdakit:toolkitLabel xml:lang="de">EIAJ</rdakit:toolkitLabel>
      <skos:definition xml:lang="de">Ein Videoformat für ein analoges Band, das 1969 von der Electronic Industries Association of Japan für den gewerblichen Gebrauch entwickelt wurde.</skos:definition>
      <rdakit:toolkitDefinition xml:lang="de">Ein Videoformat für ein analoges Band, das 1969 von der Electronic Industries Association of Japan für den gewerblichen Gebrauch entwickelt wurde.</rdakit:toolkitDefinition>
      <skos:prefLabel xml:lang="fi">EIAJ</skos:prefLabel>
      <rdakit:toolkitLabel xml:lang="fi">EIAJ</rdakit:toolkitLabel>
      <skos:definition xml:lang="fi">Analogisen nauhan videoformaatti, jonka  Electronic Industries Association of Japan kehitti ammattilaiskäyttöön vuonna 1969.</skos:definition>
      <rdakit:toolkitDefinition xml:lang="fi">Analogisen nauhan videoformaatti, jonka  Electronic Industries Association of Japan kehitti ammattilaiskäyttöön vuonna 1969.</rdakit:toolkitDefinition>
      <skos:prefLabel xml:lang="ca">EIAJ</skos:prefLabel>
      <rdakit:toolkitLabel xml:lang="ca">EIAJ</rdakit:toolkitLabel>
      <skos:definition xml:lang="ca">Format vídeo per a cinta analògica desenvolupat per a ús professional Electronic Industries Association of Japan el 1969.</skos:definition>
      <rdakit:toolkitDefinition xml:lang="ca">Format vídeo per a cinta analògica desenvolupat per a ús professional Electronic Industries Association of Japan el 1969.</rdakit:toolkitDefinition>
      <skos:prefLabel xml:lang="da">EIAJ</skos:prefLabel>
      <rdakit:toolkitLabel xml:lang="da">EIAJ</rdakit:toolkitLabel>
      <skos:definition xml:lang="da">Videoformat til analoge bånd udviklet til professionel brug af Electronic Industries Association of Japan i 1969.</skos:definition>
      <rdakit:toolkitDefinition xml:lang="da">Videoformat til analoge bånd udviklet til professionel brug af Electronic Industries Association of Japan i 1969.</rdakit:toolkitDefinition>
      <skos:prefLabel xml:lang="fr">EIAJ</skos:prefLabel>
      <rdakit:toolkitLabel xml:lang="fr">EIAJ</rdakit:toolkitLabel>
      <skos:definition xml:lang="fr">Format vidéo pour bande analogique conçu pour un usage professionnel par la Electronic Industries Association of Japan en 1969.</skos:definition>
      <rdakit:toolkitDefinition xml:lang="fr">Format vidéo pour bande analogique conçu pour un usage professionnel par la Electronic Industries Association of Japan en 1969.</rdakit:toolkitDefinition>
      <skos:prefLabel xml:lang="no">EIAJ</skos:prefLabel>
      <rdakit:toolkitLabel xml:lang="no">EIAJ</rdakit:toolkitLabel>
      <skos:definition xml:lang="no">Et videoformat for analoge videobånd utviklet av Electronic Industries Association of Japan i 1969 for profesjonell bruk.</skos:definition>
      <rdakit:toolkitDefinition xml:lang="no">Et videoformat for analoge videobånd utviklet av Electronic Industries Association of Japan i 1969 for profesjonell bruk.</rdakit:toolkitDefinition>
    </skos:Concept>
<!-- Concept: Hi-8 mm  -->
    <skos:Concept rdf:about="http://rdaregistry.info/termList/videoFormat/1008" xml:lang="en">
      <skos:inScheme rdf:resource="http://rdaregistry.info/termList/videoFormat"/>
      <reg:status rdf:resource="http://metadataregistry.org/uri/RegStatus/1001"/>
      <reg:identifier rdf:resource="http://metadataregistry.org/concepts/906"/>
      <skos:prefLabel xml:lang="en">Hi-8 mm</skos:prefLabel>
      <rdakit:toolkitLabel xml:lang="en">Hi-8 mm</rdakit:toolkitLabel>
      <skos:definition xml:lang="en">A video format for analogue tape that is part of the 8 mm format.</skos:definition>
      <rdakit:toolkitDefinition xml:lang="en">A video format for analogue tape that is part of the 8 mm format.</rdakit:toolkitDefinition>
      <skos:prefLabel xml:lang="de">Hi-8 mm</skos:prefLabel>
      <rdakit:toolkitLabel xml:lang="de">Hi-8 mm</rdakit:toolkitLabel>
      <skos:definition xml:lang="de">Ein Videoformat für ein analoges Band, das Teil des 8 mm Formats ist.</skos:definition>
      <rdakit:toolkitDefinition xml:lang="de">Ein Videoformat für ein analoges Band, das Teil des 8 mm Formats ist.</rdakit:toolkitDefinition>
      <skos:prefLabel xml:lang="fi">Hi-8 mm</skos:prefLabel>
      <rdakit:toolkitLabel xml:lang="fi">Hi-8 mm</rdakit:toolkitLabel>
      <skos:definition xml:lang="fi">Analogisen nauhan videoformaatti joka on osa 8 mm -formaattia.</skos:definition>
      <rdakit:toolkitDefinition xml:lang="fi">Analogisen nauhan videoformaatti joka on osa 8 mm -formaattia.</rdakit:toolkitDefinition>
      <skos:prefLabel xml:lang="ca">Hi-8 mm</skos:prefLabel>
      <rdakit:toolkitLabel xml:lang="ca">Hi-8 mm</rdakit:toolkitLabel>
      <skos:definition xml:lang="ca">Format vídeo per a cinta analògica que és part del format 8 mm.</skos:definition>
      <rdakit:toolkitDefinition xml:lang="ca">Format vídeo per a cinta analògica que és part del format 8 mm.</rdakit:toolkitDefinition>
      <skos:prefLabel xml:lang="da">Hi-8 mm</skos:prefLabel>
      <rdakit:toolkitLabel xml:lang="da">Hi-8 mm</rdakit:toolkitLabel>
      <skos:definition xml:lang="da">Videoformat til analoge bånd der er en del af 8 mm formatet.</skos:definition>
      <rdakit:toolkitDefinition xml:lang="da">Videoformat til analoge bånd der er en del af 8 mm formatet.</rdakit:toolkitDefinition>
      <skos:prefLabel xml:lang="fr">Hi-8 mm</skos:prefLabel>
      <rdakit:toolkitLabel xml:lang="fr">Hi-8 mm</rdakit:toolkitLabel>
      <skos:definition xml:lang="fr">Format vidéo pour bande analogique qui fait partie du format 8 mm.</skos:definition>
      <rdakit:toolkitDefinition xml:lang="fr">Format vidéo pour bande analogique qui fait partie du format 8 mm.</rdakit:toolkitDefinition>
      <skos:prefLabel xml:lang="no">Hi-8 mm</skos:prefLabel>
      <rdakit:toolkitLabel xml:lang="no">Hi-8 mm</rdakit:toolkitLabel>
      <skos:definition xml:lang="no">Et videoformat for analoge videobånd som er del av 8 mm-formatet.</skos:definition>
      <rdakit:toolkitDefinition xml:lang="no">Et videoformat for analoge videobånd som er del av 8 mm-formatet.</rdakit:toolkitDefinition>
    </skos:Concept>
<!-- Concept: Laser optical  -->
    <skos:Concept rdf:about="http://rdaregistry.info/termList/videoFormat/1009" xml:lang="en">
      <skos:inScheme rdf:resource="http://rdaregistry.info/termList/videoFormat"/>
      <reg:status rdf:resource="http://metadataregistry.org/uri/RegStatus/1001"/>
      <reg:identifier rdf:resource="http://metadataregistry.org/concepts/907"/>
      <skos:prefLabel xml:lang="en">Laser optical</skos:prefLabel>
      <rdakit:toolkitLabel xml:lang="en">Laser optical</rdakit:toolkitLabel>
      <skos:definition xml:lang="en">A video format for optical disc that is read by a laser.</skos:definition>
      <rdakit:toolkitDefinition xml:lang="en">A video format for optical disc that is read by a laser.</rdakit:toolkitDefinition>
      <skos:prefLabel xml:lang="de">Laser optical</skos:prefLabel>
      <rdakit:toolkitLabel xml:lang="de">Laser optical</rdakit:toolkitLabel>
      <skos:definition xml:lang="de">Ein Videoformat für eine Bildplatte, die von einem Laser abgelesen wird.</skos:definition>
      <rdakit:toolkitDefinition xml:lang="de">Ein Videoformat für eine Bildplatte, die von einem Laser abgelesen wird.</rdakit:toolkitDefinition>
      <skos:prefLabel xml:lang="fi">optinen levy</skos:prefLabel>
      <rdakit:toolkitLabel xml:lang="fi">optinen levy</rdakit:toolkitLabel>
      <skos:definition xml:lang="fi">Optisen levyn laserluettava videoformaatti.</skos:definition>
      <rdakit:toolkitDefinition xml:lang="fi">Optisen levyn laserluettava videoformaatti.</rdakit:toolkitDefinition>
      <skos:prefLabel xml:lang="ca">Làser òptic</skos:prefLabel>
      <rdakit:toolkitLabel xml:lang="ca">Làser òptic</rdakit:toolkitLabel>
      <skos:definition xml:lang="ca">Format vídeo per a disc òptic que es llegeix amb un làser.</skos:definition>
      <rdakit:toolkitDefinition xml:lang="ca">Format vídeo per a disc òptic que es llegeix amb un làser.</rdakit:toolkitDefinition>
      <skos:prefLabel xml:lang="da">Laser optical</skos:prefLabel>
      <rdakit:toolkitLabel xml:lang="da">Laser optical</rdakit:toolkitLabel>
      <skos:definition xml:lang="da">Videoformat til optisk disk, der læses af en laser.</skos:definition>
      <rdakit:toolkitDefinition xml:lang="da">Videoformat til optisk disk, der læses af en laser.</rdakit:toolkitDefinition>
      <skos:prefLabel xml:lang="fr">optique à laser</skos:prefLabel>
      <rdakit:toolkitLabel xml:lang="fr">optique à laser</rdakit:toolkitLabel>
      <skos:definition xml:lang="fr">Format vidéo pour disque optique qui est lu par un laser.</skos:definition>
      <rdakit:toolkitDefinition xml:lang="fr">Format vidéo pour disque optique qui est lu par un laser.</rdakit:toolkitDefinition>
      <skos:prefLabel xml:lang="no">laseroptisk</skos:prefLabel>
      <rdakit:toolkitLabel xml:lang="no">laseroptisk</rdakit:toolkitLabel>
      <skos:definition xml:lang="no">Et videoformat for optiske plater som leses av laser.</skos:definition>
      <rdakit:toolkitDefinition xml:lang="no">Et videoformat for optiske plater som leses av laser.</rdakit:toolkitDefinition>
    </skos:Concept>
<!-- Concept: M-II  -->
    <skos:Concept rdf:about="http://rdaregistry.info/termList/videoFormat/1010" xml:lang="en">
      <skos:inScheme rdf:resource="http://rdaregistry.info/termList/videoFormat"/>
      <reg:status rdf:resource="http://metadataregistry.org/uri/RegStatus/1001"/>
      <reg:identifier rdf:resource="http://metadataregistry.org/concepts/908"/>
      <skos:prefLabel xml:lang="en">M-II</skos:prefLabel>
      <rdakit:toolkitLabel xml:lang="en">M-II</rdakit:toolkitLabel>
      <skos:definition xml:lang="en">A video format for analogue tape developed for professional use by Panasonic in 1986.</skos:definition>
      <rdakit:toolkitDefinition xml:lang="en">A video format for analogue tape developed for professional use by Panasonic in 1986.</rdakit:toolkitDefinition>
      <skos:prefLabel xml:lang="de">M-II</skos:prefLabel>
      <rdakit:toolkitLabel xml:lang="de">M-II</rdakit:toolkitLabel>
      <skos:definition xml:lang="de">Ein Videoformat für ein analoges Band, das 1986 von Panasonic für den gewerblichen Gebrauch entwickelt wurde.</skos:definition>
      <rdakit:toolkitDefinition xml:lang="de">Ein Videoformat für ein analoges Band, das 1986 von Panasonic für den gewerblichen Gebrauch entwickelt wurde.</rdakit:toolkitDefinition>
      <skos:prefLabel xml:lang="fi">M-II</skos:prefLabel>
      <rdakit:toolkitLabel xml:lang="fi">M-II</rdakit:toolkitLabel>
      <skos:definition xml:lang="fi">Analogisen nauhan videoformaatti, jonka Panasonic kehitti ammattilaiskäyttöön vuonna 1986.</skos:definition>
      <rdakit:toolkitDefinition xml:lang="fi">Analogisen nauhan videoformaatti, jonka Panasonic kehitti ammattilaiskäyttöön vuonna 1986.</rdakit:toolkitDefinition>
      <skos:prefLabel xml:lang="ca">M-II</skos:prefLabel>
      <rdakit:toolkitLabel xml:lang="ca">M-II</rdakit:toolkitLabel>
      <skos:definition xml:lang="ca">Format vídeo per a cinta analògica desenvolupat per a ús professional per Panasonic  el 1988.</skos:definition>
      <rdakit:toolkitDefinition xml:lang="ca">Format vídeo per a cinta analògica desenvolupat per a ús professional per Panasonic  el 1988.</rdakit:toolkitDefinition>
      <skos:prefLabel xml:lang="da">M-II</skos:prefLabel>
      <rdakit:toolkitLabel xml:lang="da">M-II</rdakit:toolkitLabel>
      <skos:definition xml:lang="da">Videoformat til analoge bånd udviklet til professional brug af Panasonic i 1986.</skos:definition>
      <rdakit:toolkitDefinition xml:lang="da">Videoformat til analoge bånd udviklet til professional brug af Panasonic i 1986.</rdakit:toolkitDefinition>
      <skos:prefLabel xml:lang="fr">M-II</skos:prefLabel>
      <rdakit:toolkitLabel xml:lang="fr">M-II</rdakit:toolkitLabel>
      <skos:definition xml:lang="fr">Format vidéo pour bande analogique conçu pour un usage professionnel par Panasonic en 1986.</skos:definition>
      <rdakit:toolkitDefinition xml:lang="fr">Format vidéo pour bande analogique conçu pour un usage professionnel par Panasonic en 1986.</rdakit:toolkitDefinition>
      <skos:prefLabel xml:lang="no">M-II</skos:prefLabel>
      <rdakit:toolkitLabel xml:lang="no">M-II</rdakit:toolkitLabel>
      <skos:definition xml:lang="no">Et videoformat for analoge videobånd utviklet av Panasonic i 1986 for profesjonell bruk.</skos:definition>
      <rdakit:toolkitDefinition xml:lang="no">Et videoformat for analoge videobånd utviklet av Panasonic i 1986 for profesjonell bruk.</rdakit:toolkitDefinition>
    </skos:Concept>
<!-- Concept: Quadruplex  -->
    <skos:Concept rdf:about="http://rdaregistry.info/termList/videoFormat/1011" xml:lang="en">
      <skos:inScheme rdf:resource="http://rdaregistry.info/termList/videoFormat"/>
      <reg:status rdf:resource="http://metadataregistry.org/uri/RegStatus/1001"/>
      <reg:identifier rdf:resource="http://metadataregistry.org/concepts/909"/>
      <skos:prefLabel xml:lang="en">Quadruplex</skos:prefLabel>
      <rdakit:toolkitLabel xml:lang="en">Quadruplex</rdakit:toolkitLabel>
      <skos:definition xml:lang="en">A video format for analogue tape developed for professional use by Ampex in 1956.</skos:definition>
      <rdakit:toolkitDefinition xml:lang="en">A video format for analogue tape developed for professional use by Ampex in 1956.</rdakit:toolkitDefinition>
      <skos:prefLabel xml:lang="de">Quadruplex</skos:prefLabel>
      <rdakit:toolkitLabel xml:lang="de">Quadruplex</rdakit:toolkitLabel>
      <skos:definition xml:lang="de">Ein Videoformat für ein analoges Band, das 1956 von Ampex für den gewerblichen Gebrauch entwickelt wurde.</skos:definition>
      <rdakit:toolkitDefinition xml:lang="de">Ein Videoformat für ein analoges Band, das 1956 von Ampex für den gewerblichen Gebrauch entwickelt wurde.</rdakit:toolkitDefinition>
      <skos:prefLabel xml:lang="fi">Quadruplex</skos:prefLabel>
      <rdakit:toolkitLabel xml:lang="fi">Quadruplex</rdakit:toolkitLabel>
      <skos:definition xml:lang="fi">Analogisen nauhan videoformaatti, jonka Ampex kehitti ammattilaiskäyttöön vuonna 1956.</skos:definition>
      <rdakit:toolkitDefinition xml:lang="fi">Analogisen nauhan videoformaatti, jonka Ampex kehitti ammattilaiskäyttöön vuonna 1956.</rdakit:toolkitDefinition>
      <skos:prefLabel xml:lang="ca">Quàdruplex</skos:prefLabel>
      <rdakit:toolkitLabel xml:lang="ca">Quàdruplex</rdakit:toolkitLabel>
      <skos:definition xml:lang="ca">Format vídeo per a cinta analògica desenvolupat per a ús professional per Ampex  el 1956.</skos:definition>
      <rdakit:toolkitDefinition xml:lang="ca">Format vídeo per a cinta analògica desenvolupat per a ús professional per Ampex  el 1956.</rdakit:toolkitDefinition>
      <skos:prefLabel xml:lang="da">Quadruplex</skos:prefLabel>
      <rdakit:toolkitLabel xml:lang="da">Quadruplex</rdakit:toolkitLabel>
      <skos:definition xml:lang="da">Videoformat til analoge bånd udviklet til professionel brug af Ampex i 1956.</skos:definition>
      <rdakit:toolkitDefinition xml:lang="da">Videoformat til analoge bånd udviklet til professionel brug af Ampex i 1956.</rdakit:toolkitDefinition>
      <skos:prefLabel xml:lang="fr">Quadruplex</skos:prefLabel>
      <rdakit:toolkitLabel xml:lang="fr">Quadruplex</rdakit:toolkitLabel>
      <skos:definition xml:lang="fr">Format vidéo pour bande analogique conçu pour un usage professionnel par Ampex en 1956.</skos:definition>
      <rdakit:toolkitDefinition xml:lang="fr">Format vidéo pour bande analogique conçu pour un usage professionnel par Ampex en 1956.</rdakit:toolkitDefinition>
      <skos:prefLabel xml:lang="no">Quadruplex</skos:prefLabel>
      <rdakit:toolkitLabel xml:lang="no">Quadruplex</rdakit:toolkitLabel>
      <skos:definition xml:lang="no">Et videoformat for analoge videobånd utviklet av Ampex i 1956 for profesjonell bruk.</skos:definition>
      <rdakit:toolkitDefinition xml:lang="no">Et videoformat for analoge videobånd utviklet av Ampex i 1956 for profesjonell bruk.</rdakit:toolkitDefinition>
    </skos:Concept>
<!-- Concept: Super-VHS  -->
    <skos:Concept rdf:about="http://rdaregistry.info/termList/videoFormat/1012" xml:lang="en">
      <skos:inScheme rdf:resource="http://rdaregistry.info/termList/videoFormat"/>
      <reg:status rdf:resource="http://metadataregistry.org/uri/RegStatus/1001"/>
      <reg:identifier rdf:resource="http://metadataregistry.org/concepts/910"/>
      <skos:prefLabel xml:lang="en">Super-VHS</skos:prefLabel>
      <rdakit:toolkitLabel xml:lang="en">Super-VHS</rdakit:toolkitLabel>
      <skos:definition xml:lang="en">A video format for analogue tape based on VHS that increases horizontal resolution to 420 lines.</skos:definition>
      <rdakit:toolkitDefinition xml:lang="en">A video format for analogue tape based on VHS that increases horizontal resolution to 420 lines.</rdakit:toolkitDefinition>
      <skos:prefLabel xml:lang="de">Super-VHS</skos:prefLabel>
      <rdakit:toolkitLabel xml:lang="de">Super-VHS</rdakit:toolkitLabel>
      <skos:definition xml:lang="de">Ein Videoformat für ein analoges Band, basierend auf VHS, das die horizontale Auflösung auf 420 Zeilen erhöht.</skos:definition>
      <rdakit:toolkitDefinition xml:lang="de">Ein Videoformat für ein analoges Band, basierend auf VHS, das die horizontale Auflösung auf 420 Zeilen erhöht.</rdakit:toolkitDefinition>
      <skos:prefLabel xml:lang="fi">Super-VHS</skos:prefLabel>
      <rdakit:toolkitLabel xml:lang="fi">Super-VHS</rdakit:toolkitLabel>
      <skos:definition xml:lang="fi">Analogisen nauhan VHS:lle perustuva videoformaatti, joka nostaa horisontaalisen resoluution raitojen määrän 420:een.</skos:definition>
      <rdakit:toolkitDefinition xml:lang="fi">Analogisen nauhan VHS:lle perustuva videoformaatti, joka nostaa horisontaalisen resoluution raitojen määrän 420:een.</rdakit:toolkitDefinition>
      <skos:prefLabel xml:lang="ca">Super-VHS</skos:prefLabel>
      <rdakit:toolkitLabel xml:lang="ca">Super-VHS</rdakit:toolkitLabel>
      <skos:definition xml:lang="ca">Format vídeo per a cinta analògica basat en el VHS que incrementa la resolució horitzontal a 420 línies.</skos:definition>
      <rdakit:toolkitDefinition xml:lang="ca">Format vídeo per a cinta analògica basat en el VHS que incrementa la resolució horitzontal a 420 línies.</rdakit:toolkitDefinition>
      <skos:prefLabel xml:lang="da">Super-VHS</skos:prefLabel>
      <rdakit:toolkitLabel xml:lang="da">Super-VHS</rdakit:toolkitLabel>
      <skos:definition xml:lang="da">Videoformat til analoge bånd baseret på VHS, der øger den horisontale opløsning på 420 linjer.</skos:definition>
      <rdakit:toolkitDefinition xml:lang="da">Videoformat til analoge bånd baseret på VHS, der øger den horisontale opløsning på 420 linjer.</rdakit:toolkitDefinition>
      <skos:prefLabel xml:lang="fr">Super-VHS</skos:prefLabel>
      <rdakit:toolkitLabel xml:lang="fr">Super-VHS</rdakit:toolkitLabel>
      <skos:definition xml:lang="fr">Format vidéo pour bande analogique basé sur le format VHS et qui augmente la résolution horizontale à 420 lignes.</skos:definition>
      <rdakit:toolkitDefinition xml:lang="fr">Format vidéo pour bande analogique basé sur le format VHS et qui augmente la résolution horizontale à 420 lignes.</rdakit:toolkitDefinition>
      <skos:prefLabel xml:lang="no">Super-VHS</skos:prefLabel>
      <rdakit:toolkitLabel xml:lang="no">Super-VHS</rdakit:toolkitLabel>
      <skos:definition xml:lang="no">Et videoformat for analoge videobånd som er basert på VHS og øker den horisontale oppløsningen til 420 linjer.</skos:definition>
      <rdakit:toolkitDefinition xml:lang="no">Et videoformat for analoge videobånd som er basert på VHS og øker den horisontale oppløsningen til 420 linjer.</rdakit:toolkitDefinition>
    </skos:Concept>
<!-- Concept: Type C  -->
    <skos:Concept rdf:about="http://rdaregistry.info/termList/videoFormat/1013" xml:lang="en">
      <skos:inScheme rdf:resource="http://rdaregistry.info/termList/videoFormat"/>
      <reg:status rdf:resource="http://metadataregistry.org/uri/RegStatus/1001"/>
      <reg:identifier rdf:resource="http://metadataregistry.org/concepts/911"/>
      <skos:prefLabel xml:lang="en">Type C</skos:prefLabel>
      <rdakit:toolkitLabel xml:lang="en">Type C</rdakit:toolkitLabel>
      <skos:definition xml:lang="en">A video format for analogue tape developed for professional use by Ampex and Sony in 1976.</skos:definition>
      <rdakit:toolkitDefinition xml:lang="en">A video format for analogue tape developed for professional use by Ampex and Sony in 1976.</rdakit:toolkitDefinition>
      <skos:prefLabel xml:lang="de">Type C</skos:prefLabel>
      <rdakit:toolkitLabel xml:lang="de">Type C</rdakit:toolkitLabel>
      <skos:definition xml:lang="de">Ein Videoformat für ein analoges Band, das 1976 von Ampex und Sony für den gewerblichen Gebrauch entwickelt wurde.</skos:definition>
      <rdakit:toolkitDefinition xml:lang="de">Ein Videoformat für ein analoges Band, das 1976 von Ampex und Sony für den gewerblichen Gebrauch entwickelt wurde.</rdakit:toolkitDefinition>
      <skos:prefLabel xml:lang="fi">C-tyyppi</skos:prefLabel>
      <skos:altLabel xml:lang="fi">1&quot; C-formaatti</skos:altLabel>
      <rdakit:toolkitLabel xml:lang="fi">C-tyyppi</rdakit:toolkitLabel>
      <skos:definition xml:lang="fi">Analogisen nauhan videoformaatti, jonka Ampex ja Sony kehittivät ammattilaiskäyttöön vuonna 1976.</skos:definition>
      <rdakit:toolkitDefinition xml:lang="fi">Analogisen nauhan videoformaatti, jonka Ampex ja Sony kehittivät ammattilaiskäyttöön vuonna 1976.</rdakit:toolkitDefinition>
      <skos:prefLabel xml:lang="ca">Tipus C</skos:prefLabel>
      <rdakit:toolkitLabel xml:lang="ca">Tipus C</rdakit:toolkitLabel>
      <skos:definition xml:lang="ca">Format vídeo per a cinta analògica desenvolupat per a ús professional per Ampex el 1976.</skos:definition>
      <rdakit:toolkitDefinition xml:lang="ca">Format vídeo per a cinta analògica desenvolupat per a ús professional per Ampex el 1976.</rdakit:toolkitDefinition>
      <skos:prefLabel xml:lang="da">Type C</skos:prefLabel>
      <rdakit:toolkitLabel xml:lang="da">Type C</rdakit:toolkitLabel>
      <skos:definition xml:lang="da">Videoformat til analoge bånd udviklet til professional brug af Ampex  og Sony i 1976.</skos:definition>
      <rdakit:toolkitDefinition xml:lang="da">Videoformat til analoge bånd udviklet til professional brug af Ampex  og Sony i 1976.</rdakit:toolkitDefinition>
      <skos:prefLabel xml:lang="fr">Type C</skos:prefLabel>
      <rdakit:toolkitLabel xml:lang="fr">Type C</rdakit:toolkitLabel>
      <skos:definition xml:lang="fr">Format vidéo pour bande analogique conçu pour un usage professionnel par Ampex et Sony en 1976.</skos:definition>
      <rdakit:toolkitDefinition xml:lang="fr">Format vidéo pour bande analogique conçu pour un usage professionnel par Ampex et Sony en 1976.</rdakit:toolkitDefinition>
      <skos:prefLabel xml:lang="no">Type C</skos:prefLabel>
      <rdakit:toolkitLabel xml:lang="no">Type C</rdakit:toolkitLabel>
      <skos:definition xml:lang="no">Et videoformat for analoge videobånd utviklet av Ampex og Sony i 1976 for profesjonell bruk.</skos:definition>
      <rdakit:toolkitDefinition xml:lang="no">Et videoformat for analoge videobånd utviklet av Ampex og Sony i 1976 for profesjonell bruk.</rdakit:toolkitDefinition>
    </skos:Concept>
<!-- Concept: U-matic  -->
    <skos:Concept rdf:about="http://rdaregistry.info/termList/videoFormat/1014" xml:lang="en">
      <skos:inScheme rdf:resource="http://rdaregistry.info/termList/videoFormat"/>
      <reg:status rdf:resource="http://metadataregistry.org/uri/RegStatus/1001"/>
      <reg:identifier rdf:resource="http://metadataregistry.org/concepts/912"/>
      <skos:prefLabel xml:lang="en">U-matic</skos:prefLabel>
      <rdakit:toolkitLabel xml:lang="en">U-matic</rdakit:toolkitLabel>
      <skos:definition xml:lang="en">A video format for analogue tape developed for professional use by Sony in 1969.</skos:definition>
      <rdakit:toolkitDefinition xml:lang="en">A video format for analogue tape developed for professional use by Sony in 1969.</rdakit:toolkitDefinition>
      <skos:prefLabel xml:lang="de">U-matic</skos:prefLabel>
      <rdakit:toolkitLabel xml:lang="de">U-matic</rdakit:toolkitLabel>
      <skos:definition xml:lang="de">Ein Videoformat für ein analoges Band, das 1969 von Sony  für den gewerblichen Gebrauch entwickelt wurde.</skos:definition>
      <rdakit:toolkitDefinition xml:lang="de">Ein Videoformat für ein analoges Band, das 1969 von Sony  für den gewerblichen Gebrauch entwickelt wurde.</rdakit:toolkitDefinition>
      <skos:prefLabel xml:lang="fi">U-matic</skos:prefLabel>
      <rdakit:toolkitLabel xml:lang="fi">U-matic</rdakit:toolkitLabel>
      <skos:definition xml:lang="fi">Analogisen nauhan videoformaatti, jonka Sony kehitti ammattilaiskäyttöön vuonna 1969.</skos:definition>
      <rdakit:toolkitDefinition xml:lang="fi">Analogisen nauhan videoformaatti, jonka Sony kehitti ammattilaiskäyttöön vuonna 1969.</rdakit:toolkitDefinition>
      <skos:prefLabel xml:lang="ca">U-matic</skos:prefLabel>
      <rdakit:toolkitLabel xml:lang="ca">U-matic</rdakit:toolkitLabel>
      <skos:definition xml:lang="ca">Format vídeo per a cinta analògica desenvolupat per a ús professional per Sony el 1969.</skos:definition>
      <rdakit:toolkitDefinition xml:lang="ca">Format vídeo per a cinta analògica desenvolupat per a ús professional per Sony el 1969.</rdakit:toolkitDefinition>
      <skos:prefLabel xml:lang="da">U-matic</skos:prefLabel>
      <rdakit:toolkitLabel xml:lang="da">U-matic</rdakit:toolkitLabel>
      <skos:definition xml:lang="da">Videoformat til analoge bånd udviklet til professionel brug af Sony i 1969.</skos:definition>
      <rdakit:toolkitDefinition xml:lang="da">Videoformat til analoge bånd udviklet til professionel brug af Sony i 1969.</rdakit:toolkitDefinition>
      <skos:prefLabel xml:lang="fr">U-matic</skos:prefLabel>
      <rdakit:toolkitLabel xml:lang="fr">U-matic</rdakit:toolkitLabel>
      <skos:definition xml:lang="fr">Format vidéo pour bande analogique conçu pour un usage professionnel par Sony en 1969.</skos:definition>
      <rdakit:toolkitDefinition xml:lang="fr">Format vidéo pour bande analogique conçu pour un usage professionnel par Sony en 1969.</rdakit:toolkitDefinition>
      <skos:prefLabel xml:lang="no">U-matic</skos:prefLabel>
      <rdakit:toolkitLabel xml:lang="no">U-matic</rdakit:toolkitLabel>
      <skos:definition xml:lang="no">Et videoformat for analoge videobånd utviklet av Sony i 1969 for profesjonell bruk.</skos:definition>
      <rdakit:toolkitDefinition xml:lang="no">Et videoformat for analoge videobånd utviklet av Sony i 1969 for profesjonell bruk.</rdakit:toolkitDefinition>
    </skos:Concept>
<!-- Concept: VHS  -->
    <skos:Concept rdf:about="http://rdaregistry.info/termList/videoFormat/1015" xml:lang="en">
      <skos:inScheme rdf:resource="http://rdaregistry.info/termList/videoFormat"/>
      <reg:status rdf:resource="http://metadataregistry.org/uri/RegStatus/1001"/>
      <reg:identifier rdf:resource="http://metadataregistry.org/concepts/913"/>
      <skos:prefLabel xml:lang="en">VHS</skos:prefLabel>
      <skos:altLabel xml:lang="en">Video Home System</skos:altLabel>
      <rdakit:toolkitLabel xml:lang="en">VHS</rdakit:toolkitLabel>
      <skos:definition xml:lang="en">A video format for analogue tape developed for consumer use by JVC in the 1970s.</skos:definition>
      <rdakit:toolkitDefinition xml:lang="en">A video format for analogue tape developed for consumer use by JVC in the 1970s.</rdakit:toolkitDefinition>
      <skos:prefLabel xml:lang="de">VHS</skos:prefLabel>
      <rdakit:toolkitLabel xml:lang="de">VHS</rdakit:toolkitLabel>
      <skos:definition xml:lang="de">Ein Videoformat für ein analoges Band, das in den 1970ern von JVC für den privaten Gebrauch entwickelt wurde.</skos:definition>
      <rdakit:toolkitDefinition xml:lang="de">Ein Videoformat für ein analoges Band, das in den 1970ern von JVC für den privaten Gebrauch entwickelt wurde.</rdakit:toolkitDefinition>
      <skos:prefLabel xml:lang="fi">VHS</skos:prefLabel>
      <rdakit:toolkitLabel xml:lang="fi">VHS</rdakit:toolkitLabel>
      <skos:definition xml:lang="fi">Analogisen nauhan videoformaatti, jonka JVC kehitti kuluttajakäyttöön 1970-luvulla.</skos:definition>
      <rdakit:toolkitDefinition xml:lang="fi">Analogisen nauhan videoformaatti, jonka JVC kehitti kuluttajakäyttöön 1970-luvulla.</rdakit:toolkitDefinition>
      <skos:prefLabel xml:lang="ca">VHS</skos:prefLabel>
      <skos:altLabel xml:lang="ca">Video Home System</skos:altLabel>
      <rdakit:toolkitLabel xml:lang="ca">VHS</rdakit:toolkitLabel>
      <skos:definition xml:lang="ca">Format vídeo per a cinta analògica desenvolupat per a ús domèstic per JVC els anys 1970.</skos:definition>
      <rdakit:toolkitDefinition xml:lang="ca">Format vídeo per a cinta analògica desenvolupat per a ús domèstic per JVC els anys 1970.</rdakit:toolkitDefinition>
      <skos:prefLabel xml:lang="da">VHS</skos:prefLabel>
      <rdakit:toolkitLabel xml:lang="da">VHS</rdakit:toolkitLabel>
      <skos:definition xml:lang="da">Vidoeformat til analoge bånd udviklet til privat brug af JVC i 1970'erne.</skos:definition>
      <rdakit:toolkitDefinition xml:lang="da">Vidoeformat til analoge bånd udviklet til privat brug af JVC i 1970'erne.</rdakit:toolkitDefinition>
      <skos:prefLabel xml:lang="fr">VHS</skos:prefLabel>
      <rdakit:toolkitLabel xml:lang="fr">VHS</rdakit:toolkitLabel>
      <skos:definition xml:lang="fr">Format vidéo pour bande analogique conçu pour un usage grand public par JVC dans les années 1970.</skos:definition>
      <rdakit:toolkitDefinition xml:lang="fr">Format vidéo pour bande analogique conçu pour un usage grand public par JVC dans les années 1970.</rdakit:toolkitDefinition>
      <skos:prefLabel xml:lang="no">VHS</skos:prefLabel>
      <skos:altLabel xml:lang="no">Video Home System</skos:altLabel>
      <rdakit:toolkitLabel xml:lang="no">VHS</rdakit:toolkitLabel>
      <skos:definition xml:lang="no">Et videoformat for analoge videobånd for hjemmebruk utviklet av JVC i på 1970-tallet.</skos:definition>
      <rdakit:toolkitDefinition xml:lang="no">Et videoformat for analoge videobånd for hjemmebruk utviklet av JVC i på 1970-tallet.</rdakit:toolkitDefinition>
    </skos:Concept>

<!-- Status properties used in this document  -->
    <skos:Concept rdf:about="http://metadataregistry.org/uri/RegStatus/1001">
        <skos:prefLabel xml:lang="en">Published</skos:prefLabel>
    </skos:Concept>

</rdf:RDF>
